<?xml version="1.0"?>
<rdf:RDF xml:base="http://sparql.cwrc.ca/ontologies/cwrc#" 
  xmlns="http://sparql.cwrc.ca/ontologies/cwrc#" 
  xmlns:as="http://www.w3.org/ns/activitystreams#" 
  xmlns:bio="http://purl.org/vocab/bio/0.1/" 
  xmlns:cc="http://creativecommons.org/ns#" 
  xmlns:cwrc="http://sparql.cwrc.ca/ontologies/cwrc#" 
  xmlns:dbpedia="http://dbpedia.org/resource/" 
  xmlns:dc="http://purl.org/dc/terms/" 
  xmlns:dcterms="http://purl.org/dc/terms/" 
  xmlns:doap="http://usefulinc.com/ns/doap#" 
  xmlns:foaf="http://xmlns.com/foaf/0.1/" 
  xmlns:loc="http://id.loc.gov/vocabulary/relators/" 
  xmlns:locl ="http://id.loc.gov/vocabulary/languages/"
  xmlns:nif="http://persistence.uni-leipzig.org/nlp2rdf/ontologies/nif-core#" 
  xmlns:oa="http://www.w3.org/ns/oa#" 
  xmlns:owl="http://www.w3.org/2002/07/owl#" 
  xmlns:prov="http://www.w3.org/ns/prov#" 
  xmlns:rdf="http://www.w3.org/1999/02/22-rdf-syntax-ns#" 
  xmlns:rdfs="http://www.w3.org/2000/01/rdf-schema#" 
  xmlns:rel="http://purl.org/vocab/relationship/" 
  xmlns:skos="http://www.w3.org/2004/02/skos/core#" 
  xmlns:skosxl="http://www.w3.org/2008/05/skos-xl#" 
  xmlns:time="http://www.w3.org/2006/time#" 
  xmlns:vann="http://purl.org/vocab/vann/" 
  xmlns:voaf="http://purl.org/vocommons/voaf#" 
  xmlns:void="http://rdfs.org/ns/void#" 
  xmlns:vs="http://www.w3.org/2003/06/sw-vocab-status/ns#" 
  xmlns:xsd="http://www.w3.org/2001/XMLSchema#">
  <owl:Ontology rdf:about="">
    <rdf:type rdf:resource="http://purl.org/vocommons/voaf#Vocabulary"/>
    <vann:preferredNamespacePrefix>cwrc</vann:preferredNamespacePrefix>
    <vann:preferredNamespaceUri>http://sparql.cwrc.ca/ontology/cwrc#</vann:preferredNamespaceUri>
    <dc:title xml:lang="en">The CWRC Ontology</dc:title>
    <rdfs:label xml:lang="en">The CWRC Ontology</rdfs:label>
    <foaf:name xml:lang="en">The CWRC Ontology</foaf:name>
    <dc:title xml:lang="fr">L'Ontologie CWRC</dc:title>
    <rdfs:label xml:lang="fr">L'Ontologie CWRC</rdfs:label>
    <foaf:name xml:lang="fr">L'Ontologie CWRC</foaf:name>
    <dc:description xml:lang="en">The CWRC Ontology is the ontology of the Canadian Writing Research Collaboratory.</dc:description>
    <skos:definition xml:lang="en">The CWRC Ontology is the ontology of the Canadian Writing Research Collaboratory.</skos:definition>
    <rdfs:comment xml:lang="en">The CWRC Ontology is the ontology of the Canadian Writing Research Collaboratory.</rdfs:comment>
    <dc:description xml:lang="fr">L'Ontologie CWRC est l'ontologie du Collaboratoire scientifique des écrits du Canada.</dc:description>
    <skos:definition xml:lang="fr">L'Ontologie CWRC est l'ontologie du Collaboratoire scientifique des écrits du Canada.</skos:definition>
    <rdfs:comment xml:lang="fr">L'Ontologie CWRC est l'ontologie du Collaboratoire scientifique des écrits du Canada.</rdfs:comment>
    <owl:versionInfo>0.99.3</owl:versionInfo>
    <owl:priorVersion rdf:resource="http://sparql.cwrc.ca/ontology/cwrc-2017-03-18"/>
    <dc:date rdf:datatype="http://www.w3.org/2001/XMLSchema#date">ONTOLOGY_DATE</dc:date>
    <dc:rights rdf:resource="http://creativecommons.org/licenses/by-nc/4.0/"/>
    <vs:term_status xml:lang="en">Testing</vs:term_status>
    <dc:creator>
      <foaf:Person rdf:about="#JohnSimpson">
        <foaf:name>John Simpson</foaf:name>
      </foaf:Person>
    </dc:creator>
    <dc:creator>
      <foaf:Person rdf:about="#AbigelLemak">
        <foaf:name>Abigel Lemak</foaf:name>
      </foaf:Person>
    </dc:creator>
    <dc:creator>
      <foaf:Person rdf:about="#JadePenancier">
        <foaf:name>Jade Penancier</foaf:name>
      </foaf:Person>
    </dc:creator>
    <dc:creator>
      <foaf:Person rdf:about="#KimMartin">
        <foaf:name>Kim Martin</foaf:name>
      </foaf:Person>
    </dc:creator>
    <dc:creator rdf:resource="#SusanBrown"/>
    <dc:creator>
      <foaf:Person rdf:about="#ColinFaulkner">
        <foaf:name>Colin Faulkner</foaf:name>
      </foaf:Person>
    </dc:creator>
    <dc:creator>
      <foaf:Person rdf:about="#RobWarren">
        <foaf:name>Robert Warren</foaf:name>
        <owl:sameAs rdf:resource="http://rdf.muninn-project.org/ww1/2011/11/11/Person/Warren"/>
      </foaf:Person>
    </dc:creator>
    <dc:creator>
      <foaf:Person rdf:about="#AlliyyaMo">
        <foaf:name>Alliyya Mo</foaf:name>
      </foaf:Person>
    </dc:creator>
    <dc:publisher>
      <foaf:Organization rdf:about="#cwrc">
        <foaf:name xml:lang="fr">Le Collaboratoire scientifique des écrits du Canada</foaf:name>
        <foaf:name xml:lang="en">The Canadian Writing Research Collaboratory</foaf:name>
        <foaf:logo rdf:resource="http://sparql.cwrc.ca/images/CWRCLogo-Horz-FullColour.png"/>
      </foaf:Organization>
    </dc:publisher>
    <loc:pdr>
      <foaf:Person rdf:about="#SusanBrown">
        <foaf:name>Susan Brown</foaf:name>
        <owl:sameAs rdf:resource="http://orcid.org/0000-0002-0267-7344"/>
      </foaf:Person>
    </loc:pdr>
    <loc:ctb>
      <foaf:Person rdf:about="#ConstanceCrompton">
        <foaf:name>Constance Crompton</foaf:name>
      </foaf:Person>
    </loc:ctb>
    <loc:fnd>
      <foaf:Organization rdf:about="#sshrc">
        <foaf:name xml:lang="en">Social Sciences and Humanities Research Council</foaf:name>
        <foaf:name xml:lang="fr">Conseil de recherches en sciences humaines</foaf:name>
        <foaf:nick>SSHRC</foaf:nick>
      </foaf:Organization>
    </loc:fnd>
    <vann:preferredNamespacePrefix>cwrc</vann:preferredNamespacePrefix>
    <void:inDataset rdf:resource="#datasetdefinition"/>
    <foaf:logo rdf:resource="http://sparql.cwrc.ca/images/CWRCLogo-Horz-FullColour.png"/>
    <dc:subject rdf:resource="http://id.loc.gov/authorities/subjects/sh85019388"/>
    <dc:subject rdf:resource="http://id.loc.gov/authorities/subjects/sh85043777"/>
    <dc:subject rdf:resource="http://id.loc.gov/authorities/subjects/sh85013838"/>
    <dc:subject rdf:resource="http://id.loc.gov/authorities/subjects/sh85077519"/>
    <dc:subject rdf:resource="http://id.loc.gov/authorities/subjects/sh2009007122"/>
  </owl:Ontology>
  <!-- http://id.loc.gov/vocabulary/relators/ctb -->
  <void:Dataset rdf:about="#datasetdefinition">
    <dc:title xml:lang="en">The CWRC Ontology</dc:title>
    <rdfs:label xml:lang="en">The CWRC Ontology</rdfs:label>
    <foaf:name xml:lang="en">The CWRC Ontology</foaf:name>
    <dc:title xml:lang="fr">L'Ontologie CWRC</dc:title>
    <rdfs:label xml:lang="fr">L'Ontologie CWRC</rdfs:label>
    <foaf:name xml:lang="fr">L'Ontologie CWRC</foaf:name>
    <dc:description xml:lang="en">The CWRC Ontology is the ontology of the Canadian Writing Research Collaboratory.</dc:description>
    <skos:definition xml:lang="en">The CWRC Ontology is the ontology of the Canadian Writing Research Collaboratory.</skos:definition>
    <rdfs:comment xml:lang="en">The CWRC Ontology is the ontology of the Canadian Writing Research Collaboratory.</rdfs:comment>
    <dc:description xml:lang="fr">L'Ontologie CWRC est l'ontologie du Collaboratoire scientifique des écrits du Canada.</dc:description>
    <skos:definition xml:lang="fr">L'Ontologie CWRC est l'ontologie du Collaboratoire scientifique des écrits du Canada.</skos:definition>
    <rdfs:comment xml:lang="fr">L'Ontologie CWRC est l'ontologie du Collaboratoire scientifique des écrits du Canada.</rdfs:comment>
    <!-- -->
    <cc:license rdf:resource="http://creativecommons.org/licenses/by-nc/4.0/"/>
    <cc:Jurisdiction rdf:resource="http://dbpedia.org/resource/Canada"/>
    <cc:attributionURL rdf:resource="http://www.cwrc.ca/"/>
    <dc:creator rdf:resource="#JohnSimpson"/>
    <dc:creator rdf:resource="#AbiLemak"/>
    <dc:creator rdf:resource="#ColinFaulkner"/>
    <dc:creator rdf:resource="#RobWarren"/>
    <dc:publisher rdf:resource="#cwrc"/>
    <dc:creator rdf:resource="#JadePenancier"/>
    <dc:creator rdf:resource="#AlliyyaMo"/>
    <dc:creator rdf:resource="#KimMartin"/>
    <dc:creator rdf:resource="#SusanBrown"/>
    <loc:ctb rdf:resource="#ConstanceCrompton"/>
    <loc:ctb rdf:resource="#originalOrlandoAuthor"/>
    <loc:pdr rdf:resource="#SusanBrown"/>
    <loc:fnd rdf:resource="#sshrc"/>
    <rdfs:isDefinedBy rdf:resource="http://sparql.cwrc.ca/ontologies/cwrc-ONTOLOGY_DATE"/>
    <foaf:logo rdf:resource="http://www.cwrc.ca/wp-content/uploads/2010/11/CWRC_logo_v074.gif"/>
    <dc:subject rdf:resource="http://id.loc.gov/authorities/subjects/sh85019388"/>
    <dc:subject rdf:resource="http://id.loc.gov/authorities/subjects/sh85043777"/>
    <dc:subject rdf:resource="http://id.loc.gov/authorities/subjects/sh85013838"/>
    <dc:subject rdf:resource="http://id.loc.gov/authorities/subjects/sh85077519"/>
    <dc:subject rdf:resource="http://id.loc.gov/authorities/subjects/sh2009007122"/>
  </void:Dataset>
  <skos:Concept rdf:about="#originalOrlandoAuthor">
    <rdfs:label xml:lang="en">Members of the Orlando Project</rdfs:label>
    <rdfs:label xml:lang="fr">Les membres du projet Orlando</rdfs:label>
    <rdf:type rdf:resource="http://xmlns.com/foaf/0.1/Group"/>
    <foaf:name xml:lang="en">Members of the Orlando Project.</foaf:name>
    <foaf:homepage rdf:resource="http://orlando.cambridge.org/public/svDocumentation?formname=t&amp;d_id=CREDITSANDACKNOWLEDGEMENTS"/>
    <skos:definition xml:lang="en">The collection of all persons having written entries for The Orlando Project.</skos:definition>
    <skos:definition xml:lang="fr">La collection de tous les auteurs du Projet Orlando.</skos:definition>
    <rdfs:isDefinedBy rdf:resource="http://sparql.cwrc.ca/ontologies/cwrc-ONTOLOGY_DATE"/>
    <void:inDataset rdf:resource="#datasetdefinition"/>
    <void:triples>TOTAL_TRIPLES_CWRC_ONTOLOGY</void:triples>
    <void:entities>TOTAL_ENTITIES_CWRC_ONTOLOGY</void:entities>
  </skos:Concept>
  <!-- End Boilerplate -->
  <owl:Class rdf:ID="Event">
    <foaf:name>Event</foaf:name>
    <rdfs:label xml:lang="en">event (historical)</rdfs:label>
    <rdfs:label xml:lang="fr">évènement (historique)</rdfs:label>
    <rdfs:label xml:lang="de">event</rdfs:label>
    <skos:definition xml:lang="en">An event that occurs in space and time.</skos:definition>
    <rdf:type rdf:resource="http://www.w3.org/2006/time/TemporalEntity"/>
    <owl:sameAs rdf:resource="http://erlangen-crm.org/current/E5.Event"/>
    <owl:sameAs rdf:resource="http://linkedevents.org/ontology/Event"/>
    <owl:sameAs rdf:resource="http://en.wikipedia.org/wiki/Event"/>
    <rdfs:isDefinedBy rdf:resource="http://sparql.cwrc.ca/ontologies/cwrc-ONTOLOGY_DATE"/>
    <rdf:type rdf:resource="http://www.w3.org/2004/02/skos/core#Concept"/>
    <void:inDataset rdf:resource="#datasetdefinition"/>
  </owl:Class>
  <owl:ObjectProperty rdf:ID="hasActor">
    <rdfs:label xml:lang="en">has actor</rdfs:label>
    <rdfs:comment xml:lang="en">An Actor in this event.</rdfs:comment>
    <rdfs:range rdf:resource="#Event"/>
    <rdfs:range rdf:resource="#Actor"/>
    <rdfs:isDefinedBy rdf:resource="http://sparql.cwrc.ca/ontologies/cwrc-ONTOLOGY_DATE"/>
    <rdf:type rdf:resource="http://www.w3.org/2004/02/skos/core#Concept"/>
    <void:inDataset rdf:resource="#datasetdefinition"/>
  </owl:ObjectProperty>
  <owl:Class rdf:ID="Actor">
    <rdfs:label xml:lang="en">actor</rdfs:label>
    <rdfs:comment xml:lang="en">A person performing a certain role within an event.</rdfs:comment>
    <owl:sameAs rdf:resource="http://erlangen-crm.org/current/E39.Actor"/>
    <rdfs:isDefinedBy rdf:resource="http://sparql.cwrc.ca/ontologies/cwrc-ONTOLOGY_DATE"/>
    <rdf:type rdf:resource="http://www.w3.org/2004/02/skos/core#Concept"/>
    <void:inDataset rdf:resource="#datasetdefinition"/>
  </owl:Class>
  <owl:ObjectProperty rdf:ID="identity">
    <rdfs:label xml:lang="en">identity</rdfs:label>
    <rdfs:comment xml:lang="en">The identity of the person who committed the act.</rdfs:comment>
    <rdfs:domain rdf:resource="#Actor"/>
    <rdfs:range rdf:resource="#Person"/>
    <rdfs:isDefinedBy rdf:resource="http://sparql.cwrc.ca/ontologies/cwrc-ONTOLOGY_DATE"/>
    <rdf:type rdf:resource="http://www.w3.org/2004/02/skos/core#Concept"/>
    <void:inDataset rdf:resource="#datasetdefinition"/>
  </owl:ObjectProperty>
  <owl:ObjectProperty rdf:ID="inRole">
    <rdfs:label xml:lang="en">in role</rdfs:label>
    <rdfs:comment xml:lang="en">The role taken on by this actor.</rdfs:comment>
    <rdfs:domain rdf:resource="#Actor"/>
    <rdfs:range rdf:resource="#Role"/>
    <rdfs:isDefinedBy rdf:resource="http://sparql.cwrc.ca/ontologies/cwrc-ONTOLOGY_DATE"/>
    <rdf:type rdf:resource="http://www.w3.org/2004/02/skos/core#Concept"/>
    <void:inDataset rdf:resource="#datasetdefinition"/>
  </owl:ObjectProperty>
  <!-- Events -->
  <owl:Class rdf:ID="Address">
    <rdfs:label xml:lang="en">address</rdfs:label>
    <rdfs:label xml:lang="fr">adresse</rdfs:label>
    <skos:definition xml:lang="en">A mailling or street address.</skos:definition>
    <skos:definition xml:lang="fr">Une adresse postale ou de rue.</skos:definition>
    <rdfs:comment xml:lang="en">The postal address is the equivalent of a schema.org address and inherits all of the data from that vocabulary to markup a modern postral address.</rdfs:comment>
    <owl:sameAs rdf:resource="http://schema.org/PostalAddress"/>
    <rdfs:subClassOf rdf:resource="#Place"/>
    <rdfs:isDefinedBy rdf:resource="http://sparql.cwrc.ca/ontologies/cwrc-ONTOLOGY_DATE"/>
    <rdf:type rdf:resource="http://www.w3.org/2004/02/skos/core#Concept"/>
    <void:inDataset rdf:resource="#datasetdefinition"/>
  </owl:Class>
  <owl:Class rdf:ID="Place">
    <rdfs:label xml:lang="en">place</rdfs:label>
    <rdfs:label xml:lang="fr">endroit</rdfs:label>
    <foaf:name xml:lang="en">Place</foaf:name>
    <foaf:name xml:lang="fr">Endroit</foaf:name>
    <skos:definition xml:lang="en">A named place, wheter incorporated, settled or occupied.</skos:definition>
    <skos:definition xml:lang="en">Un endroit nommé, qu'il soit déclaré, investi ou occupé.</skos:definition>
    <rdfs:comment xml:lang="en">Could be a populated place according to Geonames, but not necessarily so. Some places, such as cross-roads are named without having a population or settlement per say. The geonames is incosistent in this regards in that a populated place can be abandonned.</rdfs:comment>
    <owl:equivalentClass rdf:resource="http://www.geonames.org/ontology#Feature"/>
    <owl:equivalentClass rdf:resource="http://dbpedia.org/ontology/Place"/>
    <owl:equivalentClass rdf:resource="http://schema.org/Place"/>
    <rdfs:subClassOf rdf:resource="http://www.w3.org/2003/01/geo/wgs84_pos#SpatialThing"/>
    <owl:sameAs rdf:resource="http://geovocab.org/spatial#Feature"/>
    <owl:sameAs rdf:resource="http://www.opengis.net/ont/geosparql#Feature"/>
    <rdfs:isDefinedBy rdf:resource="http://sparql.cwrc.ca/ontologies/cwrc-ONTOLOGY_DATE"/>
    <rdf:type rdf:resource="http://www.w3.org/2004/02/skos/core#Concept"/>
    <void:inDataset rdf:resource="#datasetdefinition"/>
  </owl:Class>
  <owl:DeprecatedClass rdf:ID="CulturalFormation">
    <rdfs:label xml:lang="en">cultural formation </rdfs:label>
    <rdfs:label xml:lang="fr">formation culturelle</rdfs:label>
    <rdf:type rdf:resource="http://www.w3.org/2004/02/skos/core#Concept"/>
    <skos:definition xml:lang="en">Cultural formation refers to the processes of lived social subjectivities of people and is often combined with predicates indicating the identity positions as they relate to the following discursive constructions of Class, Religion, Ethnicity, Gender, GeographicalHeritage, LinguisticAbility, NationalHeritage, NationalIdentity, PoliticalAffiliation, RaceColour, Sexuality. These categories are not understood as transhistorical or isolated categories. Rather, they facilitate analysis of how such situationally contingent, changing, and negotiated labels are assigned to or adopted by a particular individual. The tensions endemic to practices of classification demand critical engagement and inquiry into the situatedness of particular cultural identities.</skos:definition>
    <skos:definition xml:lang="fr"/>
    <rdfs:isDefinedBy rdf:resource="http://sparql.cwrc.ca/ontologies/cwrc-ONTOLOGY_DATE"/>
    <void:inDataset rdf:resource="#datasetdefinition"/>
    <owl:equivalentClass rdf:resource="#CulturalForm"/>
    <dc:isReplacedBy rdf:resource="#CulturalForm"/>
    <vs:term_status xml:lang="en">deprecated</vs:term_status>
  </owl:DeprecatedClass>
  <owl:Class rdf:ID="CulturalForm">
    <rdfs:label xml:lang="en">cultural form</rdfs:label>
    <rdfs:label xml:lang="fr">forme culturelle</rdfs:label>
    <rdf:type rdf:resource="http://www.w3.org/2004/02/skos/core#Concept"/>
    <skos:definition xml:lang="en">Cultural forms refers to the processes of lived social subjectivities of people and is often combined with predicates indicating the identity positions as they relate to the following discursive constructions of Class, Religion, Ethnicity, Gender, GeographicalHeritage, LinguisticAbility, NationalHeritage, NationalIdentity, PoliticalAffiliation, RaceColour, Sexuality. These categories are not understood as transhistorical or isolated categories. Rather, they facilitate analysis of how such situationally contingent, changing, and negotiated labels are assigned to or adopted by a particular individual. The tensions endemic to practices of classification demand critical engagement and inquiry into the situatedness of particular cultural identities.</skos:definition>
    <skos:definition xml:lang="fr"/>
    <rdfs:isDefinedBy rdf:resource="http://sparql.cwrc.ca/ontologies/cwrc-ONTOLOGY_DATE"/>
    <void:inDataset rdf:resource="#datasetdefinition"/>
  </owl:Class>
  <owl:ObjectProperty rdf:ID="hasCulturalForms">
    <rdfs:label xml:lang="en">has a cultural form</rdfs:label>
    <rdfs:label xml:lang="fr">a une forme culturelle</rdfs:label>
    <skos:definition xml:lang="en">This sub-class of culturalFormation associates specific concepts and categories with the process of identity formation through cultural processes. Such associations may be or have been embraced by the subject her/himself or attributed by others. The concepts and categories classed as culturalForms are understood to overlap with each other conceptually and in terms of the labels used.</skos:definition>
    <skos:definition xml:lang="fr">Cette sous-classe de culturalFormation associe des concepts et des catégories spécifiques au processus de formation identitaire à travers les processus culturels. Le sujet elle/lui-même peut ou a pu s’approprier de telles associations, ou d’autres personnes les lui ont attribuées. Les concepts et les catégories classés dans culturalForms se chevauchent en théorie et en terme d'étiquettes utilisés.</skos:definition>
    <rdfs:isDefinedBy rdf:resource="http://sparql.cwrc.ca/ontologies/cwrc-ONTOLOGY_DATE"/>
    <void:inDataset rdf:resource="#datasetdefinition"/>
  </owl:ObjectProperty>
  <!-- Will inherit oa:hasBody and oa:hasTarget from the Annotation -->
  <owl:Class rdf:ID="Context">
    <rdf:type rdf:resource="http://www.w3.org/ns/oa#Annotation"/>
    <rdfs:label xml:lang="en">context</rdfs:label>
    <rdfs:label xml:lang="fr">contexte</rdfs:label>
    <rdf:type rdf:resource="http://www.w3.org/2004/02/skos/core#Concept"/>
    <skos:definition xml:lang="en">A context relates.... </skos:definition>
    <skos:definition xml:lang="fr"/>
    <rdfs:isDefinedBy rdf:resource="http://sparql.cwrc.ca/ontologies/cwrc-ONTOLOGY_DATE"/>
    <void:inDataset rdf:resource="#datasetdefinition"/>
  </owl:Class>
  <!-- Cheat to ensure that the provenance is hooked into the Cultural Context -->
  <rdf:Description rdf:about="http://www.w3.org/ns/prov#derivedFrom">
    <rdfs:range rdf:resource="#Context"/>
  </rdf:Description>
  <owl:Class rdf:ID="RaceEthnicityContext">
    <rdfs:label xml:lang="en">race ethnicity context</rdfs:label>
    <rdfs:label xml:lang="fr">contexte racial et/ou ethnique</rdfs:label>
    <rdf:type rdf:resource="http://www.w3.org/2004/02/skos/core#Concept"/>
    <rdfs:subClassOf rdf:resource="#Context"/>
    <skos:definition xml:lang="en">raceEthnicityContext is a significant sub-class within culturalForms. It indicates the presence of information and discussions of a person's subject position with regards to race and ethnicity by working in conjunction with subject specific sub-elements (raceColour, nationalHeritage, geogHeritage, ethnicity). The following discussion applies to both the general discursive context of raceAndEthnicity as well as the specific sub-class categories. Despite the ways in which categories of race and ethnicity frequently serve heinous interests, their ideological and material impacts in the formation of identities requires recognition. These are shifting, historically constituted, and interestedly deployed categories whose use must be situated contextually and which are understood here finally as discursive or representational. Because of this this ontology does not try to lay out an exact, fully defined, or mutually exclusive set of categories: this is an impossibility given their shifting use and the overlap among them. Those applying this class and its subclasses are encouraged not to let privileged identities operate as an unspoken given or to use this class solely in relation to the marginalized. Those concerned about &quot;white&quot; and &quot;black&quot; as homogenizing categories are encouraged to reach for specificity through multiplicity and representations of intersectionality. RaceAndEthnicity is a sub-class within culturalFormation. It has four related content sub-classes: raceColour, nationalHeritage, geogHeritage, and ethnicity.</skos:definition>
    <skos:definition xml:lang="fr">raceEthnicityContext est une sous-classe importante de culturalForms. Elle indique la présence d’informations et de discussions sur le sujet concernant son appartenance raciale et ethnique, conjointement avec les sous-éléments spécifiques au sujet (raceColour, nationalHeritage, geogHeritage, ethnicity). La discussion qui suit s’applique au contexte discursif général de raceAndEthnicity ainsi qu’aux catégories spécifiques de cette sous-classe. Même si les catégories de race et d'ethnicité sont fréquemment manipulées au service d'intérêts déplorables, elles doivent être prises en compte à cause de leur répercussions idéologiques et matérielles sur la formation identitaire. Ces catégories sont changeantes, historiquement constituées, développées de façon intéressée, doivent être employées en contexte et sont ici entendues comme discursives et représentationnelles. C'est pour ces raisons que l'ontologie ne prétend pas offrir un ensemble de catégories exactes, complètement définies, ou mutuellement exclusives, ce que leur emploi instable et leur chevauchement ne permettent pas. Celles/ceux qui appliquent ces catégories et sous-catégories sont encouragé/es à ne pas faire fonctionner les identités privilégiées comme si elles étaient consensuelles et évidentes, ou à utiliser cette classe seulement pour les marginaux. Celles/ceux préoccupés par le fait que &quot;blanc&quot; et &quot;noir&quot; sont des catégories homogénéisantes sont encouragés à atteindre la spécificité à travers la multiplicité et les représentations intersectionnelles. RaceAndEthnicity est sous-classe de culturalFormation. Elle a quatre sous-classes qui lui sont liées: raceColour, nationalHeritage, geogHeritage et ethnicity.</skos:definition>
    <rdfs:isDefinedBy rdf:resource="http://sparql.cwrc.ca/ontologies/cwrc-ONTOLOGY_DATE"/>
    <void:inDataset rdf:resource="#datasetdefinition"/>
    <dc:subject rdf:resource="#Ethnicity"/>
    <dc:subject rdf:resource="#RaceColour"/>
  </owl:Class>
  <owl:Class rdf:ID="SexualityContext">
    <rdfs:label xml:lang="en">sexuality context</rdfs:label>
    <rdfs:label xml:lang="fr">contexte de sexualité</rdfs:label>
    <rdf:type rdf:resource="http://www.w3.org/2004/02/skos/core#Concept"/>
    <rdfs:subClassOf rdf:resource="#Context"/>
    <skos:definition xml:lang="en">hasSexualityContext is a significant sub-class within culturalForms. It indicates the presence of information and discussions of a person's subject position with regards to their sexuality and sexual identity. A subclass of Cultural Formation, hasSexualityContext provides depth to more granual categorizations of a person through hasSexuality or hasSexuality. It is not meant to capture individual sexual experiences and relationships, which are covered by intimateRelationships. Specific relationships may be invoked here to indicate the effect on a subject's life and understanding of her own sexuality. This effort to to contextualize gestures towards some of the complicated issues around sexuality, for example, the politics of outing, the historical specificity of some categories such as &quot;congenital invert,&quot; or the multiple forms of relating to one's own sexuality. Capturing discussions of her sexuality within this element, will help users interested in the historical, ideological and gendered constructions of sexuality. There are important politics of privacy with respect to the disclosure of a subject's sexuality, sexual orientation and sexual identity. As far as living persons are concerned, our practice is to draw only on widely circulated public sources or disclosures from the subject her/himself in order to avoid inadvertently outing someone. See Campbell and Cowan 2016</skos:definition>
    <skos:definition xml:lang="fr">sexualityContext est une sous-classe importante de culturalForms. Elle indique la présence de données ou de discussions sur la subjectivité d’une personne en ce qui concerne sa sexualité et son identité sexuelle. Sous-classe de culturalForms, sexualityContext approfondit la catégorisation granulaire d’une personne à travers hasSexuality ou hasSexuality. Elle n’est pas vouée à répertorier les expériences sexuelles et relations personnelles, qui sont comprises dans intimateRelationships. Des relations spécifiques pourront être évoquées ici pour indiquer les conséquences qu’elles ont eu dans la vie du sujet ou la compréhension de sa propre sexualité. Cet effort de contextualisation est un mouvement vers des questions complexes autours de la sexualité, comme par exemple les politiques de délation autour de la sexualité, la spécificité historique de certaines catégories comme “inversion sexuelle”, ou les multiples formes liées à la sexualité d’une personne. Les utilisatrices/teurs intéressé/es par la construction historique, idéologique et genrée de la sexualité pour se servir de cet élément qui rend compte des débats autour de ce thème. Nous reconnaissons l'importance des politiques de confidentialité au regard de la divulgation de la sexualité, de l’orientation et de l’identité sexuelles du sujet. En ce qui concerne les personnes toujours en vie, notre pratique est de ne nous appuyer que sur des sources ou des déclarations publiques venant du sujet elle/lui-même, afin d’éviter de dévoiler par inadvertance des informations privées sur sa sexualité. Voir Campbell and Cowan 2016. (http://ir.lib.uwo.ca/cgi/viewcontent.cgi?article=1085&amp;context=fimspub). </skos:definition>
    <rdfs:isDefinedBy rdf:resource="http://sparql.cwrc.ca/ontologies/cwrc-ONTOLOGY_DATE"/>
    <void:inDataset rdf:resource="#datasetdefinition"/>
    <dc:subject rdf:resource="#Sexuality"/>
    <dc:subject rdf:resource="#Gender"/>
  </owl:Class>
  <!--  (http://ir.lib.uwo.ca/cgi/viewcontent.cgi?article=1085&context=fimspub) -->
  <owl:Class rdf:ID="LanguageContext">
    <rdfs:label xml:lang="en">language context</rdfs:label>
    <rdfs:label xml:lang="fr">contexte linguistique</rdfs:label>
    <rdf:type rdf:resource="http://www.w3.org/2004/02/skos/core#Concept"/>
    <rdfs:subClassOf rdf:resource="#Context"/>
    <dc:subject rdf:resource="#LinguisticAbility"/>
    <skos:definition xml:lang="en"/>
    <skos:definition xml:lang="fr"/>
    <rdfs:isDefinedBy rdf:resource="http://sparql.cwrc.ca/ontologies/cwrc-ONTOLOGY_DATE"/>
    <void:inDataset rdf:resource="#datasetdefinition"/>
    <dc:subject rdf:resource="#Language"/>
  </owl:Class>
  <owl:Class rdf:ID="SocialClassContext">
    <rdfs:label xml:lang="en">social class context</rdfs:label>
    <rdfs:label xml:lang="fr">contexte de classe sociale</rdfs:label>
    <rdf:type rdf:resource="http://www.w3.org/2004/02/skos/core#Concept"/>
    <rdfs:subClassOf rdf:resource="#Context"/>
    <dc:subject rdf:resource="#SocialClassIdentity"/>
    <skos:definition xml:lang="en"/>
    <skos:definition xml:lang="fr"/>
    <rdfs:isDefinedBy rdf:resource="http://sparql.cwrc.ca/ontologies/cwrc-ONTOLOGY_DATE"/>
    <void:inDataset rdf:resource="#datasetdefinition"/>
    <dc:subject rdf:resource="#SocialClassIdentity"/>
  </owl:Class>
  <owl:Class rdf:ID="ReligionContext">
    <rdfs:label xml:lang="en">religious context</rdfs:label>
    <rdfs:label xml:lang="fr">contexte religieux</rdfs:label>
    <rdf:type rdf:resource="http://www.w3.org/2004/02/skos/core#Concept"/>
    <rdfs:subClassOf rdf:resource="#Context"/>
    <dc:subject rdf:resource="#Religion"/>
    <skos:definition xml:lang="en"/>
    <skos:definition xml:lang="fr"/>
    <rdfs:isDefinedBy rdf:resource="http://sparql.cwrc.ca/ontologies/cwrc-ONTOLOGY_DATE"/>
    <void:inDataset rdf:resource="#datasetdefinition"/>
    <dc:subject rdf:resource="#Religion"/>
  </owl:Class>
  <owl:Class rdf:ID="NationalityContext">
    <rdfs:label xml:lang="en">nationality context</rdfs:label>
    <rdfs:label xml:lang="fr">contexte de nationalité</rdfs:label>
    <rdf:type rdf:resource="http://www.w3.org/2004/02/skos/core#Concept"/>
    <rdfs:subClassOf rdf:resource="#Context"/>
    <dc:subject rdf:resource="#NationalHeritage"/>
    <dc:subject rdf:resource="#NationalIdentity"/>
    <dc:subject rdf:resource="#GeographicalHeritage"/>
    <skos:definition xml:lang="en"/>
    <skos:definition xml:lang="fr"/>
    <rdfs:isDefinedBy rdf:resource="http://sparql.cwrc.ca/ontologies/cwrc-ONTOLOGY_DATE"/>
    <void:inDataset rdf:resource="#datasetdefinition"/>
  </owl:Class>
  <owl:Class rdf:ID="PoliticalContext">
    <rdfs:label xml:lang="en">political context</rdfs:label>
    <rdfs:label xml:lang="fr">contexte politique</rdfs:label>
    <rdf:type rdf:resource="http://www.w3.org/2004/02/skos/core#Concept"/>
    <rdfs:subClassOf rdf:resource="#Context"/>
    <dc:subject rdf:resource="#PoliticalAffiliation"/>
    <skos:definition xml:lang="en"/>
    <skos:definition xml:lang="fr"/>
    <rdfs:isDefinedBy rdf:resource="http://sparql.cwrc.ca/ontologies/cwrc-ONTOLOGY_DATE"/>
    <void:inDataset rdf:resource="#datasetdefinition"/>
  </owl:Class>
  <owl:Class rdf:ID="EthnicityContext">
    <rdfs:label xml:lang="en">racial, colour or ethnicity context</rdfs:label>
    <rdfs:label xml:lang="fr">contexte racial, de couleur de peau ou d'ethnicité</rdfs:label>
    <rdf:type rdf:resource="http://www.w3.org/2004/02/skos/core#Concept"/>
    <rdfs:subClassOf rdf:resource="#Context"/>
    <dc:subject rdf:resource="#Ethnicity"/>
    <dc:subject rdf:resource="#RaceColour"/>
    <skos:definition xml:lang="en"/>
    <skos:definition xml:lang="fr"/>
    <rdfs:isDefinedBy rdf:resource="http://sparql.cwrc.ca/ontologies/cwrc-ONTOLOGY_DATE"/>
    <void:inDataset rdf:resource="#datasetdefinition"/>
    <dc:subject rdf:resource="#Ethnicity"/>
  </owl:Class>
  <owl:Class rdf:ID="GenderContext">
    <rdfs:label xml:lang="en">Gender Context</rdfs:label>
    <rdfs:label xml:lang="fr">Contexte de Genre</rdfs:label>
    <rdf:type rdf:resource="http://www.w3.org/2004/02/skos/core#Concept"/>
    <rdfs:subClassOf rdf:resource="#Context"/>
    <dc:subject rdf:resource="#Gender"/>
    <skos:definition xml:lang="en"/>
    <skos:definition xml:lang="fr"/>
    <rdfs:isDefinedBy rdf:resource="http://sparql.cwrc.ca/ontologies/cwrc-ONTOLOGY_DATE"/>
    <void:inDataset rdf:resource="#datasetdefinition"/>
  </owl:Class>
  <!-- End contexts -->
  <owl:Class rdf:ID="NationalHeritage">
    <rdfs:label xml:lang="en">National Heritage</rdfs:label>
    <rdfs:label xml:lang="fr">Héritage National</rdfs:label>
    <rdf:type rdf:resource="http://www.w3.org/2004/02/skos/core#Concept"/>
    <rdfs:subClassOf rdf:resource="#CulturalForm"/>
    <skos:definition xml:lang="en">A subclass of culturalForms, this escrbes a person's national heritage and is not the same as citizenship.</skos:definition>
    <skos:definition xml:lang="fr"/>
    <rdfs:isDefinedBy rdf:resource="http://sparql.cwrc.ca/ontologies/cwrc-ONTOLOGY_DATE"/>
    <void:inDataset rdf:resource="#datasetdefinition"/>
  </owl:Class>
  <owl:DeprecatedClass rdf:about="#EnglishNationalHeritage">
    <rdfs:label xml:lang="en">English</rdfs:label>
    <rdfs:label xml:lang="fr">Anglais</rdfs:label>
    <rdf:type rdf:resource="http://www.w3.org/2004/02/skos/core#Concept"/>
    <skos:definition xml:lang="en"/>
    <skos:definition xml:lang="fr"/>
    <rdfs:isDefinedBy rdf:resource="http://sparql.cwrc.ca/ontologies/cwrc-ONTOLOGY_DATE"/>
    <void:inDataset rdf:resource="#datasetdefinition"/>
    <owl:equivalentClass rdf:resource="#englishNationalHeritage"/>
    <dc:isReplacedBy rdf:resource="#englishNationalHeritage"/>
    <vs:term_status xml:lang="en">deprecated</vs:term_status>
  </owl:DeprecatedClass>
  <cwrc:NationalHeritage rdf:about="#englishNationalHeritage">
    <rdfs:label xml:lang="en">English</rdfs:label>
    <rdfs:label xml:lang="fr">Anglais</rdfs:label>
    <rdf:type rdf:resource="http://www.w3.org/2004/02/skos/core#Concept"/>
    <skos:definition xml:lang="en"/>
    <skos:definition xml:lang="fr"/>
    <rdfs:isDefinedBy rdf:resource="http://sparql.cwrc.ca/ontologies/cwrc-ONTOLOGY_DATE"/>
    <void:inDataset rdf:resource="#datasetdefinition"/>
  </cwrc:NationalHeritage>

  <cwrc:NationalIdentity rdf:about="#jewishNationalIdentity">
    <rdfs:label xml:lang="en">Jewish</rdfs:label>
    <rdfs:label xml:lang="fr">Juif</rdfs:label>
    <rdf:type rdf:resource="http://www.w3.org/2004/02/skos/core#Concept"/>
    <skos:definition xml:lang="en"/>
    <skos:definition xml:lang="fr"/>
    <skos:broader rdf:resource="#jewishlabel"/>
    <rdfs:isDefinedBy rdf:resource="http://sparql.cwrc.ca/ontologies/cwrc-ONTOLOGY_DATE"/>
    <void:inDataset rdf:resource="#datasetdefinition"/>
  </cwrc:NationalIdentity>
  <owl:Class rdf:ID="NationalIdentity">
    <rdfs:label xml:lang="en">National Identity</rdfs:label>
    <rdfs:label xml:lang="fr">Identité Nationale</rdfs:label>
    <rdf:type rdf:resource="http://www.w3.org/2004/02/skos/core#Concept"/>
    <rdfs:subClassOf rdf:resource="#CulturalForm"/>
    <skos:definition xml:lang="en">A subclass of culturalForms, this descrbes a person's nationality/ies and is not the same as citizenship.</skos:definition>
    <skos:definition xml:lang="fr"/>
    <rdfs:isDefinedBy rdf:resource="http://sparql.cwrc.ca/ontologies/cwrc-ONTOLOGY_DATE"/>
    <void:inDataset rdf:resource="#datasetdefinition"/>
  </owl:Class>
  <owl:DeprecatedClass rdf:about="#EnglishNationalIdentity">
    <rdfs:label xml:lang="en">English</rdfs:label>
    <rdfs:label xml:lang="fr">Anglais</rdfs:label>
    <rdf:type rdf:resource="http://www.w3.org/2004/02/skos/core#Concept"/>
    <skos:definition xml:lang="en"/>
    <skos:definition xml:lang="fr"/>
    <rdfs:isDefinedBy rdf:resource="http://sparql.cwrc.ca/ontologies/cwrc-ONTOLOGY_DATE"/>
    <void:inDataset rdf:resource="#datasetdefinition"/>
    <owl:equivalentClass rdf:resource="#englishNationalIdentity"/>
    <dc:isReplacedBy rdf:resource="#englishNationalIdentity"/>
    <vs:term_status xml:lang="en">deprecated</vs:term_status>
  </owl:DeprecatedClass>
  <cwrc:NationalIdentity rdf:about="#englishNationalIdentity">
    <rdfs:label xml:lang="en">English</rdfs:label>
    <rdfs:label xml:lang="fr">Anglais</rdfs:label>
    <rdf:type rdf:resource="http://www.w3.org/2004/02/skos/core#Concept"/>
    <skos:definition xml:lang="en"/>
    <skos:definition xml:lang="fr"/>
    <rdfs:isDefinedBy rdf:resource="http://sparql.cwrc.ca/ontologies/cwrc-ONTOLOGY_DATE"/>
    <void:inDataset rdf:resource="#datasetdefinition"/>
  </cwrc:NationalIdentity>
  <owl:Class rdf:ID="Language">
    <rdfs:label xml:lang="en">Linguistic Ability</rdfs:label>
    <rdfs:label xml:lang="fr">aptitudelinguistique</rdfs:label>
    <foaf:name xml:lang="en">linguistic ability</foaf:name>
    <rdf:type rdf:resource="http://www.w3.org/2004/02/skos/core#Concept"/>
    <rdfs:subClassOf rdf:resource="#CulturalForm"/>
    <skos:definition xml:lang="en">These terms do not differentiate between spoken and/or written. For operational reasons this class is a direct equivalent to ISO639 language code as published by the Library of Congress.</skos:definition>
    <skos:definition xml:lang="fr">Écrit ou Parlé. Pour des raisons opérationnelles, cette classe est équivalente à la classe de langage iso639 publiée par le Library of Congress.</skos:definition>
    <rdfs:isDefinedBy rdf:resource="http://sparql.cwrc.ca/ontologies/cwrc-ONTOLOGY_DATE"/>
    <void:inDataset rdf:resource="#datasetdefinition"/>
    <owl:sameAs rdf:resource="http://id.loc.gov/vocabulary/iso639-1/iso639-1_Language"/>
  </owl:Class>
  <cwrc:Language rdf:about="#EnglishLanguage">
    <rdfs:label xml:lang="en">English</rdfs:label>
    <rdfs:label xml:lang="fr">Anglais</rdfs:label>
    <rdf:type rdf:resource="http://www.w3.org/2004/02/skos/core#Concept"/>
    <skos:definition xml:lang="en"/>
    <skos:definition xml:lang="fr"/>
    <rdfs:isDefinedBy rdf:resource="http://sparql.cwrc.ca/ontologies/cwrc-ONTOLOGY_DATE"/>
    <void:inDataset rdf:resource="#datasetdefinition"/>
  </cwrc:Language>
  <cwrc:Language rdf:about="#FrenchLanguage">
    <rdfs:label xml:lang="en">French</rdfs:label>
    <rdfs:label xml:lang="fr">Français</rdfs:label>
    <rdf:type rdf:resource="http://www.w3.org/2004/02/skos/core#Concept"/>
    <skos:definition xml:lang="en"/>
    <skos:definition xml:lang="fr"/>
    <rdfs:isDefinedBy rdf:resource="http://sparql.cwrc.ca/ontologies/cwrc-ONTOLOGY_DATE"/>
    <void:inDataset rdf:resource="#datasetdefinition"/>
  </cwrc:Language>
  <owl:Class rdf:ID="GeographicalHeritage">
    <rdfs:label xml:lang="en">Geographical Heritage</rdfs:label>
    <rdfs:label xml:lang="fr">Héritage Géographique</rdfs:label>
    <rdf:type rdf:resource="http://www.w3.org/2004/02/skos/core#Concept"/>
    <rdfs:subClassOf rdf:resource="#CulturalForm"/>
    <skos:definition xml:lang="en">GeographicalHeritage is a subclass of CulturalForm that captures information about the geographical origins of a person's family which often contributes to an understanding of their racial and ethnic background. It offers a way to capture women identified as &quot;South-Asian,&quot; for example, when no more precise national heritage is indicated. See raceAndEthnicity for a detailed description of the complexities of this element.</skos:definition>
    <skos:definition xml:lang="fr">GeographicalHeritage est une sous-classe de CulturalForms qui contient des informations sur les origines géographiques de la famille d'une personne, ce qui contribue souvent à la compréhension de ses origines ethnique et raciale. Cela permet de saisir l’identité de femmes qui se déclarent “sud-asiatiques” par exemple, quand aucune autre précision n'est fournie concernant l'héritage national. Voir raceEthnicityContext pour un compte-rendu détaillé de la complexité de cet élément.</skos:definition>
    <rdfs:isDefinedBy rdf:resource="http://sparql.cwrc.ca/ontologies/cwrc-ONTOLOGY_DATE"/>
    <void:inDataset rdf:resource="#datasetdefinition"/>
  </owl:Class>
  <cwrc:GeographicalHeritage rdf:about="#england">
    <rdfs:label xml:lang="en">England</rdfs:label>
    <rdfs:label xml:lang="fr">Angleterre</rdfs:label>
    <foaf:name xml:lang="en">England (Geographical Heritage)</foaf:name>
    <skos:definition xml:lang="en"/>
    <skos:definition xml:lang="fr"/>
    <skos:broader rdf:resource="#jewishLabel"/>
    <rdfs:isDefinedBy rdf:resource="http://sparql.cwrc.ca/ontologies/cwrc-ONTOLOGY_DATE"/>
    <void:inDataset rdf:resource="#datasetdefinition"/>
  </cwrc:GeographicalHeritage>
  <cwrc:GeographicalHeritage rdf:about="#jewishGeographicalHeritage">
    <rdfs:label xml:lang="en">Jewish</rdfs:label>
    <rdfs:label xml:lang="fr">Juif</rdfs:label>
    <foaf:name xml:lang="en">Jewish (Geographical Heritage)</foaf:name>
    <skos:definition xml:lang="en"/>
    <skos:definition xml:lang="fr"/>
    <skos:broader rdf:resource="#jewishLabel"/>
    <rdfs:isDefinedBy rdf:resource="http://sparql.cwrc.ca/ontologies/cwrc-ONTOLOGY_DATE"/>
    <void:inDataset rdf:resource="#datasetdefinition"/>
  </cwrc:GeographicalHeritage>
  <owl:Class rdf:ID="Gender">
    <rdfs:label xml:lang="en">gender</rdfs:label>
    <rdfs:label xml:lang="fr">genre</rdfs:label>
    <rdf:type rdf:resource="http://www.w3.org/2004/02/skos/core#Concept"/>
    <rdfs:subClassOf rdf:resource="#CulturalForm"/>
    <skos:definition xml:lang="en">A subclass of culturalForms for noting a person's gender whether attributed or self-defined. Although in popular culture gender and biological sex are conflated and understood to be binary, the concept of gender stresses the relationality, constructedness, and performativity of gendered identities and gendered behaviour, whose categories are historically contingent and shifting, and the boundaries between them blurry. Cf. Simone de Beauvoir: &quot;One is not born, but rather becomes, a woman,&quot; along with many other theorists of gender including Judith Butler, 1990. Gender is understood as fluid, situational, and sometimes plural, and it is related to though not commensurate with sexual identity and orientation. It is related to but not defined by specific forms of embodiment. Rather than seeing biological sex as a pre-social or natural given, the body is understood as a site of inscription (cf. Elizabeth Grosz 1994) which is also socially constructed and indeed epigenetically shaped by environmental factors (N. Katherine Hayles 2012). This ontology therefore does not provide separate terms for sex as distinct from gender. Instead, the slashes conjoining terms associated with gender and those conventionally associated with sex indicate the constant slippage between gender and sex in the way that these categories circulate through discourses, actions, and institutions. Far from indicating a universal facet of experience, gender intersects with other identity categories and axes of oppression such as class, race or colour, or geographical heritage to produced quite different interests and experiences among people of the same gender, as with the intersection of religion and white masculine identity in the Muscular Christianity movement in nineteenth-century Britain. Being a woman of colour may thus compound the impacts of gender oppression (Kimberlé Crenshaw 1989).</skos:definition>
    <skos:definition xml:lang="fr">Cette  sous-classe de culturalForms indique le genre d’une personne, qu’il soit attribué par cette dernière ou auto-défini. Même si dans la culture populaire le genre et le sexe biologique sont confondus et binaires, le concept de genre souligne la relativité, la constructivité et la performativité des identités et des comportements genrés, réparties en catégories historiquement contingentes, changeantes et aux frontières floues. Cf Simone de Beauvoir: “On ne naît pas femme, on le devient,” et d’autres nombreuses théoriciennes du genre, dont Judith Butler en 1990. Le genre est entendu comme fluide, situationnel, parfois pluriel, et est relié à, l’identité et l’orientation sexuelles même s’ils ne doivent pas être confondus. Il est relié à des formes spécifiques d’incarnation ou à des comportements physiques, sans pour autant être défini par eux. Plutôt que de voir le sexe biologique comme présocial et attribué par nature,  le corps est compris comme un lieu d’inscriptions (cf Elizabeth Grosz 1994) qui est aussi socialement construit et épigénétiquement modelé par des facteurs environnementaux (N. Katherine Hayles 2012). Cette ontologie ne fournit donc pas de termes séparés pour le genre et le sexe. Les barres obliques qui lient les termes associés aux genres et ceux conventionnellement attribués au sexe indiquent plutôt le glissement constant de ces catégories au fil des discours, des actions et des institutions. Loin d’indiquer une part d’expérience universelle, le genre s’entrecroise avec d’autres catégories d’identité et axes d’oppression comme la classe, la race, la couleur, ou l’héritage géographique pour produire des intérêts et des expériences bien différentes pour les personnes d’un même genre. Un exemple est l’intersection de la religion et de l’identité masculine du mouvement de la Chrétienté Musculaire formé au Royaume-Uni au 19ème siècle. Dans ce contexte, être une femme de couleur devait aggraver les oppressions liées au genre (Kimberlé Crenshaw 1989).</skos:definition>
    <rdfs:isDefinedBy rdf:resource="http://sparql.cwrc.ca/ontologies/cwrc-ONTOLOGY_DATE"/>
    <void:inDataset rdf:resource="#datasetdefinition"/>
  </owl:Class>
  <cwrc:Gender rdf:about="#genderManMale">
    <rdfs:label xml:lang="en">man/male</rdfs:label>
    <rdfs:label xml:lang="fr">homme/mâle</rdfs:label>
    <foaf:name xml:lang="en">man/male (gender)</foaf:name>
    <skos:definition xml:lang="en"/>
    <rdf:type rdf:resource="http://www.w3.org/2004/02/skos/core#Concept"/>
    <rdfs:isDefinedBy rdf:resource="http://sparql.cwrc.ca/ontologies/cwrc-ONTOLOGY_DATE"/>
    <void:inDataset rdf:resource="#datasetdefinition"/>
  </cwrc:Gender>
  <cwrc:Gender rdf:about="#genderWomanFemale">
    <rdfs:label xml:lang="en">Woman/Female</rdfs:label>
    <rdfs:label xml:lang="fr">Femme/Femelle</rdfs:label>
    <foaf:name xml:lang="en">Woman/Female (gender)</foaf:name>
    <skos:definition xml:lang="en"/>
    <rdf:type rdf:resource="http://www.w3.org/2004/02/skos/core#Concept"/>
    <rdfs:isDefinedBy rdf:resource="http://sparql.cwrc.ca/ontologies/cwrc-ONTOLOGY_DATE"/>
    <void:inDataset rdf:resource="#datasetdefinition"/>
  </cwrc:Gender>
  <cwrc:Gender rdf:about="#genderTransMan">
    <rdfs:label xml:lang="en">Transman/Transmale</rdfs:label>
    <rdfs:label xml:lang="fr">Homme Trans</rdfs:label>
    <foaf:name xml:lang="en">Transman/Transmale (gender)</foaf:name>
    <skos:definition xml:lang="en"/>
    <rdf:type rdf:resource="http://www.w3.org/2004/02/skos/core#Concept"/>
    <rdfs:isDefinedBy rdf:resource="http://sparql.cwrc.ca/ontologies/cwrc-ONTOLOGY_DATE"/>
    <void:inDataset rdf:resource="#datasetdefinition"/>
  </cwrc:Gender>
  <cwrc:Gender rdf:about="#genderTransWoman">
    <rdfs:label xml:lang="en">Transwoman/Transfemale</rdfs:label>
    <rdfs:label xml:lang="fr">Femme Trans</rdfs:label>
    <foaf:name xml:lang="en">Transwoman/Transfemale (gender)</foaf:name>
    <skos:definition xml:lang="en"/>
    <rdf:type rdf:resource="http://www.w3.org/2004/02/skos/core#Concept"/>
    <rdfs:isDefinedBy rdf:resource="http://sparql.cwrc.ca/ontologies/cwrc-ONTOLOGY_DATE"/>
    <void:inDataset rdf:resource="#datasetdefinition"/>
  </cwrc:Gender>
  <owl:Class rdf:ID="GenderQueer">
    <rdfs:label xml:lang="en">GenderQueer</rdfs:label>
    <rdfs:label xml:lang="fr">Non-binaire</rdfs:label>
    <skos:note>Listed as non-binary? in french</skos:note>
    <rdf:type rdf:resource="http://www.w3.org/2004/02/skos/core#Concept"/>
    <rdfs:isDefinedBy rdf:resource="http://sparql.cwrc.ca/ontologies/cwrc-ONTOLOGY_DATE"/>
    <void:inDataset rdf:resource="#datasetdefinition"/>
  </owl:Class>
  <owl:Class rdf:ID="Androgynous">
    <rdfs:label xml:lang="en">Androgynous</rdfs:label>
    <rdfs:label xml:lang="fr">Androgyne</rdfs:label>
    <rdf:type rdf:resource="http://www.w3.org/2004/02/skos/core#Concept"/>
    <rdfs:isDefinedBy rdf:resource="http://sparql.cwrc.ca/ontologies/cwrc-ONTOLOGY_DATE"/>
    <void:inDataset rdf:resource="#datasetdefinition"/>
  </owl:Class>
  <owl:Class rdf:ID="Sexuality">
    <rdfs:label xml:lang="en">sexuality</rdfs:label>
    <rdfs:label xml:lang="fr">sexualité</rdfs:label>
    <rdf:type rdf:resource="http://www.w3.org/2004/02/skos/core#Concept"/>
    <rdfs:subClassOf rdf:resource="#CulturalForm"/>
    <skos:definition xml:lang="en">These terms capture in a word or phrase identifications of sexuality (i.e., &quot;lesbian,&quot; &quot;monogamous,&quot; &quot;heterosexual&quot;) not as a means of shutting down but advancing investigation and critical analysis of these identifications. The association assumes that sexual identity does not function in an essentialist manner but can be plural and fluid, so multiple designations can be applied to a single person. Assertions of sexual itentity may come from the subject her/himself or from others. They may be in tension or mutually exclusive, and they may reflect different life stages. Linking to the term &quot;lesbian&quot; as a sexualIdentity class, for instance, does not signify that the subject was in any definitive sense a lesbian; such identifications are often impossible for reasons of historical gaps and silences. As far as living persons are concerned, our practice is to draw only on widely circulated public sources or disclosures from the subject her/himself in order to avoid inadvertently outing someone. See Campbell and Cowan 2016</skos:definition>
    <skos:definition xml:lang="fr">Ces termes identifient en un mot ou en une phrase la sexualité d'un sujet (par exemple “lesbienne”, “monogame”, “hétérosexuel/le”), non pas pour fermer la discussion, mais pour développer l’étude et l’analyse critique de ces catégories. L’association à une sexualité suppose que celle-ci n’est pas vécue de manière essentialiste, mais est plutôt plurielle et fluide; plusieurs désignations peuvent ainsi être appliquées à une seule personne. Le sujet elle/lui-même ou d'autres personnes peuvent émettre des assertions sur son identité sexuelle. Celles-ci peuvent se trouver en tension, se montrer incompatibles, et reflètent le changement du sujet au cours du sa vie. Par exemple, lier le terme “lesbienne” à la classe sexualIdentiy ne signifie pas que le sujet était définitivement lesbienne, car une telle identification est souvent impossible à cause des lacunes et silences historiques. En ce qui concerne les personnes toujours en vie, nous ne nous appuyons que sur des sources ou des déclarations publiques faites par le sujet elle/lui-même afin d’éviter de dévoiler sa sexualité par inadvertance. Voir Campbell et Cowan 2016. 
</skos:definition>
    <owl:sameAs rdf:resource="http://homosaurus.org/terms/sexualIdentity"/>
    <rdfs:isDefinedBy rdf:resource="http://sparql.cwrc.ca/ontologies/cwrc-ONTOLOGY_DATE"/>
    <void:inDataset rdf:resource="#datasetdefinition"/>
  </owl:Class>
  <owl:DeprecatedClass rdf:ID="SexualIdentity">
    <rdfs:label xml:lang="en">Sexual Identity</rdfs:label>
    <rdfs:label xml:lang="fr">Identité Sexuelle</rdfs:label>
    <rdf:type rdf:resource="http://www.w3.org/2004/02/skos/core#Concept"/>
    <rdfs:subClassOf rdf:resource="#CulturalForm"/>
    <rdfs:comment xml:lang="en">Deprecated in favour of #Sexuality term.</rdfs:comment>
    <owl:sameAs rdf:resource="http://homosaurus.org/terms/sexualIdentity"/>
    <rdfs:isDefinedBy rdf:resource="http://sparql.cwrc.ca/ontologies/cwrc-ONTOLOGY_DATE"/>
    <void:inDataset rdf:resource="#datasetdefinition"/>
    <owl:equivalentClass rdf:resource="#Sexuality"/>
    <dc:isReplacedBy rdf:resource="#Sexuality"/>
    <vs:term_status xml:lang="en">deprecated</vs:term_status>
  </owl:DeprecatedClass>
  <!--  (http://ir.lib.uwo.ca/cgi/viewcontent.cgi?article=1085&context=fimspub) -->
  <cwrc:Sexuality rdf:about="#heterosexual">
    <rdfs:label xml:lang="en">Heterosexual</rdfs:label>
    <rdfs:label xml:lang="fr">Hétérosexuelle</rdfs:label>
    <foaf:name xml:lang="en">Heterosexual (Sexual Identity)</foaf:name>
    <skos:definition xml:lang="en"/>
    <skos:definition xml:lang="fr"/>
    <rdf:type rdf:resource="http://www.w3.org/2004/02/skos/core#Concept"/>
    <owl:sameAs rdf:resource="http://homosaurus.org/terms/heterosexualIdentity"/>
    <rdfs:isDefinedBy rdf:resource="http://sparql.cwrc.ca/ontologies/cwrc-ONTOLOGY_DATE"/>
    <void:inDataset rdf:resource="#datasetdefinition"/>
  </cwrc:Sexuality>
  <cwrc:Sexuality rdf:about="#homosexual">
    <rdfs:label xml:lang="en">Homosexual</rdfs:label>
    <rdfs:label xml:lang="fr">Homosexuelle</rdfs:label>
    <foaf:name xml:lang="en">Homosexual (Sexual Identity)</foaf:name>
    <skos:definition xml:lang="en"/>
    <skos:definition xml:lang="fr"/>
    <rdf:type rdf:resource="http://www.w3.org/2004/02/skos/core#Concept"/>
    <rdfs:isDefinedBy rdf:resource="http://sparql.cwrc.ca/ontologies/cwrc-ONTOLOGY_DATE"/>
    <void:inDataset rdf:resource="#datasetdefinition"/>
  </cwrc:Sexuality>
  <cwrc:Sexuality rdf:about="#lesbian">
    <rdfs:label xml:lang="en">Lesbian</rdfs:label>
    <rdfs:label xml:lang="fr">Lesbienne</rdfs:label>
    <foaf:name xml:lang="en">Lesbian (Sexual Identity)</foaf:name>
    <skos:definition xml:lang="en"/>
    <skos:definition xml:lang="fr"/>
    <rdf:type rdf:resource="http://www.w3.org/2004/02/skos/core#Concept"/>
    <owl:sameAs rdf:resource="http://homosaurus.org/terms/lesbianIdentity"/>
    <rdfs:isDefinedBy rdf:resource="http://sparql.cwrc.ca/ontologies/cwrc-ONTOLOGY_DATE"/>
    <void:inDataset rdf:resource="#datasetdefinition"/>
  </cwrc:Sexuality>
  <owl:DeprecatedClass rdf:ID="SexIdentity">
    <rdfs:label xml:lang="en">sex identity</rdfs:label>
    <rdfs:label xml:lang="fr">identité sexe</rdfs:label>
    <rdf:type rdf:resource="http://www.w3.org/2004/02/skos/core#Concept"/>
    <rdfs:subClassOf rdf:resource="#CulturalForm"/>
    <rdfs:comment xml:lang="en">Deprecated in favour of class Gender.</rdfs:comment>
    <rdfs:isDefinedBy rdf:resource="http://sparql.cwrc.ca/ontologies/cwrc-ONTOLOGY_DATE"/>
    <void:inDataset rdf:resource="#datasetdefinition"/>
    <owl:equivalentClass rdf:resource="#Gender"/>
    <dc:isReplacedBy rdf:resource="#Gender"/>
    <vs:term_status xml:lang="en">deprecated</vs:term_status>
  </owl:DeprecatedClass>
  <rdf:Description rdf:about="#maleSex">
    <rdfs:label xml:lang="en">Male</rdfs:label>
    <rdfs:label xml:lang="fr">Mâle</rdfs:label>
    <foaf:name xml:lang="en">Male (Sex)</foaf:name>
    <skos:definition xml:lang="en"/>
    <skos:definition xml:lang="fr"/>
    <rdf:type rdf:resource="http://www.w3.org/2004/02/skos/core#Concept"/>
    <rdfs:isDefinedBy rdf:resource="http://sparql.cwrc.ca/ontologies/cwrc-ONTOLOGY_DATE"/>
    <void:inDataset rdf:resource="#datasetdefinition"/>
    <rdfs:comment xml:lang="en">Deprecated in favour of instance #genderManMale.</rdfs:comment>
    <owl:deprecated rdf:datatype="http://www.w3.org/2001/XMLSchema#boolean">true</owl:deprecated>
    <owl:equivalentClass rdf:resource="#genderManMale"/>
    <dc:isReplacedBy rdf:resource="#genderManMale"/>
    <vs:term_status xml:lang="en">deprecated</vs:term_status>
  </rdf:Description>
  <rdf:Description rdf:about="#femaleSex">
    <rdfs:label xml:lang="en">Female</rdfs:label>
    <rdfs:label xml:lang="fr">Femelle</rdfs:label>
    <foaf:name xml:lang="en">Female (Sex)</foaf:name>
    <skos:definition xml:lang="en"/>
    <skos:definition xml:lang="fr"/>
    <rdf:type rdf:resource="http://www.w3.org/2004/02/skos/core#Concept"/>
    <rdfs:isDefinedBy rdf:resource="http://sparql.cwrc.ca/ontologies/cwrc-ONTOLOGY_DATE"/>
    <void:inDataset rdf:resource="#datasetdefinition"/>
    <rdfs:comment xml:lang="en">Deprecated in favour of instance #genderWomanFemale.</rdfs:comment>
    <owl:deprecated rdf:datatype="http://www.w3.org/2001/XMLSchema#boolean">true</owl:deprecated>
    <owl:equivalentClass rdf:resource="#genderWomanFemale"/>
    <dc:isReplacedBy rdf:resource="#genderWomanFemale"/>
    <vs:term_status xml:lang="en">deprecated</vs:term_status>
  </rdf:Description>
  <rdf:Description rdf:about="#unknownSex">
    <rdfs:label xml:lang="en">Unknown</rdfs:label>
    <rdfs:label xml:lang="fr">Inconnue</rdfs:label>
    <foaf:name xml:lang="en">Unknown (Sex)</foaf:name>
    <skos:definition xml:lang="en"/>
    <skos:definition xml:lang="fr"/>
    <rdf:type rdf:resource="http://www.w3.org/2004/02/skos/core#Concept"/>
    <rdfs:isDefinedBy rdf:resource="http://sparql.cwrc.ca/ontologies/cwrc-ONTOLOGY_DATE"/>
    <void:inDataset rdf:resource="#datasetdefinition"/>
    <rdfs:comment xml:lang="en">Deprecated with no current equivalence.</rdfs:comment>
    <owl:deprecated rdf:datatype="http://www.w3.org/2001/XMLSchema#boolean">true</owl:deprecated>
    <vs:term_status xml:lang="en">deprecated</vs:term_status>
  </rdf:Description>
  <owl:Class rdf:ID="RaceColour">
    <rdfs:label xml:lang="en">race and/or colour</rdfs:label>
    <rdfs:label xml:lang="fr">race et/ou couleur de peau</rdfs:label>
    <rdf:type rdf:resource="http://www.w3.org/2004/02/skos/core#Concept"/>
    <rdfs:subClassOf rdf:resource="#CulturalForm"/>
    <skos:definition xml:lang="en"/>
    <skos:definition xml:lang="fr"/>
    <rdfs:isDefinedBy rdf:resource="http://sparql.cwrc.ca/ontologies/cwrc-ONTOLOGY_DATE"/>
    <void:inDataset rdf:resource="#datasetdefinition"/>
  </owl:Class>
  <owl:DeprecatedClass rdf:about="#whiteRace">
    <rdfs:label xml:lang="en">white</rdfs:label>
    <rdfs:label xml:lang="fr">blanc</rdfs:label>
    <foaf:name xml:lang="en">White (Race Colour)</foaf:name>
    <skos:definition xml:lang="en"/>
    <skos:definition xml:lang="fr"/>
    <rdf:type rdf:resource="http://www.w3.org/2004/02/skos/core#Concept"/>
    <rdfs:subClassOf rdf:resource="#whiteLabel"/>
    <rdfs:isDefinedBy rdf:resource="http://sparql.cwrc.ca/ontologies/cwrc-ONTOLOGY_DATE"/>
    <void:inDataset rdf:resource="#datasetdefinition"/>
    <owl:equivalentClass rdf:resource="#whiteRaceColour"/>
    <dc:isReplacedBy rdf:resource="#whiteRaceColour"/>
    <vs:term_status xml:lang="en">deprecated</vs:term_status>
  </owl:DeprecatedClass>
  <cwrc:RaceColour rdf:about="#whiteRaceColour">
    <rdfs:label xml:lang="en">white</rdfs:label>
    <rdfs:label xml:lang="fr">blanc</rdfs:label>
    <foaf:name xml:lang="en">White (Race Colour)</foaf:name>
    <skos:definition xml:lang="en"/>
    <skos:definition xml:lang="fr"/>
    <rdf:type rdf:resource="http://www.w3.org/2004/02/skos/core#Concept"/>
    <rdfs:subClassOf rdf:resource="#whiteLabel"/>
    <rdfs:isDefinedBy rdf:resource="http://sparql.cwrc.ca/ontologies/cwrc-ONTOLOGY_DATE"/>
    <void:inDataset rdf:resource="#datasetdefinition"/>
  </cwrc:RaceColour>
  <cwrc:RaceColour rdf:about="#eurasianRace">
    <rdfs:label xml:lang="en">eurasian</rdfs:label>
    <rdfs:label xml:lang="fr">eurasien</rdfs:label>
    <foaf:name xml:lang="en">Eurasian (Race Colour)</foaf:name>
    <skos:definition xml:lang="en"/>
    <skos:definition xml:lang="fr"/>
    <rdf:type rdf:resource="http://www.w3.org/2004/02/skos/core#Concept"/>
    <rdfs:isDefinedBy rdf:resource="http://sparql.cwrc.ca/ontologies/cwrc-ONTOLOGY_DATE"/>
    <void:inDataset rdf:resource="#datasetdefinition"/>
  </cwrc:RaceColour>
  <owl:Class rdf:ID="RaceEthnicity">
    <rdfs:label xml:lang="en">race and/or ethnicity</rdfs:label>
    <rdfs:label xml:lang="fr">race et/ou ethnicité</rdfs:label>
    <rdf:type rdf:resource="http://www.w3.org/2004/02/skos/core#Concept"/>
    <rdfs:subClassOf rdf:resource="#CulturalForm"/>
    <skos:definition xml:lang="en"/>
    <skos:definition xml:lang="fr"/>
    <rdfs:isDefinedBy rdf:resource="http://sparql.cwrc.ca/ontologies/cwrc-ONTOLOGY_DATE"/>
    <void:inDataset rdf:resource="#datasetdefinition"/>
  </owl:Class>
  <owl:Class rdf:ID="Ethnicity">
    <rdfs:label xml:lang="en">ethnicity</rdfs:label>
    <rdfs:label xml:lang="fr">ethnicité</rdfs:label>
    <rdf:type rdf:resource="http://www.w3.org/2004/02/skos/core#Concept"/>
    <rdfs:subClassOf rdf:resource="#CulturalForm"/>
    <skos:definition xml:lang="en">Ethnicity is a subclass of CulturalForm that captures information about a person's ethnic position. Ethnicity is a sub-element within culturalFormation and raceAndEthnicity. See raceAndEthnicity for a detailed description of the complexities of this discursive construction and the social practices surrounding it.</skos:definition>
    <skos:definition xml:lang="fr"/>
    <rdfs:isDefinedBy rdf:resource="http://sparql.cwrc.ca/ontologies/cwrc-ONTOLOGY_DATE"/>
    <void:inDataset rdf:resource="#datasetdefinition"/>
  </owl:Class>
  <cwrc:Ethnicity rdf:about="#whiteEthnicity">
    <rdfs:label xml:lang="en">white</rdfs:label>
    <rdfs:label xml:lang="fr">blanc</rdfs:label>
    <foaf:name xml:lang="en">White (Ethnicity)</foaf:name>
    <skos:definition xml:lang="en"/>
    <skos:definition xml:lang="fr"/>
    <rdfs:subClassOf rdf:resource="#whiteLabel"/>
    <rdfs:isDefinedBy rdf:resource="http://sparql.cwrc.ca/ontologies/cwrc-ONTOLOGY_DATE"/>
    <void:inDataset rdf:resource="#datasetdefinition"/>
  </cwrc:Ethnicity>
  <owl:DeprecatedClass rdf:about="#JewishEthnicity">
    <rdfs:label xml:lang="en">Jewish</rdfs:label>
    <rdfs:label xml:lang="fr">Juif</rdfs:label>
    <foaf:name xml:lang="en">Jewish (Ethnicity)</foaf:name>
    <skos:definition xml:lang="en"/>
    <skos:definition xml:lang="fr"/>
    <skos:broader rdf:resource="#jewishLabel"/>
    <rdfs:isDefinedBy rdf:resource="http://sparql.cwrc.ca/ontologies/cwrc-ONTOLOGY_DATE"/>
    <void:inDataset rdf:resource="#datasetdefinition"/>
    <owl:equivalentClass rdf:resource="#jewishEthnicity"/>
    <dc:isReplacedBy rdf:resource="#jewishEthnicity"/>
    <vs:term_status xml:lang="en">deprecated</vs:term_status>
  </owl:DeprecatedClass>
  <cwrc:Ethnicity rdf:about="#jewishEthnicity">
    <rdfs:label xml:lang="en">Jewish</rdfs:label>
    <rdfs:label xml:lang="fr">Juif</rdfs:label>
    <foaf:name xml:lang="en">Jewish (Ethnicity)</foaf:name>
    <skos:definition xml:lang="en"/>
    <skos:definition xml:lang="fr"/>
    <skos:broader rdf:resource="#jewishLabel"/>
    <rdfs:isDefinedBy rdf:resource="http://sparql.cwrc.ca/ontologies/cwrc-ONTOLOGY_DATE"/>
    <void:inDataset rdf:resource="#datasetdefinition"/>
    <rdfs:subClassOf rdf:resource="#jewishLabel"/>
    <rdfs:isDefinedBy rdf:resource="http://sparql.cwrc.ca/ontologies/cwrc-ONTOLOGY_DATE"/>
    <void:inDataset rdf:resource="#datasetdefinition"/>
  </cwrc:Ethnicity>
  <!-- Religion -->
  <owl:Class rdf:ID="Religion">
    <rdfs:label xml:lang="en">Religion</rdfs:label>
    <rdfs:label xml:lang="fr">Religion</rdfs:label>
    <rdf:type rdf:resource="http://www.w3.org/2004/02/skos/core#ConceptScheme"/>
    <rdfs:subClassOf rdf:resource="#CulturalForm"/>
    <skos:definition xml:lang="en">A subclass of CulturalForm, this describes a person's religion(s) or belief system(s). Note that while atheism denotes the absence of religion, we use the Religion label for convinience.</skos:definition>
    <skos:definition xml:lang="fr"/>
    <rdfs:isDefinedBy rdf:resource="http://sparql.cwrc.ca/ontologies/cwrc-ONTOLOGY_DATE"/>
    <void:inDataset rdf:resource="#datasetdefinition"/>
    <rdf:type rdf:resource="http://www.w3.org/2004/02/skos/core#ConceptScheme"/>
  </owl:Class>
  <cwrc:Religion rdf:about="#anglicanChurch">
    <rdfs:label xml:lang="en">Church of England</rdfs:label>
    <rdfs:label xml:lang="zh-hant">英國聖公會 (英國國教)</rdfs:label>
    <rdfs:label xml:lang="zh-latn-pinyin-x-hanyu">yīng guó shèng gōng huì</rdfs:label>
    <rdfs:label xml:lang="zh-latn-pinyin-x-notone">ying guo sheng gong hui</rdfs:label>
    <rdfs:label xml:lang="zh-latn-wadegile">ying kuo sheng kung hui</rdfs:label>
    <rdfs:label xml:lang="nl">Anglicaans (kerk van Engeland)</rdfs:label>
    <rdfs:label xml:lang="es">Anglicanismo</rdfs:label>
    <rdfs:label xml:lang="es">Iglesia de Inglaterra</rdfs:label>
    <rdfs:label xml:lang="fr">Église d'Angleterre</rdfs:label>
    <skos:definition xml:lang="en">A Christian denomination having both Protestant and Catholic aspects that originated with Henry VIII's break with the Roman Catholic Church (ca. 1532-34). As the official state Church of England, the monarch of England is still formally considered its head. While at first it remained mainly Catholic in character, reforms came under Edward IV and Elizabeth I who introduced doctrine that was more Protestant in nature, namely new editions of the Book of Common Prayer and the Thirty-nine Articles. Although an overall attitude of toleration exists in the modern Anglican Church, tension remains between its Protestant and Catholic inclinations as well as with newer liberal and evangelical influences. Anglicanism is based on episcopal authority and parish structure is fundamental to the organization of the church. The term is used with regard to the Church of England; with regard to the Episcopal Church in America, use &quot;Episcopal.&quot; <![CDATA[<a href="#_getty_2017">(Getty, 2017)</a>]]></skos:definition>
    <skos:definition xml:lang="nl">Te gebruiken om te verwijzen naar de anglicaanse kerk (Church of England); gebruik 'episcopaal' om te verwijzen naar de episcopale kerk in Amerika. De term verwijst naar een christelijke geloofsrichting met zowel protestantse als katholieke elementen die ontstond na de breuk tussen de Engelse koning Hendrik VIII en de rooms-katholieke kerk (circa 1532-34). Het anglicanisme is de officiële Britse staatsgodsdienst, en de Britse soevereine vorst is nog altijd het officiële hoofd van de anglicaanse kerk. Aanvankelijk droeg de kerk nog een overwegend katholiek karakter, maar onder Edward IV en Elizabeth I werden er hervormingen doorgevoerd en werd een meer protestants georiënteerde geloofsleer geïntroduceerd, met een nieuwe versie van het Book of Common Prayer en de Negenendertig Artikelen. Hoewel de huidige anglicaanse kerk in het algemeen wordt gekenmerkt door een tolerante houding, zijn de spanningen tussen protestants en katholiek gezinde stromingen binnen de kerk nooit verdwenen en heerst er weerstand tegen nieuwe vrijzinnige en evangelische invloeden. Het anglicanisme berust op episcopaal gezag en op een structuur van parochies, welke van fundamenteel belang is voor de kerkelijke organisatie. <![CDATA[<a href="#_getty_2017">(Getty, 2017)</a>]]></skos:definition>
    <skos:definition xml:lang="es">Úsese con referencia a la Iglesia de Inglaterra y también con referencia a la Iglesia Episcopal de Estados Unidos (úsese Iglesia Episcopal). Este término s erefiere a a una denominación cristiana que contiene elementos católicos y protestantes en varios aspectos y que se originó con el rey Enrique VIII quien rompió con la Iglesia Católica Romana (ca. 1532-1534) Es la iglesia oficial de Inglaterra, la Monarquía Inglesa es aún formalmente considerada su cabeza.Mientras en sus comienzos conservaba su carácter católico, con las reformas realizadas bajo Eduardo IV e Isabel I quienes introdujeron una doctrina que está más cerca del protestantismo y que se encuentra contenida en nuevas ediciones del Libro de Oraciones Comunes y en los Treinta y nueve Artículos. Aunque el anglicanismo  tiene actualmente una actitud de total tolerancia, aún persisten tensiones con las iglesias protestantes y católicas así como de últimas influencias liberales y evangélicas.El Anglicanismo está basado en la autoridad episcopal y se sustenta en una estructura de parroquias que resulta fundamental para la organización de la Iglesia. <![CDATA[<a href="#_getty_2017">(Getty, 2017)</a>]]></skos:definition>
    <skos:definition xml:lang="zh-hant">英王亨利八世與羅馬天主教教會(西元1532-34年)分裂所創的基督教派別，同時含有新教與天主教元素。作為官方英國國教，其正式教會首腦仍為英國國王。起初較具天主教特色，在愛德華四世與伊莉莎白一世時改革，加入較具新教本質的教條，即：新版的公禱書(Book of Common Prayer)及三十九條信綱(Thirty-nine Articles)。雖然現代的英國聖公會大體上態度已越顯寬容，但教會內的新教派系與天主教派系關係仍緊繃，也仍不樂於接受較新的自由與福音派影響。英國聖公會奠基於主教的權威上，牧師教區的結構對教會組織十分重要。此詞彙用於指稱英國國教；美國區的主教派教會，則稱為「美國聖公會(Episcopal)」。 <![CDATA[<a href="#_getty_2017">(Getty, 2017)</a>]]></skos:definition>
    <prov:derivedFrom rdf:resource="http://vocab.getty.edu/aat/300153822"/>
    <rdfs:comment xml:lang="en">The description for this term is indebted to the Getty Art &amp; Architecture Thesaurus.</rdfs:comment>
    <skos:definition xml:lang="fr">L'anglicanisme est une confession chrétienne présente principalement dans les pays qui ont pu être imprégnés par la culture anglaise incluant notamment, outre l'Angleterre, les anciennes colonies britanniques en Amérique et en Afrique. On retrouve tout de même plusieurs communauté anglicanes dans le monde, notamment en France. L'origine de cette confession remonte à la période antique de l'Église d'Angleterre, lorsque celle-ci était unie canoniquement et juridiquement à l'évêque de Rome. Puis, au XVIe siècle, lorsque le roi d'Angleterre Henri VIII rompit avec le pape de Rome pour causes politiques et théologiques. Ainsi, Henri VIII ne créa rien de nouveau : il extirpa l'autorité du pape de son royaume, sans pour autant modifier ou jeter de nouvelles bases théologiques pour l'Église, et remplaça l'autorité papale par la sienne propre. Depuis la reine Elizabeth Ire, le monarque a le titre de « gouverneur suprême », mais n'a qu'un rôle de maintien de l'ordre et du bon déroulement de la vie ecclésiale, mais aucune réelle autorité décisionnelle comme celle d'un évêque ou d'un synode. L'Archevêque de Canterbury porte le titre de « primat de toute l'Angleterre » et l'archevêque d'York porte quant à lui le titre de « primat de l'Angleterre ». L'Église anglicane, tout comme l'Église orthodoxe, est une communion d'églises autocéphales, mais néanmoins interdépendantes. Bien que plusieurs églises anglicanes existent à travers le monde, comme c'est le cas pour l'Église catholique romaine (présente en France, en Espagne, etc.), ou encore pour l'Église orthodoxe (présente en Russie, en Serbie, etc.), il ne s'agit que d'une seule Église. Elles sont rassemblées dans la Communion anglicane , au sein de laquelle l'Église d'Angleterre et son primat, l'archevêque de Canterbury, ne jouissent que d'une primauté d'honneur. Ces églises sont en pleine communion (doctrinale, spirituelle, épiscopale, sacramentelle) les unes avec les autres et représentent ensemble environ 85 millions de fidèles. Les Églises de la Communion anglicane ont une structure épiscopale. Elles se disent à la fois catholiques et réformées, et l'anglicanisme a souvent été présenté comme une via media entre le catholicisme romain et le protestantisme. Elles se présentent comme des Églises catholiques non romaines, parce qu'elles se veulent en continuité avec la tradition apostolique (ainsi la patristique est très développée dans le monde anglican) et affirment avoir conservé la succession apostolique. L'Église orthodoxe du patriarcat œcuménique de Constantinople a reconnu la validité de la succession apostolique en 1922 ; cependant, d'autres patriarcats, comme celui de Russie, ne saurait reconnaître une quelconque succession apostolique, en autre par le fait de l'ordination épiscopale de femme, depuis janvier 2015. L'Église catholique romaine ne leur reconnait pas cette qualité : ainsi par la lettre apostolique Apostolicae Curae le pape Léon XIII déclare en 1896 « nulles et sans valeur » les ordinations anglicanes (doctrine confirmée par le motu proprio Ad Tuendam Fidem en 1998). Les archevêques anglicans de Canterbury et d'York ont donné leur réponse dans Saepius officio. Pour autant, lors du concile Vatican II est affirmée la « place particulière » des Anglicans, « qui gardent en partie les traditions et les structures catholiques ». Par ailleurs, les Églises anglicanes se disent réformées parce qu'elles ont adhéré à certains principes nouveaux issus de la Réforme protestante en matière de doctrine et de liturgie.À l'origine, la doctrine anglicane est énoncée dans les Trente-neuf articles (Bill of XXXIX articles) qui ont longtemps eu une valeur impérative. L'éventail entre les positions doctrinales s'est ensuite élargi et donne lieu à de nombreuses classifications (Haute Église, Basse Église, Broad Church (en), Anglo-catholicisme, Évangélisme…). Alors que pendant longtemps la coexistence apaisée entre de telles positions divergentes était considérée comme une spécificité de l'anglicanisme, la communion est depuis la fin du XXe siècle soumise à de forts tiraillements sur certaines questions, notamment l'ordination des femmes et la position par rapport à l'homosexualité. <![CDATA[<a href="#_dbpedia_2017">(DBpedia, 2017)</a>]]></skos:definition>
    <prov:derivedFrom rdf:resource="http://dbpedia.org/page/Anglicanism"/>
    <rdfs:comment xml:lang="fr">La description de ce terme est basée sur celle de DBPedia.</rdfs:comment>
    <rdf:type rdf:resource="http://www.w3.org/2004/02/skos/core#Concept"/>
    <rdf:type rdf:resource="http://xmlns.com/foaf/0.1/Organization"/>
    <skos:inScheme rdf:resource="#Religion"/>
    <skos:broaderTransitive rdf:resource="#christianity"/>
    <rdfs:isDefinedBy rdf:resource="http://sparql.cwrc.ca/ontologies/cwrc-ONTOLOGY_DATE"/>
    <void:inDataset rdf:resource="#datasetdefinition"/>
  </cwrc:Religion>
  <cwrc:Religion rdf:about="#baptistChurch">
    <rdfs:label xml:lang="en">Baptist</rdfs:label>
    <rdfs:label xml:lang="zh-hant">浸禮宗</rdfs:label>
    <rdfs:label xml:lang="zh-hant">浸禮派</rdfs:label>
    <rdfs:label xml:lang="zh-hant">浸信會</rdfs:label>
    <rdfs:label xml:lang="zh-latn-pinyin-x-hanyu">jìn lǐ zōng</rdfs:label>
    <rdfs:label xml:lang="zh-latn-pinyin-x-notone">jin li zong</rdfs:label>
    <rdfs:label xml:lang="zh-latn-wadegile">chin li tsung</rdfs:label>
    <rdfs:label xml:lang="nl">Baptisme</rdfs:label>
    <rdfs:label xml:lang="es">Baptismo</rdfs:label>
    <rdfs:label xml:lang="es">Baptistas</rdfs:label>
    <rdfs:label xml:lang="fr">Baptisme</rdfs:label>
    <skos:definition xml:lang="en">Refers to a Protestant denomination centered around the belief that the sacrament of baptism should only be administered to adult members after a personal profession of belief in Jesus Christ. Baptism in this faith is usually done by full immersion. Emphasis is placed on biblical scripture and preaching. The Baptist denomination is primarily derived from early 17th-century England and Wales where it quickly spread although there are some links with the Anabaptists of the 16th century. Baptist churches very rapidly increased in the late 19th century in the United States. <![CDATA[<a href="#_getty_2017">(Getty, 2017)</a>]]></skos:definition>
    <skos:definition xml:lang="nl">Verwijst naar een protestantse gezindte waarbij het geloof centraal staat dat het sacrament van de doop alleen moet worden toegediend aan volwassen leden na een persoonlijke belijdenis van geloof in Jezus Christus. De doop vindt bij deze gezindte doorgaans plaats door volledige onderdompeling. De nadruk ligt op Bijbelse geschriften en preken. Het baptisme is in hoofdzaak ontstaan in de vroege 17de eeuw in Engeland en Wales waar het zich snel verspreidde, hoewel er enige verbanden zijn met de anabaptisten van de 16de eeuw. In de late 19de eeuw nam het aantal baptistische kerken in de Verenigde Staten snel toe. <![CDATA[<a href="#_getty_2017">(Getty, 2017)</a>]]></skos:definition>
    <skos:definition xml:lang="es">Se refiere a la religión protestante centrada en torno a la creencia que el sacramento del bautismo debería ser administrado sólo a miembros adultos tras una manifestación personal de creencia en Jesucristo. El bautismo en esta fe es usualmente hecho por inmersión total. El énfasis es puesto en las Escrituras Bíblicas y la oración. La denominación baptista deriva principalmente de la Inglaterra y Gales del siglo XVII en donde rápidamente se difundió a pesar que hay algunas conexiones con los Anabaptistas del siglo XVI. La iglesia baptista creció rápidamente en el siglo XIX en los Estados Unidos. <![CDATA[<a href="#_getty_2017">(Getty, 2017)</a>]]></skos:definition>
    <skos:definition xml:lang="zh-hant">一支新教派別，相信只有親自聲明信仰基督的成人才可受洗。此教的洗禮通常需全身浸洗。重視聖經經文與佈道。浸信會與十六世紀的重浸派有些淵源，但主要源於十七世紀初的英格蘭與威爾斯，在這兩處快速廣傳。其教會於十九世紀末在美國急速增加。 <![CDATA[<a href="#_getty_2017">(Getty, 2017)</a>]]></skos:definition>
    <prov:derivedFrom rdf:resource="http://vocab.getty.edu/aat/300153825"/>
    <rdfs:comment xml:lang="en">The description for this term is indebted to the Getty Art &amp; Architecture Thesaurus.</rdfs:comment>
    <skos:definition xml:lang="fr">Le baptisme est un courant chrétien évangélique issu d'un réveil démarré par les pasteurs anglais John Smyth en Hollande en 1609, puis Thomas Helwys en Angleterre en 1612. Ce mouvement se caractérise par l'importance donnée à la Bible, à la nouvelle naissance, au baptême adulte en tant que témoignage volontaire, un esprit missionnaire, un engagement moral de vie ainsi que par l’autonomie locale des églises, la séparation de l’Église et de l’État, et finalement l’autorité de la congrégation (congrégationalisme). Selon les chiffres du Pew Research Center, en 2011, le mouvement recense 72 millions de croyants. <![CDATA[<a href="#_dbpedia_2017">(DBpedia, 2017)</a>]]></skos:definition>
    <prov:derivedFrom rdf:resource="http://dbpedia.org/page/Baptists"/>
    <rdfs:comment xml:lang="fr">La description de ce terme est basée sur celle de DBPedia.</rdfs:comment>
    <rdf:type rdf:resource="http://www.w3.org/2004/02/skos/core#Concept"/>
    <skos:inScheme rdf:resource="#Religion"/>
    <skos:broaderTransitive rdf:resource="#christianity"/>
    <rdfs:isDefinedBy rdf:resource="http://sparql.cwrc.ca/ontologies/cwrc-ONTOLOGY_DATE"/>
    <void:inDataset rdf:resource="#datasetdefinition"/>
  </cwrc:Religion>
  <cwrc:Religion rdf:about="#buddhism">
    <rdfs:label xml:lang="en">Buddhism</rdfs:label>
    <rdfs:label xml:lang="nl">Boeddhisme</rdfs:label>
    <rdfs:label xml:lang="es">Budismo</rdfs:label>
    <skos:altLabel xml:lang="en">Buddhist</skos:altLabel>
    <rdfs:label xml:lang="zh-hant">佛教</rdfs:label>
    <rdfs:label xml:lang="zh-latn-pinyin-x-hanyu">fó jiào</rdfs:label>
    <rdfs:label xml:lang="zh-latn-pinyin-x-notone">fo jiao</rdfs:label>
    <rdfs:label xml:lang="zh-latn-wadegile">fo chiao</rdfs:label>
    <rdfs:label xml:lang="fr">Bouddhisme</rdfs:label>
    <skos:definition xml:lang="en">Refers to the philosophy and religion based on the enlightenment and teachings of the Buddha Gautama in the early sixth century BCE in the northeastern region of modern India. Playing dominant roles in the art and culture of Southeast Asia and East Asia, this religion is based on the transcendence of human suffering and pain through the acceptance of the limitations of individuality, the surrender of worldly desires and cravings that cause disappointment and sorrow, and the deliverance from the impermanence of living and individual ego based on wealth, social position, or family through the process of enlightenment (nirvana). The religion also centers around 'anatman', or no-self, the idea that the self is in a state of action or a series of changing manifestations rather than in a state of fixed, metaphysical substance. The structure of the religion is based on the Triratna (&quot;Three Jewels&quot; of Buddha), a tripartite schematic for living based on three elements: Buddha (the teacher), dharma (the teaching), and sangha (community). <![CDATA[<a href="#_getty_2017">(Getty, 2017)</a>]]></skos:definition>
    <skos:definition xml:lang="es">Se refiere a la filosofía y religión basada en la iluminación y enseñanza del Buddha Gautama en el siglo VI a.C temprano en la región nordeste de la India Moderna. Jugando un rol dominante en el arte y la cultura del Asia Sudeste y Asia Oriental, esta religión está basada en la trascendencia del sufrimiento y dolor humano a través de la aceptación de las limitaciones de individualidad, la rendición de deseos mundanos y anhelos que causan desilusión y aflicción y la liberación desde la transitoriedad of living and individual ego based on wealth, social position, or family through the process of enlightenment (nirvana). The religion also centers around anatman, or no-self, the idea that the self is in a state of action or a series of changing manifestations rather than in a state of fixed, metaphysical substance. The structure of the religion is based on the Triratna (&quot;Three Jewels&quot; of Buddha), a tripartite schematic for living based on three elements: Buddha (the teacher), dharma (the teaching), and sangha (community). <![CDATA[<a href="#_getty_2017">(Getty, 2017)</a>]]></skos:definition>
    <skos:definition xml:lang="nl">Verwijst naar de filosofie en religie die zijn gebaseerd op de verlichting en leer van Boeddha Gautama in de vroege 6de eeuw v. Chr. in het Noord-Oosten van het moderne India. Deze religie, die een dominante rol speelt in de kunst en cultuur van Zuidoost-Azië en Oost-Azië, is gebaseerd op het overstijgen van menselijk lijden en pijn door het accepteren van de grenzen van de individualiteit, het opgeven van wereldse verlangens en wensen die voor teleurstellingen en verdriet zorgen en het loslaten van het niet-permanente van het leven en het afzonderlijke ego met de bijbehorende welvaart, sociale positie of familierelaties, allemaal door het proces van de verlichting (nirvana). Bij deze religie staat ook 'anatman' centraal, het idee dat 'het zelf' altijd in ontwikkeling is of deel uitmaakt van een reeks veranderende verschijningsvormen in plaats van een vaste, metafysische substantie. De structuur van de religie is gebaseerd op de Triratna ('drie juwelen' van boeddha), een drieledige structuur voor het leven gebaseerd op drie elementen: boeddha (de leraar), dharma (de leer) en sangha (de gemeenschap). <![CDATA[<a href="#_getty_2017">(Getty, 2017)</a>]]></skos:definition>
    <skos:definition xml:lang="zh-hant">根據釋迦牟尼佛之開悟與教誨的哲學和宗教，在西元前六世紀初起源於現今印度東北部。佛教於東南亞及東亞的藝術與文化層面扮演主要角色，相信透過接受自身的局限，以及放棄會引起失望與悲傷的世俗欲求及渴望，能夠使人類的苦痛得以昇華，而在開悟（涅盤）過程中得以從短暫的生命以及建築在財富、社會地位與家庭上的個人自尊中獲得解脫。此宗教的中心思想為「無我」，認為自我是處於活動狀態或是一連串的形式改變，而非固定的形上實體狀態。佛教的架構奠基於「三寶」，即生命三元素：佛(老師)、法(規範)、僧(眾)。 <![CDATA[<a href="#_getty_2017">(Getty, 2017)</a>]]></skos:definition>
    <prov:derivedFrom rdf:resource="http://vocab.getty.edu/aat/300073738"/>
    <rdfs:comment xml:lang="en">The description for this term is indebted to the Getty Art &amp; Architecture Thesaurus.</rdfs:comment>
    <skos:definition xml:lang="fr">Le bouddhisme est, selon les points de vue en Occident, une religion (notamment une religion d'État) ou une philosophie, voire les deux, dont les origines remontent en Inde au Ve siècleav. J.-C. à la suite de l'éveil de Siddhartha Gautama et de son enseignement. Le bouddhisme comptait en 2005 entre 230 millions et 500 millions d'adeptes, ce qui en fait la quatrième religion mondiale, derrière (dans l'ordre décroissant) le christianisme, l'islam, et l'hindouisme. Le bouddhisme présente un ensemble ramifié de pratiques méditatives, de pratiques éthiques, de théories psychologiques, philosophiques, cosmogoniques et cosmologiques, abordées dans la perspective de la bodhi, « l'éveil ». À l'instar du jaïnisme, le bouddhisme est à l'origine une tradition shramana, et non brahmanique comme l'est l'hindouisme. Les notions de dieu et de divinité dans le bouddhisme sont particulières : bien que le bouddhisme soit souvent perçu comme une religion sans dieu créateur, la notion étant absente de la plupart des formes du bouddhisme, la vénération et le culte du Bouddha historique Siddhartha Gautama en tant que bhagavat joue un rôle important dans le Theravāda et également dans le Mahāyāna, dans lesquels il est un être éveillé ayant trois aspects ou manifestations (trikāya). <![CDATA[<a href="#_dbpedia_2017">(DBpedia, 2017)</a>]]></skos:definition>
    <prov:derivedFrom rdf:resource="http://dbpedia.org/page/Buddhism"/>
    <rdfs:comment xml:lang="fr">La description de ce terme est basée sur celle de DBPedia.</rdfs:comment>
    <rdf:type rdf:resource="http://www.w3.org/2004/02/skos/core#Concept"/>
    <skos:inScheme rdf:resource="#Religion"/>
    <rdfs:isDefinedBy rdf:resource="http://sparql.cwrc.ca/ontologies/cwrc-ONTOLOGY_DATE"/>
    <void:inDataset rdf:resource="#datasetdefinition"/>
    <skos:broaderTransitive rdf:resource="#occultism"/>
  </cwrc:Religion>
  <cwrc:Religion rdf:about="#catholicChurch">
    <rdfs:label xml:lang="en">Roman Catholic</rdfs:label>
    <rdfs:label xml:lang="nl">Rooms-Katholicisme</rdfs:label>
    <rdfs:label xml:lang="nl">Katholiek</rdfs:label>
    <rdfs:label xml:lang="nl">Katholicisme</rdfs:label>
    <rdfs:label xml:lang="es">Catolicismo Romano</rdfs:label>
    <rdfs:label xml:lang="es">Catolicismo</rdfs:label>
    <rdfs:label xml:lang="fr">Catholicisme</rdfs:label>
    <skos:definition xml:lang="en">Refers to the branch of Christianity characterized by a uniform, highly developed ritual canon and organizational structure with doctrinal roots based in the teachings of the Apostles of Jesus Christ in the first century, in the Alexandrian school of theology, and in Augustinian thought. In this religious branch, faith is considered an acceptance of revelation; revelation appears as doctrine. In juridical terms, it refers to the branch of Christianity distinguished as a unified, monolithic sacramental system under the governance of papal authority. Throughout much of its history, the seat of the Pope has been in Rome, thus &quot;Roman Catholicism&quot; is often used to distinguish this concept from the Orthodox Catholic church. <![CDATA[<a href="#_getty_2017">(Getty, 2017)</a>]]></skos:definition>
    <skos:definition xml:lang="es">Se refiere a la rama del cristianismo caracterizada por un canon ritual uniforme y altamente desarrollado y una estructura organizacional con raíces doctrinales basadas en las enseñanzas de los Apostoles de Jesucristo en la primera centuria, en la Escuela Alejandrina de teología, y en el pensamiento agustiniano. En esta rama de la religión, la fe es considerada como una aceptación de revelación; la revelación aparece como doctrina. Se refiere a la rama del cristianismo caracterizada por un canon ritual uniforme y altamente desarrollado y una estructura organizacional con raíces doctrinales basadas en las enseñanzas de los Apóstoles de Jesucristo en el primer siglo, en la Escuela Alejandrina de teología, y en el pensamiento agustiniano. En esta rama de la religión, la fe es considerada como una aceptación de revelación; la revelación aparece como doctrina. En términos jurídicos, se refiere a la rama del Cristianismo distinguido como sistema sacramental unificado, monolítico bajo gobierno de la autoridad papal. A través de la mayor parte de su historia, &quot;la silla del papal” ha estado en Roma, mediante este concepto el Catolicismo Romano se distingue de la Iglesia Católica Ortodoxa. <![CDATA[<a href="#_getty_2017">(Getty, 2017)</a>]]></skos:definition>
    <skos:definition xml:lang="nl">Verwijst naar de richting van het christendom die zich kenmerkt door een uniforme, hoogontwikkelde rituele canon en organisatiestructuur met een doctrine die wortelt in de leer van de apostelen van Jezus Christus in de 1ste eeuw, in de theologie van de Alexandrijnse school en in het augustijner gedachtegoed. In deze godsdienstige richting wordt het geloof beschouwd als een aanvaarding van de openbaring; de openbaring heeft de vorm van een doctrine. In juridische zin verwijst de term naar de richting van het christendom die zich onderscheidt als een verenigd, monolithisch sacramenteel systeem onder het bestuur van het pauselijk gezag. Gedurende het grootste deel van de geschiedenis van dit systeem was de paus gevestigd in Rome en daarom wordt 'rooms-katholicisme' vaak gebruikt om dit begrip te onderscheiden van de orthodoxe katholieke kerk. <![CDATA[<a href="#_getty_2017">(Getty, 2017)</a>]]></skos:definition>
    <prov:derivedFrom rdf:resource="http://vocab.getty.edu/aat/300073730"/>
    <rdfs:comment xml:lang="en">The description for this term is indebted to the Getty Art &amp; Architecture Thesaurus.</rdfs:comment>
    <skos:definition xml:lang="fr">L’Église catholique, ou Église catholique, apostolique et romaine, est la plus grande Église chrétienne avec plus d'un milliard de fidèles. Elle réunit l’ensemble des chrétiens en communion avec le pape et les évêques qui sont considérés par les catholiques comme étant les successeurs des apôtres de Jésus-Christ. L'Église catholique est l'une des plus vieilles institutions religieuses au monde et a joué un rôle important dans l'histoire, surtout du monde occidental. La foi de l'Église catholique est résumée par le symbole de Nicée et elle se caractérise par la célébration des sept sacrements dont le plus important est l'Eucharistie célébré liturgiquement durant la messe. Selon son propre catéchisme, l'Église catholique est composée de trois parties qui ne forment qu'une seule Église placée sous Jésus-Christ : l'Église militante, l'Église triomphante et l'Église souffrante correspondant respectivement à l'ensemble des fidèles sur terre, l'ensemble des saints qui sont au ciel et l'ensemble des âmes qui sont au purgatoire. L'Église catholique sur terre se conçoit comme une communion d'Églises locales ou particulières, c'est-à-dire ayant chacune un territoire et un évêque à sa tête. Celles-ci sont chacune pleinement l'Église catholique dans la mesure où elles sont en communion avec le pape, qui est l'évêque de Rome et considéré comme étant le successeur de saint Pierre, et en communion les unes avec les autres. L'Église catholique se définit comme une institution à la fois humaine et divine : « société parfaite en dépit de l'imperfection de ses membres ». En plus d'être l'ensemble des baptisés, elle est aussi une institution et un clergé organisés de façon hiérarchique. Une très grande majorité des catholiques (au moins 98 %) sont de l'Église latine, mais il existe aussi des catholiques de différentes Églises catholiques orientales. <![CDATA[<a href="#_dbpedia_2017">(DBpedia, 2017)</a>]]></skos:definition>
    <prov:derivedFrom rdf:resource="http://dbpedia.org/page/Catholic_Church"/>
    <rdfs:comment xml:lang="fr">La description de ce terme est basée sur celle de DBPedia.</rdfs:comment>
    <rdf:type rdf:resource="http://www.w3.org/2004/02/skos/core#Concept"/>
    <rdf:type rdf:resource="http://xmlns.com/foaf/0.1/Organization"/>
    <skos:inScheme rdf:resource="#Religion"/>
    <skos:broaderTransitive rdf:resource="#christianity"/>
    <rdfs:isDefinedBy rdf:resource="http://sparql.cwrc.ca/ontologies/cwrc-ONTOLOGY_DATE"/>
    <void:inDataset rdf:resource="#datasetdefinition"/>
  </cwrc:Religion>
  <cwrc:Religion rdf:about="#christianity">
    <rdfs:label xml:lang="en">Christianity</rdfs:label>
    <rdfs:label xml:lang="zh-hant">基督教</rdfs:label>
    <rdfs:label xml:lang="zh-latn-pinyin-x-hanyu">jī dū jiāo</rdfs:label>
    <rdfs:label xml:lang="zh-latn-pinyin-x-notone">ji du jiao</rdfs:label>
    <rdfs:label xml:lang="zh-latn-wadegile">chi tu chiao</rdfs:label>
    <rdfs:label xml:lang="nl">Christendom</rdfs:label>
    <rdfs:label xml:lang="nl">Christelijk</rdfs:label>
    <rdfs:label xml:lang="es">Cristianismo</rdfs:label>
    <rdfs:label xml:lang="fr">Christianisme</rdfs:label>
    <skos:definition xml:lang="en">Refers to the world religion and culture that developed in the first century CE, driven by the teachings of Jesus Christ of Nazareth. Its roots are in the Judaic tradition and the Old Testament. The tenets include a belief in the death and redemptive resurrection of Jesus. The religion incorporates a tradition of faith, ritual, and a form of church authority or leadership. <![CDATA[<a href="#_getty_2017">(Getty, 2017)</a>]]></skos:definition>
    <skos:definition xml:lang="es">Se refiere a la religión y cultura que se desarrolló en la primera centuria, guiado por la creencia y reverencia por la vida, enseñanza, muerte y resurrección redentiva de Jesucristo de Nazaret. La religión incorpora una tradición de fe, ritual y una forma de iglesia de autoridad y liderazgo. <![CDATA[<a href="#_getty_2017">(Getty, 2017)</a>]]></skos:definition>
    <skos:definition xml:lang="nl">Verwijst naar de wereldreligie en -cultuur die in de eerste eeuw n. Chr. tot ontwikkeling kwam op basis van de leer van Jezus Christus van Nazareth. De wortels van deze religie liggen in de joodse traditie en het Oude Testament. Een van de kenmerkende grondbeginselen is het geloof in de dood en wederopstanding van Jezus. De religie omvat een traditie van geloof, rituelen en een vorm van kerkelijke autoriteit of leiderschap. <![CDATA[<a href="#_getty_2017">(Getty, 2017)</a>]]></skos:definition>
    <skos:definition xml:lang="zh-hant">發展於西元一世紀的世界宗教與文化，跟隨拿薩勒(Nazareth)耶穌基督的教誨。源於猶太傳統及舊約聖經。教義包括相信耶穌之死與救贖復活。此教融合信仰傳統、儀式，及某種形式的教會權威或領導。 <![CDATA[<a href="#_getty_2017">(Getty, 2017)</a>]]></skos:definition>
    <prov:derivedFrom rdf:resource="http://vocab.getty.edu/aat/300073711"/>
    <rdfs:comment xml:lang="en">The description for this term is indebted to the Getty Art &amp; Architecture Thesaurus.</rdfs:comment>
    <skos:definition xml:lang="fr">Le christianisme est une religion abrahamique fondée sur l'enseignement, la personne et la vie de Jésus de Nazareth tels qu'ils sont interprétés par la tradition chrétienne à partir du Nouveau Testament de la Bible. Il s'agit d'une religion du salut considérant Jésus-Christ comme le Messie annoncé par les prophètes dans l'Ancien Testament qui vient sauver l'humanité du Mal et la faire participer à la vie de Dieu. La foi en la résurrection de Jésus est au cœur du christianisme car elle signifie le début d'une humanité nouvelle libérée du Mal. Les premières communautés chrétiennes naissent au Ier siècle en Judée et dans les grandes villes de la diaspora juive telles que Rome, Éphèse, Antioche et Alexandrie. Le christianisme se développe dès le IIe siècle dans l'Empire romain, dont il devient la religion officielle au IVe siècle, mais aussi en Perse, en Inde et en Éthiopie. Au Moyen-Âge, le christianisme devint majoritaire en Europe, tandis qu'il s'amenuise face à l'islam dans les régions où il est né. Depuis le XVIe siècle, il est devenu la religion la plus importante de la planète par son expansion en Amérique et, plus tard, en Afrique. Il est actuellement présent dans tous les pays du monde. Les Églises chrétiennes sont classiquement regroupées en trois principales branches : le catholicisme, le christianisme orthodoxe et le protestantisme représentant respectivement 50%, 12% et 37% du total des chrétiens en 2010. À la mi-2015, le nombre total de chrétiens dans le monde est évalué à 2,419 milliards, ce qui en fait la religion comptant le plus grand nombre de fidèles au monde devant l'islam qui en compte environ 1,6 milliard. <![CDATA[<a href="#_dbpedia_2017">(DBpedia, 2017)</a>]]></skos:definition>
    <prov:derivedFrom rdf:resource="http://dbpedia.org/page/Christianity"/>
    <rdfs:comment xml:lang="fr">La description de ce terme est basée sur celle de DBPedia.</rdfs:comment>
    <rdf:type rdf:resource="http://www.w3.org/2004/02/skos/core#Concept"/>
    <skos:inScheme rdf:resource="#Religion"/>
    <rdfs:isDefinedBy rdf:resource="http://sparql.cwrc.ca/ontologies/cwrc-ONTOLOGY_DATE"/>
    <void:inDataset rdf:resource="#datasetdefinition"/>
    <skos:broaderTransitive rdf:resource="#abrahamicReligions"/>
  </cwrc:Religion>
  <cwrc:Religion rdf:about="#churchOfChristianScience">
    <rdfs:label xml:lang="en">Christian Science</rdfs:label>
    <rdfs:label xml:lang="nl">Christenwetenschap</rdfs:label>
    <rdfs:label xml:lang="es">Ciencia Cristiana</rdfs:label>
    <rdfs:label xml:lang="fr">Science CHRÉTIENNE</rdfs:label>
    <skos:definition xml:lang="en">Refers to a Christian denomination and movement founded by Mary Baker Eddy (1821-1910) that seeks to reinstate the Christian message of salvation from all evil, including sickness and disease as well as sin. Eddy, a semi-invalid who was interested in cures not involving medicine, claimed a recovery from a bad injury without medical assistance in 1866. Afterwards, she devoted herself to restoring the healing emphasis of early Christianity. In 1875 she finished writing the first edition of the 'Science and Health with Key to the Scriptures.' This work and the Bible are the principal texts of the movement and importance has been laid on establishing reading rooms where these works can make their own appeal to readers. The 'Christian Science Monitor' is also published by the denomination. Christian Science believes that ignorance is at the root of human unease and thus 'dis-ease.' Instead of seeking medical treatment, special Christian Science healers are to be consulted for spiritual healing. Health, happiness, and holiness can be restored by applying to all aspects of life practices and attitudes in keeping with the principal of divine harmony. The first Church of Christ, Scientist was founded in 1879 in Boston and its headquarters remain there. <![CDATA[<a href="#_getty_2017">(Getty, 2017)</a>]]></skos:definition>
    <skos:definition xml:lang="es">Se refiere a una secta y movimiento cristiano fundado por Mary Baker Eddy (1821-1910) que busca reincorporar el mensaje cristiano de salvación de todo mal, incluso la enfermedad y padecimiento así como el pecado. Eddy, un semi-inválido que estaba interesado en curas que no involucraran medicina, afirmó que se había recuperado de una lesión grave sin la ayuda médica en 1866. Después, se consagró a restaurar el énfasis curativo de la primera cristiandad. En 1875 ella terminó escribiendo la primera edición del &quot;la Ciencia y Salud con Llave a las Escrituras&quot;. Este trabajo y la Biblia son los textos principales del movimiento y importancia se ha puesto en establecer salas de lectura donde estos trabajos pueden hacer su propia apelación a los lectores. El &quot;Instructivo de ciencia cristiano&quot; también fue publicado por la secta. La Ciencia Cristiana cree que la ignorancia es la raíz de los padecimientos humanos y por lo tanto de la enfermedad. En lugar de buscar tratamiento médico, los sanadores de la Ciencia Cristiana especiales serán consultados para la curación espiritual. La salud, felicidad, y santidad pueden ser restauradas aplicando a todos los aspectos de la vida prácticas y actitudes en concordancia con la armonía divina. La primera Iglesia Científica de Cristo, se fundó en 1879 en Boston y su centro principal permanece allí. <![CDATA[<a href="#_getty_2017">(Getty, 2017)</a>]]></skos:definition>
    <skos:definition xml:lang="nl">Verwijst naar een christelijke gezindte en beweging die is gesticht door Mary Baker Eddy (1821-1910) en die streeft naar herbevestiging van de christelijke boodschap van verlossing van al het kwaad, met inbegrip van ziekte en zonde. Eddy, die half invalide was en geïnteresseerd in genezing zonder medicijnen, beweerde dat zij in 1866 zonder medische hulp was hersteld van zwaar letsel. Daarna wijdde zij zich aan het herstel van de nadruk op gebedsgenezing die het vroege christendom had gekenmerkt. In 1875 voltooide zij de eerste editie van haar boek 'Science and Health with Key to the Scriptures'. Dit werk en de Bijbel zijn de voornaamste geschriften van de beweging, die veel belang hecht aan de inrichting van leesruimten waar deze boeken een eigen beroep op de lezers kunnen doen. Ook de 'Christian Science Monitor' wordt door het kerkgenootschap uitgegeven. Volgens de leer van Christian Science is onwetendheid de wortel van het menselijk ongemak, de menselijke ziekte. In plaats van medische behandeling te zoeken moet men gebedsgenezers van Christian Science raadplegen voor spirituele genezing. Gezondheid, geluk en heiligheid kunnen worden hersteld door alle aspecten van de levenspraktijk en -houding aan te spreken in overeenstemming met het beginsel van goddelijke harmonie. De eerste Church of Christ, Scientist werd in 1879 in Boston gesticht en het hoofdkwartier van de beweging is daar nog altijd gevestigd. <![CDATA[<a href="#_getty_2017">(Getty, 2017)</a>]]></skos:definition>
    <prov:derivedFrom rdf:resource="http://vocab.getty.edu/aat/300264476"/>
    <rdfs:comment xml:lang="en">The description for this term is indebted to the Getty Art &amp; Architecture Thesaurus.</rdfs:comment>
    <skos:definition xml:lang="fr">La Science chrétienne (ou Christian Science en anglais) se définit elle-même comme la « Science du Christ ». Sa fondatrice, la théologienne américaine Mary Baker Eddy, estime avoir redécouvert en 1866 les lois appliquées par Jésus dans la guérison des malades et la résolution des aléas de la vie, lois toujours démontrables aujourd'hui. Son observation des guérisons et résolutions diverses obtenues sur la base de sa théorie en prouve, selon elle, la validité. Ainsi, la Science chrétienne est « chrétienne » en ce sens qu’elle repose sur les enseignements de Jésus de Nazareth, tels qu'exposés dans le Nouveau Testament. La Science chrétienne se veut une religion pratique permettant l'application de lois divines démontrables. Afin d'assurer la diffusion de cette science, Mary Baker Eddy fonde en 1879 une Église sans credo, appelée « Église du Christ, Scientiste » (en anglais The First Church of Christ, Scientist), rassemblant de nos jours 1 800 églises dans 82 pays et quelques centaines de milliers de pratiquants, principalement aux États-Unis. Reconnue comme association cultuelle dans de nombreux pays, notamment aux États-Unis, la Science chrétienne précise que, malgré la confusion possible entre les deux noms, elle n’a rien de commun avec l’Église de Scientologie; de plus, bien qu'elle partage nombre de concepts métaphysiques avec les églises de la Nouvelle Pensée comme Unité, la Science divine et la Science religieuse, ce qui amène certains historiens et sociologues à les aborder ensemble dans leurs travaux, la Science chrétienne et ces églises ne se reconnaissent pas mutuellement comme faisant partie de la même mouvance. La principale critique de la Science chrétienne est qu'elle a un caractère alternatif et non complémentaire au traitement médical. Ainsi, les guérisons alléguées sont obtenues en dehors de tout contrôle médical. Ses guérisons de maladies fonctionnelles ou organiques sont considérées comme relevant de l’effet placebo par les détracteurs de la Science chrétienne (ce qui n’est d’ailleurs pas tellement en contradiction avec la Science chrétienne, qui ne considère la maladie que comme le résultat de simples croyances erronées, qu’il faudrait donc corriger pour recouvrer la santé.). La principale défense de la Science chrétienne est que chacun est libre de choisir la méthode de guérison qu'il juge la plus efficace et qu'il n'existe aucune contrainte à ce sujet. Les sympathisants mettent en avant les guérisons qu’ils disent avoir obtenues et réfutent toute idée de rejet de la médecine conventionnelle. <![CDATA[<a href="#_dbpedia_2017">(DBpedia, 2017)</a>]]></skos:definition>
    <prov:derivedFrom rdf:resource="http://dbpedia.org/page/Christian_Science"/>
    <rdfs:comment xml:lang="fr">La description de ce terme est basée sur celle de DBPedia.</rdfs:comment>
    <rdf:type rdf:resource="http://www.w3.org/2004/02/skos/core#Concept"/>
    <skos:inScheme rdf:resource="#Religion"/>
    <skos:broaderTransitive rdf:resource="#christianity"/>
    <rdfs:isDefinedBy rdf:resource="http://sparql.cwrc.ca/ontologies/cwrc-ONTOLOGY_DATE"/>
    <void:inDataset rdf:resource="#datasetdefinition"/>
  </cwrc:Religion>
  <cwrc:Religion rdf:about="#hinduism">
    <rdfs:label xml:lang="en">Hinduism</rdfs:label>
    <rdfs:label xml:lang="fr">Hindou</rdfs:label>
    <rdfs:label xml:lang="zh-hant">印度教</rdfs:label>
    <rdfs:label xml:lang="zh-latn-pinyin-x-hanyu">yìn dù jiào</rdfs:label>
    <rdfs:label xml:lang="zh-latn-pinyin-x-notone">yin du jiao</rdfs:label>
    <rdfs:label xml:lang="zh-latn-wadegile">yin tu chiao</rdfs:label>
    <rdfs:label xml:lang="nl">Hindoeïsme</rdfs:label>
    <rdfs:label xml:lang="es">Hinduismo</rdfs:label>
    <rdfs:label xml:lang="fr">hindouisme</rdfs:label>
    <skos:definition xml:lang="en">General term for the set of intellectual and philosophical tenets and highly diverse beliefs and practices that define the civilization, art, literature, society, and politics of the Indian subcontinent. Hinduism is not a common set of rigid beliefs , but varies significantly between different regions; it includes Shaivism, Vaishnavism, Srauta, and numerous other traditions. Among other practices and philosophies, Hinduism includes a wide spectrum of laws and prescriptions of &quot;daily morality&quot; based on karma, dharma, and societal norms. The highest divine powers are seen as complementary to one another and not exclusive. Hinduism does not have a particular founder or central authority. Hindu literature is rich and varied, with no one text considered uniquely authoritative. The Vedas, dating to the Vedic period (ca. 1200-500 BCE), are the earliest extant writings. Religious law books and epics such as the Ramayana and the Mahabharata have been and continue to be highly influential. <![CDATA[<a href="#_getty_2017">(Getty, 2017)</a>]]></skos:definition>
    <skos:definition xml:lang="es">Se refiere al conjunto de creencias y prácticas altamente diversas que generalmente denotan la civilización y cultura India de los dos mil últimos años. La religión influye fuertemente en el arte, la literatura, la política y al sociedad hinduista. Presenta la creencia y la práctica de ritos mágicos, cultos animales, creencia en demonios, cultos a deidades, incluyendo dioses locales y dioses centrales, misticismo, ascetismo y una apreciación y respeto por otras formas de cultos o creencias religiosas. La verdad de la religión no esta concebida como un término dogmático, sino que la verdad supera toda definición verbal. En vez de un sistema de doctrinas, el énfasis se pone en la manera correcta de vivir (dharma). Hay variaciones significativas entre diversas regiones. La mayoría de las formas de hinduismo enfatizan el concepto del reencarnación o de la transmigración; la liberación (moksha) desde el ciclo del samsara es la última meta espiritual del hindú. Brahma, Vishnu y Shiva son las deidades hindúes principales, juntos forman la tríada, el Trimurti. Existen muchos otros deidades de menor rango. El Hinduismo no tiene un fundador en particular o un iniciado, allí no hay una autoridad central. La literatura hindú es rica y variada, sin un texto considerado únicamente autoritario. El Vedas, fechando en el período de Vedic (ca. 1200-500 a. C), es la escritura más temprana existente. Los libros de ley y las epopeyas religiosas tales como el Ramayana y el Mahabharata han sido y continúan siendo altamente influyentes. <![CDATA[<a href="#_getty_2017">(Getty, 2017)</a>]]></skos:definition>
    <skos:definition xml:lang="nl">Verwijst naar de reeks uiterst diverse geloven en gebruiken die in het algemeen verwijzen naar de Indiase beschaving en cultuur van de afgelopen tweeduizend jaar. De religie heeft een sterke invloed op de Indiase kunst, literatuur, maatschappij en politiek. Het hindoeïsme omvat diverse religieuze geloven en gebruiken en in plaats van andere goden, andere godsdiensten en andere religieuze concepten als fout of onverenigbaar te zien, worden de hoogste goddelijke machten gezien als elkaar aanvullend. De religieuze waarheid wordt niet gezien in dogmatische termen aangezien wordt geloofd dat de waarheid alle woordelijke definities overstijgt. In plaats van op een reeks doctrines ligt de nadruk op de juiste manier van leven (dharma). Er zijn aanzienlijke verschillen per regio. In de meeste vormen van het hindoeïsme ligt de nadruk op het concept van reïncarnatie of zielsverhuizing; de bevrijding (moksha) van de cyclus van samsara is het uiteindelijke spirituele doel van hindoes. Brahma, Visjnoe en Shiva zijn de belangrijkste hindoeïstische godheden en vormen gezamenlijk een drie-eenheid, de Trimurti. Verder is er een groot aantal lagere goden. Het hindoeïsme heeft geen specifieke oprichter of ontstaansmoment en er is geen centrale autoriteit. De hindoeïstische literatuur is erg rijk en gevarieerd en geen enkele specifieke tekst wordt als gezaghebbend beschouwd. De Veda's, die afkomstig zijn uit de Vedische periode (ca. 1200-500 v. Chr.), zijn de oudste overgebleven geschriften. Religieuze wetboeken en heldendichten zoals de Ramayana en de Mahabharata zijn altijd erg invloedrijk geweest. <![CDATA[<a href="#_getty_2017">(Getty, 2017)</a>]]></skos:definition>
    <skos:definition xml:lang="zh-hant">代表過去兩千年來印度文明與文化的一套極多樣的信仰與實踐方式。此宗教對印度藝術、文學、社會與政治有極大影響。印度教包含多元的宗教信仰及實踐方式，因此不會認為其他的神明、其他形式的敬拜及宗教觀是錯誤或者互不相容，反而認為最高的神力是彼此互補的。他們相信真理超越所有言語定義，因此不應武斷認定何謂宗教真理。重視生活的正確方式(法)，而非一連串的教條。不同宗教之間差異甚鉅。大部分的印度教形式強調輪迴觀念；從生死疾苦等輪迴中解脫是印度教徒最終的心靈目標。婆羅摩、毗濕奴、濕婆是印度教主要的三個神明(三相神) 。還有很多其他小神。印度教沒有確切的建立者及開始時間，也沒有中央權威。印度教文學豐富且多樣，但沒有哪一部作品被認為是權威。追溯自吠陀時期(西元前500年到西元1200年)的吠陀經是現存最早的經典。宗教法律典籍及史詩如《羅摩耶那史詩》及《摩訶婆羅達》仍舊極具影響力。 <![CDATA[<a href="#_getty_2017">(Getty, 2017)</a>]]></skos:definition>
    <prov:derivedFrom rdf:resource="http://vocab.getty.edu/aat/300073727"/>
    <rdfs:comment xml:lang="en">The description for this term is indebted to the Getty Art &amp; Architecture Thesaurus.</rdfs:comment>
    <skos:definition xml:lang="fr">L’hindouisme (hindi : hindu dharm ; devanāgarī : हिन्दू धर्म ; « religion hindoue »), ou Sanatana Dharma (sanskrit IAST : sanātanadharma ; devanāgarī : सनातनधर्म ; « Loi Éternelle »), est l'une des plus vieilles religions du monde encore pratiquées, qui n'a ni fondateur ni Église. Avec près d'un milliard de fidèles dans 84 pays, c'est actuellement la troisième religion la plus pratiquée dans le monde après le christianisme et l'islam. Elle est issue du sous-continent indien qui reste son principal foyer de peuplement. La particularité de l'hindouisme est de n'avoir ni prophètes ni dogmes centraux. Cependant, les hindous contemporains croient en l'autorité du Veda, qui, selon la tradition, fut révélé aux hommes, grâce à la « vision » des Rishi. Le terme persan hindu (du sanskrit Sindhu) désignait au départ, pour les musulmans qui pénétrèrent en Inde, les habitants du bassin de l'Indus. L'hindouisme se présente comme un ensemble de concepts philosophiques issus d'une tradition remontant à la protohistoire indienne, la pratique hindouiste étant sans doute issue d'une tradition orale très ancienne, proche de l'animisme. On retient parfois une tripartition historique qui fait de l'hindouisme la dernière phase du développement des religions en Inde, après le védisme aryen (~1500 à 900 av. J.-C.) et le brahmanisme (~900 à 400 av. J.-C.). Au-delà du syncrétisme théologique, l'hindouisme d'avant les invasions islamiques et le colonialisme européen qui soumirent l'Inde à leur autorité était un vecteur pour toutes les sciences : le droit, la politique, l'architecture, l'astronomie, la philosophie, la médecine, etc., comme d'autres savoirs qui avaient en commun le substrat religieux. <![CDATA[<a href="#_dbpedia_2017">(DBpedia, 2017)</a>]]></skos:definition>
    <prov:derivedFrom rdf:resource="http://dbpedia.org/page/Hinduism"/>
    <rdfs:comment xml:lang="fr">La description de ce terme est basée sur celle de DBPedia.</rdfs:comment>
    <rdf:type rdf:resource="http://www.w3.org/2004/02/skos/core#Concept"/>
    <skos:inScheme rdf:resource="#Religion"/>
    <rdfs:isDefinedBy rdf:resource="http://sparql.cwrc.ca/ontologies/cwrc-ONTOLOGY_DATE"/>
    <void:inDataset rdf:resource="#datasetdefinition"/>
    <skos:broaderTransitive rdf:resource="#occultism"/>
  </cwrc:Religion>
  <cwrc:Religion rdf:about="#islam">
    <rdfs:label xml:lang="en">Islamism</rdfs:label>
    <rdfs:label xml:lang="es">Islam</rdfs:label>
    <rdfs:label xml:lang="zh-hant">伊斯蘭教</rdfs:label>
    <rdfs:label xml:lang="zh-hant">回教</rdfs:label>
    <rdfs:label xml:lang="zh-latn-pinyin-x-hanyu">yī sī lán jiāo</rdfs:label>
    <rdfs:label xml:lang="zh-latn-pinyin-x-notone">yi si lan jiao</rdfs:label>
    <rdfs:label xml:lang="zh-latn-wadegile">i ssu lan chiao</rdfs:label>
    <rdfs:label xml:lang="nl">Islam</rdfs:label>
    <rdfs:label xml:lang="fr">Religion Mahométane</rdfs:label>
    <rdfs:label xml:lang="fr">Mahométisme</rdfs:label>
    <rdfs:label xml:lang="es">Islamismo</rdfs:label>
    <rdfs:label xml:lang="fr">islam</rdfs:label>
    <skos:definition xml:lang="en">Refers to the religious beliefs and social practices founded in the seventh century by the Arabian Prophet Muhammad, held to be the last of a series of major prophets, which include, according to Islamic dogma, Adam, Noah, and Jesus. It later spread throughout the Middle East, Africa, Europe, and parts of Asia. It is characterized by the belief in the fundamental idea that a devotee 'surrenders' and submits his will to Allah, the prime creator and sustainer of the universe and all creation. In Islam, God is unique and has no partner or intermediary as in the Christian Trinity. Social service and the active alleviation of suffering in others is considered the only path to salvation and prayer and sacred ritual alone are inadequate forms of submission to Allah. The Qur'an (Koran), the sacred text of the religion, is a compilation of revelations from Allah believed to have been received by Muhammad. <![CDATA[<a href="#_getty_2017">(Getty, 2017)</a>]]></skos:definition>
    <skos:definition xml:lang="es">Se refiere a creencias religiosas y prácticas sociales fundadas en el siglo VII por el Profeta árabe Mahoma, supuestamente el último de una serie de grandes profetas, incluídos, de acuerdo al dogma Islámico, Adán, Noé y Jesús. Posteriormente se difundió a través del Medio Oriente, África, Europa y parte de Asia. Se caracteriza por la creencia en la idea fundamental que un devoto se &quot;rinde&quot; y somete la voluntad de Alá, el principal creador y mantenedor del universo y toda creación. En el Islam, Dios es único y no tiene parentesco o intermediario como la trinidad cristiana. El servicio social y las actividades que alivian el sufrimiento de otros es considerado el único camino a la salvación y la oración y ritual sagrado a solas es una inadecuado forma de sumisión para Alá. El Coran (Koran), consagrado el texto de las religiones, es una compilación relevante de las creencias de Alá que fueron recibidas de Mahoma. <![CDATA[<a href="#_getty_2017">(Getty, 2017)</a>]]></skos:definition>
    <skos:definition xml:lang="nl">Verwijst naar het samenstel van religieuze overtuigingen en sociale gebruiken dat in de 7de eeuw is ontstaan op basis van de leer van de Arabische profeet Mohammed, die wordt beschouwd als de laatste in een reeks van grote profeten; volgens de islamitische leer zijn dit onder anderen Adam, Noach en Jezus. De islam heeft zich later verspreid in het Midden-Oosten, Afrika, Europa en delen van Azië. De islam wordt gekenmerkt door het geloof in het fundamentele idee dat een gelovige zich 'overgeeft' en zich onderwerpt aan Allah, de schepper van het universum en de schepping als geheel. God is uniek en heeft geen partner of tussenpersoon zoals bij de christelijke drie-eenheid. Maatschappelijke dienstbaarheid en het actief verlichten van het lijden van anderen wordt beschouwd als de enige weg naar verlossing en gebeden en heilige rituelen zijn op zichzelf onvoldoende vormen van overgave aan Allah. De Qur'an (Koran), het heilige geschrift van de religie, is een verzameling onthullingen die, zo gelooft men, door Allah aan Mohammed zijn geopenbaard. <![CDATA[<a href="#_getty_2017">(Getty, 2017)</a>]]></skos:definition>
    <skos:definition xml:lang="zh-hant">由阿拉伯先知穆罕默德於七世紀創建的宗教信仰與社會實踐方式。根據伊斯蘭教條，穆罕默德是繼亞當、挪亞、耶穌後最後一個主要的先知。此教之後廣傳中東、非洲、歐洲、及部份亞洲。基本思想為信徒交出自己的意志給阿拉(宇宙及所有創造物的最高造物者與支撐者)。就伊斯蘭教而言，神是獨一無二的，且并非如基督教三位一體的觀點般有夥伴或是媒介。社會服務及積極幫助受苦者被認為是通往救贖的唯一路徑，若只有祈禱及神聖儀式則不算完全奉獻予阿拉。可蘭經是此教的聖典，記載穆罕默德從阿拉得來的神示。 <![CDATA[<a href="#_getty_2017">(Getty, 2017)</a>]]></skos:definition>
    <prov:derivedFrom rdf:resource="http://vocab.getty.edu/aat/300073715"/>
    <rdfs:comment xml:lang="en">The description for this term is indebted to the Getty Art &amp; Architecture Thesaurus.</rdfs:comment>
    <skos:definition xml:lang="fr">L'islam (arabe : الإسلام) est une religion abrahamique s'appuyant sur le dogme du monothéisme absolu (l'adoration du Dieu unique sans lui attribuer aucun associé) et prenant sa source dans le Coran, considéré comme le recueil de la parole de Dieu (arabe : الله, Allah) révélée à Mahomet, proclamé par les adhérents de l'islam comme étant le dernier prophète de Dieu, au VIIe siècle en Arabie. Un adepte de l'islam est appelé un musulman. L'islam revendique pour fondement et enseignement principal le tawhid (monothéisme, unicité et indivisibilité), c'est-à-dire le monothéisme le plus épuré où le culte est voué exclusivement à Dieu, sans lui attribuer aucun fils. Les musulmans croient que Dieu est un et incomparable et que le but de l'existence est d'adorer Dieu. Les musulmans croient également que l'islam est la version complète et universelle d'une foi primordiale qui a été révélée à plusieurs reprises par le passé à travers les prophètes, incluant Adam, Noé, Abraham, Moïse et Jésus. Ainsi, elle se présente comme un retour sur les pas d'Abraham (appelé, en arabe, Ibrahim par les musulmans) du point de vue de la croyance, le Coran le définissant comme étant l'étalon-pied, la lieue de la Kaaba, le mille d'Abraham (milla ta Ibrahim), c'est-à-dire une soumission exclusive à la volonté d'Allah. Le Coran reconnaît l'origine divine de l'ensemble des livres sacrés du judaïsme et du christianisme, tout en estimant qu'ils seraient, dans leurs interprétations actuelles, le résultat d'une falsification partielle : le Suhuf-i-Ibrahim (les Feuillets d'Abraham), la Tawrat (le Pentateuque ou la Torah), le Zabur de David et Salomon (identifié au Livre des Psaumes) et l'Injil (l'Évangile). Outre le Coran, la majorité des musulmans se réfèrent à des transmissions de paroles, actes et approbations de Mahomet, récits appelés hadîths, pour l'établissement de règles juridiques (fiqh) permettant la compréhension et l'accomplissement des adorations du musulman au quotidien. Les différentes branches de l'islam ne s'accordent pas sur les compilations de hadiths à retenir comme authentiques. Le Coran et les hadiths dits « recevables » sont deux des quatre sources de la loi islamique, la charia, les deux autres étant l'unanimité (ijma’) et l'analogie (qiyas). En 2010, le nombre de musulmans dans le monde est estimé à 1,6 milliard, soit 23,4 % de la population mondiale, ce qui fait de l'islam la deuxième religion du monde après le christianisme et devant l'hindouisme. C’est, chronologiquement parlant, le troisième grand courant monothéiste de la famille des religions abrahamiques, après le judaïsme et le christianisme avec lesquels il possède un certain nombre d'éléments communs. L’islam se répartit en différents courants, dont les principaux sont le sunnisme, qui représente entre 80 et 85 % des musulmans, et le chiisme, rencontré principalement en Irak et en Iran. <![CDATA[<a href="#_dbpedia_2017">(DBpedia, 2017)</a>]]></skos:definition>
    <prov:derivedFrom rdf:resource="http://dbpedia.org/page/Islam"/>
    <rdfs:comment xml:lang="fr">La description de ce terme est basée sur celle de DBPedia.</rdfs:comment>
    <rdf:type rdf:resource="http://www.w3.org/2004/02/skos/core#Concept"/>
    <skos:inScheme rdf:resource="#Religion"/>
    <rdfs:isDefinedBy rdf:resource="http://sparql.cwrc.ca/ontologies/cwrc-ONTOLOGY_DATE"/>
    <void:inDataset rdf:resource="#datasetdefinition"/>
    <skos:broaderTransitive rdf:resource="#abrahamicReligions"/>
  </cwrc:Religion>
  <cwrc:Religion rdf:about="#judaism">
    <rdfs:label xml:lang="en">Jewish</rdfs:label>
    <rdfs:label xml:lang="zh-hant">猶太教</rdfs:label>
    <rdfs:label xml:lang="zh-latn-pinyin-x-hanyu">yóu tài jiāo</rdfs:label>
    <rdfs:label xml:lang="zh-latn-pinyin-x-notone">you tai jiao</rdfs:label>
    <rdfs:label xml:lang="zh-latn-wadegile">yu t'ai chiao</rdfs:label>
    <rdfs:label xml:lang="nl">Jodendom</rdfs:label>
    <rdfs:label xml:lang="nl">Joods</rdfs:label>
    <rdfs:label xml:lang="es">Judaísmo</rdfs:label>
    <rdfs:label xml:lang="fr">Judaïsme</rdfs:label>
    <skos:definition xml:lang="en">Refers to the monotheistic religion of the Jewish people, central to which is the belief that the ancient Israelites experienced God's presence in human events. Jews believe that the one God delivered the Israelites out of bondage in Egypt, revealed the structure of communal and individual life to them, and chose them to be a holy nation of people able to set an example for all humankind. The Hebrew Bible and Talmud are the two primary sources for Judaism's spiritual and ethical principles. The religion, which traces its origins to Abraham, places more emphasis on expressing beliefs through ritual rather than through abstract doctrine. The Sabbath, beginning on sunset on Friday and ending at sunset on Saturday, is the central religious observance; there is also an annual cycle of religious festivals and days of fasting. Judaism has had a diverse history of development over almost 4000 years, with a number of resulting branches in modern times, namely Orthodox, Conservative, and Reform. <![CDATA[<a href="#_getty_2017">(Getty, 2017)</a>]]></skos:definition>
    <skos:definition xml:lang="es">Se refiere a la religión monoteista del pueblo judío, para los cuales es central la creencia que los antiguos israelitas experimentaron la presencia de Dios en los eventos humanos. Los judíos creen que el Dios único salvó los israelistas de la esclavitud en Egipto, revelándoles la estructura de la vida comunal e individual y eligiéndolos para ser una nación sagrada de personas capaces de dar un ejemplo para toda la humanidad. La Biblia Hebrea y el Talmud son dos fuentes primarias de la espiritualidad judía y de los principios éticos.Los orígenes de la religión se remontan a los tiempos de Abraham, poniendo mayor énfasis en expresar la creencia con rituales más bien que con doctrinas abstractas. El Shabbat, que comienza con la puesta de sol del viernes y termina con la puesta de sol del sábado, es la observancia religiosa central; hay también un ciclo anual de fiestas religiosas y días de ayuno. El judaísmo ha tenido un desarrollo diverso a lo largo de la historia de casi 4.000 años, con un gran número de ramas resultantes en épocas modernas, concretamente ortodoxas, conservadoras, y reformistas. <![CDATA[<a href="#_getty_2017">(Getty, 2017)</a>]]></skos:definition>
    <skos:definition xml:lang="nl">Verwijst naar de monotheïstische religie van het joodse volk, waarbij het geloof centraal staat dat de oude Israëlieten de aanwezigheid van God ervoeren in menselijke gebeurtenissen. Joden geloven dat één God de Israëlieten uit hun gevangenschap in Egypte heeft bevrijd, de structuur van een gemeenschappelijk en individueel leven aan hen heeft onthuld en hen heeft uitverkoren als een heilig volk dat als voorbeeld moest dienen voor de gehele mensheid. De Hebreeuwse bijbel en de Talmoed zijn de belangrijkste bronnen voor de spirituele en ethische principes van het jodendom. Deze religie, waarvan de oorsprong teruggaat naar de tijd van Abraham, legt meer de nadruk op het tot uitdrukking brengen van het geloof in de vorm van rituelen dan in de vorm van abstracte doctrines. De sabbat, die begint bij zonsondergang op vrijdag en eindigt bij zonsondergang op zaterdag, is een centraal element van de religie; er is ook een jaarlijkse cyclus van religieuze feestdagen en vastendagen. Het jodendom heeft een zeer uiteenlopende ontwikkelingsgeschiedenis die bijna 4000 jaar beslaat en is uitgemond in diverse stromingen: de orthodoxe, conservatieve en reformistische stroming. <![CDATA[<a href="#_getty_2017">(Getty, 2017)</a>]]></skos:definition>
    <skos:definition xml:lang="zh-hant">猶太人的一神論宗教，相信古代以色列人於人類事件中體驗到神的存在。猶太人相信這唯一的神使他們脫離埃及的奴役，向他們揭示公共及個人生活的結構，並選擇他們為聖國子民，以為全人類樹立榜樣。《希伯來聖經(Hebrew Bible)》與《塔爾穆德(Talmud)》為猶太教精神與道德原則的兩大來源。猶太教源於亞伯拉罕，較強調以儀式而非抽象的教條表達信仰。遵循信仰的重心為安息日，從週五的日落開始到週日的日出結束；另外每年還有宗教節慶和齋戒日。猶太教經過將近四千年的發展，衍生出許多現代的分支，即正統派猶太教(Orthodox)、保守派猶太教(Conservative)，與改革派猶太教(Reform.)。 <![CDATA[<a href="#_getty_2017">(Getty, 2017)</a>]]></skos:definition>
    <prov:derivedFrom rdf:resource="http://vocab.getty.edu/aat/300073723"/>
    <rdfs:comment xml:lang="en">The description for this term is indebted to the Getty Art &amp; Architecture Thesaurus.</rdfs:comment>
    <skos:definition xml:lang="fr">Pour l'Encyclopædia Britannica, le mot judaïsme recouvre la religion des Juifs, ainsi que la théologie, la loi et les traditions culturelles du peuple juif, constitué des descendants des Israélites provenant de l'antique terre d'Israël et des quelques minorités les ayant rejoints par la conversion et s'étant mélangées à eux au fil de leur diaspora de deux millénaires. Pour un juif orthodoxe comme Daniel Boyarin, le judaïsme est « l'ensemble des rituels et des autres pratiques, des croyances et des valeurs, des loyautés historiques et politiques qui constituent l'allégeance au peuple d'Israël », mais le judaïsme n’est ni une religion ni une foi, selon Boyarin. Ainsi Bernard-Henri Lévy affirme que « la tâche des Juifs comme tels est d’être irréligieux », dans la mesure où la religion, telle qu'on la conçoit en théologie, édifiée par une croyance, par des dogmes, par une instance suprême, centrale et doctrinale, n’appartient pas à l’esprit du judaïsme, selon lui. Le judaïsme comporte des éléments religieux, mais ne s'y limite pas puisqu'il contient des coutumes non spécifiquement religieuses – outre des codes de conduite, des lois, des rites – et qu’il fonde plus largement encore une « culture juive ». Néanmoins, par convention, on parle habituellement du judaïsme comme d’une « religion », mais il ne faut pas l’entendre au sens strict, selon des historiens des religions comme Simon Claude Mimouni ou Daniel Boyarin, ou des philosophes comme Léo Strauss ou Bernard-Henri Lévy. Selon ses textes fondateurs, en particulier le Tanakh, la foi des anciens Israélites et de leurs descendants les Juifs, est fondée sur une alliance contractée entre Dieu et Abraham, qui a ensuite été renouvelée entre Dieu et Moïse. Les juifs fondent le judaïsme sur la religion abrahamique qui fleurira ensuite dans la Loi mosaïque (la Torah, les Nevi'im et les Ketouvim), collectivement désignés par l'acronyme Tanakh, dont le texte constitue la Miqra ou Bible hébraïque. Cette religion se fonde sur le culte du Dieu d'Abraham, d'Isaac et de Jacob, au Nom ineffable, qu'elle conçoit comme une Essence éternelle (YHWH), qui détient tous les pouvoirs (Elohim), transcendant le Seigneur des Seigneurs (Adonaï) qu'elle considère Un et Unique et qu'elle qualifie ainsi : omnipotent, omniscient, omniprésent, juste et miséricordieux. Cette religion professe aussi que le rassemblement de toutes les puissances (Elohim) manifesta le créateur du monde qui continue de s'impliquer dans sa destinée en faisant irruption dans l'Histoire dont il révèle la dimension d'Histoire Sainte, comme lorsqu'il fit sortir d'Égypte les enfants d'Israël. Les cohanim, ou prêtres, du Temple de Jérusalem, par deux fois détruit, assuraient son culte. Certains groupes juifs, comme les Ésséniens, s'opposaient à la centralité du culte à Jérusalem. La seconde destruction du Temple de Jérusalem et la dispersion des juifs dans le monde donna naissance à plusieurs traditions religieuses juives. Si la majorité des juifs se regroupèrent autour de l'élaboration du Talmud par les rabbanim, un mouvement strictement scripturaliste, dit Karaïsme, s'opposa à la codification de la tradition orale, tandis que d'autres groupes éloignés, comme les Beta d'Israël en Éthiopie, ignorèrent cette évolution et se développèrent en vase clos. Le judaïsme est l'une des plus anciennes traditions religieuses du monothéisme exclusif encore pratiquées aujourd'hui. Les valeurs et l'histoire du peuple juif sont à la source des deux autres religions abrahamiques, le christianisme et l'islam. Il n'est toutefois pas à la base du samaritanisme, qui est une tradition israélite très tôt distincte du judaïsme de Jérusalem, ni du zoroastrisme, lui-même issu du mazdéisme. <![CDATA[<a href="#_dbpedia_2017">(DBpedia, 2017)</a>]]></skos:definition>
    <prov:derivedFrom rdf:resource="http://dbpedia.org/page/Judaism"/>
    <rdfs:comment xml:lang="fr">La description de ce terme est basée sur celle de DBPedia.</rdfs:comment>
    <rdf:type rdf:resource="http://www.w3.org/2004/02/skos/core#Concept"/>
    <skos:inScheme rdf:resource="#Religion"/>
    <skos:broader rdf:resource="#jewishLabel"/>
    <rdfs:isDefinedBy rdf:resource="http://sparql.cwrc.ca/ontologies/cwrc-ONTOLOGY_DATE"/>
    <void:inDataset rdf:resource="#datasetdefinition"/>
    <skos:broaderTransitive rdf:resource="#abrahamicReligions"/>
  </cwrc:Religion>
  <owl:DeprecatedClass rdf:about="#jewishReligion">
    <rdfs:label xml:lang="en">Jewish</rdfs:label>
    <rdfs:label xml:lang="zh-hant">猶太教</rdfs:label>
    <rdfs:label xml:lang="zh-latn-pinyin-x-hanyu">yóu tài jiāo</rdfs:label>
    <rdfs:label xml:lang="zh-latn-pinyin-x-notone">you tai jiao</rdfs:label>
    <rdfs:label xml:lang="zh-latn-wadegile">yu t'ai chiao</rdfs:label>
    <rdfs:label xml:lang="nl">Jodendom</rdfs:label>
    <rdfs:label xml:lang="nl">Joods</rdfs:label>
    <rdfs:label xml:lang="es">Judaísmo</rdfs:label>
    <rdfs:label xml:lang="fr">Judaïsme</rdfs:label>
    <skos:definition xml:lang="en">Refers to the monotheistic religion of the Jewish people, central to which is the belief that the ancient Israelites experienced God's presence in human events. Jews believe that the one God delivered the Israelites out of bondage in Egypt, revealed the structure of communal and individual life to them, and chose them to be a holy nation of people able to set an example for all humankind. The Hebrew Bible and Talmud are the two primary sources for Judaism's spiritual and ethical principles. The religion, which traces its origins to Abraham, places more emphasis on expressing beliefs through ritual rather than through abstract doctrine. The Sabbath, beginning on sunset on Friday and ending at sunset on Saturday, is the central religious observance; there is also an annual cycle of religious festivals and days of fasting. Judaism has had a diverse history of development over almost 4000 years, with a number of resulting branches in modern times, namely Orthodox, Conservative, and Reform. <![CDATA[<a href="#_getty_2017">(Getty, 2017)</a>]]></skos:definition>
    <skos:definition xml:lang="es">Se refiere a la religión monoteista del pueblo judío, para los cuales es central la creencia que los antiguos israelitas experimentaron la presencia de Dios en los eventos humanos. Los judíos creen que el Dios único salvó los israelistas de la esclavitud en Egipto, revelándoles la estructura de la vida comunal e individual y eligiéndolos para ser una nación sagrada de personas capaces de dar un ejemplo para toda la humanidad. La Biblia Hebrea y el Talmud son dos fuentes primarias de la espiritualidad judía y de los principios éticos.Los orígenes de la religión se remontan a los tiempos de Abraham, poniendo mayor énfasis en expresar la creencia con rituales más bien que con doctrinas abstractas. El Shabbat, que comienza con la puesta de sol del viernes y termina con la puesta de sol del sábado, es la observancia religiosa central; hay también un ciclo anual de fiestas religiosas y días de ayuno. El judaísmo ha tenido un desarrollo diverso a lo largo de la historia de casi 4.000 años, con un gran número de ramas resultantes en épocas modernas, concretamente ortodoxas, conservadoras, y reformistas. <![CDATA[<a href="#_getty_2017">(Getty, 2017)</a>]]></skos:definition>
    <skos:definition xml:lang="nl">Verwijst naar de monotheïstische religie van het joodse volk, waarbij het geloof centraal staat dat de oude Israëlieten de aanwezigheid van God ervoeren in menselijke gebeurtenissen. Joden geloven dat één God de Israëlieten uit hun gevangenschap in Egypte heeft bevrijd, de structuur van een gemeenschappelijk en individueel leven aan hen heeft onthuld en hen heeft uitverkoren als een heilig volk dat als voorbeeld moest dienen voor de gehele mensheid. De Hebreeuwse bijbel en de Talmoed zijn de belangrijkste bronnen voor de spirituele en ethische principes van het jodendom. Deze religie, waarvan de oorsprong teruggaat naar de tijd van Abraham, legt meer de nadruk op het tot uitdrukking brengen van het geloof in de vorm van rituelen dan in de vorm van abstracte doctrines. De sabbat, die begint bij zonsondergang op vrijdag en eindigt bij zonsondergang op zaterdag, is een centraal element van de religie; er is ook een jaarlijkse cyclus van religieuze feestdagen en vastendagen. Het jodendom heeft een zeer uiteenlopende ontwikkelingsgeschiedenis die bijna 4000 jaar beslaat en is uitgemond in diverse stromingen: de orthodoxe, conservatieve en reformistische stroming. <![CDATA[<a href="#_getty_2017">(Getty, 2017)</a>]]></skos:definition>
    <skos:definition xml:lang="zh-hant">猶太人的一神論宗教，相信古代以色列人於人類事件中體驗到神的存在。猶太人相信這唯一的神使他們脫離埃及的奴役，向他們揭示公共及個人生活的結構，並選擇他們為聖國子民，以為全人類樹立榜樣。《希伯來聖經(Hebrew Bible)》與《塔爾穆德(Talmud)》為猶太教精神與道德原則的兩大來源。猶太教源於亞伯拉罕，較強調以儀式而非抽象的教條表達信仰。遵循信仰的重心為安息日，從週五的日落開始到週日的日出結束；另外每年還有宗教節慶和齋戒日。猶太教經過將近四千年的發展，衍生出許多現代的分支，即正統派猶太教(Orthodox)、保守派猶太教(Conservative)，與改革派猶太教(Reform.)。 <![CDATA[<a href="#_getty_2017">(Getty, 2017)</a>]]></skos:definition>
    <prov:derivedFrom rdf:resource="http://vocab.getty.edu/aat/300073723"/>
    <rdfs:comment xml:lang="en">The description for this term is indebted to the Getty Art &amp; Architecture Thesaurus.</rdfs:comment>
    <skos:definition xml:lang="fr">Pour l'Encyclopædia Britannica, le mot judaïsme recouvre la religion des Juifs, ainsi que la théologie, la loi et les traditions culturelles du peuple juif, constitué des descendants des Israélites provenant de l'antique terre d'Israël et des quelques minorités les ayant rejoints par la conversion et s'étant mélangées à eux au fil de leur diaspora de deux millénaires. Pour un juif orthodoxe comme Daniel Boyarin, le judaïsme est « l'ensemble des rituels et des autres pratiques, des croyances et des valeurs, des loyautés historiques et politiques qui constituent l'allégeance au peuple d'Israël », mais le judaïsme n’est ni une religion ni une foi, selon Boyarin. Ainsi Bernard-Henri Lévy affirme que « la tâche des Juifs comme tels est d’être irréligieux », dans la mesure où la religion, telle qu'on la conçoit en théologie, édifiée par une croyance, par des dogmes, par une instance suprême, centrale et doctrinale, n’appartient pas à l’esprit du judaïsme, selon lui. Le judaïsme comporte des éléments religieux, mais ne s'y limite pas puisqu'il contient des coutumes non spécifiquement religieuses – outre des codes de conduite, des lois, des rites – et qu’il fonde plus largement encore une « culture juive ». Néanmoins, par convention, on parle habituellement du judaïsme comme d’une « religion », mais il ne faut pas l’entendre au sens strict, selon des historiens des religions comme Simon Claude Mimouni ou Daniel Boyarin, ou des philosophes comme Léo Strauss ou Bernard-Henri Lévy. Selon ses textes fondateurs, en particulier le Tanakh, la foi des anciens Israélites et de leurs descendants les Juifs, est fondée sur une alliance contractée entre Dieu et Abraham, qui a ensuite été renouvelée entre Dieu et Moïse. Les juifs fondent le judaïsme sur la religion abrahamique qui fleurira ensuite dans la Loi mosaïque (la Torah, les Nevi'im et les Ketouvim), collectivement désignés par l'acronyme Tanakh, dont le texte constitue la Miqra ou Bible hébraïque. Cette religion se fonde sur le culte du Dieu d'Abraham, d'Isaac et de Jacob, au Nom ineffable, qu'elle conçoit comme une Essence éternelle (YHWH), qui détient tous les pouvoirs (Elohim), transcendant le Seigneur des Seigneurs (Adonaï) qu'elle considère Un et Unique et qu'elle qualifie ainsi : omnipotent, omniscient, omniprésent, juste et miséricordieux. Cette religion professe aussi que le rassemblement de toutes les puissances (Elohim) manifesta le créateur du monde qui continue de s'impliquer dans sa destinée en faisant irruption dans l'Histoire dont il révèle la dimension d'Histoire Sainte, comme lorsqu'il fit sortir d'Égypte les enfants d'Israël. Les cohanim, ou prêtres, du Temple de Jérusalem, par deux fois détruit, assuraient son culte. Certains groupes juifs, comme les Ésséniens, s'opposaient à la centralité du culte à Jérusalem. La seconde destruction du Temple de Jérusalem et la dispersion des juifs dans le monde donna naissance à plusieurs traditions religieuses juives. Si la majorité des juifs se regroupèrent autour de l'élaboration du Talmud par les rabbanim, un mouvement strictement scripturaliste, dit Karaïsme, s'opposa à la codification de la tradition orale, tandis que d'autres groupes éloignés, comme les Beta d'Israël en Éthiopie, ignorèrent cette évolution et se développèrent en vase clos. Le judaïsme est l'une des plus anciennes traditions religieuses du monothéisme exclusif encore pratiquées aujourd'hui. Les valeurs et l'histoire du peuple juif sont à la source des deux autres religions abrahamiques, le christianisme et l'islam. Il n'est toutefois pas à la base du samaritanisme, qui est une tradition israélite très tôt distincte du judaïsme de Jérusalem, ni du zoroastrisme, lui-même issu du mazdéisme. <![CDATA[<a href="#_dbpedia_2017">(DBpedia, 2017)</a>]]></skos:definition>
    <prov:derivedFrom rdf:resource="http://dbpedia.org/page/Judaism"/>
    <rdfs:comment xml:lang="fr">La description de ce terme est basée sur celle de DBPedia.</rdfs:comment>
    <rdf:type rdf:resource="http://www.w3.org/2004/02/skos/core#Concept"/>
    <skos:inScheme rdf:resource="#Religion"/>
    <skos:broader rdf:resource="#jewishLabel"/>
    <rdfs:isDefinedBy rdf:resource="http://sparql.cwrc.ca/ontologies/cwrc-ONTOLOGY_DATE"/>
    <void:inDataset rdf:resource="#datasetdefinition"/>
    <skos:broaderTransitive rdf:resource="#abrahamicReligions"/>
    <owl:equivalentClass rdf:resource="#judaism"/>
    <dc:isReplacedBy rdf:resource="#judaism"/>
    <vs:term_status xml:lang="en">deprecated</vs:term_status>
  </owl:DeprecatedClass>
  <cwrc:Religion rdf:about="#presbyterianism">
    <rdfs:label xml:lang="en">Presbyterianism</rdfs:label>
    <rdfs:label xml:lang="zh-hant">長老宗</rdfs:label>
    <rdfs:label xml:lang="zh-hant">長老制</rdfs:label>
    <rdfs:label xml:lang="zh-hant">長老教會</rdfs:label>
    <rdfs:label xml:lang="zh-latn-pinyin-x-hanyu">zhǎng lǎo zōng</rdfs:label>
    <rdfs:label xml:lang="zh-latn-pinyin-x-notone">zhang lao zong</rdfs:label>
    <rdfs:label xml:lang="zh-latn-wadegile">chang lao tsung</rdfs:label>
    <rdfs:label xml:lang="nl">Presbyterianisme</rdfs:label>
    <rdfs:label xml:lang="nl">Prebyteriaan</rdfs:label>
    <rdfs:label xml:lang="es">Presbiterianismo</rdfs:label>
    <rdfs:label xml:lang="fr">Presbytarianisme</rdfs:label>
    <skos:definition xml:lang="en">One of the main Protestant groups that arose out of the 16th-century Reformation. Generally speaking, modern Presbyterian churches trace their origins to the Calvinist churches of the British Isles, the European counterparts of which came to be known by the more inclusive name of Reformed. The term presbyterian also denotes a collegiate type of church government led by pastors and lay leaders called elders or presbyters. Strictly speaking, all Presbyterian churches are a part of the Reformed, or Calvinist, tradition, although not all Reformed churches are presbyterian in their form of government. <![CDATA[<a href="#_getty_2017">(Getty, 2017)</a>]]></skos:definition>
    <skos:definition xml:lang="nl">Een van de belangrijkste protestantse groeperingen die voortkwamen uit de 16de-eeuwse Reformatie. In het algemeen hebben moderne presbyteriaanse kerken hun oorsprong in de calvinistische kerken op de Britse eilanden, waarvan de Europese tegenhangers bekend zijn geworden onder de meer algemene naam 'gereformeerden'. De term 'presbyteriaans' verwijst ook naar een collegiaal type kerkbestuur onder leiding van pastors en leken die ouderlingen of presbyters worden genoemd. Strikt genomen maken alle presbyteriaanse kerken deel uit van de gereformeerde of calvinistische traditie, maar zijn niet alle gereformeerde kerken presbyteriaans in hun bestuursvorm. <![CDATA[<a href="#_getty_2017">(Getty, 2017)</a>]]></skos:definition>
    <skos:definition xml:lang="es">Uno de los principales grupos protestantes que surgió de la Reforma del siglo XVI. Hablando en general, las Iglesias Presbiterianas modernas señalan sus orígenes en las iglesias calvinistas de las Islas Británicas, la contraparte Europea la que fue conocida por el nombre más global de &quot;Reformada&quot;. El término presbiterianismo también denota un tipo colegiado de gobierno de iglesia liderado por el pastor y lideres laicos llamados ancianos o presbiteros. Estrictamente hablando, todas las iglesias presbiterianas son parte de la Iglesia .El término presbiterianismo también denota un tipo colegiado de gobierno de iglesia liderado por el pastor y lideres laicos llamados ancianos o presbiteros. Estrictamente hablando, todas las iglesias presbiterianas son parte de la Reforma o Calvinismo, tradición, aunque no todas las iglesias Reformadas son presbiterianas en su gubernamentalidad. <![CDATA[<a href="#_getty_2017">(Getty, 2017)</a>]]></skos:definition>
    <skos:definition xml:lang="zh-hant">自十六世紀宗教改革興起的主要新教團體的一派。一般說來，現代的長老教會可追溯至不列顛群島的喀爾文(Calvinis)教派，其在歐洲的對應教派則被稱為較具涵蓋性的歸正派(Reformed)。長老教會一詞，亦表示其管理方式如同大學，由稱作長老或教士的牧師及信徒領導。嚴格來說，所有長老教會皆為歸正派或喀爾文教派傳統的一部分，但並非所有歸正教會的管理方式皆如同長老教會一般。 <![CDATA[<a href="#_getty_2017">(Getty, 2017)</a>]]></skos:definition>
    <prov:derivedFrom rdf:resource="http://vocab.getty.edu/aat/300153854"/>
    <rdfs:comment xml:lang="en">The description for this term is indebted to the Getty Art &amp; Architecture Thesaurus.</rdfs:comment>
    <skos:definition xml:lang="fr">Le presbytérianisme est une forme du protestantisme liée à l'Écosse. <![CDATA[<a href="#_dbpedia_2017">(DBpedia, 2017)</a>]]></skos:definition>
    <prov:derivedFrom rdf:resource="http://dbpedia.org/page/Presbyterianism"/>
    <rdfs:comment xml:lang="fr">La description de ce terme est basée sur celle de DBPedia.</rdfs:comment>
    <rdf:type rdf:resource="http://www.w3.org/2004/02/skos/core#Concept"/>
    <skos:inScheme rdf:resource="#Religion"/>
    <skos:broaderTransitive rdf:resource="#christianity"/>
    <rdfs:isDefinedBy rdf:resource="http://sparql.cwrc.ca/ontologies/cwrc-ONTOLOGY_DATE"/>
    <void:inDataset rdf:resource="#datasetdefinition"/>
  </cwrc:Religion>
  <cwrc:Religion rdf:about="#protestantism">
    <rdfs:label xml:lang="en">Protestantism</rdfs:label>
    <rdfs:label xml:lang="zh-hant">新教</rdfs:label>
    <rdfs:label xml:lang="zh-hant">抗羅宗</rdfs:label>
    <rdfs:label xml:lang="zh-latn-pinyin-x-hanyu">xīn jiāo</rdfs:label>
    <rdfs:label xml:lang="zh-latn-pinyin-x-notone">xin jiao</rdfs:label>
    <rdfs:label xml:lang="zh-latn-wadegile">hsin chiao</rdfs:label>
    <rdfs:label xml:lang="nl">protestantisme</rdfs:label>
    <rdfs:label xml:lang="nl">protestant</rdfs:label>
    <rdfs:label xml:lang="es">protestantismo</rdfs:label>
    <rdfs:label xml:lang="fr">protestantisme</rdfs:label>
    <skos:definition xml:lang="en">The general term for types of Christian faith originating from the Reformation. Although the early forms of Protestantism were those who followed Luther, Calvin, and Zwingli, the term now includes most non-Roman Catholic or non-Orthodox denominations. Protestants want to be closer to the style of faith of the early Church which they feel has been obscured in Catholic practices. The term derives from the word 'protestari' which means not only to protest but to avow or confess. Common characteristics of Protestantism include the justification by faith alone, the authority of scripture, and the priesthood of all believers, in which not only the clergy are able to hear the confession of sin. <![CDATA[<a href="#_getty_2017">(Getty, 2017)</a>]]></skos:definition>
    <skos:definition xml:lang="es">El término general para tipos de fe cristiana originadas a partir de la Reforma. Aunque las formas tempranas del protestantismo fueron aquellas que obedecían a Lutero, Calvino y Zwinglio, el término ahora incluye la mayoría de las denominaciones no Romanas o no Ortodoxas. El caracter común de los protestantes incluye la justificación de la fe por la fe, la autoridad de la sagrada escritura  y el sacerdocio de todos los fieles, por el que cada creyente puede oir la confesión de los pecados, no siendo exclusivo del clero. protestantes quieren estar cerca al estilo de fe de la primera Iglesia el cual sienten ha sido opacado en las prácticas católicas. El término deriva desde la palabra &quot;protestari&quot; que significa no sólo protestar sino que reconocer o confesar. Característica común. <![CDATA[<a href="#_getty_2017">(Getty, 2017)</a>]]></skos:definition>
    <skos:definition xml:lang="nl">De algemene term voor typen christelijk geloof die zijn ontstaan tijdens de Reformatie. Hoewel de vroegste vormen van protestantisme werden beoefend door de volgelingen van Luther, Calvijn en Zwingli, wordt de term tegenwoordig gebruikt voor de meeste overtuigingen die niet rooms-katholiek of orthodox zijn. Protestanten willen dichter bij de geloofsstijl van de vroege kerk staan, die volgens hen in de katholieke praktijk overschaduwd is geraakt. De term is afkomstig van het woord 'protestari', wat niet alleen 'protesteren' betekent, maar ook 'belijden'. Enkele algemene kenmerken van het protestantisme zijn: rechtvaardiging door het geloof alleen, de berusting van alle gezag bij de Bijbel en de leer dat alle gelovigen zelf hun zonden aan God kunnen belijden, waarbij het aanhoren van de biecht niet alleen aan priesters is voorbehouden. <![CDATA[<a href="#_getty_2017">(Getty, 2017)</a>]]></skos:definition>
    <skos:definition xml:lang="zh-hant">泛稱源自宗教改革的各式基督信仰。雖然早期的新教形式是指遵循路德(Luther)、喀爾文(Calvin)，以及茨溫利(Zwingli)的派別，但現在新教這個詞彙包含了大部分非羅馬天主教或非正教的派別。新教徒希望能更接近早期教會信仰，認為天主教將之變得晦澀難解。本詞彙衍生自”protestari”，不僅意指抗議，更要坦白或懺悔。新教的常見特色包括因純信而稱義、經典的權威性、信徒皆牧師，所以不是只有牧師才能聽取認罪懺悔。 <![CDATA[<a href="#_getty_2017">(Getty, 2017)</a>]]></skos:definition>
    <prov:derivedFrom rdf:resource="http://vocab.getty.edu/aat/300073735"/>
    <skos:definition xml:lang="fr">Le protestantisme est l'une des principales branches du christianisme avec le catholicisme et l'orthodoxie. Entendu largement, le protestantisme est l'ensemble des groupements « issus, directement ou non, de la Réforme et qui rejettent l'autorité du pape ». Selon cette perspective, le protestantisme englobe des mouvements variés allant des luthériens passant par les évangéliques, jusqu'aux quakers. <![CDATA[<a href="#_getty_2017">(DBpedia, 2017)</a>]]></skos:definition>
    <prov:derivedFrom rdf:resource="http://dbpedia.org/page/Protestantism"/>
    <rdf:type rdf:resource="http://www.w3.org/2004/02/skos/core#Concept"/>
    <rdfs:comment xml:lang="en">The description for this term is indebted to the Getty Art &amp; Architecture Thesaurus.</rdfs:comment>
    <skos:inScheme rdf:resource="#Religion"/>
    <skos:broaderTransitive rdf:resource="#christianity"/>
    <rdfs:isDefinedBy rdf:resource="http://sparql.cwrc.ca/ontologies/cwrc-ONTOLOGY_DATE"/>
    <void:inDataset rdf:resource="#datasetdefinition"/>
  </cwrc:Religion>
  <cwrc:Religion rdf:about="#agnosticism">
    <rdfs:label xml:lang="en">Agnosticism</rdfs:label>
    <rdfs:label xml:lang="fr">agnosticisme</rdfs:label>
    <skos:definition xml:lang="en">Agnosticism is the view that, the truth values of certain claims – especially metaphysical and religious claims such as whether God, the divine or the supernatural exist – are unknown and perhaps unknowable. According to the philosopher William L. Rowe: "In the popular sense of the term, an agnostic is someone who neither believes nor disbelieves in God, whereas an atheist disbelieves in God." Agnosticism is a doctrine or set of tenets rather than a religion as such. Thomas Henry Huxley, an English biologist, coined the word "agnostic" in 1869.Earlier thinkers, however, had written works that promoted agnostic points of view, such as Sanjaya Belatthaputta, a 5th-century BCE Indian philosopher who expressed agnosticism about any afterlife; and Protagoras, a 5th-century BCE Greek philosopher who expressed agnosticism about "the gods". The Nasadiya Sukta in the Rigveda is agnostic about the origin of the universe. <![CDATA[<a href="#_dbpedia_2017">(DBpedia, 2017)</a>]]></skos:definition>
    <skos:definition xml:lang="fr">L’agnosticisme ou pensée de l'interrogation est une attitude de pensée considérant la vérité de certaines propositions concernant notamment l'existence de Dieu ou des dieux comme inconnaissable : à la différence des croyants, considérant probable ou certaine l'existence de telles divinités, ou des athées l'estimant improbable ou impossible, les agnostiques refusent de trancher. Si le degré de scepticisme varie selon les individus, les agnostiques s'accordent pour dire qu'il n'existe pas de preuve définitive en faveur de l'existence ou de l'inexistence du divin, et affirment l'impossibilité de se prononcer. Si les agnostiques refusent de se prononcer quant à l'existence d'une intelligence supérieure, ils n'accordent, en revanche, ou du moins tendent à n'accorder, aucune transcendance et aucune valeur sacrée aux religions (prophète, messie, textes sacrés...) et à leurs institutions (clergé, rituels et prescriptions diverses...). Ceux-ci voient en effet les religions comme de pures constructions sociales et culturelles qui auraient surtout pour fonction historique d'assurer la cohésion et l'ordre dans les sociétés humaines traditionnelles via par exemple la menace de l'enfer, la promesse du paradis ou encore la notion de péché ou par le mécanisme du bouc émissaire. En d'autres termes, les religions, aux yeux d'un agnostique, seraient bien trop « humaines » de par leurs modes de fonctionnement et de par les dynamiques anthropologiques sur lesquelles elles se basent (soutien psychologique face à la mort, analogie très anthropocentrique d'un Dieu bâtisseur de l'univers...) pour qu'elles aient un quelconque lien direct avec toute forme d'intelligence supérieure, tout en n'excluant pas non plus pour certains le fait que ce soit malgré tout possible. D'où cette interrogation constante propre à l'agnostique. <![CDATA[<a href="#_dbpedia_2017">(DBpedia, 2017)</a>]]></skos:definition>
    <rdf:type rdf:resource="http://www.w3.org/2004/02/skos/core#Concept"/>
    <skos:inScheme rdf:resource="#Religion"/>
    <rdfs:isDefinedBy rdf:resource="http://sparql.cwrc.ca/ontologies/cwrc-ONTOLOGY_DATE"/>
    <void:inDataset rdf:resource="#datasetdefinition"/>
    <skos:broaderTransitive rdf:resource="#occultism"/>
  </cwrc:Religion>
  <cwrc:Religion rdf:about="#atheism">
    <rdfs:label xml:lang="en">Atheism</rdfs:label>
    <rdfs:label xml:lang="fr">athéisme</rdfs:label>
    <skos:definition xml:lang="en">Atheism is, in a broad sense, the rejection of belief in the existence of deities. In a narrower sense, atheism is specifically the position that there are no deities. Most inclusively, atheism is the absence of belief that any deities exist. Atheism is contrasted with theism, which, in its most general form, is the belief that at least one deity exists. The term "atheism" originated from the Greek ἄθεος (atheos), meaning &quot;without god(s)&quot;, used as a pejorative term applied to those thought to reject the gods worshiped by the larger society. With the spread of freethought, skeptical inquiry, and subsequent increase in criticism of religion, application of the term narrowed in scope. The first individuals to identify themselves using the word &quot;atheist&quot; lived in the 18th century during the Age of Enlightenment. The French Revolution, noted for its &quot;unprecedented atheism,&quot; witnessed the first major political movement in history to advocate for the supremacy of human reason. Arguments for atheism range from the philosophical to social and historical approaches. Rationales for not believing in deities include arguments that there is a lack of empirical evidence; the problem of evil; the argument from inconsistent revelations; the rejection of concepts that cannot be falsified; and the argument from nonbelief. Although some atheists have adopted secular philosophies (eg. humanism and skepticism), there is no one ideology or set of behaviors to which all atheists adhere. Many atheists hold that atheism is a more parsimonious worldview than theism and therefore that the burden of proof lies not on the atheist to disprove the existence of God but on the theist to provide a rationale for theism. Since conceptions of atheism vary, accurate estimations of current numbers of atheists are difficult. Several comprehensive global polls on the subject have been conducted by Gallup International: their 2015 poll featured over 64,000 respondents and indicated that 11% were &quot;convinced atheists&quot; whereas an earlier 2012 poll found that 13% of respondents were &quot;convinced atheists.&quot; An older survey by the BBC, in 2004, recorded atheists as comprising 8% of the world's population. Other older estimates have indicated that atheists comprise 2% of the world's population, while the irreligious add a further 12%. According to these polls, Europe and East Asia are the regions with the highest rates of atheism. In 2015, 61% of people in China reported that they were atheists. The figures for a 2010 Eurobarometer survey in the European Union (EU) reported that 20% of the EU population claimed not to believe in &quot;any sort of spirit, God or life force&quot;. <![CDATA[<a href="#_dbpedia_2017">(DBpedia, 2017)</a>]]></skos:definition>
    <skos:definition xml:lang="fr">L’athéisme est une attitude ou une doctrine qui nie l’existence de quelque dieu ou divinité que ce soit, contrairement, par exemple, au déisme et au théisme qui soutiennent ces existences, ou à l’agnosticisme qui considère que personne ne peut répondre à ces questions. C'est une position philosophique qui peut être formulée ainsi : il n'existe rien qui ressemble de près ou de loin à ce que les croyants appellent un « dieu », ou « Dieu ». <![CDATA[<a href="#_dbpedia_2017">(DBpedia, 2017)</a>]]></skos:definition>
    <prov:derivedFrom rdf:resource="http://dbpedia.org/page/Atheism"/>
    <rdfs:comment xml:lang="fr">La description de ce terme est basée sur celle de DBPedia.</rdfs:comment>
    <rdf:type rdf:resource="http://www.w3.org/2004/02/skos/core#Concept"/>
    <skos:inScheme rdf:resource="#Religion"/>
    <rdfs:isDefinedBy rdf:resource="http://sparql.cwrc.ca/ontologies/cwrc-ONTOLOGY_DATE"/>
    <void:inDataset rdf:resource="#datasetdefinition"/>
  </cwrc:Religion>
  <cwrc:Religion rdf:about="#churchOfEngland">
    <rdfs:label xml:lang="en">Church of England</rdfs:label>
    <rdfs:label xml:lang="fr"/>
    <skos:definition xml:lang="en"/>
    <skos:definition xml:lang="fr"/>
    <rdf:type rdf:resource="http://www.w3.org/2004/02/skos/core#Concept"/>
    <rdf:type rdf:resource="http://xmlns.com/foaf/0.1/Organization"/>
    <skos:inScheme rdf:resource="#Religion"/>
    <skos:broaderTransitive rdf:resource="#christianity"/>
    <rdfs:isDefinedBy rdf:resource="http://sparql.cwrc.ca/ontologies/cwrc-ONTOLOGY_DATE"/>
    <void:inDataset rdf:resource="#datasetdefinition"/>
  </cwrc:Religion>
  <cwrc:Religion rdf:about="#congregationalChurch">
    <rdfs:label xml:lang="en">Congregational Church</rdfs:label>
    <rdfs:label xml:lang="fr">Églises congrégationalistes</rdfs:label>
    <skos:definition xml:lang="en">Congregational churches are Protestant Christian churches practicing congregationalist church governance, in which each congregation independently and autonomously runs its own affairs. Congregationalism is often considered to be a part of the wider Reformed tradition. Many Congregational churches claim their descent from Protestant denominations formed on a theory of union published by the theologian Robert Browne in 1582. These arose from the ideas of nonconforming Protestants during the Puritan Reformation of the Church of England. In Great Britain, the early Congregationalists were called Separatists or Independents to distinguish them from the similarly Calvinistic Presbyterians. Congregational churches were widely established in the Plymouth Colony and the Massachusetts Bay Colony (later New England), and together wrote the Cambridge Platform of 1648 which described the autonomy of the church and its association with others. Within the United States, the model of Congregational churches was carried by migrating settlers from New England into New York, then into the Old North West, and further. With their insistence on independent local bodies, they became important in many social reform movements, including abolitionism, temperance, and women's suffrage. Modern Congregationalism in the United States is largely split into three bodies: the United Church of Christ, the National Association of Congregational Christian Churches and the Conservative Congregational Christian Conference, which is the most theologically conservative. Congregationalism, as defined by the Pew Research Center, is estimated to represent 0.5% of the worldwide Protestant population. <![CDATA[<a href="#_dbpedia_2017">(DBpedia, 2017)</a>]]></skos:definition>
    <skos:definition xml:lang="fr">Les Églises congrégationalistes sont des églises protestantes de tradition réformée, pratiquant une forme d’organisation d’église où chaque paroisse se gère de manière entièrement autonome et indépendante. Le congrégationalisme se caractérise plus comme un mouvement que comme une dénomination chrétienne en raison de sa conviction fondamentale en faveur de l’autonomie complète de chaque paroisse. Malgré la forte diversité théologique inhérente à leur forme d'organisation, la plupart des congrégationalistes se considèrent d'abord comme des réformés, soit traditionnels soit néo-orthodoxes (barthiens). Les congrégationalistes, selon la définition du centre de recherche indépendant Pew Research Center, représentent environ 0,5% de la population protestante mondiale, soit 4 millions de chrétiens répartis essentiellement dans les grands pays anglophones (Royaume-Uni, États-Unis, Canada, Australie, Afrique du sud, Irlande) et dans quelques « terres de mission » (Argentine, Bulgarie, Îles Samoa). Leur rôle historique et leur influence, notamment aux États-Unis, excèdent largement ces chiffres. <![CDATA[<a href="#_dbpedia_2017">(DBpedia, 2017)</a>]]></skos:definition>
    <prov:derivedFrom rdf:resource="http://dbpedia.org/page/Congregational_church"/>
    <rdfs:comment xml:lang="fr">La description de ce terme est basée sur celle de DBPedia.</rdfs:comment>
    <rdf:type rdf:resource="http://www.w3.org/2004/02/skos/core#Concept"/>
    <skos:inScheme rdf:resource="#Religion"/>
    <skos:broaderTransitive rdf:resource="#christianity"/>
    <rdfs:isDefinedBy rdf:resource="http://sparql.cwrc.ca/ontologies/cwrc-ONTOLOGY_DATE"/>
    <void:inDataset rdf:resource="#datasetdefinition"/>
  </cwrc:Religion>
  <cwrc:Religion rdf:about="#churchOfIreland">
    <rdfs:label xml:lang="en">Church of Ireland</rdfs:label>
    <rdfs:label xml:lang="fr">Église d'Irlande</rdfs:label>
    <skos:definition xml:lang="en">The Church of Ireland (Irish: Eaglais na hÉireann Scots: Kirk o Airlann) is a Christian church in Ireland and an autonomous province of the Anglican Communion. It is organised on an all-Ireland basis and is the second-largest Christian church on the island after the Catholic Church. Like other Anglican churches, it has retained elements of pre-Reformation practice, notably its episcopal polity, while rejecting the primacy of the Bishop of Rome. Nevertheless, in theological and liturgical matters, it incorporates many principles of the Reformation, particularly those espoused during the English Reformation. The church self identifies as being both Catholic and Reformed. Within the church, differences exist between those members who are more Catholic-leaning (high church) and those who are more Protestant-leaning (low church or evangelical). For historical and cultural reasons, the Church of Ireland is generally identified as a Protestant church. The Church of Ireland is the second-largest in the Republic of Ireland, with around 130,000 members, and the third-largest in Northern Ireland, with around 260,000 members. <![CDATA[<a href="#_dbpedia_2017">(DBpedia, 2017)</a>]]></skos:definition>
    <skos:definition xml:lang="fr">L'Église d'Irlande (irlandais : Eaglais na hÉireann, anglais : Church of Ireland) est une communauté religieuse autonome de la communion anglicane, dont le rayon d'action touche la République d'Irlande et l'Irlande du Nord. Comme d'autres Églises anglicanes, elle s'affirme « catholique » et « réformée ». Quand l'Église d'Angleterre rompt avec le Pape et l'Église catholique romaine, l'Église d'Irlande évolue également vers la Réforme, gardant son statut juridique et ses possessions, si sa doctrine change. Ainsi, de nos jours, l'Église, dans ses cathédrales et ses églises, conserve largement l'héritage des constructions médiévales de l'île. La nouvelle Église indépendante n'est cependant pas suivie par la majorité de la population ; l'Église catholique romaine conserve le soutien de la plus grande partie des habitants, et ce jusqu'à aujourd'hui. En dépit de son caractère minoritaire, cependant, l'Église d'Irlande conserve le statut de religion d'État jusqu'au désétablissement de 1869, quand Gladstone abolit l'Acte d'établissement. Le nombre d'églises est tombé brusquement au cours du XXe siècle, particulièrement en République d'Irlande, après l'indépendance ; le dernier recensement de la République montre un exemple rare de résistance à la crise de la foi. Aujourd'hui, l'Église d'Irlande est, après l'Église catholique, la deuxième plus importante Église de l'île d'Irlande. C'est également la plus importante Église protestante de la République d'Irlande et le deuxième plus importante d'Irlande du Nord, après l'Église presbytérienne d'Irlande. Elle est gouvernée par un synode général du clergé et des laïcs et organisée en douze diocèses. Elle a à sa tête l'archevêque d'Armagh, qui porte le titre de "Primat de toute l'Irlande". L'archevêque actuel est Richard Clarke qui a succédé le à Alan Harper ; l'autre archevêque est celui de Dublin John Neill. <![CDATA[<a href="#_dbpedia_2017">(DBpedia, 2017)</a>]]></skos:definition>
    <prov:derivedFrom rdf:resource="http://dbpedia.org/page/Church_of_Ireland"/>
    <rdfs:comment xml:lang="fr">La description de ce terme est basée sur celle de DBPedia.</rdfs:comment>
    <rdf:type rdf:resource="http://www.w3.org/2004/02/skos/core#Concept"/>
    <skos:inScheme rdf:resource="#Religion"/>
    <skos:broaderTransitive rdf:resource="#christianity"/>
    <rdfs:isDefinedBy rdf:resource="http://sparql.cwrc.ca/ontologies/cwrc-ONTOLOGY_DATE"/>
    <void:inDataset rdf:resource="#datasetdefinition"/>
  </cwrc:Religion>
  <cwrc:Religion rdf:about="#dissenters">
    <rdfs:label xml:lang="en">Dissenters</rdfs:label>
    <rdfs:label xml:lang="fr">dissidents (ou non-conformistes)</rdfs:label>
    <skos:definition xml:lang="en"/>
    <skos:definition xml:lang="fr"/>
    <rdf:type rdf:resource="http://www.w3.org/2004/02/skos/core#Concept"/>
    <skos:inScheme rdf:resource="#Religion"/>
    <rdfs:isDefinedBy rdf:resource="http://sparql.cwrc.ca/ontologies/cwrc-ONTOLOGY_DATE"/>
    <void:inDataset rdf:resource="#datasetdefinition"/>
    <skos:broaderTransitive rdf:resource="#churchOfEngland"/>
  </cwrc:Religion>
  <cwrc:Religion rdf:about="#dissentingChurches">
    <rdfs:label xml:lang="en">Dissenting Churches</rdfs:label>
    <rdfs:label xml:lang="fr">Églises dissidentes</rdfs:label>
    <skos:definition xml:lang="en"/>
    <skos:definition xml:lang="fr"/>
    <rdf:type rdf:resource="http://www.w3.org/2004/02/skos/core#Concept"/>
    <skos:inScheme rdf:resource="#Religion"/>
    <rdfs:isDefinedBy rdf:resource="http://sparql.cwrc.ca/ontologies/cwrc-ONTOLOGY_DATE"/>
    <void:inDataset rdf:resource="#datasetdefinition"/>
    <skos:broaderTransitive rdf:resource="#churchOfEngland"/>
  </cwrc:Religion>
  <cwrc:Religion rdf:about="#fifthMonarchists">
    <rdfs:label xml:lang="en">Fifth Monarchists</rdfs:label>
    <rdfs:label xml:lang="fr">Cinquièmes Monarchistes</rdfs:label>
    <skos:definition xml:lang="en">The Fifth Monarchists or Fifth Monarchy Men were active from 1649 to 1660 during the Interregnum, following the English Civil Wars of the 17th century. They took their name from a prophecy in the Book of Daniel that four ancient monarchies (Babylonian, Persian, Macedonian, and Roman) would precede the kingdom of Christ. They also referred to the year 1666 and its relationship to the biblical Number of the Beast indicating the end of earthly rule by carnal human beings. They were one of a number of nonconformist dissenting groups that emerged around this time. <![CDATA[<a href="#_dbpedia_2017">(DBpedia, 2017)</a>]]></skos:definition>
    <skos:definition xml:lang="fr">Les hommes de la Cinquième Monarchie, ou Cinquièmes Monarchistes (Fifth Monarchy Men ou Fifth Monarchists en anglais) sont une faction idéologique de la Première Révolution anglaise, active de 1649 à 1661. Ils tiennent leur nom de leur croyance en la fondation prochaine d'un royaume planétaire par Jésus retournant sur terre. <![CDATA[<a href="#_dbpedia_2017">(DBpedia, 2017)</a>]]></skos:definition>
    <prov:derivedFrom rdf:resource="http://dbpedia.org/page/Fifth_Monarchists"/>
    <rdfs:comment xml:lang="fr">La description de ce terme est basée sur celle de DBPedia.</rdfs:comment>
    <rdf:type rdf:resource="http://www.w3.org/2004/02/skos/core#Concept"/>
    <skos:broaderTransitive rdf:resource="#millenarianism"/>
    <skos:inScheme rdf:resource="#Religion"/>
    <rdfs:isDefinedBy rdf:resource="http://sparql.cwrc.ca/ontologies/cwrc-ONTOLOGY_DATE"/>
    <void:inDataset rdf:resource="#datasetdefinition"/>
    <skos:broaderTransitive rdf:resource="#dissenters"/>
  </cwrc:Religion>
  <cwrc:Religion rdf:about="#lollards">
    <rdfs:label xml:lang="en">Lollards</rdfs:label>
    <rdfs:label xml:lang="fr">Lollards</rdfs:label>
    <skos:definition xml:lang="en">Lollardy (Lollardry, Lollardism) was a political and religious movement that existed from the mid-14th century to the English Reformation. It was initially led by John Wycliffe, a prominent theologian who was dismissed from the University of Oxford in 1381 for criticism of the Church, especially in his doctrine on the Eucharist. The Lollards' demands were primarily for reform of Western Christianity. <![CDATA[<a href="#_dbpedia_2017">(DBpedia, 2017)</a>]]></skos:definition>
    <skos:definition xml:lang="fr">Les Lollards sont les membres ou sympathisants d'un mouvement de contestation religieuse et sociale apparu en Angleterre au XIVe siècle. — John Ball <![CDATA[<a href="#_dbpedia_2017">(DBpedia, 2017)</a>]]> </skos:definition>
    <prov:derivedFrom rdf:resource="http://dbpedia.org/resource/Lollardy"/>
    <rdfs:comment xml:lang="fr">La description de ce terme est basée sur celle de DBPedia.</rdfs:comment>
    <rdf:type rdf:resource="http://www.w3.org/2004/02/skos/core#Concept"/>
    <skos:inScheme rdf:resource="#Religion"/>
    <rdfs:isDefinedBy rdf:resource="http://sparql.cwrc.ca/ontologies/cwrc-ONTOLOGY_DATE"/>
    <void:inDataset rdf:resource="#datasetdefinition"/>
    <skos:broaderTransitive rdf:resource="#catholicChurch"/>
  </cwrc:Religion>
  <cwrc:Religion rdf:about="#methodistChurch">
    <rdfs:label xml:lang="en">Methodist Church</rdfs:label>
    <rdfs:label xml:lang="fr">Église méthodiste</rdfs:label>
    <skos:definition xml:lang="en"/>
    <skos:definition xml:lang="fr"/>
    <rdf:type rdf:resource="http://www.w3.org/2004/02/skos/core#Concept"/>
    <skos:inScheme rdf:resource="#Religion"/>
    <skos:broaderTransitive rdf:resource="#christianity"/>
    <rdfs:isDefinedBy rdf:resource="http://sparql.cwrc.ca/ontologies/cwrc-ONTOLOGY_DATE"/>
    <void:inDataset rdf:resource="#datasetdefinition"/>
  </cwrc:Religion>
  <cwrc:Religion rdf:about="#millenarianism">
    <rdfs:label xml:lang="en">Millenarianism</rdfs:label>
    <rdfs:label xml:lang="fr">millénarisme, ou chiliasme</rdfs:label>
    <skos:definition xml:lang="en">Millenarianism (also millenarism), from Latin mīllēnārius "containing a thousand", is the belief by a religious, social, or political group or movement in a coming major transformation of society, after which all things will be changed. Millenarianism is a concept or theme that exists in many cultures and religions. <![CDATA[<a href="#_dbpedia_2017">(DBpedia, 2017)</a>]]></skos:definition>
    <skos:definition xml:lang="fr">Le millénarisme, ou chiliasme (ou encore, mais de façon erronée, chialisme), est une doctrine religieuse qui soutient l'idée d'un règne terrestre du Messie, après que celui-ci aura chassé l'Antéchrist et préalablement au Jugement dernier.Cette pensée est présente dans certains courants du judaïsme, dans l'Apocalypse de Jean, dans les écrits des Pères apostoliques et dans l'islam sunnite et chiite.Toujours par extension, le mot peut servir à désigner dans le langage courant des types de pensée non plus religieuses mais politiques. <![CDATA[<a href="#_dbpedia_2017">(DBpedia, 2017)</a>]]></skos:definition>
    <prov:derivedFrom rdf:resource="http://dbpedia.org/resource/Millenarianism"/>
    <rdfs:comment xml:lang="fr">La description de ce terme est basée sur celle de DBPedia.</rdfs:comment>
    <rdf:type rdf:resource="http://www.w3.org/2004/02/skos/core#Concept"/>
    <skos:inScheme rdf:resource="#Religion"/>
    <rdfs:isDefinedBy rdf:resource="http://sparql.cwrc.ca/ontologies/cwrc-ONTOLOGY_DATE"/>
    <void:inDataset rdf:resource="#datasetdefinition"/>
    <skos:broaderTransitive rdf:resource="#occultism"/>
  </cwrc:Religion>
  <cwrc:Religion rdf:about="#neo-thomism">
    <rdfs:label xml:lang="en">Neo-thomism</rdfs:label>
    <rdfs:label xml:lang="fr">néothomisme</rdfs:label>
    <skos:definition xml:lang="en">Neo-Scholasticism (also known as neo-scholastic Thomism or neo-Thomism because of the great influence of the writings of St. Thomas Aquinas on the movement), is a revival and development of medieval scholasticism in Roman Catholic theology and philosophy which began in the second half of the 19th century. <![CDATA[<a href="#_dbpedia_2017">(DBpedia, 2017)</a>]]></skos:definition>
    <prov:derivedFrom rdf:resource="http://dbpedia.org/page/Neo-Scholasticism"/>
    <rdfs:comment xml:lang="fr">La description de ce terme est basée sur celle de DBPedia.</rdfs:comment>
    <skos:definition xml:lang="fr"/>
    <rdf:type rdf:resource="http://www.w3.org/2004/02/skos/core#Concept"/>
    <skos:inScheme rdf:resource="#Religion"/>
    <rdfs:isDefinedBy rdf:resource="http://sparql.cwrc.ca/ontologies/cwrc-ONTOLOGY_DATE"/>
    <void:inDataset rdf:resource="#datasetdefinition"/>
    <skos:broaderTransitive rdf:resource="#catholicChurch"/>
  </cwrc:Religion>
  <cwrc:Religion rdf:about="#occultism">
    <rdfs:label xml:lang="en">Occultism/Theosophism</rdfs:label>
    <rdfs:label xml:lang="fr">occultisme</rdfs:label>
    <skos:definition xml:lang="en">Any religious or philosophic ideology based on mystical insight into the nature of God and/or divine truth. This insight is attained only through direct experience of the divine. The term is sometimes used to specifically refer to the principles of the Theosophical Society founded in New York in 1875 by Madame Blavatsky and H. S. Olcott which incorporated aspects of Buddhism and Brahmanism.</skos:definition>
    <!-- Missing source -->
    <skos:definition xml:lang="fr"/>
    <rdf:type rdf:resource="http://www.w3.org/2004/02/skos/core#Concept"/>
    <skos:inScheme rdf:resource="#Religion"/>
    <rdfs:isDefinedBy rdf:resource="http://sparql.cwrc.ca/ontologies/cwrc-ONTOLOGY_DATE"/>
    <void:inDataset rdf:resource="#datasetdefinition"/>
  </cwrc:Religion>
  <cwrc:Religion rdf:about="#pagan">
    <rdfs:label xml:lang="en">Pagan</rdfs:label>
    <rdfs:label xml:lang="fr">païen (ou payen)</rdfs:label>
    <skos:definition xml:lang="en">Paganism is a term that developed among the Christian community of southern Europe during late antiquity to describe religions other than their own, Judaism, or Islam–the three Abrahamic religions. Throughout Christendom, it continued to be used, typically in a derogatory sense. In the 19th century, it was re-adopted as a self-descriptor by members of various artistic groups inspired by the ancient world. In the 20th century, it came to be applied as a self-description by practitioners of contemporary pagan, or neo-pagan, religious movements. There has been much scholarly argument as to the origin of the term paganism. Paganism has also been understood by some[who?] to include any non-Abrahamic religions, but this is generally[who?] seen as insulting by adherents of those religions. While paganism is often considered to exclude monotheism and to express a worldview that is pantheistic, polytheistic, or animistic, there are some monotheistic pagans. Once monotheistic religions, such as Christianity and Islam, started to become more prominent (in processes known as Christianization and Islamization), names to encompass polytheistic worshipers started to develop; some of these include Hellene, pagan, and heathen, and at times these names were used as slurs. Modern knowledge of old pagan religions comes from several sources, including: anthropological field research records, the evidence of archaeological artifacts, and the historical accounts of ancient writers regarding cultures known to the classical world. Before the rise of monotheistic religions, most people practiced some type of polytheism. Many of these religions started to die out, and eventually they became extinct. In some cases, elements of polytheistic belief systems continued to exist in folklore. Paganism would later be studied during the Renaissance and Romantic era. Forms of these religions, influenced by various historical pagan beliefs of pre-modern Europe, exist today and are known as contemporary or modern paganism, also referred to as Neo-paganism. <![CDATA[<a href="#_dbpedia_2017">(DBpedia, 2017)</a>]]></skos:definition>
    <skos:definition xml:lang="fr">Paganisme est un terme générique employé depuis le VIe siècle par des chrétiens pour désigner la religion de ceux qui ne sont ni chrétiens, ni juifs, ni musulmans. Il remonte au latin paganus (païen). Au VIe siècle, ce mot pouvait servir à désigner les habitants des campagnes par opposition à ceux des villes ou bien les civils par opposition aux militaires. D'abord employé comme sobriquet populaire par des chrétiens pour désigner ceux qui ne sont pas baptisés, le terme a ensuite été adopté dans la littérature chrétienne. Même s'il y désigne toujours ceux qui ne sont pas chrétiens, son acception y est cependant ambiguë. Il est parfois employé de façon péjorative pour désigner ceux qui sont tenus pour être des ignorants, parfois de façon neutre pour désigner les philosophes grecs, parfois encore pour désigner des chrétiens jugés mal convertis ou tièdes dans leur foi. À partir de 370, des lois impériales regroupées au Ve siècle dans le code théodosien emploient le terme paganus pour désigner ceux qui pratiquent la magie, ceux qui sont considérés comme superstitieux ou dans l'erreur. Le terme a depuis conservé une connotation péjorative. De nombreux Pères de l'Église ayant écrit « contre les païens », le paganisme a eu une première existence sous forme de fiction littéraire, comme s'il s'agissait de la religion de ceux qui ne sont pas chrétiens. Le paganisme tel qu'il a été exposé par les Pères de l'Église n'était cependant pas à proprement parler une religion, il s'agit plutôt de l'ensemble sans homogénéité des positions philosophiques et des croyances rejetées par les Pères de l'Église. Le paganisme est ainsi, dans l'antiquité tardive, une attitude combattue par des chrétiens puis par les autorités, mais elle n'est revendiquée par personne. C'est surtout à l'époque moderne, avec l'essor de l'histoire des religions que le paganisme commence à être perçu et étudié comme une religion parmi d'autres. Le paganisme peut aujourd'hui être revendiqué sous forme de néo-paganisme, ou bien comme une position philosophique tel que l'a fait Marc Augé dans Le génie du paganisme. Le mot paganus n'a pas son correspondant chez les écrivains chrétiens de langue grecque qui utilisent le terme moins péjoratif de « nations » ou « religions nationales » (ethnikoï) (décalque de l'hébreu). <![CDATA[<a href="#_dbpedia_2017">(DBpedia, 2017)</a>]]></skos:definition>
    <rdf:type rdf:resource="http://www.w3.org/2004/02/skos/core#Concept"/>
    <skos:inScheme rdf:resource="#Religion"/>
    <rdfs:isDefinedBy rdf:resource="http://sparql.cwrc.ca/ontologies/cwrc-ONTOLOGY_DATE"/>
    <void:inDataset rdf:resource="#datasetdefinition"/>
    <skos:broaderTransitive rdf:resource="#occultism"/>
  </cwrc:Religion>
  <cwrc:Religion rdf:about="#plymouthBrethren">
    <rdfs:label xml:lang="en">Plymouth Brethren</rdfs:label>
    <rdfs:label xml:lang="fr">Frères de Schwarzenau</rdfs:label>
    <rdfs:label xml:lang="fr">Assemblées de Frères</rdfs:label>
    <skos:definition xml:lang="en">The Plymouth Brethren are a conservative, low church, nonconformist, Evangelical Christian movement whose history can be traced to Dublin, Ireland in the late 1820s, originating from Anglicanism. Among other beliefs, the group emphasizes sola scriptura, the belief that the Bible is the supreme authority for church doctrine and practice over and above &quot;the [mere] tradition of men&quot; (Mark 7:8). Brethren generally see themselves not as a denomination but as a network, or even as a collection of overlapping networks, of like-minded independent churches. (The Brethren would generally prefer that their gatherings be referred to as &quot;assemblies&quot; rather than &quot;churches&quot; but, in the interests of simplicity, this article uses both terms interchangeably.) The movement refused for many years to take any denominational name to itself, a stance that some still maintain. The title &quot;The Brethren,&quot; however, is one that many of their number are comfortable with, in that the Bible designates all believers as &quot;brethren&quot;. (&quot;[O]ne is your Master, even Christ; and all ye are brethren.&quot; Matthew 23:8)<![CDATA[<a href="#_dbpedia_2017">(DBpedia, 2017)</a>]]></skos:definition>
    <skos:definition xml:lang="fr">Le courant des Assemblées de Frères ou Plymouth Brethren ou encore Frères de Plymouth constitue l'une des branches du protestantisme évangélique. Ce mouvement est né à Dublin et en Grande-Bretagne vers 1830 et a connu une importante scission en 1848 qui a abouti à distinguer un courant « ouvert » d'une part, les « Open Brethren », et un courant « exclusif » d'autre part, appelé aussi « darbyste ». La branche la plus « étroite » a suivi John Nelson Darby et la branche plus ouverte des leaders comme George Müller et Henry Craik. Ces deux courants se sont développés dans le monde et notamment en France pour faire partie des cinq principales dénominations évangéliques sur quarante-trois significatives. <![CDATA[<a href="#_dbpedia_2017">(DBpedia, 2017)</a>]]></skos:definition>
    <prov:derivedFrom rdf:resource="http://dbpedia.org/page/Plymouth_Brethren"/>
    <rdfs:comment xml:lang="fr">La description de ce terme est basée sur celle de DBPedia.</rdfs:comment>
    <rdf:type rdf:resource="http://www.w3.org/2004/02/skos/core#Concept"/>
    <skos:inScheme rdf:resource="#Religion"/>
    <rdfs:isDefinedBy rdf:resource="http://sparql.cwrc.ca/ontologies/cwrc-ONTOLOGY_DATE"/>
    <void:inDataset rdf:resource="#datasetdefinition"/>
    <skos:broaderTransitive rdf:resource="#anglicanChurch"/>
  </cwrc:Religion>
  <cwrc:Religion rdf:about="#quakers">
    <rdfs:label xml:lang="en">Quaker</rdfs:label>
    <rdfs:label xml:lang="fr">quaker</rdfs:label>
    <skos:definition xml:lang="en">Quakers (or Friends) are members of a group of religious Christian movements which is known as the Religious Society of Friends in Europe, Australia, New Zealand and parts of North America; and known as the Friends Church in Africa, Asia, South America and parts of the US. The movements were originally, and are still predominantly based on Christianity. Members of the movements profess the priesthood of all believers, a doctrine derived from the First Epistle of Peter. They include those with evangelical, holiness, liberal, and traditional Quaker understandings of Christianity. To differing extents, the different movements that make up the Religious Society of Friends/Friends Church avoid creeds and hierarchical structures. In 2007, there were approximately 359,000 adult Quakers. <![CDATA[<a href="#_dbpedia_2017">(DBpedia, 2017)</a>]]></skos:definition>
    <skos:definition xml:lang="fr">La Société religieuse des Amis est un mouvement religieux fondé en Angleterre au XVIIe siècle par des dissidents de l'Église anglicane. Les membres de ce mouvement sont communément connus sous le nom de quakers () mais ils se nomment entre eux « Amis » et « Amies ». Le mouvement est souvent nommé simplement Société des Amis et le surnom de « quaker » apparaît le plus souvent dans la dénomination officielle, sous la forme Société religieuse des Amis (quakers). Les historiens s'accordent à désigner George Fox comme le principal fondateur ou le plus important meneur des débuts du mouvement. Depuis sa création en Angleterre, le mouvement s'est d'abord répandu dans les pays de colonisation anglo-saxonne. Au XXe siècle, des missionnaires quakers ont propagé leur religion en Amérique latine et en Afrique. Aujourd'hui, les quakers déclarent être au nombre d'environ 350 000 dans le monde. La Société des Amis se différencie de la plupart des autres groupes issus du christianisme par l'absence de credo et de toute structure hiérarchique. Pour les quakers, la croyance religieuse appartient à la sphère personnelle et chacun est libre de ses convictions. Le concept de « lumière intérieure » (inner light) est cependant partagé par la plupart d'entre eux, quelle que soit la signification donnée à ces mots. De nombreux quakers reconnaissent le christianisme mais ne ressentent pas leur foi comme entrant dans les catégories chrétiennes traditionnelles. On trouve aujourd'hui dans la Société des Amis des pratiques très diverses, y compris un large courant évangélique. <![CDATA[<a href="#_dbpedia_2017">(DBpedia, 2017)</a>]]></skos:definition>
    <skos:definition xml:lang="nl">Het Religieus Genootschap der Vrienden, beter bekend als quakers, verouderd Nederlands kwakers, vormt een groep ondogmatische gelovigen, die zijn wortels vindt in de christelijke traditie. Het leven en de overgeleverde uitspraken van Jezus vormen een belangrijke inspiratiebron. <![CDATA[<a href="#_dbpedia_2017">(DBpedia, 2017)</a>]]></skos:definition>
    <prov:derivedFrom rdf:resource="http://dbpedia.org/resource/Quakers"/>
    <rdfs:comment xml:lang="fr">La description de ce terme est basée sur celle de DBPedia.</rdfs:comment>
    <skos:broaderTransitive rdf:resource="#churchOfEngland"/>
    <rdf:type rdf:resource="http://www.w3.org/2004/02/skos/core#Concept"/>
    <skos:inScheme rdf:resource="#Religion"/>
    <rdfs:isDefinedBy rdf:resource="http://sparql.cwrc.ca/ontologies/cwrc-ONTOLOGY_DATE"/>
    <void:inDataset rdf:resource="#datasetdefinition"/>
    <skos:broaderTransitive rdf:resource="#dissenters"/>
  </cwrc:Religion>
  <cwrc:Religion rdf:about="#rationalDissenter">
    <rdfs:label xml:lang="en">Rational Dissenter</rdfs:label>
    <rdfs:label xml:lang="fr"/>
    <!-- #outstanding, btw -->
    <skos:definition xml:lang="en"></skos:definition>
    <skos:definition xml:lang="fr"/>
    <rdf:type rdf:resource="http://www.w3.org/2004/02/skos/core#Concept"/>
    <skos:inScheme rdf:resource="#Religion"/>
    <rdfs:isDefinedBy rdf:resource="http://sparql.cwrc.ca/ontologies/cwrc-ONTOLOGY_DATE"/>
    <void:inDataset rdf:resource="#datasetdefinition"/>
    <skos:broaderTransitive rdf:resource="#dissenters"/>
  </cwrc:Religion>
  <cwrc:Religion rdf:about="#societyOfFriends">
    <rdfs:label xml:lang="en">Society of Friends</rdfs:label>
    <rdfs:label xml:lang="fr">Société religieuse des Amis</rdfs:label>
    <skos:definition xml:lang="en"/>
    <skos:definition xml:lang="fr"/>
    <rdf:type rdf:resource="http://www.w3.org/2004/02/skos/core#Concept"/>
    <skos:inScheme rdf:resource="#Religion"/>
    <skos:broaderTransitive rdf:resource="#christianity"/>
    <rdfs:isDefinedBy rdf:resource="http://sparql.cwrc.ca/ontologies/cwrc-ONTOLOGY_DATE"/>
    <void:inDataset rdf:resource="#datasetdefinition"/>
  </cwrc:Religion>
  <cwrc:Religion rdf:about="#spiritualism">
    <rdfs:label xml:lang="en">Spiritualism</rdfs:label>
    <rdfs:label xml:lang="fr">spiritualisme</rdfs:label>
    <skos:definition xml:lang="en"/>
    <skos:definition xml:lang="fr"/>
    <rdf:type rdf:resource="http://www.w3.org/2004/02/skos/core#Concept"/>
    <rdfs:subClassOf rdf:resource="http://dbpedia.org/resource/Spiritualism"/>
    <skos:inScheme rdf:resource="#Religion"/>
    <rdfs:isDefinedBy rdf:resource="http://sparql.cwrc.ca/ontologies/cwrc-ONTOLOGY_DATE"/>
    <void:inDataset rdf:resource="#datasetdefinition"/>
    <skos:broaderTransitive rdf:resource="#occultism"/>
  </cwrc:Religion>
  <cwrc:Religion rdf:about="#tractarianMovement">
    <rdfs:label xml:lang="en">Tractarian Movement</rdfs:label>
    <rdfs:label xml:lang="fr">tractarianisme</rdfs:label>
    <skos:definition xml:lang="en"/>
    <skos:definition xml:lang="fr"/>
    <rdf:type rdf:resource="http://www.w3.org/2004/02/skos/core#Concept"/>
    <skos:inScheme rdf:resource="#Religion"/>
    <skos:broaderTransitive rdf:resource="#churchOfEngland"/>
    <rdfs:subClassOf rdf:resource="http://dbpedia.org/resource/Oxford_Movement"/>
    <rdfs:isDefinedBy rdf:resource="http://sparql.cwrc.ca/ontologies/cwrc-ONTOLOGY_DATE"/>
    <void:inDataset rdf:resource="#datasetdefinition"/>
  </cwrc:Religion>
  <cwrc:Religion rdf:about="#unitarianChurch">
    <rdfs:label xml:lang="en">Unitarian Church</rdfs:label>
    <rdfs:label xml:lang="fr">Église unitarienne</rdfs:label>
    <skos:definition xml:lang="en">Unitarian church usually refers to a church (either a single church or a group of churches and/or its followers) which follows Unitarianism, a Christian theology. It can also more broadly refer to a church which is a member of an umbrella group with "Unitarian" in its title, such as the Unitarian Universalist Association in the U.S., the Canadian Unitarian Council, and similar bodies. <![CDATA[<a href="#_dbpedia_2017">(DBpedia, 2017)</a>]]></skos:definition>
    <prov:derivedFrom rdf:resource="http://dbpedia.org/resource/Unitarian_church"/>
    <rdfs:comment xml:lang="fr">La description de ce terme est basée sur celle de DBPedia.</rdfs:comment>
    <skos:definition xml:lang="fr"/>
    <rdf:type rdf:resource="http://www.w3.org/2004/02/skos/core#Concept"/>
    <rdf:value>unitarianChurch</rdf:value>
    <skos:broaderTransitive rdf:resource="#christianity"/>
    <rdfs:isDefinedBy rdf:resource="http://sparql.cwrc.ca/ontologies/cwrc-ONTOLOGY_DATE"/>
    <void:inDataset rdf:resource="#datasetdefinition"/>
  </cwrc:Religion>
  <cwrc:Religion rdf:about="#unitarianism">
    <rdfs:label xml:lang="en">Unitarianism</rdfs:label>
    <skos:altLabel xml:lang="en">Unitarian Movement</skos:altLabel>
    <skos:altLabel xml:lang="en">Unitarian</skos:altLabel>
    <rdfs:label xml:lang="nl">unitarisme</rdfs:label>
    <rdfs:label xml:lang="es">unitarismo</rdfs:label>
    <rdfs:label xml:lang="es">unitarios</rdfs:label>
    <rdfs:label xml:lang="fr">unitarisme</rdfs:label>
    <skos:definition xml:lang="en">The liberal Protestant movement that arose in Europe during the 16th century Reformation, was embodied in a church in Transylvania, and achieved denominational status in the 19th century in the United Kingdom, the United States, and Canada. It is characterized by a denial of the orthodox Christian doctrines of the Trinity and the divinity of Jesus, the free use of reason in religion, and the belief that God exists in one person. In 1961, in the United States and Canada, it merged with the Universalist denomination to form &quot;Unitarian Universalism.&quot;  Use also generally for the theological doctrines of the unified nature of God and the humanity of Jesus, first expressed in second- and third-century monarchism and in the teachings of Arius in the third and fourth centuries, and later in the radical Neoplatonist thinkers of the Reformation such as Michael Servetus, Faustus Socinus, and Ferenc David. <![CDATA[<a href="#_getty_2017">(Getty, 2017)</a>]]></skos:definition>
    <skos:definition xml:lang="nl">In het bijzonder te gebruiken voor de vrijzinnig protestantse beweging die in Europa opkwam tijdens de Reformatie in de 16de eeuw, werd belichaamd door een kerk in Transsylvanië en een confessionele status verkreeg in Groot-Brittannië, de Verenigde Staten en Canada tijdens de 19de eeuw. De beweging wordt gekenmerkt door de afwijzing van de orthodox christelijke leer van de Drie-eenheid en de goddelijke Christus, het vrije gebruik van de rede in religieuze zaken en het geloof dat God bestaat in één persoon. In 1961 fuseerde deze beweging in de Verenigde Staten en Canada met de universalistische beweging, waardoor het ‘unitaristisch universalisme’ ontstond. Ook in het algemeen te gebruiken voor de theologische leer van de eenheid van God en het mens-zijn van Jezus, zoals voor het eerst verwoord in het monarchisme van de 2de en 3de eeuw en in de leer van Arius in de 3de en 4de eeuw, en later in de leer van de radicale neoplatonisten uit de Reformatie zoals Michael Servetus, Faustus Socinus en Ferenc David. <![CDATA[<a href="#_getty_2017">(Getty, 2017)</a>]]></skos:definition>
    <skos:definition xml:lang="es">Úsese específicamente para el movimiento protestante liberal que surgió en Europa durante la Reforma del siglo XVI, que tuvo su manifestación en una iglesia en Transilvania, y que logró un estatus confesional en el siglo XIX en el Reino Unido, los Estados Unidos y Canadá. Es caracterizado por una desaprobación de las doctrinas cristianas ortodoxas de la Trinidad y la divinidad de Jesús, el libre uso de la razón en la religión y la creencia que Dios existe en una persona. En 1961, en los Estados Unidos y Canadá s <![CDATA[<a href="#_getty_2017">(Getty, 2017)</a>]]></skos:definition>
    <prov:derivedFrom rdf:resource="http://vocab.getty.edu/aat/300263305"/>
    <rdfs:comment xml:lang="en">The description for this term is indebted to the Getty Art &amp; Architecture Thesaurus.</rdfs:comment>
    <skos:definition xml:lang="fr">L’unitarisme est une doctrine qui affirme que le Dieu du christianisme est une seule personne, et non pas une seule nature ou "ousie" en trois hypostases comme l'affirme le dogme de la Trinité : Père, Fils et Esprit. Selon le dogme de la Trinité, ces trois personnes divines participent d'une seule nature divine unique . Le « trinitarisme » est la doctrine officielle du christianisme depuis le premier concile de Nicée (325) et le concile de Chalcédoine (451). <![CDATA[<a href="#_dbpedia_2017">(DBpedia, 2017)</a>]]></skos:definition>
    <prov:derivedFrom rdf:resource="http://dbpedia.org/page/Unitarianism"/>
    <rdfs:comment xml:lang="fr">La description de ce terme est basée sur celle de DBPedia.</rdfs:comment>

    <rdf:type rdf:resource="http://www.w3.org/2004/02/skos/core#Concept"/>
    <rdf:value>unitarianMovement</rdf:value>
    <skos:inScheme rdf:resource="#Religion"/>
    <skos:broaderTransitive rdf:resource="#protestantism"/>
    <rdfs:subClassOf rdf:resource="http://dbpedia.org/resource/Unitarianism"/>
    <rdfs:isDefinedBy rdf:resource="http://sparql.cwrc.ca/ontologies/cwrc-ONTOLOGY_DATE"/>
    <void:inDataset rdf:resource="#datasetdefinition"/>
  </cwrc:Religion>
  <cwrc:Religion rdf:about="#abrahamicReligions">
    <rdfs:label xml:lang="en">Abrahamic religions</rdfs:label>
    <rdfs:label xml:lang="fr">Religions abrahamiques</rdfs:label>
    <skos:definition xml:lang="en">Abrahamic religions, emphasizing and tracing their common origin to the tribal patriarch Abraham or recognizing a spiritual tradition identified with him, comprising one of the major divisions in comparative religion, along with Indian, Iranian, and East Asian religions. Judaism, Christianity and Islam are the largest Abrahamic religions.The largest Abrahamic religions in chronological order of founding are Judaism (2nd millennium BCE), Christianity (1st century CE) and Islam (7th century CE). <![CDATA[<a href="#_dbpedia_2017">(DBpedia, 2017)</a>]]></skos:definition>
    <skos:definition xml:lang="fr">L'expression religion abrahamique désigne principalement le judaïsme, le christianisme dont les Saintes Écritures, respectivement le Tanakh, la Bible évoquent la figure d'Abraham et l'islam avec le Coran, celle d'Ibrahim.En français, cette expression est apparue vers 1950 dans des études d'islamologie pour désigner, d'une part, la religion d'Abraham telle qu'elle se conçoit dans l'islam et d'autre part les trois religions que sont le judaïsme, le christianisme et l'islam. <![CDATA[<a href="#_dbpedia_2017">(DBpedia, 2017)</a>]]></skos:definition>
    <prov:derivedFrom rdf:resource="http://dbpedia.org/page/Abrahamic_religions"/>
    <rdfs:comment xml:lang="fr">La description de ce terme est basée sur celle de DBPedia.</rdfs:comment>
    <rdfs:isDefinedBy rdf:resource="http://sparql.cwrc.ca/ontologies/cwrc-ONTOLOGY_DATE"/>
    <void:inDataset rdf:resource="#datasetdefinition"/>
    <rdf:type rdf:resource="http://www.w3.org/2004/02/skos/core#Concept"/>
    <skos:broaderTransitive rdf:resource="#occultism"/>
  </cwrc:Religion>
  <!-- Social Classes -->
  <owl:Class rdf:ID="SocialClassIdentity">
    <rdfs:label xml:lang="en">social class identity</rdfs:label>
    <rdfs:label xml:lang="fr">identité classe sociale</rdfs:label>
    <rdf:type rdf:resource="http://www.w3.org/2004/02/skos/core#Concept"/>
    <rdfs:subClassOf rdf:resource="#CulturalForm"/>
    <skos:definition xml:lang="en">A subclass of culturalForms, Social Class terms associate subjects with a specific social group, recognizing that such categories and their application to individuals are contested and can change over time. The association may be or have been embraced by the subject by the subject her/himself or attributed by others. Unlike Notes typed as socialClassContext, which contain detailed discussion of a subject's class position, socialClass links to a word or phrase signifying a particular construction of class, with particular reference to earlier historical periods in the British Isles. Social class has been variously constructed and theorized, and for women is further complicated by the fact that women were understood to take their social status from fathers and/or husbands. The terminology used here reflects quite basic social groupings that intersect with other factors such as wealth.</skos:definition>
    <skos:definition xml:lang="fr"/>
    <rdfs:isDefinedBy rdf:resource="http://sparql.cwrc.ca/ontologies/cwrc-ONTOLOGY_DATE"/>
    <void:inDataset rdf:resource="#datasetdefinition"/>
    <rdf:type rdf:resource="http://www.w3.org/2004/02/skos/core#ConceptScheme"/>
  </owl:Class>
  <cwrc:SocialClassIdentity rdf:about="#lowerMiddleClass">
    <rdfs:label xml:lang="en">lower middle class</rdfs:label>
    <rdfs:label xml:lang="fr">classe moyenne inférieure</rdfs:label>
    <rdf:type rdf:resource="http://www.w3.org/2004/02/skos/core#Concept"/>
    <rdfs:subClassOf rdf:resource="#CulturalForm"/>
    <skos:definition xml:lang="en">Employees, clerical workers, teachers, governesses. Note, however, that some teachers go into Professional (Mr. Chips) and women starting schools and then managing them also go into Professional.</skos:definition>
    <skos:definition xml:lang="fr"/>
    <rdfs:isDefinedBy rdf:resource="http://sparql.cwrc.ca/ontologies/cwrc-ONTOLOGY_DATE"/>
    <void:inDataset rdf:resource="#datasetdefinition"/>
  </cwrc:SocialClassIdentity>
  <cwrc:SocialClassIdentity rdf:about="#entrepreneurial-industrialist">
    <rdfs:label xml:lang="en">entrepreneurial</rdfs:label>
    <rdfs:label xml:lang="fr">entrepreneur</rdfs:label>
    <rdf:type rdf:resource="http://www.w3.org/2004/02/skos/core#Concept"/>
    <rdfs:subClassOf rdf:resource="#CulturalForm"/>
    <skos:definition xml:lang="en">Involves larges-scale enterprises such as running factories, or backing such enterprises through investing money, for instance, Elizabeth Montagu or Beatrice Webb.</skos:definition>
    <skos:definition xml:lang="fr"/>
    <!-- Fix the examples -->
    <rdfs:isDefinedBy rdf:resource="http://sparql.cwrc.ca/ontologies/cwrc-ONTOLOGY_DATE"/>
    <void:inDataset rdf:resource="#datasetdefinition"/>
  </cwrc:SocialClassIdentity>
  <cwrc:SocialClassIdentity rdf:about="#professional">
    <rdfs:label xml:lang="en">professional</rdfs:label>
    <rdfs:label xml:lang="fr">professionnel</rdfs:label>
    <rdf:type rdf:resource="http://www.w3.org/2004/02/skos/core#Concept"/>
    <rdfs:subClassOf rdf:resource="#CulturalForm"/>
    <skos:definition xml:lang="en">Includes doctors, lawyers, guild members, and those of high calling such as members of the clergy (Church of England). It implies social respect and intellectual requirements. Examples are Ann Hunter, who was married to a surgeon, and Virginia Woolf, daughter of an intellectual.</skos:definition>
    <skos:definition xml:lang="fr"/>
    <rdfs:isDefinedBy rdf:resource="http://sparql.cwrc.ca/ontologies/cwrc-ONTOLOGY_DATE"/>
    <void:inDataset rdf:resource="#datasetdefinition"/>
  </cwrc:SocialClassIdentity>
  <cwrc:SocialClassIdentity rdf:about="#managerial">
    <rdfs:label xml:lang="en">managerial</rdfs:label>
    <rdfs:label xml:lang="fr">gestionnaire</rdfs:label>
    <rdf:type rdf:resource="http://www.w3.org/2004/02/skos/core#Concept"/>
    <rdfs:subClassOf rdf:resource="#CulturalForm"/>
    <skos:definition xml:lang="en">Someone whose station in life comes from the fact that they are running something but not putting their money into it, e.g. salaried civil service, bankers, hospital administrators.</skos:definition>
    <skos:definition xml:lang="fr"/>
    <rdfs:isDefinedBy rdf:resource="http://sparql.cwrc.ca/ontologies/cwrc-ONTOLOGY_DATE"/>
    <void:inDataset rdf:resource="#datasetdefinition"/>
  </cwrc:SocialClassIdentity>
  <cwrc:SocialClassIdentity rdf:about="#nobility">
    <rdfs:label xml:lang="en">nobility</rdfs:label>
    <rdfs:label xml:lang="fr">noblesse</rdfs:label>
    <rdf:type rdf:resource="http://www.w3.org/2004/02/skos/core#Concept"/>
    <rdfs:subClassOf rdf:resource="#CulturalForm"/>
    <skos:definition xml:lang="en">This group refers to those holding a title or of close family relation to someone holding a title (such as Lady Mary Wortley Montagu, Lord Byron, or Nancy Mitford).</skos:definition>
    <skos:definition xml:lang="fr"/>
    <rdfs:isDefinedBy rdf:resource="http://sparql.cwrc.ca/ontologies/cwrc-ONTOLOGY_DATE"/>
    <void:inDataset rdf:resource="#datasetdefinition"/>
  </cwrc:SocialClassIdentity>
  <cwrc:SocialClassIdentity rdf:about="#gentry">
    <rdfs:label xml:lang="en">gentry</rdfs:label>
    <rdfs:label xml:lang="fr">noblesse non titrée</rdfs:label>
    <rdf:type rdf:resource="http://www.w3.org/2004/02/skos/core#Concept"/>
    <rdfs:subClassOf rdf:resource="#CulturalForm"/>
    <skos:definition xml:lang="en">Gentry indicates someone who is property-owning or related to the same; property can be land or stocks and bonds. It begins in the idea of owning arms and having a coat of arms. but is distinguished from nobility in so far as money is not necessarily related to blood and title. Disinterested gentlemen are of this class (i.e. Mr. Bennett in Jane Austen). Gentlewomen belong to this class, even thought they may not themselves own much property but instead be supported by a father or brother, or they may be distressed, which is to say, impoverished gentlewomen, as in the case of Jane Eyre or Austen's Jane Fairfax. <![CDATA[<a href="#_dbpedia_2017">(DBpedia, 2017)</a>]]></skos:definition>
    <skos:definition xml:lang="fr">La landed gentry est le nom donné à la bonne société anglaise, et en particulier à la noblesse non titrée. Elle est de bonne éducation et « a des valeurs ». Les membres de la gentry sont légalement des gentlemen, esquire, et peuvent recevoir des décorations, titres de noblesses, héréditaires ou viagier (chevaliers, baronnets). Cette classe, composée à la fois de la haute bourgeoisie et de la noblesse titrée ou non, se développe au XVIe siècle, à une époque de mobilité sociale accentuée. À l'origine, ce sont des notables provinciaux, propriétaires, qui s'enrichissent grâce à leurs domaines (qu'ils n'exploitent pas directement). Du point de vue juridique, la gentry n'a pas un statut comparable à celui qu'a eu la noblesse continentale au cours des siècles, et on ne parle donc pas légalement de nobility (sauf en Écosse qui a un système plus proche du système continental). En effet, en Angleterre (au sens strict), seuls les pairs ont légalement le titre de noble et tous les attributs légaux qui vont avec. Ainsi, dans une famille qui descend d'un pair du royaume, seul le chef de famille est légalement « noble », les autres sont gentry. Néanmoins, la gentry a tous les attributs sociaux de la noblesse, et est donc reconnue comme noble au sens complet par la CILANE (« Commission d'information et de liaison des associations nobles d'Europe », voir Association d'entraide de la noblesse française). Le statut juridique de la gentility est donné par la lettre patente donnée par les rois d'armes par délégation du souverain. C'est cette lettre patente qui leur donne à eux seuls le droit de porter des armoiries, de se déclarer « of gentle birth. » Dans la distinction traditionnelle nobilitas maior et nobilitas minor, les pairs représentent le premier groupe, la gentry le second. <![CDATA[<a href="#_dbpedia_2017">(DBpedia, 2017)</a>]]></skos:definition>
    <owl:sameAs rdf:resource="http://dbpedia.org/resource/Gentry"/>
    <rdfs:isDefinedBy rdf:resource="http://sparql.cwrc.ca/ontologies/cwrc-ONTOLOGY_DATE"/>
    <void:inDataset rdf:resource="#datasetdefinition"/>
  </cwrc:SocialClassIdentity>
  <owl:DeprecatedClass rdf:about="#entrepreneurial-industrialism">
    <rdfs:label xml:lang="en">entrepreneurial industrialism</rdfs:label>
    <rdfs:label xml:lang="fr">entrepreneuriat industriel</rdfs:label>
    <skos:definition xml:lang="en"/>
    <skos:definition xml:lang="fr"/>
    <rdf:type rdf:resource="http://www.w3.org/2004/02/skos/core#Concept"/>
    <rdfs:isDefinedBy rdf:resource="http://sparql.cwrc.ca/ontologies/cwrc-ONTOLOGY_DATE"/>
    <void:inDataset rdf:resource="#datasetdefinition"/>
    <owl:equivalentClass rdf:resource="#entrepreneurial-industrialist"/>
    <dc:isReplacedBy rdf:resource="#entrepreneurial-industrialist"/>
    <vs:term_status xml:lang="en">deprecated</vs:term_status>
  </owl:DeprecatedClass>
  <cwrc:SocialClassIdentity rdf:about="#indigent">
    <rdfs:label xml:lang="en">indigent</rdfs:label>
    <rdfs:label xml:lang="fr">indigents</rdfs:label>
    <rdf:type rdf:resource="http://www.w3.org/2004/02/skos/core#Concept"/>
    <rdfs:subClassOf rdf:resource="#CulturalForm"/>
    <skos:definition xml:lang="en">This social group is poor, destitute, unemployed, supported by charity, or on social security.</skos:definition>
    <skos:definition xml:lang="fr"/>
    <rdfs:isDefinedBy rdf:resource="http://sparql.cwrc.ca/ontologies/cwrc-ONTOLOGY_DATE"/>
    <void:inDataset rdf:resource="#datasetdefinition"/>
  </cwrc:SocialClassIdentity>
  <cwrc:SocialClassIdentity rdf:about="#shopkeepers">
    <rdfs:label xml:lang="en">shopkeepers</rdfs:label>
    <rdfs:label xml:lang="fr">commerçants</rdfs:label>
    <rdf:type rdf:resource="http://www.w3.org/2004/02/skos/core#Concept"/>
    <rdfs:subClassOf rdf:resource="#CulturalForm"/>
    <skos:definition xml:lang="en">Owns and runs a pub or shop. Similar to an industrialist but to a lesser degree of magnitude.</skos:definition>
    <skos:definition xml:lang="fr"/>
    <rdfs:isDefinedBy rdf:resource="http://sparql.cwrc.ca/ontologies/cwrc-ONTOLOGY_DATE"/>
    <void:inDataset rdf:resource="#datasetdefinition"/>
  </cwrc:SocialClassIdentity>
  <cwrc:SocialClassIdentity rdf:about="#yeoman-farmer">
    <rdfs:label xml:lang="en">yeoman farmer</rdfs:label>
    <rdfs:label xml:lang="fr">agriculteur vivrier</rdfs:label>
    <rdf:type rdf:resource="http://www.w3.org/2004/02/skos/core#Concept"/>
    <rdfs:subClassOf rdf:resource="#CulturalForm"/>
    <skos:definition xml:lang="en">Own just enough land to support themselves if they do most of the work themselves (ie Elizabeth Ham, Mary Webb).</skos:definition>
    <skos:definition xml:lang="fr"/>
    <rdfs:isDefinedBy rdf:resource="http://sparql.cwrc.ca/ontologies/cwrc-ONTOLOGY_DATE"/>
    <void:inDataset rdf:resource="#datasetdefinition"/>
  </cwrc:SocialClassIdentity>
  <cwrc:SocialClassIdentity rdf:about="#upper-middleClass">
    <rdfs:label xml:lang="en">upper middle class</rdfs:label>
    <rdfs:label xml:lang="fr">classe moyenne supérieure</rdfs:label>
    <rdf:type rdf:resource="http://www.w3.org/2004/02/skos/core#Concept"/>
    <rdfs:subClassOf rdf:resource="#CulturalForm"/>
    <skos:definition xml:lang="en"/>
    <skos:definition xml:lang="fr"/>
    <rdfs:comment xml:lang="en">This term is a CWRC specific addition not in the original Orlando tag set.</rdfs:comment>
    <rdfs:isDefinedBy rdf:resource="http://sparql.cwrc.ca/ontologies/cwrc-ONTOLOGY_DATE"/>
    <void:inDataset rdf:resource="#datasetdefinition"/>
  </cwrc:SocialClassIdentity>
  <cwrc:SocialClassIdentity rdf:about="#skilledCraftpersonArtisan">
    <rdfs:label xml:lang="en">skilled craftperson/artisan</rdfs:label>
    <rdfs:label xml:lang="fr">artisan</rdfs:label>
    <rdf:type rdf:resource="http://www.w3.org/2004/02/skos/core#Concept"/>
    <rdfs:subClassOf rdf:resource="#CulturalForm"/>
    <skos:definition xml:lang="en">Goldsmith, tailor, shoemaker, milliner, dressmaker.</skos:definition>
    <skos:definition xml:lang="fr"/>
    <!-- Fix examples -->
    <rdfs:isDefinedBy rdf:resource="http://sparql.cwrc.ca/ontologies/cwrc-ONTOLOGY_DATE"/>
    <void:inDataset rdf:resource="#datasetdefinition"/>
  </cwrc:SocialClassIdentity>
  <cwrc:SocialClassIdentity rdf:about="#urban-industrialUnskilled">
    <rdfs:label xml:lang="en">urban-industrial unskilled</rdfs:label>
    <rdfs:label xml:lang="fr">ouvrier non qualifié</rdfs:label>
    <rdf:type rdf:resource="http://www.w3.org/2004/02/skos/core#Concept"/>
    <rdfs:subClassOf rdf:resource="#CulturalForm"/>
    <skos:definition xml:lang="en">This category includes factory workers and workers in urban or large-scale industries without defined trades or professional qualifications, and those in low-wage and low-status service sector jobs, such as the restaurant or fast-food industry, in industrial or post-industrial societies.</skos:definition>
    <skos:definition xml:lang="fr"/>
    <!-- Fix dfinition -->
    <rdfs:isDefinedBy rdf:resource="http://sparql.cwrc.ca/ontologies/cwrc-ONTOLOGY_DATE"/>
    <void:inDataset rdf:resource="#datasetdefinition"/>
  </cwrc:SocialClassIdentity>
  <cwrc:SocialClassIdentity rdf:about="#rural-unskilled">
    <rdfs:label xml:lang="en">rural-unskilled</rdfs:label>
    <rdfs:label xml:lang="fr">travailleurs ruraus non qualifiés</rdfs:label>
    <rdf:type rdf:resource="http://www.w3.org/2004/02/skos/core#Concept"/>
    <rdfs:subClassOf rdf:resource="#CulturalForm"/>
    <skos:definition xml:lang="en">This generally indicates farm laborers, mostly male in earlier periods, and includes migrant farm workers.</skos:definition>
    <skos:definition xml:lang="fr"/>
    <!-- Fix dfinition -->
    <rdfs:isDefinedBy rdf:resource="http://sparql.cwrc.ca/ontologies/cwrc-ONTOLOGY_DATE"/>
    <void:inDataset rdf:resource="#datasetdefinition"/>
  </cwrc:SocialClassIdentity>
  <cwrc:SocialClassIdentity rdf:about="#servants">
    <rdfs:label xml:lang="en">servants</rdfs:label>
    <rdfs:label xml:lang="fr">domestiques</rdfs:label>
    <rdf:type rdf:resource="http://www.w3.org/2004/02/skos/core#Concept"/>
    <rdfs:subClassOf rdf:resource="#CulturalForm"/>
    <skos:definition xml:lang="en">Domestic servants typically live in the home with the family or institution that employs them, although the lowest class of servants might work only casually and hence not receive room and board. This type of labour, very common before the twentieth century, is distinct from that of service positions such as shop assistants, flight attendances, and restaurant workers.</skos:definition>
    <skos:definition xml:lang="fr"/>
    <!-- Fix dfinition -->
    <rdfs:isDefinedBy rdf:resource="http://sparql.cwrc.ca/ontologies/cwrc-ONTOLOGY_DATE"/>
    <void:inDataset rdf:resource="#datasetdefinition"/>
  </cwrc:SocialClassIdentity>
  <owl:Class rdf:ID="LinguisticAbility">
    <rdfs:label xml:lang="en">linguistic ability (spoken and/or writen)</rdfs:label>
    <rdfs:label xml:lang="fr">aptitude linguistique (écrit ou parlé)</rdfs:label>
    <rdf:type rdf:resource="http://www.w3.org/2004/02/skos/core#Concept"/>
    <rdfs:subClassOf rdf:resource="#CulturalForm"/>
    <skos:definition xml:lang="en"/>
    <skos:definition xml:lang="fr"/>
    <rdfs:isDefinedBy rdf:resource="http://sparql.cwrc.ca/ontologies/cwrc-ONTOLOGY_DATE"/>
    <void:inDataset rdf:resource="#datasetdefinition"/>
  </owl:Class>
  <owl:Class rdf:ID="PoliticalAffiliation">
    <rdfs:label xml:lang="en">political affiliation</rdfs:label>
    <rdfs:label xml:lang="fr">affiliation politique</rdfs:label>
    <rdf:type rdf:resource="http://www.w3.org/2004/02/skos/core#Concept"/>
    <rdfs:subClassOf rdf:resource="#CulturalForm"/>
    <skos:definition xml:lang="en">This subclass of CulturalForm tracks the affiliations, connections and associations which designate a person's political involvement. These affiliations can be both formal connections to a party or organization and informal political positions held by the writer. We hope to point our readers towards women writers associated with different political positions and help researchers make links between political beliefs and writing. For this reason, we are defining political affiliations broadly and include things like &quot;against capital punishment&quot; or &quot;strong supporter of the Empire&quot; in addition to more straightforward affiliations such as &quot;marxist&quot; or &quot;conservative.&quot;</skos:definition>
    <skos:definition xml:lang="fr"/>
    <rdfs:isDefinedBy rdf:resource="http://sparql.cwrc.ca/ontologies/cwrc-ONTOLOGY_DATE"/>
    <void:inDataset rdf:resource="#datasetdefinition"/>
  </owl:Class>
  <cwrc:RaceColour rdf:about="#black">
    <rdfs:label xml:lang="en">black (race)</rdfs:label>
    <rdfs:label xml:lang="fr">noir (race)</rdfs:label>
    <skos:definition xml:lang="en"/>
    <skos:definition xml:lang="fr"/>
    <rdfs:isDefinedBy rdf:resource="http://sparql.cwrc.ca/ontologies/cwrc-ONTOLOGY_DATE"/>
    <void:inDataset rdf:resource="#datasetdefinition"/>
  </cwrc:RaceColour>
  <owl:ObjectProperty rdf:ID="personalProperty">
    <rdfs:label xml:lang="en">personal property</rdfs:label>
    <rdfs:label xml:lang="fr">propriété de la personne</rdfs:label>
    <skos:definition xml:lang="en"/>
    <skos:definition xml:lang="fr"/>
    <rdfs:isDefinedBy rdf:resource="http://sparql.cwrc.ca/ontologies/cwrc-ONTOLOGY_DATE"/>
    <void:inDataset rdf:resource="#datasetdefinition"/>
  </owl:ObjectProperty>
  <owl:ObjectProperty rdf:ID="personalPropertySelfDeclared">
    <rdfs:label xml:lang="en">personal property (self reported)</rdfs:label>
    <rdfs:label xml:lang="fr">propriété de la personne (autodéclarée)</rdfs:label>
    <rdfs:subPropertyOf rdf:resource="#personalProperty"/>
    <skos:definition xml:lang="en"/>
    <skos:definition xml:lang="fr"/>
    <rdfs:isDefinedBy rdf:resource="http://sparql.cwrc.ca/ontologies/cwrc-ONTOLOGY_DATE"/>
    <void:inDataset rdf:resource="#datasetdefinition"/>
  </owl:ObjectProperty>
  <owl:ObjectProperty rdf:ID="hasGender">
    <rdfs:label xml:lang="en">has gender</rdfs:label>
    <rdfs:label xml:lang="fr">est de genre</rdfs:label>
    <rdfs:subPropertyOf rdf:resource="#personalProperty"/>
    <rdfs:range rdf:resource="#Gender"/>
    <skos:definition xml:lang="en"/>
    <skos:definition xml:lang="fr"/>
    <rdfs:isDefinedBy rdf:resource="http://sparql.cwrc.ca/ontologies/cwrc-ONTOLOGY_DATE"/>
    <void:inDataset rdf:resource="#datasetdefinition"/>
  </owl:ObjectProperty>
  <owl:ObjectProperty rdf:ID="hasGenderSelfDeclared">
    <rdfs:label xml:lang="en">has gender (self declared)</rdfs:label>
    <rdfs:label xml:lang="fr">est de genre (autodéclaré)</rdfs:label>
    <rdfs:subPropertyOf rdf:resource="#personalPropertySelfDeclared"/>
    <rdfs:range rdf:resource="#Gender"/>
    <skos:definition xml:lang="en"/>
    <skos:definition xml:lang="fr"/>
    <rdfs:isDefinedBy rdf:resource="http://sparql.cwrc.ca/ontologies/cwrc-ONTOLOGY_DATE"/>
    <void:inDataset rdf:resource="#datasetdefinition"/>
  </owl:ObjectProperty>
  <owl:ObjectProperty rdf:ID="hasNationality">
    <rdfs:label xml:lang="en">has nationality</rdfs:label>
    <rdfs:label xml:lang="fr">de nationalité</rdfs:label>
    <rdfs:subPropertyOf rdf:resource="#personalProperty"/>
    <rdfs:range rdf:resource="#NationalIdentity"/>
    <skos:definition xml:lang="en"/>
    <skos:definition xml:lang="fr"/>
    <rdfs:isDefinedBy rdf:resource="http://sparql.cwrc.ca/ontologies/cwrc-ONTOLOGY_DATE"/>
    <void:inDataset rdf:resource="#datasetdefinition"/>
  </owl:ObjectProperty>
  <owl:ObjectProperty rdf:ID="hasNationalitySelfDeclared">
    <rdfs:label xml:lang="en">has nationality (self declared)</rdfs:label>
    <rdfs:label xml:lang="fr">de nationalité (autodéclarée)</rdfs:label>
    <rdfs:subPropertyOf rdf:resource="#personalPropertySelfDeclared"/>
    <rdfs:range rdf:resource="#NationalIdentity"/>
    <skos:definition xml:lang="en"/>
    <skos:definition xml:lang="fr"/>
    <rdfs:isDefinedBy rdf:resource="http://sparql.cwrc.ca/ontologies/cwrc-ONTOLOGY_DATE"/>
    <void:inDataset rdf:resource="#datasetdefinition"/>
  </owl:ObjectProperty>
  <owl:ObjectProperty rdf:ID="hasRaceColour">
    <rdfs:label xml:lang="en">has race</rdfs:label>
    <rdfs:label xml:lang="fr">est de race</rdfs:label>
    <rdfs:subPropertyOf rdf:resource="#personalProperty"/>
    <rdfs:range rdf:resource="#RaceColour"/>
    <skos:definition xml:lang="en">A subclass of raceEthnicityContext, this describes a person's racial identity.</skos:definition>
    <skos:definition xml:lang="fr"/>
    <rdfs:isDefinedBy rdf:resource="http://sparql.cwrc.ca/ontologies/cwrc-ONTOLOGY_DATE"/>
    <void:inDataset rdf:resource="#datasetdefinition"/>
  </owl:ObjectProperty>
  <owl:ObjectProperty rdf:ID="hasRaceColourSelfDeclared">
    <rdfs:label xml:lang="en">has race (self declared)</rdfs:label>
    <rdfs:label xml:lang="fr">est de race (autodéclarée)</rdfs:label>
    <rdfs:subPropertyOf rdf:resource="#personalPropertySelfDeclared"/>
    <rdfs:range rdf:resource="#Race"/>
    <skos:definition xml:lang="en">A subclass of raceEthnicityContext, this describes a person's self-reported racial identity.</skos:definition>
    <skos:definition xml:lang="fr"/>
    <rdfs:isDefinedBy rdf:resource="http://sparql.cwrc.ca/ontologies/cwrc-ONTOLOGY_DATE"/>
    <void:inDataset rdf:resource="#datasetdefinition"/>
  </owl:ObjectProperty>
  <owl:ObjectProperty rdf:ID="hasEthnicity">
    <rdfs:label xml:lang="en">has ethnicity</rdfs:label>
    <rdfs:label xml:lang="fr">d'ethnicité</rdfs:label>
    <rdfs:subPropertyOf rdf:resource="#personalProperty"/>
    <rdfs:range rdf:resource="#Ethnicity"/>
    <skos:definition xml:lang="en"/>
    <skos:definition xml:lang="fr"/>
    <rdfs:isDefinedBy rdf:resource="http://sparql.cwrc.ca/ontologies/cwrc-ONTOLOGY_DATE"/>
    <void:inDataset rdf:resource="#datasetdefinition"/>
  </owl:ObjectProperty>
  <owl:ObjectProperty rdf:ID="hasEthnicitySelfDefined">
    <rdfs:label xml:lang="en">has ethnicity (self defined)</rdfs:label>
    <rdfs:label xml:lang="fr">d'ethnicité (autodéclarée)</rdfs:label>
    <rdfs:subPropertyOf rdf:resource="#personalPropertySelfDefined"/>
    <rdfs:range rdf:resource="#Ethnicity"/>
    <skos:definition xml:lang="en"/>
    <skos:definition xml:lang="fr"/>
    <rdfs:isDefinedBy rdf:resource="http://sparql.cwrc.ca/ontologies/cwrc-ONTOLOGY_DATE"/>
    <void:inDataset rdf:resource="#datasetdefinition"/>
  </owl:ObjectProperty>
  <owl:ObjectProperty rdf:ID="hasReligion">
    <rdfs:label xml:lang="en">has religious affiliation</rdfs:label>
    <rdfs:label xml:lang="fr">est de confession</rdfs:label>
    <rdfs:subPropertyOf rdf:resource="#personalProperty"/>
    <rdfs:range rdf:resource="#Religion"/>
    <skos:definition xml:lang="en"/>
    <skos:definition xml:lang="fr"/>
    <rdfs:isDefinedBy rdf:resource="http://sparql.cwrc.ca/ontologies/cwrc-ONTOLOGY_DATE"/>
    <void:inDataset rdf:resource="#datasetdefinition"/>
  </owl:ObjectProperty>
  <owl:ObjectProperty rdf:ID="hasReligionSelfDefined">
    <rdfs:label xml:lang="en">has religious affilication (self defined)</rdfs:label>
    <rdfs:label xml:lang="fr">religion (autodéclarée)</rdfs:label>
    <rdfs:subPropertyOf rdf:resource="#personalPropertySelfDefined"/>
    <rdfs:range rdf:resource="#Religion"/>
    <skos:definition xml:lang="en"/>
    <skos:definition xml:lang="fr"/>
    <rdfs:isDefinedBy rdf:resource="http://sparql.cwrc.ca/ontologies/cwrc-ONTOLOGY_DATE"/>
    <void:inDataset rdf:resource="#datasetdefinition"/>
  </owl:ObjectProperty>
  <owl:ObjectProperty rdf:ID="hasSocialClass">
    <rdfs:label xml:lang="en">has social class</rdfs:label>
    <rdfs:label xml:lang="fr">de classe sociale</rdfs:label>
    <rdfs:subPropertyOf rdf:resource="#personalProperty"/>
    <rdfs:range rdf:resource="#SocialClass"/>
    <skos:definition xml:lang="en"/>
    <skos:definition xml:lang="fr"/>
    <rdfs:isDefinedBy rdf:resource="http://sparql.cwrc.ca/ontologies/cwrc-ONTOLOGY_DATE"/>
    <void:inDataset rdf:resource="#datasetdefinition"/>
  </owl:ObjectProperty>
  <owl:ObjectProperty rdf:ID="hasSocialClassSelfDefined">
    <rdfs:label xml:lang="en">has social class (self defined)</rdfs:label>
    <rdfs:label xml:lang="fr">de classe sociale (autodéclarés)</rdfs:label>
    <rdfs:subPropertyOf rdf:resource="#personalPropertySelfDefined"/>
    <rdfs:range rdf:resource="#SocialClass"/>
    <skos:definition xml:lang="en"/>
    <skos:definition xml:lang="fr"/>
    <rdfs:isDefinedBy rdf:resource="http://sparql.cwrc.ca/ontologies/cwrc-ONTOLOGY_DATE"/>
    <void:inDataset rdf:resource="#datasetdefinition"/>
  </owl:ObjectProperty>
  <owl:ObjectProperty rdf:ID="hasLinguisticAbility">
    <rdfs:label xml:lang="en">language known</rdfs:label>
    <rdfs:label xml:lang="fr">connait la langue</rdfs:label>
    <rdfs:subPropertyOf rdf:resource="#personalProperty"/>
    <rdfs:range rdf:resource="#LinguisticAbility"/>
    <skos:definition xml:lang="en">Knowlege of the language for writing or reading.</skos:definition>
    <skos:definition xml:lang="fr"/>
    <rdfs:isDefinedBy rdf:resource="http://sparql.cwrc.ca/ontologies/cwrc-ONTOLOGY_DATE"/>
    <void:inDataset rdf:resource="#datasetdefinition"/>
  </owl:ObjectProperty>
  <owl:ObjectProperty rdf:ID="hasLinguisticAbilitySelfDeclared">
    <rdfs:label xml:lang="en">language known (self declared)</rdfs:label>
    <rdfs:label xml:lang="fr">connait la langue (autodéclaré)</rdfs:label>
    <rdfs:subPropertyOf rdf:resource="#personalPropertySelfDeclared"/>
    <rdfs:range rdf:resource="#LinguisticAbility"/>
    <skos:definition xml:lang="en"/>
    <skos:definition xml:lang="fr"/>
    <rdfs:isDefinedBy rdf:resource="http://sparql.cwrc.ca/ontologies/cwrc-ONTOLOGY_DATE"/>
    <void:inDataset rdf:resource="#datasetdefinition"/>
  </owl:ObjectProperty>
  <owl:ObjectProperty rdf:ID="hasNativeLinguisticAbility">
    <rdfs:label xml:lang="en">natively known language</rdfs:label>
    <rdfs:label xml:lang="fr">a une langue maternelle</rdfs:label>
    <rdfs:subPropertyOf rdf:resource="#hasLinguisticAbility"/>
    <rdfs:range rdf:resource="#LinguisticAbility"/>
    <skos:definition xml:lang="en">Knowledge of the language for writing or reading.</skos:definition>
    <skos:definition xml:lang="fr"/>
    <rdfs:isDefinedBy rdf:resource="http://sparql.cwrc.ca/ontologies/cwrc-ONTOLOGY_DATE"/>
    <void:inDataset rdf:resource="#datasetdefinition"/>
  </owl:ObjectProperty>
  <owl:ObjectProperty rdf:ID="hasNativeLinguisticAbilitySelfDeclared">
    <rdfs:label xml:lang="en">natively known language (self declared)</rdfs:label>
    <rdfs:label xml:lang="fr">a une langue maternelle (autodéclaré)</rdfs:label>
    <rdfs:subPropertyOf rdf:resource="#hasLinguisticAbilitySelfDeclared"/>
    <rdfs:range rdf:resource="#LinguisticAbility"/>
    <skos:definition xml:lang="en"/>
    <skos:definition xml:lang="fr"/>
    <rdfs:isDefinedBy rdf:resource="http://sparql.cwrc.ca/ontologies/cwrc-ONTOLOGY_DATE"/>
    <void:inDataset rdf:resource="#datasetdefinition"/>
  </owl:ObjectProperty>
  <owl:ObjectProperty rdf:ID="hasSexuality">
    <rdfs:label xml:lang="en">has sexual orientation</rdfs:label>
    <rdfs:label xml:lang="fr">a une orientation sexuelle</rdfs:label>
    <rdfs:subPropertyOf rdf:resource="#personalProperty"/>
    <rdfs:range rdf:resource="#Sexuality"/>
    <skos:definition xml:lang="en"/>
    <skos:definition xml:lang="fr"/>
    <rdfs:isDefinedBy rdf:resource="http://sparql.cwrc.ca/ontologies/cwrc-ONTOLOGY_DATE"/>
    <void:inDataset rdf:resource="#datasetdefinition"/>
  </owl:ObjectProperty>
  <owl:ObjectProperty rdf:ID="hasSexualitySelfDeclared">
    <rdfs:label xml:lang="en">has sexual orientation (self declared)</rdfs:label>
    <rdfs:label xml:lang="fr">a une orientation sexuelle (autodéclarée)</rdfs:label>
    <rdfs:subPropertyOf rdf:resource="#personalPropertySelfDeclared"/>
    <rdfs:range rdf:resource="#Sexuality"/>
    <skos:definition xml:lang="en"/>
    <skos:definition xml:lang="fr"/>
    <rdfs:isDefinedBy rdf:resource="http://sparql.cwrc.ca/ontologies/cwrc-ONTOLOGY_DATE"/>
    <void:inDataset rdf:resource="#datasetdefinition"/>
  </owl:ObjectProperty>
  <owl:ObjectProperty rdf:ID="hasGeographicHeritage">
    <rdfs:label xml:lang="en">has Geographic Heritage</rdfs:label>
    <rdfs:label xml:lang="fr">A un héritage géographique</rdfs:label>
    <rdfs:subPropertyOf rdf:resource="#personalProperty"/>
    <rdfs:range rdf:resource="#GeographicHeritage"/>
    <skos:definition xml:lang="en"/>
    <skos:definition xml:lang="fr"/>
    <rdfs:isDefinedBy rdf:resource="http://sparql.cwrc.ca/ontologies/cwrc-ONTOLOGY_DATE"/>
    <void:inDataset rdf:resource="#datasetdefinition"/>
  </owl:ObjectProperty>
  <owl:ObjectProperty rdf:ID="hasGeographicHeritageSelfDeclared">
    <rdfs:label xml:lang="en">has geographic heritage (self declared)</rdfs:label>
    <rdfs:label xml:lang="fr">a un héritage géographique (autodéclaré)</rdfs:label>
    <rdfs:subPropertyOf rdf:resource="#personalProperty"/>
    <rdfs:range rdf:resource="#GeographicHeritage"/>
    <skos:definition xml:lang="en"/>
    <skos:definition xml:lang="fr"/>
    <rdfs:isDefinedBy rdf:resource="http://sparql.cwrc.ca/ontologies/cwrc-ONTOLOGY_DATE"/>
    <void:inDataset rdf:resource="#datasetdefinition"/>
  </owl:ObjectProperty>
  <!-- Labels -->
  <skos:ConceptScheme rdf:about="#TextLabels">
    <rdfs:label xml:lang="en">text labels</rdfs:label>
    <rdfs:label xml:lang="fr">blanc</rdfs:label>
    <skos:definition xml:lang="en">Collection of all ambiguous labels within the Orlando markup.</skos:definition>
    <skos:definition xml:lang="fr"/>
    <rdfs:isDefinedBy rdf:resource="http://sparql.cwrc.ca/ontologies/cwrc-ONTOLOGY_DATE"/>
    <void:inDataset rdf:resource="#datasetdefinition"/>
  </skos:ConceptScheme>
  <!-- add rdfvalue to everything -->
  <skos:Concept rdf:about="#whiteLabel">
    <rdfs:label xml:lang="en">white</rdfs:label>
    <rdfs:label xml:lang="fr">blanc</rdfs:label>
    <foaf:name xml:lang="en">white</foaf:name>
    <skos:definition xml:lang="en"/>
    <skos:definition xml:lang="fr"/>
    <rdf:type rdf:resource="http://www.w3.org/2008/05/skos-xl#Label"/>
    <owl:oneOf rdf:parseType="Collection">
      <owl:Thing rdf:about="#whiteEthnicity"/>
      <owl:Thing rdf:about="#whiteRace"/>
    </owl:oneOf>
    <skos:inScheme rdf:resource="#TextLabels"/>
    <rdfs:isDefinedBy rdf:resource="http://sparql.cwrc.ca/ontologies/cwrc-ONTOLOGY_DATE"/>
    <void:inDataset rdf:resource="#datasetdefinition"/>
  </skos:Concept>
  <skos:Concept rdf:about="#blackLabel">
    <rdfs:label xml:lang="en">black</rdfs:label>
    <rdfs:label xml:lang="fr">noir</rdfs:label>
    <foaf:name xml:lang="en">black</foaf:name>
    <skos:definition xml:lang="en"/>
    <skos:definition xml:lang="fr"/>
    <rdf:type rdf:resource="http://www.w3.org/2008/05/skos-xl#Label"/>
    <skos:inScheme rdf:resource="#TextLabels"/>
    <rdfs:isDefinedBy rdf:resource="http://sparql.cwrc.ca/ontologies/cwrc-ONTOLOGY_DATE"/>
    <void:inDataset rdf:resource="#datasetdefinition"/>
  </skos:Concept>
  <skos:Concept rdf:about="#englishLabel">
    <rdf:value>english</rdf:value>
    <rdfs:label xml:lang="en">english</rdfs:label>
    <rdfs:label xml:lang="fr">englais</rdfs:label>
    <foaf:name xml:lang="en">english</foaf:name>
    <skos:definition xml:lang="en"/>
    <skos:definition xml:lang="fr"/>
    <rdf:type rdf:resource="http://www.w3.org/2008/05/skos-xl#Label"/>
    <owl:oneOf rdf:parseType="Collection">
      <owl:Thing rdf:about="#EnglishNationalHeritage"/>
      <owl:Thing rdf:about="#EnglishLanguage"/>
      <owl:Thing rdf:about="#EnglishNationalIdentity"/>
    </owl:oneOf>
    <skos:inScheme rdf:resource="#TextLabels"/>
    <rdfs:isDefinedBy rdf:resource="http://sparql.cwrc.ca/ontologies/cwrc-ONTOLOGY_DATE"/>
    <void:inDataset rdf:resource="#datasetdefinition"/>
  </skos:Concept>
  <skos:Concept rdf:about="#manLabel">
    <rdf:value>man</rdf:value>
    <rdfs:label xml:lang="en">man</rdfs:label>
    <rdfs:label xml:lang="fr">homme</rdfs:label>
    <foaf:name xml:lang="en">Man (Label)</foaf:name>
    <skos:definition xml:lang="en"/>
    <skos:definition xml:lang="fr"/>
    <rdf:type rdf:resource="http://www.w3.org/2008/05/skos-xl#Label"/>
    <owl:oneOf rdf:parseType="Collection">
      <owl:Thing rdf:about="#genderManMale"/>
    </owl:oneOf>
    <skos:inScheme rdf:resource="#TextLabels"/>
    <rdfs:isDefinedBy rdf:resource="http://sparql.cwrc.ca/ontologies/cwrc-ONTOLOGY_DATE"/>
    <void:inDataset rdf:resource="#datasetdefinition"/>
  </skos:Concept>
  <skos:Concept rdf:about="#womanLabel">
    <rdf:value>woman</rdf:value>
    <rdfs:label xml:lang="en">woman</rdfs:label>
    <rdfs:label xml:lang="fr">femme</rdfs:label>
    <foaf:name xml:lang="en">Woman (Label)</foaf:name>
    <skos:definition xml:lang="en"/>
    <skos:definition xml:lang="fr"/>
    <rdf:type rdf:resource="http://www.w3.org/2008/05/skos-xl#Label"/>
    <owl:oneOf rdf:parseType="Collection">
      <owl:Thing rdf:about="#genderWomanFemale"/>
    </owl:oneOf>
    <skos:inScheme rdf:resource="#TextLabels"/>
    <rdfs:isDefinedBy rdf:resource="http://sparql.cwrc.ca/ontologies/cwrc-ONTOLOGY_DATE"/>
    <void:inDataset rdf:resource="#datasetdefinition"/>
  </skos:Concept>
  <skos:Concept rdf:about="#maleLabel">
    <rdf:value>male</rdf:value>
    <rdfs:label xml:lang="en">male</rdfs:label>
    <rdfs:label xml:lang="fr">male</rdfs:label>
    <foaf:name xml:lang="en">Male (Label)</foaf:name>
    <skos:definition xml:lang="en"/>
    <skos:definition xml:lang="fr"/>
    <rdf:type rdf:resource="http://www.w3.org/2008/05/skos-xl#Label"/>
    <owl:oneOf rdf:parseType="Collection">
      <owl:Thing rdf:about="#genderManMale"/>
      <owl:Thing rdf:about="#maleSex"/>
    </owl:oneOf>
    <skos:inScheme rdf:resource="#TextLabels"/>
    <rdfs:isDefinedBy rdf:resource="http://sparql.cwrc.ca/ontologies/cwrc-ONTOLOGY_DATE"/>
    <void:inDataset rdf:resource="#datasetdefinition"/>
  </skos:Concept>
  <skos:Concept rdf:about="#FemaleLabel">
    <rdf:value>female</rdf:value>
    <rdfs:label xml:lang="en">female</rdfs:label>
    <rdfs:label xml:lang="fr">femelle</rdfs:label>
    <foaf:name xml:lang="en">Female (Label)</foaf:name>
    <skos:definition xml:lang="en"/>
    <skos:definition xml:lang="fr"/>
    <rdf:type rdf:resource="http://www.w3.org/2008/05/skos-xl#Label"/>
    <owl:oneOf rdf:parseType="Collection">
      <owl:Thing rdf:about="#genderWomanFemale"/>
      <owl:Thing rdf:about="#femaleSex"/>
    </owl:oneOf>
    <skos:inScheme rdf:resource="#TextLabels"/>
    <rdfs:isDefinedBy rdf:resource="http://sparql.cwrc.ca/ontologies/cwrc-ONTOLOGY_DATE"/>
    <void:inDataset rdf:resource="#datasetdefinition"/>
  </skos:Concept>
  <skos:Concept rdf:about="#jewishLabel">
    <rdfs:label xml:lang="en">Jewish</rdfs:label>
    <rdfs:label xml:lang="fr">Juif</rdfs:label>
    <foaf:name xml:lang="en">Jewish</foaf:name>
    <skos:definition xml:lang="en"/>
    <skos:definition xml:lang="fr"/>
    <rdf:type rdf:resource="http://www.w3.org/2008/05/skos-xl#Label"/>
    <owl:oneOf rdf:parseType="Collection">
      <owl:Thing rdf:about="#judaism"/>
      <owl:Thing rdf:about="#jewishEthnicity"/>
      <owl:Thing rdf:about="#jewishGeographicalHeritage"/>
      <owl:Thing rdf:about="#jewishNationalIdentity"/>
    </owl:oneOf>
    <skos:inScheme rdf:resource="#TextLabels"/>
    <rdfs:isDefinedBy rdf:resource="http://sparql.cwrc.ca/ontologies/cwrc-ONTOLOGY_DATE"/>
    <void:inDataset rdf:resource="#datasetdefinition"/>
  </skos:Concept>
  <skos:Concept rdf:about="#englandLabel">
    <rdfs:label xml:lang="en">England</rdfs:label>
    <rdfs:label xml:lang="fr">Angleterre</rdfs:label>
    <foaf:name xml:lang="en">England</foaf:name>
    <skos:definition xml:lang="en"/>
    <skos:definition xml:lang="fr"/>
    <rdf:type rdf:resource="http://www.w3.org/2008/05/skos-xl#Label"/>
    <owl:oneOf rdf:parseType="Collection">
      <owl:Thing rdf:about="#england"/>
    </owl:oneOf>
    <skos:inScheme rdf:resource="#TextLabels"/>
    <rdfs:isDefinedBy rdf:resource="http://sparql.cwrc.ca/ontologies/cwrc-ONTOLOGY_DATE"/>
    <void:inDataset rdf:resource="#datasetdefinition"/>
  </skos:Concept>
  <!-- Genres -->
  <owl:Class rdf:ID="Genre">
    <rdfs:label xml:lang="en">literary genre</rdfs:label>
    <rdfs:label xml:lang="fr">genre littéraire</rdfs:label>
    <rdf:type rdf:resource="http://www.w3.org/2004/02/skos/core#ConceptScheme"/>
    <skos:definition xml:lang="en"/>
    <skos:definition xml:lang="fr"/>
    <owl:sameAs rdf:resource="http://dbpedia.org/resource/Literary_genre"/>
    <rdfs:isDefinedBy rdf:resource="http://sparql.cwrc.ca/ontologies/cwrc-ONTOLOGY_DATE"/>
    <void:inDataset rdf:resource="#datasetdefinition"/>
  </owl:Class>
  <owl:ObjectProperty rdf:ID="hasGenre">
    <rdfs:label xml:lang="en">has genre</rdfs:label>
    <rdfs:label xml:lang="fr">a un genre</rdfs:label>
    <skos:definition xml:lang="en"/>
    <skos:definition xml:lang="fr"/>
    <rdfs:isDefinedBy rdf:resource="http://sparql.cwrc.ca/ontologies/cwrc-ONTOLOGY_DATE"/>
    <void:inDataset rdf:resource="#datasetdefinition"/>
  </owl:ObjectProperty>
  <!-- Moved to cwrc_genre.owl for now -->


</rdf:RDF>
