<?xml version="1.0" encoding="UTF-8"?>
<rdf:RDF xml:base="http://sparql.cwrc.ca/ontologies/genre#"
  xmlns="http://sparql.cwrc.ca/ontologies/genre#"
  xmlns:as="http://www.w3.org/ns/activitystreams#"
  xmlns:cc="http://creativecommons.org/ns#"
  xmlns:cwrc="http://sparql.cwrc.ca/ontologies/cwrc#"
  xmlns:dbpedia="http://dbpedia.org/resource/"
  xmlns:dcterms="http://purl.org/dc/terms/"
  xmlns:doap="http://usefulinc.com/ns/doap#"
  xmlns:eurovoc="http://eurovoc.europa.eu/"
  xmlns:foaf="http://xmlns.com/foaf/0.1/"
  xmlns:genre="http://sparql.cwrc.ca/ontologies/genre#"
  xmlns:geonames="http://sws.geonames.org/"
  xmlns:loc="http://id.loc.gov/vocabulary/relators/"
  xmlns:nif="http://persistence.uni-leipzig.org/nlp2rdf/ontologies/nif-core#"
  xmlns:oa="http://www.w3.org/ns/oa#"
  xmlns:owl="http://www.w3.org/2002/07/owl#"
  xmlns:prov="http://www.w3.org/ns/prov#"
  xmlns:rdf="http://www.w3.org/1999/02/22-rdf-syntax-ns#"
  xmlns:rdfs="http://www.w3.org/2000/01/rdf-schema#"
  xmlns:skos="http://www.w3.org/2004/02/skos/core#"
  xmlns:skosxl="http://www.w3.org/2008/05/skos-xl#"
  xmlns:time="http://www.w3.org/2006/time#"
  xmlns:vann="http://purl.org/vocab/vann/"
  xmlns:void="http://rdfs.org/ns/void#"
  xmlns:vs="http://www.w3.org/2003/06/sw-vocab-status/ns#"
  xmlns:xsd="http://www.w3.org/2001/XMLSchema#">
  <owl:Ontology rdf:about="">
    <rdf:type rdf:resource="http://purl.org/vocommons/voaf#Vocabulary"/>
    <vann:preferredNamespacePrefix>genre</vann:preferredNamespacePrefix>
    <vann:preferredNamespaceUri>http://sparql.cwrc.ca/ontologies/genre#</vann:preferredNamespaceUri>
    <dcterms:title xml:lang="en">The CWRC Genre Ontology</dcterms:title>
    <rdfs:isDefinedBy rdf:resource="http://sparql.cwrc.ca/ontologies/genre-ONTOLOGY_DATE"/>
    <rdfs:label xml:lang="en">The CWRC Genre Ontology</rdfs:label>
    <foaf:name xml:lang="en">The CWRC Genre Ontology</foaf:name>
    <dcterms:title xml:lang="fr">L'Ontologie des genres CWRC</dcterms:title>
    <rdfs:label xml:lang="fr">L'Ontologie des genres CWRC</rdfs:label>
    <foaf:name xml:lang="fr">L'Ontologie des genres CWRC</foaf:name>
    <dcterms:description xml:lang="en">The CWRC Genre Ontology is the ontology used by the Canadian Writing Research Collaboratory to assign Genres to different types of cultural objects, particularly but not exclusively written ones.</dcterms:description>
    <skos:definition xml:lang="en">The CWRC Genre Ontology is the ontology used by the Canadian Writing Research Collaboratory to assign Genres to different types of cultural objects, particularly but not exclusively written ones.</skos:definition>
    <rdfs:comment xml:lang="en">The CWRC Genre Ontology is the ontology used by the Canadian Writing Research Collaboratory to assign  Genres to different types of cultural objects, particularly but not exclusively written ones.</rdfs:comment>
    <dcterms:description xml:lang="fr">L'Ontologie des genres CWRC est l'ontologie utilisée par le Collaboratoire scientifique des écrits du Canada pour assigner des genres à des écrits littéraires.</dcterms:description>
    <skos:definition xml:lang="fr">L'Ontologie des genres CWRC est l'ontologie utilisée par le Collaboratoire scientifique des écrits du Canada pour assigner des genres à des écrits littéraires.</skos:definition>
    <rdfs:comment xml:lang="fr">L'Ontologie des genres CWRC est l'ontologie utilisée par le Collaboratoire scientifique des écrits du Canada pour assigner des genres à des écrits littéraires.</rdfs:comment>
    <owl:versionInfo>0.7</owl:versionInfo>
    <owl:priorVersion rdf:resource="http://sparql.cwrc.ca/ontologies/genre-2019-07-09"/>
    <dcterms:date rdf:datatype="http://www.w3.org/2001/XMLSchema#date">ONTOLOGY_DATE</dcterms:date>
    <dcterms:rights rdf:resource="https://creativecommons.org/licenses/by/3.0/"/>
    <vs:term_status xml:lang="en">Testing</vs:term_status>
    <dcterms:creator>
      <cwrc:NaturalPerson rdf:about="http://sparql.cwrc.ca/ontologies/cwrc#AbigelLemak">
        <foaf:name>Abigel Lemak</foaf:name>
        <owl:sameAs rdf:resource="https://orcid.org/0000-0002-4275-5140"/>
      </cwrc:NaturalPerson>
    </dcterms:creator>
    <dcterms:creator>
      <cwrc:NaturalPerson rdf:about="http://sparql.cwrc.ca/ontologies/cwrc#JadePenancier">
        <foaf:name>Jade Penancier</foaf:name>
      </cwrc:NaturalPerson>
    </dcterms:creator>
    <dcterms:creator>
      <cwrc:NaturalPerson rdf:about="http://sparql.cwrc.ca/ontologies/cwrc#KimMartin">
        <foaf:name>Kim Martin</foaf:name>
        <owl:sameAs rdf:resource="https://orcid.org/0000-0003-0945-0158"/>
      </cwrc:NaturalPerson>
    </dcterms:creator>
    <dcterms:creator>
      <cwrc:NaturalPerson rdf:about="http://sparql.cwrc.ca/ontologies/cwrc#MicaelaJimenez">
        <foaf:name>Micaela Jimenez</foaf:name>
      </cwrc:NaturalPerson>
    </dcterms:creator>
    <dcterms:creator rdf:resource="http://sparql.cwrc.ca/ontologies/cwrc#SusanBrown"/>
    <dcterms:creator>
      <cwrc:NaturalPerson rdf:about="http://sparql.cwrc.ca/ontologies/cwrc#RobWarren">
        <foaf:name>Robert Warren</foaf:name>
        <owl:sameAs rdf:resource="http://rdf.muninn-project.org/ww1/2011/11/11/Person/Warren"/>
        <foaf:homepage rdf:resource="http://www.dbdump.org/"/>
      </cwrc:NaturalPerson>
    </dcterms:creator>
    <dcterms:creator>
      <cwrc:NaturalPerson rdf:about="http://sparql.cwrc.ca/ontologies/cwrc#AlliyyaMo">
        <foaf:name>Alliyya Mo</foaf:name>
        <owl:sameAs rdf:resource="https://orcid.org/0000-0002-6159-7694"/>
      </cwrc:NaturalPerson>
    </dcterms:creator>
    <dcterms:creator>
      <cwrc:NaturalPerson rdf:about="http://sparql.cwrc.ca/ontologies/cwrc#JasmineDrudgeWillson">
        <foaf:name>Jasmine Drudge-Willson</foaf:name>
      </cwrc:NaturalPerson>
    </dcterms:creator>
    <dcterms:creator>
      <cwrc:NaturalPerson rdf:about="http://sparql.cwrc.ca/ontologies/cwrc#JoelCummings">
        <foaf:name>Joel Cummings</foaf:name>
        <owl:sameAs rdf:resource="https://orcid.org/0000-0002-9100-3316"/>
      </cwrc:NaturalPerson>
    </dcterms:creator>
    <dcterms:creator>
      <cwrc:NaturalPerson rdf:about="http://sparql.cwrc.ca/ontologies/cwrc#DebStacey">
        <foaf:name>Deborah Stacey</foaf:name>
        <foaf:homepage rdf:resource="http://www.dastacey.ca/"/>
        <owl:sameAs rdf:resource="https://orcid.org/0000-0002-2019-9905"/>
      </cwrc:NaturalPerson>
    </dcterms:creator>
    <dcterms:creator>
      <cwrc:NaturalPerson rdf:about="http://sparql.cwrc.ca/ontologies/cwrc#HannahStewart">
        <foaf:name>Hannah Stewart</foaf:name>
      </cwrc:NaturalPerson>
    </dcterms:creator>
    <dcterms:creator>
      <cwrc:NaturalPerson rdf:about="http://sparql.cwrc.ca/ontologies/cwrc#ThomasSmith">
        <foaf:name>Thomas Smith</foaf:name>
      </cwrc:NaturalPerson>
    </dcterms:creator>
    <dcterms:creator>
      <cwrc:NaturalPerson rdf:about="http://sparql.cwrc.ca/ontologies/cwrc#MichaelaRye">
        <foaf:name>Michaela Rye</foaf:name>
      </cwrc:NaturalPerson>
    </dcterms:creator>
    <dcterms:publisher>
      <foaf:Organization rdf:about="http://sparql.cwrc.ca/ontologies/cwrc#cwrc">
        <foaf:name xml:lang="fr">Le Collaboratoire scientifique des écrits du Canada</foaf:name>
        <foaf:name xml:lang="en">The Canadian Writing Research Collaboratory</foaf:name>
        <foaf:logo rdf:resource="http://sparql.cwrc.ca/images/CWRCLogo-Horz-FullColour.png"/>
      </foaf:Organization>
    </dcterms:publisher>
    <loc:pdr>
      <cwrc:NaturalPerson rdf:about="http://sparql.cwrc.ca/ontologies/cwrc#SusanBrown">
        <foaf:name>Susan Brown</foaf:name>
        <owl:sameAs rdf:resource="http://orcid.org/0000-0002-0267-7344"/>
        <foaf:homepage rdf:resource="http://www.uoguelph.ca/~sbrown/"/>
      </cwrc:NaturalPerson>
    </loc:pdr>
    <loc:ctb>
      <cwrc:NaturalPerson rdf:about="http://sparql.cwrc.ca/ontologies/cwrc#DianeJakacki">
        <foaf:name>Diane Jakacki</foaf:name>
        <owl:sameAs rdf:resource="https://orcid.org/0000-0002-7836-1223"/>
      </cwrc:NaturalPerson>
    </loc:ctb>
    <loc:ctb>
      <cwrc:NaturalPerson rdf:about="http://sparql.cwrc.ca/ontologies/cwrc#CarolynBlack">
        <foaf:name>Carolyn Black</foaf:name>
      </cwrc:NaturalPerson>
    </loc:ctb>
    <loc:fnd>
      <foaf:Organization rdf:about="http://sparql.cwrc.ca/ontologies/cwrc#sshrc">
        <foaf:name xml:lang="en">Social Sciences and Humanities Research Council</foaf:name>
        <foaf:name xml:lang="fr">Conseil de recherches en sciences humaines</foaf:name>
        <foaf:nick>SSHRC</foaf:nick>
      </foaf:Organization>
    </loc:fnd>
    <void:inDataset rdf:resource="#datasetdefinition"/>
    <foaf:logo rdf:resource="http://sparql.cwrc.ca/images/CWRCLogo-Horz-FullColour.png"/>
    <dcterms:subject rdf:resource="http://id.loc.gov/authorities/subjects/sh85077490"/>
  </owl:Ontology>
  <void:Dataset rdf:about="#datasetdefinition">
    <dcterms:title xml:lang="en">The CWRC Literary Genre Ontology</dcterms:title>
    <rdfs:isDefinedBy rdf:resource="http://sparql.cwrc.ca/ontologies/genre-ONTOLOGY_DATE"/>
    <rdfs:label xml:lang="en">The CWRC Literary Genre Ontology</rdfs:label>
    <foaf:name xml:lang="en">The CWRC Literary Genre Ontology</foaf:name>
    <dcterms:title xml:lang="fr">L'Ontologie des genres littéraires CWRC</dcterms:title>
    <rdfs:label xml:lang="fr">L'Ontologie des genres littéraires CWRC</rdfs:label>
    <foaf:name xml:lang="fr">L'Ontologie des genres littéraires CWRC</foaf:name>
    <dcterms:description xml:lang="en">The CWRC Literary Genre Ontology is the ontology used by the Canadian Writing Research Collaboratory to assign Literary Genres to different documents.</dcterms:description>
    <skos:definition xml:lang="en">The CWRC Literary Genre Ontology is the ontology used by the Canadian Writing Research Collaboratory to assign Literary Genres to different documents.</skos:definition>
    <rdfs:comment xml:lang="en">The CWRC Literary Genre Ontology is the ontology used by the Canadian Writing Research Collaboratory to assign Literary Genres to different documents.</rdfs:comment>
    <dcterms:description xml:lang="fr">L'Ontologie des genres littéraires CWRC est l'ontologie utilisée par le Collaboratoire scientifique des écrits du Canada pour assigner des genres à des écrits littéraires.</dcterms:description>
    <skos:definition xml:lang="fr">L'Ontologie des genres littéraires CWRC est l'ontologie utilisée par le Collaboratoire scientifique des écrits du Canada pour assigner des genres à des écrits littéraires.</skos:definition>
    <rdfs:comment xml:lang="fr">L'Ontologie des genres littéraires CWRC est l'ontologie utilisée par le Collaboratoire scientifique des écrits du Canada pour assigner des genres à des écrits littéraires.</rdfs:comment>
    <cc:license rdf:resource="https://creativecommons.org/licenses/by/3.0/"/>
    <cc:Jurisdiction rdf:resource="http://dbpedia.org/resource/Canada"/>
    <cc:attributionURL rdf:resource="http://www.cwrc.ca/"/>
    <dcterms:publisher rdf:resource="http://sparql.cwrc.ca/ontologies/cwrc#cwrc"/>
    <dcterms:creator rdf:resource="http://sparql.cwrc.ca/ontologies/cwrc#MicaelaJimenez"/>
    <dcterms:creator rdf:resource="http://sparql.cwrc.ca/ontologies/cwrc#RobWarren"/>
    <dcterms:creator rdf:resource="http://sparql.cwrc.ca/ontologies/cwrc#JadePenancier"/>
    <dcterms:creator rdf:resource="http://sparql.cwrc.ca/ontologies/cwrc#AlliyyaMo"/>
    <dcterms:creator rdf:resource="http://sparql.cwrc.ca/ontologies/cwrc#DebStacey"/>
    <dcterms:creator rdf:resource="http://sparql.cwrc.ca/ontologies/cwrc#JoelCummings"/>
    <dcterms:creator rdf:resource="http://sparql.cwrc.ca/ontologies/cwrc#SusanBrown"/>
    <dcterms:creator rdf:resource="http://sparql.cwrc.ca/ontologies/cwrc#HannahStewart"/>
    <dcterms:creator rdf:resource="http://sparql.cwrc.ca/ontologies/cwrc#ThomasSmith"/>
    <dcterms:creator rdf:resource="http://sparql.cwrc.ca/ontologies/cwrc#MichaelaRye"/>
    <loc:ctb rdf:resource="http://sparql.cwrc.ca/ontologies/cwrc#DianeJakacki"/>
    <loc:ctb rdf:resource="http://sparql.cwrc.ca/ontologies/cwrc#CarolynBlack"/>
    <loc:pdr rdf:resource="http://sparql.cwrc.ca/ontologies/cwrc#SusanBrown"/>
    <loc:fnd rdf:resource="http://sparql.cwrc.ca/ontologies/cwrc#sshrc"/>
    <rdfs:isDefinedBy rdf:resource="http://sparql.cwrc.ca/ontologies/genre-ONTOLOGY_DATE"/>
    <foaf:logo rdf:resource="http://www.cwrc.ca/wp-content/uploads/2010/11/CWRC_logo_v074.gif"/>
    <dcterms:subject rdf:resource="http://id.loc.gov/authorities/subjects/sh85077490"/>
    <void:triples>TOTAL_TRIPLES</void:triples>
    <void:entities>TOTAL_ENTITIES</void:entities>
  </void:Dataset>
  <skos:Concept rdf:about="http://sparql.cwrc.ca/ontologies/cwrc#originalOrlandoAuthor">
    <rdfs:isDefinedBy rdf:resource="http://sparql.cwrc.ca/ontologies/genre-ONTOLOGY_DATE"/>
    <rdfs:label xml:lang="en">Members of the Orlando Project</rdfs:label>
    <rdfs:label xml:lang="fr">Les membres du projet Orlando</rdfs:label>
    <rdf:type rdf:resource="http://xmlns.com/foaf/0.1/Group"/>
    <foaf:name xml:lang="en">Members of the Orlando Project.</foaf:name>
    <foaf:homepage rdf:resource="http://orlando.cambridge.org/public/svDocumentation?formname=t&amp;d_id=CREDITSANDACKNOWLEDGEMENTS"/>
    <skos:definition xml:lang="en">The collection of all persons having written entries for The Orlando Project.</skos:definition>
    <skos:definition xml:lang="fr">La collection de tous les auteurs du Projet Orlando.</skos:definition>
    <rdfs:isDefinedBy rdf:resource="http://sparql.cwrc.ca/ontologies/genre-ONTOLOGY_DATE"/>
    <void:inDataset rdf:resource="#datasetdefinition"/>
  </skos:Concept>
  <owl:ObjectProperty rdf:ID="hasMedium">
    <rdfs:isDefinedBy rdf:resource="http://sparql.cwrc.ca/ontologies/genre-ONTOLOGY_DATE"/>
    <rdfs:label xml:lang="en">has medium</rdfs:label>
    <skos:definition xml:lang="en">Describes the material used to produce a cultural work and/or the governing substance that defines a particular object, digital or otherwise. Objects may have multiple media.</skos:definition>
    <owl:inverseOf rdf:resource="#mediumOf"/>
    <void:inDataset rdf:resource="#datasetdefinition"/>
    <rdfs:range rdf:resource="#Medium"/>
  </owl:ObjectProperty>
  <owl:ObjectProperty rdf:ID="mediumOf">
    <rdfs:isDefinedBy rdf:resource="http://sparql.cwrc.ca/ontologies/genre-ONTOLOGY_DATE"/>
    <rdfs:label xml:lang="en">medium of</rdfs:label>
    <owl:inverseOf rdf:resource="#hasMedium"/>
    <void:inDataset rdf:resource="#datasetdefinition"/>
    <rdfs:range rdf:resource="#Medium"/>
  </owl:ObjectProperty>
  <owl:ObjectProperty rdf:ID="hasGenre">
    <rdfs:isDefinedBy rdf:resource="http://sparql.cwrc.ca/ontologies/genre-ONTOLOGY_DATE"/>
    <rdfs:label xml:lang="en">has genre</rdfs:label>
    <rdfs:label xml:lang="fr">a un genre</rdfs:label>
    <skos:definition xml:lang="en">Describes a cultural work as classified by this genre. A single work may be classified as belonging to multiple genres, which may overlap or even seem to be contradictory, such as @@#verseNovel@@s also classified as @@#poetry@@ and @@#fiction@@. </skos:definition>
    <skos:definition xml:lang="fr">Décrit le genre d'une personne. De même que pour les autres formes culturelles, une même personne peut cumuler plus d'une propriété ou description de ce type. Pour plus d'informations sur cette propriété, voir @@#Genre@@.</skos:definition>
    <rdfs:isDefinedBy rdf:resource="http://sparql.cwrc.ca/ontologies/genre-ONTOLOGY_DATE"/>
    <skos:narrower rdf:resource="http://id.loc.gov/ontologies/bibframe/genreForm"/>
    <void:inDataset rdf:resource="#datasetdefinition"/>
    <!-- <rdfs:domain rdf:resource="#title"/> -->
    <rdfs:range rdf:resource="#Genre"/>
  </owl:ObjectProperty>
  <owl:ObjectProperty rdf:ID="genreOf">
    <rdfs:isDefinedBy rdf:resource="http://sparql.cwrc.ca/ontologies/genre-ONTOLOGY_DATE"/>
    <rdfs:label xml:lang="en">genre of</rdfs:label>
    <rdfs:label xml:lang="fr">genre de</rdfs:label>
    <owl:inverseOf rdf:resource="#hasGenre"/>
    <void:inDataset rdf:resource="#datasetdefinition"/>
  </owl:ObjectProperty>
  <owl:ObjectProperty rdf:ID="hasForm">
    <rdfs:label xml:lang="en">has form</rdfs:label>
    <rdfs:label xml:lang="fr">a un form</rdfs:label>
    <skos:definition xml:lang="en">Describes the form of a cultural artifact, including material form; type of publication such as serialization; or organization of content such as record. Objects often have multiple forms.</skos:definition>
    <skos:definition xml:lang="fr"></skos:definition>
    <rdfs:isDefinedBy rdf:resource="http://sparql.cwrc.ca/ontologies/genre-ONTOLOGY_DATE"/>
    <skos:narrower rdf:resource="http://id.loc.gov/ontologies/bibframe/genreForm"/>
    <void:inDataset rdf:resource="#datasetdefinition"/>
    <rdfs:range rdf:resource="#Form"/>
  </owl:ObjectProperty>
  <owl:ObjectProperty rdf:ID="formOf">
    <rdfs:isDefinedBy rdf:resource="http://sparql.cwrc.ca/ontologies/genre-ONTOLOGY_DATE"/>
    <rdfs:label xml:lang="en">form of</rdfs:label>
    <rdfs:label xml:lang="fr">form de</rdfs:label>
    <owl:inverseOf rdf:resource="#hasForm"/>
    <rdfs:isDefinedBy rdf:resource="http://sparql.cwrc.ca/ontologies/genre-ONTOLOGY_DATE"/>
    <void:inDataset rdf:resource="#datasetdefinition"/>
  </owl:ObjectProperty>

  <genre:SatiricalGenre rdf:about="#antiromance">
    <rdfs:label xml:lang="en">anti-romance</rdfs:label>
    <rdfs:label xml:lang="fr"/>
    <skos:definition xml:lang="en">"An anti-romance, sometimes referred to as a satire, is a type of story characterized by having an apathetic or self-doubting anti-hero cast as the protagonist, who fails in the object of his journey or struggle. Most anti-romances take place in urban settings, and frequently feature insanity, depression, and the meaning of reality as major themes. An anti-romance is the antithesis of a romance." <![CDATA[<a href="#cwrc:727d97bc-af78-4122-94be-aa78b2e97d5a">(DBpedia, 2019)</a>]]></skos:definition>
    <skos:definition xml:lang="fr"/>
    <owl:sameAs rdf:resource="http://dbpedia.org/resource/Anti-romance"/>
    <rdfs:isDefinedBy rdf:resource="http://sparql.cwrc.ca/ontologies/genre-ONTOLOGY_DATE"/>
  </genre:SatiricalGenre>
  <genre:NovelisticGenre rdf:about="#kunstlerroman">
    <rdfs:label xml:lang="en">kunstlerroman</rdfs:label>
    <rdfs:label xml:lang="fr"/>
    <skos:hiddenLabel xml:lang="en">KUNSTLERROMAN</skos:hiddenLabel>
    <skos:definition xml:lang="fr"/>
    <skos:definition xml:lang="en">A @@#bildungsroman@@ in which the protagonist is an writer or some other type of artist.</skos:definition>
    <skos:narrower rdf:resource="#bildungsroman"/>
    <rdfs:isDefinedBy rdf:resource="http://sparql.cwrc.ca/ontologies/genre-ONTOLOGY_DATE"/>
  </genre:NovelisticGenre>
  <genre:ThematicGenre rdf:about="#pornography">
    <rdfs:label xml:lang="en">pornography</rdfs:label>
    <rdfs:label xml:lang="fr"/>
    <skos:definition xml:lang="fr"/>
    <skos:definition xml:lang="en">Creative works involving content that is sexually oriented and often arousing to their audiences; often distinguished from erotica by being more sexually explicit, or involving a power differential and the domination, objectification, or exploitation of women. Notwithstanding this common association, there are proponents of feminist pornography as a liberating genre, but anti-pornography feminists see a strong link between pornography and rape culture and understand pornography itself a form of violence against women. A pithy formulation is Robin Morgan's "Pornography is the theory, and rape is the practice" <![CDATA[<a href="#cwrc:97cff38b-7268-46fe-b33d-10b0c0623510">(Morgan 139)</a>]]>. See @@https://en.wikipedia.org/wiki/Pornography@@, @@https://en.wikipedia.org/wiki/Feminist_pornography@@, and @@https://en.wikipedia.org/wiki/Feminist_views_on_pornography#Anti-pornography_feminism@@</skos:definition>
    <rdfs:seeAlso rdf:resource="http://dbpedia.org/resource/Pornography"/>
    <rdfs:seeAlso rdf:resource="http://dbpedia.org/resource/Feminist_pornography"/>
    <rdfs:seeAlso rdf:resource="http://dbpedia.org/resource/Feminist_views_on_pornography"/>
    <skos:narrower rdf:resource="#eroticaOrPornography"/>
    <skos:related rdf:resource="#erotica"/>
    <rdfs:isDefinedBy rdf:resource="http://sparql.cwrc.ca/ontologies/genre-ONTOLOGY_DATE"/>
  </genre:ThematicGenre>
  <genre:ThematicGenre rdf:about="#eroticaOrPornography">
    <rdfs:label xml:lang="en">erotica or pornography</rdfs:label>
    <rdfs:label xml:lang="fr"/>
    <skos:hiddenLabel xml:lang="en">EROTICAPORNOGRAPHY</skos:hiddenLabel>
    <skos:definition xml:lang="fr"/>
    <skos:definition xml:lang="en">Creative works involving content that is sexually oriented, at times explicit, and often arousing to their audiences. Distinctions between erotica and pornography are historically and contextually influenced, often hotly contested, and reflect the subject position of the person making the classification. Many feminists including Gloria Steinem (cited in Wikipedia "Erotica") saw the two as distinguished by respect and reciprocity on the one hand and gender domination and objectification on the other, whereas Susanne Kappeler argued that common practices of representation are bound up in power differentials that can be pornographic without necessarily involving gender <![CDATA[<a href="#cwrc:26b39b85-62f3-484c-a2e8-e249b476b927">(Kappeler)</a>]]>. Notwithstanding the feminist anti-pornography movement of the 1980s associated with thinkers such as Andrea Dworkin, both erotica and pornography have been championed by pro-sex feminists. See @@https://en.wikipedia.org/wiki/Erotica@@, @@https://en.wikipedia.org/wiki/Pornography@@ and @@https://en.wikipedia.org/wiki/Feminist_pornography@@.</skos:definition>
    <rdfs:seeAlso rdf:resource="http://dbpedia.org/resource/Erotica"/>
    <rdfs:seeAlso rdf:resource="http://dbpedia.org/resource/Pornography"/>
    <rdfs:seeAlso rdf:resource="http://dbpedia.org/resource/Feminist_pornography"/>
    <rdfs:isDefinedBy rdf:resource="http://sparql.cwrc.ca/ontologies/genre-ONTOLOGY_DATE"/>
  </genre:ThematicGenre>
  <genre:EmbeddedWork rdf:about="#editorialWork">
    <rdfs:label xml:lang="en">editorial work</rdfs:label>
    <skos:hiddenLabel xml:lang="en">EDITING</skos:hiddenLabel>
    <rdfs:label xml:lang="fr"/>
    <skos:definition xml:lang="fr"/>
    <skos:definition xml:lang="en">An often invisible and unacknowledged type of cultural labour, paid or unpaid, that ranges from the selection and preparation of works, in a range of media including text, image, and film, for publication to the preparation of minutely researched scholarly editions by textual scholars. It can express care and attachment to a community <![CDATA[<a href="#cwrc:d4130c87-b761-46d3-b85c-96ed84d3e4f5">(Eichhorn and Milne)</a>]]> or  Editorial work has a shaping impact on cultural production and may manifest in changes to a cultural artifact that are distinct, as with the addition of explanatory notes, or embedded in traces throughout. See @@https://en.wikipedia.org/wiki/Editing@@</skos:definition>
    <rdfs:seeAlso rdf:resource="http://dbpedia.org/resource/Editing"/>
    <rdfs:isDefinedBy rdf:resource="http://sparql.cwrc.ca/ontologies/genre-ONTOLOGY_DATE"/>
  </genre:EmbeddedWork>
  <genre:FictionalGenre rdf:about="#characterSketch">
    <rdfs:label xml:lang="en">character sketch</rdfs:label>
    <rdfs:label xml:lang="fr"/>
    <skos:hiddenLabel xml:lang="en">CHARACTER</skos:hiddenLabel>
    <skos:definition xml:lang="fr"/>
    <skos:definition xml:lang="en">"A character sketch is an abbreviated portrayal of a particular characteristic of people. The term originates in portraiture, where the character sketch is a common academic exercise. Following the translation of Theophrastus's Characters into English, a number of British and American painters attempted to illustrate the "types" of humanity. As late as William Hogarth, portraitists were doing studies of (in his case) Nine heads. The artist performing a character sketch attempts to capture an expression or gesture that goes beyond coincident actions and gets to the essence of the individual." <![CDATA[<a href="#cwrc:727d97bc-af78-4122-94be-aa78b2e97d5a">(DBpedia, 2019)</a>]]></skos:definition>
    <rdfs:comment xml:lang="en">The description for this term is indebted to DBpedia. </rdfs:comment>
    <owl:sameAs rdf:resource="http://dbpedia.org/resource/Character_sketch"/>
    <rdfs:isDefinedBy rdf:resource="http://sparql.cwrc.ca/ontologies/genre-ONTOLOGY_DATE"/>
  </genre:FictionalGenre>
  <genre:FictionalGenre rdf:about="#realist">
    <rdfs:label xml:lang="fr">réaliste</rdfs:label>
    <dcterms:references rdf:resource="http://www.oxfordreference.com/view/10.1093/acref/9780199208272.001.0001/acref-9780199208272-e-954?rskey=CNr3ZX%26result=951"/>
    <rdfs:isDefinedBy rdf:resource="http://sparql.cwrc.ca/ontologies/genre-ONTOLOGY_DATE"/>
    <rdfs:label xml:lang="en">realist</rdfs:label>
    <skos:definition xml:lang="fr">«Terme général pour qualifier les œuvres d'art dans lesquelles la représentation du monde extérieur s'appuie ou semble s'appuyer sur une observation directe de celui-ci; ces oeuvres incluent ou mettent en valeur ses défauts et ses imperfections plutôt que d'en souligner la beauté ou d'idéaliser certains de ses aspetcs. Bien qu'une oeuvre puisse être à la fois réaliste et naturaliste, le naturalisme est susceptible d'idéaliser les défauts ou la laideur des thèmes abordés. Concernant le style formel et la période d'apparition des caractéristiques générales du réalisme, comme dans la peinture de Gustave Courbet, utilisez "Realist (dans les styles de beaux arts modernes européens)".»  <![CDATA[<a href="#cwrc:db2f8571-a773-4068-a35f-34262950bb8f">(Getty, 2017)</a>]]></skos:definition>
    <rdfs:comment xml:lang="en">This term and its description were created from data gathered from the Oxford Dictionary of Literary Terms, 4th ed.</rdfs:comment>
    <skos:definition xml:lang="en">"Fiction that attempts to capture life as it is, rejecting idealism in favour of exposing in detail the realities, including the flaws, of its characters and their lives."  <![CDATA[<a href="#cwrc:4c227091-6bf0-4325-b846-9733fae19e61">(Oxford, 2015)</a>]]></skos:definition>
  </genre:FictionalGenre>
  <genre:FictionalGenre rdf:about="#fairytale">
    <owl:sameAs rdf:resource="http://vocab.getty.edu/aat/300185684"/>
    <rdfs:comment xml:lang="en">The description for this term is indebted to DBpedia. </rdfs:comment>
    <owl:sameAs rdf:resource="http://id.loc.gov/authorities/genreForms/gf2014026329"/>
    <skos:definition xml:lang="fr">Récits se déroulant dans un passé lointain et racontant des événements impossibles dans la réalité, souvent magiques et avec des fées, mais avec des humains comme héros et héroïnes.</skos:definition>
    <rdfs:isDefinedBy rdf:resource="http://sparql.cwrc.ca/ontologies/genre-ONTOLOGY_DATE"/>
    <rdfs:label xml:lang="en">fairytale</rdfs:label>
    <skos:definition xml:lang="en">"Narratives set in the distant past recounting events impossible in the real world, often magical and with fairies, but with humans as heroes and heroines."  <![CDATA[<a href="#cwrc:db2f8571-a773-4068-a35f-34262950bb8f">(Getty, 2017)</a>]]></skos:definition>
    <rdfs:label xml:lang="fr">conte de fées</rdfs:label>
  </genre:FictionalGenre>
  <genre:ThematicGenre rdf:about="#guidebook">
    <skos:definition xml:lang="en">"Handbooks for the guidance of strangers or visitors in a district, town, building, etc., giving a description of the roads, places, or objects of interest to be found there."  <![CDATA[<a href="#cwrc:db2f8571-a773-4068-a35f-34262950bb8f">(Getty, 2017)</a>]]></skos:definition>
    <rdfs:comment xml:lang="en">The description for this term is indebted to the Getty Art &amp; Architecture Thesaurus.</rdfs:comment>
    <rdfs:label xml:lang="fr">guide de voyage</rdfs:label>
    <owl:sameAs rdf:resource="http://vocab.getty.edu/aat/300026300"/>
    <owl:sameAs rdf:resource="http://id.loc.gov/authorities/genreForms/gf2014026108"/>
    <skos:definition xml:lang="fr">Manuels destinés à guider des étrangers ou des visiteurs dans un quartier, une ville, un bâtiment, etc., en décrivant les routes, les lieux ou les sujets d'intérêt qui s'y trouvent.</skos:definition>
    <rdfs:isDefinedBy rdf:resource="http://sparql.cwrc.ca/ontologies/genre-ONTOLOGY_DATE"/>
    <rdfs:label xml:lang="en">guidebook</rdfs:label>
  </genre:ThematicGenre>
  <genre:ScholarlyGenre rdf:about="#treatise">
    <skos:definition xml:lang="en">"Formal and systematic written expositions of the principles of a subject, generally longer and more detailed than essays."  <![CDATA[<a href="#cwrc:db2f8571-a773-4068-a35f-34262950bb8f">(Getty, 2017)</a>]]></skos:definition>
    <owl:sameAs rdf:resource="http://dbpedia.org/resource/Treatise"/>
    <rdfs:isDefinedBy rdf:resource="http://sparql.cwrc.ca/ontologies/genre-ONTOLOGY_DATE"/>
    <rdfs:label xml:lang="en">treatise</rdfs:label>
    <rdfs:comment xml:lang="en">The description for this term is indebted to the Getty Art &amp; Architecture Thesaurus.</rdfs:comment>
    <skos:definition xml:lang="fr">«Un traité est un manuel d'instructions ou un livre standard dans n'importe quelle branche qui forme un sujet d'études. Ils se différencient les uns des autres, aussi bien par le public ciblé que par le sujet abordé. Les traités sont habituellement édités par des imprimeurs spécialisés, dans le but de répondre aux besoins de formation, sur n'importe quel thème susceptible de faire l'objet d'un enseignement. Il s'agit d'un important commerce qui nécessite des ventes massives, afin de rendre ces publications rentables. Bien que la plupart des traités soient uniquement édités sous forme de livres reliés, certains sont désormais consultables sur internet. Les traités sont apparus avec le développement de l'imprimerie de Johannes Gutenberg, sous la forme de méthodes d'enseignement.»  <![CDATA[<a href="#cwrc:727d97bc-af78-4122-94be-aa78b2e97d5a">(DBpedia, 2017)</a>]]></skos:definition>
  </genre:ScholarlyGenre>
  <genre:NovelisticGenre rdf:about="#novella">
    <skos:definition xml:lang="fr">Brèves histoires en prose populaires à la Renaissance, et ensuite formes de de prose intermédiaires entre le roman et la nouvelle.</skos:definition>
    <owl:sameAs rdf:resource="http://id.loc.gov/authorities/genreForms/gf2015026019"/>
    <owl:sameAs rdf:resource="http://vocab.getty.edu/aat/300202569"/>
    <rdfs:label xml:lang="fr">novella</rdfs:label>
    <rdfs:comment xml:lang="en">The description for this term is indebted to the Getty Art &amp; Architecture Thesaurus.</rdfs:comment>
    <skos:definition xml:lang="en">"Short prose tales popular in the Renaissance and for later prose narratives intermediate between novels and short stories."  <![CDATA[<a href="#cwrc:db2f8571-a773-4068-a35f-34262950bb8f">(Getty, 2017)</a>]]></skos:definition>
    <rdfs:isDefinedBy rdf:resource="http://sparql.cwrc.ca/ontologies/genre-ONTOLOGY_DATE"/>
    <rdfs:label xml:lang="en">novella</rdfs:label>
  </genre:NovelisticGenre>
  <genre:DialogueOrDebateGenre rdf:about="#polemic">
    <skos:definition xml:lang="fr">«Le terme de polémique (du grec πολεμικός, polêmikôs « qui concerne la guerre », « disposé à la guerre », polêmikon museion, musée de la guerre, « batailleur, querelleur ») désigne une discussion, un débat, une controverse qui traduit de façon violente ou passionnée, et le plus souvent par écrit, des opinions contraires sur toutes espèces de sujets (politique, scientifique, littéraire, religieux, etc.). Il fait aujourd'hui l'objet d'emplois multiples.»  <![CDATA[<a href="#cwrc:727d97bc-af78-4122-94be-aa78b2e97d5a">(DBpedia, 2017)</a>]]></skos:definition>
    <owl:sameAs rdf:resource="http://vocab.getty.edu/aat/300252982"/>
    <skos:definition xml:lang="en">"Aggressive, forcefully presented arguments, often disputing a policy or opinion."  <![CDATA[<a href="#cwrc:db2f8571-a773-4068-a35f-34262950bb8f">(Getty, 2017)</a>]]></skos:definition>
    <rdfs:comment xml:lang="en">The description for this term is indebted to DBpedia. </rdfs:comment>
    <rdfs:isDefinedBy rdf:resource="http://sparql.cwrc.ca/ontologies/genre-ONTOLOGY_DATE"/>
    <rdfs:label xml:lang="en">polemic</rdfs:label>
  </genre:DialogueOrDebateGenre>
  <genre:PrintMedium rdf:about="#offprint">
    <skos:closeMatch rdf:resource="http://dbpedia.org/resource/Offprint"/>
    <rdfs:isDefinedBy rdf:resource="http://sparql.cwrc.ca/ontologies/genre-ONTOLOGY_DATE"/>
    <rdfs:label xml:lang="en">offprint</rdfs:label>
    <owl:sameAs rdf:resource="http://id.loc.gov/vocabulary/marcgt/off.html"/>
    <skos:definition xml:lang="en">An offprint is a separate printing of a work that originally appeared as part of a larger publication, usually one of composite authorship such as an academic journal, magazine, or edited book. <![CDATA[<a href="#cwrc:727d97bc-af78-4122-94be-aa78b2e97d5a">(DBpedia, 2019)</a>]]></skos:definition>
  </genre:PrintMedium>
  <genre:FictionalGenre rdf:about="#magicRealist">
    <rdfs:isDefinedBy rdf:resource="http://sparql.cwrc.ca/ontologies/genre-ONTOLOGY_DATE"/>
    <rdfs:label xml:lang="en">magic realist</rdfs:label>
    <owl:sameAs rdf:resource="http://dbpedia.org/resource/Magic_realism"/>
    <skos:definition xml:lang="en">"A style of fiction popularized in Latin-American writing from the mid-twentieth century, in which magical or fantastical elements are not treated as unusual, but rather occur alongside realistic elements as a natural part of the narrative."  <![CDATA[<a href="#cwrc:7ff0c640-f273-46f5-be8d-e50aa27dce59">(Encyclopædia Britannica, 2017)</a>]]></skos:definition>
    <skos:definition xml:lang="fr">«Le réalisme magique est une appellation utilisée par la critique littéraire et la critique d’art depuis 1925 pour rendre compte de productions où des éléments perçus et décrétés comme « magiques », « surnaturels » et « irrationnels » qui surgissent dans un environnement défini comme « réaliste », à savoir un cadre historique, géographique et culturel vraisemblable. Ainsi la réalité reconnaissable devient-elle le lieu naturel de manifestations paranormales et oniriques. Aujourd'hui, cette appellation est surtout associée à certains auteurs de la littérature latino-américaine du XXe siècle comme les Mexicains Carlos Fuentes et Juan Rulfo, les Argentins Adolfo Bioy Casares et Julio Cortázar, le Bolivien Jaime Sáenz et le Colombien Gabriel García Márquez, prix Nobel de littérature en 1982, dont le roman Cent ans de solitude publié en 1967, est cité comme exemplaire. L’origine de ce terme et sa portée sont pourtant beaucoup plus généraux et ont été utilisés pour qualifier une grande variété de romans, de poèmes, de peintures et de réalisations cinématographiques. Par ailleurs, le réalisme magique connaît plusieurs déclinaisons et peut caractériser divers styles, esthétiques, genres, courants et mouvements en Asie, en Europe ou en Amérique. De manière plus récente, il est rapproché de la world literature. Généralement, il cherche à tisser des liens étroits entre des courants habituellement opposés tels que le naturalisme, le merveilleux et le fantastique afin de peindre une réalité transfigurée par l'imaginaire et dans laquelle le rationalisme est rejeté. Néanmoins, il n'existe pas de définition rigoureuse et son application dépend de la démarche intellectuelle et stylistique de l'écrivain ou l'artiste qui y a recours.»  <![CDATA[<a href="#cwrc:727d97bc-af78-4122-94be-aa78b2e97d5a">(DBpedia, 2017)</a>]]> </skos:definition>
    <owl:sameAs rdf:resource="http://id.loc.gov/authorities/genreForms/gf2014026424"/>
    <rdfs:label xml:lang="fr">réalisme magique</rdfs:label>
    <rdfs:comment xml:lang="en">This term and its description were created from data gathered from the Encyclopædia Britannica.</rdfs:comment>
  </genre:FictionalGenre>
  <genre:DramaticGenre rdf:about="#panegyric">
    <skos:definition xml:lang="en">"A speech or poem designed to praise another person or group. In ancient Greek and Roman rhetoric, it was one branch of public speaking, with established rules and conventions found in the works of Menander and Hermogenes. Famous examples include Pliny's eulogy on Emperor Trajan and Isocrates' oration on the Olympic games of 380."  <![CDATA[<a href="cwrc:509015ff-7641-473e-94c5-688e06952bb7">(L. K Wheeler, 2017)</a>]]></skos:definition>
    <rdfs:isDefinedBy rdf:resource="http://sparql.cwrc.ca/ontologies/genre-ONTOLOGY_DATE"/>
    <rdfs:label xml:lang="en">panegyric</rdfs:label>
    <dcterms:references rdf:resource="http://web.cn.edu/kwheeler/lit_terms_p.html"/>
    <skos:definition xml:lang="fr">«L’éloge panégyrique ou simplement le panégyrique, du latin emprunté au grec panêguris, « assemblée de tout le peuple », est au sens strict un discours public à la louange d'un personnage illustre, d'une nation, ou d'une chose et, dans l'occident chrétien, un sermon faisant l'éloge d'un saint. Le terme a pris aujourd'hui le sens plus général de louange ou d’apologie, et s’utilise parfois dans le sens péjoratif d’éloge emphatique ou exagéré.»  <![CDATA[<a href="#cwrc:727d97bc-af78-4122-94be-aa78b2e97d5a">(DBpedia, 2017)</a>]]></skos:definition>
    <rdfs:comment xml:lang="en">This term and its description were created from data gathered from DBpedia.</rdfs:comment>
    <skos:related rdf:resource="http://id.loc.gov/authorities/genreForms/gf2014026095"/>
    <rdfs:label xml:lang="fr">panégyrique</rdfs:label>
  </genre:DramaticGenre>
  <genre:AutobiographicalGenre rdf:about="#slaveNarrative">
    <rdfs:label xml:lang="fr">récit d'esclave</rdfs:label>
    <rdfs:isDefinedBy rdf:resource="http://sparql.cwrc.ca/ontologies/genre-ONTOLOGY_DATE"/>
    <rdfs:label xml:lang="en">slave narrative</rdfs:label>
    <skos:altLabel xml:lang="en">slavery</skos:altLabel>
    <owl:sameAs rdf:resource="http://id.loc.gov/authorities/genreForms/gf2014026176"/>
    <owl:sameAs rdf:resource="http://dbpedia.org/resource/Slave_narrative"/>
    <skos:definition xml:lang="en">"An autobiographical account of the life of an escaped or freed slave. Typically written and published in the Americas and used as a form of protest against the slave trade."  <![CDATA[<a href="#cwrc:4c227091-6bf0-4325-b846-9733fae19e61">(Oxford, 2015)</a>]]></skos:definition>
    <skos:definition xml:lang="fr">«Le récit d'esclave est type d’œuvre littéraires écrites par des esclaves, essentiellement africains au Royaume-Uni et dans ses colonies, y compris ensuite les États-Unis, le Canada, et les états caribéens. Quelque six mille anciens esclaves d'Amérique du nord et des caraïbes écrivirent sur leur vie durant les XVIIIe siècle et XIXe siècle, avec environ 150 récits publiés individuellement en livres ou en pamphlets. Aux États-Unis durant la grande dépression (années 1930), plus de 2 300 récits oraux de vie sous l'esclavage furent collectés par des écrivains financés et publiés par la Work Projects Administration (WPA) de l'administration du président Roosevelt. 26 de ses enregistrements audios sont aujourd'hui conservés à la bibliothèque du Congrès.»  <![CDATA[<a href="#cwrc:727d97bc-af78-4122-94be-aa78b2e97d5a">(DBpedia, 2017)</a>]]></skos:definition>
    <rdfs:comment xml:lang="en">This term and its description were created from data gathered from the Oxford Dictionary of Literary Terms, 4th ed.</rdfs:comment>
  </genre:AutobiographicalGenre>
  <genre:PoeticGenre rdf:about="#dramaticMonologue">
    <rdfs:comment xml:lang="en">The description for this term is indebted to DBpedia. </rdfs:comment>
    <skos:definition xml:lang="fr">«Un monologue dramatique est en France, à la fin du Moyen Âge, un type de poème comique à vocation scénique. À l’instar des jongleurs, l’acteur seul en scène incarnait plusieurs personnages stéréotypés. Il est considéré comme un des quatre grands genres comiques de la fin du Moyen Âge avec la sotie, le sermon joyeux et la farce. Dans l'Angleterre du XIXe siècle, le terme monologue dramatique (dramatic mononologue) désignait un type de poème, fort apprécié par de nombreux poètes de l'époque victorienne, dans lequel un personnage, de fiction ou historique, exprime ses sentiments, ses actions ou ses motifs dans un monologue. Celui-ci, dont les paroles sont souvent influencées par le contexte critique dans lequel elles sont prononcées, s'adresse en général à un auditoire silencieux.Des exemples de monologues dramatiques sont My Last Duchess de Robert Browning, The Captain of the 1984 Top of the Form Team de Carol Ann Duffy, ou encore Lady Lazarus de Sylvia Plath.»  <![CDATA[<a href="#cwrc:727d97bc-af78-4122-94be-aa78b2e97d5a">(DBpedia, 2017)</a>]]></skos:definition>
    <rdfs:isDefinedBy rdf:resource="http://sparql.cwrc.ca/ontologies/genre-ONTOLOGY_DATE"/>
    <rdfs:label xml:lang="en">dramatic monologue</rdfs:label>
    <owl:sameAs rdf:resource="http://id.loc.gov/authorities/genreForms/gf2014026298"/>
    <skos:definition xml:lang="en">"Dramatic monologue, also known as a persona poem, is a type of poetry written in the form of a speech of an individual character."  <![CDATA[<a href="#cwrc:727d97bc-af78-4122-94be-aa78b2e97d5a">(DBpedia, 2017)</a>]]></skos:definition>
    <owl:sameAs rdf:resource="http://dbpedia.org/resource/Dramatic_monologue"/>
    <rdf:type rdf:resource="#DramaticGenre"/>
  </genre:PoeticGenre>
  <genre:ThematicGenre rdf:about="#popular">
    <skos:definition xml:lang="en">"Visual arts produced by or for the general public, often reflecting fads and as a response to the daily environment; works produced for mass audiences as distinct from fine art and folk art."  <![CDATA[<a href="#cwrc:db2f8571-a773-4068-a35f-34262950bb8f">(Getty, 2017)</a>]]></skos:definition>
    <rdfs:label xml:lang="fr">populaire</rdfs:label>
    <rdfs:comment xml:lang="en">The description for this term is indebted to the Getty Art &amp; Architecture Thesaurus.</rdfs:comment>
    <skos:definition xml:lang="fr">Arts visuels élaborés par ou pour le grand public qui reflètent souvent des tendances et font écho à la vie quotidienne. Œuvres produites pour le public de masse et qui se distinguent des beaux arts et de l'artisanat.</skos:definition>
    <rdfs:isDefinedBy rdf:resource="http://sparql.cwrc.ca/ontologies/genre-ONTOLOGY_DATE"/>
    <rdfs:label xml:lang="en">popular</rdfs:label>
    <owl:sameAs rdf:resource="http://vocab.getty.edu/aat/300311927"/>
  </genre:ThematicGenre>
  <genre:InformationalGenre rdf:about="#genealogy">
    <rdfs:comment xml:lang="en">The description for this term is indebted to the Getty Art &amp; Architecture Thesaurus.</rdfs:comment>
    <skos:related rdf:resource="http://id.loc.gov/authorities/genreForms/gf2014026100"/>
    <skos:definition xml:lang="en">"Accounts or histories of the descent of persons, families, or other groups, from an ancestor or ancestors; enumerations of ancestors and their descendants in the natural order of succession."  <![CDATA[<a href="#cwrc:db2f8571-a773-4068-a35f-34262950bb8f">(Getty, 2017)</a>]]></skos:definition>
    <rdfs:label xml:lang="fr">généalogie</rdfs:label>
    <skos:definition xml:lang="fr">«La généalogie (du grec γενεά genea, « génération » et λόγος logos, « connaissance ») est la « liste des membres d'une famille établissant une filiation » ou la pratique qui a pour objet la recherche de la parenté et de la filiation des personnes. La généalogie est considérée comme une science auxiliaire de l'histoire. Historiquement, elle était utilisée par les gens aisés pour établir la noblesse de sang d'un individu.»  <![CDATA[<a href="#cwrc:727d97bc-af78-4122-94be-aa78b2e97d5a">(DBpedia, 2017)</a>]]></skos:definition>
    <rdfs:isDefinedBy rdf:resource="http://sparql.cwrc.ca/ontologies/genre-ONTOLOGY_DATE"/>
    <rdfs:label xml:lang="en">genealogy</rdfs:label>
    <owl:sameAs rdf:resource="http://vocab.getty.edu/aat/300027015"/>
  </genre:InformationalGenre>
  <genre:DramaticGenre rdf:about="#bergamasque">
    <rdfs:label xml:lang="fr">bergamasque</rdfs:label>
    <rdfs:isDefinedBy rdf:resource="http://sparql.cwrc.ca/ontologies/genre-ONTOLOGY_DATE"/>
    <rdfs:label xml:lang="en">bergamasque</rdfs:label>
    <skos:definition xml:lang="fr">«La bergamasque est une danse traditionnelle provenant de la ville de Bergame dans le nord de l'Italie. Son existence est attestée depuis le début du XVIe siècle. Danse de couples disposés en cercle jusqu'au XVIIe siècle, vive et sautillante, elle est souvent utilisée dans la commedia dell'arte. La bergamasque d'un compositeur français se trouve dans le Thesaurus harmonicus (1603) de Jean-Baptiste Besard.»  <![CDATA[<a href="#cwrc:727d97bc-af78-4122-94be-aa78b2e97d5a">(DBpedia, 2017)</a>]]></skos:definition>
    <rdfs:comment xml:lang="en">This term and its description were created from data gathered from DBpedia.</rdfs:comment>
    <dcterms:references rdf:resource="https://www.merriam-webster.com/dictionary/Bergamasque"/>
    <skos:definition xml:lang="en">"A folk dance originating in Bergamo, Italy, in the 16th century, but often included in theatre productions unrelated to Italian culture."  <![CDATA[<a href="#cwrc:0a58baf2-e7d5-47d7-9853-c8140dbbfeed">(Merriam-Webster, 2017)</a>]]></skos:definition>
  </genre:DramaticGenre>
  <genre:ScholarlyGenre rdf:about="#dissertation">
    <rdfs:comment xml:lang="en">This term and its description were created from data gathered from the Getty Art &amp; Architecture Thesaurus.</rdfs:comment>
    <owl:sameAs rdf:resource="http://id.loc.gov/authorities/genreForms/gf2014026039"/>
    <rdfs:isDefinedBy rdf:resource="http://sparql.cwrc.ca/ontologies/genre-ONTOLOGY_DATE"/>
    <rdfs:label xml:lang="en">dissertation</rdfs:label>
    <skos:definition xml:lang="fr">Textes écrits ou enregistrement d'une présentation sur un sujet, généralement préparés et présentés en tant que devoir final pour obtenir un diplôme, s'appuyant généralement sur des recherches indépendantes démontrant l'expertis et la méthode académique du candidat.</skos:definition>
    <owl:sameAs rdf:resource="http://vocab.getty.edu/aat/300028029"/>
    <rdfs:label xml:lang="fr">mémoire, thèse</rdfs:label>
    <skos:definition xml:lang="en">"Written treatises, or the records of a discourse on a subject, usually prepared and presented as the final requirement for a degree or diploma and typically based on independent research and giving evidence of the candidate's mastery of the subject and of scholarly method."  <![CDATA[<a href="#cwrc:db2f8571-a773-4068-a35f-34262950bb8f">(Getty, 2017)</a>]]></skos:definition>
  </genre:ScholarlyGenre>
  <genre:InformationalGenre rdf:about="#epitaph">
    <skos:definition xml:lang="fr">«Une épitaphe (du grec ἐπιτάφος / epi, « sur » et taphos, « tombeau », par exemple des jeux funèbres ou une oraison funèbre) est une inscription funéraire, placée sur une pierre tombale ou un monument funéraire. Cela peut être un objet donné à une civilisation comme signe de paix. Dans la Grèce antique, l’épitaphe est un genre littéraire : c’est un éloge funèbre ancien. En littérature française, l'épitaphe est aussi un genre littéraire rimé : c'est surtout ce que l'on aimerait inscrire sur la pierre tombale de quelqu'un que l'on admire, ou, au contraire, que l'on n'apprécie guère. Supposée être inscrite sur le tombeau lui-même, une épitaphe peut débuter par ci-gît ou par la formule plus moderne ici repose ou par leur pluriel ci-gisent et ici reposent.»  <![CDATA[<a href="#cwrc:727d97bc-af78-4122-94be-aa78b2e97d5a">(DBpedia, 2017)</a>]]></skos:definition>
    <rdfs:label xml:lang="fr">épitaphe</rdfs:label>
    <rdfs:comment xml:lang="en">This term and its description were created from data gathered from DBpedia.</rdfs:comment>
    <owl:sameAs rdf:resource="http://dbpedia.org/resource/Epitaph"/>
    <rdfs:isDefinedBy rdf:resource="http://sparql.cwrc.ca/ontologies/genre-ONTOLOGY_DATE"/>
    <rdfs:label xml:lang="en">epitaph</rdfs:label>
    <skos:definition xml:lang="en">"An epitaph (from Greek ἐπιτάφιος epitaphios "a funeral oration" from ἐπί epi "at, over" and τάφος taphos "tomb") is a short text honoring a deceased person. Strictly speaking, it refers to text that is inscribed on a tombstone or plaque, but it may also be used in a figurative sense. Some epitaphs are specified by the person themselves before their death, while others are chosen by those responsible for the burial. An epitaph may be written in prose or in poem verse; poets have been known to compose their own epitaphs prior to their death."  <![CDATA[<a href="#cwrc:c5e7bace-95bb-4820-bd7d-6bb97c1badc5">(DBpedia, 2018)</a>]]></skos:definition>
  </genre:InformationalGenre>
  <genre:ReligiousGenre rdf:about="#hagiography">
    <owl:sameAs rdf:resource="http://id.loc.gov/authorities/genreForms/gf2015026032"/>
    <skos:definition xml:lang="fr">«L’hagiographie (du grec ancien ἅγιος / hágios (« saint ») et γράφειν / gráphein (« écrire »)) est l'écriture de la vie et / ou de l'œuvre des saints. Pour un texte particulier, on ne parle que rarement d'« une hagiographie » (sauf dans le sens figuré), mais plutôt d'un texte hagiographique ou tout simplement d'une vie de saint. Le texte hagiographique étant destiné à être lu, soit lors de l'office des moines soit en public dans le cadre de la prédication, on lui donne souvent le nom de légende (du latin legenda, « ce qui doit être lu », terme utilisé dans son acception la plus littérale et non dans son sens péjoratif actuel de récit dépourvu de tout enracinement dans l'histoire événementielle). Un texte hagiographique recouvre plusieurs genres littéraires ou artistiques parmi lesquels on compte en premier lieu la vita, c'est-à-dire le récit biographique de la vie du saint. Une fresque à épisode est également une hagiographie, de même qu'une simple notice résumant la vie du bienheureux. Par rapport à une biographie, l'hagiographie est un genre littéraire qui veut mettre en avant le caractère de sainteté du personnage dont on raconte la vie. L'écrivain, l'hagiographe n'a pas d'abord une démarche d'historien, surtout lorsque le genre hagiographique s'est déployé. Aussi les hagiographies anciennes sont parsemées de passages merveilleux à l'historicité douteuse. De plus, des typologies de saints existaient au Moyen Âge, ce qui a conduit les hagiographes à se conformer à ces modèles et à faire de nombreux emprunts à des récits antérieurs. L'hagiographie est ainsi un récit fortement stéréotypé dont la fonction pastorale est de servir à l'instruction et l'édification religieuse, mais qui peut avoir aussi une fonction normative, politique et de propagande religieuse. D'une manière plus polémique, on parle aussi d'hagiographie pour désigner un écrit (une biographie, l'analyse d'un système philosophique, etc.) trop favorable à son objet, c'est-à-dire manquant de recul et/ou ne laissant guère de place à la critique.»  <![CDATA[<a href="#cwrc:727d97bc-af78-4122-94be-aa78b2e97d5a">(DBpedia, 2017)</a>]]></skos:definition>
    <rdfs:comment xml:lang="en">The description for this term is indebted to DBpedia. </rdfs:comment>
    <skos:definition xml:lang="en">"Saints' lives as a branch of literature or legend."  <![CDATA[<a href="#cwrc:db2f8571-a773-4068-a35f-34262950bb8f">(Getty, 2017)</a>]]></skos:definition>
    <rdfs:isDefinedBy rdf:resource="http://sparql.cwrc.ca/ontologies/genre-ONTOLOGY_DATE"/>
    <rdfs:label xml:lang="en">hagiography</rdfs:label>
    <owl:sameAs rdf:resource="http://vocab.getty.edu/aat/300201063"/>
    <rdf:type rdf:resource="#LiteraryGenre"/>
  </genre:ReligiousGenre>
  <genre:MovingMedium rdf:about="#videoRecording">
    <rdfs:isDefinedBy rdf:resource="http://sparql.cwrc.ca/ontologies/genre-ONTOLOGY_DATE"/>
    <rdfs:label xml:lang="en">video recording</rdfs:label>
    <skos:related rdf:resource="http://vocab.getty.edu/aat/300028682"/>
    <skos:definition xml:lang="en">"Video is an electronic medium for the recording, copying, playback, broadcasting, and display of moving visual media. Video systems vary greatly in the resolution of the display and refresh rate. Video can be carried on a variety of media, including radio broadcast, tapes, DVDs, computer files etc." <![CDATA[<a href="#cwrc:727d97bc-af78-4122-94be-aa78b2e97d5a">(DBpedia, 2019)</a>]]></skos:definition>
    <rdf:type rdf:resource="#VisualArtMedium"/>
  </genre:MovingMedium>
  <genre:NarrativeGenre rdf:about="#myth">
    <skos:definition xml:lang="en">"Legendary stories without a determinable basis of fact or natural explanation, typically concerning a being, hero, deity, or event and explains some practice, rite, or phenomenon of nature."  <![CDATA[<a href="#cwrc:db2f8571-a773-4068-a35f-34262950bb8f">(Getty, 2017)</a>]]></skos:definition>
    <owl:sameAs rdf:resource="http://dbpedia.org/resource/Myth"/>
    <rdfs:isDefinedBy rdf:resource="http://sparql.cwrc.ca/ontologies/genre-ONTOLOGY_DATE"/>
    <rdfs:label xml:lang="en">myth</rdfs:label>
    <rdfs:comment xml:lang="en">The description for this term is indebted to DBpedia. </rdfs:comment>
    <skos:definition xml:lang="fr">«Un mythe est un récit qui se veut explicatif et surtout fondateur d'une pratique sociale. Il est porté à l'origine par une tradition orale, qui propose une explication pour certains aspects fondamentaux du monde et de la société qui a forgé ou qui véhicule ces mythes : L'étude des mythes est appelée mythologie. Le terme mythe est souvent employé pour désigner une croyance manifestement erronée au premier abord, mais qui peut se rapporter à des éléments concrets exprimés de façon symbolique et partagée par un nombre significatif de personnes. Le mythe se distingue de la légende (qui suppose quelques faits historiques identifiables), du conte (qui se veut inventif sans expliquer), et du roman (qui "explique" avec peu de fondements).»  <![CDATA[<a href="#cwrc:727d97bc-af78-4122-94be-aa78b2e97d5a">(DBpedia, 2017)</a>]]></skos:definition>
  </genre:NarrativeGenre>
  <genre:MovingMedium rdf:about="#animation">
    <skos:definition xml:lang="en">"Animation is the process of making the illusion of motion and change by means of the rapid display of a sequence of static images that minimally differ from each other. The illusion—as in motion pictures in general—is thought to rely on the phi phenomenon. Animators are artists who specialize in the creation of animation.Animation can be recorded with either analogue media, a flip book, motion picture film, video tape, digital media, including formats with animated GIF, Flash animation and digital video. To display animation, a digital camera, computer, or projector are used along with new technologies that are produced. Animation creation methods include the traditional animation creation method and those involving stop motion animation of two and three-dimensional objects, paper cutouts, puppets and clay figures. Images are displayed in a rapid succession, usually 24, 25, 30, or 60 frames per second." <![CDATA[<a href="#cwrc:727d97bc-af78-4122-94be-aa78b2e97d5a">(DBpedia, 2019)</a>]]></skos:definition>
    <rdfs:isDefinedBy rdf:resource="http://sparql.cwrc.ca/ontologies/genre-ONTOLOGY_DATE"/>
    <rdfs:label xml:lang="en">animation</rdfs:label>
    <rdf:type rdf:resource="#VisualArtMedium"/>
  </genre:MovingMedium>
  <genre:EmbeddedWork rdf:about="#prefatoryPiece">
    <rdfs:isDefinedBy rdf:resource="http://sparql.cwrc.ca/ontologies/genre-ONTOLOGY_DATE"/>
    <rdfs:label xml:lang="en">prefatory piece</rdfs:label>
    <rdfs:label xml:lang="fr">préface</rdfs:label>
    <rdfs:comment xml:lang="en">This term and its description were created from data gathered from the Getty Art &amp; Architecture Thesaurus.</rdfs:comment>
    <skos:definition xml:lang="fr">«Une préface (du latin præ : avant et fari : parler) est, en littérature, un texte d’introduction et de présentation. Placé en tête d’un livre, il en fait connaître les vues, le plan, prévient des objections, répond à des critiques ou encore donne une idée sur le message que veut transmettre l'auteur à travers ce livre (ex : la pauvreté de la société, l'inégalité, la prostitution, la violence, etc.). La préface est courte lorsqu'elle devient un avertissement et largement développée dans le cadre des prolégomènes. On oppose à la préface la postface.»  <![CDATA[<a href="#cwrc:727d97bc-af78-4122-94be-aa78b2e97d5a">(DBpedia, 2017)</a>]]></skos:definition>
    <skos:definition xml:lang="en">"Texts preceding the main literary work and containing comments about such matters as the reason for or circumstances of the author's writing the work, or comments by another about the author or the work."  <![CDATA[<a href="#cwrc:db2f8571-a773-4068-a35f-34262950bb8f">(Getty, 2017)</a>]]></skos:definition>
    <owl:sameAs rdf:resource="http://dbpedia.org/resource/Preface"/>
  </genre:EmbeddedWork>
  <genre:FictionalGenre rdf:about="#schoolFiction">
    <rdfs:label xml:lang="fr">fiction scolaire</rdfs:label>
    <rdfs:comment xml:lang="en">This term and its description were created from data gathered from DBpedia.</rdfs:comment>
    <rdfs:isDefinedBy rdf:resource="http://sparql.cwrc.ca/ontologies/genre-ONTOLOGY_DATE"/>
    <rdfs:label xml:lang="en">school fiction</rdfs:label>
    <skos:definition xml:lang="en">"The school story is a fiction genre centering on older pre-adolescent and adolescent school life, at its most popular in the first half of the twentieth century. While examples do exist in other countries, it is most commonly set in English boarding schools and mostly written in girls' and boys' subgenres, reflecting the single-sex education typical until the 1950s. It focuses largely on friendship, honor and loyalty between pupils. Plots involving sports events, bullies, secrets, rivalry and bravery are often used to shape the school story."  <![CDATA[<a href="#cwrc:727d97bc-af78-4122-94be-aa78b2e97d5a">(DBpedia, 2017)</a>]]></skos:definition>
    <owl:sameAs rdf:resource="http://dbpedia.org/resource/School_story"/>
  </genre:FictionalGenre>
  <genre:ReligiousGenre rdf:about="#conversionNarrative">
    <skos:definition xml:lang="en">"Broadly speaking, a conversion narrative is a narrative that relates the operation of conversion, usually religious. As a specific aspect of American literary and religious history, the conversion narrative was an important facet of Puritan sacred and secular society in New England during a period stretching roughly from 1630 to the end of the First Great Awakening." <![CDATA[<a href="#cwrc:50024824-8252-4a95-b62e-797911907f20">(DBpedia, 2021)</a>]]></skos:definition>
    <rdfs:comment xml:lang="en">This term and its description were created from data gathered from DBpedia.</rdfs:comment>
    <owl:sameAs rdf:resource="https://dbpedia.org/page/Conversion_narrative"/>
    <rdfs:isDefinedBy rdf:resource="http://sparql.cwrc.ca/ontologies/genre-ONTOLOGY_DATE"/>
    <rdfs:label xml:lang="en">conversion narrative</rdfs:label>
  </genre:ReligiousGenre>
  <genre:DramaticGenre rdf:about="#drama">
    <rdfs:comment xml:lang="en">The description for this term is indebted to Dr. L. Kip Wheeler of Carson-Newman University. </rdfs:comment>
    <owl:sameAs rdf:resource="http://id.loc.gov/authorities/genreForms/gf2014026297"/>
    <skos:broader rdf:resource="http://sparql.cwrc.ca/ontologies/genre.html#theatreForYoungAudiences"/>
    <rdfs:label xml:lang="fr">genre dramatique</rdfs:label>
    <rdfs:isDefinedBy rdf:resource="http://sparql.cwrc.ca/ontologies/genre-ONTOLOGY_DATE"/>
    <rdfs:label xml:lang="en">drama</rdfs:label>
    <dcterms:references rdf:resource="http://web.cn.edu/kwheeler/lit_terms_d.html"/>
    <skos:definition xml:lang="en">"A composition in prose or verse presenting, in pantomime and dialogue, a narrative involving conflict between a character or characters and some external or internal force (see conflict). Playwrights usually design dramas for presentation on a stage in front of an audience. Aristotle called drama "imitated human action." Drama may have originated in religious ceremonies. Thespis of Attica (sixth century BCE) was the first recorded composer of a tragedy. Tragedies in their earliest stage were performed by a single actor who interacted with the chorus. The playwright Aeschylus added a second actor on the stage (deuteragonist) to allow additional conflict and dialogue. Sophocles and Euripides added a third (tritagonist). Medieval drama may have evolved independently from rites commemorating the birth and death of Christ. During the late medieval period and the early Renaissance, drama gradually altered to the form we know today. The mid-sixteenth century in England in particular was one of the greatest periods of world drama. In traditional Greek drama, as defined by Aristotle, a play was to consist of five acts and follow the three dramatic unities. In more recent drama (i.e., during the last two centuries), plays have frequently consisted of three acts, and playwrights have felt more comfortable disregarding the confines of Aristotelian rules involving verisimilitude. See also unities, comedy, tragedy, revenge play, miracle play, morality play, and mystery play. An individual work of drama is called a play."  <![CDATA[<a href="cwrc:509015ff-7641-473e-94c5-688e06952bb7">(L. K Wheeler, 2017)</a>]]></skos:definition>
    <skos:definition xml:lang="fr">(du grec "drama", action) Formes littéraires, presque toujours sous forme de dialogues (en vers ou un prose) destinés à être joués par des acteurs lors d'une représentation scénique.</skos:definition>
  </genre:DramaticGenre>
  <genre:NovelisticGenre rdf:about="#sentimental">
    <skos:definition xml:lang="en">"The sentimental novel or the novel of sensibility is an 18th-century literary genre which celebrates the emotional and intellectual concepts of sentiment, sentimentalism, and sensibility. Sentimentalism, which is to be distinguished from sensibility, was a fashion in both poetry and prose fiction beginning in the eighteenth century in reaction to the rationalism of the Augustan Age. Sentimental novels relied on emotional response, both from their readers and characters. They feature scenes of distress and tenderness, and the plot is arranged to advance both emotions and actions. The result is a valorization of "fine feeling," displaying the characters as a model for refined, sensitive emotional effect. The ability to display feelings was thought to show character and experience, and to shape social life and relations."  <![CDATA[<a href="#cwrc:727d97bc-af78-4122-94be-aa78b2e97d5a">(DBpedia, 2017)</a>]]></skos:definition>
    <rdfs:isDefinedBy rdf:resource="http://sparql.cwrc.ca/ontologies/genre-ONTOLOGY_DATE"/>
    <rdfs:label xml:lang="en">sentimental</rdfs:label>
    <skos:definition xml:lang="fr">Le XIXe siècle est marqué par la formidable expansion de la presse et des technologies de la communication. La production s’accélère dans tous les secteurs de la culture : la musique, les spectacles, bientôt le cinéma. Un public de nouveaux lecteurs émerge. L’Angleterre est un des premiers pays à faire du livre un objet destiné au grand public. Publié en 1740, Pamela, ou la Vertu récompensée de Samuel Richardson, roman d'amour à succès, est un des premiers best-sellers, avec cinq éditions imprimées en onze mois. De son côté, Jane Austen est considérée comme l'un des précurseurs du genre avec Orgueil et Préjugés, paru en 1813. En France, l’apparition du roman-feuilleton à partir de 1840 marque la naissance du roman populaire. Le roman sentimental se développe dans le dernier quart du XIXe siècle, lorsque l’Église s’alarme du goût du peuple alphabétisé pour la lecture de romans. Elle choisit alors de l’encadrer. Les feuilletons issus des périodiques tels que Les Veillées des chaumières ou Le Petit Écho de la mode proposent alors un roman d’amour qui élève l’âme et l’esprit. M. Maryan a ainsi écrit plus de quatre-vingt-dix-sept romans d’éducation. Toujours optimistes, ces ouvrages préparent les jeunes filles au mariage. Le roman sentimental connaît un large développement après la Première Guerre mondiale. Les principaux éditeurs en sont Joseph Ferenczi, Jules Tallandier et Jules Rouff. Ils produisent de multiples collections de petits romans : petits par le format, la pagination et le coût modique. Jusque dans les années 1980, la Librairie Jules Tallandier restera un des éditeurs majeurs dans ce domaine. Elle va codifier la littérature sentimentale, destinée à exprimer une vision enchantée de l’existence. Les Delly, pseudonyme des frère et sœur Frédéric et Jeanne-Marie Petitjean, sont des auteurs emblématiques du genre.</skos:definition>
    <owl:sameAs rdf:resource="http://dbpedia.org/resource/Sentimental_novel"/>
    <rdf:type rdf:resource="#ThematicGenre"/>
    <rdfs:comment xml:lang="en">The description for this term is indebted to DBpedia. </rdfs:comment>
    <owl:sameAs rdf:resource="http://id.loc.gov/authorities/genreForms/gf2014026536"/>
    <rdfs:label xml:lang="fr">littérature sentimentale</rdfs:label>
  </genre:NovelisticGenre>
  <genre:DigitalMedium rdf:about="#multimedia">
    <skos:altLabel xml:lang="en">software, multimedia</skos:altLabel>
    <skos:altLabel xml:lang="en">mixed media</skos:altLabel>
    <rdfs:comment xml:lang="en">This term and its description were created from data gathered from the Getty Art &amp; Architecture Thesaurus.</rdfs:comment>
    <skos:related rdf:resource="http://vocab.getty.edu/aat/300047910"/>
    <rdfs:isDefinedBy rdf:resource="http://sparql.cwrc.ca/ontologies/genre-ONTOLOGY_DATE"/>
    <rdfs:label xml:lang="en">multimedia</rdfs:label>
    <skos:definition xml:lang="en">"Contemporary works of art that employ several distinct art forms, such as sculpture and music or painting and light art."  <![CDATA[<a href="#cwrc:db2f8571-a773-4068-a35f-34262950bb8f">(Getty, 2017)</a>]]></skos:definition>
    <rdfs:label xml:lang="fr">multimédia</rdfs:label>
    <skos:definition xml:lang="fr">Oeuvre matérialisée par son support quel qu'il soit ou son mode de communication, constituée de différents éléments (logiciel, graphisme, musique, son, scénario, images fixes ou animées, etc.) assemblés pour former un ensemble à l'identité propre.</skos:definition>
    <owl:sameAs rdf:resource="http://vocab.getty.edu/aat/300047910"/>
  </genre:DigitalMedium>
  <genre:PoeticGenre rdf:about="#boutsRimes">
    <rdfs:isDefinedBy rdf:resource="http://sparql.cwrc.ca/ontologies/genre-ONTOLOGY_DATE"/>
    <rdfs:label xml:lang="en">bouts-rimés</rdfs:label>
    <skos:definition xml:lang="en">"The result of a game popularized in 17th-century France in which a poet must write a logical poem using a list of random rhyming words written by someone else."  <![CDATA[<a href="#cwrc:4c227091-6bf0-4325-b846-9733fae19e61">(Oxford, 2015)</a>]]></skos:definition>
    <rdfs:comment xml:lang="en">This term and its description were created from data gathered from the Oxford Dictionary of Literary Terms, 4th ed.</rdfs:comment>
    <dcterms:references rdf:resource="http://www.oxfordreference.com/view/10.1093/acref/9780199208272.001.0001/acref-9780199208272-e-142?rskey=3RXM0b%26result=141"/>
    <rdfs:label xml:lang="fr">bout-rimé</rdfs:label>
  </genre:PoeticGenre>
  <genre:IntertextualGenre rdf:about="#sequel">
    <rdfs:comment xml:lang="en">The description for this term is indebted to Dr. L. Kip Wheeler of Carson-Newman University. </rdfs:comment>
    <dcterms:references rdf:resource="http://web.cn.edu/kwheeler/lit_terms_s.html"/>
    <rdfs:isDefinedBy rdf:resource="http://sparql.cwrc.ca/ontologies/genre-ONTOLOGY_DATE"/>
    <rdfs:label xml:lang="en">sequel</rdfs:label>
    <rdfs:label xml:lang="fr">oeuvres en série</rdfs:label>
    <skos:definition xml:lang="en">"(from Latin sequi, to follow): A literary work complete in itself, but continuing the narrative of an earlier work. It is a new story that extends or develops characters and situations found in an earlier work. Two sequels following an original work (together) are called a trilogy. Three sequels following an original work together are called a tetralogy.Often sequels have a reputation for inferior artistry compared to the original publication since they are often hastily written from the desire to capitalize on earlier financial success. Examples include Mark Twain's Tom Sawyer Abroad, which is a sequel to The Adventures of Tom Sawyer, and Alexandra Ripley's Scarlett, which is a sequel to Mitchell's Gone With the Wind. In the late twentieth century, it became common retroactively to write "prequels," a later book with the same geographic setting or characters, but which takes place in an earlier time."  <![CDATA[<a href="cwrc:509015ff-7641-473e-94c5-688e06952bb7">(L. K Wheeler, 2017)</a>]]></skos:definition>
    <skos:definition xml:lang="fr">«La suite d'une œuvre littéraire, cinématographique, télévisuelle, d'une bande dessinée ou d'un jeu vidéo, est une œuvre se déroulant dans le même univers de fiction que la première œuvre, et qui raconte une histoire ayant lieu après celle qui est narrée dans cette œuvre originelle.»  <![CDATA[<a href="#cwrc:727d97bc-af78-4122-94be-aa78b2e97d5a">(DBpedia, 2017)</a>]]></skos:definition>
  </genre:IntertextualGenre>
  <genre:FictionalGenre rdf:about="#dreamVision">
    <rdfs:isDefinedBy rdf:resource="http://sparql.cwrc.ca/ontologies/genre-ONTOLOGY_DATE"/>
    <rdfs:label xml:lang="en">dream vision</rdfs:label>
    <dcterms:references rdf:resource="http://www.oxfordreference.com/view/10.1093/acref/9780199208272.001.0001/acref-9780199208272-e-351?rskey=MMt5zw%26result=351"/>
    <rdfs:comment xml:lang="en">This term and its description were created from data gathered from the Oxford Dictionary of Literary Terms, 4th ed.</rdfs:comment>
    <skos:definition xml:lang="en">"Literature, typically a poem and frequently an allegory or symbolic tale, in which the plot is a dream recounted by a narrator who dreamed it."  <![CDATA[<a href="#cwrc:4c227091-6bf0-4325-b846-9733fae19e61">(Oxford, 2015)</a>]]></skos:definition>
    <skos:definition xml:lang="fr">Forme littéraire, souvent sous forme de poème allégorique ou de conte symbolique, dans lequel l'intrigue est le rêve du narrateur.</skos:definition>
    <rdfs:label xml:lang="fr">vision onirique</rdfs:label>
  </genre:FictionalGenre>
  <genre:PhilosophicalGenre rdf:about="#philosophy">
    <dcterms:references rdf:resource="http://web.cn.edu/kwheeler/lit_terms_p.html"/>
    <skos:definition xml:lang="fr">«La philosophie, du grec ancien φιλοσοφία (composé de φιλεῖν, philein : « aimer » ; et de σοφία, sophia : « sagesse »), signifie littéralement : « l'amour de la sagesse ». C'est une activité et une discipline existant depuis l'Antiquité en Occident et en Orient, se présentant comme un questionnement, une interprétation et une réflexion sur le monde et l'existence humaine. Différents buts peuvent lui être attribués : la recherche de la vérité ; la méditation sur le bien, le beau, le juste ; la quête du sens de la vie et du bonheur.»  <![CDATA[<a href="#cwrc:727d97bc-af78-4122-94be-aa78b2e97d5a">(DBpedia, 2017)</a>]]></skos:definition>
    <skos:definition xml:lang="en">"(Greek, "Love of wisdom"): The methodical and systematic exploration of what we know, how we know it, and why it is important that we know it. Too frequently, students use the term somewhat nebulously. They often mistakenly state, "My philosophy about X is . . ." when they really mean, "My opinion about X is . . ." or "My attitude toward X is . . ." Traditional areas of Western philosophic inquiry include the following areas."  <![CDATA[<a href="cwrc:509015ff-7641-473e-94c5-688e06952bb7">(L. K Wheeler, 2017)</a>]]></skos:definition>
    <rdfs:comment xml:lang="en">This term and its description were created from data gathered from DBpedia.</rdfs:comment>
    <rdfs:isDefinedBy rdf:resource="http://sparql.cwrc.ca/ontologies/genre-ONTOLOGY_DATE"/>
    <rdfs:label xml:lang="en">philosophy</rdfs:label>
    <rdfs:label xml:lang="fr">philosophie</rdfs:label>
  </genre:PhilosophicalGenre>
  <genre:IntertextualGenre rdf:about="#answer">
    <rdfs:isDefinedBy rdf:resource="http://sparql.cwrc.ca/ontologies/genre-ONTOLOGY_DATE"/>
    <rdfs:label xml:lang="en">answer</rdfs:label>
    <rdf:type rdf:resource="#DialogueOrDebateGenre"/>
    <skos:definition xml:lang="fr">Forme d'intertextualité, texte dans lequel un auteur se prononce en réponse à l'œuvre d'un autre écrivain, généralement en opposition aux propos qu'elle contient. Prend souvent la forme d'un essai ou d'une lettre.</skos:definition>
    <rdfs:label xml:lang="fr">réponse</rdfs:label>
    <skos:definition xml:lang="en">A form of intertextuality in which an author writes a response to a work by another writer, typically to argue against the statements of that work. Often takes the form of an essay or letter.</skos:definition>
  </genre:IntertextualGenre>
  <genre:HistoricalGenre rdf:about="#oralHistory">
    <rdfs:isDefinedBy rdf:resource="http://sparql.cwrc.ca/ontologies/genre-ONTOLOGY_DATE"/>
    <rdfs:label xml:lang="en">oral history</rdfs:label>
    <skos:definition xml:lang="en">"Oral history is the collection and study of historical information about individuals, families, important events, or everyday life using audiotapes, videotapes, or transcriptions of planned interviews. These interviews are conducted with people who participated in or observed past events and whose memories and perceptions of these are to be preserved as an aural record for future generations. Oral history strives to obtain information from different perspectives and most of these cannot be found in written sources. Oral history also refers to information gathered in this manner and to a written work (published or unpublished) based on such data, often preserved in archives and large libraries. The term is sometimes used in a more general sense to refer to any information about past events that people who experienced them tell anybody else, but professional historians usually consider this to be oral tradition. However, as the Columbia Encyclopedia explains: Primitive societies have long relied on oral tradition to preserve a record of the past in the absence of written histories. In Western society, the use of oral material goes back to the early Greek historians Herodotus and Thucydides, both of whom made extensive use of oral reports from witnesses. The modern concept of oral history was developed in the 1940s by Allan Nevins and his associates at Columbia University." <![CDATA[<a href="#cwrc:727d97bc-af78-4122-94be-aa78b2e97d5a">(DBpedia, 2019)</a>]]></skos:definition>
    <rdf:type rdf:resource="#NarrativeGenre"/>
  </genre:HistoricalGenre>
  <genre:FictionalGenre rdf:about="#allegory">
    <rdfs:isDefinedBy rdf:resource="http://sparql.cwrc.ca/ontologies/genre-ONTOLOGY_DATE"/>
    <rdfs:label xml:lang="en">allegory</rdfs:label>
    <rdfs:comment xml:lang="en">The description for this term is indebted to DBpedia. </rdfs:comment>
    <owl:sameAs rdf:resource="http://vocab.getty.edu/aat/300202507"/>
    <skos:definition xml:lang="fr">«Une allégorie (du grec : ἄλλον / állon, « autre chose », et ἀγορεύειν / agoreúein, « parler en public ») est une forme de représentation indirecte qui emploie une chose (une personne, un être animé ou inanimé, une action) comme signe d'une autre chose, cette dernière étant souvent une idée abstraite ou une notion morale difficile à représenter directement. Elle représente donc une idée abstraite par du concret. En littérature, l'allégorie est une figure rhétorique qui consiste à exprimer une idée en utilisant une histoire ou une représentation qui doit servir de support comparatif. La signification étymologique est : « une autre manière de dire », au moyen d'une image figurative ou figurée.»  <![CDATA[<a href="#cwrc:727d97bc-af78-4122-94be-aa78b2e97d5a">(DBpedia, 2017)</a>]]></skos:definition>
    <skos:definition xml:lang="en">"Literary works, art works, or other creative works that employ allegory to express complex abstract ideas, for example works that employ symbolic, fictional figures and actions to express truths or generalizations about human conduct or experience."  <![CDATA[<a href="#cwrc:db2f8571-a773-4068-a35f-34262950bb8f">(Getty, 2017)</a>]]></skos:definition>
    <rdfs:label xml:lang="fr">allégorie</rdfs:label>
    <rdfs:comment xml:lang="fr">La description de ce terme est basée sur celle de DBPedia.</rdfs:comment>
  </genre:FictionalGenre>
  <genre:FictionalGenre rdf:about="#fiction">
    <owl:sameAs rdf:resource="http://id.loc.gov/authorities/genreForms/gf2014026333"/>
    <rdfs:comment xml:lang="en">The description for this term is indebted to the Getty Art &amp; Architecture Thesaurus.</rdfs:comment>
    <rdfs:label xml:lang="fr">fiction</rdfs:label>
    <rdfs:isDefinedBy rdf:resource="http://sparql.cwrc.ca/ontologies/genre-ONTOLOGY_DATE"/>
    <rdfs:label xml:lang="en">fiction</rdfs:label>
    <skos:hiddenLabel xml:lang="en">NATIONALISTFICTION</skos:hiddenLabel>
    <skos:definition xml:lang="en">"Genre that refers to works evoked from the imagination of the writer and not conferred as fact. In literature, fiction generally refers to the novel, novella, short story, and poetic forms."  <![CDATA[<a href="#cwrc:db2f8571-a773-4068-a35f-34262950bb8f">(Getty, 2017)</a>]]></skos:definition>
    <owl:sameAs rdf:resource="http://vocab.getty.edu/aat/300055918"/>
    <skos:definition xml:lang="fr">Genre that refers to works evoked from the imagination of the writer and not conferred as fact. In literature, fiction generally refers to the novel, novella, short story, and poetic forms.</skos:definition>
  </genre:FictionalGenre>
  <genre:EpistolaryGenre rdf:about="#lettersFromTheDeadToTheLiving">
    <skos:definition xml:lang="fr">Histoires illustrant des leçons morales sous forme de lettres dans lesquelles les morts s'efforcent de persuader des proches toujours en vie de se repentir et d'améliorer leur conduite. Inclut souvent des caractéristiques propre à la fiction divertissante, comme le portrait de personnage, le récit, le suspense, la surprise, l'humour et les romances, y compris des transgressions de toutes sortes.</skos:definition>
    <rdfs:label xml:lang="fr">lettres des morts aux vivants</rdfs:label>
    <skos:definition xml:lang="en">Moralised case-histories in the form of letters in which the dead strive to reclaim the living beloved by persuading them to repent and reform. Often include features of lively fiction: character-drawing, narrative, suspense, surprise, humour, and love-situations including transgression of all kinds.</skos:definition>
    <rdfs:isDefinedBy rdf:resource="http://sparql.cwrc.ca/ontologies/genre-ONTOLOGY_DATE"/>
    <rdfs:label xml:lang="en">letters from the dead to the living</rdfs:label>
  </genre:EpistolaryGenre>
  <genre:ThematicGenre rdf:about="#military">
    <rdfs:isDefinedBy rdf:resource="http://sparql.cwrc.ca/ontologies/genre-ONTOLOGY_DATE"/>
    <rdfs:label xml:lang="en">military</rdfs:label>
    <skos:definition xml:lang="en">A thematic genre concerned with such matters as military lives, experiences, or history, whether at war or during peace time.</skos:definition>
    <skos:related rdf:resource="#"/>
  </genre:ThematicGenre>
  <genre:StandaloneWork rdf:about="#scrapbook">
    <skos:related rdf:resource="http://vocab.getty.edu/aat/300027341"/>
    <rdfs:comment xml:lang="en">This term and its description were created from data gathered from DBpedia.</rdfs:comment>
    <skos:definition xml:lang="fr">«Un album photos est un livre regroupant un ensemble de photographies. Certains albums ont des compartiments dans lesquels les photos sont rangées, d'autres, généralement plus anciens, contiennent simplement des feuilles de papier épais sur lesquelles les photos peuvent être collées. Il est également possible et facile de créer un album photo avec les photos numériques. De nombreux logiciels offrent cette possibilité.»  <![CDATA[<a href="#cwrc:727d97bc-af78-4122-94be-aa78b2e97d5a">(DBpedia, 2017)</a>]]></skos:definition>
    <rdfs:label xml:lang="fr">album</rdfs:label>
    <rdfs:isDefinedBy rdf:resource="http://sparql.cwrc.ca/ontologies/genre-ONTOLOGY_DATE"/>
    <rdfs:label xml:lang="en">scrapbook</rdfs:label>
    <owl:sameAs rdf:resource="http://dbpedia.org/resource/Photograph_album"/>
    <skos:definition xml:lang="en">"Blank books or albums designed so that a variety of items may be affixed to the pages, including photographs, clippings, and other memorabilia."  <![CDATA[<a href="#cwrc:db2f8571-a773-4068-a35f-34262950bb8f">(Getty, 2017)</a>]]></skos:definition>
  </genre:StandaloneWork>
  <genre:FeministGenre rdf:about="#feministTheory">
    <skos:definition xml:lang="fr">«La théorie féministe est un aspect du féminisme porté sur la théorisation et la réflexion philosophique. Son but est de comprendre la nature de l'inégalité entre les genres. Elle examine la place des femmes en faisant référence à des domaines des sciences sociales comme l'anthropologie, la sociologie, la communication, la psychanalyse, la philosophie, etc.»  <![CDATA[<a href="#cwrc:727d97bc-af78-4122-94be-aa78b2e97d5a">(DBpedia, 2017)</a>]]></skos:definition>
    <owl:sameAs rdf:resource="https://en.wikipedia.org/wiki/Feminist_theory"/>
    <rdf:type rdf:resource="#PhilosophicalGenre"/>
    <rdfs:label xml:lang="fr">théorie féministe</rdfs:label>
    <rdf:type rdf:resource="#ScholarlyGenre"/>
    <skos:definition xml:lang="en">"Feminist theory is the extension of feminism into theoretical, fictional, or philosophical discourse. It aims to understand the nature of gender inequality. It examines women's and men's social roles, experience, interests, chores, and feminist politics in a variety of fields, such as anthropology and sociology, communication, psychoanalysis, home economics, literature, education, and philosophy."  <![CDATA[<a href="#cwrc:727d97bc-af78-4122-94be-aa78b2e97d5a">(DBpedia, 2017)</a>]]></skos:definition>
    <rdfs:isDefinedBy rdf:resource="http://sparql.cwrc.ca/ontologies/genre-ONTOLOGY_DATE"/>
    <rdfs:label xml:lang="en">feminist theory</rdfs:label>
    <owl:sameAs rdf:resource="http://dbpedia.org/resource/Feminist_theory"/>
  </genre:FeministGenre>
  <genre:FictionalGenre rdf:about="#scienceFiction">
    <rdfs:isDefinedBy rdf:resource="http://sparql.cwrc.ca/ontologies/genre-ONTOLOGY_DATE"/>
    <rdfs:label xml:lang="en">science fiction</rdfs:label>
    <skos:definition xml:lang="fr">«La science-fiction est un genre narratif, principalement un genre littéraire et un genre cinématographique. Il est structuré par des hypothèses sur ce que pourrait être le futur ou ce qu'aurait pu être le présent voire le passé (planètes éloignées, mondes parallèles, uchronie...), en partant des connaissances actuelles (scientifiques, technologiques, ethnologiques...). Elle se distingue du fantastique qui inclut une dimension inexplicable et de la fantasy qui fait souvent intervenir la magie.»  <![CDATA[<a href="#cwrc:727d97bc-af78-4122-94be-aa78b2e97d5a">(DBpedia, 2017)</a>]]></skos:definition>
    <rdfs:comment xml:lang="en">The description for this term is indebted to DBpedia. </rdfs:comment>
    <skos:definition xml:lang="en">"Science fiction is a genre of speculative fiction dealing with imaginative concepts such as futuristic settings, futuristic science and technology, space travel, time travel, faster than light travel, parallel universes and extraterrestrial life. Science fiction often explores the potential consequences of scientific and other innovations, and has been called a "literature of ideas." It usually eschews the supernatural, and unlike the related genre of fantasy, historically science fiction stories were intended to have at least a faint grounding in science-based fact or theory at the time the story was created, but this connection has become tenuous or non-existent in much of science fiction."  <![CDATA[<a href="#cwrc:727d97bc-af78-4122-94be-aa78b2e97d5a">(DBpedia, 2017)</a>]]></skos:definition>
    <owl:sameAs rdf:resource="http://id.loc.gov/authorities/genreForms/gf2014026529"/>
    <owl:sameAs rdf:resource="http://dbpedia.org/resource/Science_fiction"/>
  </genre:FictionalGenre>
  <genre:NovelisticGenre rdf:about="#industrialNovel">
    <skos:definition xml:lang="fr">«Le roman industriel est un genre littéraire qui fait son apparition au début de l'ère victorienne en Grande-Bretagne. Classé dans la catégorie plus vaste du roman social, il décrit le déclin d’un monde essentiellement rural gagné par de nouvelles formes de production et d'urbanisation et aborde les difficultés dans lesquelles se débattent les ouvriers non seulement pour survivre mais aussi pour défendre leur humanité pendant et après la révolution industrielle. Certains romans industriels témoignent de sympathie pour le chartisme et les formes d’action pacifiques comme la grève.»  <![CDATA[<a href="#cwrc:727d97bc-af78-4122-94be-aa78b2e97d5a">(DBpedia, 2017)</a>]]></skos:definition>
    <rdfs:comment xml:lang="en">This term and its description were created from data gathered from the Penguin Dictionary of Literary Terms &amp; Literary Theory, 4th ed.</rdfs:comment>
    <skos:related rdf:resource="http://id.loc.gov/authorities/genreForms/gf2017026040"/>
    <owl:sameAs rdf:resource="http://dbpedia.org/resource/Industrial_novel"/>
    <skos:definition xml:lang="en">"A novel that exposes the living or working conditions of the 19th century-working class as a result of the industrial revolution. The shocking circumstances—extreme poverty, deplorable factory conditions, widespread disease, over-crowded housing, etc.—are typically described in great detail. Solutions are often proposed, but the main goal of an industrial novel is to make the plight of the lower class known to the middle and upper classes in order to promote social change."  <![CDATA[<a href="#cwrc:2f09376c-f784-4a46-9f04-5a21aa311f27">(Penguin, 1999)</a>]]></skos:definition>
    <rdfs:isDefinedBy rdf:resource="http://sparql.cwrc.ca/ontologies/genre-ONTOLOGY_DATE"/>
    <rdfs:label xml:lang="en">industrial novel</rdfs:label>
    <rdfs:label xml:lang="fr">roman industriel</rdfs:label>
    <rdf:type rdf:resource="#ThematicGenre"/>
    <rdf:type rdf:resource="#PoliticalGenre"/>
  </genre:NovelisticGenre>
  <genre:IntertextualGenre rdf:about="#translation">
    <skos:closeMatch rdf:resource="http://vocab.getty.edu/aat/300027389"/>
    <rdfs:isDefinedBy rdf:resource="http://sparql.cwrc.ca/ontologies/genre-ONTOLOGY_DATE"/>
    <rdfs:label xml:lang="en">translation</rdfs:label>
    <skos:definition xml:lang="fr">Versions traduites du'un texte.</skos:definition>
    <rdfs:label xml:lang="fr">traduction</rdfs:label>
    <rdfs:comment xml:lang="en">The description for this term is indebted to Dr. L. Kip Wheeler of Carson-Newman University. </rdfs:comment>
    <skos:definition xml:lang="en">Translated versions of a text. <![CDATA[<a href="#cwrc:db2f8571-a773-4068-a35f-34262950bb8f">(Getty, 2019)</a>]]></skos:definition>
  </genre:IntertextualGenre>
  <genre:DramaticGenre rdf:about="#theatreOfCruelty">
    <rdfs:label xml:lang="fr">théâtre de la cruauté</rdfs:label>
    <owl:sameAs rdf:resource="http://dbpedia.org/resource/Theatre_of_Cruelty"/>
    <skos:definition xml:lang="en">"The Theatre of Cruelty (French: Théâtre de la Cruauté) is a form of theatre developed by avant-garde playwright, actor, essayist, and theorist, Antonin Artaud, in The Theatre and its Double. Originally a member of the surrealist movement, Artaud eventually began to develop his own theatrical theories. The Theatre of Cruelty can be seen as break with traditional Western theatre, and a means by which artists assault the senses of the audience, and allow them to feel the unexpressed emotions of the subconscious. While Artaud was only able to produce one play in his lifetime that reflected the tenets of the Theatre of Cruelty, the works of many theatre artists reflect his theories."  <![CDATA[<a href="#cwrc:727d97bc-af78-4122-94be-aa78b2e97d5a">(DBpedia, 2017)</a>]]></skos:definition>
    <rdfs:comment xml:lang="en">This term and its description were created from data gathered from DBpedia.</rdfs:comment>
    <skos:definition xml:lang="fr">«Le théâtre de la cruauté est une expression introduite par Antonin Artaud pour désigner la forme dramatique à laquelle il travailla dans son essai Le Théâtre et son double. Derrière « cruauté » il faut entendre « souffrance d'exister ». L'acteur doit brûler les planches comme un supplicié sur son bûcher. Selon Artaud, le théâtre doit retrouver sa dimension sacrée, métaphysique et porter le spectateur jusqu'à la transe.»  <![CDATA[<a href="#cwrc:727d97bc-af78-4122-94be-aa78b2e97d5a">(DBpedia, 2017)</a>]]></skos:definition>
    <rdfs:isDefinedBy rdf:resource="http://sparql.cwrc.ca/ontologies/genre-ONTOLOGY_DATE"/>
    <rdfs:label xml:lang="en">theatre of cruelty</rdfs:label>
  </genre:DramaticGenre>
  <genre:PerformanceMedium rdf:about="#charade">
    <skos:related rdf:resource="http://id.loc.gov/authorities/genreForms/gf2014026533"/>
    <rdfs:label xml:lang="fr">charade</rdfs:label>
    <rdfs:isDefinedBy rdf:resource="http://sparql.cwrc.ca/ontologies/genre-ONTOLOGY_DATE"/>
    <rdfs:label xml:lang="en">charade</rdfs:label>
    <skos:definition xml:lang="fr">Divertissement verbal qui consiste à faire deviner un mot sommairement défini (appelé mon tout ou mon entier) d'après la définition d'un homonyme (appelé mon premier, mon second, etc.) de chacune de ses syllabes.</skos:definition>
    <dcterms:references rdf:resource="https://www.britannica.com/topic/charade-game"/>
    <skos:definition xml:lang="en">"A form of riddle in which clues are given about each syllable of a word so that the entire word may be guessed. Originally, these riddles were written, often in the form of a poem, but it soon gained popularity as a parlour game in which the clues were mimed rather than written in verse."  <![CDATA[<a href="#cwrc:7ff0c640-f273-46f5-be8d-e50aa27dce59">(Encyclopædia Britannica, 2017)</a>]]></skos:definition>
    <rdfs:comment xml:lang="en">This term and its description were created from data gathered from the Encyclopædia Britannica.</rdfs:comment>
  </genre:PerformanceMedium>
  <genre:PoeticGenre rdf:about="#eclogue">
    <skos:definition xml:lang="en">"An eclogue is a poem in a classical style on a pastoral subject. Poems in the genre are sometimes also called bucolics."  <![CDATA[<a href="#cwrc:727d97bc-af78-4122-94be-aa78b2e97d5a">(DBpedia, 2017)</a>]]></skos:definition>
    <skos:definition xml:lang="fr">«Une églogue est un poème de style classique consacré à un sujet pastoral. Les poèmes de ce genre littéraire sont parfois qualifiés de » bucoliques »."  <![CDATA[<a href="#cwrc:727d97bc-af78-4122-94be-aa78b2e97d5a">(DBpedia, 2017)</a>]]></skos:definition>
    <owl:sameAs rdf:resource="http://id.loc.gov/authorities/genreForms/gf2014026476"/>
    <owl:sameAs rdf:resource="http://dbpedia.org/resource/Eclogue"/>
    <rdfs:comment xml:lang="en">The description for this term is indebted to DBpedia. </rdfs:comment>
    <rdfs:isDefinedBy rdf:resource="http://sparql.cwrc.ca/ontologies/genre-ONTOLOGY_DATE"/>
    <rdfs:label xml:lang="en">eclogue</rdfs:label>
  </genre:PoeticGenre>
  <genre:PoeticGenre rdf:about="#verseNovel">
    <rdfs:label xml:lang="fr">roman en vers</rdfs:label>
    <skos:definition xml:lang="fr">Un roman en vers est un type de narration poétique dans laquelle un récit de la longueur d'un roman est raconté sous la forme de la poésie plutôt que de la prose. L'auteur peut utiliser des formes métriques simples ou complexes, mais incluera normalement un grand nombre de personnages, des voix multiples, un dialogue, une narration, une description et une action de manière romanesque.</skos:definition>
    <rdfs:comment xml:lang="en">The description for this term is indebted to DBpedia. </rdfs:comment>
    <owl:sameAs rdf:resource="http://dbpedia.org/resource/Verse_novel"/>
    <owl:sameAs rdf:resource="http://id.loc.gov/authorities/genreForms/gf2014026457"/>
    <rdfs:isDefinedBy rdf:resource="http://sparql.cwrc.ca/ontologies/genre-ONTOLOGY_DATE"/>
    <rdfs:label xml:lang="en">verse novel</rdfs:label>
    <rdf:type rdf:resource="#NovelisticGenre"/>
    <skos:definition xml:lang="en">"A verse novel is a type of narrative poetry in which a novel-length narrative is told through the medium of poetry rather than prose. Either simple or complex stanzaic verse-forms may be used, but there will usually be a large cast, multiple voices, dialogue, narration, description, and action in a novelistic manner."  <![CDATA[<a href="#cwrc:727d97bc-af78-4122-94be-aa78b2e97d5a">(DBpedia, 2017)</a>]]></skos:definition>
  </genre:PoeticGenre>
  <genre:ThematicGenre rdf:about="#temperance">
    <skos:definition xml:lang="en">"The temperance movement is a social movement against the consumption of alcoholic beverages. Temperance movements typically criticize excessive alcohol consumption, promote complete abstinence (teetotalism), or use its political influence to press the government to enact alcohol laws to regulate the availability of alcohol or even its complete prohibition." <![CDATA[<a href="#cwrc:727d97bc-af78-4122-94be-aa78b2e97d5a">(DBpedia, 2019)</a>]]></skos:definition>
    <rdfs:isDefinedBy rdf:resource="http://sparql.cwrc.ca/ontologies/genre-ONTOLOGY_DATE"/>
    <rdfs:label xml:lang="en">temperance</rdfs:label>
    <rdf:type rdf:resource="#PoliticalGenre"/>
  </genre:ThematicGenre>
  <genre:ThematicGenre rdf:about="#pastoral">
    <owl:sameAs rdf:resource="http://vocab.getty.edu/aat/300250491"/>
    <skos:definition xml:lang="en">"Genre that depicts or evokes idyllic life in the country; in works of pictorial art, often scenes of shepherds and shepherdesses in idealized arcadian landscapes."  <![CDATA[<a href="#cwrc:db2f8571-a773-4068-a35f-34262950bb8f">(Getty, 2017)</a>]]></skos:definition>
    <owl:sameAs rdf:resource="http://id.loc.gov/authorities/genreForms/gf2014026475"/>
    <rdfs:label xml:lang="fr">littérature pastorale</rdfs:label>
    <rdfs:isDefinedBy rdf:resource="http://sparql.cwrc.ca/ontologies/genre-ONTOLOGY_DATE"/>
    <rdfs:label xml:lang="en">pastoral</rdfs:label>
    <skos:definition xml:lang="fr">Genre qui représente ou évoque la vie paysanne de façon idyllique. Dans les œuvres d'art picturales, les scènes pastorales représentent généralement des bergers et des bergères dans des paysages arcadiens idéalisés.</skos:definition>
    <rdfs:comment xml:lang="en">The description for this term is indebted to the Getty Art &amp; Architecture Thesaurus.</rdfs:comment>
  </genre:ThematicGenre>
  <genre:PoeticGenre rdf:about="#haiku">
    <rdfs:comment xml:lang="en">This term and its description were created from data gathered from DBpedia.</rdfs:comment>
    <rdfs:isDefinedBy rdf:resource="http://sparql.cwrc.ca/ontologies/genre-ONTOLOGY_DATE"/>
    <rdfs:label xml:lang="en">haiku</rdfs:label>
    <skos:definition xml:lang="fr">«Le haïku (俳句, haiku), terme créé par le poète Masaoka Shiki (1867-1902), est une forme poétique très codifiée d'origine japonaise et dont la paternité, dans son esprit actuel, est attribuée au poète Bashō Matsuo (1644-1694). Le haïku doit donner une notion de saison (le kigo) et doit comporter une césure (le kireji). Si le haïku n'indique ni saison, ni moment particulier, on l'appellera un moki ou encore haïku libre, tels les poèmes de Taneda Santôka (1882-1940) ou ceux de Ozaki Hôsai (1885-1926).»  <![CDATA[<a href="#cwrc:727d97bc-af78-4122-94be-aa78b2e97d5a">(DBpedia, 2017)</a>]]></skos:definition>
    <owl:sameAs rdf:resource="http://id.loc.gov/authorities/genreForms/gf2014026366"/>
    <owl:sameAs rdf:resource="http://dbpedia.org/resource/Haiku"/>
    <skos:definition xml:lang="en">"(plural: haiku, from archaic Japanese): The term haiku is a fairly late addition to Japanese poetry. The poet Shiki coined the term in the nineteenth century from a longer, more traditional phrase, haikai renga no hokku ("the introductory lines of light linked verse"). To understand the haiku's history as a genre, peruse the vocabulary entries for its predecessors, the hokku and the haikai renga or renku. The haiku follows several conventions: Many Japanese poets have used the form, the two acknowledged masters being Bashó (a nom de plume for Matsuo Munefusa, 1644-94); and Kobayashi Issa (a nom de plume for Kobayashi Nobuyuki). The Imagist Movement in 20th century English literature has been profoundly influenced by haiku. The list of poets who attempted the haiku or admired the genre includes Ezra Pound, Amy Lowell, Robert Frost, Conrad Aiken, and W. B. Yeats. Contrast haiku with the tanka and the senryu. See also hokku, below, and haikai, above. See also kigo and imagism. You can click here to download a PDF handout summarizing this discussion of haiku, or you can click here to download PDF samples of haiku."  <![CDATA[<a href="cwrc:509015ff-7641-473e-94c5-688e06952bb7">(L. K Wheeler, 2017)</a>]]></skos:definition>
    <rdfs:label xml:lang="fr">haïku</rdfs:label>
  </genre:PoeticGenre>
  <genre:TextualMedium rdf:about="#chapter">
    <skos:definition xml:lang="en">"Main divisions or sections of a book, typically designated in some way, such as with a special heading, title, number, or layout." <![CDATA[<a href="#cwrc:bd595bc4-5991-4c51-98d9-9ab52c416f4f">(Getty, 2021)</a>]]></skos:definition>
    <rdfs:comment xml:lang="en">The description for this term is indebted to the Getty Art &amp; Architecture Thesaurus.</rdfs:comment>
    <owl:sameAs rdf:resource="http://vocab.getty.edu/aat/300311699"/>
    <rdfs:isDefinedBy rdf:resource="http://sparql.cwrc.ca/ontologies/genre-ONTOLOGY_DATE"/>
    <rdfs:label xml:lang="en">chapter</rdfs:label>
  </genre:TextualMedium>
  <genre:DramaticGenre rdf:about="#tragedy">
    <rdfs:comment xml:lang="en">The description for this term is indebted to the Getty Art &amp; Architecture Thesaurus.</rdfs:comment>
    <owl:sameAs rdf:resource="http://id.loc.gov/authorities/genreForms/gf2014026576"/>
    <skos:definition xml:lang="fr">«La tragédie est un genre théâtral dont l’origine remonte au théâtre grec antique. Contrairement à la comédie, elle met en scène des personnages de rangs élevés et se dénoue très souvent par la mort d’un ou de plusieurs personnages.Elle a un rôle cathartique (prévenir les gens de ne pas faire le Mal en suscitant terreur et pitié).»  <![CDATA[<a href="#cwrc:727d97bc-af78-4122-94be-aa78b2e97d5a">(DBpedia, 2017)</a>]]></skos:definition>
    <rdfs:isDefinedBy rdf:resource="http://sparql.cwrc.ca/ontologies/genre-ONTOLOGY_DATE"/>
    <rdfs:label xml:lang="en">tragedy</rdfs:label>
    <owl:sameAs rdf:resource="http://dbpedia.org/resource/Tragedy"/>
    <rdfs:label xml:lang="fr">tragédie</rdfs:label>
    <skos:definition xml:lang="en">"Literary works of serious and dignified character that reach disastrous or sorrowful conclusions."  <![CDATA[<a href="#cwrc:db2f8571-a773-4068-a35f-34262950bb8f">(Getty, 2017)</a>]]></skos:definition>
  </genre:DramaticGenre>
  <genre:ReligiousGenre rdf:about="#sermon">
    <skos:definition xml:lang="en">"A sermon is an oration, lecture, or talk by a member of a religious institution or clergy. Sermons address a Biblical, theological, religious, or moral topic, usually expounding on a type of belief, law or behavior within both past and present contexts. Elements of the sermon often include exposition, exhortation and practical application. In Christianity, a sermon (also known as a homily within some churches) is usually delivered in a place of worship from an elevated architectural feature, variously known as a pulpit, a lectern, or an ambo. The word "sermon" comes from a Middle English word which was derived from Old French, which in turn came from the Latin word sermō meaning "discourse". The word can mean "conversation", which could mean that early sermons were delivered in the form of question and answer, and that only later did it come to mean a monologue. However, the Bible contains many speeches without interlocution, which some take to be sermons: Moses in Deuteronomy 1-33 ; Jesus' sermon on the mount in Matthew 5-7 (though the gospel writers do not specifically call it a sermon; the popular descriptor for Christ's speech there came much later); Peter after Pentecost in Acts 2:14-40 (though this speech was delivered to nonbelievers and as such is not quite parallel to the popular definition of a sermon). In modern language, the word "sermon" is used in secular terms, pejoratively, to describe a lengthy or tedious speech delivered with great passion, by any person, to an uninterested audience. A sermonette is a short sermon (usually associated with television broadcasting, as stations would present a sermonette before signing off for the night)."  <![CDATA[<a href="#cwrc:727d97bc-af78-4122-94be-aa78b2e97d5a">(DBpedia, 2017)</a>]]></skos:definition>
    <skos:definition xml:lang="fr">«Le sermon est un discours de prédication prononcé dans des circonstances religieuses.»  <![CDATA[<a href="#cwrc:727d97bc-af78-4122-94be-aa78b2e97d5a">(DBpedia, 2017)</a>]]></skos:definition>
    <owl:sameAs rdf:resource="http://id.loc.gov/authorities/genreForms/gf2015026051"/>
    <owl:sameAs rdf:resource="http://dbpedia.org/resource/Sermon"/>
    <rdfs:comment xml:lang="en">The description for this term is indebted to DBpedia. </rdfs:comment>
    <rdfs:isDefinedBy rdf:resource="http://sparql.cwrc.ca/ontologies/genre-ONTOLOGY_DATE"/>
    <rdfs:label xml:lang="en">sermon</rdfs:label>
    <rdf:type rdf:resource="#PerformanceMedium"/>
  </genre:ReligiousGenre>
  <genre:ReligiousGenre rdf:about="#churchOrder">
    <skos:definition xml:lang="en">"Regulations and directions on church governance that are decreed according to ecclesiastical or scriptural authority."<![CDATA[<a href="#cwrc:788072dc-a6e5-44b1-b72b-873846d117a8">(Library of Congress, 2022)</a>]]></skos:definition>
    <owl:sameAs rdf:resource="http://id.loc.gov/authorities/genreForms/gf2015026054"/>
    <rdfs:comment xml:lang="en">The description for this term is indebted to The Library of Congress.</rdfs:comment>
    <rdfs:isDefinedBy rdf:resource="http://sparql.cwrc.ca/ontologies/genre-ONTOLOGY_DATE"/>
    <rdfs:label xml:lang="en">church order</rdfs:label>
  </genre:ReligiousGenre>
  <genre:DidacticGenre rdf:about="#bestiary">
    <rdfs:label xml:lang="fr">bestiaire</rdfs:label>
    <rdfs:isDefinedBy rdf:resource="http://sparql.cwrc.ca/ontologies/genre-ONTOLOGY_DATE"/>
    <rdfs:label xml:lang="en">bestiary</rdfs:label>
    <rdfs:comment xml:lang="en">The description for this term is indebted to the Getty Art &amp; Architecture Thesaurus.</rdfs:comment>
    <skos:definition xml:lang="en">"Collections of moralized fables, especially as written in the Middle Ages, about actual or mythical animals."  <![CDATA[<a href="#cwrc:db2f8571-a773-4068-a35f-34262950bb8f">(Getty, 2017)</a>]]></skos:definition>
    <owl:sameAs rdf:resource="http://www.universalis.fr/encyclopedie/bestiaires/"/>
    <skos:definition xml:lang="fr">«Collections de fables à moral mettant en scène des animaux réels ou mythiques et principalement écrites au Moyen-Âge.»  <![CDATA[<a href="#cwrc:db2f8571-a773-4068-a35f-34262950bb8f">(Getty, 2017)</a>]]></skos:definition>
  </genre:DidacticGenre>
  <genre:ComedicGenre rdf:about="#comedyOfIntrigue">
    <skos:definition xml:lang="en">"A dramatic form popularized in the 16th century in which the comedy depends on complex plots, surprising twists, and ridiculous situations. The characters and their development tend to be secondary to plot in importance."  <![CDATA[<a href="#cwrc:2f09376c-f784-4a46-9f04-5a21aa311f27">(Penguin, 1999)</a>]]></skos:definition>
    <rdfs:isDefinedBy rdf:resource="http://sparql.cwrc.ca/ontologies/genre-ONTOLOGY_DATE"/>
    <rdfs:label xml:lang="en">comedy of intrigue</rdfs:label>
    <rdfs:comment xml:lang="en">This term and its description were created from data gathered from the Penguin Dictionary of Literary Terms &amp; Literary Theory, 4th ed.</rdfs:comment>
    <rdfs:label xml:lang="fr">comédie d'intrigue</rdfs:label>
    <skos:definition xml:lang="fr">Genre de comédie rendue populaire au 16ème siècle, dans laquelle la pièce repose sur des intrigues complexes, des revirement surprenants et des situations ridicules. Les personnages et leur développement ont généralement une importance seconde par rapport à l'intrigue.</skos:definition>
  </genre:ComedicGenre>
  <genre:SongGenre rdf:about="#oratorio">
    <owl:sameAs rdf:resource="http://dbpedia.org/resource/Oratorio"/>
    <skos:definition xml:lang="en">"A lengthy musical composition for voice and orchestra, typically narrative and religious in nature. Unlike an opera, it is not a theatrical performance and does not include costumes or sets."  <![CDATA[<a href="#cwrc:4c227091-6bf0-4325-b846-9733fae19e61">(Oxford, 2015)</a>]]></skos:definition>
    <owl:sameAs rdf:resource="http://id.loc.gov/authorities/genreForms/gf2014026977"/>
    <rdfs:isDefinedBy rdf:resource="http://sparql.cwrc.ca/ontologies/genre-ONTOLOGY_DATE"/>
    <rdfs:label xml:lang="en">oratorio</rdfs:label>
    <rdfs:label xml:lang="fr">oratorio</rdfs:label>
    <rdfs:comment xml:lang="en">This term and its description were created from data gathered from the Oxford Dictionary of English, 3rd ed.</rdfs:comment>
    <skos:definition xml:lang="fr">«Un oratorio est une œuvre lyrique dramatique représentée sans mise en scène, ni costumes, ni décors. Généralement composé pour voix solistes, chœur et orchestre symphonique, avec parfois un narrateur, son sujet est le plus souvent religieux (épisode extrait de la Bible, de la vie de Jésus, d’un(e) saint(e)… ) mais peut être aussi profane (héros mythologique, sujet historique, hymne à la nature…). Formellement assez proche de la cantate et de l’opéra, l'oratorio comprend généralement une ouverture, des récitatifs, des airs et des chœurs.»  <![CDATA[<a href="#cwrc:727d97bc-af78-4122-94be-aa78b2e97d5a">(DBpedia, 2017)</a>]]></skos:definition>
    <rdf:type rdf:resource="#ReligiousGenre"/>
    <rdf:type rdf:resource="#NarrativeGenre"/>
  </genre:SongGenre>
  <genre:DramaticGenre rdf:about="#theatreOfTheAbsurd">
    <rdfs:label xml:lang="fr">théâtre de l'absurde</rdfs:label>
    <rdfs:comment xml:lang="en">This term and its description were created from data gathered from DBpedia.</rdfs:comment>
    <owl:sameAs rdf:resource="http://dbpedia.org/resource/Theatre_of_the_Absurd"/>
    <skos:definition xml:lang="fr">«Le théâtre de l’absurde est un style de théâtre apparu au XXe siècle, à l'époque de la Seconde Guerre mondiale, qui se caractérise par une rupture totale par rapport aux genres plus classiques, tels que la tragédie ou la comédie. C'est un genre traitant fréquemment de l’absurdité de l’Homme et de la vie en général, celle-ci menant toujours à une fin tragique. L’origine de ce mouvement est sans conteste essentiellement liée à la chute de l’humanisme et au traumatisme causé par la Première Guerre mondiale. Ce mouvement littéraire s'est inspiré des surréalistes et des dadaïstes mais est radicalement opposé au réalisme.»  <![CDATA[<a href="#cwrc:727d97bc-af78-4122-94be-aa78b2e97d5a">(DBpedia, 2017)</a>]]></skos:definition>
    <rdfs:isDefinedBy rdf:resource="http://sparql.cwrc.ca/ontologies/genre-ONTOLOGY_DATE"/>
    <rdfs:label xml:lang="en">theatre of the absurd</rdfs:label>
    <skos:definition xml:lang="en">"The Theatre of the Absurd (French: théâtre de l'absurde) is a post–World War II designation for particular plays of absurdist fiction written by a number of primarily European playwrights in the late 1950s, as well as one for the style of theatre which has evolved from their work. Their work focused largely on the idea of existentialism and expressed what happens when human existence has no meaning or purpose and therefore all communication breaks down, in fact alerting their audiences to pursue the opposite. Logical construction and argument gives way to irrational and illogical speech and to its ultimate conclusion, silence."  <![CDATA[<a href="#cwrc:727d97bc-af78-4122-94be-aa78b2e97d5a">(DBpedia, 2017)</a>]]></skos:definition>
  </genre:DramaticGenre>
  <genre:ChildrensLiteratureGenre rdf:about="#youngAdultWriting">
    <rdfs:label xml:lang="fr">littérature jeunes adultes</rdfs:label>
    <rdfs:isDefinedBy rdf:resource="http://sparql.cwrc.ca/ontologies/genre-ONTOLOGY_DATE"/>
    <rdfs:label xml:lang="en">young adult writing</rdfs:label>
    <skos:definition xml:lang="en">Writing aimed at a young adult audience.</skos:definition>
    <skos:definition xml:lang="fr">Littérature destinée à un public de jeunes adultes.</skos:definition>
  </genre:ChildrensLiteratureGenre>
  <genre:PoeticGenre rdf:about="#performancePoetry">
    <skos:definition xml:lang="fr">«La lecture performée ou lecture-performance est une lecture publique de textes poétiques ou littéraires effectuée le plus souvent par son auteur dans un esprit qui s'apparente à celui de la performance et qui peut convoquer tous les arts et techniques du théâtre et de la scène où la poésie et la littérature sont cependant toujours au premier plan. Christian Prigent, Serge Pey et Charles Pennequin en sont les premiers représentants. Édith Azam est aujourd'hui la conseillère lecture-performance au festival Voix de la Méditerranée de Lodève.»  <![CDATA[<a href="#cwrc:727d97bc-af78-4122-94be-aa78b2e97d5a">(DBpedia, 2017)</a>]]></skos:definition>
    <skos:definition xml:lang="en">"Performance poetry is poetry that is specifically composed for or during a performance before an audience. During the 1980s, the term came into popular usage to describe poetry written or composed for performance rather than print distribution."  <![CDATA[<a href="#cwrc:727d97bc-af78-4122-94be-aa78b2e97d5a">(DBpedia, 2017)</a>]]></skos:definition>
    <rdfs:isDefinedBy rdf:resource="http://sparql.cwrc.ca/ontologies/genre-ONTOLOGY_DATE"/>
    <rdfs:label xml:lang="en">performance poetry</rdfs:label>
    <rdfs:comment xml:lang="en">The description for this term is indebted to DBpedia. </rdfs:comment>
    <owl:sameAs rdf:resource="http://id.loc.gov/authorities/genreForms/gf2014026552"/>
    <owl:sameAs rdf:resource="http://dbpedia.org/resource/Performance_poetry"/>
  </genre:PoeticGenre>
  <genre:ReligiousGenre rdf:about="#psalm">
    <skos:definition xml:lang="fr">Chacun des cent cinquante poèmes religieux, jadis attribués au roi David, qui composent l'un des livres de la Bible et sont récités ou chantés dans les liturgies juives ou chrétiennes (abrév. ps.).</skos:definition>
    <rdfs:label xml:lang="fr">psaume</rdfs:label>
    <owl:sameAs rdf:resource="http://id.loc.gov/authorities/genreForms/gf2015026079"/>
    <rdf:type rdf:resource="#SongGenre"/>
    <rdfs:comment xml:lang="en">This term and its description were created from data gathered from the Dictionnaire Vivant de la Langue Française.</rdfs:comment>
    <rdf:type rdf:resource="#PoeticGenre"/>
    <skos:definition xml:lang="en">"Sacred songs that may be sung or recited in religious worship, particularly those contained in the Book of Psalms in the Old Testament and Hebrew Scriptures."  <![CDATA[<a href="#cwrc:db2f8571-a773-4068-a35f-34262950bb8f">(Getty, 2017)</a>]]></skos:definition>
    <owl:sameAs rdf:resource="http://vocab.getty.edu/aat/300400527"/>
    <rdfs:isDefinedBy rdf:resource="http://sparql.cwrc.ca/ontologies/genre-ONTOLOGY_DATE"/>
    <rdfs:label xml:lang="en">psalm</rdfs:label>
  </genre:ReligiousGenre>
  <genre:PerformanceMedium rdf:about="#dance">
    <skos:definition xml:lang="en">"(See also: List of basic dance topics) Dance is a performance art form consisting of purposefully selected sequences of human movement. This movement has aesthetic and symbolic value, and is acknowledged as dance by performers and observers within a particular culture. Dance can be categorized and described by its choreography, by its repertoire of movements, or by its historical period or place of origin. An important distinction is to be drawn between the contexts of theatrical and participatory dance, although these two categories are not always completely separate; both may have special functions, whether social, ceremonial, competitive, erotic, martial, or sacred/liturgical. Other forms of human movement are sometimes said to have a dance-like quality, including martial arts, gymnastics, figure skating, synchronized swimming and many other forms of athletics." <![CDATA[<a href="#cwrc:727d97bc-af78-4122-94be-aa78b2e97d5a">(DBpedia, 2019)</a>]]></skos:definition>
    <rdfs:isDefinedBy rdf:resource="http://sparql.cwrc.ca/ontologies/genre-ONTOLOGY_DATE"/>
    <rdfs:label xml:lang="en">dance</rdfs:label>
    <skos:related rdf:resource="http://vocab.getty.edu/aat/300054144"/>
  </genre:PerformanceMedium>
  <genre:ThematicGenre rdf:about="#migration">
    <skos:definition xml:lang="en">"A text or other form of media concerned with the topic of the changing of permanent residence (conventionally understood as being for at least one year) by discrete populations." <![CDATA[<a href="#cwrc:bd595bc4-5991-4c51-98d9-9ab52c416f4f">(Getty, 2021)</a>]]></skos:definition>
    <rdfs:comment xml:lang="en">The description for this term is indebted to the Getty Art &amp; Architecture Thesaurus.</rdfs:comment>
    
    <rdfs:isDefinedBy rdf:resource="http://sparql.cwrc.ca/ontologies/genre-ONTOLOGY_DATE"/>
    <rdfs:label xml:lang="en">migration</rdfs:label>
    <skos:altLabel xml:lang="en">immigration writing</skos:altLabel>
    <rdf:type rdf:resource="#PoliticalGenre"/>
  </genre:ThematicGenre>
  <genre:DialogueOrDebateGenre rdf:about="#dialogueOrDebate">
    <rdfs:comment xml:lang="en">This term and its description were created from data gathered from data.bnf.fr.</rdfs:comment>
    <rdfs:label xml:lang="fr">dialogue ou débat</rdfs:label>
    <skos:definition xml:lang="fr">Oeuvre littéraire en forme de conversation entre deux ou plusieurs personnes, où l'exposé contradictoire des idées permet à l'auteur d'exposer ses opinions morales, philosophiques, religieuses, etc.</skos:definition>
    <rdfs:isDefinedBy rdf:resource="http://sparql.cwrc.ca/ontologies/genre-ONTOLOGY_DATE"/>
    <rdfs:label xml:lang="en">dialogue or debate</rdfs:label>
    <dcterms:references rdf:resource="http://www.oxfordreference.com/view/10.1093/acref/9780199208272.001.0001/acref-9780199208272-e-310?rskey=TydJW0%26result=301"/>
    <skos:definition xml:lang="en">"A text made up of a conversation between two or more characters, often in which the characters take up opposing sides of an argument."  <![CDATA[<a href="#cwrc:4c227091-6bf0-4325-b846-9733fae19e61">(Oxford, 2015)</a>]]></skos:definition>
    <owl:sameAs rdf:resource="http://id.loc.gov/authorities/genreForms/gf2014026083"/>
  </genre:DialogueOrDebateGenre>
  <genre:ThematicGenre rdf:about="#domestic">
    <rdfs:isDefinedBy rdf:resource="http://sparql.cwrc.ca/ontologies/genre-ONTOLOGY_DATE"/>
    <rdfs:label xml:lang="en">domestic</rdfs:label>
    <skos:definition xml:lang="en">"Domestic realism normally refers to the genre of nineteenth-century novels popular with women readers. This body of writing is also known as "sentimental fiction" or "woman's fiction". The genre is mainly reflected in the novel though short-stories and non-fiction works such as Harriet Beecher Stowe's "Our Country Neighbors" and The New Housekeeper's Manual written by Stowe and her sister-in-law Catharine Beecher are works of domestic realism. The style's particular characteristics are: "1. Plot focuses on a heroine who embodies one of two types of exemplar: the angel and the practical woman (Reynolds) who sometimes exist in the same work. Baym says that this heroine is contrasted with the passive woman (incompetent, cowardly, ignorant; often the heroine's mother is this type) and the "belle," who is deprived of a proper education. 2. The heroine struggles for self-mastery, learning the pain of conquering her own passions (Tompkins, Sensational Designs, 172). 3. The heroine learns to balance society's demands for self-denial with her own desire for autonomy, a struggle often addressed in terms of religion. 4. She suffers at the hands of abusers of power before establishing a network of surrogate kin. 5. The plots "repeatedly identify immersion in feeling as one of the great temptations and dangers for a developing woman. They show that feeling must be controlled. . . " (Baym 25). Frances Cogan notes that the heroines thus undergo a full education within which to realize feminine obligations (The All-American Girl). 6. The tales generally end with marriage, usually one of two possible kinds: A. Reforming the bad or "wild" male, as in Augusta Evans's St. Elmo (1867) B. Marrying the solid male who already meets her qualifications.Examples: Maria Cummins, The Lamplighter (1854) and Susan Warner, The Wide, Wide World (1850) 7. The novels may use a "language of tears" that evokes sympathy from the readers. 8. Richard Brodhead (Cultures of Letters) sees class as an important issue, as the ideal family or heroine is poised between a lower-class family exemplifying poverty and domestic disorganization and upper-class characters exemplifying an idle, frivolous existence (94)." An example of this style of novel is Jane Smiley's A Thousand Acres in which the main character's confinement is emphasized in such a way. Some early exponents of the genre of domestic realism were Jane Austen and Elizabeth Barrett Browning."  <![CDATA[<a href="#cwrc:727d97bc-af78-4122-94be-aa78b2e97d5a">(DBpedia, 2017)</a>]]></skos:definition>
    <rdf:type rdf:resource="#NovelisticGenre"/>
    <rdfs:label xml:lang="fr">réalisme domestique</rdfs:label>
    <skos:definition xml:lang="fr">Le réalisme domestique se réfère généralement au genre des romans du dix-neuvième siècle populaires auprès des lectrices des femmes. Ce corps d'écriture est également connu sous le nom de "fiction sentimentale" Ou "la fiction de la femme". Le genre se reflète principalement dans le roman, bien que des histoires courtes et des œuvres non-fiction telles que Harriet Beecher Stowe's Our Country Neighbours &amp; quot; Et The New Housekeeper's Manual écrit par Stowe et sa belle-sœur Catharine Beecher sont des œuvres de réalisme domestique. Les caractéristiques particulières du style sont: &amp; quot; 1. Plot se concentre sur une héroïne qui incarne l'un des deux types d'exemples: l'ange et la femme pratique (Reynolds) qui existent parfois dans le même travail. Baym dit que cette héroïne est contrastée avec la femme passive (incompétente, lâche, ignorante, souvent la mère de l'héroïne est de ce type) et la «belle», qui est privée d'une éducation adéquate. 2. L'héroïne lutte pour la maîtrise de soi, apprenant la douleur causée par la nécessité de vaincre ses propres passions (Tompkins, Sensational Designs, 172). 3. L'héroïne apprend à trouver un équilibre entre l’impératif social du sacrifice de soi et son propre désir d'autonomie, une lutte souvent abordée en terme de religion. 4. Elle souffre aux mains d’auteurs de maltraitance, avant d'établir un réseau de parents de substitution. 5. Les intrigues "identifient à plusieurs reprises l’immersion dans la vie sentimentale comme synonyme de grandes tentations et de dangers pour une femme en développement. Ils montrent que les sentiments doivent être contrôlés. . . " (Baym 25). Frances Cogan note que les héroïnes sont suivent une éducation complète dans le but de remplir des obligations féminines (The All-American Girl). 6. Les histoires finissent habituellement par un mariage, correspondant en général à un des deux types possibles: A. Celui qui réhabilite un personnage masculin mauvais ou "sauvage", comme dans le Saint-Elmo d'Augusta Evans (1867) B. Celui qui marrie la protagoniste avec un homme stable qui répond déjà à ses exigences.Exemples: Maria Cummins, The Lamplighter (1854) et Susan Warner, The Wide, Wide World (1850) 7. Les romans peuvent utiliser un "langage larmoyant" qui provoque la sympathie des lecteurs. 8. Richard Brodhead (Cultures of Letters) voit la classe comme une question importante, car la famille idéale ou l'héroïne se situe entre une famille de classe inférieure illustrant la pauvreté et la désorganisation domestique et des personnages de classe supérieure illustrant une existence inactive et frivole (94). " Un exemple de ce style de roman est A Thousand Acres de Jane Smiley, dans lequel le confinement du personnage principal est souligné d’une telle manière. On compte Jane Austen et Elizabeth Barrett Browning comme des premières représentantes du réalisme domestique.</skos:definition>
    <owl:sameAs rdf:resource="http://dbpedia.org/resource/Domestic_realism"/>
    <rdfs:comment xml:lang="en">The description for this term is indebted to DBpedia. </rdfs:comment>
  </genre:ThematicGenre>
  <genre:PoeticGenre rdf:about="#elegy">
    <skos:definition xml:lang="en">"Mournful, melancholy, or plaintive poems, especially funeral songs or laments for the dead."  <![CDATA[<a href="#cwrc:db2f8571-a773-4068-a35f-34262950bb8f">(Getty, 2017)</a>]]></skos:definition>
    <rdfs:isDefinedBy rdf:resource="http://sparql.cwrc.ca/ontologies/genre-ONTOLOGY_DATE"/>
    <rdfs:label xml:lang="en">elegy</rdfs:label>
    <skos:definition xml:lang="fr">«L’élégie (en grec ancien ἐλεγεία / elegeía, signifiant « chant de mort ») fut une forme de poème dans l'Antiquité, avant de devenir un genre poétique à partir de la Renaissance. Dans l’Antiquité, était appelé « élégie » tout poème alternant hexamètres et pentamètres en distiques : ce sont les vers élégiaques. De nos jours, l’élégie est considérée comme un genre au sein de la poésie lyrique, en tant que poème de longueur et de forme variables caractérisé par son ton plaintif particulièrement adapté à l’évocation d’un mort ou à l’expression d’une souffrance amoureuse due à un abandon ou à une absence.»  <![CDATA[<a href="#cwrc:727d97bc-af78-4122-94be-aa78b2e97d5a">(DBpedia, 2017)</a>]]></skos:definition>
    <rdfs:label xml:lang="fr">élégie</rdfs:label>
    <rdfs:comment xml:lang="en">The description for this term is indebted to the Getty Art &amp; Architecture Thesaurus.</rdfs:comment>
    <owl:sameAs rdf:resource="http://id.loc.gov/authorities/genreForms/gf2014026307"/>
    <owl:sameAs rdf:resource="http://dbpedia.org/resource/Elegy"/>
  </genre:PoeticGenre>
  <genre:ThematicGenre rdf:about="#gardening">
    <skos:definition xml:lang="fr">Texte non fictif qui traite du jardinage.</skos:definition>
    <rdfs:label xml:lang="fr">jardinage</rdfs:label>
    <rdfs:isDefinedBy rdf:resource="http://sparql.cwrc.ca/ontologies/genre-ONTOLOGY_DATE"/>
    <rdfs:label xml:lang="en">gardening</rdfs:label>
    <skos:hiddenLabel xml:lang="en">GARDENINGBOOK</skos:hiddenLabel>
    <skos:definition xml:lang="en">A text, typically non-fiction, dealing with the subject of gardening.</skos:definition>
  </genre:ThematicGenre>
  <genre:PerformanceMedium rdf:about="#puppetry">
    <rdfs:isDefinedBy rdf:resource="http://sparql.cwrc.ca/ontologies/genre-ONTOLOGY_DATE"/>
    <rdfs:label xml:lang="en">puppetry</rdfs:label>
    <skos:definition xml:lang="en">"Puppetry is a form of theatre or performance that involves the manipulation of puppets—inanimate objects, often resembling some type of human or animal figure, that are animated or manipulated by a human called a puppeteer. Such a performance is also known as a puppet play. The puppeteer uses movements of her hands, arms, or control devices such as rods or strings to move the body, head, limbs, and in some cases the mouth and eyes of the puppet. The puppeteer often speaks in the voice of the character of the puppet, and then synchronizes the movements of the puppet's mouth with this spoken part. The actions, gestures and spoken parts acted out by the puppets are typically used in storytelling. There are many different varieties of puppets, and they are made of a wide range of materials, depending on their form and intended use. They can be extremely complex or very simple in their construction. The simplest puppets are finger puppets, which are tiny puppets that fit onto a single finger, and sock puppets, which are formed from a sock and operated by inserting one's hand inside the sock, with the opening and closing of the hand simulating the movement of the puppet's "mouth". A hand puppet is controlled by one hand which occupies the interior of the puppet and moves the puppet around (Punch and Judy puppets are familiar examples of hand puppets). A "live-hand puppet" is similar to a hand puppet but is larger and requires two puppeteer for each puppet. Marionettes are suspended and controlled by a number of strings, plus sometimes a central rod attached to a control bar held from above by the puppeteer. Puppetry is a very ancient form of theatre which was first recorded in the 5th century BC in Ancient Greece. Some forms of puppetry may have originated as long ago as 3000 years BC. Puppetry takes many forms, but they all share the process of animating inanimate performing objects to tell a story. Puppetry is used in almost all human societies both as entertainment – in performance – and ceremonially in rituals and celebrations such as carnivals." <![CDATA[<a href="#cwrc:727d97bc-af78-4122-94be-aa78b2e97d5a">(DBpedia, 2019)</a>]]></skos:definition>
    <skos:related rdf:resource="http://vocab.getty.edu/aat/300248147"/>
  </genre:PerformanceMedium>
  <genre:AutobiographicalGenre rdf:about="#memoir">
    <skos:related rdf:resource="http://id.loc.gov/authorities/genreForms/gf2014026047"/>
    <rdfs:isDefinedBy rdf:resource="http://sparql.cwrc.ca/ontologies/genre-ONTOLOGY_DATE"/>
    <rdfs:label xml:lang="en">memoir</rdfs:label>
    <skos:definition xml:lang="en">"A memoir (from French: mémoire: memoria, meaning memory or reminiscence) is a collection of memories that an individual writes about moments or events, both public or private, that took place in the subject's life. The assertions made in the work are understood to be factual. While memoir has historically been defined as a subcategory of biography or autobiography since the late 20th century, the genre is differentiated in form, presenting a narrowed focus. A biography or autobiography tells the story "of a life", while a memoir often tells "a story from a life", such as touchstone events and turning points from the author's life. The author of a memoir may be referred to as a "memoirist."" <![CDATA[<a href="#cwrc:727d97bc-af78-4122-94be-aa78b2e97d5a">(DBpedia, 2019)</a>]]></skos:definition>
  </genre:AutobiographicalGenre>
  <genre:DramaticGenre rdf:about="#monologue">
    <rdfs:isDefinedBy rdf:resource="http://sparql.cwrc.ca/ontologies/genre-ONTOLOGY_DATE"/>
    <rdfs:label xml:lang="en">monologue</rdfs:label>
    <owl:sameAs rdf:resource="http://id.loc.gov/authorities/genreForms/gf2014026440"/>
    <skos:definition xml:lang="fr">«Un monologue (du grec mono : "un seul", et logos : "discours") est une ou plusieurs phrases auto-adressées à haute voix, rapportant les pensées du locuteur au style direct.Il faut distinguer le véritable monologue non seulement, cela va de soi, du roman autobiographique à la première personne, qui suppose un décalage de temps, même minime ("Aujourd'hui maman est morte") entre la narration et le narré, mais aussi d'une forme d'écriture fictionnelle moderne, la représentation du flux intérieur sous la forme je ou tu.»  <![CDATA[<a href="#cwrc:727d97bc-af78-4122-94be-aa78b2e97d5a">(DBpedia, 2017)</a>]]></skos:definition>
    <skos:definition xml:lang="en">"In theatre, a monologue (from Greek μονόλογος from μόνος mónos, "alone, solitary" and λόγος lógos, "speech") is a speech presented by a single character, most often to express their mental thoughts aloud, though sometimes also to directly address another character or the audience. Monologues are common across the range of dramatic media (plays, films, etc.), as well as in non-dramatic media such as poetry. Monologues share much in common with several other literary devices including soliloquies, apostrophes, and aside. There are, however, distinctions between each of these devices."  <![CDATA[<a href="#cwrc:727d97bc-af78-4122-94be-aa78b2e97d5a">(DBpedia, 2017)</a>]]></skos:definition>
    <owl:sameAs rdf:resource="http://dbpedia.org/resource/Monologue"/>
    <rdfs:comment xml:lang="en">The description for this term is indebted to DBpedia. </rdfs:comment>
  </genre:DramaticGenre>
  <genre:ComedicGenre rdf:about="#blackComedy">
    <rdfs:comment xml:lang="en">The description for this term is indebted to DBpedia. </rdfs:comment>
    <skos:definition xml:lang="fr">«L’humour noir est une forme d’humour qui souligne avec cruauté, amertume et parfois désespoir l’absurdité du monde, face à laquelle il constitue quelques fois une forme de défense.»  <![CDATA[<a href="#cwrc:727d97bc-af78-4122-94be-aa78b2e97d5a">(DBpedia, 2017)</a>]]></skos:definition>
    <owl:sameAs rdf:resource="http://dbpedia.org/resource/Black_comedy"/>
    <skos:definition xml:lang="en">"A black comedy (or dark comedy) is a comic work that employs morbid humor, which, in its simplest form, is humor that makes light of subject matter usually considered taboo. Black humor corresponds to the earlier concept of gallows humor. Black comedy is often controversial due to its subject matter."  <![CDATA[<a href="#cwrc:727d97bc-af78-4122-94be-aa78b2e97d5a">(DBpedia, 2017)</a>]]></skos:definition>
    <owl:sameAs rdf:resource="http://id.loc.gov/authorities/genreForms/gf2014026248"/>
    <rdfs:comment xml:lang="fr">La description de ce terme est basée sur celle de DBPedia.</rdfs:comment>
    <rdfs:isDefinedBy rdf:resource="http://sparql.cwrc.ca/ontologies/genre-ONTOLOGY_DATE"/>
    <rdfs:label xml:lang="en">black comedy</rdfs:label>
    <rdfs:label xml:lang="fr">humour noir</rdfs:label>
  </genre:ComedicGenre>
  <genre:ReferenceWorkGenre rdf:about="#encyclopaedia">
    <skos:definition xml:lang="fr">Livres, séries de livres ou de disques contenant des articles informatifs, habituellement classés par ordre alphabétique, portant sur différents domaines du savoir général, ou se limitant à un domaine ou un sujet spécifique.</skos:definition>
    <owl:sameAs rdf:resource="http://id.loc.gov/authorities/genreForms/gf2014026092"/>
    <skos:definition xml:lang="en">"Books, set of books, or disks, containing informational articles on subjects in every field of knowledge, or limited to a special field or subject, usually arranged in alphabetical order."  <![CDATA[<a href="#cwrc:db2f8571-a773-4068-a35f-34262950bb8f">(Getty, 2017)</a>]]></skos:definition>
    <owl:sameAs rdf:resource="http://vocab.getty.edu/aat/300129439"/>
    <rdfs:label xml:lang="fr">encyclopédie</rdfs:label>
    <rdfs:comment xml:lang="en">The description for this term is indebted to the Getty Art &amp; Architecture Thesaurus.</rdfs:comment>
    <rdfs:isDefinedBy rdf:resource="http://sparql.cwrc.ca/ontologies/genre-ONTOLOGY_DATE"/>
    <rdfs:label xml:lang="en">encyclopaedia</rdfs:label>
  </genre:ReferenceWorkGenre>
  <genre:PoeticGenre rdf:about="#lais">
    <rdfs:comment xml:lang="en">This term and its description were created from data gathered from DBpedia.</rdfs:comment>
    <rdfs:isDefinedBy rdf:resource="http://sparql.cwrc.ca/ontologies/genre-ONTOLOGY_DATE"/>
    <rdfs:label xml:lang="en">lais</rdfs:label>
    <skos:definition xml:lang="fr">«Le lai est un poème à forme fixe apparu au XIIe siècle et qui a désigné successivement des genres de poésie assez différents. Au Moyen Âge, ce mot était employé au sens de « chant » (ou plutôt récit chanté) ou de « mélodie » ; on connaît le lai narratif, ancêtre du fabliau, et le lai lyrique. L’origine du lai et de son nom est peut-être née d’anciens souvenirs littéraires celtiques (liais en gallois ou laoith en gaélique) car les vieilles légendes de la « matière de Bretagne » y tiennent une grande place, mais on y trouve toujours aussi la matière de France et la matière de Rome.»  <![CDATA[<a href="#cwrc:727d97bc-af78-4122-94be-aa78b2e97d5a">(DBpedia, 2017)</a>]]></skos:definition>
    <rdfs:label xml:lang="fr">lai</rdfs:label>
    <skos:definition xml:lang="en">"A laisse is a type of stanza, of varying length, found in medieval French literature, specifically medieval French epic poetry (the chanson de geste), such as The Song of Roland. In early works, each laisse was made up of (mono) assonanced verses, although the appearance of (mono) rhymed laisses was increasingly common in later poems. Within a poem, the length of each separate laisse is variable (whereas the metric length of the verses is invariable, each verse having the same syllable length, typically decasyllables or, occasionally, alexandrines. The laisse is characterized by stereotyped phrases and formulas and frequently repeated themes and motifs, including repetitions of material from one laisse to another. Such repetitions and formulaic structures are common of orality and oral-formulaic composition. When medieval poets repeated content (with different wording or assonance/rhyme) from one laisse to another, such "similar" laisses are called laisses similaires in French."  <![CDATA[<a href="#cwrc:727d97bc-af78-4122-94be-aa78b2e97d5a">(DBpedia, 2017)</a>]]></skos:definition>
    <owl:sameAs rdf:resource="http://id.loc.gov/authorities/genreForms/gf2014026404"/>
    <owl:sameAs rdf:resource="http://dbpedia.org/resource/Lai"/>
  </genre:PoeticGenre>
  <genre:ThematicGenre rdf:about="#harlequinade">
    <skos:definition xml:lang="fr">Livres populaires aux 18ème et 19ème siècles, représentant à l'origine des harlequins, et dans lesquels des parties des pages qu'on soulève révèlent de nouvelles images, précisément placées sur les parties restantes des images précédentes.</skos:definition>
    <skos:definition xml:lang="en">"Books popular in the 18th and 19th centuries, originally often depicting harlequins, in which folded parts of pages are lifted to reveal new pictures, fitted neatly onto the remaining parts of the previous pictures."  <![CDATA[<a href="#cwrc:db2f8571-a773-4068-a35f-34262950bb8f">(Getty, 2017)</a>]]></skos:definition>
    <rdfs:comment xml:lang="en">This term and its description were created from data gathered from the Getty Art &amp; Architecture Thesaurus.</rdfs:comment>
    <owl:sameAs rdf:resource="http://vocab.getty.edu/aat/300212205"/>
    <rdfs:isDefinedBy rdf:resource="http://sparql.cwrc.ca/ontologies/genre-ONTOLOGY_DATE"/>
    <rdfs:label xml:lang="en">harlequinade</rdfs:label>
    <rdfs:label xml:lang="fr">harlequinade</rdfs:label>
  </genre:ThematicGenre>
  <genre:DramaticGenre rdf:about="#closetDrama">
    <rdfs:isDefinedBy rdf:resource="http://sparql.cwrc.ca/ontologies/genre-ONTOLOGY_DATE"/>
    <rdfs:label xml:lang="en">closet drama</rdfs:label>
    <rdfs:label xml:lang="fr">pièce en chambre</rdfs:label>
    <rdfs:comment xml:lang="en">This term and its description were created from data gathered from the Oxford Dictionary of Literary Terms, 4th ed.</rdfs:comment>
    <dcterms:references rdf:resource="http://www.oxfordreference.com/view/10.1093/acref/9780199208272.001.0001/acref-9780199208272-e-214?rskey=qZ7ZtK%26result=211"/>
    <skos:definition xml:lang="en">"A drama, often written in verse and frequently with extensive stage directions, that is meant to be read in private rather than performed for an audience."  <![CDATA[<a href="#cwrc:4c227091-6bf0-4325-b846-9733fae19e61">(Oxford, 2015)</a>]]></skos:definition>
  </genre:DramaticGenre>
  <genre:DidacticGenre rdf:about="#parable">
    <rdfs:isDefinedBy rdf:resource="http://sparql.cwrc.ca/ontologies/genre-ONTOLOGY_DATE"/>
    <rdfs:label xml:lang="en">parable</rdfs:label>
    <rdfs:comment xml:lang="en">The description for this term is indebted to DBpedia. </rdfs:comment>
    <skos:definition xml:lang="en">"Short, fictitious stories that illustrate a moral attitude or religious principle."  <![CDATA[<a href="#cwrc:db2f8571-a773-4068-a35f-34262950bb8f">(Getty, 2017)</a>]]></skos:definition>
    <skos:definition xml:lang="fr">«Une parabole (du grec παραϐολή, « rapprochement, comparaison ») est une des variétés de l’allégorie. La parabole est une figure de rhétorique consistant en une courte histoire qui utilise les événements quotidiens pour illustrer un enseignement, une morale ou une doctrine. Tandis que celle-ci, en général, présente directement le fait qu’elle a en vue, la parabole offre, sous ses couleurs véritables, un fait qui doit servir à la démonstration d’une vérité d’un autre ordre, avec laquelle elle a une relation plus ou moins facile à saisir. « Substituez dans la parabole, dit l’abbé Girard, le véritable fait à celui qu’elle expose, vous changerez le fond du discours : substituez dans l’allégorie les véritables couleurs à celles qu’elle emprunte, vous ne changerez que la forme. » On la trouve également dans le discours argumentatif lorsqu’un récit illustre la thèse défendue pour faciliter la compréhension du lecteur. La parabole est également un récit allégorique qui permet de dispenser un enseignement moral ou religieux. Présente dans la Bible où elle joue le rôle de l’apologue et de la fable, surtout les Évangiles, qui l'ont empruntée au midrash hébreu, la parabole est reprise dans les sermons des orateurs chrétiens. Le Nouveau Testament en contient un très grand nombre : le grain de sénevé ou l’Église, le Bon Samaritain ou l’amour de l’humanité, le levain ou la grâce, les loups ravisseurs sous des peaux d’agneaux ou les instituteurs de fausses doctrines, le travail des ouvriers de la vigne ou les œuvres du salut, le mauvais riche ou l’obligation de l’aumône, le bon pasteur, etc. Les paraboles sont plus fréquentes encore dans la littérature bouddhique ; les Avadanas, le Hitopadekas donnent à peine l’idée des recueils plus vastes dont ils sont extraits et dont l’un s’appelle le Yu-Lin, c’est-à-dire la « Forêt de comparaisons». Dans les littératures modernes, les Allemands ont surtout cultivé la parabole ; Lessing, Herder, Krummacher y ont particulièrement réussi. Dans le Bouc émissaire, page 270, René Girard remarque que « paraballo signifie jeter quelque chose en pâture à la foule pour apaiser son appétit de violence, de préférence une victime, un condamné à mort ; c'est ainsi qu'on se tire soi-même d'une situation épineuse, de toute évidence. C'est pour empêcher la foule de se retourner contre l'orateur que celui-ci recourt à la parabole, c'est-à-dire à la métaphore. »»  <![CDATA[<a href="#cwrc:727d97bc-af78-4122-94be-aa78b2e97d5a">(DBpedia, 2017)</a>]]></skos:definition>
    <owl:sameAs rdf:resource="http://vocab.getty.edu/aat/300185342"/>
    <owl:sameAs rdf:resource="http://id.loc.gov/authorities/genreForms/gf2014026467"/>
  </genre:DidacticGenre>
  <genre:DramaticGenre rdf:about="#epicTheatre">
    <skos:definition xml:lang="en">"Epic theatre is a theatrical movement arising in the early to mid-20th century from the theories and practice of a number of theatre practitioners who responded to the political climate of the time through the creation of new political dramas. Epic theatre is not meant to refer to the scale or the scope of the work, but rather to the form that it takes. Epic theatre emphasizes the audience's perspective and reaction to the piece through a variety of techniques that deliberately cause them to individually engage in a different way. The purpose of epic theatre is not to encourage an audience to suspend their disbelief, but rather to force them to see their world as it is." <![CDATA[<a href="#cwrc:50024824-8252-4a95-b62e-797911907f20">(DBpedia, 2021)</a>]]></skos:definition>
    <rdfs:comment xml:lang="en">This term and its description were created from data gathered from DBpedia.</rdfs:comment>
    <skos:closeMatch rdf:resource="https://dbpedia.org/page/Epic_theatre"/>
    <skos:related rdf:resource="https://sparql.cwrc.ca/ontologies/genre.html#epic"/>
    <rdfs:isDefinedBy rdf:resource="http://sparql.cwrc.ca/ontologies/genre-ONTOLOGY_DATE"/>
    <rdfs:label xml:lang="en">epic theatre</rdfs:label>
  </genre:DramaticGenre>
  <genre:DigitalMedium rdf:about="#digital">
    <skos:definition xml:lang="en">"Related to a device, instrument, information storage, work, or other application, operating according to the principles or methods using signals, information, or data represented by a series of discrete values (commonly the numbers 0 and 1), such as for electronic storage or processing." <![CDATA[<a href="#cwrc:bd595bc4-5991-4c51-98d9-9ab52c416f4f">(Getty, 2021)</a>]]></skos:definition>
    <rdfs:comment xml:lang="en">The description for this term is indebted to the Getty Art &amp; Architecture Thesaurus.</rdfs:comment>
    <owl:sameAs rdf:resource="http://vocab.getty.edu/aat/300404196"/>
    <rdfs:isDefinedBy rdf:resource="http://sparql.cwrc.ca/ontologies/genre-ONTOLOGY_DATE"/>
    <skos:broader rdf:resource="https://sparql.cwrc.ca/ontologies/genre.html#bornDigital"/>
    <skos:broader rdf:resource="https://sparql.cwrc.ca/ontologies/genre.html#webpage"/>
    <rdfs:label xml:lang="en">digital</rdfs:label>
  </genre:DigitalMedium>
  <genre:RomanceGenre rdf:about="#romance">
    <owl:sameAs rdf:resource="http://id.loc.gov/authorities/genreForms/gf2014026516"/>
    <skos:definition xml:lang="fr">Œuvre habituellement fictionnelle, qui tirent leur origines des romans chevaleresques du Moyen Âge et de la Renaissance représentant des chevaliers et des aventures merveilleuses. La romance traite des relations sentimentales, familiales et sexuelles, et s'articule souvent autours de récits hétéronormés qui se concluent par une union romantique ou un mariage. La catégorie comprend les œuvres reconnues pour leur qualité littéraire, ainsi que la littérature commerciale ou de genre produite pour un public de masse. Les sous-genres de la romance comprennent la littérature gothique, la romance historique et celles écrites durant la Régence anglaise.</skos:definition>
    <owl:sameAs rdf:resource="http://vocab.getty.edu/aat/300191065"/>
    <rdfs:isDefinedBy rdf:resource="http://sparql.cwrc.ca/ontologies/genre-ONTOLOGY_DATE"/>
    <rdfs:label xml:lang="en">literary romance</rdfs:label>
    <rdfs:comment xml:lang="en">The description for this term is indebted to the Getty Art &amp; Architecture Thesaurus.</rdfs:comment>
    <skos:definition xml:lang="en">"Poetic or prosaic literary forms derived from medieval narratives of love, legendary or heroic adventures, and chivalry. Extends to narratives about important religious figures, or fantastic or supernatural events."  <![CDATA[<a href="#cwrc:db2f8571-a773-4068-a35f-34262950bb8f">(Getty, 2017)</a>]]></skos:definition>
    <rdfs:label xml:lang="fr">romance</rdfs:label>
  </genre:RomanceGenre>
  <genre:ThematicGenre rdf:about="#orientalist">
    <rdf:type rdf:resource="#InformationalGenre"/>
    <rdfs:comment xml:lang="en">This term and its description were created from data gathered from DBpedia.</rdfs:comment>
    <rdfs:isDefinedBy rdf:resource="http://sparql.cwrc.ca/ontologies/genre-ONTOLOGY_DATE"/>
    <rdfs:label xml:lang="en">orientalist</rdfs:label>
    <rdfs:label xml:lang="fr">orientalisme</rdfs:label>
    <skos:hiddenLabel xml:lang="en">ORIENTAL</skos:hiddenLabel>
    <skos:definition xml:lang="fr">«L'orientalisme est un mouvement littéraire et artistique né en Occident au XIXe siècle. Il existe cependant un orientalisme prémoderne humaniste et classique qui remonte à la fin du Moyen Âge et au début de la Renaissance, lorsque les explorations commencèrent, avec par exemple Marco Polo, et qui atteint son apogée avec les turqueries et le goût oriental du XVIIIe siècle baroque puis rococo. Ce goût oriental hérite aussi du contact de l'époque des Croisades avec le monde islamique. Cet article traite donc plutôt de l'orientalisme à partir du XIXe siècle. C'est un mouvement qui marque l'intérêt de cette époque pour les cultures d'Afrique du Nord, turque et arabe, et toutes les régions dominées par l'Empire ottoman, jusqu'au Caucase.»  <![CDATA[<a href="#cwrc:727d97bc-af78-4122-94be-aa78b2e97d5a">(DBpedia, 2017)</a>]]></skos:definition>
    <skos:definition xml:lang="en">"Writing about the East by Western writers and with a Western perspective, encompassing everything from fiction to scientific writing. In Orientalist writing, even if not looked down upon as inferior, Eastern cultures are represented as foreign and exotic, and in need of translation, interpretation, or explanation."  <![CDATA[<a href="#cwrc:2f09376c-f784-4a46-9f04-5a21aa311f27">(Penguin, 1999)</a>]]></skos:definition>
  </genre:ThematicGenre>
  <genre:MysteryGenre rdf:about="#detective">
    <rdfs:label xml:lang="fr">roman policier</rdfs:label>
    <skos:closeMatch rdf:resource="http://dbpedia.org/resource/Detective_fiction"/>
    <skos:definition xml:lang="fr">«Le genre policier, ou polar, est un genre caractérisant certaines œuvres narratives et qui se distingue par sa mise en scène d'une énigme que le protagoniste tente de résoudre, souvent par une enquête de police. En ressortent notamment, en littérature le roman policier, au cinéma le film policier et à la télévision la série télévisée policière.»  <![CDATA[<a href="#cwrc:727d97bc-af78-4122-94be-aa78b2e97d5a">(DBpedia, 2017)</a>]]></skos:definition>
    <rdfs:comment xml:lang="en">This term and its description were created from data gathered from DBpedia.</rdfs:comment>
    <rdfs:isDefinedBy rdf:resource="http://sparql.cwrc.ca/ontologies/genre-ONTOLOGY_DATE"/>
    <rdfs:label xml:lang="en">detective</rdfs:label>
    <owl:sameAs rdf:resource="http://id.loc.gov/authorities/genreForms/gf2014026280"/>
    <skos:definition xml:lang="en">Detective fiction is a subgenre of crime fiction and mystery fiction in which an investigator or a detective—either professional or amateur—investigates a crime, often murder. <![CDATA[<a href="#cwrc:727d97bc-af78-4122-94be-aa78b2e97d5a">(DBpedia, 2019)</a>]]></skos:definition>
  </genre:MysteryGenre>
  <genre:JournalForm rdf:about="#column">
    <skos:definition xml:lang="en">"Written articles appearing regularly in a series in a newspaper." <![CDATA[<a href="#cwrc:bd595bc4-5991-4c51-98d9-9ab52c416f4f">(Getty, 2021)</a>]]></skos:definition>
    <rdfs:comment xml:lang="en">The description for this term is indebted to the Getty Art &amp; Architecture Thesaurus.</rdfs:comment>
    <owl:sameAs rdf:resource="http://vocab.getty.edu/aat/300026441"/>
    <rdfs:isDefinedBy rdf:resource="http://sparql.cwrc.ca/ontologies/genre-ONTOLOGY_DATE"/>
    <rdfs:label xml:lang="en">column</rdfs:label>
    <skos:related rdf:resource="http://vocab.getty.edu/aat/300026441"/>
  </genre:JournalForm>
  <genre:ThematicGenre rdf:about="#robinsonades">
    <rdfs:isDefinedBy rdf:resource="http://sparql.cwrc.ca/ontologies/genre-ONTOLOGY_DATE"/>
    <rdfs:label xml:lang="en">robinsonades</rdfs:label>
    <owl:sameAs rdf:resource="http://id.loc.gov/authorities/genreForms/gf2014026514"/>
    <skos:definition xml:lang="en">"Robinsonade (/ˌrɒbɪnsəˈneɪd/) is a literary genre that takes its name from the 1719 novel Robinson Crusoe by Daniel Defoe. The success of this novel spawned so many imitations that its name was used to define a genre, which is sometimes described simply as a "desert island story" or a "castaway narrative." The word "robinsonade" was coined by the German writer Johann Gottfried Schnabel in the Preface of his 1731 work Die Insel Felsenburg (The Island Stronghold). It is often viewed as a subgenre of survivalist fiction." <![CDATA[<a href="#cwrc:727d97bc-af78-4122-94be-aa78b2e97d5a">(DBpedia, 2019)</a>]]></skos:definition>
  </genre:ThematicGenre>
  <genre:StandaloneWork rdf:about="#giftbook">
    <rdfs:comment xml:lang="en">The description for this term is indebted to the Getty Art &amp; Architecture Thesaurus.</rdfs:comment>
    <owl:sameAs rdf:resource="http://id.loc.gov/authorities/genreForms/gf2017026072"/>
    <owl:sameAs rdf:resource="http://vocab.getty.edu/aat/300202541"/>
    <rdfs:label xml:lang="fr">livre d'étrenne</rdfs:label>
    <skos:definition xml:lang="fr">Livres, généralement des anthologies littéraires illustrées publiées une fois par an, destinées à être offertes et populaires au 19ème siècle. Pour les oeuvres produites afin de marquer une occasion, utilisez "souvenirs" (livres).</skos:definition>
    <skos:definition xml:lang="en">"Books, usually illustrated literary anthologies, intended to be given as gifts and often published annually; popular in the 19th century. For works produced to mark an occasion, use "keepsakes (books)."  <![CDATA[<a href="#cwrc:db2f8571-a773-4068-a35f-34262950bb8f">(Getty, 2017)</a>]]></skos:definition>
    <rdfs:isDefinedBy rdf:resource="http://sparql.cwrc.ca/ontologies/genre-ONTOLOGY_DATE"/>
    <rdfs:label xml:lang="en">giftbook</rdfs:label>
  </genre:StandaloneWork>
  <genre:DigitalMedium rdf:about="#computerProgram">
    <owl:sameAs rdf:resource="http://vocab.getty.edu/aat/300312188"/>
    <rdfs:comment xml:lang="en">The description for this term is indebted to the Getty Art &amp; Architecture Thesaurus.</rdfs:comment>
    <rdfs:label xml:lang="fr">programme informatique</rdfs:label>
    <rdfs:isDefinedBy rdf:resource="http://sparql.cwrc.ca/ontologies/genre-ONTOLOGY_DATE"/>
    <rdfs:label xml:lang="en">computer program</rdfs:label>
    <skos:related rdf:resource="http://vocab.getty.edu/aat/300312188"/>
    <skos:definition xml:lang="fr">" Compilation d'instructions codées, ou séquence de code qui lorsqu'on l'exécute permet de faire réaliser une tâche spécifique à une machine, le plus souvent un ordinateur." </skos:definition>
    <skos:definition xml:lang="en">"A compilation of coded instructions or sequence of code that, when run, achieves a certain task in a mechanism, usually a computer."  <![CDATA[<a href="#cwrc:db2f8571-a773-4068-a35f-34262950bb8f">(Getty, 2017)</a>]]></skos:definition>
  </genre:DigitalMedium>
  <genre:ScholarlyGenre rdf:about="#essay">
    <owl:sameAs rdf:resource="http://id.loc.gov/authorities/genreForms/gf2014026094"/>
    <rdfs:isDefinedBy rdf:resource="http://sparql.cwrc.ca/ontologies/genre-ONTOLOGY_DATE"/>
    <rdfs:label xml:lang="en">essay</rdfs:label>
    <skos:definition xml:lang="fr">«En littérature, un essai est une œuvre de réflexion portant sur les sujets les plus divers et exposée de manière personnelle, voire subjective par l'auteur. Contrairement à l'étude, l'essai peut être polémique ou partisan. C'est un texte littéraire qui se prête bien à la réflexion philosophique, mais aussi à d'autres domaines : essais historiques, essais scientifiques, essais politiques, etc. L'auteur d’un essai est appelé « essayiste ». Le terme « essai » est dérivé du latin exagium, un poids ou appareil de mesure.»  <![CDATA[<a href="#cwrc:727d97bc-af78-4122-94be-aa78b2e97d5a">(DBpedia, 2017)</a>]]></skos:definition>
    <owl:sameAs rdf:resource="http://vocab.getty.edu/aat/300026291"/>
    <rdfs:label xml:lang="fr">essai</rdfs:label>
    <skos:definition xml:lang="en">"Short literary compositions on single subjects, often presenting the personal view of the author."  <![CDATA[<a href="#cwrc:db2f8571-a773-4068-a35f-34262950bb8f">(Getty, 2017)</a>]]></skos:definition>
    <rdfs:comment xml:lang="en">The description for this term is indebted to DBpedia. </rdfs:comment>
  </genre:ScholarlyGenre>
  <genre:CartographicForm rdf:about="#map">
    <rdfs:isDefinedBy rdf:resource="http://sparql.cwrc.ca/ontologies/genre-ONTOLOGY_DATE"/>
    <rdfs:label xml:lang="en">map</rdfs:label>
    <rdfs:label xml:lang="fr">carte</rdfs:label>
    <skos:definition xml:lang="fr">Désigne des représentations graphiques ou photogrammétriques de la surface de la Terre ou d'une partie de celle-ci, y compris les caractéristiques physiques et les délimitations politiques, où chaque point correspond à une position géographique ou céleste selon une échelle ou une projection définie. Le terme peut également se référer à des représentations similaires d'autres planètes, de soleils, d'autres corps célestes ou des zones du ciel. Les cartes sont généralement représentées sur un support plat, tel que du papier, un mur ou un écran d'ordinateur.</skos:definition>
    <skos:related rdf:resource="http://vocab.getty.edu/aat/300028094"/>
    <owl:sameAs rdf:resource="http://id.loc.gov/authorities/genreForms/gf2011026387"/>
    <rdfs:comment xml:lang="en">This term and its description were created from data gathered from the Getty Art &amp; Architecture Thesaurus.</rdfs:comment>
    <owl:sameAs rdf:resource="http://vocab.getty.edu/aat/300028094"/>
    <skos:definition xml:lang="en">"Refers to graphic or photogrammetric representations of the Earth's surface or a part of it, including physical features and political boundaries, where each point corresponds to a geographical or celestial position according to a definite scale or projection. The term may also refer to similar depictions of other planets, suns, other heavenly bodies, or areas of the heavens. Maps are typically depicted on a flat medium, such as on paper, a wall, or a computer screen."  <![CDATA[<a href="#cwrc:db2f8571-a773-4068-a35f-34262950bb8f">(Getty, 2017)</a>]]></skos:definition>
  </genre:CartographicForm>
  <genre:NovelisticGenre rdf:about="#novel">
    <skos:definition xml:lang="en">"Invented prose narratives of considerable length and a certain complexity that deal imaginatively with human experience through a connected sequence of events involving a group of persons in a specific setting."  <![CDATA[<a href="#cwrc:db2f8571-a773-4068-a35f-34262950bb8f">(Getty, 2017)</a>]]></skos:definition>
    <owl:sameAs rdf:resource="http://dbpedia.org/ontology/Novel"/>
    <owl:sameAs rdf:resource="http://id.loc.gov/authorities/genreForms/gf2015026020"/>
    <rdfs:isDefinedBy rdf:resource="http://sparql.cwrc.ca/ontologies/genre-ONTOLOGY_DATE"/>
    <rdfs:label xml:lang="en">novel</rdfs:label>
    <skos:definition xml:lang="fr">«Le roman est un genre littéraire, caractérisé pour l'essentiel par une narration fictionnelle plus ou moins longue.»  <![CDATA[<a href="#cwrc:727d97bc-af78-4122-94be-aa78b2e97d5a">(DBpedia, 2017)</a>]]></skos:definition>
    <rdfs:label xml:lang="fr">roman</rdfs:label>
    <rdfs:comment xml:lang="en">This term and its description were created from data gathered from DBpedia.</rdfs:comment>
  </genre:NovelisticGenre>
  <genre:DramaticGenre rdf:about="#oneActPlay">
    <skos:definition xml:lang="en">"A one-act play is a play that has only one act, as distinct from plays that occur over several acts. One-act plays may consist of one or more scenes." <![CDATA[<a href="#cwrc:8b528b2b-1cd5-4249-9195-b08111ab826c">(Wikidata, 2021)</a>]]></skos:definition>
    <rdfs:comment xml:lang="en">This term and its description were created from data gathered from Wikidata.</rdfs:comment>
    <owl:sameAs rdf:resource="https://www.wikidata.org/wiki/Q1194583"/>
    <owl:sameAs rdf:resource="http://id.loc.gov/authorities/genreForms/gf2014026462"/>
    <rdfs:isDefinedBy rdf:resource="http://sparql.cwrc.ca/ontologies/genre-ONTOLOGY_DATE"/>
    <rdfs:label xml:lang="en">one-act-play</rdfs:label>
  </genre:DramaticGenre>
  <genre:IllustratedForm rdf:about="#colouringBook">
    <owl:sameAs rdf:resource="http://vocab.getty.edu/aat/300026449"/>
    <skos:definition xml:lang="en">"Books containing outline drawings, for coloring in with crayons, watercolor, colored pencils, or other media, usually intended for use by children."  <![CDATA[<a href="#cwrc:db2f8571-a773-4068-a35f-34262950bb8f">(Getty, 2017)</a>]]></skos:definition>
    <rdfs:comment xml:lang="en">The description for this term is indebted to the Getty Art &amp; Architecture Thesaurus.</rdfs:comment>
    <rdfs:isDefinedBy rdf:resource="http://sparql.cwrc.ca/ontologies/genre-ONTOLOGY_DATE"/>
    <rdfs:label xml:lang="en">colouring book</rdfs:label>
    <skos:definition xml:lang="fr">"Livres contenant des dessins à colorier à l'aide de crayons gras, aquarelles, crayons de couleur ou autres techniques, généralement destinés aux enfants." </skos:definition>
    <owl:sameAs rdf:resource="http://id.loc.gov/authorities/genreForms/gf2017026082"/>
    <rdfs:label xml:lang="fr">livre de coloriage</rdfs:label>
  </genre:IllustratedForm>
  <genre:PoeticGenre rdf:about="#fabliau">
    <rdfs:comment xml:lang="en">This term and its description were created from data gathered from DBpedia.</rdfs:comment>
    <rdfs:isDefinedBy rdf:resource="http://sparql.cwrc.ca/ontologies/genre-ONTOLOGY_DATE"/>
    <rdfs:label xml:lang="en">fabliau</rdfs:label>
    <skos:definition xml:lang="en">"A humorous, frequently ribald or "dirty" narrative popular with French poets, who traditionally wrote the story in octosyllabic couplets. The tales frequently revolve around trickery, practical jokes, sexual mishaps, scatology, mistaken identity, and bodily humor. Chaucer included several fabliaux in The Canterbury Tales, including the stories of the Shipman, the Friar, the Miller, the Reeve, and the Cook. Examples from French literature include Les Quatre Souhais Saint Martin, Audigier, and Beranger au Long Cul (Beranger of the Long Ass)."  <![CDATA[<a href="cwrc:509015ff-7641-473e-94c5-688e06952bb7">(L. K Wheeler, 2017)</a>]]></skos:definition>
    <skos:definition xml:lang="fr">«Fabliau (du picard, lui-même issu du latin fabula qui donna en français « fable », signifie littéralement « petit récit ») est le nom qu'on donne dans la littérature française du Moyen Âge à de petites histoires simples et amusantes, définies par Bédier comme des contes à rire en vers. Leur vocation est de distraire ou faire rire les auditeurs et lecteurs, mais ils peuvent prétendre offrir une leçon morale, parfois ambiguë.»  <![CDATA[<a href="#cwrc:727d97bc-af78-4122-94be-aa78b2e97d5a">(DBpedia, 2017)</a>]]></skos:definition>
    <dcterms:references rdf:resource="http://web.cn.edu/kwheeler/lit_terms_f.html"/>
    <rdfs:label xml:lang="fr">fabliau</rdfs:label>
  </genre:PoeticGenre>
  <genre:PoliticalGenre rdf:about="#tractPamphlet">
    <rdfs:comment xml:lang="en">This term and its description were created from data gathered from DBpedia.</rdfs:comment>
    <skos:definition xml:lang="en">"Writing printed on a single sheet of paper or in a small booklet, designed to be distributed to the public. The subject matter is typically religious or political, and aims to persuade the reader of a certain point of view."  <![CDATA[<a href="#cwrc:db2f8571-a773-4068-a35f-34262950bb8f">(Getty, 2017)</a>]]></skos:definition>
    <skos:definition xml:lang="fr">«Un tract, un prospectus ou en français feuille volante, en anglais flyer (le terme pamphlet est également utilisé au Québec, et le terme manifeste en suisse francophone) est un texte ou une publicité sur support papier qui est distribué de la main à la main dans les espaces publics, en particulier sur les trottoirs, ou directement déposé dans les boîtes aux lettres par des personnes employées à cette tâche ou agissant par militantisme afin de faire passer des idées, de promouvoir un produit ou d'annoncer un événement artistique, culturel ou politique. Lorsque l'objet est purement commercial, on parle plutôt de prospectus.»  <![CDATA[<a href="#cwrc:727d97bc-af78-4122-94be-aa78b2e97d5a">(DBpedia, 2017)</a>]]></skos:definition>
    <rdfs:isDefinedBy rdf:resource="http://sparql.cwrc.ca/ontologies/genre-ONTOLOGY_DATE"/>
    <rdfs:label xml:lang="en">tract pamphlet</rdfs:label>
    <owl:sameAs rdf:resource="http://vocab.getty.edu/aat/300027211"/>
    <rdfs:label xml:lang="fr">tract</rdfs:label>
    <owl:sameAs rdf:resource="http://id.loc.gov/authorities/genreForms/gf2015026053"/>
    <rdf:type rdf:resource="#ReligiousGenre"/>
  </genre:PoliticalGenre>
  <genre:InformationalGenre rdf:about="#survey">
    <rdfs:isDefinedBy rdf:resource="http://sparql.cwrc.ca/ontologies/genre-ONTOLOGY_DATE"/>
    <skos:definition xml:lang="en">"Documentation of examinations, inspections, or questionnaires conducted in order to achieve a comprehensive view, as of a place, a group of related items, or to ascertain condition or value."<![CDATA[<a href="#cwrc:bd595bc4-5991-4c51-98d9-9ab52c416f4f">(Getty, 2021)</a>]]></skos:definition>
    <rdfs:comment xml:lang="en">The description for this term is indebted to the Getty Art &amp; Architecture Thesaurus.</rdfs:comment>
    <owl:sameAs rdf:resource="http://vocab.getty.edu/aat/300226986"/>
    <rdfs:label xml:lang="en">survey</rdfs:label>
  </genre:InformationalGenre>
  <genre:InformationalGenre rdf:about="#register">
    <rdfs:isDefinedBy rdf:resource="http://sparql.cwrc.ca/ontologies/genre-ONTOLOGY_DATE"/>
    <skos:definition xml:lang="en">"Lists of names, addresses, events, dates, etc., usually presented in a single chronological or numerical sequence (e.g., parish or guild registers, birth/death/marriage)."<![CDATA[<a href="#cwrc:788072dc-a6e5-44b1-b72b-873846d117a8">(Library of Congress, 2022)</a>]]></skos:definition>
    <rdfs:comment xml:lang="en">The description for this term is indebted to The Library of Congress.</rdfs:comment>
    <owl:sameAs rdf:resource="http://id.loc.gov/authorities/genreForms/gf2014026166"/>
    <rdfs:label xml:lang="en">register</rdfs:label>
  </genre:InformationalGenre>
  <genre:FinancialRecordsGenre rdf:about="#accountBook">
    <rdfs:isDefinedBy rdf:resource="http://sparql.cwrc.ca/ontologies/genre-ONTOLOGY_DATE"/>
    <skos:definition xml:lang="en">"Accounting journals, Accounting ledgers, Books of account, Journals, Accounting, Ledgers, Accounting, Records (Documents)."<![CDATA[<a href="#cwrc:788072dc-a6e5-44b1-b72b-873846d117a8">(Library of Congress, 2022)</a>]]></skos:definition>
    <rdfs:comment xml:lang="en">The description for this term is indebted to The Library of Congress.</rdfs:comment>
    <owl:sameAs rdf:resource="http://id.loc.gov/authorities/genreForms/gf2017026136"/>
    <rdfs:label xml:lang="en">account book</rdfs:label>
  </genre:FinancialRecordsGenre>  
  <genre:PerformanceMedium rdf:about="#cabaret">
    <rdfs:isDefinedBy rdf:resource="http://sparql.cwrc.ca/ontologies/genre-ONTOLOGY_DATE"/>
    <rdfs:label xml:lang="en">cabaret</rdfs:label>
    <rdfs:comment xml:lang="en">This term and its description were created from data gathered from the Oxford Dictionary of English, 3rd ed.</rdfs:comment>
    <dcterms:references rdf:resource="http://www.oxfordreference.com/view/10.1093/acref/9780199571123.001.0001/m_en_gb0114080?rskey=xIWuHx%26result=12581"/>
    <rdfs:label xml:lang="fr">spectacle de cabaret</rdfs:label>
    <skos:definition xml:lang="en">"Various forms of entertainment, often involving dancing, singing, or comedy acts, performed at a venue such as a nightclub in which the audience is seated at tables. Live music played in restaurants or public houses would not usually be considered cabaret without an additional component."  <![CDATA[<a href="#cwrc:4c227091-6bf0-4325-b846-9733fae19e61">(Oxford, 2015)</a>]]></skos:definition>
    <skos:definition xml:lang="fr">Formes de spectacles divers, incluant souvent de la danse, du chant ou de la comédie, représentés dans une salle de spectacle, généralement un cabaret, où le public est assis à des tables. La musique jouée dans les restaurants ou les tavernes n'est généralement pas considérée comme un spectacle de cabaret, à moins qu'elle présente des éléments distinctifs.</skos:definition>
  </genre:PerformanceMedium>
  <genre:InformationalGenre rdf:about="#governmentReport">
    <rdfs:label xml:lang="fr">rapport gouvernemental</rdfs:label>
    <skos:definition xml:lang="fr">Publication officielle émise par un gouvernement, couvrant une large variété de sujets.</skos:definition>
    <skos:definition xml:lang="en">An official government publication covering any of a wide variety of subjects.</skos:definition>
    <rdfs:isDefinedBy rdf:resource="http://sparql.cwrc.ca/ontologies/genre-ONTOLOGY_DATE"/>
    <rdfs:label xml:lang="en">government report</rdfs:label>
    <skos:hiddenLabel xml:lang="en">PARLIAMENTARYREPORT</skos:hiddenLabel>
  </genre:InformationalGenre>
  <genre:GovernmentRecordsGenre rdf:about="#municipalOrdinance">
    <skos:definition xml:lang="en">"Laws established by cities, towns, or other local governmental entities. For rules or administrative provisions adopted by an organization for its internal governance and its external dealings." <![CDATA[<a href="#cwrc:788072dc-a6e5-44b1-b72b-873846d117a8">(Library of Congress, 2022)</a>]]></skos:definition>
    <rdfs:comment xml:lang="en">The description for this term is indebted to The Library of Congress.</rdfs:comment>
    <owl:sameAs rdf:resource="http://id.loc.gov/authorities/genreForms/gf2011026412"/>
    <rdfs:isDefinedBy rdf:resource="http://sparql.cwrc.ca/ontologies/genre-ONTOLOGY_DATE"/>
    <rdfs:label xml:lang="en">municipal ordinance</rdfs:label>
  </genre:GovernmentRecordsGenre> 
  <genre:InformationalGenre rdf:about="#administrativeDecision">
    <skos:definition xml:lang="en">"Decisions and opinions of administrative agencies."<![CDATA[<a href="#cwrc:788072dc-a6e5-44b1-b72b-873846d117a8">(Library of Congress, 2022)</a>]]></skos:definition>
    <rdfs:comment xml:lang="en">The description for this term is indebted to The Library of Congress.</rdfs:comment>
    <rdfs:isDefinedBy rdf:resource="http://sparql.cwrc.ca/ontologies/genre-ONTOLOGY_DATE"/>
    <owl:sameAs rdf:resource="http://id.loc.gov/authorities/genreForms/gf2011026029"/>
    <rdfs:label xml:lang="en">administrative decision</rdfs:label>
  </genre:InformationalGenre>  
  <genre:DidacticGenre rdf:about="#conductLiterature">
    <rdfs:isDefinedBy rdf:resource="http://sparql.cwrc.ca/ontologies/genre-ONTOLOGY_DATE"/>
    <rdfs:label xml:lang="en">conduct literature</rdfs:label>
    <rdfs:label xml:lang="fr">livre de conduite</rdfs:label>
    <rdfs:comment xml:lang="en">This term and its description were created from data gathered from the Penguin Dictionary of Literary Terms &amp; Literary Theory, 4th ed.</rdfs:comment>
    <skos:definition xml:lang="en">"Prescriptive literature, usually directed to a specific gender, that outlines the rules of appropriate behaviour according to the gender roles and societal norms prevalent at the time of writing. Conduct books became very popular in the 18th century."  <![CDATA[<a href="#cwrc:2f09376c-f784-4a46-9f04-5a21aa311f27">(Penguin, 1999)</a>]]></skos:definition>
    <skos:definition xml:lang="fr">«Un conduct book (littéralement : « livre de conduite », ou « manuel de conduite ») est un genre littéraire anglais, très répandu à la fin du XVIIIe siècle et au début du XIXe siècle et dont le but est de former le lecteur aux respects des convenances et aux règles de la vie en société. On peut rapprocher de ce genre les conduct novels, les romans d'apprentissage, qui poursuivent le même but au travers d'une histoire romancée.»  <![CDATA[<a href="#cwrc:727d97bc-af78-4122-94be-aa78b2e97d5a">(DBpedia, 2017)</a>]]></skos:definition>
    <owl:sameAs rdf:resource="http://dbpedia.org/resource/Conduct_book"/>
  </genre:DidacticGenre>
  <genre:PerformanceMedium rdf:about="#speech">
    <rdfs:label xml:lang="fr">discours</rdfs:label>
    <rdfs:comment xml:lang="en">The description for this term is indebted to the Getty Art &amp; Architecture Thesaurus.</rdfs:comment>
    <owl:sameAs rdf:resource="http://vocab.getty.edu/aat/300026671"/>
    <owl:sameAs rdf:resource="http://id.loc.gov/authorities/genreForms/gf2011026363"/>
    <skos:definition xml:lang="fr">Documents qui fournissent la transcription écrite d'une adresse publique ou d'une conversation.</skos:definition>
    <rdfs:isDefinedBy rdf:resource="http://sparql.cwrc.ca/ontologies/genre-ONTOLOGY_DATE"/>
    <rdfs:label xml:lang="en">speech</rdfs:label>
    <skos:definition xml:lang="en">"Documents containing the text of any public address or talk"  <![CDATA[<a href="#cwrc:db2f8571-a773-4068-a35f-34262950bb8f">(Getty, 2017)</a>]]></skos:definition>
  </genre:PerformanceMedium>
  <genre:ReligiousGenre rdf:about="#prayer">
    <rdfs:label xml:lang="fr">prière</rdfs:label>
    <skos:definition xml:lang="fr">Documents contenant des requêtes respectueusement adressées à une divinité ou à une autre entité spirituelle.</skos:definition>
    <owl:sameAs rdf:resource="http://vocab.getty.edu/aat/300026452"/>
    <rdfs:comment xml:lang="en">This term and its description were created from data gathered from the Getty Art &amp; Architecture Thesaurus.</rdfs:comment>
    <owl:sameAs rdf:resource="http://id.loc.gov/authorities/genreForms/gf2015026049"/>
    <rdfs:isDefinedBy rdf:resource="http://sparql.cwrc.ca/ontologies/genre-ONTOLOGY_DATE"/>
    <rdfs:label xml:lang="en">prayer</rdfs:label>
    <skos:definition xml:lang="en">"Reverent petitions, usually in verse or prose, to a deity or other spiritual entity."  <![CDATA[<a href="#cwrc:db2f8571-a773-4068-a35f-34262950bb8f">(Getty, 2017)</a>]]></skos:definition>
  </genre:ReligiousGenre>
  <genre:SocialScienceGenre rdf:about="#socialScience">
    <skos:definition xml:lang="en">Writing dealing with the study of human societies and relationships across several fields of scientific study, including anthropology, political science, and sociology.</skos:definition>
    <rdfs:label xml:lang="fr">sciences sociales</rdfs:label>
    <skos:definition xml:lang="fr">Travaux écrits qui étudient les sociétés et les rapports humains à travers plusieurs disciplines scientifiques incluant l'anthropologie, les sciences politiques et la sociologie.</skos:definition>
    <rdfs:isDefinedBy rdf:resource="http://sparql.cwrc.ca/ontologies/genre-ONTOLOGY_DATE"/>
    <rdfs:label xml:lang="en">social science</rdfs:label>
  </genre:SocialScienceGenre>
  <genre:ProverbForm rdf:about="#aphorism">
    <owl:sameAs rdf:resource="http://vocab.getty.edu/aat/300253001"/>
    <rdfs:isDefinedBy rdf:resource="http://sparql.cwrc.ca/ontologies/genre-ONTOLOGY_DATE"/>
    <rdfs:label xml:lang="en">aphorism</rdfs:label>
    <skos:definition xml:lang="fr">" Déclarations de principes ou de préceptes concises et lapidaires, souvent d'un auteur connu, différant des "proverbes" qui sont des propos répétés dans la langue orale et qui incarnent souvent la sagesse populaire d'un groupe ou d'une nation. " </skos:definition>
    <rdfs:label xml:lang="fr">aphorisme</rdfs:label>
    <skos:definition xml:lang="en">"Short, pithy statements of principle or precepts, often of known authorship; distinguished from "proverbs" which are statements repeated colloquially and which often embody the folk wisdom of a group or nation."  <![CDATA[<a href="#cwrc:db2f8571-a773-4068-a35f-34262950bb8f">(Getty, 2017)</a>]]></skos:definition>
    <rdfs:comment xml:lang="en">The description for this term is indebted to the Getty Art &amp; Architecture Thesaurus.</rdfs:comment>
  </genre:ProverbForm>
  <genre:NarrativeGenre rdf:about="#folkTale">
    <skos:altLabel xml:lang="en">folklore</skos:altLabel>
    <rdfs:isDefinedBy rdf:resource="http://sparql.cwrc.ca/ontologies/genre-ONTOLOGY_DATE"/>
    <rdfs:label xml:lang="en">folk tale</rdfs:label>
    <skos:definition xml:lang="en">"Traditional stories or legends in a given culture that are passed down over time, often orally." <![CDATA[<a href="#cwrc:a0414fff-d3ba-4d20-9d13-623b4ddc077f">(Getty, 2022)</a>]]></skos:definition>
    <rdfs:comment xml:lang="en">This term and its description were created from data gathered from the Getty Art &amp; Architecture Thesaurus.</rdfs:comment>
    <owl:sameAs rdf:resource="http://vocab.getty.edu/aat/300055922"/>
  </genre:NarrativeGenre>
  <genre:PhilosophicalGenre rdf:about="#philosophical">
    <skos:definition xml:lang="en">Writing engaging in philosophical questions, that may or may not be considered philosophy per se.</skos:definition>
    <rdfs:label xml:lang="fr">philosophique</rdfs:label>
    <rdfs:isDefinedBy rdf:resource="http://sparql.cwrc.ca/ontologies/genre-ONTOLOGY_DATE"/>
    <rdfs:label xml:lang="en">philosophical</rdfs:label>
    <skos:definition xml:lang="fr">Textes qui abordent des questions philosophiques, qui sont ou non considérés comme de la philosophie à proprement parler.</skos:definition>
  </genre:PhilosophicalGenre>
  <genre:CalendarForm rdf:about="#calendar">
    <skos:definition xml:lang="en">"A calendar is a system of organizing days for social, religious, commercial or administrative purposes. This is done by giving names to periods of time, typically days, weeks, months, and years. A date is the designation of a single, specific day within such a system. A calendar is also a physical record (often paper) of such a system. A calendar can also mean a list of planned events, such as a court calendar or a partly or fully chronological list of documents, such as a calendar of wills. Periods in a calendar (such as years and months) are usually, though not necessarily, synchronized with the cycle of the sun or the moon. The most common type of pre-modern calendar was the lunisolar calendar, a lunar calendar that occasionally adds one intercalary month to remain synchronised with the solar year over the long term. The calendar in most widespread use today is the Gregorian calendar, introduced in the 16th century by Pope Gregory XIII as a modification of the Julian calendar, which was itself a modification of the ancient Roman calendar.The term calendar itself is taken from calendae, the term for the first day of the month in the Roman calendar, related to the verb calare "to call out", referring to the "calling" of the new moon when it was first seen.Latin calendarium meant "account book, register" (as accounts were settled and debts were collected on the calends of each month). The Latin term was adopted in Old French as calendier and from there in Middle English as calender by the 13th century (the spelling calendar is early modern)." <![CDATA[<a href="#cwrc:727d97bc-af78-4122-94be-aa78b2e97d5a">(DBpedia, 2019)</a>]]></skos:definition>
    <rdfs:isDefinedBy rdf:resource="http://sparql.cwrc.ca/ontologies/genre-ONTOLOGY_DATE"/>
    <rdfs:label xml:lang="en">calendar</rdfs:label>
  </genre:CalendarForm>
  <genre:PoeticGenre rdf:about="#lyric">
    <owl:sameAs rdf:resource="http://www.universalis.fr/encyclopedie/lyrisme/"/>
    <rdfs:comment xml:lang="en">This term and its description were created from data gathered from Encyclopaedia Universalis.</rdfs:comment>
    <skos:definition xml:lang="fr">Terme dérivé de la lyre, instrument de musique symbole du pouvoir de la poésie remontant au mythe d'Orphée dans l'Antiquité. L'adjectif "lyrique" apparaît en France au XVIe siècle, mais devient de plus en plus utilisé au XIXe pour décrire le romantisme. Il réfère souvent à un type de poésie particulièrement centrée sur la subjectivité du poète et l'expression de ses sentiments. Toutefois, il n'est pas réductible à cet aspect, et peut être résumé en trois concepts majeurs: subjectivité, chant et idéalité. Dans la critique littéraire, le lyrique est un registre qui peut aussi être étudié dans d'autres formes littéraires, comme le roman.</skos:definition>
    <owl:sameAs rdf:resource="http://id.loc.gov/authorities/genreForms/gf2014026422"/>
    <skos:definition xml:lang="en">"Lyric Essay is a subgenre of essay writing, which combines qualities of poetry, essay, memoir, and research writing. The lyric essay is considered high art, and often requires work and association on behalf of the reader. Proponents of the lyric essay classification insist it differs from prose poetry in its reliance on association rather than line breaks and juxtaposition."  <![CDATA[<a href="#cwrc:727d97bc-af78-4122-94be-aa78b2e97d5a">(DBpedia, 2017)</a>]]></skos:definition>
    <rdfs:label xml:lang="fr">lyrique</rdfs:label>
    <rdfs:isDefinedBy rdf:resource="http://sparql.cwrc.ca/ontologies/genre-ONTOLOGY_DATE"/>
    <rdfs:label xml:lang="en">lyric</rdfs:label>
  </genre:PoeticGenre>
  <genre:PoeticGenre rdf:about="#ballad">
    <rdfs:comment xml:lang="en">The description for this term is indebted to DBpedia.</rdfs:comment>
    <rdfs:isDefinedBy rdf:resource="http://sparql.cwrc.ca/ontologies/genre-ONTOLOGY_DATE"/>
    <rdfs:label xml:lang="en">ballad</rdfs:label>
    <owl:sameAs rdf:resource="http://id.loc.gov/authorities/genreForms/gf2014026648"/>
    <skos:definition xml:lang="fr">«Ballade désigne, au sens ancien, un poème médiéval à forme fixe composé de trois couplets et d'une demi-strophe appelée envoi, chacune étant terminée par un vers refrain, qui rappelle la forme chantée des origines. L'histoire de la poésie retient en particulier les ballades aux strophes carrées (le nombre de vers est égal au nombre de syllabes de chaque vers) de huit ou dix vers et aux thèmes très variés qu'ont composées des poètes comme Guillaume de Machaut, Eustache Deschamps (fin xiv siècle), Christine de Pisan et François Villon (début et milieu du xve siècle) ou encore Clément Marot au xvie, alors que la Pléiade rejette le genre de la ballade comme vieilli, privilégiant des formes nouvelles comme le sonnet ou l'ode.»  <![CDATA[<a href="#cwrc:727d97bc-af78-4122-94be-aa78b2e97d5a">(DBpedia, 2017)</a>]]></skos:definition>
    <rdfs:comment xml:lang="fr">La description de ce terme est basée sur celle de DBPedia.</rdfs:comment>
    <rdfs:label xml:lang="fr">ballade</rdfs:label>
    <skos:definition xml:lang="en">A ballad /ˈbæləd/ is a form of verse, often a narrative set to music. Ballads derive from the medieval French chanson balladée or ballade, which were originally "dancing songs". Ballads were particularly characteristic of the popular poetry and song of the British Isles from the later medieval period until the 19th century and used extensively across Europe and later the Americas, Australia and North Africa. <![CDATA[<a href="#cwrc:727d97bc-af78-4122-94be-aa78b2e97d5a">(DBpedia, 2017)</a>]]></skos:definition>
    <skos:closeMatch rdf:resource="http://dbpedia.org/resource/Ballad"/>
  </genre:PoeticGenre>
  <genre:ThematicGenre rdf:about="#eulogy">
    <rdfs:isDefinedBy rdf:resource="http://sparql.cwrc.ca/ontologies/genre-ONTOLOGY_DATE"/>
    <rdfs:label xml:lang="en">eulogy</rdfs:label>
    <owl:sameAs rdf:resource="http://dbpedia.org/resource/Eulogy"/>
    <rdfs:comment xml:lang="en">The description for this term is indebted to DBpedia. </rdfs:comment>
    <skos:definition xml:lang="en">"A eulogy (from εὐλογία, eulogia, Classical Greek for "praise") is a speech or writing in praise of a person(s) or thing(s), especially one who recently died or retired or as a term of endearment. Eulogies may be given as part of funeral services. They take place in a funeral home during or after a wake. However, some denominations either discourage or do not permit eulogies at services to maintain respect for traditions. Eulogies can also praise people who are still alive. This normally takes place on special occasions like birthdays, office parties, retirement celebrations, etc. Eulogies should not be confused with elegies, which are poems written in tribute to the dead; nor with obituaries, which are published biographies recounting the lives of those who have recently died; nor with obsequies, which refer generally to the rituals surrounding funerals. Catholic priests are prohibited by the rubrics of the Mass from presenting a eulogy for the deceased in place of a homily during a funeral Mass. The modern use of the word eulogy was first documented in the 15th century and came from the Medieval Latin term “eulogium” (Merriam-Webster 2012). “Eulogium” at that time has since turned into the shorter “eulogy” of today. Eulogies are usually delivered by a family member or a close family friend in the case of a dead person. For a living eulogy given in such cases as a retirement, a senior colleague could perhaps deliver it. On occasions, eulogies are given to those who are severely ill or elderly in order to express words of love and gratitude before they die. Eulogies are not limited to merely people, however; Places or things can also be given eulogies (which anyone can deliver), but these are less common than those delivered to people, whether living or deceased."  <![CDATA[<a href="#cwrc:727d97bc-af78-4122-94be-aa78b2e97d5a">(DBpedia, 2017)</a>]]></skos:definition>
    <skos:definition xml:lang="fr">«L’éloge (masculin du latin elogium, avec l’influence du grec εὐλογία) est un genre littéraire hérité de l'Antiquité, où il est très présent, qui consiste à vanter les mérites d'un individu ou d'une institution. Il s'agit d'un discours public ou donné comme tel, destiné à l'édification commune ; à cette fin, il recourt à l'exploitation des ressources du discours épidictique héritées de la rhétorique classique. Il existe plusieurs sortes d'éloges:»</skos:definition>
  </genre:ThematicGenre>
  <genre:RecordForm rdf:about="#record">
    <owl:sameAs rdf:resource="http://dbpedia.org/resource/Document"/>
    <owl:sameAs rdf:resource="http://id.loc.gov/authorities/genreForms/gf2014026163"/>
    <skos:definition xml:lang="en">"Evidence about an object or the past, regardless of medium, as preserved in a record or document. As defined by the Library of Congress, records are "Documents in any form created or received by an agency, institution, organization, or individual, accumulated in the normal conduct of business or affairs."  <![CDATA[<a href="http://id.loc.gov/authorities/genreForms/g(f2014026163.html">Library of Congress, 2018)</a>]]> Wikipedia says, "A document is a written, drawn, presented or recorded representation of thoughts. Originating from the Latin Documentum meaning lesson - the verb doceō means to teach, and is pronounced similarly, in the past it was usually used as a term for a written proof used as evidence. In the computer age, a document is usually used to describe a primarily textual file, along with its structure and design, such as fonts, colors and additional images."  <![CDATA[<a href="https://en.wikipedia.org/wiki/Document">(Wikipedia, 2018)</a>]]> Information scientist Suzanne Breit defines a document as "any concrete or symbolic indication, preserved or recorded, for reconstructing or for proving a phenomenon, whether physical or mental."  <![CDATA[<a href="#cwrc:3A9ee53c63-e387-4fc0-ad17-df5a84dddb4">(Breit, 1951; translated)</a>]]></skos:definition>
    <rdfs:isDefinedBy rdf:resource="http://sparql.cwrc.ca/ontologies/genre-ONTOLOGY_DATE"/>
    <rdfs:label xml:lang="en">record</rdfs:label>
    <rdfs:label xml:lang="fr">notice</rdfs:label>
    <skos:definition xml:lang="fr">«Un document renvoie à un ensemble formé par un support et une information, celle-ci enregistrée de manière persistante. Il a une valeur explicative, descriptive ou de preuve. Vecteur matériel de la pensée humaine, il joue un rôle essentiel dans la plupart des sociétés contemporaines, tant pour le fonctionnement de leurs administrations que dans l'élaboration de leurs savoirs.»  <![CDATA[<a href="http://fr.dbpedia.org/resource/Document">(Breit, 1951</a>; <a href="http://martinetl.free.fr/suzannebriet/questcequeladocumentation/briet.pdf">pdf)</a>]]> «[T]out indice concret ou symbolique, conservé out enregistré, aux fins de représenter, de reconstituer ou de prouver un phénomène ou physique out intellectuel» <![CDATA[<a href="#cwrc:3A9ee53c63-e387-4fc0-ad17-df5a84dddb4">(Breit, 1951)</a>]]></skos:definition>
    <rdfs:comment xml:lang="en">This term and its description were created from data gathered from DBpedia.</rdfs:comment>
  </genre:RecordForm>
  <genre:MusicalGenre rdf:about="#hymn">
    <rdfs:label xml:lang="fr">hymne (poétique)</rdfs:label>
    <skos:definition xml:lang="en">"A religious song consisting of one or more repeating rhythmical stanzas. In classical Roman literature, hymns to Minerva and Jupiter survive. The Greek poet Sappho wrote a number of hymns to Aphrodite. More recently a vast number of hymns appear in Catholic and Protestant religious lyrics. A particularly vibrant tradition of hymn-writing comes from the South's African-American population during the nineteenth century. In the realm of fiction, C.S. Lewis creates hymns for the Solid Ones in The Great Divorce, and Tolkien creates Elvish hymns such as "O Elbereth" in The Lord of the Rings, typically with quatrain structure alternating with couplet stanzas. In the example of "O Elbereth," the hymn honors one of the Maiar spirits. See also paean."  <![CDATA[<a href="cwrc:509015ff-7641-473e-94c5-688e06952bb7">(L. K Wheeler, 2017)</a>]]></skos:definition>
    <rdfs:comment xml:lang="en">The description for this term is indebted to Dr. L. Kip Wheeler of Carson-Newman University. </rdfs:comment>
    <rdfs:isDefinedBy rdf:resource="http://sparql.cwrc.ca/ontologies/genre-ONTOLOGY_DATE"/>
    <rdfs:label xml:lang="en">hymn</rdfs:label>
    <owl:sameAs rdf:resource="http://id.loc.gov/authorities/genreForms/gf2014026872"/>
    <rdf:type rdf:resource="#PoeticGenre"/>
    <skos:definition xml:lang="fr">Des chants d'éloge en l'honneur des dieux, de pays, de personnes célèbres ou d'autres objets de haute estime, en particulier les textes métrique en strophes non bibliques destinés à être chantés durant les services religieux.</skos:definition>
    <dcterms:references rdf:resource="http://web.cn.edu/kwheeler/lit_terms_h.html"/>
    <rdf:type rdf:resource="#ReligiousGenre"/>
  </genre:MusicalGenre>
  <genre:EmbeddedWork rdf:about="#afterword">
    <rdfs:isDefinedBy rdf:resource="http://sparql.cwrc.ca/ontologies/genre-ONTOLOGY_DATE"/>
    <rdfs:label xml:lang="en">afterword</rdfs:label>
    <skos:definition xml:lang="en">"A section that appears towards the end of a book, does not form part of the main body, and often concludes or summarizes."  <![CDATA[<a href="#cwrc:4c227091-6bf0-4325-b846-9733fae19e61">(Oxford, 2015)</a>]]></skos:definition>
    <rdfs:label xml:lang="fr">postface</rdfs:label>
    <owl:sameAs rdf:resource="http://dbpedia.org/resource/Postface"/>
    <skos:definition xml:lang="fr">«Une postface est un texte ajouté à la fin d'un livre ou d'un écrit pour en guise de supplément ou de conclusion, généralement pour émettre un commentaire, une explication ou un avertissement. La postface peut être rédigée par l'auteur d'un document ou par une autre personne. La postface est séparée du corps principal de l'ouvrage et est placée dans les pages annexes, c'est-à-dire à la fin du document. La postface, bien qu'elle puise faire office de conclusion, présente des informations qui ne sont pas essentielles à l'intégralité de l'ouvrage, mais qui sont toutefois jugées pertinentes. On oppose la préface, située dans les liminaires, à la postface.»  <![CDATA[<a href="#cwrc:727d97bc-af78-4122-94be-aa78b2e97d5a">(DBpedia, 2017)</a>]]></skos:definition>
    <rdfs:comment xml:lang="en">This term and its description were created from data gathered from DBpedia.</rdfs:comment>
  </genre:EmbeddedWork>
  <genre:OperaGenre rdf:about="#opera">
    <rdf:type rdf:resource="#PerformanceMedium"/>
    <owl:sameAs rdf:resource="http://id.loc.gov/authorities/genreForms/gf2014026976"/>
    <rdfs:label xml:lang="fr">opéra</rdfs:label>
    <skos:definition xml:lang="en">"Dramatic musical performances in which most roles are sung with instrumental accompanyment, usually including arias, recitives, and choruses. Typically, they are intended to be staged with costumes, sets, and dramatic movement."  <![CDATA[<a href="#cwrc:db2f8571-a773-4068-a35f-34262950bb8f">(Getty, 2017)</a>]]></skos:definition>
    <skos:definition xml:lang="fr">«Un opéra est une œuvre destinée à être chantée sur une scène, appartenant à un genre musical vocal du même nom ; l'opéra est l’une des formes du théâtre musical occidental regroupées sous l’appellation d’art lyrique. L'œuvre, chantée par des interprètes possédant un registre vocal déterminé en fonction du rôle et accompagnés par un orchestre, parfois symphonique, parfois de chambre, parfois destiné exclusivement au seul répertoire d'opéra, est constituée d'un livret mis en musique sous forme d'airs, de récitatifs, de chœurs, d'intermèdes souvent précédés d'une ouverture, et parfois agrémentée de ballets. Le genre musical est décliné selon les pays et les époques et recouvre des œuvres d’appellations et de formes différentes. Aujourd’hui, les œuvres sont jouées dans des salles d’opéra spécifiquement affectées ou tout simplement sur des scènes de théâtre ou dans des salles de concerts. Les représentations sont organisées par des institutions du secteur public ou privé, parfois désignées sous le vocable de « maison d'opéra », qui peuvent regrouper les compagnies d’artistes (orchestre, chœur et ballet) et les services administratifs et techniques nécessaires à l’organisation des saisons culturelles. (fr») <![CDATA[<a href="#cwrc:727d97bc-af78-4122-94be-aa78b2e97d5a">(DBpedia, 2017)</a>]]></skos:definition>
    <rdfs:comment xml:lang="en">This term and its description were created from data gathered from the Getty Art &amp; Architecture Thesaurus.</rdfs:comment>
    <owl:sameAs rdf:resource="http://dbpedia.org/resource/Opera"/>
    <rdfs:isDefinedBy rdf:resource="http://sparql.cwrc.ca/ontologies/genre-ONTOLOGY_DATE"/>
    <rdfs:label xml:lang="en">opera</rdfs:label>
  </genre:OperaGenre>
  <genre:ScholarlyGenre rdf:about="#artCriticism">
    <rdfs:comment xml:lang="en">This term and its description were created from data gathered from the Getty Art &amp; Architecture Thesaurus.</rdfs:comment>
    <rdfs:isDefinedBy rdf:resource="http://sparql.cwrc.ca/ontologies/genre-ONTOLOGY_DATE"/>
    <rdfs:label xml:lang="en">art criticism</rdfs:label>
    <rdfs:label xml:lang="fr">critique d'art</rdfs:label>
    <owl:sameAs rdf:resource="http://id.loc.gov/authorities/genreForms/gf2018026112"/>
    <skos:definition xml:lang="fr">"L'étude ou la pratique analytique, descriptive et évualtive d'oeuvres d'art et d'expositions." </skos:definition>
    <skos:definition xml:lang="en">"The study or practice of the analytical description, interpretation, and evaluation of visual art works and exhibitions."  <![CDATA[<a href="#cwrc:db2f8571-a773-4068-a35f-34262950bb8f">(Getty, 2017)</a>]]></skos:definition>
    <owl:sameAs rdf:resource="http://vocab.getty.edu/aat/300168233"/>
  </genre:ScholarlyGenre>
  <genre:InformationalGenre rdf:about="#profileOfAuthor">
    <rdfs:isDefinedBy rdf:resource="http://sparql.cwrc.ca/ontologies/genre-ONTOLOGY_DATE"/>
    <rdfs:label xml:lang="en">profile of author</rdfs:label>
    <skos:definition xml:lang="en">"A summary of relevant details about an author, including, but not limited to: significant works, awards and other accomplishment, professional background or education, biographical information, or personal details."</skos:definition>
  </genre:InformationalGenre>
  <genre:EpistolaryGenre rdf:about="#epistle">
    <skos:definition xml:lang="en">"Literary genre taking the form of letters, usually of a literary, formal, or public nature. Examples are the epistles in the Biblical New Testament."  <![CDATA[<a href="#cwrc:db2f8571-a773-4068-a35f-34262950bb8f">(Getty, 2017)</a>]]></skos:definition>
    <owl:sameAs rdf:resource="http://dbpedia.org/resource/Epistle"/>
    <rdfs:isDefinedBy rdf:resource="http://sparql.cwrc.ca/ontologies/genre-ONTOLOGY_DATE"/>
    <rdfs:label xml:lang="en">epistle</rdfs:label>
    <rdfs:label xml:lang="fr">épître></rdfs:label>
    <skos:definition xml:lang="fr">«Le terme épître, issu du latin epistula, du grec επιστολη (epistolē), désigne une lettre (au sens de correspondance).Il a pris le sens aujourd'hui d'un court traité philosophique ou religieux exposé sous forme épistolaire. Ce sont de courts traités le plus souvent philosophiques. Ce peuvent être aussi des « conversations en l'absence » de l'interlocuteur sur des aspects sociaux ou moraux de l'existence. Au fil du temps, l’épître devient, en littérature, un discours en vers du genre académique ou didactique. Elle prend rapidement le sens d’épigramme nettement moins acerbe que la satire.Le mot « épître » est un nom commun féminin. Le Nouveau Testamen» contient plusieur"  <![CDATA[<a href="#cwrc:727d97bc-af78-4122-94be-aa78b2e97d5a">(DBpedia, 2017)</a>]]></skos:definition>
    <rdfs:comment xml:lang="en">The description for this term is indebted to DBpedia. </rdfs:comment>
  </genre:EpistolaryGenre>
  <genre:FictionalGenre rdf:about="#bisexualFiction">
    <rdfs:isDefinedBy rdf:resource="http://sparql.cwrc.ca/ontologies/genre-ONTOLOGY_DATE"/>
    <rdfs:label xml:lang="en">bisexual fiction</rdfs:label>
    <skos:definition xml:lang="en">Fiction dealing with bisexuality.</skos:definition>
    <owl:sameAs rdf:resource="http://id.loc.gov/authorities/genreForms/gf2018026053"/>
    <skos:definition xml:lang="fr">Fiction abordant le thème de la bisexualité.</skos:definition>
    <rdfs:label xml:lang="fr">fiction bisexuelle</rdfs:label>
    <rdf:type rdf:resource="#LGBTQPlusGenre"/>
  </genre:FictionalGenre>
  <genre:ReferenceWorkGenre rdf:about="#biographicalDictionary">
    <rdfs:isDefinedBy rdf:resource="http://sparql.cwrc.ca/ontologies/genre-ONTOLOGY_DATE"/>
    <rdfs:label xml:lang="en">biographical dictionary</rdfs:label>
    <skos:definition xml:lang="fr">Texte de référence contenant des entrées biographiques à propos de plusieurs personnes, souvent reliées par un thème commun (par exemple, un dictionnaire biographique de femmes) et généralement classées par ordre alphabétique.</skos:definition>
    <skos:definition xml:lang="en">A reference text containing biographical entries on multiple people, often with a common link between them (for example, a biographical dictionary of women), and typically arranged alphabetically.</skos:definition>
    <rdfs:label xml:lang="fr">dictionaire biographique</rdfs:label>
  </genre:ReferenceWorkGenre>
  <genre:ThematicGenre rdf:about="#love">
    <rdfs:label xml:lang="fr">amour</rdfs:label>
    <skos:definition xml:lang="en">Generic modifier for a representation that deals primarily with the subject of love.</skos:definition>
    <rdfs:isDefinedBy rdf:resource="http://sparql.cwrc.ca/ontologies/genre-ONTOLOGY_DATE"/>
    <rdfs:label xml:lang="en">love</rdfs:label>
    <skos:definition xml:lang="fr">Dénomination générique pour les textes dont le sujet principal contient une forme de représentation de l'amour.</skos:definition>
  </genre:ThematicGenre>
  <genre:StillImageMedium rdf:about="#painting">
    <skos:definition xml:lang="en">"Unique works in which images are formed primarily by the direct application of pigments suspended in oil, water, egg yolk, molten wax, or other liquid, arranged in masses of color, onto a generally two-dimensional surface." <![CDATA[<a href="#cwrc:bd595bc4-5991-4c51-98d9-9ab52c416f4f">(Getty, 2021)</a>]]></skos:definition>
    <rdfs:comment xml:lang="en">This term and its description were created from data gathered from the Getty Art &amp; Architecture Thesaurus.</rdfs:comment>
    <owl:sameAs rdf:resource="http://vocab.getty.edu/aat/300033618"/>
    <skos:related rdf:resource="http://vocab.getty.edu/aat/300033618"/>
    <rdfs:isDefinedBy rdf:resource="http://sparql.cwrc.ca/ontologies/genre-ONTOLOGY_DATE"/>
    <rdfs:label xml:lang="en">painting</rdfs:label>
    <rdf:type rdf:resource="#VisualArtMedium"/>
  </genre:StillImageMedium>
  <genre:ReferenceWorkGenre rdf:about="#manual">
    <rdfs:isDefinedBy rdf:resource="http://sparql.cwrc.ca/ontologies/genre-ONTOLOGY_DATE"/>
    <rdfs:label xml:lang="en">manual</rdfs:label>
    <skos:definition xml:lang="en">"Books or treatises, often compendious, containing rules or instructions needed to perform tasks, operations, processes, occupations, arts, or studies, and intended to be used as reference while the task or study is performed."  <![CDATA[<a href="#cwrc:db2f8571-a773-4068-a35f-34262950bb8f">(Getty, 2017)</a>]]></skos:definition>
    <rdfs:label xml:lang="fr">manuel</rdfs:label>
    <skos:altLabel xml:lang="en">companion</skos:altLabel>
    <owl:sameAs rdf:resource="http://vocab.getty.edu/aat/300026395"/>
    <skos:definition xml:lang="fr">Livres ou traités, souvent concis, contenant des règles ou des instructions nécessaires à la réalisation de tâches, d"opérations, de processus, de professions, d'arts ou d'études, et destinés à être utilisés comme référence pendant la réalisation de la tâche ou de l'apprentissage.</skos:definition>
    <rdfs:comment xml:lang="en">The description for this term is indebted to the Getty Art &amp; Architecture Thesaurus.</rdfs:comment>
    <owl:sameAs rdf:resource="http://id.loc.gov/authorities/genreForms/gf2014026109"/>
  </genre:ReferenceWorkGenre>
  <genre:ScholarlyGenre rdf:about="#musicology">
    <skos:definition xml:lang="en">"Writing dealing with the scientific study of music."  <![CDATA[<a href="#cwrc:db2f8571-a773-4068-a35f-34262950bb8f">(Getty, 2017)</a>]]></skos:definition>
    <rdfs:comment xml:lang="en">This term and its description were created from data gathered from DBpedia.</rdfs:comment>
    <rdfs:label xml:lang="fr">musicologie</rdfs:label>
    <skos:definition xml:lang="fr">«La musicologie est une discipline qui étudie les phénomènes en relation avec la musique, dans leur essence (sémiologie musicale, analyse, théorie), leur évolution (histoire des idées et des théories musicales) et dans leur rapport avec l'être humain et la société, domaines plus particulièrement abordés par l'ethnomusicologie et la sociologie de la musique. La seconde catégorie est d'ordre conceptuel, et tend surtout à comparer les statuts de l'œuvre musicale d'hier et de celle d'aujourd'hui, et à analyser toute l'évolution de la musique selon cette optique.»  <![CDATA[<a href="#cwrc:727d97bc-af78-4122-94be-aa78b2e97d5a">(DBpedia, 2017)</a>]]></skos:definition>
    <rdfs:isDefinedBy rdf:resource="http://sparql.cwrc.ca/ontologies/genre-ONTOLOGY_DATE"/>
    <rdfs:label xml:lang="en">musicology</rdfs:label>
    <owl:sameAs rdf:resource="http://vocab.getty.edu/aat/300054240"/>
  </genre:ScholarlyGenre>
  <genre:PoeticGenre rdf:about="#epic">
    <skos:definition xml:lang="fr">Provenant du nom "épopoée", le genre épique désigne aujourd'hui les formes artistiques et littéraires (prose, poésie, théâtre, fillms, et autres) dans lesquelles l'histoire a pour thèmes principaux la grandeur et l'héroïsme.</skos:definition>
    <owl:sameAs rdf:resource="http://vocab.getty.edu/aat/300404209"/>
    <skos:definition xml:lang="en">"Meaning extended from "epic poetry," in modern usage refers to literary art forms, such as prose, poetry, plays, films, and other works where the story has a theme of grandeur and heroism."  <![CDATA[<a href="#cwrc:db2f8571-a773-4068-a35f-34262950bb8f">(Getty, 2017)</a>]]></skos:definition>
    <rdfs:label xml:lang="fr">épique</rdfs:label>
    <owl:sameAs rdf:resource="http://id.loc.gov/authorities/genreForms/gf2014026310"/>
    <rdfs:comment xml:lang="en">The description for this term is indebted to the Getty Art &amp; Architecture Thesaurus.</rdfs:comment>
    <rdfs:isDefinedBy rdf:resource="http://sparql.cwrc.ca/ontologies/genre-ONTOLOGY_DATE"/>
    <rdfs:label xml:lang="en">epic</rdfs:label>
  </genre:PoeticGenre>
  <genre:PoeticGenre rdf:about="#georgic">
    <rdfs:isDefinedBy rdf:resource="http://sparql.cwrc.ca/ontologies/genre-ONTOLOGY_DATE"/>
    <rdfs:label xml:lang="en">georgic</rdfs:label>
    <rdfs:label xml:lang="fr">géorgique</rdfs:label>
    <dcterms:references rdf:resource="http://www.oxfordreference.com/view/10.1093/acref/9780199208272.001.0001/acref-9780199208272-e-496?rskey=qEr6Vu%26result=491"/>
    <rdfs:comment xml:lang="en">This term and its description were created from data gathered from the Oxford Dictionary of Literary Terms, 4th ed.</rdfs:comment>
    <skos:definition xml:lang="fr">Poésie à propos de la vie rurale qui donne des conseils pratiques au sujet de l'agriculture. Contrairement à la poésie pastorale, elle ne dépeint pas la campagne comme une lieu d'évasion idyllique, mais se concentre plutôt sur la nécessité du travail extérieur.</skos:definition>
    <skos:definition xml:lang="en">"Poetry about rural life that gives practical advice on the subject of agriculture. Unlike pastoral poetry, it does not portray the countryside as an idyllic escape, but rather focuses on the necessity of outdoor labour."  <![CDATA[<a href="#cwrc:4c227091-6bf0-4325-b846-9733fae19e61">(Oxford, 2015)</a>]]></skos:definition>
  </genre:PoeticGenre>
  <genre:PoeticGenre rdf:about="#anagram">
    <rdfs:label xml:lang="fr">anagramme</rdfs:label>
    <owl:sameAs rdf:resource="http://vocab.getty.edu/aat/300202515"/>
    <rdfs:isDefinedBy rdf:resource="http://sparql.cwrc.ca/ontologies/genre-ONTOLOGY_DATE"/>
    <rdfs:label xml:lang="en">anagram</rdfs:label>
    <skos:definition xml:lang="en">"Anagrammatic poetry is poetry with the constrained form that either each line or each verse is an anagram of all other lines or verses in the poem. A poet that specializes in anagrams is an anagrammarian. Writing anagrammatic poetry is a form of a constrained writing similar to writing pangrams or long alliterations."  <![CDATA[<a href="#cwrc:727d97bc-af78-4122-94be-aa78b2e97d5a">(DBpedia, 2017)</a>]]></skos:definition>
    <rdfs:comment xml:lang="en">This term and its description were created from data gathered from DBpedia.</rdfs:comment>
    <skos:definition xml:lang="fr">«Une anagramme (le mot est féminin) – du grec ανά, « en arrière », et γράμμα, « lettre », anagramma : « renversement de lettres » – est une construction fondée sur une figure de style qui inverse ou permute les lettres d'un mot ou d'un groupe de mots pour en extraire un sens ou un mot nouveau. Jeu littéraire, l'anagramme peut aussi avoir une valeur ésotérique. Elle a fait l'objet de l'attention autant des linguistes – à l'instar de Ferdinand de Saussure – que des psychanalystes et des poètes contemporains.»  <![CDATA[<a href="#cwrc:727d97bc-af78-4122-94be-aa78b2e97d5a">(DBpedia, 2017)</a>]]></skos:definition>
    <owl:sameAs rdf:resource="http://id.loc.gov/authorities/genreForms/gf2014026043"/>
  </genre:PoeticGenre>
  <genre:AutobiographicalGenre rdf:about="#diary">
    <rdfs:isDefinedBy rdf:resource="http://sparql.cwrc.ca/ontologies/genre-ONTOLOGY_DATE"/>
    <rdfs:label xml:lang="en">diary</rdfs:label>
    <skos:definition xml:lang="fr">"Désigne les livres contenant les comptes rendus journaliers et personnels des expériences, états d'esprit et observations de l'auteur. Utiliser journaux (comptes rendus)" lorsqu'on se réfère au compte rendus d'évènements et de transactions d'un individu ou d'une organisation.  " </skos:definition>
    <rdfs:label xml:lang="fr">journal intime</rdfs:label>
    <rdfs:comment xml:lang="en">The description for this term is indebted to the Getty Art &amp; Architecture Thesaurus.</rdfs:comment>
    <skos:definition xml:lang="en">"Refers to books containing the daily, personal accounts of the writer's own experiences, attitudes, and observations. Use "journals (accounts)" when referring to an individual's or an organization's account of occurrences or transactions."  <![CDATA[<a href="#cwrc:db2f8571-a773-4068-a35f-34262950bb8f">(Getty, 2017)</a>]]></skos:definition>
    <owl:sameAs rdf:resource="http://vocab.getty.edu/aat/300027112"/>
    <owl:sameAs rdf:resource="http://id.loc.gov/authorities/genreForms/gf2014026085"/>
  </genre:AutobiographicalGenre>
  <genre:InformationalGenre rdf:about="#obituary">
    <owl:sameAs rdf:resource="http://id.loc.gov/authorities/genreForms/gf2014026134"/>
    <rdfs:label xml:lang="fr">élégie</rdfs:label>
    <skos:definition xml:lang="en">"An obituary (obit for short) is a news article that reports the recent death of a person, typically along with an account of the person's life and information about the upcoming funeral."  <![CDATA[<a href="#cwrc:727d97bc-af78-4122-94be-aa78b2e97d5a">(DBpedia, 2018)</a>]]></skos:definition>
    <owl:sameAs rdf:resource="http://dbpedia.org/resource/Obituary"/>
    <skos:definition xml:lang="fr">«L’élégie (en grec ancien ἐλεγεία / elegeía, signifiant « chant de mort ») fut une forme de poème dans l'Antiquité, avant de devenir un genre poétique à partir de la Renaissance. Dans l’Antiquité, était appelé « élégie » tout poème alternant hexamètres et pentamètres en distiques : ce sont les vers élégiaques. De nos jours, l’élégie est considérée comme un genre au sein de la poésie lyrique, en tant que poème de longueur et de forme variables caractérisé par son ton plaintif particulièrement adapté à l’évocation d’un mort ou à l’expression d’une souffrance amoureuse due à un abandon ou à une absence.»  <![CDATA[<a href="#cwrc:727d97bc-af78-4122-94be-aa78b2e97d5a">(DBpedia, 2017)</a>]]></skos:definition>
    <rdfs:comment xml:lang="en">This term and its description were created from data gathered from DBpedia.</rdfs:comment>
    <rdfs:isDefinedBy rdf:resource="http://sparql.cwrc.ca/ontologies/genre-ONTOLOGY_DATE"/>
    <rdfs:label xml:lang="en">obituary</rdfs:label>
  </genre:InformationalGenre>
  <genre:DramaticGenre rdf:about="#masque">
    <dcterms:references rdf:resource="http://web.cn.edu/kwheeler/lit_terms_m.html"/>
    <skos:definition xml:lang="fr">«Le masque (de l'anglais « masque ») est une forme de spectacle de cour qui fit son apparition en Angleterre sous le règne d'Elisabeth I (1558-1603).»  <![CDATA[<a href="#cwrc:727d97bc-af78-4122-94be-aa78b2e97d5a">(DBpedia, 2017)</a>]]></skos:definition>
    <owl:sameAs rdf:resource="http://id.loc.gov/authorities/genreForms/gf2014026428"/>
    <rdf:type rdf:resource="#PerformanceMedium"/>
    <rdfs:comment xml:lang="en">This term and its description were created from data gathered from DBpedia.</rdfs:comment>
    <rdfs:label xml:lang="fr">masque</rdfs:label>
    <skos:definition xml:lang="en">"Not to be confused with a masquerade, a masque is a type of elaborate court entertainment popular in the times of Queen Elizabeth I, King James I, and Charles I--i.e., the early 17th Century after Queen Elizabeth's death. The masque as a performance grew out of medieval plays, but it was more spectacle than drama proper. The content was suitable for amateur actors rather than professional performers. The masques tended to use long speeches and little action. They combined poetic drama, singing, dancing, music, and splendid costumes and settings. The imagery was influential on later poets and poems, such as Andrew Marvell, who makes use of masque-imagery in "Upon Appleton House."  <![CDATA[<a href="cwrc:509015ff-7641-473e-94c5-688e06952bb7">(L. K Wheeler, 2017)</a>]]></skos:definition>
    <rdfs:isDefinedBy rdf:resource="http://sparql.cwrc.ca/ontologies/genre-ONTOLOGY_DATE"/>
    <rdfs:label xml:lang="en">masque</rdfs:label>
  </genre:DramaticGenre>
  <genre:PoeticGenre rdf:about="#poetry">
    <rdfs:isDefinedBy rdf:resource="http://sparql.cwrc.ca/ontologies/genre-ONTOLOGY_DATE"/>
    <rdfs:label xml:lang="en">poetry</rdfs:label>
    <rdfs:comment xml:lang="en">The description for this term is indebted to DBpedia. </rdfs:comment>
    <owl:sameAs rdf:resource="http://dbpedia.org/resource/Poetry"/>
    <owl:sameAs rdf:resource="http://id.loc.gov/authorities/genreForms/gf2014026481"/>
    <skos:definition xml:lang="en">"Poetry is a form of literature that uses aesthetic and rhythmic qualities of language—such as phonaesthetics, sound symbolism, and metre—to evoke meanings in addition to, or in place of, the prosaic ostensible meaning."  <![CDATA[<a href="#cwrc:727d97bc-af78-4122-94be-aa78b2e97d5a">(DBpedia, 2017)</a>]]></skos:definition>
    <rdfs:label xml:lang="fr">poésie</rdfs:label>
    <skos:definition xml:lang="fr">«La poésie est un genre littéraire très ancien aux formes variées, écrites généralement en vers, mais qui admettent aussi la prose, et qui privilégient l'expressivité de la forme, les mots disant plus qu'eux-mêmes par leur choix (sens et sonorités) et leur agencement (rythmes, métrique, figures de style). Sa définition se révèle difficile et varie selon les époques, au point que chaque siècle a pu lui trouver une fonction et une expression différente, à quoi s'ajoute l'approche propre à la personnalité de chaque poète. Le terme « poésie » et ses dérivés viennent du grec ancien ποίησις, et s'écrivait, jusqu'en 1878 poësie (le tréma marquait une disjonction entre les voyelles o et e). ποιεῖν (poiein) signifie « faire, créer » : le poète est donc un créateur, un inventeur de formes expressives, ce que révèlent aussi les termes du Moyen Âge, comme trouvère et troubadour. Le poète, héritier d'une longue tradition orale, privilégie la musicalité et le rythme, d'où, dans la plupart des textes poétiques, le recours à une forme versifiée qui confère de la densité à la langue. Le poète recherche aussi l'expressivité par le poids accordé aux mots comme par l'utilisation des figures de style et au premier chef des images et des figures d'analogie, recherchées pour leur force suggestive. La poésie s'est constamment renouvelée au cours des siècles avec des orientations différentes selon les époques, les civilisations et les individus. On peut par exemple distinguer le poète artiste soucieux d'abord de beauté formelle, le poète « lyrique » qui cultive le « chant de l'âme », le poète prophète, découvreur du monde et « voyant » ou le poète engagé, sans cependant réduire un créateur à une étiquette simplificatrice.»  <![CDATA[<a href="#cwrc:727d97bc-af78-4122-94be-aa78b2e97d5a">(DBpedia, 2017)</a>]]></skos:definition>
  </genre:PoeticGenre>
  <genre:PoliticalGenre rdf:about="#proletarianWriting">
    <rdfs:label xml:lang="fr">littérature prolétarienne</rdfs:label>
    <skos:definition xml:lang="fr">«La littérature prolétarienne est un courant littéraire qu'Henry Poulaille, fondateur du « Groupe des écrivains prolétariens de langue française », connu aussi sous le nom d'« école prolétarienne » (terme que Poulaille désapprouvait), fut le premier à définir et organiser en France dans les années 1930. Est défini comme auteur prolétarien tout auteur : * né de parents ouvriers ou paysans, * autodidacte (ayant quitté tôt l'école pour travailler, ou à la rigueur ayant bénéficié d'une bourse - en général pour devenir instituteur dans le système primaire, « l'école des pauvres », à l'époque où deux systèmes scolaires cohabitaient), * et qui témoigne dans ses écrits des conditions d'existence de sa classe sociale. La définition première précise aussi que l'auteur prolétarien doit continuer de gagner sa vie comme ouvrier ou comme paysan, mais plusieurs auteurs faisant exception à cette règle (à commencer par Poulaille lui-même qui a exercé divers métiers de 13 à 27 ans, mais s'est consacré ensuite à des activités moins « ouvrières » dans l'édition et le journalisme) sont cependant considérés comme auteurs prolétariens, du fait que leurs ouvrages et leur action restent orientés vers la défense du prolétariat et d'une expression littéraire spécifiquement ouvrière.»  <![CDATA[<a href="#cwrc:727d97bc-af78-4122-94be-aa78b2e97d5a">(DBpedia, 2017)</a>]]></skos:definition>
    <skos:definition xml:lang="en">Writing by members of the working-classes or poor, including that by those who consider themselves members of the proletariat, and sometimes also writing produced to raise awareness of poor economic or labour conditions. <![CDATA[<a href="#cwrc:727d97bc-af78-4122-94be-aa78b2e97d5a">(DBpedia, 2019)</a>]]></skos:definition>
    <rdfs:comment xml:lang="en">This term and its description were created from data gathered from DBpedia.</rdfs:comment>
    <skos:closeMatch rdf:resource="http://dbpedia.org/resource/Proletarian_literature"/>
    <rdfs:isDefinedBy rdf:resource="http://sparql.cwrc.ca/ontologies/genre-ONTOLOGY_DATE"/>
    <rdfs:label xml:lang="en">proletarian writing</rdfs:label>
  </genre:PoliticalGenre>
  <genre:ThematicGenre rdf:about="#gothic">
    <skos:definition xml:lang="fr">Fictions romantiques dont l'atmosphère est mystérieuse et angoissante, racontant souvent une histoire d'amour. Le genre a été introduit en Angleterre aux alentours de 1765, mais s'est aussitôt popularisé ailleurs en Europe, atteignant son apogée dans les années 1790. Le genre a connu de nombreux renouvellements au cours des siècles suivants. Le genre est ainsi nommé car les premiers exemples de romans gothiques se déroulaients souvent partiellement au sein de bâtiments médiévaux et de ruines, comme les châteaux ou les monastères.</skos:definition>
    <owl:sameAs rdf:resource="http://id.loc.gov/authorities/genreForms/gf2014026360"/>
    <owl:sameAs rdf:resource="http://vocab.getty.edu/aat/300266777"/>
    <rdfs:comment xml:lang="en">The description for this term is indebted to the Getty Art &amp; Architecture Thesaurus.</rdfs:comment>
    <rdfs:isDefinedBy rdf:resource="http://sparql.cwrc.ca/ontologies/genre-ONTOLOGY_DATE"/>
    <rdfs:label xml:lang="en">gothic</rdfs:label>
    <rdfs:label xml:lang="fr">gothique</rdfs:label>
    <skos:definition xml:lang="en">"Romantic fictions having a prevailing atmosphere of mystery and terror, often combined with a love story. The genre was introduced in England ca. 1765, but soon became popular elsewhere in Europe, reaching its heyday in the 1790s. The genre has undergone frequent revivals in subsequent centuries. It is called "Gothic" because the early examples were often set in part among medieval buildings and ruins, such as castles or monasteries."  <![CDATA[<a href="#cwrc:db2f8571-a773-4068-a35f-34262950bb8f">(Getty, 2017)</a>]]></skos:definition>
  </genre:ThematicGenre>
  <genre:NovelisticGenre rdf:about="#nationalTale">
    <rdfs:comment xml:lang="en">This term and its description were created from data gathered from The Cambridge Companion to the Irish Novel.</rdfs:comment>
    <skos:definition xml:lang="en">"A romantic genre developed in early nineteenth-century, particularly associated with Ireland and Scotland, in which historical content is woven into narratives treating such subjects as the formation or defence of a nation, political conflict with a bearing on nationhood, and national identity or culture."  <![CDATA[<a href="#cwrc:076686ab-eab5-4dcf-a6c0-4949d23feb5c">(Foster, 2006)</a>]]></skos:definition>
    <rdfs:isDefinedBy rdf:resource="http://sparql.cwrc.ca/ontologies/genre-ONTOLOGY_DATE"/>
    <rdfs:label xml:lang="en">national tale</rdfs:label>
    <rdfs:label xml:lang="fr">national tale</rdfs:label>
    <dcterms:references rdf:resource="https://books.google.ca/books?id=b2uvkN2taiQC&amp;printsec=frontcover&amp;redir_esc=y#v=onepage&amp;q&amp;f=false"/>
    <skos:definition xml:lang="fr">Genre romantique développé au début du XIXe siècle, en particulier associé à l'Irlande et à l'Écosse, dans lequel la dimension historique s'inscrit dans des récits autour de sujets tels que la formation ou la défense d'une nation, ou le conflit politique à propos de la nationalité, de l'identité et de la culture nationale .</skos:definition>
    <rdf:type rdf:resource="#HistoricalGenre"/>
  </genre:NovelisticGenre>
  <genre:FictionalGenre rdf:about="#shortStory">
    <skos:definition xml:lang="en">"Relatively brief invented prose narratives."  <![CDATA[<a href="#cwrc:db2f8571-a773-4068-a35f-34262950bb8f">(Getty, 2017)</a>]]></skos:definition>
    <rdfs:isDefinedBy rdf:resource="http://sparql.cwrc.ca/ontologies/genre-ONTOLOGY_DATE"/>
    <rdfs:label xml:lang="en">short story</rdfs:label>
    <rdfs:label xml:lang="fr">nouvelle</rdfs:label>
    <skos:definition xml:lang="fr">«Une nouvelle est un récit habituellement court. Apparu à la fin du Moyen Âge, ce genre littéraire était alors proche du roman et d'inspiration réaliste, se distinguant peu du conte. À partir du XIXe siècle, les auteurs ont progressivement développé d'autres possibilités du genre, en s'appuyant sur la concentration de l'histoire pour renforcer l'effet de celle-ci sur le lecteur, par exemple par un dénouement surprenant. Les thèmes se sont également élargis : la nouvelle est devenue une forme privilégiée de la littérature fantastique, policière, et de science-fiction.»  <![CDATA[<a href="#cwrc:727d97bc-af78-4122-94be-aa78b2e97d5a">(DBpedia, 2017)</a>]]></skos:definition>
    <owl:sameAs rdf:resource="http://dbpedia.org/resource/Short_story"/>
    <rdfs:comment xml:lang="en">This term and its description were created from data gathered from DBpedia.</rdfs:comment>
    <owl:sameAs rdf:resource="http://id.loc.gov/authorities/genreForms/gf2014026542"/>
  </genre:FictionalGenre>
  <genre:AutobiographicalGenre rdf:about="#captivityNarrative">
    <owl:sameAs rdf:resource="http://id.loc.gov/authorities/genreForms/gf2014026056"/>
    <skos:definition xml:lang="en">"Captivity narratives are usually stories of people captured by enemies whom they consider uncivilized, or whose beliefs and customs they oppose. The best-known captivity narratives are those concerning the indigenous peoples of North America. These narratives (and questions about their accuracy) have an enduring place in literature, history, ethnography, and the study of Native peoples. However, captivity narratives have also come to play a major role in the study of contemporary religious movements, thanks to scholars of religion like David G. Bromley and James R. Lewis. In this article, both main types of captivity narratives are considered. Traditionally, historians have made limited use of certain captivity narratives. They have regarded the genre with suspicion because of its ideological underpinnings. As a result of new scholarly approaches, historians with a more certain grasp of Native American cultures are distinguishing between plausible statements of fact and value-laden judgements in order to study the narratives as rare sources from "inside" Native societies. Contemporary historians such as Linda Colley and anthropologists such as Pauline Turner Strong have also found the narratives useful in analyzing how the colonists constructed the "other", as well as what the narratives reveal about the settlers' sense of themselves and their culture, and the experience of crossing the line to another. Colley has studied the long history of English captivity in other cultures, both the Barbary pirate captives who preceded those in North America, and British captives in cultures such as India, after the North American experience. Certain North American captivity narratives involving Native peoples were published from the 18th through the 19th centuries, but they reflected a well-established genre in English literature. There had already been English accounts of captivity by Barbary pirates, or in the Middle East, which established some of the major elements of the form. Following the American experience, additional accounts were written after British people were captured during exploration and settlement in India and East Asia. Other types of captivity narratives, such as those recounted by apostates from religious movements (i.e. "cult survivor" tales), have remained an enduring feature of modern media, and currently appear in books, periodicals, film, and television. The unifying factor in most captivity narratives, whether they stem from geopolitical or religious conflicts, is that the captive portrays the captors' way of life as alien, undesirable, and incompatible with the captive's own (typically dominant) culture. This underscores the utility of captivity narratives in garnering support for social control measures, such as removing Native Americans to "reservations", or stigmatizing participation in religious movements – whether Catholicism in the nineteenth century, or ISKCON in the twentieth. Captivity narratives tend to be culturally chauvinistic, viewing an "alien" culture through the lens of the narrator's preferred culture, thus making (possibly unfair) value judgements like "Puritans good, Indians bad.""  <![CDATA[<a href="#cwrc:727d97bc-af78-4122-94be-aa78b2e97d5a">(DBpedia, 2017)</a>]]></skos:definition>
    <rdfs:isDefinedBy rdf:resource="http://sparql.cwrc.ca/ontologies/genre-ONTOLOGY_DATE"/>
    <rdfs:label xml:lang="en">captivity narrative</rdfs:label>
    <rdfs:comment xml:lang="en">The description for this term is indebted to DBpedia. </rdfs:comment>
    <skos:definition xml:lang="fr">Les récits de captivité sont généralement des histoires de personnes capturées par des ennemis qu'ils considèrent comme incivilisés, ou dont les croyances et les coutumes sont opposées aux leurs. Les récits de captivité les plus connus sont ceux concernant les peuples autochtones d'Amérique du Nord. Ces récits (et la question de leur exactitude) ont depuis longtemps leur place dans la littérature, l'histoire, l'ethnographie et l'étude des peuples autochtones. Cependant, les récits de captivité ont également joué un rôle majeur dans l'étude des mouvements religieux contemporains, grâce à des spécialistes de la religion comme David G. Bromley et James R. Lewis. Dans cet article, les deux principaux types de récits de captivité sont considérés. Dans la tradition, l''utilisation de certains récits de captivité par les historiens est restée limitée. Ils ont considéré le genre avec suspicion en raison de ses fondements idéologiques. À la suite de nouvelles approches académiques, des historiens possédant une meilleure compréhension des cultures amérindiennes distinguent les énoncés plausibles de faits et de jugements chargés valeurs afin d'étudier les récits comme de rares sources provenant de "l'intérieur" des sociétés autochtones. Des historiennes contemporaines telles que Linda Colley et des anthropologues comme Pauline Turner Strong ont également trouvé les récits utiles à l'analyse de la construction de "l'Autre" par les colons, et de ce que les récits révèlent de la perception qu'ils ont d'eux-mêmes, de leur culture et de l'expérience de la rencontre avec l'autre. Colley a étudié la longue histoire de la captivité anglaise dans d'autres cultures, à la fois celle des pirates barbaresques précédents ceux d'Amérique du Nord et celle des captifs britanniques en Inde, après l'expérience nord-américaine. Certains récits de captivité nord-américains impliquant des peuples autochtones furent publiés du 18ème au 19ème siècle, et reflétaient un genre déjà bien établi dans la littérature anglaise. Des récits sur la captivité par les pirates barbaresque ou au Moyen-Orient étaient déjà parus en anglais, établissant certains des principaux éléments du genre. À la suite de l'expérience américaine, des récits supplémentaires avaient été écrits après la capture de Britanniques lors de l'exploration et de l'implantation en Inde et en Asie de l'Est. D'autres types de récits de captivité, tels que ceux racontés par les apostats de mouvements religieux (ou "réctis de survivants de sectes"), sont restés une caractéristique récurrente des média modernes et apparaissent aujourd'hui dans les livres, les périodiques, le cinéma et la télévision. Le dénominateur commun des récits de captivité, qu'ils soient la conséquence de conflits géopolitiques ou religieux, est que le captif dépeint le mode de vie des ravisseurs comme différente, indésirable et incompatible avec la propre culture (généralement dominante) du captit. Cela souligne l'utilité des récits de captivité dans le recueil de mesures en faveur du contrôle social, comme la séclusion d'Amérindiens dans "réserves", ou la participation stigmatisante à des mouvements religieux - que ce soit le catholicisme 19ème, ou le ISKCON au 20ème Les récits de captivité ont tendance à être culturellement chauvins, percevant la culture "étrangère" du point de vue subjectif du narrateur, qui comprend des jugements de valeur (éventuellement injustes) du type les "les Puritains sont bons, les Indiens sont mauvais".</skos:definition>
    <owl:sameAs rdf:resource="http://dbpedia.org/resource/Captivity_narrative"/>
    <rdfs:label xml:lang="fr">récit de captivité</rdfs:label>
  </genre:AutobiographicalGenre>
  <genre:EpistolaryGenre rdf:about="#letter">
    <skos:definition xml:lang="en-gb">"Letters written to a newspaper or magazine to present a position, make a correction, or respond to another story or letter."  <![CDATA[<a href="#cwrc:db2f8571-a773-4068-a35f-34262950bb8f">(Getty, 2017)</a>]]></skos:definition>
    <skos:altLabel xml:lang="en">correspondence</skos:altLabel>
    <rdfs:isDefinedBy rdf:resource="http://sparql.cwrc.ca/ontologies/genre-ONTOLOGY_DATE"/>
    <rdfs:label xml:lang="en">letter</rdfs:label>
    <owl:sameAs rdf:resource="http://vocab.getty.edu/aat/300026879"/>
    <rdfs:comment xml:lang="en">This term and its description were created from data gathered from the Getty Art &amp; Architecture Thesaurus.</rdfs:comment>
    <rdfs:label xml:lang="fr">lettre</rdfs:label>
    <skos:definition xml:lang="fr">Pièces de correspondance qui sont légèrement plus formelles que le mémorandum ou des notes, habituellement écrites sur papier et destinées à être envoyées à un destinataire.</skos:definition>
  </genre:EpistolaryGenre>
  <genre:NovelisticGenre rdf:about="#silverForkNovel">
    <rdfs:comment xml:lang="en">This term and its description were created from data gathered from the Oxford Dictionary of Literary Terms, 4th ed.</rdfs:comment>
    <skos:definition xml:lang="en">"A mocking term for a popular literary genre depicting life in upper-class British society in the 1820s-1840s."  <![CDATA[<a href="#cwrc:4c227091-6bf0-4325-b846-9733fae19e61">(Oxford, 2015)</a>]]></skos:definition>
    <rdfs:isDefinedBy rdf:resource="http://sparql.cwrc.ca/ontologies/genre-ONTOLOGY_DATE"/>
    <rdfs:label xml:lang="en">silver-fork novel</rdfs:label>
    <dcterms:references rdf:resource="http://www.oxfordreference.com/view/10.1093/acref/9780199208272.001.0001/acref-9780199208272-e-1057?rskey=bq3DDS%26result=1061"/>
  </genre:NovelisticGenre>
  <genre:ReferenceWorkGenre rdf:about="#thesaurus">
    <owl:sameAs rdf:resource="http://dbpedia.org/resource/Thesaurus"/>
    <skos:definition xml:lang="en">"A semantic network of unique concepts, including relationships between synonyms, broader and narrower contexts, and other related concepts. Thesauri may be monolingual or multilingual. Thesauri may have the following three relationships between terms: equivalence (synonyms), hierarchical (whole/part), and associative (various types of other relationships)."  <![CDATA[<a href="#cwrc:db2f8571-a773-4068-a35f-34262950bb8f">(Getty, 2017)</a>]]></skos:definition>
    <rdfs:label xml:lang="fr">thesaurus</rdfs:label>
    <rdfs:isDefinedBy rdf:resource="http://sparql.cwrc.ca/ontologies/genre-ONTOLOGY_DATE"/>
    <rdfs:label xml:lang="en">thesaurus</rdfs:label>
    <owl:sameAs rdf:resource="http://id.loc.gov/authorities/genreForms/gf2014026195"/>
    <rdfs:comment xml:lang="en">This term and its description were created from data gathered from the Getty Art &amp; Architecture Thesaurus.</rdfs:comment>
    <skos:definition xml:lang="fr">«Synonyme de Dictionnaire (Dictionarium) : Dictionnarium seu Thesaurus... du XVI° au XVII ° s. À la Renaissance, le thesaurus, venant du grec thesauros, et traduction latine du mot trésor, est un dictionnaire de mots dans les langues anciennes, le mot trésor étant réservé à la langue alors contemporaine, le français. Les premiers thesaurus furent ceux des Estienne, Robert Estienne, imprimeur et libraire du Roi, et Henri Estienne, et voisins des dictionnaires de grec et de latin comme le Dictionnarium Latino-Gallicum (1538), le Dictionnaire françois-latin, (1540). Ce nom a peut-être été emprunté à Hésiode, « La langue est un trésor de mots » car le mot thesaurus existait déjà dans le domaine de l'encyclopédie dans la littérature médiévale (voir Thesaurus:homonymie) ou signifiant comme aujourd’hui un recueil de textes.»  <![CDATA[<a href="#cwrc:727d97bc-af78-4122-94be-aa78b2e97d5a">(DBpedia, 2017)</a>]]></skos:definition>
  </genre:ReferenceWorkGenre>
  <genre:FictionalGenre rdf:about="#utopia">
    <skos:definition xml:lang="en">"An imaginary place or government in which political and social perfection has been reached in the material world as opposed to some spiritual afterlife as discussed in the Christian Bible or the Elysian fields of The Odyssey. The citizens of such utopias are typically universally clean, virtuous, healthy, and happy, or at least those who are criminals are always captured and appropriately punished. A utopian society is one that has cured all social ills. See discussion under Utopian literature, below. Contrast with dystopia. UTOPIAN"  <![CDATA[<a href="cwrc:509015ff-7641-473e-94c5-688e06952bb7">(L. K Wheeler, 2017)</a>]]></skos:definition>
    <owl:sameAs rdf:resource="http://id.loc.gov/authorities/genreForms/gf2014026583"/>
    <rdfs:comment xml:lang="en">This term and its description were created from data gathered from DBpedia.</rdfs:comment>
    <dcterms:references rdf:resource="http://web.cn.edu/kwheeler/lit_terms_u.html"/>
    <skos:definition xml:lang="fr">«L’utopie (mot forgé par l'écrivain anglais Thomas More, du grec οὐ-τόπος « en aucun lieu ») est une représentation d'une réalité idéale et sans défaut. C'est un genre d'apologue qui se traduit, dans les écrits, par un régime politique idéal (qui gouvernerait parfaitement les hommes), une société parfaite (sans injustice par exemple, comme la Callipolis de Platon ou la découverte de l'Eldorado dans Candide) ou encore une communauté d'individus vivant heureux et en harmonie (l'abbaye de Thélème dans Gargantua de Rabelais en 1534), souvent écrites pour dénoncer les injustices et dérives de leurs temps.»  <![CDATA[<a href="#cwrc:727d97bc-af78-4122-94be-aa78b2e97d5a">(DBpedia, 2017)</a>]]></skos:definition>
    <rdfs:isDefinedBy rdf:resource="http://sparql.cwrc.ca/ontologies/genre-ONTOLOGY_DATE"/>
    <rdfs:label xml:lang="en">utopia</rdfs:label>
    <rdfs:label xml:lang="fr">utopie</rdfs:label>
  </genre:FictionalGenre>
  <genre:ScriptForm rdf:about="#filmScript">
    <skos:definition xml:lang="en">"Written forms of stories prepared for motion picture productions, including description of characters, details of scenes and settings, dialogue, and stage directions." <![CDATA[<a href="#cwrc:bd595bc4-5991-4c51-98d9-9ab52c416f4f">(Getty, 2021)</a>]]></skos:definition>
    <rdfs:comment xml:lang="en">This term and its description were created from data gathered from the Getty Art &amp; Architecture Thesaurus.</rdfs:comment>
    <owl:sameAs rdf:resource="http://vocab.getty.edu/aat/300026491"/>
    <rdfs:isDefinedBy rdf:resource="http://sparql.cwrc.ca/ontologies/genre-ONTOLOGY_DATE"/>
    <rdfs:label xml:lang="en">film script</rdfs:label>
  </genre:ScriptForm>
  <genre:PoliticalGenre rdf:about="#suffragist">
    <skos:definition xml:lang="en">"Suffrage, political franchise, or simply franchise is the right to vote in public, political elections (although the term is sometimes used for any right to vote). The right to run for office is sometimes called candidate eligibility, and the combination of both rights is sometimes called full suffrage. In many languages, the right to vote is called the active right to vote and the right to run for office is called the passive right to vote. In English, these are sometimes called active suffrage and passive suffrage. Suffrage is often conceived in terms of elections for representatives. However, suffrage applies equally to referenda and initiatives. Suffrage describes not only the legal right to vote, but also the practical question of whether a question will be put to a vote. The utility of suffrage is reduced when important questions are decided unilaterally by elected or non-elected representatives. In most democracies, eligible voters can vote in elections of representatives. Voting on issues by referendum may also be available. For example, in Switzerland this is permitted at all levels of government. In the United States, some states such as California and Washington have exercised their shared sovereignty to offer citizens the opportunity to write, propose, and vote on referendums and initiatives; other states have not. The United States federal government does not offer any initiatives at all. Suffrage is granted to qualifying citizens once they have reached the voting age. What constitutes a qualifying citizen depends on the government's decision, but most democracies no longer extend differing rights to vote on the basis of sex or race. Resident non-citizens can vote in some countries, which may be restricted to citizens of closely linked countries (e.g., Commonwealth citizens and European Union citizens)." <![CDATA[<a href="#cwrc:727d97bc-af78-4122-94be-aa78b2e97d5a">(DBpedia, 2019)</a>]]></skos:definition>
    <rdfs:isDefinedBy rdf:resource="http://sparql.cwrc.ca/ontologies/genre-ONTOLOGY_DATE"/>
    <rdfs:label xml:lang="en">suffragist</rdfs:label>
  </genre:PoliticalGenre>
  <genre:PerformanceMedium rdf:about="#ballet">
    <rdfs:label xml:lang="fr">ballet</rdfs:label>
    <skos:definition xml:lang="fr">«Le ballet est un genre dramatique dont l'action est figurée par des pantomimes et des danses. Ses origines remontent à la Renaissance italienne (XVe siècle). Primitivement développé à la cour d'Italie, le ballet a reçu ses lettres de noblesse en France, puis en Russie, en tant que danse-spectacle. Au XVIIe siècle, le développement important qu'a connu le ballet à la cour de Louis XIV explique l'origine française de la plupart des termes de vocabulaire de la danse. Comme l'opéra, il peut être organisé de deux manières »: <![CDATA[<a href="#cwrc:727d97bc-af78-4122-94be-aa78b2e97d5a">(DBpedia, 2017)</a>]]></skos:definition>
    <rdfs:comment xml:lang="en">This term and its description were created from data gathered from the Getty Art &amp; Architecture Thesaurus.</rdfs:comment>
    <skos:definition xml:lang="en">"Dramatic entertainments consisting of dance and mime performed to music. Ballets are characterized by stylized poses and steps that are combined with light and flowing figures and movements, such as leaps and turns; often combined with music, scenery, costume, and sometimes pantomime or speech to convey a story, theme, or atmosphere to the audience."  <![CDATA[<a href="#cwrc:db2f8571-a773-4068-a35f-34262950bb8f">(Getty, 2017)</a>]]></skos:definition>
    <rdfs:isDefinedBy rdf:resource="http://sparql.cwrc.ca/ontologies/genre-ONTOLOGY_DATE"/>
    <rdfs:label xml:lang="en">ballet</rdfs:label>
    <skos:related rdf:resource="http://vocab.getty.edu/aat/300389780"/>
    <owl:sameAs rdf:resource="http://vocab.getty.edu/aat/300389780"/>
  </genre:PerformanceMedium>
  <genre:ScholarlyGenre rdf:about="#scientificWriting">
    <skos:altLabel xml:lang="en">science</skos:altLabel>
    <skos:definition xml:lang="en">Writing relating to scientific research, often reporting the findings of a particular scientific study.</skos:definition>
    <rdfs:label xml:lang="fr">écrits scientifiques</rdfs:label>
    <rdfs:isDefinedBy rdf:resource="http://sparql.cwrc.ca/ontologies/genre-ONTOLOGY_DATE"/>
    <rdfs:label xml:lang="en">scientific writing</rdfs:label>
    <skos:definition xml:lang="fr">Travaux écrits en lien avec la recherche scientifique, qui livrent généralement des comptes rendus de découvertes faites dans le cadre d'une étude scientifique spécifique.</skos:definition>
  </genre:ScholarlyGenre>
  <genre:FictionalGenre rdf:about="#mystery">
    <skos:definition xml:lang="fr">Dans le roman à énigme, le détective cherche le coupable au sein d’un groupe de suspects tour à tour présenté par l’auteur. D’un interrogatoire l’autre, on suit donc le détective dans sa quête de vérité, pour le voir aboutir généralement au fameux dévoilement de l’affaire, le plus souvent dans une scène finale où il expose les clés de son raisonnement. Il devient très vite admis que l’auteur s’amuse avec son lecteur, lui donnant la possibilité de jouer lui aussi les détectives et de parvenir aux mêmes conclusions que son héros.</skos:definition>
    <dcterms:references rdf:resource="http://web.cn.edu/kwheeler/lit_terms_m.html"/>
    <rdfs:label xml:lang="fr">roman à énigme</rdfs:label>
    <rdfs:isDefinedBy rdf:resource="http://sparql.cwrc.ca/ontologies/genre-ONTOLOGY_DATE"/>
    <rdfs:label xml:lang="en">mystery</rdfs:label>
    <skos:definition xml:lang="en">"A novel focused on suspense and solving a mystery--especially a murder, theft, kidnapping, or some other crime. The protagonist faces inexplicable events, threats, assaults, and unknown forces or antagonists. Conventionally, the hero is a keenly observant individual (such as Sherlock Holmes) and the police are depicted as incompetent or incapable of solving the crime by themselves. Many of the works of Sir Arthur Conan Doyle, Edgar Allan Poe, and Agatha Christie are mystery novels."  <![CDATA[<a href="cwrc:509015ff-7641-473e-94c5-688e06952bb7">(L. K Wheeler, 2017)</a>]]></skos:definition>
    <owl:sameAs rdf:resource="http://id.loc.gov/authorities/genreForms/gf2014026280"/>
    <rdfs:comment xml:lang="en">This term and its description were created from data gathered from polars.org.</rdfs:comment>
  </genre:FictionalGenre>
  <genre:ComedicGenre rdf:about="#burletta">
    <rdfs:label xml:lang="fr">burletta</rdfs:label>
    <rdfs:isDefinedBy rdf:resource="http://sparql.cwrc.ca/ontologies/genre-ONTOLOGY_DATE"/>
    <rdfs:label xml:lang="en">burletta</rdfs:label>
    <skos:definition xml:lang="en">"A form of comic drama set to music, first popularized in the 1700s."  <![CDATA[<a href="#cwrc:2f09376c-f784-4a46-9f04-5a21aa311f27">(Penguin, 1999)</a>]]></skos:definition>
    <skos:definition xml:lang="fr">«Burletta (« petite plaisanterie » en italien, parfois aussi burla ou burlettina), est un terme musical pour qualifier un bref opéra comique italien (ou, plus tard anglais). Le terme est utilisé au XVIIIe siècle pour désigner les intermezzos comiques entre les actes d'un opéra seria mais est parfois donné à des œuvres de plus grande envergure. La serva padrona de Pergolese est appelée burletta lors de sa création à Londres en 1750.»  <![CDATA[<a href="#cwrc:727d97bc-af78-4122-94be-aa78b2e97d5a">(DBpedia, 2017)</a>]]></skos:definition>
    <owl:sameAs rdf:resource="http://dbpedia.org/resource/Burletta"/>
  </genre:ComedicGenre>
  <genre:ThematicGenre rdf:about="#western">
    <skos:definition xml:lang="en">"Western is a genre of fiction set primarily in the latter half of the 19th and early 20th century in the western United States. It has expanded to include narratives with different settings (such as Space Westerns) that nonetheless share themes associated with the Western. The genre often involves narratives or conflicts associated with the expansion of settler culture and conflicts among settlers or with Indigenous peoples."<![CDATA[<a href="#cwrc:50024824-8252-4a95-b62e-797911907f20">(DBpedia, 2021)</a>]]></skos:definition>
    <rdfs:comment xml:lang="en">The description for this term is indebted to DBpedia.</rdfs:comment>
    <skos:closeMatch rdf:resource="https://dbpedia.org/page/Western_(genre)"/>
    <owl:sameAs rdf:resource="http://id.loc.gov/authorities/genreForms/gf2014026594"/>
    <rdfs:isDefinedBy rdf:resource="http://sparql.cwrc.ca/ontologies/genre-ONTOLOGY_DATE"/>
    <rdfs:label xml:lang="en">western</rdfs:label>
  </genre:ThematicGenre>
  <genre:NovelisticGenre rdf:about="#sensationNovel">
    <skos:definition xml:lang="fr">«Le roman à sensation est un genre littéraire né dans la deuxième moitié du XIXe siècle en Grande-Bretagne. Ce genre littéraire est une évolution des romans mélodramatiques, qui utilisaient un ensemble de personnages stéréotypés, et des romans Newgate, qui avaient pour thème principal la vie de célèbres criminels. East Lynne de Ellen Wood's, paru en 1861, fut le premier roman à être étiqueté comme roman à sensation par la critique. Le courant comprend trois auteurs majeurs : Ellen Woods, Wilkie Collins (La Femme en blanc, 1859; La Pierre de lune, 1868) et Mary Elizabeth Braddon (Le secret de Lady Audley, 1862). Les romans à sensation avaient pour thèmes des sujets choquants comme l'adultère, le vol, l'enlèvement, la bigamie, la fabrication de fausse monnaie, la séduction et le meurtre. Le genre se distinguait des autres mouvements de l'époque, comme le mouvement Gothique, par l'utilisation de ces thèmes dans un contexte domestique, voire familial, allant ainsi à l'encontre de l'idée largement répandue à l'époque victorienne que les événements sensationnels étaient totalement étrangers à la vie confortable des classes moyennes qui composaient la plus grande partie du lectorat de l'époque. William S. Gilbert fit une satire du genre en 1871 avec son opéra comique A Sensation Novel.»  <![CDATA[<a href="#cwrc:727d97bc-af78-4122-94be-aa78b2e97d5a">(DBpedia, 2017)</a>]]></skos:definition>
    <rdfs:comment xml:lang="en">The description for this term is indebted to DBpedia. </rdfs:comment>
    <rdfs:isDefinedBy rdf:resource="http://sparql.cwrc.ca/ontologies/genre-ONTOLOGY_DATE"/>
    <rdfs:label xml:lang="en">sensation novel</rdfs:label>
    <skos:definition xml:lang="en">"The sensation novel was a literary genre of fiction popular in Great Britain in the 1860s and 1870s, following on from earlier melodramatic novels and the Newgate novels, which focused on tales woven around criminal biographies. It also drew on the gothic and romantic genres of fiction. The sensation novel's appearance notably follows the Industrial Revolution, which made books available on a mass scale for people of all social standings and increased the sensation novel's popularity. Sensation novels used both modes of romance and realism to the extreme where in the past they had traditionally been contradictory modes of literature. The sensation novelists commonly wrote stories that were allegorical and abstract; the abstract nature of the stories gave the authors room to explore scenarios that wrestled with the social anxieties of the Victorian Era. The loss of identity is seen in many sensation fiction stories because this was a common social anxiety; in Britain, there was an increased use in record keeping and therefore people questioned the meaning and permanence of identity. The social anxiety regarding identity is reflected in stories, such as, The Woman in White and Lady Audley's Secret. The genre of sensation fiction was established by the publications of the following novels The Woman in White by Wilkie Collins in 1859; East Lynne by Ellen Wood in 1861; Lady Audley's Secret by Mary Elizabeth Braddon in 1862. Perhaps the earliest use of the term, sensation fiction, as a name for such novels appears in the 1861 edition of the Saunders, Otley, &amp; co.'s Literary Budget. The neo-Victorian novel of New Zealand author Eleanor Catton, The Luminaries, which won the 2013 Man Booker Prize, has been described as being heavily based on sensation literature, with its plot devices of "suspect wills and forged documents, secret marriages, illegitimacy and opium"  <![CDATA[<a href="#cwrc:727d97bc-af78-4122-94be-aa78b2e97d5a">(DBpedia, 2017)</a>]]></skos:definition>
    <rdf:type rdf:resource="#MysteryGenre"/>
    <owl:sameAs rdf:resource="http://dbpedia.org/resource/Sensation_novel"/>
  </genre:NovelisticGenre>
  <genre:FictionalGenre rdf:about="#sketch">
    <rdfs:isDefinedBy rdf:resource="http://sparql.cwrc.ca/ontologies/genre-ONTOLOGY_DATE"/>
    <rdfs:label xml:lang="en">sketch</rdfs:label>
    <rdfs:label xml:lang="fr">croquis</rdfs:label>
    <skos:definition xml:lang="en">A short, often but not necessarily humorous depiction of a person, incident, or a subject, by analogy with an artistic sketch often cursory and suggestive rather than fully fleshed out. Subjects may be identifiable or fictional. See @@https://en.wikipedia.org/wiki/Sketch_story@@.</skos:definition>
    <rdfs:seeAlso rdf:resource="http://dbpedia.org/resource/Sketch_story"/>
    <skos:definition xml:lang="fr"/>
  </genre:FictionalGenre>
  <genre:ReligiousGenre rdf:about="#passionPlay">
    <owl:sameAs rdf:resource="http://id.loc.gov/authorities/genreForms/gf2014026472"/>
    <skos:definition xml:lang="en">"The Passion Play or Easter pageant is a dramatic presentation depicting the Passion of Jesus Christ: his trial, suffering and death. It is a traditional part of Lent in several Christian denominations, particularly in Catholic tradition." <![CDATA[<a href="#cwrc:727d97bc-af78-4122-94be-aa78b2e97d5a">(DBpedia, 2019)</a>]]></skos:definition>
    <rdfs:isDefinedBy rdf:resource="http://sparql.cwrc.ca/ontologies/genre-ONTOLOGY_DATE"/>
    <rdfs:label xml:lang="en">passion play</rdfs:label>
    <rdf:type rdf:resource="#PerformanceMedium"/>
  </genre:ReligiousGenre>
  <genre:ReligiousGenre rdf:about="#catechism">
    <skos:definition xml:lang="fr">«Dans la religion chrétienne, le catéchisme désigne l'instruction des doctrines de la foi chrétienne, particulièrement destinée aux enfants. Il prend souvent la forme d'une exposé officiel des articles de la foi, servant d'outil de base pour la catéchèse, qui est l'ensemble des actions destinées à éduquer des enfants, des jeunes et des adultes à la doctrine chrétienne. La catéchèse est une des composantes de la mission évangélique du christianisme.»  <![CDATA[<a href="#cwrc:727d97bc-af78-4122-94be-aa78b2e97d5a">(DBpedia, 2017)</a>]]></skos:definition>
    <owl:sameAs rdf:resource="http://vocab.getty.edu/aat/300026460"/>
    <skos:definition xml:lang="en">"A catechism (/ˈkætəˌkizəm/; from Greek: κατηχέω, to teach orally), is a summary or exposition of doctrine and served as a learning introduction to the Sacraments traditionally used in catechesis, or Christian religious teaching of children and adult converts. Catechisms are doctrinal manuals - often in the form of questions followed by answers to be memorised - a format in non-religious or secular contexts as well. The term catechumen refers to the designated recipient of the catechetical work or instruction. In the Catholic Church, catachumens were usually placed separately during Holy Mass from those who received the Sacrament of Baptism. Early catecheticals emerged from Graeco-Roman mystery religions, especially the late cult of Mithras meant to educate their members into the secretive teachings, which competed with the Christian Church as an underground religion in the 1st to 4th centuries CE and allegedly shared its many ritual practices. Today, they are characteristic of Western Christianity but are also present in Eastern Christianity."  <![CDATA[<a href="#cwrc:727d97bc-af78-4122-94be-aa78b2e97d5a">(DBpedia, 2017)</a>]]></skos:definition>
    <rdfs:label xml:lang="fr">catéchisme</rdfs:label>
    <rdfs:isDefinedBy rdf:resource="http://sparql.cwrc.ca/ontologies/genre-ONTOLOGY_DATE"/>
    <rdfs:label xml:lang="en">catechism</rdfs:label>
    <rdfs:comment xml:lang="en">The description for this term is indebted to DBpedia. </rdfs:comment>
    <owl:sameAs rdf:resource="http://id.loc.gov/authorities/genreForms/gf2015026029"/>
    <rdfs:comment xml:lang="fr">La description de ce terme est basée sur celle de DBPedia.</rdfs:comment>
    <rdf:type rdf:resource="#DidacticGenre"/>
  </genre:ReligiousGenre>
  <genre:StandaloneWork rdf:about="#book">
    <rdfs:isDefinedBy rdf:resource="http://sparql.cwrc.ca/ontologies/genre-ONTOLOGY_DATE"/>
    <rdfs:label xml:lang="en">book</rdfs:label>
    <skos:definition xml:lang="en">The book, often considered synonymous with the codex, can be understood variously as an object, a form of content, an idea, or an interface <![CDATA[<a href="#cwrc:c6ec4483-c3b8-42a2-81b2-4a1c2727d12e">(Borsuk, 2018)</a>]]>. Commonly understood as a medium <![CDATA[<a href="#cwrc:4b7ec4be-c188-463c-9159-6ead04cc02eb">(Wikipedia, 2021)</a>]]>, the book is characterized by pages of writing that are bound or grouped together and intended to be read as a unified work. The content and interfaces of mainstream e-books are overdetermined by both the materiality and idea of the book.</skos:definition>
    <rdfs:comment xml:lang="en">The description for this term is indebted to Wikipedia and Aramanth Borsuk of The University of Washington. </rdfs:comment>
  </genre:StandaloneWork>
  <genre:ThematicGenre rdf:about="#exploration">
    <rdfs:isDefinedBy rdf:resource="http://sparql.cwrc.ca/ontologies/genre-ONTOLOGY_DATE"/>
    <rdfs:label xml:lang="en">exploration</rdfs:label>
    <skos:definition xml:lang="en">Indicates works wherein a subject interacts with ostensibly new flora, fauna, peoples, and places. Such narratives often reflect colonialist and imperialist mentalities and stereotypes.</skos:definition>
    <skos:broader rdf:resource="#travel"/>
  </genre:ThematicGenre>
  <genre:PoliticalGenre rdf:about="#propaganda">
    <rdfs:label xml:lang="fr">propagande</rdfs:label>
    <owl:sameAs rdf:resource="http://vocab.getty.edu/aat/300055539"/>
    <skos:definition xml:lang="en">"Ideas, facts, or allegations spread deliberately to support one cause or individual or to damage another."  <![CDATA[<a href="#cwrc:db2f8571-a773-4068-a35f-34262950bb8f">(Getty, 2017)</a>]]></skos:definition>
    <rdfs:comment xml:lang="en">The description for this term is indebted to the Getty Art &amp; Architecture Thesaurus.</rdfs:comment>
    <rdfs:isDefinedBy rdf:resource="http://sparql.cwrc.ca/ontologies/genre-ONTOLOGY_DATE"/>
    <rdfs:label xml:lang="en">propaganda</rdfs:label>
    <skos:definition xml:lang="fr">«La propagande est un concept désignant un ensemble de techniques de persuasion, mis en œuvre pour propager avec tous les moyens disponibles une idée, une opinion, une idéologie ou une doctrine et stimuler l'adoption de comportements prédéterminés au sein d'un public-cible. Ces techniques sont exercées sur une population afin de l'influencer, voire de l'endoctriner[réf. insuffisante]. La propagande se distingue de la publicité, laquelle vise la promotion de produits commerciaux. Néanmoins, la publicité utilise des techniques similaires à celles utilisées par la propagande . Nonobstant la similarité de certaines de leurs caractéristiques, les liens entre propagande et publicité sont largement discutés. La propagande est étudiée en milieu universitaire à partir du début du XXe siècle, principalement en histoire, mais aussi en psychologie (particulièrement en psychologie sociale) et en communication (notamment concernant les médias de masse).»  <![CDATA[<a href="#cwrc:727d97bc-af78-4122-94be-aa78b2e97d5a">(DBpedia, 2017)</a>]]></skos:definition>
  </genre:PoliticalGenre>
  <genre:DramaticGenre rdf:about="#radioDrama">
    <owl:sameAs rdf:resource="http://dbpedia.org/resource/Radio_drama"/>
    <rdfs:label xml:lang="fr">théâtre radiophonique</rdfs:label>
    <skos:definition xml:lang="en">"Radio drama (or audio drama, audio play, radio play, radio theater, or audio theater) is a dramatized, purely acoustic performance, broadcast on radio. With no visual component, radio drama depends on dialogue, music and sound effects to help the listener imagine the characters and story."  <![CDATA[<a href="#cwrc:727d97bc-af78-4122-94be-aa78b2e97d5a">(DBpedia, 2017)</a>]]></skos:definition>
    <owl:sameAs rdf:resource="http://id.loc.gov/authorities/genreForms/gf2014026499"/>
    <rdfs:isDefinedBy rdf:resource="http://sparql.cwrc.ca/ontologies/genre-ONTOLOGY_DATE"/>
    <rdfs:label xml:lang="en">radio drama</rdfs:label>
    <rdfs:comment xml:lang="en">This term and its description were created from data gathered from DBpedia.</rdfs:comment>
    <skos:definition xml:lang="fr">«Le théâtre radiophonique ou radio-théâtre est une adaptation du médium théâtral au médium radiophonique.À partir du début des années 1950, le théâtre radiophonique subit la concurrence de la dramatique radio, puisque le premier terme disparait.»  <![CDATA[<a href="#cwrc:727d97bc-af78-4122-94be-aa78b2e97d5a">(DBpedia, 2017)</a>]]></skos:definition>
  </genre:DramaticGenre>
  <genre:DramaticGenre rdf:about="#agitprop">
    <rdfs:comment xml:lang="en">The description for this term is indebted to the Getty Art &amp; Architecture Thesaurus.</rdfs:comment>
    <owl:sameAs rdf:resource="http://vocab.getty.edu/aat/300055540"/>
    <skos:definition xml:lang="fr">"Le terme est dérivé de "propagande d'agitation" et incite à l'action politique. En référence à l'art visuel, il renvoie plus particulièrement au mouvement artistique en essor durant la période qui suit la révolution bolchévique en URSS.  " </skos:definition>
    <rdfs:label xml:lang="fr">agitprop</rdfs:label>
    <skos:definition xml:lang="en">"Derived from agitation propaganda, meaning intended to inspire political action. With reference to visual art, refers to the specific art movement arising in Soviet Russia following the Bolshevik revolution."  <![CDATA[<a href="#cwrc:db2f8571-a773-4068-a35f-34262950bb8f">(Getty, 2017)</a>]]></skos:definition>
    <rdf:type rdf:resource="#PoliticalGenre"/>
    <rdfs:isDefinedBy rdf:resource="http://sparql.cwrc.ca/ontologies/genre-ONTOLOGY_DATE"/>
    <rdfs:label xml:lang="en">agitprop</rdfs:label>
  </genre:DramaticGenre>
  <genre:DramaticGenre rdf:about="#melodrama">
    <dcterms:references rdf:resource="http://web.cn.edu/kwheeler/lit_terms_m.html"/>
    <skos:definition xml:lang="fr">«Le mélodrame, du grec μέλος = chant ou musique + δράμα = action théâtrale, est un genre théâtral dramatique et populaire, qui signifie étymologiquement drame avec musique très populaire au XIXe siècle, se caractérisant par des situations invraisemblables et des personnages manichéens (bons contre méchants).»  <![CDATA[<a href="#cwrc:727d97bc-af78-4122-94be-aa78b2e97d5a">(DBpedia, 2017)</a>]]></skos:definition>
    <rdfs:label xml:lang="fr">mélodrame</rdfs:label>
    <owl:sameAs rdf:resource="http://id.loc.gov/authorities/genreForms/gf2014026432"/>
    <rdfs:isDefinedBy rdf:resource="http://sparql.cwrc.ca/ontologies/genre-ONTOLOGY_DATE"/>
    <rdfs:label xml:lang="en">melodrama</rdfs:label>
    <skos:definition xml:lang="en">"A dramatic form characterized by excessive sentiment, exaggerated emotion, sensational and thrilling action, and an artificially happy ending. Melodramas originally referred to romantic plays featuring music, singing, and dancing, but by the eighteenth century they connoted simplified and coincidental plots, bathos, and happy endings. These melodramatic traits are present in Gothic novels, western stories, popular films, and television crime shows, to name but a few more recent examples."  <![CDATA[<a href="cwrc:509015ff-7641-473e-94c5-688e06952bb7">(L. K Wheeler, 2017)</a>]]></skos:definition>
  </genre:DramaticGenre>
  <genre:EmbeddedWork rdf:about="#epilogue">
    <skos:definition xml:lang="fr">«L’épilogue (du grec επι (epi) : au-dessus et λογος (logos) : discours) est la dernière partie, la conclusion d’une œuvre (discours, roman, film, pièce théâtrale, etc.). Il désigne plus particulièrement au théâtre classique un discours récapitulatif à la fin de la pièce. Il est surtout un hors-d’œuvre, un adieu au public. La Fontaine, croyant avoir fini son œuvre des Fables au VIe livre, prend congé du lecteur dans cet épilogue : Bornons ici cette carrière,Les longs ouvrages me font peur ;Loin d’épuiser une matière,On n’en doit prendre que la fleur»… <![CDATA[<a href="#cwrc:727d97bc-af78-4122-94be-aa78b2e97d5a">(DBpedia, 2017)</a>]]></skos:definition>
    <rdfs:label xml:lang="fr">épilogue</rdfs:label>
    <rdfs:comment xml:lang="en">The description for this term is indebted to Dr. L. Kip Wheeler of Carson-Newman University.</rdfs:comment>
    <owl:sameAs rdf:resource="http://dbpedia.org/resource/Epilogue"/>
    <rdfs:isDefinedBy rdf:resource="http://sparql.cwrc.ca/ontologies/genre-ONTOLOGY_DATE"/>
    <rdfs:label xml:lang="en">epilogue</rdfs:label>
    <owl:sameAs rdf:resource="http://id.loc.gov/authorities/genreForms/gf2018026101"/>
    <skos:definition xml:lang="en">"A conclusion added to a literary work such as a novel, play, or long poem. It is the opposite of a prologue. Often, the epilogue refers to the moral of a fable. Sometimes, it is a speech made by one of the actors at the end of a play asking for the indulgence of the critics and the audience. Shakespeare's A Midsummer Night's Dream contains one of the most famous epilogues. Contrast with prologue. Do not confuse the term with eclogue."  <![CDATA[<a href="cwrc:509015ff-7641-473e-94c5-688e06952bb7">(L. K Wheeler, 2017)</a>]]></skos:definition>
  </genre:EmbeddedWork>
  <genre:RecordForm rdf:about="#bibliographicRecord">
    <skos:definition xml:lang="en">"An entry in a bibliographic index (or a library catalog) which represents and describes a specific resource." <![CDATA[<a href="#cwrc:50024824-8252-4a95-b62e-797911907f20">(DBpedia, 2021)</a>]]></skos:definition>
    <rdfs:comment xml:lang="en">The description for this term is indebted to DBpedia.</rdfs:comment>
    <owl:sameAs rdf:resource="https://dbpedia.org/page/Bibliographic_record"/>
    <rdfs:isDefinedBy rdf:resource="http://sparql.cwrc.ca/ontologies/genre-ONTOLOGY_DATE"/>
    <rdfs:label xml:lang="en">bibliographic record</rdfs:label>
  </genre:RecordForm>
  <genre:ReligiousGenre rdf:about="#scripture">
    <skos:definition xml:lang="en">"Religious texts (also known as scripture, or scriptures, from the Latin scriptura, meaning "a writing" ) are the texts which various religious traditions consider to be sacred, or central to their religious tradition. Religious texts may be used to evoke a deeper connection with the divine, convey spiritual truths, promote mystical experience, foster communal identity, and to guide individual and communal spiritual practice. Many religions and spiritual movements believe that their sacred texts are divinely or supernaturally revealed or inspired. The monotheistic faiths view their texts as the "Word of God" and divine revelation." <![CDATA[<a href="#cwrc:727d97bc-af78-4122-94be-aa78b2e97d5a">(DBpedia, 2019)</a>]]></skos:definition>
    <rdfs:isDefinedBy rdf:resource="http://sparql.cwrc.ca/ontologies/genre-ONTOLOGY_DATE"/>
    <rdfs:label xml:lang="en">scripture</rdfs:label>
    <rdf:type rdf:resource="#LiteraryGenre"/>
  </genre:ReligiousGenre>
  <genre:DramaticGenre rdf:about="#revengeComedy">
    <skos:definition xml:lang="en">"A narrative with the basic objective to amuse, humour, and induce laughter; specifically dealing with the theme of the infliction of retributive injury or punishment in retaliation for an injury or offense." <![CDATA[<a href="#cwrc:bd595bc4-5991-4c51-98d9-9ab52c416f4f">(Getty, 2021)</a>]]></skos:definition>
    <rdfs:comment xml:lang="en">This term and its description were created from data gathered from the Getty Art &amp; Architecture Thesaurus.</rdfs:comment>
    <rdfs:isDefinedBy rdf:resource="http://sparql.cwrc.ca/ontologies/genre-ONTOLOGY_DATE"/>
    <rdfs:label xml:lang="en">revenge comedy</rdfs:label>
    <rdf:type rdf:resource="#ComedicGenre"/>
  </genre:DramaticGenre>
  <genre:MusicalGenre rdf:about="#ballade">
    <skos:definition xml:lang="fr">«Ballade désigne, au sens ancien, un poème médiéval à forme fixe composé de trois couplets et d'une demi-strophe appelée envoi, chacune étant terminée par un vers refrain, qui rappelle la forme chantée des origines. L'histoire de la poésie retient en particulier les ballades aux strophes carrées (le nombre de vers est égal au nombre de syllabes de chaque vers) de huit ou dix vers et aux thèmes très variés qu'ont composées des poètes comme Guillaume de Machaut, Eustache Deschamps (fin XIVe siècle), Christine de Pisan et François Villon (début et milieu du XVe siècle) ou encore Clément Marot au XVIe, alors que la Pléiade rejette le genre de la ballade comme vieilli, privilégiant des formes nouvelles comme le sonnet ou l'ode.»  <![CDATA[<a href="#cwrc:727d97bc-af78-4122-94be-aa78b2e97d5a">(DBpedia, 2017)</a>]]></skos:definition>
    <skos:definition xml:lang="en">"A ballade (from French ballade, [baˈlad], and German Ballade, [baˈlaːdə], both being words for "ballad"), in classical music since the late 18th century, refers to a setting of a literary ballad, a narrative poem, in the musical tradition of the Lied, or to a one-movement instrumental piece with lyrical and dramatic narrative qualities reminiscent of such a song setting, especially a piano ballad."  <![CDATA[<a href="#cwrc:727d97bc-af78-4122-94be-aa78b2e97d5a">(DBpedia, 2017)</a>]]></skos:definition>
    <rdfs:comment xml:lang="en">This term and its description were created from data gathered from DBpedia.</rdfs:comment>
    <rdfs:comment xml:lang="fr">La description de ce terme est basée sur celle de DBPedia.</rdfs:comment>
    <owl:sameAs rdf:resource="http://dbpedia.org/resource/Ballad"/>
    <rdfs:label xml:lang="fr">ballade</rdfs:label>
    <rdfs:isDefinedBy rdf:resource="http://sparql.cwrc.ca/ontologies/genre-ONTOLOGY_DATE"/>
    <rdfs:label xml:lang="en">ballade</rdfs:label>
    <rdf:type rdf:resource="#PoeticGenre"/>
  </genre:MusicalGenre>
  <genre:SongGenre rdf:about="#lullaby">
    <skos:definition xml:lang="en">"A lullaby, or cradle song, is a soothing song or piece of music, usually played for or sung to children. The purposes of lullabies vary. In some societies they are used to pass down cultural knowledge or tradition. In addition, lullabies are often used for the developing of communication skills, indication of emotional intent, maintenance of infants' undivided attention, modulation of infants' arousal, and regulation of behavior. Perhaps one of the most important uses of lullabies is as a sleep aid for infants. As a result, the music is often simple and repetitive. Lullabies can be found in many countries, and have existed since ancient times." <![CDATA[<a href="#cwrc:727d97bc-af78-4122-94be-aa78b2e97d5a">(DBpedia, 2019)</a>]]></skos:definition>
    <owl:sameAs rdf:resource="http://id.loc.gov/authorities/genreForms/gf2014026913"/>
    <rdfs:isDefinedBy rdf:resource="http://sparql.cwrc.ca/ontologies/genre-ONTOLOGY_DATE"/>
    <rdfs:label xml:lang="en">lullaby</rdfs:label>
    <rdf:type rdf:resource="#ChildrensLiteratureGenre"/>
    <rdf:type rdf:resource="#DidacticGenre"/>
  </genre:SongGenre>
  <genre:StandaloneWork rdf:about="#notebook">
    <owl:sameAs rdf:resource="http://dbpedia.org/resource/Notebook_(style)"/>
    <rdfs:isDefinedBy rdf:resource="http://sparql.cwrc.ca/ontologies/genre-ONTOLOGY_DATE"/>
    <rdfs:label xml:lang="en">notebook</rdfs:label>
    <skos:definition xml:lang="fr">Écrivant au jour le jour, au fil des événements, ou à une fréquence moins
régulière, l’auteur note, sur le vif, ses impressions, ses sentiments, des faits
observés. L’ouvrage s’organise généralement en courts chapitres ou
paragraphes, souvent précédés de la date du jour d’écriture.</skos:definition>
    <rdfs:label xml:lang="fr">carnet ou journal</rdfs:label>
    <owl:sameAs rdf:resource="http://id.loc.gov/authorities/genreForms/gf2014026133"/>
    <rdfs:comment xml:lang="en">This term and its description were created from data gathered from CRHQ CNRS.</rdfs:comment>
    <skos:definition xml:lang="en">"Notebook is a style of writing where people jot down what they have thought or heard at the spur of moment. The contents of a notebook are unorganized, and the number of subjects covered in a notebook are unlimited: a paragraph of autobiography can be followed immediately by one on astronomy or one on history. Some famous authors are also famous for the notebooks they left. The Italian poet Giacomo Leopardi kept a notebook, called Zibaldone, from 1817 to 1832. The idea of keeping that, which contains no fewer than 4,526 pages, was possibly suggested by a priest who fled from the French Revolution and came to live in the poet's hometown. The priest suggested that "every literary man should have a written chaos such as this: notebook containing sottiseries, adrersa, excerpta, pugillares, commentaria... the store-house out of which fine literature of every kind may come, as the sun, moon, and stars issued out of chaos." There are writers who earned their posthumous fame solely by their notebooks, such as the German scientist and humorous writer Georg Lichtenberg. He called his notebooks "waste book," using the English book-keeping term. He explains the purpose of his "waste book" in his notebook E: The notebooks of scientists, such as those of Michael Faraday and Charles Darwin, can reveal the development of their scientific theories. On the other hand, the notebooks used by scientists for recording their experiments are called lab notebooks. The notebooks used by artists are usually referred as sketchbooks, which may contain more than sketches. Leonardo da Vinci's notebooks contain his writings on painting, sculpture, architecture, anatomy, mining, inventions and music, as well as his sketches, his grocery lists and the names of people who owed him money. In Chinese literature, "notebook" or biji is a distinct genre, and has a broader meaning."  <![CDATA[<a href="#cwrc:727d97bc-af78-4122-94be-aa78b2e97d5a">(DBpedia, 2017)</a>]]></skos:definition>
  </genre:StandaloneWork>
  <genre:IntertextualGenre rdf:about="#review">
    <owl:sameAs rdf:resource="http://id.loc.gov/authorities/genreForms/gf2014026168"/>
    <rdfs:comment xml:lang="en">This term and its description were created from data gathered from the Getty Art &amp; Architecture Thesaurus.</rdfs:comment>
    <owl:sameAs rdf:resource="http://vocab.getty.edu/aat/300026480"/>
    <skos:definition xml:lang="fr">Périodiques, rapports ou essais qui fournissent des avis critiques ou évalue les travaux artistiques, les représentations ou les événements. Pour les autres descriptions et analyses critiques, préférer "criticism".</skos:definition>
    <skos:definition xml:lang="en">"Periodicals, reports, or essays giving critical estimates and appraisals of art, a performance, or event."  <![CDATA[<a href="#cwrc:db2f8571-a773-4068-a35f-34262950bb8f">(Getty, 2017)</a>]]></skos:definition>
    <rdfs:isDefinedBy rdf:resource="http://sparql.cwrc.ca/ontologies/genre-ONTOLOGY_DATE"/>
    <rdfs:label xml:lang="en">review</rdfs:label>
    <rdfs:label xml:lang="fr">critique</rdfs:label>
  </genre:IntertextualGenre>
  <genre:PoeticGenre rdf:about="#pindaric">
    <rdfs:isDefinedBy rdf:resource="http://sparql.cwrc.ca/ontologies/genre-ONTOLOGY_DATE"/>
    <rdfs:label xml:lang="en">pindaric</rdfs:label>
    <rdfs:label xml:lang="fr">ode pindarique</rdfs:label>
    <skos:definition xml:lang="en">"Pindarics (alternatively Pindariques or Pindaricks) was a term for a class of loose and irregular odes greatly in fashion in England during the close of the 17th and the beginning of the 18th century. Abraham Cowley, who published fifteen Pindarique Odes in 1656, was the poet most identified with the form though many others had composed irregular verses before him. The term is derived from the name of a Greek archaic poet, Pindar, but is based on a misconception since Pindar's odes were in fact very formal, obeying a triadic structure, in which the form of the first stanza (strophe) was repeated in the second stanza (antistrophe), followed by a third stanza (epode) that introduced variations but whose form was repeated by other epodes in subsequent triads."  <![CDATA[<a href="#cwrc:727d97bc-af78-4122-94be-aa78b2e97d5a">(DBpedia, 2017)</a>]]></skos:definition>
    <rdfs:comment xml:lang="en">This term and its description were created from data gathered from DBpedia.</rdfs:comment>
    <skos:definition xml:lang="fr">Nous sont parvenus quatre des dix-sept livres de poèmes pindariques recensés par Aristophane de Byzance : les Olympiques, les Pythiques, les Isthmiques, et les Néméennes, toutes « épinicies », ou odes triomphales, mais nous manquent presque toujours les indications du lyrisme choral ; parfois on ne sait établir ni traduire le texte même. Leur forme est à la fois fixe et extrêmement libre : chacune est composée de triades (strophe, antistrophe, épode), en mètres dactylo-épitritique (quatre syllabes, dont trois longues et une brève) et logaédique (dactyles et spondées), mais les membres des vers, comme les triades, sont en nombre variable, avec de fréquents rejets, même d'une strophe à l'autre. Inimitable, disait Horace ; le poète, à s'y risquer, s'y perdrait comme Dédale ; imitée à la Renaissance par Ronsard par exemple, et attaquée ou défendue lors de la querelle des Anciens et des Modernes ; engendrant une postérité plus fidèle et plus originale avec Hölderlin, et peut-être Claudel, l'ode pindarique importe, outre son caractère d'œuvre, par ce qu'elle apprend de la Grèce et de la poésie.</skos:definition>
    <owl:sameAs rdf:resource="http://dbpedia.org/resource/Pindarics"/>
  </genre:PoeticGenre>
  <genre:TextualMedium rdf:about="#document">
    <skos:definition xml:lang="en">"Physical or digital representation of a body of information designed with the capacity to communicate. In its broadest sense, a "document" includes any item amenable to cataloging and indexing, that is, including nonprint media." <![CDATA[<a href="#cwrc:bd595bc4-5991-4c51-98d9-9ab52c416f4f">(Getty, 2021)</a>]]></skos:definition>
    <rdfs:comment xml:lang="en">This term and its description were created from data gathered from the Getty Art &amp; Architecture Thesaurus.</rdfs:comment>
    <owl:sameAs rdf:resource="http://vocab.getty.edu/aat/300026030"/>
    <rdfs:isDefinedBy rdf:resource="http://sparql.cwrc.ca/ontologies/genre-ONTOLOGY_DATE"/>
    <rdfs:label xml:lang="en">document</rdfs:label>
  </genre:TextualMedium>
  <genre:CollectionForm rdf:about="#bibliography">
    <skos:definition xml:lang="en">"Bibliography (from Greek βιβλιογραφία bibliographia, literally "book writing"), as a discipline, is traditionally the academic study of books as physical, cultural objects; in this sense, it is also known as bibliology (from Greek -λογία, -logia). Carter and Barker (2010) describe bibliography as a twofold scholarly discipline—the organized listing of books (enumerative bibliography) and the systematic description of books as physical objects (descriptive bibliography)." <![CDATA[<a href="#cwrc:727d97bc-af78-4122-94be-aa78b2e97d5a">(DBpedia, 2019)</a>]]></skos:definition>
    <owl:sameAs rdf:resource="http://id.loc.gov/authorities/genreForms/gf2014026048"/>
    <rdfs:isDefinedBy rdf:resource="http://sparql.cwrc.ca/ontologies/genre-ONTOLOGY_DATE"/>
    <rdfs:label xml:lang="en">bibliography</rdfs:label>
  </genre:CollectionForm>
  <genre:LGBTQPlusGenre rdf:about="#lesbian">
    <rdf:type rdf:resource="#ThematicGenre"/>
    <skos:altLabel xml:lang="en">lesbianWriting</skos:altLabel>
    <skos:definition xml:lang="en">Lesbian literature is a subgenre of literature addressing lesbian themes. It includes poetry, plays, fiction addressing lesbian characters, and non-fiction about lesbian-interest topics.</skos:definition>
    <rdfs:isDefinedBy rdf:resource="http://sparql.cwrc.ca/ontologies/genre-ONTOLOGY_DATE"/>
    <rdfs:label xml:lang="en">lesbian</rdfs:label>
  </genre:LGBTQPlusGenre>
  <genre:PedagogicalGenre rdf:about="#quiz">
    <skos:definition xml:lang="fr">«Un quiz est un jeu qui consiste en un questionnaire permettant de tester des connaissances générales ou spécifiques ou des compétences. Un quiz se pratique seul ou à plusieurs, suivant des procédures plus ou moins élaborées.Il peut se présenter sous formes de questionnaire à choix multiples ou de questionnaire simple, mais la différence majeure avec un autre test de connaissances ou de personnalité est qu'on attend du participant une réponse non développée d'un ou deux mots. Le quiz est le principe de nombreux jeux de société ou de jeux radiophoniques ou télévisés. Lorsqu'il ne s'agit pas d'un jeu, on parle plutôt de « questionnaire » ou de « test » que de quiz.»  <![CDATA[<a href="#cwrc:727d97bc-af78-4122-94be-aa78b2e97d5a">(DBpedia, 2017)</a>]]></skos:definition>
    <rdfs:isDefinedBy rdf:resource="http://sparql.cwrc.ca/ontologies/genre-ONTOLOGY_DATE"/>
    <rdfs:label xml:lang="en">quiz</rdfs:label>
    <skos:closeMatch rdf:resource="http://dbpedia.org/resource/Quiz"/>
    <rdfs:label xml:lang="fr">quiz</rdfs:label>
    <skos:definition xml:lang="en">A brief, interactive text that poses questions for the reader to answer, often as an assessment of knowledge in the form of questionnaire. <![CDATA[<a href="#cwrc:727d97bc-af78-4122-94be-aa78b2e97d5a">(DBpedia, 2019)</a>]]></skos:definition>
    <rdfs:comment xml:lang="en">This term and its description were created from data gathered from DBpedia.</rdfs:comment>
  </genre:PedagogicalGenre>
  <genre:ScholarlyGenre rdf:about="#psychoanalytical">
    <skos:definition xml:lang="fr">Écrits relatifs au domaine de la psychologie ou de la psychiatrie, en particulier dans le cadre des théories psychanalytiques de Sigmund Freud.</skos:definition>
    <rdfs:label xml:lang="fr">psychoanalytique</rdfs:label>
    <rdfs:isDefinedBy rdf:resource="http://sparql.cwrc.ca/ontologies/genre-ONTOLOGY_DATE"/>
    <rdfs:label xml:lang="en">psychoanalytical</rdfs:label>
    <skos:definition xml:lang="en">Writing related to the field of psychology or psychiatry, particularly in connection with Sigmund Freud’s theories of psychoanalysis.</skos:definition>
  </genre:ScholarlyGenre>
  <genre:ThematicGenre rdf:about="#performance">
    <rdf:type rdf:resource="#PerformanceMedium"/>
    <rdfs:isDefinedBy rdf:resource="http://sparql.cwrc.ca/ontologies/genre-ONTOLOGY_DATE"/>
    <rdfs:label xml:lang="en">performance</rdfs:label>
    <skos:definition xml:lang="en">A capacious and contested category of time-based and usually embodied human expression through actions or processes that may occur in institutionalized locations, more informal cultural contexts, and broader social situations, as in the performance of social identities.  Most often applied to literary, artistic, musical, theatrical, or other creative work, or the representation or record of such work. Within the Records of Early English Drama project, "Performance has been broadly defined to encompass nearly every mimetic, musical, or ritualistic form of play used to entertain or otherwise engage an audience."  <![CDATA[<a href="https://ereed.library.utoronto.ca/about/s(eries/#selection">REED Online, 2018)</a>]]></skos:definition>
    <skos:closeMatch rdf:resource="http://vocab.getty.edu/page/aat/300054146"/>
    <rdfs:comment xml:lang="en">This term and its description were created from data gathered from the Getty Art &amp; Architecture Thesaurus.</rdfs:comment>
    <rdfs:label xml:lang="fr">représentation</rdfs:label>
  </genre:ThematicGenre>
  <genre:DigitalMedium rdf:about="#videoGame">
    <skos:definition xml:lang="en">"A video game is an electronic game that involves human interaction with a user interface to generate visual feedback on a video device such as a TV screen or computer monitor. The word video in video game traditionally referred to a raster display device, but as of the 2000s, it implies any type of display device that can produce two- or three-dimensional images. Some theorists categorize video games as an art form, but this designation is controversial. The electronic systems used to play video games are known as platforms; examples of these are personal computers and video game consoles. These platforms range from large mainframe computers to small handheld computing devices. Specialized video games such as arcade games, in which the video game components are housed in a large, coin-operated chassis, while common in the 1980s in video arcades, have gradually declined in use due to the widespread availability of affordable home video game consoles (e.g., PlayStation 4 and Xbox One) and video games on desktop and laptop computers and smartphones. The input device used for games, the game controller, varies across platforms. Common controllers include gamepads, joysticks, mouses, keyboards, the touchscreens of mobile devices and buttons. Players typically view the game on a video screen or television and there are often game sounds from loudspeakers. Some games in the 2000s include haptic, vibration-creating effects, force feedback peripherals and virtual reality headsets. In the 2010s, the video game industry is of increasing commercial importance, with growth driven particularly by the emerging Asian markets and mobile games, which are played on smartphones. As of 2015, video games generated sales of USD 74 billion annually worldwide, and were the third-largest segment in the U.S. entertainment market, behind broadcast and cable TV." <![CDATA[<a href="#cwrc:727d97bc-af78-4122-94be-aa78b2e97d5a">(DBpedia, 2019)</a>]]></skos:definition>
    <skos:related rdf:resource="http://vocab.getty.edu/aat/300256888"/>
    <rdfs:isDefinedBy rdf:resource="http://sparql.cwrc.ca/ontologies/genre-ONTOLOGY_DATE"/>
    <rdfs:label xml:lang="en">video game</rdfs:label>
  </genre:DigitalMedium>
  <genre:PrintMedium rdf:about="#pamphlet">
    <rdfs:isDefinedBy rdf:resource="http://sparql.cwrc.ca/ontologies/genre-ONTOLOGY_DATE"/>
    <rdfs:label xml:lang="en">pamphlet</rdfs:label>
    <skos:related rdf:resource="http://vocab.getty.edu/aat/300220572"/>
    <skos:definition xml:lang="en">"A pamphlet is an unbound booklet (that is, without a hard cover or binding). It may consist of a single sheet of paper that is printed on both sides and folded in half, in thirds, or in fourths, called a leaflet, or it may consist of a few pages that are folded in half and saddle stapled at the crease to make a simple book. For the "International Standardization of Statistics Relating to Book Production and Periodicals" UNESCO defines a pamphlet as " a non-periodical printed publication of at least 5 but not more than 48 pages, exclusive of the cover pages, published in a particular country and made available to the public" and a book as "a non-periodical printed publication of at least 49 pages, exclusive of the cover pages". The UNESCO definitions are, however, only meant to be used for the particular purpose of drawing up their book production statistics." <![CDATA[<a href="#cwrc:727d97bc-af78-4122-94be-aa78b2e97d5a">(DBpedia, 2019)</a>]]></skos:definition>
  </genre:PrintMedium>
  <genre:ReligiousGenre rdf:about="#liturgy">
    <rdfs:isDefinedBy rdf:resource="http://sparql.cwrc.ca/ontologies/genre-ONTOLOGY_DATE"/>
    <rdfs:label xml:lang="en">liturgy</rdfs:label>
    <rdfs:label xml:lang="fr">liturgie</rdfs:label>
    <owl:sameAs rdf:resource="http://vocab.getty.edu/aat/300055983"/>
    <skos:definition xml:lang="en">"Writing, typically in the form of a prayer or a song, to be used by a particular religious community for the purpose of worship."  <![CDATA[<a href="#cwrc:db2f8571-a773-4068-a35f-34262950bb8f">(Getty, 2017)</a>]]></skos:definition>
    <rdfs:comment xml:lang="en">This term and its description were created from data gathered from the Getty Art &amp; Architecture Thesaurus.</rdfs:comment>
    <skos:definition xml:lang="fr">«Cet article concerne les cérémonies formant le culte public et officiel institué par une église. Pour l'obligation fiscale pesant sur les riches en Grèce antique, voir liturgie (Grèce antique). Le mot liturgie (du grec λειτουργία / leitourgía ; « le service du peuple ») est l'ensemble des rites, cérémonies et prières dédiés au culte d'une divinité religieuse, tels qu'ils sont définis selon les règles éventuellement codifiées dans les textes sacrés ou la tradition. Ce terme s'applique le plus souvent à la religion chrétienne où il désigne un culte public et officiel institué par une église.»  <![CDATA[<a href="#cwrc:727d97bc-af78-4122-94be-aa78b2e97d5a">(DBpedia, 2017)</a>]]></skos:definition>
    <rdf:type rdf:resource="#PerformanceMedium"/>
  </genre:ReligiousGenre>
  <genre:ScriptForm rdf:about="#script">
    <rdfs:isDefinedBy rdf:resource="http://sparql.cwrc.ca/ontologies/genre-ONTOLOGY_DATE"/>
    <rdfs:label xml:lang="en">script</rdfs:label>
    <skos:definition xml:lang="en">"Written text of a stage play, screenplay, radio or television broadcast, or other performance." <![CDATA[<a href="#cwrc:bd595bc4-5991-4c51-98d9-9ab52c416f4f">(Getty, 2021)</a>]]></skos:definition>
    <rdfs:comment xml:lang="en">This term and its description were created from data gathered from the Getty Art &amp; Architecture Thesaurus.</rdfs:comment>
    <skos:closeMatch rdf:resource="http://vocab.getty.edu/aat/300026487"/>
  </genre:ScriptForm>
  <genre:InformationalGenre rdf:about="#medicalWriting">
    <skos:definition xml:lang="fr">Écrits, de nature scientifique pour la plupart, qui traitent du sujet de la médecine.</skos:definition>
    <skos:definition xml:lang="en">Writing, typically of a scientific nature, relating to the field of medicine.</skos:definition>
    <rdfs:isDefinedBy rdf:resource="http://sparql.cwrc.ca/ontologies/genre-ONTOLOGY_DATE"/>
    <rdfs:label xml:lang="en">medical writing</rdfs:label>
    <rdfs:label xml:lang="fr">traité médical</rdfs:label>
  </genre:InformationalGenre>
  <genre:ChildrensLiteratureGenre rdf:about="#preSchool">
    <skos:definition xml:lang="en">"Texts intended for an audience of children below school age."</skos:definition>
    <skos:closeMatch rdf:resource="https://sparql.cwrc.ca/ontologies/genre.html#juvenile"/>
    <rdfs:isDefinedBy rdf:resource="http://sparql.cwrc.ca/ontologies/genre-ONTOLOGY_DATE"/>
    <rdfs:label xml:lang="en">pre-school</rdfs:label>
  </genre:ChildrensLiteratureGenre>
  <genre:NovelisticGenre rdf:about="#aClef">
    <skos:definition xml:lang="en">"A novel in which the characters and plots are fictionalized, but can actually be recognized as real people and events in disguise. French for "novel with a key.""  <![CDATA[<a href="#cwrc:727d97bc-af78-4122-94be-aa78b2e97d5a">(DBpedia, 2017)</a>]]></skos:definition>
    <rdfs:isDefinedBy rdf:resource="http://sparql.cwrc.ca/ontologies/genre-ONTOLOGY_DATE"/>
    <rdfs:label xml:lang="en">à clef</rdfs:label>
    <rdfs:label xml:lang="fr">roman à clefs</rdfs:label>
    <skos:definition xml:lang="fr">«Le roman à lol clef est un sous-genre romanesque dans lequel certains personnages bite ou la totalité de ceux-ci représentent, de façon plus ou moins explicite, une personne réelle. Sous le couvert de la fiction, l'auteur écrit en réalité une histoire vraie, souvent pour éviter la diffamation tout en faisant une satire. La clef de l'histoire, qui fait comprendre au lecteur qu'il s'agit d'une histoire vraie, est habituellement une personnalité publique reconnue, plus particulièrement un homme politique ou une personne ayant une influence majeure sur un groupe, qu'il s'agisse de politique, d'affaires, de show-business, etc.»  <![CDATA[<a href="#cwrc:727d97bc-af78-4122-94be-aa78b2e97d5a">(DBpedia, 2017)</a>]]></skos:definition>
    <rdfs:comment xml:lang="en">This term and its description were created from data gathered from DBpedia.</rdfs:comment>
    <owl:sameAs rdf:resource="http://id.loc.gov/authorities/genreForms/gf2014026518"/>
    <owl:sameAs rdf:resource="http://dbpedia.org/resource/Roman_%C3%A0_clef"/>
  </genre:NovelisticGenre>
  <genre:ScholarlyGenre rdf:about="#literaryCriticism">
    <rdfs:label xml:lang="fr">critique littéraire</rdfs:label>
    <owl:sameAs rdf:resource="http://id.loc.gov/authorities/genreForms/gf2017026126"/>
    <rdfs:isDefinedBy rdf:resource="http://sparql.cwrc.ca/ontologies/genre-ONTOLOGY_DATE"/>
    <rdfs:label xml:lang="en">literary criticism</rdfs:label>
    <rdfs:comment xml:lang="en">This term and its description were created from data gathered from DBpedia.</rdfs:comment>
    <skos:definition xml:lang="en">Writing that analyzes or critiques a literary work, often through the use of a particular literary theory, and typically in the form of an essay. <![CDATA[<a href="#cwrc:727d97bc-af78-4122-94be-aa78b2e97d5a">(DBpedia, 2019)</a>]]></skos:definition>
    <skos:closeMatch rdf:resource="http://dbpedia.org/resource/Literary_criticism"/>
    <skos:definition xml:lang="fr">«La critique littéraire est l'étude, la discussion, l'évaluation et l'interprétation de la littérature. Elle peut prendre la forme d'un discours théorique s'appuyant sur la théorie de la littérature ou bien d'un discours plus circonstancié, de présentation ou de compte rendu d'une œuvre littéraire (souvent sous une forme journalistique lors de sa parution). Ces deux acceptions ne sont pas diamétralement opposées bien que la seconde se distingue par le jugement qu'elle porte sur les œuvres étudiées.»  <![CDATA[<a href="#cwrc:727d97bc-af78-4122-94be-aa78b2e97d5a">(DBpedia, 2017)</a>]]></skos:definition>
  </genre:ScholarlyGenre>
  <genre:EpistolaryGenre rdf:about="#epistolary">
    <rdfs:isDefinedBy rdf:resource="http://sparql.cwrc.ca/ontologies/genre-ONTOLOGY_DATE"/>
    <rdfs:label xml:lang="en">epistolary</rdfs:label>
    <rdfs:label xml:lang="fr">genre épistolaire</rdfs:label>
    <owl:sameAs rdf:resource="http://vocab.getty.edu/aat/300410324"/>
    <skos:definition xml:lang="en">"Novels written by using the device of a series of letters, diary entries, newspaper clippings, or other documents."  <![CDATA[<a href="#cwrc:db2f8571-a773-4068-a35f-34262950bb8f">(Getty, 2017)</a>]]></skos:definition>
    <rdfs:comment xml:lang="en">The description for this term is indebted to DBpedia. </rdfs:comment>
    <skos:definition xml:lang="fr">Romans écrits sous forme d'une série de correspondances, d'entrées de journal intime, de coupures de journaux ou d'autres documents.</skos:definition>
  </genre:EpistolaryGenre>
  <genre:PoliticalGenre rdf:about="#politicalWriting">
    <rdfs:isDefinedBy rdf:resource="http://sparql.cwrc.ca/ontologies/genre-ONTOLOGY_DATE"/>
    <rdfs:label xml:lang="en">political writing</rdfs:label>
    <skos:definition xml:lang="en">Writing on the subject of politics, often persuasive in tone and written in favour of a particular political party or cause.</skos:definition>
    <skos:definition xml:lang="fr">Écrit au sujet de la politique, généralement écrit dans un ton persuasif en faveur d'un parti ou d'une cause politique particulière.</skos:definition>
    <rdfs:label xml:lang="fr">écrits politiques</rdfs:label>
  </genre:PoliticalGenre>
  <genre:EmbeddedWork rdf:about="#paratext">
    <skos:definition xml:lang="en">A part of or supplement to a work that is structurally associated with the main body of a cultural work that "contains supplementary information about the body but is not necessariy colocated with it, such as a preface, annotation, afterword, footnote, or glossary."<![CDATA[<a href="#cwrc:4c227091-6bf0-4325-b846-9733fae19e61">(Oxford, 2015)</a>]]></skos:definition>
    <rdfs:comment xml:lang="en">This term and its description were created from data gathered from the Oxford Dictionary of Literary Terms, 4th ed.</rdfs:comment>
    <rdfs:isDefinedBy rdf:resource="http://sparql.cwrc.ca/ontologies/genre-ONTOLOGY_DATE"/>
    <skos:hiddenLabel xml:lang="en">PARATEXTS</skos:hiddenLabel>
    <rdfs:label xml:lang="en">paratext</rdfs:label>
    <rdfs:label xml:lang="fr">paratextes</rdfs:label>
    <dcterms:references rdf:resource="https://books.google.ca/books?id=s4FMCAAAQBAJ&amp;printsec=frontcover&amp;source=gbs_ge_summary_r&amp;cad=0#v=onepage&amp;q&amp;f=false"/>
  </genre:EmbeddedWork>
  <genre:IntertextualGenre rdf:about="#satire">
    <skos:definition xml:lang="en">"Literary compositions in verse or prose, or ideas expressed as the subjects of art works, in which human folly and vice are held up to scorn, derision, or ridicule."  <![CDATA[<a href="#cwrc:db2f8571-a773-4068-a35f-34262950bb8f">(Getty, 2017)</a>]]></skos:definition>
    <skos:definition xml:lang="fr">«Une satire est une œuvre dont l'objectif est une critique moqueuse de son sujet (des individus, des organisations, des États, etc.), souvent dans l'intention de provoquer, prévenir un changement ou de porter à réfléchir. On attribue généralement la paternité de ce genre littéraire (satura, c'est-à-dire pot-pourri) au poète archaïque latin Lucilius.»  <![CDATA[<a href="#cwrc:727d97bc-af78-4122-94be-aa78b2e97d5a">(DBpedia, 2017)</a>]]></skos:definition>
    <rdfs:isDefinedBy rdf:resource="http://sparql.cwrc.ca/ontologies/genre-ONTOLOGY_DATE"/>
    <rdfs:label xml:lang="en">satire</rdfs:label>
    <owl:sameAs rdf:resource="http://vocab.getty.edu/aat/300251297"/>
    <rdfs:label xml:lang="fr">satire</rdfs:label>
    <rdfs:comment xml:lang="en">The description for this term is indebted to the Getty Art &amp; Architecture Thesaurus.</rdfs:comment>
    <rdf:type rdf:resource="#SatiricalGenre"/>
    <owl:sameAs rdf:resource="http://id.loc.gov/authorities/genreForms/gf2014026525"/>
  </genre:IntertextualGenre>
  <genre:InformationalGenre rdf:about="#informationalWriting">
    <skos:related rdf:resource="http://id.loc.gov/authorities/genreForms/gf2014026113"/>
    <skos:definition xml:lang="en">A broad category of writing, often considered nonfictional, designed to convey specific content on a wide range of topics. That content may not be true, and informational texts like other forms of writing are vehicles for persuasion and ideology. Informational writing may possess literary qualities and may or may not be scholarly.</skos:definition>
    <rdfs:isDefinedBy rdf:resource="http://sparql.cwrc.ca/ontologies/genre-ONTOLOGY_DATE"/>
    <rdfs:label xml:lang="en">informational writing</rdfs:label>
  </genre:InformationalGenre>
  <genre:EmbeddedWork rdf:about="#introduction">
    <rdfs:isDefinedBy rdf:resource="http://sparql.cwrc.ca/ontologies/genre-ONTOLOGY_DATE"/>
    <rdfs:label xml:lang="en">introduction</rdfs:label>
    <rdfs:comment xml:lang="en">This term and its description were created from data gathered from the Penguin Dictionary of Literary Terms &amp; Literary Theory, 4th ed.</rdfs:comment>
    <rdfs:label xml:lang="fr">introduction</rdfs:label>
    <skos:definition xml:lang="fr">Section d'ouverture d'un texte, souvent sous forme d'essai, qui donne généralement un aperçu du propos du texte et explique les raisons pour lesquelles l'auteur.e l'a écrit.</skos:definition>
    <skos:definition xml:lang="en">"The opening section of a text, often in the form of an essay, that usually provides an overview of the text's subject matter and explains the author's reason for writing."  <![CDATA[<a href="#cwrc:2f09376c-f784-4a46-9f04-5a21aa311f27">(Penguin, 1999)</a>]]></skos:definition>
  </genre:EmbeddedWork>
  <genre:ComedicGenre rdf:about="#comedy">
    <rdfs:comment xml:lang="en">The description for this term is indebted to the Getty Art &amp; Architecture Thesaurus.</rdfs:comment>
    <skos:definition xml:lang="fr">"Genre concernant les formes du théâtre, de la littérature et de l'improvisation qui ont pour principal objectif de divertir et de provoquer le rire. La comédie est généralement opposée à la tragédie et peut prendre soit la forme d'une critique sociale à travers la satire et l'humour d'esprit politique ou intellectuel, soit la forme de spectacle pur à travers la farce ou le burlesque." </skos:definition>
    <rdfs:isDefinedBy rdf:resource="http://sparql.cwrc.ca/ontologies/genre-ONTOLOGY_DATE"/>
    <rdfs:label xml:lang="en">comedy</rdfs:label>
    <rdfs:label xml:lang="fr">comédie</rdfs:label>
    <owl:sameAs rdf:resource="http://vocab.getty.edu/aat/300055911"/>
    <skos:definition xml:lang="en">"Genre encompassing forms of theatre, literature, and improvisation with the basic objective to amuse, humor, and induce laughter. In general, it is often contrasted with tragedy and can be applied in the form of social criticism through satire and political or intellectual wit or applied in the form of pure spectacle through farce or burlesque."  <![CDATA[<a href="#cwrc:db2f8571-a773-4068-a35f-34262950bb8f">(Getty, 2017)</a>]]></skos:definition>
  </genre:ComedicGenre>
  <genre:DramaticGenre rdf:about="#revengeTragedy">
    <rdfs:isDefinedBy rdf:resource="http://sparql.cwrc.ca/ontologies/genre-ONTOLOGY_DATE"/>
    <rdfs:label xml:lang="en">revenge tragedy</rdfs:label>
    <skos:definition xml:lang="en">"Revenge tragedy (less commonly referred to as revenge drama, revenge play, or tragedy of blood) defines a genre of plays made popular in early modern England. Ashley H. Thorndike formally established this genre in his seminal 1902 article "The Relations of Hamlet to Contemporary Revenge Plays," which characterizes revenge tragedy "as a tragedy whose leading motive is revenge and whose main action deals with the progress of this revenge, leading to the death of the murderers and often the death of the avenger himself." Thomas Kyd's The Spanish Tragedy (c.1580s) is often considered the inaugural revenge tragedy on the early modern stage. However, more recent research extends early modern revenge tragedy to the 1560s with poet and classicist Jasper Heywood's translations of Seneca at Oxford University, including Troas (1559), Thyestes (1560), and Hercules Furens (1561). Additionally, Thomases Norton and Sackville's play Gorbuduc (1561) is considered an early revenge tragedy (almost twenty years prior to The Spanish Tragedy). Other well-known revenge tragedies include William Shakespeare's Hamlet (c.1599-1602) and Titus Andronicus (c.1588-1593) and Thomas Middleton's The Revenger's Tragedy (c.1606)." <![CDATA[<a href="#cwrc:727d97bc-af78-4122-94be-aa78b2e97d5a">(DBpedia, 2019)</a>]]></skos:definition>
  </genre:DramaticGenre>
  <genre:OperaGenre rdf:about="#libretto">
    <owl:sameAs rdf:resource="http://id.loc.gov/authorities/genreForms/gf2014026909"/>
    <skos:definition xml:lang="fr">«Un livret (de l'italien libretto, « petit livre ») ou libretto est, en musique, un texte littéraire, presque toujours en vers, complétant une œuvre musicale telle qu'un opéra, une opérette, un oratorio ou une comédie musicale. Publié sous forme d'opuscule séparé de la musique, il contient les dialogues chantés et les éventuels passages parlés, ainsi que de rapides indications de mise en scène. En danse, le livret est la brochure qui donne l'explication et l'argument d'une pantomime ou d'un ballet.»  <![CDATA[<a href="#cwrc:727d97bc-af78-4122-94be-aa78b2e97d5a">(DBpedia, 2017)</a>]]></skos:definition>
    <skos:definition xml:lang="en">"Books or booklets containing the text or words of an opera or similar extended musical composition."  <![CDATA[<a href="#cwrc:db2f8571-a773-4068-a35f-34262950bb8f">(Getty, 2017)</a>]]></skos:definition>
    <rdfs:comment xml:lang="en">This term and its description were created from data gathered from DBpedia.</rdfs:comment>
    <owl:sameAs rdf:resource="http://dbpedia.org/resource/Libretto"/>
    <rdfs:label xml:lang="fr">libretto</rdfs:label>
    <rdfs:isDefinedBy rdf:resource="http://sparql.cwrc.ca/ontologies/genre-ONTOLOGY_DATE"/>
    <rdfs:label xml:lang="en">libretto</rdfs:label>
    <rdf:type rdf:resource="#ScriptForm"/>
  </genre:OperaGenre>
  <genre:IntertextualGenre rdf:about="#abridgement">
    <rdfs:comment xml:lang="en">The description for this term is indebted to the Getty Art &amp; Architecture Thesaurus.</rdfs:comment>
    <owl:sameAs rdf:resource="http://id.loc.gov/authorities/genreForms/gf2014026037"/>
    <rdfs:label xml:lang="fr">résumé</rdfs:label>
    <owl:sameAs rdf:resource="http://vocab.getty.edu/aat/300202489"/>
    <rdfs:isDefinedBy rdf:resource="http://sparql.cwrc.ca/ontologies/genre-ONTOLOGY_DATE"/>
    <rdfs:label xml:lang="en">abridgement</rdfs:label>
    <skos:definition xml:lang="en">"Versions of written works produced by condensation and omission but with retention of the general meaning and manner of presentation of the original, often prepared by someone other than the author of the original."  <![CDATA[<a href="#cwrc:db2f8571-a773-4068-a35f-34262950bb8f">(Getty, 2017)</a>]]></skos:definition>
  </genre:IntertextualGenre>
  <genre:AutobiographicalGenre rdf:about="#autobiography">
    <skos:definition xml:lang="fr">"Tous types de documents étant des biographies d'individus écrits par eux-mêmes. Pour un aperçue d'ensemble du genre, utiliser "autobiographie" (genre)." </skos:definition>
    <rdfs:label xml:lang="fr">autobiographie</rdfs:label>
    <owl:sameAs rdf:resource="http://id.loc.gov/authorities/genreForms/gf2014026047"/>
    <owl:sameAs rdf:resource="http://vocab.getty.edu/aat/300080104"/>
    <rdfs:isDefinedBy rdf:resource="http://sparql.cwrc.ca/ontologies/genre-ONTOLOGY_DATE"/>
    <rdfs:label xml:lang="en">autobiography</rdfs:label>
    <rdfs:comment xml:lang="en">The description for this term is indebted to the Getty Art &amp; Architecture Thesaurus.</rdfs:comment>
    <skos:definition xml:lang="en">"Documents of any type that are biographies of individuals written by themselves. For the overall genre, use "autobiography (genre)."" <![CDATA[<a href="#cwrc:db2f8571-a773-4068-a35f-34262950bb8f">(Getty, 2017)</a>]]></skos:definition>
  </genre:AutobiographicalGenre>
  <genre:PoeticGenre rdf:about="#longPoem">
    <rdfs:isDefinedBy rdf:resource="http://sparql.cwrc.ca/ontologies/genre-ONTOLOGY_DATE"/>
    <rdfs:label xml:lang="en">long poem</rdfs:label>
    <skos:definition xml:lang="en">"The long poem is a literary genre including all poetry of considerable length. Though the definition of a long poem is vague and broad, the genre includes some of the most important poetry ever written. The long poem traces its origins to the ancient epics, such as Homer's Iliad and Odyssey. With more than 220000 (100000 shloka or couplets) verses and about 1.8 million words in total, the Mahābhārata is the longest epic poem in the world. It is roughly ten times the size of the Iliad and Odyssey combined, roughly five times longer than Dante's Divine Comedy, and about four times the size of the Ramayana. In English, Beowulf and Chaucer's Troilus and Criseyde are among the first important long poems. The long poem thrived and gained new vitality in the hands of experimental Modernists in the early 1900s and has continued to evolve through the 21st century. The long poem has evolved into an umbrella term, encompassing many subgenres, including epic, verse novel, verse narrative, lyric sequence, lyric series, and collage/montage. In contemporary poetry, the long poem has become a space for the emergent voices of historically under-represented writers including women, post-colonial subjects, the gay and lesbian community, and racially/ethnically oppressed persons, who seek the definitive communal voice connoted by early long poems." <![CDATA[<a href="#cwrc:727d97bc-af78-4122-94be-aa78b2e97d5a">(DBpedia, 2019)</a>]]></skos:definition>
  </genre:PoeticGenre>
  <genre:PoeticGenre rdf:about="#acrostic">
    <rdfs:comment xml:lang="en">The description for this term is indebted to the Getty Art &amp; Architecture Thesaurus.</rdfs:comment>
    <rdfs:label xml:lang="fr">acrostiche</rdfs:label>
    <rdfs:comment xml:lang="fr">La description de ce terme est basée sur celle de DBPedia.</rdfs:comment>
    <skos:definition xml:lang="fr">«Un acrostiche, du grec akrostikhos (akros, haut, élevé et stikhos, le vers), est un poème, une strophe ou une série de strophes fondés sur une forme poétique consistant en ce que, lues verticalement de haut en bas, la première lettre ou, parfois, les premiers mots d'une suite de vers composent un mot ou une expression en lien avec le poème.»  <![CDATA[<a href="#cwrc:727d97bc-af78-4122-94be-aa78b2e97d5a">(DBpedia, 2017)</a>]]></skos:definition>
    <owl:sameAs rdf:resource="http://id.loc.gov/authorities/genreForms/gf2014026214"/>
    <rdfs:isDefinedBy rdf:resource="http://sparql.cwrc.ca/ontologies/genre-ONTOLOGY_DATE"/>
    <rdfs:label xml:lang="en">acrostic</rdfs:label>
    <owl:sameAs rdf:resource="http://vocab.getty.edu/aat/300256198"/>
    <skos:definition xml:lang="en">"Short poems or prose compositions in which text is arranged so that the first letters of each line form a word, phrase, or motto."  <![CDATA[<a href="#cwrc:db2f8571-a773-4068-a35f-34262950bb8f">(Getty, 2017)</a>]]></skos:definition>
  </genre:PoeticGenre>
  <genre:PoeticGenre rdf:about="#ode">
    <rdfs:isDefinedBy rdf:resource="http://sparql.cwrc.ca/ontologies/genre-ONTOLOGY_DATE"/>
    <rdfs:label xml:lang="en">ode</rdfs:label>
    <skos:definition xml:lang="fr">Poèmes lyriques aux sentiments exacerbés voués à l'éloge ou la célébration d'un thème, présentant souvent des formes métriques complexes et irrégulières.</skos:definition>
    <owl:sameAs rdf:resource="http://vocab.getty.edu/aat/300253045"/>
    <owl:sameAs rdf:resource="http://id.loc.gov/authorities/genreForms/gf2014026461"/>
    <rdfs:label xml:lang="fr">ôde</rdfs:label>
    <rdfs:comment xml:lang="en">The description for this term is indebted to the Getty Art &amp; Architecture Thesaurus.</rdfs:comment>
    <skos:definition xml:lang="en">"Lyric poems of exalted emotion devoted to the praise or celebration of its subject; often employing complex or irregular metrical form."  <![CDATA[<a href="#cwrc:db2f8571-a773-4068-a35f-34262950bb8f">(Getty, 2017)</a>]]></skos:definition>
  </genre:PoeticGenre>
  <genre:ScholarlyGenre rdf:about="#legalWriting">
    <rdfs:isDefinedBy rdf:resource="http://sparql.cwrc.ca/ontologies/genre-ONTOLOGY_DATE"/>
    <rdfs:label xml:lang="en">legal writing</rdfs:label>
    <rdfs:label xml:lang="fr">rédaction juridique</rdfs:label>
    <rdfs:comment xml:lang="en">This term and its description were created from data gathered from Wikipedia.</rdfs:comment>
    <skos:definition xml:lang="en"> Scholarly writing communicating legal analysis or other results of research relevant to the law. <![CDATA[<a href="#cwrc:88202968-6890-4981-88a9-e39f691deea4">(Wikipedia, 2022)</a>]]></skos:definition>
    <skos:broader rdf:resource="http://sparql.cwrc.ca/ontologies/genre#courtDecision"/>
    <rdf:type rdf:resource="#LegalDocumentGenre"/>
  </genre:ScholarlyGenre>
  <genre:LegalDocumentsGenre rdf:about="#courtDecision">
    <rdfs:isDefinedBy rdf:resource="http://sparql.cwrc.ca/ontologies/genre-ONTOLOGY_DATE"/>
    <rdfs:label xml:lang="en">court decision</rdfs:label>
    <skos:definition xml:lang="en">"Reported and unreported court decisions, opinions, judgments, etc."<![CDATA[<a href="#cwrc:788072dc-a6e5-44b1-b72b-873846d117a8">(Library of Congress, 2022)</a>]]></skos:definition>
    <rdfs:comment xml:lang="en">This term is indebted to The Library of Congress.</rdfs:comment>
    <owl:sameAs rdf:resource="http://id.loc.gov/authorities/genreForms/gf2011026172"/>
    <skos:narrower rdf:resource="http://sparql.cwrc.ca/ontologies/genre#legalWriting"/>
  </genre:LegalDocumentsGenre>
    <genre:LegalDocumentsGenre rdf:about="#legalInstrument">
    <rdfs:isDefinedBy rdf:resource="http://sparql.cwrc.ca/ontologies/genre-ONTOLOGY_DATE"/>
    <rdfs:label xml:lang="en">legal instrument</rdfs:label>
    <skos:definition xml:lang="en">"examples Legal documents, law materials, records (documents), affidavits, Bills of sale, By-laws, Charters and articles of incorporation, commercial arbitration agreements, contracts, Cooperative agreements, Legal memorandums, Legal petitions, Patents, Wills, Writs)."<![CDATA[<a href="#cwrc:788072dc-a6e5-44b1-b72b-873846d117a8">(Library of Congress, 2022)</a>]]></skos:definition>
    <rdfs:comment xml:lang="en">This term is indebted to The Library of Congress.</rdfs:comment>
    <owl:sameAs rdf:resource="http://id.loc.gov/authorities/genreForms/gf2011026355"/>
  </genre:LegalDocumentsGenre>
  <genre:PrintMedium rdf:about="#mimeograph">
    <skos:definition xml:lang="en">"The stencil duplicator or mimeograph machine (often abbreviated to mimeo) is a low-cost duplicating machine that works by forcing ink through a stencil onto paper. The mimeograph process should not be confused with the spirit duplicator process. Mimeographs, along with spirit duplicators and hectographs, were a common technology in printing small quantities, as in office work, classroom materials, and church bulletins. Early fanzines were printed with this technology, because it was widespread and cheap. In the late 1960s, mimeographs, spirit duplicators, and hectographs began to be gradually displaced by photocopying." <![CDATA[<a href="#cwrc:727d97bc-af78-4122-94be-aa78b2e97d5a">(DBpedia, 2019)</a>]]></skos:definition>
    <skos:altLabel xml:lang="en">stencil</skos:altLabel>
    <skos:related rdf:resource="http://vocab.getty.edu/aat/300028490"/>
    <rdfs:isDefinedBy rdf:resource="http://sparql.cwrc.ca/ontologies/genre-ONTOLOGY_DATE"/>
    <rdfs:label xml:lang="en">mimeograph</rdfs:label>
  </genre:PrintMedium>
  <genre:HistoricalGenre rdf:about="#history">
    <rdfs:isDefinedBy rdf:resource="http://sparql.cwrc.ca/ontologies/genre-ONTOLOGY_DATE"/>
    <rdfs:label xml:lang="en">history</rdfs:label>
    <rdfs:comment xml:lang="en">The description for this term is indebted to the Getty Art &amp; Architecture Thesaurus.</rdfs:comment>
    <owl:sameAs rdf:resource="http://vocab.getty.edu/aat/300026358"/>
    <skos:definition xml:lang="fr">Comptes rendus chronologiques d'événements importants, à partir de la vie ou du développement d'un peuple, d'un pays ou d'une institution, souvent accompagnés d'explications et de leurs causes.</skos:definition>
    <skos:definition xml:lang="en">"Chronological records of significant events, as of the life or development of a people, country, or institution, often with an explanation of the causes."  <![CDATA[<a href="#cwrc:db2f8571-a773-4068-a35f-34262950bb8f">(Getty, 2017)</a>]]></skos:definition>
    <rdfs:label xml:lang="fr">histoire</rdfs:label>
  </genre:HistoricalGenre>
  <genre:ThematicGenre rdf:about="#regional">
    <rdfs:comment xml:lang="en">Encyclopédie du Canada</rdfs:comment>
    <skos:definition xml:lang="en">Regional writing reflects the details of a specific region, whether in prose or poetry. Regionalism is often associated with rural areas and "local colour", and often allied with realism insofar as it seeks to distinguish one region clearly from others. At its best, as when practiced by Thomas Hardy, William Faulkner, Sara Jeannette Duncan, or Margaret Laurence, regionalism conveys not merely the superficialities or prosaic details of an area but a profound sense of the impact of place on individual characters and destinies.</skos:definition>
    <rdfs:isDefinedBy rdf:resource="http://sparql.cwrc.ca/ontologies/genre-ONTOLOGY_DATE"/>
    <rdfs:label xml:lang="en">regional</rdfs:label>
    <rdfs:label xml:lang="fr">littérature régionale</rdfs:label>
    <dcterms:references rdf:resource="http://www.encyclopediecanadienne.ca/fr/article/regionalisme-dans-la-litterature/"/>
    <skos:definition xml:lang="fr">La littérature régionale au sens strict se rattache aux conventions du réalisme parce qu'elle tente de distinguer avec précision les caractéristiques d'une région clairement définissable, soit une région rurale ou encore étroitement liée à la terre. Comme le montrent les oeuvres de Thomas Hardy, de William Faulkner, de Sara Jeannette Duncan, et de Margaret Laurence de ce type de littérature régionale, dans sa forme la plus accomplie, n'est pas synonyme de détails superficiels ou de style prosaïque mais plutôt d'une exploration profonde de l'influence qu'exercent des régions particulières dans le destin d'individus précis.</skos:definition>
  </genre:ThematicGenre>
  <genre:ReligiousGenre rdf:about="#religious">
    <rdfs:label xml:lang="fr">religieux</rdfs:label>
    <skos:definition xml:lang="en">Writing dealing with religion or spirituality.</skos:definition>
    <rdfs:isDefinedBy rdf:resource="http://sparql.cwrc.ca/ontologies/genre-ONTOLOGY_DATE"/>
    <rdfs:label xml:lang="en">religious</rdfs:label>
    <skos:definition xml:lang="fr">Écrits traitent de la religion ou de la spiritualité.</skos:definition>
  </genre:ReligiousGenre>
  <genre:PoeticGenre rdf:about="#epyllion">
    <rdfs:label xml:lang="fr">epyllion</rdfs:label>
    <rdfs:isDefinedBy rdf:resource="http://sparql.cwrc.ca/ontologies/genre-ONTOLOGY_DATE"/>
    <rdfs:label xml:lang="en">epyllion</rdfs:label>
    <skos:definition xml:lang="en">"Brief narrative poems in dactylic hexameter of ancient Greece, imitated by Romans and others. Usually dealing with mythological and romantic themes. They are characterized by lively description, miniaturistic attitude, scholarly allusion, and an elevated tone similar to that of the elegy."  <![CDATA[<a href="#cwrc:db2f8571-a773-4068-a35f-34262950bb8f">(Getty, 2017)</a>]]></skos:definition>
    <owl:sameAs rdf:resource="http://vocab.getty.edu/aat/300410360"/>
    <rdfs:comment xml:lang="en">This term and its description were created from data gathered from DBpedia.</rdfs:comment>
    <skos:definition xml:lang="fr">«Un épyllion (en grec ancien ἐπύλλιον / epúllion diminutif de ἔπος / épos [« parole » racine d'ἐποποιία / epopoiía : « épopée »]) est, dans la littérature grecque et latine, une épopée très brève. C'est un poème narratif de quelques centaines d'hexamètres portant généralement sur la vie d'un héros ou d'une héroïne mythique et plus particulièrement sur ses amours.»  <![CDATA[<a href="#cwrc:727d97bc-af78-4122-94be-aa78b2e97d5a">(DBpedia, 2017)</a>]]></skos:definition>
  </genre:PoeticGenre>
  <genre:DidacticGenre rdf:about="#sageWriting">
    <rdfs:comment xml:lang="en">The description for this term is indebted to DBpedia. </rdfs:comment>
    <owl:sameAs rdf:resource="http://dbpedia.org/resource/Sage_writing"/>
    <skos:definition xml:lang="en">"Sage writing was a genre of creative nonfiction popular in the Victorian era. The concept originates with John Holloway's 1953 book The Victorian Sage: Studies in Argument. Sage writing is a development from ancient wisdom literature in which the writer chastises and instructs the reader about contemporary social issues, often utilizing discourses of philosophy, history, politics, and economics in non-technical ways. Prominent examples of the genre include writings by Thomas Carlyle, Matthew Arnold, John Ruskin, and Henry David Thoreau. Some 20th-century writers, such as Joan Didion and New Journalists such as Norman Mailer and Tom Wolfe, have also been identified as sage writers."  <![CDATA[<a href="#cwrc:727d97bc-af78-4122-94be-aa78b2e97d5a">(DBpedia, 2017)</a>]]></skos:definition>
    <rdfs:isDefinedBy rdf:resource="http://sparql.cwrc.ca/ontologies/genre-ONTOLOGY_DATE"/>
    <rdfs:label xml:lang="en">sage writing</rdfs:label>
    <rdfs:label xml:lang="fr">sage writing</rdfs:label>
    <skos:definition xml:lang="fr">Le "sage writing" était un genre non fictionel populaire à l'ère victorienne. Son nom vient de de John Holloway paru en 1953, The Victorian Sage: Studies in Argument. Le "sage writing" s'inspire de la littérature de sagesse antique dans laquelle l'auteur donne des leçons et des enseignements à son lecteur concernant des questions sociales contemporaines, souvent en utilisant dans un style accessible et non savant les discours philosophiques, historiques, politiques et et économiques. Les représentants les plus connus du "sage writing" sont Thomas Carlyle, Matthew Arnold, John Ruskin et Henry David Thoreau. Certains écrivains du 20ème siècle comme Joan Didion et les New Journalists Norman Mailer et Tom Wolfe sont également considérés comme appartenant à ce genre.</skos:definition>
  </genre:DidacticGenre>
  <genre:FictionalGenre rdf:about="#picaresque">
    <rdfs:isDefinedBy rdf:resource="http://sparql.cwrc.ca/ontologies/genre-ONTOLOGY_DATE"/>
    <rdfs:label xml:lang="en">picaresque</rdfs:label>
    <owl:sameAs rdf:resource="http://id.loc.gov/authorities/genreForms/gf2014026479"/>
    <owl:sameAs rdf:resource="http://dbpedia.org/resource/Picaresque_novel"/>
    <rdfs:comment xml:lang="en">The description for this term is indebted to DBpedia. </rdfs:comment>
    <skos:definition xml:lang="fr">«Le roman picaresque (de l'espagnol pícaro, « misérable », « futé ») est un genre littéraire né en Espagne au XVIe siècle et qui a connu sa plus florissante époque dans ce pays. Un roman picaresque se compose d'un récit sur le mode autobiographique de l’histoire de héros miséreux, généralement des jeunes gens vivant en marge de la société et à ses dépens. Au cours d’aventures souvent extravagantes supposées plus pittoresques et surtout plus variées que celles des honnêtes gens, qui sont autant de prétextes à présenter des tableaux de la vie vulgaire et des scènes de mœurs, le héros entre en contact avec toutes les couches de la société.»  <![CDATA[<a href="#cwrc:727d97bc-af78-4122-94be-aa78b2e97d5a">(DBpedia, 2017)</a>]]></skos:definition>
    <skos:definition xml:lang="en">"The picaresque novel (Spanish: "picaresca," from "pícaro," for "rogue" or "rascal") is a genre of prose fiction which depicts the adventures of a roguish hero of low social class who lives by his wits in a corrupt society. Picaresque novels typically adopt a realistic style, with elements of comedy and satire. This style of novel originated in 16th-century Spain and flourished throughout Europe in the 17th and 18th centuries. It continues to influence modern literature. According to the traditional view of Thrall and Hibbard (first published in 1936), seven qualities distinguish the picaresque novel or narrative form, all or some of which may be employed for effect by the author. (1) A picaresque narrative is usually written in first person as an autobiographical account. (2) The main character is often of low character or social class. He or she gets by with wit and rarely deigns to hold a job. (3) There is no plot. The story is told in a series of loosely connected adventures or episodes. (4) There is little if any character development in the main character. Once a picaro, always a picaro. His or her circumstances may change but they rarely result in a change of heart. (5) The picaro's story is told with a plainness of language or realism. (6) Satire might sometimes be a prominent element. (7) The behavior of a picaresque hero or heroine stops just short of criminality. Carefree or immoral rascality positions the picaresque hero as a sympathetic outsider, untouched by the false rules of society. However, Trall and Hibbert's thesis has been questioned by scholars[specify] interested in how genre functions, rather than how it looks on the surface."  <![CDATA[<a href="#cwrc:727d97bc-af78-4122-94be-aa78b2e97d5a">(DBpedia, 2017)</a>]]></skos:definition>
  </genre:FictionalGenre>
  <genre:NarrativeGenre rdf:about="#legend">
    <skos:definition xml:lang="en">"Stories handed down by tradition from earlier times, usually concerned with a real person, place, or event, and popularly regarded as historical although not entirely verifiable." <![CDATA[<a href="#cwrc:a0414fff-d3ba-4d20-9d13-623b4ddc077f">(Getty, 2022)</a>]]></skos:definition>
    <rdfs:comment xml:lang="en">The description for this term is indebted to the Getty Art &amp; Architecture Thesaurus.</rdfs:comment>
    <owl:sameAs rdf:resource="http://vocab.getty.edu/aat/300055923"/>
    <skos:altLabel xml:lang="en">folktale</skos:altLabel>
    <rdfs:isDefinedBy rdf:resource="http://sparql.cwrc.ca/ontologies/genre-ONTOLOGY_DATE"/>
    <rdfs:label xml:lang="en">legend</rdfs:label>
  </genre:NarrativeGenre>
  <genre:DramaticGenre rdf:about="#guerillaTheatre">
    <rdfs:isDefinedBy rdf:resource="http://sparql.cwrc.ca/ontologies/genre-ONTOLOGY_DATE"/>
    <rdfs:label xml:lang="en">guerilla theatre</rdfs:label>
    <skos:definition xml:lang="en">"Guerrilla theatre, generally rendered "guerrilla theater" in the US, is a form of guerrilla communication originated in 1965 by the San Francisco Mime Troupe, who, in spirit of the Che Guevara writings from which the term guerrilla is taken, engaged in performances in public places committed to "revolutionary sociopolitical change." The group performances, aimed against the Vietnam war and capitalism, sometimes contained nudity, profanity and taboo subjects that were shocking to some members of the audiences of the time. Guerrilla (Spanish for "little war"), as applied to theatrical events, describes the act of spontaneous, surprise performances in unlikely public spaces to an unsuspecting audience. Typically these performances intend to draw attention to a political/social issue through satire, protest, and carnivalesque techniques. Many of these performances were a direct result of the radical social movements of the late 1960s through mid-1970s. Guerrilla Theater, also referred to as guerrilla performance, has been sometimes related to the agitprop theater of the 1930s, but it is differentiated from agitprop by the inclusion of Dada performance tactics." <![CDATA[<a href="#cwrc:727d97bc-af78-4122-94be-aa78b2e97d5a">(DBpedia, 2019)</a>]]></skos:definition>
  </genre:DramaticGenre>
  <genre:PoliticalGenre rdf:about="#petition">
    <skos:definition xml:lang="fr">«Le droit de pétition est le droit accordé aux populations de faire une demande directe au souverain, ou au représentant de l'exécutif. Par extension, il est possible de faire une pétition envers toute personne morale disposant d'un pouvoir. Une pétition se présente le plus souvent sous la forme d'un ensemble de signatures au bas d'un texte. Ces signatures sont généralement recueillies dans la rue par des volontaires. Avec l'arrivée d'Internet, un certain nombre de sites permettent d'organiser une pétition et de recueillir les signatures en ligne.»  <![CDATA[<a href="#cwrc:727d97bc-af78-4122-94be-aa78b2e97d5a">(DBpedia, 2017)</a>]]></skos:definition>
    <rdfs:isDefinedBy rdf:resource="http://sparql.cwrc.ca/ontologies/genre-ONTOLOGY_DATE"/>
    <rdfs:label xml:lang="en">petition</rdfs:label>
    <skos:definition xml:lang="en">"Includes any written requests and lists of signatures submitted to an authority to appeal for the performance of specific action."  <![CDATA[<a href="#cwrc:db2f8571-a773-4068-a35f-34262950bb8f">(Getty, 2017)</a>]]></skos:definition>
    <skos:related rdf:resource="http://id.loc.gov/authorities/genreForms/gf2011026358"/>
    <rdfs:label xml:lang="fr">pétition</rdfs:label>
    <owl:sameAs rdf:resource="http://vocab.getty.edu/aat/300027219"/>
    <rdfs:comment xml:lang="en">The description for this term is indebted to the Getty Art &amp; Architecture Thesaurus.</rdfs:comment>
  </genre:PoliticalGenre>
  <genre:ProverbForm rdf:about="#proverb">
    <rdfs:isDefinedBy rdf:resource="http://sparql.cwrc.ca/ontologies/genre-ONTOLOGY_DATE"/>
    <rdfs:label xml:lang="en">proverb</rdfs:label>
    <skos:definition xml:lang="en">"A proverb (from Latin: proverbium) is a simple and concrete saying, popularly known and repeated, that expresses a truth based on common sense or experience. They are often metaphorical. A proverb that describes a basic rule of conduct may also be known as a maxim. Proverbs fall into the category of formulaic language. Proverbs are often borrowed from similar languages and cultures, and sometimes come down to the present through more than one language. Both the Bible (including, but not limited to the Book of Proverbs) and medieval Latin (aided by the work of Erasmus) have played a considerable role in distributing proverbs across Europe. Mieder has concluded that cultures that treat the Bible as their "major spiritual book contain between three hundred and five hundred proverbs that stem from the Bible." However, almost every culture has examples of its own unique proverbs." <![CDATA[<a href="#cwrc:727d97bc-af78-4122-94be-aa78b2e97d5a">(DBpedia, 2019)</a>]]></skos:definition>
  </genre:ProverbForm>
  <genre:DramaticGenre rdf:about="#kitchenSinkDrama">
    <skos:definition xml:lang="en">"Originating in Britain in the 1950s, realistic drama centred on the domestic lives of working-class characters."  <![CDATA[<a href="#cwrc:4c227091-6bf0-4325-b846-9733fae19e61">(Oxford, 2015)</a>]]></skos:definition>
    <dcterms:references rdf:resource="http://www.oxfordreference.com/view/10.1093/acref/9780199208272.001.0001/acref-9780199208272-e-629?rskey=HtykbC%26result=621"/>
    <skos:definition xml:lang="fr">Drame réaliste centré sur la vie domestique de personnages de la classe ouvrière, apparu en Angleterre dans les années 50.</skos:definition>
    <rdfs:comment xml:lang="en">This term and its description were created from data gathered from the Oxford Dictionary of Literary Terms, 4th ed.</rdfs:comment>
    <rdfs:label xml:lang="fr">kitchen sink drama</rdfs:label>
    <rdfs:isDefinedBy rdf:resource="http://sparql.cwrc.ca/ontologies/genre-ONTOLOGY_DATE"/>
    <rdfs:label xml:lang="en">kitchen sink drama</rdfs:label>
  </genre:DramaticGenre>
  <genre:DramaticGenre rdf:about="#pageant">
    <skos:definition xml:lang="fr">Divertissements, souvent représentés en plein air, illustrant des thèmes sous forme de spectacles plutôt que par une trame narrative continue.</skos:definition>
    <owl:sameAs rdf:resource="http://vocab.getty.edu/aat/300069240"/>
    <skos:definition xml:lang="en">"Entertainments, frequently held in the open air, illustrating themes by means of spectacle rather than by consecutive narrative and dramatic characterization."  <![CDATA[<a href="#cwrc:db2f8571-a773-4068-a35f-34262950bb8f">(Getty, 2017)</a>]]></skos:definition>
    <rdfs:isDefinedBy rdf:resource="http://sparql.cwrc.ca/ontologies/genre-ONTOLOGY_DATE"/>
    <rdfs:label xml:lang="en">pageant</rdfs:label>
    <rdfs:label xml:lang="fr">procession</rdfs:label>
    <rdfs:comment xml:lang="en">This term and its description were created from data gathered from the Getty Art &amp; Architecture Thesaurus.</rdfs:comment>
    <owl:sameAs rdf:resource="http://id.loc.gov/authorities/genreForms/gf2014026464"/>
  </genre:DramaticGenre>
  <genre:ScholarlyGenre rdf:about="#scholarlyWriting">
    <rdfs:isDefinedBy rdf:resource="http://sparql.cwrc.ca/ontologies/genre-ONTOLOGY_DATE"/>
    <rdfs:label xml:lang="en">scholarly writing</rdfs:label>
    <skos:definition xml:lang="fr">Travaux écrits d'un intellectuel, amateur ou professionnel, normalement centré sur un domain ou un sujet spécifique dans lequel l'auteure est experte.</skos:definition>
    <rdfs:label xml:lang="fr">érudition</rdfs:label>
    <skos:definition xml:lang="en">Writing by a scholar, either amateur or professional, typically focused on a specific field or topic in which the author is an expert.</skos:definition>
    <skos:altLabel xml:lang="en">academic writing</skos:altLabel>
  </genre:ScholarlyGenre>
  <genre:DramaticGenre rdf:about="#tragicomedy">
    <rdfs:comment xml:lang="en">The description for this term is indebted to DBpedia. </rdfs:comment>
    <owl:sameAs rdf:resource="http://id.loc.gov/authorities/genreForms/gf2014026577"/>
    <skos:definition xml:lang="fr">«La tragi-comédie est une forme théâtrale caractérisée par une action romanesque, des personnages de haute extraction, un dénouement heureux et un refus des règles de la tragédie. Le terme est apparu en France chez le dramaturge Robert Garnier vers la fin du XVIe siècle, orthographié tragecomedie ; le terme nous vient de Plaute, qui désigne son Amphitryon comme une "tragi-comoedia" (au vers 59). Ce genre a connu un très grand succès en France dans les années 1630-1640. Il est assez difficile de définir les limites de la tragi-comédie à cette époque parce que les auteurs revendiquaient le refus de toute règle. On pouvait alors voir dans la tragi-comédie une sorte de tragédie à fin heureuse parce que la tragédie n'était définie que par son personnel noble et mythologique. Dans les années 1640, les partisans d'un théâtre beaucoup plus normé prennent de plus en plus d'importance et la tragédie répondant aux règles classiques prend le dessus sur la tragi-comédie. Le cas du Le Cid de Corneille est un exemple intéressant à cet égard car il a été publié en 1637 en tant que tragi-comédie et requalifié en tragédie dès 1648 alors que Corneille n'avait pas encore effectué de modification majeure de la pièce. On peut donc considérer que ce n'est pas la pièce mais la perception qu'on avait des différents genres théâtraux qui a évolué entre ces deux dates. En effet, l'intrigue du Cid comporte de nombreux éléments caractéristiques d'une tragi-comédie : il raconte une histoire d'amour dans laquelle un obstacle empêche à un moment donné la réunion des deux amants. À la fin de la pièce, cet obstacle sera levé et le dénouement sera heureux et nuptial ce qui est à l'époque une caractéristique des comédies et des tragi-comédies. La Querelle du Cid aura contribué à fixer les règles de la tragédie même si Le Cid conserve ses caractéristiques à savoir l'accumulation des événements , les coups de théâtre, les changements de décor successif et le dénouement heureux. On a beaucoup reproché à Corneille l'invraisemblance de la fin et un respect très discutable des trois unités. De fait, même s'il est déjà influencé par les règles qui commencent à s'imposer à la fin des années 1630, Corneille conserve dans cette pièce une liberté de composition héritée de la tragi-comédie et que l'on ne trouvera plus dans ses tragédies ultérieures. Pour autant, la pièce annonce la dramaturgie classique parce que les conflits omniprésents qui la constituent ne se manifestent pas à travers de combats spectaculaires sur scène mais à travers le travail du langage. Ainsi le duel entre Rodrigue et Don Gomes s'achève très vite alors que les célébrissimes stances du Cid rendent compte longuement du conflit intérieur qui travaille Rodrigue. Ce refus du spectaculaire au profit d'un travail sur le discours et les sentiments des personnages sera caractéristique de l'esthétique classique et explique que le Cid en soit resté un exemple majeur alors qu'il est encore très influencé par le genre de la tragi-comédie qui s'oppose aux caractéristiques de l'écriture classique. Philippe Quinault , poète et librettiste français, a aussi contribué au succès de ce genre en participant à la création de la tragédie-ballet Psyché en 1671 écrit par Molière aidé de Corneille. Le mélange des genres fut peu représenté par la suite dans le théâtre français, tout au plus trouve-t-on des pièces ou les genres s'alternent sans se mêler. Victor Hugo tente pourtant d'imposer avec son théâtre romantique une écriture entre sublime et grotesque, mais il faudra attendre le XXe siècle et le théâtre de l'absurde pour que le public accepte de concevoir que le rire ne nuit pas obligatoirement à la profondeur dramatique.»  <![CDATA[<a href="#cwrc:727d97bc-af78-4122-94be-aa78b2e97d5a">(DBpedia, 2017)</a>]]></skos:definition>
    <dcterms:references rdf:resource="http://web.cn.edu/kwheeler/lit_terms_t.html"/>
    <skos:definition xml:lang="en">"Tragicomedy is a literary genre that blends aspects of both tragic and comic forms. Most often seen in dramatic literature, the term can variously describe either a tragic play which contains enough comic elements to lighten the overall mood or a serious play with a happy ending."  <![CDATA[<a href="#cwrc:727d97bc-af78-4122-94be-aa78b2e97d5a">(DBpedia, 2017)</a>]]></skos:definition>
    <rdfs:isDefinedBy rdf:resource="http://sparql.cwrc.ca/ontologies/genre-ONTOLOGY_DATE"/>
    <rdfs:label xml:lang="en">tragicomedy</rdfs:label>
  </genre:DramaticGenre>
  <genre:PoeticGenre rdf:about="#heroic">
    <skos:definition xml:lang="en">"Form of poetry comprising long narratives celebrating on a grand scale the adventures and deeds of one or more heroic figures, ordinarily concerning a serious subject significant to a culture or nation. Classical epic poetry employs dactylic hexameter and recounts a journey."  <![CDATA[<a href="#cwrc:db2f8571-a773-4068-a35f-34262950bb8f">(Getty, 2017)</a>]]></skos:definition>
    <rdfs:label xml:lang="fr">poème épique</rdfs:label>
    <skos:related rdf:resource="http://id.loc.gov/authorities/genreForms/gf2014026310"/>
    <owl:sameAs rdf:resource="http://vocab.getty.edu/aat/300404208"/>
    <skos:definition xml:lang="fr">Forme de poésie qui présente de longs récits célébrant les aventures et les actes d'une ou plusieurs figures héroïques, d'ordinaire concernant un sujet sérieux important pour une culture ou une nation. La poésie épique classique emploie l'hexamètre dactylique et raconte un voyage.</skos:definition>
    <rdfs:isDefinedBy rdf:resource="http://sparql.cwrc.ca/ontologies/genre-ONTOLOGY_DATE"/>
    <rdfs:label xml:lang="en">heroic</rdfs:label>
    <rdfs:comment xml:lang="en">The description for this term is indebted to the Getty Art &amp; Architecture Thesaurus.</rdfs:comment>
  </genre:PoeticGenre>
  <genre:FictionalGenre rdf:about="#animalStory">
    <skos:definition xml:lang="en">"Literary works in which an animal or animals are the primary characters." <![CDATA[<a href="#cwrc:bd595bc4-5991-4c51-98d9-9ab52c416f4f">(Getty, 2021)</a>]]></skos:definition>
    <rdfs:comment xml:lang="en">The description for this term is indebted to the Getty Art &amp; Architecture Thesaurus.</rdfs:comment>
    <owl:sameAs rdf:resource="http://vocab.getty.edu/aat/300254800"/>
    <rdfs:isDefinedBy rdf:resource="http://sparql.cwrc.ca/ontologies/genre-ONTOLOGY_DATE"/>
    <rdfs:label xml:lang="en">animal story</rdfs:label>
  </genre:FictionalGenre>
  <genre:IllustratedForm rdf:about="#comicbook">
    <skos:definition xml:lang="en">"Sequence of illustrations containing a story or stories (called "comics," because some are humorous), often serialized, published in booklet form."  <![CDATA[<a href="#cwrc:db2f8571-a773-4068-a35f-34262950bb8f">(Getty, 2017)</a>]]></skos:definition>
    <rdfs:comment xml:lang="en">The description for this term is indebted to the Getty Art &amp; Architecture Thesaurus.</rdfs:comment>
    <owl:sameAs rdf:resource="http://vocab.getty.edu/aat/300203177"/>
    <rdfs:isDefinedBy rdf:resource="http://sparql.cwrc.ca/ontologies/genre-ONTOLOGY_DATE"/>
    <rdfs:label xml:lang="en">comicbook</rdfs:label>
    <rdfs:label xml:lang="fr">bande dessinée</rdfs:label>
    <skos:definition xml:lang="fr">" Séquence d'illustrations contenant une ou des histoires (appelées «comics», car certaines sont humoristiques), souvent sérialisées et publiées sous forme de brochure." </skos:definition>
    <owl:sameAs rdf:resource="http://id.loc.gov/authorities/genreForms/gf2014026266"/>
  </genre:IllustratedForm>
  <genre:DramaticGenre rdf:about="#pantomime">
    <skos:definition xml:lang="fr">Jeu, art du pantomime; technique d'expression dramatique suivant laquelle les situations, les sentiments, les idées sont rendus par des attitudes, des gestes, des jeux de physionomie, sans recours à la parole.</skos:definition>
    <owl:sameAs rdf:resource="https://dvlf.uchicago.edu/mot/pantomime"/>
    <rdfs:comment xml:lang="en">This term and its description were created from data gathered from DBpedia.</rdfs:comment>
    <skos:related rdf:resource="http://id.loc.gov/authorities/genreForms/gf2018026117"/>
    <skos:definition xml:lang="en">"Pantomime (informally panto) is a type of musical comedy stage production, designed for family entertainment. It was developed in England and is still performed there, generally during the Christmas and New Year season and, to a lesser extent, in other English-speaking countries. Modern pantomime includes songs, slapstick comedy and dancing, employs gender-crossing actors, and combines topical humour with a story loosely based on a well-known fairy tale, fable or folk tale. It is a participatory form of theatre, in which the audience is expected to sing along with certain parts of the music and shout out phrases to the performers."  <![CDATA[<a href="#cwrc:727d97bc-af78-4122-94be-aa78b2e97d5a">(DBpedia, 2017)</a>]]></skos:definition>
    <rdfs:isDefinedBy rdf:resource="http://sparql.cwrc.ca/ontologies/genre-ONTOLOGY_DATE"/>
    <rdfs:label xml:lang="en">pantomime</rdfs:label>
    <rdfs:label xml:lang="fr">pantomime</rdfs:label>
  </genre:DramaticGenre>
  <genre:CalendarForm rdf:about="#almanac">
    <skos:definition xml:lang="en">"Publications, usually annuals, containing a variety of useful facts of miscellaneous nature, or statistical information; originally included projections of coming days, months, and holidays." <![CDATA[<a href="#cwrc:bd595bc4-5991-4c51-98d9-9ab52c416f4f">(Getty, 2021)</a>]]></skos:definition>
    <rdfs:comment xml:lang="en">The description for this term is indebted to the Getty Art &amp; Architecture Thesaurus.</rdfs:comment>
    <owl:sameAs rdf:resource="http://vocab.getty.edu/aat/300026705"/> 
    <rdfs:isDefinedBy rdf:resource="http://sparql.cwrc.ca/ontologies/genre-ONTOLOGY_DATE"/>
    <rdfs:label xml:lang="en">almanac</rdfs:label>
  </genre:CalendarForm>
  <genre:PerformanceMedium rdf:about="#physicalTheatre">
    <skos:definition xml:lang="en">"Physical theater is a genre of theatrical performance that pursues storytelling through primarily physical means. Several performance traditions all describe themselves as "physical theater", but the unifying aspect is a reliance on physical motion of the performers rather than or combined with text to convey the story. In a basic sense, you talk through hand gestures, body language, thought track and many more physical features." <![CDATA[<a href="#cwrc:727d97bc-af78-4122-94be-aa78b2e97d5a">(DBpedia, 2019)</a>]]></skos:definition>
    <rdfs:isDefinedBy rdf:resource="http://sparql.cwrc.ca/ontologies/genre-ONTOLOGY_DATE"/>
    <rdfs:label xml:lang="en">physical theatre</rdfs:label>
  </genre:PerformanceMedium>
  <genre:DidacticGenre rdf:about="#didactic">
    <skos:definition xml:lang="fr">Écrits "moralisateurs" ou qui cherchent ouvertement à convaincre le lecteur en lui offrant une leçon. Les homélies médiévales et les essais moraux victoriens sont souvent considérés comme des exemples de la littérature didactique, mais on peut prétendre que toute littérature est didactique d'une façon ou d'une autre, car la parole écrite implique ou suggère fréquemment une prise de position autoriale. Parfois, la leçon est manifestement religieuse, comme dans le cas des sermons, ou en littérature comme pour  Le Paradis perdu de Milton, qui cherche à "justifier les voies de Dieu envers les hommes". D'une manière plus subtile, une grande partie de la littérature romantique suggère une critique de la vie urbaine et mécanisée de Londres au 19ème siècle.</skos:definition>
    <rdfs:label xml:lang="fr">ouvrage didactique</rdfs:label>
    <rdfs:isDefinedBy rdf:resource="http://sparql.cwrc.ca/ontologies/genre-ONTOLOGY_DATE"/>
    <rdfs:label xml:lang="en">didactic</rdfs:label>
    <dcterms:references rdf:resource="http://web.cn.edu/kwheeler/lit_terms_d.html"/>
    <rdfs:comment xml:lang="en">The description for this term is indebted to Dr. L. Kip Wheeler of Carson-Newman University. </rdfs:comment>
    <skos:definition xml:lang="en">"Writing that is "preachy" or seeks overtly to convince a reader of a particular point or lesson. Medieval homilies and Victorian moral essays are often held up as examples of didactic literature, but one might argue that all literature is didactic to one extent or another since the written word frequently implies or suggests an authorial attitude. Sometimes, the lesson is overtly religious, as in the case of sermons or in literature like Milton's Paradise Lost, which seeks to "justify God's ways to men." In a more subtle way, much of Romantic literature hints at a critique of urbanized and mechanized life in 19th-century London."  <![CDATA[<a href="cwrc:509015ff-7641-473e-94c5-688e06952bb7">(L. K Wheeler, 2017)</a>]]></skos:definition>
  </genre:DidacticGenre>
  <genre:DramaticGenre rdf:about="#afterpiece">
    <rdfs:label xml:lang="fr">afterpiece</rdfs:label>
    <rdfs:isDefinedBy rdf:resource="http://sparql.cwrc.ca/ontologies/genre-ONTOLOGY_DATE"/>
    <rdfs:label xml:lang="en">afterpiece</rdfs:label>
    <rdfs:comment xml:lang="en">This term and its description were created from data gathered from the Penguin Dictionary of Literary Terms &amp; Literary Theory, 4th ed.</rdfs:comment>
    <skos:definition xml:lang="en">"A short drama performed after a main play, popularized in the 1700s as justification for a new half-price entrance fee charged to latecomers. Typically a comedic one-act, regardless of the genre of the preceding play."  <![CDATA[<a href="#cwrc:2f09376c-f784-4a46-9f04-5a21aa311f27">(Penguin, 1999)</a>]]></skos:definition>
    <skos:definition xml:lang="fr">Courte pièce de théâtre représentée à la suite d'une pièce principale, rendue populaire au 18ᵉ siècle afin de justifier pour un supplément s'élevant à la moitié du prix d'entrée qui était facturé aux retardataires. L'afterpiece était généralement une comédie en un acte sans relation avec le genre de la pièce qui précédait.</skos:definition>
  </genre:DramaticGenre>
  <genre:ChildrensLiteratureGenre rdf:about="#childrensLiterature">
    <rdfs:label xml:lang="fr">littérature de jeunesse</rdfs:label>
    <skos:definition xml:lang="fr">"Littérature écrite et publiée pour les enfants." </skos:definition>
    <rdfs:comment xml:lang="en">The description for this term is indebted to the Getty Art &amp; Architecture Thesaurus.</rdfs:comment>
    <rdfs:isDefinedBy rdf:resource="http://sparql.cwrc.ca/ontologies/genre-ONTOLOGY_DATE"/>
    <rdfs:label xml:lang="en">childrens literature</rdfs:label>
    <skos:definition xml:lang="en">"Literature written and published for children."  <![CDATA[<a href="#cwrc:db2f8571-a773-4068-a35f-34262950bb8f">(Getty, 2017)</a>]]></skos:definition>
    <owl:sameAs rdf:resource="http://vocab.getty.edu/aat/300263209"/>
    <skos:closeMatch rdf:resource="https://sparql.cwrc.ca/ontologies/genre.html#juvenile"/>
    <skos:broader rdf:resource="http://sparql.cwrc.ca/ontologies/genre.html#theatreForYoungAudiences"/>
  </genre:ChildrensLiteratureGenre>
  <genre:ThematicGenre rdf:about="#seaStory">
    <rdfs:isDefinedBy rdf:resource="http://sparql.cwrc.ca/ontologies/genre-ONTOLOGY_DATE"/>
    <rdfs:label xml:lang="en">sea story</rdfs:label>
    <skos:definition xml:lang="en">"Nautical fiction, frequently also naval fiction, sea fiction, naval adventure fiction or maritime fiction, is a genre of literature with a setting on or near the sea, that focuses on the human relationship to the sea and sea voyages and highlights nautical culture in these environments. The settings of nautical fiction vary greatly, including merchant ships, liners, naval ships, fishing vessels, life boats, etc., along with sea ports and fishing villages. When describing nautical fiction, scholars most frequently refer to novels, novellas, and short stories, sometimes under the name of sea novels or sea stories. These works are sometimes adapted for the theatre, film and television. The development of nautical fiction follows with the development of the English language novel and while the tradition is mainly British and North American, there are also significant works from literatures in Japan, France, Scandinavia, and other Western traditions. Though the treatment of themes and settings related to the sea and maritime culture is common throughout the history of western literature, nautical fiction, as a distinct genre, was first pioneered by James Fenimore Cooper (The Pilot, 1824) and Frederick Marryat (Frank Mildmay, 1829 and Mr Midshipman Easy 1836) at the beginning of the 19th century. There were 18th century and earlier precursors that have nautical settings, but few are as richly developed as subsequent works in this genre. The genre has evolved to include notable literary works like Herman Melville's Moby Dick (1851), Joseph Conrad's Lord Jim (1899–1900), popular fiction like C.S. Forester's Hornblower series (1937–67), and works by authors that straddle the divide between popular and literary fiction, like Patrick O'Brian's Aubrey-Maturin series (1970–2004). Because of the historical dominance of nautical culture by men, they are usually the central characters, except for works that feature ships carrying women passengers. For this reason, nautical fiction is often marketed for men. Nautical fiction usually includes distinctive themes, such as a focus on masculinity and heroism, investigations of social hierarchies, and the psychological struggles of the individual in the hostile environment of the sea. Stylistically, readers of the genre expect an emphasis on adventure, accurate representation of maritime culture, and use of nautical language. Works of nautical fiction often include elements overlapping with other genres, including historical fiction, adventure fiction, war fiction, children's literature, travel narratives (such as the Robinsonade), the social problem novel and psychological fiction." <![CDATA[<a href="#cwrc:727d97bc-af78-4122-94be-aa78b2e97d5a">(DBpedia, 2019)</a>]]></skos:definition>
  </genre:ThematicGenre>
  <genre:JournalForm rdf:about="#newspaper">
    <rdfs:isDefinedBy rdf:resource="http://sparql.cwrc.ca/ontologies/genre-ONTOLOGY_DATE"/>
    <rdfs:label xml:lang="en">newspaper</rdfs:label>
    <skos:definition xml:lang="en">"A newspaper is a serial publication containing news, other informative articles (), and advertising. A newspaper is usually but not exclusively printed on relatively inexpensive, low-grade paper such as newsprint. The news organizations that publish newspapers are themselves often metonymically called newspapers. Most newspapers are now published online as well as in print. The online versions are called online newspapers or news sites. Newspapers are typically published daily or weekly. News magazines are also weekly, but they have a magazine format. General-interest newspapers typically publish news articles and feature articles on national and international news as well as local news. The news includes political events and personalities, business and finance, crime, severe weather, and natural disasters; health and medicine, science, and technology; sports; and entertainment, society, food and cooking, clothing and home fashion, and the arts. Typically the paper is divided into sections for each of those major groupings (labeled A, B, C, and so on, with pagination prefixes yielding page numbers A1-A20, B1-B20, C1-C20, and so on). Most traditional papers also feature an editorial page containing editorials written by an editor, op-eds written by guest writers, and columns that express the personal opinions of columnists, usually offering analysis and synthesis that attempts to translate the raw data of the news into information telling the reader "what it all means" and persuading them to concur. A wide variety of material has been published in newspapers. Besides the aforementioned news and opinions, they include weather forecasts; criticism and reviews of the arts (including literature, film, television, theater, fine arts, and architecture) and of local services such as restaurants; obituaries; entertainment features such as crosswords, horoscopes, editorial cartoons, gag cartoons, and comic strips; advice, food, and other columns; and radio and television listings (program schedules). Most newspapers are businesses, and they pay their expenses (such as journalists' wages, printing costs, and distribution costs) with a mixture of subscription revenue, newsstand sales, and advertising revenue (other businesses or individuals pay to place advertisements in the pages, including display ads, classified ads, and their online equivalents). Some newspapers are government-run or at least government-funded; their reliance on advertising revenue and on profitability is less critical to their survival. The editorial independence of a newspaper is thus always subject to the interests of someone, whether owners, advertisers, or a government. Some newspapers with high editorial independence, high journalism quality, and large circulation are viewed as newspapers of record. Many newspapers, besides employing journalists on their own payrolls, also subscribe to news agencies (wire services) (such as the Associated Press, Reuters, or Agence France-Presse), which employ journalists to find, assemble, and report the news, then sell the content to the various newspapers. This is a way to avoid duplicating the expense of reporting. Circa 2005, there were approximately 6,580 daily newspaper titles in the world selling 395 million print copies a day (in the U.S., 1,450 titles selling 55 million copies). The late 2000s–early 2010s global recession, combined with the rapid growth of free web-based alternatives, has helped cause a decline in advertising and circulation, as many papers had to retrench operations to increase profitability. The decline in advertising revenues affected both the print and online media as well as all other mediums; print advertising was once lucrative but has greatly declined, and the prices of online advertising are often lower than those of their print precursors. Besides remodeling advertising, the internet (especially the web) has also challenged the business models of the print-only era by democratizing and crowdsourcing both publishing in general (sharing information with others) and, more specifically, journalism (the work of finding, assembling, and reporting the news). In addition, the rise of news aggregators, which bundle linked articles from many online newspapers and other sources, influences the flow of web traffic. Increasing paywalling of online newspapers may be counteracting those effects." <![CDATA[<a href="#cwrc:727d97bc-af78-4122-94be-aa78b2e97d5a">(DBpedia, 2019)</a>]]></skos:definition>
    <skos:related rdf:resource="http://vocab.getty.edu/aat/300026656"/>
  </genre:JournalForm>
  <genre:IllustratedForm rdf:about="#illustrated">
    <skos:definition xml:lang="en">"Document containing drawings or other pictures intended to elucidate a description, story, or other written material." <![CDATA[<a href="#cwrc:bd595bc4-5991-4c51-98d9-9ab52c416f4f">(Getty, 2021)</a>]]></skos:definition>
    <rdfs:comment xml:lang="en">The description for this term is indebted to the Getty Art &amp; Architecture Thesaurus.</rdfs:comment>
    <rdfs:isDefinedBy rdf:resource="http://sparql.cwrc.ca/ontologies/genre-ONTOLOGY_DATE"/>
    <rdfs:label xml:lang="en">illustrated</rdfs:label>
  </genre:IllustratedForm>
  <genre:ComedicGenre rdf:about="#farce">
    <owl:sameAs rdf:resource="http://dbpedia.org/resource/Farce"/>
    <owl:sameAs rdf:resource="http://id.loc.gov/authorities/genreForms/gf2014026335"/>
    <rdfs:isDefinedBy rdf:resource="http://sparql.cwrc.ca/ontologies/genre-ONTOLOGY_DATE"/>
    <rdfs:label xml:lang="en">farce</rdfs:label>
    <skos:definition xml:lang="fr">«La farce est un genre théâtral né au Moyen Âge, qui a comme but de faire rire et qui a souvent des caractéristiques grossières. Son origine remonte à l'Antiquité gréco-romaine, et on en trouve déjà des traces chez Aristophane et Plaute, et surtout dans les atellanes latines.»  <![CDATA[<a href="#cwrc:727d97bc-af78-4122-94be-aa78b2e97d5a">(DBpedia, 2017)</a>]]></skos:definition>
    <rdfs:label xml:lang="fr">farce</rdfs:label>
    <skos:definition xml:lang="en">"(from Latin Farsus, "stuffed"): A farce is a form of low comedy designed to provoke laughter through highly exaggerated caricatures of people in improbable or silly situations. Traits of farce include (1) physical bustle such as slapstick, (2) sexual misunderstandings and mix-ups, and (3) broad verbal humor such as puns. Many literary critics (especially in the Victorian period) have tended to view farce as inferior to "high comedy" that involves brilliant dialogue. Many of Shakespeare's early works, such as The Taming of the Shrew, are considered farces. Contrast with comedy of manners."  <![CDATA[<a href="cwrc:509015ff-7641-473e-94c5-688e06952bb7">(L. K Wheeler, 2017)</a>]]></skos:definition>
    <skos:altLabel xml:lang="en">farce</skos:altLabel>
    <rdfs:comment xml:lang="en">The description for this term is indebted to Dr. L. Kip Wheeler of Carson-Newman University. </rdfs:comment>
  </genre:ComedicGenre>
  <genre:PoliticalGenre rdf:about="#manifesto">
    <rdfs:isDefinedBy rdf:resource="http://sparql.cwrc.ca/ontologies/genre-ONTOLOGY_DATE"/>
    <rdfs:label xml:lang="en">manifesto</rdfs:label>
    <rdfs:comment xml:lang="en">The description for this term is indebted to the Getty Art &amp; Architecture Thesaurus.</rdfs:comment>
    <rdfs:label xml:lang="fr">manifeste</rdfs:label>
    <skos:definition xml:lang="en">"Formal written declarations, promulgated by a sovereign or by the executive authority of a state or nation, such as to proclaim its reasons and motives for declaring a war, or other international action; also public declarations or proclamations of political, social, artistic, or other principles."  <![CDATA[<a href="#cwrc:db2f8571-a773-4068-a35f-34262950bb8f">(Getty, 2017)</a>]]></skos:definition>
    <skos:definition xml:lang="fr">«Un manifeste est une déclaration écrite et publique par laquelle un gouvernement, une personne, un parti ou un courant artistique expose un programme d'action ou une position, le plus souvent politique ou esthétique.»  <![CDATA[<a href="#cwrc:727d97bc-af78-4122-94be-aa78b2e97d5a">(DBpedia, 2017)</a>]]></skos:definition>
    <owl:sameAs rdf:resource="http://id.loc.gov/authorities/genreForms/gf2017027243"/>
    <owl:sameAs rdf:resource="http://dbpedia.org/resource/Manifesto"/>
  </genre:PoliticalGenre>
  <genre:JournalisticGenre rdf:about="#journalism">
    <skos:definition xml:lang="fr">«Le journalisme (/ʒuʀnalism/) est l'activité qui consiste à recueillir, vérifier ou commenter des faits pour les porter à l'attention du public dans les médias en respectant une même déontologie du journalisme, reposant sur la protection des sources d'information, du correspondant de guerre au journalisme d'investigation, sans oublier les autres spécialisations : dessinateur de presse, journaliste reporter d'images (JRI), photojournaliste, secrétaire de rédaction, critique musical ou éditorialiste.»  <![CDATA[<a href="#cwrc:727d97bc-af78-4122-94be-aa78b2e97d5a">(DBpedia, 2017)</a>]]></skos:definition>
    <skos:definition xml:lang="en">"Content prepared for a newspaper, magazine, news website, or other form of news media, typically with the purpose of recording facts about a person or event."  <![CDATA[<a href="#cwrc:0a58baf2-e7d5-47d7-9853-c8140dbbfeed">(Merriam-Webster, 2017)</a>]]></skos:definition>
    <rdfs:comment xml:lang="en">This term and its description were created from data gathered from the Merriam-Webster dictionary.</rdfs:comment>
    <rdfs:isDefinedBy rdf:resource="http://sparql.cwrc.ca/ontologies/genre-ONTOLOGY_DATE"/>
    <rdfs:label xml:lang="en">journalism</rdfs:label>
    <owl:sameAs rdf:resource="http://dbpedia.org/resource/Journalism"/>
    <rdfs:label xml:lang="fr">journalisme</rdfs:label>
  </genre:JournalisticGenre>
  <genre:EmbeddedWork rdf:about="#annotation">
    <rdfs:label xml:lang="fr">annotation</rdfs:label>
    <skos:definition xml:lang="fr">"Notes ajoutées en tant que commentaires ou explications, comme celles qui accompagnent les entrées d'une bibliographie, une liste de lecture, ou un catalogue voué à décrire, expliquer ou évaluer la publication à laquelle on se réfère. " </skos:definition>
    <skos:definition xml:lang="en">"Notes added as comment or explanation, such as those accompanying an entry in a bibliography, reading list, or catalogue intended to describe, explain, or evaluate the publication referred to."  <![CDATA[<a href="#cwrc:db2f8571-a773-4068-a35f-34262950bb8f">(Getty, 2017)</a>]]></skos:definition>
    <rdfs:comment xml:lang="en">The description for this term is indebted to the Getty Art &amp; Architecture Thesaurus.</rdfs:comment>
    <rdfs:isDefinedBy rdf:resource="http://sparql.cwrc.ca/ontologies/genre-ONTOLOGY_DATE"/>
    <rdfs:label xml:lang="en">annotation</rdfs:label>
    <owl:sameAs rdf:resource="http://vocab.getty.edu/aat/300026100"/>
  </genre:EmbeddedWork>
  <genre:ChildrensLiteratureGenre rdf:about="#nurseryRhyme">
    <rdfs:comment xml:lang="en">The description for this term is indebted to the Getty Art &amp; Architecture Thesaurus.</rdfs:comment>
    <owl:sameAs rdf:resource="http://vocab.getty.edu/aat/300202593"/>
    <owl:sameAs rdf:resource="http://id.loc.gov/authorities/genreForms/gf2014026459"/>
    <skos:definition xml:lang="en">"Tales in rhymed verse for children."  <![CDATA[<a href="#cwrc:db2f8571-a773-4068-a35f-34262950bb8f">(Getty, 2017)</a>]]></skos:definition>
    <rdf:type rdf:resource="#PoeticGenre"/>
    <rdfs:isDefinedBy rdf:resource="http://sparql.cwrc.ca/ontologies/genre-ONTOLOGY_DATE"/>
    <rdfs:label xml:lang="en">nursery rhyme</rdfs:label>
  </genre:ChildrensLiteratureGenre>
  <genre:NarrativeGenre rdf:about="#testimony">
    <rdfs:label xml:lang="fr">témoignage</rdfs:label>
    <rdfs:isDefinedBy rdf:resource="http://sparql.cwrc.ca/ontologies/genre-ONTOLOGY_DATE"/>
    <rdfs:label xml:lang="en">testimony</rdfs:label>
    <skos:definition xml:lang="fr">Déclarations solennelles, écrites ou verbales, habituellement faites par un témoin sous serment dans le cadre d'une interrogatoire conduit par un avocat ou un représentant de la fonction publique, et ensuite retranscrit par écrit dans un compte rendu.</skos:definition>
    <owl:sameAs rdf:resource="http://vocab.getty.edu/aat/300027861"/>
    <rdfs:comment xml:lang="en">The description for this term is indebted to the Getty Art &amp; Architecture Thesaurus.</rdfs:comment>
    <skos:definition xml:lang="en">"Solemn declarations, written or verbal; usually made orally by a witness under oath in response to interrogation by a lawyer or authorized public official, then reduced to writing for the record."  <![CDATA[<a href="#cwrc:db2f8571-a773-4068-a35f-34262950bb8f">(Getty, 2017)</a>]]></skos:definition>
  </genre:NarrativeGenre>
  <genre:EmbeddedWork rdf:about="#prologue">
    <skos:definition xml:lang="en">"(1) In original Greek tragedy, the prologue was either the action or a set of introductory speeches before the first entry (parados) of the chorus. Here, a single actor's monologue or a dialogue between two actors would establish the play's background events. (2) In later literature, a prologue is a section of any introductory material before the first chapter or the main material of a prose work, or any such material before the first stanza of a poetic work."  <![CDATA[<a href="cwrc:509015ff-7641-473e-94c5-688e06952bb7">(L. K Wheeler, 2017)</a>]]></skos:definition>
    <rdfs:label xml:lang="fr">prologue</rdfs:label>
    <skos:definition xml:lang="fr">«Le prologue (du grec προ (pro) : avant, et λóγος (logos) : discours) est la première partie d’une œuvre littéraire ou la première scène d’une œuvre dramatique, faisant office de préface, d’introduction ou de préambule, et servant à situer les personnages et l’action de l’œuvre en exposant divers points essentiels à connaître pour l’intelligence de la pièce.»  <![CDATA[<a href="#cwrc:727d97bc-af78-4122-94be-aa78b2e97d5a">(DBpedia, 2017)</a>]]></skos:definition>
    <rdfs:isDefinedBy rdf:resource="http://sparql.cwrc.ca/ontologies/genre-ONTOLOGY_DATE"/>
    <rdfs:label xml:lang="en">prologue</rdfs:label>
    <rdfs:comment xml:lang="en">This term and its description were created from data gathered from DBpedia.</rdfs:comment>
    <owl:sameAs rdf:resource="http://id.loc.gov/authorities/genreForms/gf2018026101"/>
    <owl:sameAs rdf:resource="http://dbpedia.org/resource/Prologue"/>
  </genre:EmbeddedWork>
  <genre:MusicalNotationForm rdf:about="#notatedMusic">
    <skos:definition xml:lang="en">"Sheet music is a handwritten or printed form of music notation that uses modern musical symbols to indicate the pitches (melodies), rhythms and/or chords of a song or instrumental musical piece. Like its analogs – printed books or pamphlets in English, Arabic or other languages – the medium of sheet music typically is paper (or, in earlier centuries, papyrus or parchment), although the access to musical notation since the 1980s has included the presentation of musical notation on computer screens and the development of scorewriter computer programs that can notate a song or piece electronically, and, in some cases, "play back" the notated music using a synthesizer or virtual instruments. Use of the term "sheet" is intended to differentiate written or printed forms of music from sound recordings (on vinyl record, cassette, CD), radio or TV broadcasts or recorded live performances, which may capture film or video footage of the performance as well as the audio component. In everyday use, "sheet music" (or simply "music") can refer to the print publication of commercial sheet music in conjunction with the release of a new film, TV show, record album, or other special or popular event which involves music. The first printed sheet music made with a printing press was made in 1473. Sheet music is the basic form in which Western classical music is notated so that it can be learned and performed by solo singers or instrumentalists or musical ensembles. Many forms of traditional and popular Western music are commonly learned by singers and musicians "by ear", rather than by using sheet music (although in many cases, traditional and pop music may also be available in sheet music form). "Score" is a common alternative (and more generic) term for sheet music, and there are several types of scores, as discussed below. The term "score" can also refer to theatre music, orchestral music or songs written for a play, musical, opera or ballet, or to music or songs written for a television programme or film; for the last of these, see Film score." <![CDATA[<a href="#cwrc:727d97bc-af78-4122-94be-aa78b2e97d5a">(DBpedia, 2019)</a>]]></skos:definition>
    <rdfs:isDefinedBy rdf:resource="http://sparql.cwrc.ca/ontologies/genre-ONTOLOGY_DATE"/>
    <rdfs:label xml:lang="en">notated music</rdfs:label>
  </genre:MusicalNotationForm>
  <genre:NovelisticGenre rdf:about="#bildungsroman">
    <skos:definition xml:lang="fr">«Le roman d'apprentissage, appelé aussi roman de formation ou roman d’éducation, est un genre littéraire romanesque né en Allemagne au XVIIIe siècle (à ne pas confondre avec le roman de jeunesse). Il s'oppose cependant à la fonction première du romanesque qui est de nous transporter dans un monde de rêve et d'évasion. On parle ainsi de « roman initiatique » ou de « conte initiatique ». En allemand, le roman de formation est nommé « Bildungsroman ». Ce terme est dû au philologue allemand Johann Carl Simon Morgenstern, qui voyait dans le Bildungsroman « l'essence du roman par opposition au récit épique ». On emploie aussi l'expression « Entwicklungsroman » (roman de développement personnel). Un roman d'apprentissage a pour thème le cheminement évolutif d'un héros, souvent jeune, jusqu'à ce qu'il atteigne l'idéal de l'homme accompli et cultivé. Le héros découvre en général un domaine particulier dans lequel il fait ses armes. Mais en réalité, c'est une conception de la vie en elle-même qu'il se forge progressivement. En effet, derrière l'apprentissage d'un domaine, le jeune héros découvre les grands événements de l'existence (la mort, l'amour, la haine, l'altérité, pour prendre quelques exemples). Ainsi, dans L'Éducation sentimentale (Flaubert, 1869), le jeune Frédéric connaît les premiers émois de l'amour : et réfléchissant sur les sentiments qu'il porte à Mme Arnoux, Frédéric se construit une idée de l'existence. Le roman d'apprentissage est un roman qui décrit la maturation du héros. Il manque d'expérience au départ et traverse des obstacles ou des épreuves afin de mûrir et d'en tirer des leçons.»  <![CDATA[<a href="#cwrc:727d97bc-af78-4122-94be-aa78b2e97d5a">(DBpedia, 2017)</a>]]></skos:definition>
    <rdfs:comment xml:lang="en">The description for this term is indebted to DBpedia. </rdfs:comment>
    <owl:sameAs rdf:resource="http://id.loc.gov/authorities/genreForms/gf2014026243"/>
    <skos:definition xml:lang="en">"Novels of a traditional German genre that focuses on the spiritual development or formative years of an individual. Now in broad use to refer to this type of novel written in any language or in any culture."  <![CDATA[<a href="#cwrc:db2f8571-a773-4068-a35f-34262950bb8f">(Getty, 2017)</a>]]></skos:definition>
    <owl:sameAs rdf:resource="http://dbpedia.org/resource/Bildungsroman"/>
    <rdfs:label xml:lang="fr">bildungsroman</rdfs:label>
    <rdfs:comment xml:lang="fr">La description de ce terme est basée sur celle de DBPedia.</rdfs:comment>
    <rdfs:isDefinedBy rdf:resource="http://sparql.cwrc.ca/ontologies/genre-ONTOLOGY_DATE"/>
    <rdfs:label xml:lang="en">bildungsroman</rdfs:label>
  </genre:NovelisticGenre>
  <genre:ComedicGenre rdf:about="#riddle">
    <rdfs:isDefinedBy rdf:resource="http://sparql.cwrc.ca/ontologies/genre-ONTOLOGY_DATE"/>
    <rdfs:label xml:lang="en">riddle</rdfs:label>
    <skos:definition xml:lang="fr">Jeu d'esprit mettant à l'épreuve la sagacité de l'interlocuteur qui doit trouver la réponse à une interrogation dont le sens est caché sous une parabole ou une métaphore.</skos:definition>
    <skos:definition xml:lang="en">"(from Old English roedel, from roedan meaning "to give council" or "to read"): A universal form of literature in which a puzzling question or a conundrum is presented to the reader. The reader is often challenged to solve this enigma, which requires ingenuity in discovering the hidden meaning. A riddle may involve puns, symbolism, synecdoche, personification (especially prosopopoeia), or unusual imagery. For instance, a Norse riddle asks, "Tell me what I am. Thirty white horses round a red hill. First they champ. Then they stamp. Now they stand still." The answer is the speaker's teeth; these thirty white horses circle the "red hill" of the tongue; they champ and stamp while the riddler speaks, but stand still at the end of his riddle. Another famous example is the riddle of the sphinx from Sophocles' Oedipus Trilogy. The sphinx asks Oedipus, "What goes on four feet, on two feet, and then three. But the more feet it goes on, the weaker is he?" The answer is a human being, which crawls as an infant, walks erect on two feet as an adult, and totters on a staff (the third leg) in old age. The earliest known English riddles are recorded in the Exeter Book, and they probably date back to the 8th century. Examples, however, can be found in Greek, Sanskrit, Hebrew, Arabic, Persian, and Chinese, and many other languages. Authors of Anglo-Latin riddles include Aldhelm of Sherborne, Archbishop Tatwine of Canterbury, and Abbot Eusebius of Wearmouth. A large Renaissance collection can also be found in Nicolas Reusner's Aenigmatographia (1602)."  <![CDATA[<a href="cwrc:509015ff-7641-473e-94c5-688e06952bb7">(L. K Wheeler, 2017)</a>]]></skos:definition>
    <rdfs:comment xml:lang="en">This term and its description were created from data gathered from the Dictionnaire Vivant de la Langue Française.</rdfs:comment>
    <rdfs:label xml:lang="fr">éngime</rdfs:label>
    <owl:sameAs rdf:resource="https://dvlf.uchicago.edu/mot/%C3%A9nigme"/>
  </genre:ComedicGenre>
  <genre:FictionalGenre rdf:about="#dystopia">
    <skos:definition xml:lang="fr">Une dystopie est un récit de fiction dépeignant une société imaginaire organisée de telle façon qu'elle empêche ses membres d'atteindre le bonheur. Une dystopie peut également être considérée, entre autres, comme une utopie qui vire au cauchemar et conduit donc à une contre-utopie. L'auteur entend ainsi mettre en garde le lecteur en montrant les conséquences néfastes d’une idéologie (ou d’une pratique) présente à notre époque. L'impact que ces romans ont eu sur la science-fiction a souvent amené à qualifier de dystopie toute œuvre d'anticipation sociale décrivant un avenir sombre.</skos:definition>
    <rdfs:comment xml:lang="en">The description for this term is indebted to Dr. L. Kip Wheeler of Carson-Newman University. </rdfs:comment>
    <dcterms:references rdf:resource="http://web.cn.edu/kwheeler/lit_terms_d.html"/>
    <skos:definition xml:lang="en">"(from Greek, dys topos, "bad place"): The opposite of a utopia, a dystopia is an imaginary society in fictional writing that represents, as M. H. Abrams puts it, "a very unpleasant imaginary world in which ominous tendencies of our present social, political, and technological order are projected in some disastrous future culmination" (Glossary 218). For instance, while a utopia presents readers with a place where all the citizens are happy and ruled by a virtuous, efficient, rational government, a dystopia presents readers with a world where all citizens are universally unhappy, manipulated, and repressed by a sinister, sadistic totalitarian state. This government exists at best to further its own power and at worst seeks actively to destroy its own citizens' creativity, health, and happiness. Examples of fictional dystopias include Aldous Huxley's Brave New World, George Orwell's 1984, Margaret Atwood's The Handmaid's Tale, and Ursula Le Guin's The Dispossessed."  <![CDATA[<a href="cwrc:509015ff-7641-473e-94c5-688e06952bb7">(L. K Wheeler, 2017)</a>]]></skos:definition>
    <rdfs:isDefinedBy rdf:resource="http://sparql.cwrc.ca/ontologies/genre-ONTOLOGY_DATE"/>
    <rdfs:label xml:lang="en">dystopia</rdfs:label>
    <owl:sameAs rdf:resource="http://id.loc.gov/authorities/genreForms/gf2014026302"/>
    <rdfs:label xml:lang="fr">dystopie</rdfs:label>
  </genre:FictionalGenre>
  <genre:PrintMedium rdf:about="#microform">
    <rdfs:isDefinedBy rdf:resource="http://sparql.cwrc.ca/ontologies/genre-ONTOLOGY_DATE"/>
    <rdfs:label xml:lang="en">microform</rdfs:label>
    <skos:related rdf:resource="http://vocab.getty.edu/aat/300028589"/>
    <skos:definition xml:lang="en">"Microforms are any forms, either films or paper, containing microreproductions of documents for transmission, storage, reading, and printing. Microform images are commonly reduced to about one twenty-fifth of the original document size. For special purposes, greater optical reductions may be used. All microform images may be provided as positives or negatives, more often the latter. Three formats are common: microfilm (reels), aperture cards and microfiche (flat sheets). Microcards, a format no longer produced, were similar to microfiche, but printed on cardboard rather than photographic film." <![CDATA[<a href="#cwrc:727d97bc-af78-4122-94be-aa78b2e97d5a">(DBpedia, 2019)</a>]]></skos:definition>
  </genre:PrintMedium>
  <genre:SongGenre rdf:about="#anthem">
    <rdfs:comment xml:lang="en">This term and its description were created from data gathered from the Oxford Dictionary of Literary Terms, 4th ed.</rdfs:comment>
    <dcterms:references rdf:resource="http://www.oxfordreference.com/view/10.1093/acref/9780199208272.001.0001/acref-9780199208272-e-61?rskey=9jlyTO%26result=61"/>
    <rdfs:isDefinedBy rdf:resource="http://sparql.cwrc.ca/ontologies/genre-ONTOLOGY_DATE"/>
    <rdfs:label xml:lang="en">anthem</rdfs:label>
    <rdfs:label xml:lang="fr">hymne (politique)</rdfs:label>
    <owl:sameAs rdf:resource="http://id.loc.gov/authorities/genreForms/gf2014026635"/>
    <skos:definition xml:lang="en">"A song in which the lyrics promote pride in and allegiance to the identity and values of a particular group, such as a nation, sports team, or social cause."  <![CDATA[<a href="#cwrc:4c227091-6bf0-4325-b846-9733fae19e61">(Oxford, 2015)</a>]]></skos:definition>
    <skos:definition xml:lang="fr">Une chanson dont les paroles promeuvent la fidélité à l'identité et aux valeurs d'un groupe particulier —une nation, une équipe sportive ou une cause sociale— ainsi que la fierté d'y adhérer.</skos:definition>
    <rdf:type rdf:resource="#PoliticalGenre"/>
    <rdf:type rdf:resource="#ThematicGenre"/>
  </genre:SongGenre>
  <genre:DramaticGenre rdf:about="#filmTvScript">
    <rdfs:label xml:lang="fr">script</rdfs:label>
    <rdfs:comment xml:lang="en">This term and its description were created from data gathered from the Getty Art &amp; Architecture Thesaurus.</rdfs:comment>
    <owl:sameAs rdf:resource="http://vocab.getty.edu/aat/300026487"/>
    <rdfs:isDefinedBy rdf:resource="http://sparql.cwrc.ca/ontologies/genre-ONTOLOGY_DATE"/>
    <rdfs:label xml:lang="en">film tv script</rdfs:label>
    <rdf:type rdf:resource="#ScriptForm"/>
    <skos:definition xml:lang="fr">Textes de théâtre, scénario, et scripts pour télévision ou la radio.</skos:definition>
    <skos:altLabel xml:lang="en">tv script</skos:altLabel>
    <skos:definition xml:lang="en">"Written texts of stage plays, screenplays, and radio or television broadcasts."  <![CDATA[<a href="#cwrc:db2f8571-a773-4068-a35f-34262950bb8f">(Getty, 2017)</a>]]></skos:definition>
  </genre:DramaticGenre>
  <genre:ThematicGenre rdf:about="#juvenilia">
    <skos:definition xml:lang="en">"Literary or artistic works produced by persons in their childhood or youth; usually used to set those works apart from later, mature works."  <![CDATA[<a href="#cwrc:db2f8571-a773-4068-a35f-34262950bb8f">(Getty, 2017)</a>]]></skos:definition>
    <rdfs:comment xml:lang="en">The description for this term is indebted to the Getty Art &amp; Architecture Thesaurus.</rdfs:comment>
    <rdfs:isDefinedBy rdf:resource="http://sparql.cwrc.ca/ontologies/genre-ONTOLOGY_DATE"/>
    <rdfs:label xml:lang="en">juvenilia</rdfs:label>
    <owl:sameAs rdf:resource="http://vocab.getty.edu/aat/300028883"/>
    <rdfs:label xml:lang="fr">oeuvres de jeunesse</rdfs:label>
    <skos:definition xml:lang="fr">Œuvres littéraires ou artistiques produites par des personnes dans leur enfance ou leur jeunesse; le terme est généralement utilisé pour distinguer ces œuvres des travaux matures plus tardifs.</skos:definition>
  </genre:ThematicGenre>
  <genre:ThematicGenre rdf:about="#ruralIdyll">
    <rdfs:isDefinedBy rdf:resource="http://sparql.cwrc.ca/ontologies/genre-ONTOLOGY_DATE"/>
    <rdfs:label xml:lang="en">rural idyll</rdfs:label>
    <skos:definition xml:lang="en">"An idyll or idyl (/ˈaɪdəl/ or /ˈɪdəl/; from Greek εἰδύλλιον, eidullion, "short poem") is a short poem, descriptive of rustic life, written in the style of Theocritus' short pastoral poems, the Idylls. Unlike Homer, Theocritus did not engage in heroes and warfare. His idylls are limited to a small intimate world, and describe scenes from everyday life. Later imitators include the Roman poets Virgil and Catullus, Italian poets Torquato Tasso, Sannazaro and Leopardi, the English poet Alfred, Lord Tennyson (Idylls of the King), and Nietzsche's Idylls from Messina. Goethe called his poem Hermann and Dorothea—which Schiller considered the very climax in Goethe's production—an idyll." <![CDATA[<a href="#cwrc:727d97bc-af78-4122-94be-aa78b2e97d5a">(DBpedia, 2019)</a>]]></skos:definition>
    <rdf:type rdf:resource="#PoeticGenre"/>
  </genre:ThematicGenre>
  <genre:PedagogicalGenre rdf:about="#pedagogy">
    <owl:sameAs rdf:resource="http://dbpedia.org/resource/Pedagogy"/>
    <rdfs:comment xml:lang="en">This term and its description were created from data gathered from DBpedia.</rdfs:comment>
    <skos:definition xml:lang="en">"Writing dealing with the theory and practice of teaching."  <![CDATA[<a href="#cwrc:4c227091-6bf0-4325-b846-9733fae19e61">(Oxford, 2015)</a>]]></skos:definition>
    <rdfs:label xml:lang="fr">pédagogie</rdfs:label>
    <skos:definition xml:lang="fr">«La pédagogie (du grec παιδαγωγία, direction ou éducation des enfants) désigne l'art de l'éducation. Le terme rassemble les méthodes et pratiques d'enseignement requises pour transmettre des connaissances, c'est-à-dire un savoir, un savoir-faire ou un savoir-être. Plus généralement, l'expression « Faire preuve de pédagogie » signifie l'aptitude à enseigner et à transmettre à un individu ou un groupe d'individus — de tous âges et de toutes conditions — un savoir ou une expérience par l'usage des méthodes les plus adaptées à l'audience concernée.»  <![CDATA[<a href="#cwrc:727d97bc-af78-4122-94be-aa78b2e97d5a">(DBpedia, 2017)</a>]]></skos:definition>
    <rdfs:isDefinedBy rdf:resource="http://sparql.cwrc.ca/ontologies/genre-ONTOLOGY_DATE"/>
    <rdfs:label xml:lang="en">pedagogy</rdfs:label>
  </genre:PedagogicalGenre>
  <genre:PoeticGenre rdf:about="#villanelle">
    <skos:definition xml:lang="fr">«D’origine italienne, la villanelle, de l’italien villanella dérivant du latin villanus (paysan), est, en littérature, une sorte de petite poésie pastorale à forme fixe et divisée en couplets qui finissent par le même refrain. En musique, c’est une ancienne danse rustique accompagnée de chant ainsi qu’une mélodie, un air d’instruments composé sur le modèle de cette danse.»  <![CDATA[<a href="#cwrc:727d97bc-af78-4122-94be-aa78b2e97d5a">(DBpedia, 2017)</a>]]></skos:definition>
    <owl:sameAs rdf:resource="http://dbpedia.org/resource/Villanelle"/>
    <rdfs:comment xml:lang="en">The description for this term is indebted to Dr. L. Kip Wheeler of Carson-Newman University. </rdfs:comment>
    <rdfs:label xml:lang="fr">villanelle</rdfs:label>
    <skos:definition xml:lang="en">"A versatile genre of poetry consisting of nineteen lines--five tercets and a concluding quatrain. The form requires that whole lines be repeated in a specific order, and that only two rhyming sounds occur in the course of the poem. A number of English poets, including Oscar Wilde, W. E. Henley, and W. H. Auden have experimented with it. Here is an example of an opening stanza to one poem by W. E. Henley: Probably the most famous English villanelle is Dylan Thomas's "Do Not Go Gentle Into That Good Night."  <![CDATA[<a href="cwrc:509015ff-7641-473e-94c5-688e06952bb7">(L. K Wheeler, 2017)</a>]]></skos:definition>
    <rdfs:isDefinedBy rdf:resource="http://sparql.cwrc.ca/ontologies/genre-ONTOLOGY_DATE"/>
    <rdfs:label xml:lang="en">villanelle</rdfs:label>
    <owl:sameAs rdf:resource="http://id.loc.gov/authorities/genreForms/gf2014026587"/>
  </genre:PoeticGenre>
  <genre:FictionalGenre rdf:about="#ghostStory">
    <rdfs:comment xml:lang="en">The description for this term is indebted to DBpedia. </rdfs:comment>
    <skos:definition xml:lang="fr">«Les histoires de fantôme sont un sous-genre du fantastique. Dans ces histoires, le fantôme est souvent le héros et a une personnalité et une identité bien à lui. Le genre peut aussi donner lieu à des récits centrés uniquement sur les fantômes ou les morts.»  <![CDATA[<a href="#cwrc:727d97bc-af78-4122-94be-aa78b2e97d5a">(DBpedia, 2017)</a>]]></skos:definition>
    <skos:definition xml:lang="en">"Prose tales of the supernatural in which the living encounter manifestations of the spirits of the dead."  <![CDATA[<a href="#cwrc:db2f8571-a773-4068-a35f-34262950bb8f">(Getty, 2017)</a>]]></skos:definition>
    <owl:sameAs rdf:resource="http://vocab.getty.edu/aat/300254823"/>
    <owl:sameAs rdf:resource="http://id.loc.gov/authorities/genreForms/gf2014026357"/>
    <rdfs:isDefinedBy rdf:resource="http://sparql.cwrc.ca/ontologies/genre-ONTOLOGY_DATE"/>
    <rdfs:label xml:lang="en">ghost story</rdfs:label>
  </genre:FictionalGenre>
  <genre:DramaticGenre rdf:about="#camp">
    <skos:definition xml:lang="en">"Camp is an aesthetic style and sensibility that regards something as appealing because of its bad taste and ironic value. Camp aesthetics disrupt many of modernism's notions of what art is and what can be classified as high art by inverting aesthetic attributes such as beauty, value, and taste through an invitation of a different kind of apprehension and consumption. Camp can also be a social practice. For many it is considered a style and performance identity for several types of entertainment including film, cabaret and pantomime. Where high art necessarily incorporates beauty and value, camp necessarily needs to be lively, audacious and dynamic. "Camp aesthetics delights in impertinence." Camp opposes satisfaction and seeks to challenge. Camp art is related to—and often confused with—kitsch, and things with camp appeal may also be described as "cheesy". When the usage appeared in 1909, it denoted ostentatious, exaggerated, affected, theatrical, and/or effeminate behavior, and by the middle of the 1970s, the definition comprised: banality, artifice, mediocrity and ostentation so extreme as to have perversely sophisticated appeal. American writer Susan Sontag's essay "Notes on 'Camp'" (1964) emphasized its key elements as: artifice, frivolity, naive middle-class pretentiousness, and 'shocking' excess. Camp as an aesthetic has been popular from the 1960s to the present. Camp aesthetics were popularised by filmmakers George and Mike Kuchar, Jack Smith and his film Flaming Creatures, and later John Waters, including the last's Pink Flamingos, Hairspray, and Polyester. Celebrities that are associated with camp personas include drag queens and performers such as Dame Edna Everage, Divine, RuPaul, Paul Lynde, and Liberace. Camp was a part of the anti-academic defense of popular culture in the 1960s and gained popularity in the 1980s with the widespread adoption of postmodern views on art and culture." <![CDATA[<a href="#cwrc:727d97bc-af78-4122-94be-aa78b2e97d5a">(DBpedia, 2019)</a>]]></skos:definition>
    <rdfs:isDefinedBy rdf:resource="http://sparql.cwrc.ca/ontologies/genre-ONTOLOGY_DATE"/>
    <rdfs:label xml:lang="en">camp</rdfs:label>
  </genre:DramaticGenre>
  <genre:EmbeddedWork rdf:about="#appendix">
    <skos:definition xml:lang="en">"An addendum, in general, is an addition required to be made to a document by its author subsequent to its printing or publication. It comes from the Latin verbal phrase addendum est, being the gerundive form of the verb addo, addere, addidi, additum, "to give to, add to", meaning "(that which) must be added". Addenda is from the plural form addenda sunt, "(those things) which must be added". (See also memorandum, agenda, corrigenda.)" <![CDATA[<a href="#cwrc:727d97bc-af78-4122-94be-aa78b2e97d5a">(DBpedia, 2019)</a>]]></skos:definition>
    <rdfs:isDefinedBy rdf:resource="http://sparql.cwrc.ca/ontologies/genre-ONTOLOGY_DATE"/>
    <rdfs:label xml:lang="en">appendix</rdfs:label>
  </genre:EmbeddedWork>
  <genre:MusicalGenre rdf:about="#music">
    <rdfs:comment xml:lang="en">This term and its description were created from data gathered from the Getty Art &amp; Architecture Thesaurus.</rdfs:comment>
    <owl:sameAs rdf:resource="http://id.loc.gov/authorities/genreForms/gf2014026952"/>
    <rdfs:isDefinedBy rdf:resource="http://sparql.cwrc.ca/ontologies/genre-ONTOLOGY_DATE"/>
    <rdfs:label xml:lang="en">music</rdfs:label>
    <rdfs:label xml:lang="fr">musique</rdfs:label>
    <skos:definition xml:lang="en">"Performing arts genre having to do with the combining of vocal or instrumental sounds in measured time to communicate emotions, ideas, or states of mind, usually according to cultural standards of rhythm, melody, and, in most Western music, harmony."  <![CDATA[<a href="#cwrc:db2f8571-a773-4068-a35f-34262950bb8f">(Getty, 2017)</a>]]></skos:definition>
    <owl:sameAs rdf:resource="http://vocab.getty.edu/page/aat/300054146"/>
  </genre:MusicalGenre>
  <genre:HistoricalGenre rdf:about="#historicalWriting">
    <skos:definition xml:lang="en">"Refers to maps that indicate political administrative boundaries or other characteristics of a region at periods of time before the present. They typically include historical names for places, historical population dispositions, and the historical state of physical features."  <![CDATA[<a href="#cwrc:db2f8571-a773-4068-a35f-34262950bb8f">(Getty, 2017)</a>]]></skos:definition>
    <rdfs:isDefinedBy rdf:resource="http://sparql.cwrc.ca/ontologies/genre-ONTOLOGY_DATE"/>
    <rdfs:label xml:lang="en">historical writing</rdfs:label>
    <rdfs:comment xml:lang="en">The description for this term is indebted to the Getty Art &amp; Architecture Thesaurus.</rdfs:comment>
    <skos:definition xml:lang="fr">«La fiction historique est un genre de fiction qui situe le récit dans le cadre historique précis d'un passé proche ou lointain. Des exemples connus de fiction historique sont le roman Sinouhé l'Égyptien, la bande dessinée L'Épervier ou le film Meurtre dans un jardin anglais. D'autres romans tels que Les Piliers de la Terre se placent également dans un contexte réaliste, respectant scrupuleusement les faits historiques, tout en déroulant un fil principal à caractère fictionnel : Ainsi, le livre reprend le thème du Moyen Âge central et narre la vie d'un bâtisseur de l'époque.»  <![CDATA[<a href="#cwrc:727d97bc-af78-4122-94be-aa78b2e97d5a">(DBpedia, 2017)</a>]]></skos:definition>
    <rdfs:label xml:lang="fr">écrivage historique</rdfs:label>
    <skos:hiddenLabel xml:lang="en">HISTORICAL</skos:hiddenLabel>
    <owl:sameAs rdf:resource="http://dbpedia.org/resource/Historical_fiction"/>
  </genre:HistoricalGenre>
  <genre:DramaticGenre rdf:about="#revue">
    <rdfs:label xml:lang="en">revue</rdfs:label>
    <rdfs:label xml:lang="fr">revue (variétés)</rdfs:label>
    <skos:definition xml:lang="en">"A revue (from French 'magazine' or 'overview') is a type of multi-act popular theatrical entertainment that combines music, dance and sketches. The revue has its roots in 19th century popular entertainment and melodrama but grew into a substantial cultural presence of its own during its golden years from 1916 to 1932. Though most famous for their visual spectacle, revues frequently satirized contemporary figures, news or literature. Similar to the related subforms of operetta and musical theatre, the revue art form brings together music, dance and sketches to create a compelling show. In contrast to these, however, revue does not have an overarching storyline. Rather, a general theme serves as the motto for a loosely-related series of acts that alternate between solo performances and dance" <![CDATA[<a href="#cwrc:727d97bc-af78-4122-94be-aa78b2e97d5a">(DBpedia, 2019)</a>]]></skos:definition>
    <skos:definition xml:lang="fr">«Une revue est un genre théâtral qui associe musique, danse et sketches qui font la satire de personnes contemporaines, de l'actualité ou de la littérature. Comme les formes apparentées de l'opérette et de la comédie musicale, la revue allie musique, danse et comédie pour former un spectacle complet. Contrairement à celles-ci, elle ne possède cependant pas d'histoire suivie. Un thème général est plutôt utilisé pour un enchaînement de numéros au cours desquels solos et ensembles de danse se relaient.»  <![CDATA[<a href="#cwrc:727d97bc-af78-4122-94be-aa78b2e97d5a">(DBpedia, 2017)</a>]]></skos:definition>
    <rdfs:comment xml:lang="en">This term and its description were created from data gathered from DBpedia.</rdfs:comment>
    <owl:sameAs rdf:resource="http://dbpedia.org/resource/Revue"/>
    <owl:sameAs rdf:resource="http://id.loc.gov/authorities/genreForms/gf2014027050"/>
    <rdfs:isDefinedBy rdf:resource="http://sparql.cwrc.ca/ontologies/genre-ONTOLOGY_DATE"/>
  </genre:DramaticGenre>
  <genre:PoeticGenre rdf:about="#epigram">
    <rdfs:isDefinedBy rdf:resource="http://sparql.cwrc.ca/ontologies/genre-ONTOLOGY_DATE"/>
    <rdfs:label xml:lang="en">epigram</rdfs:label>
    <owl:sameAs rdf:resource="http://dbpedia.org/resource/Epigram"/>
    <skos:definition xml:lang="fr">«À l’origine, une épigramme, du grec ancien ἐπίγραμμα (epígramma), « inscription », est une inscription, d’abord en prose, puis en vers, qu’on gravait sur les monuments, les statues, les tombeaux et les trophées, pour perpétuer le souvenir d’un héros ou d’un événement. À partir du IVe siècleav. J.-C., l’épigramme devient une petite pièce de poésie sur un sujet quelconque, imitant par sa brièveté les inscriptions, offrant une pensée ingénieuse ou délicate exprimée avec grâce et précision. Enfin, à partir du XVIe siècle, le genre se spécialise dans le mot d’esprit : l’épigramme renferme généralement une pointe grivoise ou assassine. Les plus anciennes épigrammes ne revêtent qu'un caractère pratique, visant à identifier le propriétaire ou la personne dédiant l’objet. Le premier auteur d’épigrammes, selon la tradition grecque, est Simonide de Céos (Hérodote, VII, 228, 4), qui vit à la fin du VIe siècleav. J.-C. C'est de cette même époque que date la première épigramme signée connue ; il s'agit d’une dédicace d’Ion de Chios à Delphes.»  <![CDATA[<a href="#cwrc:727d97bc-af78-4122-94be-aa78b2e97d5a">(DBpedia, 2017)</a>]]></skos:definition>
    <skos:definition xml:lang="en">"Refers to short satiric poems or any similar pointed sayings."  <![CDATA[<a href="#cwrc:db2f8571-a773-4068-a35f-34262950bb8f">(Getty, 2017)</a>]]></skos:definition>
    <owl:sameAs rdf:resource="http://id.loc.gov/authorities/genreForms/gf2014026312"/>
    <rdfs:comment xml:lang="en">The description for this term is indebted to DBpedia. </rdfs:comment>
  </genre:PoeticGenre>
  <genre:HistoricalGenre rdf:about="#localHistory">
    <skos:definition xml:lang="en">"Histories that are distinctly localized in subject matter or source materials, focusing on specific neighborhoods, communities, counties, or other specific subdivisions of larger geopolitical bodies." <![CDATA[<a href="#cwrc:bd595bc4-5991-4c51-98d9-9ab52c416f4f">(Getty, 2021)</a>]]></skos:definition>
    <rdfs:comment xml:lang="en">The description for this term is indebted to the Getty Art &amp; Architecture Thesaurus.</rdfs:comment>
    <owl:sameAs rdf:resource="http://vocab.getty.edu/aat/300251993"/>
    <rdfs:isDefinedBy rdf:resource="http://sparql.cwrc.ca/ontologies/genre-ONTOLOGY_DATE"/>
    <rdfs:label xml:lang="en">local history</rdfs:label>
  </genre:HistoricalGenre>
  <genre:LifeWritingGenre rdf:about="#lifeWriting">
    <rdfs:isDefinedBy rdf:resource="http://sparql.cwrc.ca/ontologies/genre-ONTOLOGY_DATE"/>
    <rdfs:label xml:lang="en">life writing</rdfs:label>
    <skos:definition xml:lang="en">"Life writing is the recording of memories, and experiences, whether one's own or another's. This applies to many genres and practices, under which can be found autobiography, biography, memoir, diaries, letters, testimonies, personal essays and, more recently, digital forms such as blogs and email."  <![CDATA[<a href="#cwrc:727d97bc-af78-4122-94be-aa78b2e97d5a">(DBpedia, 2017)</a>]]></skos:definition>
    <owl:sameAs rdf:resource="http://dbpedia.org/resource/Life_writing"/>
    <rdfs:comment xml:lang="en">The description for this term is indebted to DBpedia. </rdfs:comment>
  </genre:LifeWritingGenre>
  <genre:TextualMedium rdf:about="#looseLeaf">
    <skos:definition xml:lang="en">"A loose leaf is a piece of paper that is not bound in place, but typically punched so as to be organized in a ring binder. Loose leaves may be sold as free sheets, or made up into notepads, where perforations allow them to be removed easily." <![CDATA[<a href="#cwrc:727d97bc-af78-4122-94be-aa78b2e97d5a">(DBpedia, 2019)</a>]]></skos:definition>
    <skos:related rdf:resource="http://vocab.getty.edu/aat/300257592"/>
    <rdfs:isDefinedBy rdf:resource="http://sparql.cwrc.ca/ontologies/genre-ONTOLOGY_DATE"/>
    <rdfs:label xml:lang="en">loose-leaf</rdfs:label>
  </genre:TextualMedium>
  <genre:InformationalGenre rdf:about="#biography">
    <skos:definition xml:lang="en">"The genre of nonfiction that concerns accounts of the lives of individuals."  <![CDATA[<a href="#cwrc:db2f8571-a773-4068-a35f-34262950bb8f">(Getty, 2017)</a>]]></skos:definition>
    <rdfs:isDefinedBy rdf:resource="http://sparql.cwrc.ca/ontologies/genre-ONTOLOGY_DATE"/>
    <rdfs:label xml:lang="en">biography</rdfs:label>
    <rdfs:comment xml:lang="fr">La description de ce terme est basée sur celle de DBPedia.</rdfs:comment>
    <owl:sameAs rdf:resource="http://vocab.getty.edu/aat/300404015"/>
    <skos:definition xml:lang="fr">«Une biographie (une bio), du grec ancien βίος, « la vie » et γραφή, « écrire », est un écrit qui a pour objet l'histoire d'une vie particulière. Elle peut être écrite par la personne elle-même (autobiographie) ou par une autre personne.»  <![CDATA[<a href="#cwrc:727d97bc-af78-4122-94be-aa78b2e97d5a">(DBpedia, 2017)</a>]]></skos:definition>
    <owl:sameAs rdf:resource="http://id.loc.gov/authorities/genreForms/gf2014026049"/>
    <rdfs:comment xml:lang="en">The description for this term is indebted to DBpedia. </rdfs:comment>
    <rdfs:label xml:lang="fr">biographie </rdfs:label>
  </genre:InformationalGenre>
  <genre:SerialForm rdf:about="#serial">
    <rdfs:isDefinedBy rdf:resource="http://sparql.cwrc.ca/ontologies/genre-ONTOLOGY_DATE"/>
    <rdfs:label xml:lang="en">serial</rdfs:label>
    <skos:definition xml:lang="en">A broad category indicating works in a range of media and genres published in parts, whether a television series or a serial podcast.
For fiction published in installments there are also specific terms for those issued as separate publications @@#serialVolume@@ or within sequential issues of the same periodical publication.
</skos:definition>
  </genre:SerialForm>
  <genre:SerialForm rdf:about="#bookSeries">
    <rdfs:isDefinedBy rdf:resource="http://sparql.cwrc.ca/ontologies/genre-ONTOLOGY_DATE"/>
    <rdfs:label xml:lang="en">book series</rdfs:label>
    <skos:definition xml:lang="en">"A book series is a sequence of books having certain characteristics in common that are formally identified together as a group. Book series can be organized in different ways, such as written by the same author, or marketed as a group by their publisher." <![CDATA[<a href="#cwrc:727d97bc-af78-4122-94be-aa78b2e97d5a">(DBpedia, 2017)</a>]]></skos:definition>
  </genre:SerialForm>
  <genre:SerialForm rdf:about="#serialVolume">
    <rdfs:isDefinedBy rdf:resource="http://sparql.cwrc.ca/ontologies/genre-ONTOLOGY_DATE"/>
    <rdfs:label xml:lang="en">serial volume</rdfs:label>
    <skos:definition xml:lang="en">Serialized in print in the form of standalone numbers or volumes.</skos:definition>
    <skos:broader rdf:resource="#serial"/>
  </genre:SerialForm>
  <genre:SerialForm rdf:about="#serialPeriodical">
    <rdfs:isDefinedBy rdf:resource="http://sparql.cwrc.ca/ontologies/genre-ONTOLOGY_DATE"/>
    <rdfs:label xml:lang="en">serial periodical</rdfs:label>
    <skos:definition xml:lang="en">Serialized in print embedded within a larger periodical such as a magazine or newspaper.</skos:definition>
    <skos:broader rdf:resource="#serial"/>
  </genre:SerialForm>
  <genre:SoundRecordingMedium rdf:about="#soundRecordingMusical">
    <skos:definition xml:lang="en">"Discs, tapes, filaments, or other media on which music has been recorded. Music is defined as a performing arts genre having to do with the combining of vocal or instrumental sounds in measured time to communicate emotions, ideas, or states of mind, usually according to cultural standards of rhythm, melody, and, in most Western music, harmony."<![CDATA[<a href="#cwrc:bd595bc4-5991-4c51-98d9-9ab52c416f4f">(Getty, 2021)</a>]]></skos:definition>
    <rdfs:comment xml:lang="en">The description for this term is indebted to the Getty Art &amp; Architecture Thesaurus.</rdfs:comment>
    <skos:related rdf:resource="http://sparql.cwrc.ca/ontologies/genre.html#SoundRecordingMedium"/>
    <rdfs:isDefinedBy rdf:resource="http://sparql.cwrc.ca/ontologies/genre-ONTOLOGY_DATE"/>
    <rdfs:label xml:lang="en">sound recording - musical</rdfs:label>
  </genre:SoundRecordingMedium>
  <genre:SongGenre rdf:about="#folkSong">
    <skos:definition xml:lang="en">"A song recorded or transcribed after being preserved for generations by a particular culture through an oral tradition, or more recent songs composed in the style of that tradition."  <![CDATA[<a href="#cwrc:4c227091-6bf0-4325-b846-9733fae19e61">(Oxford, 2015)</a>]]></skos:definition>
    <skos:definition xml:lang="fr">Chanson enregistrée ou retranscrite après avoir été transmire de génération en génération suivant une tradition orale au sein d'une culture spécifique, ou chansons plus récentes composées dans le style de cette tradition.</skos:definition>
    <dcterms:references rdf:resource="http://www.oxfordreference.com/view/10.1093/acref/9780199208272.001.0001/acref-9780199208272-e-470?rskey=icg8D9%26result=461"/>
    <rdfs:label xml:lang="fr">chanson populaire</rdfs:label>
    <owl:sameAs rdf:resource="http://id.loc.gov/authorities/genreForms/gf2014026811"/>
    <rdfs:isDefinedBy rdf:resource="http://sparql.cwrc.ca/ontologies/genre-ONTOLOGY_DATE"/>
    <rdfs:label xml:lang="en">folk song</rdfs:label>
    <rdfs:comment xml:lang="en">This term and its description were created from data gathered from the Oxford Dictionary of Literary Terms, 4th ed.</rdfs:comment>
  </genre:SongGenre>
  <genre:PerformanceMedium rdf:about="#lecture">
    <skos:definition xml:lang="en">"Expositions of a given subject delivered before an audience or class, or recorded and broadcast or streamed, especially for the purposes of instruction." <![CDATA[<a href="#cwrc:bd595bc4-5991-4c51-98d9-9ab52c416f4f">(Getty, 2021)</a>]]></skos:definition>
    <rdfs:comment xml:lang="en">The description for this term is indebted to the Getty Art &amp; Architecture Thesaurus.</rdfs:comment>
    <owl:sameAs rdf:resource="http://vocab.getty.edu/aat/300026673"/>
    <owl:sameAs rdf:resource="http://id.loc.gov/authorities/genreForms/gf2014026122"/>
    <rdfs:isDefinedBy rdf:resource="http://sparql.cwrc.ca/ontologies/genre-ONTOLOGY_DATE"/>
    <rdfs:label xml:lang="en">lecture</rdfs:label>
  </genre:PerformanceMedium>
  <genre:IntertextualGenre rdf:about="#imitation">
    <skos:definition xml:lang="fr">Forme d'intertextualité dans laquelle un.e auteur.e adopte intentionnellement le style d'un.e autre auteur.e, ou emprunte des éléments importants du travail de quelqu'un d'autre.</skos:definition>
    <rdfs:isDefinedBy rdf:resource="http://sparql.cwrc.ca/ontologies/genre-ONTOLOGY_DATE"/>
    <rdfs:label xml:lang="en">imitation</rdfs:label>
    <rdfs:comment xml:lang="en">This term and its description were created from data gathered from the Penguin Dictionary of Literary Terms &amp; Literary Theory, 4th ed.</rdfs:comment>
    <skos:definition xml:lang="en">"A form of intertextuality in which a writer intentionally adopts the style of another writer or borrows important elements of someone else's work."  <![CDATA[<a href="#cwrc:2f09376c-f784-4a46-9f04-5a21aa311f27">(Penguin, 1999)</a>]]></skos:definition>
    <rdfs:label xml:lang="fr">imitation</rdfs:label>
  </genre:IntertextualGenre>
  <genre:FictionalGenre rdf:about="#fantasy">
    <owl:sameAs rdf:resource="http://vocab.getty.edu/aat/300380290"/>
    <skos:definition xml:lang="en">"Literary genre in which works are of a whimsical or visionary nature, having suppositions that are speculation or resting on no solid grounds."  <![CDATA[<a href="#cwrc:db2f8571-a773-4068-a35f-34262950bb8f">(Getty, 2017)</a>]]></skos:definition>
    <skos:definition xml:lang="fr">La fantasy, ou fantasie (terme issu de l’anglais fantasy : « imagination » ; à ne pas confondre avec la fantaisie musicale, ni avec le terme allemand phantasie qui désigne le concept psychologique de fantasme), est un genre littéraire présentant un ou plusieurs éléments surnaturels qui relèvent souvent du mythe et qui sont souvent incarnés par l’irruption ou l’utilisation de la magie. La fantasy fait partie des littératures de l'imaginaire. Dans la fantasy comme dans le merveilleux, le surnaturel est généralement accepté, voire utilisé pour définir les règles d'un monde imaginaire, et n'est pas nécessairement objet de doute ou de peur. Cela distingue la fantasy du fantastique où le surnaturel fait intrusion dans les règles du monde habituel, et de l'horreur où il suscite peur et angoisse. Par extension, à partir du genre littéraire, on parle aussi de fantasy à propos d'illustrations, de bandes dessinées, de films, de jeux, etc.</skos:definition>
    <rdfs:isDefinedBy rdf:resource="http://sparql.cwrc.ca/ontologies/genre-ONTOLOGY_DATE"/>
    <rdfs:label xml:lang="en">fantasy</rdfs:label>
    <rdfs:comment xml:lang="en">The description for this term is indebted to the Getty Art &amp; Architecture Thesaurus.</rdfs:comment>
  </genre:FictionalGenre>
  <genre:SongGenre rdf:about="#song">
    <rdfs:label xml:lang="fr">chanson</rdfs:label>
    <skos:definition xml:lang="en">"A lyric poem with a number of repeating stanzas (called refrains), written to be set to music in either vocal performance or with accompaniment of musical instruments."  <![CDATA[<a href="cwrc:509015ff-7641-473e-94c5-688e06952bb7">(L. K Wheeler, 2017)</a>]]></skos:definition>
    <skos:definition xml:lang="fr">«Une chanson ou un chant est une œuvre musicale composée d'un texte et d'une mélodie destinée à être interprétée par la voix humaine. Cette interprétation peut se faire sans accompagnement instrumental, c'est-à-dire a cappella, ou au contraire être accompagnée d'un ou plusieurs instruments (guitare, piano, groupe, voire un big band ou un grand orchestre symphonique). Elle peut être à une voix (monodie) ou à plusieurs (polyphonie) comme dans un choral.»  <![CDATA[<a href="#cwrc:727d97bc-af78-4122-94be-aa78b2e97d5a">(DBpedia, 2017)</a>]]></skos:definition>
    <rdfs:isDefinedBy rdf:resource="http://sparql.cwrc.ca/ontologies/genre-ONTOLOGY_DATE"/>
    <rdfs:label xml:lang="en">song</rdfs:label>
    <owl:sameAs rdf:resource="http://dbpedia.org/resource/Song"/>
    <rdfs:comment xml:lang="en">The description for this term is indebted to Dr. L. Kip Wheeler of Carson-Newman University. </rdfs:comment>
    <owl:sameAs rdf:resource="http://id.loc.gov/authorities/genreForms/gf2014027103"/>
    <rdf:type rdf:resource="#PoeticGenre"/>
  </genre:SongGenre>
  <genre:EmbeddedWork rdf:about="#dedication">
    <skos:definition xml:lang="en">"A short bit of text conventionally appearing before the start of a novel or poem in which the author or poet addresses some individual, invoking his or her gratitude or thanks to that individual. Frequently, the dedication is to a spouse, friend, loved one, child, mentor, or individual who inspired the work. Several of the Inklings dedicated specific fictional works to each other (or in the case of C.S. Lewis, to children of fellow Inklings). Among scholars, one of the most significant types of dedications is a festschrift. A festschrift is a collection of essays or studies in book form, dedicated to a former teacher or professor in his or her advanced age. The individual scholarly writings come from his or her students, who typically collaborate to organize the work and contact the publisher, and they present the collection to the teacher upon its publication."  <![CDATA[<a href="cwrc:509015ff-7641-473e-94c5-688e06952bb7">(L. K Wheeler, 2017)</a>]]></skos:definition>
    <skos:definition xml:lang="fr">«Une dédicace est une épître ou simple inscription placée par un auteur en tête d’un livre pour mettre son œuvre sous le patronage d’une personne illustre ou influente, ou pour témoigner de ses sentiments de gratitude ou d’amitié, ou enfin, à certaines époques, pour en tirer profit.»  <![CDATA[<a href="#cwrc:727d97bc-af78-4122-94be-aa78b2e97d5a">(DBpedia, 2017)</a>]]></skos:definition>
    <rdfs:isDefinedBy rdf:resource="http://sparql.cwrc.ca/ontologies/genre-ONTOLOGY_DATE"/>
    <rdfs:label xml:lang="en">dedication</rdfs:label>
    <rdfs:label xml:lang="fr">dédicace</rdfs:label>
    <owl:sameAs rdf:resource="http://dbpedia.org/resource/Dedication_(publishing)"/>
    <rdfs:comment xml:lang="en">The description for this term is indebted to Dr. L. Kip Wheeler of Carson-Newman University. </rdfs:comment>
  </genre:EmbeddedWork>
  <genre:ScholarlyGenre rdf:about= "#phdThesis">
    <rdfs:isDefinedBy rdf:resource="http://sparql.cwrc.ca/ontologies/genre-ONTOLOGY_DATE"/>
    <rdfs:label xml:lang="en">Ph.D. dissertation</rdfs:label>
    <skos:altLabel xml:lang="en">Ph.D. thesis</skos:altLabel>
    <skos:definition xml:lang="en">"Papers, research results, or other documents presenting the author's research and submitted in support of candidature for a Ph.D." <![CDATA[<a href="#cwrc:bd595bc4-5991-4c51-98d9-9ab52c416f4f">(Getty, 2021)</a>]]></skos:definition>
    <rdfs:comment xml:lang="en">The description for this term is indebted to the Getty Art &amp; Architecture Thesaurus.</rdfs:comment>
  </genre:ScholarlyGenre>
  <genre:PoeticGenre rdf:about="#dub">
    <skos:definition xml:lang="en">"Dub poetry is a form of performance poetry of West Indian origin, which evolved out of dub music consisting of spoken word over reggae rhythms in Jamaica in the 1970s.Unlike dee jaying (also known as toasting), which also features the use of the spoken word, the dub poet's performance is normally prepared, rather than the extemporized chat of the dancehall dee jay. In musical setting, the dub poet usually appears on stage with a band performing music specifically written to accompany each poem, rather than simply perform over the top of dub plates, or riddims, in the dancehall fashion. Musicality is built into dub poems, yet, dub poets generally perform without backing music, delivering chanted speech with pronounced rhythmic accentuation and dramatic stylization of gesture. Sometimes dub music effects, e.g. echo, reverb, are dubbed spontaneously by a poet into live versions of a poem. Many dub poets also employ call-and-response devices to engage audiences." <![CDATA[<a href="#cwrc:727d97bc-af78-4122-94be-aa78b2e97d5a">(DBpedia, 2019)</a>]]></skos:definition>
    <rdfs:isDefinedBy rdf:resource="http://sparql.cwrc.ca/ontologies/genre-ONTOLOGY_DATE"/>
    <rdfs:label xml:lang="en">dub</rdfs:label>
  </genre:PoeticGenre>
  <genre:NarrativeGenre rdf:about="#fable">
    <rdfs:label xml:lang="fr">fable</rdfs:label>
    <skos:definition xml:lang="en">"Fictitious narratives usually with animals or inanimate objects as protagonists, intended to convey a hidden meaning regarding human conduct."  <![CDATA[<a href="#cwrc:db2f8571-a773-4068-a35f-34262950bb8f">(Getty, 2017)</a>]]></skos:definition>
    <skos:definition xml:lang="fr">Récits fictifs habituellement avec des animaux ou des objets inanimés comme protagonistes, destinés à véhiculer une signification cachée concernant la conduite humaine.</skos:definition>
    <rdfs:isDefinedBy rdf:resource="http://sparql.cwrc.ca/ontologies/genre-ONTOLOGY_DATE"/>
    <rdfs:label xml:lang="en">fable</rdfs:label>
    <owl:sameAs rdf:resource="http://vocab.getty.edu/aat/300055917"/>
    <rdfs:comment xml:lang="en">The description for this term is indebted to Dr. L. Kip Wheeler of Carson-Newman University. </rdfs:comment>
  </genre:NarrativeGenre>
  <genre:OperaGenre rdf:about="#balladOpera">
    <skos:definition xml:lang="fr">«Le ballad opera est un genre de spectacles caractéristiques de la scène anglaise du XVIIIe siècle, écrits en réaction à la prééminence de l'opéra italien sur les scènes d'alors. Il s'agissait de pièces musicales satiriques, qui suivaient certaines des conventions de l'opéra, mais sans récitatifs. Les textes de ces pièces étaient mis en musique sur des hymnes religieux, des mélodies populaires d'alors, des airs d'opéras connus, et surtout, sur des romances, des ballads populaires, qui ont donné leur nom au genre. Le fondateur du genre, et le plus fameux des ballad operas, est The Beggar's Opera, de John Gay et Johann Christoph Pepusch.»  <![CDATA[<a href="#cwrc:727d97bc-af78-4122-94be-aa78b2e97d5a">(DBpedia, 2017)</a>]]></skos:definition>
    <skos:definition xml:lang="en">"A drama combining song and spoken dialogue, popularized in the 1700s by John Gay’s The Beggar’s Opera. It can be seen as a precursor to the modern musical."  <![CDATA[<a href="#cwrc:2f09376c-f784-4a46-9f04-5a21aa311f27">(Penguin, 1999)</a>]]></skos:definition>
    <rdf:type rdf:resource="#DramaticGenre"/>
    <rdfs:label xml:lang="fr">ballad opera ou opéra-ballade</rdfs:label>
    <rdfs:comment xml:lang="en">This term and its description were created from data gathered from the Penguin Dictionary of Literary Terms &amp; Literary Theory, 4th ed.</rdfs:comment>
    <rdfs:isDefinedBy rdf:resource="http://sparql.cwrc.ca/ontologies/genre-ONTOLOGY_DATE"/>
    <rdfs:label xml:lang="en">ballad opera</rdfs:label>
    <owl:sameAs rdf:resource="http://dbpedia.org/resource/Ballad_opera"/>
    <owl:sameAs rdf:resource="http://id.loc.gov/authorities/genreForms/gf2014026645"/>
  </genre:OperaGenre>
  <genre:RomanceGenre rdf:about="#courtshipFiction">
    <rdfs:isDefinedBy rdf:resource="http://sparql.cwrc.ca/ontologies/genre-ONTOLOGY_DATE"/>
    <rdfs:label xml:lang="en">courtship fiction</rdfs:label>
    <rdf:type rdf:resource="#FictionalGenre"/>
    <skos:definition xml:lang="en">Fiction in which courtship is a major part of the plot.</skos:definition>
  </genre:RomanceGenre>
  <genre:PoeticGenre rdf:about="#occasionalPoetry">
    <skos:definition xml:lang="fr">Poésie composée en l'honneur d'une occasion particulière. Dans l'histoire de la littérature, elle est souvent étudiée en relation avec l'oralité, la performance et le mécénat.</skos:definition>
    <rdfs:label xml:lang="fr">poésie de circonstance</rdfs:label>
    <rdfs:isDefinedBy rdf:resource="http://sparql.cwrc.ca/ontologies/genre-ONTOLOGY_DATE"/>
    <rdfs:label xml:lang="en">occasional poetry</rdfs:label>
    <owl:sameAs rdf:resource="http://id.loc.gov/authorities/genreForms/gf2014026460"/>
    <skos:definition xml:lang="en">Occasional poetry is poetry composed for a particular occasion. In the history of literature, it is often studied in connection with orality, performance, and patronage. <![CDATA[<a href="#cwrc:727d97bc-af78-4122-94be-aa78b2e97d5a">(DBpedia, 2019)</a>]]></skos:definition>
    <rdfs:comment xml:lang="en">The description for this term is indebted to DBpedia. </rdfs:comment>
    <skos:closeMatch rdf:resource="http://dbpedia.org/resource/Occasional_poetry"/>
  </genre:PoeticGenre>
  <genre:JournalForm rdf:about="#journal">
    <skos:definition xml:lang="en">A journal or magazine is a regular publication which may be devoted to material of general interest, a particular subject, or a professional or academic field.</skos:definition>
    <owl:sameAs rdf:resource="http://id.loc.gov/authorities/genreForms/gf2014026139"/>
    <rdfs:isDefinedBy rdf:resource="http://sparql.cwrc.ca/ontologies/genre-ONTOLOGY_DATE"/>
    <rdfs:label xml:lang="en">journal</rdfs:label>
  </genre:JournalForm>
  <genre:StandaloneWork rdf:about="#sketchBook">
    <skos:definition xml:lang="fr">«Un carnet de croquis est un carnet utilisé par les dessinateurs, peintres et graveurs pour exécuter dessins et esquisses hors de leur atelier. Il peut être utilisé pour une modeste création ou pour préparer l’exécution d'une œuvre plus complexe. Généralement, le carnet de croquis est utilisé avec les outils de dessin : crayons, feutres, mine de plomb, pierre noire, aquarelle ou gouache. C'est souvent une ressource recherchée en histoire de l'art, pour comprendre le cheminement d'un artiste dans une œuvre ; points de passage, modèles qui inspireront les éléments de composition de l'œuvre finale.»  <![CDATA[<a href="#cwrc:727d97bc-af78-4122-94be-aa78b2e97d5a">(DBpedia, 2017)</a>]]></skos:definition>
    <owl:sameAs rdf:resource="http://id.loc.gov/authorities/genreForms/gf2017027262"/>
    <skos:definition xml:lang="en">"Books or pads of blank sheets used or intended for sketching, which are informal or rough drawings."  <![CDATA[<a href="#cwrc:db2f8571-a773-4068-a35f-34262950bb8f">(Getty, 2017)</a>]]></skos:definition>
    <rdfs:label xml:lang="fr">carnet de croquis</rdfs:label>
    <rdfs:isDefinedBy rdf:resource="http://sparql.cwrc.ca/ontologies/genre-ONTOLOGY_DATE"/>
    <rdfs:label xml:lang="en">sketch book</rdfs:label>
    <rdfs:comment xml:lang="en">The description for this term is indebted to the Getty Art &amp; Architecture Thesaurus.</rdfs:comment>
    <owl:sameAs rdf:resource="http://vocab.getty.edu/aat/300027354"/>
  </genre:StandaloneWork>
  <genre:CartographicForm rdf:about="#cartographicMaterials">
    <skos:definition xml:lang="en">"Any materials representing, in whole or part, the earth or any celestial body at any scale." <![CDATA[<a href="#cwrc:bd595bc4-5991-4c51-98d9-9ab52c416f4f">(Getty, 2021)</a>]]></skos:definition>
    <rdfs:comment xml:lang="en">The description for this term is indebted to the Getty Art &amp; Architecture Thesaurus.</rdfs:comment>
    <owl:sameAs rdf:resource="http://vocab.getty.edu/aat/300028052"/>
    <rdfs:isDefinedBy rdf:resource="http://sparql.cwrc.ca/ontologies/genre-ONTOLOGY_DATE"/>
    <rdfs:label xml:lang="en">cartographic materials</rdfs:label>
  </genre:CartographicForm>
  <genre:ThematicGenre rdf:about="#diasporic">
    <skos:altLabel xml:lang="en">diaspora</skos:altLabel>
    <skos:closeMatch rdf:resource="http://sparql.cwrc.ca/ontologies/genre.html#migration"/>
    <skos:definition xml:lang="en">"Written works or other forms of media that deals with the experiences of populations who have spread or become dispersed beyond their traditional homeland or point of origin, by either voluntary or forced means." <![CDATA[<a href="#cwrc:bd595bc4-5991-4c51-98d9-9ab52c416f4f">(Getty, 2021)</a>]]></skos:definition>
    <rdfs:comment xml:lang="en">The description for this term is indebted to the Getty Art &amp; Architecture Thesaurus.</rdfs:comment>
    <owl:sameAs rdf:resource="http://vocab.getty.edu/aat/300417673"/>
    <skos:closeMatch rdf:resource="http://sparql.cwrc.ca/ontologies/genre.html#immigration"/>
    <skos:closeMatch rdf:resource="https://sparql.cwrc.ca/ontologies/genre.html#migration"/>
    <rdfs:isDefinedBy rdf:resource="http://sparql.cwrc.ca/ontologies/genre-ONTOLOGY_DATE"/>
    <rdfs:label xml:lang="en">diasporic</rdfs:label>
    <rdf:type rdf:resource="#PoliticalGenre"/>
  </genre:ThematicGenre>
  <genre:PoeticGenre rdf:about="#epithalamium">
    <owl:sameAs rdf:resource="http://dbpedia.org/resource/Epithalamium"/>
    <skos:definition xml:lang="fr">«L'épithalame (en grec ancien ἐπιθαλάμιον / epithalámion) est une sorte de poème lyrique composé chez les Anciens à l'occasion d'un mariage et à la louange des nouveaux époux. En Grèce, il était chanté par un chœur, soit de jeunes vierges seules, soit de jeunes filles[réf. nécessaire] et de jeunes garçons, avec accompagnement de danses. On le nommait aussi catakoemèse (de catakoimân, envoyer dormir).»  <![CDATA[<a href="#cwrc:727d97bc-af78-4122-94be-aa78b2e97d5a">(DBpedia, 2017)</a>]]></skos:definition>
    <owl:sameAs rdf:resource="http://id.loc.gov/authorities/genreForms/gf2014026317"/>
    <rdfs:comment xml:lang="en">The description for this term is indebted to DBpedia. </rdfs:comment>
    <rdfs:isDefinedBy rdf:resource="http://sparql.cwrc.ca/ontologies/genre-ONTOLOGY_DATE"/>
    <rdfs:label xml:lang="en">epithalamium</rdfs:label>
    <skos:definition xml:lang="en">"An epithalamiumLatin form of Greek (ἐπιθαλάμιον epithalamion from ἐπί epi "upon," and θάλαμος thalamos nuptial chamber) is a poem written specifically for the bride on the way to her marital chamber. This form continued in popularity through the history of the classical world; the Roman poet Catullus wrote a famous epithalamium, which was translated from or at least inspired by a now-lost work of Sappho. According to Origen, Song of Songs, might be an epithalamium on the marriage of Solomon with Pharaoh’s daughter."  <![CDATA[<a href="#cwrc:727d97bc-af78-4122-94be-aa78b2e97d5a">(DBpedia, 2017)</a>]]></skos:definition>
  </genre:PoeticGenre>
  <genre:PrintMedium rdf:about="#chapbook">
    <rdfs:isDefinedBy rdf:resource="http://sparql.cwrc.ca/ontologies/genre-ONTOLOGY_DATE"/>
    <rdfs:label xml:lang="en">chapbook</rdfs:label>
    <skos:definition xml:lang="fr">"Petits livres ou brochures généralement imprimés à bon marché et contenant des textes tels que des contes populaires, des traités, des ballades ou des comptines, auparavant vendus par des chapmen." </skos:definition>
    <owl:sameAs rdf:resource="http://vocab.getty.edu/aat/300152367"/>
    <skos:definition xml:lang="en">"Small books or pamphlets, usually cheaply printed and containing such texts as popular tales, treatises, ballads, or nursery rhymes, formerly peddled by chapmen."  <![CDATA[<a href="#cwrc:db2f8571-a773-4068-a35f-34262950bb8f">(Getty, 2017)</a>]]></skos:definition>
    <skos:related rdf:resource="http://vocab.getty.edu/aat/300152367"/>
    <rdfs:comment xml:lang="en">The description for this term is indebted to the Getty Art &amp; Architecture Thesaurus.</rdfs:comment>
    <rdfs:label xml:lang="fr">chapbook</rdfs:label>
  </genre:PrintMedium>
  <genre:EmbeddedWork rdf:about="#fascicle">
    <skos:definition xml:lang="en">A bundle or bound set of pages, usually a portion of a book that is published in parts or installments, but used more rarely to refer to unpublished bundles such as Emily Dickinson’s fascicles.</skos:definition>
    <rdfs:isDefinedBy rdf:resource="http://sparql.cwrc.ca/ontologies/genre-ONTOLOGY_DATE"/>
    <rdfs:label xml:lang="en">fascicle</rdfs:label>
    <owl:sameAs rdf:resource="http://vocab.getty.edu/aat/300265628"/>
  </genre:EmbeddedWork>
  <genre:PoeticGenre rdf:about="#poeticDrama">
    <rdfs:isDefinedBy rdf:resource="http://sparql.cwrc.ca/ontologies/genre-ONTOLOGY_DATE"/>
    <rdfs:label xml:lang="en">poetic drama</rdfs:label>
    <skos:definition xml:lang="en">"Verse drama is any drama written as verse to be spoken; another possible general term is poetic drama. For a very long period, verse drama was the dominant form of drama in Europe (and was also important in non-European cultures). Greek tragedy and Racine's plays are written in verse, as is almost all of Shakespeare's drama, Ben Jonson, John Fletcher and others like Goethe's Faust. Verse drama is particularly associated with the seriousness of tragedy, providing an artistic reason to write in this form, as well as the practical one that verse lines are easier for the actors to memorize exactly. In the second half of the twentieth century verse drama fell almost completely out of fashion with dramatists writing in English (the plays of Christopher Fry and T. S. Eliot being possibly the end of a long tradition)." <![CDATA[<a href="#cwrc:727d97bc-af78-4122-94be-aa78b2e97d5a">(DBpedia, 2019)</a>]]></skos:definition>
    <owl:sameAs rdf:resource="http://id.loc.gov/authorities/genreForms/gf2014026585"/>
  </genre:PoeticGenre>
  <genre:PoeticGenre rdf:about="#versePoem">
    <skos:definition xml:lang="en">"In the uncountable (mass noun) sense verse refers to "poetry" as contrasted to prose. Where the common unit of verse is based on meter or rhyme, , ."" <![CDATA[<a href="#cwrc:727d97bc-af78-4122-94be-aa78b2e97d5a">(DBpedia, 2019)</a>]]></skos:definition>
    <rdfs:isDefinedBy rdf:resource="http://sparql.cwrc.ca/ontologies/genre-ONTOLOGY_DATE"/>
    <rdfs:label xml:lang="en">verse poem</rdfs:label>
  </genre:PoeticGenre>
  <genre:NarrativeGenre rdf:about="#episodicLiterature">
    <skos:definition xml:lang="en">"Episodic storytelling is when a story is narrated through episodes, as opposed to chapters, which are typically seen in novels. The term used in literature to refer to a body of work composed of episodes or similar installments is serial. Serials are also known as episodic fiction. Multiple episodes are usually grouped together into a series through a unifying story arc. Episodes may not always contain the same characters, but each episode draws from a broader group of characters, or cast, all of whom exist in the same story world." <![CDATA[<a href="#cwrc:727d97bc-af78-4122-94be-aa78b2e97d5a">(DBpedia, 2019)</a>]]></skos:definition>
    <rdfs:isDefinedBy rdf:resource="http://sparql.cwrc.ca/ontologies/genre-ONTOLOGY_DATE"/>
    <rdfs:label xml:lang="en">episodic literature</rdfs:label>
  </genre:NarrativeGenre>
  <genre:IntertextualGenre rdf:about="#adaptation">
    <rdfs:isDefinedBy rdf:resource="http://sparql.cwrc.ca/ontologies/genre-ONTOLOGY_DATE"/>
    <rdfs:label xml:lang="en">adaptation</rdfs:label>
    <skos:definition xml:lang="en">W"ritten works or works derived from written works, where the second work is an alteration or amendment a text to make it suitable for another purpose. An example of an adaptation is a version of an earlier text made to better agree with a philosophy other than that intended by the original. Other examples are written works adapted for another medium, such as film, broadcasting, or stage production." <![CDATA[<a href="#cwrc:db2f8571-a773-4068-a35f-34262950bb8f">(Getty, 2017)</a>]]></skos:definition>
    <skos:definition xml:lang="fr">Œuvres écrites ou travaux dérivés d'œuvres écrites, qui sont des altérations ou des modifications d'un texte pour qu'il convienne à d'autres fins. Par exemple, un texte ancien peut être réécrit pour transmettre une morale différente de celle qui était initialement prévue. Les œuvres écrites pour être adaptées à un autre support, tel que l'audiovisuel, la télévision ou le théâtre sont des exemples d'adaptation.</skos:definition>
    <rdfs:label xml:lang="fr">adaptation</rdfs:label>
    <owl:sameAs rdf:resource="http://id.loc.gov/authorities/genreForms/gf2014026041"/>
    <rdfs:comment xml:lang="en">The description for this term is indebted to the Getty Art &amp; Architecture Thesaurus.</rdfs:comment>
    <skos:closeMatch rdf:resource="http://vocab.getty.edu/aat/300410356"/>
  </genre:IntertextualGenre>
  <genre:TextualMedium rdf:about="#manuscript">
    <skos:definition xml:lang="en">"A manuscript (abbreviated MS for singular and MSS for plural) is any document written by hand or typewritten, as opposed to being mechanically printed or reproduced in some automated way. More recently, it is understood to be an author's written, typed, or word-processed copy of a work, as distinguished from the print of the same. Before the arrival of printing, all documents and books were manuscripts. Manuscripts are not defined by their contents, which may combine writing with mathematical calculations, maps, explanatory figures or illustrations. Manuscripts may be in book form, scrolls or in codex format. Illuminated manuscripts are enriched with pictures, border decorations, elaborately embossed initial letters or full-page illustrations." <![CDATA[<a href="#cwrc:727d97bc-af78-4122-94be-aa78b2e97d5a">(DBpedia, 2019)</a>]]></skos:definition>
    <skos:related rdf:resource="http://vocab.getty.edu/aat/300028569"/>
    <rdfs:isDefinedBy rdf:resource="http://sparql.cwrc.ca/ontologies/genre-ONTOLOGY_DATE"/>
    <rdfs:label xml:lang="en">manuscript</rdfs:label>
  </genre:TextualMedium>
  <genre:ThematicGenre rdf:about="#juvenile">
    <skos:definition xml:lang="en">"Literary or artistic works produced by persons in their childhood or youth; usually used to set those works apart from later, mature works." <![CDATA[<a href="#cwrc:bd595bc4-5991-4c51-98d9-9ab52c416f4f">(Getty, 2021)</a>]]></skos:definition>
    <rdfs:comment xml:lang="en">The description for this term is indebted to the Getty Art &amp; Architecture Thesaurus.</rdfs:comment>
    <owl:sameAs rdf:resource="http://vocab.getty.edu/aat/300028883"/>
    <skos:closeMatch rdf:resource="https://sparql.cwrc.ca/ontologies/genre.html#childrensLiterature"/>
    <skos:closeMatch rdf:resource="https://sparql.cwrc.ca/ontologies/genre.html#preSchool"/>
    <rdfs:isDefinedBy rdf:resource="http://sparql.cwrc.ca/ontologies/genre-ONTOLOGY_DATE"/>
    <rdfs:label xml:lang="en">juvenile</rdfs:label>
  </genre:ThematicGenre>
  <genre:PoeticGenre rdf:about="#topographicalPoetry">
    <rdfs:comment xml:lang="en">This term and its description were created from data gathered from data.bnf.</rdfs:comment>
    <owl:sameAs rdf:resource="http://id.loc.gov/authorities/genreForms/gf2018026132"/>
    <rdfs:isDefinedBy rdf:resource="http://sparql.cwrc.ca/ontologies/genre-ONTOLOGY_DATE"/>
    <rdfs:label xml:lang="en">topographical poetry</rdfs:label>
    <rdfs:label xml:lang="fr">poésie des lieux</rdfs:label>
    <skos:definition xml:lang="en">"Topographical poetry or loco-descriptive poetry is a genre of poetry that describes, and often praises, a landscape or place. John Denham's 1642 poem "Cooper's Hill" established the genre, which peaked in popularity in 18th-century England. Examples of topographical verse date, however, to the late classical period, and can be found throughout the medieval era and during the Renaissance. Though the earliest examples come mostly from continental Europe, the topographical poetry in the tradition originating with Denham concerns itself with the classics, and many of the various types of topographical verse, such as river, ruin, or hilltop poems were established by the early 17th century. Alexander Pope's "Windsor Forest" (1713) and John Dyer's "Grongar Hill' (1762) are two other oft-mentioned examples. More recently, Matthew Arnold's "The Scholar Gipsy" (1853) praises the Oxfordshire countryside, and W. H. Auden's "In Praise of Limestone" (1948) uses a limestone landscape as an allegory. Subgenres of topographical poetry include the country house poem, written in 17th-century England to compliment a wealthy patron, and the prospect poem, describing the view from a distance or a temporal view into the future, with the sense of opportunity or expectation. When understood broadly as landscape poetry and when assessed from its establishment to the present, topographical poetry can take on many formal situations and types of places. Kenneth Baker identifies 37 varieties and compiles poems from the 16th through the 20th centuries—from Edmund Spenser to Sylvia Plath—correspondent to each type, from "Walks and Surveys," to "Mountains, Hills, and the View from Above," to "Violation of Nature and the Landscape," to "Spirits and Ghosts." Common aesthetic registers of which topographical poetry make use include pastoral imagery, the sublime, and the picturesque. These latter two registers subsume imagery of rivers, ruins, moonlight, birdsong, and clouds, peasants, mountains, caves, and waterscapes."  <![CDATA[<a href="#cwrc:727d97bc-af78-4122-94be-aa78b2e97d5a">(DBpedia, 2017)</a>]]></skos:definition>
    <owl:sameAs rdf:resource="http://dbpedia.org/resource/Topographical_poetry"/>
    <skos:definition xml:lang="fr">Recueils de poésie célébrant des lieux situés dans différentes parties du monde.</skos:definition>
  </genre:PoeticGenre>
  <genre:PoliticalGenre rdf:about="#feminist">
    <skos:definition xml:lang="fr">Textes qui peuvent être considérés comme féministes dans la mesure où ils abordent de façon critique et consciente les inégalités entre hommes et femmes, ou parmi les individus d'identités genrées diverses. Un texte, fictif ou non, entre généralement dans cette catégorie s'il reflète des théories féministes ou est engagé dans des mouvements politiques féministes. Les aspects féministes d'un texte peuvent être explicites ou implicites, et sont fortement sujets à débat étant donné la grande pluralité de type de féminisme.</skos:definition>
    <rdf:type rdf:resource="#ThematicGenre"/>
    <rdfs:comment xml:lang="en">The description for this term is indebted to Dr. L. Kip Wheeler of Carson-Newman University. </rdfs:comment>
    <dcterms:references rdf:resource="http://web.cn.edu/kwheeler/lit_terms_f.html"/>
    <rdf:type rdf:resource="#FeministGenre"/>
    <rdfs:label xml:lang="fr">féministe</rdfs:label>
    <rdfs:isDefinedBy rdf:resource="http://sparql.cwrc.ca/ontologies/genre-ONTOLOGY_DATE"/>
    <rdfs:label xml:lang="en">feminist</rdfs:label>
    <skos:definition xml:lang="en">"Writing concerned with the unique experience of being a woman or alternatively writing designed to challenge existing preconceptions of gender. Examples of feminist writings include Christine de Pisan's medieval work, The City of Ladies; Aemilia Lanyer's Renaissance treatise, Salve Deus, Rex Judaeorum (which presented the then-shocking idea that Adam was just as much to blame for the fall of man as Eve was in the Genesis account); Mary Wollstonecraft's Vindication, and Susan B. Anthony's nineteenth-century essays (which presented the equally shocking idea that women in America and Canada should have the right to vote). Many female students in my class preface their discussions of feminist writings by stating, "I'm not a feminist, but ..." This tendency always puzzled me, since it implies that feminism is something negative, radical, or always liberal. Worse yet, it implies that it's bad for women to want crazy, misguided things like education, equal health insurance, similar pay to what men earn in similar professions, freedom from harassment, and funding for medical problems concerning women, such as breast and uterine cancer research, which are the primary concerns of feminism. Somewhere toward the end of the twentieth-century, detractors of such writers have caricatured these demands as "man-hating" or "anti-family." As an antidote to such thinking, keep in mind the broader definition: a feminist is anyone who thinks that women are people too."  <![CDATA[<a href="cwrc:509015ff-7641-473e-94c5-688e06952bb7">(L. K Wheeler, 2017)</a>]]></skos:definition>
  </genre:PoliticalGenre>
  <genre:NarrativeGenre rdf:about="#cautionaryTale">
    <skos:definition xml:lang="en">"Stories, verses, or writings usually intended for children, admonishing or warning of the consequences of misbehavior or foolishness; also, in various disciplines, refers to writings warning of possible methodological pitfalls." <![CDATA[<a href="#cwrc:bd595bc4-5991-4c51-98d9-9ab52c416f4f">(Getty, 2021)</a>]]></skos:definition>
    <rdfs:comment xml:lang="en">This term and its description were created from data gathered from the Getty Art &amp; Architecture Thesaurus.</rdfs:comment>
    <owl:sameAs rdf:resource="http://vocab.getty.edu/aat/300255312"/>
    <rdfs:isDefinedBy rdf:resource="http://sparql.cwrc.ca/ontologies/genre-ONTOLOGY_DATE"/>
    <rdfs:label xml:lang="en">cautionary tale</rdfs:label>
  </genre:NarrativeGenre>
  <genre:PoeticGenre rdf:about="#graveyardPoetry">
    <rdfs:comment xml:lang="en">This term and its description were created from data gathered from the Oxford Dictionary of Literary Terms, 4th ed.</rdfs:comment>
    <rdfs:label xml:lang="fr">graveyard poetry</rdfs:label>
    <owl:sameAs rdf:resource="http://id.loc.gov/authorities/genreForms/gf2014026364"/>
    <skos:definition xml:lang="fr">Mouvement poétique rattaché au romantisme britannique du 18ème siècle, traitant de la mort et de l'immortalité. Le nom provient du cadre habituel décrit et traité dans ces poèmes, le cimetière.</skos:definition>
    <rdfs:isDefinedBy rdf:resource="http://sparql.cwrc.ca/ontologies/genre-ONTOLOGY_DATE"/>
    <rdfs:label xml:lang="en">graveyard poetry</rdfs:label>
    <dcterms:references rdf:resource="http://www.oxfordreference.com/view/10.1093/acref/9780199208272.001.0001/acref-9780199208272-e-511?rskey=ejri5r%26result=511"/>
    <skos:definition xml:lang="en">"An 18th-century poetic form dealing with the subjects of death and immortality. The name originates from the setting typical of these poems: the graveyard."  <![CDATA[<a href="#cwrc:4c227091-6bf0-4325-b846-9733fae19e61">(Oxford, 2015)</a>]]></skos:definition>
  </genre:PoeticGenre>
  <genre:PoeticGenre rdf:about="#sonnet">
    <rdfs:isDefinedBy rdf:resource="http://sparql.cwrc.ca/ontologies/genre-ONTOLOGY_DATE"/>
    <rdfs:label xml:lang="en">sonnet</rdfs:label>
    <rdfs:label xml:lang="fr">sonnet</rdfs:label>
    <skos:definition xml:lang="en">"Poems consisting of 14 decasyllabic lines, often in a rhyming scheme. The sonnet form is considered to be of Italian origin, appearing in the 13th century in Sicily, after which it spread to Tuscany, where Petrarch perfected the form with his Canzioniere, a series of 317 sonnets to his idealized love, Laura. The Petrarchian sonnet has historically been the most widely used of the form, although the Elizabethan form (3 quatrains, with a final rhyming couplet) is also common."  <![CDATA[<a href="#cwrc:db2f8571-a773-4068-a35f-34262950bb8f">(Getty, 2017)</a>]]></skos:definition>
    <owl:sameAs rdf:resource="http://vocab.getty.edu/aat/300266382"/>
    <rdfs:comment xml:lang="en">This term and its description were created from data gathered from DBpedia.</rdfs:comment>
    <owl:sameAs rdf:resource="http://id.loc.gov/authorities/genreForms/gf2014026549"/>
    <skos:definition xml:lang="fr">«Un sonnet (de l'italien sonnetto ou sonetto aujourd'hui) est une forme de poème comportant quatorze vers dont la répartition typographique peut varier — deux quatrains et deux tercets ou un seul sizain final par exemple — et dont le schéma des rimes varie également, soit librement soit en suivant des dispositions régulières. La longueur du vers n'est pas fixe en français. Le sonnet est un genre qui a été pratiqué dans une bonne partie de l'Europe, tant dans les poésies syllabiques que rythmiques.»  <![CDATA[<a href="#cwrc:727d97bc-af78-4122-94be-aa78b2e97d5a">(DBpedia, 2017)</a>]]></skos:definition>
  </genre:PoeticGenre>
  <genre:PoeticGenre rdf:about="#clerihew">
    <rdfs:isDefinedBy rdf:resource="http://sparql.cwrc.ca/ontologies/genre-ONTOLOGY_DATE"/>
    <rdfs:label xml:lang="en">clerihew</rdfs:label>
    <skos:definition xml:lang="en">"A clerihew is a whimsical, four-line biographical poem invented by Edmund Clerihew Bentley. The first line is the name of the poem's subject, usually a famous person put in an absurd light. The rhyme scheme is AABB, and the rhymes are often forced. The line length and metre are irregular. Bentley invented the clerihew in school and then popularized it in books."  <![CDATA[<a href="#cwrc:727d97bc-af78-4122-94be-aa78b2e97d5a">(DBpedia, 2017)</a>]]></skos:definition>
    <rdfs:label xml:lang="fr">clerihew</rdfs:label>
    <rdfs:comment xml:lang="en">The description for this term is indebted to DBpedia. </rdfs:comment>
    <skos:definition xml:lang="fr">"Un clerihew est un poème biographique et excentrique de quatre vers inventé par Edmund Clerihew Bentley. La première ligne est le nom du sujet du poème, généralement une personne célèbre mise en scène de façon absurde. Le schéma des rimes est AABB, et celles-ci sont souvent forcées. La longueur du vers et le mètre sont irréguliers. Bentley a inventé le clerihew à l'école et l'a ensuite popularisé dans des livres." </skos:definition>
    <owl:sameAs rdf:resource="http://id.loc.gov/authorities/genreForms/gf2014026261"/>
    <owl:sameAs rdf:resource="http://dbpedia.org/resource/Clerihew"/>
  </genre:PoeticGenre>
  <genre:InformationalGenre rdf:about="#documentary">
    <skos:definition xml:lang="fr">Enregistrements écrits, oraux, sonores ou photographiques, ou représentations dans d'autres média qui expliquent ou recréent des événements réels, des épisodes, des histoires de vie ou d'autres informations factuelles d'une façon qui se veut objective et précise.</skos:definition>
    <rdfs:isDefinedBy rdf:resource="http://sparql.cwrc.ca/ontologies/genre-ONTOLOGY_DATE"/>
    <rdfs:label xml:lang="en">documentary</rdfs:label>
    <owl:sameAs rdf:resource="http://vocab.getty.edu/aat/300249172"/>
    <rdfs:comment xml:lang="en">This term and its description were created from data gathered from the Getty Art &amp; Architecture Thesaurus.</rdfs:comment>
    <skos:definition xml:lang="en">"Written, oral, sound, or photographic recordings, or presentations in other media that explain or re-create actual events, eras, life stories, or other factual information in a manner purporting to be objective and accurate."  <![CDATA[<a href="#cwrc:db2f8571-a773-4068-a35f-34262950bb8f">(Getty, 2017)</a>]]></skos:definition>
    <rdfs:label xml:lang="fr">documentaire</rdfs:label>
  </genre:InformationalGenre>
  <genre:PoeticGenre rdf:about="#narrativePoetry">
    <owl:sameAs rdf:resource="http://id.loc.gov/authorities/genreForms/gf2014026448"/>
    <skos:definition xml:lang="en">"Narrative poetry is a form of poetry that tells a story, often making use of the voices of a narrator and characters as well; the entire story is usually written in metred verse. Narrative poems do not have to follow rhythmic patterns. The poems that make up this genre may be short or long, and the story it relates to may be complex. It is usually well it normally dramatic, with objectives, diverse characters, and metre. Narrative poems include epics, ballads, idylls, and lays. Some narrative poetry takes the form of a novel in verse. An example of this is The Ring and the Book by Robert Browning. In terms of narrative poetry, a romance is a narrative poem that tells a story of chivalry. Examples include the Romance of the Rose or Tennyson's Idylls of the King. Although these examples use medieval and Arthurian materials, romances may also tell stories from classical mythology. Shorter narrative poems are often similar in style to the short story. Sometimes these short narratives are collected into interrelated groups, as with Chaucer's The Canterbury Tales. Some literatures contain prose naose narratives, and the Old Norse sagas include both incidental poetry and the biographies of poets. An example is "The Cremation of Sam McGee" by Robert Service."  <![CDATA[<a href="#cwrc:727d97bc-af78-4122-94be-aa78b2e97d5a">(DBpedia, 2017)</a>]]></skos:definition>
    <rdfs:comment xml:lang="en">The description for this term is indebted to DBpedia. </rdfs:comment>
    <skos:definition xml:lang="fr">«La poésie narrative est un courant de la poésie italienne contemporaine dont les principaux représentants sont Carlo Bordini, Mauro Fabi et Andrea di Consoli. Cette poésie, qui sans renoncer à sa dimension expérimentale ou à une certaine forme de lyrisme exploite des matériaux divers - en usant du collage ou en incluant des fragments discursifs ou narratifs - et s'appuie sur le rythme et l'oralité non pour cacher le sens, mais pour le révéler.»  <![CDATA[<a href="#cwrc:727d97bc-af78-4122-94be-aa78b2e97d5a">(DBpedia, 2017)</a>]]></skos:definition>
    <rdfs:isDefinedBy rdf:resource="http://sparql.cwrc.ca/ontologies/genre-ONTOLOGY_DATE"/>
    <rdfs:label xml:lang="en">narrative poetry</rdfs:label>
    <owl:sameAs rdf:resource="http://dbpedia.org/resource/Narrative_poetry"/>
  </genre:PoeticGenre>
  <genre:ScriptForm rdf:about="#radioScript">
    <rdfs:isDefinedBy rdf:resource="http://sparql.cwrc.ca/ontologies/genre-ONTOLOGY_DATE"/>
    <rdfs:label xml:lang="en">radio script</rdfs:label>
    <skos:definition xml:lang="en">"Texts for a broadcast announcement, talk, play, or other productions intended for radio." <![CDATA[<a href="#cwrc:bd595bc4-5991-4c51-98d9-9ab52c416f4f">(Getty, 2021)</a>]]></skos:definition>
    <rdfs:comment xml:lang="en">This term and its description were created from data gathered from the Getty Art &amp; Architecture Thesaurus.</rdfs:comment>
    <owl:sameAs rdf:resource="http://vocab.getty.edu/aat/300026489"/>
  </genre:ScriptForm>
  <genre:ScholarlyGenre rdf:about="#research">
    <rdfs:isDefinedBy rdf:resource="http://sparql.cwrc.ca/ontologies/genre-ONTOLOGY_DATE"/>
    <rdfs:label xml:lang="en">research</rdfs:label>
  </genre:ScholarlyGenre>
  <genre:IntertextualGenre rdf:about="#parody">
    <rdfs:comment xml:lang="en">The description for this term is indebted to DBpedia. </rdfs:comment>
    <skos:definition xml:lang="en">"A parody (/ˈpærədi/; also called spoof, send-up, take-off or lampoon), in use, is a work created to imitate, make fun of, or comment on an original work, its subject, author, style, or some other target, by means of satiric or ironic imitation. As the literary theorist Linda Hutcheon puts it, "parody … is imitation, not always at the expense of the parodied text." Another critic, Simon Dentith, defines parody as "any cultural practice which provides a relatively polemical allusive imitation of another cultural production or practice."Parody may be found in art or culture, including literature, music (although "parody" in music has an earlier, somewhat different meaning than for other art forms), animation, gaming and film. The writer and critic John Gross observes in his Oxford Book of Parodies, that parody seems to flourish on territory somewhere between pastiche ("a composition in another artist's manner, without satirical intent") and burlesque (which "fools around with the material of high literature and adapts it to low ends"). Meanwhile, the Encyclopédie of Denis Diderot distinguishes between the parody and the burlesque, "A good parody is a fine amusement, capable of amusing and instructing the most sensible and polished minds; the burlesque is a miserable buffoonery which can only please the populace." Historically, when a formula grows tired, as in the case of the moralistic melodramas in the 1910s, it retains value only as a parody, as demonstrated by the Buster Keaton shorts that mocked that genre. In his 1960 anthology of parody from the 14th through 20th centuries, critic Dwight Macdonald offered this metaphor: "Parody is making a new wine that tastes like the old but has a slightly lethal effect."  <![CDATA[<a href="#cwrc:727d97bc-af78-4122-94be-aa78b2e97d5a">(DBpedia, 2017)</a>]]></skos:definition>
    <owl:sameAs rdf:resource="http://id.loc.gov/authorities/genreForms/gf2014026470"/>
    <skos:definition xml:lang="fr">«La parodie est une forme d'humour qui utilise le cadre, les personnages, le style et le fonctionnement d'une œuvre ou une institution pour s'en moquer. Elle se base entre autres sur l'inversion et l'exagération des caractéristiques appartenant au sujet parodié. Selon Dominique Maingueneau, la parodie constitue une « stratégie de réinvestissement d'un texte ou d'un genre de discours dans d'autres » : il s'agit d'une stratégie de « subversion », visant à disqualifier l'auteur du texte ou du genre source, tandis que la stratégie opposée (la « captation », imitation positive) permet de « transférer sur le discours réinvestisseur l'autorité attachée au texte ou au genre source ».»  <![CDATA[<a href="#cwrc:727d97bc-af78-4122-94be-aa78b2e97d5a">(DBpedia, 2017)</a>]]></skos:definition>
    <owl:sameAs rdf:resource="http://dbpedia.org/resource/Parody"/>
    <rdfs:isDefinedBy rdf:resource="http://sparql.cwrc.ca/ontologies/genre-ONTOLOGY_DATE"/>
    <rdfs:label xml:lang="en">parody</rdfs:label>
  </genre:IntertextualGenre>
  <genre:PedagogicalGenre rdf:about="#textbook">
    <skos:definition xml:lang="en">"Books used as standard works for the formal study of a particular subject."  <![CDATA[<a href="#cwrc:db2f8571-a773-4068-a35f-34262950bb8f">(Getty, 2017)</a>]]></skos:definition>
    <skos:definition xml:lang="fr">«Le manuel scolaire (du latin manus, « la main »), considéré au XIXe siècle comme le livre résumant tous les autres est un ouvrage didactique ayant un format maniable et regroupant l'essentiel des connaissances relatives à un domaine donné. Le manuel scolaire est destiné à être utilisé en classe comme support de cours avec l'aide directe ou indirecte d'un enseignant. Il doit tenir compte du caractère progressif de l'apprentissage (âge des élèves, capacité cognitive).»  <![CDATA[<a href="#cwrc:727d97bc-af78-4122-94be-aa78b2e97d5a">(DBpedia, 2017)</a>]]></skos:definition>
    <rdfs:label xml:lang="fr">manuel scolaire</rdfs:label>
    <rdfs:comment xml:lang="en">The description for this term is indebted to the Getty Art &amp; Architecture Thesaurus.</rdfs:comment>
    <rdfs:isDefinedBy rdf:resource="http://sparql.cwrc.ca/ontologies/genre-ONTOLOGY_DATE"/>
    <rdfs:label xml:lang="en">textbook</rdfs:label>
    <owl:sameAs rdf:resource="http://vocab.getty.edu/aat/300026384"/>
    <owl:sameAs rdf:resource="http://id.loc.gov/authorities/genreForms/gf2014026191"/>
  </genre:PedagogicalGenre>
  <genre:DigitalMedium rdf:about="#bornDigital">
    <skos:definition xml:lang="en">"Material or content created in electronic form and saved as digital data, having had no initial or interstitial state as an analog or physical product." <![CDATA[<a href="#cwrc:bd595bc4-5991-4c51-98d9-9ab52c416f4f">(Getty, 2021)</a>]]></skos:definition>
    <rdfs:comment xml:lang="en">The description for this term is indebted to the Getty Art &amp; Architecture Thesaurus.</rdfs:comment>
    <owl:sameAs rdf:resource="http://vocab.getty.edu/aat/300374824"/>
    <skos:related rdf:resource="http://vocab.getty.edu/aat/300374824"/>
    <rdfs:isDefinedBy rdf:resource="http://sparql.cwrc.ca/ontologies/genre-ONTOLOGY_DATE"/>
    <skos:narrower rdf:resource="https://sparql.cwrc.ca/ontologies/genre.html#digital"/>
    <rdfs:label xml:lang="en">born digital</rdfs:label>
  </genre:DigitalMedium>
  <genre:ThematicGenre rdf:about="#lgbtq">
    <skos:definition xml:lang="en">"LGBT, or GLBT, is an initialism that stands for lesbian, gay, bisexual, and transgender. In use since the 1990s, the term is an adaptation of the initialism LGB, which was used to replace the term gay in reference to the LGBT community beginning in the mid-to-late 1980s. Activists believed that the term gay community did not accurately represent all those to whom it referred. The initialism has become mainstream as a self-designation; it has been adopted by the majority of sexuality and gender identity-based community centers and media in the United States, as well as some other English-speaking countries. The term is used also in some other countries, particularly those which languages use the initialism, such as Argentina, France and Turkey. The initialism LGBT is intended to emphasize a diversity of sexuality and gender identity-based cultures. It may be used to refer to anyone who is non-heterosexual or non-cisgender, instead of exclusively to people who are lesbian, gay, bisexual, or transgender. To recognize this inclusion, a popular variant adds the letter Q for those who identify as queer or are questioning their sexual identity; LGBTQ has been recorded since 1996. Those who wish to include intersex people in LGBT groups suggest an extended initialism LGBTI. This initialism is used in all parts of "The Activist's Guide" of the Yogyakarta Principles in Action. Some people combine the two acronyms and use the term LGBTIQ. Whether or not LGBT people openly identify themselves may depend on local political concerns and whether they live in a discriminatory environment, as well as on the status of LGBT rights where they live." <![CDATA[<a href="#cwrc:727d97bc-af78-4122-94be-aa78b2e97d5a">(DBpedia, 2019)</a>]]></skos:definition>
    <rdfs:isDefinedBy rdf:resource="http://sparql.cwrc.ca/ontologies/genre-ONTOLOGY_DATE"/>
    <rdfs:label xml:lang="en">lgbtq</rdfs:label>
    <rdf:type rdf:resource="#LGBTQPlusGenre"/>
  </genre:ThematicGenre>
  <genre:StillImageMedium rdf:about="#photograph">
    <skos:related rdf:resource="http://vocab.getty.edu/aat/300046300"/>
    <rdfs:isDefinedBy rdf:resource="http://sparql.cwrc.ca/ontologies/genre-ONTOLOGY_DATE"/>
    <rdfs:label xml:lang="en">photograph</rdfs:label>
    <skos:definition xml:lang="en">"A photograph or photo is an image created by light falling on a light-sensitive surface, usually photographic film or an electronic medium such as a CCD or a CMOS chip. Most photographs are created using a camera, which uses a lens to focus the scene's visible wavelengths of light into a reproduction of what the human eye would see. The process and practice of creating photographs is called photography. The word "photograph" was coined in 1839 by Sir John Herschel and is based on the Greek φῶς (phos), meaning "light", and γραφή (graphê), meaning "drawing, writing", together meaning "drawing with light"." <![CDATA[<a href="#cwrc:727d97bc-af78-4122-94be-aa78b2e97d5a">(DBpedia, 2019)</a>]]></skos:definition>
    <rdf:type rdf:resource="#VisualArtMedium"/>
  </genre:StillImageMedium>
  <genre:ThematicGenre rdf:about="#comingOut">
    <rdfs:label xml:lang="fr">coming out</rdfs:label>
    <skos:definition xml:lang="en">Pertaining to the process of coming out sexually.</skos:definition>
    <skos:definition xml:lang="fr">Qui se rapporte au processus de révélation publique de sa sexualité.</skos:definition>
    <rdfs:isDefinedBy rdf:resource="http://sparql.cwrc.ca/ontologies/genre-ONTOLOGY_DATE"/>
    <rdfs:label xml:lang="en">coming out</rdfs:label>
    <rdf:type rdf:resource="#LGBTQPlusGenre"/>
  </genre:ThematicGenre>
  <genre:MusicalGenre rdf:about="#musicalWriting">
    <rdfs:isDefinedBy rdf:resource="http://sparql.cwrc.ca/ontologies/genre-ONTOLOGY_DATE"/>
    <rdfs:label xml:lang="en">musical writing</rdfs:label>
    <skos:definition xml:lang="en">Writing associated with some form of music.</skos:definition>
    <rdf:type rdf:resource="#InformationalGenre"/>
  </genre:MusicalGenre>
  <genre:ComedicGenre rdf:about="#comedyOfManners">
    <skos:definition xml:lang="en">"The comedy of manners is an entertainment form which satirizes the manners and affectations of a social class or of multiple classes, often represented by stereotypical stock characters. For example, the miles gloriosus ("boastful soldier") in ancient times, the fop and the rake during the English Restoration, or an old person pretending to be young. Restoration comedy is used as a synonym for "comedy of manners". The plot of the comedy, often concerned with scandal, is generally less important than its witty dialogue. A great writer of comedies of manners was Oscar Wilde, his most famous play being The Importance of Being Earnest. The comedy of manners was first developed in the new comedy of the Ancient Greek playwright Menander. His style, elaborate plots, and stock characters were imitated by the Roman playwrights Plautus and Terence, whose comedies were widely known and copied during the Renaissance. The best-known comedies of manners, however, may well be those of the French playwright Molière, who satirized the hypocrisy and pretension of the ancien régime in such plays as L'École des femmes (The School for Wives, 1662), Le Misanthrope (The Misanthrope, 1666), and most famously Tartuffe (1664)."  <![CDATA[<a href="#cwrc:727d97bc-af78-4122-94be-aa78b2e97d5a">(DBpedia, 2017)</a>]]></skos:definition>
    <rdfs:comment xml:lang="en">The description for this term is indebted to DBpedia. </rdfs:comment>
    <owl:sameAs rdf:resource="http://id.loc.gov/authorities/genreForms/gf2014026263"/>
    <owl:sameAs rdf:resource="http://dbpedia.org/resource/Comedy_of_manners"/>
    <rdfs:isDefinedBy rdf:resource="http://sparql.cwrc.ca/ontologies/genre-ONTOLOGY_DATE"/>
    <rdfs:label xml:lang="en">comedy of manners</rdfs:label>
    <skos:definition xml:lang="fr">«La comédie de mœurs est un sous-genre de la comédie qui se développe à partir du XVIe siècle. Y sont dénoncés les travers d'une époque, d'un groupe ou d'une classe sociale, généralement dominante. La comédie de mœurs est souvent caractérisée par une critique sociale qui reste superficielle. Généralement la dimension satirique ne vise qu'un travers particulier ou une convention risible très ciblée de la communauté dépeinte. En ce sens, la comédie de mœurs ne remet souvent rien de fondamental en cause dans la structure sociale ni dans la représentation dominante de l'époque. La critique s'efface vite et devient récupérable par l'ordre en place, comme dans les pièces d'Émile Augier ou d'Alexandre Dumas fils. Cependant, le dénouement peut aussi être impressionnant, comme celui des Affaires sont les affaires du libertaire Octave Mirbeau (1903), parfois qualifié de "shakespearien". Plusieurs comédies très connues de Molière sont des comédies de mœurs : Les Précieuses ridicules ou encore Les Femmes savantes mais aussi L'École des femmes. Pour Molière, la comédie de mœurs représente un lieu privilégié pour la satire sociale.»  <![CDATA[<a href="#cwrc:727d97bc-af78-4122-94be-aa78b2e97d5a">(DBpedia, 2017)</a>]]></skos:definition>
  </genre:ComedicGenre>
  <genre:ReligiousGenre rdf:about="#biblicalParaphrase">
    <rdfs:label xml:lang="fr">paraphrase biblique</rdfs:label>
    <skos:definition xml:lang="fr">Texte qui reprend les paroles de la Bible, souvent dans l'objectif d'en améliorer la clarté ou de la rendre plus accessibleau large public.</skos:definition>
    <rdfs:isDefinedBy rdf:resource="http://sparql.cwrc.ca/ontologies/genre-ONTOLOGY_DATE"/>
    <rdfs:label xml:lang="en">biblical paraphrase</rdfs:label>
    <skos:definition xml:lang="en">A work that rewords the text of the Bible, often to improve clarity or to make it accessible to a wider audience.</skos:definition>
    <rdf:type rdf:resource="#LiteraryGenre"/>
  </genre:ReligiousGenre>
  <genre:DramaticGenre rdf:about="#improvisation">
    <rdfs:isDefinedBy rdf:resource="http://sparql.cwrc.ca/ontologies/genre-ONTOLOGY_DATE"/>
    <rdfs:label xml:lang="en">improvisation</rdfs:label>
    <skos:definition xml:lang="en">"Improvisation is the process of devising a solution to a requirement by making-do, despite absence of resources that might be expected to produce a solution. In a technical context, this can mean adapting a device for some use other than that which it was designed for, or building a device from unusual components in an ad-hoc fashion. Improvisation as a context of performing arts is a very spontaneous performance without specific preparation. The skills of improvisation can apply to many different faculties, across all artistic, scientific, physical, cognitive, academic, and non-academic disciplines. Musical improvisation is usually defined as the composition of music while simultaneously singing or playing an instrument. Improvisational comedy is a theatre art performed throughout the world and has had on-again, off-again status throughout history. Dance improvisation is frequently used as a choreographic tool. Choreography is also frequently used as a tool for improvisation. Improvisation was originally rarely used on dramatic television. A major exception was the situation comedy Mork &amp; Mindy where star Robin Williams, famed for this kind of performing, was allotted specific sections in each episode where he was allowed to perform freely. Improvisation also exists outside the arts. Improvisation in engineering is to solve a problem with the tools and materials immediately at hand. Improvised weapons are often used by guerrillas, insurgents and criminals." <![CDATA[<a href="#cwrc:727d97bc-af78-4122-94be-aa78b2e97d5a">(DBpedia, 2019)</a>]]></skos:definition>
  </genre:DramaticGenre>
  <genre:FictionalGenre rdf:about="#adventureWriting">
    <skos:definition xml:lang="fr">Fiction remplie de péripéties dans laquelle la ou le protagoniste échappe à son quotidien pour entreprendre un voyage ou une quête. En chemin, elle ou il est exposé.e à des événements extraordinaires et à des dangers physiques qui mettent à l'épreuve ses vertus, par exemple la bravoure.</skos:definition>
    <dcterms:references rdf:resource="http://www.oxfordreference.com/view/10.1093/acref/9780199208272.001.0001/acref-9780199208272-e-15?rskey=BDrsna%26result=11"/>
    <rdfs:label xml:lang="fr">roman d'aventures</rdfs:label>
    <skos:definition xml:lang="en">"Action-filled fiction in which a protagonist is removed from her or his ordinary life to undertake some sort of journey or quest. Along the way, the protagonist is exposed to extraordinary events and physical dangers that put his or her virtues, such as bravery, to the test."  <![CDATA[<a href="#cwrc:4c227091-6bf0-4325-b846-9733fae19e61">(Oxford, 2015)</a>]]></skos:definition>
    <rdfs:isDefinedBy rdf:resource="http://sparql.cwrc.ca/ontologies/genre-ONTOLOGY_DATE"/>
    <rdfs:label xml:lang="en">adventure writing</rdfs:label>
    <rdfs:comment xml:lang="en">This term and its description were created from data gathered from the Oxford Dictionary of Literary Terms, 4th ed.</rdfs:comment>
  </genre:FictionalGenre>
  <genre:ThreeDimensionalMedium rdf:about="#threeDimensionalObject">
    <skos:definition xml:lang="en">"A three-dimensional object can be measured in three different directions, typically height, length, and width." <![CDATA[<a href="#cwrc:157432b9-b7a2-465a-b24a-863f2a441e94">(Collins, 2021)</a>]]></skos:definition>
    <rdfs:comment xml:lang="en">This term and its description were created from data gathered from the Collins Dictionary.</rdfs:comment>
    <dcterms:references rdf:resource="https://www.collinsdictionary.com/dictionary/english/three-dimensional"/>
    <rdfs:isDefinedBy rdf:resource="http://sparql.cwrc.ca/ontologies/genre-ONTOLOGY_DATE"/>
    <rdfs:label xml:lang="en">three dimensional object</rdfs:label>
  </genre:ThreeDimensionalMedium>
  <genre:DramaticGenre rdf:about="#moralityOrMysteryPlay">
    <dcterms:references rdf:resource="http://www.oxfordreference.com/view/10.1093/acref/9780199208272.001.0001/acref-9780199208272-e-753?rskey=XphoRT%26result=751"/>
    <rdfs:isDefinedBy rdf:resource="http://sparql.cwrc.ca/ontologies/genre-ONTOLOGY_DATE"/>
    <rdfs:label xml:lang="en">morality or mystery play</rdfs:label>
    <skos:hiddenLabel xml:lang="en">MORALITYMYSTERYPLAY</skos:hiddenLabel>
    <owl:sameAs rdf:resource="http://id.loc.gov/authorities/genreForms/gf2014026442"/>
    <skos:definition xml:lang="en">"Religious dramas or pageants, typically written anonymously, that were popular in medieval Europe. Mystery plays represent one or more scenes from the Bible, and were first performed in the 13th century, often using a wagon as a stage to allow a performance to take place in various locations, . Morality plays were first popularized in the 15th century, and are allegorical rather than directly representational works in which personified vices and virtues compete to win a human soul for eternity."  <![CDATA[<a href="#cwrc:4c227091-6bf0-4325-b846-9733fae19e61">(Oxford, 2015)</a>]]></skos:definition>
    <rdfs:comment xml:lang="en">This term and its description were created from data gathered from the Oxford Dictionary of Literary Terms, 4th ed.</rdfs:comment>
  </genre:DramaticGenre>
  <genre:PoliticalGenre rdf:about="#politicalStatement">
    <rdfs:isDefinedBy rdf:resource="http://sparql.cwrc.ca/ontologies/genre-ONTOLOGY_DATE"/>
    <rdfs:label xml:lang="en">political Statement</rdfs:label>
    <skos:definition xml:lang="en">"Written work or other form of media that is intended to influence or comment upon a political issue." <![CDATA[<a href="#cwrc:4b7ec4be-c188-463c-9159-6ead04cc02eb">(Wikipedia, 2021)</a>]]></skos:definition>
    <rdfs:comment xml:lang="en">This term and its description were created from data gathered from Wikipedia.</rdfs:comment>
  </genre:PoliticalGenre>
  <genre:StillImageMedium rdf:about="#drawing">
    <skos:definition xml:lang="en">"A drawing instrument releases small amount of material onto a surface, leaving a visible mark. The most common support for drawing is paper, although other materials, such as cardboard, plastic, leather, canvas, and board, may be used. Temporary drawings may be made on a blackboard or whiteboard or indeed almost anything. The medium has been a popular and fundamental means of public expression throughout human history. It is one of the simplest and most efficient means of communicating visual ideas. The wide availability of drawing instruments makes drawing one of the most common artistic activities. In addition to its more artistic forms, drawing is frequently used in commercial illustration, animation, architecture, engineering and technical drawing. A quick, freehand drawing, usually not intended as a finished work, is sometimes called a sketch. An artist who practices or works in technical drawing may be called a drafter, draftsman or a draughtsman." <![CDATA[<a href="#cwrc:727d97bc-af78-4122-94be-aa78b2e97d5a">(DBpedia, 2019)</a>]]></skos:definition>
    <skos:related rdf:resource="http://vocab.getty.edu/aat/300033973"/>
    <rdfs:isDefinedBy rdf:resource="http://sparql.cwrc.ca/ontologies/genre-ONTOLOGY_DATE"/>
    <rdfs:label xml:lang="en">drawing</rdfs:label>
    <rdf:type rdf:resource="#VisualArtMedium"/>
  </genre:StillImageMedium>
  <genre:ThematicGenre rdf:about="#travel">
    <rdfs:label xml:lang="fr">voyage</rdfs:label>
    <rdfs:comment xml:lang="en">This term and its description were created from data gathered from Wikipedia.</rdfs:comment>
    <skos:definition xml:lang="en">About experiences away from home, typically containing descriptions of the scenery and culture of places visited. Sometimes includes biographical content, such as travel literature written in the form of a personal journal or diary.</skos:definition>
    <rdfs:isDefinedBy rdf:resource="http://sparql.cwrc.ca/ontologies/genre-ONTOLOGY_DATE"/>
    <rdfs:label xml:lang="en">travel writing</rdfs:label>
    <skos:definition xml:lang="fr">Un récit de voyage ou relation de voyage est un genre littéraire dans lequel l'auteur rend compte d'un ou des voyages, des peuples rencontrés, des émotions ressenties, des choses vues et entendues. Contrairement au roman, le récit de voyage privilégie le réel à la fiction. Pour mériter le titre de « récit » et avoir rang de littérature, la narration doit être structurée et aller au-delà de la simple énumération des dates et des lieux (comme un journal intime ou un livre de bord d'un navire). Cette littérature doit rendre compte d'impressions, d'aventures, de l'exploration ou de la conquête de pays lointains.</skos:definition>
    <skos:closeMatch rdf:resource="https://fr.wikipedia.org/wiki/R%C3%A9cit_de_voyage"/>
    <rdf:type rdf:resource="#NarrativeGenre"/>
  </genre:ThematicGenre>
  <genre:DialogueOrDebateGenre rdf:about="#dialogueOfTheDead">
    <skos:definition xml:lang="en">"A popular style of fiction in the 17th and 18th centuries featuring conversations between the ghosts of well-known figures. Based on the satirical Dialogues of the Dead by Lucian (120-around 180 CE), but not necessarily satirical themselves."  <![CDATA[<a href="#cwrc:93fc3195-0bd5-4161-a123-0352d96c42ab">(Mazella, 2007)</a>]]></skos:definition>
    <skos:definition xml:lang="fr">Mise en scène littéraire de la parole de personnages illustres dans l'au-delà, pratiquée dans l'Antiquité grecque, et jusqu'à nos jours.</skos:definition>
    <rdfs:isDefinedBy rdf:resource="http://sparql.cwrc.ca/ontologies/genre-ONTOLOGY_DATE"/>
    <rdfs:label xml:lang="en">dialogue of the dead</rdfs:label>
    <rdfs:label xml:lang="fr">dialogue des morts</rdfs:label>
    <dcterms:references rdf:resource="https://books.google.ca/books?id=8zBk8k35SFEC&amp;printsec=frontcover#v=onepage&amp;q&amp;f=false"/>
    <rdfs:comment xml:lang="en">This term and its description were created from data gathered from data.bnf.fr.</rdfs:comment>
  </genre:DialogueOrDebateGenre>
  <genre:AlphabetForm rdf:about="#alphabet">
    <skos:definition xml:lang="en"> "Books designed to display the letters of the alphabet, often with accompanying illustrations; may be used to teach the alphabet or as vehicles for an illustrator's art."  <![CDATA[<a href="#cwrc:bd595bc4-5991-4c51-98d9-9ab52c416f4f">(Getty, 2021)</a>]]></skos:definition>
    <rdfs:comment xml:lang="en">The description for this term is indebted to the Getty Art &amp; Architecture Thesaurus.</rdfs:comment>
    <owl:sameAs rdf:resource="http://vocab.getty.edu/aat/300202510"/>
    <rdfs:isDefinedBy rdf:resource="http://sparql.cwrc.ca/ontologies/genre-ONTOLOGY_DATE"/>
    <rdfs:label xml:lang="en">alphabet</rdfs:label>
  </genre:AlphabetForm>
  <genre:VisualArtMedium rdf:about="#visualArt">
    <rdfs:isDefinedBy rdf:resource="http://sparql.cwrc.ca/ontologies/genre-ONTOLOGY_DATE"/>
    <rdfs:label xml:lang="en">visual art</rdfs:label>
    <skos:definition xml:lang="en">"The visual arts are art forms such as ceramics, drawing, painting, sculpture, printmaking, design, crafts, photography, video, filmmaking, literature, and architecture. Many artistic disciplines (performing arts, conceptual art, textile arts) involve aspects of the visual arts as well as arts of other types. Also included within the visual arts are the applied arts such as industrial design, graphic design, fashion design, interior design and decorative art. Current usage of the term "visual arts" includes fine art as well as the applied, decorative arts and crafts, but this was not always the case. Before the Arts and Crafts Movement in Britain and elsewhere at the turn of the 20th century, the term 'artist' was often restricted to a person working in the fine arts (such as painting, sculpture, or printmaking) and not the handicraft, craft, or applied art media. The distinction was emphasized by artists of the Arts and Crafts Movement, who valued vernacular art forms as much as high forms. Art schools made a distinction between the fine arts and the crafts, maintaining that a craftsperson could not be considered a practitioner of the arts. The increasing tendency to privilege painting, and to a lesser degree sculpture, above other arts has been a feature of Western art as well as East Asian art. In both regions painting has been seen as relying to the highest degree on the imagination of the artist, and the furthest removed from manual labour - in Chinese painting the most highly valued styles were those of "scholar-painting", at least in theory practiced by gentleman amateurs. The Western hierarchy of genres reflected similar attitudes." <![CDATA[<a href="#cwrc:727d97bc-af78-4122-94be-aa78b2e97d5a">(DBpedia, 2019)</a>]]></skos:definition>
  </genre:VisualArtMedium>
  <genre:ReferenceWorkGenre rdf:about="#dictionary">
    <rdfs:comment xml:lang="en">The description for this term is indebted to the Getty Art &amp; Architecture Thesaurus.</rdfs:comment>
    <owl:sameAs rdf:resource="http://vocab.getty.edu/aat/300026186"/>
    <skos:definition xml:lang="fr">"Sources de références, contenant des listes alphabétiques dans lesquelles chaque mot est associé à des informations données. Elles incluent généralement les différentes significations, la prononciation, l'étymologie et des conseils sur l'usage des mots. " </skos:definition>
    <owl:sameAs rdf:resource="http://id.loc.gov/authorities/genreForms/gf2014026086"/>
    <rdfs:label xml:lang="fr">dictionnaire</rdfs:label>
    <rdfs:isDefinedBy rdf:resource="http://sparql.cwrc.ca/ontologies/genre-ONTOLOGY_DATE"/>
    <rdfs:label xml:lang="en">dictionary</rdfs:label>
    <skos:definition xml:lang="en">"Reference sources containing alphabetical lists of words with information given for each word; generally including meanings, pronunciation, etymology, and often usage guidance."  <![CDATA[<a href="#cwrc:db2f8571-a773-4068-a35f-34262950bb8f">(Getty, 2017)</a>]]></skos:definition>
  </genre:ReferenceWorkGenre>
  <genre:InformationalGenre rdf:about="#interview">
    <skos:definition xml:lang="en">"An interview is a conversation where questions are asked and answers are given. In common parlance, the word "interview" refers to a one-on-one conversation with one person acting in the role of the interviewer and the other in the role of the interviewee. The interviewer asks questions, the interviewee responds, with participants taking turns talking. Interviews usually involve a transfer of information from interviewee to interviewer, which is usually the primary purpose of the interview, although information transfers can happen in both directions simultaneously. One can contrast an interview which involves bi-directional communication with a one-way flow of information, such as a speech or oration. Interviews usually take place face to face and in person, although modern communications technologies such as the Internet have enabled conversations to happen in which parties are separated geographically, such as with videoconferencing software, and of course telephone interviews can happen without visual contact. Interviews almost always involve spoken conversation between two or more parties, although in some instances a "conversation" can happen between two persons who type questions and answers back and forth. Interviews can range from unstructured or free-wheeling and open-ended conversations in which there is no predetermined plan with prearranged questions, to highly structured conversations in which specific questions occur in a specified order. They can follow diverse formats; for example, in a ladder interview, a respondent's answers typically guide subsequent interviews, with the object being to explore a respondent's subconscious motives. Typically the interviewer has some way of recording the information that is gleaned from the interviewee, often by writing with a pencil and paper, sometimes transcribing with a video or audio recorder, depending on the context and extent of information and the length of the interview. Interviews have a duration in time, in the sense that the interview has a beginning and an ending." <![CDATA[<a href="#cwrc:727d97bc-af78-4122-94be-aa78b2e97d5a">(DBpedia, 2019)</a>]]></skos:definition>
    <rdfs:isDefinedBy rdf:resource="http://sparql.cwrc.ca/ontologies/genre-ONTOLOGY_DATE"/>
    <rdfs:label xml:lang="en">interview</rdfs:label>
  </genre:InformationalGenre>
  <genre:AdvertisementForm rdf:about="#advertisement">
    <skos:definition xml:lang="en">"Public notices or paid announcements, often promoting something for commercial purposes."<![CDATA[<a href="#cwrc:bd595bc4-5991-4c51-98d9-9ab52c416f4f">(Getty, 2021)</a>]]></skos:definition>
    <rdfs:comment xml:lang="en">The description for this term is indebted to the Getty Art &amp; Architecture Thesaurus.</rdfs:comment>
    <rdfs:isDefinedBy rdf:resource="http://sparql.cwrc.ca/ontologies/genre-ONTOLOGY_DATE"/>
    <rdfs:label xml:lang="en">advertisement</rdfs:label>
    <owl:sameAs rdf:resource="http://vocab.getty.edu/aat/300193993"/>
  </genre:AdvertisementForm>
  <genre:ComedicGenre rdf:about="#comedyOfHumours">
    <skos:definition xml:lang="en">"The comedy of humours refers to a genre of dramatic comedy that focuses on a character or range of characters, each of whom exhibits two or more overriding traits or 'humours' that dominates their personality, desires and conduct. This comic technique may be found in Aristophanes, but the English playwrights Ben Jonson and George Chapman popularized the genre in the closing years of the sixteenth century. In the later half of the seventeenth century, it was combined with the comedy of manners in Restoration comedy. In Jonson’s Every Man in His Humour (acted 1598), which made this type of play popular, all the words and acts of Kitely are controlled by an overpowering suspicion that his wife is unfaithful; George Downright, a country squire, must be "frank" above all things; the country gull in town determines his every decision by his desire to "catch on" to the manners of the city gallant. In his Induction to Every Man out of His Humour (1599) Jonson explains his character-formula thus: Some one peculiar qualityDoth so possess a man, that it doth drawAll his affects, his spirits, and his powers,In their confluctions, all to run one way. The comedy of humours owes something to earlier vernacular comedy but more to a desire to imitate the classical comedy of Plautus and Terence and to combat the vogue of romantic comedy, as developed by William Shakespeare. The satiric purpose of the comedy of humours and its realistic method lead to more serious character studies with Jonson’s The Alchemist. The humours each had been associated with physical and mental characteristics; the result was a system that was quite subtle in its capacity for describing types of personality." <![CDATA[<a href="#cwrc:727d97bc-af78-4122-94be-aa78b2e97d5a">(DBpedia, 2019)</a>]]></skos:definition>
    <rdfs:isDefinedBy rdf:resource="http://sparql.cwrc.ca/ontologies/genre-ONTOLOGY_DATE"/>
    <rdfs:label xml:lang="en">comedy of humours</rdfs:label>
  </genre:ComedicGenre>
  <genre:PoeticGenre rdf:about="#apology">
    <rdfs:comment xml:lang="en">This term and its description were created from data gathered from the Oxford Dictionary of Literary Terms, 4th ed.</rdfs:comment>
    <owl:sameAs rdf:resource="http://dbpedia.org/resource/Apologia"/>
    <rdfs:isDefinedBy rdf:resource="http://sparql.cwrc.ca/ontologies/genre-ONTOLOGY_DATE"/>
    <rdfs:label xml:lang="en">apology</rdfs:label>
    <rdfs:label xml:lang="fr">apologie</rdfs:label>
    <skos:definition xml:lang="fr">«Dans son sens originel, l'apologie est un genre littéraire visant à argumenter en défense contre les attaques visant une personne ou une doctrine. L'Apologie de Socrate est un exemple du genre, où Platon met en scène Socrate se défendant lui-même lors du procès qui déboucha sur sa condamnation à mort. Utilisée dans l'Antiquité par des orateurs et des avocats, l'apologie est aussi un moyen de réagir à des attaques publiques.»  <![CDATA[<a href="#cwrc:727d97bc-af78-4122-94be-aa78b2e97d5a">(DBpedia, 2017)</a>]]></skos:definition>
    <skos:definition xml:lang="en">"A text in which a writer defends the possibly controversial opinions contained in his or her writing."  <![CDATA[<a href="#cwrc:4c227091-6bf0-4325-b846-9733fae19e61">(Oxford, 2015)</a>]]></skos:definition>
  </genre:PoeticGenre>
  <genre:ReligiousGenre rdf:about="#prophecy">
    <owl:sameAs rdf:resource="http://id.loc.gov/authorities/genreForms/gf2015026059"/>
    <owl:sameAs rdf:resource="http://dbpedia.org/resource/Prophecy"/>
    <skos:definition xml:lang="en">"Prophecy involves a process in which one or more messages allegedly communicated to a prophet are then communicated to other people. Such messages typically involve] inspiration, interpretation, or revelation of events to come (compare divine knowledge). Historically, clairvoyance has been used[by whom?] as an adjunct to prophecy."  <![CDATA[<a href="#cwrc:727d97bc-af78-4122-94be-aa78b2e97d5a">(DBpedia, 2017)</a>]]></skos:definition>
    <skos:definition xml:lang="fr">«Dans les religions abrahamiques, une prophétie consiste en des paroles ou des écrits divinement inspirés qu'une personne reçoit par révélation. Pour les chrétiens, le témoignage de Jésus est l'esprit de la prophétie (Apocalypse 19:10). Une prophétie peut avoir trait au passé, au présent ou à l'avenir. Quand une personne prophétise, elle dit ou écrit ce que Dieu veut qu'elle sache, pour son propre bien ou pour le bien des autres. La prophétie n'est pas l'apanage des prophètes. Une personne peut recevoir une prophétie ou une révélation pour sa vie personnelle.»  <![CDATA[<a href="#cwrc:727d97bc-af78-4122-94be-aa78b2e97d5a">(DBpedia, 2017)</a>]]></skos:definition>
    <rdfs:comment xml:lang="en">The description for this term is indebted to DBpedia. </rdfs:comment>
    <rdfs:isDefinedBy rdf:resource="http://sparql.cwrc.ca/ontologies/genre-ONTOLOGY_DATE"/>
    <rdfs:label xml:lang="en">prophecy</rdfs:label>
  </genre:ReligiousGenre>
  <genre:FictionalGenre rdf:about="#vignette">
    <rdfs:label xml:lang="fr">micronouvelle</rdfs:label>
    <skos:definition xml:lang="en">"In theatrical script writing, sketch stories, and poetry, a vignette is a short impressionistic scene that focuses on one moment or gives a trenchant impression about a character, idea, setting, or object.[citation needed] This type of scene is more common in recent postmodern theater, where less emphasis is placed on adhering to the conventions of theatrical structure and story development. Vignettes have been particularly influenced by contemporary notions of a scene as shown in film, video and television scripting. It is also a part of something bigger than itself: for example, a vignette about a house belonging to a collection of vignettes or a whole story, such as The House On Mango Street, by Sandra Cisneros. A blog can provide a form of vignette."  <![CDATA[<a href="#cwrc:727d97bc-af78-4122-94be-aa78b2e97d5a">(DBpedia, 2017)</a>]]></skos:definition>
    <skos:definition xml:lang="fr">«La micronouvelle (parfois aussi appelée microroman) est un récit imaginaire, suggestif, parfois caustique, rédigé en un nombre extrêmement restreint de mots. C'est la forme la plus concise de récit littéraire prosaïque, parfois proche du poème par le rythme qu'il imprime. L'ironie et l'interactivité qui la caractérisent la rattachent au postmodernisme en littérature. Elle est connue dans les littératures anglaise et hispanique sous les locutions micro-fiction, short-short story et microconte. La microfiction, aussi appelée nanofiction ou fiction éclair, est « l’ancêtre » de la micronouvelle. Adaptée à la littérature française, parfois sur Twitter (aussi dite « twittérature ») pour son fonctionnement aux nombres très limités de mots qui se prête parfaitement à la micronouvelle, par des auteurs comme Fuentealba, Berthiaume, Gechter, Bastin, Le Blanc et Fréchette, elle passe aujourd'hui sous la plume d'auteurs comme Thierry Crouzet, Bernard Pivot, Alexandre Jardin, et Michel Trembla»y <![CDATA[<a href="#cwrc:727d97bc-af78-4122-94be-aa78b2e97d5a">(DBpedia, 2017)</a>]]></skos:definition>
    <owl:sameAs rdf:resource="http://dbpedia.org/resource/Vignette_(literature)"/>
    <rdfs:comment xml:lang="en">The description for this term is indebted to DBpedia. </rdfs:comment>
    <rdfs:isDefinedBy rdf:resource="http://sparql.cwrc.ca/ontologies/genre-ONTOLOGY_DATE"/>
    <rdfs:label xml:lang="en">vignette</rdfs:label>
  </genre:FictionalGenre>
  <genre:IllustratedForm rdf:about="#photoEssay">
    <skos:definition xml:lang="en">"A photo-essay is a set or series of photographs that are made to create series of emotions in the viewer. A photo essay will often show pictures in deep emotional stages. Photo essays range from purely photographic works to photographs with captions or small comments to full text essays illustrated with photographs. Examples of photo essays include: 
*  An article in a publication, sometimes a full page or a two-page spread 
*  A book or other complete publication. 
*  A web page or portion of a web site. 
*  A single montage or collage of photographic images, with text or other additions, intended to be viewed both as a whole and as individual photographs. Such a work may also fall in the category of mixed media. 
*  An art show which is staged at a particular time and location. Some such shows also fall into other categories category. 
*  In fashion publishing especially, a photo-editorial – an editorial-style article dominated by or entirely consisting of a series of thematic photographs Photographers known for their photo-essays include: 
*  W. Eugene Smith 
*  Ansel Adams 
* Adams's Born Free and Equal (1944) documented Japanese Americans held at the Manzanar War Relocation Center during World War II. 
*  James Nachtwey Photo-essays moved from printed press to the net." <![CDATA[<a href="#cwrc:727d97bc-af78-4122-94be-aa78b2e97d5a">(DBpedia, 2019)</a>]]></skos:definition>
    <rdfs:isDefinedBy rdf:resource="http://sparql.cwrc.ca/ontologies/genre-ONTOLOGY_DATE"/>
    <rdfs:label xml:lang="en">photo essay</rdfs:label>
  </genre:IllustratedForm>
  <genre:IntertextualGenre rdf:about="#reflection">
    <rdfs:isDefinedBy rdf:resource="http://sparql.cwrc.ca/ontologies/genre-ONTOLOGY_DATE"/>
    <rdfs:label xml:lang="en">reflection</rdfs:label>
    <skos:definition xml:lang="en">"Writing that describes a real or imaginary scene, event, interaction, passing thought, or memory, to which it adds a personal or critical reflection on its meaning." <![CDATA[<a href="#cwrc:50024824-8252-4a95-b62e-797911907f20">(DBpedia, 2021)</a>]]></skos:definition>
    <rdfs:comment xml:lang="en">The description for this term is indebted to DBpedia.</rdfs:comment>
    <skos:closeMatch rdf:resource="https://dbpedia.org/page/Reflective_writing"/>  
  </genre:IntertextualGenre>
  <genre:CollectionForm rdf:about="#collection">
    <skos:definition xml:lang="en">"Physical or virtual repositories comprising accumulated groups of objects or materials having a focal characteristic and that have been brought together by an individual or organization." <![CDATA[<a href="#cwrc:bd595bc4-5991-4c51-98d9-9ab52c416f4f">(Getty, 2021)</a>]]></skos:definition>
    <rdfs:comment xml:lang="en">The description for this term is indebted to the Getty Art &amp; Architecture Thesaurus.</rdfs:comment>
    <owl:sameAs rdf:resource="http://vocab.getty.edu/aat/300443858"/>
    <rdfs:isDefinedBy rdf:resource="http://sparql.cwrc.ca/ontologies/genre-ONTOLOGY_DATE"/>
    <rdfs:label xml:lang="en">collection</rdfs:label>
  </genre:CollectionForm>
  <genre:FictionalGenre rdf:about="#novelOfSensibility">
    <skos:definition xml:lang="en">"Also known as a sentimental novel, a novel of sensibility is an emotionally extravagant novel of a kind that became popular in Europe in the late 18th century, which exhibits the close connections between virtue and sensibility." <![CDATA[<a href="#cwrc:ef6d40f5-0c3c-45e0-bb04-a4cf93665e35">(Oxford, 2021)</a>]]></skos:definition>
    <rdfs:comment xml:lang="en">The description for this term is indebted to Oxford University Press.</rdfs:comment>
    <rdfs:isDefinedBy rdf:resource="http://sparql.cwrc.ca/ontologies/genre-ONTOLOGY_DATE"/>
    <rdfs:label xml:lang="en">novel of sensibility</rdfs:label>
    <skos:hiddenLabel xml:lang="en">sensibility</skos:hiddenLabel>
  </genre:FictionalGenre>
  <genre:ReligiousGenre rdf:about="#devotional">
    <rdfs:label xml:lang="fr">littérature de dévotion</rdfs:label>
    <skos:definition xml:lang="fr">La littérature de dévotion chrétienne est une écriture religieuse qui n'est ni doctrinale ni théologique, mais conçue pour les individus à lire pour leur édification personnelle et leur formation spirituelle. Le théologien Karl Holl a suggéré que la littérature de dévotion s'est définitivement développée au moment du piétisme pendant la seconde moitié du 17ème siècle.</skos:definition>
    <rdfs:isDefinedBy rdf:resource="http://sparql.cwrc.ca/ontologies/genre-ONTOLOGY_DATE"/>
    <rdfs:label xml:lang="en">devotional</rdfs:label>
    <skos:definition xml:lang="en">"Christian devotional literature (also called devotionals or Christian living literature) is religious writing that is neither doctrinal nor theological, but designed for individuals to read for their personal edification and spiritual formation. Theologian Karl Holl has suggested that devotional literature came into full development at the time of Pietism during the second half of the 17th century."  <![CDATA[<a href="#cwrc:727d97bc-af78-4122-94be-aa78b2e97d5a">(DBpedia, 2017)</a>]]></skos:definition>
    <owl:sameAs rdf:resource="http://dbpedia.org/resource/Christian_devotional_literature"/>
    <rdfs:comment xml:lang="en">The description for this term is indebted to DBpedia. </rdfs:comment>
    <owl:sameAs rdf:resource="http://id.loc.gov/authorities/genreForms/gf2015026057"/>
    <rdf:type rdf:resource="#LiteraryGenre"/>
  </genre:ReligiousGenre>
  <genre:AutobiographicalGenre rdf:about="#sexualAwakeningFiction">
    <rdfs:label xml:lang="fr">éveil à la sexualité</rdfs:label>
    <skos:definition xml:lang="en">Fiction in which a character, typically an adolescent, experiences sexual desires for the first time or has a first sexual encounter.</skos:definition>
    <rdfs:isDefinedBy rdf:resource="http://sparql.cwrc.ca/ontologies/genre-ONTOLOGY_DATE"/>
    <rdfs:label xml:lang="en">sexual awakening fiction</rdfs:label>
    <skos:definition xml:lang="fr">Œuvres de fiction dans lesquelles un personnage, généralement un adolescent, éprouve des désirs sexuels pour la première fois ou connait sa première expérience sexuelle.</skos:definition>
  </genre:AutobiographicalGenre>
  <genre:PoliticalGenre rdf:about="#conditionOfEnglandNovel">
    <rdfs:label xml:lang="fr">condition of england novel</rdfs:label>
    <skos:definition xml:lang="fr">Forme de fiction narrative, nommée ainsi d'après une phrase du "Chartisme" de Thomas Carlyle (1839), qui traite des questions sociales et politiques victoriennes en mettant l'accent sur l'agitation politique et les conflits entre classes sociales, qui cherche généralement à provoquer l'empathie pour les pauvres et la compréhension des inégalités et des injustices sociales. Ce mouvement est très proche du roman industriel en raison de son intérêt pour les conséquences de la révolution industrielle.</skos:definition>
    <rdfs:isDefinedBy rdf:resource="http://sparql.cwrc.ca/ontologies/genre-ONTOLOGY_DATE"/>
    <rdfs:label xml:lang="en">condition of england novel</rdfs:label>
    <skos:definition xml:lang="en">A form of narrative fiction, named for a phrase from Thomas Carlyle's “Chartism” (1839), that addresses Victorian social and political issues with a focus on political unrest and class conflict, and typically seeks to instill empathy for the poor and understanding of social iniquities and injustices.
Closely related to the industrial novel because of its interest in the impact of the industrial revolution.</skos:definition>
    <rdf:type rdf:resource="#NovelisticGenre"/>
    <rdf:type rdf:resource="#FictionalGenre"/>
  </genre:PoliticalGenre>
  <genre:ComedicGenre rdf:about="#comedyOfMenace">
    <rdfs:label xml:lang="fr">comédie de menace</rdfs:label>
    <rdfs:comment xml:lang="en">This term and its description were created from data gathered from the Penguin Dictionary of Literary Terms &amp; Literary Theory, 4th ed.</rdfs:comment>
    <rdfs:isDefinedBy rdf:resource="http://sparql.cwrc.ca/ontologies/genre-ONTOLOGY_DATE"/>
    <rdfs:label xml:lang="en">comedy of menace</rdfs:label>
    <skos:definition xml:lang="fr">Type de drame comique dans lequel l'humour noir dérive de la peur, irrationnelle ou non, des personnages principaux en réponse à la menace de quelque force obscure.</skos:definition>
    <skos:definition xml:lang="en">"A type of comedic drama in which the dark humour stems from the main characters’ fear, irrational or not, that some dark force threatens them."  <![CDATA[<a href="#cwrc:2f09376c-f784-4a46-9f04-5a21aa311f27">(Penguin, 1999)</a>]]></skos:definition>
  </genre:ComedicGenre>
  <genre:DramaticGenre rdf:about="#collectiveCreation">
    <skos:definition xml:lang="en">"Devised theatre - frequently called collective creation - is a method of theatre-making in which the script or (if it is a predominantly physical work) performance score originates from collaborative, often improvisatory work by a performing ensemble." <![CDATA[<a href="#cwrc:50024824-8252-4a95-b62e-797911907f20">(DBpedia, 2021)</a>]]></skos:definition>
    <rdfs:comment xml:lang="en">This term and its description were created from data gathered from DBpedia.</rdfs:comment>
    <owl:sameAs rdf:resource="https://dbpedia.org/page/Devised_theatre"/>
    <rdfs:isDefinedBy rdf:resource="http://sparql.cwrc.ca/ontologies/genre-ONTOLOGY_DATE"/>
    <rdfs:label xml:lang="en">collective creation</rdfs:label>
  </genre:DramaticGenre>
  <genre:ScholarlyGenre rdf:about="#criticism">
    <rdfs:isDefinedBy rdf:resource="http://sparql.cwrc.ca/ontologies/genre-ONTOLOGY_DATE"/>
    <rdfs:label xml:lang="en">criticism</rdfs:label>
    <skos:definition xml:lang="en">"Analyzing and evaluating the characteristics of man-made objects, literary works and documents, actions or projects. For critical descriptions or analyses of relatively recent works or events," <![CDATA[<a href="#cwrc:db2f8571-a773-4068-a35f-34262950bb8f">(Getty, 2019)</a>]]></skos:definition>
    <rdfs:comment xml:lang="en">The description for this term is indebted to the Getty Art &amp; Architecture Thesaurus.</rdfs:comment>
    <owl:sameAs rdf:resource="http://vocab.getty.edu/aat/300055851"/>
  </genre:ScholarlyGenre>
  <genre:FictionalGenre rdf:about="#thriller">
    <rdfs:label xml:lang="fr">thriller</rdfs:label>
    <owl:sameAs rdf:resource="http://dbpedia.org/resource/Thriller_(genre)"/>
    <owl:sameAs rdf:resource="http://id.loc.gov/authorities/genreForms/gf2014026571"/>
    <skos:definition xml:lang="fr">«Le thriller (anglicisme, de l'anglais to thrill : « frémir ») est un genre artistique utilisant le suspense ou la tension narrative pour provoquer chez le lecteur ou le spectateur une excitation ou une appréhension et le tenir en haleine jusqu'au dénouement de l'intrigue. Ce genre est très utilisé dans la littérature, le cinéma ou la télévision et se subdivise en de nombreux , chacun possédant ses propres codes. Les procédés narratifs sont souvent les mêmes, qu'ils soient utilisés au cinéma ou dans la littérature, avec notamment les fausses-pistes et la rétention d'informations afin d'embrouiller le lecteur/spectateur, ou l'utilisation des cliffhangers entre les différents chapitres, scènes ou épisodes. Au cinéma, le genre est aussi caractérisé par des scènes de poursuite ou de combat, qui y sont parfois traitées différemment que dans les films d'action. Les thèmes sont nombreux. Au sein des thrillers policiers (crime thriller), on peut citer les demandes de rançons, les prises d'otages, les enlèvements, les casses et la vengeance, ainsi que les enquêtes policières qui en découlent et la technique du whodunit, quel que soit le point-de-vue de l’œuvre (celui du policier, de la victime ou du criminel). Les thrillers psychologiques (psychological thrillers) sont caractérisés par des manipulations psychologiques, des traques ou harcèlements liées à des obsessions, des emprisonnements ou confinements dans des endroits dangereux ou piégés, frisant parfois avec le genre de l'horreur. Dans les thrillers paranoïaques (paranoid thrillers), des éléments tels que les théories du complot, les fausses accusations et la paranoïa clinique sont récurrents. Contrairement aux récits d'aventures ou d'action, le thriller est principalement caractérisé par le méchant de l'histoire qui va mettre des obstacles sur la route du héros.»  <![CDATA[<a href="#cwrc:727d97bc-af78-4122-94be-aa78b2e97d5a">(DBpedia, 2017)</a>]]></skos:definition>
    <skos:definition xml:lang="en">"Fiction full of action and suspense in which the protagonist is threatened by some sort of danger, often through the actions of a villain or criminal. The protagonist must usually employ both physical skill and wit to escape danger and outsmart the villain."  <![CDATA[<a href="#cwrc:4c227091-6bf0-4325-b846-9733fae19e61">(Oxford, 2015)</a>]]></skos:definition>
    <rdfs:isDefinedBy rdf:resource="http://sparql.cwrc.ca/ontologies/genre-ONTOLOGY_DATE"/>
    <rdfs:label xml:lang="en">thriller</rdfs:label>
    <rdfs:comment xml:lang="en">This term and its description were created from data gathered from the Oxford Dictionary of Literary Terms, 4th ed.</rdfs:comment>
  </genre:FictionalGenre>
  <genre:SatiricalGenre rdf:about="#lampoon">
    <rdfs:comment xml:lang="en">The description for this term is indebted to Dr. L. Kip Wheeler of Carson-Newman University. </rdfs:comment>
    <skos:definition xml:lang="en">"A coarse or crude satire ridiculing the appearance or character of another person."  <![CDATA[<a href="cwrc:509015ff-7641-473e-94c5-688e06952bb7">(L. K Wheeler, 2017)</a>]]></skos:definition>
    <owl:sameAs rdf:resource="http://dbpedia.org/resource/Libelle_(literary_genre)"/>
    <rdfs:label xml:lang="fr">libelle</rdfs:label>
    <skos:definition xml:lang="fr">«Un libelle est un petit livre de caractère satirique, insultant ou diffamatoire.»  <![CDATA[<a href="#cwrc:727d97bc-af78-4122-94be-aa78b2e97d5a">(DBpedia, 2017)</a>]]></skos:definition>
    <rdfs:isDefinedBy rdf:resource="http://sparql.cwrc.ca/ontologies/genre-ONTOLOGY_DATE"/>
    <rdfs:label xml:lang="en">lampoon</rdfs:label>
  </genre:SatiricalGenre>
  <genre:SocialScienceGenre rdf:about="#criminology">
    <rdfs:isDefinedBy rdf:resource="http://sparql.cwrc.ca/ontologies/genre-ONTOLOGY_DATE"/>
    <rdfs:label xml:lang="en">criminology</rdfs:label>
    <skos:definition xml:lang="en">Scholarship, typically non-fiction, dealing with the study of crime, criminals, and criminal justice.</skos:definition>
    <skos:definition xml:lang="fr">Science de l'étude des crimes, des criminels et de la justice pénale, généralement non fictionnelle.</skos:definition>
    <rdfs:label xml:lang="fr">criminologie</rdfs:label>
  </genre:SocialScienceGenre>
  <genre:DigitalMedium rdf:about="#website">
    <rdfs:isDefinedBy rdf:resource="http://sparql.cwrc.ca/ontologies/genre-ONTOLOGY_DATE"/>
    <rdfs:label xml:lang="en">website</rdfs:label>
    <skos:related rdf:resource="http://vocab.getty.edu/aat/300265431"/>
    <skos:definition xml:lang="en">"A website, also written as web site, is a collection of related web pages, including multimedia content, typically identified with a common domain name, and published on at least one web server. A web site may be accessible via a public Internet Protocol (IP) network, such as the Internet, or a private local area network (LAN), by referencing a uniform resource locator (URL) that identifies the site. Websites have many functions and can be used in various fashions; a website can be a personal website, a commercial website for a company, a government website or a non-profit organization website. Websites can be the work of an individual, a business or other organization, and are typically dedicated to a particular topic or purpose, ranging from entertainment and social networking to providing news and education. All publicly accessible websites collectively constitute the World Wide Web, while private websites, such as a company's website for its employees, are typically a part of an intranet. Web pages, which are the building blocks of websites, are documents, typically composed in plain text interspersed with formatting instructions of Hypertext Markup Language (HTML, XHTML). They may incorporate elements from other websites with suitable markup anchors. Web pages are accessed and transported with the Hypertext Transfer Protocol (HTTP), which may optionally employ encryption (HTTP Secure, HTTPS) to provide security and privacy for the user. The user's application, often a web browser, renders the page content according to its HTML markup instructions onto a display terminal. Hyperlinking between web pages conveys to the reader the site structure and guides the navigation of the site, which often starts with a home page containing a directory of the site web content. Some websites require user registration or subscription to access content. Examples of subscription websites include many business sites, parts of news websites, academic journal websites, gaming websites, file-sharing websites, message boards, web-based email, social networking websites, websites providing real-time stock market data, as well as sites providing various other services. As of 2016, end users can access websites on a range of devices, including desktop and laptop computers, tablet computers, smartphones and smart TVs." <![CDATA[<a href="#cwrc:727d97bc-af78-4122-94be-aa78b2e97d5a">(DBpedia, 2019)</a>]]></skos:definition>
  </genre:DigitalMedium>
  <genre:MovingMedium rdf:about="#film">
    <skos:definition xml:lang="en">"("Movie" and "Moving picture" redirect here. For other uses, see Movie (disambiguation) and Moving picture (disambiguation).) A film, also called a movie, motion picture, theatrical film or photoplay, is a series of still images which, when shown on a screen, creates the illusion of moving images due to the phi phenomenon. This optical illusion causes the audience to perceive continuous motion between separate objects viewed rapidly in succession. The process of filmmaking is both an art and an industry. A film is created by photographing actual scenes with a motion picture camera; by photographing drawings or miniature models using traditional animation techniques; by means of CGI and computer animation; or by a combination of some or all of these techniques and other visual effects. The word "cinema", short for cinematography, is often used to refer to the industry of films and filmmaking or to the art of filmmaking itself. The contemporary definition of cinema is the art of simulating experiences to communicate ideas, stories, perceptions, feelings, beauty or atmosphere by the means of recorded or programmed moving images along with other sensory stimulations. Films were originally recorded onto plastic film through a photochemical process, and then shown through a movie projector onto a large screen. The adoption of CGI-based special effects led to the use of digital intermediates. Most contemporary films are now fully digital through the entire process of production, distribution, and exhibition from start to finish. Films recorded in a photochemical form traditionally included an analogous optical soundtrack, which is a graphic recording of the spoken words, music and other sounds that accompany the images. It runs along a portion of the film exclusively reserved for it and is not projected. Films are cultural artifacts created by specific cultures. They reflect those cultures, and, in turn, affect them. Film is considered to be an important art form, a source of popular entertainment, and a powerful medium for educating—or indoctrinating—citizens. The visual basis of film gives it a universal power of communication. Some films have become popular worldwide attractions by using dubbing or subtitles to translate the dialog into the language of the viewer. Some have criticized the film industry's glorification of violence and its potentially negative treatment of women. The individual images that make up a film are called frames. During projection of traditional films, a rotating shutter causes intervals of darkness as each frame in turn is moved into position to be projected, but the viewer does not notice the interruptions because of an effect known as persistence of vision, whereby the eye retains a visual image for a fraction of a second after the source has been removed. The perception of motion is due to a psychological effect called phi phenomenon. The name "film" originates from the fact that photographic film (also called film stock) has historically been the medium for recording and displaying motion pictures. Many other terms exist for an individual motion picture, including picture, picture show, moving picture, photoplay and flick. The most common term in the United States is movie, while in Europe film is preferred. Terms for the field in general include the big screen, the silver screen, the movies and cinema; the latter is commonly used in scholarly texts and critical essays, especially by European writers. In early years, the word sheet was sometimes used instead of screen." <![CDATA[<a href="#cwrc:727d97bc-af78-4122-94be-aa78b2e97d5a">(DBpedia, 2019)</a>]]></skos:definition>
    <rdfs:isDefinedBy rdf:resource="http://sparql.cwrc.ca/ontologies/genre-ONTOLOGY_DATE"/>
    <rdfs:label xml:lang="en">film</rdfs:label>
    <rdf:type rdf:resource="#VisualArtMedium"/>
  </genre:MovingMedium>
  <genre:InformationalGenre rdf:about="#cookbook">
    <owl:sameAs rdf:resource="http://id.loc.gov/authorities/genreForms/gf2011026169"/>
    <skos:definition xml:lang="fr">«Un livre de cuisine est un recueil de recettes ou de considérations gastronomiques.»  <![CDATA[<a href="#cwrc:727d97bc-af78-4122-94be-aa78b2e97d5a">(DBpedia, 2017)</a>]]></skos:definition>
    <rdfs:comment xml:lang="en">The description for this term is indebted to DBpedia. </rdfs:comment>
    <owl:sameAs rdf:resource="http://vocab.getty.edu/aat/300026109"/>
    <rdfs:isDefinedBy rdf:resource="http://sparql.cwrc.ca/ontologies/genre-ONTOLOGY_DATE"/>
    <rdfs:label xml:lang="en">cookbook</rdfs:label>
    <skos:definition xml:lang="en">"Reference publications containing collections of recipes with ancillary content on selection of ingredients or the broader context of the types of cooking presented. Contemporary cookbooks may  focus on cultural or regional themes."  <![CDATA[<a href="#cwrc:db2f8571-a773-4068-a35f-34262950bb8f">(Getty, 2017)</a>]]></skos:definition>
  </genre:InformationalGenre>
  <genre:ThreeDimensionalMedium rdf:about="#realia">
    <skos:definition xml:lang="en">"In library classification systems, the term realia refers to three-dimensional objects from real life such as coins, tools, and textiles, that do not easily fit into the orderly categories of printed material. They can be either man-made (artifacts, tools, utensils, etc.) or naturally occurring (specimens, samples, etc.), usually borrowed, purchased, or received as donation by a teacher, library, or museum for use in classroom instruction or in exhibits. Archival and manuscript collections often receive items of memorabilia such as badges, emblems, insignias, jewelry, leather goods, needlework, etc., in connection with gifts of personal papers. Most government or institutional archives reject gifts of non-documentary objects unless they have a documentary value. When accepting large bequests of mixed objects they normally have the donors sign legal documents giving permission to the archive to destroy, exchange, sell or dispose in any way those objects which, according to the best judgement of the archivist, are not manuscripts (which can include typescripts or printouts) or are not immediately useful for understanding the manuscripts." <![CDATA[<a href="#cwrc:727d97bc-af78-4122-94be-aa78b2e97d5a">(DBpedia, 2019)</a>]]></skos:definition>
    <rdfs:isDefinedBy rdf:resource="http://sparql.cwrc.ca/ontologies/genre-ONTOLOGY_DATE"/>
    <rdfs:label xml:lang="en">realia</rdfs:label>
  </genre:ThreeDimensionalMedium>
  <genre:ReferenceWorkGenre rdf:about="#directory">
    <skos:definition xml:lang="en">"Enumerations of names, addresses, and other data about specific groups of persons or organizations; may appear in alphabetic or graphic format."  <![CDATA[<a href="#cwrc:db2f8571-a773-4068-a35f-34262950bb8f">(Getty, 2017)</a>]]></skos:definition>
    <rdfs:isDefinedBy rdf:resource="http://sparql.cwrc.ca/ontologies/genre-ONTOLOGY_DATE"/>
    <rdfs:label xml:lang="en">directory</rdfs:label>
    <rdfs:label xml:lang="fr">répertoire</rdfs:label>
    <owl:sameAs rdf:resource="http://vocab.getty.edu/aat/300026234"/>
    <rdfs:comment xml:lang="en">The description for this term is indebted to the Getty Art &amp; Architecture Thesaurus.</rdfs:comment>
    <skos:definition xml:lang="fr">"Énumérations de noms, d'adresses et d'autres données concernant des groupes spécifiques de personnes ou des organisations; apparaît sous forme alphabétique ou graphique. " </skos:definition>
    <owl:sameAs rdf:resource="http://id.loc.gov/authorities/genreForms/gf2014026087"/>
  </genre:ReferenceWorkGenre>
  <genre:PrintMedium rdf:about="#broadside">
    <rdfs:isDefinedBy rdf:resource="http://sparql.cwrc.ca/ontologies/genre-ONTOLOGY_DATE"/>
    <rdfs:label xml:lang="en">broadside</rdfs:label>
    <dcterms:references rdf:resource="http://www.oxfordreference.com/view/10.1093/acref/9780199208272.001.0001/acref-9780199208272-e-149?rskey=LdAUjx%26result=141"/>
    <rdfs:label xml:lang="fr">broadside</rdfs:label>
    <skos:definition xml:lang="en">"Large sheets of paper with a poem or song, especially a ballad, printed on only one side."  <![CDATA[<a href="#cwrc:4c227091-6bf0-4325-b846-9733fae19e61">(Oxford, 2015)</a>]]></skos:definition>
    <owl:sameAs rdf:resource="http://id.loc.gov/authorities/genreForms/gf2014026152"/>
    <skos:definition xml:lang="fr">Grandes affiches contenant un poème ou une chanson, plus particulièrement une ballade, imprimée d'un seul côté.</skos:definition>
    <rdfs:comment xml:lang="en">This term and its description were created from data gathered from the Oxford Dictionary of Literary Terms, 4th ed.</rdfs:comment>
  </genre:PrintMedium>
  <genre:PedagogicalGenre rdf:about="#instructionalText">
    <skos:definition xml:lang="en">"Print materials used for the purpose of imparting knowledge, attitudes, or skills to others." <![CDATA[<a href="#cwrc:bd595bc4-5991-4c51-98d9-9ab52c416f4f">(Getty, 2021)</a>]]></skos:definition>
    <rdfs:comment xml:lang="en">The description for this term is indebted to the Getty Art &amp; Architecture Thesaurus.</rdfs:comment>
    <rdfs:isDefinedBy rdf:resource="http://sparql.cwrc.ca/ontologies/genre-ONTOLOGY_DATE"/>
    <rdfs:label xml:lang="en">instructional text</rdfs:label>
  </genre:PedagogicalGenre>
  <genre:ScriptForm rdf:about="#playScript">
    <rdfs:isDefinedBy rdf:resource="http://sparql.cwrc.ca/ontologies/genre-ONTOLOGY_DATE"/>
    <rdfs:label xml:lang="en">play script</rdfs:label>
    <skos:definition xml:lang="en">"Written forms of stories prepared for stage plays, including description of characters, details of scenes and settings, dialogue, and stage directions." <![CDATA[<a href="#cwrc:bd595bc4-5991-4c51-98d9-9ab52c416f4f">(Getty, 2021)</a>]]></skos:definition>
    <owl:sameAs rdf:resource="http://vocab.getty.edu/aat/300026491"/>
    <rdfs:comment xml:lang="en">The description for this term is indebted to the Getty Art &amp; Architecture Thesaurus.</rdfs:comment>
</genre:ScriptForm>
  <genre:ReligiousGenre rdf:about="#sundaySchoolStory">
    <skos:definition xml:lang="en">"Stories paraphrasing Biblical texts or closely based on Biblical events; used in educational institutions associated with Christian churches, to provide religious education to children on Sundays." <![CDATA[<a href="#cwrc:bd595bc4-5991-4c51-98d9-9ab52c416f4f">(Getty, 2021)</a>]]></skos:definition>
    <rdfs:comment xml:lang="en">The description for this term is indebted to the Getty Art &amp; Architecture Thesaurus.</rdfs:comment>
    <rdfs:isDefinedBy rdf:resource="http://sparql.cwrc.ca/ontologies/genre-ONTOLOGY_DATE"/>
    <rdfs:label xml:lang="en">sunday school story</rdfs:label>
    <rdf:type rdf:resource="#ChildrensLiteratureGenre"/>
  </genre:ReligiousGenre>
  <genre:ThreeDimensionalMedium rdf:about="#archivalMaterial">
    <skos:definition xml:lang="en">"The physical materials that make up the mass of an archive." <![CDATA[<a href="#cwrc:bd595bc4-5991-4c51-98d9-9ab52c416f4f">(Getty, 2021)</a>]]></skos:definition>
    <rdfs:comment xml:lang="en">The description for this term is indebted to the Getty Art &amp; Architecture Thesaurus.</rdfs:comment>
    <skos:closeMatch rdf:resource="http://vocab.getty.edu/aat/300379505"/>
    <skos:related rdf:resource="http://vocab.getty.edu/aat/300379505"/>
    <rdfs:isDefinedBy rdf:resource="http://sparql.cwrc.ca/ontologies/genre-ONTOLOGY_DATE"/>
    <rdfs:label xml:lang="en">archival material</rdfs:label>
  </genre:ThreeDimensionalMedium>
  <genre:JournalForm rdf:about="#periodicalFeature">
    <rdfs:isDefinedBy rdf:resource="http://sparql.cwrc.ca/ontologies/genre-ONTOLOGY_DATE"/>
    <rdfs:label xml:lang="en">periodical feature</rdfs:label>
    <skos:definition xml:lang="en">"The central article in an issue of a publication issued at regular intervals, but not daily, containing articles on various subjects by different authors." <![CDATA[<a href="#cwrc:bd595bc4-5991-4c51-98d9-9ab52c416f4f">(Getty, 2021)</a>]]></skos:definition>
    <rdfs:comment xml:lang="en">The description for this term is indebted to the Getty Art &amp; Architecture Thesaurus.</rdfs:comment>
  </genre:JournalForm>
  <genre:CollectionForm rdf:about="#commonplaceBook">
    <skos:definition xml:lang="en">"Commonplace books (or commonplaces) are a way to compile knowledge, usually by writing information into books. Such books are essentially scrapbooks filled with items of every kind: recipes, quotes, letters, poems, tables of weights and measures, proverbs, prayers, legal formulas. Commonplaces are used by readers, writers, students, and scholars as an aid for remembering useful concepts or facts they have learned. Each commonplace book is unique to its creator's particular interests. They became significant in Early Modern Europe. "Commonplace" is a translation of the Latin term locus communis (from Greek tópos koinós, see literary topos) which means "a theme or argument of general application", such as a statement of proverbial wisdom. In this original sense, commonplace books were collections of such sayings, such as John Milton's commonplace book. Scholars have expanded this usage to include any manuscript that collects material along a common theme by an individual. Commonplace books are not diaries nortravelogues, with which they can be contrasted:English Enlightenment philosopher John Locke wrote the 1706 book A New Method of Making Common-Place-Books, "in which techniques for entering proverbs, quotations, ideas, speeches were formulated. Locke gave specific advice on how to arrange material by subject and category, using such key topics as love, politics, or religion. Commonplace books, it must be stressed, are not journals, which are chronological and introspective." By the early eighteenth century they had become an information management device in which a note-taker stored quotations, observations and definitions. They were even used by influential scientists. Carl Linnaeus, for instance, used commonplacing techniques to invent and arrange the nomenclature of his Systema Naturae (which is the basis for the system used by scientists today)." <![CDATA[<a href="#cwrc:727d97bc-af78-4122-94be-aa78b2e97d5a">(DBpedia, 2019)</a>]]></skos:definition>
    <rdfs:isDefinedBy rdf:resource="http://sparql.cwrc.ca/ontologies/genre-ONTOLOGY_DATE"/>
    <rdfs:label xml:lang="en">commonplace book</rdfs:label>
  </genre:CollectionForm>
  <genre:InformationalGenre rdf:about="#summary">
    <skos:definition xml:lang="en">"Brief statements condensing substantive points in a longer document." <![CDATA[<a href="#cwrc:bd595bc4-5991-4c51-98d9-9ab52c416f4f">(Getty, 2021)</a>]]></skos:definition>
    <rdfs:comment xml:lang="en">The description for this term is indebted to the Getty Art &amp; Architecture Thesaurus.</rdfs:comment>
    <owl:sameAs rdf:resource="http://vocab.getty.edu/aat/300139067"/>
    <rdfs:isDefinedBy rdf:resource="http://sparql.cwrc.ca/ontologies/genre-ONTOLOGY_DATE"/>
    <rdfs:label xml:lang="en">summary</rdfs:label>
  </genre:InformationalGenre>
  <genre:PerformanceMedium rdf:about="#theatreForYoungAudiences">
    <skos:definition xml:lang="en">"Genre of performing arts concerning theatrical or dramatic entertainment, often intended for stage presentation, and specifically intended for an audience of children." <![CDATA[<a href="#cwrc:bd595bc4-5991-4c51-98d9-9ab52c416f4f">(Getty, 2021)</a>]]></skos:definition>
    <rdfs:comment xml:lang="en">The description for this term is indebted to the Getty Art &amp; Architecture Thesaurus.</rdfs:comment>
    <skos:narrower rdf:resource="https://sparql.cwrc.ca/ontologies/genre.html#drama"/>
    <skos:narrower rdf:resource="https://sparql.cwrc.ca/ontologies/genre.html#childrensLiterature"/>
    <rdfs:isDefinedBy rdf:resource="http://sparql.cwrc.ca/ontologies/genre-ONTOLOGY_DATE"/>
    <rdfs:label xml:lang="en">theatre for young audiences</rdfs:label>
  </genre:PerformanceMedium>
  <genre:CollectionForm rdf:about="#anthology">
    <skos:definition xml:lang="en">"Collections of choice extracts, from the writings of one author, or various authors, and usually having a common characteristic such as subject matter or literary form."  <![CDATA[<a href="#cwrc:db2f8571-a773-4068-a35f-34262950bb8f">(Getty, 2017)</a>]]></skos:definition>
    <rdfs:isDefinedBy rdf:resource="http://sparql.cwrc.ca/ontologies/genre-ONTOLOGY_DATE"/>
    <rdfs:label xml:lang="en">anthology</rdfs:label>
    <owl:sameAs rdf:resource="http://vocab.getty.edu/aat/300026037"/>
    <rdfs:comment xml:lang="en">The description for this term is indebted to the Getty Art &amp; Architecture Thesaurus.</rdfs:comment>
    <skos:related rdf:resource="http://id.loc.gov/authorities/genreForms/gf2011026051"/>
    <skos:related rdf:resource="http://id.loc.gov/authorities/genreForms/gf2011026487"/>
    <rdfs:label xml:lang="fr">anthologie</rdfs:label>
    <skos:definition xml:lang="fr">"Collections d'extraits choisis parmi les écrits d'un ou de plusieurs auteurs, ayant habituellement une caractéristique commune telle que le sujet abordé ou la forme littéraire. " </skos:definition>
    <skos:related rdf:resource="http://id.loc.gov/authorities/genreForms/gf2011026052"/>
  </genre:CollectionForm>
  <genre:ThematicGenre rdf:about="#paranormal">
    <rdfs:isDefinedBy rdf:resource="http://sparql.cwrc.ca/ontologies/genre-ONTOLOGY_DATE"/>
    <rdfs:label xml:lang="en">paranormal</rdfs:label>
    <skos:definition xml:lang="en">"Paranormal events are phenomena described in popular culture, folklore, and other non-scientific bodies of knowledge, whose existence within these contexts is described to lie beyond normal experience or scientific explanation. A paranormal phenomenon is different from hypothetical concepts such as dark matter and dark energy. Unlike paranormal phenomena, these hypothetical concepts are based on empirical observations and experimental data gained through the scientific method. The most notable paranormal beliefs include those that pertain to ghosts, extraterrestrial life, unidentified flying objects, psychic abilities or extrasensory perception, and cryptids." <![CDATA[<a href="#cwrc:727d97bc-af78-4122-94be-aa78b2e97d5a">(DBpedia, 2019)</a>]]></skos:definition>
  </genre:ThematicGenre>
  <genre:IllustratedForm rdf:about="#graphicNovel">
    <skos:definition xml:lang="en">A book made up of comics content, which generally consists of an extended story with sequential art. Although the word "novel" normally refers to long fictional works, the term "graphic novel" is applied broadly and includes fiction or non-fiction, <![CDATA[<a href="#cwrc:50024824-8252-4a95-b62e-797911907f20">(DBpedia, 2021)</a>]]> as well as comics previously published as serials, or works that were created specifically for book form. The term is also used more broadly to refer to collections or anthologies of comics published in book form. <![CDATA[<a href="#cwrc:bd595bc4-5991-4c51-98d9-9ab52c416f4f">(Getty, 2021)</a>]]> It is, at least in the United States, distinguished from the term "comic book", which is generally used for comics periodicals. <![CDATA[<a href="#cwrc:50024824-8252-4a95-b62e-797911907f20">(DBpedia, 2021)</a>]]></skos:definition>
    <rdfs:comment xml:lang="en">This term and its description were created from data gathered from DBpedia and the Getty Art &amp; Architecture Thesaurus.</rdfs:comment>
    <owl:sameAs rdf:resource="https://dbpedia.org/page/Graphic_novel"/>
    <owl:sameAs rdf:resource="http://vocab.getty.edu/aat/300265568"/>
    <owl:sameAs rdf:resource="http://id.loc.gov/authorities/genreForms/gf2014026362"/>
    <rdfs:isDefinedBy rdf:resource="http://sparql.cwrc.ca/ontologies/genre-ONTOLOGY_DATE"/>
    <rdfs:label xml:lang="en">graphic novel</rdfs:label>
  </genre:IllustratedForm>
  <genre:ThreeDimensionalMedium rdf:about="#mixedMaterials">
    <skos:definition xml:lang="en">"Indication of multiple materials being used for a group, set, or other configuration of multiple works, including visual works, audio works, written works, or other types of works. For the indication of multiple materials being used on one single work, use "mixed media."" <![CDATA[<a href="#cwrc:bd595bc4-5991-4c51-98d9-9ab52c416f4f">(Getty, 2021)</a>]]></skos:definition>
    <rdfs:comment xml:lang="en">This term and its description were created from data gathered from DBpedia and the Getty Art &amp; Architecture Thesaurus.</rdfs:comment>
    <owl:sameAs rdf:resource="http://vocab.getty.edu/aat/300404821"/>
    <skos:related rdf:resource="http://vocab.getty.edu/aat/300163347"/>
    <rdfs:isDefinedBy rdf:resource="http://sparql.cwrc.ca/ontologies/genre-ONTOLOGY_DATE"/>
    <rdfs:label xml:lang="en">mixed materials</rdfs:label>
  </genre:ThreeDimensionalMedium>
  <genre:InformationalGenre rdf:about="#programNotes">
    <skos:definition xml:lang="en">"A concert program or programme is a selection and ordering, or programming, of pieces to be performed at an occasion, or concert. Programs may be influenced by the available ensemble of instruments, by performer ability or skill, by theme (historical, programmatic, or technical), by musical concerns (such as form), or by allowable time. For example, a brass ensemble will perform an "all brass" program, the pieces of which may be chosen by a theme, such as "all Bach", and the chosen pieces may be ordered so that they build in intensity as the concert progresses. Concert programs may be put together by ensembles, conductors, or ensemble directors, and are often explained in program notes. The program note is a standard element of a concert where contemporary or classical music is being performed. Program notes serve two purposes: to provide historical and background information on the piece and, if necessary, the composer, and to give the audience some sense of what to expect, and what possibly what to listen for, when listening to the work. With the presentation of contemporary pieces, it is common to include notes provided by the composer. Programs may include information about, and quotes or commentary from, the composer, conductor, or performers, as well as provide context regarding the musical era. Programs may also include information about the programmatic or absolute content of the music, including analysis, and may point out details such as themes, musical motifs, and sections or movements." <![CDATA[<a href="#cwrc:727d97bc-af78-4122-94be-aa78b2e97d5a">(DBpedia, 2019)</a>]]></skos:definition>
    <rdfs:isDefinedBy rdf:resource="http://sparql.cwrc.ca/ontologies/genre-ONTOLOGY_DATE"/>
    <rdfs:label xml:lang="en">program notes</rdfs:label>
  </genre:InformationalGenre>
  <genre:ThematicGenre rdf:about="#thematicWriting">
    <rdfs:isDefinedBy rdf:resource="http://sparql.cwrc.ca/ontologies/genre-ONTOLOGY_DATE"/>
    <rdfs:label xml:lang="en">thematic writing</rdfs:label>
    <rdfs:label xml:lang="fr">écriture thématique</rdfs:label>
    <skos:definition xml:lang="en">"Indicates a type of writing associated with some aspect of the text’s content or purpose, broadly conceived."  <![CDATA[<a href="#cwrc:727d97bc-af78-4122-94be-aa78b2e97d5a">(DBpedia, 2017)</a>]]></skos:definition>
    <rdfs:comment xml:lang="en">This term and its description were created from data gathered from DBpedia.</rdfs:comment>
  </genre:ThematicGenre>
  <genre:PoeticGenre rdf:about="#freeVerse">
    <skos:definition xml:lang="en">"An open form of poetry, which does not use consistent meter patterns, rhyme, or any musical pattern." <![CDATA[<a href="#cwrc:50024824-8252-4a95-b62e-797911907f20">(DBpedia, 2021)</a>]]></skos:definition>
    <rdfs:comment xml:lang="en">This term and its description were created from data gathered from DBpedia.</rdfs:comment>
    <owl:sameAs rdf:resource="https://dbpedia.org/page/Free_verse"/>
    <owl:sameAs rdf:resource="http://id.loc.gov/authorities/genreForms/gf2014026348"/>
    <rdfs:isDefinedBy rdf:resource="http://sparql.cwrc.ca/ontologies/genre-ONTOLOGY_DATE"/>
    <rdfs:label xml:lang="en">free verse</rdfs:label>
  </genre:PoeticGenre>
  <genre:InformationalGenre rdf:about="#chronology">
    <skos:definition xml:lang="en">"Tables, lists, or treatises listing events, biographies, milestones, or other items in serial temporal order relative to given dates or time periods."  <![CDATA[<a href="#cwrc:db2f8571-a773-4068-a35f-34262950bb8f">(Getty, 2017)</a>]]></skos:definition>
    <rdfs:comment xml:lang="en">The description for this term is indebted to the Getty Art &amp; Architecture Thesaurus.</rdfs:comment>
    <owl:sameAs rdf:resource="http://vocab.getty.edu/page/aat/300252008"/>
    <rdfs:isDefinedBy rdf:resource="http://sparql.cwrc.ca/ontologies/genre-ONTOLOGY_DATE"/>
    <rdfs:label xml:lang="en">chronology</rdfs:label>
    <owl:sameAs rdf:resource="http://id.loc.gov/authorities/genreForms/gf2014026062"/>
  </genre:InformationalGenre>
  <genre:ThematicGenre rdf:about="#war">
    <skos:definition xml:lang="en">A themtic genre concerning engagement with war in a range of forms and media and from a range of perspectives, including both front-line experiences, the lives of those imprisoned by war, experiences of living and working at a remove from battle. Includes historical and documentary approaches.</skos:definition>
    <rdfs:isDefinedBy rdf:resource="http://sparql.cwrc.ca/ontologies/genre-ONTOLOGY_DATE"/>
    <rdfs:label xml:lang="en">war</rdfs:label>
    <skos:related rdf:resource="#military"/>
    <rdf:type rdf:resource="#PoliticalGenre"/>
  </genre:ThematicGenre>
  <genre:SatiricalGenre rdf:about="#mockForms">
    <skos:definition xml:lang="en">Writing that uses the conventions of a specific genre satirically in order to mock or parody that genre.</skos:definition>
    <skos:definition xml:lang="fr">Œuvres qui reprennent les conventions d'un genre spécifique dans une perspective satirique, dans le but de le parodier ou de le tourner en ridicule.</skos:definition>
    <rdfs:isDefinedBy rdf:resource="http://sparql.cwrc.ca/ontologies/genre-ONTOLOGY_DATE"/>
    <rdfs:label xml:lang="en">mock forms</rdfs:label>
    <rdfs:label xml:lang="fr">imitations parodiques</rdfs:label>
  </genre:SatiricalGenre>
  <genre:InformationalGenre rdf:about="#nonFiction">
    <skos:definition xml:lang="en">"Nonfiction or non-fiction is content (often, in the form of a story) whose creator, in good faith, assumes responsibility for the truth or accuracy of the events, people, and/or information presented. In contrast, a story whose creator explicitly leaves open if and how the work refers to reality is usually classified as fiction. Nonfiction, which may be presented either objectively or subjectively, is traditionally one of the two main divisions of narratives (and, specifically, prose writing), the other traditional division being fiction, which contrasts with nonfiction by dealing in information, events, and characters expected to be partly or largely imaginary. Nonfiction's specific factual assertions and descriptions may or may not be accurate, and can give either a true or a false account of the subject in question. However, authors of such accounts genuinely believe or claim them to be truthful at the time of their composition or, at least, pose them to a convinced audience as historically or empirically factual. Reporting the beliefs of others in a nonfiction format is not necessarily an endorsement of the ultimate veracity of those beliefs, it is simply saying it is true that people believe them (for such topics as mythology). Nonfiction can also be written about fiction, typically known as literary criticism, giving information and analysis on these other works. Nonfiction need not necessarily be written text, since pictures and film can also purport to present a factual account of a subject." <![CDATA[<a href="#cwrc:727d97bc-af78-4122-94be-aa78b2e97d5a">(DBpedia, 2019)</a>]]></skos:definition>
    <rdfs:isDefinedBy rdf:resource="http://sparql.cwrc.ca/ontologies/genre-ONTOLOGY_DATE"/>
    <rdfs:label xml:lang="en">non-fiction</rdfs:label>
  </genre:InformationalGenre>
  <genre:NarrativeGenre rdf:about="#questNarrative">
    <rdfs:isDefinedBy rdf:resource="http://sparql.cwrc.ca/ontologies/genre-ONTOLOGY_DATE"/>
    <rdfs:label xml:lang="en">quest narrative</rdfs:label>
    <skos:definition xml:lang="en">"A story that involves a journey toward a specific mission or a goal, often symbolic or allegorical." <![CDATA[<a href="#cwrc:4b7ec4be-c188-463c-9159-6ead04cc02eb">(Wikipedia, 2021)</a>]]></skos:definition>
    <rdfs:comment xml:lang="en">This term and its description were created from data gathered from Wikipedia.</rdfs:comment>
  </genre:NarrativeGenre>
  <genre:ThreeDimensionalMedium rdf:about="#ephemera">
    <rdfs:isDefinedBy rdf:resource="http://sparql.cwrc.ca/ontologies/genre-ONTOLOGY_DATE"/>
    <rdfs:label xml:lang="en">ephemera</rdfs:label>
    <skos:related rdf:resource="http://vocab.getty.edu/aat/300028881"/>
    <skos:definition xml:lang="en">"Ephemera (singular: ephemeron) are any transitory written or printed matter not meant to be retained or preserved. The word derives from the Greek ephemeros, meaning "lasting only one day, short-lived". Some collectible ephemera are advertising trade cards, airsickness bags, bookmarks, catalogues, greeting cards, letters, pamphlets, postcards, posters, prospectuses, defunct stock certificates or tickets, and zines." <![CDATA[<a href="#cwrc:727d97bc-af78-4122-94be-aa78b2e97d5a">(DBpedia, 2019)</a>]]></skos:definition>
  </genre:ThreeDimensionalMedium>
  <genre:ScholarlyGenre rdf:about="#M.A.ResearchPaper">
    <skos:definition xml:lang="en">"Papers presenting the author's research and submitted in support of candidature for a Master's Degree." <![CDATA[<a href="#cwrc:bd595bc4-5991-4c51-98d9-9ab52c416f4f">(Getty, 2021)</a>]]></skos:definition>
    <rdfs:comment xml:lang="en">The description for this term is indebted to the Getty Art &amp; Architecture Thesaurus.</rdfs:comment>
    <rdfs:isDefinedBy rdf:resource="http://sparql.cwrc.ca/ontologies/genre-ONTOLOGY_DATE"/>
    <rdfs:label xml:lang="en">M.A. research paper</rdfs:label>
  </genre:ScholarlyGenre>
  <genre:ReligiousGenre rdf:about="#theology">
    <skos:definition xml:lang="en">A branch of religious writing attempting to deal systematically with the study of a deity or deities or religious beliefs; the science of religion. <![CDATA[<a href="#cwrc:727d97bc-af78-4122-94be-aa78b2e97d5a">(DBpedia, 2019)</a>]]></skos:definition>
    <rdfs:comment xml:lang="en">This term and its description were created from data gathered from DBpedia.</rdfs:comment>
    <skos:definition xml:lang="fr">«La théologie (en grec ancien θεολογία, littéralement « discours rationnel sur la divinité ou le divin, le Θεός [Theos] ») est un ensemble de champs disciplinaires qui touchent d'une manière ou d'une autre à l'idée de Dieu ou de divin. Selon la tradition dont il est question, les définitions de la théologie peuvent varier grandement.»  <![CDATA[<a href="#cwrc:727d97bc-af78-4122-94be-aa78b2e97d5a">(DBpedia, 2017)</a>]]></skos:definition>
    <skos:closeMatch rdf:resource="http://dbpedia.org/resource/Theology"/>
    <rdfs:label xml:lang="fr">théologie</rdfs:label>
    <rdfs:isDefinedBy rdf:resource="http://sparql.cwrc.ca/ontologies/genre-ONTOLOGY_DATE"/>
    <rdfs:label xml:lang="en">theology</rdfs:label>
  </genre:ReligiousGenre>
  <genre:CatalogueForm rdf:about="#exhibitionCatalogue">
    <skos:definition xml:lang="fr">Publications qui fournissent des informations sur les oeuvres présentées lors d'une exposition.</skos:definition>
    <owl:sameAs rdf:resource="http://id.loc.gov/authorities/genreForms/gf2014026098"/>
    <owl:sameAs rdf:resource="http://vocab.getty.edu/aat/300026096"/>
    <rdfs:comment xml:lang="en">The description for this term is indebted to the Getty Art &amp; Architecture Thesaurus.</rdfs:comment>
    <skos:definition xml:lang="en">"Publications that document the works displayed in an exhibition."  <![CDATA[<a href="#cwrc:db2f8571-a773-4068-a35f-34262950bb8f">(Getty, 2017)</a>]]></skos:definition>
    <rdfs:isDefinedBy rdf:resource="http://sparql.cwrc.ca/ontologies/genre-ONTOLOGY_DATE"/>
    <rdfs:label xml:lang="en">exhibition catalogue</rdfs:label>
    <rdfs:label xml:lang="fr">catalogue d'exposition</rdfs:label>
  </genre:CatalogueForm>
  <genre:RecordForm rdf:about="#index">
    <rdfs:isDefinedBy rdf:resource="http://sparql.cwrc.ca/ontologies/genre-ONTOLOGY_DATE"/>
    <rdfs:label xml:lang="en">index</rdfs:label>
    <skos:definition xml:lang="en">"An index (plural: usually indexes, more rarely indices; see below) is a list of words or phrases ('headings') and associated pointers ('locators') to where useful material relating to that heading can be found in a document or on a page. In a traditional back-of-the-book index the headings will include names of people, places and events, and concepts selected by a person as being relevant and of interest to a possible reader of the book. The pointers are typically page numbers, paragraph numbers or section numbers. In a library catalog the words are authors, titles, subject headings, etc., and the pointers are call numbers. Internet search engines, such as Google, and full text searching help provide access to information but are not as selective as an index, as they provide non-relevant links, and may miss relevant information if it is not phrased in exactly the way they expect. Perhaps the most advanced investigation of problems related to book indexes is made in the development of topic maps, which started as a way of representing the knowledge structures inherent in traditional back-of-the-book indexes." <![CDATA[<a href="#cwrc:727d97bc-af78-4122-94be-aa78b2e97d5a">(DBpedia, 2019)</a>]]></skos:definition>
  </genre:RecordForm>
  <genre:DramaticGenre rdf:about="#costumeDrama">
    <rdfs:isDefinedBy rdf:resource="http://sparql.cwrc.ca/ontologies/genre-ONTOLOGY_DATE"/>
    <rdfs:label xml:lang="en">costume drama</rdfs:label>
    <skos:definition xml:lang="en">"A historical period drama (also known as a historical drama, period drama or period piece) is a work of art set in, or reminiscent of, an earlier time period. The term is usually used in the context of film and television. It is an informal crossover term that can apply to several genres but is most often heard in the context of historical fiction and romances, adventure films, and swashbucklers. The implication is that the audience is attracted as much by the lavish costumes as by the content. In the performing arts, a period piece is a work set in a particular era. This informal term covers all countries, all periods and all genres. It may be as long and general as the medieval era or as limited as one decade—the Roaring Twenties, for example." <![CDATA[<a href="#cwrc:727d97bc-af78-4122-94be-aa78b2e97d5a">(DBpedia, 2019)</a>]]></skos:definition>
  </genre:DramaticGenre>
  <genre:StandaloneWork rdf:about="#artistsBook">
    <skos:related rdf:resource="http://vocab.getty.edu/aat/300123016"/>
    <rdfs:isDefinedBy rdf:resource="http://sparql.cwrc.ca/ontologies/genre-ONTOLOGY_DATE"/>
    <rdfs:label xml:lang="en">artist's book</rdfs:label>
    <skos:definition xml:lang="en">"Artists' books (or art books) are works of art that utilize the form of the book. They are often published in small editions, though they are sometimes produced as one-of-a-kind objects." <![CDATA[<a href="#cwrc:727d97bc-af78-4122-94be-aa78b2e97d5a">(DBpedia, 2019)</a>]]></skos:definition>
  </genre:StandaloneWork>
  <genre:SoundRecordingMedium rdf:about="#soundRecordingNonmusical">
    <skos:definition xml:lang="en">"Discs, tapes, filaments, or other media on which sound, excluding musical sound, has been recorded."<![CDATA[<a href="#cwrc:bd595bc4-5991-4c51-98d9-9ab52c416f4f">(Getty, 2021)</a>]]></skos:definition>
    <rdfs:comment xml:lang="en">The description for this term is indebted to the Getty Art &amp; Architecture Thesaurus.</rdfs:comment>
    <skos:related rdf:resource="http://sparql.cwrc.ca/ontologies/genre.html#SoundRecordingMedium"/>
    <rdfs:isDefinedBy rdf:resource="http://sparql.cwrc.ca/ontologies/genre-ONTOLOGY_DATE"/>
    <rdfs:label xml:lang="en">sound recording – nonmusical</rdfs:label>
  </genre:SoundRecordingMedium>
  <genre:ThematicGenre rdf:about="#nationalist">
    <skos:definition xml:lang="en">"A text that deals with a sense of national consciousness exalting one nation, typically above others, and placing primary emphasis on promotion of its culture and interests as opposed to those of other nations or supranational groups." <![CDATA[<a href="#cwrc:bd595bc4-5991-4c51-98d9-9ab52c416f4f">(Getty, 2021)</a>]]></skos:definition>
    <rdfs:comment xml:lang="en">The description for this term is indebted to the Getty Art &amp; Architecture Thesaurus.</rdfs:comment>
    <rdfs:isDefinedBy rdf:resource="http://sparql.cwrc.ca/ontologies/genre-ONTOLOGY_DATE"/>
    <rdfs:label xml:lang="en">nationalist</rdfs:label>
    <skos:related rdf:resource="http://dbpedia.org/resource/Nationalism"/>
    <rdf:type rdf:resource="#PoliticalGenre"/>
    <skos:hiddenLabel xml:lang="en">NATIONALISTFICTION</skos:hiddenLabel>
  </genre:ThematicGenre>
  <genre:DigitalMedium rdf:about="#webpage">
    <skos:definition xml:lang="en">"Hypertext documents of text, images, and other embedded media or scripts that are accessible via the World Wide Web, hosted on a web site." <![CDATA[<a href="#cwrc:bd595bc4-5991-4c51-98d9-9ab52c416f4f">(Getty, 2021)</a>]]></skos:definition>
    <rdfs:comment xml:lang="en">The description for this term is indebted to the Getty Art &amp; Architecture Thesaurus.</rdfs:comment>
    <owl:sameAs rdf:resource="http://vocab.getty.edu/aat/300264578"/>
    <skos:narrower rdf:resource="https://sparql.cwrc.ca/ontologies/genre.html#digital"/>
    <rdfs:isDefinedBy rdf:resource="http://sparql.cwrc.ca/ontologies/genre-ONTOLOGY_DATE"/>
    <rdfs:label xml:lang="en">webpage</rdfs:label>
  </genre:DigitalMedium>
  <genre:HistoricalGenre rdf:about="#historicalOverview">
    <skos:definition xml:lang="en">"Written works or other forms of media that describe or summarize a specific historical period or set of events, and their significance."</skos:definition>
    <rdfs:isDefinedBy rdf:resource="http://sparql.cwrc.ca/ontologies/genre-ONTOLOGY_DATE"/>
    <rdfs:label xml:lang="en">historical overview</rdfs:label>
  </genre:HistoricalGenre>
  <genre:PedagogicalGenre rdf:about="#grammar">
    <skos:definition xml:lang="en">"GRAMMAR: Another term for transformational grammar."  <![CDATA[<a href="cwrc:509015ff-7641-473e-94c5-688e06952bb7">(L. K Wheeler, 2017)</a>]]></skos:definition>
    <skos:definition xml:lang="fr">«La grammaire est l'étude systématique des éléments constitutifs d'une langue. Par extension, on nomme aussi grammaire un manuel ou un ensemble de documents décrivant des règles grammaticales.»  <![CDATA[<a href="#cwrc:727d97bc-af78-4122-94be-aa78b2e97d5a">(DBpedia, 2017)</a>]]></skos:definition>
    <rdfs:isDefinedBy rdf:resource="http://sparql.cwrc.ca/ontologies/genre-ONTOLOGY_DATE"/>
    <rdfs:label xml:lang="en">grammar</rdfs:label>
    <rdfs:label xml:lang="fr">grammaire</rdfs:label>
    <dcterms:references rdf:resource="http://web.cn.edu/kwheeler/lit_terms_g.html"/>
    <rdfs:comment xml:lang="en">The description for this term is indebted to Dr. L. Kip Wheeler of Carson-Newman University. </rdfs:comment>
  </genre:PedagogicalGenre>
  <genre:ThematicGenre rdf:about="#business">
    <skos:definition xml:lang="en">"Written works or other forms of media concerning the broad area of commercial or mercantile activity involving the exchange of commodities, services, or financial resources." <![CDATA[<a href="#cwrc:bd595bc4-5991-4c51-98d9-9ab52c416f4f">(Getty, 2021)</a>]]></skos:definition>
    <rdfs:comment xml:lang="en">The description for this term is indebted to the Getty Art &amp; Architecture Thesaurus.</rdfs:comment>
    <owl:sameAs rdf:resource="http://vocab.getty.edu/aat/300054343"/>
    <rdfs:isDefinedBy rdf:resource="http://sparql.cwrc.ca/ontologies/genre-ONTOLOGY_DATE"/>
    <rdfs:label xml:lang="en">business</rdfs:label>
  </genre:ThematicGenre>
  <genre:CatalogueForm rdf:about="#catalogue">
    <skos:definition xml:lang="en">"Enumeration of items, such as a file of bibliographic records or a list of art objects, usually arranged systematically and with descriptive details; may be in book or pamphlet form, on cards, or online. Catalogs are created according to specific and uniform principles of construction and usually under the control of an authority file."<![CDATA[<a href="#cwrc:bd595bc4-5991-4c51-98d9-9ab52c416f4f">(Getty, 2021)</a>]]></skos:definition>
    <rdfs:comment xml:lang="en">The description for this term is indebted to the Getty Art &amp; Architecture Thesaurus.</rdfs:comment>
    <owl:sameAs rdf:resource="http://vocab.getty.edu/aat/300026059"/>
    <rdfs:isDefinedBy rdf:resource="http://sparql.cwrc.ca/ontologies/genre-ONTOLOGY_DATE"/>
    <rdfs:label xml:lang="en">catalogue</rdfs:label>
  </genre:CatalogueForm>
  <genre:ThematicGenre rdf:about="#architecturalWriting">
    <skos:altLabel xml:lang="en">architecture</skos:altLabel>
    <skos:definition xml:lang="en">Written works concerning the art or science of designing and building structures, especially habitable structures, in accordance with principles determined by aesthetic and practical or material considerations. <![CDATA[<a href="#cwrc:bd595bc4-5991-4c51-98d9-9ab52c416f4f">(Getty, 2021)</a>]]></skos:definition>
    <rdfs:comment xml:lang="en">The description for this term is indebted to the Getty Art &amp; Architecture Thesaurus.</rdfs:comment>
    <rdfs:isDefinedBy rdf:resource="http://sparql.cwrc.ca/ontologies/genre-ONTOLOGY_DATE"/>
    <rdfs:label xml:lang="en">architectural writing</rdfs:label>
    <rdf:type rdf:resource="#InformationalGenre"/>
    <rdf:type rdf:resource="#ScholarlyGenre"/>
  </genre:ThematicGenre>
  <genre:PoeticGenre rdf:about="#anacreontic">
    <skos:definition xml:lang="en">"Anacreontics are verses in a meter used by the Greek poet Anacreon in his poems dealing with love and wine. His later Greek imitators (whose surviving poems are known as the Anacreontea) took up the same themes and used the Anacreontic meter. In modern poetry, Anacreontics are short lyrical pieces that keep the Anacreontic subject matter but not the meter." <![CDATA[<a href="#cwrc:727d97bc-af78-4122-94be-aa78b2e97d5a">(DBpedia, 2019)</a>]]></skos:definition>
    <rdfs:isDefinedBy rdf:resource="http://sparql.cwrc.ca/ontologies/genre-ONTOLOGY_DATE"/>
    <rdfs:label xml:lang="en">anacreontic</rdfs:label>
  </genre:PoeticGenre>
  <genre:ScholarlyGenre rdf:about="#maThesis">
    <rdfs:isDefinedBy rdf:resource="http://sparql.cwrc.ca/ontologies/genre-ONTOLOGY_DATE"/>
    <rdfs:label xml:lang="en">M.A. thesis</rdfs:label>
  </genre:ScholarlyGenre>
  <genre:PoeticGenre rdf:about="#prosePoem">
    <skos:definition xml:lang="en">"Prose poetry is poetry written in prose instead of using verse but preserving poetic qualities such as heightened imagery, parataxis and emotional effects." <![CDATA[<a href="#cwrc:727d97bc-af78-4122-94be-aa78b2e97d5a">(DBpedia, 2019)</a>]]></skos:definition>
    <owl:sameAs rdf:resource="http://id.loc.gov/authorities/genreForms/gf2014026488"/>
    <rdfs:isDefinedBy rdf:resource="http://sparql.cwrc.ca/ontologies/genre-ONTOLOGY_DATE"/>
    <rdfs:label xml:lang="en">prose poem</rdfs:label>
  </genre:PoeticGenre>
  <genre:CartographicForm rdf:about="#atlas">
    <skos:definition xml:lang="en">"Volumes of maps, with or without descriptive text, which may be issued to supplement or accompany texts or be published independently." <![CDATA[<a href="#cwrc:bd595bc4-5991-4c51-98d9-9ab52c416f4f">(Getty, 2021)</a>]]></skos:definition>
    <rdfs:comment xml:lang="en">The description for this term is indebted to the Getty Art &amp; Architecture Thesaurus.</rdfs:comment>
    <owl:sameAs rdf:resource="http://vocab.getty.edu/aat/300028053"/>
    <rdfs:isDefinedBy rdf:resource="http://sparql.cwrc.ca/ontologies/genre-ONTOLOGY_DATE"/>
    <rdfs:label xml:lang="en">atlas</rdfs:label>
    <owl:sameAs rdf:resource="http://id.loc.gov/authorities/genreForms/gf2011026058"/>
  </genre:CartographicForm>
  <genre:NarrativeGenre rdf:about="#eyeWitness">
    <skos:definition xml:lang="en">"An account of an incident or crime, given by a bystander or victim." <![CDATA[<a href="#cwrc:4b7ec4be-c188-463c-9159-6ead04cc02eb">(Wikipedia, 2021)</a>]]></skos:definition>
    <rdfs:comment xml:lang="en">This term and its description were created from data gathered from Wikipedia.</rdfs:comment>
    <rdfs:isDefinedBy rdf:resource="http://sparql.cwrc.ca/ontologies/genre-ONTOLOGY_DATE"/>
    <rdfs:label xml:lang="en">eye-witness</rdfs:label>
  </genre:NarrativeGenre>
  <genre:InformationalGenre rdf:about="#announcement">
    <skos:definition xml:lang="en">"Printed, spoken, or published statements or notices that inform the reader of an event or other news."  <![CDATA[<a href="#cwrc:bd595bc4-5991-4c51-98d9-9ab52c416f4f">(Getty, 2021)</a>]]></skos:definition>
    <rdfs:comment xml:lang="en">The description for this term is indebted to the Getty Art &amp; Architecture Thesaurus.</rdfs:comment>
    <owl:sameAs rdf:resource="http://vocab.getty.edu/aat/300026707"/>
    <rdfs:isDefinedBy rdf:resource="http://sparql.cwrc.ca/ontologies/genre-ONTOLOGY_DATE"/>
    <rdfs:label xml:lang="en">announcement</rdfs:label>
  </genre:InformationalGenre>
  <genre:PoliticalGenre rdf:about="#socialReform">
    <skos:definition xml:lang="en">"Written work or other form of media with a focus on a social problem that critiques the situation and aims to improve it or bring it closer to an ideal, whether held by the author individual, by a social movement or theory, or a particular community." <![CDATA[<a href="#cwrc:4b7ec4be-c188-463c-9159-6ead04cc02eb">(Wikipedia, 2021)</a>]]></skos:definition>
    <rdfs:comment xml:lang="en">This term and its description were created from data gathered from Wikipedia.</rdfs:comment>
    <rdfs:isDefinedBy rdf:resource="http://sparql.cwrc.ca/ontologies/genre-ONTOLOGY_DATE"/>
    <rdfs:label xml:lang="en">social reform</rdfs:label>
  </genre:PoliticalGenre>
  <genre:ThematicGenre rdf:about="#erotica">
    <rdfs:label xml:lang="en">erotica</rdfs:label>
    <rdfs:label xml:lang="fr"/>
    <skos:definition xml:lang="fr"/>
    <skos:definition xml:lang="en">Creative works involving content that is sexually oriented and often arousing to their audiences; often distinguished from pornography by being less sexually explicit, more egalitarian, and providing a greater sense of narrative or context. See @@#eroticaOrPornography@@ and @@https://en.wikipedia.org/wiki/Erotica@@</skos:definition>
    <skos:related rdf:resource="#pornography"/>
    <skos:narrower rdf:resource="#eroticaOrPornography"/>
    <rdfs:seeAlso rdf:resource="http://dbpedia.org/resource/Erotica"/>
    <skos:narrower rdf:resource="#eroticaOrPornography"/>
    <skos:related rdf:resource="#erotica"/>
    <rdfs:isDefinedBy rdf:resource="http://sparql.cwrc.ca/ontologies/genre-ONTOLOGY_DATE"/>
  </genre:ThematicGenre>
  <genre:ThematicGenre rdf:about="#environmental">
    <skos:definition xml:lang="en">"A text that focuses on the natural world or physical surroundings in general, either as a whole or within a particular geographical area, particularly as affected by human activity." <![CDATA[<a href="#cwrc:bd595bc4-5991-4c51-98d9-9ab52c416f4f">(Getty, 2021)</a>]]></skos:definition>
    <rdfs:comment xml:lang="en">The description for this term is indebted to the Getty Art &amp; Architecture Thesaurus.</rdfs:comment>
    <rdfs:isDefinedBy rdf:resource="http://sparql.cwrc.ca/ontologies/genre-ONTOLOGY_DATE"/>
    <rdfs:label xml:lang="en">environmental</rdfs:label>
  </genre:ThematicGenre>
  <genre:EmbeddedWork rdf:about="#partExcerpt">
    <rdfs:isDefinedBy rdf:resource="http://sparql.cwrc.ca/ontologies/genre-ONTOLOGY_DATE"/>
    <rdfs:label xml:lang="en">part/excerpt</rdfs:label>
    <skos:definition xml:lang="en">"Portions of a larger work, such as a literary work or motion picture, reproduced or excised without further change from their original context." <![CDATA[<a href="#cwrc:bd595bc4-5991-4c51-98d9-9ab52c416f4f">(Getty, 2021)</a>]]></skos:definition>
    <owl:sameAs rdf:resource="http://vocab.getty.edu/aat/300026939"/>
    <rdfs:comment xml:lang="en">The description for this term is indebted to the Getty Art &amp; Architecture Thesaurus.</rdfs:comment>
  </genre:EmbeddedWork>
  <genre:IntertextualGenre rdf:about="#commentary">
    <skos:definition xml:lang="en">"Treatises or series of comments that systematically explain or annotate another work." <![CDATA[<a href="#cwrc:bd595bc4-5991-4c51-98d9-9ab52c416f4f">(Getty, 2021)</a>]]></skos:definition>
    <rdfs:comment xml:lang="en">The description for this term is indebted to the Getty Art &amp; Architecture Thesaurus.</rdfs:comment>
    <owl:sameAs rdf:resource="http://vocab.getty.edu/aat/300026098"/>
    <rdfs:isDefinedBy rdf:resource="http://sparql.cwrc.ca/ontologies/genre-ONTOLOGY_DATE"/>
    <rdfs:label xml:lang="en">commentary</rdfs:label>
  </genre:IntertextualGenre>
  <genre:ThematicGenre rdf:about="#sensational">
    <rdfs:isDefinedBy rdf:resource="http://sparql.cwrc.ca/ontologies/genre-ONTOLOGY_DATE"/>
    <rdfs:label xml:lang="en">sensational</rdfs:label>
    <skos:definition xml:lang="en">"A kind of novel that flourished in Britain in the 1860s, exploiting the element of suspense in stories of crime and mystery. The sensation novel has been seen as an early kind of thriller in that it exposes dark secrets and conspiracies, but is distinguished from the classic detective story by its lack of a central detective figure." <![CDATA[<a href="#cwrc:ef6d40f5-0c3c-45e0-bb04-a4cf93665e35">(Oxford, 2021)</a>]]></skos:definition>
    <rdfs:comment xml:lang="en">The description for this term is indebted to Oxford Reference.</rdfs:comment>
    <dcterms:references rdf:resource="https://www.oxfordreference.com/view/10.1093/oi/authority.20110803100454745"/>
  </genre:ThematicGenre>
  <owl:Class rdf:about="#CatalogueForm">
    <rdfs:subClassOf rdf:resource="#Form"/>
    <skos:definition xml:lang="en">Indicates "enumerations of items, such as a file of bibliographic records or a list of art objects, usually arranged systematically and with descriptive details; may be in book or pamphlet form, on cards, or online." <![CDATA[<a href="#cwrc:db2f8571-a773-4068-a35f-34262950bb8f">(Getty, 2019)</a>]]></skos:definition>
    <skos:closeMatch rdf:resource="http://vocab.getty.edu/aat/300026059"/>
    <rdfs:isDefinedBy rdf:resource="http://sparql.cwrc.ca/ontologies/genre-ONTOLOGY_DATE"/>
    <rdfs:label xml:lang="en">Catalogue Form</rdfs:label>
    <owl:sameAs rdf:resource="http://id.loc.gov/authorities/genreForms/gf2014026057"/>
  </owl:Class>
  <owl:Class rdf:about="#JournalForm">
    <rdfs:subClassOf rdf:resource="#SerialForm"/>
    <skos:definition xml:lang="en">"Periodical literature (also called a periodical publication or simply a periodical) is a published work that appears in a new edition on a regular schedule. The most familiar counter-examples are the newspaper, often published daily, or weekly. The most familiar example is the magazine, typically published weekly, monthly, or as a quarterly. Other examples are newsletters, literary magazines (literary journals), academic journals (including scientific journals), science magazines, and yearbooks."<![CDATA[<a href="#cwrc:727d97bc-af78-4122-94be-aa78b2e97d5a">(DBpedia, 2019)</a>]]></skos:definition>
    <skos:closeMatch rdf:resource="http://dbpedia.org/resource/Periodical_literature"/>
    <rdfs:isDefinedBy rdf:resource="http://sparql.cwrc.ca/ontologies/genre-ONTOLOGY_DATE"/>
    <rdfs:label xml:lang="en">Journal Form</rdfs:label>
    <owl:sameAs rdf:resource="http://id.loc.gov/authorities/genreForms/gf2014026057"/>
  </owl:Class>
  <owl:Class rdf:about="#SeriesForm">
    <rdfs:subClassOf rdf:resource="#SerialForm"/>
    <skos:definition xml:lang="en">A publication that appears in a series, usually at regular intervals. It may be combined with other forms to indicate medium, as in a book series or television series. See @@https://en.wikipedia.org/wiki/Series@@ 
    Note: Used to class texts encoded using the “s” (series) value for the level attribute in the Text Encoding Initiative Schema. See @@https://tei-c.org/release/doc/tei-p5-doc/en/html/ref-title.html@@.
    </skos:definition>
    <rdfs:isDefinedBy rdf:resource="http://sparql.cwrc.ca/ontologies/genre-ONTOLOGY_DATE"/>
    <rdfs:label xml:lang="en">Series Form</rdfs:label>
    <owl:sameAs rdf:resource="http://id.loc.gov/authorities/genreForms/gf2014026057"/>
  </owl:Class>
  <owl:Class rdf:about="#PedagogicalGenre">
    <rdfs:isDefinedBy rdf:resource="http://sparql.cwrc.ca/ontologies/genre-ONTOLOGY_DATE"/>
    <rdfs:label xml:lang="en">Pedagogical Genre</rdfs:label>
    <rdfs:subClassOf rdf:resource="#ScholarlyGenre"/>
    <skos:definition xml:lang="en">Indicates works intended for educational purposes.</skos:definition>
  </owl:Class>
  <owl:Class rdf:about="#PoliticalGenre">
    <skos:definition xml:lang="en">Indicates works concerned with "the distribution of power and resources within a given community (a usually hierarchically organized population) as well as the interrelationship(s) between communities." <![CDATA[<a href="#cwrc:727d97bc-af78-4122-94be-aa78b2e97d5a">(DBpedia, 2019)</a>]]></skos:definition>
    <rdfs:subClassOf rdf:resource="#Genre"/>
    <skos:closeMatch rdf:resource="http://dbpedia.org/resource/Politics"/>
    <rdfs:isDefinedBy rdf:resource="http://sparql.cwrc.ca/ontologies/genre-ONTOLOGY_DATE"/>
    <rdfs:label xml:lang="en">Political Genre</rdfs:label>
  </owl:Class>
  <owl:Class rdf:about="#FeministGenre">
    <rdfs:isDefinedBy rdf:resource="http://sparql.cwrc.ca/ontologies/genre-ONTOLOGY_DATE"/>
    <rdfs:label xml:lang="en">Feminist Genre</rdfs:label>
    <skos:closeMatch rdf:resource="http://dbpedia.org/resource/Feminism"/>
    <rdfs:subClassOf rdf:resource="#PoliticalGenre"/>
    <skos:definition xml:lang="en">Indicates works engaging with "a range of political movements, ideologies, and social movements that share a common goal: to define, establish, and achieve political, economic, personal, and social rights" and equality for all genders. <![CDATA[<a href="#cwrc:727d97bc-af78-4122-94be-aa78b2e97d5a">(DBpedia, 2019)</a>]]></skos:definition>
  </owl:Class>
  <owl:Class rdf:about="#CalendarForm">
    <skos:definition xml:lang="en">Indicates "registers of days or other contrivances for reckoning days, months, years, etc., such as a table showing the division of a given year into its months, weeks, days, years, or other divisions of time." <![CDATA[<a href="#cwrc:db2f8571-a773-4068-a35f-34262950bb8f">(Getty, 2019)</a>]]></skos:definition>
    <rdfs:isDefinedBy rdf:resource="http://sparql.cwrc.ca/ontologies/genre-ONTOLOGY_DATE"/>
    <rdfs:label xml:lang="en">Calendar Form</rdfs:label>
    <owl:sameAs rdf:resource="http://vocab.getty.edu/aat/300026741"/>
    <rdfs:subClassOf rdf:resource="#Form"/>
  </owl:Class>
  <owl:Class rdf:about="#ScriptForm">
    <skos:closeMatch rdf:resource="http://vocab.getty.edu/aat/300026487"/>
    <rdfs:subClassOf rdf:resource="#Form"/>
    <skos:definition xml:lang="en">Indicates "written texts of stage plays, screenplays, and radio or television broadcasts." <![CDATA[<a href="#cwrc:db2f8571-a773-4068-a35f-34262950bb8f">(Getty, 2019)</a>]]></skos:definition>
    <rdfs:isDefinedBy rdf:resource="http://sparql.cwrc.ca/ontologies/genre-ONTOLOGY_DATE"/>
    <rdfs:label xml:lang="en">Script Form</rdfs:label>
  </owl:Class>
  <owl:Class rdf:about="#VisualArtMedium">
    <rdfs:isDefinedBy rdf:resource="http://sparql.cwrc.ca/ontologies/genre-ONTOLOGY_DATE"/>
    <rdfs:label xml:lang="en">Visual Art Medium</rdfs:label>
    <rdfs:subClassOf rdf:resource="#VisualMedium"/>
    <skos:definition xml:lang="en">Indicates media "that are meant to be perceived primarily through the sense of sight, were created by the use of skill and imagination, and possess an aesthetic that is valued and of a quality and type that would be collected by art museums or private collectors." <![CDATA[<a href="#cwrc:db2f8571-a773-4068-a35f-34262950bb8f">(Getty, 2019)</a>]]></skos:definition>
    <owl:sameAs rdf:resource="http://vocab.getty.edu/aat/300054154"/>
  </owl:Class>
  <owl:Class rdf:about="#IntertextualGenre">
    <rdfs:isDefinedBy rdf:resource="http://sparql.cwrc.ca/ontologies/genre-ONTOLOGY_DATE"/>
    <rdfs:label xml:lang="en">Intertextual Genre</rdfs:label>
    <skos:closeMatch rdf:resource="http://dbpedia.org/resource/Intertextuality"/>
    <rdfs:subClassOf rdf:resource="#Genre"/>
    <skos:definition xml:lang="en">Indicates works that shape "a text's meaning by another text." <![CDATA[<a href="#cwrc:727d97bc-af78-4122-94be-aa78b2e97d5a">(DBpedia, 2019)</a>]]></skos:definition>
  </owl:Class>
  <owl:Class rdf:about="#EpistolaryGenre">
    <skos:closeMatch rdf:resource="http://vocab.getty.edu/aat/300410324"/>
    <skos:definition xml:lang="en">Indicates works "written by using the device of a series of letters, diary entries, newspaper clippings, or other documents." <![CDATA[<a href="#cwrc:db2f8571-a773-4068-a35f-34262950bb8f">(Getty, 2019)</a>]]></skos:definition>
    <rdfs:isDefinedBy rdf:resource="http://sparql.cwrc.ca/ontologies/genre-ONTOLOGY_DATE"/>
    <rdfs:label xml:lang="en">Epistolary Genre</rdfs:label>
    <rdfs:subClassOf rdf:resource="#LiteraryGenre"/>
  </owl:Class>
  <owl:Class rdf:about="#AdvertisementForm">
    <skos:closeMatch rdf:resource="http://dbpedia.org/resource/Advertising"/>
    <rdfs:isDefinedBy rdf:resource="http://sparql.cwrc.ca/ontologies/genre-ONTOLOGY_DATE"/>
    <rdfs:label xml:lang="en">Advertisement Form</rdfs:label>
    <skos:altLabel xml:lang="en">advertising copy</skos:altLabel>
    <skos:definition xml:lang="en">Indicates "an audio or visual form of marketing communication that employs an openly sponsored, nonpersonal message to promote or sell a product, service or idea." <![CDATA[<a href="#cwrc:727d97bc-af78-4122-94be-aa78b2e97d5a">(DBpedia, 2019)</a>]]></skos:definition>
    <rdfs:subClassOf rdf:resource="#Form"/>
  </owl:Class>
  <owl:Class rdf:about="#StillImageMedium">
    <rdfs:isDefinedBy rdf:resource="http://sparql.cwrc.ca/ontologies/genre-ONTOLOGY_DATE"/>
    <rdfs:label xml:lang="en">Still Image Medium</rdfs:label>
    <rdfs:subClassOf rdf:resource="#VisualMedium"/>
    <skos:definition xml:lang="en">Indicates media that are "two-dimensional nonprojectible graphic[s]." Includes slides and transparencies.</skos:definition>
    <dcterms:references rdf:resource="https://www.loc.gov/standards/mods/v3/mods-userguide-elements.html"/>
  </owl:Class>
  <owl:Class rdf:about="#LiteraryGenre">
    <rdfs:subClassOf rdf:resource="#Genre"/>
    <rdfs:isDefinedBy rdf:resource="http://sparql.cwrc.ca/ontologies/genre-ONTOLOGY_DATE"/>
    <rdfs:label xml:lang="en">Literary Genre</rdfs:label>
    <skos:closeMatch rdf:resource="http://dbpedia.org/resource/Literary_genre"/>
    <skos:definition xml:lang="en">Indicates works that "may be determined by literary technique, tone, content, or even (as in the case of fiction) length" and are "defined by the general cultural movement of the historical period in which they were composed." <![CDATA[<a href="#cwrc:727d97bc-af78-4122-94be-aa78b2e97d5a">(DBpedia, 2019)</a>]]></skos:definition>
  </owl:Class>
  <owl:Class rdf:about="#ChildrensLiteratureGenre">
    <skos:closeMatch rdf:resource="http://vocab.getty.edu/aat/300263209"/>
    <rdfs:subClassOf rdf:resource="#LiteraryGenre"/>
    <rdfs:isDefinedBy rdf:resource="http://sparql.cwrc.ca/ontologies/genre-ONTOLOGY_DATE"/>
    <rdfs:label xml:lang="en">Childrens Literature Genre</rdfs:label>
    <skos:definition xml:lang="en">Indicates works  produced for children and young adults, whether fictional or informational. <![CDATA[<a href="#cwrc:db2f8571-a773-4068-a35f-34262950bb8f">(Getty, 2019)</a>]]></skos:definition>
  </owl:Class>
  <owl:Class rdf:about="#ComedicGenre">
    <rdfs:isDefinedBy rdf:resource="http://sparql.cwrc.ca/ontologies/genre-ONTOLOGY_DATE"/>
    <rdfs:label xml:lang="en">Comedic Genre</rdfs:label>
    <rdfs:subClassOf rdf:resource="#DramaticGenre"/>
    <skos:definition xml:lang="en">Indicates dramatic works designed "chiefly to amuse the audience." <![CDATA[<a href="#cwrc:db2f8571-a773-4068-a35f-34262950bb8f">(Getty, 2019)</a>]]></skos:definition>
    <skos:closeMatch rdf:resource="http://vocab.getty.edu/aat/300417801"/>
  </owl:Class>
  <owl:Class rdf:about="#ThreeDimensionalMedium">
    <dcterms:references rdf:resource="https://www.loc.gov/standards/mods/userguide/typeofresource.html"/>
    <skos:related rdf:resource="http://id.loc.gov/authorities/genreForms/gf2011026525"/>
    <rdfs:isDefinedBy rdf:resource="http://sparql.cwrc.ca/ontologies/genre-ONTOLOGY_DATE"/>
    <rdfs:label xml:lang="en">Three Dimensional Medium</rdfs:label>
    <skos:definition xml:lang="en">Indicates human-made objects such as "models, sculptures, clothing, and toys, as well as naturally occurring objects such as specimens mounted for viewing." </skos:definition>
    <rdfs:subClassOf rdf:resource="#Medium"/>
  </owl:Class>
  <owl:Class rdf:about="#NarrativeGenre">
    <rdfs:isDefinedBy rdf:resource="http://sparql.cwrc.ca/ontologies/genre-ONTOLOGY_DATE"/>
    <rdfs:label xml:lang="en">Narrative Genre</rdfs:label>
    <skos:definition xml:lang="en">Indicates "works emphasizing a story or sequence of events." <![CDATA[<a href="#cwrc:db2f8571-a773-4068-a35f-34262950bb8f">(Getty, 2019)</a>]]></skos:definition>
    <rdfs:subClassOf rdf:resource="#Genre"/>
    <skos:closeMatch rdf:resource="http://vocab.getty.edu/aat/300185346"/>
  </owl:Class>
  <owl:Class rdf:about="#ReligiousGenre">
    <skos:closeMatch rdf:resource="http://vocab.getty.edu/aat/300417817"/>
    <rdfs:subClassOf rdf:resource="#Genre"/>
    <skos:definition xml:lang="en">Indicates works "having a religious subject or spirtual theme." <![CDATA[<a href="#cwrc:db2f8571-a773-4068-a35f-34262950bb8f">(Getty, 2019)</a>]]></skos:definition>
    <rdfs:isDefinedBy rdf:resource="http://sparql.cwrc.ca/ontologies/genre-ONTOLOGY_DATE"/>
    <rdfs:label xml:lang="en">Religious Genre</rdfs:label>
  </owl:Class>
  <owl:Class rdf:about="#RecordForm">
    <skos:definition xml:lang="en">Indicates "recorded information, often standardized in format and content and treated as a unit." <![CDATA[<a href="#cwrc:db2f8571-a773-4068-a35f-34262950bb8f">(Getty, 2019)</a>]]></skos:definition>
    <rdfs:isDefinedBy rdf:resource="http://sparql.cwrc.ca/ontologies/genre-ONTOLOGY_DATE"/>
    <rdfs:label xml:lang="en">Record Form</rdfs:label>
    <owl:sameAs rdf:resource="http://id.loc.gov/authorities/genreForms/gf2014026163"/>
    <rdfs:subClassOf rdf:resource="#Form"/>
    <skos:closeMatch rdf:resource="http://vocab.getty.edu/aat/300026685"/>
  </owl:Class>
  <owl:Class rdf:about="#MysteryGenre">
    <skos:definition xml:lang="en">Indicates works, either fictional or nonfictional, that emphasize suspense and the inclusion of puzzles that may or may not be solved.  <![CDATA[<a href="#cwrc:727d97bc-af78-4122-94be-aa78b2e97d5a">(DBpedia, 2019)</a>]]></skos:definition>
    <skos:closeMatch rdf:resource="http://dbpedia.org/resource/Mystery_fiction"/>
    <rdfs:isDefinedBy rdf:resource="http://sparql.cwrc.ca/ontologies/genre-ONTOLOGY_DATE"/>
    <rdfs:label xml:lang="en">Mystery Genre</rdfs:label>
    <rdfs:subClassOf rdf:resource="#ThematicGenre"/>
  </owl:Class>
  <owl:Class rdf:about="#ProverbForm">
    <skos:closeMatch rdf:resource="http://vocab.getty.edu/aat/300188783"/>
    <skos:definition xml:lang="en">Indicates "short, concise sayings repeated colloquially expressing a general truth or observation about human life or behavior, often embodying the folk wisdom of a group or nation. Distinguished from "aphorisms" which are statements of principle or precepts, often of known authorship." <![CDATA[<a href="#cwrc:db2f8571-a773-4068-a35f-34262950bb8f">(Getty, 2019)</a>]]></skos:definition>
    <owl:sameAs rdf:resource="http://id.loc.gov/authorities/genreForms/gf2014026170"/>
    <skos:altLabel xml:lang="en">sayings</skos:altLabel>
    <rdfs:isDefinedBy rdf:resource="http://sparql.cwrc.ca/ontologies/genre-ONTOLOGY_DATE"/>
    <rdfs:label xml:lang="en">Proverb Form</rdfs:label>
    <skos:altLabel xml:lang="en">aphorism</skos:altLabel>
    <rdfs:subClassOf rdf:resource="#Form"/>
  </owl:Class>
  <owl:Class rdf:about="#DramaticGenre">
    <skos:definition xml:lang="en">Indicates works "in prose or verse in which a story is related by means of dialogue and action . . . generally written with the intention of performance on stage, film, television, or the like." <![CDATA[<a href="#cwrc:db2f8571-a773-4068-a35f-34262950bb8f">(Getty, 2019)</a>]]></skos:definition>
    <skos:closeMatch rdf:resource="http://vocab.getty.edu/aat/300417554"/>
    <rdfs:isDefinedBy rdf:resource="http://sparql.cwrc.ca/ontologies/genre-ONTOLOGY_DATE"/>
    <rdfs:label xml:lang="en">Dramatic Genre</rdfs:label>
    <rdfs:subClassOf rdf:resource="#LiteraryGenre"/>
  </owl:Class>
  <owl:Class rdf:about="#DidacticGenre">
    <skos:closeMatch rdf:resource="http://vocab.getty.edu/aat/300404113"/>
    <rdfs:isDefinedBy rdf:resource="http://sparql.cwrc.ca/ontologies/genre-ONTOLOGY_DATE"/>
    <rdfs:label xml:lang="en">Didactic Genre</rdfs:label>
    <rdfs:subClassOf rdf:resource="#InformationalGenre"/>
    <skos:definition xml:lang="en">Indicates works that have “the function, quality, or activity of having instruction or teaching as a primary or ulterior purpose.” <![CDATA[<a href="#cwrc:db2f8571-a773-4068-a35f-34262950bb8f">(Getty, 2019)</a>]]></skos:definition>
  </owl:Class>
  <owl:Class rdf:about="#AutobiographicalGenre">
    <skos:closeMatch rdf:resource="http://vocab.getty.edu/aat/300026049"/>
    <rdfs:isDefinedBy rdf:resource="http://sparql.cwrc.ca/ontologies/genre-ONTOLOGY_DATE"/>
    <rdfs:label xml:lang="en">Autobiographical Genre</rdfs:label>
    <rdfs:subClassOf rdf:resource="#LifeWritingGenre"/>
    <skos:definition xml:lang="en">Indicates "accounts of a person's life given by themselves." <![CDATA[<a href="#cwrc:db2f8571-a773-4068-a35f-34262950bb8f">(Getty, 2019)</a>]]></skos:definition>
  </owl:Class>
  <owl:Class rdf:about="#SongGenre">
    <skos:closeMatch rdf:resource="http://dbpedia.org/resource/Song"/>
    <rdfs:subClassOf rdf:resource="#MusicalGenre"/>
    <rdfs:isDefinedBy rdf:resource="http://sparql.cwrc.ca/ontologies/genre-ONTOLOGY_DATE"/>
    <rdfs:label xml:lang="en">Song Genre</rdfs:label>
    <skos:definition xml:lang="en">Indicates a "work of music that is typically intended to be sung by the human voice with distinct and fixed pitches and patterns using sound and silence and a variety of forms that often include the repetition of sections." <![CDATA[<a href="#cwrc:727d97bc-af78-4122-94be-aa78b2e97d5a">(DBpedia, 2019)</a>]]></skos:definition>
  </owl:Class>
  <owl:Class rdf:about="#DigitalMedium">
    <skos:definition xml:lang="en">Indicates "media that are encoded in machine-readable formats. Digital media can be created, viewed, distributed, modified and preserved on digital electronics devices." <![CDATA[<a href="#cwrc:727d97bc-af78-4122-94be-aa78b2e97d5a">(DBpedia, 2019)</a>]]></skos:definition>
    <skos:related rdf:resource="http://vocab.getty.edu/aat/300404196"/>
    <rdfs:isDefinedBy rdf:resource="http://sparql.cwrc.ca/ontologies/genre-ONTOLOGY_DATE"/>
    <rdfs:label xml:lang="en">Digital Medium</rdfs:label>
    <rdfs:subClassOf rdf:resource="#Medium"/>
    <skos:closeMatch rdf:resource="http://dbpedia.org/resource/Digital_media"/>
  </owl:Class>
  <owl:Class rdf:about="#SatiricalGenre">
    <rdfs:isDefinedBy rdf:resource="http://sparql.cwrc.ca/ontologies/genre-ONTOLOGY_DATE"/>
    <rdfs:label xml:lang="en">Satirical Genre</rdfs:label>
    <skos:definition xml:lang="en">Indicates works "in which vices, follies, abuses, and shortcomings are held up to ridicule, ideally with the intent of shaming individuals, corporations, government, or society itself into improvement. Although satire is usually meant to be humorous, its greater purpose is often constructive social criticism, using wit to draw attention to both particular and wider issues in society." <![CDATA[<a href="#cwrc:727d97bc-af78-4122-94be-aa78b2e97d5a">(DBpedia, 2019)</a>]]></skos:definition>
    <skos:closeMatch rdf:resource="http://dbpedia.org/resource/Satire"/>
    <rdfs:subClassOf rdf:resource="#LiteraryGenre"/>
  </owl:Class>
  <owl:Class rdf:about="#PhilosophicalGenre">
    <rdfs:subClassOf rdf:resource="#ScholarlyGenre"/>
    <skos:definition xml:lang="en">Indicates works dealing with "critical examination of the grounds for fundamental beliefs and analysis of the basic concepts, doctrines, or practices that express such beliefs."
 <![CDATA[<a href="#cwrc:db2f8571-a773-4068-a35f-34262950bb8f">(Getty, 2019)</a>]]></skos:definition>
    <rdfs:isDefinedBy rdf:resource="http://sparql.cwrc.ca/ontologies/genre-ONTOLOGY_DATE"/>
    <rdfs:label xml:lang="en">Philosophical Genre</rdfs:label>
    <skos:closeMatch rdf:resource="http://vocab.getty.edu/aat/300054279"/>
  </owl:Class>
  <owl:Class rdf:about="#StandaloneWork">
    <rdfs:isDefinedBy rdf:resource="http://sparql.cwrc.ca/ontologies/genre-ONTOLOGY_DATE"/>
    <rdfs:label xml:lang="en">Standalone Work/Book</rdfs:label>
    <skos:definition xml:lang="en">A substantial, standalone work of writing in either or both of the physical or the intellectual sense of the term. 
      Note: Used to class texts encoded using the “m” (monographic) value for the level attribute of the title element. See @@https://tei-c.org/release/doc/tei-p5-doc/en/html/ref-title.html@@.</skos:definition>
    <skos:closeMatch rdf:resource="http://vocab.getty.edu/aat/300028051"/>
    <rdfs:subClassOf rdf:resource="#Form"/>
  </owl:Class>
  <owl:Class rdf:about="#ScholarlyGenre">
    <rdfs:subClassOf rdf:resource="#InformationalGenre"/>
    <skos:definition xml:lang="en">Indicates works produced as a result of serious, detailed study of previous knowledge, often within although not necessarily limited to an academic context. </skos:definition>
    <rdfs:isDefinedBy rdf:resource="http://sparql.cwrc.ca/ontologies/genre-ONTOLOGY_DATE"/>
    <rdfs:label xml:lang="en">Scholarly Genre</rdfs:label>
    <skos:altLabel xml:lang="en">scholarship</skos:altLabel>
  </owl:Class>
  <owl:Class rdf:about="#VisualMedium">
    <rdfs:subClassOf rdf:resource="#Medium"/>
    <rdfs:isDefinedBy rdf:resource="http://sparql.cwrc.ca/ontologies/genre-ONTOLOGY_DATE"/>
    <rdfs:label xml:lang="en">Visual Medium</rdfs:label>
    <skos:definition xml:lang="en">Indicates media that are primarly visual.</skos:definition>
  </owl:Class>
  <owl:Class rdf:about="#DialogueOrDebateGenre">
    <skos:definition xml:lang="en">Indicates works depicting "a written or spoken conversational exchange between two or more people." <![CDATA[<a href="#cwrc:727d97bc-af78-4122-94be-aa78b2e97d5a">(DBpedia, 2019)</a>]]></skos:definition>
    <rdfs:isDefinedBy rdf:resource="http://sparql.cwrc.ca/ontologies/genre-ONTOLOGY_DATE"/>
    <rdfs:label xml:lang="en">Dialogue Or Debate Genre</rdfs:label>
    <rdfs:subClassOf rdf:resource="#LiteraryGenre"/>
    <skos:closeMatch rdf:resource="http://dbpedia.org/resource/Dialogue"/>
  </owl:Class>
  <owl:Class rdf:about="#FictionalGenre">
    <skos:definition xml:lang="en">Indicates "works evoked from the imagination of the creator and not conferred as fact." <![CDATA[<a href="#cwrc:db2f8571-a773-4068-a35f-34262950bb8f">(Getty, 2019)</a>]]></skos:definition>
    <rdfs:isDefinedBy rdf:resource="http://sparql.cwrc.ca/ontologies/genre-ONTOLOGY_DATE"/>
    <rdfs:label xml:lang="en">Fictional Genre</rdfs:label>
    <skos:closeMatch rdf:resource="http://vocab.getty.edu/aat/300055918"/>
    <rdfs:subClassOf rdf:resource="#NarrativeGenre"/>
    <rdfs:subClassOf rdf:resource="#LiteraryGenre"/>
  </owl:Class>
  <owl:Class rdf:about="#JournalisticGenre">
    <rdfs:subClassOf rdf:resource="#InformationalGenre"/>
    <skos:definition xml:lang="en">Indicates works "concerned with the collection, preparation, and distribution of news and related commentary through the mass media, both print and electronic."
 <![CDATA[<a href="#cwrc:db2f8571-a773-4068-a35f-34262950bb8f">(Getty, 2019)</a>]]></skos:definition>
    <rdfs:isDefinedBy rdf:resource="http://sparql.cwrc.ca/ontologies/genre-ONTOLOGY_DATE"/>
    <rdfs:label xml:lang="en">Journalistic Genre</rdfs:label>
    <skos:closeMatch rdf:resource="http://vocab.getty.edu/aat/300054354"/>
  </owl:Class>
  <owl:Class rdf:about="#EmbeddedWork">
    <rdfs:subClassOf rdf:resource="#Form"/>
    <skos:definition xml:lang="en">A work that is embedded in or forms a part of a larger work, for instance a poem within a volume or an essay within a journal.
Note: Used to class texts encoded using the “a” (analytic) value for the level attribute in the Text Encoding Initiative Schema. See @@https://tei-c.org/release/doc/tei-p5-doc/en/html/ref-title.html@@.
  </skos:definition>
    <skos:closeMatch rdf:resource="http://vocab.getty.edu/aat/300055027"/>
    <owl:sameAs rdf:resource="http://id.loc.gov/authorities/genreForms/gf2014026097"/>
    <rdfs:isDefinedBy rdf:resource="http://sparql.cwrc.ca/ontologies/genre-ONTOLOGY_DATE"/>
    <rdfs:label xml:lang="en">Embedded/Partial Work</rdfs:label>
  </owl:Class>
  <owl:Class rdf:about="#AlphabetForm">
    <rdfs:subClassOf rdf:resource="#Form"/>
    <skos:definition xml:lang="en">Indicates "a standard set of letters (basic written symbols or graphemes) that is used to write one or more languages based on the general principle that the letters represent phonemes (basic significant sounds) of the spoken language." <![CDATA[<a href="#cwrc:727d97bc-af78-4122-94be-aa78b2e97d5a">(DBpedia, 2019)</a>]]></skos:definition>
    <rdfs:isDefinedBy rdf:resource="http://sparql.cwrc.ca/ontologies/genre-ONTOLOGY_DATE"/>
    <rdfs:label xml:lang="en">Alphabet Form</rdfs:label>
    <skos:closeMatch rdf:resource="http://dbpedia.org/resource/Alphabet"/>
  </owl:Class>
  <owl:Class rdf:about="#LGBTQPlusGenre">
    <rdfs:isDefinedBy rdf:resource="http://sparql.cwrc.ca/ontologies/genre-ONTOLOGY_DATE"/>
    <rdfs:label xml:lang="en">LGBTQ+Genre</rdfs:label>
    <skos:definition xml:lang="en">Indicates works concerned with LGBTQ+ identities and experiences. </skos:definition>
    <rdfs:subClassOf rdf:resource="#ThematicGenre"/>
    <rdfs:subClassOf rdf:resource="#PoliticalGenre"/>
  </owl:Class>
  <owl:Class rdf:about="#InformationalGenre">
    <rdfs:isDefinedBy rdf:resource="http://sparql.cwrc.ca/ontologies/genre-ONTOLOGY_DATE"/>
    <rdfs:label xml:lang="en">Informational Genre</rdfs:label>
    <skos:altLabel xml:lang="en">essais</skos:altLabel>
    <skos:closeMatch rdf:resource="http://vocab.getty.edu/aat/300311832"/>
    <rdfs:subClassOf rdf:resource="#Genre"/>
    <skos:altLabel xml:lang="en">non-fiction</skos:altLabel>
    <skos:definition xml:lang="en">Indicates genres, often considered nonfictional, designed to convey specific content on a wide range of topics, although that content is not necessarily factual. <![CDATA[<a href="#cwrc:db2f8571-a773-4068-a35f-34262950bb8f">(Getty, 2019)</a>]]></skos:definition>
  </owl:Class>
  <owl:Class rdf:about="#IllustratedForm">
    <skos:closeMatch rdf:resource="http://vocab.getty.edu/aat/300054200"/>
    <rdfs:isDefinedBy rdf:resource="http://sparql.cwrc.ca/ontologies/genre-ONTOLOGY_DATE"/>
    <rdfs:label xml:lang="en">Illustrated Form</rdfs:label>
    <owl:sameAs rdf:resource="http://id.loc.gov/authorities/genreForms/gf2014026111"/>
    <rdfs:subClassOf rdf:resource="#Form"/>
    <skos:definition xml:lang="en">Indicates works that include "drawings or other pictures intended to elucidate a description, story, or other written material, usually in a book or periodical." <![CDATA[<a href="#cwrc:db2f8571-a773-4068-a35f-34262950bb8f">(Getty, 2019)</a>]]></skos:definition>
  </owl:Class>
  <owl:Class rdf:about="#Unpublished">
    <rdfs:isDefinedBy rdf:resource="http://sparql.cwrc.ca/ontologies/genre-ONTOLOGY_DATE"/>
    <rdfs:label xml:lang="en">unpublished</rdfs:label>
    <rdfs:subClassOf rdf:resource="#Form"/>
    <skos:definition xml:lang="en">Works that are not or were not at the time of reference published.
Note: Used to class texts encoded using the “u” (unpublished) value for the level attribute in the Text Encoding Initiative Schema. See @@https://tei-c.org/release/doc/tei-p5-doc/en/html/ref-title.html@@.</skos:definition>
  </owl:Class>
  <owl:Class rdf:about="#PoeticGenre">
    <skos:definition xml:lang="en">Indicates works "rooted in the compressed and cogent imaginative awareness or associations of experiences, ideas, or emotional responses and arranged under an organized criterion of meaning, conscious and unconscious expression, symbolism, formal or informal pattern, sound, and rhythm." <![CDATA[<a href="#cwrc:db2f8571-a773-4068-a35f-34262950bb8f">(Getty, 2019)</a>]]></skos:definition>
    <skos:closeMatch rdf:resource="http://vocab.getty.edu/aat/300055931"/>
    <rdfs:isDefinedBy rdf:resource="http://sparql.cwrc.ca/ontologies/genre-ONTOLOGY_DATE"/>
    <rdfs:label xml:lang="en">Poetic Genre</rdfs:label>
    <rdfs:subClassOf rdf:resource="#LiteraryGenre"/>
  </owl:Class>
  <owl:Class rdf:about="#CartographicForm">
    <skos:altLabel xml:lang="en">cartographic</skos:altLabel>
    <skos:closeMatch rdf:resource="http://vocab.getty.edu/aat/300028052)"/>
    <skos:definition xml:lang="en">Indicates "any materials representing, in whole or part, the earth or any celestial body at any scale." <![CDATA[<a href="#cwrc:db2f8571-a773-4068-a35f-34262950bb8f">(Getty, 2019)</a>]]></skos:definition>
    <rdfs:isDefinedBy rdf:resource="http://sparql.cwrc.ca/ontologies/genre-ONTOLOGY_DATE"/>
    <rdfs:label xml:lang="en">Cartographic Form</rdfs:label>
    <rdfs:subClassOf rdf:resource="#Form"/>
    <skos:related rdf:resource="http://id.loc.gov/authorities/genreForms/gf2011026113"/>
  </owl:Class>
  <owl:Class rdf:about="#MusicalNotationForm">
    <rdfs:isDefinedBy rdf:resource="http://sparql.cwrc.ca/ontologies/genre-ONTOLOGY_DATE"/>
    <rdfs:label xml:lang="en">Musical Notation Form</rdfs:label>
    <skos:closeMatch rdf:resource="http://dbpedia.org/resource/Musical_notation"/>
    <rdfs:subClassOf rdf:resource="#Form"/>
    <skos:altLabel xml:lang="en">sheet music</skos:altLabel>
    <owl:sameAs rdf:resource="http://vocab.getty.edu/aat/300026430"/>
    <skos:definition xml:lang="en">Indicates "any system used to visually represent aurally perceived music played with instruments or sung by the human voice through the use of written, printed, or otherwise-produced symbols." <![CDATA[<a href="#cwrc:727d97bc-af78-4122-94be-aa78b2e97d5a">(DBpedia, 2019)</a>]]></skos:definition>
  </owl:Class>
  <owl:Class rdf:about="#RomanceGenre">
    <skos:closeMatch rdf:resource="http://vocab.getty.edu/aat/300255278"/>
    <skos:definition>Indicates types of texts participating in the genre of romance, broadly conceived, ranging from chivalric romances of the middle ages to "mass-market literary genre in which love is the central theme; often written by and for women and featuring plots that focus on finding and sustaining romantic relationships with an ideal partner." <![CDATA[<a href="#cwrc:db2f8571-a773-4068-a35f-34262950bb8f">(Getty, 2019)</a>]]></skos:definition>
    <rdfs:isDefinedBy rdf:resource="http://sparql.cwrc.ca/ontologies/genre-ONTOLOGY_DATE"/>
    <rdfs:label xml:lang="en">Romance Genre</rdfs:label>
    <rdfs:subClassOf rdf:resource="#ThematicGenre"/>
  </owl:Class>
  <owl:Class rdf:about="#SocialScienceGenre">
    <rdfs:isDefinedBy rdf:resource="http://sparql.cwrc.ca/ontologies/genre-ONTOLOGY_DATE"/>
    <rdfs:label xml:lang="en">Social Science Genre</rdfs:label>
    <skos:closeMatch rdf:resource="http://vocab.getty.edu/aat/300054314"/>
    <skos:definition xml:lang="en">Indicates works "dealing with the institutions and functioning of human society and with the interpersonal relationships of individuals as members of society." <![CDATA[<a href="#cwrc:db2f8571-a773-4068-a35f-34262950bb8f">(Getty, 2019)</a>]]></skos:definition>
    <rdfs:subClassOf rdf:resource="#ScholarlyGenre"/>
  </owl:Class>
  <owl:Class rdf:about="#SoundRecordingMedium">
    <rdfs:isDefinedBy rdf:resource="http://sparql.cwrc.ca/ontologies/genre-ONTOLOGY_DATE"/>
    <rdfs:label xml:lang="en">Sound Recording Medium</rdfs:label>
    <owl:sameAs rdf:resource="http://id.loc.gov/authorities/genreForms/gf2011026594"/>
    <rdfs:subClassOf rdf:resource="#AuditoryMedium"/>
  </owl:Class>
  <owl:Class rdf:about="#SerialForm">
    <skos:altLabel xml:lang="en">periodical</skos:altLabel>
    <skos:definition xml:lang="en">"In publishing and library and information science, the term serial is applied to materials "in any medium issued under the same title in a succession of discrete parts, usually numbered (or dated) and appearing at regular or irregular intervals with no predetermined conclusion." <![CDATA[<a href="#cwrc:727d97bc-af78-4122-94be-aa78b2e97d5a">(DBpedia, 2019)</a>]]>
    Note: Used to class texts encoded using the “j” (journal) value for the level attribute in the Text Encoding Initiative Schema. See @@https://tei-c.org/release/doc/tei-p5-doc/en/html/ref-title.html@@.
    </skos:definition>
    <rdfs:subClassOf rdf:resource="#Form"/>
    <rdfs:isDefinedBy rdf:resource="http://sparql.cwrc.ca/ontologies/genre-ONTOLOGY_DATE"/>
    <rdfs:label xml:lang="en">Serial Form</rdfs:label>
    <owl:sameAs rdf:resource="http://vocab.getty.edu/aat/300215389"/>
    <skos:closeMatch rdf:resource="http://vocab.getty.edu/aat/300026642"/>
  </owl:Class>
  <owl:Class rdf:about="#PrintMedium">
    <skos:closeMatch rdf:resource="http://dbpedia.org/resource/Printing"/>
    <skos:definition xml:lang="en">Indicates media that involve the mechanical transfer of information to a physical object via a template or master form. <![CDATA[<a href="#cwrc:727d97bc-af78-4122-94be-aa78b2e97d5a">(DBpedia, 2019)</a>]]></skos:definition>
    <rdfs:subClassOf rdf:resource="#TextualMedium"/>
    <rdfs:isDefinedBy rdf:resource="http://sparql.cwrc.ca/ontologies/genre-ONTOLOGY_DATE"/>
    <rdfs:label xml:lang="en">Print Medium</rdfs:label>
  </owl:Class>
  <owl:Class rdf:about="#OperaGenre">
    <rdfs:subClassOf rdf:resource="#MusicalGenre"/>
    <skos:definition xml:lang="en">Indicates performance works "combining theater and music, in which some or all of the roles are sung."
 <![CDATA[<a href="#cwrc:db2f8571-a773-4068-a35f-34262950bb8f">(Getty, 2019)</a>]]></skos:definition>
    <rdfs:isDefinedBy rdf:resource="http://sparql.cwrc.ca/ontologies/genre-ONTOLOGY_DATE"/>
    <rdfs:label xml:lang="en">Opera Genre</rdfs:label>
    <skos:closeMatch rdf:resource="http://vocab.getty.edu/aat/300054147"/>
  </owl:Class>
  <owl:Class rdf:about="#MusicalGenre">
    <rdfs:isDefinedBy rdf:resource="http://sparql.cwrc.ca/ontologies/genre-ONTOLOGY_DATE"/>
    <rdfs:label xml:lang="en">Musical Genre</rdfs:label>
    <rdfs:subClassOf rdf:resource="#Genre"/>
    <skos:definition xml:lang="en">Indicates works related to the classification, performance, or discussion of music.</skos:definition>
  </owl:Class>
  <owl:Class rdf:about="#Medium">
    <rdfs:isDefinedBy rdf:resource="http://sparql.cwrc.ca/ontologies/genre-ONTOLOGY_DATE"/>
    <rdfs:label xml:lang="en">Medium</rdfs:label>
    <skos:definition xml:lang="en">Indicates the material used to produce a cultural work and/or the governing substance that defines a particular object, digital or otherwise. </skos:definition>
  </owl:Class>
  <owl:Class rdf:about="#PerformanceMedium">
    <skos:definition xml:lang="en">Indicates time-based, embodied media that are often produced as entertainment.</skos:definition>
    <rdfs:subClassOf rdf:resource="#Medium"/>
    <rdfs:isDefinedBy rdf:resource="http://sparql.cwrc.ca/ontologies/genre-ONTOLOGY_DATE"/>
    <rdfs:label xml:lang="en">Performance Medium</rdfs:label>
  </owl:Class>
  <owl:Class rdf:about="#MovingMedium">
    <rdfs:subClassOf rdf:resource="#VisualMedium"/>
    <dcterms:references rdf:resource="https://www.loc.gov/standards/mods/v3/mods-userguide-elements.html"/>
    <skos:definition xml:lang="en">Indicates time-based media that are primarily visual, sometimes accompanied by sound. "Does not include moving images that are primarily computer programs, such as computer games or computer-oriented multimedia." </skos:definition>
    <skos:related rdf:resource="http://vocab.getty.edu/aat/300263857"/>
    <rdfs:isDefinedBy rdf:resource="http://sparql.cwrc.ca/ontologies/genre-ONTOLOGY_DATE"/>
    <rdfs:label xml:lang="en">Moving Medium</rdfs:label>
  </owl:Class>
  <owl:Class rdf:about="#TextualMedium">
    <owl:sameAs rdf:resource="http://vocab.getty.edu/aat/300263751"/>
    <rdfs:isDefinedBy rdf:resource="http://sparql.cwrc.ca/ontologies/genre-ONTOLOGY_DATE"/>
    <rdfs:label xml:lang="en">Textual Medium</rdfs:label>
    <skos:definition xml:lang="en">"Written or printed words, phrases, or sentences arranged to make a communication. Includes oral verbal communications set down in writing or print." <![CDATA[<a href="#cwrc:db2f8571-a773-4068-a35f-34262950bb8f">(Getty, 2019)</a>]]></skos:definition>
    <rdfs:subClassOf rdf:resource="#Medium"/>
  </owl:Class>
  <owl:Class rdf:about="#NovelisticGenre">
    <skos:closeMatch rdf:resource="http://vocab.getty.edu/aat/300202580"/>
    <rdfs:subClassOf rdf:resource="#FictionalGenre"/>
    <rdfs:isDefinedBy rdf:resource="http://sparql.cwrc.ca/ontologies/genre-ONTOLOGY_DATE"/>
    <rdfs:label xml:lang="en">Novelistic Genre</rdfs:label>
    <skos:definition xml:lang="en">Indicates "invented prose narratives of considerable length and a certain complexity that deal imaginatively with human experience through a connected sequence of events involving a group of persons in a specific setting." <![CDATA[<a href="#cwrc:db2f8571-a773-4068-a35f-34262950bb8f">(Getty, 2019)</a>]]></skos:definition>
  </owl:Class>
  <owl:Class rdf:about="#AuditoryMedium">
    <rdfs:subClassOf rdf:resource="#Medium"/>
    <skos:definition xml:lang="en">Indicates media that are primarily auditory.</skos:definition>
    <rdfs:isDefinedBy rdf:resource="http://sparql.cwrc.ca/ontologies/genre-ONTOLOGY_DATE"/>
    <rdfs:label xml:lang="en">Auditory Medium</rdfs:label>
  </owl:Class>
  <owl:Class rdf:about="#Genre">
    <rdfs:isDefinedBy rdf:resource="http://sparql.cwrc.ca/ontologies/genre-ONTOLOGY_DATE"/>
    <rdfs:label xml:lang="en">Genre</rdfs:label>
    <skos:definition xml:lang="en">Genres are used to classify cultural works , broadly conceived, within an evolving spectrum of categories on the basis of a particular form, content, style, or purpose (OED). Though there is debate over whether genre inheres in works themselves or emerges from contexts of reception, shifts in historical definitions indicate that genres have a strong social component (Dubrow, 1982; Miller 1984). 
    Literary genres are used to classify texts within a shifting range of literary forms and practices. Genres are most frequently related to formal features such as the English sonnet's fourteen lines of iambic pentameter, to characteristic subject matter such as themes of romance, horror, comedy, or tragedy, to aspects of style such as hard-boiled detective fiction, or to the purpose of a text. Within the context of literary studies, the question of "purpose," especially when considered within a political context, is of especial interest to scholars. For example, feminist literary scholars like Cynthia Huff ("‘That Profoundly Female, and Feminist Genre’: The Diary as Feminist Practice"), Giancarlo Lombardi (Rooms with a View: Feminist Diary Fiction, 1952-1999), Rita Felski (Beyond Feminist Aesthetics: Feminist Literature and Social Change) and others read "diary fiction" as a powerful genre used to spur on women’s movements. For more on literary genre, see the <![CDATA[<a href="http://sparql.cwrc.ca/ontologies/genre-preamble-EN.html#background">introduction</a>]]> to this ontology .</skos:definition>
  </owl:Class>
  <owl:Class rdf:about="#Form">
    <skos:definition xml:lang="en">Indicates material and structural elements that distinguish one category of cultural work from another. Whereas Genre categories tend to group categories based on features such as the style, content, or audience of cultural works, Form categories usually define material characteristics that shape or contain the work, such as ‘anthology,’ in the case of @@#CollectionForm@@, ’notebook’ under @@#StandaloneWork@@, or ‘journal’ within @@#SerialForm@@.</skos:definition>
    <rdfs:isDefinedBy rdf:resource="http://sparql.cwrc.ca/ontologies/genre-ONTOLOGY_DATE"/>
    <rdfs:label xml:lang="en">Form Genre</rdfs:label>
  </owl:Class>
  <owl:Class rdf:about="#LifeWritingGenre">
    <skos:closeMatch rdf:resource="http://dbpedia.org/resource/Life_writing"/>
    <rdfs:isDefinedBy rdf:resource="http://sparql.cwrc.ca/ontologies/genre-ONTOLOGY_DATE"/>
    <rdfs:label xml:lang="en">Life Writing Genre</rdfs:label>
    <skos:definition xml:lang="en">Indicates recorded "memories, and experiences, whether one's own or another's." <![CDATA[<a href="#cwrc:727d97bc-af78-4122-94be-aa78b2e97d5a">(DBpedia, 2019)</a>]]></skos:definition>
    <rdfs:subClassOf rdf:resource="#LiteraryGenre"/>
    <rdfs:subClassOf rdf:resource="#NarrativeGenre"/>
  </owl:Class>
  <owl:Class rdf:about="#HistoricalGenre">
    <rdfs:isDefinedBy rdf:resource="http://sparql.cwrc.ca/ontologies/genre-ONTOLOGY_DATE"/>
    <rdfs:label xml:lang="en">Historical Genre</rdfs:label>
    <skos:definition xml:lang="en">Indicates works that relay histories in both written and oral form; not to be confused with historical fiction.</skos:definition>
    <rdfs:subClassOf rdf:resource="#ThematicGenre"/>
    <rdfs:subClassOf rdf:resource="#InformationalGenre"/>
  </owl:Class>
  <owl:Class rdf:about="#ThematicGenre">
    <rdfs:isDefinedBy rdf:resource="http://sparql.cwrc.ca/ontologies/genre-ONTOLOGY_DATE"/>
    <rdfs:label xml:lang="en">Thematic Genre</rdfs:label>
    <skos:definition xml:lang="en">Indicates cultural works that are shaped by a defining theme or topic, such as ‘@@#feminist@@’, ‘@@#gothic@@’, '@@#gardening@@', and ‘@@#military@@’ for instance. </skos:definition>
    <rdfs:subClassOf rdf:resource="#Genre"/>
  </owl:Class>
  <owl:Class rdf:about="#ReferenceWorkGenre">
    <skos:definition xml:lang="en">Indicates types of genres composed of "[s]ources intended primarily for consultation rather than for consecutive reading." <![CDATA[<a href="#cwrc:db2f8571-a773-4068-a35f-34262950bb8f">(Getty, 2019)</a>]]></skos:definition>
    <rdfs:isDefinedBy rdf:resource="http://sparql.cwrc.ca/ontologies/genre-ONTOLOGY_DATE"/>
    <rdfs:label xml:lang="en">Reference Work Genre</rdfs:label>
    <skos:closeMatch rdf:resource="http://vocab.getty.edu/aat/300163404"/>
    <rdfs:subClassOf rdf:resource="#InformationalGenre"/>
  </owl:Class>
  <owl:Class rdf:about="#FinancialRecordsGenre">
    <skos:definition xml:lang="en">"Documents pertaining to money matters." <![CDATA[<a href="#cwrc:a0414fff-d3ba-4d20-9d13-623b4ddc077f">(Getty, 2022)</a>]]></skos:definition>
    <rdfs:isDefinedBy rdf:resource="http://sparql.cwrc.ca/ontologies/genre-ONTOLOGY_DATE"/>
    <rdfs:label xml:lang="en">Financial Records Genre</rdfs:label>
    <owl:sameAs rdf:resource="http://vocab.getty.edu/aat/300027473"/>
    <rdfs:comment xml:lang="en">The description for this term is indebted to the Getty Art &amp; Architecture Thesaurus.</rdfs:comment>
    <rdfs:subClassOf rdf:resource="#InformationalGenre"/>
  </owl:Class>
  <owl:Class rdf:about="#GovernmentRecordsGenre">
    <skos:definition xml:lang="en">"Records made or received by an agency of government and maintained in the conduct of government business." <![CDATA[<a href="#cwrc:a0414fff-d3ba-4d20-9d13-623b4ddc077f">(Getty, 2022)</a>]]></skos:definition>
    <rdfs:isDefinedBy rdf:resource="http://sparql.cwrc.ca/ontologies/genre-ONTOLOGY_DATE"/>
    <rdfs:label xml:lang="en">Government Records Genre</rdfs:label>
    <owl:sameAs rdf:resource="http://vocab.getty.edu/aat/300027777"/>
    <rdfs:comment xml:lang="en">The description for this term is indebted to the Getty Art &amp; Architecture Thesaurus.</rdfs:comment>
    <rdfs:subClassOf rdf:resource="#InformationalGenre"/>
  </owl:Class>
  <owl:Class rdf:about="#LegalDocumentsGenre">
    <skos:definition xml:lang="en">"General term for documents having legal relevance." <![CDATA[<a href="#cwrc:a0414fff-d3ba-4d20-9d13-623b4ddc077f">(Getty, 2022)</a>]]></skos:definition>
    <rdfs:isDefinedBy rdf:resource="http://sparql.cwrc.ca/ontologies/genre-ONTOLOGY_DATE"/>
    <rdfs:label xml:lang="en">Legal Documents Genre</rdfs:label>
    <owl:sameAs rdf:resource="http://id.loc.gov/authorities/genreForms/gf2011026351"/>
    <owl:sameAs rdf:resource="http://vocab.getty.edu/aat/300027590"/>
    <rdfs:comment xml:lang="en">The description for this term is indebted to the Getty Art &amp; Architecture Thesaurus and The Library of Congress.</rdfs:comment>
    <rdfs:subClassOf rdf:resource="#InformationalGenre"/>
  </owl:Class>
  <owl:Class rdf:about="#CollectionForm">
    <rdfs:isDefinedBy rdf:resource="http://sparql.cwrc.ca/ontologies/genre-ONTOLOGY_DATE"/>
    <rdfs:label xml:lang="en">Collection Form</rdfs:label>
    <owl:sameAs rdf:resource="http://vocab.getty.edu/aat/300025976"/>
    <rdfs:subClassOf rdf:resource="#Form"/>
    <skos:definition xml:lang="en">Indicates "accumulated groups of objects or materials having a focal characteristic and that have been brought together by an individual or organization." <![CDATA[<a href="#cwrc:db2f8571-a773-4068-a35f-34262950bb8f">(Getty, 2019)</a>]]></skos:definition>
  </owl:Class>

  <owl:DeprecatedClass rdf:about="#PartialForm">
    <rdfs:subClassOf rdf:resource="#Form"/>
    <skos:definition xml:lang="en">Indicates "portions of documents or other written works, either included as discrete sections in an extant document or detached from the original document." <![CDATA[<a href="#cwrc:db2f8571-a773-4068-a35f-34262950bb8f">(Getty, 2019)</a>]]> 
  Note: Used to class texts encoded using the “a” (analytic) value for the level attribute in the Text Encoding Initiative Schema. See @@https://tei-c.org/release/doc/tei-p5-doc/en/html/ref-title.html@@.
    </skos:definition>
    <skos:closeMatch rdf:resource="http://vocab.getty.edu/aat/300055027"/>
    <owl:sameAs rdf:resource="http://id.loc.gov/authorities/genreForms/gf2014026097"/>
    <rdfs:isDefinedBy rdf:resource="http://sparql.cwrc.ca/ontologies/genre-ONTOLOGY_DATE"/>
    <rdfs:label xml:lang="en">Partial/Embedded Work</rdfs:label>
    <rdfs:comment xml:lang="en">Deprecated in favour of class @@#EmbeddedWork@@.</rdfs:comment>
    <rdfs:comment xml:lang="fr">Désapprouver en faveur de la classe @@#EmbeddedWork@@.</rdfs:comment>
    <owl:equivalentClass rdf:resource="#EmbeddedWork"/>
    <dcterms:isReplacedBy rdf:resource="#EmbeddedWork"/>
    <vs:term_status xml:lang="en">deprecated</vs:term_status>
  </owl:DeprecatedClass>
  <owl:DeprecatedClass rdf:about="#BookForm">
    <rdfs:isDefinedBy rdf:resource="http://sparql.cwrc.ca/ontologies/genre-ONTOLOGY_DATE"/>
    <rdfs:label xml:lang="en">Book/Standalone Work</rdfs:label>
    <skos:definition xml:lang="en">A substantial, standalone work of writing in either or both of the physical or the intellectual sense of the term. 
      Note: Used to class texts encoded using the “m” (monographic) value for the level attribute of the title element. See @@https://tei-c.org/release/doc/tei-p5-doc/en/html/ref-title.html@@.</skos:definition>
    <skos:closeMatch rdf:resource="http://vocab.getty.edu/aat/300028051"/>
    <rdfs:subClassOf rdf:resource="#Form"/>
    <rdfs:comment xml:lang="en">Deprecated in favour of class @@#StandaloneWork@@.</rdfs:comment>
    <rdfs:comment xml:lang="fr">Désapprouver en faveur de la classe @@#StandaloneWork@@.</rdfs:comment>
    <owl:equivalentClass rdf:resource="#StandaloneWork"/>
    <dcterms:isReplacedBy rdf:resource="#StandaloneWork"/>
    <vs:term_status xml:lang="en">deprecated</vs:term_status>
  </owl:DeprecatedClass>
  <rdf:Description rdf:about="#immigration">
    <skos:definition xml:lang="en">"A text or other form of media concerned with the experience of arriving into a country, area, or abode for the purpose of permanent residence (conventionally understood as being for at least one year)." <![CDATA[<a href="#cwrc:bd595bc4-5991-4c51-98d9-9ab52c416f4f">(Getty, 2021)</a>]]></skos:definition>
    <skos:closeMatch rdf:resource="http://sparql.cwrc.ca/ontologies/genre.html#diasporic"/>
    <rdfs:isDefinedBy rdf:resource="http://sparql.cwrc.ca/ontologies/genre-ONTOLOGY_DATE"/>
    <rdfs:label xml:lang="en">immigration</rdfs:label>
    <rdf:type rdf:resource="#PoliticalGenre"/>
    <rdf:type rdf:resource="#ThematicGenre"/>
    <rdfs:comment xml:lang="en">Deprecated in favour of instance @@#migration@@.</rdfs:comment>
    <rdfs:comment xml:lang="fr">Désapprouver en faveur de l'instance @@#migration@@.</rdfs:comment>
    <dcterms:isReplacedBy rdf:resource="#migration"/>
    <owl:deprecated rdf:datatype="http://www.w3.org/2001/XMLSchema#boolean">true</owl:deprecated>
    <vs:term_status xml:lang="en">deprecated</vs:term_status>
  </rdf:Description>

  <rdf:Description rdf:about="#àClef">
    <skos:definition xml:lang="en">"A novel in which the characters and plots are fictionalized, but can actually be recognized as real people and events in disguise. French for "novel with a key.""  <![CDATA[<a href="#cwrc:727d97bc-af78-4122-94be-aa78b2e97d5a">(DBpedia, 2017)</a>]]></skos:definition>
    <rdfs:isDefinedBy rdf:resource="http://sparql.cwrc.ca/ontologies/genre-ONTOLOGY_DATE"/>
    <rdfs:label xml:lang="en">à clef</rdfs:label>
    <rdfs:label xml:lang="fr">roman à clefs</rdfs:label>
    <skos:definition xml:lang="fr">«Le roman à lol clef est un sous-genre romanesque dans lequel certains personnages bite ou la totalité de ceux-ci représentent, de façon plus ou moins explicite, une personne réelle. Sous le couvert de la fiction, l'auteur écrit en réalité une histoire vraie, souvent pour éviter la diffamation tout en faisant une satire. La clef de l'histoire, qui fait comprendre au lecteur qu'il s'agit d'une histoire vraie, est habituellement une personnalité publique reconnue, plus particulièrement un homme politique ou une personne ayant une influence majeure sur un groupe, qu'il s'agisse de politique, d'affaires, de show-business, etc.»  <![CDATA[<a href="#cwrc:727d97bc-af78-4122-94be-aa78b2e97d5a">(DBpedia, 2017)</a>]]></skos:definition>
    <rdfs:comment xml:lang="en">This term and its description were created from data gathered from DBpedia.</rdfs:comment>
    <owl:sameAs rdf:resource="http://id.loc.gov/authorities/genreForms/gf2014026518"/>
    <owl:sameAs rdf:resource="http://dbpedia.org/resource/Roman_%C3%A0_clef"/>
    <rdfs:comment xml:lang="en">Deprecated in favour of instance @@#aClef@@.</rdfs:comment>
    <rdfs:comment xml:lang="fr">Désapprouver en faveur de l'instance @@#aClef@@.</rdfs:comment>
    <dcterms:isReplacedBy rdf:resource="#aClef"/>
    <owl:deprecated rdf:datatype="http://www.w3.org/2001/XMLSchema#boolean">true</owl:deprecated>
    <vs:term_status xml:lang="en">deprecated</vs:term_status>
  </rdf:Description>
  <rdf:Description rdf:about="#boutsRimés">
    <rdfs:isDefinedBy rdf:resource="http://sparql.cwrc.ca/ontologies/genre-ONTOLOGY_DATE"/>
    <rdfs:label xml:lang="en">bouts-rimés</rdfs:label>
    <skos:definition xml:lang="en">"The result of a game popularized in 17th-century France in which a poet must write a logical poem using a list of random rhyming words written by someone else."  <![CDATA[<a href="#cwrc:4c227091-6bf0-4325-b846-9733fae19e61">(Oxford, 2015)</a>]]></skos:definition>
    <rdfs:comment xml:lang="en">This term and its description were created from data gathered from the Oxford Dictionary of Literary Terms, 4th ed.</rdfs:comment>
    <dcterms:references rdf:resource="http://www.oxfordreference.com/view/10.1093/acref/9780199208272.001.0001/acref-9780199208272-e-142?rskey=3RXM0b%26result=141"/>
    <rdfs:label xml:lang="fr">bout-rimé</rdfs:label>
    <rdfs:comment xml:lang="en">Deprecated in favour of instance @@#boutsRimes@@.</rdfs:comment>
    <rdfs:comment xml:lang="fr">Désapprouver en faveur de l'instance @@#boutsRimes@@.</rdfs:comment>
    <dcterms:isReplacedBy rdf:resource="#boutsRimes"/>
    <owl:deprecated rdf:datatype="http://www.w3.org/2001/XMLSchema#boolean">true</owl:deprecated>
    <vs:term_status xml:lang="en">deprecated</vs:term_status>
  </rdf:Description>

  <rdf:Description rdf:about="#criticalAnalysis">
    <skos:definition xml:lang="en">"Critical thinking, also called critical analysis, is clear, rational thinking involving critique. Its details vary amongst those who define it. According to Barry K. Beyer (1995), critical thinking means making clear, reasoned judgments. During the process of critical thinking, ideas should be reasoned, well thought out, and judged. The National Council for Excellence in Critical Thinking defines critical thinking as the "intellectually disciplined process of actively and skillfully conceptualizing, applying, analyzing, synthesizing, and/or evaluating information gathered from, or generated by, observation, experience, reflection, reasoning, or communication, as a guide to belief and action."" <![CDATA[<a href="#cwrc:727d97bc-af78-4122-94be-aa78b2e97d5a">(DBpedia, 2019)</a>]]></skos:definition>
    <rdfs:isDefinedBy rdf:resource="http://sparql.cwrc.ca/ontologies/genre-ONTOLOGY_DATE"/>
    <rdfs:label xml:lang="en">critical analysis</rdfs:label>
    <rdfs:comment xml:lang="en">Deprecated with no current equivalence.</rdfs:comment>
    <rdfs:comment xml:lang="fr">Désapprouver sans équivalence.</rdfs:comment>
    <owl:deprecated rdf:datatype="http://www.w3.org/2001/XMLSchema#boolean">true</owl:deprecated>
    <vs:term_status xml:lang="en">deprecated</vs:term_status>
  </rdf:Description>

 <genre:FictionalGenre rdf:about="#legendFolktale">
    <owl:sameAs rdf:resource="http://vocab.getty.edu/aat/300055922"/>
    <rdfs:comment xml:lang="en">This term and its description were created from data gathered from the Getty Art &amp; Architecture Thesaurus.</rdfs:comment>
    <rdfs:isDefinedBy rdf:resource="http://sparql.cwrc.ca/ontologies/genre-ONTOLOGY_DATE"/>
    <rdfs:label xml:lang="en">legend folktale</rdfs:label>
    <skos:definition xml:lang="en">"Stories that have been maintained over time, usually by a particular culture through an oral tradition. Often understood within originating cultures as historical accounts although they differ from Western record-keeping."  <![CDATA[<a href="#cwrc:db2f8571-a773-4068-a35f-34262950bb8f">(Getty, 2017)</a>]]></skos:definition>
    <skos:altLabel xml:lang="en">folklore</skos:altLabel>
    <skos:related rdf:resource="http://id.loc.gov/authorities/genreForms/gf2014026344"/>
    <skos:definition xml:lang="fr">Histoires conservées au fil du temps, généralement transmise au sein d'une culture particulière par le biais de la tradition orale. Elles sont souvent interprétées comme des faits historiques dans les sociétés anciennes, même si elles diffèrent de la conception occidentale de l'Histoire.</skos:definition>
    <rdfs:label xml:lang="fr">légende conte folklorique</rdfs:label>
    <rdfs:comment xml:lang="en">Deprecated with no current equivalence. This term was split into two terms: @@#legend@@ and @@#folkTale@@.</rdfs:comment>
    <owl:deprecated rdf:datatype="http://www.w3.org/2001/XMLSchema#boolean">true</owl:deprecated>
    <vs:term_status xml:lang="en">deprecated</vs:term_status>
  </genre:FictionalGenre>

</rdf:RDF>
