<?xml version="1.0" encoding="UTF-8"?>
<rdf:RDF xml:base="http://sparql.cwrc.ca/ontologies/genre#"
  xmlns="http://sparql.cwrc.ca/ontologies/genre#"
  xmlns:as="http://www.w3.org/ns/activitystreams#"
  xmlns:cc="http://creativecommons.org/ns#"
  xmlns:cwrc="http://sparql.cwrc.ca/ontologies/cwrc#"
  xmlns:dbpedia="http://dbpedia.org/resource/"
  xmlns:dcterms="http://purl.org/dc/terms/"
  xmlns:doap="http://usefulinc.com/ns/doap#"
  xmlns:eurovoc="http://eurovoc.europa.eu/"
  xmlns:foaf="http://xmlns.com/foaf/0.1/"
  xmlns:genre="http://sparql.cwrc.ca/ontologies/genre#"
  xmlns:geonames="http://sws.geonames.org/"
  xmlns:loc="http://id.loc.gov/vocabulary/relators/"
  xmlns:nif="http://persistence.uni-leipzig.org/nlp2rdf/ontologies/nif-core#"
  xmlns:oa="http://www.w3.org/ns/oa#"
  xmlns:owl="http://www.w3.org/2002/07/owl#"
  xmlns:prov="http://www.w3.org/ns/prov#"
  xmlns:rdf="http://www.w3.org/1999/02/22-rdf-syntax-ns#"
  xmlns:rdfs="http://www.w3.org/2000/01/rdf-schema#"
  xmlns:skos="http://www.w3.org/2004/02/skos/core#"
  xmlns:skosxl="http://www.w3.org/2008/05/skos-xl#"
  xmlns:time="http://www.w3.org/2006/time#"
  xmlns:vann="http://purl.org/vocab/vann/"
  xmlns:void="http://rdfs.org/ns/void#"
  xmlns:vs="http://www.w3.org/2003/06/sw-vocab-status/ns#"
  xmlns:xsd="http://www.w3.org/2001/XMLSchema#">
  <owl:Ontology rdf:about="">
    <rdf:type rdf:resource="http://purl.org/vocommons/voaf#Vocabulary"/>
    <vann:preferredNamespacePrefix>genre</vann:preferredNamespacePrefix>
    <vann:preferredNamespaceUri>http://sparql.cwrc.ca/ontologies/genre#</vann:preferredNamespaceUri>
    <dcterms:title xml:lang="en">The CWRC Literary Genre Ontology</dcterms:title>
    <rdfs:label xml:lang="en">The CWRC Literary Genre Ontology</rdfs:label>
    <foaf:name xml:lang="en">The CWRC Literary Genre Ontology</foaf:name>
    <dcterms:title xml:lang="fr">L'Ontologie des genres littéraires CWRC</dcterms:title>
    <rdfs:label xml:lang="fr">L'Ontologie des genres littéraires CWRC</rdfs:label>
    <foaf:name xml:lang="fr">L'Ontologie des genres littéraires CWRC</foaf:name>
    <dcterms:description xml:lang="en">The CWRC Literary Genre Ontology is the ontology used by the Canadian Writing Research Collaboratory to assign Literary Genres to different documents.</dcterms:description>
    <skos:definition xml:lang="en">The CWRC Literary Genre Ontology is the ontology used by the Canadian Writing Research Collaboratory to assign Literary Genres to different documents.</skos:definition>
    <rdfs:comment xml:lang="en">The CWRC Literary Genre Ontology is the ontology used by the Canadian Writing Research Collaboratory to assign Literary Genres to different documents.</rdfs:comment>
    <dcterms:description xml:lang="fr">L'Ontologie des genres littéraires CWRC est l'ontologie utilisée par le Collaboratoire scientifique des écrits du Canada pour assigner des genres à des écrits littéraires.</dcterms:description>
    <skos:definition xml:lang="fr">L'Ontologie des genres littéraires CWRC est l'ontologie utilisée par le Collaboratoire scientifique des écrits du Canada pour assigner des genres à des écrits littéraires.</skos:definition>
    <rdfs:comment xml:lang="fr">L'Ontologie des genres littéraires CWRC est l'ontologie utilisée par le Collaboratoire scientifique des écrits du Canada pour assigner des genres à des écrits littéraires.</rdfs:comment>
    <owl:versionInfo>0.3</owl:versionInfo>
    <owl:priorVersion rdf:resource="http://sparql.cwrc.ca/ontologies/genre-2018-08-31"/>
    <dcterms:date rdf:datatype="http://www.w3.org/2001/XMLSchema#date">ONTOLOGY_DATE</dcterms:date>
    <dcterms:rights rdf:resource="https://creativecommons.org/licenses/by/3.0/"/>
    <vs:term_status xml:lang="en">Testing</vs:term_status>
    <dcterms:creator>
      <cwrc:NaturalPerson rdf:about="#AbigelLemak">
        <foaf:name>Abigel Lemak</foaf:name>
      </cwrc:NaturalPerson>
    </dcterms:creator>
    <dcterms:creator>
      <cwrc:NaturalPerson rdf:about="#JadePenancier">
        <foaf:name>Jade Penancier</foaf:name>
      </cwrc:NaturalPerson>
    </dcterms:creator>
    <dcterms:creator>
      <cwrc:NaturalPerson rdf:about="#KimMartin">
        <foaf:name>Kim Martin</foaf:name>
      </cwrc:NaturalPerson>
    </dcterms:creator>
    <dcterms:creator>
      <cwrc:NaturalPerson rdf:about="#MicaelaJimenez">
        <foaf:name>Micaela Jimenez</foaf:name>
      </cwrc:NaturalPerson>
    </dcterms:creator>
    <dcterms:creator rdf:resource="#SusanBrown"/>
    <dcterms:creator>
      <cwrc:NaturalPerson rdf:about="#RobWarren">
        <foaf:name>Robert Warren</foaf:name>
        <owl:sameAs rdf:resource="http://rdf.muninn-project.org/ww1/2011/11/11/Person/Warren"/>
        <foaf:homepage rdf:resource="http://www.dbdump.org/"/>
      </cwrc:NaturalPerson>
    </dcterms:creator>
    <dcterms:creator>
      <cwrc:NaturalPerson rdf:about="#AlliyyaMo">
        <foaf:name>Alliyya Mo</foaf:name>
      </cwrc:NaturalPerson>
    </dcterms:creator>
    <dcterms:creator>
      <cwrc:NaturalPerson rdf:about="#JasmineDrudgeWillson">
        <foaf:name>Jasmine Drudge-Willson</foaf:name>
      </cwrc:NaturalPerson>
    </dcterms:creator>
    <dcterms:creator>
      <cwrc:NaturalPerson rdf:about="#JoelCummings">
        <foaf:name>Joel Cummings</foaf:name>
      </cwrc:NaturalPerson>
    </dcterms:creator>
    <dcterms:creator>
      <cwrc:NaturalPerson rdf:about="#DebStacey">
        <foaf:name>Deborah Stacey</foaf:name>
        <foaf:homepage rdf:resource="http://ontology.socs.uoguelph.ca/"/>
      </cwrc:NaturalPerson>
    </dcterms:creator>
    <dcterms:publisher>
      <foaf:Organization rdf:about="#cwrc">
        <foaf:name xml:lang="fr">Le Collaboratoire scientifique des écrits du Canada</foaf:name>
        <foaf:name xml:lang="en">The Canadian Writing Research Collaboratory</foaf:name>
        <foaf:logo rdf:resource="http://sparql.cwrc.ca/images/CWRCLogo-Horz-FullColour.png"/>
      </foaf:Organization>
    </dcterms:publisher>
    <loc:pdr>
      <cwrc:NaturalPerson rdf:about="#SusanBrown">
        <foaf:name>Susan Brown</foaf:name>
        <owl:sameAs rdf:resource="http://orcid.org/0000-0002-0267-7344"/>
        <foaf:homepage rdf:resource="http://www.uoguelph.ca/~sbrown/"/>
      </cwrc:NaturalPerson>
    </loc:pdr>
    <loc:fnd>
      <foaf:Organization rdf:about="#sshrc">
        <foaf:name xml:lang="en">Social Sciences and Humanities Research Council</foaf:name>
        <foaf:name xml:lang="fr">Conseil de recherches en sciences humaines</foaf:name>
        <foaf:nick>SSHRC</foaf:nick>
      </foaf:Organization>
    </loc:fnd>
    <void:inDataset rdf:resource="#datasetdefinition"/>
    <foaf:logo rdf:resource="http://sparql.cwrc.ca/images/CWRCLogo-Horz-FullColour.png"/>
    <dcterms:subject rdf:resource="http://id.loc.gov/authorities/subjects/sh85077490"/>
  </owl:Ontology>
  <void:Dataset rdf:about="#datasetdefinition">
    <dcterms:title xml:lang="en">The CWRC Literary Genre Ontology</dcterms:title>
    <rdfs:label xml:lang="en">The CWRC Literary Genre Ontology</rdfs:label>
    <foaf:name xml:lang="en">The CWRC Literary Genre Ontology</foaf:name>
    <dcterms:title xml:lang="fr">L'Ontologie des genres littéraires CWRC</dcterms:title>
    <rdfs:label xml:lang="fr">L'Ontologie des genres littéraires CWRC</rdfs:label>
    <foaf:name xml:lang="fr">L'Ontologie des genres littéraires CWRC</foaf:name>
    <dcterms:description xml:lang="en">The CWRC Literary Genre Ontology is the ontology used by the Canadian Writing Research Collaboratory to assign Literary Genres to different documents.</dcterms:description>
    <skos:definition xml:lang="en">The CWRC Literary Genre Ontology is the ontology used by the Canadian Writing Research Collaboratory to assign Literary Genres to different documents.</skos:definition>
    <rdfs:comment xml:lang="en">The CWRC Literary Genre Ontology is the ontology used by the Canadian Writing Research Collaboratory to assign Literary Genres to different documents.</rdfs:comment>
    <dcterms:description xml:lang="fr">L'Ontologie des genres littéraires CWRC est l'ontologie utilisée par le Collaboratoire scientifique des écrits du Canada pour assigner des genres à des écrits littéraires.</dcterms:description>
    <skos:definition xml:lang="fr">L'Ontologie des genres littéraires CWRC est l'ontologie utilisée par le Collaboratoire scientifique des écrits du Canada pour assigner des genres à des écrits littéraires.</skos:definition>
    <rdfs:comment xml:lang="fr">L'Ontologie des genres littéraires CWRC est l'ontologie utilisée par le Collaboratoire scientifique des écrits du Canada pour assigner des genres à des écrits littéraires.</rdfs:comment>
    <cc:license rdf:resource="https://creativecommons.org/licenses/by/3.0/"/>
    <cc:Jurisdiction rdf:resource="http://dbpedia.org/resource/Canada"/>
    <cc:attributionURL rdf:resource="http://www.cwrc.ca/"/>
    <dcterms:publisher rdf:resource="#cwrc"/>
    <dcterms:creator rdf:resource="#MicaelaJimenez"/>
    <dcterms:creator rdf:resource="#RobWarren"/>
    <dcterms:creator rdf:resource="#JadePenancier"/>
    <dcterms:creator rdf:resource="#AlliyyaMo"/>
    <dcterms:creator rdf:resource="#DebStacey"/>
    <dcterms:creator rdf:resource="#JoelCummings"/>
    <dcterms:creator rdf:resource="#SusanBrown"/>
    <loc:pdr rdf:resource="#SusanBrown"/>
    <loc:fnd rdf:resource="#sshrc"/>
    <rdfs:isDefinedBy rdf:resource="http://sparql.cwrc.ca/ontologies/genre-ONTOLOGY_DATE"/>
    <foaf:logo rdf:resource="http://www.cwrc.ca/wp-content/uploads/2010/11/CWRC_logo_v074.gif"/>
    <dcterms:subject rdf:resource="http://id.loc.gov/authorities/subjects/sh85077490"/>
    <void:triples>TOTAL_TRIPLES_CWRC_ONTOLOGY</void:triples>
    <void:entities>TOTAL_ENTITIES_CWRC_ONTOLOGY</void:entities>
  </void:Dataset>
  <skos:Concept rdf:about="#originalOrlandoAuthor">
    <rdfs:label xml:lang="en">Members of the Orlando Project</rdfs:label>
    <rdfs:label xml:lang="fr">Les membres du projet Orlando</rdfs:label>
    <rdf:type rdf:resource="http://xmlns.com/foaf/0.1/Group"/>
    <foaf:name xml:lang="en">Members of the Orlando Project.</foaf:name>
    <foaf:homepage rdf:resource="http://orlando.cambridge.org/public/svDocumentation?formname=t&amp;d_id=CREDITSANDACKNOWLEDGEMENTS"/>
    <skos:definition xml:lang="en">The collection of all persons having written entries for The Orlando Project.</skos:definition>
    <skos:definition xml:lang="fr">La collection de tous les auteurs du Projet Orlando.</skos:definition>
    <rdfs:isDefinedBy rdf:resource="http://sparql.cwrc.ca/ontologies/genre-ONTOLOGY_DATE"/>
    <void:inDataset rdf:resource="#datasetdefinition"/>
  </skos:Concept>
  <owl:ObjectProperty rdf:ID="hasGenre">
    <rdfs:label xml:lang="en">has genre</rdfs:label>
    <rdfs:label xml:lang="fr">a un genre</rdfs:label>
    <skos:definition xml:lang="en">The cultural work in question is classified by this genre. A single work may be classified as belonging to multiple genres, which may overlap or even seem to be contradictory, such as @@#verseNovel@@s also classified as @@#poetry@@ and @@#fiction@@.</skos:definition>
    <skos:definition xml:lang="fr">Décrit le genre d'une personne. De même que pour les autres formes culturelles, une même personne peut cumuler plus d'une propriété ou description de ce type. Pour plus d'informations sur cette propriété, voir @@#Genre@@.</skos:definition>
    <rdfs:range rdf:resource="#Genre"/>
    <rdfs:isDefinedBy rdf:resource="http://sparql.cwrc.ca/ontologies/genre-ONTOLOGY_DATE"/>
    <void:inDataset rdf:resource="#datasetdefinition"/>
  </owl:ObjectProperty>
  <owl:ObjectProperty rdf:ID="genreOf">
    <rdfs:label xml:lang="en">genre of</rdfs:label>
    <rdfs:label xml:lang="fr">genre de</rdfs:label>
    <rdfs:domain rdf:resource="#Genre"/>
    <owl:inverseOf rdf:resource="#hasGenre"/>
    <rdfs:isDefinedBy rdf:resource="http://sparql.cwrc.ca/ontologies/genre-ONTOLOGY_DATE"/>
    <void:inDataset rdf:resource="#datasetdefinition"/>
  </owl:ObjectProperty>
  <void:Dataset rdf:about="#datasetdefinition">
    <dcterms:title xml:lang="en">The CWRC Ontology</dcterms:title>
    <rdfs:label xml:lang="en">The CWRC Ontology</rdfs:label>
    <foaf:name xml:lang="en">The CWRC Ontology</foaf:name>
    <dcterms:title xml:lang="fr">L'Ontologie CWRC</dcterms:title>
    <rdfs:label xml:lang="fr">L'Ontologie CWRC</rdfs:label>
    <foaf:name xml:lang="fr">L'Ontologie CWRC</foaf:name>
    <dcterms:description xml:lang="en">The CWRC Ontology is the ontology of the Canadian Writing Research Collaboratory.</dcterms:description>
    <skos:definition xml:lang="en">The CWRC Ontology is the ontology of the Canadian Writing Research Collaboratory.</skos:definition>
    <rdfs:comment xml:lang="en">The CWRC Ontology is the ontology of the Canadian Writing Research Collaboratory.</rdfs:comment>
    <dcterms:description xml:lang="fr">L'Ontologie CWRC est l'ontologie du Collaboratoire scientifique des écrits du Canada.</dcterms:description>
    <skos:definition xml:lang="fr">L'Ontologie CWRC est l'ontologie du Collaboratoire scientifique des écrits du Canada.</skos:definition>
    <rdfs:comment xml:lang="fr">L'Ontologie CWRC est l'ontologie du Collaboratoire scientifique des écrits du Canada.</rdfs:comment>
    <!-- -->
    <cc:license rdf:resource="https://creativecommons.org/licenses/by/3.0/"/>
    <cc:Jurisdiction rdf:resource="http://dbpedia.org/resource/Canada"/>
    <cc:attributionURL rdf:resource="http://www.cwrc.ca/"/>
    <dcterms:publisher rdf:resource="#cwrc"/>
    <dcterms:creator rdf:resource="#SusanBrown"/>
    <dcterms:creator rdf:resource="#JoelCummings"/>
    <dcterms:creator rdf:resource="#MicaelaJimenez"/>
    <dcterms:creator rdf:resource="#AbigelLemak"/>
    <dcterms:creator rdf:resource="#KimMartin"/>
    <dcterms:creator rdf:resource="#AlliyyaMo"/>
    <dcterms:creator rdf:resource="#JadePenancier"/>
    <dcterms:creator rdf:resource="#DebStacey"/>
    <dcterms:creator rdf:resource="#RobWarren"/>
    <loc:ctb rdf:resource="#ConstanceCrompton"/>
    <loc:ctb rdf:resource="#originalOrlandoAuthor"/>
    <loc:pdr rdf:resource="#SusanBrown"/>
    <loc:fnd rdf:resource="#sshrc"/>
    <rdfs:isDefinedBy rdf:resource="http://sparql.cwrc.ca/ontologies/genre-ONTOLOGY_DATE"/>
    <foaf:logo rdf:resource="http://www.cwrc.ca/wp-content/uploads/2010/11/CWRC_logo_v074.gif"/>
    <dcterms:subject rdf:resource="http://id.loc.gov/authorities/subjects/sh85019388"/>
    <dcterms:subject rdf:resource="http://id.loc.gov/authorities/subjects/sh85043777"/>
    <dcterms:subject rdf:resource="http://id.loc.gov/authorities/subjects/sh85013838"/>
    <dcterms:subject rdf:resource="http://id.loc.gov/authorities/subjects/sh85077519"/>
    <dcterms:subject rdf:resource="http://id.loc.gov/authorities/subjects/sh2009007122"/>
    <void:triples>TOTAL_TRIPLES_CWRC_ONTOLOGY</void:triples>
    <void:entities>TOTAL_ENTITIES_CWRC_ONTOLOGY</void:entities>
  </void:Dataset>
  <genre:ReferenceWorkGenre rdf:about="http://sparql.cwrc.ca/ontologies/genre#dictionary">
    <rdfs:label xml:lang="fr">dictionnaire</rdfs:label>
    <skos:definition xml:lang="en">"Reference sources containing alphabetical lists of words with information given for each word; generally including meanings, pronunciation, etymology, and often usage guidance." <![CDATA[(<a href="#cwrc:db2f8571-a773-4068-a35f-34262950bb8f">Getty, 2017</a>)]]></skos:definition>
    <skos:definition xml:lang="fr">"Sources de références, contenant des listes alphabétiques dans lesquelles chaque mot est associé à des informations données. Elles incluent généralement les différentes significations, la prononciation, l'étymologie et des conseils sur l'usage des mots. "</skos:definition>
    <rdfs:label xml:lang="en">dictionary</rdfs:label>
    <owl:sameAs rdf:resource="http://vocab.getty.edu/aat/300026186"/>
    <owl:sameAs rdf:resource="http://id.loc.gov/authorities/genreForms/gf2014026086"/>
    <rdfs:comment xml:lang="en">The description for this term is indebted to the Getty Art &amp; Architecture Thesaurus.</rdfs:comment>
  </genre:ReferenceWorkGenre>
  <genre:PoeticGenre rdf:about="http://sparql.cwrc.ca/ontologies/genre#lyric">
    <rdfs:label xml:lang="fr">lyrique</rdfs:label>
    <skos:definition xml:lang="fr">Terme dérivé de la lyre, instrument de musique symbole du pouvoir de la poésie remontant au mythe d'Orphée dans l'Antiquité. L'adjectif "lyrique" apparaît en France au XVIe siècle, mais devient de plus en plus utilisé au XIXe pour décrire le romantisme. Il réfère souvent à un type de poésie particulièrement centrée sur la subjectivité du poète et l'expression de ses sentiments. Toutefois, il n'est pas réductible à cet aspect, et peut être résumé en trois concepts majeurs: subjectivité, chant et idéalité. Dans la critique littéraire, le lyrique est un registre qui peut aussi être étudié dans d'autres formes littéraires, comme le roman.</skos:definition>
    <owl:sameAs rdf:resource="http://www.universalis.fr/encyclopedie/lyrisme/"/>
    <rdfs:label xml:lang="en">lyric</rdfs:label>
    <owl:sameAs rdf:resource="http://id.loc.gov/authorities/genreForms/gf2014026422"/>
    <skos:definition xml:lang="en">"Lyric Essay is a subgenre of essay writing, which combines qualities of poetry, essay, memoir, and research writing. The lyric essay is considered high art, and often requires work and association on behalf of the reader. Proponents of the lyric essay classification insist it differs from prose poetry in its reliance on association rather than line breaks and juxtaposition." <![CDATA[(<a href="#cwrc:727d97bc-af78-4122-94be-aa78b2e97d5a">DBpedia, 2017</a>)]]></skos:definition>
    <rdfs:comment xml:lang="en">The description for this term is indebted to DBpedia. </rdfs:comment>
  </genre:PoeticGenre>
  <genre:ChildrensLiteratureGenre rdf:about="http://sparql.cwrc.ca/ontologies/genre#childrensLiterature">
    <skos:definition xml:lang="en">"Literature written and published for children." <![CDATA[(<a href="#cwrc:db2f8571-a773-4068-a35f-34262950bb8f">Getty, 2017</a>)]]></skos:definition>
    <owl:sameAs rdf:resource="http://vocab.getty.edu/aat/300263209"/>
    <rdfs:label xml:lang="fr">littérature de jeunesse</rdfs:label>
    <skos:definition xml:lang="fr">"Littérature écrite et publiée pour les enfants."</skos:definition>
    <rdfs:comment xml:lang="en">The description for this term is indebted to the Getty Art &amp; Architecture Thesaurus.</rdfs:comment>
    <rdfs:label xml:lang="en">childrens literature</rdfs:label>
  </genre:ChildrensLiteratureGenre>
  <genre:ThematicWritingGenre rdf:about="http://sparql.cwrc.ca/ontologies/genre#regional">
    <rdfs:label xml:lang="fr">littérature régionale</rdfs:label>
    <skos:definition xml:lang="fr">La littérature régionale au sens strict se rattache aux conventions du réalisme parce qu'elle tente de distinguer avec précision les caractéristiques d'une région clairement définissable, soit une région rurale ou encore étroitement liée à la terre. Comme le montrent les oeuvres de Thomas Hardy, de William Faulkner, de Sara Jeannette Duncan, et de Margaret Laurence de ce type de littérature régionale, dans sa forme la plus accomplie, n'est pas synonyme de détails superficiels ou de style prosaïque mais plutôt d'une exploration profonde de l'influence qu'exercent des régions particulières dans le destin d'individus précis.</skos:definition>
    <rdfs:comment xml:lang="en">Encyclopédie du Canada</rdfs:comment>
    <skos:definition xml:lang="en">Regional writing reflects the details of a specific region, whether in prose or poetry. Regionalism is often associated with rural areas and "local colour", and often allied with realism insofar as it seeks to distinguish one region clearly from others. At its best, as when practiced by Thomas Hardy, William Faulkner, Sara Jeannette Duncan, or Margaret Laurence, regionalism conveys not merely the superficialities or prosaic details of an area but a profound sense of the impact of place on individual characters and destinies.</skos:definition>
    <rdfs:label xml:lang="en">regional</rdfs:label>
    <dcterms:references rdf:resource="http://www.encyclopediecanadienne.ca/fr/article/regionalisme-dans-la-litterature/"/>
  </genre:ThematicWritingGenre>
  <genre:InformationalGenre rdf:about="http://sparql.cwrc.ca/ontologies/genre#chronology">
    <owl:sameAs rdf:resource="http://id.loc.gov/authorities/genreForms/gf2014026062"/>
    <owl:sameAs rdf:resource="http://vocab.getty.edu/page/aat/300252008"/>
    <rdfs:comment xml:lang="en">The description for this term is indebted to the Getty Art &amp; Architecture Thesaurus.</rdfs:comment>
    <skos:definition xml:lang="en">"Tables, lists, or treatises listing events, biographies, milestones, or other items in serial temporal order relative to given dates or time periods." <![CDATA[(<a href="#cwrc:db2f8571-a773-4068-a35f-34262950bb8f">Getty, 2017</a>)]]></skos:definition>
    <rdfs:label xml:lang="en">chronology</rdfs:label>
  </genre:InformationalGenre>
  <genre:FeministGenre rdf:about="http://sparql.cwrc.ca/ontologies/genre#feminist">
    <skos:definition xml:lang="fr">Textes qui peuvent être considérés comme féministes dans la mesure où ils abordent de façon critique et consciente les inégalités entre hommes et femmes, ou parmi les individus d'identités genrées diverses. Un texte, fictif ou non, entre généralement dans cette catégorie s'il reflète des théories féministes ou est engagé dans des mouvements politiques féministes. Les aspects féministes d'un texte peuvent être explicites ou implicites, et sont fortement sujets à débat étant donné la grande pluralité de type de féminisme.</skos:definition>
    <rdf:type rdf:resource="http://sparql.cwrc.ca/ontologies/genre#PoliticalWritingGenre"/>
    <rdfs:label xml:lang="fr">féministe</rdfs:label>
    <skos:definition xml:lang="en">"Writing concerned with the unique experience of being a woman or alternatively writing designed to challenge existing preconceptions of gender. Examples of feminist writings include Christine de Pisan's medieval work, The City of Ladies; Aemilia Lanyer's Renaissance treatise, Salve Deus, Rex Judaeorum (which presented the then-shocking idea that Adam was just as much to blame for the fall of man as Eve was in the Genesis account); Mary Wollstonecraft's Vindication, and Susan B. Anthony's nineteenth-century essays (which presented the equally shocking idea that women in America and Canada should have the right to vote). Many female students in my class preface their discussions of feminist writings by stating, "I'm not a feminist, but ..." This tendency always puzzled me, since it implies that feminism is something negative, radical, or always liberal. Worse yet, it implies that it's bad for women to want crazy, misguided things like education, equal health insurance, similar pay to what men earn in similar professions, freedom from harassment, and funding for medical problems concerning women, such as breast and uterine cancer research, which are the primary concerns of feminism. Somewhere toward the end of the twentieth-century, detractors of such writers have caricatured these demands as "man-hating" or "anti-family." As an antidote to such thinking, keep in mind the broader definition: a feminist is anyone who thinks that women are people too." <![CDATA[(<a href="cwrc:509015ff-7641-473e-94c5-688e06952bb7">L. K Wheeler, 2017</a>)]]></skos:definition>
    <rdfs:label xml:lang="en">feminist</rdfs:label>
    <rdf:type rdf:resource="http://sparql.cwrc.ca/ontologies/genre#ThematicWritingGenre"/>
    <rdfs:comment xml:lang="en">The description for this term is indebted to Dr. L. Kip Wheeler of Carson-Newman University. </rdfs:comment>
    <dcterms:references rdf:resource="http://web.cn.edu/kwheeler/lit_terms_f.html"/>
  </genre:FeministGenre>
  <genre:InformationalGenre rdf:about="http://sparql.cwrc.ca/ontologies/genre#obituary">
    <rdfs:label xml:lang="en">obituary</rdfs:label>
    <skos:definition xml:lang="fr">«L’élégie (en grec ancien ἐλεγεία / elegeía, signifiant « chant de mort ») fut une forme de poème dans l'Antiquité, avant de devenir un genre poétique à partir de la Renaissance. Dans l’Antiquité, était appelé « élégie » tout poème alternant hexamètres et pentamètres en distiques : ce sont les vers élégiaques. De nos jours, l’élégie est considérée comme un genre au sein de la poésie lyrique, en tant que poème de longueur et de forme variables caractérisé par son ton plaintif particulièrement adapté à l’évocation d’un mort ou à l’expression d’une souffrance amoureuse due à un abandon ou à une absence.» <![CDATA[(<a href="#cwrc:727d97bc-af78-4122-94be-aa78b2e97d5a">DBpedia, 2017</a>)]]></skos:definition>
    <skos:definition xml:lang="en">"An obituary (obit for short) is a news article that reports the recent death of a person, typically along with an account of the person's life and information about the upcoming funeral." <![CDATA[(<a href="#cwrc:727d97bc-af78-4122-94be-aa78b2e97d5a">DBpedia, 2018</a>)]]></skos:definition>
    <rdfs:comment xml:lang="en">The description for this term is indebted to DBpedia. </rdfs:comment>
    <owl:sameAs rdf:resource="http://dbpedia.org/page/Obituary"/>
    <rdfs:label xml:lang="fr">élégie</rdfs:label>
    <owl:sameAs rdf:resource="http://id.loc.gov/authorities/genreForms/gf2014026134"/>
  </genre:InformationalGenre>
  <genre:ReligiousGenre rdf:about="http://sparql.cwrc.ca/ontologies/genre#devotional">
    <rdfs:label xml:lang="en">devotional</rdfs:label>
    <owl:sameAs rdf:resource="http://dbpedia.org/resource/Christian_devotional_literature"/>
    <skos:definition xml:lang="fr">La littérature de dévotion chrétienne est une écriture religieuse qui n'est ni doctrinale ni théologique, mais conçue pour les individus à lire pour leur édification personnelle et leur formation spirituelle. Le théologien Karl Holl a suggéré que la littérature de dévotion s'est définitivement développée au moment du piétisme pendant la seconde moitié du 17ème siècle.</skos:definition>
    <rdfs:comment xml:lang="en">The description for this term is indebted to DBpedia. </rdfs:comment>
    <owl:sameAs rdf:resource="http://id.loc.gov/authorities/genreForms/gf2015026057"/>
    <rdfs:label xml:lang="fr">littérature de dévotion</rdfs:label>
    <skos:definition xml:lang="en">"Christian devotional literature (also called devotionals or Christian living literature) is religious writing that is neither doctrinal nor theological, but designed for individuals to read for their personal edification and spiritual formation. Theologian Karl Holl has suggested that devotional literature came into full development at the time of Pietism during the second half of the 17th century." <![CDATA[(<a href="#cwrc:727d97bc-af78-4122-94be-aa78b2e97d5a">DBpedia, 2017</a>)]]></skos:definition>
  </genre:ReligiousGenre>
  <genre:SatiricalGenre rdf:about="http://sparql.cwrc.ca/ontologies/genre#lampoon">
    <skos:definition xml:lang="fr">«Un libelle est un petit livre de caractère satirique, insultant ou diffamatoire.» <![CDATA[(<a href="#cwrc:727d97bc-af78-4122-94be-aa78b2e97d5a">DBpedia, 2017</a>)]]></skos:definition>
    <rdfs:comment xml:lang="en">The description for this term is indebted to Dr. L. Kip Wheeler of Carson-Newman University. </rdfs:comment>
    <dcterms:references rdf:resource="http://web.cn.edu/kwheeler/lit_terms_l.html"/>
    <rdfs:label xml:lang="fr">libelle</rdfs:label>
    <rdfs:label xml:lang="en">lampoon</rdfs:label>
    <skos:definition xml:lang="en">"A coarse or crude satire ridiculing the appearance or character of another person." <![CDATA[(<a href="cwrc:509015ff-7641-473e-94c5-688e06952bb7">L. K Wheeler, 2017</a>)]]></skos:definition>
  </genre:SatiricalGenre>
  <genre:DramaticGenre rdf:about="http://sparql.cwrc.ca/ontologies/genre#theatreOfCruelty">
    <rdfs:label xml:lang="fr">théâtre de la cruauté</rdfs:label>
    <owl:sameAs rdf:resource="http://dbpedia.org/resource/Theatre_of_Cruelty"/>
    <skos:definition xml:lang="en">"The Theatre of Cruelty (French: Théâtre de la Cruauté) is a form of theatre developed by avant-garde playwright, actor, essayist, and theorist, Antonin Artaud, in The Theatre and its Double. Originally a member of the surrealist movement, Artaud eventually began to develop his own theatrical theories. The Theatre of Cruelty can be seen as break with traditional Western theatre, and a means by which artists assault the senses of the audience, and allow them to feel the unexpressed emotions of the subconscious. While Artaud was only able to produce one play in his lifetime that reflected the tenets of the Theatre of Cruelty, the works of many theatre artists reflect his theories." <![CDATA[(<a href="#cwrc:727d97bc-af78-4122-94be-aa78b2e97d5a">DBpedia, 2017</a>)]]></skos:definition>
    <skos:definition xml:lang="fr">«Le théâtre de la cruauté est une expression introduite par Antonin Artaud pour désigner la forme dramatique à laquelle il travailla dans son essai Le Théâtre et son double. Derrière « cruauté » il faut entendre « souffrance d'exister ». L'acteur doit brûler les planches comme un supplicié sur son bûcher. Selon Artaud, le théâtre doit retrouver sa dimension sacrée, métaphysique et porter le spectateur jusqu'à la transe.» <![CDATA[(<a href="#cwrc:727d97bc-af78-4122-94be-aa78b2e97d5a">DBpedia, 2017</a>)]]></skos:definition>
    <rdfs:label xml:lang="en">theatre of cruelty</rdfs:label>
    <rdfs:comment xml:lang="en">This term and its description were created from data gathered from DBpedia.</rdfs:comment>
  </genre:DramaticGenre>
  <genre:BookForm rdf:about="http://sparql.cwrc.ca/ontologies/genre#artistsBook">
    <rdfs:label xml:lang="en">artist's book</rdfs:label>
    <skos:related rdf:resource="http://vocab.getty.edu/aat/300123016"/>
  </genre:BookForm>
  <genre:ComedicGenre rdf:about="http://sparql.cwrc.ca/ontologies/genre#riddle">
    <rdfs:comment xml:lang="en">The description for this term is indebted to Dr. L. Kip Wheeler of Carson-Newman University. </rdfs:comment>
    <skos:definition xml:lang="en">"(from Old English roedel, from roedan meaning "to give council" or "to read"): A universal form of literature in which a puzzling question or a conundrum is presented to the reader. The reader is often challenged to solve this enigma, which requires ingenuity in discovering the hidden meaning. A riddle may involve puns, symbolism, synecdoche, personification (especially prosopopoeia), or unusual imagery. For instance, a Norse riddle asks, "Tell me what I am. Thirty white horses round a red hill. First they champ. Then they stamp. Now they stand still." The answer is the speaker's teeth; these thirty white horses circle the "red hill" of the tongue; they champ and stamp while the riddler speaks, but stand still at the end of his riddle. Another famous example is the riddle of the sphinx from Sophocles' Oedipus Trilogy. The sphinx asks Oedipus, "What goes on four feet, on two feet, and then three. But the more feet it goes on, the weaker is he?" The answer is a human being, which crawls as an infant, walks erect on two feet as an adult, and totters on a staff (the third leg) in old age. The earliest known English riddles are recorded in the Exeter Book, and they probably date back to the 8th century. Examples, however, can be found in Greek, Sanskrit, Hebrew, Arabic, Persian, and Chinese, and many other languages. Authors of Anglo-Latin riddles include Aldhelm of Sherborne, Archbishop Tatwine of Canterbury, and Abbot Eusebius of Wearmouth. A large Renaissance collection can also be found in Nicolas Reusner's Aenigmatographia (1602)." <![CDATA[(<a href="cwrc:509015ff-7641-473e-94c5-688e06952bb7">L. K Wheeler, 2017</a>)]]></skos:definition>
    <rdfs:label xml:lang="fr">éngime</rdfs:label>
    <rdfs:label xml:lang="en">riddle</rdfs:label>
    <owl:sameAs rdf:resource="https://dvlf.uchicago.edu/mot/%C3%A9nigme"/>
    <skos:definition xml:lang="fr">Jeu d'esprit mettant à l'épreuve la sagacité de l'interlocuteur qui doit trouver la réponse à une interrogation dont le sens est caché sous une parabole ou une métaphore.</skos:definition>
  </genre:ComedicGenre>
  <genre:ThematicWritingGenre rdf:about="http://sparql.cwrc.ca/ontologies/genre#gothic">
    <rdfs:comment xml:lang="en">The description for this term is indebted to the Getty Art &amp; Architecture Thesaurus.</rdfs:comment>
    <owl:sameAs rdf:resource="http://vocab.getty.edu/aat/300266777"/>
    <owl:sameAs rdf:resource="http://id.loc.gov/authorities/genreForms/gf2014026360"/>
    <skos:definition xml:lang="fr">Fictions romantiques dont l'atmosphère est mystérieuse et angoissante, racontant souvent une histoire d'amour. Le genre a été introduit en Angleterre aux alentours de 1765, mais s'est aussitôt popularisé ailleurs en Europe, atteignant son apogée dans les années 1790. Le genre a connu de nombreux renouvellements au cours des siècles suivants. Le genre est ainsi nommé car les premiers exemples de romans gothiques se déroulaients souvent partiellement au sein de bâtiments médiévaux et de ruines, comme les châteaux ou les monastères.</skos:definition>
    <rdfs:label xml:lang="fr">gothique</rdfs:label>
    <skos:definition xml:lang="en">"Romantic fictions having a prevailing atmosphere of mystery and terror, often combined with a love story. The genre was introduced in England ca. 1765, but soon became popular elsewhere in Europe, reaching its heyday in the 1790s. The genre has undergone frequent revivals in subsequent centuries. It is called "Gothic" because the early examples were often set in part among medieval buildings and ruins, such as castles or monasteries." <![CDATA[(<a href="#cwrc:db2f8571-a773-4068-a35f-34262950bb8f">Getty, 2017</a>)]]></skos:definition>
    <rdfs:label xml:lang="en">gothic</rdfs:label>
  </genre:ThematicWritingGenre>
  <genre:NarrativeGenre rdf:about="http://sparql.cwrc.ca/ontologies/genre#fable">
    <rdfs:comment xml:lang="en">The description for this term is indebted to the Getty Art &amp; Architecture Thesaurus.</rdfs:comment>
    <skos:definition xml:lang="en">"A brief story illustrating human tendencies through animal characters. Unlike the parables, fables often include talking animals or animated objects as the principal characters. The interaction of these animals or objects reveals general truths about human nature, i.e., a person can learn practical lessons from the fictional antics in a fable. However, unlike a parable, the lesson learned is not necessarily allegorical. Each animal is not necessarily a symbol for something else. Instead, the reader learns the lesson as an exemplum--an example of what one should or should not do. The sixth century (BCE) Greek writer Aesop is most credited as an author of fables, but Phaedrus and Babrius in the first century (CE) expanded on his works to produce the tales we know today. A famous collection of Indian fables was the Sanskrit Bidpai (circa 300 CE), and in the medieval period, Marie de France (c. 1200 CE) composed 102 fables in verse. After the 1600s, fables increasingly became common as a form of children's literature. See also allegory, beast fable, and parable. Click here for a PDF handout discussing the difference between fables and parables." <![CDATA[(<a href="cwrc:509015ff-7641-473e-94c5-688e06952bb7">L. K Wheeler, 2017</a>)]]></skos:definition>
    <dcterms:references rdf:resource="http://web.cn.edu/kwheeler/lit_terms_f.html"/>
    <skos:definition xml:lang="fr">Récits fictifs habituellement avec des animaux ou des objets inanimés comme protagonistes, destinés à véhiculer une signification cachée concernant la conduite humaine.</skos:definition>
    <rdfs:label xml:lang="fr">fable</rdfs:label>
    <rdfs:label xml:lang="en">fable</rdfs:label>
  </genre:NarrativeGenre>
  <genre:ThematicWritingGenre rdf:about="http://sparql.cwrc.ca/ontologies/genre#erotica">
    <rdfs:label xml:lang="en">erotica</rdfs:label>
  </genre:ThematicWritingGenre>
  <genre:PrintMedium rdf:about="http://sparql.cwrc.ca/ontologies/genre#broadside">
    <rdfs:comment xml:lang="en">This term and its description were created from data gathered from the Oxford Dictionary of Literary Terms, 4th ed.</rdfs:comment>
    <rdfs:label xml:lang="en">broadside</rdfs:label>
    <rdfs:label xml:lang="fr">broadside</rdfs:label>
    <dcterms:references rdf:resource="http://www.oxfordreference.com/view/10.1093/acref/9780199208272.001.0001/acref-9780199208272-e-149?rskey=LdAUjx%26result=141"/>
    <skos:definition xml:lang="en">"Large sheets of paper with a poem or song, especially a ballad, printed on only one side." <![CDATA[(<a href="#cwrc:4c227091-6bf0-4325-b846-9733fae19e61">Oxford, 2015</a>)]]></skos:definition>
    <skos:definition xml:lang="fr">Grandes affiches contenant un poème ou une chanson, plus particulièrement une ballade, imprimée d'un seul côté.</skos:definition>
    <owl:sameAs rdf:resource="http://id.loc.gov/authorities/genreForms/gf2014026152"/>
  </genre:PrintMedium>
  <genre:PoliticalWritingGenre rdf:about="http://sparql.cwrc.ca/ontologies/genre#proletarianWriting">
    <skos:definition xml:lang="en">Writing by members of the working-classes or poor, including that by those who consider themselves members of the proletariat, and sometimes also writing produced to raise awareness of poor economic or labour conditions.</skos:definition>
    <rdfs:label xml:lang="fr">littérature prolétarienne</rdfs:label>
    <skos:definition xml:lang="fr">«La littérature prolétarienne est un courant littéraire qu'Henry Poulaille, fondateur du « Groupe des écrivains prolétariens de langue française », connu aussi sous le nom d'« école prolétarienne » (terme que Poulaille désapprouvait), fut le premier à définir et organiser en France dans les années 1930. Est défini comme auteur prolétarien tout auteur : * né de parents ouvriers ou paysans, * autodidacte (ayant quitté tôt l'école pour travailler, ou à la rigueur ayant bénéficié d'une bourse - en général pour devenir instituteur dans le système primaire, « l'école des pauvres », à l'époque où deux systèmes scolaires cohabitaient), * et qui témoigne dans ses écrits des conditions d'existence de sa classe sociale. La définition première précise aussi que l'auteur prolétarien doit continuer de gagner sa vie comme ouvrier ou comme paysan, mais plusieurs auteurs faisant exception à cette règle (à commencer par Poulaille lui-même qui a exercé divers métiers de 13 à 27 ans, mais s'est consacré ensuite à des activités moins « ouvrières » dans l'édition et le journalisme) sont cependant considérés comme auteurs prolétariens, du fait que leurs ouvrages et leur action restent orientés vers la défense du prolétariat et d'une expression littéraire spécifiquement ouvrière.» <![CDATA[(<a href="#cwrc:727d97bc-af78-4122-94be-aa78b2e97d5a">DBpedia, 2017</a>)]]></skos:definition>
    <skos:closeMatch rdf:resource="http://dbpedia.org/resource/Proletarian_literature"/>
    <rdfs:comment xml:lang="en">This term and its description were created from data gathered from DBpedia.</rdfs:comment>
    <rdfs:label xml:lang="en">proletarian writing</rdfs:label>
  </genre:PoliticalWritingGenre>
  <genre:DramaticGenre rdf:about="http://sparql.cwrc.ca/ontologies/genre#masque">
    <skos:definition xml:lang="en">"Not to be confused with a masquerade, a masque is a type of elaborate court entertainment popular in the times of Queen Elizabeth I, King James I, and Charles I--i.e., the early 17th Century after Queen Elizabeth's death. The masque as a performance grew out of medieval plays, but it was more spectacle than drama proper. The content was suitable for amateur actors rather than professional performers. The masques tended to use long speeches and little action. They combined poetic drama, singing, dancing, music, and splendid costumes and settings. The imagery was influential on later poets and poems, such as Andrew Marvell, who makes use of masque-imagery in "Upon Appleton House." <![CDATA[(<a href="cwrc:509015ff-7641-473e-94c5-688e06952bb7">L. K Wheeler, 2017</a>)]]></skos:definition>
    <rdfs:label xml:lang="fr">masque</rdfs:label>
    <rdfs:comment xml:lang="en">The description for this term is indebted to Dr. L. Kip Wheeler of Carson-Newman University. </rdfs:comment>
    <rdfs:label xml:lang="en">masque</rdfs:label>
    <owl:sameAs rdf:resource="http://dbpedia.org/resource/Masque"/>
    <owl:sameAs rdf:resource="http://id.loc.gov/authorities/genreForms/gf2014026428"/>
    <rdf:type rdf:resource="http://sparql.cwrc.ca/ontologies/genre#PerformanceMedium"/>
    <skos:definition xml:lang="fr">«Le masque (de l'anglais « masque ») est une forme de spectacle de cour qui fit son apparition en Angleterre sous le règne d'Elisabeth I (1558-1603).» <![CDATA[(<a href="#cwrc:727d97bc-af78-4122-94be-aa78b2e97d5a">DBpedia, 2017</a>)]]></skos:definition>
  </genre:DramaticGenre>
  <genre:DidacticGenre rdf:about="http://sparql.cwrc.ca/ontologies/genre#bestiary">
    <rdfs:label xml:lang="fr">bestiaire</rdfs:label>
    <rdfs:comment xml:lang="en">The description for this term is indebted to the Getty Art &amp; Architecture Thesaurus.</rdfs:comment>
    <owl:sameAs rdf:resource="http://vocab.getty.edu/aat/300201056"/>
    <rdfs:label xml:lang="en">bestiary</rdfs:label>
    <skos:definition xml:lang="fr">«Collections de fables à moral mettant en scène des animaux réels ou mythiques et principalement écrites au Moyen-Âge.» <![CDATA[(<a href="#cwrc:db2f8571-a773-4068-a35f-34262950bb8f">Getty, 2017</a>)]]></skos:definition>
    <skos:definition xml:lang="en">"Collections of moralized fables, especially as written in the Middle Ages, about actual or mythical animals." <![CDATA[(<a href="#cwrc:db2f8571-a773-4068-a35f-34262950bb8f">Getty, 2017</a>)]]></skos:definition>
  </genre:DidacticGenre>
  <genre:DigitalMedium rdf:about="http://sparql.cwrc.ca/ontologies/genre#multimedia">
    <skos:definition xml:lang="en">"Contemporary works of art that employ several distinct art forms, such as sculpture and music or painting and light art." <![CDATA[(<a href="#cwrc:db2f8571-a773-4068-a35f-34262950bb8f">Getty, 2017</a>)]]></skos:definition>
    <skos:definition xml:lang="fr">Oeuvre matérialisée par son support quel qu'il soit ou son mode de communication, constituée de différents éléments (logiciel, graphisme, musique, son, scénario, images fixes ou animées, etc.) assemblés pour former un ensemble à l'identité propre.</skos:definition>
    <skos:altLabel xml:lang="en">software, multimedia</skos:altLabel>
    <skos:related rdf:resource="http://vocab.getty.edu/aat/300047910"/>
    <owl:sameAs rdf:resource="http://data.culture.fr/thesaurus/page/ark:/67717/T69-7979"/>
    <skos:altLabel xml:lang="en">mixed media</skos:altLabel>
    <rdfs:comment xml:lang="en">This term and its description were created from data gathered from the Thésaurus de la désignation des objets mobiliers (2014).</rdfs:comment>
    <rdfs:label xml:lang="fr">multimédia</rdfs:label>
    <rdfs:label xml:lang="en">multimedia</rdfs:label>
  </genre:DigitalMedium>
  <genre:ThematicWritingGenre rdf:about="http://sparql.cwrc.ca/ontologies/genre#juvenilia">
    <skos:definition xml:lang="fr">Œuvres littéraires ou artistiques produites par des personnes dans leur enfance ou leur jeunesse; le terme est généralement utilisé pour distinguer ces œuvres des travaux matures plus tardifs.</skos:definition>
    <rdfs:comment xml:lang="en">The description for this term is indebted to the Getty Art &amp; Architecture Thesaurus.</rdfs:comment>
    <rdfs:label xml:lang="fr">oeuvres de jeunesse</rdfs:label>
    <skos:definition xml:lang="en">"Literary or artistic works produced by persons in their childhood or youth; usually used to set those works apart from later, mature works." <![CDATA[(<a href="#cwrc:db2f8571-a773-4068-a35f-34262950bb8f">Getty, 2017</a>)]]></skos:definition>
    <rdfs:label xml:lang="en">juvenilia</rdfs:label>
    <owl:sameAs rdf:resource="http://vocab.getty.edu/aat/300028883"/>
  </genre:ThematicWritingGenre>
  <genre:ThematicWritingGenre rdf:about="http://sparql.cwrc.ca/ontologies/genre#orientalist">
    <skos:definition xml:lang="en">"Writing about the East by Western writers and with a Western perspective, encompassing everything from fiction to scientific writing. In Orientalist writing, even if not looked down upon as inferior, Eastern cultures are represented as foreign and exotic, and in need of translation, interpretation, or explanation." <![CDATA[(<a href="#cwrc:2f09376c-f784-4a46-9f04-5a21aa311f27">Penguin, 1999</a>)]]></skos:definition>
    <rdfs:label xml:lang="en">orientalist</rdfs:label>
    <owl:sameAs rdf:resource="http://dbpedia.org/resource/Orientalism"/>
    <rdfs:comment xml:lang="en">This term and its description were created from data gathered from the Penguin Dictionary of Literary Terms &amp; Literary Theory, 4th ed.</rdfs:comment>
    <rdfs:label xml:lang="fr">orientalisme</rdfs:label>
    <rdf:type rdf:resource="http://sparql.cwrc.ca/ontologies/genre#InformationalGenre"/>
    <skos:definition xml:lang="fr">«L'orientalisme est un mouvement littéraire et artistique né en Occident au XIXe siècle. Il existe cependant un orientalisme prémoderne humaniste et classique qui remonte à la fin du Moyen Âge et au début de la Renaissance, lorsque les explorations commencèrent, avec par exemple Marco Polo, et qui atteint son apogée avec les turqueries et le goût oriental du XVIIIe siècle baroque puis rococo. Ce goût oriental hérite aussi du contact de l'époque des Croisades avec le monde islamique. Cet article traite donc plutôt de l'orientalisme à partir du XIXe siècle. C'est un mouvement qui marque l'intérêt de cette époque pour les cultures d'Afrique du Nord, turque et arabe, et toutes les régions dominées par l'Empire ottoman, jusqu'au Caucase.» <![CDATA[(<a href="#cwrc:727d97bc-af78-4122-94be-aa78b2e97d5a">DBpedia, 2017</a>)]]></skos:definition>
  </genre:ThematicWritingGenre>
  <genre:MovingMedium rdf:about="http://sparql.cwrc.ca/ontologies/genre#videoRecording">
    <rdfs:label xml:lang="en">video recording</rdfs:label>
    <skos:related rdf:resource="http://vocab.getty.edu/aat/300028682"/>
  </genre:MovingMedium>
  <genre:NovelisticGenre rdf:about="http://sparql.cwrc.ca/ontologies/genre#sensationNovel">
    <skos:definition xml:lang="fr">«Le roman à sensation est un genre littéraire né dans la deuxième moitié du XIXe siècle en Grande-Bretagne. Ce genre littéraire est une évolution des romans mélodramatiques, qui utilisaient un ensemble de personnages stéréotypés, et des romans Newgate, qui avaient pour thème principal la vie de célèbres criminels. East Lynne de Ellen Wood's, paru en 1861, fut le premier roman à être étiqueté comme roman à sensation par la critique. Le courant comprend trois auteurs majeurs : Ellen Woods, Wilkie Collins (La Femme en blanc, 1859; La Pierre de lune, 1868) et Mary Elizabeth Braddon (Le secret de Lady Audley, 1862). Les romans à sensation avaient pour thèmes des sujets choquants comme l'adultère, le vol, l'enlèvement, la bigamie, la fabrication de fausse monnaie, la séduction et le meurtre. Le genre se distinguait des autres mouvements de l'époque, comme le mouvement Gothique, par l'utilisation de ces thèmes dans un contexte domestique, voire familial, allant ainsi à l'encontre de l'idée largement répandue à l'époque victorienne que les événements sensationnels étaient totalement étrangers à la vie confortable des classes moyennes qui composaient la plus grande partie du lectorat de l'époque. William S. Gilbert fit une satire du genre en 1871 avec son opéra comique A Sensation Novel.» <![CDATA[(<a href="#cwrc:727d97bc-af78-4122-94be-aa78b2e97d5a">DBpedia, 2017</a>)]]></skos:definition>
    <owl:sameAs rdf:resource="http://dbpedia.org/resource/Sensation_novel"/>
    <skos:definition xml:lang="en">"The sensation novel was a literary genre of fiction popular in Great Britain in the 1860s and 1870s, following on from earlier melodramatic novels and the Newgate novels, which focused on tales woven around criminal biographies. It also drew on the gothic and romantic genres of fiction. The sensation novel's appearance notably follows the Industrial Revolution, which made books available on a mass scale for people of all social standings and increased the sensation novel's popularity. Sensation novels used both modes of romance and realism to the extreme where in the past they had traditionally been contradictory modes of literature. The sensation novelists commonly wrote stories that were allegorical and abstract; the abstract nature of the stories gave the authors room to explore scenarios that wrestled with the social anxieties of the Victorian Era. The loss of identity is seen in many sensation fiction stories because this was a common social anxiety; in Britain, there was an increased use in record keeping and therefore people questioned the meaning and permanence of identity. The social anxiety regarding identity is reflected in stories, such as, The Woman in White and Lady Audley's Secret. The genre of sensation fiction was established by the publications of the following novels The Woman in White by Wilkie Collins in 1859; East Lynne by Ellen Wood in 1861; Lady Audley's Secret by Mary Elizabeth Braddon in 1862. Perhaps the earliest use of the term, sensation fiction, as a name for such novels appears in the 1861 edition of the Saunders, Otley, &amp; co.'s Literary Budget. The neo-Victorian novel of New Zealand author Eleanor Catton, The Luminaries, which won the 2013 Man Booker Prize, has been described as being heavily based on sensation literature, with its plot devices of "suspect wills and forged documents, secret marriages, illegitimacy and opium" <![CDATA[(<a href="#cwrc:727d97bc-af78-4122-94be-aa78b2e97d5a">DBpedia, 2017</a>)]]></skos:definition>
    <rdfs:comment xml:lang="en">The description for this term is indebted to DBpedia. </rdfs:comment>
    <rdf:type rdf:resource="http://sparql.cwrc.ca/ontologies/genre#MysteryGenre"/>
    <rdfs:label xml:lang="en">sensation novel</rdfs:label>
  </genre:NovelisticGenre>
  <genre:DramaticGenre rdf:about="http://sparql.cwrc.ca/ontologies/genre#sketch">
    <skos:definition xml:lang="en">"Short literary compositions on single subjects, often presenting the personal view of the author." <![CDATA[(<a href="#cwrc:db2f8571-a773-4068-a35f-34262950bb8f">Getty, 2017</a>)]]></skos:definition>
    <rdfs:label xml:lang="fr">croquis</rdfs:label>
    <owl:sameAs rdf:resource="http://dbpedia.org/resource/Croquis"/>
    <rdfs:comment xml:lang="en">The description for this term is indebted to the Getty Art &amp; Architecture Thesaurus.</rdfs:comment>
    <rdfs:label xml:lang="en">sketch</rdfs:label>
    <skos:definition xml:lang="fr">«Un croquis est un dessin fait rapidement, à main levée, sans recherche de détails dans le but de dégager à grands traits, l'essentiel du sujet, du motif ; souvent fait d'après nature, il alimente le carnet de voyage dessiné dit « de croquis ».» <![CDATA[(<a href="#cwrc:727d97bc-af78-4122-94be-aa78b2e97d5a">DBpedia, 2017</a>)]]></skos:definition>
  </genre:DramaticGenre>
  <genre:SatiricalGenre rdf:about="http://sparql.cwrc.ca/ontologies/genre#mockForms">
    <rdfs:label xml:lang="en">mock forms</rdfs:label>
    <skos:definition xml:lang="fr">Œuvres qui reprennent les conventions d'un genre spécifique dans une perspective satirique, dans le but de le parodier ou de le tourner en ridicule.</skos:definition>
    <rdfs:label xml:lang="fr">imitations parodiques</rdfs:label>
    <skos:definition xml:lang="en">Writing that uses the conventions of a specific genre satirically in order to mock or parody that genre.</skos:definition>
  </genre:SatiricalGenre>
  <genre:ReligiousGenre rdf:about="http://sparql.cwrc.ca/ontologies/genre#liturgy">
    <owl:sameAs rdf:resource="http://vocab.getty.edu/aat/300055983"/>
    <rdfs:comment xml:lang="en">This term and its description were created from data gathered from the Getty Art &amp; Architecture Thesaurus.</rdfs:comment>
    <skos:definition xml:lang="fr">«Cet article concerne les cérémonies formant le culte public et officiel institué par une église. Pour l'obligation fiscale pesant sur les riches en Grèce antique, voir liturgie (Grèce antique). Le mot liturgie (du grec λειτουργία / leitourgía ; « le service du peuple ») est l'ensemble des rites, cérémonies et prières dédiés au culte d'une divinité religieuse, tels qu'ils sont définis selon les règles éventuellement codifiées dans les textes sacrés ou la tradition. Ce terme s'applique le plus souvent à la religion chrétienne où il désigne un culte public et officiel institué par une église.» <![CDATA[(<a href="#cwrc:727d97bc-af78-4122-94be-aa78b2e97d5a">DBpedia, 2017</a>)]]></skos:definition>
    <skos:definition xml:lang="en">"Writing, typically in the form of a prayer or a song, to be used by a particular religious community for the purpose of worship." <![CDATA[(<a href="#cwrc:db2f8571-a773-4068-a35f-34262950bb8f">Getty, 2017</a>)]]></skos:definition>
    <rdfs:label xml:lang="en">liturgy</rdfs:label>
    <rdfs:label xml:lang="fr">liturgie</rdfs:label>
  </genre:ReligiousGenre>
  <genre:BookForm rdf:about="http://sparql.cwrc.ca/ontologies/genre#scrapbook">
    <skos:definition xml:lang="en">"Blank books or albums designed so that a variety of items may be affixed to the pages, including photographs, clippings, and other memorabilia." <![CDATA[(<a href="#cwrc:db2f8571-a773-4068-a35f-34262950bb8f">Getty, 2017</a>)]]></skos:definition>
    <rdfs:label xml:lang="en">scrapbook</rdfs:label>
    <rdfs:label xml:lang="fr">album</rdfs:label>
    <rdfs:comment xml:lang="en">This term and its description were created from data gathered from DBpedia.</rdfs:comment>
    <skos:definition xml:lang="fr">«Un album photos est un livre regroupant un ensemble de photographies. Certains albums ont des compartiments dans lesquels les photos sont rangées, d'autres, généralement plus anciens, contiennent simplement des feuilles de papier épais sur lesquelles les photos peuvent être collées. Il est également possible et facile de créer un album photo avec les photos numériques. De nombreux logiciels offrent cette possibilité.» <![CDATA[(<a href="#cwrc:727d97bc-af78-4122-94be-aa78b2e97d5a">DBpedia, 2017</a>)]]></skos:definition>
    <owl:sameAs rdf:resource="http://vocab.getty.edu/aat/300027341"/>
    <skos:related rdf:resource="http://vocab.getty.edu/aat/300027341"/>
  </genre:BookForm>
  <genre:ComedicGenre rdf:about="http://sparql.cwrc.ca/ontologies/genre#blackComedy">
    <rdfs:comment xml:lang="en">The description for this term is indebted to DBpedia. </rdfs:comment>
    <rdfs:label xml:lang="en">black comedy</rdfs:label>
    <rdfs:comment xml:lang="fr">La description de ce terme est basée sur celle de DBPedia.</rdfs:comment>
    <skos:definition xml:lang="fr">«L’humour noir est une forme d’humour qui souligne avec cruauté, amertume et parfois désespoir l’absurdité du monde, face à laquelle il constitue quelques fois une forme de défense.» <![CDATA[(<a href="#cwrc:727d97bc-af78-4122-94be-aa78b2e97d5a">DBpedia, 2017</a>)]]></skos:definition>
    <rdfs:label xml:lang="fr">humour noir</rdfs:label>
    <owl:sameAs rdf:resource="http://dbpedia.org/resource/Black_comedy"/>
    <owl:sameAs rdf:resource="http://id.loc.gov/authorities/genreForms/gf2014026248"/>
    <skos:definition xml:lang="en">"A black comedy (or dark comedy) is a comic work that employs morbid humor, which, in its simplest form, is humor that makes light of subject matter usually considered taboo. Black humor corresponds to the earlier concept of gallows humor. Black comedy is often controversial due to its subject matter." <![CDATA[(<a href="#cwrc:727d97bc-af78-4122-94be-aa78b2e97d5a">DBpedia, 2017</a>)]]></skos:definition>
  </genre:ComedicGenre>
  <genre:FictionalGenre rdf:about="http://sparql.cwrc.ca/ontologies/genre#courtshipFiction">
    <skos:definition xml:lang="en">Fiction in which courtship is a major part of the plot.</skos:definition>
    <rdfs:label xml:lang="en">courtship fiction</rdfs:label>
    <rdf:type rdf:resource="http://sparql.cwrc.ca/ontologies/genre#RomanceGenre"/>
  </genre:FictionalGenre>
  <genre:PoeticGenre rdf:about="http://sparql.cwrc.ca/ontologies/genre#anagram">
    <rdfs:label xml:lang="en">anagram</rdfs:label>
    <owl:sameAs rdf:resource="http://dbpedia.org/resource/Anagrammatic_poem"/>
    <rdfs:label xml:lang="fr">anagramme</rdfs:label>
    <skos:definition xml:lang="en">"Anagrammatic poetry is poetry with the constrained form that either each line or each verse is an anagram of all other lines or verses in the poem. A poet that specializes in anagrams is an anagrammarian. Writing anagrammatic poetry is a form of a constrained writing similar to writing pangrams or long alliterations." <![CDATA[(<a href="#cwrc:727d97bc-af78-4122-94be-aa78b2e97d5a">DBpedia, 2017</a>)]]></skos:definition>
    <owl:sameAs rdf:resource="http://id.loc.gov/authorities/genreForms/gf2014026043"/>
    <skos:definition xml:lang="fr">«Une anagramme (le mot est féminin) – du grec ανά, « en arrière », et γράμμα, « lettre », anagramma : « renversement de lettres » – est une construction fondée sur une figure de style qui inverse ou permute les lettres d'un mot ou d'un groupe de mots pour en extraire un sens ou un mot nouveau. Jeu littéraire, l'anagramme peut aussi avoir une valeur ésotérique. Elle a fait l'objet de l'attention autant des linguistes – à l'instar de Ferdinand de Saussure – que des psychanalystes et des poètes contemporains.» <![CDATA[(<a href="#cwrc:727d97bc-af78-4122-94be-aa78b2e97d5a">DBpedia, 2017</a>)]]></skos:definition>
    <rdfs:comment xml:lang="en">The description for this term is indebted to DBpedia. </rdfs:comment>
  </genre:PoeticGenre>
  <genre:PoeticGenre rdf:about="http://sparql.cwrc.ca/ontologies/genre#epic">
    <rdfs:label xml:lang="fr">épique</rdfs:label>
    <owl:sameAs rdf:resource="http://id.loc.gov/authorities/genreForms/gf2014026310"/>
    <rdfs:label xml:lang="en">epic</rdfs:label>
    <skos:definition xml:lang="en">"Meaning extended from "epic poetry," in modern usage refers to literary art forms, such as prose, poetry, plays, films, and other works where the story has a theme of grandeur and heroism." <![CDATA[(<a href="#cwrc:db2f8571-a773-4068-a35f-34262950bb8f">Getty, 2017</a>)]]></skos:definition>
    <rdfs:comment xml:lang="en">The description for this term is indebted to the Getty Art &amp; Architecture Thesaurus.</rdfs:comment>
    <owl:sameAs rdf:resource="http://vocab.getty.edu/aat/300404209"/>
    <skos:definition xml:lang="fr">Provenant du nom "épopoée", le genre épique désigne aujourd'hui les formes artistiques et littéraires (prose, poésie, théâtre, fillms, et autres) dans lesquelles l'histoire a pour thèmes principaux la grandeur et l'héroïsme.</skos:definition>
  </genre:PoeticGenre>
  <genre:FictionalGenre rdf:about="http://sparql.cwrc.ca/ontologies/genre#adventureWriting">
    <skos:definition xml:lang="en">"Action-filled fiction in which a protagonist is removed from her or his ordinary life to undertake some sort of journey or quest. Along the way, the protagonist is exposed to extraordinary events and physical dangers that put his or her virtues, such as bravery, to the test." <![CDATA[(<a href="#cwrc:4c227091-6bf0-4325-b846-9733fae19e61">Oxford, 2015</a>)]]></skos:definition>
    <rdfs:comment xml:lang="en">This term and its description were created from data gathered from the Oxford Dictionary of Literary Terms, 4th ed.</rdfs:comment>
    <dcterms:references rdf:resource="http://www.oxfordreference.com/view/10.1093/acref/9780199208272.001.0001/acref-9780199208272-e-15?rskey=BDrsna%26result=11"/>
    <rdfs:label xml:lang="fr">roman d'aventures</rdfs:label>
    <skos:definition xml:lang="fr">Fiction remplie de péripéties dans laquelle la ou le protagoniste échappe à son quotidien pour entreprendre un voyage ou une quête. En chemin, elle ou il est exposé.e à des événements extraordinaires et à des dangers physiques qui mettent à l'épreuve ses vertus, par exemple la bravoure.</skos:definition>
    <rdfs:label xml:lang="en">adventure writing</rdfs:label>
  </genre:FictionalGenre>
  <genre:SocialScienceGenre rdf:about="http://sparql.cwrc.ca/ontologies/genre#socialScience">
    <skos:definition xml:lang="en">Writing dealing with the study of human societies and relationships across several fields of scientific study, including anthropology, political science, and sociology.</skos:definition>
    <skos:definition xml:lang="fr">Travaux écrits qui étudient les sociétés et les rapports humains à travers plusieurs disciplines scientifiques incluant l'anthropologie, les sciences politiques et la sociologie.</skos:definition>
    <rdfs:label xml:lang="fr">sciences sociales</rdfs:label>
    <rdfs:label xml:lang="en">social science</rdfs:label>
  </genre:SocialScienceGenre>
  <genre:ScriptForm rdf:about="http://sparql.cwrc.ca/ontologies/genre#script">
    <rdfs:label xml:lang="en">script</rdfs:label>
  </genre:ScriptForm>
  <genre:IllustratedForm rdf:about="http://sparql.cwrc.ca/ontologies/genre#graphicNovel">
    <rdfs:label xml:lang="en">graphic novel</rdfs:label>
    <owl:sameAs rdf:resource="http://id.loc.gov/authorities/genreForms/gf2014026362"/>
  </genre:IllustratedForm>
  <genre:ReferenceWorkGenre rdf:about="http://sparql.cwrc.ca/ontologies/genre#manual">
    <owl:sameAs rdf:resource="http://vocab.getty.edu/aat/300026395"/>
    <rdfs:label xml:lang="en">manual</rdfs:label>
    <skos:definition xml:lang="en">"Books or treatises, often compendious, containing rules or instructions needed to perform tasks, operations, processes, occupations, arts, or studies, and intended to be used as reference while the task or study is performed." <![CDATA[(<a href="#cwrc:db2f8571-a773-4068-a35f-34262950bb8f">Getty, 2017</a>)]]></skos:definition>
    <skos:altLabel xml:lang="en">companion</skos:altLabel>
    <owl:sameAs rdf:resource="http://id.loc.gov/authorities/genreForms/gf2014026109"/>
    <rdfs:label xml:lang="fr">manuel</rdfs:label>
    <skos:definition xml:lang="fr">Livres ou traités, souvent concis, contenant des règles ou des instructions nécessaires à la réalisation de tâches, d"opérations, de processus, de professions, d'arts ou d'études, et destinés à être utilisés comme référence pendant la réalisation de la tâche ou de l'apprentissage.</skos:definition>
    <rdfs:comment xml:lang="en">The description for this term is indebted to the Getty Art &amp; Architecture Thesaurus.</rdfs:comment>
  </genre:ReferenceWorkGenre>
  <genre:PedagogicalGenre rdf:about="http://sparql.cwrc.ca/ontologies/genre#pedagogy">
    <rdfs:label xml:lang="en">pedagogy</rdfs:label>
    <rdfs:comment xml:lang="en">This term and its description were created from data gathered from the Oxford Dictionary of English, 3rd ed.</rdfs:comment>
    <skos:definition xml:lang="en">"Writing dealing with the theory and practice of teaching." <![CDATA[(<a href="#cwrc:4c227091-6bf0-4325-b846-9733fae19e61/">Oxford, 2015</a>)]]></skos:definition>
    <skos:definition xml:lang="fr">«La pédagogie (du grec παιδαγωγία, direction ou éducation des enfants) désigne l'art de l'éducation. Le terme rassemble les méthodes et pratiques d'enseignement requises pour transmettre des connaissances, c'est-à-dire un savoir, un savoir-faire ou un savoir-être. Plus généralement, l'expression « Faire preuve de pédagogie » signifie l'aptitude à enseigner et à transmettre à un individu ou un groupe d'individus — de tous âges et de toutes conditions — un savoir ou une expérience par l'usage des méthodes les plus adaptées à l'audience concernée.» <![CDATA[(<a href="#cwrc:727d97bc-af78-4122-94be-aa78b2e97d5a">DBpedia, 2017</a>)]]></skos:definition>
    <dcterms:references rdf:resource="http://www.oxfordreference.com/view/10.1093/acref/9780199571123.001.0001/m_en_gb0614030?rskey=II64E5%26result=68781"/>
    <rdfs:label xml:lang="fr">pédagogie</rdfs:label>
  </genre:PedagogicalGenre>
  <genre:PhilosophicalGenre rdf:about="http://sparql.cwrc.ca/ontologies/genre#philosophy">
    <rdfs:comment xml:lang="en">This term and its description were created from data gathered from DBpedia.</rdfs:comment>
    <rdfs:label xml:lang="fr">philosophie</rdfs:label>
    <skos:definition xml:lang="en">"(Greek, "Love of wisdom"): The methodical and systematic exploration of what we know, how we know it, and why it is important that we know it. Too frequently, students use the term somewhat nebulously. They often mistakenly state, "My philosophy about X is . . ." when they really mean, "My opinion about X is . . ." or "My attitude toward X is . . ." Traditional areas of Western philosophic inquiry include the following areas." <![CDATA[(<a href="cwrc:509015ff-7641-473e-94c5-688e06952bb7">L. K Wheeler, 2017</a>)]]></skos:definition>
    <rdfs:label xml:lang="en">philosophy</rdfs:label>
    <skos:definition xml:lang="fr">«La philosophie, du grec ancien φιλοσοφία (composé de φιλεῖν, philein : « aimer » ; et de σοφία, sophia : « sagesse »), signifie littéralement : « l'amour de la sagesse ». C'est une activité et une discipline existant depuis l'Antiquité en Occident et en Orient, se présentant comme un questionnement, une interprétation et une réflexion sur le monde et l'existence humaine. Différents buts peuvent lui être attribués : la recherche de la vérité ; la méditation sur le bien, le beau, le juste ; la quête du sens de la vie et du bonheur.» <![CDATA[(<a href="#cwrc:727d97bc-af78-4122-94be-aa78b2e97d5a">DBpedia, 2017</a>)]]></skos:definition>
    <owl:sameAs rdf:resource="http://dbpedia.org/resource/Philosophy"/>
  </genre:PhilosophicalGenre>
  <genre:IntertextualGenre rdf:about="http://sparql.cwrc.ca/ontologies/genre#parody">
    <rdfs:comment xml:lang="en">The description for this term is indebted to DBpedia. </rdfs:comment>
    <owl:sameAs rdf:resource="http://id.loc.gov/authorities/genreForms/gf2014026470"/>
    <rdfs:label xml:lang="en">parody</rdfs:label>
    <skos:definition xml:lang="en">"A parody (/ˈpærədi/; also called spoof, send-up, take-off or lampoon), in use, is a work created to imitate, make fun of, or comment on an original work, its subject, author, style, or some other target, by means of satiric or ironic imitation. As the literary theorist Linda Hutcheon puts it, "parody … is imitation, not always at the expense of the parodied text." Another critic, Simon Dentith, defines parody as "any cultural practice which provides a relatively polemical allusive imitation of another cultural production or practice."Parody may be found in art or culture, including literature, music (although "parody" in music has an earlier, somewhat different meaning than for other art forms), animation, gaming and film. The writer and critic John Gross observes in his Oxford Book of Parodies, that parody seems to flourish on territory somewhere between pastiche ("a composition in another artist's manner, without satirical intent") and burlesque (which "fools around with the material of high literature and adapts it to low ends"). Meanwhile, the Encyclopédie of Denis Diderot distinguishes between the parody and the burlesque, "A good parody is a fine amusement, capable of amusing and instructing the most sensible and polished minds; the burlesque is a miserable buffoonery which can only please the populace." Historically, when a formula grows tired, as in the case of the moralistic melodramas in the 1910s, it retains value only as a parody, as demonstrated by the Buster Keaton shorts that mocked that genre. In his 1960 anthology of parody from the 14th through 20th centuries, critic Dwight Macdonald offered this metaphor: "Parody is making a new wine that tastes like the old but has a slightly lethal effect." <![CDATA[(<a href="#cwrc:727d97bc-af78-4122-94be-aa78b2e97d5a">DBpedia, 2017</a>)]]></skos:definition>
    <owl:sameAs rdf:resource="http://dbpedia.org/resource/Parody"/>
    <skos:definition xml:lang="fr">«La parodie est une forme d'humour qui utilise le cadre, les personnages, le style et le fonctionnement d'une œuvre ou une institution pour s'en moquer. Elle se base entre autres sur l'inversion et l'exagération des caractéristiques appartenant au sujet parodié. Selon Dominique Maingueneau, la parodie constitue une « stratégie de réinvestissement d'un texte ou d'un genre de discours dans d'autres » : il s'agit d'une stratégie de « subversion », visant à disqualifier l'auteur du texte ou du genre source, tandis que la stratégie opposée (la « captation », imitation positive) permet de « transférer sur le discours réinvestisseur l'autorité attachée au texte ou au genre source ».» <![CDATA[(<a href="#cwrc:727d97bc-af78-4122-94be-aa78b2e97d5a">DBpedia, 2017</a>)]]></skos:definition>
  </genre:IntertextualGenre>
  <genre:ThreeDimensionalMedium rdf:about="http://sparql.cwrc.ca/ontologies/genre#threeDimensionalObject">
    <rdfs:label xml:lang="en">three dimensional object</rdfs:label>
  </genre:ThreeDimensionalMedium>
  <genre:PoeticGenre rdf:about="http://sparql.cwrc.ca/ontologies/genre#ballad">
    <skos:closeMatch rdf:resource="http://dbpedia.org/resource/Ballad"/>
    <rdfs:label xml:lang="en">ballad</rdfs:label>
    <rdfs:comment xml:lang="en">The description for this term is indebted to DBpedia.</rdfs:comment>
    <owl:sameAs rdf:resource="http://id.loc.gov/authorities/genreForms/gf2014026648"/>
    <skos:definition xml:lang="fr">«Ballade désigne, au sens ancien, un poème médiéval à forme fixe composé de trois couplets et d'une demi-strophe appelée envoi, chacune étant terminée par un vers refrain, qui rappelle la forme chantée des origines. L'histoire de la poésie retient en particulier les ballades aux strophes carrées (le nombre de vers est égal au nombre de syllabes de chaque vers) de huit ou dix vers et aux thèmes très variés qu'ont composées des poètes comme Guillaume de Machaut, Eustache Deschamps (fin xiv siècle), Christine de Pisan et François Villon (début et milieu du xve siècle) ou encore Clément Marot au xvie, alors que la Pléiade rejette le genre de la ballade comme vieilli, privilégiant des formes nouvelles comme le sonnet ou l'ode.» <![CDATA[(<a href="#cwrc:727d97bc-af78-4122-94be-aa78b2e97d5a">DBpedia, 2017</a>)]]></skos:definition>
    <rdfs:label xml:lang="fr">ballade</rdfs:label>
    <rdfs:comment xml:lang="fr">La description de ce terme est basée sur celle de DBPedia.</rdfs:comment>
    <skos:definition xml:lang="en">A ballad /ˈbæləd/ is a form of verse, often a narrative set to music. Ballads derive from the medieval French chanson balladée or ballade, which were originally "dancing songs". Ballads were particularly characteristic of the popular poetry and song of the British Isles from the later medieval period until the 19th century and used extensively across Europe and later the Americas, Australia and North Africa.<![CDATA[(<a href="#cwrc:727d97bc-af78-4122-94be-aa78b2e97d5a">DBpedia, 2017</a>)]]></skos:definition>
  </genre:PoeticGenre>
  <genre:PoeticGenre rdf:about="http://sparql.cwrc.ca/ontologies/genre#pindaric">
    <rdfs:label xml:lang="fr">ode pindarique</rdfs:label>
    <skos:definition xml:lang="fr">Nous sont parvenus quatre des dix-sept livres de poèmes pindariques recensés par Aristophane de Byzance : les Olympiques, les Pythiques, les Isthmiques, et les Néméennes, toutes « épinicies », ou odes triomphales, mais nous manquent presque toujours les indications du lyrisme choral ; parfois on ne sait établir ni traduire le texte même. Leur forme est à la fois fixe et extrêmement libre : chacune est composée de triades (strophe, antistrophe, épode), en mètres dactylo-épitritique (quatre syllabes, dont trois longues et une brève) et logaédique (dactyles et spondées), mais les membres des vers, comme les triades, sont en nombre variable, avec de fréquents rejets, même d'une strophe à l'autre. Inimitable, disait Horace ; le poète, à s'y risquer, s'y perdrait comme Dédale ; imitée à la Renaissance par Ronsard par exemple, et attaquée ou défendue lors de la querelle des Anciens et des Modernes ; engendrant une postérité plus fidèle et plus originale avec Hölderlin, et peut-être Claudel, l'ode pindarique importe, outre son caractère d'œuvre, par ce qu'elle apprend de la Grèce et de la poésie.</skos:definition>
    <rdfs:label xml:lang="en">pindaric</rdfs:label>
    <owl:sameAs rdf:resource="http://www.universalis.fr/encyclopedie/ode-pindarique/"/>
    <rdfs:comment xml:lang="en">This term and its description were created from data gathered from DBpedia.</rdfs:comment>
    <skos:definition xml:lang="en">"Pindarics (alternatively Pindariques or Pindaricks) was a term for a class of loose and irregular odes greatly in fashion in England during the close of the 17th and the beginning of the 18th century. Abraham Cowley, who published fifteen Pindarique Odes in 1656, was the poet most identified with the form though many others had composed irregular verses before him. The term is derived from the name of a Greek archaic poet, Pindar, but is based on a misconception since Pindar's odes were in fact very formal, obeying a triadic structure, in which the form of the first stanza (strophe) was repeated in the second stanza (antistrophe), followed by a third stanza (epode) that introduced variations but whose form was repeated by other epodes in subsequent triads." <![CDATA[(<a href="#cwrc:727d97bc-af78-4122-94be-aa78b2e97d5a">DBpedia, 2017</a>)]]></skos:definition>
  </genre:PoeticGenre>
  <genre:PoeticGenre rdf:about="http://sparql.cwrc.ca/ontologies/genre#occasionalPoetry">
    <rdfs:label xml:lang="fr">poésie de circonstance</rdfs:label>
    <rdfs:comment xml:lang="en">The description for this term is indebted to DBpedia. </rdfs:comment>
    <owl:sameAs rdf:resource="http://id.loc.gov/authorities/genreForms/gf2014026460"/>
    <skos:definition xml:lang="en">Occasional poetry is poetry composed for a particular occasion. In the history of literature, it is often studied in connection with orality, performance, and patronage.</skos:definition>
    <rdfs:label xml:lang="en">occasional poetry</rdfs:label>
    <skos:definition xml:lang="fr">Poésie composée en l'honneur d'une occasion particulière. Dans l'histoire de la littérature, elle est souvent étudiée en relation avec l'oralité, la performance et le mécénat.</skos:definition>
    <skos:closeMatch rdf:resource="http://dbpedia.org/resource/Occasional_poetry"/>
  </genre:PoeticGenre>
  <genre:DramaticGenre rdf:about="http://sparql.cwrc.ca/ontologies/genre#balladOpera">
    <owl:sameAs rdf:resource="http://dbpedia.org/resource/Ballad_opera"/>
    <rdfs:label xml:lang="en">ballad opera</rdfs:label>
    <skos:definition xml:lang="fr">«Le ballad opera est un genre de spectacles caractéristiques de la scène anglaise du XVIIIe siècle, écrits en réaction à la prééminence de l'opéra italien sur les scènes d'alors. Il s'agissait de pièces musicales satiriques, qui suivaient certaines des conventions de l'opéra, mais sans récitatifs. Les textes de ces pièces étaient mis en musique sur des hymnes religieux, des mélodies populaires d'alors, des airs d'opéras connus, et surtout, sur des romances, des ballads populaires, qui ont donné leur nom au genre. Le fondateur du genre, et le plus fameux des ballad operas, est The Beggar's Opera, de John Gay et Johann Christoph Pepusch.» <![CDATA[(<a href="#cwrc:727d97bc-af78-4122-94be-aa78b2e97d5a">DBpedia, 2017</a>)]]></skos:definition>
    <rdfs:comment xml:lang="en">This term and its description were created from data gathered from DBpedia.</rdfs:comment>
    <rdfs:label xml:lang="fr">ballad opera ou opéra-ballade</rdfs:label>
    <skos:definition xml:lang="en">"A drama combining song and spoken dialogue, popularized in the 1700s by John Gay’s The Beggar’s Opera. It can be seen as a precursor to the modern musical." <![CDATA[(<a href="#cwrc:2f09376c-f784-4a46-9f04-5a21aa311f27">Penguin, 1999</a>)]]></skos:definition>
    <owl:sameAs rdf:resource="http://id.loc.gov/authorities/genreForms/gf2014026645"/>
    <rdf:type rdf:resource="http://sparql.cwrc.ca/ontologies/genre#OperaGenre"/>
  </genre:DramaticGenre>
  <genre:InformationalGenre rdf:about="http://sparql.cwrc.ca/ontologies/genre#medicalWriting">
    <skos:definition xml:lang="en">Writing, typically of a scientific nature, relating to the field of medicine.</skos:definition>
    <rdfs:label xml:lang="fr">traité médical</rdfs:label>
    <skos:definition xml:lang="fr">Écrits, de nature scientifique pour la plupart, qui traitent du sujet de la médecine.</skos:definition>
    <rdfs:label xml:lang="en">medical writing</rdfs:label>
  </genre:InformationalGenre>
  <genre:DramaticGenre rdf:about="http://sparql.cwrc.ca/ontologies/genre#radioDrama">
    <skos:definition xml:lang="fr">«Le théâtre radiophonique ou radio-théâtre est une adaptation du médium théâtral au médium radiophonique.À partir du début des années 1950, le théâtre radiophonique subit la concurrence de la dramatique radio, puisque le premier terme disparait.» <![CDATA[(<a href="#cwrc:727d97bc-af78-4122-94be-aa78b2e97d5a">DBpedia, 2017</a>)]]></skos:definition>
    <rdfs:label xml:lang="fr">théâtre radiophonique</rdfs:label>
    <owl:sameAs rdf:resource="http://dbpedia.org/resource/Radio_drama"/>
    <rdfs:comment xml:lang="en">This term and its description were created from data gathered from DBpedia.</rdfs:comment>
    <owl:sameAs rdf:resource="http://id.loc.gov/authorities/genreForms/gf2014026499"/>
    <skos:definition xml:lang="en">"Radio drama (or audio drama, audio play, radio play, radio theater, or audio theater) is a dramatized, purely acoustic performance, broadcast on radio. With no visual component, radio drama depends on dialogue, music and sound effects to help the listener imagine the characters and story." <![CDATA[(<a href="#cwrc:727d97bc-af78-4122-94be-aa78b2e97d5a">DBpedia, 2017</a>)]]></skos:definition>
    <rdfs:label xml:lang="en">radio drama</rdfs:label>
  </genre:DramaticGenre>
  <genre:ScholarlyGenre rdf:about="http://sparql.cwrc.ca/ontologies/genre#artCriticism">
    <rdfs:comment xml:lang="en">This term and its description were created from data gathered from the Getty Art &amp; Architecture Thesaurus.</rdfs:comment>
    <rdfs:label xml:lang="fr">critique d'art</rdfs:label>
    <skos:definition xml:lang="fr">"L'étude ou la pratique analytique, descriptive et évualtive d'oeuvres d'art et d'expositions."</skos:definition>
    <owl:sameAs rdf:resource="http://id.loc.gov/authorities/genreForms/gf2018026112"/>
    <rdfs:label xml:lang="en">art criticism</rdfs:label>
    <skos:definition xml:lang="en">"The study or practice of the analytical description, interpretation, and evaluation of visual art works and exhibitions." <![CDATA[(<a href="#cwrc:db2f8571-a773-4068-a35f-34262950bb8f">Getty, 2017</a>)]]></skos:definition>
    <owl:sameAs rdf:resource="http://vocab.getty.edu/aat/300168233"/>
  </genre:ScholarlyGenre>
  <genre:NovelisticGenre rdf:about="http://sparql.cwrc.ca/ontologies/genre#bildungsroman">
    <owl:sameAs rdf:resource="http://dbpedia.org/resource/Bildungsroman"/>
    <skos:definition xml:lang="fr">«Le roman d'apprentissage, appelé aussi roman de formation ou roman d’éducation, est un genre littéraire romanesque né en Allemagne au XVIIIe siècle (à ne pas confondre avec le roman de jeunesse). Il s'oppose cependant à la fonction première du romanesque qui est de nous transporter dans un monde de rêve et d'évasion. On parle ainsi de « roman initiatique » ou de « conte initiatique ». En allemand, le roman de formation est nommé « Bildungsroman ». Ce terme est dû au philologue allemand Johann Carl Simon Morgenstern, qui voyait dans le Bildungsroman « l'essence du roman par opposition au récit épique ». On emploie aussi l'expression « Entwicklungsroman » (roman de développement personnel). Un roman d'apprentissage a pour thème le cheminement évolutif d'un héros, souvent jeune, jusqu'à ce qu'il atteigne l'idéal de l'homme accompli et cultivé. Le héros découvre en général un domaine particulier dans lequel il fait ses armes. Mais en réalité, c'est une conception de la vie en elle-même qu'il se forge progressivement. En effet, derrière l'apprentissage d'un domaine, le jeune héros découvre les grands événements de l'existence (la mort, l'amour, la haine, l'altérité, pour prendre quelques exemples). Ainsi, dans L'Éducation sentimentale (Flaubert, 1869), le jeune Frédéric connaît les premiers émois de l'amour : et réfléchissant sur les sentiments qu'il porte à Mme Arnoux, Frédéric se construit une idée de l'existence. Le roman d'apprentissage est un roman qui décrit la maturation du héros. Il manque d'expérience au départ et traverse des obstacles ou des épreuves afin de mûrir et d'en tirer des leçons.» <![CDATA[(<a href="#cwrc:727d97bc-af78-4122-94be-aa78b2e97d5a">DBpedia, 2017</a>)]]></skos:definition>
    <rdfs:comment xml:lang="fr">La description de ce terme est basée sur celle de DBPedia.</rdfs:comment>
    <rdfs:label xml:lang="fr">bildungsroman</rdfs:label>
    <owl:sameAs rdf:resource="http://id.loc.gov/authorities/genreForms/gf2014026243"/>
    <rdfs:label xml:lang="en">bildungsroman</rdfs:label>
    <skos:definition xml:lang="en">"Novels of a traditional German genre that focuses on the spiritual development or formative years of an individual. Now in broad use to refer to this type of novel written in any language or in any culture." <![CDATA[(<a href="#cwrc:db2f8571-a773-4068-a35f-34262950bb8f">Getty, 2017</a>)]]></skos:definition>
    <rdfs:comment xml:lang="en">The description for this term is indebted to DBpedia. </rdfs:comment>
  </genre:NovelisticGenre>
  <genre:DidacticGenre rdf:about="http://sparql.cwrc.ca/ontologies/genre#conductLiterature">
    <rdfs:comment xml:lang="en">This term and its description were created from data gathered from DBpedia.</rdfs:comment>
    <skos:definition xml:lang="fr">«Un conduct book (littéralement : « livre de conduite », ou « manuel de conduite ») est un genre littéraire anglais, très répandu à la fin du XVIIIe siècle et au début du XIXe siècle et dont le but est de former le lecteur aux respects des convenances et aux règles de la vie en société. On peut rapprocher de ce genre les conduct novels, les romans d'apprentissage, qui poursuivent le même but au travers d'une histoire romancée.» <![CDATA[(<a href="#cwrc:727d97bc-af78-4122-94be-aa78b2e97d5a">DBpedia, 2017</a>)]]></skos:definition>
    <rdfs:label xml:lang="fr">livre de conduite</rdfs:label>
    <rdfs:label xml:lang="en">conduct literature</rdfs:label>
    <skos:definition xml:lang="en">"Prescriptive literature, usually directed to a specific gender, that outlines the rules of appropriate behaviour according to the gender roles and societal norms prevalent at the time of writing. Conduct books became very popular in the 18th century." <![CDATA[(<a href="#cwrc:2f09376c-f784-4a46-9f04-5a21aa311f27">Penguin, 1999</a>)]]></skos:definition>
    <owl:sameAs rdf:resource="http://dbpedia.org/resource/Conduct_book"/>
  </genre:DidacticGenre>
  <genre:SerialForm rdf:about="http://sparql.cwrc.ca/ontologies/genre#serial">
    <rdfs:label xml:lang="en">serial</rdfs:label>
  </genre:SerialForm>
  <genre:DramaticGenre rdf:about="http://sparql.cwrc.ca/ontologies/genre#kitchenSinkDrama">
    <dcterms:references rdf:resource="http://www.oxfordreference.com/view/10.1093/acref/9780199208272.001.0001/acref-9780199208272-e-629?rskey=HtykbC%26result=621"/>
    <rdfs:label xml:lang="fr">kitchen sink drama</rdfs:label>
    <skos:definition xml:lang="en">"Originating in Britain in the 1950s, realistic drama centred on the domestic lives of working-class characters." <![CDATA[(<a href="#cwrc:4c227091-6bf0-4325-b846-9733fae19e61">Oxford, 2015</a>)]]></skos:definition>
    <rdfs:label xml:lang="en">kitchen sink drama</rdfs:label>
    <rdfs:comment xml:lang="en">This term and its description were created from data gathered from the Oxford Dictionary of Literary Terms, 4th ed.</rdfs:comment>
    <skos:definition xml:lang="fr">Drame réaliste centré sur la vie domestique de personnages de la classe ouvrière, apparu en Angleterre dans les années 50.</skos:definition>
  </genre:DramaticGenre>
  <genre:DidacticGenre rdf:about="http://sparql.cwrc.ca/ontologies/genre#sageWriting">
    <skos:definition xml:lang="fr">Le "sage writing" était un genre non fictionel populaire à l'ère victorienne. Son nom vient de de John Holloway paru en 1953, The Victorian Sage: Studies in Argument. Le "sage writing" s'inspire de la littérature de sagesse antique dans laquelle l'auteur donne des leçons et des enseignements à son lecteur concernant des questions sociales contemporaines, souvent en utilisant dans un style accessible et non savant les discours philosophiques, historiques, politiques et et économiques. Les représentants les plus connus du "sage writing" sont Thomas Carlyle, Matthew Arnold, John Ruskin et Henry David Thoreau. Certains écrivains du 20ème siècle comme Joan Didion et les New Journalists Norman Mailer et Tom Wolfe sont également considérés comme appartenant à ce genre.</skos:definition>
    <rdfs:label xml:lang="fr">sage writing</rdfs:label>
    <rdfs:comment xml:lang="en">The description for this term is indebted to DBpedia. </rdfs:comment>
    <skos:definition xml:lang="en">"Sage writing was a genre of creative nonfiction popular in the Victorian era. The concept originates with John Holloway's 1953 book The Victorian Sage: Studies in Argument. Sage writing is a development from ancient wisdom literature in which the writer chastises and instructs the reader about contemporary social issues, often utilizing discourses of philosophy, history, politics, and economics in non-technical ways. Prominent examples of the genre include writings by Thomas Carlyle, Matthew Arnold, John Ruskin, and Henry David Thoreau. Some 20th-century writers, such as Joan Didion and New Journalists such as Norman Mailer and Tom Wolfe, have also been identified as sage writers." <![CDATA[(<a href="#cwrc:727d97bc-af78-4122-94be-aa78b2e97d5a">DBpedia, 2017</a>)]]></skos:definition>
    <rdfs:label xml:lang="en">sage writing</rdfs:label>
    <owl:sameAs rdf:resource="http://dbpedia.org/resource/Sage_writing"/>
  </genre:DidacticGenre>
  <genre:ComedicGenre rdf:about="http://sparql.cwrc.ca/ontologies/genre#comedyOfManners">
    <skos:definition xml:lang="en">"The comedy of manners is an entertainment form which satirizes the manners and affectations of a social class or of multiple classes, often represented by stereotypical stock characters. For example, the miles gloriosus ("boastful soldier") in ancient times, the fop and the rake during the English Restoration, or an old person pretending to be young. Restoration comedy is used as a synonym for "comedy of manners". The plot of the comedy, often concerned with scandal, is generally less important than its witty dialogue. A great writer of comedies of manners was Oscar Wilde, his most famous play being The Importance of Being Earnest. The comedy of manners was first developed in the new comedy of the Ancient Greek playwright Menander. His style, elaborate plots, and stock characters were imitated by the Roman playwrights Plautus and Terence, whose comedies were widely known and copied during the Renaissance. The best-known comedies of manners, however, may well be those of the French playwright Molière, who satirized the hypocrisy and pretension of the ancien régime in such plays as L'École des femmes (The School for Wives, 1662), Le Misanthrope (The Misanthrope, 1666), and most famously Tartuffe (1664)." <![CDATA[(<a href="#cwrc:727d97bc-af78-4122-94be-aa78b2e97d5a">DBpedia, 2017</a>)]]></skos:definition>
    <skos:definition xml:lang="fr">«La comédie de mœurs est un sous-genre de la comédie qui se développe à partir du XVIe siècle. Y sont dénoncés les travers d'une époque, d'un groupe ou d'une classe sociale, généralement dominante. La comédie de mœurs est souvent caractérisée par une critique sociale qui reste superficielle. Généralement la dimension satirique ne vise qu'un travers particulier ou une convention risible très ciblée de la communauté dépeinte. En ce sens, la comédie de mœurs ne remet souvent rien de fondamental en cause dans la structure sociale ni dans la représentation dominante de l'époque. La critique s'efface vite et devient récupérable par l'ordre en place, comme dans les pièces d'Émile Augier ou d'Alexandre Dumas fils. Cependant, le dénouement peut aussi être impressionnant, comme celui des Affaires sont les affaires du libertaire Octave Mirbeau (1903), parfois qualifié de "shakespearien". Plusieurs comédies très connues de Molière sont des comédies de mœurs : Les Précieuses ridicules ou encore Les Femmes savantes mais aussi L'École des femmes. Pour Molière, la comédie de mœurs représente un lieu privilégié pour la satire sociale.» <![CDATA[(<a href="#cwrc:727d97bc-af78-4122-94be-aa78b2e97d5a">DBpedia, 2017</a>)]]></skos:definition>
    <rdfs:label xml:lang="en">comedy of manners</rdfs:label>
    <owl:sameAs rdf:resource="http://id.loc.gov/authorities/genreForms/gf2014026263"/>
    <owl:sameAs rdf:resource="http://dbpedia.org/resource/Comedy_of_manners"/>
    <rdfs:comment xml:lang="en">The description for this term is indebted to DBpedia. </rdfs:comment>
  </genre:ComedicGenre>
  <genre:ScholarlyGenre rdf:about="http://sparql.cwrc.ca/ontologies/genre#scholarlyWriting">
    <skos:altLabel xml:lang="en">academic writing</skos:altLabel>
    <rdfs:label xml:lang="en">scholarly writing</rdfs:label>
    <rdfs:label xml:lang="fr">érudition</rdfs:label>
    <skos:definition xml:lang="en">Writing by a scholar, either amateur or professional, typically focused on a specific field or topic in which the author is an expert.</skos:definition>
    <skos:definition xml:lang="fr">Travaux écrits d'un intellectuel, amateur ou professionnel, normalement centré sur un domain ou un sujet spécifique dans lequel l'auteure est experte.</skos:definition>
  </genre:ScholarlyGenre>
  <genre:FictionalGenre rdf:about="http://sparql.cwrc.ca/ontologies/genre#scienceFiction">
    <skos:definition xml:lang="en">"Science fiction is a genre of speculative fiction dealing with imaginative concepts such as futuristic settings, futuristic science and technology, space travel, time travel, faster than light travel, parallel universes and extraterrestrial life. Science fiction often explores the potential consequences of scientific and other innovations, and has been called a "literature of ideas." It usually eschews the supernatural, and unlike the related genre of fantasy, historically science fiction stories were intended to have at least a faint grounding in science-based fact or theory at the time the story was created, but this connection has become tenuous or non-existent in much of science fiction." <![CDATA[(<a href="#cwrc:727d97bc-af78-4122-94be-aa78b2e97d5a">DBpedia, 2017</a>)]]></skos:definition>
    <rdfs:comment xml:lang="en">The description for this term is indebted to DBpedia. </rdfs:comment>
    <owl:sameAs rdf:resource="http://dbpedia.org/resource/Science_fiction"/>
    <owl:sameAs rdf:resource="http://id.loc.gov/authorities/genreForms/gf2014026529"/>
    <skos:definition xml:lang="fr">«La science-fiction est un genre narratif, principalement un genre littéraire et un genre cinématographique. Il est structuré par des hypothèses sur ce que pourrait être le futur ou ce qu'aurait pu être le présent voire le passé (planètes éloignées, mondes parallèles, uchronie...), en partant des connaissances actuelles (scientifiques, technologiques, ethnologiques...). Elle se distingue du fantastique qui inclut une dimension inexplicable et de la fantasy qui fait souvent intervenir la magie.» <![CDATA[(<a href="#cwrc:727d97bc-af78-4122-94be-aa78b2e97d5a">DBpedia, 2017</a>)]]></skos:definition>
    <rdfs:label xml:lang="en">science fiction</rdfs:label>
  </genre:FictionalGenre>
  <genre:PrintMedium rdf:about="http://sparql.cwrc.ca/ontologies/genre#chapbook">
    <skos:definition xml:lang="en">"Small books or pamphlets, usually cheaply printed and containing such texts as popular tales, treatises, ballads, or nursery rhymes, formerly peddled by chapmen." <![CDATA[(<a href="#cwrc:db2f8571-a773-4068-a35f-34262950bb8f">Getty, 2017</a>)]]></skos:definition>
    <skos:definition xml:lang="fr">"Petits livres ou brochures généralement imprimés à bon marché et contenant des textes tels que des contes populaires, des traités, des ballades ou des comptines, auparavant vendus par des chapmen."</skos:definition>
    <rdfs:comment xml:lang="en">The description for this term is indebted to the Getty Art &amp; Architecture Thesaurus.</rdfs:comment>
    <skos:related rdf:resource="http://vocab.getty.edu/aat/300152367"/>
    <rdfs:label xml:lang="en">chapbook</rdfs:label>
    <rdfs:label xml:lang="fr">chapbook</rdfs:label>
    <owl:sameAs rdf:resource="http://vocab.getty.edu/aat/300152367"/>
  </genre:PrintMedium>
  <genre:FictionalGenre rdf:about="http://sparql.cwrc.ca/ontologies/genre#novelOfSensibility">
    <rdfs:label xml:lang="en">novel of sensibility</rdfs:label>
  </genre:FictionalGenre>
  <genre:ReligiousGenre rdf:about="http://sparql.cwrc.ca/ontologies/genre#prophecy">
    <owl:sameAs rdf:resource="http://dbpedia.org/resource/Prophecy"/>
    <skos:definition xml:lang="en">"Prophecy involves a process in which one or more messages allegedly communicated to a prophet are then communicated to other people. Such messages typically involve] inspiration, interpretation, or revelation of events to come (compare divine knowledge). Historically, clairvoyance has been used[by whom?] as an adjunct to prophecy." <![CDATA[(<a href="#cwrc:727d97bc-af78-4122-94be-aa78b2e97d5a">DBpedia, 2017</a>)]]></skos:definition>
    <skos:definition xml:lang="fr">«Dans les religions abrahamiques, une prophétie consiste en des paroles ou des écrits divinement inspirés qu'une personne reçoit par révélation. Pour les chrétiens, le témoignage de Jésus est l'esprit de la prophétie (Apocalypse 19:10). Une prophétie peut avoir trait au passé, au présent ou à l'avenir. Quand une personne prophétise, elle dit ou écrit ce que Dieu veut qu'elle sache, pour son propre bien ou pour le bien des autres. La prophétie n'est pas l'apanage des prophètes. Une personne peut recevoir une prophétie ou une révélation pour sa vie personnelle.» <![CDATA[(<a href="#cwrc:727d97bc-af78-4122-94be-aa78b2e97d5a">DBpedia, 2017</a>)]]></skos:definition>
    <rdfs:label xml:lang="en">prophecy</rdfs:label>
    <rdfs:comment xml:lang="en">The description for this term is indebted to DBpedia. </rdfs:comment>
    <owl:sameAs rdf:resource="http://id.loc.gov/authorities/genreForms/gf2015026059"/>
  </genre:ReligiousGenre>
  <genre:NovelisticGenre rdf:about="http://sparql.cwrc.ca/ontologies/genre#sentimental">
    <skos:definition xml:lang="fr">Le XIXe siècle est marqué par la formidable expansion de la presse et des technologies de la communication. La production s’accélère dans tous les secteurs de la culture : la musique, les spectacles, bientôt le cinéma. Un public de nouveaux lecteurs émerge. L’Angleterre est un des premiers pays à faire du livre un objet destiné au grand public. Publié en 1740, Pamela, ou la Vertu récompensée de Samuel Richardson, roman d'amour à succès, est un des premiers best-sellers, avec cinq éditions imprimées en onze mois. De son côté, Jane Austen est considérée comme l'un des précurseurs du genre avec Orgueil et Préjugés, paru en 1813. En France, l’apparition du roman-feuilleton à partir de 1840 marque la naissance du roman populaire. Le roman sentimental se développe dans le dernier quart du XIXe siècle, lorsque l’Église s’alarme du goût du peuple alphabétisé pour la lecture de romans. Elle choisit alors de l’encadrer. Les feuilletons issus des périodiques tels que Les Veillées des chaumières ou Le Petit Écho de la mode proposent alors un roman d’amour qui élève l’âme et l’esprit. M. Maryan a ainsi écrit plus de quatre-vingt-dix-sept romans d’éducation. Toujours optimistes, ces ouvrages préparent les jeunes filles au mariage. Le roman sentimental connaît un large développement après la Première Guerre mondiale. Les principaux éditeurs en sont Joseph Ferenczi, Jules Tallandier et Jules Rouff. Ils produisent de multiples collections de petits romans : petits par le format, la pagination et le coût modique. Jusque dans les années 1980, la Librairie Jules Tallandier restera un des éditeurs majeurs dans ce domaine. Elle va codifier la littérature sentimentale, destinée à exprimer une vision enchantée de l’existence. Les Delly, pseudonyme des frère et sœur Frédéric et Jeanne-Marie Petitjean, sont des auteurs emblématiques du genre.</skos:definition>
    <owl:sameAs rdf:resource="http://dbpedia.org/resource/Sentimental_novel"/>
    <rdfs:comment xml:lang="en">This term and its description were created from data gathered from Encyclopaedia Universalis.</rdfs:comment>
    <owl:sameAs rdf:resource="http://id.loc.gov/authorities/genreForms/gf2014026536"/>
    <rdf:type rdf:resource="http://sparql.cwrc.ca/ontologies/genre#ThematicWritingGenre"/>
    <rdfs:label xml:lang="fr">littérature sentimentale</rdfs:label>
    <skos:definition xml:lang="en">"The sentimental novel or the novel of sensibility is an 18th-century literary genre which celebrates the emotional and intellectual concepts of sentiment, sentimentalism, and sensibility. Sentimentalism, which is to be distinguished from sensibility, was a fashion in both poetry and prose fiction beginning in the eighteenth century in reaction to the rationalism of the Augustan Age. Sentimental novels relied on emotional response, both from their readers and characters. They feature scenes of distress and tenderness, and the plot is arranged to advance both emotions and actions. The result is a valorization of "fine feeling," displaying the characters as a model for refined, sensitive emotional effect. The ability to display feelings was thought to show character and experience, and to shape social life and relations." <![CDATA[(<a href="#cwrc:727d97bc-af78-4122-94be-aa78b2e97d5a">DBpedia, 2017</a>)]]></skos:definition>
    <rdfs:label xml:lang="en">sentimental</rdfs:label>
  </genre:NovelisticGenre>
  <genre:ThreeDimensionalMedium rdf:about="http://sparql.cwrc.ca/ontologies/genre#realia">
    <rdfs:label xml:lang="en">realia</rdfs:label>
  </genre:ThreeDimensionalMedium>
  <genre:IllustratedForm rdf:about="http://sparql.cwrc.ca/ontologies/genre#comicbook">
    <owl:sameAs rdf:resource="http://vocab.getty.edu/aat/300203177"/>
    <owl:sameAs rdf:resource="http://id.loc.gov/authorities/genreForms/gf2014026266"/>
    <rdfs:label xml:lang="en">comicbook</rdfs:label>
    <skos:definition xml:lang="fr">" Séquence d'illustrations contenant une ou des histoires (appelées «comics», car certaines sont humoristiques), souvent sérialisées et publiées sous forme de brochure."</skos:definition>
    <skos:definition xml:lang="en">"Sequence of illustrations containing a story or stories (called "comics," because some are humorous), often serialized, published in booklet form." <![CDATA[(<a href="#cwrc:db2f8571-a773-4068-a35f-34262950bb8f">Getty, 2017</a>)]]></skos:definition>
    <rdfs:comment xml:lang="en">The description for this term is indebted to the Getty Art &amp; Architecture Thesaurus.</rdfs:comment>
    <rdfs:label xml:lang="fr">bande dessinée</rdfs:label>
  </genre:IllustratedForm>
  <genre:ComedicGenre rdf:about="http://sparql.cwrc.ca/ontologies/genre#comedyOfIntrigue">
    <rdfs:comment xml:lang="en">This term and its description were created from data gathered from the Penguin Dictionary of Literary Terms &amp; Literary Theory, 4th ed.</rdfs:comment>
    <skos:definition xml:lang="en">"A dramatic form popularized in the 16th century in which the comedy depends on complex plots, surprising twists, and ridiculous situations. The characters and their development tend to be secondary to plot in importance." <![CDATA[(<a href="#cwrc:2f09376c-f784-4a46-9f04-5a21aa311f27">Penguin, 1999</a>)]]></skos:definition>
    <rdfs:label xml:lang="en">comedy of intrigue</rdfs:label>
    <rdfs:label xml:lang="fr">comédie d'intrigue</rdfs:label>
    <skos:definition xml:lang="fr">Genre de comédie rendue populaire au 16ème siècle, dans laquelle la pièce repose sur des intrigues complexes, des revirement surprenants et des situations ridicules. Les personnages et leur développement ont généralement une importance seconde par rapport à l'intrigue.</skos:definition>
  </genre:ComedicGenre>
  <genre:PoeticGenre rdf:about="http://sparql.cwrc.ca/ontologies/genre#georgic">
    <rdfs:label xml:lang="fr">géorgique</rdfs:label>
    <skos:definition xml:lang="en">"Poetry about rural life that gives practical advice on the subject of agriculture. Unlike pastoral poetry, it does not portray the countryside as an idyllic escape, but rather focuses on the necessity of outdoor labour." <![CDATA[(<a href="#cwrc:4c227091-6bf0-4325-b846-9733fae19e61">Oxford, 2015</a>)]]></skos:definition>
    <rdfs:comment xml:lang="en">This term and its description were created from data gathered from the Oxford Dictionary of Literary Terms, 4th ed.</rdfs:comment>
    <rdfs:label xml:lang="en">georgic</rdfs:label>
    <skos:definition xml:lang="fr">Poésie à propos de la vie rurale qui donne des conseils pratiques au sujet de l'agriculture. Contrairement à la poésie pastorale, elle ne dépeint pas la campagne comme une lieu d'évasion idyllique, mais se concentre plutôt sur la nécessité du travail extérieur.</skos:definition>
    <dcterms:references rdf:resource="http://www.oxfordreference.com/view/10.1093/acref/9780199208272.001.0001/acref-9780199208272-e-496?rskey=qEr6Vu%26result=491"/>
  </genre:PoeticGenre>
  <genre:FictionalGenre rdf:about="http://sparql.cwrc.ca/ontologies/genre#shortStory">
    <rdfs:label xml:lang="fr">nouvelle</rdfs:label>
    <owl:sameAs rdf:resource="http://id.loc.gov/authorities/genreForms/gf2014026542"/>
    <skos:definition xml:lang="en">"Relatively brief invented prose narratives." <![CDATA[(<a href="#cwrc:db2f8571-a773-4068-a35f-34262950bb8f">Getty, 2017</a>)]]></skos:definition>
    <rdfs:label xml:lang="en">short story</rdfs:label>
    <rdfs:comment xml:lang="en">The description for this term is indebted to the Getty Art &amp; Architecture Thesaurus.</rdfs:comment>
    <owl:sameAs rdf:resource="http://vocab.getty.edu/aat/300202607"/>
    <skos:definition xml:lang="fr">«Une nouvelle est un récit habituellement court. Apparu à la fin du Moyen Âge, ce genre littéraire était alors proche du roman et d'inspiration réaliste, se distinguant peu du conte. À partir du XIXe siècle, les auteurs ont progressivement développé d'autres possibilités du genre, en s'appuyant sur la concentration de l'histoire pour renforcer l'effet de celle-ci sur le lecteur, par exemple par un dénouement surprenant. Les thèmes se sont également élargis : la nouvelle est devenue une forme privilégiée de la littérature fantastique, policière, et de science-fiction.» <![CDATA[(<a href="#cwrc:727d97bc-af78-4122-94be-aa78b2e97d5a">DBpedia, 2017</a>)]]></skos:definition>
  </genre:FictionalGenre>
  <genre:PoeticGenre rdf:about="http://sparql.cwrc.ca/ontologies/genre#apology">
    <dcterms:references rdf:resource="http://www.oxfordreference.com/view/10.1093/acref/9780199208272.001.0001/acref-9780199208272-e-81?rskey=cEhQEO%26result=81"/>
    <skos:definition xml:lang="fr">«Dans son sens originel, l'apologie est un genre littéraire visant à argumenter en défense contre les attaques visant une personne ou une doctrine. L'Apologie de Socrate est un exemple du genre, où Platon met en scène Socrate se défendant lui-même lors du procès qui déboucha sur sa condamnation à mort. Utilisée dans l'Antiquité par des orateurs et des avocats, l'apologie est aussi un moyen de réagir à des attaques publiques.» <![CDATA[(<a href="#cwrc:727d97bc-af78-4122-94be-aa78b2e97d5a">DBpedia, 2017</a>)]]></skos:definition>
    <rdfs:label xml:lang="fr">apologie</rdfs:label>
    <skos:definition xml:lang="en">"A text in which a writer defends the possibly controversial opinions contained in his or her writing." <![CDATA[(<a href="#cwrc:4c227091-6bf0-4325-b846-9733fae19e61">Oxford, 2015</a>)]]></skos:definition>
    <rdfs:label xml:lang="en">apology</rdfs:label>
    <rdfs:comment xml:lang="en">This term and its description were created from data gathered from DBpedia.</rdfs:comment>
  </genre:PoeticGenre>
  <genre:PoeticGenre rdf:about="http://sparql.cwrc.ca/ontologies/genre#freeVerse">
    <owl:sameAs rdf:resource="http://id.loc.gov/authorities/genreForms/gf2014026348"/>
    <rdfs:label xml:lang="en">free verse</rdfs:label>
  </genre:PoeticGenre>
  <genre:MusicalNotationForm rdf:about="http://sparql.cwrc.ca/ontologies/genre#notatedMusic">
    <rdfs:label xml:lang="en">notated music</rdfs:label>
  </genre:MusicalNotationForm>
  <genre:MusicalGenre rdf:about="http://sparql.cwrc.ca/ontologies/genre#ballade">
    <owl:sameAs rdf:resource="http://dbpedia.org/resource/Ballade_(classical_music)"/>
    <rdfs:comment xml:lang="fr">La description de ce terme est basée sur celle de DBPedia.</rdfs:comment>
    <rdfs:label xml:lang="en">ballade</rdfs:label>
    <skos:definition xml:lang="en">"A ballade (from French ballade, [baˈlad], and German Ballade, [baˈlaːdə], both being words for "ballad"), in classical music since the late 18th century, refers to a setting of a literary ballad, a narrative poem, in the musical tradition of the Lied, or to a one-movement instrumental piece with lyrical and dramatic narrative qualities reminiscent of such a song setting, especially a piano ballad." <![CDATA[(<a href="#cwrc:727d97bc-af78-4122-94be-aa78b2e97d5a">DBpedia, 2017</a>)]]></skos:definition>
    <rdfs:label xml:lang="fr">ballade</rdfs:label>
    <rdfs:comment xml:lang="en">The description for this term is indebted to DBpedia. </rdfs:comment>
    <skos:definition xml:lang="fr">«Ballade désigne, au sens ancien, un poème médiéval à forme fixe composé de trois couplets et d'une demi-strophe appelée envoi, chacune étant terminée par un vers refrain, qui rappelle la forme chantée des origines. L'histoire de la poésie retient en particulier les ballades aux strophes carrées (le nombre de vers est égal au nombre de syllabes de chaque vers) de huit ou dix vers et aux thèmes très variés qu'ont composées des poètes comme Guillaume de Machaut, Eustache Deschamps (fin XIVe siècle), Christine de Pisan et François Villon (début et milieu du XVe siècle) ou encore Clément Marot au XVIe, alors que la Pléiade rejette le genre de la ballade comme vieilli, privilégiant des formes nouvelles comme le sonnet ou l'ode.» <![CDATA[(<a href="#cwrc:727d97bc-af78-4122-94be-aa78b2e97d5a">DBpedia, 2017</a>)]]></skos:definition>
  </genre:MusicalGenre>
  <genre:BookForm rdf:about="http://sparql.cwrc.ca/ontologies/genre#sketchBook">
    <owl:sameAs rdf:resource="http://id.loc.gov/authorities/genreForms/gf2017027262"/>
    <skos:definition xml:lang="en">"Books or pads of blank sheets used or intended for sketching, which are informal or rough drawings." <![CDATA[(<a href="#cwrc:db2f8571-a773-4068-a35f-34262950bb8f">Getty, 2017</a>)]]></skos:definition>
    <rdfs:label xml:lang="fr">carnet de croquis</rdfs:label>
    <skos:definition xml:lang="fr">«Un carnet de croquis est un carnet utilisé par les dessinateurs, peintres et graveurs pour exécuter dessins et esquisses hors de leur atelier. Il peut être utilisé pour une modeste création ou pour préparer l’exécution d'une œuvre plus complexe. Généralement, le carnet de croquis est utilisé avec les outils de dessin : crayons, feutres, mine de plomb, pierre noire, aquarelle ou gouache. C'est souvent une ressource recherchée en histoire de l'art, pour comprendre le cheminement d'un artiste dans une œuvre ; points de passage, modèles qui inspireront les éléments de composition de l'œuvre finale.» <![CDATA[(<a href="#cwrc:727d97bc-af78-4122-94be-aa78b2e97d5a">DBpedia, 2017</a>)]]></skos:definition>
    <rdfs:label xml:lang="en">sketch book</rdfs:label>
    <rdfs:comment xml:lang="en">This term and its description were created from data gathered from DBpedia.</rdfs:comment>
    <owl:sameAs rdf:resource="http://dbpedia.org/resource/Sketchbook"/>
  </genre:BookForm>
  <genre:DigitalMedium rdf:about="http://sparql.cwrc.ca/ontologies/genre#videoGame">
    <rdfs:label xml:lang="en">video game</rdfs:label>
    <skos:related rdf:resource="http://vocab.getty.edu/aat/300256888"/>
  </genre:DigitalMedium>
  <genre:ReferenceWorkGenre rdf:about="http://sparql.cwrc.ca/ontologies/genre#thesaurus">
    <owl:sameAs rdf:resource="http://id.loc.gov/authorities/genreForms/gf2014026195"/>
    <rdfs:label xml:lang="en">thesaurus</rdfs:label>
    <rdfs:label xml:lang="fr">thesaurus</rdfs:label>
    <owl:sameAs rdf:resource="http://dbpedia.org/resource/Thesaurus"/>
    <rdfs:comment xml:lang="en">This term and its description were created from data gathered from the Getty Art &amp; Architecture Thesaurus.</rdfs:comment>
    <skos:definition xml:lang="fr">«Synonyme de Dictionnaire (Dictionarium) : Dictionnarium seu Thesaurus... du XVI° au XVII ° s. À la Renaissance, le thesaurus, venant du grec thesauros, et traduction latine du mot trésor, est un dictionnaire de mots dans les langues anciennes, le mot trésor étant réservé à la langue alors contemporaine, le français. Les premiers thesaurus furent ceux des Estienne, Robert Estienne, imprimeur et libraire du Roi, et Henri Estienne, et voisins des dictionnaires de grec et de latin comme le Dictionnarium Latino-Gallicum (1538), le Dictionnaire françois-latin, (1540). Ce nom a peut-être été emprunté à Hésiode, « La langue est un trésor de mots » car le mot thesaurus existait déjà dans le domaine de l'encyclopédie dans la littérature médiévale (voir Thesaurus:homonymie) ou signifiant comme aujourd’hui un recueil de textes.» <![CDATA[(<a href="#cwrc:727d97bc-af78-4122-94be-aa78b2e97d5a">DBpedia, 2017</a>)]]></skos:definition>
    <skos:definition xml:lang="en">"A semantic network of unique concepts, including relationships between synonyms, broader and narrower contexts, and other related concepts. Thesauri may be monolingual or multilingual. Thesauri may have the following three relationships between terms: equivalence (synonyms), hierarchical (whole/part), and associative (various types of other relationships)." <![CDATA[(<a href="#cwrc:db2f8571-a773-4068-a35f-34262950bb8f">Getty, 2017</a>)]]></skos:definition>
  </genre:ReferenceWorkGenre>
  <genre:SerialForm rdf:about="http://sparql.cwrc.ca/ontologies/genre#newspaper">
    <rdfs:label xml:lang="en">newspaper</rdfs:label>
    <skos:related rdf:resource="http://vocab.getty.edu/aat/300026656"/>
  </genre:SerialForm>
  <genre:AutobiographicalGenre rdf:about="http://sparql.cwrc.ca/ontologies/genre#diary">
    <rdfs:label xml:lang="fr">journal intime</rdfs:label>
    <rdfs:comment xml:lang="en">The description for this term is indebted to the Getty Art &amp; Architecture Thesaurus.</rdfs:comment>
    <owl:sameAs rdf:resource="http://vocab.getty.edu/aat/300027112"/>
    <owl:sameAs rdf:resource="http://id.loc.gov/authorities/genreForms/gf2014026085"/>
    <skos:definition xml:lang="fr">"Désigne les livres contenant les comptes rendus journaliers et personnels des expériences, états d'esprit et observations de l'auteur. Utiliser journaux (comptes rendus)" lorsqu'on se réfère au compte rendus d'évènements et de transactions d'un individu ou d'une organisation.  "</skos:definition>
    <skos:definition xml:lang="en">"Refers to books containing the daily, personal accounts of the writer's own experiences, attitudes, and observations. Use "journals (accounts)" when referring to an individual's or an organization's account of occurrences or transactions." <![CDATA[(<a href="#cwrc:db2f8571-a773-4068-a35f-34262950bb8f">Getty, 2017</a>)]]></skos:definition>
    <rdfs:label xml:lang="en">diary</rdfs:label>
  </genre:AutobiographicalGenre>
  <genre:ComedicGenre rdf:about="http://sparql.cwrc.ca/ontologies/genre#comedyOfMenace">
    <skos:definition xml:lang="fr">Type de drame comique dans lequel l'humour noir dérive de la peur, irrationnelle ou non, des personnages principaux en réponse à la menace de quelque force obscure.</skos:definition>
    <rdfs:comment xml:lang="en">This term and its description were created from data gathered from the Penguin Dictionary of Literary Terms &amp; Literary Theory, 4th ed.</rdfs:comment>
    <skos:definition xml:lang="en">"A type of comedic drama in which the dark humour stems from the main characters’ fear, irrational or not, that some dark force threatens them." <![CDATA[(<a href="#cwrc:2f09376c-f784-4a46-9f04-5a21aa311f27">Penguin, 1999</a>)]]></skos:definition>
    <rdfs:label xml:lang="fr">comédie de menace</rdfs:label>
    <rdfs:label xml:lang="en">comedy of menace</rdfs:label>
  </genre:ComedicGenre>
  <genre:NarrativeGenre rdf:about="http://sparql.cwrc.ca/ontologies/genre#folkTale">
    <skos:altLabel xml:lang="en">folklore</skos:altLabel>
    <rdfs:label xml:lang="en">folk tale</rdfs:label>
  </genre:NarrativeGenre>
  <genre:FictionalGenre rdf:about="http://sparql.cwrc.ca/ontologies/genre#dreamVision">
    <rdfs:label xml:lang="fr">vision onirique</rdfs:label>
    <rdfs:comment xml:lang="en">This term and its description were created from data gathered from the Oxford Dictionary of Literary Terms, 4th ed.</rdfs:comment>
    <skos:definition xml:lang="en">"Literature, typically a poem and frequently an allegory or symbolic tale, in which the plot is a dream recounted by a narrator who dreamed it." <![CDATA[(<a href="#cwrc:4c227091-6bf0-4325-b846-9733fae19e61">Oxford, 2015</a>)]]></skos:definition>
    <rdfs:label xml:lang="en">dream vision</rdfs:label>
    <skos:definition xml:lang="fr">Forme littéraire, souvent sous forme de poème allégorique ou de conte symbolique, dans lequel l'intrigue est le rêve du narrateur.</skos:definition>
    <dcterms:references rdf:resource="http://www.oxfordreference.com/view/10.1093/acref/9780199208272.001.0001/acref-9780199208272-e-351?rskey=MMt5zw%26result=351"/>
  </genre:FictionalGenre>
  <genre:SerialForm rdf:about="http://sparql.cwrc.ca/ontologies/genre#fascicle">
    <owl:sameAs rdf:resource="http://vocab.getty.edu/aat/300265628"/>
    <rdfs:label xml:lang="en">fascicle</rdfs:label>
  </genre:SerialForm>
  <genre:FictionalGenre rdf:about="http://sparql.cwrc.ca/ontologies/genre#fantasy">
    <skos:definition xml:lang="fr">La fantasy, ou fantasie (terme issu de l’anglais fantasy : « imagination » ; à ne pas confondre avec la fantaisie musicale, ni avec le terme allemand phantasie qui désigne le concept psychologique de fantasme), est un genre littéraire présentant un ou plusieurs éléments surnaturels qui relèvent souvent du mythe et qui sont souvent incarnés par l’irruption ou l’utilisation de la magie. La fantasy fait partie des littératures de l'imaginaire. Dans la fantasy comme dans le merveilleux, le surnaturel est généralement accepté, voire utilisé pour définir les règles d'un monde imaginaire, et n'est pas nécessairement objet de doute ou de peur. Cela distingue la fantasy du fantastique où le surnaturel fait intrusion dans les règles du monde habituel, et de l'horreur où il suscite peur et angoisse. Par extension, à partir du genre littéraire, on parle aussi de fantasy à propos d'illustrations, de bandes dessinées, de films, de jeux, etc.</skos:definition>
    <owl:sameAs rdf:resource="http://vocab.getty.edu/aat/300380290"/>
    <rdfs:comment xml:lang="en">The description for this term is indebted to DBpedia. </rdfs:comment>
    <skos:definition xml:lang="en">"Literary genre in which works are of a whimsical or visionary nature, having suppositions that are speculation or resting on no solid grounds." <![CDATA[(<a href="#cwrc:db2f8571-a773-4068-a35f-34262950bb8f">Getty, 2017</a>)]]></skos:definition>
    <rdfs:label xml:lang="en">fantasy</rdfs:label>
  </genre:FictionalGenre>
  <genre:ReligiousGenre rdf:about="http://sparql.cwrc.ca/ontologies/genre#sermon">
    <rdfs:label xml:lang="en">sermon</rdfs:label>
    <skos:definition xml:lang="en">"A sermon is an oration, lecture, or talk by a member of a religious institution or clergy. Sermons address a Biblical, theological, religious, or moral topic, usually expounding on a type of belief, law or behavior within both past and present contexts. Elements of the sermon often include exposition, exhortation and practical application. In Christianity, a sermon (also known as a homily within some churches) is usually delivered in a place of worship from an elevated architectural feature, variously known as a pulpit, a lectern, or an ambo. The word "sermon" comes from a Middle English word which was derived from Old French, which in turn came from the Latin word sermō meaning "discourse". The word can mean "conversation", which could mean that early sermons were delivered in the form of question and answer, and that only later did it come to mean a monologue. However, the Bible contains many speeches without interlocution, which some take to be sermons: Moses in Deuteronomy 1-33 ; Jesus' sermon on the mount in Matthew 5-7 (though the gospel writers do not specifically call it a sermon; the popular descriptor for Christ's speech there came much later); Peter after Pentecost in Acts 2:14-40 (though this speech was delivered to nonbelievers and as such is not quite parallel to the popular definition of a sermon). In modern language, the word "sermon" is used in secular terms, pejoratively, to describe a lengthy or tedious speech delivered with great passion, by any person, to an uninterested audience. A sermonette is a short sermon (usually associated with television broadcasting, as stations would present a sermonette before signing off for the night)." <![CDATA[(<a href="#cwrc:727d97bc-af78-4122-94be-aa78b2e97d5a">DBpedia, 2017</a>)]]></skos:definition>
    <rdfs:comment xml:lang="en">The description for this term is indebted to DBpedia. </rdfs:comment>
    <owl:sameAs rdf:resource="http://dbpedia.org/resource/Sermon"/>
    <skos:definition xml:lang="fr">«Le sermon est un discours de prédication prononcé dans des circonstances religieuses.» <![CDATA[(<a href="#cwrc:727d97bc-af78-4122-94be-aa78b2e97d5a">DBpedia, 2017</a>)]]></skos:definition>
    <owl:sameAs rdf:resource="http://id.loc.gov/authorities/genreForms/gf2015026051"/>
  </genre:ReligiousGenre>
  <genre:PoeticGenre rdf:about="http://sparql.cwrc.ca/ontologies/genre#graveyardPoetry">
    <owl:sameAs rdf:resource="http://id.loc.gov/authorities/genreForms/gf2014026364"/>
    <rdfs:label xml:lang="en">graveyard poetry</rdfs:label>
    <rdfs:label xml:lang="fr">graveyard poetry</rdfs:label>
    <rdfs:comment xml:lang="en">This term and its description were created from data gathered from the Oxford Dictionary of Literary Terms, 4th ed.</rdfs:comment>
    <dcterms:references rdf:resource="http://www.oxfordreference.com/view/10.1093/acref/9780199208272.001.0001/acref-9780199208272-e-511?rskey=ejri5r%26result=511"/>
    <skos:definition xml:lang="en">"An 18th-century poetic form dealing with the subjects of death and immortality. The name originates from the setting typical of these poems: the graveyard." <![CDATA[(<a href="#cwrc:4c227091-6bf0-4325-b846-9733fae19e61">Oxford, 2015</a>)]]></skos:definition>
    <skos:definition xml:lang="fr">Mouvement poétique rattaché au romantisme britannique du 18ème siècle, traitant de la mort et de l'immortalité. Le nom provient du cadre habituel décrit et traité dans ces poèmes, le cimetière.</skos:definition>
  </genre:PoeticGenre>
  <genre:InformationalGenre rdf:about="http://sparql.cwrc.ca/ontologies/genre#documentary">
    <skos:definition xml:lang="fr">Enregistrements écrits, oraux, sonores ou photographiques, ou représentations dans d'autres média qui expliquent ou recréent des événements réels, des épisodes, des histoires de vie ou d'autres informations factuelles d'une façon qui se veut objective et précise.</skos:definition>
    <skos:definition xml:lang="en">"Written, oral, sound, or photographic recordings, or presentations in other media that explain or re-create actual events, eras, life stories, or other factual information in a manner purporting to be objective and accurate." <![CDATA[(<a href="#cwrc:db2f8571-a773-4068-a35f-34262950bb8f">Getty, 2017</a>)]]></skos:definition>
    <rdfs:label xml:lang="en">documentary</rdfs:label>
    <rdfs:label xml:lang="fr">documentaire</rdfs:label>
    <rdfs:comment xml:lang="en">This term and its description were created from data gathered from the Getty Art &amp; Architecture Thesaurus.</rdfs:comment>
    <owl:sameAs rdf:resource="http://vocab.getty.edu/aat/300249172"/>
  </genre:InformationalGenre>
  <genre:NarrativeGenre rdf:about="http://sparql.cwrc.ca/ontologies/genre#myth">
    <rdfs:label xml:lang="en">myth</rdfs:label>
    <rdfs:comment xml:lang="en">The description for this term is indebted to the Getty Art &amp; Architecture Thesaurus.</rdfs:comment>
    <skos:definition xml:lang="en">"Legendary stories without a determinable basis of fact or natural explanation, typically concerning a being, hero, deity, or event and explains some practice, rite, or phenomenon of nature." <![CDATA[(<a href="#cwrc:db2f8571-a773-4068-a35f-34262950bb8f">Getty, 2017</a>)]]></skos:definition>
    <skos:definition xml:lang="fr">«Un mythe est un récit qui se veut explicatif et surtout fondateur d'une pratique sociale. Il est porté à l'origine par une tradition orale, qui propose une explication pour certains aspects fondamentaux du monde et de la société qui a forgé ou qui véhicule ces mythes : L'étude des mythes est appelée mythologie. Le terme mythe est souvent employé pour désigner une croyance manifestement erronée au premier abord, mais qui peut se rapporter à des éléments concrets exprimés de façon symbolique et partagée par un nombre significatif de personnes. Le mythe se distingue de la légende (qui suppose quelques faits historiques identifiables), du conte (qui se veut inventif sans expliquer), et du roman (qui "explique" avec peu de fondements).» <![CDATA[(<a href="#cwrc:727d97bc-af78-4122-94be-aa78b2e97d5a">DBpedia, 2017</a>)]]></skos:definition>
    <owl:sameAs rdf:resource="http://dbpedia.org/resource/Myth"/>
  </genre:NarrativeGenre>
  <genre:ReligiousGenre rdf:about="http://sparql.cwrc.ca/ontologies/genre#hagiography">
    <rdfs:label xml:lang="en">hagiography</rdfs:label>
    <owl:sameAs rdf:resource="http://id.loc.gov/authorities/genreForms/gf2015026032"/>
    <skos:definition xml:lang="en">"Saints' lives as a branch of literature or legend." <![CDATA[(<a href="#cwrc:db2f8571-a773-4068-a35f-34262950bb8f">Getty, 2017</a>)]]></skos:definition>
    <skos:definition xml:lang="fr">«L’hagiographie (du grec ancien ἅγιος / hágios (« saint ») et γράφειν / gráphein (« écrire »)) est l'écriture de la vie et / ou de l'œuvre des saints. Pour un texte particulier, on ne parle que rarement d'« une hagiographie » (sauf dans le sens figuré), mais plutôt d'un texte hagiographique ou tout simplement d'une vie de saint. Le texte hagiographique étant destiné à être lu, soit lors de l'office des moines soit en public dans le cadre de la prédication, on lui donne souvent le nom de légende (du latin legenda, « ce qui doit être lu », terme utilisé dans son acception la plus littérale et non dans son sens péjoratif actuel de récit dépourvu de tout enracinement dans l'histoire événementielle). Un texte hagiographique recouvre plusieurs genres littéraires ou artistiques parmi lesquels on compte en premier lieu la vita, c'est-à-dire le récit biographique de la vie du saint. Une fresque à épisode est également une hagiographie, de même qu'une simple notice résumant la vie du bienheureux. Par rapport à une biographie, l'hagiographie est un genre littéraire qui veut mettre en avant le caractère de sainteté du personnage dont on raconte la vie. L'écrivain, l'hagiographe n'a pas d'abord une démarche d'historien, surtout lorsque le genre hagiographique s'est déployé. Aussi les hagiographies anciennes sont parsemées de passages merveilleux à l'historicité douteuse. De plus, des typologies de saints existaient au Moyen Âge, ce qui a conduit les hagiographes à se conformer à ces modèles et à faire de nombreux emprunts à des récits antérieurs. L'hagiographie est ainsi un récit fortement stéréotypé dont la fonction pastorale est de servir à l'instruction et l'édification religieuse, mais qui peut avoir aussi une fonction normative, politique et de propagande religieuse. D'une manière plus polémique, on parle aussi d'hagiographie pour désigner un écrit (une biographie, l'analyse d'un système philosophique, etc.) trop favorable à son objet, c'est-à-dire manquant de recul et/ou ne laissant guère de place à la critique.» <![CDATA[(<a href="#cwrc:727d97bc-af78-4122-94be-aa78b2e97d5a">DBpedia, 2017</a>)]]></skos:definition>
    <owl:sameAs rdf:resource="http://vocab.getty.edu/aat/300055909"/>
    <rdfs:comment xml:lang="en">The description for this term is indebted to DBpedia. </rdfs:comment>
  </genre:ReligiousGenre>
  <genre:ThematicWritingGenre rdf:about="http://sparql.cwrc.ca/ontologies/genre#diasporic">
    <rdfs:label xml:lang="en">diasporic</rdfs:label>
    <skos:altLabel xml:lang="en">diaspora</skos:altLabel>
  </genre:ThematicWritingGenre>
  <genre:ThematicWritingGenre rdf:about="http://sparql.cwrc.ca/ontologies/genre#performance">
    <rdfs:label xml:lang="en">performance</rdfs:label>
    <rdf:type rdf:resource="http://sparql.cwrc.ca/ontologies/genre#PerformanceMedium"/>
    <skos:definition xml:lang="en">A capacious and contested category of time-based and usually embodied human expression through actions or processes that may occur in institutionalized locations, more informal cultural contexts, and broader social situations, as in the performance of social identities.  Most often applied to literary, artistic, musical, theatrical, or other creative work, or the representation or record of such work. Within the Records of Early English Drama project, "Performance has been broadly defined to encompass nearly every mimetic, musical, or ritualistic form of play used to entertain or otherwise engage an audience." <![CDATA[(<a href="https://ereed.library.utoronto.ca/about/series/#selection">REED Online, 2018</a>)]]></skos:definition>
    <rdfs:comment xml:lang="en">This term and its description were created from data gathered from the Getty Art &amp; Architecture Thesaurus.</rdfs:comment>
    <skos:closeMatch rdf:resource="http://vocab.getty.edu/page/aat/300054146"/>
    <rdfs:label xml:lang="fr">représentation</rdfs:label>
  </genre:ThematicWritingGenre>
  <genre:NarrativeGenre rdf:about="http://sparql.cwrc.ca/ontologies/genre#testimony">
    <skos:definition xml:lang="fr">Déclarations solennelles, écrites ou verbales, habituellement faites par un témoin sous serment dans le cadre d'une interrogatoire conduit par un avocat ou un représentant de la fonction publique, et ensuite retranscrit par écrit dans un compte rendu.</skos:definition>
    <rdfs:label xml:lang="fr">témoignage</rdfs:label>
    <rdfs:label xml:lang="en">testimony</rdfs:label>
    <owl:sameAs rdf:resource="http://vocab.getty.edu/aat/300027861"/>
    <rdfs:comment xml:lang="en">The description for this term is indebted to the Getty Art &amp; Architecture Thesaurus.</rdfs:comment>
    <skos:definition xml:lang="en">"Solemn declarations, written or verbal; usually made orally by a witness under oath in response to interrogation by a lawyer or authorized public official, then reduced to writing for the record." <![CDATA[(<a href="#cwrc:db2f8571-a773-4068-a35f-34262950bb8f">Getty, 2017</a>)]]></skos:definition>
  </genre:NarrativeGenre>
  <genre:PhilosophicalGenre rdf:about="http://sparql.cwrc.ca/ontologies/genre#feministTheory">
    <owl:sameAs rdf:resource="http://dbpedia.org/resource/Feminist_theory"/>
    <rdfs:label xml:lang="en">feminist theory</rdfs:label>
    <rdf:type rdf:resource="http://sparql.cwrc.ca/ontologies/genre#FeministGenre"/>
    <rdf:type rdf:resource="http://sparql.cwrc.ca/ontologies/genre#ScholarlyGenre"/>
    <skos:definition xml:lang="en">"Feminist theory is the extension of feminism into theoretical, fictional, or philosophical discourse. It aims to understand the nature of gender inequality. It examines women's and men's social roles, experience, interests, chores, and feminist politics in a variety of fields, such as anthropology and sociology, communication, psychoanalysis, home economics, literature, education, and philosophy." <![CDATA[(<a href="#cwrc:727d97bc-af78-4122-94be-aa78b2e97d5a">DBpedia, 2017</a>)]]></skos:definition>
    <owl:sameAs rdf:resource="https://en.wikipedia.org/wiki/Feminist_theory"/>
    <rdfs:label xml:lang="fr">théorie féministe</rdfs:label>
    <skos:definition xml:lang="fr">«La théorie féministe est un aspect du féminisme porté sur la théorisation et la réflexion philosophique. Son but est de comprendre la nature de l'inégalité entre les genres. Elle examine la place des femmes en faisant référence à des domaines des sciences sociales comme l'anthropologie, la sociologie, la communication, la psychanalyse, la philosophie, etc.» <![CDATA[(<a href="#cwrc:727d97bc-af78-4122-94be-aa78b2e97d5a">DBpedia, 2017</a>)]]></skos:definition>
  </genre:PhilosophicalGenre>
  <genre:FictionalGenre rdf:about="http://sparql.cwrc.ca/ontologies/genre#vignette">
    <rdfs:label xml:lang="fr">micronouvelle</rdfs:label>
    <skos:definition xml:lang="fr">«La micronouvelle (parfois aussi appelée microroman) est un récit imaginaire, suggestif, parfois caustique, rédigé en un nombre extrêmement restreint de mots. C'est la forme la plus concise de récit littéraire prosaïque, parfois proche du poème par le rythme qu'il imprime. L'ironie et l'interactivité qui la caractérisent la rattachent au postmodernisme en littérature. Elle est connue dans les littératures anglaise et hispanique sous les locutions micro-fiction, short-short story et microconte. La microfiction, aussi appelée nanofiction ou fiction éclair, est « l’ancêtre » de la micronouvelle. Adaptée à la littérature française, parfois sur Twitter (aussi dite « twittérature ») pour son fonctionnement aux nombres très limités de mots qui se prête parfaitement à la micronouvelle, par des auteurs comme Fuentealba, Berthiaume, Gechter, Bastin, Le Blanc et Fréchette, elle passe aujourd'hui sous la plume d'auteurs comme Thierry Crouzet, Bernard Pivot, Alexandre Jardin, et Michel Trembla»y<![CDATA[(<a href="#cwrc:727d97bc-af78-4122-94be-aa78b2e97d5a">DBpedia, 2017</a>)]]></skos:definition>
    <skos:definition xml:lang="en">"In theatrical script writing, sketch stories, and poetry, a vignette is a short impressionistic scene that focuses on one moment or gives a trenchant impression about a character, idea, setting, or object.[citation needed] This type of scene is more common in recent postmodern theater, where less emphasis is placed on adhering to the conventions of theatrical structure and story development. Vignettes have been particularly influenced by contemporary notions of a scene as shown in film, video and television scripting. It is also a part of something bigger than itself: for example, a vignette about a house belonging to a collection of vignettes or a whole story, such as The House On Mango Street, by Sandra Cisneros. A blog can provide a form of vignette." <![CDATA[(<a href="#cwrc:727d97bc-af78-4122-94be-aa78b2e97d5a">DBpedia, 2017</a>)]]></skos:definition>
    <owl:sameAs rdf:resource="http://dbpedia.org/resource/Vignette_(literature)"/>
    <rdfs:comment xml:lang="en">This term and its description were created from data gathered from DBpedia.</rdfs:comment>
    <rdfs:label xml:lang="en">vignette</rdfs:label>
  </genre:FictionalGenre>
  <genre:BookForm rdf:about="http://sparql.cwrc.ca/ontologies/genre#giftbook">
    <skos:definition xml:lang="en">"Books, usually illustrated literary anthologies, intended to be given as gifts and often published annually; popular in the 19th century. For works produced to mark an occasion, use "keepsakes (books)." <![CDATA[(<a href="#cwrc:db2f8571-a773-4068-a35f-34262950bb8f">Getty, 2017</a>)]]></skos:definition>
    <owl:sameAs rdf:resource="http://id.loc.gov/authorities/genreForms/gf2017026072"/>
    <skos:definition xml:lang="fr">Livres, généralement des anthologies littéraires illustrées publiées une fois par an, destinées à être offertes et populaires au 19ème siècle. Pour les oeuvres produites afin de marquer une occasion, utilisez "souvenirs" (livres).</skos:definition>
    <rdfs:label xml:lang="en">giftbook</rdfs:label>
    <rdfs:comment xml:lang="en">The description for this term is indebted to the Getty Art &amp; Architecture Thesaurus.</rdfs:comment>
    <owl:sameAs rdf:resource="http://vocab.getty.edu/aat/300202541"/>
    <rdfs:label xml:lang="fr">livre d'étrenne</rdfs:label>
  </genre:BookForm>
  <genre:OperaGenre rdf:about="http://sparql.cwrc.ca/ontologies/genre#libretto">
    <owl:sameAs rdf:resource="http://vocab.getty.edu/aat/300026424"/>
    <owl:sameAs rdf:resource="http://id.loc.gov/authorities/genreForms/gf2014026909"/>
    <rdfs:label xml:lang="en">libretto</rdfs:label>
    <skos:definition xml:lang="fr">«Un livret (de l'italien libretto, « petit livre ») ou libretto est, en musique, un texte littéraire, presque toujours en vers, complétant une œuvre musicale telle qu'un opéra, une opérette, un oratorio ou une comédie musicale. Publié sous forme d'opuscule séparé de la musique, il contient les dialogues chantés et les éventuels passages parlés, ainsi que de rapides indications de mise en scène. En danse, le livret est la brochure qui donne l'explication et l'argument d'une pantomime ou d'un ballet.» <![CDATA[(<a href="#cwrc:727d97bc-af78-4122-94be-aa78b2e97d5a">DBpedia, 2017</a>)]]></skos:definition>
    <rdfs:label xml:lang="fr">libretto</rdfs:label>
    <rdfs:comment xml:lang="en">The description for this term is indebted to the Getty Art &amp; Architecture Thesaurus.</rdfs:comment>
    <skos:definition xml:lang="en">"Books or booklets containing the text or words of an opera or similar extended musical composition." <![CDATA[(<a href="#cwrc:db2f8571-a773-4068-a35f-34262950bb8f">Getty, 2017</a>)]]></skos:definition>
  </genre:OperaGenre>
  <genre:DramaticGenre rdf:about="http://sparql.cwrc.ca/ontologies/genre#pantomime">
    <skos:definition xml:lang="en">"Pantomime (informally panto) is a type of musical comedy stage production, designed for family entertainment. It was developed in England and is still performed there, generally during the Christmas and New Year season and, to a lesser extent, in other English-speaking countries. Modern pantomime includes songs, slapstick comedy and dancing, employs gender-crossing actors, and combines topical humour with a story loosely based on a well-known fairy tale, fable or folk tale. It is a participatory form of theatre, in which the audience is expected to sing along with certain parts of the music and shout out phrases to the performers." <![CDATA[(<a href="#cwrc:727d97bc-af78-4122-94be-aa78b2e97d5a">DBpedia, 2017</a>)]]></skos:definition>
    <rdfs:comment xml:lang="en">This term and its description were created from data gathered from DBpedia.</rdfs:comment>
    <rdfs:label xml:lang="en">pantomime</rdfs:label>
    <skos:related rdf:resource="http://id.loc.gov/authorities/genreForms/gf2018026117"/>
    <rdfs:label xml:lang="fr">pantomime</rdfs:label>
    <skos:definition xml:lang="fr">Jeu, art du pantomime; technique d'expression dramatique suivant laquelle les situations, les sentiments, les idées sont rendus par des attitudes, des gestes, des jeux de physionomie, sans recours à la parole.</skos:definition>
    <owl:sameAs rdf:resource="https://dvlf.uchicago.edu/mot/pantomime"/>
  </genre:DramaticGenre>
  <genre:ThematicWritingGenre rdf:about="http://sparql.cwrc.ca/ontologies/genre#travelWriting">
    <rdfs:label xml:lang="en">travel writing</rdfs:label>
    <skos:definition xml:lang="en">Writing about time spent abroad, typically containing descriptions of the scenery and culture of places visited. Sometimes includes biographical content, such as travel literature written in the form of a personal journal or diary.</skos:definition>
    <rdfs:comment xml:lang="en">This term and its description were created from data gathered from Wikipedia.</rdfs:comment>
    <skos:closeMatch rdf:resource="https://fr.wikipedia.org/wiki/R%C3%A9cit_de_voyage"/>
    <rdfs:label xml:lang="fr">récit de voyage</rdfs:label>
    <skos:definition xml:lang="fr">Un récit de voyage ou relation de voyage est un genre littéraire dans lequel l'auteur rend compte d'un ou des voyages, des peuples rencontrés, des émotions ressenties, des choses vues et entendues. Contrairement au roman, le récit de voyage privilégie le réel à la fiction. Pour mériter le titre de « récit » et avoir rang de littérature, la narration doit être structurée et aller au-delà de la simple énumération des dates et des lieux (comme un journal intime ou un livre de bord d'un navire). Cette littérature doit rendre compte d'impressions, d'aventures, de l'exploration ou de la conquête de pays lointains.</skos:definition>
  </genre:ThematicWritingGenre>
  <genre:ThematicWritingGenre rdf:about="http://sparql.cwrc.ca/ontologies/genre#environmental">
    <rdfs:label xml:lang="en">environmental</rdfs:label>
  </genre:ThematicWritingGenre>
  <genre:PerformanceMedium rdf:about="http://sparql.cwrc.ca/ontologies/genre#cabaret">
    <dcterms:references rdf:resource="http://www.oxfordreference.com/view/10.1093/acref/9780199571123.001.0001/m_en_gb0114080?rskey=xIWuHx%26result=12581"/>
    <rdfs:label xml:lang="en">cabaret</rdfs:label>
    <skos:definition xml:lang="en">"Various forms of entertainment, often involving dancing, singing, or comedy acts, performed at a venue such as a nightclub in which the audience is seated at tables. Live music played in restaurants or public houses would not usually be considered cabaret without an additional component." <![CDATA[(<a href="#cwrc:4c227091-6bf0-4325-b846-9733fae19e61/">Oxford, 2015</a>)]]></skos:definition>
    <skos:definition xml:lang="fr">Formes de spectacles divers, incluant souvent de la danse, du chant ou de la comédie, représentés dans une salle de spectacle, généralement un cabaret, où le public est assis à des tables. La musique jouée dans les restaurants ou les tavernes n'est généralement pas considérée comme un spectacle de cabaret, à moins qu'elle présente des éléments distinctifs.</skos:definition>
    <rdfs:comment xml:lang="en">This term and its description were created from data gathered from the Oxford Dictionary of English, 3rd ed.</rdfs:comment>
    <rdfs:label xml:lang="fr">spectacle de cabaret</rdfs:label>
  </genre:PerformanceMedium>
  <genre:FictionalGenre rdf:about="http://sparql.cwrc.ca/ontologies/genre#legendFolktale">
    <rdfs:comment xml:lang="en">This term and its description were created from data gathered from the Getty Art &amp; Architecture Thesaurus.</rdfs:comment>
    <skos:definition xml:lang="en">"Stories that have been maintained over time, usually by a particular culture through an oral tradition. Often understood within originating cultures as historical accounts although they differ from Western record-keeping." <![CDATA[(<a href="#cwrc:db2f8571-a773-4068-a35f-34262950bb8f">Getty, 2017</a>)]]></skos:definition>
    <skos:altLabel xml:lang="en">folklore</skos:altLabel>
    <skos:related rdf:resource="http://id.loc.gov/authorities/genreForms/gf2014026344"/>
    <rdfs:label xml:lang="en">legend folktale</rdfs:label>
    <skos:definition xml:lang="fr">Histoires conservées au fil du temps, généralement transmise au sein d'une culture particulière par le biais de la tradition orale. Elles sont souvent interprétées comme des faits historiques dans les sociétés anciennes, même si elles diffèrent de la conception occidentale de l'Histoire.</skos:definition>
    <owl:sameAs rdf:resource="http://vocab.getty.edu/aat/300055922"/>
    <rdfs:label xml:lang="fr">légende conte folklorique</rdfs:label>
  </genre:FictionalGenre>
  <genre:PerformanceMedium rdf:about="http://sparql.cwrc.ca/ontologies/genre#puppetry">
    <skos:related rdf:resource="http://vocab.getty.edu/aat/300248147"/>
    <rdfs:label xml:lang="en">puppetry</rdfs:label>
  </genre:PerformanceMedium>
  <genre:PoeticGenre rdf:about="http://sparql.cwrc.ca/ontologies/genre#epithalamium">
    <owl:sameAs rdf:resource="http://id.loc.gov/authorities/genreForms/gf2014026317"/>
    <skos:definition xml:lang="en">"An epithalamiumLatin form of Greek (ἐπιθαλάμιον epithalamion from ἐπί epi "upon," and θάλαμος thalamos nuptial chamber) is a poem written specifically for the bride on the way to her marital chamber. This form continued in popularity through the history of the classical world; the Roman poet Catullus wrote a famous epithalamium, which was translated from or at least inspired by a now-lost work of Sappho. According to Origen, Song of Songs, might be an epithalamium on the marriage of Solomon with Pharaoh’s daughter." <![CDATA[(<a href="#cwrc:727d97bc-af78-4122-94be-aa78b2e97d5a">DBpedia, 2017</a>)]]></skos:definition>
    <skos:definition xml:lang="fr">«L'épithalame (en grec ancien ἐπιθαλάμιον / epithalámion) est une sorte de poème lyrique composé chez les Anciens à l'occasion d'un mariage et à la louange des nouveaux époux. En Grèce, il était chanté par un chœur, soit de jeunes vierges seules, soit de jeunes filles[réf. nécessaire] et de jeunes garçons, avec accompagnement de danses. On le nommait aussi catakoemèse (de catakoimân, envoyer dormir).» <![CDATA[(<a href="#cwrc:727d97bc-af78-4122-94be-aa78b2e97d5a">DBpedia, 2017</a>)]]></skos:definition>
    <rdfs:comment xml:lang="en">The description for this term is indebted to DBpedia. </rdfs:comment>
    <owl:sameAs rdf:resource="http://dbpedia.org/resource/Epithalamium"/>
    <rdfs:label xml:lang="en">epithalamium</rdfs:label>
  </genre:PoeticGenre>
  <genre:InformationalGenre rdf:about="http://sparql.cwrc.ca/ontologies/genre#cookbook">
    <rdfs:comment xml:lang="en">The description for this term is indebted to DBpedia. </rdfs:comment>
    <rdfs:label xml:lang="en">cookbook</rdfs:label>
    <skos:definition xml:lang="fr">«Un livre de cuisine est un recueil de recettes ou de considérations gastronomiques.» <![CDATA[(<a href="#cwrc:727d97bc-af78-4122-94be-aa78b2e97d5a">DBpedia, 2017</a>)]]></skos:definition>
    <owl:sameAs rdf:resource="http://id.loc.gov/authorities/genreForms/gf2011026169"/>
    <owl:sameAs rdf:resource="http://vocab.getty.edu/aat/300026109"/>
    <skos:definition xml:lang="en">"Reference publications containing collections of recipes with ancillary content on selection of ingredients or the broader context of the types of cooking presented. Contemporary cookbooks may  focus on cultural or regional themes." <![CDATA[(<a href="#cwrc:db2f8571-a773-4068-a35f-34262950bb8f">Getty, 2017</a>)]]></skos:definition>
  </genre:InformationalGenre>
  <genre:HistoricalGenre rdf:about="http://sparql.cwrc.ca/ontologies/genre#nationalTale">
    <rdf:type rdf:resource="http://sparql.cwrc.ca/ontologies/genre#NovelisticGenre"/>
    <skos:definition xml:lang="en">"A romantic genre developed in early nineteenth-century, particularly associated with Ireland and Scotland, in which historical content is woven into narratives treating such subjects as the formation or defence of a nation, political conflict with a bearing on nationhood, and national identity or culture." <![CDATA[(<a href="#cwrc:076686ab-eab5-4dcf-a6c0-4949d23feb5c">Foster, 2006</a>)]]></skos:definition>
    <rdfs:comment xml:lang="en">This term and its description were created from data gathered from The Cambridge Companion to the Irish Novel.</rdfs:comment>
    <rdfs:label xml:lang="en">national tale</rdfs:label>
    <dcterms:references rdf:resource="https://books.google.ca/books?id=b2uvkN2taiQC&amp;printsec=frontcover&amp;redir_esc=y#v=onepage&amp;q&amp;f=false"/>
    <skos:definition xml:lang="fr">Genre romantique développé au début du XIXe siècle, en particulier associé à l'Irlande et à l'Écosse, dans lequel la dimension historique s'inscrit dans des récits autour de sujets tels que la formation ou la défense d'une nation, ou le conflit politique à propos de la nationalité, de l'identité et de la culture nationale .</skos:definition>
    <rdfs:label xml:lang="fr">national tale</rdfs:label>
  </genre:HistoricalGenre>
  <genre:IntertextualGenre rdf:about="http://sparql.cwrc.ca/ontologies/genre#sequel">
    <skos:definition xml:lang="fr">«La suite d'une œuvre littéraire, cinématographique, télévisuelle, d'une bande dessinée ou d'un jeu vidéo, est une œuvre se déroulant dans le même univers de fiction que la première œuvre, et qui raconte une histoire ayant lieu après celle qui est narrée dans cette œuvre originelle.» <![CDATA[(<a href="#cwrc:727d97bc-af78-4122-94be-aa78b2e97d5a">DBpedia, 2017</a>)]]></skos:definition>
    <rdfs:label xml:lang="en">sequel</rdfs:label>
    <rdfs:comment xml:lang="en">This term and its description were created from data gathered from DBpedia.</rdfs:comment>
    <skos:definition xml:lang="en">"(from Latin sequi, to follow): A literary work complete in itself, but continuing the narrative of an earlier work. It is a new story that extends or develops characters and situations found in an earlier work. Two sequels following an original work (together) are called a trilogy. Three sequels following an original work together are called a tetralogy.Often sequels have a reputation for inferior artistry compared to the original publication since they are often hastily written from the desire to capitalize on earlier financial success. Examples include Mark Twain's Tom Sawyer Abroad, which is a sequel to The Adventures of Tom Sawyer, and Alexandra Ripley's Scarlett, which is a sequel to Mitchell's Gone With the Wind. In the late twentieth century, it became common retroactively to write "prequels," a later book with the same geographic setting or characters, but which takes place in an earlier time." <![CDATA[(<a href="cwrc:509015ff-7641-473e-94c5-688e06952bb7">L. K Wheeler, 2017</a>)]]></skos:definition>
    <owl:sameAs rdf:resource="http://dbpedia.org/resource/Sequel"/>
    <rdfs:label xml:lang="fr">oeuvres en série</rdfs:label>
  </genre:IntertextualGenre>
  <genre:PoeticGenre rdf:about="http://sparql.cwrc.ca/ontologies/genre#haiku">
    <rdfs:comment xml:lang="en">The description for this term is indebted to Dr. L. Kip Wheeler of Carson-Newman University. </rdfs:comment>
    <owl:sameAs rdf:resource="http://dbpedia.org/resource/Haiku"/>
    <owl:sameAs rdf:resource="http://id.loc.gov/authorities/genreForms/gf2014026366"/>
    <skos:definition xml:lang="fr">«Le haïku (俳句, haiku), terme créé par le poète Masaoka Shiki (1867-1902), est une forme poétique très codifiée d'origine japonaise et dont la paternité, dans son esprit actuel, est attribuée au poète Bashō Matsuo (1644-1694). Le haïku doit donner une notion de saison (le kigo) et doit comporter une césure (le kireji). Si le haïku n'indique ni saison, ni moment particulier, on l'appellera un moki ou encore haïku libre, tels les poèmes de Taneda Santôka (1882-1940) ou ceux de Ozaki Hôsai (1885-1926).» <![CDATA[(<a href="#cwrc:727d97bc-af78-4122-94be-aa78b2e97d5a">DBpedia, 2017</a>)]]></skos:definition>
    <rdfs:label xml:lang="en">haiku</rdfs:label>
    <rdfs:label xml:lang="fr">haïku</rdfs:label>
    <skos:definition xml:lang="en">"(plural: haiku, from archaic Japanese): The term haiku is a fairly late addition to Japanese poetry. The poet Shiki coined the term in the nineteenth century from a longer, more traditional phrase, haikai renga no hokku ("the introductory lines of light linked verse"). To understand the haiku's history as a genre, peruse the vocabulary entries for its predecessors, the hokku and the haikai renga or renku. The haiku follows several conventions: Many Japanese poets have used the form, the two acknowledged masters being Bashó (a nom de plume for Matsuo Munefusa, 1644-94); and Kobayashi Issa (a nom de plume for Kobayashi Nobuyuki). The Imagist Movement in 20th century English literature has been profoundly influenced by haiku. The list of poets who attempted the haiku or admired the genre includes Ezra Pound, Amy Lowell, Robert Frost, Conrad Aiken, and W. B. Yeats. Contrast haiku with the tanka and the senryu. See also hokku, below, and haikai, above. See also kigo and imagism. You can click here to download a PDF handout summarizing this discussion of haiku, or you can click here to download PDF samples of haiku." <![CDATA[(<a href="cwrc:509015ff-7641-473e-94c5-688e06952bb7">L. K Wheeler, 2017</a>)]]></skos:definition>
  </genre:PoeticGenre>
  <genre:FictionalGenre rdf:about="http://sparql.cwrc.ca/ontologies/genre#schoolFiction">
    <rdfs:label xml:lang="en">school fiction</rdfs:label>
    <skos:definition xml:lang="en">"The school story is a fiction genre centering on older pre-adolescent and adolescent school life, at its most popular in the first half of the twentieth century. While examples do exist in other countries, it is most commonly set in English boarding schools and mostly written in girls' and boys' subgenres, reflecting the single-sex education typical until the 1950s. It focuses largely on friendship, honor and loyalty between pupils. Plots involving sports events, bullies, secrets, rivalry and bravery are often used to shape the school story." <![CDATA[(<a href="#cwrc:727d97bc-af78-4122-94be-aa78b2e97d5a">DBpedia, 2017</a>)]]></skos:definition>
    <rdfs:label xml:lang="fr">fiction scolaire</rdfs:label>
    <owl:sameAs rdf:resource="http://dbpedia.org/resource/School_story"/>
    <rdfs:comment xml:lang="en">This term and its description were created from data gathered from DBpedia.</rdfs:comment>
  </genre:FictionalGenre>
  <genre:PoeticGenre rdf:about="http://sparql.cwrc.ca/ontologies/genre#clerihew">
    <rdfs:label xml:lang="en">clerihew</rdfs:label>
    <skos:definition xml:lang="fr">"Un clerihew est un poème biographique et excentrique de quatre vers inventé par Edmund Clerihew Bentley. La première ligne est le nom du sujet du poème, généralement une personne célèbre mise en scène de façon absurde. Le schéma des rimes est AABB, et celles-ci sont souvent forcées. La longueur du vers et le mètre sont irréguliers. Bentley a inventé le clerihew à l'école et l'a ensuite popularisé dans des livres."</skos:definition>
    <skos:definition xml:lang="en">"A clerihew is a whimsical, four-line biographical poem invented by Edmund Clerihew Bentley. The first line is the name of the poem's subject, usually a famous person put in an absurd light. The rhyme scheme is AABB, and the rhymes are often forced. The line length and metre are irregular. Bentley invented the clerihew in school and then popularized it in books." <![CDATA[(<a href="#cwrc:727d97bc-af78-4122-94be-aa78b2e97d5a">DBpedia, 2017</a>)]]></skos:definition>
    <owl:sameAs rdf:resource="http://id.loc.gov/authorities/genreForms/gf2014026261"/>
    <rdfs:label xml:lang="fr">clerihew</rdfs:label>
    <rdfs:comment xml:lang="en">The description for this term is indebted to DBpedia. </rdfs:comment>
    <owl:sameAs rdf:resource="http://dbpedia.org/resource/Clerihew"/>
  </genre:PoeticGenre>
  <genre:PoeticGenre rdf:about="http://sparql.cwrc.ca/ontologies/genre#narrativePoetry">
    <rdfs:label xml:lang="en">narrative poetry</rdfs:label>
    <owl:sameAs rdf:resource="http://id.loc.gov/authorities/genreForms/gf2014026448"/>
    <skos:definition xml:lang="en">"Narrative poetry is a form of poetry that tells a story, often making use of the voices of a narrator and characters as well; the entire story is usually written in metred verse. Narrative poems do not have to follow rhythmic patterns. The poems that make up this genre may be short or long, and the story it relates to may be complex. It is usually well it normally dramatic, with objectives, diverse characters, and metre. Narrative poems include epics, ballads, idylls, and lays. Some narrative poetry takes the form of a novel in verse. An example of this is The Ring and the Book by Robert Browning. In terms of narrative poetry, a romance is a narrative poem that tells a story of chivalry. Examples include the Romance of the Rose or Tennyson's Idylls of the King. Although these examples use medieval and Arthurian materials, romances may also tell stories from classical mythology. Shorter narrative poems are often similar in style to the short story. Sometimes these short narratives are collected into interrelated groups, as with Chaucer's The Canterbury Tales. Some literatures contain prose naose narratives, and the Old Norse sagas include both incidental poetry and the biographies of poets. An example is "The Cremation of Sam McGee" by Robert Service." <![CDATA[(<a href="#cwrc:727d97bc-af78-4122-94be-aa78b2e97d5a">DBpedia, 2017</a>)]]></skos:definition>
    <skos:definition xml:lang="fr">«La poésie narrative est un courant de la poésie italienne contemporaine dont les principaux représentants sont Carlo Bordini, Mauro Fabi et Andrea di Consoli. Cette poésie, qui sans renoncer à sa dimension expérimentale ou à une certaine forme de lyrisme exploite des matériaux divers - en usant du collage ou en incluant des fragments discursifs ou narratifs - et s'appuie sur le rythme et l'oralité non pour cacher le sens, mais pour le révéler.» <![CDATA[(<a href="#cwrc:727d97bc-af78-4122-94be-aa78b2e97d5a">DBpedia, 2017</a>)]]></skos:definition>
    <owl:sameAs rdf:resource="http://dbpedia.org/resource/Narrative_poetry"/>
    <rdfs:comment xml:lang="en">The description for this term is indebted to DBpedia. </rdfs:comment>
  </genre:PoeticGenre>
  <genre:DramaticGenre rdf:about="http://sparql.cwrc.ca/ontologies/genre#pageant">
    <skos:definition xml:lang="en">"Entertainments, frequently held in the open air, illustrating themes by means of spectacle rather than by consecutive narrative and dramatic characterization." <![CDATA[(<a href="#cwrc:db2f8571-a773-4068-a35f-34262950bb8f">Getty, 2017</a>)]]></skos:definition>
    <skos:definition xml:lang="fr">Divertissements, souvent représentés en plein air, illustrant des thèmes sous forme de spectacles plutôt que par une trame narrative continue.</skos:definition>
    <rdfs:comment xml:lang="en">This term and its description were created from data gathered from the Getty Art &amp; Architecture Thesaurus.</rdfs:comment>
    <owl:sameAs rdf:resource="http://id.loc.gov/authorities/genreForms/gf2014026464"/>
    <rdfs:label xml:lang="fr">procession</rdfs:label>
    <owl:sameAs rdf:resource="http://vocab.getty.edu/aat/300069240"/>
    <rdfs:label xml:lang="en">pageant</rdfs:label>
  </genre:DramaticGenre>
  <genre:PoeticGenre rdf:about="http://sparql.cwrc.ca/ontologies/genre#fabliau">
    <rdfs:label xml:lang="en">fabliau</rdfs:label>
    <rdfs:comment xml:lang="en">This term and its description were created from data gathered from DBpedia.</rdfs:comment>
    <skos:definition xml:lang="en">"A humorous, frequently ribald or "dirty" narrative popular with French poets, who traditionally wrote the story in octosyllabic couplets. The tales frequently revolve around trickery, practical jokes, sexual mishaps, scatology, mistaken identity, and bodily humor. Chaucer included several fabliaux in The Canterbury Tales, including the stories of the Shipman, the Friar, the Miller, the Reeve, and the Cook. Examples from French literature include Les Quatre Souhais Saint Martin, Audigier, and Beranger au Long Cul (Beranger of the Long Ass)." <![CDATA[(<a href="cwrc:509015ff-7641-473e-94c5-688e06952bb7">L. K Wheeler, 2017</a>)]]></skos:definition>
    <rdfs:label xml:lang="fr">fabliau</rdfs:label>
    <skos:definition xml:lang="fr">«Fabliau (du picard, lui-même issu du latin fabula qui donna en français « fable », signifie littéralement « petit récit ») est le nom qu'on donne dans la littérature française du Moyen Âge à de petites histoires simples et amusantes, définies par Bédier comme des contes à rire en vers. Leur vocation est de distraire ou faire rire les auditeurs et lecteurs, mais ils peuvent prétendre offrir une leçon morale, parfois ambiguë.» <![CDATA[(<a href="#cwrc:727d97bc-af78-4122-94be-aa78b2e97d5a">DBpedia, 2017</a>)]]></skos:definition>
    <dcterms:references rdf:resource="http://web.cn.edu/kwheeler/lit_terms_f.html"/>
  </genre:PoeticGenre>
  <genre:ChildrensLiteratureGenre rdf:about="http://sparql.cwrc.ca/ontologies/genre#youngAdultWriting">
    <rdfs:label xml:lang="fr">littérature jeunes adultes</rdfs:label>
    <rdfs:label xml:lang="en">young adult writing</rdfs:label>
    <skos:definition xml:lang="en">Writing aimed at a young adult audience.</skos:definition>
    <skos:definition xml:lang="fr">Littérature destinée à un public de jeunes adultes.</skos:definition>
  </genre:ChildrensLiteratureGenre>
  <genre:DramaticGenre rdf:about="http://sparql.cwrc.ca/ontologies/genre#tragicomedy">
    <owl:sameAs rdf:resource="http://id.loc.gov/authorities/genreForms/gf2014026577"/>
    <owl:sameAs rdf:resource="http://dbpedia.org/resource/Tragicomedy"/>
    <skos:definition xml:lang="en">"Tragicomedy is a literary genre that blends aspects of both tragic and comic forms. Most often seen in dramatic literature, the term can variously describe either a tragic play which contains enough comic elements to lighten the overall mood or a serious play with a happy ending." <![CDATA[(<a href="#cwrc:727d97bc-af78-4122-94be-aa78b2e97d5a">DBpedia, 2017</a>)]]></skos:definition>
    <rdfs:label xml:lang="en">tragicomedy</rdfs:label>
    <rdfs:comment xml:lang="en">The description for this term is indebted to DBpedia. </rdfs:comment>
    <skos:definition xml:lang="fr">«La tragi-comédie est une forme théâtrale caractérisée par une action romanesque, des personnages de haute extraction, un dénouement heureux et un refus des règles de la tragédie. Le terme est apparu en France chez le dramaturge Robert Garnier vers la fin du XVIe siècle, orthographié tragecomedie ; le terme nous vient de Plaute, qui désigne son Amphitryon comme une "tragi-comoedia" (au vers 59). Ce genre a connu un très grand succès en France dans les années 1630-1640. Il est assez difficile de définir les limites de la tragi-comédie à cette époque parce que les auteurs revendiquaient le refus de toute règle. On pouvait alors voir dans la tragi-comédie une sorte de tragédie à fin heureuse parce que la tragédie n'était définie que par son personnel noble et mythologique. Dans les années 1640, les partisans d'un théâtre beaucoup plus normé prennent de plus en plus d'importance et la tragédie répondant aux règles classiques prend le dessus sur la tragi-comédie. Le cas du Le Cid de Corneille est un exemple intéressant à cet égard car il a été publié en 1637 en tant que tragi-comédie et requalifié en tragédie dès 1648 alors que Corneille n'avait pas encore effectué de modification majeure de la pièce. On peut donc considérer que ce n'est pas la pièce mais la perception qu'on avait des différents genres théâtraux qui a évolué entre ces deux dates. En effet, l'intrigue du Cid comporte de nombreux éléments caractéristiques d'une tragi-comédie : il raconte une histoire d'amour dans laquelle un obstacle empêche à un moment donné la réunion des deux amants. À la fin de la pièce, cet obstacle sera levé et le dénouement sera heureux et nuptial ce qui est à l'époque une caractéristique des comédies et des tragi-comédies. La Querelle du Cid aura contribué à fixer les règles de la tragédie même si Le Cid conserve ses caractéristiques à savoir l'accumulation des événements , les coups de théâtre, les changements de décor successif et le dénouement heureux. On a beaucoup reproché à Corneille l'invraisemblance de la fin et un respect très discutable des trois unités. De fait, même s'il est déjà influencé par les règles qui commencent à s'imposer à la fin des années 1630, Corneille conserve dans cette pièce une liberté de composition héritée de la tragi-comédie et que l'on ne trouvera plus dans ses tragédies ultérieures. Pour autant, la pièce annonce la dramaturgie classique parce que les conflits omniprésents qui la constituent ne se manifestent pas à travers de combats spectaculaires sur scène mais à travers le travail du langage. Ainsi le duel entre Rodrigue et Don Gomes s'achève très vite alors que les célébrissimes stances du Cid rendent compte longuement du conflit intérieur qui travaille Rodrigue. Ce refus du spectaculaire au profit d'un travail sur le discours et les sentiments des personnages sera caractéristique de l'esthétique classique et explique que le Cid en soit resté un exemple majeur alors qu'il est encore très influencé par le genre de la tragi-comédie qui s'oppose aux caractéristiques de l'écriture classique. Philippe Quinault , poète et librettiste français, a aussi contribué au succès de ce genre en participant à la création de la tragédie-ballet Psyché en 1671 écrit par Molière aidé de Corneille. Le mélange des genres fut peu représenté par la suite dans le théâtre français, tout au plus trouve-t-on des pièces ou les genres s'alternent sans se mêler. Victor Hugo tente pourtant d'imposer avec son théâtre romantique une écriture entre sublime et grotesque, mais il faudra attendre le XXe siècle et le théâtre de l'absurde pour que le public accepte de concevoir que le rire ne nuit pas obligatoirement à la profondeur dramatique.» <![CDATA[(<a href="#cwrc:727d97bc-af78-4122-94be-aa78b2e97d5a">DBpedia, 2017</a>)]]></skos:definition>
  </genre:DramaticGenre>
  <genre:MysteryGenre rdf:about="http://sparql.cwrc.ca/ontologies/genre#detective">
    <skos:closeMatch rdf:resource="http://dbpedia.org/resource/Crime_fiction"/>
    <skos:definition xml:lang="en">Detective fiction is a subgenre of crime fiction and mystery fiction in which an investigator or a detective—either professional or amateur—investigates a crime, often murder.</skos:definition>
    <rdfs:label xml:lang="en">detective</rdfs:label>
    <rdfs:label xml:lang="fr">roman policier</rdfs:label>
    <skos:definition xml:lang="fr">«Le genre policier, ou polar, est un genre caractérisant certaines œuvres narratives et qui se distingue par sa mise en scène d'une énigme que le protagoniste tente de résoudre, souvent par une enquête de police. En ressortent notamment, en littérature le roman policier, au cinéma le film policier et à la télévision la série télévisée policière.» <![CDATA[(<a href="#cwrc:727d97bc-af78-4122-94be-aa78b2e97d5a">DBpedia, 2017</a>)]]></skos:definition>
    <owl:sameAs rdf:resource="http://id.loc.gov/authorities/genreForms/gf2014026280"/>
    <rdfs:comment xml:lang="en">The description for this term is indebted to DBpedia. </rdfs:comment>
  </genre:MysteryGenre>
  <genre:SerialForm rdf:about="http://sparql.cwrc.ca/ontologies/genre#column">
    <rdfs:label xml:lang="en">column</rdfs:label>
    <skos:related rdf:resource="http://vocab.getty.edu/aat/300026441"/>
  </genre:SerialForm>
  <genre:DramaticGenre rdf:about="http://sparql.cwrc.ca/ontologies/genre#filmTvScript">
    <rdf:type rdf:resource="http://sparql.cwrc.ca/ontologies/genre#ScriptForm"/>
    <skos:definition xml:lang="fr">Textes de théâtre, scénario, et scripts pour télévision ou la radio.</skos:definition>
    <rdfs:label xml:lang="en">film tv script</rdfs:label>
    <skos:definition xml:lang="en">"Written texts of stage plays, screenplays, and radio or television broadcasts." <![CDATA[(<a href="#cwrc:db2f8571-a773-4068-a35f-34262950bb8f">Getty, 2017</a>)]]></skos:definition>
    <skos:altLabel xml:lang="en">tv script</skos:altLabel>
    <owl:sameAs rdf:resource="http://vocab.getty.edu/aat/300026487"/>
    <rdfs:comment xml:lang="en">This term and its description were created from data gathered from the Getty Art &amp; Architecture Thesaurus.</rdfs:comment>
    <rdfs:label xml:lang="fr">script</rdfs:label>
  </genre:DramaticGenre>
  <genre:ThematicWritingGenre rdf:about="http://sparql.cwrc.ca/ontologies/genre#temperance">
    <rdfs:label xml:lang="en">temperance</rdfs:label>
  </genre:ThematicWritingGenre>
  <genre:AutobiographicalGenre rdf:about="http://sparql.cwrc.ca/ontologies/genre#autobiography">
    <owl:sameAs rdf:resource="http://id.loc.gov/authorities/genreForms/gf2014026047"/>
    <owl:sameAs rdf:resource="http://vocab.getty.edu/aat/300080104"/>
    <rdfs:comment xml:lang="en">The description for this term is indebted to the Getty Art &amp; Architecture Thesaurus.</rdfs:comment>
    <skos:definition xml:lang="en">"Documents of any type that are biographies of individuals written by themselves. For the overall genre, use "autobiography (genre).""<![CDATA[(<a href="#cwrc:db2f8571-a773-4068-a35f-34262950bb8f">Getty, 2017</a>)]]></skos:definition>
    <rdfs:label xml:lang="en">autobiography</rdfs:label>
    <skos:definition xml:lang="fr">"Tous types de documents étant des biographies d'individus écrits par eux-mêmes. Pour un aperçue d'ensemble du genre, utiliser "autobiographie" (genre)."</skos:definition>
    <rdfs:label xml:lang="fr">autobiographie</rdfs:label>
  </genre:AutobiographicalGenre>
  <genre:PoeticGenre rdf:about="http://sparql.cwrc.ca/ontologies/genre#villanelle">
    <rdfs:label xml:lang="fr">villanelle</rdfs:label>
    <rdfs:label xml:lang="en">villanelle</rdfs:label>
    <rdfs:comment xml:lang="en">This term and its description were created from data gathered from DBpedia.</rdfs:comment>
    <skos:definition xml:lang="en">"A versatile genre of poetry consisting of nineteen lines--five tercets and a concluding quatrain. The form requires that whole lines be repeated in a specific order, and that only two rhyming sounds occur in the course of the poem. A number of English poets, including Oscar Wilde, W. E. Henley, and W. H. Auden have experimented with it. Here is an example of an opening stanza to one poem by W. E. Henley: Probably the most famous English villanelle is Dylan Thomas's "Do Not Go Gentle Into That Good Night." <![CDATA[(<a href="cwrc:509015ff-7641-473e-94c5-688e06952bb7">L. K Wheeler, 2017</a>)]]></skos:definition>
    <skos:definition xml:lang="fr">«D’origine italienne, la villanelle, de l’italien villanella dérivant du latin villanus (paysan), est, en littérature, une sorte de petite poésie pastorale à forme fixe et divisée en couplets qui finissent par le même refrain. En musique, c’est une ancienne danse rustique accompagnée de chant ainsi qu’une mélodie, un air d’instruments composé sur le modèle de cette danse.» <![CDATA[(<a href="#cwrc:727d97bc-af78-4122-94be-aa78b2e97d5a">DBpedia, 2017</a>)]]></skos:definition>
    <dcterms:references rdf:resource="http://web.cn.edu/kwheeler/lit_terms_v.html"/>
    <owl:sameAs rdf:resource="http://id.loc.gov/authorities/genreForms/gf2014026587"/>
  </genre:PoeticGenre>
  <genre:CatalogueForm rdf:about="http://sparql.cwrc.ca/ontologies/genre#catalogue">
    <rdfs:label xml:lang="en">catalogue</rdfs:label>
  </genre:CatalogueForm>
  <genre:RecordForm rdf:about="http://sparql.cwrc.ca/ontologies/genre#record">
    <skos:definition xml:lang="fr">«Un document renvoie à un ensemble formé par un support et une information, celle-ci enregistrée de manière persistante. Il a une valeur explicative, descriptive ou de preuve. Vecteur matériel de la pensée humaine, il joue un rôle essentiel dans la plupart des sociétés contemporaines, tant pour le fonctionnement de leurs administrations que dans l'élaboration de leurs savoirs.» <![CDATA[(<a href="http://fr.dbpedia.org/page/Document">Breit, 1951</a>; <a href="http://martinetl.free.fr/suzannebriet/questcequeladocumentation/briet.pdf">pdf</a>) «[T]out indice concret ou symbolique, conservé out enregistré, aux fins de représenter, de reconstituer ou de prouver un phénomène ou physique out intellectuel»<![CDATA[(<a href="#cwrc:3A9ee53c63-e387-4fc0-ad17-df5a84dddb4">Breit, 1951</a>)]]></skos:definition>
    <rdfs:label xml:lang="fr">notice</rdfs:label>
    <rdfs:label xml:lang="en">record</rdfs:label>
    <skos:definition xml:lang="en">"Evidence about an object or the past, regardless of medium, as preserved in a record or document. As defined by the Library of Congress, records are "Documents in any form created or received by an agency, institution, organization, or individual, accumulated in the normal conduct of business or affairs." <![CDATA[(<a href="http://id.loc.gov/authorities/genreForms/gf2014026163.html">Library of Congress, 2018</a>) Wikipedia says, "A document is a written, drawn, presented or recorded representation of thoughts. Originating from the Latin Documentum meaning lesson - the verb doceō means to teach, and is pronounced similarly, in the past it was usually used as a term for a written proof used as evidence. In the computer age, a document is usually used to describe a primarily textual file, along with its structure and design, such as fonts, colors and additional images." <![CDATA[(<a href="https://en.wikipedia.org/wiki/Document">Wikipedia, 2018</a>) Information scientist Suzanne Breit defines a document as "any concrete or symbolic indication, preserved or recorded, for reconstructing or for proving a phenomenon, whether physical or mental." <![CDATA[(<a href="#cwrc:3A9ee53c63-e387-4fc0-ad17-df5a84dddb4">Breit, 1951; translated</a>)]]></skos:definition>
    <rdfs:comment xml:lang="en">This term and its description were created from data gathered from DBpedia.</rdfs:comment>
    <owl:sameAs rdf:resource="http://id.loc.gov/authorities/genreForms/gf2014026163"/>
    <owl:sameAs rdf:resource="http://dbpedia.org/resource/Document"/>
  </genre:RecordForm>
  <genre:InformationalGenre rdf:about="http://sparql.cwrc.ca/ontologies/genre#interview">
    <rdfs:label xml:lang="en">interview</rdfs:label>
  </genre:InformationalGenre>
  <genre:IntertextualGenre rdf:about="http://sparql.cwrc.ca/ontologies/genre#abridgement">
    <rdfs:label xml:lang="en">abridgement</rdfs:label>
    <owl:sameAs rdf:resource="http://id.loc.gov/authorities/genreForms/gf2014026037"/>
    <skos:definition xml:lang="en">"Versions of written works produced by condensation and omission but with retention of the general meaning and manner of presentation of the original, often prepared by someone other than the author of the original." <![CDATA[(<a href="#cwrc:db2f8571-a773-4068-a35f-34262950bb8f">Getty, 2017</a>)]]></skos:definition>
    <rdfs:label xml:lang="fr">résumé</rdfs:label>
    <rdfs:comment xml:lang="en">The description for this term is indebted to the Getty Art &amp; Architecture Thesaurus.</rdfs:comment>
    <owl:sameAs rdf:resource="http://vocab.getty.edu/aat/300202489"/>
  </genre:IntertextualGenre>
  <genre:CollectionForm rdf:about="http://sparql.cwrc.ca/ontologies/genre#anthology">
    <skos:related rdf:resource="http://id.loc.gov/authorities/genreForms/gf2011026487"/>
    <rdfs:comment xml:lang="en">The description for this term is indebted to the Getty Art &amp; Architecture Thesaurus.</rdfs:comment>
    <skos:related rdf:resource="http://id.loc.gov/authorities/genreForms/gf2011026051"/>
    <skos:related rdf:resource="http://id.loc.gov/authorities/genreForms/gf2011026052"/>
    <skos:definition xml:lang="en">"Collections of choice extracts, from the writings of one author, or various authors, and usually having a common characteristic such as subject matter or literary form." <![CDATA[(<a href="#cwrc:db2f8571-a773-4068-a35f-34262950bb8f">Getty, 2017</a>)]]></skos:definition>
    <skos:definition xml:lang="fr">"Collections d'extraits choisis parmi les écrits d'un ou de plusieurs auteurs, ayant habituellement une caractéristique commune telle que le sujet abordé ou la forme littéraire. "</skos:definition>
    <owl:sameAs rdf:resource="http://vocab.getty.edu/aat/300026037"/>
    <rdfs:label xml:lang="fr">anthologie</rdfs:label>
    <rdfs:label xml:lang="en">anthology</rdfs:label>
  </genre:CollectionForm>
  <genre:AutobiographicalGenre rdf:about="http://sparql.cwrc.ca/ontologies/genre#slaveNarrative">
    <rdfs:label xml:lang="en">slave narrative</rdfs:label>
    <rdfs:label xml:lang="fr">récit d'esclave</rdfs:label>
    <skos:altLabel xml:lang="en">slavery</skos:altLabel>
    <skos:definition xml:lang="en">"An autobiographical account of the life of an escaped or freed slave. Typically written and published in the Americas and used as a form of protest against the slave trade." <![CDATA[(<a href="#cwrc:4c227091-6bf0-4325-b846-9733fae19e61">Oxford, 2015</a>)]]></skos:definition>
    <owl:sameAs rdf:resource="http://dbpedia.org/resource/Slave_narrative"/>
    <skos:definition xml:lang="fr">«Le récit d'esclave est type d’œuvre littéraires écrites par des esclaves, essentiellement africains au Royaume-Uni et dans ses colonies, y compris ensuite les États-Unis, le Canada, et les états caribéens. Quelque six mille anciens esclaves d'Amérique du nord et des caraïbes écrivirent sur leur vie durant les XVIIIe siècle et XIXe siècle, avec environ 150 récits publiés individuellement en livres ou en pamphlets. Aux États-Unis durant la grande dépression (années 1930), plus de 2 300 récits oraux de vie sous l'esclavage furent collectés par des écrivains financés et publiés par la Work Projects Administration (WPA) de l'administration du président Roosevelt. 26 de ses enregistrements audios sont aujourd'hui conservés à la bibliothèque du Congrès.» <![CDATA[(<a href="#cwrc:727d97bc-af78-4122-94be-aa78b2e97d5a">DBpedia, 2017</a>)]]></skos:definition>
    <owl:sameAs rdf:resource="http://id.loc.gov/authorities/genreForms/gf2014026176"/>
    <rdfs:comment xml:lang="en">This term and its description were created from data gathered from DBpedia.</rdfs:comment>
  </genre:AutobiographicalGenre>
  <genre:SocialScienceGenre rdf:about="http://sparql.cwrc.ca/ontologies/genre#criminology">
    <skos:definition xml:lang="fr">Science de l'étude des crimes, des criminels et de la justice pénale, généralement non fictionnelle.</skos:definition>
    <rdfs:label xml:lang="fr">criminologie</rdfs:label>
    <skos:definition xml:lang="en">Scholarship, typically non-fiction, dealing with the study of crime, criminals, and criminal justice.</skos:definition>
    <rdfs:label xml:lang="en">criminology</rdfs:label>
  </genre:SocialScienceGenre>
  <genre:PoeticGenre rdf:about="http://sparql.cwrc.ca/ontologies/genre#lais">
    <rdfs:label xml:lang="fr">lai</rdfs:label>
    <owl:sameAs rdf:resource="http://dbpedia.org/resource/Lai"/>
    <rdfs:comment xml:lang="en">The description for this term is indebted to DBpedia. </rdfs:comment>
    <owl:sameAs rdf:resource="http://id.loc.gov/authorities/genreForms/gf2014026404"/>
    <skos:definition xml:lang="fr">«Le lai est un poème à forme fixe apparu au XIIe siècle et qui a désigné successivement des genres de poésie assez différents. Au Moyen Âge, ce mot était employé au sens de « chant » (ou plutôt récit chanté) ou de « mélodie » ; on connaît le lai narratif, ancêtre du fabliau, et le lai lyrique. L’origine du lai et de son nom est peut-être née d’anciens souvenirs littéraires celtiques (liais en gallois ou laoith en gaélique) car les vieilles légendes de la « matière de Bretagne » y tiennent une grande place, mais on y trouve toujours aussi la matière de France et la matière de Rome.» <![CDATA[(<a href="#cwrc:727d97bc-af78-4122-94be-aa78b2e97d5a">DBpedia, 2017</a>)]]></skos:definition>
    <skos:definition xml:lang="en">"A laisse is a type of stanza, of varying length, found in medieval French literature, specifically medieval French epic poetry (the chanson de geste), such as The Song of Roland. In early works, each laisse was made up of (mono) assonanced verses, although the appearance of (mono) rhymed laisses was increasingly common in later poems. Within a poem, the length of each separate laisse is variable (whereas the metric length of the verses is invariable, each verse having the same syllable length, typically decasyllables or, occasionally, alexandrines. The laisse is characterized by stereotyped phrases and formulas and frequently repeated themes and motifs, including repetitions of material from one laisse to another. Such repetitions and formulaic structures are common of orality and oral-formulaic composition. When medieval poets repeated content (with different wording or assonance/rhyme) from one laisse to another, such "similar" laisses are called laisses similaires in French." <![CDATA[(<a href="#cwrc:727d97bc-af78-4122-94be-aa78b2e97d5a">DBpedia, 2017</a>)]]></skos:definition>
    <rdfs:label xml:lang="en">lais</rdfs:label>
  </genre:PoeticGenre>
  <genre:NovelisticGenre rdf:about="http://sparql.cwrc.ca/ontologies/genre#domestic">
    <skos:definition xml:lang="en">"Domestic realism normally refers to the genre of nineteenth-century novels popular with women readers. This body of writing is also known as "sentimental fiction" or "woman's fiction". The genre is mainly reflected in the novel though short-stories and non-fiction works such as Harriet Beecher Stowe's "Our Country Neighbors" and The New Housekeeper's Manual written by Stowe and her sister-in-law Catharine Beecher are works of domestic realism. The style's particular characteristics are: "1. Plot focuses on a heroine who embodies one of two types of exemplar: the angel and the practical woman (Reynolds) who sometimes exist in the same work. Baym says that this heroine is contrasted with the passive woman (incompetent, cowardly, ignorant; often the heroine's mother is this type) and the "belle," who is deprived of a proper education. 2. The heroine struggles for self-mastery, learning the pain of conquering her own passions (Tompkins, Sensational Designs, 172). 3. The heroine learns to balance society's demands for self-denial with her own desire for autonomy, a struggle often addressed in terms of religion. 4. She suffers at the hands of abusers of power before establishing a network of surrogate kin. 5. The plots "repeatedly identify immersion in feeling as one of the great temptations and dangers for a developing woman. They show that feeling must be controlled. . . " (Baym 25). Frances Cogan notes that the heroines thus undergo a full education within which to realize feminine obligations (The All-American Girl). 6. The tales generally end with marriage, usually one of two possible kinds: A. Reforming the bad or "wild" male, as in Augusta Evans's St. Elmo (1867) B. Marrying the solid male who already meets her qualifications.Examples: Maria Cummins, The Lamplighter (1854) and Susan Warner, The Wide, Wide World (1850) 7. The novels may use a "language of tears" that evokes sympathy from the readers. 8. Richard Brodhead (Cultures of Letters) sees class as an important issue, as the ideal family or heroine is poised between a lower-class family exemplifying poverty and domestic disorganization and upper-class characters exemplifying an idle, frivolous existence (94)." An example of this style of novel is Jane Smiley's A Thousand Acres in which the main character's confinement is emphasized in such a way. Some early exponents of the genre of domestic realism were Jane Austen and Elizabeth Barrett Browning." <![CDATA[(<a href="#cwrc:727d97bc-af78-4122-94be-aa78b2e97d5a">DBpedia, 2017</a>)]]></skos:definition>
    <rdfs:label xml:lang="en">domestic</rdfs:label>
    <rdf:type rdf:resource="http://sparql.cwrc.ca/ontologies/genre#ThematicWritingGenre"/>
    <owl:sameAs rdf:resource="http://dbpedia.org/resource/Domestic_realism"/>
    <rdfs:comment xml:lang="en">The description for this term is indebted to DBpedia. </rdfs:comment>
    <skos:definition xml:lang="fr">Le réalisme domestique se réfère généralement au genre des romans du dix-neuvième siècle populaires auprès des lectrices des femmes. Ce corps d'écriture est également connu sous le nom de "fiction sentimentale" Ou "la fiction de la femme". Le genre se reflète principalement dans le roman, bien que des histoires courtes et des œuvres non-fiction telles que Harriet Beecher Stowe's Our Country Neighbours &amp; quot; Et The New Housekeeper's Manual écrit par Stowe et sa belle-sœur Catharine Beecher sont des œuvres de réalisme domestique. Les caractéristiques particulières du style sont: &amp; quot; 1. Plot se concentre sur une héroïne qui incarne l'un des deux types d'exemples: l'ange et la femme pratique (Reynolds) qui existent parfois dans le même travail. Baym dit que cette héroïne est contrastée avec la femme passive (incompétente, lâche, ignorante, souvent la mère de l'héroïne est de ce type) et la «belle», qui est privée d'une éducation adéquate. 2. L'héroïne lutte pour la maîtrise de soi, apprenant la douleur causée par la nécessité de vaincre ses propres passions (Tompkins, Sensational Designs, 172). 3. L'héroïne apprend à trouver un équilibre entre l’impératif social du sacrifice de soi et son propre désir d'autonomie, une lutte souvent abordée en terme de religion. 4. Elle souffre aux mains d’auteurs de maltraitance, avant d'établir un réseau de parents de substitution. 5. Les intrigues "identifient à plusieurs reprises l’immersion dans la vie sentimentale comme synonyme de grandes tentations et de dangers pour une femme en développement. Ils montrent que les sentiments doivent être contrôlés. . . " (Baym 25). Frances Cogan note que les héroïnes sont suivent une éducation complète dans le but de remplir des obligations féminines (The All-American Girl). 6. Les histoires finissent habituellement par un mariage, correspondant en général à un des deux types possibles: A. Celui qui réhabilite un personnage masculin mauvais ou "sauvage", comme dans le Saint-Elmo d'Augusta Evans (1867) B. Celui qui marrie la protagoniste avec un homme stable qui répond déjà à ses exigences.Exemples: Maria Cummins, The Lamplighter (1854) et Susan Warner, The Wide, Wide World (1850) 7. Les romans peuvent utiliser un "langage larmoyant" qui provoque la sympathie des lecteurs. 8. Richard Brodhead (Cultures of Letters) voit la classe comme une question importante, car la famille idéale ou l'héroïne se situe entre une famille de classe inférieure illustrant la pauvreté et la désorganisation domestique et des personnages de classe supérieure illustrant une existence inactive et frivole (94). " Un exemple de ce style de roman est A Thousand Acres de Jane Smiley, dans lequel le confinement du personnage principal est souligné d’une telle manière. On compte Jane Austen et Elizabeth Barrett Browning comme des premières représentantes du réalisme domestique.</skos:definition>
    <rdfs:label xml:lang="fr">réalisme domestique</rdfs:label>
  </genre:NovelisticGenre>
  <genre:ThreeDimensionalMedium rdf:about="http://sparql.cwrc.ca/ontologies/genre#ephemera">
    <skos:related rdf:resource="http://vocab.getty.edu/aat/300028881"/>
    <rdfs:label xml:lang="en">ephemera</rdfs:label>
  </genre:ThreeDimensionalMedium>
  <genre:ThematicWritingGenre rdf:about="http://sparql.cwrc.ca/ontologies/genre#pastoral">
    <rdfs:label xml:lang="fr">littérature pastorale</rdfs:label>
    <owl:sameAs rdf:resource="http://vocab.getty.edu/aat/300250491"/>
    <rdfs:comment xml:lang="en">The description for this term is indebted to the Getty Art &amp; Architecture Thesaurus.</rdfs:comment>
    <rdfs:label xml:lang="en">pastoral</rdfs:label>
    <owl:sameAs rdf:resource="http://id.loc.gov/authorities/genreForms/gf2014026475"/>
    <skos:definition xml:lang="fr">Genre qui représente ou évoque la vie paysanne de façon idyllique. Dans les œuvres d'art picturales, les scènes pastorales représentent généralement des bergers et des bergères dans des paysages arcadiens idéalisés.</skos:definition>
    <skos:definition xml:lang="en">"Genre that depicts or evokes idyllic life in the country; in works of pictorial art, often scenes of shepherds and shepherdesses in idealized arcadian landscapes." <![CDATA[(<a href="#cwrc:db2f8571-a773-4068-a35f-34262950bb8f">Getty, 2017</a>)]]></skos:definition>
  </genre:ThematicWritingGenre>
  <genre:ParatextualGenre rdf:about="http://sparql.cwrc.ca/ontologies/genre#epilogue">
    <rdfs:comment xml:lang="en">The description for this term is indebted to Dr. L. Kip Wheeler of Carson-Newman University. </rdfs:comment>
    <rdfs:label xml:lang="fr">épilogue</rdfs:label>
    <owl:sameAs rdf:resource="http://id.loc.gov/authorities/genreForms/gf2018026101"/>
    <rdfs:label xml:lang="en">epilogue</rdfs:label>
    <skos:definition xml:lang="fr">«L’épilogue (du grec επι (epi) : au-dessus et λογος (logos) : discours) est la dernière partie, la conclusion d’une œuvre (discours, roman, film, pièce théâtrale, etc.). Il désigne plus particulièrement au théâtre classique un discours récapitulatif à la fin de la pièce. Il est surtout un hors-d’œuvre, un adieu au public. La Fontaine, croyant avoir fini son œuvre des Fables au VIe livre, prend congé du lecteur dans cet épilogue : Bornons ici cette carrière,Les longs ouvrages me font peur ;Loin d’épuiser une matière,On n’en doit prendre que la fleur»…<![CDATA[(<a href="#cwrc:727d97bc-af78-4122-94be-aa78b2e97d5a">DBpedia, 2017</a>)]]></skos:definition>
    <skos:definition xml:lang="en">"A conclusion added to a literary work such as a novel, play, or long poem. It is the opposite of a prologue. Often, the epilogue refers to the moral of a fable. Sometimes, it is a speech made by one of the actors at the end of a play asking for the indulgence of the critics and the audience. Shakespeare's A Midsummer Night's Dream contains one of the most famous epilogues. Contrast with prologue. Do not confuse the term with eclogue." <![CDATA[(<a href="cwrc:509015ff-7641-473e-94c5-688e06952bb7">L. K Wheeler, 2017</a>)]]></skos:definition>
    <owl:sameAs rdf:resource="http://dbpedia.org/resource/Epilogue"/>
  </genre:ParatextualGenre>
  <genre:DidacticGenre rdf:about="http://sparql.cwrc.ca/ontologies/genre#didactic">
    <rdfs:label xml:lang="fr">ouvrage didactique</rdfs:label>
    <skos:definition xml:lang="en">"Writing that is "preachy" or seeks overtly to convince a reader of a particular point or lesson. Medieval homilies and Victorian moral essays are often held up as examples of didactic literature, but one might argue that all literature is didactic to one extent or another since the written word frequently implies or suggests an authorial attitude. Sometimes, the lesson is overtly religious, as in the case of sermons or in literature like Milton's Paradise Lost, which seeks to "justify God's ways to men." In a more subtle way, much of Romantic literature hints at a critique of urbanized and mechanized life in 19th-century London." <![CDATA[(<a href="cwrc:509015ff-7641-473e-94c5-688e06952bb7">L. K Wheeler, 2017</a>)]]></skos:definition>
    <skos:definition xml:lang="fr">Écrits "moralisateurs" ou qui cherchent ouvertement à convaincre le lecteur en lui offrant une leçon. Les homélies médiévales et les essais moraux victoriens sont souvent considérés comme des exemples de la littérature didactique, mais on peut prétendre que toute littérature est didactique d'une façon ou d'une autre, car la parole écrite implique ou suggère fréquemment une prise de position autoriale. Parfois, la leçon est manifestement religieuse, comme dans le cas des sermons, ou en littérature comme pour  Le Paradis perdu de Milton, qui cherche à "justifier les voies de Dieu envers les hommes". D'une manière plus subtile, une grande partie de la littérature romantique suggère une critique de la vie urbaine et mécanisée de Londres au 19ème siècle.</skos:definition>
    <rdfs:label xml:lang="en">didactic</rdfs:label>
    <rdfs:comment xml:lang="en">The description for this term is indebted to Dr. L. Kip Wheeler of Carson-Newman University. </rdfs:comment>
    <dcterms:references rdf:resource="http://web.cn.edu/kwheeler/lit_terms_d.html"/>
  </genre:DidacticGenre>
  <genre:PrintMedium rdf:about="http://sparql.cwrc.ca/ontologies/genre#pamphlet">
    <rdfs:label xml:lang="en">pamphlet</rdfs:label>
    <skos:related rdf:resource="http://vocab.getty.edu/aat/300220572"/>
  </genre:PrintMedium>
  <genre:ThematicWritingGenre rdf:about="http://sparql.cwrc.ca/ontologies/genre#harlequinade">
    <rdfs:label xml:lang="fr">harlequinade</rdfs:label>
    <rdfs:comment xml:lang="en">This term and its description were created from data gathered from the Getty Art &amp; Architecture Thesaurus.</rdfs:comment>
    <skos:definition xml:lang="en">"Books popular in the 18th and 19th centuries, originally often depicting harlequins, in which folded parts of pages are lifted to reveal new pictures, fitted neatly onto the remaining parts of the previous pictures." <![CDATA[(<a href="#cwrc:db2f8571-a773-4068-a35f-34262950bb8f">Getty, 2017</a>)]]></skos:definition>
    <rdfs:label xml:lang="en">harlequinade</rdfs:label>
    <owl:sameAs rdf:resource="http://vocab.getty.edu/aat/300212205"/>
    <skos:definition xml:lang="fr">Livres populaires aux 18ème et 19ème siècles, représentant à l'origine des harlequins, et dans lesquels des parties des pages qu'on soulève révèlent de nouvelles images, précisément placées sur les parties restantes des images précédentes.</skos:definition>
  </genre:ThematicWritingGenre>
  <genre:DramaticGenre rdf:about="http://sparql.cwrc.ca/ontologies/genre#monologue">
    <rdfs:label xml:lang="en">monologue</rdfs:label>
    <owl:sameAs rdf:resource="http://id.loc.gov/authorities/genreForms/gf2014026440"/>
    <rdfs:comment xml:lang="en">The description for this term is indebted to DBpedia. </rdfs:comment>
    <owl:sameAs rdf:resource="http://dbpedia.org/resource/Monologue"/>
    <skos:definition xml:lang="en">"In theatre, a monologue (from Greek μονόλογος from μόνος mónos, "alone, solitary" and λόγος lógos, "speech") is a speech presented by a single character, most often to express their mental thoughts aloud, though sometimes also to directly address another character or the audience. Monologues are common across the range of dramatic media (plays, films, etc.), as well as in non-dramatic media such as poetry. Monologues share much in common with several other literary devices including soliloquies, apostrophes, and aside. There are, however, distinctions between each of these devices." <![CDATA[(<a href="#cwrc:727d97bc-af78-4122-94be-aa78b2e97d5a">DBpedia, 2017</a>)]]></skos:definition>
    <skos:definition xml:lang="fr">«Un monologue (du grec mono : "un seul", et logos : "discours") est une ou plusieurs phrases auto-adressées à haute voix, rapportant les pensées du locuteur au style direct.Il faut distinguer le véritable monologue non seulement, cela va de soi, du roman autobiographique à la première personne, qui suppose un décalage de temps, même minime ("Aujourd'hui maman est morte") entre la narration et le narré, mais aussi d'une forme d'écriture fictionnelle moderne, la représentation du flux intérieur sous la forme je ou tu.» <![CDATA[(<a href="#cwrc:727d97bc-af78-4122-94be-aa78b2e97d5a">DBpedia, 2017</a>)]]></skos:definition>
  </genre:DramaticGenre>
  <genre:InformationalGenre rdf:about="http://sparql.cwrc.ca/ontologies/genre#epitaph">
    <skos:definition xml:lang="en">"An epitaph (from Greek ἐπιτάφιος epitaphios "a funeral oration" from ἐπί epi "at, over" and τάφος taphos "tomb") is a short text honoring a deceased person. Strictly speaking, it refers to text that is inscribed on a tombstone or plaque, but it may also be used in a figurative sense. Some epitaphs are specified by the person themselves before their death, while others are chosen by those responsible for the burial. An epitaph may be written in prose or in poem verse; poets have been known to compose their own epitaphs prior to their death." <![CDATA[(<a href="#cwrc:c5e7bace-95bb-4820-bd7d-6bb97c1badc5">DBpedia, 2018</a>)]]></skos:definition>
    <rdfs:label xml:lang="fr">épitaphe</rdfs:label>
    <rdfs:label xml:lang="en">epitaph</rdfs:label>
    <rdfs:comment xml:lang="en">This term and its description were created from data gathered from DBpedia.</rdfs:comment>
    <skos:definition xml:lang="fr">«Une épitaphe (du grec ἐπιτάφος / epi, « sur » et taphos, « tombeau », par exemple des jeux funèbres ou une oraison funèbre) est une inscription funéraire, placée sur une pierre tombale ou un monument funéraire. Cela peut être un objet donné à une civilisation comme signe de paix. Dans la Grèce antique, l’épitaphe est un genre littéraire : c’est un éloge funèbre ancien. En littérature française, l'épitaphe est aussi un genre littéraire rimé : c'est surtout ce que l'on aimerait inscrire sur la pierre tombale de quelqu'un que l'on admire, ou, au contraire, que l'on n'apprécie guère. Supposée être inscrite sur le tombeau lui-même, une épitaphe peut débuter par ci-gît ou par la formule plus moderne ici repose ou par leur pluriel ci-gisent et ici reposent.» <![CDATA[(<a href="#cwrc:727d97bc-af78-4122-94be-aa78b2e97d5a">DBpedia, 2017</a>)]]></skos:definition>
    <owl:sameAs rdf:resource="http://dbpedia.org/resource/Epitaph"/>
  </genre:InformationalGenre>
  <genre:RomanceGenre rdf:about="http://sparql.cwrc.ca/ontologies/genre#romance">
    <skos:definition xml:lang="fr">Œuvre habituellement fictionnelle, qui tirent leur origines des romans chevaleresques du Moyen Âge et de la Renaissance représentant des chevaliers et des aventures merveilleuses. La romance traite des relations sentimentales, familiales et sexuelles, et s'articule souvent autours de récits hétéronormés qui se concluent par une union romantique ou un mariage. La catégorie comprend les œuvres reconnues pour leur qualité littéraire, ainsi que la littérature commerciale ou de genre produite pour un public de masse. Les sous-genres de la romance comprennent la littérature gothique, la romance historique et celles écrites durant la Régence anglaise.</skos:definition>
    <rdfs:label xml:lang="en">romance</rdfs:label>
    <owl:sameAs rdf:resource="http://id.loc.gov/authorities/genreForms/gf2014026516"/>
    <skos:definition xml:lang="en">"Poetic or prosaic literary forms derived from medieval narratives of love, legendary or heroic adventures, and chivalry. Extends to narratives about important religious figures, or fantastic or supernatural events." <![CDATA[(<a href="#cwrc:db2f8571-a773-4068-a35f-34262950bb8f">Getty, 2017</a>)]]></skos:definition>
    <owl:sameAs rdf:resource="http://vocab.getty.edu/aat/300191065"/>
    <rdfs:label xml:lang="fr">romance</rdfs:label>
    <rdfs:comment xml:lang="en">The description for this term is indebted to the Getty Art &amp; Architecture Thesaurus.</rdfs:comment>
  </genre:RomanceGenre>
  <genre:NovelisticGenre rdf:about="http://sparql.cwrc.ca/ontologies/genre#conditionOfEnglandNovel">
    <rdfs:label xml:lang="fr">condition of england novel</rdfs:label>
    <rdf:type rdf:resource="http://sparql.cwrc.ca/ontologies/genre#PoliticalWritingGenre"/>
    <rdfs:label xml:lang="en">condition of england novel</rdfs:label>
    <skos:definition xml:lang="fr">Forme de fiction narrative, nommée ainsi d'après une phrase du "Chartisme" de Thomas Carlyle (1839), qui traite des questions sociales et politiques victoriennes en mettant l'accent sur l'agitation politique et les conflits entre classes sociales, qui cherche généralement à provoquer l'empathie pour les pauvres et la compréhension des inégalités et des injustices sociales. Ce mouvement est très proche du roman industriel en raison de son intérêt pour les conséquences de la révolution industrielle.</skos:definition>
    <skos:definition xml:lang="en">A form of narrative fiction, named for a phrase from Thomas Carlyle's “Chartism” (1839), that addresses Victorian social and political issues with a focus on political unrest and class conflict, and typically seeks to instill empathy for the poor and understanding of social iniquities and injustices.
Closely related to the industrial novel because of its interest in the impact of the industrial revolution.</skos:definition>
  </genre:NovelisticGenre>
  <genre:FictionalGenre rdf:about="http://sparql.cwrc.ca/ontologies/genre#fairytale">
    <rdfs:label xml:lang="fr">conte de fées</rdfs:label>
    <owl:sameAs rdf:resource="http://id.loc.gov/authorities/genreForms/gf2014026329"/>
    <skos:definition xml:lang="en">"Narratives set in the distant past recounting events impossible in the real world, often magical and with fairies, but with humans as heroes and heroines." <![CDATA[(<a href="#cwrc:db2f8571-a773-4068-a35f-34262950bb8f">Getty, 2017</a>)]]></skos:definition>
    <rdfs:label xml:lang="en">fairytale</rdfs:label>
    <owl:sameAs rdf:resource="http://dbpedia.org/resource/Fairytale_fantasy"/>
    <skos:definition xml:lang="fr">Récits se déroulant dans un passé lointain et racontant des événements impossibles dans la réalité, souvent magiques et avec des fées, mais avec des humains comme héros et héroïnes.</skos:definition>
    <rdfs:comment xml:lang="en">The description for this term is indebted to the Getty Art &amp; Architecture Thesaurus.</rdfs:comment>
  </genre:FictionalGenre>
  <genre:FictionalGenre rdf:about="http://sparql.cwrc.ca/ontologies/genre#magicRealist">
    <owl:sameAs rdf:resource="http://id.loc.gov/authorities/genreForms/gf2014026424"/>
    <skos:definition xml:lang="fr">«Le réalisme magique est une appellation utilisée par la critique littéraire et la critique d’art depuis 1925 pour rendre compte de productions où des éléments perçus et décrétés comme « magiques », « surnaturels » et « irrationnels » qui surgissent dans un environnement défini comme « réaliste », à savoir un cadre historique, géographique et culturel vraisemblable. Ainsi la réalité reconnaissable devient-elle le lieu naturel de manifestations paranormales et oniriques. Aujourd'hui, cette appellation est surtout associée à certains auteurs de la littérature latino-américaine du XXe siècle comme les Mexicains Carlos Fuentes et Juan Rulfo, les Argentins Adolfo Bioy Casares et Julio Cortázar, le Bolivien Jaime Sáenz et le Colombien Gabriel García Márquez, prix Nobel de littérature en 1982, dont le roman Cent ans de solitude publié en 1967, est cité comme exemplaire. L’origine de ce terme et sa portée sont pourtant beaucoup plus généraux et ont été utilisés pour qualifier une grande variété de romans, de poèmes, de peintures et de réalisations cinématographiques. Par ailleurs, le réalisme magique connaît plusieurs déclinaisons et peut caractériser divers styles, esthétiques, genres, courants et mouvements en Asie, en Europe ou en Amérique. De manière plus récente, il est rapproché de la world literature. Généralement, il cherche à tisser des liens étroits entre des courants habituellement opposés tels que le naturalisme, le merveilleux et le fantastique afin de peindre une réalité transfigurée par l'imaginaire et dans laquelle le rationalisme est rejeté. Néanmoins, il n'existe pas de définition rigoureuse et son application dépend de la démarche intellectuelle et stylistique de l'écrivain ou l'artiste qui y a recours.» <![CDATA[(<a href="#cwrc:727d97bc-af78-4122-94be-aa78b2e97d5a">DBpedia, 2017</a>)]]></skos:definition>
    <rdfs:label xml:lang="fr">réalisme magique</rdfs:label>
    <dcterms:references rdf:resource="https://www.britannica.com/art/magic-realism"/>
    <skos:definition xml:lang="en">"A style of fiction popularized in Latin-American writing from the mid-twentieth century, in which magical or fantastical elements are not treated as unusual, but rather occur alongside realistic elements as a natural part of the narrative." <![CDATA[(<a href="#cwrc:7ff0c640-f273-46f5-be8d-e50aa27dce59">Encyclopædia Britannica, 2017</a>)]]></skos:definition>
    <rdfs:comment xml:lang="en">This term and its description were created from data gathered from the Encyclopædia Britannica.</rdfs:comment>
    <rdfs:label xml:lang="en">magic realist</rdfs:label>
  </genre:FictionalGenre>
  <genre:ReligiousGenre rdf:about="http://sparql.cwrc.ca/ontologies/genre#biblicalParaphrase">
    <rdfs:label xml:lang="en">biblical paraphrase</rdfs:label>
    <skos:definition xml:lang="en">A work that rewords the text of the Bible, often to improve clarity or to make it accessible to a wider audience.</skos:definition>
    <skos:definition xml:lang="fr">Texte qui reprend les paroles de la Bible, souvent dans l'objectif d'en améliorer la clarté ou de la rendre plus accessibleau large public.</skos:definition>
    <rdfs:label xml:lang="fr">paraphrase biblique</rdfs:label>
  </genre:ReligiousGenre>
  <genre:ThematicWritingGenre rdf:about="http://sparql.cwrc.ca/ontologies/genre#love">
    <skos:definition xml:lang="en">Generic modifier for a representation that deals primarily with the subject of love.</skos:definition>
    <skos:definition xml:lang="fr">Dénomination générique pour les textes dont le sujet principal contient une forme de représentation de l'amour.</skos:definition>
    <rdfs:comment xml:lang="en">The description for this term is indebted to DBpedia. </rdfs:comment>
    <rdfs:label xml:lang="en">love</rdfs:label>
    <skos:closeMatch rdf:resource="http://dbpedia.org/resource/Christo"/>
    <rdfs:label xml:lang="fr">amour</rdfs:label>
  </genre:ThematicWritingGenre>
  <genre:ThematicWritingGenre rdf:about="http://sparql.cwrc.ca/ontologies/genre#seaStory">
    <rdfs:label xml:lang="en">sea story</rdfs:label>
  </genre:ThematicWritingGenre>
  <genre:NovelisticGenre rdf:about="http://sparql.cwrc.ca/ontologies/genre#verseNovel">
    <rdfs:label xml:lang="en">verse novel</rdfs:label>
    <owl:sameAs rdf:resource="http://dbpedia.org/resource/Verse_novel"/>
    <rdfs:label xml:lang="fr">roman en vers</rdfs:label>
    <rdf:type rdf:resource="http://sparql.cwrc.ca/ontologies/genre#PoeticGenre"/>
    <skos:definition xml:lang="en">"A verse novel is a type of narrative poetry in which a novel-length narrative is told through the medium of poetry rather than prose. Either simple or complex stanzaic verse-forms may be used, but there will usually be a large cast, multiple voices, dialogue, narration, description, and action in a novelistic manner." <![CDATA[(<a href="#cwrc:727d97bc-af78-4122-94be-aa78b2e97d5a">DBpedia, 2017</a>)]]></skos:definition>
    <skos:definition xml:lang="fr">Un roman en vers est un type de narration poétique dans laquelle un récit de la longueur d'un roman est raconté sous la forme de la poésie plutôt que de la prose. L'auteur peut utiliser des formes métriques simples ou complexes, mais incluera normalement un grand nombre de personnages, des voix multiples, un dialogue, une narration, une description et une action de manière romanesque.</skos:definition>
    <rdfs:comment xml:lang="en">The description for this term is indebted to DBpedia. </rdfs:comment>
    <owl:sameAs rdf:resource="http://id.loc.gov/authorities/genreForms/gf2014026457"/>
  </genre:NovelisticGenre>
  <genre:DigitalMedium rdf:about="http://sparql.cwrc.ca/ontologies/genre#website">
    <rdfs:label xml:lang="en">website</rdfs:label>
    <skos:related rdf:resource="http://vocab.getty.edu/aat/300265431"/>
  </genre:DigitalMedium>
  <genre:PedagogicalGenre rdf:about="http://sparql.cwrc.ca/ontologies/genre#instructionalText">
    <rdfs:label xml:lang="en">instructional text</rdfs:label>
  </genre:PedagogicalGenre>
  <genre:ThematicWritingGenre rdf:about="http://sparql.cwrc.ca/ontologies/genre#gardening">
    <rdfs:label xml:lang="en">gardening</rdfs:label>
    <skos:definition xml:lang="fr">Texte non fictif qui traite du jardinage.</skos:definition>
    <rdfs:label xml:lang="fr">jardinage</rdfs:label>
    <skos:definition xml:lang="en">A text, typically non-fiction, dealing with the subject of gardening.</skos:definition>
  </genre:ThematicWritingGenre>
  <genre:ScholarlyGenre rdf:about="http://sparql.cwrc.ca/ontologies/genre#essay">
    <rdfs:label xml:lang="fr">essai</rdfs:label>
    <owl:sameAs rdf:resource="http://dbpedia.org/resource/Essay"/>
    <rdfs:label xml:lang="en">essay</rdfs:label>
    <skos:definition xml:lang="fr">«En littérature, un essai est une œuvre de réflexion portant sur les sujets les plus divers et exposée de manière personnelle, voire subjective par l'auteur. Contrairement à l'étude, l'essai peut être polémique ou partisan. C'est un texte littéraire qui se prête bien à la réflexion philosophique, mais aussi à d'autres domaines : essais historiques, essais scientifiques, essais politiques, etc. L'auteur d’un essai est appelé « essayiste ». Le terme « essai » est dérivé du latin exagium, un poids ou appareil de mesure.» <![CDATA[(<a href="#cwrc:727d97bc-af78-4122-94be-aa78b2e97d5a">DBpedia, 2017</a>)]]></skos:definition>
    <owl:sameAs rdf:resource="http://id.loc.gov/authorities/genreForms/gf2014026094"/>
    <skos:definition xml:lang="en">"Short literary compositions on single subjects, often presenting the personal view of the author." <![CDATA[(<a href="#cwrc:db2f8571-a773-4068-a35f-34262950bb8f">Getty, 2017</a>)]]></skos:definition>
    <rdfs:comment xml:lang="en">The description for this term is indebted to DBpedia. </rdfs:comment>
  </genre:ScholarlyGenre>
  <genre:PartialForm rdf:about="http://sparql.cwrc.ca/ontologies/genre#partExcerpt">
    <rdfs:label xml:lang="en">part/excerpt</rdfs:label>
  </genre:PartialForm>
  <genre:PrintMedium rdf:about="http://sparql.cwrc.ca/ontologies/genre#offprint">
    <skos:closeMatch rdf:resource="http://dbpedia.org/resource/Offprint"/>
    <skos:definition xml:lang="en">An offprint is a separate printing of a work that originally appeared as part of a larger publication, usually one of composite authorship such as an academic journal, magazine, or edited book.</skos:definition>
    <owl:sameAs rdf:resource="http://id.loc.gov/vocabulary/marcgt/off.html"/>
    <rdfs:label xml:lang="en">offprint</rdfs:label>
  </genre:PrintMedium>
  <genre:SerialForm rdf:about="http://sparql.cwrc.ca/ontologies/genre#journal">
    <owl:sameAs rdf:resource="http://id.loc.gov/authorities/genreForms/gf2014026139"/>
    <rdfs:label xml:lang="en">journal</rdfs:label>
  </genre:SerialForm>
  <genre:IntertextualGenre rdf:about="http://sparql.cwrc.ca/ontologies/genre#imitation">
    <rdfs:label xml:lang="en">imitation</rdfs:label>
    <skos:definition xml:lang="fr">Forme d'intertextualité dans laquelle un.e auteur.e adopte intentionnellement le style d'un.e autre auteur.e, ou emprunte des éléments importants du travail de quelqu'un d'autre.</skos:definition>
    <rdfs:comment xml:lang="en">This term and its description were created from data gathered from the Penguin Dictionary of Literary Terms &amp; Literary Theory, 4th ed.</rdfs:comment>
    <skos:definition xml:lang="en">"A form of intertextuality in which a writer intentionally adopts the style of another writer or borrows important elements of someone else's work." <![CDATA[(<a href="#cwrc:2f09376c-f784-4a46-9f04-5a21aa311f27">Penguin, 1999</a>)]]></skos:definition>
    <rdfs:label xml:lang="fr">imitation</rdfs:label>
  </genre:IntertextualGenre>
  <genre:PrintMedium rdf:about="http://sparql.cwrc.ca/ontologies/genre#microform">
    <skos:related rdf:resource="http://vocab.getty.edu/aat/300028589"/>
    <rdfs:label xml:lang="en">microform</rdfs:label>
  </genre:PrintMedium>
  <genre:FictionalGenre rdf:about="http://sparql.cwrc.ca/ontologies/genre#bisexualFiction">
    <skos:definition xml:lang="en">Fiction dealing with bisexuality.</skos:definition>
    <rdfs:label xml:lang="en">bisexual fiction</rdfs:label>
    <skos:definition xml:lang="fr">Fiction abordant le thème de la bisexualité.</skos:definition>
    <owl:sameAs rdf:resource="http://id.loc.gov/authorities/genreForms/gf2018026053"/>
    <rdfs:label xml:lang="fr">fiction bisexuelle</rdfs:label>
  </genre:FictionalGenre>
  <genre:PedagogicalGenre rdf:about="http://sparql.cwrc.ca/ontologies/genre#grammar">
    <rdfs:label xml:lang="en">grammar</rdfs:label>
    <rdfs:label xml:lang="fr">grammaire</rdfs:label>
    <rdfs:comment xml:lang="en">The description for this term is indebted to Dr. L. Kip Wheeler of Carson-Newman University. </rdfs:comment>
    <skos:definition xml:lang="fr">«La grammaire est l'étude systématique des éléments constitutifs d'une langue. Par extension, on nomme aussi grammaire un manuel ou un ensemble de documents décrivant des règles grammaticales.» <![CDATA[(<a href="#cwrc:727d97bc-af78-4122-94be-aa78b2e97d5a">DBpedia, 2017</a>)]]></skos:definition>
    <skos:definition xml:lang="en">"GRAMMAR: Another term for transformational grammar." <![CDATA[(<a href="cwrc:509015ff-7641-473e-94c5-688e06952bb7">L. K Wheeler, 2017</a>)]]></skos:definition>
    <dcterms:references rdf:resource="http://web.cn.edu/kwheeler/lit_terms_g.html"/>
  </genre:PedagogicalGenre>
  <genre:IntertextualGenre rdf:about="http://sparql.cwrc.ca/ontologies/genre#adaptation">
    <rdfs:label xml:lang="fr">adaptation</rdfs:label>
    <skos:closeMatch rdf:resource="http://vocab.getty.edu/aat/300410356"/>
    <skos:definition xml:lang="en">W"ritten works or works derived from written works, where the second work is an alteration or amendment a text to make it suitable for another purpose. An example of an adaptation is a version of an earlier text made to better agree with a philosophy other than that intended by the original. Other examples are written works adapted for another medium, such as film, broadcasting, or stage production."<![CDATA[(<a href="#cwrc:db2f8571-a773-4068-a35f-34262950bb8f">Getty, 2017</a>)]]></skos:definition>
    <owl:sameAs rdf:resource="http://id.loc.gov/authorities/genreForms/gf2014026041"/>
    <skos:definition xml:lang="fr">Œuvres écrites ou travaux dérivés d'œuvres écrites, qui sont des altérations ou des modifications d'un texte pour qu'il convienne à d'autres fins. Par exemple, un texte ancien peut être réécrit pour transmettre une morale différente de celle qui était initialement prévue. Les œuvres écrites pour être adaptées à un autre support, tel que l'audiovisuel, la télévision ou le théâtre sont des exemples d'adaptation.</skos:definition>
    <rdfs:comment xml:lang="en">The description for this term is indebted to the Getty Art &amp; Architecture Thesaurus.</rdfs:comment>
    <rdfs:label xml:lang="en">adaptation</rdfs:label>
  </genre:IntertextualGenre>
  <genre:LifeWritingGenre rdf:about="http://sparql.cwrc.ca/ontologies/genre#lifeWriting">
    <rdfs:comment xml:lang="en">The description for this term is indebted to DBpedia. </rdfs:comment>
    <rdfs:label xml:lang="en">life writing</rdfs:label>
    <skos:definition xml:lang="en">"Life writing is the recording of memories, and experiences, whether one's own or another's. This applies to many genres and practices, under which can be found autobiography, biography, memoir, diaries, letters, testimonies, personal essays and, more recently, digital forms such as blogs and email." <![CDATA[(<a href="#cwrc:727d97bc-af78-4122-94be-aa78b2e97d5a">DBpedia, 2017</a>)]]></skos:definition>
    <owl:sameAs rdf:resource="http://dbpedia.org/resource/Life_writing"/>
  </genre:LifeWritingGenre>
  <genre:PoeticGenre rdf:about="http://sparql.cwrc.ca/ontologies/genre#heroic">
    <owl:sameAs rdf:resource="http://vocab.getty.edu/aat/300404208"/>
    <skos:definition xml:lang="en">"Form of poetry comprising long narratives celebrating on a grand scale the adventures and deeds of one or more heroic figures, ordinarily concerning a serious subject significant to a culture or nation. Classical epic poetry employs dactylic hexameter and recounts a journey." <![CDATA[(<a href="#cwrc:db2f8571-a773-4068-a35f-34262950bb8f">Getty, 2017</a>)]]></skos:definition>
    <rdfs:label xml:lang="en">heroic</rdfs:label>
    <skos:definition xml:lang="fr">Forme de poésie qui présente de longs récits célébrant les aventures et les actes d'une ou plusieurs figures héroïques, d'ordinaire concernant un sujet sérieux important pour une culture ou une nation. La poésie épique classique emploie l'hexamètre dactylique et raconte un voyage.</skos:definition>
    <skos:related rdf:resource="http://id.loc.gov/authorities/genreForms/gf2014026310"/>
    <rdfs:label xml:lang="fr">poème épique</rdfs:label>
    <rdfs:comment xml:lang="en">The description for this term is indebted to the Getty Art &amp; Architecture Thesaurus.</rdfs:comment>
  </genre:PoeticGenre>
  <genre:PoeticGenre rdf:about="http://sparql.cwrc.ca/ontologies/genre#dramaticMonologue">
    <owl:sameAs rdf:resource="http://dbpedia.org/resource/Dramatic_monologue"/>
    <owl:sameAs rdf:resource="http://id.loc.gov/authorities/genreForms/gf2014026298"/>
    <skos:definition xml:lang="en">"Dramatic monologue, also known as a persona poem, is a type of poetry written in the form of a speech of an individual character. M.H. Abrams notes the following three features of the dramatic monologue as it applies to poetry." <![CDATA[(<a href="#cwrc:727d97bc-af78-4122-94be-aa78b2e97d5a">DBpedia, 2017</a>)]]></skos:definition>
    <skos:definition xml:lang="fr">«Un monologue dramatique est en France, à la fin du Moyen Âge, un type de poème comique à vocation scénique. À l’instar des jongleurs, l’acteur seul en scène incarnait plusieurs personnages stéréotypés. Il est considéré comme un des quatre grands genres comiques de la fin du Moyen Âge avec la sotie, le sermon joyeux et la farce. Dans l'Angleterre du XIXe siècle, le terme monologue dramatique (dramatic mononologue) désignait un type de poème, fort apprécié par de nombreux poètes de l'époque victorienne, dans lequel un personnage, de fiction ou historique, exprime ses sentiments, ses actions ou ses motifs dans un monologue. Celui-ci, dont les paroles sont souvent influencées par le contexte critique dans lequel elles sont prononcées, s'adresse en général à un auditoire silencieux.Des exemples de monologues dramatiques sont My Last Duchess de Robert Browning, The Captain of the 1984 Top of the Form Team de Carol Ann Duffy, ou encore Lady Lazarus de Sylvia Plath.» <![CDATA[(<a href="#cwrc:727d97bc-af78-4122-94be-aa78b2e97d5a">DBpedia, 2017</a>)]]></skos:definition>
    <rdfs:comment xml:lang="en">The description for this term is indebted to DBpedia. </rdfs:comment>
    <rdfs:label xml:lang="en">dramatic monologue</rdfs:label>
  </genre:PoeticGenre>
  <genre:CartographicForm rdf:about="http://sparql.cwrc.ca/ontologies/genre#map">
    <skos:definition xml:lang="en">"Refers to graphic or photogrammetric representations of the Earth's surface or a part of it, including physical features and political boundaries, where each point corresponds to a geographical or celestial position according to a definite scale or projection. The term may also refer to similar depictions of other planets, suns, other heavenly bodies, or areas of the heavens. Maps are typically depicted on a flat medium, such as on paper, a wall, or a computer screen." <![CDATA[(<a href="#cwrc:db2f8571-a773-4068-a35f-34262950bb8f">Getty, 2017</a>)]]></skos:definition>
    <owl:sameAs rdf:resource="http://id.loc.gov/authorities/genreForms/gf2011026387"/>
    <rdfs:label xml:lang="fr">carte</rdfs:label>
    <rdfs:label xml:lang="en">map</rdfs:label>
    <rdfs:comment xml:lang="en">This term and its description were created from data gathered from the Getty Art &amp; Architecture Thesaurus.</rdfs:comment>
    <skos:related rdf:resource="http://vocab.getty.edu/aat/300028094"/>
    <owl:sameAs rdf:resource="http://vocab.getty.edu/aat/300028094"/>
    <skos:definition xml:lang="fr">Désigne des représentations graphiques ou photogrammétriques de la surface de la Terre ou d'une partie de celle-ci, y compris les caractéristiques physiques et les délimitations politiques, où chaque point correspond à une position géographique ou céleste selon une échelle ou une projection définie. Le terme peut également se référer à des représentations similaires d'autres planètes, de soleils, d'autres corps célestes ou des zones du ciel. Les cartes sont généralement représentées sur un support plat, tel que du papier, un mur ou un écran d'ordinateur.</skos:definition>
  </genre:CartographicForm>
  <genre:ThematicWritingGenre rdf:about="http://sparql.cwrc.ca/ontologies/genre#thematicWriting">
    <skos:definition xml:lang="en">"Indicates a type of writing associated with some aspect of the text’s content or purpose, broadly conceived." <![CDATA[(<a href="#cwrc:727d97bc-af78-4122-94be-aa78b2e97d5a">DBpedia, 2017</a>)]]></skos:definition>
    <rdfs:label xml:lang="fr">écriture thématique</rdfs:label>
    <rdfs:comment xml:lang="en">This term and its description were created from data gathered from DBpedia.</rdfs:comment>
    <rdfs:label xml:lang="en">thematic writing</rdfs:label>
  </genre:ThematicWritingGenre>
  <genre:ParatextualGenre rdf:about="http://sparql.cwrc.ca/ontologies/genre#prefatoryPiece">
    <rdfs:label xml:lang="fr">préface</rdfs:label>
    <rdfs:comment xml:lang="en">This term and its description were created from data gathered from the Getty Art &amp; Architecture Thesaurus.</rdfs:comment>
    <skos:definition xml:lang="fr">«Une préface (du latin præ : avant et fari : parler) est, en littérature, un texte d’introduction et de présentation. Placé en tête d’un livre, il en fait connaître les vues, le plan, prévient des objections, répond à des critiques ou encore donne une idée sur le message que veut transmettre l'auteur à travers ce livre (ex : la pauvreté de la société, l'inégalité, la prostitution, la violence, etc.). La préface est courte lorsqu'elle devient un avertissement et largement développée dans le cadre des prolégomènes. On oppose à la préface la postface.» <![CDATA[(<a href="#cwrc:727d97bc-af78-4122-94be-aa78b2e97d5a">DBpedia, 2017</a>)]]></skos:definition>
    <rdfs:label xml:lang="en">prefatory piece</rdfs:label>
    <skos:definition xml:lang="en">"Texts preceding the main literary work and containing comments about such matters as the reason for or circumstances of the author's writing the work, or comments by another about the author or the work." <![CDATA[(<a href="#cwrc:db2f8571-a773-4068-a35f-34262950bb8f">Getty, 2017</a>)]]></skos:definition>
    <owl:sameAs rdf:resource="http://dbpedia.org/resource/Preface"/>
  </genre:ParatextualGenre>
  <genre:IntertextualGenre rdf:about="http://sparql.cwrc.ca/ontologies/genre#review">
    <skos:definition xml:lang="en">"Periodicals, reports, or essays giving critical estimates and appraisals of art, a performance, or event." <![CDATA[(<a href="#cwrc:db2f8571-a773-4068-a35f-34262950bb8f">Getty, 2017</a>)]]></skos:definition>
    <skos:definition xml:lang="fr">Périodiques, rapports ou essais qui fournissent des avis critiques ou évalue les travaux artistiques, les représentations ou les événements. Pour les autres descriptions et analyses critiques, préférer "criticism".</skos:definition>
    <owl:sameAs rdf:resource="http://id.loc.gov/authorities/genreForms/gf2014026168"/>
    <owl:sameAs rdf:resource="http://vocab.getty.edu/aat/300026480"/>
    <rdfs:label xml:lang="en">review</rdfs:label>
    <rdfs:label xml:lang="fr">critique</rdfs:label>
    <rdfs:comment xml:lang="en">This term and its description were created from data gathered from the Getty Art &amp; Architecture Thesaurus.</rdfs:comment>
  </genre:IntertextualGenre>
  <genre:FictionalGenre rdf:about="http://sparql.cwrc.ca/ontologies/genre#allegory">
    <skos:definition xml:lang="fr">«Une allégorie (du grec : ἄλλον / állon, « autre chose », et ἀγορεύειν / agoreúein, « parler en public ») est une forme de représentation indirecte qui emploie une chose (une personne, un être animé ou inanimé, une action) comme signe d'une autre chose, cette dernière étant souvent une idée abstraite ou une notion morale difficile à représenter directement. Elle représente donc une idée abstraite par du concret. En littérature, l'allégorie est une figure rhétorique qui consiste à exprimer une idée en utilisant une histoire ou une représentation qui doit servir de support comparatif. La signification étymologique est : « une autre manière de dire », au moyen d'une image figurative ou figurée.» <![CDATA[(<a href="#cwrc:727d97bc-af78-4122-94be-aa78b2e97d5a">DBpedia, 2017</a>)]]></skos:definition>
    <rdfs:label xml:lang="en">allegory</rdfs:label>
    <rdfs:comment xml:lang="fr">La description de ce terme est basée sur celle de DBPedia.</rdfs:comment>
    <skos:definition xml:lang="en">"Literary works, art works, or other creative works that employ allegory to express complex abstract ideas, for example works that employ symbolic, fictional figures and actions to express truths or generalizations about human conduct or experience." <![CDATA[(<a href="#cwrc:db2f8571-a773-4068-a35f-34262950bb8f">Getty, 2017</a>)]]></skos:definition>
    <rdfs:label xml:lang="fr">allégorie</rdfs:label>
    <rdfs:comment xml:lang="en">The description for this term is indebted to DBpedia. </rdfs:comment>
    <owl:sameAs rdf:resource="http://dbpedia.org/resource/Allegory"/>
  </genre:FictionalGenre>
  <genre:NarrativeGenre rdf:about="http://sparql.cwrc.ca/ontologies/genre#questNarrative">
    <rdfs:label xml:lang="en">quest narrative</rdfs:label>
  </genre:NarrativeGenre>
  <genre:FictionalGenre rdf:about="http://sparql.cwrc.ca/ontologies/genre#dystopia">
    <rdfs:comment xml:lang="en">The description for this term is indebted to Dr. L. Kip Wheeler of Carson-Newman University. </rdfs:comment>
    <owl:sameAs rdf:resource="http://id.loc.gov/authorities/genreForms/gf2014026302"/>
    <skos:definition xml:lang="en">"(from Greek, dys topos, "bad place"): The opposite of a utopia, a dystopia is an imaginary society in fictional writing that represents, as M. H. Abrams puts it, "a very unpleasant imaginary world in which ominous tendencies of our present social, political, and technological order are projected in some disastrous future culmination" (Glossary 218). For instance, while a utopia presents readers with a place where all the citizens are happy and ruled by a virtuous, efficient, rational government, a dystopia presents readers with a world where all citizens are universally unhappy, manipulated, and repressed by a sinister, sadistic totalitarian state. This government exists at best to further its own power and at worst seeks actively to destroy its own citizens' creativity, health, and happiness. Examples of fictional dystopias include Aldous Huxley's Brave New World, George Orwell's 1984, Margaret Atwood's The Handmaid's Tale, and Ursula Le Guin's The Dispossessed." <![CDATA[(<a href="cwrc:509015ff-7641-473e-94c5-688e06952bb7">L. K Wheeler, 2017</a>)]]></skos:definition>
    <skos:definition xml:lang="fr">Une dystopie est un récit de fiction dépeignant une société imaginaire organisée de telle façon qu'elle empêche ses membres d'atteindre le bonheur. Une dystopie peut également être considérée, entre autres, comme une utopie qui vire au cauchemar et conduit donc à une contre-utopie. L'auteur entend ainsi mettre en garde le lecteur en montrant les conséquences néfastes d’une idéologie (ou d’une pratique) présente à notre époque. L'impact que ces romans ont eu sur la science-fiction a souvent amené à qualifier de dystopie toute œuvre d'anticipation sociale décrivant un avenir sombre.</skos:definition>
    <rdfs:label xml:lang="en">dystopia</rdfs:label>
    <dcterms:references rdf:resource="http://web.cn.edu/kwheeler/lit_terms_d.html"/>
    <rdfs:label xml:lang="fr">dystopie</rdfs:label>
  </genre:FictionalGenre>
  <genre:InformationalGenre rdf:about="http://sparql.cwrc.ca/ontologies/genre#announcement">
    <rdfs:label xml:lang="en">announcement</rdfs:label>
  </genre:InformationalGenre>
  <genre:TextualMedium rdf:about="http://sparql.cwrc.ca/ontologies/genre#manuscript">
    <skos:related rdf:resource="http://vocab.getty.edu/aat/300028569"/>
    <rdfs:label xml:lang="en">manuscript</rdfs:label>
  </genre:TextualMedium>
  <genre:ThreeDimensionalMedium rdf:about="http://sparql.cwrc.ca/ontologies/genre#archivalMaterial">
    <skos:related rdf:resource="http://vocab.getty.edu/aat/300379505"/>
    <rdfs:label xml:lang="en">archival material</rdfs:label>
  </genre:ThreeDimensionalMedium>
  <genre:NarrativeGenre rdf:about="http://sparql.cwrc.ca/ontologies/genre#legend">
    <skos:altLabel xml:lang="en">folktale</skos:altLabel>
    <rdfs:label xml:lang="en">legend</rdfs:label>
  </genre:NarrativeGenre>
  <genre:CollectionForm rdf:about="http://sparql.cwrc.ca/ontologies/genre#bibliography">
    <rdfs:label xml:lang="en">bibliography</rdfs:label>
    <owl:sameAs rdf:resource="http://id.loc.gov/authorities/genreForms/gf2014026048"/>
  </genre:CollectionForm>
  <genre:HistoricalGenre rdf:about="http://sparql.cwrc.ca/ontologies/genre#historicalOverview">
    <rdfs:label xml:lang="en">historical overview</rdfs:label>
  </genre:HistoricalGenre>
  <genre:PoeticGenre rdf:about="http://sparql.cwrc.ca/ontologies/genre#boutsRimés">
    <rdfs:comment xml:lang="en">This term and its description were created from data gathered from the Oxford Dictionary of Literary Terms, 4th ed.</rdfs:comment>
    <rdfs:label xml:lang="en">bouts-rimés</rdfs:label>
    <skos:definition xml:lang="en">"The result of a game popularized in 17th-century France in which a poet must write a logical poem using a list of random rhyming words written by someone else." <![CDATA[(<a href="#cwrc:4c227091-6bf0-4325-b846-9733fae19e61">Oxford, 2015</a>)]]></skos:definition>
    <dcterms:references rdf:resource="http://www.oxfordreference.com/view/10.1093/acref/9780199208272.001.0001/acref-9780199208272-e-142?rskey=3RXM0b%26result=141"/>
    <rdfs:label xml:lang="fr">bout-rimé</rdfs:label>
  </genre:PoeticGenre>
  <genre:NovelisticGenre rdf:about="http://sparql.cwrc.ca/ontologies/genre#àClef">
    <rdfs:label xml:lang="fr">roman à clefs</rdfs:label>
    <rdfs:label xml:lang="en">à clef</rdfs:label>
    <skos:definition xml:lang="fr">«Le roman à lol clef est un sous-genre romanesque dans lequel certains personnages bite ou la totalité de ceux-ci représentent, de façon plus ou moins explicite, une personne réelle. Sous le couvert de la fiction, l'auteur écrit en réalité une histoire vraie, souvent pour éviter la diffamation tout en faisant une satire. La clef de l'histoire, qui fait comprendre au lecteur qu'il s'agit d'une histoire vraie, est habituellement une personnalité publique reconnue, plus particulièrement un homme politique ou une personne ayant une influence majeure sur un groupe, qu'il s'agisse de politique, d'affaires, de show-business, etc.» <![CDATA[(<a href="#cwrc:727d97bc-af78-4122-94be-aa78b2e97d5a">DBpedia, 2017</a>)]]></skos:definition>
    <skos:definition xml:lang="en">"A novel in which the characters and plots are fictionalized, but can actually be recognized as real people and events in disguise. French for "novel with a key."" <![CDATA[(<a href="#cwrc:727d97bc-af78-4122-94be-aa78b2e97d5a">DBpedia, 2017</a>)]]></skos:definition>
    <owl:sameAs rdf:resource="http://id.loc.gov/authorities/genreForms/gf2014026518"/>
    <rdfs:comment xml:lang="en">This term and its description were created from data gathered from DBpedia.</rdfs:comment>
    <owl:sameAs rdf:resource="http://dbpedia.org/resource/Roman_%C3%A0_clef"/>
  </genre:NovelisticGenre>
  <genre:ScholarlyGenre rdf:about="http://sparql.cwrc.ca/ontologies/genre#criticalAnalysis">
    <rdfs:label xml:lang="en">critical analysis</rdfs:label>
  </genre:ScholarlyGenre>
  <genre:FictionalGenre rdf:about="http://sparql.cwrc.ca/ontologies/genre#realist">
    <skos:definition xml:lang="en">"Fiction that attempts to capture life as it is, rejecting idealism in favour of exposing in detail the realities, including the flaws, of its characters and their lives." <![CDATA[(<a href="#cwrc:4c227091-6bf0-4325-b846-9733fae19e61">Oxford, 2015</a>)]]></skos:definition>
    <rdfs:comment xml:lang="en">The description for this term is indebted to the Getty Art &amp; Architecture Thesaurus.</rdfs:comment>
    <owl:sameAs rdf:resource="http://vocab.getty.edu/aat/300056550"/>
    <rdfs:label xml:lang="en">realist</rdfs:label>
    <skos:definition xml:lang="fr">«Terme général pour qualifier les œuvres d'art dans lesquelles la représentation du monde extérieur s'appuie ou semble s'appuyer sur une observation directe de celui-ci; ces oeuvres incluent ou mettent en valeur ses défauts et ses imperfections plutôt que d'en souligner la beauté ou d'idéaliser certains de ses aspetcs. Bien qu'une oeuvre puisse être à la fois réaliste et naturaliste, le naturalisme est susceptible d'idéaliser les défauts ou la laideur des thèmes abordés. Concernant le style formel et la période d'apparition des caractéristiques générales du réalisme, comme dans la peinture de Gustave Courbet, utilisez "Realist (dans les styles de beaux arts modernes européens)".» <![CDATA[(<a href="#cwrc:db2f8571-a773-4068-a35f-34262950bb8f">Getty, 2017</a>)]]></skos:definition>
    <rdfs:label xml:lang="fr">réaliste</rdfs:label>
  </genre:FictionalGenre>
  <genre:PoliticalWritingGenre rdf:about="http://sparql.cwrc.ca/ontologies/genre#petition">
    <owl:sameAs rdf:resource="http://dbpedia.org/resource/Petition"/>
    <skos:definition xml:lang="fr">«Le droit de pétition est le droit accordé aux populations de faire une demande directe au souverain, ou au représentant de l'exécutif. Par extension, il est possible de faire une pétition envers toute personne morale disposant d'un pouvoir. Une pétition se présente le plus souvent sous la forme d'un ensemble de signatures au bas d'un texte. Ces signatures sont généralement recueillies dans la rue par des volontaires. Avec l'arrivée d'Internet, un certain nombre de sites permettent d'organiser une pétition et de recueillir les signatures en ligne.» <![CDATA[(<a href="#cwrc:727d97bc-af78-4122-94be-aa78b2e97d5a">DBpedia, 2017</a>)]]></skos:definition>
    <rdfs:label xml:lang="en">petition</rdfs:label>
    <rdfs:label xml:lang="fr">pétition</rdfs:label>
    <skos:definition xml:lang="en">"Includes any written requests and lists of signatures submitted to an authority to appeal for the performance of specific action." <![CDATA[(<a href="#cwrc:db2f8571-a773-4068-a35f-34262950bb8f">Getty, 2017</a>)]]></skos:definition>
    <rdfs:comment xml:lang="en">The description for this term is indebted to the Getty Art &amp; Architecture Thesaurus.</rdfs:comment>
    <skos:related rdf:resource="http://id.loc.gov/authorities/genreForms/gf2011026358"/>
  </genre:PoliticalWritingGenre>
  <genre:PerformanceMedium rdf:about="http://sparql.cwrc.ca/ontologies/genre#passionPlay">
    <rdfs:label xml:lang="en">passion play</rdfs:label>
    <owl:sameAs rdf:resource="http://id.loc.gov/authorities/genreForms/gf2014026472"/>
    <rdf:type rdf:resource="http://sparql.cwrc.ca/ontologies/genre#ReligiousGenre"/>
  </genre:PerformanceMedium>
  <genre:ParatextualGenre rdf:about="http://sparql.cwrc.ca/ontologies/genre#dedication">
    <rdfs:comment xml:lang="en">The description for this term is indebted to Dr. L. Kip Wheeler of Carson-Newman University. </rdfs:comment>
    <skos:definition xml:lang="en">"A short bit of text conventionally appearing before the start of a novel or poem in which the author or poet addresses some individual, invoking his or her gratitude or thanks to that individual. Frequently, the dedication is to a spouse, friend, loved one, child, mentor, or individual who inspired the work. Several of the Inklings dedicated specific fictional works to each other (or in the case of C.S. Lewis, to children of fellow Inklings). Among scholars, one of the most significant types of dedications is a festschrift. A festschrift is a collection of essays or studies in book form, dedicated to a former teacher or professor in his or her advanced age. The individual scholarly writings come from his or her students, who typically collaborate to organize the work and contact the publisher, and they present the collection to the teacher upon its publication." <![CDATA[(<a href="cwrc:509015ff-7641-473e-94c5-688e06952bb7">L. K Wheeler, 2017</a>)]]></skos:definition>
    <rdfs:label xml:lang="fr">dédicace</rdfs:label>
    <skos:definition xml:lang="fr">«Une dédicace est une épître ou simple inscription placée par un auteur en tête d’un livre pour mettre son œuvre sous le patronage d’une personne illustre ou influente, ou pour témoigner de ses sentiments de gratitude ou d’amitié, ou enfin, à certaines époques, pour en tirer profit.» <![CDATA[(<a href="#cwrc:727d97bc-af78-4122-94be-aa78b2e97d5a">DBpedia, 2017</a>)]]></skos:definition>
    <dcterms:references rdf:resource="http://web.cn.edu/kwheeler/lit_terms_d.html"/>
    <rdfs:label xml:lang="en">dedication</rdfs:label>
  </genre:ParatextualGenre>
  <genre:CartographicForm rdf:about="http://sparql.cwrc.ca/ontologies/genre#cartographicMaterials">
    <rdfs:label xml:lang="en">cartographic materials</rdfs:label>
  </genre:CartographicForm>
  <genre:PoeticGenre rdf:about="http://sparql.cwrc.ca/ontologies/genre#epigram">
    <rdfs:label xml:lang="en">epigram</rdfs:label>
    <owl:sameAs rdf:resource="http://id.loc.gov/authorities/genreForms/gf2014026312"/>
    <skos:definition xml:lang="en">"Refers to short satiric poems or any similar pointed sayings." <![CDATA[(<a href="#cwrc:db2f8571-a773-4068-a35f-34262950bb8f">Getty, 2017</a>)]]></skos:definition>
    <owl:sameAs rdf:resource="http://vocab.getty.edu/aat/300202533"/>
    <rdfs:comment xml:lang="en">The description for this term is indebted to DBpedia. </rdfs:comment>
    <skos:definition xml:lang="fr">«À l’origine, une épigramme, du grec ancien ἐπίγραμμα (epígramma), « inscription », est une inscription, d’abord en prose, puis en vers, qu’on gravait sur les monuments, les statues, les tombeaux et les trophées, pour perpétuer le souvenir d’un héros ou d’un événement. À partir du IVe siècleav. J.-C., l’épigramme devient une petite pièce de poésie sur un sujet quelconque, imitant par sa brièveté les inscriptions, offrant une pensée ingénieuse ou délicate exprimée avec grâce et précision. Enfin, à partir du XVIe siècle, le genre se spécialise dans le mot d’esprit : l’épigramme renferme généralement une pointe grivoise ou assassine. Les plus anciennes épigrammes ne revêtent qu'un caractère pratique, visant à identifier le propriétaire ou la personne dédiant l’objet. Le premier auteur d’épigrammes, selon la tradition grecque, est Simonide de Céos (Hérodote, VII, 228, 4), qui vit à la fin du VIe siècleav. J.-C. C'est de cette même époque que date la première épigramme signée connue ; il s'agit d’une dédicace d’Ion de Chios à Delphes.» <![CDATA[(<a href="#cwrc:727d97bc-af78-4122-94be-aa78b2e97d5a">DBpedia, 2017</a>)]]></skos:definition>
  </genre:PoeticGenre>
  <genre:PoeticGenre rdf:about="http://sparql.cwrc.ca/ontologies/genre#topographicalPoetry">
    <skos:definition xml:lang="fr">Recueils de poésie célébrant des lieux situés dans différentes parties du monde.</skos:definition>
    <owl:sameAs rdf:resource="http://id.loc.gov/authorities/genreForms/gf2018026132"/>
    <rdfs:label xml:lang="en">topographical poetry</rdfs:label>
    <rdfs:comment xml:lang="en">The description for this term is indebted to DBpedia. </rdfs:comment>
    <rdfs:label xml:lang="fr">poésie des lieux</rdfs:label>
    <skos:definition xml:lang="en">"Topographical poetry or loco-descriptive poetry is a genre of poetry that describes, and often praises, a landscape or place. John Denham's 1642 poem "Cooper's Hill" established the genre, which peaked in popularity in 18th-century England. Examples of topographical verse date, however, to the late classical period, and can be found throughout the medieval era and during the Renaissance. Though the earliest examples come mostly from continental Europe, the topographical poetry in the tradition originating with Denham concerns itself with the classics, and many of the various types of topographical verse, such as river, ruin, or hilltop poems were established by the early 17th century. Alexander Pope's "Windsor Forest" (1713) and John Dyer's "Grongar Hill' (1762) are two other oft-mentioned examples. More recently, Matthew Arnold's "The Scholar Gipsy" (1853) praises the Oxfordshire countryside, and W. H. Auden's "In Praise of Limestone" (1948) uses a limestone landscape as an allegory. Subgenres of topographical poetry include the country house poem, written in 17th-century England to compliment a wealthy patron, and the prospect poem, describing the view from a distance or a temporal view into the future, with the sense of opportunity or expectation. When understood broadly as landscape poetry and when assessed from its establishment to the present, topographical poetry can take on many formal situations and types of places. Kenneth Baker identifies 37 varieties and compiles poems from the 16th through the 20th centuries—from Edmund Spenser to Sylvia Plath—correspondent to each type, from "Walks and Surveys," to "Mountains, Hills, and the View from Above," to "Violation of Nature and the Landscape," to "Spirits and Ghosts." Common aesthetic registers of which topographical poetry make use include pastoral imagery, the sublime, and the picturesque. These latter two registers subsume imagery of rivers, ruins, moonlight, birdsong, and clouds, peasants, mountains, caves, and waterscapes." <![CDATA[(<a href="#cwrc:727d97bc-af78-4122-94be-aa78b2e97d5a">DBpedia, 2017</a>)]]></skos:definition>
    <owl:sameAs rdf:resource="http://data.bnf.fr/11978314/poesie_des_lieux/"/>
  </genre:PoeticGenre>
  <genre:ComedicGenre rdf:about="http://sparql.cwrc.ca/ontologies/genre#farce">
    <skos:definition xml:lang="en">"(from Latin Farsus, "stuffed"): A farce is a form of low comedy designed to provoke laughter through highly exaggerated caricatures of people in improbable or silly situations. Traits of farce include (1) physical bustle such as slapstick, (2) sexual misunderstandings and mix-ups, and (3) broad verbal humor such as puns. Many literary critics (especially in the Victorian period) have tended to view farce as inferior to "high comedy" that involves brilliant dialogue. Many of Shakespeare's early works, such as The Taming of the Shrew, are considered farces. Contrast with comedy of manners." <![CDATA[(<a href="cwrc:509015ff-7641-473e-94c5-688e06952bb7">L. K Wheeler, 2017</a>)]]></skos:definition>
    <rdfs:comment xml:lang="en">This term and its description were created from data gathered from DBpedia.</rdfs:comment>
    <skos:altLabel xml:lang="en">farce</skos:altLabel>
    <owl:sameAs rdf:resource="http://dbpedia.org/resource/Farce"/>
    <rdfs:label xml:lang="fr">farce</rdfs:label>
    <owl:sameAs rdf:resource="http://id.loc.gov/authorities/genreForms/gf2014026335"/>
    <skos:definition xml:lang="fr">«La farce est un genre théâtral né au Moyen Âge, qui a comme but de faire rire et qui a souvent des caractéristiques grossières. Son origine remonte à l'Antiquité gréco-romaine, et on en trouve déjà des traces chez Aristophane et Plaute, et surtout dans les atellanes latines.» <![CDATA[(<a href="#cwrc:727d97bc-af78-4122-94be-aa78b2e97d5a">DBpedia, 2017</a>)]]></skos:definition>
    <rdfs:label xml:lang="en">farce</rdfs:label>
  </genre:ComedicGenre>
  <genre:ThematicWritingGenre rdf:about="http://sparql.cwrc.ca/ontologies/genre#architecturalWriting">
    <skos:altLabel xml:lang="en">architecture</skos:altLabel>
    <rdfs:label xml:lang="en">architectural writing</rdfs:label>
  </genre:ThematicWritingGenre>
  <genre:DialogueOrDebateGenre rdf:about="http://sparql.cwrc.ca/ontologies/genre#polemic">
    <rdfs:label xml:lang="en">polemic</rdfs:label>
    <owl:sameAs rdf:resource="http://vocab.getty.edu/aat/300252982"/>
    <rdfs:comment xml:lang="en">The description for this term is indebted to DBpedia. </rdfs:comment>
    <skos:definition xml:lang="fr">«Le terme de polémique (du grec πολεμικός, polêmikôs « qui concerne la guerre », « disposé à la guerre », polêmikon museion, musée de la guerre, « batailleur, querelleur ») désigne une discussion, un débat, une controverse qui traduit de façon violente ou passionnée, et le plus souvent par écrit, des opinions contraires sur toutes espèces de sujets (politique, scientifique, littéraire, religieux, etc.). Il fait aujourd'hui l'objet d'emplois multiples.» <![CDATA[(<a href="#cwrc:727d97bc-af78-4122-94be-aa78b2e97d5a">DBpedia, 2017</a>)]]></skos:definition>
    <skos:definition xml:lang="en">"Aggressive, forcefully presented arguments, often disputing a policy or opinion." <![CDATA[(<a href="#cwrc:db2f8571-a773-4068-a35f-34262950bb8f">Getty, 2017</a>)]]></skos:definition>
  </genre:DialogueOrDebateGenre>
  <genre:DialogueOrDebateGenre rdf:about="http://sparql.cwrc.ca/ontologies/genre#dialogueOrDebate">
    <skos:definition xml:lang="en">"A text made up of a conversation between two or more characters, often in which the characters take up opposing sides of an argument." <![CDATA[(<a href="#cwrc:4c227091-6bf0-4325-b846-9733fae19e61">Oxford, 2015</a>)]]></skos:definition>
    <rdfs:label xml:lang="en">dialogue or debate</rdfs:label>
    <dcterms:references rdf:resource="http://www.oxfordreference.com/view/10.1093/acref/9780199208272.001.0001/acref-9780199208272-e-310?rskey=TydJW0%26result=301"/>
    <rdfs:label xml:lang="fr">dialogue ou débat</rdfs:label>
    <owl:sameAs rdf:resource="http://id.loc.gov/authorities/genreForms/gf2014026083"/>
    <rdfs:comment xml:lang="en">This term and its description were created from data gathered from data.bnf.fr.</rdfs:comment>
    <skos:definition xml:lang="fr">Oeuvre littéraire en forme de conversation entre deux ou plusieurs personnes, où l'exposé contradictoire des idées permet à l'auteur d'exposer ses opinions morales, philosophiques, religieuses, etc.</skos:definition>
  </genre:DialogueOrDebateGenre>
  <genre:ThematicWritingGenre rdf:about="http://sparql.cwrc.ca/ontologies/genre#comingOut">
    <rdfs:label xml:lang="fr">coming out</rdfs:label>
    <rdfs:label xml:lang="en">coming out</rdfs:label>
    <skos:definition xml:lang="fr">Qui se rapporte au processus de révélation publique de sa sexualité.</skos:definition>
    <skos:definition xml:lang="en">Pertaining to the process of coming out sexually.</skos:definition>
  </genre:ThematicWritingGenre>
  <genre:AutobiographicalGenre rdf:about="http://sparql.cwrc.ca/ontologies/genre#memoir">
    <skos:related rdf:resource="http://id.loc.gov/authorities/genreForms/gf2014026047"/>
    <rdfs:label xml:lang="en">memoir</rdfs:label>
  </genre:AutobiographicalGenre>
  <genre:PoeticGenre rdf:about="http://sparql.cwrc.ca/ontologies/genre#eclogue">
    <owl:sameAs rdf:resource="http://id.loc.gov/authorities/genreForms/gf2014026476"/>
    <skos:definition xml:lang="en">"An eclogue is a poem in a classical style on a pastoral subject. Poems in the genre are sometimes also called bucolics." <![CDATA[(<a href="#cwrc:727d97bc-af78-4122-94be-aa78b2e97d5a">DBpedia, 2017</a>)
]]></skos:definition>
    <rdfs:comment xml:lang="en">The description for this term is indebted to DBpedia. </rdfs:comment>
    <owl:sameAs rdf:resource="http://dbpedia.org/resource/Eclogue"/>
    <skos:definition xml:lang="fr">«Une églogue est un poème de style classique consacré à un sujet pastoral. Les poèmes de ce genre littéraire sont parfois qualifiés de » bucoliques »." <![CDATA[(<a href="#cwrc:727d97bc-af78-4122-94be-aa78b2e97d5a">DBpedia, 2017</a>)
]]></skos:definition>
    <rdfs:label xml:lang="en">eclogue</rdfs:label>
  </genre:PoeticGenre>
  <genre:FictionalGenre rdf:about="http://sparql.cwrc.ca/ontologies/genre#thriller">
    <dcterms:references rdf:resource="http://www.oxfordreference.com/view/10.1093/acref/9780199208272.001.0001/acref-9780199208272-e-1146?rskey=Bizyon%26result=1151"/>
    <rdfs:label xml:lang="en">thriller</rdfs:label>
    <owl:sameAs rdf:resource="http://id.loc.gov/authorities/genreForms/gf2014026571"/>
    <skos:definition xml:lang="en">"Fiction full of action and suspense in which the protagonist is threatened by some sort of danger, often through the actions of a villain or criminal. The protagonist must usually employ both physical skill and wit to escape danger and outsmart the villain." <![CDATA[(<a href="#cwrc:4c227091-6bf0-4325-b846-9733fae19e61">Oxford, 2015</a>)]]></skos:definition>
    <skos:definition xml:lang="fr">«Le thriller (anglicisme, de l'anglais to thrill : « frémir ») est un genre artistique utilisant le suspense ou la tension narrative pour provoquer chez le lecteur ou le spectateur une excitation ou une appréhension et le tenir en haleine jusqu'au dénouement de l'intrigue. Ce genre est très utilisé dans la littérature, le cinéma ou la télévision et se subdivise en de nombreux , chacun possédant ses propres codes. Les procédés narratifs sont souvent les mêmes, qu'ils soient utilisés au cinéma ou dans la littérature, avec notamment les fausses-pistes et la rétention d'informations afin d'embrouiller le lecteur/spectateur, ou l'utilisation des cliffhangers entre les différents chapitres, scènes ou épisodes. Au cinéma, le genre est aussi caractérisé par des scènes de poursuite ou de combat, qui y sont parfois traitées différemment que dans les films d'action. Les thèmes sont nombreux. Au sein des thrillers policiers (crime thriller), on peut citer les demandes de rançons, les prises d'otages, les enlèvements, les casses et la vengeance, ainsi que les enquêtes policières qui en découlent et la technique du whodunit, quel que soit le point-de-vue de l’œuvre (celui du policier, de la victime ou du criminel). Les thrillers psychologiques (psychological thrillers) sont caractérisés par des manipulations psychologiques, des traques ou harcèlements liées à des obsessions, des emprisonnements ou confinements dans des endroits dangereux ou piégés, frisant parfois avec le genre de l'horreur. Dans les thrillers paranoïaques (paranoid thrillers), des éléments tels que les théories du complot, les fausses accusations et la paranoïa clinique sont récurrents. Contrairement aux récits d'aventures ou d'action, le thriller est principalement caractérisé par le méchant de l'histoire qui va mettre des obstacles sur la route du héros.» <![CDATA[(<a href="#cwrc:727d97bc-af78-4122-94be-aa78b2e97d5a">DBpedia, 2017</a>)]]></skos:definition>
    <rdfs:label xml:lang="fr">thriller</rdfs:label>
    <rdfs:comment xml:lang="en">This term and its description were created from data gathered from the Oxford Dictionary of Literary Terms, 4th ed.</rdfs:comment>
  </genre:FictionalGenre>
  <genre:InformationalGenre rdf:about="http://sparql.cwrc.ca/ontologies/genre#informationalWriting">
    <rdfs:label xml:lang="en">informational writing</rdfs:label>
    <skos:definition xml:lang="en">A broad category of writing, often considered nonfictional, designed to convey specific content on a wide range of topics. That content may not be true, and informational texts like other forms of writing are vehicles for persuasion and ideology. Informational writing may possess literary qualities and may or may not be scholarly.</skos:definition>
    <skos:related rdf:resource="http://id.loc.gov/authorities/genreForms/gf2014026113"/>
  </genre:InformationalGenre>
  <genre:ProverbForm rdf:about="http://sparql.cwrc.ca/ontologies/genre#aphorism">
    <rdfs:label xml:lang="fr">aphorisme</rdfs:label>
    <skos:definition xml:lang="en">"Short, pithy statements of principle or precepts, often of known authorship; distinguished from "proverbs" which are statements repeated colloquially and which often embody the folk wisdom of a group or nation." <![CDATA[(<a href="#cwrc:db2f8571-a773-4068-a35f-34262950bb8f">Getty, 2017</a>)]]></skos:definition>
    <skos:definition xml:lang="fr">" Déclarations de principes ou de préceptes concises et lapidaires, souvent d'un auteur connu, différant des "proverbes" qui sont des propos répétés dans la langue orale et qui incarnent souvent la sagesse populaire d'un groupe ou d'une nation. "</skos:definition>
    <rdfs:label xml:lang="en">aphorism</rdfs:label>
    <owl:sameAs rdf:resource="http://vocab.getty.edu/aat/300253001"/>
    <rdfs:comment xml:lang="en">The description for this term is indebted to the Getty Art &amp; Architecture Thesaurus.</rdfs:comment>
  </genre:ProverbForm>
  <genre:ParatextualGenre rdf:about="http://sparql.cwrc.ca/ontologies/genre#annotation">
    <rdfs:label xml:lang="en">annotation</rdfs:label>
    <skos:definition xml:lang="fr">"Notes ajoutées en tant que commentaires ou explications, comme celles qui accompagnent les entrées d'une bibliographie, une liste de lecture, ou un catalogue voué à décrire, expliquer ou évaluer la publication à laquelle on se réfère. "</skos:definition>
    <rdfs:label xml:lang="fr">annotation</rdfs:label>
    <owl:sameAs rdf:resource="http://vocab.getty.edu/aat/300026100"/>
    <skos:definition xml:lang="en">"Notes added as comment or explanation, such as those accompanying an entry in a bibliography, reading list, or catalogue intended to describe, explain, or evaluate the publication referred to." <![CDATA[(<a href="#cwrc:db2f8571-a773-4068-a35f-34262950bb8f">Getty, 2017</a>)]]></skos:definition>
    <rdfs:comment xml:lang="en">The description for this term is indebted to the Getty Art &amp; Architecture Thesaurus.</rdfs:comment>
  </genre:ParatextualGenre>
  <genre:DramaticGenre rdf:about="http://sparql.cwrc.ca/ontologies/genre#melodrama">
    <rdfs:label xml:lang="fr">mélodrame</rdfs:label>
    <skos:definition xml:lang="en">"A dramatic form characterized by excessive sentiment, exaggerated emotion, sensational and thrilling action, and an artificially happy ending. Melodramas originally referred to romantic plays featuring music, singing, and dancing, but by the eighteenth century they connoted simplified and coincidental plots, bathos, and happy endings. These melodramatic traits are present in Gothic novels, western stories, popular films, and television crime shows, to name but a few more recent examples." <![CDATA[(<a href="cwrc:509015ff-7641-473e-94c5-688e06952bb7">L. K Wheeler, 2017</a>)]]></skos:definition>
    <owl:sameAs rdf:resource="http://id.loc.gov/authorities/genreForms/gf2014026432"/>
    <owl:sameAs rdf:resource="http://dbpedia.org/resource/Melodrama"/>
    <skos:definition xml:lang="fr">«Le mélodrame, du grec μέλος = chant ou musique + δράμα = action théâtrale, est un genre théâtral dramatique et populaire, qui signifie étymologiquement drame avec musique très populaire au XIXe siècle, se caractérisant par des situations invraisemblables et des personnages manichéens (bons contre méchants).» <![CDATA[(<a href="#cwrc:727d97bc-af78-4122-94be-aa78b2e97d5a">DBpedia, 2017</a>)]]></skos:definition>
    <rdfs:label xml:lang="en">melodrama</rdfs:label>
  </genre:DramaticGenre>
  <genre:InformationalGenre rdf:about="http://sparql.cwrc.ca/ontologies/genre#governmentReport">
    <skos:definition xml:lang="en">An official government publication covering any of a wide variety of subjects.</skos:definition>
    <skos:definition xml:lang="fr">Publication officielle émise par un gouvernement, couvrant une large variété de sujets.</skos:definition>
    <rdfs:label xml:lang="fr">rapport gouvernemental</rdfs:label>
    <rdfs:label xml:lang="en">government report</rdfs:label>
  </genre:InformationalGenre>
  <genre:ScholarlyGenre rdf:about="http://sparql.cwrc.ca/ontologies/genre#literaryCriticism">
    <skos:definition xml:lang="fr">«La critique littéraire est l'étude, la discussion, l'évaluation et l'interprétation de la littérature. Elle peut prendre la forme d'un discours théorique s'appuyant sur la théorie de la littérature ou bien d'un discours plus circonstancié, de présentation ou de compte rendu d'une œuvre littéraire (souvent sous une forme journalistique lors de sa parution). Ces deux acceptions ne sont pas diamétralement opposées bien que la seconde se distingue par le jugement qu'elle porte sur les œuvres étudiées.» <![CDATA[(<a href="#cwrc:727d97bc-af78-4122-94be-aa78b2e97d5a">DBpedia, 2017</a>)]]></skos:definition>
    <rdfs:label xml:lang="en">literary criticism</rdfs:label>
    <skos:definition xml:lang="en">Writing that analyzes or critiques a literary work, often through the use of a particular literary theory, and typically in the form of an essay.</skos:definition>
    <rdfs:comment xml:lang="en">This term and its description were created from data gathered from DBpedia.</rdfs:comment>
    <skos:closeMatch rdf:resource="http://dbpedia.org/resource/Literary_criticism"/>
    <owl:sameAs rdf:resource="http://id.loc.gov/authorities/genreForms/gf2017026126"/>
    <rdfs:label xml:lang="fr">critique littéraire</rdfs:label>
  </genre:ScholarlyGenre>
  <genre:NarrativeGenre rdf:about="http://sparql.cwrc.ca/ontologies/genre#episodicLiterature">
    <rdfs:label xml:lang="en">episodic literature</rdfs:label>
  </genre:NarrativeGenre>
  <genre:FictionalGenre rdf:about="http://sparql.cwrc.ca/ontologies/genre#utopia">
    <skos:definition xml:lang="en">"An imaginary place or government in which political and social perfection has been reached in the material world as opposed to some spiritual afterlife as discussed in the Christian Bible or the Elysian fields of The Odyssey. The citizens of such utopias are typically universally clean, virtuous, healthy, and happy, or at least those who are criminals are always captured and appropriately punished. A utopian society is one that has cured all social ills. See discussion under Utopian literature, below. Contrast with dystopia. UTOPIAN" <![CDATA[(<a href="cwrc:509015ff-7641-473e-94c5-688e06952bb7">L. K Wheeler, 2017</a>)]]></skos:definition>
    <skos:definition xml:lang="fr">«L’utopie (mot forgé par l'écrivain anglais Thomas More, du grec οὐ-τόπος « en aucun lieu ») est une représentation d'une réalité idéale et sans défaut. C'est un genre d'apologue qui se traduit, dans les écrits, par un régime politique idéal (qui gouvernerait parfaitement les hommes), une société parfaite (sans injustice par exemple, comme la Callipolis de Platon ou la découverte de l'Eldorado dans Candide) ou encore une communauté d'individus vivant heureux et en harmonie (l'abbaye de Thélème dans Gargantua de Rabelais en 1534), souvent écrites pour dénoncer les injustices et dérives de leurs temps.» <![CDATA[(<a href="#cwrc:727d97bc-af78-4122-94be-aa78b2e97d5a">DBpedia, 2017</a>)]]></skos:definition>
    <dcterms:references rdf:resource="http://web.cn.edu/kwheeler/lit_terms_u.html"/>
    <rdfs:label xml:lang="en">utopia</rdfs:label>
    <rdfs:label xml:lang="fr">utopie</rdfs:label>
    <rdfs:comment xml:lang="en">This term and its description were created from data gathered from DBpedia.</rdfs:comment>
    <owl:sameAs rdf:resource="http://id.loc.gov/authorities/genreForms/gf2014026583"/>
  </genre:FictionalGenre>
  <genre:InformationalGenre rdf:about="http://sparql.cwrc.ca/ontologies/genre#profileOfAuthor">
    <rdfs:label xml:lang="en">profile of author</rdfs:label>
  </genre:InformationalGenre>
  <genre:ScholarlyGenre rdf:about="http://sparql.cwrc.ca/ontologies/genre#musicology">
    <owl:sameAs rdf:resource="http://vocab.getty.edu/aat/300054240"/>
    <rdfs:label xml:lang="en">musicology</rdfs:label>
    <skos:definition xml:lang="fr">«La musicologie est une discipline qui étudie les phénomènes en relation avec la musique, dans leur essence (sémiologie musicale, analyse, théorie), leur évolution (histoire des idées et des théories musicales) et dans leur rapport avec l'être humain et la société, domaines plus particulièrement abordés par l'ethnomusicologie et la sociologie de la musique. La seconde catégorie est d'ordre conceptuel, et tend surtout à comparer les statuts de l'œuvre musicale d'hier et de celle d'aujourd'hui, et à analyser toute l'évolution de la musique selon cette optique.» <![CDATA[(<a href="#cwrc:727d97bc-af78-4122-94be-aa78b2e97d5a">DBpedia, 2017</a>)]]></skos:definition>
    <rdfs:label xml:lang="fr">musicologie</rdfs:label>
    <skos:definition xml:lang="en">"Writing dealing with the scientific study of music." <![CDATA[(<a href="#cwrc:db2f8571-a773-4068-a35f-34262950bb8f">Getty, 2017</a>)]]></skos:definition>
    <rdfs:comment xml:lang="en">This term and its description were created from data gathered from DBpedia.</rdfs:comment>
  </genre:ScholarlyGenre>
  <genre:DramaticGenre rdf:about="http://sparql.cwrc.ca/ontologies/genre#moralityOrMysteryPlay">
    <skos:definition xml:lang="en">"Religious dramas or pageants, typically written anonymously, that were popular in medieval Europe. Mystery plays represent one or more scenes from the Bible, and were first performed in the 13th century, often using a wagon as a stage to allow a performance to take place in various locations, . Morality plays were first popularized in the 15th century, and are allegorical rather than directly representational works in which personified vices and virtues compete to win a human soul for eternity." <![CDATA[(<a href="#cwrc:4c227091-6bf0-4325-b846-9733fae19e61">Oxford, 2015</a>)]]></skos:definition>
    <dcterms:references rdf:resource="http://www.oxfordreference.com/view/10.1093/acref/9780199208272.001.0001/acref-9780199208272-e-745?rskey=1MnHpb%26result=741"/>
    <owl:sameAs rdf:resource="http://id.loc.gov/authorities/genreForms/gf2014026442"/>
    <rdfs:comment xml:lang="en">This term and its description were created from data gathered from the Oxford Dictionary of Literary Terms, 4th ed.</rdfs:comment>
    <rdfs:label xml:lang="en">morality or mystery play</rdfs:label>
  </genre:DramaticGenre>
  <genre:ReferenceWorkGenre rdf:about="http://sparql.cwrc.ca/ontologies/genre#directory">
    <owl:sameAs rdf:resource="http://id.loc.gov/authorities/genreForms/gf2014026087"/>
    <owl:sameAs rdf:resource="http://vocab.getty.edu/aat/300026234"/>
    <rdfs:label xml:lang="en">directory</rdfs:label>
    <rdfs:comment xml:lang="en">The description for this term is indebted to the Getty Art &amp; Architecture Thesaurus.</rdfs:comment>
    <rdfs:label xml:lang="fr">répertoire</rdfs:label>
    <skos:definition xml:lang="fr">"Énumérations de noms, d'adresses et d'autres données concernant des groupes spécifiques de personnes ou des organisations; apparaît sous forme alphabétique ou graphique. "</skos:definition>
    <skos:definition xml:lang="en">"Enumerations of names, addresses, and other data about specific groups of persons or organizations; may appear in alphabetic or graphic format." <![CDATA[(<a href="#cwrc:db2f8571-a773-4068-a35f-34262950bb8f">Getty, 2017</a>)]]></skos:definition>
  </genre:ReferenceWorkGenre>
  <genre:PoliticalWritingGenre rdf:about="http://sparql.cwrc.ca/ontologies/genre#manifesto">
    <rdfs:label xml:lang="en">manifesto</rdfs:label>
    <owl:sameAs rdf:resource="http://id.loc.gov/authorities/genreForms/gf2017027243"/>
    <owl:sameAs rdf:resource="http://vocab.getty.edu/aat/300026393"/>
    <rdfs:label xml:lang="fr">manifeste</rdfs:label>
    <rdfs:comment xml:lang="en">This term and its description were created from data gathered from DBpedia.</rdfs:comment>
    <skos:definition xml:lang="fr">«Un manifeste est une déclaration écrite et publique par laquelle un gouvernement, une personne, un parti ou un courant artistique expose un programme d'action ou une position, le plus souvent politique ou esthétique.» <![CDATA[(<a href="#cwrc:727d97bc-af78-4122-94be-aa78b2e97d5a">DBpedia, 2017</a>)]]></skos:definition>
    <skos:definition xml:lang="en">"Formal written declarations, promulgated by a sovereign or by the executive authority of a state or nation, such as to proclaim its reasons and motives for declaring a war, or other international action; also public declarations or proclamations of political, social, artistic, or other principles." <![CDATA[(<a href="#cwrc:db2f8571-a773-4068-a35f-34262950bb8f">Getty, 2017</a>)]]></skos:definition>
  </genre:PoliticalWritingGenre>
  <genre:PhilosophicalGenre rdf:about="http://sparql.cwrc.ca/ontologies/genre#philosophical">
    <rdfs:label xml:lang="fr">philosophique</rdfs:label>
    <rdfs:label xml:lang="en">philosophical</rdfs:label>
    <skos:definition xml:lang="fr">Textes qui abordent des questions philosophiques, qui sont ou non considérés comme de la philosophie à proprement parler.</skos:definition>
    <skos:definition xml:lang="en">Writing engaging in philosophical questions, that may or may not be considered philosophy per se.</skos:definition>
  </genre:PhilosophicalGenre>
  <genre:AutobiographicalGenre rdf:about="http://sparql.cwrc.ca/ontologies/genre#sexualAwakeningFiction">
    <rdfs:label xml:lang="fr">éveil à la sexualité</rdfs:label>
    <skos:definition xml:lang="en">Fiction in which a character, typically an adolescent, experiences sexual desires for the first time or has a first sexual encounter.</skos:definition>
    <skos:definition xml:lang="fr">Œuvres de fiction dans lesquelles un personnage, généralement un adolescent, éprouve des désirs sexuels pour la première fois ou connait sa première expérience sexuelle.</skos:definition>
    <rdfs:label xml:lang="en">sexual awakening fiction</rdfs:label>
  </genre:AutobiographicalGenre>
  <genre:DramaticGenre rdf:about="http://sparql.cwrc.ca/ontologies/genre#closetDrama">
    <dcterms:references rdf:resource="http://www.oxfordreference.com/view/10.1093/acref/9780199208272.001.0001/acref-9780199208272-e-214?rskey=qZ7ZtK%26result=211"/>
    <rdfs:label xml:lang="fr">pièce en chambre</rdfs:label>
    <rdfs:label xml:lang="en">closet drama</rdfs:label>
    <skos:definition xml:lang="en">"A drama, often written in verse and frequently with extensive stage directions, that is meant to be read in private rather than performed for an audience." <![CDATA[(<a href="#cwrc:4c227091-6bf0-4325-b846-9733fae19e61">Oxford, 2015</a>)]]></skos:definition>
    <rdfs:comment xml:lang="en">This term and its description were created from data gathered from the Oxford Dictionary of Literary Terms, 4th ed.</rdfs:comment>
  </genre:DramaticGenre>
  <genre:EpistolaryGenre rdf:about="http://sparql.cwrc.ca/ontologies/genre#lettersFromTheDeadToTheLiving">
    <rdfs:label xml:lang="en">letters from the dead to the living</rdfs:label>
    <skos:definition xml:lang="en">Moralised case-histories in the form of letters in which the dead strive to reclaim the living beloved by persuading them to repent and reform. Often include features of lively fiction: character-drawing, narrative, suspense, surprise, humour, and love-situations including transgression of all kinds.</skos:definition>
    <rdfs:label xml:lang="fr">lettres des morts aux vivants</rdfs:label>
    <skos:definition xml:lang="fr">Histoires illustrant des leçons morales sous forme de lettres dans lesquelles les morts s'efforcent de persuader des proches toujours en vie de se repentir et d'améliorer leur conduite. Inclut souvent des caractéristiques propre à la fiction divertissante, comme le portrait de personnage, le récit, le suspense, la surprise, l'humour et les romances, y compris des transgressions de toutes sortes.</skos:definition>
  </genre:EpistolaryGenre>
  <genre:ThematicWritingGenre rdf:about="http://sparql.cwrc.ca/ontologies/genre#sensational">
    <rdfs:label xml:lang="en">sensational</rdfs:label>
  </genre:ThematicWritingGenre>
  <genre:DramaticGenre rdf:about="http://sparql.cwrc.ca/ontologies/genre#panegyric">
    <skos:related rdf:resource="http://id.loc.gov/authorities/genreForms/gf2014026095"/>
    <rdfs:label xml:lang="en">panegyric</rdfs:label>
    <skos:definition xml:lang="en">"A speech or poem designed to praise another person or group. In ancient Greek and Roman rhetoric, it was one branch of public speaking, with established rules and conventions found in the works of Menander and Hermogenes. Famous examples include Pliny's eulogy on Emperor Trajan and Isocrates' oration on the Olympic games of 380." <![CDATA[(<a href="cwrc:509015ff-7641-473e-94c5-688e06952bb7">L. K Wheeler, 2017</a>)]]></skos:definition>
    <skos:definition xml:lang="fr">«L’éloge panégyrique ou simplement le panégyrique, du latin emprunté au grec panêguris, « assemblée de tout le peuple », est au sens strict un discours public à la louange d'un personnage illustre, d'une nation, ou d'une chose et, dans l'occident chrétien, un sermon faisant l'éloge d'un saint. Le terme a pris aujourd'hui le sens plus général de louange ou d’apologie, et s’utilise parfois dans le sens péjoratif d’éloge emphatique ou exagéré.» <![CDATA[(<a href="#cwrc:727d97bc-af78-4122-94be-aa78b2e97d5a">DBpedia, 2017</a>)]]></skos:definition>
    <rdfs:label xml:lang="fr">panégyrique</rdfs:label>
    <dcterms:references rdf:resource="http://web.cn.edu/kwheeler/lit_terms_p.html"/>
    <rdfs:comment xml:lang="en">This term and its description were created from data gathered from DBpedia.</rdfs:comment>
  </genre:DramaticGenre>
  <genre:ScriptForm rdf:about="http://sparql.cwrc.ca/ontologies/genre#radioScript">
    <rdfs:label xml:lang="en">radio script</rdfs:label>
  </genre:ScriptForm>
  <genre:ThematicWritingGenre rdf:about="http://sparql.cwrc.ca/ontologies/genre#western">
    <owl:sameAs rdf:resource="http://id.loc.gov/authorities/genreForms/gf2014026594"/>
    <rdfs:label xml:lang="en">western</rdfs:label>
  </genre:ThematicWritingGenre>
  <genre:PoliticalWritingGenre rdf:about="http://sparql.cwrc.ca/ontologies/genre#tractPamphlet">
    <skos:definition xml:lang="en">"Writing printed on a single sheet of paper or in a small booklet, designed to be distributed to the public. The subject matter is typically religious or political, and aims to persuade the reader of a certain point of view." <![CDATA[(<a href="#cwrc:db2f8571-a773-4068-a35f-34262950bb8f">Getty, 2017</a>)]]></skos:definition>
    <rdfs:label xml:lang="en">tract pamphlet</rdfs:label>
    <skos:definition xml:lang="fr">«Un tract, un prospectus ou en français feuille volante, en anglais flyer (le terme pamphlet est également utilisé au Québec, et le terme manifeste en suisse francophone) est un texte ou une publicité sur support papier qui est distribué de la main à la main dans les espaces publics, en particulier sur les trottoirs, ou directement déposé dans les boîtes aux lettres par des personnes employées à cette tâche ou agissant par militantisme afin de faire passer des idées, de promouvoir un produit ou d'annoncer un événement artistique, culturel ou politique. Lorsque l'objet est purement commercial, on parle plutôt de prospectus.» <![CDATA[(<a href="#cwrc:727d97bc-af78-4122-94be-aa78b2e97d5a">DBpedia, 2017</a>)]]></skos:definition>
    <owl:sameAs rdf:resource="http://dbpedia.org/resource/Flyer_(pamphlet)"/>
    <rdfs:label xml:lang="fr">tract</rdfs:label>
    <owl:sameAs rdf:resource="http://id.loc.gov/authorities/genreForms/gf2015026053"/>
    <rdfs:comment xml:lang="en">This term and its description were created from data gathered from DBpedia.</rdfs:comment>
  </genre:PoliticalWritingGenre>
  <genre:ThematicWritingGenre rdf:about="http://sparql.cwrc.ca/ontologies/genre#war">
    <rdfs:label xml:lang="en">war</rdfs:label>
  </genre:ThematicWritingGenre>
  <genre:DramaticGenre rdf:about="http://sparql.cwrc.ca/ontologies/genre#afterpiece">
    <skos:definition xml:lang="fr">Courte pièce de théâtre représentée à la suite d'une pièce principale, rendue populaire au 18ᵉ siècle afin de justifier pour un supplément s'élevant à la moitié du prix d'entrée qui était facturé aux retardataires. L'afterpiece était généralement une comédie en un acte sans relation avec le genre de la pièce qui précédait.</skos:definition>
    <rdfs:label xml:lang="fr">afterpiece</rdfs:label>
    <skos:definition xml:lang="en">"A short drama performed after a main play, popularized in the 1700s as justification for a new half-price entrance fee charged to latecomers. Typically a comedic one-act, regardless of the genre of the preceding play." <![CDATA[(<a href="#cwrc:2f09376c-f784-4a46-9f04-5a21aa311f27">Penguin, 1999</a>)]]></skos:definition>
    <rdfs:label xml:lang="en">afterpiece</rdfs:label>
    <rdfs:comment xml:lang="en">This term and its description were created from data gathered from the Penguin Dictionary of Literary Terms &amp; Literary Theory, 4th ed.</rdfs:comment>
  </genre:DramaticGenre>
  <genre:SongGenre rdf:about="http://sparql.cwrc.ca/ontologies/genre#anthem">
    <rdfs:comment xml:lang="en">This term and its description were created from data gathered from the Oxford Dictionary of Literary Terms, 4th ed.</rdfs:comment>
    <rdfs:label xml:lang="en">anthem</rdfs:label>
    <skos:definition xml:lang="en">"A song in which the lyrics promote pride in and allegiance to the identity and values of a particular group, such as a nation, sports team, or social cause." <![CDATA[(<a href="#cwrc:4c227091-6bf0-4325-b846-9733fae19e61">Oxford, 2015</a>)]]></skos:definition>
    <skos:definition xml:lang="fr">Une chanson dont les paroles promeuvent la fidélité à l'identité et aux valeurs d'un groupe particulier —une nation, une équipe sportive ou une cause sociale— ainsi que la fierté d'y adhérer.</skos:definition>
    <owl:sameAs rdf:resource="http://id.loc.gov/authorities/genreForms/gf2014026635"/>
    <dcterms:references rdf:resource="http://www.oxfordreference.com/view/10.1093/acref/9780199208272.001.0001/acref-9780199208272-e-61?rskey=9jlyTO%26result=61"/>
    <rdfs:label xml:lang="fr">hymne (politique)</rdfs:label>
  </genre:SongGenre>
  <genre:PoeticGenre rdf:about="http://sparql.cwrc.ca/ontologies/genre#elegy">
    <skos:definition xml:lang="en">"Mournful, melancholy, or plaintive poems, especially funeral songs or laments for the dead." <![CDATA[(<a href="#cwrc:db2f8571-a773-4068-a35f-34262950bb8f">Getty, 2017</a>)]]></skos:definition>
    <rdfs:comment xml:lang="en">The description for this term is indebted to the Getty Art &amp; Architecture Thesaurus.</rdfs:comment>
    <skos:definition xml:lang="fr">«L’élégie (en grec ancien ἐλεγεία / elegeía, signifiant « chant de mort ») fut une forme de poème dans l'Antiquité, avant de devenir un genre poétique à partir de la Renaissance. Dans l’Antiquité, était appelé « élégie » tout poème alternant hexamètres et pentamètres en distiques : ce sont les vers élégiaques. De nos jours, l’élégie est considérée comme un genre au sein de la poésie lyrique, en tant que poème de longueur et de forme variables caractérisé par son ton plaintif particulièrement adapté à l’évocation d’un mort ou à l’expression d’une souffrance amoureuse due à un abandon ou à une absence.» <![CDATA[(<a href="#cwrc:727d97bc-af78-4122-94be-aa78b2e97d5a">DBpedia, 2017</a>)]]></skos:definition>
    <owl:sameAs rdf:resource="http://vocab.getty.edu/aat/300026285"/>
    <owl:sameAs rdf:resource="http://id.loc.gov/authorities/genreForms/gf2014026307"/>
    <rdfs:label xml:lang="en">elegy</rdfs:label>
    <rdfs:label xml:lang="fr">élégie</rdfs:label>
  </genre:PoeticGenre>
  <genre:ParatextualGenre rdf:about="http://sparql.cwrc.ca/ontologies/genre#paratext">
    <skos:definition xml:lang="en">"Text surrounding the main body of a written work that contains supplementary information about the body, such as a preface, afterword, footnote, or glossary." <![CDATA[(<a href="#cwrc:4c227091-6bf0-4325-b846-9733fae19e61">Oxford, 2015</a>)]]></skos:definition>
    <rdfs:label xml:lang="en">paratext</rdfs:label>
    <dcterms:references rdf:resource="https://books.google.ca/books?id=s4FMCAAAQBAJ&amp;printsec=frontcover&amp;source=gbs_ge_summary_r&amp;cad=0#v=onepage&amp;q&amp;f=false"/>
    <rdfs:comment xml:lang="en">This term and its description were created from data gathered from the Oxford Dictionary of Literary Terms, 4th ed.</rdfs:comment>
    <rdfs:label xml:lang="fr">paratextes</rdfs:label>
  </genre:ParatextualGenre>
  <genre:PoliticalWritingGenre rdf:about="http://sparql.cwrc.ca/ontologies/genre#politicalStatement">
    <rdfs:label xml:lang="en">political Statement</rdfs:label>
  </genre:PoliticalWritingGenre>
  <genre:FictionalGenre rdf:about="http://sparql.cwrc.ca/ontologies/genre#fiction">
    <rdfs:label xml:lang="en">fiction</rdfs:label>
    <rdfs:label xml:lang="fr">fiction</rdfs:label>
    <skos:definition xml:lang="en">"Genre that refers to works evoked from the imagination of the writer and not conferred as fact. In literature, fiction generally refers to the novel, novella, short story, and poetic forms." <![CDATA[(<a href="#cwrc:db2f8571-a773-4068-a35f-34262950bb8f">Getty, 2017</a>)]]></skos:definition>
    <skos:definition xml:lang="fr">Genre that refers to works evoked from the imagination of the writer and not conferred as fact. In literature, fiction generally refers to the novel, novella, short story, and poetic forms.</skos:definition>
    <owl:sameAs rdf:resource="http://vocab.getty.edu/aat/300055918"/>
    <rdfs:comment xml:lang="en">The description for this term is indebted to the Getty Art &amp; Architecture Thesaurus.</rdfs:comment>
    <owl:sameAs rdf:resource="http://id.loc.gov/authorities/genreForms/gf2014026333"/>
  </genre:FictionalGenre>
  <genre:EpistolaryGenre rdf:about="http://sparql.cwrc.ca/ontologies/genre#letter">
    <skos:definition xml:lang="fr">Pièces de correspondance qui sont légèrement plus formelles que le mémorandum ou des notes, habituellement écrites sur papier et destinées à être envoyées à un destinataire.</skos:definition>
    <owl:sameAs rdf:resource="http://vocab.getty.edu/aat/300026879"/>
    <rdfs:label xml:lang="fr">lettre</rdfs:label>
    <skos:altLabel xml:lang="en">correspondence</skos:altLabel>
    <rdfs:comment xml:lang="en">This term and its description were created from data gathered from the Getty Art &amp; Architecture Thesaurus.</rdfs:comment>
    <skos:definition xml:lang="en">"Pieces of correspondence that are somewhat more formal than memoranda or notes, usually on paper and delivered." <![CDATA[(<a href="#cwrc:db2f8571-a773-4068-a35f-34262950bb8f">Getty, 2017</a>)]]></skos:definition>
    <rdfs:label xml:lang="en">letter</rdfs:label>
  </genre:EpistolaryGenre>
  <genre:IllustratedForm rdf:about="http://sparql.cwrc.ca/ontologies/genre#photoEssay">
    <rdfs:label xml:lang="en">photo essay</rdfs:label>
  </genre:IllustratedForm>
  <genre:CalendarForm rdf:about="http://sparql.cwrc.ca/ontologies/genre#calendar">
    <rdfs:label xml:lang="en">calendar</rdfs:label>
  </genre:CalendarForm>
  <genre:ChildrensLiteratureGenre rdf:about="http://sparql.cwrc.ca/ontologies/genre#nurseryRhyme">
    <owl:sameAs rdf:resource="http://vocab.getty.edu/aat/300202593"/>
    <owl:sameAs rdf:resource="http://id.loc.gov/authorities/genreForms/gf2014026459"/>
    <rdf:type rdf:resource="http://sparql.cwrc.ca/ontologies/genre#PoeticGenre"/>
    <rdfs:comment xml:lang="en">The description for this term is indebted to the Getty Art &amp; Architecture Thesaurus.</rdfs:comment>
    <rdfs:label xml:lang="en">nursery rhyme</rdfs:label>
    <skos:definition xml:lang="en">"Tales in rhymed verse for children." <![CDATA[(<a href="#cwrc:db2f8571-a773-4068-a35f-34262950bb8f">Getty, 2017</a>)]]></skos:definition>
  </genre:ChildrensLiteratureGenre>
  <genre:SongGenre rdf:about="http://sparql.cwrc.ca/ontologies/genre#oratorio">
    <skos:definition xml:lang="fr">«Un oratorio est une œuvre lyrique dramatique représentée sans mise en scène, ni costumes, ni décors. Généralement composé pour voix solistes, chœur et orchestre symphonique, avec parfois un narrateur, son sujet est le plus souvent religieux (épisode extrait de la Bible, de la vie de Jésus, d’un(e) saint(e)… ) mais peut être aussi profane (héros mythologique, sujet historique, hymne à la nature…). Formellement assez proche de la cantate et de l’opéra, l'oratorio comprend généralement une ouverture, des récitatifs, des airs et des chœurs.» <![CDATA[(<a href="#cwrc:727d97bc-af78-4122-94be-aa78b2e97d5a">DBpedia, 2017</a>)]]></skos:definition>
    <owl:sameAs rdf:resource="http://dbpedia.org/resource/Oratorio"/>
    <skos:definition xml:lang="en">"A lengthy musical composition for voice and orchestra, typically narrative and religious in nature. Unlike an opera, it is not a theatrical performance and does not include costumes or sets." <![CDATA[(<a href="#cwrc:4c227091-6bf0-4325-b846-9733fae19e61/">Oxford, 2015</a>)]]></skos:definition>
    <rdfs:label xml:lang="en">oratorio</rdfs:label>
    <rdfs:comment xml:lang="en">This term and its description were created from data gathered from DBpedia.</rdfs:comment>
    <rdfs:label xml:lang="fr">oratorio</rdfs:label>
    <owl:sameAs rdf:resource="http://id.loc.gov/authorities/genreForms/gf2014026977"/>
  </genre:SongGenre>
  <genre:DialogueOrDebateGenre rdf:about="http://sparql.cwrc.ca/ontologies/genre#dialogueOfTheDead">
    <dcterms:references rdf:resource="https://books.google.ca/books?id=8zBk8k35SFEC&amp;printsec=frontcover#v=onepage&amp;q&amp;f=false"/>
    <rdfs:label xml:lang="fr">dialogue des morts</rdfs:label>
    <rdfs:label xml:lang="en">dialogue of the dead</rdfs:label>
    <skos:definition xml:lang="en">"A popular style of fiction in the 17th and 18th centuries featuring conversations between the ghosts of well-known figures. Based on the satirical Dialogues of the Dead by Lucian (120-around 180 CE), but not necessarily satirical themselves." <![CDATA[(<a href="#cwrc:93fc3195-0bd5-4161-a123-0352d96c42ab">Mazella, 2007</a>)]]></skos:definition>
    <rdfs:comment xml:lang="en">This term and its description were created from data gathered from data.bnf.fr.</rdfs:comment>
    <skos:definition xml:lang="fr">Mise en scène littéraire de la parole de personnages illustres dans l'au-delà, pratiquée dans l'Antiquité grecque, et jusqu'à nos jours.</skos:definition>
  </genre:DialogueOrDebateGenre>
  <genre:HistoricalGenre rdf:about="http://sparql.cwrc.ca/ontologies/genre#history">
    <rdfs:label xml:lang="fr">histoire</rdfs:label>
    <owl:sameAs rdf:resource="http://vocab.getty.edu/aat/300026358"/>
    <rdfs:label xml:lang="en">history</rdfs:label>
    <skos:definition xml:lang="fr">Comptes rendus chronologiques d'événements importants, à partir de la vie ou du développement d'un peuple, d'un pays ou d'une institution, souvent accompagnés d'explications et de leurs causes.</skos:definition>
    <skos:definition xml:lang="en">"Chronological records of significant events, as of the life or development of a people, country, or institution, often with an explanation of the causes." <![CDATA[(<a href="#cwrc:db2f8571-a773-4068-a35f-34262950bb8f">Getty, 2017</a>)]]></skos:definition>
    <rdfs:comment xml:lang="en">The description for this term is indebted to the Getty Art &amp; Architecture Thesaurus.</rdfs:comment>
  </genre:HistoricalGenre>
  <genre:SatiricalGenre rdf:about="http://sparql.cwrc.ca/ontologies/genre#satire">
    <owl:sameAs rdf:resource="http://dbpedia.org/resource/Satire"/>
    <rdfs:label xml:lang="en">satire</rdfs:label>
    <skos:definition xml:lang="en">"Literary compositions in verse or prose, or ideas expressed as the subjects of art works, in which human folly and vice are held up to scorn, derision, or ridicule." <![CDATA[(<a href="#cwrc:db2f8571-a773-4068-a35f-34262950bb8f">Getty, 2017</a>)]]></skos:definition>
    <rdfs:comment xml:lang="en">The description for this term is indebted to DBpedia. </rdfs:comment>
    <rdf:type rdf:resource="http://sparql.cwrc.ca/ontologies/genre#IntertextualGenre"/>
    <owl:sameAs rdf:resource="http://id.loc.gov/authorities/genreForms/gf2014026525"/>
    <skos:definition xml:lang="fr">«Une satire est une œuvre dont l'objectif est une critique moqueuse de son sujet (des individus, des organisations, des États, etc.), souvent dans l'intention de provoquer, prévenir un changement ou de porter à réfléchir. On attribue généralement la paternité de ce genre littéraire (satura, c'est-à-dire pot-pourri) au poète archaïque latin Lucilius.» <![CDATA[(<a href="#cwrc:727d97bc-af78-4122-94be-aa78b2e97d5a">DBpedia, 2017</a>)]]></skos:definition>
    <rdfs:label xml:lang="fr">satire</rdfs:label>
  </genre:SatiricalGenre>
  <genre:EpistolaryGenre rdf:about="http://sparql.cwrc.ca/ontologies/genre#epistle">
    <rdfs:label xml:lang="fr">épître></rdfs:label>
    <skos:definition xml:lang="en">"Literary genre taking the form of letters, usually of a literary, formal, or public nature. Examples are the epistles in the Biblical New Testament." <![CDATA[(<a href="#cwrc:db2f8571-a773-4068-a35f-34262950bb8f">Getty, 2017</a>)]]></skos:definition>
    <skos:definition xml:lang="fr">«Le terme épître, issu du latin epistula, du grec επιστολη (epistolē), désigne une lettre (au sens de correspondance).Il a pris le sens aujourd'hui d'un court traité philosophique ou religieux exposé sous forme épistolaire. Ce sont de courts traités le plus souvent philosophiques. Ce peuvent être aussi des « conversations en l'absence » de l'interlocuteur sur des aspects sociaux ou moraux de l'existence. Au fil du temps, l’épître devient, en littérature, un discours en vers du genre académique ou didactique. Elle prend rapidement le sens d’épigramme nettement moins acerbe que la satire.Le mot « épître » est un nom commun féminin. Le Nouveau Testamen» contient plusieur" <![CDATA[(<a href="#cwrc:727d97bc-af78-4122-94be-aa78b2e97d5a">DBpedia, 2017</a>)
s épîtres.]]></skos:definition>
    <rdfs:label xml:lang="en">epistle</rdfs:label>
    <rdfs:comment xml:lang="en">The description for this term is indebted to DBpedia. </rdfs:comment>
    <owl:sameAs rdf:resource="http://dbpedia.org/resource/Epistle"/>
  </genre:EpistolaryGenre>
  <genre:SongGenre rdf:about="http://sparql.cwrc.ca/ontologies/genre#folkSong">
    <skos:definition xml:lang="en">"A song recorded or transcribed after being preserved for generations by a particular culture through an oral tradition, or more recent songs composed in the style of that tradition." <![CDATA[(<a href="#cwrc:4c227091-6bf0-4325-b846-9733fae19e61">Oxford, 2015</a>)]]></skos:definition>
    <skos:definition xml:lang="fr">Chanson enregistrée ou retranscrite après avoir été transmire de génération en génération suivant une tradition orale au sein d'une culture spécifique, ou chansons plus récentes composées dans le style de cette tradition.</skos:definition>
    <rdfs:comment xml:lang="en">This term and its description were created from data gathered from the Oxford Dictionary of Literary Terms, 4th ed.</rdfs:comment>
    <dcterms:references rdf:resource="http://www.oxfordreference.com/view/10.1093/acref/9780199208272.001.0001/acref-9780199208272-e-470?rskey=icg8D9%26result=461"/>
    <owl:sameAs rdf:resource="http://id.loc.gov/authorities/genreForms/gf2014026811"/>
    <rdfs:label xml:lang="en">folk song</rdfs:label>
    <rdfs:label xml:lang="fr">chanson populaire</rdfs:label>
  </genre:SongGenre>
  <genre:InformationalGenre rdf:about="http://sparql.cwrc.ca/ontologies/genre#genealogy">
    <skos:definition xml:lang="fr">«La généalogie (du grec γενεά genea, « génération » et λόγος logos, « connaissance ») est la « liste des membres d'une famille établissant une filiation » ou la pratique qui a pour objet la recherche de la parenté et de la filiation des personnes. La généalogie est considérée comme une science auxiliaire de l'histoire. Historiquement, elle était utilisée par les gens aisés pour établir la noblesse de sang d'un individu.» <![CDATA[(<a href="#cwrc:727d97bc-af78-4122-94be-aa78b2e97d5a">DBpedia, 2017</a>)]]></skos:definition>
    <owl:sameAs rdf:resource="http://vocab.getty.edu/aat/300027015"/>
    <rdfs:comment xml:lang="en">This term and its description were created from data gathered from DBpedia.</rdfs:comment>
    <rdfs:label xml:lang="fr">généalogie</rdfs:label>
    <skos:related rdf:resource="http://id.loc.gov/authorities/genreForms/gf2014026100"/>
    <skos:definition xml:lang="en">"Accounts or histories of the descent of persons, families, or other groups, from an ancestor or ancestors; enumerations of ancestors and their descendants in the natural order of succession." <![CDATA[(<a href="#cwrc:db2f8571-a773-4068-a35f-34262950bb8f">Getty, 2017</a>)]]></skos:definition>
    <rdfs:label xml:lang="en">genealogy</rdfs:label>
  </genre:InformationalGenre>
  <genre:ReligiousGenre rdf:about="http://sparql.cwrc.ca/ontologies/genre#catechism">
    <skos:definition xml:lang="fr">«Dans la religion chrétienne, le catéchisme désigne l'instruction des doctrines de la foi chrétienne, particulièrement destinée aux enfants. Il prend souvent la forme d'une exposé officiel des articles de la foi, servant d'outil de base pour la catéchèse, qui est l'ensemble des actions destinées à éduquer des enfants, des jeunes et des adultes à la doctrine chrétienne. La catéchèse est une des composantes de la mission évangélique du christianisme.» <![CDATA[(<a href="#cwrc:727d97bc-af78-4122-94be-aa78b2e97d5a">DBpedia, 2017</a>)]]></skos:definition>
    <owl:sameAs rdf:resource="http://id.loc.gov/authorities/genreForms/gf2015026029"/>
    <rdfs:comment xml:lang="fr">La description de ce terme est basée sur celle de DBPedia.</rdfs:comment>
    <owl:sameAs rdf:resource="http://vocab.getty.edu/aat/300026460"/>
    <rdfs:comment xml:lang="en">The description for this term is indebted to DBpedia. </rdfs:comment>
    <rdfs:label xml:lang="fr">catéchisme</rdfs:label>
    <skos:definition xml:lang="en">"A catechism (/ˈkætəˌkizəm/; from Greek: κατηχέω, to teach orally), is a summary or exposition of doctrine and served as a learning introduction to the Sacraments traditionally used in catechesis, or Christian religious teaching of children and adult converts. Catechisms are doctrinal manuals - often in the form of questions followed by answers to be memorised - a format in non-religious or secular contexts as well. The term catechumen refers to the designated recipient of the catechetical work or instruction. In the Catholic Church, catachumens were usually placed separately during Holy Mass from those who received the Sacrament of Baptism. Early catecheticals emerged from Graeco-Roman mystery religions, especially the late cult of Mithras meant to educate their members into the secretive teachings, which competed with the Christian Church as an underground religion in the 1st to 4th centuries CE and allegedly shared its many ritual practices. Today, they are characteristic of Western Christianity but are also present in Eastern Christianity." <![CDATA[(<a href="#cwrc:727d97bc-af78-4122-94be-aa78b2e97d5a">DBpedia, 2017</a>)]]></skos:definition>
    <rdfs:label xml:lang="en">catechism</rdfs:label>
  </genre:ReligiousGenre>
  <genre:ScholarlyGenre rdf:about="http://sparql.cwrc.ca/ontologies/genre#psychoanalytical">
    <skos:definition xml:lang="fr">Écrits relatifs au domaine de la psychologie ou de la psychiatrie, en particulier dans le cadre des théories psychanalytiques de Sigmund Freud.</skos:definition>
    <rdfs:label xml:lang="en">psychoanalytical</rdfs:label>
    <rdfs:label xml:lang="fr">psychoanalytique</rdfs:label>
    <skos:definition xml:lang="en">Writing related to the field of psychology or psychiatry, particularly in connection with Sigmund Freud’s theories of psychoanalysis.</skos:definition>
  </genre:ScholarlyGenre>
  <genre:ParatextualGenre rdf:about="http://sparql.cwrc.ca/ontologies/genre#introduction">
    <rdfs:label xml:lang="en">introduction</rdfs:label>
    <rdfs:label xml:lang="fr">introduction</rdfs:label>
    <skos:definition xml:lang="fr">Section d'ouverture d'un texte, souvent sous forme d'essai, qui donne généralement un aperçu du propos du texte et explique les raisons pour lesquelles l'auteur.e l'a écrit.</skos:definition>
    <skos:definition xml:lang="en">"The opening section of a text, often in the form of an essay, that usually provides an overview of the text's subject matter and explains the author's reason for writing." <![CDATA[(<a href="#cwrc:2f09376c-f784-4a46-9f04-5a21aa311f27">Penguin, 1999</a>)]]></skos:definition>
    <rdfs:comment xml:lang="en">This term and its description were created from data gathered from the Penguin Dictionary of Literary Terms &amp; Literary Theory, 4th ed.</rdfs:comment>
  </genre:ParatextualGenre>
  <genre:PoeticGenre rdf:about="http://sparql.cwrc.ca/ontologies/genre#acrostic">
    <rdfs:comment xml:lang="en">The description for this term is indebted to DBpedia. </rdfs:comment>
    <owl:sameAs rdf:resource="http://dbpedia.org/resource/Acrostic"/>
    <rdfs:label xml:lang="en">acrostic</rdfs:label>
    <skos:definition xml:lang="fr">«Un acrostiche, du grec akrostikhos (akros, haut, élevé et stikhos, le vers), est un poème, une strophe ou une série de strophes fondés sur une forme poétique consistant en ce que, lues verticalement de haut en bas, la première lettre ou, parfois, les premiers mots d'une suite de vers composent un mot ou une expression en lien avec le poème.» <![CDATA[(<a href="#cwrc:727d97bc-af78-4122-94be-aa78b2e97d5a">DBpedia, 2017</a>)]]></skos:definition>
    <owl:sameAs rdf:resource="http://id.loc.gov/authorities/genreForms/gf2014026214"/>
    <rdfs:comment xml:lang="fr">La description de ce terme est basée sur celle de DBPedia.</rdfs:comment>
    <skos:definition xml:lang="en">"Short poems or prose compositions in which text is arranged so that the first letters of each line form a word, phrase, or motto." <![CDATA[(<a href="#cwrc:db2f8571-a773-4068-a35f-34262950bb8f">Getty, 2017</a>)]]></skos:definition>
    <rdfs:label xml:lang="fr">acrostiche</rdfs:label>
  </genre:PoeticGenre>
  <genre:ScholarlyGenre rdf:about="http://sparql.cwrc.ca/ontologies/genre#treatise">
    <skos:definition xml:lang="fr">«Un traité est un manuel d'instructions ou un livre standard dans n'importe quelle branche qui forme un sujet d'études. Ils se différencient les uns des autres, aussi bien par le public ciblé que par le sujet abordé. Les traités sont habituellement édités par des imprimeurs spécialisés, dans le but de répondre aux besoins de formation, sur n'importe quel thème susceptible de faire l'objet d'un enseignement. Il s'agit d'un important commerce qui nécessite des ventes massives, afin de rendre ces publications rentables. Bien que la plupart des traités soient uniquement édités sous forme de livres reliés, certains sont désormais consultables sur internet. Les traités sont apparus avec le développement de l'imprimerie de Johannes Gutenberg, sous la forme de méthodes d'enseignement.» <![CDATA[(<a href="#cwrc:727d97bc-af78-4122-94be-aa78b2e97d5a">DBpedia, 2017</a>)]]></skos:definition>
    <rdfs:label xml:lang="en">treatise</rdfs:label>
    <rdfs:comment xml:lang="en">The description for this term is indebted to the Getty Art &amp; Architecture Thesaurus.</rdfs:comment>
    <owl:sameAs rdf:resource="http://vocab.getty.edu/aat/300026681"/>
    <skos:definition xml:lang="en">"Formal and systematic written expositions of the principles of a subject, generally longer and more detailed than essays." <![CDATA[(<a href="#cwrc:db2f8571-a773-4068-a35f-34262950bb8f">Getty, 2017</a>)]]></skos:definition>
  </genre:ScholarlyGenre>
  <genre:ScholarlyGenre rdf:about="http://sparql.cwrc.ca/ontologies/genre#legalWriting">
    <rdfs:label xml:lang="fr">rédaction juridique</rdfs:label>
    <skos:definition xml:lang="en">"Legal writing is a type of technical writing used by lawyers, judges, legislators, and others in law to express legal analysis and legal rights and duties. Legal writing in practice is used to advocate for or to express the resolution of a client's legal matter." <![CDATA[(<a href="#cwrc:727d97bc-af78-4122-94be-aa78b2e97d5a">DBpedia, 2017</a>)]]></skos:definition>
    <skos:definition xml:lang="fr">Type d'écrit technique destiné à être utilisé par les professionnels juridiques lors de la rédaction de textes légaux ou à propos du droit.</skos:definition>
    <rdfs:label xml:lang="en">legal writing</rdfs:label>
    <rdfs:comment xml:lang="en">This term and its description were created from data gathered from DBpedia.</rdfs:comment>
    <owl:sameAs rdf:resource="http://dbpedia.org/resource/Legal_writing"/>
  </genre:ScholarlyGenre>
  <genre:IntertextualGenre rdf:about="http://sparql.cwrc.ca/ontologies/genre#translation">
    <skos:definition xml:lang="en">"The act of conveying the meaning of words in one language by attempting to say the same thing in another language, as opposed to paraphrasing, summarizing, and transliteration." <![CDATA[(<a href="cwrc:509015ff-7641-473e-94c5-688e06952bb7">L. K Wheeler, 2017</a>)]]></skos:definition>
    <skos:definition xml:lang="fr">Versions traduites du'un texte.</skos:definition>
    <owl:sameAs rdf:resource="http://vocab.getty.edu/aat/300027389"/>
    <rdfs:label xml:lang="en">translation</rdfs:label>
    <rdfs:label xml:lang="fr">traduction</rdfs:label>
    <rdfs:comment xml:lang="en">The description for this term is indebted to Dr. L. Kip Wheeler of Carson-Newman University. </rdfs:comment>
  </genre:IntertextualGenre>
  <genre:DramaticGenre rdf:about="http://sparql.cwrc.ca/ontologies/genre#theatreOfTheAbsurd">
    <rdfs:label xml:lang="fr">théâtre de l'absurde</rdfs:label>
    <rdfs:label xml:lang="en">theatre of the absurd</rdfs:label>
    <owl:sameAs rdf:resource="http://dbpedia.org/resource/Theatre_of_the_Absurd"/>
    <skos:definition xml:lang="fr">«Le théâtre de l’absurde est un style de théâtre apparu au XXe siècle, à l'époque de la Seconde Guerre mondiale, qui se caractérise par une rupture totale par rapport aux genres plus classiques, tels que la tragédie ou la comédie. C'est un genre traitant fréquemment de l’absurdité de l’Homme et de la vie en général, celle-ci menant toujours à une fin tragique. L’origine de ce mouvement est sans conteste essentiellement liée à la chute de l’humanisme et au traumatisme causé par la Première Guerre mondiale. Ce mouvement littéraire s'est inspiré des surréalistes et des dadaïstes mais est radicalement opposé au réalisme.» <![CDATA[(<a href="#cwrc:727d97bc-af78-4122-94be-aa78b2e97d5a">DBpedia, 2017</a>)]]></skos:definition>
    <rdfs:comment xml:lang="en">This term and its description were created from data gathered from DBpedia.</rdfs:comment>
    <skos:definition xml:lang="en">"The Theatre of the Absurd (French: théâtre de l'absurde) is a post–World War II designation for particular plays of absurdist fiction written by a number of primarily European playwrights in the late 1950s, as well as one for the style of theatre which has evolved from their work. Their work focused largely on the idea of existentialism and expressed what happens when human existence has no meaning or purpose and therefore all communication breaks down, in fact alerting their audiences to pursue the opposite. Logical construction and argument gives way to irrational and illogical speech and to its ultimate conclusion, silence." <![CDATA[(<a href="#cwrc:727d97bc-af78-4122-94be-aa78b2e97d5a">DBpedia, 2017</a>)]]></skos:definition>
  </genre:DramaticGenre>
  <genre:CartographicForm rdf:about="http://sparql.cwrc.ca/ontologies/genre#atlas">
    <rdfs:label xml:lang="en">atlas</rdfs:label>
    <owl:sameAs rdf:resource="http://id.loc.gov/authorities/genreForms/gf2011026058"/>
  </genre:CartographicForm>
  <genre:ComedicGenre rdf:about="http://sparql.cwrc.ca/ontologies/genre#comedy">
    <skos:definition xml:lang="fr">"Genre concernant les formes du théâtre, de la littérature et de l'improvisation qui ont pour principal objectif de divertir et de provoquer le rire. La comédie est généralement opposée à la tragédie et peut prendre soit la forme d'une critique sociale à travers la satire et l'humour d'esprit politique ou intellectuel, soit la forme de spectacle pur à travers la farce ou le burlesque."</skos:definition>
    <rdfs:label xml:lang="en">comedy</rdfs:label>
    <skos:definition xml:lang="en">"Genre encompassing forms of theatre, literature, and improvisation with the basic objective to amuse, humor, and induce laughter. In general, it is often contrasted with tragedy and can be applied in the form of social criticism through satire and political or intellectual wit or applied in the form of pure spectacle through farce or burlesque." <![CDATA[(<a href="#cwrc:db2f8571-a773-4068-a35f-34262950bb8f">Getty, 2017</a>)]]></skos:definition>
    <owl:sameAs rdf:resource="http://vocab.getty.edu/aat/300055911"/>
    <rdfs:label xml:lang="fr">comédie</rdfs:label>
    <rdfs:comment xml:lang="en">The description for this term is indebted to the Getty Art &amp; Architecture Thesaurus.</rdfs:comment>
  </genre:ComedicGenre>
  <genre:EpistolaryGenre rdf:about="http://sparql.cwrc.ca/ontologies/genre#epistolary">
    <rdfs:label xml:lang="en">epistolary</rdfs:label>
    <rdfs:label xml:lang="fr">genre épistolaire</rdfs:label>
    <rdfs:comment xml:lang="en">The description for this term is indebted to the Getty Art &amp; Architecture Thesaurus.</rdfs:comment>
    <skos:definition xml:lang="en">"Novels written by using the device of a series of letters, diary entries, newspaper clippings, or other documents." <![CDATA[(<a href="#cwrc:db2f8571-a773-4068-a35f-34262950bb8f">Getty, 2017</a>)]]></skos:definition>
    <owl:sameAs rdf:resource="http://vocab.getty.edu/aat/300410324"/>
    <skos:definition xml:lang="fr">Romans écrits sous forme d'une série de correspondances, d'entrées de journal intime, de coupures de journaux ou d'autres documents.</skos:definition>
  </genre:EpistolaryGenre>
  <genre:ScholarlyGenre rdf:about="http://sparql.cwrc.ca/ontologies/genre#dissertation">
    <rdfs:comment xml:lang="en">This term and its description were created from data gathered from the Getty Art &amp; Architecture Thesaurus.</rdfs:comment>
    <skos:definition xml:lang="en">"Written treatises, or the records of a discourse on a subject, usually prepared and presented as the final requirement for a degree or diploma and typically based on independent research and giving evidence of the candidate's mastery of the subject and of scholarly method." <![CDATA[(<a href="#cwrc:db2f8571-a773-4068-a35f-34262950bb8f">Getty, 2017</a>)]]></skos:definition>
    <rdfs:label xml:lang="fr">mémoire, thèse</rdfs:label>
    <owl:sameAs rdf:resource="http://vocab.getty.edu/aat/300028029"/>
    <skos:definition xml:lang="fr">Textes écrits ou enregistrement d'une présentation sur un sujet, généralement préparés et présentés en tant que devoir final pour obtenir un diplôme, s'appuyant généralement sur des recherches indépendantes démontrant l'expertis et la méthode académique du candidat.</skos:definition>
    <rdfs:label xml:lang="en">dissertation</rdfs:label>
    <owl:sameAs rdf:resource="http://id.loc.gov/authorities/genreForms/gf2014026039"/>
  </genre:ScholarlyGenre>
  <genre:DigitalMedium rdf:about="http://sparql.cwrc.ca/ontologies/genre#bornDigital">
    <rdfs:label xml:lang="en">born digital</rdfs:label>
    <skos:related rdf:resource="http://vocab.getty.edu/aat/300374824"/>
  </genre:DigitalMedium>
  <genre:PedagogicalGenre rdf:about="http://sparql.cwrc.ca/ontologies/genre#quiz">
    <skos:definition xml:lang="fr">«Un quiz est un jeu qui consiste en un questionnaire permettant de tester des connaissances générales ou spécifiques ou des compétences. Un quiz se pratique seul ou à plusieurs, suivant des procédures plus ou moins élaborées.Il peut se présenter sous formes de questionnaire à choix multiples ou de questionnaire simple, mais la différence majeure avec un autre test de connaissances ou de personnalité est qu'on attend du participant une réponse non développée d'un ou deux mots. Le quiz est le principe de nombreux jeux de société ou de jeux radiophoniques ou télévisés. Lorsqu'il ne s'agit pas d'un jeu, on parle plutôt de « questionnaire » ou de « test » que de quiz.» <![CDATA[(<a href="#cwrc:727d97bc-af78-4122-94be-aa78b2e97d5a">DBpedia, 2017</a>)]]></skos:definition>
    <rdfs:comment xml:lang="en">This term and its description were created from data gathered from DBpedia.</rdfs:comment>
    <skos:definition xml:lang="en">A brief, interactive text that poses questions for the reader to answer, often as an assessment of knowledge in the form of questionnaire.</skos:definition>
    <rdfs:label xml:lang="fr">quiz</rdfs:label>
    <rdfs:label xml:lang="en">quiz</rdfs:label>
    <skos:closeMatch rdf:resource="http://dbpedia.org/resource/Quiz"/>
  </genre:PedagogicalGenre>
  <genre:ThematicWritingGenre rdf:about="http://sparql.cwrc.ca/ontologies/genre#popular">
    <skos:definition xml:lang="fr">Arts visuels élaborés par ou pour le grand public qui reflètent souvent des tendances et font écho à la vie quotidienne. Œuvres produites pour le public de masse et qui se distinguent des beaux arts et de l'artisanat.</skos:definition>
    <skos:definition xml:lang="en">"Visual arts produced by or for the general public, often reflecting fads and as a response to the daily environment; works produced for mass audiences as distinct from fine art and folk art." <![CDATA[(<a href="#cwrc:db2f8571-a773-4068-a35f-34262950bb8f">Getty, 2017</a>)]]></skos:definition>
    <owl:sameAs rdf:resource="http://vocab.getty.edu/aat/300311927"/>
    <rdfs:label xml:lang="en">popular</rdfs:label>
    <rdfs:label xml:lang="fr">populaire</rdfs:label>
    <rdfs:comment xml:lang="en">The description for this term is indebted to the Getty Art &amp; Architecture Thesaurus.</rdfs:comment>
  </genre:ThematicWritingGenre>
  <genre:PerformanceMedium rdf:about="http://sparql.cwrc.ca/ontologies/genre#ballet">
    <skos:definition xml:lang="fr">«Le ballet est un genre dramatique dont l'action est figurée par des pantomimes et des danses. Ses origines remontent à la Renaissance italienne (XVe siècle). Primitivement développé à la cour d'Italie, le ballet a reçu ses lettres de noblesse en France, puis en Russie, en tant que danse-spectacle. Au XVIIe siècle, le développement important qu'a connu le ballet à la cour de Louis XIV explique l'origine française de la plupart des termes de vocabulaire de la danse. Comme l'opéra, il peut être organisé de deux manières »:<![CDATA[(<a href="#cwrc:727d97bc-af78-4122-94be-aa78b2e97d5a">DBpedia, 2017</a>)]]></skos:definition>
    <rdfs:comment xml:lang="en">This term and its description were created from data gathered from the Getty Art &amp; Architecture Thesaurus.</rdfs:comment>
    <owl:sameAs rdf:resource="http://dbpedia.org/resource/Ballet"/>
    <rdfs:label xml:lang="fr">ballet</rdfs:label>
    <skos:related rdf:resource="http://vocab.getty.edu/aat/300389780"/>
    <skos:definition xml:lang="en">"Dramatic entertainments consisting of dance and mime performed to music. Ballets are characterized by stylized poses and steps that are combined with light and flowing figures and movements, such as leaps and turns; often combined with music, scenery, costume, and sometimes pantomime or speech to convey a story, theme, or atmosphere to the audience." <![CDATA[(<a href="#cwrc:db2f8571-a773-4068-a35f-34262950bb8f">Getty, 2017</a>)]]></skos:definition>
    <rdfs:label xml:lang="en">ballet</rdfs:label>
  </genre:PerformanceMedium>
  <genre:PoeticGenre rdf:about="http://sparql.cwrc.ca/ontologies/genre#versePoem">
    <rdfs:label xml:lang="en">verse poem</rdfs:label>
  </genre:PoeticGenre>
  <genre:MovingMedium rdf:about="http://sparql.cwrc.ca/ontologies/genre#animation">
    <rdfs:label xml:lang="en">animation</rdfs:label>
  </genre:MovingMedium>
  <genre:PoeticGenre rdf:about="http://sparql.cwrc.ca/ontologies/genre#performancePoetry">
    <skos:definition xml:lang="fr">«La lecture performée ou lecture-performance est une lecture publique de textes poétiques ou littéraires effectuée le plus souvent par son auteur dans un esprit qui s'apparente à celui de la performance et qui peut convoquer tous les arts et techniques du théâtre et de la scène où la poésie et la littérature sont cependant toujours au premier plan. Christian Prigent, Serge Pey et Charles Pennequin en sont les premiers représentants. Édith Azam est aujourd'hui la conseillère lecture-performance au festival Voix de la Méditerranée de Lodève.» <![CDATA[(<a href="#cwrc:727d97bc-af78-4122-94be-aa78b2e97d5a">DBpedia, 2017</a>)]]></skos:definition>
    <owl:sameAs rdf:resource="http://dbpedia.org/resource/Performance_poetry"/>
    <rdfs:label xml:lang="en">performance poetry</rdfs:label>
    <skos:definition xml:lang="en">"Performance poetry is poetry that is specifically composed for or during a performance before an audience. During the 1980s, the term came into popular usage to describe poetry written or composed for performance rather than print distribution." <![CDATA[(<a href="#cwrc:727d97bc-af78-4122-94be-aa78b2e97d5a">DBpedia, 2017</a>)]]></skos:definition>
    <owl:sameAs rdf:resource="http://id.loc.gov/authorities/genreForms/gf2014026552"/>
    <rdfs:comment xml:lang="en">The description for this term is indebted to DBpedia. </rdfs:comment>
  </genre:PoeticGenre>
  <genre:DigitalMedium rdf:about="http://sparql.cwrc.ca/ontologies/genre#computerProgram">
    <skos:related rdf:resource="http://vocab.getty.edu/aat/300312188"/>
    <rdfs:comment xml:lang="en">The description for this term is indebted to the Getty Art &amp; Architecture Thesaurus.</rdfs:comment>
    <skos:definition xml:lang="fr">" Compilation d'instructions codées, ou séquence de code qui lorsqu'on l'exécute permet de faire réaliser une tâche spécifique à une machine, le plus souvent un ordinateur."</skos:definition>
    <owl:sameAs rdf:resource="http://vocab.getty.edu/aat/300312188"/>
    <rdfs:label xml:lang="fr">programme informatique</rdfs:label>
    <skos:definition xml:lang="en">"A compilation of coded instructions or sequence of code that, when run, achieves a certain task in a mechanism, usually a computer." <![CDATA[(<a href="#cwrc:db2f8571-a773-4068-a35f-34262950bb8f">Getty, 2017</a>)]]></skos:definition>
    <rdfs:label xml:lang="en">computer program</rdfs:label>
  </genre:DigitalMedium>
  <genre:NovelisticGenre rdf:about="http://sparql.cwrc.ca/ontologies/genre#novel">
    <rdfs:label xml:lang="fr">roman</rdfs:label>
    <rdfs:label xml:lang="en">novel</rdfs:label>
    <skos:definition xml:lang="en">"Invented prose narratives of considerable length and a certain complexity that deal imaginatively with human experience through a connected sequence of events involving a group of persons in a specific setting." <![CDATA[(<a href="#cwrc:db2f8571-a773-4068-a35f-34262950bb8f">Getty, 2017</a>)]]></skos:definition>
    <owl:sameAs rdf:resource="http://id.loc.gov/authorities/genreForms/gf2015026020"/>
    <owl:sameAs rdf:resource="http://vocab.getty.edu/aat/300202580"/>
    <rdfs:comment xml:lang="en">The description for this term is indebted to the Getty Art &amp; Architecture Thesaurus.</rdfs:comment>
    <skos:definition xml:lang="fr">«Le roman est un genre littéraire, caractérisé pour l'essentiel par une narration fictionnelle plus ou moins longue.» <![CDATA[(<a href="#cwrc:727d97bc-af78-4122-94be-aa78b2e97d5a">DBpedia, 2017</a>)]]></skos:definition>
  </genre:NovelisticGenre>
  <genre:CalendarForm rdf:about="http://sparql.cwrc.ca/ontologies/genre#almanac">
    <rdfs:label xml:lang="en">almanac</rdfs:label>
  </genre:CalendarForm>
  <genre:PerformanceMedium rdf:about="http://sparql.cwrc.ca/ontologies/genre#charade">
    <rdfs:label xml:lang="fr">charade</rdfs:label>
    <skos:definition xml:lang="fr">Divertissement verbal qui consiste à faire deviner un mot sommairement défini (appelé mon tout ou mon entier) d'après la définition d'un homonyme (appelé mon premier, mon second, etc.) de chacune de ses syllabes.</skos:definition>
    <rdfs:comment xml:lang="en">This term and its description were created from data gathered from the Encyclopædia Britannica.</rdfs:comment>
    <skos:definition xml:lang="en">"A form of riddle in which clues are given about each syllable of a word so that the entire word may be guessed. Originally, these riddles were written, often in the form of a poem, but it soon gained popularity as a parlour game in which the clues were mimed rather than written in verse." <![CDATA[(<a href="#cwrc:7ff0c640-f273-46f5-be8d-e50aa27dce59">Encyclopædia Britannica, 2017</a>)]]></skos:definition>
    <skos:related rdf:resource="http://id.loc.gov/authorities/genreForms/gf2014026533"/>
    <owl:sameAs rdf:resource="https://dvlf.uchicago.edu/mot/charade"/>
    <rdfs:label xml:lang="en">charade</rdfs:label>
  </genre:PerformanceMedium>
  <genre:IntertextualGenre rdf:about="http://sparql.cwrc.ca/ontologies/genre#answer">
    <rdfs:label xml:lang="fr">réponse</rdfs:label>
    <skos:definition xml:lang="en">A form of intertextuality in which an author writes a response to a work by another writer, typically to argue against the statements of that work. Often takes the form of an essay or letter.</skos:definition>
    <rdf:type rdf:resource="http://sparql.cwrc.ca/ontologies/genre#DialogueOrDebateGenre"/>
    <skos:definition xml:lang="fr">Forme d'intertextualité, texte dans lequel un auteur se prononce en réponse à l'œuvre d'un autre écrivain, généralement en opposition aux propos qu'elle contient. Prend souvent la forme d'un essai ou d'une lettre.</skos:definition>
    <rdfs:label xml:lang="en">answer</rdfs:label>
  </genre:IntertextualGenre>
  <genre:PerformanceMedium rdf:about="http://sparql.cwrc.ca/ontologies/genre#speech">
    <skos:definition xml:lang="fr">Documents qui fournissent la transcription écrite d'une adresse publique ou d'une conversation.</skos:definition>
    <owl:sameAs rdf:resource="http://id.loc.gov/authorities/genreForms/gf2011026363"/>
    <rdfs:comment xml:lang="en">The description for this term is indebted to the Getty Art &amp; Architecture Thesaurus.</rdfs:comment>
    <owl:sameAs rdf:resource="http://vocab.getty.edu/aat/300026671"/>
    <rdfs:label xml:lang="en">speech</rdfs:label>
    <skos:definition xml:lang="en">"Documents containing the text of any public address or talk" <![CDATA[(<a href="#cwrc:db2f8571-a773-4068-a35f-34262950bb8f">Getty, 2017</a>)]]></skos:definition>
    <rdfs:label xml:lang="fr">discours</rdfs:label>
  </genre:PerformanceMedium>
  <genre:IntertextualGenre rdf:about="http://sparql.cwrc.ca/ontologies/genre#commentary">
    <rdfs:label xml:lang="en">commentary</rdfs:label>
  </genre:IntertextualGenre>
  <genre:FictionalGenre rdf:about="http://sparql.cwrc.ca/ontologies/genre#mystery">
    <rdfs:label xml:lang="en">mystery</rdfs:label>
    <skos:definition xml:lang="en">"A novel focused on suspense and solving a mystery--especially a murder, theft, kidnapping, or some other crime. The protagonist faces inexplicable events, threats, assaults, and unknown forces or antagonists. Conventionally, the hero is a keenly observant individual (such as Sherlock Holmes) and the police are depicted as incompetent or incapable of solving the crime by themselves. Many of the works of Sir Arthur Conan Doyle, Edgar Allan Poe, and Agatha Christie are mystery novels." <![CDATA[(<a href="cwrc:509015ff-7641-473e-94c5-688e06952bb7">L. K Wheeler, 2017</a>)]]></skos:definition>
    <rdfs:comment xml:lang="en">This term and its description were created from data gathered from polars.org.</rdfs:comment>
    <rdfs:label xml:lang="fr">roman à énigme</rdfs:label>
    <owl:sameAs rdf:resource="https://www.polars.org/spip.php?article12"/>
    <owl:sameAs rdf:resource="http://id.loc.gov/authorities/genreForms/gf2014026280"/>
    <skos:definition xml:lang="fr">Dans le roman à énigme, le détective cherche le coupable au sein d’un groupe de suspects tour à tour présenté par l’auteur. D’un interrogatoire l’autre, on suit donc le détective dans sa quête de vérité, pour le voir aboutir généralement au fameux dévoilement de l’affaire, le plus souvent dans une scène finale où il expose les clés de son raisonnement. Il devient très vite admis que l’auteur s’amuse avec son lecteur, lui donnant la possibilité de jouer lui aussi les détectives et de parvenir aux mêmes conclusions que son héros.</skos:definition>
  </genre:FictionalGenre>
  <genre:ParatextualGenre rdf:about="http://sparql.cwrc.ca/ontologies/genre#afterword">
    <rdfs:label xml:lang="fr">postface</rdfs:label>
    <rdfs:label xml:lang="en">afterword</rdfs:label>
    <rdfs:comment xml:lang="en">This term and its description were created from data gathered from DBpedia.</rdfs:comment>
    <skos:definition xml:lang="fr">«Une postface est un texte ajouté à la fin d'un livre ou d'un écrit pour en guise de supplément ou de conclusion, généralement pour émettre un commentaire, une explication ou un avertissement. La postface peut être rédigée par l'auteur d'un document ou par une autre personne. La postface est séparée du corps principal de l'ouvrage et est placée dans les pages annexes, c'est-à-dire à la fin du document. La postface, bien qu'elle puise faire office de conclusion, présente des informations qui ne sont pas essentielles à l'intégralité de l'ouvrage, mais qui sont toutefois jugées pertinentes. On oppose la préface, située dans les liminaires, à la postface.» <![CDATA[(<a href="#cwrc:727d97bc-af78-4122-94be-aa78b2e97d5a">DBpedia, 2017</a>)]]></skos:definition>
    <dcterms:references rdf:resource="http://www.oxfordreference.com/view/10.1093/acref/9780199571123.001.0001/m_en_gb0012830?rskey=tDwp66%26result=1411"/>
    <skos:definition xml:lang="en">"A section that appears towards the end of a book, does not form part of the main body, and often concludes or summarizes." <![CDATA[(<a href="#cwrc:4c227091-6bf0-4325-b846-9733fae19e61/">Oxford, 2015</a>)]]></skos:definition>
  </genre:ParatextualGenre>
  <genre:ParatextualGenre rdf:about="http://sparql.cwrc.ca/ontologies/genre#prologue">
    <owl:sameAs rdf:resource="http://id.loc.gov/authorities/genreForms/gf2018026101"/>
    <rdfs:label xml:lang="fr">prologue</rdfs:label>
    <skos:definition xml:lang="en">"(1) In original Greek tragedy, the prologue was either the action or a set of introductory speeches before the first entry (parados) of the chorus. Here, a single actor's monologue or a dialogue between two actors would establish the play's background events. (2) In later literature, a prologue is a section of any introductory material before the first chapter or the main material of a prose work, or any such material before the first stanza of a poetic work." <![CDATA[(<a href="cwrc:509015ff-7641-473e-94c5-688e06952bb7">L. K Wheeler, 2017</a>)]]></skos:definition>
    <dcterms:references rdf:resource="http://web.cn.edu/kwheeler/lit_terms_p.html"/>
    <rdfs:label xml:lang="en">prologue</rdfs:label>
    <rdfs:comment xml:lang="en">This term and its description were created from data gathered from DBpedia.</rdfs:comment>
    <skos:definition xml:lang="fr">«Le prologue (du grec προ (pro) : avant, et λóγος (logos) : discours) est la première partie d’une œuvre littéraire ou la première scène d’une œuvre dramatique, faisant office de préface, d’introduction ou de préambule, et servant à situer les personnages et l’action de l’œuvre en exposant divers points essentiels à connaître pour l’intelligence de la pièce.» <![CDATA[(<a href="#cwrc:727d97bc-af78-4122-94be-aa78b2e97d5a">DBpedia, 2017</a>)]]></skos:definition>
  </genre:ParatextualGenre>
  <genre:DramaticGenre rdf:about="http://sparql.cwrc.ca/ontologies/genre#bergamasque">
    <skos:definition xml:lang="fr">«La bergamasque est une danse traditionnelle provenant de la ville de Bergame dans le nord de l'Italie. Son existence est attestée depuis le début du XVIe siècle. Danse de couples disposés en cercle jusqu'au XVIIe siècle, vive et sautillante, elle est souvent utilisée dans la commedia dell'arte. La bergamasque d'un compositeur français se trouve dans le Thesaurus harmonicus (1603) de Jean-Baptiste Besard.» <![CDATA[(<a href="#cwrc:727d97bc-af78-4122-94be-aa78b2e97d5a">DBpedia, 2017</a>)]]></skos:definition>
    <rdfs:label xml:lang="fr">bergamasque</rdfs:label>
    <skos:definition xml:lang="en">"A folk dance originating in Bergamo, Italy, in the 16th century, but often included in theatre productions unrelated to Italian culture." <![CDATA[(<a href="#cwrc:0a58baf2-e7d5-47d7-9853-c8140dbbfeed">Merriam-Webster, 2017</a>)]]></skos:definition>
    <rdfs:label xml:lang="en">bergamasque</rdfs:label>
    <rdfs:comment xml:lang="en">This term and its description were created from data gathered from DBpedia.</rdfs:comment>
    <owl:sameAs rdf:resource="http://dbpedia.org/resource/Bergamask"/>
  </genre:DramaticGenre>
  <genre:PoeticGenre rdf:about="http://sparql.cwrc.ca/ontologies/genre#psalm">
    <skos:definition xml:lang="fr">Chacun des cent cinquante poèmes religieux, jadis attribués au roi David, qui composent l'un des livres de la Bible et sont récités ou chantés dans les liturgies juives ou chrétiennes (abrév. ps.).</skos:definition>
    <owl:sameAs rdf:resource="http://vocab.getty.edu/aat/300400527"/>
    <skos:definition xml:lang="en">"Sacred songs that may be sung or recited in religious worship, particularly those contained in the Book of Psalms in the Old Testament and Hebrew Scriptures." <![CDATA[(<a href="#cwrc:db2f8571-a773-4068-a35f-34262950bb8f">Getty, 2017</a>)]]></skos:definition>
    <owl:sameAs rdf:resource="http://id.loc.gov/authorities/genreForms/gf2015026079"/>
    <rdf:type rdf:resource="http://sparql.cwrc.ca/ontologies/genre#ReligiousGenre"/>
    <rdfs:comment xml:lang="en">This term and its description were created from data gathered from the Dictionnaire Vivant de la Langue Française.</rdfs:comment>
    <rdfs:label xml:lang="fr">psaume</rdfs:label>
    <rdfs:label xml:lang="en">psalm</rdfs:label>
  </genre:PoeticGenre>
  <genre:PoliticalWritingGenre rdf:about="http://sparql.cwrc.ca/ontologies/genre#suffragist">
    <rdfs:label xml:lang="en">suffragist</rdfs:label>
  </genre:PoliticalWritingGenre>
  <genre:BookForm rdf:about="http://sparql.cwrc.ca/ontologies/genre#book">
    <rdfs:label xml:lang="en">book</rdfs:label>
  </genre:BookForm>
  <genre:ThreeDimensionalMedium rdf:about="http://sparql.cwrc.ca/ontologies/genre#mixedMaterials">
    <rdfs:label xml:lang="en">mixed materials</rdfs:label>
    <skos:related rdf:resource="http://vocab.getty.edu/aat/300163347"/>
  </genre:ThreeDimensionalMedium>
  <genre:TextualMedium rdf:about="http://sparql.cwrc.ca/ontologies/genre#looseLeaf">
    <rdfs:label xml:lang="en">loose-leaf</rdfs:label>
    <skos:related rdf:resource="http://vocab.getty.edu/aat/300257592"/>
  </genre:TextualMedium>
  <genre:ThematicWritingGenre rdf:about="http://sparql.cwrc.ca/ontologies/genre#juvenile">
    <rdfs:label xml:lang="en">juvenile</rdfs:label>
  </genre:ThematicWritingGenre>
  <genre:ReferenceWorkGenre rdf:about="http://sparql.cwrc.ca/ontologies/genre#encyclopaedia">
    <skos:definition xml:lang="fr">Livres, séries de livres ou de disques contenant des articles informatifs, habituellement classés par ordre alphabétique, portant sur différents domaines du savoir général, ou se limitant à un domaine ou un sujet spécifique.</skos:definition>
    <owl:sameAs rdf:resource="http://vocab.getty.edu/aat/300129439"/>
    <rdfs:comment xml:lang="en">The description for this term is indebted to the Getty Art &amp; Architecture Thesaurus.</rdfs:comment>
    <owl:sameAs rdf:resource="http://id.loc.gov/authorities/genreForms/gf2014026092"/>
    <rdfs:label xml:lang="fr">encyclopédie</rdfs:label>
    <rdfs:label xml:lang="en">encyclopaedia</rdfs:label>
    <skos:definition xml:lang="en">"Books, set of books, or disks, containing informational articles on subjects in every field of knowledge, or limited to a special field or subject, usually arranged in alphabetical order." <![CDATA[(<a href="#cwrc:db2f8571-a773-4068-a35f-34262950bb8f">Getty, 2017</a>)]]></skos:definition>
  </genre:ReferenceWorkGenre>
  <genre:InformationalGenre rdf:about="http://sparql.cwrc.ca/ontologies/genre#survey">
    <rdfs:label xml:lang="en">survey</rdfs:label>
  </genre:InformationalGenre>
  <genre:PrintMedium rdf:about="http://sparql.cwrc.ca/ontologies/genre#mimeograph">
    <skos:related rdf:resource="http://vocab.getty.edu/aat/300028490"/>
    <rdfs:label xml:lang="en">mimeograph</rdfs:label>
    <skos:altLabel xml:lang="en">stencil</skos:altLabel>
  </genre:PrintMedium>
  <genre:SongGenre rdf:about="http://sparql.cwrc.ca/ontologies/genre#lullaby">
    <owl:sameAs rdf:resource="http://id.loc.gov/authorities/genreForms/gf2014026913"/>
    <rdfs:label xml:lang="en">lullaby</rdfs:label>
  </genre:SongGenre>
  <genre:ComedicGenre rdf:about="http://sparql.cwrc.ca/ontologies/genre#burletta">
    <skos:definition xml:lang="fr">«Burletta (« petite plaisanterie » en italien, parfois aussi burla ou burlettina), est un terme musical pour qualifier un bref opéra comique italien (ou, plus tard anglais). Le terme est utilisé au XVIIIe siècle pour désigner les intermezzos comiques entre les actes d'un opéra seria mais est parfois donné à des œuvres de plus grande envergure. La serva padrona de Pergolese est appelée burletta lors de sa création à Londres en 1750.» <![CDATA[(<a href="#cwrc:727d97bc-af78-4122-94be-aa78b2e97d5a">DBpedia, 2017</a>)]]></skos:definition>
    <rdfs:label xml:lang="en">burletta</rdfs:label>
    <owl:sameAs rdf:resource="http://dbpedia.org/resource/Burletta"/>
    <skos:definition xml:lang="en">"A form of comic drama set to music, first popularized in the 1700s." <![CDATA[(<a href="#cwrc:2f09376c-f784-4a46-9f04-5a21aa311f27">Penguin, 1999</a>)]]></skos:definition>
    <rdfs:label xml:lang="fr">burletta</rdfs:label>
  </genre:ComedicGenre>
  <genre:PerformanceMedium rdf:about="http://sparql.cwrc.ca/ontologies/genre#dance">
    <rdfs:label xml:lang="en">dance</rdfs:label>
    <skos:related rdf:resource="http://vocab.getty.edu/aat/300054144"/>
  </genre:PerformanceMedium>
  <genre:DramaticGenre rdf:about="http://sparql.cwrc.ca/ontologies/genre#revengeTragedy">
    <rdfs:label xml:lang="en">revenge tragedy</rdfs:label>
  </genre:DramaticGenre>
  <genre:ReligiousGenre rdf:about="http://sparql.cwrc.ca/ontologies/genre#theology">
    <rdfs:label xml:lang="fr">théologie</rdfs:label>
    <rdfs:label xml:lang="en">theology</rdfs:label>
    <skos:closeMatch rdf:resource="http://dbpedia.org/resource/Theology"/>
    <rdfs:comment xml:lang="en">This term and its description were created from data gathered from DBpedia.</rdfs:comment>
    <skos:definition xml:lang="fr">«La théologie (en grec ancien θεολογία, littéralement « discours rationnel sur la divinité ou le divin, le Θεός [Theos] ») est un ensemble de champs disciplinaires qui touchent d'une manière ou d'une autre à l'idée de Dieu ou de divin. Selon la tradition dont il est question, les définitions de la théologie peuvent varier grandement.» <![CDATA[(<a href="#cwrc:727d97bc-af78-4122-94be-aa78b2e97d5a">DBpedia, 2017</a>)]]></skos:definition>
    <skos:definition xml:lang="en">A branch of religious writing attempting to deal systematically with the study of a deity or deities or religious beliefs; the science of religion.</skos:definition>
  </genre:ReligiousGenre>
  <genre:JournalisticGenre rdf:about="http://sparql.cwrc.ca/ontologies/genre#revue">
    <owl:sameAs rdf:resource="http://vocab.getty.edu/aat/300026480"/>
    <owl:sameAs rdf:resource="http://id.loc.gov/authorities/genreForms/gf2014027050"/>
    <skos:definition xml:lang="fr">«Une revue est un genre théâtral qui associe musique, danse et sketches qui font la satire de personnes contemporaines, de l'actualité ou de la littérature. Comme les formes apparentées de l'opérette et de la comédie musicale, la revue allie musique, danse et comédie pour former un spectacle complet. Contrairement à celles-ci, elle ne possède cependant pas d'histoire suivie. Un thème général est plutôt utilisé pour un enchaînement de numéros au cours desquels solos et ensembles de danse se relaient.» <![CDATA[(<a href="#cwrc:727d97bc-af78-4122-94be-aa78b2e97d5a">DBpedia, 2017</a>)]]></skos:definition>
    <rdfs:label xml:lang="en">revue</rdfs:label>
    <rdfs:comment xml:lang="en">This term and its description were created from data gathered from DBpedia.</rdfs:comment>
    <rdfs:label xml:lang="fr">revue (variétés)</rdfs:label>
    <skos:definition xml:lang="en">"Periodicals, reports, or essays giving critical estimates and appraisals of art, a performance, or event. For other critical descriptions and analyses, prefer "criticism." <![CDATA[(<a href="#cwrc:db2f8571-a773-4068-a35f-34262950bb8f">Getty, 2017</a>)]]></skos:definition>
  </genre:JournalisticGenre>
  <genre:DramaticGenre rdf:about="http://sparql.cwrc.ca/ontologies/genre#oneActPlay">
    <owl:sameAs rdf:resource="http://id.loc.gov/authorities/genreForms/gf2014026462"/>
    <rdfs:label xml:lang="en">one-act-play</rdfs:label>
  </genre:DramaticGenre>
  <genre:PoeticGenre rdf:about="http://sparql.cwrc.ca/ontologies/genre#sonnet">
    <owl:sameAs rdf:resource="http://vocab.getty.edu/aat/300266382"/>
    <rdfs:comment xml:lang="en">This term and its description were created from data gathered from DBpedia.</rdfs:comment>
    <owl:sameAs rdf:resource="http://id.loc.gov/authorities/genreForms/gf2014026549"/>
    <skos:definition xml:lang="en">"Poems consisting of 14 decasyllabic lines, often in a rhyming scheme. The sonnet form is considered to be of Italian origin, appearing in the 13th century in Sicily, after which it spread to Tuscany, where Petrarch perfected the form with his Canzioniere, a series of 317 sonnets to his idealized love, Laura. The Petrarchian sonnet has historically been the most widely used of the form, although the Elizabethan form (3 quatrains, with a final rhyming couplet) is also common." <![CDATA[(<a href="#cwrc:db2f8571-a773-4068-a35f-34262950bb8f">Getty, 2017</a>)]]></skos:definition>
    <rdfs:label xml:lang="fr">sonnet</rdfs:label>
    <rdfs:label xml:lang="en">sonnet</rdfs:label>
    <skos:definition xml:lang="fr">«Un sonnet (de l'italien sonnetto ou sonetto aujourd'hui) est une forme de poème comportant quatorze vers dont la répartition typographique peut varier — deux quatrains et deux tercets ou un seul sizain final par exemple — et dont le schéma des rimes varie également, soit librement soit en suivant des dispositions régulières. La longueur du vers n'est pas fixe en français. Le sonnet est un genre qui a été pratiqué dans une bonne partie de l'Europe, tant dans les poésies syllabiques que rythmiques.» <![CDATA[(<a href="#cwrc:727d97bc-af78-4122-94be-aa78b2e97d5a">DBpedia, 2017</a>)]]></skos:definition>
  </genre:PoeticGenre>
  <genre:ThematicWritingGenre rdf:about="http://sparql.cwrc.ca/ontologies/genre#exploration">
    <rdfs:label xml:lang="en">exploration</rdfs:label>
  </genre:ThematicWritingGenre>
  <genre:DramaticGenre rdf:about="http://sparql.cwrc.ca/ontologies/genre#costumeDrama">
    <rdfs:label xml:lang="en">costume drama</rdfs:label>
  </genre:DramaticGenre>
  <genre:ChildrensLiteratureGenre rdf:about="http://sparql.cwrc.ca/ontologies/genre#preSchool">
    <rdfs:label xml:lang="en">pre-school</rdfs:label>
  </genre:ChildrensLiteratureGenre>
  <genre:JournalisticGenre rdf:about="http://sparql.cwrc.ca/ontologies/genre#journalism">
    <skos:definition xml:lang="en">"Content prepared for a newspaper, magazine, news website, or other form of news media, typically with the purpose of recording facts about a person or event." <![CDATA[(<a href="#cwrc:0a58baf2-e7d5-47d7-9853-c8140dbbfeed">Merriam-Webster, 2017</a>)]]></skos:definition>
    <skos:definition xml:lang="fr">«Le journalisme (/ʒuʀnalism/) est l'activité qui consiste à recueillir, vérifier ou commenter des faits pour les porter à l'attention du public dans les médias en respectant une même déontologie du journalisme, reposant sur la protection des sources d'information, du correspondant de guerre au journalisme d'investigation, sans oublier les autres spécialisations : dessinateur de presse, journaliste reporter d'images (JRI), photojournaliste, secrétaire de rédaction, critique musical ou éditorialiste.» <![CDATA[(<a href="#cwrc:727d97bc-af78-4122-94be-aa78b2e97d5a">DBpedia, 2017</a>)]]></skos:definition>
    <rdfs:comment xml:lang="en">This term and its description were created from data gathered from the Merriam-Webster dictionary.</rdfs:comment>
    <rdfs:label xml:lang="en">journalism</rdfs:label>
    <rdfs:label xml:lang="fr">journalisme</rdfs:label>
    <owl:sameAs rdf:resource="http://dbpedia.org/resource/Journalism"/>
  </genre:JournalisticGenre>
  <genre:FictionalGenre rdf:about="http://sparql.cwrc.ca/ontologies/genre#picaresque">
    <skos:definition xml:lang="fr">«Le roman picaresque (de l'espagnol pícaro, « misérable », « futé ») est un genre littéraire né en Espagne au XVIe siècle et qui a connu sa plus florissante époque dans ce pays. Un roman picaresque se compose d'un récit sur le mode autobiographique de l’histoire de héros miséreux, généralement des jeunes gens vivant en marge de la société et à ses dépens. Au cours d’aventures souvent extravagantes supposées plus pittoresques et surtout plus variées que celles des honnêtes gens, qui sont autant de prétextes à présenter des tableaux de la vie vulgaire et des scènes de mœurs, le héros entre en contact avec toutes les couches de la société.» <![CDATA[(<a href="#cwrc:727d97bc-af78-4122-94be-aa78b2e97d5a">DBpedia, 2017</a>)]]></skos:definition>
    <owl:sameAs rdf:resource="http://dbpedia.org/resource/Picaresque_novel"/>
    <rdfs:comment xml:lang="en">The description for this term is indebted to DBpedia. </rdfs:comment>
    <rdfs:label xml:lang="en">picaresque</rdfs:label>
    <owl:sameAs rdf:resource="http://id.loc.gov/authorities/genreForms/gf2014026479"/>
    <skos:definition xml:lang="en">"The picaresque novel (Spanish: "picaresca," from "pícaro," for "rogue" or "rascal") is a genre of prose fiction which depicts the adventures of a roguish hero of low social class who lives by his wits in a corrupt society. Picaresque novels typically adopt a realistic style, with elements of comedy and satire. This style of novel originated in 16th-century Spain and flourished throughout Europe in the 17th and 18th centuries. It continues to influence modern literature. According to the traditional view of Thrall and Hibbard (first published in 1936), seven qualities distinguish the picaresque novel or narrative form, all or some of which may be employed for effect by the author. (1) A picaresque narrative is usually written in first person as an autobiographical account. (2) The main character is often of low character or social class. He or she gets by with wit and rarely deigns to hold a job. (3) There is no plot. The story is told in a series of loosely connected adventures or episodes. (4) There is little if any character development in the main character. Once a picaro, always a picaro. His or her circumstances may change but they rarely result in a change of heart. (5) The picaro's story is told with a plainness of language or realism. (6) Satire might sometimes be a prominent element. (7) The behavior of a picaresque hero or heroine stops just short of criminality. Carefree or immoral rascality positions the picaresque hero as a sympathetic outsider, untouched by the false rules of society. However, Trall and Hibbert's thesis has been questioned by scholars[specify] interested in how genre functions, rather than how it looks on the surface." <![CDATA[(<a href="#cwrc:727d97bc-af78-4122-94be-aa78b2e97d5a">DBpedia, 2017</a>)]]></skos:definition>
  </genre:FictionalGenre>
  <genre:DramaticGenre rdf:about="http://sparql.cwrc.ca/ontologies/genre#camp">
    <rdfs:label xml:lang="en">camp</rdfs:label>
  </genre:DramaticGenre>
  <genre:AdvertisementForm rdf:about="http://sparql.cwrc.ca/ontologies/genre#advertisement">
    <rdfs:label xml:lang="en">advertisement</rdfs:label>
  </genre:AdvertisementForm>
  <genre:ThematicWritingGenre rdf:about="http://sparql.cwrc.ca/ontologies/genre#paranormal">
    <rdfs:label xml:lang="en">paranormal</rdfs:label>
  </genre:ThematicWritingGenre>
  <genre:MusicalGenre rdf:about="http://sparql.cwrc.ca/ontologies/genre#hymn">
    <owl:sameAs rdf:resource="http://id.loc.gov/authorities/genreForms/gf2014026872"/>
    <rdfs:label xml:lang="en">hymn</rdfs:label>
    <skos:definition xml:lang="fr">Des chants d'éloge en l'honneur des dieux, de pays, de personnes célèbres ou d'autres objets de haute estime, en particulier les textes métrique en strophes non bibliques destinés à être chantés durant les services religieux.</skos:definition>
    <skos:definition xml:lang="en">"A religious song consisting of one or more repeating rhythmical stanzas. In classical Roman literature, hymns to Minerva and Jupiter survive. The Greek poet Sappho wrote a number of hymns to Aphrodite. More recently a vast number of hymns appear in Catholic and Protestant religious lyrics. A particularly vibrant tradition of hymn-writing comes from the South's African-American population during the nineteenth century. In the realm of fiction, C.S. Lewis creates hymns for the Solid Ones in The Great Divorce, and Tolkien creates Elvish hymns such as "O Elbereth" in The Lord of the Rings, typically with quatrain structure alternating with couplet stanzas. In the example of "O Elbereth," the hymn honors one of the Maiar spirits. See also paean." <![CDATA[(<a href="cwrc:509015ff-7641-473e-94c5-688e06952bb7">L. K Wheeler, 2017</a>)]]></skos:definition>
    <dcterms:references rdf:resource="http://web.cn.edu/kwheeler/lit_terms_h.html"/>
    <rdf:type rdf:resource="http://sparql.cwrc.ca/ontologies/genre#PoeticGenre"/>
    <rdfs:label xml:lang="fr">hymne (poétique)</rdfs:label>
    <rdf:type rdf:resource="http://sparql.cwrc.ca/ontologies/genre#ReligiousGenre"/>
    <rdfs:comment xml:lang="en">The description for this term is indebted to Dr. L. Kip Wheeler of Carson-Newman University. </rdfs:comment>
  </genre:MusicalGenre>
  <genre:DidacticGenre rdf:about="http://sparql.cwrc.ca/ontologies/genre#parable">
    <rdfs:comment xml:lang="en">The description for this term is indebted to the Getty Art &amp; Architecture Thesaurus.</rdfs:comment>
    <rdfs:label xml:lang="en">parable</rdfs:label>
    <owl:sameAs rdf:resource="http://vocab.getty.edu/aat/300185342"/>
    <skos:definition xml:lang="fr">«Une parabole (du grec παραϐολή, « rapprochement, comparaison ») est une des variétés de l’allégorie. La parabole est une figure de rhétorique consistant en une courte histoire qui utilise les événements quotidiens pour illustrer un enseignement, une morale ou une doctrine. Tandis que celle-ci, en général, présente directement le fait qu’elle a en vue, la parabole offre, sous ses couleurs véritables, un fait qui doit servir à la démonstration d’une vérité d’un autre ordre, avec laquelle elle a une relation plus ou moins facile à saisir. « Substituez dans la parabole, dit l’abbé Girard, le véritable fait à celui qu’elle expose, vous changerez le fond du discours : substituez dans l’allégorie les véritables couleurs à celles qu’elle emprunte, vous ne changerez que la forme. » On la trouve également dans le discours argumentatif lorsqu’un récit illustre la thèse défendue pour faciliter la compréhension du lecteur. La parabole est également un récit allégorique qui permet de dispenser un enseignement moral ou religieux. Présente dans la Bible où elle joue le rôle de l’apologue et de la fable, surtout les Évangiles, qui l'ont empruntée au midrash hébreu, la parabole est reprise dans les sermons des orateurs chrétiens. Le Nouveau Testament en contient un très grand nombre : le grain de sénevé ou l’Église, le Bon Samaritain ou l’amour de l’humanité, le levain ou la grâce, les loups ravisseurs sous des peaux d’agneaux ou les instituteurs de fausses doctrines, le travail des ouvriers de la vigne ou les œuvres du salut, le mauvais riche ou l’obligation de l’aumône, le bon pasteur, etc. Les paraboles sont plus fréquentes encore dans la littérature bouddhique ; les Avadanas, le Hitopadekas donnent à peine l’idée des recueils plus vastes dont ils sont extraits et dont l’un s’appelle le Yu-Lin, c’est-à-dire la « Forêt de comparaisons». Dans les littératures modernes, les Allemands ont surtout cultivé la parabole ; Lessing, Herder, Krummacher y ont particulièrement réussi. Dans le Bouc émissaire, page 270, René Girard remarque que « paraballo signifie jeter quelque chose en pâture à la foule pour apaiser son appétit de violence, de préférence une victime, un condamné à mort ; c'est ainsi qu'on se tire soi-même d'une situation épineuse, de toute évidence. C'est pour empêcher la foule de se retourner contre l'orateur que celui-ci recourt à la parabole, c'est-à-dire à la métaphore. »» <![CDATA[(<a href="#cwrc:727d97bc-af78-4122-94be-aa78b2e97d5a">DBpedia, 2017</a>)]]></skos:definition>
    <skos:definition xml:lang="en">"Short, fictitious stories that illustrate a moral attitude or religious principle." <![CDATA[(<a href="#cwrc:db2f8571-a773-4068-a35f-34262950bb8f">Getty, 2017</a>)]]></skos:definition>
    <owl:sameAs rdf:resource="http://id.loc.gov/authorities/genreForms/gf2014026467"/>
  </genre:DidacticGenre>
  <genre:BookForm rdf:about="http://sparql.cwrc.ca/ontologies/genre#notebook">
    <skos:definition xml:lang="fr">Écrivant au jour le jour, au fil des événements, ou à une fréquence moins&#13;
régulière, l’auteur note, sur le vif, ses impressions, ses sentiments, des faits&#13;
observés. L’ouvrage s’organise généralement en courts chapitres ou&#13;
paragraphes, souvent précédés de la date du jour d’écriture.</skos:definition>
    <skos:definition xml:lang="en">"Notebook is a style of writing where people jot down what they have thought or heard at the spur of moment. The contents of a notebook are unorganized, and the number of subjects covered in a notebook are unlimited: a paragraph of autobiography can be followed immediately by one on astronomy or one on history. Some famous authors are also famous for the notebooks they left. The Italian poet Giacomo Leopardi kept a notebook, called Zibaldone, from 1817 to 1832. The idea of keeping that, which contains no fewer than 4,526 pages, was possibly suggested by a priest who fled from the French Revolution and came to live in the poet's hometown. The priest suggested that "every literary man should have a written chaos such as this: notebook containing sottiseries, adrersa, excerpta, pugillares, commentaria... the store-house out of which fine literature of every kind may come, as the sun, moon, and stars issued out of chaos." There are writers who earned their posthumous fame solely by their notebooks, such as the German scientist and humorous writer Georg Lichtenberg. He called his notebooks "waste book," using the English book-keeping term. He explains the purpose of his "waste book" in his notebook E: The notebooks of scientists, such as those of Michael Faraday and Charles Darwin, can reveal the development of their scientific theories. On the other hand, the notebooks used by scientists for recording their experiments are called lab notebooks. The notebooks used by artists are usually referred as sketchbooks, which may contain more than sketches. Leonardo da Vinci's notebooks contain his writings on painting, sculpture, architecture, anatomy, mining, inventions and music, as well as his sketches, his grocery lists and the names of people who owed him money. In Chinese literature, "notebook" or biji is a distinct genre, and has a broader meaning." <![CDATA[(<a href="#cwrc:727d97bc-af78-4122-94be-aa78b2e97d5a">DBpedia, 2017</a>)]]></skos:definition>
    <owl:sameAs rdf:resource="http://id.loc.gov/authorities/genreForms/gf2014026133"/>
    <rdfs:comment xml:lang="en">The description for this term is indebted to DBpedia. </rdfs:comment>
    <rdfs:label xml:lang="fr">carnet ou journal</rdfs:label>
    <rdfs:label xml:lang="en">notebook</rdfs:label>
    <owl:sameAs rdf:resource="http://dbpedia.org/resource/Notebook_(style)"/>
  </genre:BookForm>
  <genre:LGBTQPlusGenre rdf:about="http://sparql.cwrc.ca/ontologies/genre#lesbian">
    <skos:altLabel xml:lang="en">lesbianWriting</skos:altLabel>
    <rdfs:label xml:lang="en">lesbian</rdfs:label>
    <skos:definition xml:lang="en">Lesbian literature is a subgenre of literature addressing lesbian themes. It includes poetry, plays, fiction addressing lesbian characters, and non-fiction about lesbian-interest topics.</skos:definition>
    <rdf:type rdf:resource="http://sparql.cwrc.ca/ontologies/genre#ThematicWritingGenre"/>
  </genre:LGBTQPlusGenre>
  <genre:ThematicWritingGenre rdf:about="http://sparql.cwrc.ca/ontologies/genre#immigration">
    <rdfs:label xml:lang="en">immigration</rdfs:label>
  </genre:ThematicWritingGenre>
  <genre:ProverbForm rdf:about="http://sparql.cwrc.ca/ontologies/genre#proverb">
    <rdfs:label xml:lang="en">proverb</rdfs:label>
  </genre:ProverbForm>
  <genre:DramaticGenre rdf:about="http://sparql.cwrc.ca/ontologies/genre#tragedy">
    <skos:definition xml:lang="en">"Literary works of serious and dignified character that reach disastrous or sorrowful conclusions." <![CDATA[(<a href="#cwrc:db2f8571-a773-4068-a35f-34262950bb8f">Getty, 2017</a>)]]></skos:definition>
    <owl:sameAs rdf:resource="http://dbpedia.org/resource/Tragedy"/>
    <rdfs:comment xml:lang="en">The description for this term is indebted to DBpedia. </rdfs:comment>
    <rdfs:label xml:lang="fr">tragédie</rdfs:label>
    <skos:definition xml:lang="fr">«La tragédie est un genre théâtral dont l’origine remonte au théâtre grec antique. Contrairement à la comédie, elle met en scène des personnages de rangs élevés et se dénoue très souvent par la mort d’un ou de plusieurs personnages.Elle a un rôle cathartique (prévenir les gens de ne pas faire le Mal en suscitant terreur et pitié).» <![CDATA[(<a href="#cwrc:727d97bc-af78-4122-94be-aa78b2e97d5a">DBpedia, 2017</a>)]]></skos:definition>
    <owl:sameAs rdf:resource="http://id.loc.gov/authorities/genreForms/gf2014026576"/>
    <rdfs:label xml:lang="en">tragedy</rdfs:label>
  </genre:DramaticGenre>
  <genre:HistoricalGenre rdf:about="http://sparql.cwrc.ca/ontologies/genre#historicalWriting">
    <skos:definition xml:lang="fr">«La fiction historique est un genre de fiction qui situe le récit dans le cadre historique précis d'un passé proche ou lointain. Des exemples connus de fiction historique sont le roman Sinouhé l'Égyptien, la bande dessinée L'Épervier ou le film Meurtre dans un jardin anglais. D'autres romans tels que Les Piliers de la Terre se placent également dans un contexte réaliste, respectant scrupuleusement les faits historiques, tout en déroulant un fil principal à caractère fictionnel : Ainsi, le livre reprend le thème du Moyen Âge central et narre la vie d'un bâtisseur de l'époque.» <![CDATA[(<a href="#cwrc:727d97bc-af78-4122-94be-aa78b2e97d5a">DBpedia, 2017</a>)]]></skos:definition>
    <rdfs:label xml:lang="en">historical writing</rdfs:label>
    <rdfs:label xml:lang="fr">écrivage historique</rdfs:label>
    <skos:definition xml:lang="en">"Refers to maps that indicate political administrative boundaries or other characteristics of a region at periods of time before the present. They typically include historical names for places, historical population dispositions, and the historical state of physical features." <![CDATA[(<a href="#cwrc:db2f8571-a773-4068-a35f-34262950bb8f">Getty, 2017</a>)]]></skos:definition>
    <owl:sameAs rdf:resource="http://dbpedia.org/resource/Historical_fiction"/>
    <rdfs:comment xml:lang="en">This term and its description were created from data gathered from DBpedia.</rdfs:comment>
  </genre:HistoricalGenre>
  <genre:NovelisticGenre rdf:about="http://sparql.cwrc.ca/ontologies/genre#novella">
    <owl:sameAs rdf:resource="http://vocab.getty.edu/aat/300202569"/>
    <rdfs:label xml:lang="fr">novella</rdfs:label>
    <owl:sameAs rdf:resource="http://id.loc.gov/authorities/genreForms/gf2015026019"/>
    <skos:definition xml:lang="en">"Short prose tales popular in the Renaissance and for later prose narratives intermediate between novels and short stories." <![CDATA[(<a href="#cwrc:db2f8571-a773-4068-a35f-34262950bb8f">Getty, 2017</a>)]]></skos:definition>
    <rdfs:label xml:lang="en">novella</rdfs:label>
    <rdfs:comment xml:lang="en">The description for this term is indebted to the Getty Art &amp; Architecture Thesaurus.</rdfs:comment>
    <skos:definition xml:lang="fr">Brèves histoires en prose populaires à la Renaissance, et ensuite formes de de prose intermédiaires entre le roman et la nouvelle.</skos:definition>
  </genre:NovelisticGenre>
  <genre:TextualMedium rdf:about="http://sparql.cwrc.ca/ontologies/genre#document">
    <rdfs:label xml:lang="en">document</rdfs:label>
  </genre:TextualMedium>
  <genre:PoeticGenre rdf:about="http://sparql.cwrc.ca/ontologies/genre#epyllion">
    <rdfs:label xml:lang="en">epyllion</rdfs:label>
    <rdfs:comment xml:lang="en">This term and its description were created from data gathered from DBpedia.</rdfs:comment>
    <skos:definition xml:lang="fr">«Un épyllion (en grec ancien ἐπύλλιον / epúllion diminutif de ἔπος / épos [« parole » racine d'ἐποποιία / epopoiía : « épopée »]) est, dans la littérature grecque et latine, une épopée très brève. C'est un poème narratif de quelques centaines d'hexamètres portant généralement sur la vie d'un héros ou d'une héroïne mythique et plus particulièrement sur ses amours.» <![CDATA[(<a href="#cwrc:727d97bc-af78-4122-94be-aa78b2e97d5a">DBpedia, 2017</a>)]]></skos:definition>
    <owl:sameAs rdf:resource="http://dbpedia.org/resource/Epyllion"/>
    <skos:definition xml:lang="en">"Brief narrative poems in dactylic hexameter of ancient Greece, imitated by Romans and others. Usually dealing with mythological and romantic themes. They are characterized by lively description, miniaturistic attitude, scholarly allusion, and an elevated tone similar to that of the elegy." <![CDATA[(<a href="#cwrc:db2f8571-a773-4068-a35f-34262950bb8f">Getty, 2017</a>)]]></skos:definition>
    <rdfs:label xml:lang="fr">epyllion</rdfs:label>
  </genre:PoeticGenre>
  <genre:PoeticGenre rdf:about="http://sparql.cwrc.ca/ontologies/genre#poetry">
    <owl:sameAs rdf:resource="http://id.loc.gov/authorities/genreForms/gf2014026481"/>
    <skos:definition xml:lang="fr">«La poésie est un genre littéraire très ancien aux formes variées, écrites généralement en vers, mais qui admettent aussi la prose, et qui privilégient l'expressivité de la forme, les mots disant plus qu'eux-mêmes par leur choix (sens et sonorités) et leur agencement (rythmes, métrique, figures de style). Sa définition se révèle difficile et varie selon les époques, au point que chaque siècle a pu lui trouver une fonction et une expression différente, à quoi s'ajoute l'approche propre à la personnalité de chaque poète. Le terme « poésie » et ses dérivés viennent du grec ancien ποίησις, et s'écrivait, jusqu'en 1878 poësie (le tréma marquait une disjonction entre les voyelles o et e). ποιεῖν (poiein) signifie « faire, créer » : le poète est donc un créateur, un inventeur de formes expressives, ce que révèlent aussi les termes du Moyen Âge, comme trouvère et troubadour. Le poète, héritier d'une longue tradition orale, privilégie la musicalité et le rythme, d'où, dans la plupart des textes poétiques, le recours à une forme versifiée qui confère de la densité à la langue. Le poète recherche aussi l'expressivité par le poids accordé aux mots comme par l'utilisation des figures de style et au premier chef des images et des figures d'analogie, recherchées pour leur force suggestive. La poésie s'est constamment renouvelée au cours des siècles avec des orientations différentes selon les époques, les civilisations et les individus. On peut par exemple distinguer le poète artiste soucieux d'abord de beauté formelle, le poète « lyrique » qui cultive le « chant de l'âme », le poète prophète, découvreur du monde et « voyant » ou le poète engagé, sans cependant réduire un créateur à une étiquette simplificatrice.» <![CDATA[(<a href="#cwrc:727d97bc-af78-4122-94be-aa78b2e97d5a">DBpedia, 2017</a>)]]></skos:definition>
    <rdfs:label xml:lang="en">poetry</rdfs:label>
    <rdfs:comment xml:lang="en">The description for this term is indebted to DBpedia. </rdfs:comment>
    <owl:sameAs rdf:resource="http://dbpedia.org/resource/Poetry"/>
    <rdfs:label xml:lang="fr">poésie</rdfs:label>
    <skos:definition xml:lang="en">"Poetry is a form of literature that uses aesthetic and rhythmic qualities of language—such as phonaesthetics, sound symbolism, and metre—to evoke meanings in addition to, or in place of, the prosaic ostensible meaning." <![CDATA[(<a href="#cwrc:727d97bc-af78-4122-94be-aa78b2e97d5a">DBpedia, 2017</a>)]]></skos:definition>
  </genre:PoeticGenre>
  <genre:StillImageMedium rdf:about="http://sparql.cwrc.ca/ontologies/genre#photograph">
    <rdfs:label xml:lang="en">photograph</rdfs:label>
    <skos:related rdf:resource="http://vocab.getty.edu/aat/300046300"/>
  </genre:StillImageMedium>
  <genre:IllustratedForm rdf:about="http://sparql.cwrc.ca/ontologies/genre#colouringBook">
    <skos:definition xml:lang="fr">"Livres contenant des dessins à colorier à l'aide de crayons gras, aquarelles, crayons de couleur ou autres techniques, généralement destinés aux enfants."</skos:definition>
    <skos:definition xml:lang="en">"Books containing outline drawings, for coloring in with crayons, watercolor, colored pencils, or other media, usually intended for use by children." <![CDATA[(<a href="#cwrc:db2f8571-a773-4068-a35f-34262950bb8f">Getty, 2017</a>)]]></skos:definition>
    <owl:sameAs rdf:resource="http://vocab.getty.edu/aat/300026449"/>
    <rdfs:comment xml:lang="en">The description for this term is indebted to the Getty Art &amp; Architecture Thesaurus.</rdfs:comment>
    <owl:sameAs rdf:resource="http://id.loc.gov/authorities/genreForms/gf2017026082"/>
    <rdfs:label xml:lang="en">colouring book</rdfs:label>
    <rdfs:label xml:lang="fr">livre de coloriage</rdfs:label>
  </genre:IllustratedForm>
  <genre:PoeticGenre rdf:about="http://sparql.cwrc.ca/ontologies/genre#poeticDrama">
    <owl:sameAs rdf:resource="http://id.loc.gov/authorities/genreForms/gf2014026585"/>
    <rdfs:label xml:lang="en">poetic drama</rdfs:label>
  </genre:PoeticGenre>
  <genre:ThematicWritingGenre rdf:about="http://sparql.cwrc.ca/ontologies/genre#guidebook">
    <owl:sameAs rdf:resource="http://id.loc.gov/authorities/genreForms/gf2014026108"/>
    <rdfs:label xml:lang="en">guidebook</rdfs:label>
    <skos:definition xml:lang="en">"Handbooks for the guidance of strangers or visitors in a district, town, building, etc., giving a description of the roads, places, or objects of interest to be found there." <![CDATA[(<a href="#cwrc:db2f8571-a773-4068-a35f-34262950bb8f">Getty, 2017</a>)]]></skos:definition>
    <rdfs:label xml:lang="fr">guide de voyage</rdfs:label>
    <rdfs:comment xml:lang="en">The description for this term is indebted to the Getty Art &amp; Architecture Thesaurus.</rdfs:comment>
    <skos:definition xml:lang="fr">Manuels destinés à guider des étrangers ou des visiteurs dans un quartier, une ville, un bâtiment, etc., en décrivant les routes, les lieux ou les sujets d'intérêt qui s'y trouvent.</skos:definition>
    <owl:sameAs rdf:resource="http://vocab.getty.edu/aat/300026300"/>
  </genre:ThematicWritingGenre>
  <genre:InformationalGenre rdf:about="http://sparql.cwrc.ca/ontologies/genre#biography">
    <rdfs:label xml:lang="en">biography</rdfs:label>
    <skos:definition xml:lang="en">"The genre of nonfiction that concerns accounts of the lives of individuals." <![CDATA[(<a href="#cwrc:db2f8571-a773-4068-a35f-34262950bb8f">Getty, 2017</a>)]]></skos:definition>
    <rdfs:comment xml:lang="en">The description for this term is indebted to DBpedia. </rdfs:comment>
    <rdfs:comment xml:lang="fr">La description de ce terme est basée sur celle de DBPedia.</rdfs:comment>
    <skos:definition xml:lang="fr">«Une biographie (une bio), du grec ancien βίος, « la vie » et γραφή, « écrire », est un écrit qui a pour objet l'histoire d'une vie particulière. Elle peut être écrite par la personne elle-même (autobiographie) ou par une autre personne.» <![CDATA[(<a href="#cwrc:727d97bc-af78-4122-94be-aa78b2e97d5a">DBpedia, 2017</a>)]]></skos:definition>
    <owl:sameAs rdf:resource="http://vocab.getty.edu/aat/300055908"/>
    <rdfs:label xml:lang="fr">biographie </rdfs:label>
    <owl:sameAs rdf:resource="http://id.loc.gov/authorities/genreForms/gf2014026049"/>
  </genre:InformationalGenre>
  <genre:PoeticGenre rdf:about="http://sparql.cwrc.ca/ontologies/genre#longPoem">
    <rdfs:label xml:lang="en">long poem</rdfs:label>
  </genre:PoeticGenre>
  <genre:SerialForm rdf:about="http://sparql.cwrc.ca/ontologies/genre#periodicalFeature">
    <rdfs:label xml:lang="en">periodical feature</rdfs:label>
  </genre:SerialForm>
  <genre:ReligiousGenre rdf:about="http://sparql.cwrc.ca/ontologies/genre#prayer">
    <skos:definition xml:lang="fr">Documents contenant des requêtes respectueusement adressées à une divinité ou à une autre entité spirituelle.</skos:definition>
    <skos:definition xml:lang="en">"Reverent petitions, usually in verse or prose, to a deity or other spiritual entity." <![CDATA[(<a href="#cwrc:db2f8571-a773-4068-a35f-34262950bb8f">Getty, 2017</a>)]]></skos:definition>
    <owl:sameAs rdf:resource="http://id.loc.gov/authorities/genreForms/gf2015026049"/>
    <owl:sameAs rdf:resource="http://vocab.getty.edu/aat/300026452"/>
    <rdfs:label xml:lang="fr">prière</rdfs:label>
    <rdfs:comment xml:lang="en">This term and its description were created from data gathered from the Getty Art &amp; Architecture Thesaurus.</rdfs:comment>
    <rdfs:label xml:lang="en">prayer</rdfs:label>
  </genre:ReligiousGenre>
  <genre:OperaGenre rdf:about="http://sparql.cwrc.ca/ontologies/genre#opera">
    <rdfs:label xml:lang="en">opera</rdfs:label>
    <rdfs:label xml:lang="fr">opéra</rdfs:label>
    <skos:definition xml:lang="en">"Dramatic musical performances in which most roles are sung with instrumental accompanyment, usually including arias, recitives, and choruses. Typically, they are intended to be staged with costumes, sets, and dramatic movement." <![CDATA[(<a href="#cwrc:db2f8571-a773-4068-a35f-34262950bb8f">Getty, 2017</a>)]]></skos:definition>
    <rdf:type rdf:resource="http://sparql.cwrc.ca/ontologies/genre#PerformanceMedium"/>
    <owl:sameAs rdf:resource="http://vocab.getty.edu/aat/300054147"/>
    <skos:definition xml:lang="fr">«Un opéra est une œuvre destinée à être chantée sur une scène, appartenant à un genre musical vocal du même nom ; l'opéra est l’une des formes du théâtre musical occidental regroupées sous l’appellation d’art lyrique. L'œuvre, chantée par des interprètes possédant un registre vocal déterminé en fonction du rôle et accompagnés par un orchestre, parfois symphonique, parfois de chambre, parfois destiné exclusivement au seul répertoire d'opéra, est constituée d'un livret mis en musique sous forme d'airs, de récitatifs, de chœurs, d'intermèdes souvent précédés d'une ouverture, et parfois agrémentée de ballets. Le genre musical est décliné selon les pays et les époques et recouvre des œuvres d’appellations et de formes différentes. Aujourd’hui, les œuvres sont jouées dans des salles d’opéra spécifiquement affectées ou tout simplement sur des scènes de théâtre ou dans des salles de concerts. Les représentations sont organisées par des institutions du secteur public ou privé, parfois désignées sous le vocable de « maison d'opéra », qui peuvent regrouper les compagnies d’artistes (orchestre, chœur et ballet) et les services administratifs et techniques nécessaires à l’organisation des saisons culturelles. (fr»)<![CDATA[(<a href="#cwrc:727d97bc-af78-4122-94be-aa78b2e97d5a">DBpedia, 2017</a>)]]></skos:definition>
    <rdfs:comment xml:lang="en">This term and its description were created from data gathered from the Getty Art &amp; Architecture Thesaurus.</rdfs:comment>
    <owl:sameAs rdf:resource="http://id.loc.gov/authorities/genreForms/gf2014026976"/>
  </genre:OperaGenre>
  <genre:SongGenre rdf:about="http://sparql.cwrc.ca/ontologies/genre#song">
    <rdfs:comment xml:lang="en">The description for this term is indebted to Dr. L. Kip Wheeler of Carson-Newman University. </rdfs:comment>
    <owl:sameAs rdf:resource="http://dbpedia.org/resource/Song"/>
    <rdfs:label xml:lang="fr">chanson</rdfs:label>
    <owl:sameAs rdf:resource="http://id.loc.gov/authorities/genreForms/gf2014027103"/>
    <skos:definition xml:lang="fr">«Une chanson ou un chant est une œuvre musicale composée d'un texte et d'une mélodie destinée à être interprétée par la voix humaine. Cette interprétation peut se faire sans accompagnement instrumental, c'est-à-dire a cappella, ou au contraire être accompagnée d'un ou plusieurs instruments (guitare, piano, groupe, voire un big band ou un grand orchestre symphonique). Elle peut être à une voix (monodie) ou à plusieurs (polyphonie) comme dans un choral.» <![CDATA[(<a href="#cwrc:727d97bc-af78-4122-94be-aa78b2e97d5a">DBpedia, 2017</a>)]]></skos:definition>
    <rdfs:label xml:lang="en">song</rdfs:label>
    <skos:definition xml:lang="en">"A lyric poem with a number of repeating stanzas (called refrains), written to be set to music in either vocal performance or with accompaniment of musical instruments." <![CDATA[(<a href="cwrc:509015ff-7641-473e-94c5-688e06952bb7">L. K Wheeler, 2017</a>)]]></skos:definition>
  </genre:SongGenre>
  <genre:StillImageMedium rdf:about="http://sparql.cwrc.ca/ontologies/genre#drawing">
    <rdfs:label xml:lang="en">drawing</rdfs:label>
    <skos:related rdf:resource="http://vocab.getty.edu/aat/300033973"/>
  </genre:StillImageMedium>
  <genre:ThematicWritingGenre rdf:about="http://sparql.cwrc.ca/ontologies/genre#industrialNovel">
    <rdfs:label xml:lang="en">industrial novel</rdfs:label>
    <rdfs:label xml:lang="fr">roman industriel</rdfs:label>
    <skos:definition xml:lang="fr">«Le roman industriel est un genre littéraire qui fait son apparition au début de l'ère victorienne en Grande-Bretagne. Classé dans la catégorie plus vaste du roman social, il décrit le déclin d’un monde essentiellement rural gagné par de nouvelles formes de production et d'urbanisation et aborde les difficultés dans lesquelles se débattent les ouvriers non seulement pour survivre mais aussi pour défendre leur humanité pendant et après la révolution industrielle. Certains romans industriels témoignent de sympathie pour le chartisme et les formes d’action pacifiques comme la grève.» <![CDATA[(<a href="#cwrc:727d97bc-af78-4122-94be-aa78b2e97d5a">DBpedia, 2017</a>)]]></skos:definition>
    <skos:related rdf:resource="http://id.loc.gov/authorities/genreForms/gf2017026040"/>
    <rdf:type rdf:resource="http://sparql.cwrc.ca/ontologies/genre#NovelisticGenre"/>
    <rdfs:comment xml:lang="en">This term and its description were created from data gathered from DBpedia.</rdfs:comment>
    <owl:sameAs rdf:resource="http://dbpedia.org/resource/Industrial_novel"/>
    <skos:definition xml:lang="en">"A novel that exposes the living or working conditions of the 19th century-working class as a result of the industrial revolution. The shocking circumstances—extreme poverty, deplorable factory conditions, widespread disease, over-crowded housing, etc.—are typically described in great detail. Solutions are often proposed, but the main goal of an industrial novel is to make the plight of the lower class known to the middle and upper classes in order to promote social change." <![CDATA[(<a href="#cwrc:2f09376c-f784-4a46-9f04-5a21aa311f27">Penguin, 1999</a>)]]></skos:definition>
  </genre:ThematicWritingGenre>
  <genre:PoeticGenre rdf:about="http://sparql.cwrc.ca/ontologies/genre#ode">
    <rdfs:label xml:lang="fr">ôde</rdfs:label>
    <owl:sameAs rdf:resource="http://vocab.getty.edu/aat/300253045"/>
    <rdfs:label xml:lang="en">ode</rdfs:label>
    <owl:sameAs rdf:resource="http://id.loc.gov/authorities/genreForms/gf2014026461"/>
    <skos:definition xml:lang="en">"Lyric poems of exalted emotion devoted to the praise or celebration of its subject; often employing complex or irregular metrical form." <![CDATA[(<a href="#cwrc:db2f8571-a773-4068-a35f-34262950bb8f">Getty, 2017</a>)]]></skos:definition>
    <rdfs:comment xml:lang="en">The description for this term is indebted to the Getty Art &amp; Architecture Thesaurus.</rdfs:comment>
    <skos:definition xml:lang="fr">Poèmes lyriques aux sentiments exacerbés voués à l'éloge ou la célébration d'un thème, présentant souvent des formes métriques complexes et irrégulières.</skos:definition>
  </genre:PoeticGenre>
  <genre:MusicalGenre rdf:about="http://sparql.cwrc.ca/ontologies/genre#music">
    <rdfs:label xml:lang="fr">musique</rdfs:label>
    <rdfs:label xml:lang="en">music</rdfs:label>
    <owl:sameAs rdf:resource="http://id.loc.gov/authorities/genreForms/gf2014026952"/>
    <rdfs:comment xml:lang="en">This term and its description were created from data gathered from the Getty Art &amp; Architecture Thesaurus.</rdfs:comment>
    <owl:sameAs rdf:resource="http://vocab.getty.edu/page/aat/300054146"/>
    <skos:definition xml:lang="en">"Performing arts genre having to do with the combining of vocal or instrumental sounds in measured time to communicate emotions, ideas, or states of mind, usually according to cultural standards of rhythm, melody, and, in most Western music, harmony." <![CDATA[(<a href="#cwrc:db2f8571-a773-4068-a35f-34262950bb8f">Getty, 2017</a>)]]></skos:definition>
  </genre:MusicalGenre>
  <genre:DramaticGenre rdf:about="http://sparql.cwrc.ca/ontologies/genre#drama">
    <dcterms:references rdf:resource="http://web.cn.edu/kwheeler/lit_terms_d.html"/>
    <skos:definition xml:lang="en">"A composition in prose or verse presenting, in pantomime and dialogue, a narrative involving conflict between a character or characters and some external or internal force (see conflict). Playwrights usually design dramas for presentation on a stage in front of an audience. Aristotle called drama "imitated human action." Drama may have originated in religious ceremonies. Thespis of Attica (sixth century BCE) was the first recorded composer of a tragedy. Tragedies in their earliest stage were performed by a single actor who interacted with the chorus. The playwright Aeschylus added a second actor on the stage (deuteragonist) to allow additional conflict and dialogue. Sophocles and Euripides added a third (tritagonist). Medieval drama may have evolved independently from rites commemorating the birth and death of Christ. During the late medieval period and the early Renaissance, drama gradually altered to the form we know today. The mid-sixteenth century in England in particular was one of the greatest periods of world drama. In traditional Greek drama, as defined by Aristotle, a play was to consist of five acts and follow the three dramatic unities. In more recent drama (i.e., during the last two centuries), plays have frequently consisted of three acts, and playwrights have felt more comfortable disregarding the confines of Aristotelian rules involving verisimilitude. See also unities, comedy, tragedy, revenge play, miracle play, morality play, and mystery play. An individual work of drama is called a play." <![CDATA[(<a href="cwrc:509015ff-7641-473e-94c5-688e06952bb7">L. K Wheeler, 2017</a>)]]></skos:definition>
    <rdfs:comment xml:lang="en">The description for this term is indebted to Dr. L. Kip Wheeler of Carson-Newman University. </rdfs:comment>
    <rdfs:label xml:lang="fr">genre dramatique</rdfs:label>
    <rdfs:label xml:lang="en">drama</rdfs:label>
    <skos:definition xml:lang="fr">(du grec "drama", action) Formes littéraires, presque toujours sous forme de dialogues (en vers ou un prose) destinés à être joués par des acteurs lors d'une représentation scénique.</skos:definition>
    <owl:sameAs rdf:resource="http://id.loc.gov/authorities/genreForms/gf2014026297"/>
  </genre:DramaticGenre>
  <genre:ThematicWritingGenre rdf:about="http://sparql.cwrc.ca/ontologies/genre#ruralIdyll">
    <rdfs:label xml:lang="en">rural idyll</rdfs:label>
  </genre:ThematicWritingGenre>
  <genre:ThematicWritingGenre rdf:about="http://sparql.cwrc.ca/ontologies/genre#robinsonades">
    <rdfs:label xml:lang="en">robinsonades</rdfs:label>
    <owl:sameAs rdf:resource="http://id.loc.gov/authorities/genreForms/gf2014026514"/>
  </genre:ThematicWritingGenre>
  <genre:AutobiographicalGenre rdf:about="http://sparql.cwrc.ca/ontologies/genre#captivityNarrative">
    <skos:definition xml:lang="fr">Les récits de captivité sont généralement des histoires de personnes capturées par des ennemis qu'ils considèrent comme incivilisés, ou dont les croyances et les coutumes sont opposées aux leurs. Les récits de captivité les plus connus sont ceux concernant les peuples autochtones d'Amérique du Nord. Ces récits (et la question de leur exactitude) ont depuis longtemps leur place dans la littérature, l'histoire, l'ethnographie et l'étude des peuples autochtones. Cependant, les récits de captivité ont également joué un rôle majeur dans l'étude des mouvements religieux contemporains, grâce à des spécialistes de la religion comme David G. Bromley et James R. Lewis. Dans cet article, les deux principaux types de récits de captivité sont considérés. Dans la tradition, l''utilisation de certains récits de captivité par les historiens est restée limitée. Ils ont considéré le genre avec suspicion en raison de ses fondements idéologiques. À la suite de nouvelles approches académiques, des historiens possédant une meilleure compréhension des cultures amérindiennes distinguent les énoncés plausibles de faits et de jugements chargés valeurs afin d'étudier les récits comme de rares sources provenant de "l'intérieur" des sociétés autochtones. Des historiennes contemporaines telles que Linda Colley et des anthropologues comme Pauline Turner Strong ont également trouvé les récits utiles à l'analyse de la construction de "l'Autre" par les colons, et de ce que les récits révèlent de la perception qu'ils ont d'eux-mêmes, de leur culture et de l'expérience de la rencontre avec l'autre. Colley a étudié la longue histoire de la captivité anglaise dans d'autres cultures, à la fois celle des pirates barbaresques précédents ceux d'Amérique du Nord et celle des captifs britanniques en Inde, après l'expérience nord-américaine. Certains récits de captivité nord-américains impliquant des peuples autochtones furent publiés du 18ème au 19ème siècle, et reflétaient un genre déjà bien établi dans la littérature anglaise. Des récits sur la captivité par les pirates barbaresque ou au Moyen-Orient étaient déjà parus en anglais, établissant certains des principaux éléments du genre. À la suite de l'expérience américaine, des récits supplémentaires avaient été écrits après la capture de Britanniques lors de l'exploration et de l'implantation en Inde et en Asie de l'Est. D'autres types de récits de captivité, tels que ceux racontés par les apostats de mouvements religieux (ou "réctis de survivants de sectes"), sont restés une caractéristique récurrente des média modernes et apparaissent aujourd'hui dans les livres, les périodiques, le cinéma et la télévision. Le dénominateur commun des récits de captivité, qu'ils soient la conséquence de conflits géopolitiques ou religieux, est que le captif dépeint le mode de vie des ravisseurs comme différente, indésirable et incompatible avec la propre culture (généralement dominante) du captit. Cela souligne l'utilité des récits de captivité dans le recueil de mesures en faveur du contrôle social, comme la séclusion d'Amérindiens dans "réserves", ou la participation stigmatisante à des mouvements religieux - que ce soit le catholicisme 19ème, ou le ISKCON au 20ème Les récits de captivité ont tendance à être culturellement chauvins, percevant la culture "étrangère" du point de vue subjectif du narrateur, qui comprend des jugements de valeur (éventuellement injustes) du type les "les Puritains sont bons, les Indiens sont mauvais".</skos:definition>
    <owl:sameAs rdf:resource="http://dbpedia.org/resource/Captivity_narrative"/>
    <skos:definition xml:lang="en">"Captivity narratives are usually stories of people captured by enemies whom they consider uncivilized, or whose beliefs and customs they oppose. The best-known captivity narratives are those concerning the indigenous peoples of North America. These narratives (and questions about their accuracy) have an enduring place in literature, history, ethnography, and the study of Native peoples. However, captivity narratives have also come to play a major role in the study of contemporary religious movements, thanks to scholars of religion like David G. Bromley and James R. Lewis. In this article, both main types of captivity narratives are considered. Traditionally, historians have made limited use of certain captivity narratives. They have regarded the genre with suspicion because of its ideological underpinnings. As a result of new scholarly approaches, historians with a more certain grasp of Native American cultures are distinguishing between plausible statements of fact and value-laden judgements in order to study the narratives as rare sources from "inside" Native societies. Contemporary historians such as Linda Colley and anthropologists such as Pauline Turner Strong have also found the narratives useful in analyzing how the colonists constructed the "other", as well as what the narratives reveal about the settlers' sense of themselves and their culture, and the experience of crossing the line to another. Colley has studied the long history of English captivity in other cultures, both the Barbary pirate captives who preceded those in North America, and British captives in cultures such as India, after the North American experience. Certain North American captivity narratives involving Native peoples were published from the 18th through the 19th centuries, but they reflected a well-established genre in English literature. There had already been English accounts of captivity by Barbary pirates, or in the Middle East, which established some of the major elements of the form. Following the American experience, additional accounts were written after British people were captured during exploration and settlement in India and East Asia. Other types of captivity narratives, such as those recounted by apostates from religious movements (i.e. "cult survivor" tales), have remained an enduring feature of modern media, and currently appear in books, periodicals, film, and television. The unifying factor in most captivity narratives, whether they stem from geopolitical or religious conflicts, is that the captive portrays the captors' way of life as alien, undesirable, and incompatible with the captive's own (typically dominant) culture. This underscores the utility of captivity narratives in garnering support for social control measures, such as removing Native Americans to "reservations", or stigmatizing participation in religious movements – whether Catholicism in the nineteenth century, or ISKCON in the twentieth. Captivity narratives tend to be culturally chauvinistic, viewing an "alien" culture through the lens of the narrator's preferred culture, thus making (possibly unfair) value judgements like "Puritans good, Indians bad."" <![CDATA[(<a href="#cwrc:727d97bc-af78-4122-94be-aa78b2e97d5a">DBpedia, 2017</a>)]]></skos:definition>
    <rdfs:comment xml:lang="en">The description for this term is indebted to DBpedia. </rdfs:comment>
    <owl:sameAs rdf:resource="http://id.loc.gov/authorities/genreForms/gf2014026056"/>
    <rdfs:label xml:lang="en">captivity narrative</rdfs:label>
    <rdfs:label xml:lang="fr">récit de captivité</rdfs:label>
  </genre:AutobiographicalGenre>
  <genre:PedagogicalGenre rdf:about="http://sparql.cwrc.ca/ontologies/genre#textbook">
    <rdfs:label xml:lang="en">textbook</rdfs:label>
    <skos:definition xml:lang="en">"Books used as standard works for the formal study of a particular subject." <![CDATA[(<a href="#cwrc:db2f8571-a773-4068-a35f-34262950bb8f">Getty, 2017</a>)]]></skos:definition>
    <rdfs:label xml:lang="fr">manuel scolaire</rdfs:label>
    <skos:definition xml:lang="fr">«Le manuel scolaire (du latin manus, « la main »), considéré au XIXe siècle comme le livre résumant tous les autres est un ouvrage didactique ayant un format maniable et regroupant l'essentiel des connaissances relatives à un domaine donné. Le manuel scolaire est destiné à être utilisé en classe comme support de cours avec l'aide directe ou indirecte d'un enseignant. Il doit tenir compte du caractère progressif de l'apprentissage (âge des élèves, capacité cognitive).» <![CDATA[(<a href="#cwrc:727d97bc-af78-4122-94be-aa78b2e97d5a">DBpedia, 2017</a>)]]></skos:definition>
    <rdfs:comment xml:lang="en">This term and its description were created from data gathered from DBpedia.</rdfs:comment>
    <owl:sameAs rdf:resource="http://dbpedia.org/resource/Textbook"/>
    <owl:sameAs rdf:resource="http://id.loc.gov/authorities/genreForms/gf2014026191"/>
  </genre:PedagogicalGenre>
  <genre:CatalogueForm rdf:about="http://sparql.cwrc.ca/ontologies/genre#exhibitionCatalogue">
    <rdfs:label xml:lang="en">exhibition catalogue</rdfs:label>
    <skos:definition xml:lang="en">"Publications that document the works displayed in an exhibition." <![CDATA[(<a href="#cwrc:db2f8571-a773-4068-a35f-34262950bb8f">Getty, 2017</a>)]]></skos:definition>
    <owl:sameAs rdf:resource="http://id.loc.gov/authorities/genreForms/gf2014026098"/>
    <owl:sameAs rdf:resource="http://vocab.getty.edu/aat/300026096"/>
    <rdfs:label xml:lang="fr">catalogue d'exposition</rdfs:label>
    <rdfs:comment xml:lang="en">The description for this term is indebted to the Getty Art &amp; Architecture Thesaurus.</rdfs:comment>
    <skos:definition xml:lang="fr">Publications qui fournissent des informations sur les oeuvres présentées lors d'une exposition.</skos:definition>
  </genre:CatalogueForm>
  <genre:ComedicGenre rdf:about="http://sparql.cwrc.ca/ontologies/genre#comedyOfHumours">
    <rdfs:label xml:lang="en">comedy of humours</rdfs:label>
  </genre:ComedicGenre>
  <genre:ScholarlyGenre rdf:about="http://sparql.cwrc.ca/ontologies/genre#phdThesis">
    <rdfs:label xml:lang="en">phd thesis</rdfs:label>
  </genre:ScholarlyGenre>
  <genre:PoliticalWritingGenre rdf:about="http://sparql.cwrc.ca/ontologies/genre#socialReform">
    <rdfs:label xml:lang="en">social reform</rdfs:label>
  </genre:PoliticalWritingGenre>
  <genre:PoliticalWritingGenre rdf:about="http://sparql.cwrc.ca/ontologies/genre#agitprop">
    <skos:definition xml:lang="en">"Derived from agitation propaganda, meaning intended to inspire political action. With reference to visual art, refers to the specific art movement arising in Soviet Russia following the Bolshevik revolution." <![CDATA[(<a href="#cwrc:db2f8571-a773-4068-a35f-34262950bb8f">Getty, 2017</a>)]]></skos:definition>
    <rdfs:label xml:lang="en">agitprop</rdfs:label>
    <rdf:type rdf:resource="http://sparql.cwrc.ca/ontologies/genre#DramaticGenre"/>
    <skos:definition xml:lang="fr">"Le terme est dérivé de "propagande d'agitation" et incite à l'action politique. En référence à l'art visuel, il renvoie plus particulièrement au mouvement artistique en essor durant la période qui suit la révolution bolchévique en URSS.  "</skos:definition>
    <rdfs:label xml:lang="fr">agitprop</rdfs:label>
    <rdfs:comment xml:lang="en">The description for this term is indebted to the Getty Art &amp; Architecture Thesaurus.</rdfs:comment>
    <owl:sameAs rdf:resource="http://vocab.getty.edu/aat/300055540"/>
  </genre:PoliticalWritingGenre>
  <genre:NovelisticGenre rdf:about="http://sparql.cwrc.ca/ontologies/genre#silverForkNovel">
    <skos:definition xml:lang="en">"A mocking term for a popular literary genre depicting life in upper-class British society in the 1820s-1840s." <![CDATA[(<a href="#cwrc:4c227091-6bf0-4325-b846-9733fae19e61">Oxford, 2015</a>)]]></skos:definition>
    <dcterms:references rdf:resource="http://www.oxfordreference.com/view/10.1093/acref/9780199208272.001.0001/acref-9780199208272-e-1057?rskey=bq3DDS%26result=1061"/>
    <rdfs:label xml:lang="en">silver-fork novel</rdfs:label>
    <rdfs:comment xml:lang="en">This term and its description were created from data gathered from the Oxford Dictionary of Literary Terms, 4th ed.</rdfs:comment>
  </genre:NovelisticGenre>
  <genre:ThematicWritingGenre rdf:about="http://sparql.cwrc.ca/ontologies/genre#eulogy">
    <owl:sameAs rdf:resource="http://dbpedia.org/resource/Eulogy"/>
    <skos:definition xml:lang="fr">«L’éloge (masculin du latin elogium, avec l’influence du grec εὐλογία) est un genre littéraire hérité de l'Antiquité, où il est très présent, qui consiste à vanter les mérites d'un individu ou d'une institution. Il s'agit d'un discours public ou donné comme tel, destiné à l'édification commune ; à cette fin, il recourt à l'exploitation des ressources du discours épidictique héritées de la rhétorique classique. Il existe plusieurs sortes d'éloges:»</skos:definition>
    <skos:definition xml:lang="en">"A eulogy (from εὐλογία, eulogia, Classical Greek for "praise") is a speech or writing in praise of a person(s) or thing(s), especially one who recently died or retired or as a term of endearment. Eulogies may be given as part of funeral services. They take place in a funeral home during or after a wake. However, some denominations either discourage or do not permit eulogies at services to maintain respect for traditions. Eulogies can also praise people who are still alive. This normally takes place on special occasions like birthdays, office parties, retirement celebrations, etc. Eulogies should not be confused with elegies, which are poems written in tribute to the dead; nor with obituaries, which are published biographies recounting the lives of those who have recently died; nor with obsequies, which refer generally to the rituals surrounding funerals. Catholic priests are prohibited by the rubrics of the Mass from presenting a eulogy for the deceased in place of a homily during a funeral Mass. The modern use of the word eulogy was first documented in the 15th century and came from the Medieval Latin term “eulogium” (Merriam-Webster 2012). “Eulogium” at that time has since turned into the shorter “eulogy” of today. Eulogies are usually delivered by a family member or a close family friend in the case of a dead person. For a living eulogy given in such cases as a retirement, a senior colleague could perhaps deliver it. On occasions, eulogies are given to those who are severely ill or elderly in order to express words of love and gratitude before they die. Eulogies are not limited to merely people, however; Places or things can also be given eulogies (which anyone can deliver), but these are less common than those delivered to people, whether living or deceased." <![CDATA[(<a href="#cwrc:727d97bc-af78-4122-94be-aa78b2e97d5a">DBpedia, 2017</a>)]]></skos:definition>
    <rdfs:comment xml:lang="en">The description for this term is indebted to DBpedia. </rdfs:comment>
    <rdfs:label xml:lang="en">eulogy</rdfs:label>
  </genre:ThematicWritingGenre>
  <genre:PoeticGenre rdf:about="http://sparql.cwrc.ca/ontologies/genre#prosePoem">
    <rdfs:label xml:lang="en">prose poem</rdfs:label>
    <owl:sameAs rdf:resource="http://id.loc.gov/authorities/genreForms/gf2014026488"/>
  </genre:PoeticGenre>
  <genre:DramaticGenre rdf:about="http://sparql.cwrc.ca/ontologies/genre#epicTheatre">
    <rdfs:label xml:lang="en">epic theatre</rdfs:label>
  </genre:DramaticGenre>
  <genre:PoliticalWritingGenre rdf:about="http://sparql.cwrc.ca/ontologies/genre#politicalWriting">
    <skos:definition xml:lang="fr">Écrit au sujet de la politique, généralement écrit dans un ton persuasif en faveur d'un parti ou d'une cause politique particulière.</skos:definition>
    <skos:definition xml:lang="en">Writing on the subject of politics, often persuasive in tone and written in favour of a particular political party or cause.</skos:definition>
    <rdfs:label xml:lang="fr">écrits politiques</rdfs:label>
    <rdfs:label xml:lang="en">political writing</rdfs:label>
  </genre:PoliticalWritingGenre>
  <genre:ReligiousGenre rdf:about="http://sparql.cwrc.ca/ontologies/genre#religious">
    <rdfs:label xml:lang="fr">religieux</rdfs:label>
    <rdfs:label xml:lang="en">religious</rdfs:label>
    <skos:definition xml:lang="fr">Écrits traitent de la religion ou de la spiritualité.</skos:definition>
    <skos:definition xml:lang="en">Writing dealing with religion or spirituality.</skos:definition>
  </genre:ReligiousGenre>
  <genre:ReligiousGenre rdf:about="http://sparql.cwrc.ca/ontologies/genre#conversionNarrative">
    <rdfs:label xml:lang="en">conversion narrative</rdfs:label>
  </genre:ReligiousGenre>
  <genre:PoeticGenre rdf:about="http://sparql.cwrc.ca/ontologies/genre#dub">
    <rdfs:label xml:lang="en">dub</rdfs:label>
  </genre:PoeticGenre>
  <genre:ScriptForm rdf:about="http://sparql.cwrc.ca/ontologies/genre#filmScript">
    <rdfs:label xml:lang="en">film script</rdfs:label>
  </genre:ScriptForm>
  <genre:DigitalMedium rdf:about="http://sparql.cwrc.ca/ontologies/genre#webpage">
    <rdfs:label xml:lang="en">webpage</rdfs:label>
  </genre:DigitalMedium>
  <genre:ThematicWritingGenre rdf:about="http://sparql.cwrc.ca/ontologies/genre#nationalist">
    <rdfs:label xml:lang="en">nationalist</rdfs:label>
  </genre:ThematicWritingGenre>
  <genre:SoundRecordingMedium rdf:about="http://sparql.cwrc.ca/ontologies/genre#soundRecordingNonmusical">
    <rdfs:label xml:lang="en">sound recording – nonmusical</rdfs:label>
  </genre:SoundRecordingMedium>
  <genre:NarrativeGenre rdf:about="http://sparql.cwrc.ca/ontologies/genre#oralHistory">
    <rdfs:label xml:lang="en">oral history</rdfs:label>
    <rdf:type rdf:resource="http://sparql.cwrc.ca/ontologies/genre#HistoricalGenre"/>
  </genre:NarrativeGenre>
  <genre:IllustratedForm rdf:about="http://sparql.cwrc.ca/ontologies/genre#illustrated">
    <rdfs:label xml:lang="en">illustrated</rdfs:label>
  </genre:IllustratedForm>
  <genre:ThematicWritingGenre rdf:about="http://sparql.cwrc.ca/ontologies/genre#business">
    <rdfs:label xml:lang="en">business</rdfs:label>
  </genre:ThematicWritingGenre>
  <genre:ScholarlyGenre rdf:about="http://sparql.cwrc.ca/ontologies/genre#maResearchPaper">
    <rdfs:label xml:lang="en">ma research paper</rdfs:label>
  </genre:ScholarlyGenre>
  <genre:ThematicWritingGenre rdf:about="http://sparql.cwrc.ca/ontologies/genre#millitary">
    <rdfs:label xml:lang="en">millitary</rdfs:label>
  </genre:ThematicWritingGenre>
  <genre:ReligiousGenre rdf:about="http://sparql.cwrc.ca/ontologies/genre#sundaySchoolStory">
    <rdfs:label xml:lang="en">sunday school story</rdfs:label>
  </genre:ReligiousGenre>
  <genre:StillImageMedium rdf:about="http://sparql.cwrc.ca/ontologies/genre#painting">
    <rdfs:label xml:lang="en">painting</rdfs:label>
    <skos:related rdf:resource="http://vocab.getty.edu/aat/300033618"/>
  </genre:StillImageMedium>
  <genre:MusicalGenre rdf:about="http://sparql.cwrc.ca/ontologies/genre#musicalWriting">
    <rdfs:label xml:lang="en">musical writing</rdfs:label>
    <skos:definition xml:lang="en">Writing associated with some form of music.</skos:definition>
  </genre:MusicalGenre>
  <genre:NarrativeGenre rdf:about="http://sparql.cwrc.ca/ontologies/genre#cautionaryTale">
    <rdfs:label xml:lang="en">cautionary tale</rdfs:label>
  </genre:NarrativeGenre>
  <genre:PoliticalWritingGenre rdf:about="http://sparql.cwrc.ca/ontologies/genre#propaganda">
    <rdfs:label xml:lang="fr">propagande</rdfs:label>
    <skos:definition xml:lang="fr">«La propagande est un concept désignant un ensemble de techniques de persuasion, mis en œuvre pour propager avec tous les moyens disponibles une idée, une opinion, une idéologie ou une doctrine et stimuler l'adoption de comportements prédéterminés au sein d'un public-cible. Ces techniques sont exercées sur une population afin de l'influencer, voire de l'endoctriner[réf. insuffisante]. La propagande se distingue de la publicité, laquelle vise la promotion de produits commerciaux. Néanmoins, la publicité utilise des techniques similaires à celles utilisées par la propagande . Nonobstant la similarité de certaines de leurs caractéristiques, les liens entre propagande et publicité sont largement discutés. La propagande est étudiée en milieu universitaire à partir du début du XXe siècle, principalement en histoire, mais aussi en psychologie (particulièrement en psychologie sociale) et en communication (notamment concernant les médias de masse).» <![CDATA[(<a href="#cwrc:727d97bc-af78-4122-94be-aa78b2e97d5a">DBpedia, 2017</a>)]]></skos:definition>
    <skos:definition xml:lang="en">"(Latin, "things that must be sent forth"): In its original use, the term referred to a committee of cardinals the Roman Catholic church founded in 1622 (the Congregatio de propaganda fide). This group established specific educational materials to be sent with priests-in-training for foreign missions . The term is today used to refer to information, rumors, ideas, and artwork spread deliberately to help or harm another specific group, movement, belief, institution, or government. The term's connotations are mostly negative. When literature or journalism is propaganda and when it is not is hotly debated. For instance, the Roman Emperor Augustus commissioned Virgil to write The Aeneid for specific goals. He wanted Virgil to glorify Rome's greatness, instill public pride in Rome's past, and cultivate traditional Roman virtues such as loyalty to the family, the Empire, and the gods. Is this propaganda? Or patriotism? Typically, readers claim a work is propaganda when it sets forth an argument with which they personally disagree. In other cases, readers will call a work propagandistic if they can perceive that the characters or the author advances particular doctrines or principles. Harry Shaw notes: "Propaganda is attacked by most critics and general readers because it is an attempt to influence opinions and actions deliberately, but by this definition all education and most literature are propagandistic" (220)." <![CDATA[(<a href="cwrc:509015ff-7641-473e-94c5-688e06952bb7">L. K Wheeler, 2017</a>)]]></skos:definition>
    <rdfs:label xml:lang="en">propaganda</rdfs:label>
    <owl:sameAs rdf:resource="http://dbpedia.org/resource/Propaganda"/>
    <rdfs:comment xml:lang="en">The description for this term is indebted to Dr. L. Kip Wheeler of Carson-Newman University. </rdfs:comment>
  </genre:PoliticalWritingGenre>
  <genre:ReferenceWorkGenre rdf:about="http://sparql.cwrc.ca/ontologies/genre#biographicalDictionary">
    <rdfs:label xml:lang="en">biographical dictionary</rdfs:label>
    <rdfs:label xml:lang="fr">dictionaire biographique</rdfs:label>
    <skos:definition xml:lang="en">A reference text containing biographical entries on multiple people, often with a common link between them (for example, a biographical dictionary of women), and typically arranged alphabetically.</skos:definition>
    <skos:definition xml:lang="fr">Texte de référence contenant des entrées biographiques à propos de plusieurs personnes, souvent reliées par un thème commun (par exemple, un dictionnaire biographique de femmes) et généralement classées par ordre alphabétique.</skos:definition>
  </genre:ReferenceWorkGenre>
  <genre:FictionalGenre rdf:about="http://sparql.cwrc.ca/ontologies/genre#ghostStory">
    <skos:definition xml:lang="fr">«Les histoires de fantôme sont un sous-genre du fantastique. Dans ces histoires, le fantôme est souvent le héros et a une personnalité et une identité bien à lui. Le genre peut aussi donner lieu à des récits centrés uniquement sur les fantômes ou les morts.» <![CDATA[(<a href="#cwrc:727d97bc-af78-4122-94be-aa78b2e97d5a">DBpedia, 2017</a>)]]></skos:definition>
    <rdfs:comment xml:lang="en">The description for this term is indebted to DBpedia. </rdfs:comment>
    <skos:definition xml:lang="en">"Prose tales of the supernatural in which the living encounter manifestations of the spirits of the dead." <![CDATA[(<a href="#cwrc:db2f8571-a773-4068-a35f-34262950bb8f">Getty, 2017</a>)]]></skos:definition>
    <rdfs:label xml:lang="en">ghost story</rdfs:label>
    <owl:sameAs rdf:resource="http://id.loc.gov/authorities/genreForms/gf2014026357"/>
    <owl:sameAs rdf:resource="http://dbpedia.org/resource/Ghost_story"/>
  </genre:FictionalGenre>
  <genre:IntertextualGenre rdf:about="http://sparql.cwrc.ca/ontologies/genre#reflection">
    <rdfs:label xml:lang="en">reflection</rdfs:label>
  </genre:IntertextualGenre>
  <genre:ScholarlyGenre rdf:about="http://sparql.cwrc.ca/ontologies/genre#maThesis">
    <rdfs:label xml:lang="en">ma thesis</rdfs:label>
  </genre:ScholarlyGenre>
  <genre:VisualArtMedium rdf:about="http://sparql.cwrc.ca/ontologies/genre#visualArt">
    <rdfs:label xml:lang="en">visual art</rdfs:label>
  </genre:VisualArtMedium>
  <genre:AlphabetForm rdf:about="http://sparql.cwrc.ca/ontologies/genre#alphabet">
    <rdfs:label xml:lang="en">alphabet</rdfs:label>
  </genre:AlphabetForm>
  <genre:CollectionForm rdf:about="http://sparql.cwrc.ca/ontologies/genre#collection">
    <rdfs:label xml:lang="en">collection</rdfs:label>
  </genre:CollectionForm>
  <genre:TextualMedium rdf:about="http://sparql.cwrc.ca/ontologies/genre#chapter">
    <rdfs:label xml:lang="en">chapter</rdfs:label>
  </genre:TextualMedium>
  <genre:DramaticGenre rdf:about="http://sparql.cwrc.ca/ontologies/genre#guerillaTheatre">
    <rdfs:label xml:lang="en">guerilla theatre</rdfs:label>
  </genre:DramaticGenre>
  <genre:CollectionForm rdf:about="http://sparql.cwrc.ca/ontologies/genre#commonplaceBook">
    <rdfs:label xml:lang="en">commonplace book</rdfs:label>
  </genre:CollectionForm>
  <genre:ScholarlyGenre rdf:about="http://sparql.cwrc.ca/ontologies/genre#scientificWriting">
    <skos:definition xml:lang="fr">Travaux écrits en lien avec la recherche scientifique, qui livrent généralement des comptes rendus de découvertes faites dans le cadre d'une étude scientifique spécifique.</skos:definition>
    <rdfs:label xml:lang="fr">écrits scientifiques</rdfs:label>
    <skos:definition xml:lang="en">Writing relating to scientific research, often reporting the findings of a particular scientific study.</skos:definition>
    <rdfs:label xml:lang="en">scientific writing</rdfs:label>
    <skos:altLabel xml:lang="en">science</skos:altLabel>
  </genre:ScholarlyGenre>
  <genre:SoundRecordingMedium rdf:about="http://sparql.cwrc.ca/ontologies/genre#soundRecordingMusical">
    <rdfs:label xml:lang="en">sound recording - musical</rdfs:label>
  </genre:SoundRecordingMedium>
  <genre:DramaticGenre rdf:about="http://sparql.cwrc.ca/ontologies/genre#revengeComedy">
    <rdfs:label xml:lang="en">revenge comedy</rdfs:label>
    <rdf:type rdf:resource="http://sparql.cwrc.ca/ontologies/genre#ComedicGenre"/>
  </genre:DramaticGenre>
  <genre:ReligiousGenre rdf:about="http://sparql.cwrc.ca/ontologies/genre#scripture">
    <rdfs:label xml:lang="en">scripture</rdfs:label>
  </genre:ReligiousGenre>
  <genre:RecordForm rdf:about="http://sparql.cwrc.ca/ontologies/genre#index">
    <rdfs:label xml:lang="en">index</rdfs:label>
  </genre:RecordForm>
  <genre:ScholarlyGenre rdf:about="http://sparql.cwrc.ca/ontologies/genre#criticism">
    <rdfs:label xml:lang="en">criticism</rdfs:label>
  </genre:ScholarlyGenre>
  <genre:InformationalGenre rdf:about="http://sparql.cwrc.ca/ontologies/genre#programNotes">
    <rdfs:label xml:lang="en">program notes</rdfs:label>
  </genre:InformationalGenre>
  <genre:InformationalGenre rdf:about="http://sparql.cwrc.ca/ontologies/genre#summary">
    <rdfs:label xml:lang="en">summary</rdfs:label>
  </genre:InformationalGenre>
  <genre:HistoricalGenre rdf:about="http://sparql.cwrc.ca/ontologies/genre#localHistory">
    <rdfs:label xml:lang="en">local history</rdfs:label>
  </genre:HistoricalGenre>
  <genre:DramaticGenre rdf:about="http://sparql.cwrc.ca/ontologies/genre#improvisation">
    <rdfs:label xml:lang="en">improvisation</rdfs:label>
  </genre:DramaticGenre>
  <genre:PerformanceMedium rdf:about="http://sparql.cwrc.ca/ontologies/genre#lecture">
    <rdfs:label xml:lang="en">lecture</rdfs:label>
    <owl:sameAs rdf:resource="http://id.loc.gov/authorities/genreForms/gf2014026122"/>
  </genre:PerformanceMedium>
  <genre:DramaticGenre rdf:about="http://sparql.cwrc.ca/ontologies/genre#collectiveCreation">
    <rdfs:label xml:lang="en">collective creation</rdfs:label>
  </genre:DramaticGenre>
  <genre:PoeticGenre rdf:about="http://sparql.cwrc.ca/ontologies/genre#anacreontic">
    <rdfs:label xml:lang="en">anacreontic</rdfs:label>
  </genre:PoeticGenre>
  <genre:InformationalGenre rdf:about="http://sparql.cwrc.ca/ontologies/genre#nonFiction">
    <rdfs:label xml:lang="en">non-fiction</rdfs:label>
  </genre:InformationalGenre>
  <genre:MovingMedium rdf:about="http://sparql.cwrc.ca/ontologies/genre#film">
    <rdfs:label xml:lang="en">film</rdfs:label>
  </genre:MovingMedium>
  <genre:ParatextualGenre rdf:about="http://sparql.cwrc.ca/ontologies/genre#appendix">
    <rdfs:label xml:lang="en">appendix</rdfs:label>
  </genre:ParatextualGenre>
  <genre:NarrativeGenre rdf:about="http://sparql.cwrc.ca/ontologies/genre#eyeWitness">
    <rdfs:label xml:lang="en">eye-witness</rdfs:label>
  </genre:NarrativeGenre>
  <genre:ThematicWritingGenre rdf:about="http://sparql.cwrc.ca/ontologies/genre#lgbtq">
    <rdfs:label xml:lang="en">lgbtq</rdfs:label>
    <rdf:type rdf:resource="http://sparql.cwrc.ca/ontologies/genre#LGBTQPlusGenre"/>
  </genre:ThematicWritingGenre>
  <genre:RecordForm rdf:about="http://sparql.cwrc.ca/ontologies/genre#bibliographicRecord">
    <rdfs:label xml:lang="en">bibliographic record</rdfs:label>
  </genre:RecordForm>
  <genre:PerformanceMedium rdf:about="http://sparql.cwrc.ca/ontologies/genre#physicalTheatre">
    <rdfs:label xml:lang="en">physical theatre</rdfs:label>
  </genre:PerformanceMedium>
  <genre:PerformanceMedium rdf:about="http://sparql.cwrc.ca/ontologies/genre#theatreForYoungAudiences">
    <rdfs:label xml:lang="en">theatre for young audiences</rdfs:label>
  </genre:PerformanceMedium>
  <genre:ScriptForm rdf:about="http://sparql.cwrc.ca/ontologies/genre#playScript">
    <rdfs:label xml:lang="en">play script</rdfs:label>
  </genre:ScriptForm>
  <genre:DigitalMedium rdf:about="http://sparql.cwrc.ca/ontologies/genre#digital">
    <rdfs:label xml:lang="en">digital</rdfs:label>
  </genre:DigitalMedium>
  <genre:ScholarlyGenre rdf:about="http://sparql.cwrc.ca/ontologies/genre#research">
    <rdfs:label xml:lang="en">research</rdfs:label>
  </genre:ScholarlyGenre>
  <genre:FictionalGenre rdf:about="http://sparql.cwrc.ca/ontologies/genre#animalStory">
    <rdfs:label xml:lang="en">animal story</rdfs:label>
  </genre:FictionalGenre>
  <owl:Class rdf:about="http://sparql.cwrc.ca/ontologies/genre#ThreeDimensionalMedium">
    <rdfs:subClassOf rdf:resource="http://sparql.cwrc.ca/ontologies/genre#Medium"/>
    <rdfs:label xml:lang="en">Three Dimensional Medium</rdfs:label>
    <dcterms:references rdf:resource="https://www.loc.gov/standards/mods/userguide/typeofresource.html"/>
    <skos:definition xml:lang="en">Indicates human-made objects such as "models, sculptures, clothing, and toys, as well as naturally occurring objects such as specimens mounted for viewing."</skos:definition>
    <skos:related rdf:resource="http://id.loc.gov/authorities/genreForms/gf2011026525"/>
  </owl:Class>
  <owl:Class rdf:about="http://sparql.cwrc.ca/ontologies/genre#PrintMedium">
    <rdfs:subClassOf rdf:resource="http://sparql.cwrc.ca/ontologies/genre#TextualMedium"/>
    <skos:definition xml:lang="en">Indicates media that involve the mechanical transfer of information to a physical object via a template or master form.<![CDATA[(<a href="#cwrc:727d97bc-af78-4122-94be-aa78b2e97d5a">DBpedia, 2019</a>)]]></skos:definition>
    <skos:closeMatch rdf:resource="http://dbpedia.org/resource/Printing"/>
    <rdfs:label xml:lang="en">Print Medium</rdfs:label>
  </owl:Class>
  <owl:Class rdf:about="http://sparql.cwrc.ca/ontologies/genre#PedagogicalGenre">
    <skos:definition xml:lang="en">Indicates works intended for educational purposes.</skos:definition>
    <rdfs:subClassOf rdf:resource="http://sparql.cwrc.ca/ontologies/genre#ScholarlyGenre"/>
    <rdfs:label xml:lang="en">Pedagogical Genre</rdfs:label>
  </owl:Class>
  <owl:Class rdf:about="http://sparql.cwrc.ca/ontologies/genre#IllustratedForm">
    <rdfs:label xml:lang="en">Illustrated Form</rdfs:label>
    <owl:sameAs rdf:resource="http://id.loc.gov/authorities/genreForms/gf2014026111"/>
    <rdfs:subClassOf rdf:resource="http://sparql.cwrc.ca/ontologies/genre#FormGenre"/>
    <skos:closeMatch rdf:resource="http://vocab.getty.edu/aat/300054200"/>
    <skos:definition xml:lang="en">Indicates works that include "drawings or other pictures intended to elucidate a description, story, or other written material, usually in a book or periodical."<![CDATA[(<a href="#cwrc:db2f8571-a773-4068-a35f-34262950bb8f">Getty, 2019</a>)]]></skos:definition>
  </owl:Class>
  <owl:Class rdf:about="http://sparql.cwrc.ca/ontologies/genre#DialogueOrDebateGenre">
    <rdfs:subClassOf rdf:resource="http://sparql.cwrc.ca/ontologies/genre#LiteraryGenre"/>
    <skos:closeMatch rdf:resource="http://dbpedia.org/resource/Dialogue"/>
    <skos:definition xml:lang="en">Indicates works depicting "a written or spoken conversational exchange between two or more people."<![CDATA[(<a href="#cwrc:727d97bc-af78-4122-94be-aa78b2e97d5a">DBpedia, 2019</a>)]]></skos:definition>
    <rdfs:label xml:lang="en">Dialogue Or Debate Genre</rdfs:label>
  </owl:Class>
  <owl:Class rdf:about="http://sparql.cwrc.ca/ontologies/genre#IntertextualGenre">
    <rdfs:label xml:lang="en">Intertextual Genre</rdfs:label>
    <rdfs:subClassOf rdf:resource="http://sparql.cwrc.ca/ontologies/genre#Genre"/>
    <skos:closeMatch rdf:resource="http://dbpedia.org/resource/Intertextuality"/>
    <skos:definition xml:lang="en">Indicates works that shape "a text's meaning by another text."<![CDATA[(<a href="#cwrc:727d97bc-af78-4122-94be-aa78b2e97d5a">DBpedia, 2019</a>)]]></skos:definition>
  </owl:Class>
  <owl:Class rdf:about="http://sparql.cwrc.ca/ontologies/genre#NarrativeGenre">
    <skos:closeMatch rdf:resource="http://vocab.getty.edu/aat/300185346"/>
    <rdfs:label xml:lang="en">Narrative Genre</rdfs:label>
    <rdfs:subClassOf rdf:resource="http://sparql.cwrc.ca/ontologies/genre#Genre"/>
    <skos:definition xml:lang="en">Indicates "works emphasizing a story or sequence of events." <![CDATA[(<a href="#cwrc:db2f8571-a773-4068-a35f-34262950bb8f">Getty, 2019</a>)]]></skos:definition>
  </owl:Class>
  <owl:Class rdf:about="http://sparql.cwrc.ca/ontologies/genre#FormGenre">
    <rdfs:label xml:lang="en">Form Genre</rdfs:label>
    <skos:definition xml:lang="en">Indicates material and structural elements that distinguish one category of cultural work from another. Whereas Genre categories tend to group categories based on features such as the style, content, or audience of cultural works, Form categories usually define material characteristics that shape or contain the work, such as ‘anthology,’ in the case of CollectionForm, ’notebook’ under BookForm, or ‘journal’ within SerialForm.</skos:definition>
  </owl:Class>
  <owl:Class rdf:about="http://sparql.cwrc.ca/ontologies/genre#ReferenceWorkGenre">
    <rdfs:subClassOf rdf:resource="http://sparql.cwrc.ca/ontologies/genre#InformationalGenre"/>
    <skos:closeMatch rdf:resource="http://vocab.getty.edu/aat/300163404"/>
    <skos:definition xml:lang="en">Indicates types of genres composed of "[s]ources intended primarily for consultation rather than for consecutive reading."<![CDATA[(<a href="#cwrc:db2f8571-a773-4068-a35f-34262950bb8f">Getty, 2019</a>)]]></skos:definition>
    <rdfs:label xml:lang="en">Reference Work Genre</rdfs:label>
  </owl:Class>
  <owl:Class rdf:about="http://sparql.cwrc.ca/ontologies/genre#MusicalNotationForm">
    <skos:closeMatch rdf:resource="http://dbpedia.org/resource/Musical_notation"/>
    <skos:definition xml:lang="en">Indicates "any system used to visually represent aurally perceived music played with instruments or sung by the human voice through the use of written, printed, or otherwise-produced symbols."<![CDATA[(<a href="#cwrc:727d97bc-af78-4122-94be-aa78b2e97d5a">DBpedia, 2019</a>)]]></skos:definition>
    <rdfs:subClassOf rdf:resource="http://sparql.cwrc.ca/ontologies/genre#FormGenre"/>
    <owl:sameAs rdf:resource="http://vocab.getty.edu/aat/300026430"/>
    <rdfs:label xml:lang="en">Musical Notation Form</rdfs:label>
    <skos:altLabel xml:lang="en">sheet music</skos:altLabel>
  </owl:Class>
  <owl:Class rdf:about="http://sparql.cwrc.ca/ontologies/genre#AdvertisementForm">
    <rdfs:subClassOf rdf:resource="http://sparql.cwrc.ca/ontologies/genre#FormGenre"/>
    <skos:altLabel xml:lang="en">advertising copy</skos:altLabel>
    <skos:definition xml:lang="en">Indicates "an audio or visual form of marketing communication that employs an openly sponsored, nonpersonal message to promote or sell a product, service or idea."<![CDATA[(<a href="#cwrc:727d97bc-af78-4122-94be-aa78b2e97d5a">DBpedia, 2019</a>)]]></skos:definition>
    <skos:closeMatch rdf:resource="http://dbpedia.org/resource/Advertising"/>
    <rdfs:label xml:lang="en">Advertisement Form</rdfs:label>
  </owl:Class>
  <owl:Class rdf:about="http://sparql.cwrc.ca/ontologies/genre#RecordForm">
    <skos:closeMatch rdf:resource="http://vocab.getty.edu/aat/300026685"/>
    <rdfs:label xml:lang="en">Record Form</rdfs:label>
    <owl:sameAs rdf:resource="http://id.loc.gov/authorities/genreForms/gf2014026163"/>
    <skos:definition xml:lang="en">Indicates "recorded information, often standardized in format and content and treated as a unit."<![CDATA[(<a href="#cwrc:db2f8571-a773-4068-a35f-34262950bb8f">Getty, 2019</a>)]]></skos:definition>
    <rdfs:subClassOf rdf:resource="http://sparql.cwrc.ca/ontologies/genre#FormGenre"/>
  </owl:Class>
  <owl:Class rdf:about="http://sparql.cwrc.ca/ontologies/genre#SoundRecordingMedium">
    <rdfs:label xml:lang="en">Sound Recording Medium</rdfs:label>
    <owl:sameAs rdf:resource="http://id.loc.gov/authorities/genreForms/gf2011026594"/>
    <rdfs:subClassOf rdf:resource="http://sparql.cwrc.ca/ontologies/genre#AuditoryMedium"/>
  </owl:Class>
  <owl:Class rdf:about="http://sparql.cwrc.ca/ontologies/genre#SerialForm">
    <skos:altLabel xml:lang="en">periodical</skos:altLabel>
    <owl:sameAs rdf:resource="http://vocab.getty.edu/aat/300215389"/>
    <rdfs:label xml:lang="en">Serial Form</rdfs:label>
    <rdfs:subClassOf rdf:resource="http://sparql.cwrc.ca/ontologies/genre#FormGenre"/>
    <skos:definition xml:lang="en">Indicates "publications in any medium issued in successive parts bearing numerical or chronological designations and intended to be continued indefinitely."<![CDATA[(<a href="#cwrc:db2f8571-a773-4068-a35f-34262950bb8f">Getty, 2019</a>)]]></skos:definition>
    <skos:closeMatch rdf:resource="http://vocab.getty.edu/aat/300026642"/>
  </owl:Class>
  <owl:Class rdf:about="http://sparql.cwrc.ca/ontologies/genre#PerformanceMedium">
    <rdfs:subClassOf rdf:resource="http://sparql.cwrc.ca/ontologies/genre#Medium"/>
    <rdfs:label xml:lang="en">Performance Medium</rdfs:label>
    <skos:definition xml:lang="en">Indicates time-based, embodied media that are often produced as entertainment.</skos:definition>
  </owl:Class>
  <owl:Class rdf:about="http://sparql.cwrc.ca/ontologies/genre#ComedicGenre">
    <rdfs:label xml:lang="en">Comedic Genre</rdfs:label>
    <skos:closeMatch rdf:resource="http://vocab.getty.edu/aat/300417801"/>
    <rdfs:subClassOf rdf:resource="http://sparql.cwrc.ca/ontologies/genre#DramaticGenre"/>
    <skos:definition xml:lang="en">Indicates dramatic works designed "chiefly to amuse the audience."<![CDATA[(<a href="#cwrc:db2f8571-a773-4068-a35f-34262950bb8f">Getty, 2019</a>)]]></skos:definition>
  </owl:Class>
  <owl:Class rdf:about="http://sparql.cwrc.ca/ontologies/genre#EpistolaryGenre">
    <skos:definition xml:lang="en">Indicates works "written by using the device of a series of letters, diary entries, newspaper clippings, or other documents."<![CDATA[(<a href="#cwrc:db2f8571-a773-4068-a35f-34262950bb8f">Getty, 2019</a>)]]></skos:definition>
    <rdfs:subClassOf rdf:resource="http://sparql.cwrc.ca/ontologies/genre#LiteraryGenre"/>
    <skos:closeMatch rdf:resource="http://vocab.getty.edu/aat/300410324"/>
    <rdfs:label xml:lang="en">Epistolary Genre</rdfs:label>
  </owl:Class>
  <owl:Class rdf:about="http://sparql.cwrc.ca/ontologies/genre#ProverbForm">
    <rdfs:label xml:lang="en">Proverb Form</rdfs:label>
    <skos:closeMatch rdf:resource="http://vocab.getty.edu/aat/300188783"/>
    <skos:altLabel xml:lang="en">aphorism</skos:altLabel>
    <owl:sameAs rdf:resource="http://id.loc.gov/authorities/genreForms/gf2014026170"/>
    <skos:definition xml:lang="en">Indicates "short, concise sayings repeated colloquially expressing a general truth or observation about human life or behavior, often embodying the folk wisdom of a group or nation. Distinguished from "aphorisms" which are statements of principle or precepts, often of known authorship."<![CDATA[(<a href="#cwrc:db2f8571-a773-4068-a35f-34262950bb8f">Getty, 2019</a>)]]></skos:definition>
    <skos:altLabel xml:lang="en">sayings</skos:altLabel>
    <rdfs:subClassOf rdf:resource="http://sparql.cwrc.ca/ontologies/genre#FormGenre"/>
  </owl:Class>
  <owl:Class rdf:about="http://sparql.cwrc.ca/ontologies/genre#MovingMedium">
    <skos:definition xml:lang="en">Indicates time-based media that are primarily visual, sometimes accompanied by sound. "Does not include moving images that are primarily computer programs, such as computer games or computer-oriented multimedia."</skos:definition>
    <rdfs:label xml:lang="en">Moving Medium</rdfs:label>
    <rdfs:subClassOf rdf:resource="http://sparql.cwrc.ca/ontologies/genre#VisualMedium"/>
    <skos:related rdf:resource="http://vocab.getty.edu/aat/300263857"/>
    <dcterms:references rdf:resource="https://www.loc.gov/standards/mods/v3/mods-userguide-elements.html"/>
  </owl:Class>
  <owl:Class rdf:about="http://sparql.cwrc.ca/ontologies/genre#ThematicWritingGenre">
    <rdfs:label xml:lang="en">Thematic Writing Genre</rdfs:label>
    <rdfs:subClassOf rdf:resource="http://sparql.cwrc.ca/ontologies/genre#LiteraryGenre"/>
    <skos:definition xml:lang="en">Indicates works that are shaped by a defining theme or topic, such as ‘feminist,’ ‘gothic,’ 'gardening,' and ‘military,’ for instance. </skos:definition>
  </owl:Class>
  <owl:Class rdf:about="http://sparql.cwrc.ca/ontologies/genre#CartographicForm">
    <skos:related rdf:resource="http://id.loc.gov/authorities/genreForms/gf2011026113"/>
    <rdfs:label xml:lang="en">Cartographic Form</rdfs:label>
    <skos:closeMatch rdf:resource="http://vocab.getty.edu/aat/300028052)"/>
    <rdfs:subClassOf rdf:resource="http://sparql.cwrc.ca/ontologies/genre#FormGenre"/>
    <skos:altLabel xml:lang="en">cartographic</skos:altLabel>
    <skos:definition xml:lang="en">Indicates "any materials representing, in whole or part, the earth or any celestial body at any scale."<![CDATA[(<a href="#cwrc:db2f8571-a773-4068-a35f-34262950bb8f">Getty, 2019</a>)]]></skos:definition>
  </owl:Class>
  <owl:Class rdf:about="http://sparql.cwrc.ca/ontologies/genre#RomanceGenre">
    <rdfs:subClassOf rdf:resource="http://sparql.cwrc.ca/ontologies/genre#LiteraryGenre"/>
    <rdfs:label xml:lang="en">Romance Genre</rdfs:label>
    <skos:definition xml:lang="en">Indicates a "mass-market literary genre in which love is the central theme; often written by and for women and featuring plots that focus on finding and sustaining romantic relationships with an ideal partner."</skos:definition>
    <skos:closeMatch rdf:resource="http://vocab.getty.edu/aat/300255278"/>
  </owl:Class>
  <owl:Class rdf:about="http://sparql.cwrc.ca/ontologies/genre#DidacticGenre">
    <rdfs:subClassOf rdf:resource="http://sparql.cwrc.ca/ontologies/genre#ThematicWritingGenre"/>
    <skos:closeMatch rdf:resource="http://vocab.getty.edu/aat/300404113"/>
    <skos:definition xml:lang="en">Indicates works that have “the function, quality, or activity of having instruction or teaching as a primary or ulterior purpose.”</skos:definition>
    <rdfs:label xml:lang="en">Didactic Genre</rdfs:label>
  </owl:Class>
  <owl:Class rdf:about="http://sparql.cwrc.ca/ontologies/genre#PoeticGenre">
    <skos:definition xml:lang="en">Indicates works "rooted in the compressed and cogent imaginative awareness or associations of experiences, ideas, or emotional responses and arranged under an organized criterion of meaning, conscious and unconscious expression, symbolism, formal or informal pattern, sound, and rhythm."<![CDATA[(<a href="#cwrc:db2f8571-a773-4068-a35f-34262950bb8f">Getty, 2019</a>)]]></skos:definition>
    <rdfs:label xml:lang="en">Poetic Genre</rdfs:label>
    <skos:closeMatch rdf:resource="http://vocab.getty.edu/aat/300055931"/>
    <rdfs:subClassOf rdf:resource="http://sparql.cwrc.ca/ontologies/genre#LiteraryGenre"/>
  </owl:Class>
  <owl:Class rdf:about="http://sparql.cwrc.ca/ontologies/genre#NovelisticGenre">
    <skos:definition xml:lang="en">Indicates "invented prose narratives of considerable length and a certain complexity that deal imaginatively with human experience through a connected sequence of events involving a group of persons in a specific setting."<![CDATA[(<a href="#cwrc:db2f8571-a773-4068-a35f-34262950bb8f">Getty, 2019</a>)]]></skos:definition>
    <rdfs:label xml:lang="en">Novelistic Genre</rdfs:label>
    <rdfs:subClassOf rdf:resource="http://sparql.cwrc.ca/ontologies/genre#FictionalGenre"/>
    <skos:closeMatch rdf:resource="http://vocab.getty.edu/aat/300202580"/>
  </owl:Class>
  <owl:Class rdf:about="http://sparql.cwrc.ca/ontologies/genre#StillImageMedium">
    <rdfs:label xml:lang="en">Still Image Medium</rdfs:label>
    <skos:definition xml:lang="en">Indicates media that are "two-dimensional nonprojectible graphic[s]." Includes slides and transparencies.</skos:definition>
    <rdfs:subClassOf rdf:resource="http://sparql.cwrc.ca/ontologies/genre#VisualMedium"/>
    <dcterms:references rdf:resource="https://www.loc.gov/standards/mods/v3/mods-userguide-elements.html"/>
  </owl:Class>
  <owl:Class rdf:about="http://sparql.cwrc.ca/ontologies/genre#ReligiousGenre">
    <skos:definition xml:lang="en">Indicates works "having a religious subject or spirtual theme."<![CDATA[(<a href="#cwrc:db2f8571-a773-4068-a35f-34262950bb8f">Getty, 2019</a>)]]></skos:definition>
    <rdfs:label xml:lang="en">Religious Genre</rdfs:label>
    <skos:closeMatch rdf:resource="http://vocab.getty.edu/aat/300417817"/>
    <rdfs:subClassOf rdf:resource="http://sparql.cwrc.ca/ontologies/genre#LiteraryGenre"/>
  </owl:Class>
  <owl:Class rdf:about="http://sparql.cwrc.ca/ontologies/genre#FictionalGenre">
    <rdfs:subClassOf rdf:resource="http://sparql.cwrc.ca/ontologies/genre#LiteraryGenre"/>
    <rdfs:label xml:lang="en">Fictional Genre</rdfs:label>
    <rdfs:subClassOf rdf:resource="http://sparql.cwrc.ca/ontologies/genre#NarrativeGenre"/>
    <skos:definition xml:lang="en">Indicates "works evoked from the imagination of the creator and not conferred as fact."<![CDATA[(<a href="#cwrc:db2f8571-a773-4068-a35f-34262950bb8f">Getty, 2019</a>)]]></skos:definition>
    <skos:closeMatch rdf:resource="http://vocab.getty.edu/aat/300055918"/>
  </owl:Class>
  <owl:Class rdf:about="http://sparql.cwrc.ca/ontologies/genre#VisualArtMedium">
    <rdfs:subClassOf rdf:resource="http://sparql.cwrc.ca/ontologies/genre#VisualMedium"/>
    <owl:sameAs rdf:resource="http://vocab.getty.edu/aat/300054154"/>
    <skos:definition xml:lang="en">Indicates media "that are meant to be perceived primarily through the sense of sight, were created by the use of skill and imagination, and possess an aesthetic that is valued and of a quality and type that would be collected by art museums or private collectors."<![CDATA[(<a href="#cwrc:db2f8571-a773-4068-a35f-34262950bb8f">Getty, 2019</a>)]]></skos:definition>
    <rdfs:label xml:lang="en">Visual Art Medium</rdfs:label>
  </owl:Class>
  <owl:Class rdf:about="http://sparql.cwrc.ca/ontologies/genre#MusicalGenre">
    <rdfs:subClassOf rdf:resource="http://sparql.cwrc.ca/ontologies/genre#LiteraryGenre"/>
    <rdfs:label xml:lang="en">Musical Genre</rdfs:label>
    <skos:definition xml:lang="en">Indicates works related to the performance or discussion of musical pieces. </skos:definition>
  </owl:Class>
  <owl:Class rdf:about="http://sparql.cwrc.ca/ontologies/genre#LiteraryGenre">
    <skos:definition xml:lang="en">Indicates works that "may be determined by literary technique, tone, content, or even (as in the case of fiction) length" and are "defined by the general cultural movement of the historical period in which they were composed." <![CDATA[(<a href="#cwrc:727d97bc-af78-4122-94be-aa78b2e97d5a">DBpedia, 2019</a>)]]></skos:definition>
    <rdfs:subClassOf rdf:resource="http://sparql.cwrc.ca/ontologies/genre#Genre"/>
    <skos:closeMatch rdf:resource="http://dbpedia.org/resource/Literary_genre"/>
    <rdfs:label xml:lang="en">Literary Genre</rdfs:label>
  </owl:Class>
  <owl:Class rdf:about="http://sparql.cwrc.ca/ontologies/genre#Medium">
    <skos:definition xml:lang="en">Indicates the material used to produce a cultural work and/or the governing substance that defines a particular object, digital or otherwise. </skos:definition>
    <rdfs:label xml:lang="en">Medium</rdfs:label>
  </owl:Class>
  <owl:Class rdf:about="http://sparql.cwrc.ca/ontologies/genre#BookForm">
    <skos:closeMatch rdf:resource="http://vocab.getty.edu/aat/300028051"/>
    <skos:definition xml:lang="en">Indicates "items comprising a collection of leaves of paper, parchment, wood, stiffened textile, ivory, metal tablets, or other flat material, that are blank, written on, or printed, and are strung or bound together in a volume."<![CDATA[(<a href="#cwrc:db2f8571-a773-4068-a35f-34262950bb8f">Getty, 2019</a>)]]></skos:definition>
    <rdfs:label xml:lang="en">Book Form</rdfs:label>
    <rdfs:subClassOf rdf:resource="http://sparql.cwrc.ca/ontologies/genre#FormGenre"/>
  </owl:Class>
  <owl:Class rdf:about="http://sparql.cwrc.ca/ontologies/genre#AuditoryMedium">
    <rdfs:label xml:lang="en">Auditory Medium</rdfs:label>
    <rdfs:subClassOf rdf:resource="http://sparql.cwrc.ca/ontologies/genre#Medium"/>
    <skos:definition xml:lang="en">Indicates media that are primarily auditory.</skos:definition>
  </owl:Class>
  <owl:Class rdf:about="http://sparql.cwrc.ca/ontologies/genre#Genre">
    <rdfs:label xml:lang="en">Genre</rdfs:label>
    <skos:definition xml:lang="en">Genres are used to classify cultural works , broadly conceived, within an evolving spectrum of categories on the basis of a particular form, content, style, or purpose (OED). Though there is debate over whether genre inheres in works themselves or emerges from contexts of reception, shifts in historical definitions indicate that genres have a strong social component (Dubrow, 1982; Miller 1984).&#13;
&#13;
Literary genres are used to classify texts within a shifting range of literary forms and practices. Genres are most frequently related to formal features such as the English sonnet's fourteen lines of iambic pentameter, to characteristic subject matter such as themes of romance, horror, comedy, or tragedy, to aspects of style such as hard-boiled detective fiction, or to the purpose of a text. Within the context of literary studies, the question of "purpose," especially when considered within a political context, is of especial interest to scholars. For example, feminist literary scholars like Cynthia Huff ("‘That Profoundly Female, and Feminist Genre’: The Diary as Feminist Practice"), Giancarlo Lombardi (Rooms with a View: Feminist Diary Fiction, 1952-1999), Rita Felski (Beyond Feminist Aesthetics: Feminist Literature and Social Change) and others read "diary fiction" as a powerful genre used to spur on women’s movements. For more on literary genre, see the introduction to this ontology (http://sparql.cwrc.ca/ontologies/genre-preamble-EN.html#background).</skos:definition>
  </owl:Class>
  <owl:Class rdf:about="http://sparql.cwrc.ca/ontologies/genre#TextualMedium">
    <rdfs:subClassOf rdf:resource="http://sparql.cwrc.ca/ontologies/genre#Medium"/>
    <owl:sameAs rdf:resource="http://vocab.getty.edu/aat/300263751"/>
    <rdfs:label xml:lang="en">Textual Medium</rdfs:label>
    <skos:definition xml:lang="en">"Written or printed words, phrases, or sentences arranged to make a communication. Includes oral verbal communications set down in writing or print."<![CDATA[(<a href="#cwrc:db2f8571-a773-4068-a35f-34262950bb8f">Getty, 2019</a>)]]></skos:definition>
  </owl:Class>
  <owl:Class rdf:about="http://sparql.cwrc.ca/ontologies/genre#JournalisticGenre">
    <skos:closeMatch rdf:resource="http://vocab.getty.edu/aat/300054354"/>
    <rdfs:label xml:lang="en">Journalistic Genre</rdfs:label>
    <skos:definition xml:lang="en">Indicates works "concerned with the collection, preparation, and distribution of news and related commentary through the mass media, both print and electronic."&#13;
 <![CDATA[(<a href="#cwrc:db2f8571-a773-4068-a35f-34262950bb8f">Getty, 2019</a>)]]></skos:definition>
    <rdfs:subClassOf rdf:resource="http://sparql.cwrc.ca/ontologies/genre#LiteraryGenre"/>
  </owl:Class>
  <owl:Class rdf:about="http://sparql.cwrc.ca/ontologies/genre#DigitalMedium">
    <rdfs:label xml:lang="en">Digital Medium</rdfs:label>
    <skos:related rdf:resource="http://vocab.getty.edu/aat/300404196"/>
    <skos:definition xml:lang="en">Indicates "media that are encoded in machine-readable formats. Digital media can be created, viewed, distributed, modified and preserved on digital electronics devices."<![CDATA[(<a href="#cwrc:727d97bc-af78-4122-94be-aa78b2e97d5a">DBpedia, 2019</a>)]]></skos:definition>
    <rdfs:subClassOf rdf:resource="http://sparql.cwrc.ca/ontologies/genre#Medium"/>
    <skos:closeMatch rdf:resource="http://dbpedia.org/resource/Digital_media"/>
  </owl:Class>
  <owl:Class rdf:about="http://sparql.cwrc.ca/ontologies/genre#FeministGenre">
    <skos:closeMatch rdf:resource="http://dbpedia.org/resource/Feminism"/>
    <skos:definition xml:lang="en">Indicates works engaging with "a range of political movements, ideologies, and social movements that share a common goal: to define, establish, and achieve political, economic, personal, and social rights" and equality for all genders.<![CDATA[(<a href="#cwrc:727d97bc-af78-4122-94be-aa78b2e97d5a">DBpedia, 2019</a>)]]></skos:definition>
    <rdfs:subClassOf rdf:resource="http://sparql.cwrc.ca/ontologies/genre#PoliticalWritingGenre"/>
    <rdfs:label xml:lang="en">Feminist Genre</rdfs:label>
  </owl:Class>
  <owl:Class rdf:about="http://sparql.cwrc.ca/ontologies/genre#SatiricalGenre">
    <rdfs:subClassOf rdf:resource="http://sparql.cwrc.ca/ontologies/genre#LiteraryGenre"/>
    <skos:closeMatch rdf:resource="http://dbpedia.org/resource/Satire"/>
    <rdfs:label xml:lang="en">Satirical Genre</rdfs:label>
    <skos:definition xml:lang="en">Indicates works "in which vices, follies, abuses, and shortcomings are held up to ridicule, ideally with the intent of shaming individuals, corporations, government, or society itself into improvement. Although satire is usually meant to be humorous, its greater purpose is often constructive social criticism, using wit to draw attention to both particular and wider issues in society."<![CDATA[(<a href="#cwrc:727d97bc-af78-4122-94be-aa78b2e97d5a">DBpedia, 2019</a>)]]></skos:definition>
  </owl:Class>
  <owl:Class rdf:about="http://sparql.cwrc.ca/ontologies/genre#ChildrensLiteratureGenre">
    <skos:definition xml:lang="en">Indicates works  produced for children and young adults, whether fictional or informational.<![CDATA[(<a href="#cwrc:db2f8571-a773-4068-a35f-34262950bb8f">Getty, 2019</a>)]]></skos:definition>
    <rdfs:label xml:lang="en">Childrens Literature Genre</rdfs:label>
    <rdfs:subClassOf rdf:resource="http://sparql.cwrc.ca/ontologies/genre#LiteraryGenre"/>
    <skos:closeMatch rdf:resource="http://vocab.getty.edu/aat/300263209"/>
  </owl:Class>
  <owl:Class rdf:about="http://sparql.cwrc.ca/ontologies/genre#ParatextualGenre">
    <skos:closeMatch rdf:resource="http://id.loc.gov/authorities/subjects/sh2006003881"/>
    <rdfs:label xml:lang="en">Paratextual Genre</rdfs:label>
    <skos:definition xml:lang="en">Indicates "the textual elements associated with a book that are apart from the text of the work itself."</skos:definition>
    <rdfs:subClassOf rdf:resource="http://sparql.cwrc.ca/ontologies/genre#LiteraryGenre"/>
  </owl:Class>
  <owl:Class rdf:about="http://sparql.cwrc.ca/ontologies/genre#CalendarForm">
    <rdfs:subClassOf rdf:resource="http://sparql.cwrc.ca/ontologies/genre#FormGenre"/>
    <owl:sameAs rdf:resource="http://vocab.getty.edu/aat/300026741"/>
    <rdfs:label xml:lang="en">Calendar Form</rdfs:label>
    <skos:definition xml:lang="en">Indicates "registers of days or other contrivances for reckoning days, months, years, etc., such as a table showing the division of a given year into its months, weeks, days, years, or other divisions of time."<![CDATA[(<a href="#cwrc:db2f8571-a773-4068-a35f-34262950bb8f">Getty, 2019</a>)]]></skos:definition>
  </owl:Class>
  <owl:Class rdf:about="http://sparql.cwrc.ca/ontologies/genre#OperaGenre">
    <skos:closeMatch rdf:resource="http://vocab.getty.edu/aat/300054147"/>
    <skos:definition xml:lang="en">Indicates performance works "combining theater and music, in which some or all of the roles are sung."&#13;
 <![CDATA[(<a href="#cwrc:db2f8571-a773-4068-a35f-34262950bb8f">Getty, 2019</a>)]]></skos:definition>
    <rdfs:subClassOf rdf:resource="http://sparql.cwrc.ca/ontologies/genre#MusicalGenre"/>
    <rdfs:label xml:lang="en">Opera Genre</rdfs:label>
  </owl:Class>
  <owl:Class rdf:about="http://sparql.cwrc.ca/ontologies/genre#PartialForm">
    <rdfs:subClassOf rdf:resource="http://sparql.cwrc.ca/ontologies/genre#FormGenre"/>
    <skos:closeMatch rdf:resource="http://vocab.getty.edu/aat/300055027"/>
    <owl:sameAs rdf:resource="http://id.loc.gov/authorities/genreForms/gf2014026097"/>
    <rdfs:label xml:lang="en">Partial Form</rdfs:label>
    <skos:definition xml:lang="en">Indicates "portions of documents or other written works, either included as discrete sections in an extant document or detached from the original document."<![CDATA[(<a href="#cwrc:db2f8571-a773-4068-a35f-34262950bb8f">Getty, 2019</a>)]]></skos:definition>
  </owl:Class>
  <owl:Class rdf:about="http://sparql.cwrc.ca/ontologies/genre#AlphabetForm">
    <skos:definition xml:lang="en">Indicates "a standard set of letters (basic written symbols or graphemes) that is used to write one or more languages based on the general principle that the letters represent phonemes (basic significant sounds) of the spoken language."<![CDATA[(<a href="#cwrc:727d97bc-af78-4122-94be-aa78b2e97d5a">DBpedia, 2019</a>)]]></skos:definition>
    <skos:closeMatch rdf:resource="http://dbpedia.org/resource/Alphabet"/>
    <rdfs:subClassOf rdf:resource="http://sparql.cwrc.ca/ontologies/genre#FormGenre"/>
    <rdfs:label xml:lang="en">Alphabet Form</rdfs:label>
  </owl:Class>
  <owl:Class rdf:about="http://sparql.cwrc.ca/ontologies/genre#AutobiographicalGenre">
    <skos:closeMatch rdf:resource="http://vocab.getty.edu/aat/300026049"/>
    <rdfs:subClassOf rdf:resource="http://sparql.cwrc.ca/ontologies/genre#LifeWritingGenre"/>
    <skos:definition xml:lang="en">Indicates "accounts of a person's life given by themselves."<![CDATA[(<a href="#cwrc:db2f8571-a773-4068-a35f-34262950bb8f">Getty, 2019</a>)]]></skos:definition>
    <rdfs:label xml:lang="en">Autobiographical Genre</rdfs:label>
  </owl:Class>
  <owl:Class rdf:about="http://sparql.cwrc.ca/ontologies/genre#PoliticalWritingGenre">
    <rdfs:label xml:lang="en">Political Writing Genre</rdfs:label>
    <skos:closeMatch rdf:resource="http://dbpedia.org/resource/Politics"/>
    <skos:definition xml:lang="en">Indicates works concerned with "the distribution of power and resources within a given community (a usually hierarchically organized population) as well as the interrelationship(s) between communities."<![CDATA[(<a href="#cwrc:727d97bc-af78-4122-94be-aa78b2e97d5a">DBpedia, 2019</a>)]]></skos:definition>
    <rdfs:subClassOf rdf:resource="http://sparql.cwrc.ca/ontologies/genre#LiteraryGenre"/>
  </owl:Class>
  <owl:Class rdf:about="http://sparql.cwrc.ca/ontologies/genre#CollectionForm">
    <owl:sameAs rdf:resource="http://vocab.getty.edu/aat/300025976"/>
    <rdfs:subClassOf rdf:resource="http://sparql.cwrc.ca/ontologies/genre#FormGenre"/>
    <skos:definition xml:lang="en">Indicates "accumulated groups of objects or materials having a focal characteristic and that have been brought together by an individual or organization."<![CDATA[(<a href="#cwrc:db2f8571-a773-4068-a35f-34262950bb8f">Getty, 2019</a>)]]></skos:definition>
    <rdfs:label xml:lang="en">Collection Form</rdfs:label>
  </owl:Class>
  <owl:Class rdf:about="http://sparql.cwrc.ca/ontologies/genre#PhilosophicalGenre">
    <rdfs:label xml:lang="en">Philosophical Genre</rdfs:label>
    <rdfs:subClassOf rdf:resource="http://sparql.cwrc.ca/ontologies/genre#ScholarlyGenre"/>
    <skos:closeMatch rdf:resource="http://vocab.getty.edu/aat/300054279"/>
    <skos:definition xml:lang="en">Indicates works dealing with "critical examination of the grounds for fundamental beliefs and analysis of the basic concepts, doctrines, or practices that express such beliefs."&#13;
 <![CDATA[(<a href="#cwrc:db2f8571-a773-4068-a35f-34262950bb8f">Getty, 2019</a>)]]></skos:definition>
  </owl:Class>
  <owl:Class rdf:about="http://sparql.cwrc.ca/ontologies/genre#SocialScienceGenre">
    <skos:definition xml:lang="en">Indicates works "dealing with the institutions and functioning of human society and with the interpersonal relationships of individuals as members of society."<![CDATA[(<a href="#cwrc:db2f8571-a773-4068-a35f-34262950bb8f">Getty, 2019</a>)]]></skos:definition>
    <skos:closeMatch rdf:resource="http://vocab.getty.edu/aat/300054314"/>
    <rdfs:subClassOf rdf:resource="http://sparql.cwrc.ca/ontologies/genre#ScholarlyGenre"/>
    <rdfs:label xml:lang="en">Social Science Genre</rdfs:label>
  </owl:Class>
  <owl:Class rdf:about="http://sparql.cwrc.ca/ontologies/genre#InformationalGenre">
    <skos:definition xml:lang="en">Indicates genres, often considered nonfictional, designed to convey specific content on a wide range of topics, although that content is not necessarily factual.<![CDATA[(<a href="#cwrc:db2f8571-a773-4068-a35f-34262950bb8f">Getty, 2019</a>)]]></skos:definition>
    <skos:altLabel xml:lang="en">non-fiction</skos:altLabel>
    <skos:altLabel xml:lang="en">essais</skos:altLabel>
    <rdfs:subClassOf rdf:resource="http://sparql.cwrc.ca/ontologies/genre#Genre"/>
    <rdfs:label xml:lang="en">Informational Genre</rdfs:label>
    <skos:closeMatch rdf:resource="http://vocab.getty.edu/aat/300311832"/>
  </owl:Class>
  <owl:Class rdf:about="http://sparql.cwrc.ca/ontologies/genre#SongGenre">
    <rdfs:subClassOf rdf:resource="http://sparql.cwrc.ca/ontologies/genre#MusicalGenre"/>
    <skos:closeMatch rdf:resource="http://dbpedia.org/resource/Song"/>
    <skos:definition xml:lang="en">Indicates a "work of music that is typically intended to be sung by the human voice with distinct and fixed pitches and patterns using sound and silence and a variety of forms that often include the repetition of sections."<![CDATA[(<a href="#cwrc:727d97bc-af78-4122-94be-aa78b2e97d5a">DBpedia, 2019</a>)]]></skos:definition>
    <rdfs:label xml:lang="en">Song Genre</rdfs:label>
  </owl:Class>
  <owl:Class rdf:about="http://sparql.cwrc.ca/ontologies/genre#MysteryGenre">
    <rdfs:label xml:lang="en">Mystery Genre</rdfs:label>
    <skos:closeMatch rdf:resource="http://dbpedia.org/resource/Mystery_fiction"/>
    <rdfs:subClassOf rdf:resource="http://sparql.cwrc.ca/ontologies/genre#LiteraryGenre"/>
    <skos:definition xml:lang="en">Indicates works, either fictional or nonfictional, that emphasize suspense and the inclusion of puzzles that may or may not be solved.  <![CDATA[(<a href="#cwrc:727d97bc-af78-4122-94be-aa78b2e97d5a">DBpedia, 2019</a>)]]></skos:definition>
  </owl:Class>
  <owl:Class rdf:about="http://sparql.cwrc.ca/ontologies/genre#CatalogueForm">
    <rdfs:subClassOf rdf:resource="http://sparql.cwrc.ca/ontologies/genre#FormGenre"/>
    <skos:closeMatch rdf:resource="http://vocab.getty.edu/aat/300026059"/>
    <rdfs:label xml:lang="en">Catalogue Form</rdfs:label>
    <skos:definition xml:lang="en">Indicates "enumerations of items, such as a file of bibliographic records or a list of art objects, usually arranged systematically and with descriptive details; may be in book or pamphlet form, on cards, or online."<![CDATA[(<a href="#cwrc:db2f8571-a773-4068-a35f-34262950bb8f">Getty, 2019</a>)]]></skos:definition>
    <owl:sameAs rdf:resource="http://id.loc.gov/authorities/genreForms/gf2014026057"/>
  </owl:Class>
  <owl:Class rdf:about="http://sparql.cwrc.ca/ontologies/genre#ScholarlyGenre">
    <skos:altLabel xml:lang="en">scholarship</skos:altLabel>
    <skos:definition xml:lang="en">Indicates works produced as a result of serious, detailed study of previous knowledge, often within although not necessarily limited to an academic context. </skos:definition>
    <rdfs:label xml:lang="en">Scholarly Genre</rdfs:label>
    <rdfs:subClassOf rdf:resource="http://sparql.cwrc.ca/ontologies/genre#InformationalGenre"/>
  </owl:Class>
  <owl:Class rdf:about="http://sparql.cwrc.ca/ontologies/genre#LifeWritingGenre">
    <rdfs:label xml:lang="en">Life Writing Genre</rdfs:label>
    <skos:closeMatch rdf:resource="http://dbpedia.org/resource/Life_writing"/>
    <skos:definition xml:lang="en">Indicates recorded "memories, and experiences, whether one's own or another's."<![CDATA[(<a href="#cwrc:727d97bc-af78-4122-94be-aa78b2e97d5a">DBpedia, 2019</a>)]]></skos:definition>
    <rdfs:subClassOf rdf:resource="http://sparql.cwrc.ca/ontologies/genre#LiteraryGenre"/>
  </owl:Class>
  <owl:Class rdf:about="http://sparql.cwrc.ca/ontologies/genre#ScriptForm">
    <rdfs:subClassOf rdf:resource="http://sparql.cwrc.ca/ontologies/genre#FormGenre"/>
    <skos:definition xml:lang="en">Indicates "written texts of stage plays, screenplays, and radio or television broadcasts."<![CDATA[(<a href="#cwrc:db2f8571-a773-4068-a35f-34262950bb8f">Getty, 2019</a>)]]></skos:definition>
    <skos:closeMatch rdf:resource="http://vocab.getty.edu/aat/300026487"/>
    <rdfs:label xml:lang="en">Script Form</rdfs:label>
  </owl:Class>
  <owl:Class rdf:about="http://sparql.cwrc.ca/ontologies/genre#LGBTQPlusGenre">
    <rdfs:label xml:lang="en">LGBTQ+Genre</rdfs:label>
    <skos:definition xml:lang="en">Indicates works concerned with LGBTQ+ identities and experiences. </skos:definition>
    <rdfs:subClassOf rdf:resource="http://sparql.cwrc.ca/ontologies/genre#LiteraryGenre"/>
  </owl:Class>
  <owl:Class rdf:about="http://sparql.cwrc.ca/ontologies/genre#VisualMedium">
    <rdfs:subClassOf rdf:resource="http://sparql.cwrc.ca/ontologies/genre#Medium"/>
    <rdfs:label xml:lang="en">Visual Medium</rdfs:label>
    <skos:definition xml:lang="en">Indicates media that are primarly visual.</skos:definition>
  </owl:Class>
  <owl:Class rdf:about="http://sparql.cwrc.ca/ontologies/genre#HistoricalGenre">
    <rdfs:subClassOf rdf:resource="http://sparql.cwrc.ca/ontologies/genre#LiteraryGenre"/>
    <rdfs:label xml:lang="en">Historical Genre</rdfs:label>
    <skos:definition xml:lang="en">Indicates works that relay histories in both written and oral form; not to be confused with historical fiction.</skos:definition>
  </owl:Class>
  <owl:Class rdf:about="http://sparql.cwrc.ca/ontologies/genre#DramaticGenre">
    <skos:closeMatch rdf:resource="http://vocab.getty.edu/aat/300417554"/>
    <skos:definition xml:lang="en">Indicates works "in prose or verse in which a story is related by means of dialogue and action . . . generally written with the intention of performance on stage, film, television, or the like."<![CDATA[(<a href="#cwrc:db2f8571-a773-4068-a35f-34262950bb8f">Getty, 2019</a>)]]></skos:definition>
    <rdfs:subClassOf rdf:resource="http://sparql.cwrc.ca/ontologies/genre#LiteraryGenre"/>
    <rdfs:label xml:lang="en">Dramatic Genre</rdfs:label>
  </owl:Class>
</rdf:RDF>
