<?xml version="1.0" ?>
<rdf:RDF 
    xml:base="http://sparql.cwrc.ca/ontologies/genre#" 
    xmlns="http://sparql.cwrc.ca/ontologies/genre#" 
    xmlns:as="http://www.w3.org/ns/activitystreams#" 
    xmlns:cc="http://creativecommons.org/ns#" 
    xmlns:cwrc="http://sparql.cwrc.ca/ontologies/cwrc#"
    xmlns:genre="http://sparql.cwrc.ca/ontologies/genre#" 
    xmlns:dbpedia="http://dbpedia.org/resource/" 
    xmlns:dcterms="http://purl.org/dc/terms/" 
    xmlns:doap="http://usefulinc.com/ns/doap#" 
    xmlns:eurovoc="http://eurovoc.europa.eu/"
    xmlns:foaf="http://xmlns.com/foaf/0.1/" 
    xmlns:geonames="http://sws.geonames.org/"
    xmlns:loc="http://id.loc.gov/vocabulary/relators/" 
    xmlns:nif="http://persistence.uni-leipzig.org/nlp2rdf/ontologies/nif-core#" 
    xmlns:oa="http://www.w3.org/ns/oa#" 
    xmlns:owl="http://www.w3.org/2002/07/owl#" 
    xmlns:prov="http://www.w3.org/ns/prov#" 
    xmlns:rdf="http://www.w3.org/1999/02/22-rdf-syntax-ns#" 
    xmlns:rdfs="http://www.w3.org/2000/01/rdf-schema#" 
    xmlns:skos="http://www.w3.org/2004/02/skos/core#" 
    xmlns:skosxl="http://www.w3.org/2008/05/skos-xl#" 
    xmlns:time="http://www.w3.org/2006/time#" 
    xmlns:vann="http://purl.org/vocab/vann/" 
    xmlns:void="http://rdfs.org/ns/void#" 
    xmlns:vs="http://www.w3.org/2003/06/sw-vocab-status/ns#" 
    xmlns:xsd="http://www.w3.org/2001/XMLSchema#">

 
  <owl:Ontology rdf:about="">
    <rdf:type rdf:resource="http://purl.org/vocommons/voaf#Vocabulary"/>
    <vann:preferredNamespacePrefix>genre</vann:preferredNamespacePrefix>
    <vann:preferredNamespaceUri>http://sparql.cwrc.ca/ontology/genre#</vann:preferredNamespaceUri>
    <dcterms:title xml:lang="en">The CWRC Literary Genre Ontology</dcterms:title>
    <rdfs:label xml:lang="en">The CWRC Literary Genre Ontology</rdfs:label>
    <foaf:name xml:lang="en">The CWRC Literary Genre Ontology</foaf:name>
    <dcterms:title xml:lang="fr">L'Ontologie des genres littéraires CWRC</dcterms:title>
    <rdfs:label xml:lang="fr">L'Ontologie des genres littéraires CWRC</rdfs:label>
    <foaf:name xml:lang="fr">L'Ontologie des genres littéraires CWRC</foaf:name>
    <dcterms:description xml:lang="en">The CWRC Literary Genre Ontology is the ontology used by the Canadian Writing Research Collaboratory to assign Literary Genres to different documents.</dcterms:description>
    <skos:definition xml:lang="en">The CWRC Literary Genre Ontology is the ontology used by the Canadian Writing Research Collaboratory to assign Literary Genres to different documents.</skos:definition>
    <rdfs:comment xml:lang="en">The CWRC Literary Genre Ontology is the ontology used by the Canadian Writing Research Collaboratory to assign Literary Genres to different documents.</rdfs:comment>
    <dcterms:description xml:lang="fr">L'Ontologie des genres littéraires CWRC est l'ontologie utilisée par le Collaboratoire scientifique des écrits du Canada pour assigner des genres à des écrits littéraires.</dcterms:description>
    <skos:definition xml:lang="fr">L'Ontologie des genres littéraires CWRC est l'ontologie utilisée par le Collaboratoire scientifique des écrits du Canada pour assigner des genres à des écrits littéraires.</skos:definition>
    <rdfs:comment xml:lang="fr">L'Ontologie des genres littéraires CWRC est l'ontologie utilisée par le Collaboratoire scientifique des écrits du Canada pour assigner des genres à des écrits littéraires.</rdfs:comment>
    <owl:versionInfo>0.1</owl:versionInfo>
    <dcterms:date rdf:datatype="http://www.w3.org/2001/XMLSchema#date">ONTOLOGY_DATE</dcterms:date>
    <dcterms:rights rdf:resource="http://creativecommons.org/licenses/by-nc/4.0/"/>
    <vs:term_status xml:lang="en">Testing</vs:term_status>
    <dcterms:creator>
      <foaf:Person rdf:about="#JadePenancier">
        <foaf:name>Jade Penancier</foaf:name>
      </foaf:Person>
    </dcterms:creator>
    <dcterms:creator>
      <foaf:Person rdf:about="#MicaelaJimenez">
        <foaf:name>Micaela Jimenez</foaf:name>
      </foaf:Person>
    </dcterms:creator>
    <dcterms:creator rdf:resource="#SusanBrown"/>
    <dcterms:creator>
      <foaf:Person rdf:about="#RobWarren">
        <foaf:name>Robert Warren</foaf:name>
        <owl:sameAs rdf:resource="http://rdf.muninn-project.org/ww1/2011/11/11/Person/Warren"/>
        <foaf:homepage rdf:resource="http://www.muninn-project.org/" />
      </foaf:Person>
    </dcterms:creator>
    <dcterms:creator>
      <foaf:Person rdf:about="#AlliyyaMo">
        <foaf:name>Alliyya Mo</foaf:name>
      </foaf:Person>
    </dcterms:creator>
    <dcterms:publisher>
      <foaf:Organization rdf:about="#cwrc">
        <foaf:name xml:lang="fr">Le Collaboratoire scientifique des écrits du Canada</foaf:name>
        <foaf:name xml:lang="en">The Canadian Writing Research Collaboratory</foaf:name>
        <foaf:logo rdf:resource="http://sparql.cwrc.ca/images/CWRCLogo-Horz-FullColour.png"/>
      </foaf:Organization>
    </dcterms:publisher>
    <loc:pdr>
      <foaf:Person rdf:about="#SusanBrown">
        <foaf:name>Susan Brown</foaf:name>
        <owl:sameAs rdf:resource="http://orcid.org/0000-0002-0267-7344"/>
      </foaf:Person>
    </loc:pdr>
    <loc:fnd>
      <foaf:Organization rdf:about="#sshrc">
        <foaf:name xml:lang="en">Social Sciences and Humanities Research Council</foaf:name>
        <foaf:name xml:lang="fr">Conseil de recherches en sciences humaines</foaf:name>
        <foaf:nick>SSHRC</foaf:nick>
      </foaf:Organization>
    </loc:fnd>
    <void:inDataset rdf:resource="#datasetdefinition"/>
    <foaf:logo rdf:resource="http://sparql.cwrc.ca/images/CWRCLogo-Horz-FullColour.png"/>
    <dcterms:subject rdf:resource="http://id.loc.gov/authorities/subjects/sh85077490"/>
  </owl:Ontology>


  <void:Dataset rdf:about="#datasetdefinition">
    <dcterms:title xml:lang="en">The CWRC Literary Genre Ontology</dcterms:title>
    <rdfs:label xml:lang="en">The CWRC Literary Genre Ontology</rdfs:label>
    <foaf:name xml:lang="en">The CWRC Literary Genre Ontology</foaf:name>
    <dcterms:title xml:lang="fr">L'Ontologie des genres littéraires CWRC</dcterms:title>
    <rdfs:label xml:lang="fr">L'Ontologie des genres littéraires CWRC</rdfs:label>
    <foaf:name xml:lang="fr">L'Ontologie des genres littéraires CWRC</foaf:name>
    <dcterms:description xml:lang="en">The CWRC Literary Genre Ontology is the ontology used by the Canadian Writing Research Collaboratory to assign Literary Genres to different documents.</dcterms:description>
    <skos:definition xml:lang="en">The CWRC Literary Genre Ontology is the ontology used by the Canadian Writing Research Collaboratory to assign Literary Genres to different documents.</skos:definition>
    <rdfs:comment xml:lang="en">The CWRC Literary Genre Ontology is the ontology used by the Canadian Writing Research Collaboratory to assign Literary Genres to different documents.</rdfs:comment>
    <dcterms:description xml:lang="fr">L'Ontologie des genres littéraires CWRC est l'ontologie utilisée par le Collaboratoire scientifique des écrits du Canada pour assigner des genres à des écrits littéraires.</dcterms:description>
    <skos:definition xml:lang="fr">L'Ontologie des genres littéraires CWRC est l'ontologie utilisée par le Collaboratoire scientifique des écrits du Canada pour assigner des genres à des écrits littéraires.</skos:definition>
    <rdfs:comment xml:lang="fr">L'Ontologie des genres littéraires CWRC est l'ontologie utilisée par le Collaboratoire scientifique des écrits du Canada pour assigner des genres à des écrits littéraires.</rdfs:comment>
    <!-- -->
    <cc:license rdf:resource="http://creativecommons.org/licenses/by-nc/4.0/"/>
    <cc:Jurisdiction rdf:resource="http://dbpedia.org/resource/Canada"/>
    <cc:attributionURL rdf:resource="http://www.cwrc.ca/"/>
    <dcterms:publisher rdf:resource="#cwrc"/>
    <dcterms:creator rdf:resource="#MicaelaJimenez"/>
    <dcterms:creator rdf:resource="#RobWarren"/>
    <dcterms:creator rdf:resource="#JadePenancier"/>
    <dcterms:creator rdf:resource="#AlliyyaMo"/>
    <dcterms:creator rdf:resource="#SusanBrown"/>
    <loc:pdr rdf:resource="#SusanBrown"/>
    <loc:fnd rdf:resource="#sshrc"/>
    <rdfs:isDefinedBy rdf:resource="http://sparql.cwrc.ca/ontologies/genre-ONTOLOGY_DATE"/>
    <foaf:logo rdf:resource="http://www.cwrc.ca/wp-content/uploads/2010/11/CWRC_logo_v074.gif"/>
    <dcterms:subject rdf:resource="http://id.loc.gov/authorities/subjects/sh85077490"/>
    <void:triples>TOTAL_TRIPLES_CWRC_ONTOLOGY</void:triples>
    <void:entities>TOTAL_ENTITIES_CWRC_ONTOLOGY</void:entities>
  </void:Dataset>

  <skos:Concept rdf:about="#originalOrlandoAuthor">
    <rdfs:label xml:lang="en">Members of the Orlando Project</rdfs:label>
    <rdfs:label xml:lang="fr">Les membres du projet Orlando</rdfs:label>
    <rdf:type rdf:resource="http://xmlns.com/foaf/0.1/Group"/>
    <foaf:name xml:lang="en">Members of the Orlando Project.</foaf:name>
    <foaf:homepage rdf:resource="http://orlando.cambridge.org/public/svDocumentation?formname=t&amp;d_id=CREDITSANDACKNOWLEDGEMENTS"/>
    <skos:definition xml:lang="en">The collection of all persons having written entries for The Orlando Project.</skos:definition>
    <skos:definition xml:lang="fr">La collection de tous les auteurs du Projet Orlando.</skos:definition>
    <rdfs:isDefinedBy rdf:resource="http://sparql.cwrc.ca/ontologies/genre-ONTOLOGY_DATE"/>
    <void:inDataset rdf:resource="#datasetdefinition"/>
  </skos:Concept>

  <owl:Class rdf:ID="Genre">
    <rdfs:label xml:lang="en">literary genre</rdfs:label>
    <rdfs:label xml:lang="fr">genre littéraire</rdfs:label>
    <rdf:type rdf:resource="http://www.w3.org/2004/02/skos/core#ConceptScheme"/>
    <skos:definition xml:lang="en"/>
    <skos:definition xml:lang="fr"/>
    <owl:sameAs rdf:resource="http://dbpedia.org/resource/Literary_genre"/>
    <rdfs:isDefinedBy rdf:resource="http://sparql.cwrc.ca/ontologies/genre-ONTOLOGY_DATE"/>
    <void:inDataset rdf:resource="#datasetdefinition"/>
  </owl:Class>

  <owl:ObjectProperty rdf:ID="hasGenre">
    <rdfs:label xml:lang="en">has genre</rdfs:label>
    <rdfs:label xml:lang="fr">a un genre</rdfs:label>
    <skos:definition xml:lang="en"/>
    <skos:definition xml:lang="fr"/>
    <rdfs:range rdf:resource="#Genre"/>
    <rdfs:isDefinedBy rdf:resource="http://sparql.cwrc.ca/ontologies/genre-ONTOLOGY_DATE"/>
    <void:inDataset rdf:resource="#datasetdefinition"/>
  </owl:ObjectProperty>

  <void:Dataset rdf:about="#datasetdefinition">
    <dcterms:title xml:lang="en">The CWRC Ontology</dcterms:title>
    <rdfs:label xml:lang="en">The CWRC Ontology</rdfs:label>
    <foaf:name xml:lang="en">The CWRC Ontology</foaf:name>
    <dcterms:title xml:lang="fr">L'Ontologie CWRC</dcterms:title>
    <rdfs:label xml:lang="fr">L'Ontologie CWRC</rdfs:label>
    <foaf:name xml:lang="fr">L'Ontologie CWRC</foaf:name>
    <dcterms:description xml:lang="en">The CWRC Ontology is the ontology of the Canadian Writing Research Collaboratory.</dcterms:description>
    <skos:definition xml:lang="en">The CWRC Ontology is the ontology of the Canadian Writing Research Collaboratory.</skos:definition>
    <rdfs:comment xml:lang="en">The CWRC Ontology is the ontology of the Canadian Writing Research Collaboratory.</rdfs:comment>
    <dcterms:description xml:lang="fr">L'Ontologie CWRC est l'ontologie du Collaboratoire scientifique des écrits du Canada.</dcterms:description>
    <skos:definition xml:lang="fr">L'Ontologie CWRC est l'ontologie du Collaboratoire scientifique des écrits du Canada.</skos:definition>
    <rdfs:comment xml:lang="fr">L'Ontologie CWRC est l'ontologie du Collaboratoire scientifique des écrits du Canada.</rdfs:comment>
    <!-- -->
    <cc:license rdf:resource="http://creativecommons.org/licenses/by-nc/4.0/"/>
    <cc:Jurisdiction rdf:resource="http://dbpedia.org/resource/Canada"/>
    <cc:attributionURL rdf:resource="http://www.cwrc.ca/"/>
    <dcterms:publisher rdf:resource="#cwrc"/>
    <dcterms:creator rdf:resource="#MicaelaJimenez"/>
    <dcterms:creator rdf:resource="#RobWarren"/>
    <dcterms:creator rdf:resource="#JadePenancier"/>
    <dcterms:creator rdf:resource="#AlliyyaMo"/>
    <dcterms:creator rdf:resource="#SusanBrown"/>
    <loc:ctb rdf:resource="#ConstanceCrompton"/>
    <loc:ctb rdf:resource="#originalOrlandoAuthor"/>
    <loc:pdr rdf:resource="#SusanBrown"/>
    <loc:fnd rdf:resource="#sshrc"/>
    <rdfs:isDefinedBy rdf:resource="http://sparql.cwrc.ca/ontologies/genre-ONTOLOGY_DATE"/>
    <foaf:logo rdf:resource="http://www.cwrc.ca/wp-content/uploads/2010/11/CWRC_logo_v074.gif"/>
    <dcterms:subject rdf:resource="http://id.loc.gov/authorities/subjects/sh85019388"/>
    <dcterms:subject rdf:resource="http://id.loc.gov/authorities/subjects/sh85043777"/>
    <dcterms:subject rdf:resource="http://id.loc.gov/authorities/subjects/sh85013838"/>
    <dcterms:subject rdf:resource="http://id.loc.gov/authorities/subjects/sh85077519"/>
    <dcterms:subject rdf:resource="http://id.loc.gov/authorities/subjects/sh2009007122"/>
    <void:triples>TOTAL_TRIPLES_CWRC_ONTOLOGY</void:triples>
    <void:entities>TOTAL_ENTITIES_CWRC_ONTOLOGY</void:entities>
  </void:Dataset>



  <genre:Genre rdf:about="#genreAbridgement">
    <rdf:value>ABRIDGEMENT</rdf:value>
    <rdfs:label xml:lang="en">abridgement</rdfs:label>
    <rdfs:label xml:lang="fr">résumé</rdfs:label>
    <rdfs:isDefinedBy rdf:resource="http://sparql.cwrc.ca/ontologies/genre-ONTOLOGY_DATE"/>
    <void:inDataset rdf:resource="#datasetdefinition"/>
    <skos:inScheme rdf:resource="#Genre"/>
    <rdf:type rdf:resource="http://www.w3.org/2004/02/skos/core#Concept"/>
    <skos:definition xml:lang="en">Versions of written works produced by condensation and omission but with retention of the general meaning and manner of presentation of the original, often prepared by someone other than the author of the original. <![CDATA[<a href="#_getty_2017">(Getty, 2017)</a>]]></skos:definition>
    <skos:definition xml:lang="de">Version einer schriftlichen Arbeit, die durch Verdichtung und Auslassung zustande kommt, aber die eigentliche Bedeutung und Art der Darstellung des Originals beibehält; wird häufig von jemand anderem als dem Autor erstellt.  <![CDATA[<a href="#_getty_2017">(Getty, 2017)</a>]]></skos:definition>
    <skos:definition xml:lang="nl">Wordt gebruikt voor sterk ingekorte versies van geschreven werken, waarin, ondanks de vele weglatingen, de algemene inhoud en de indeling van het origineel behouden blijft. De schrijver van deze samenvattingen is vaak niet dezelfde als de auteur van het origineel. <![CDATA[<a href="#_getty_2017">(Getty, 2017)</a>]]></skos:definition>
    <skos:definition xml:lang="es">Úsese para versiones de obras escritas producidas mediante un resumen y omisiones del original pero manteniendo el significado general y su forma de presentación, a menudo preparadas por alguien diferente al autor del original. <![CDATA[<a href="#_getty_2017">(Getty, 2017)</a>]]></skos:definition>
    <skos:definition xml:lang="zh-hant">書寫作品之濃縮與省略版本，但保留原作的大體意義及呈現方式，常由原作者以外的人編纂。 <![CDATA[<a href="#_getty_2017">(Getty, 2017)</a>]]></skos:definition>
    <prov:derivedFrom rdf:resource="http://vocab.getty.edu/aat/300202489"/>
    <rdfs:comment xml:lang="en">The description for this term is indebted to the Getty Art &amp; Architecture Thesaurus.</rdfs:comment>
  </genre:Genre>
  <genre:Genre rdf:about="#genreAclef">
    <rdf:value>ACLEF</rdf:value>
    <rdfs:label xml:lang="en">aclef</rdfs:label>
    <rdfs:label xml:lang="fr">roman à clef </rdfs:label>
    <rdfs:isDefinedBy rdf:resource="http://sparql.cwrc.ca/ontologies/genre-ONTOLOGY_DATE"/>
    <void:inDataset rdf:resource="#datasetdefinition"/>
    <skos:inScheme rdf:resource="#Genre"/>
    <rdf:type rdf:resource="http://www.w3.org/2004/02/skos/core#Concept"/>
  </genre:Genre>
  <genre:Genre rdf:about="#genreAcrostic">
    <rdf:value>ACROSTIC</rdf:value>
    <rdfs:label xml:lang="en">acrostic</rdfs:label>
    <rdfs:label xml:lang="fr">acrostiche</rdfs:label>
    <rdfs:isDefinedBy rdf:resource="http://sparql.cwrc.ca/ontologies/genre-ONTOLOGY_DATE"/>
    <void:inDataset rdf:resource="#datasetdefinition"/>
    <skos:inScheme rdf:resource="#Genre"/>
    <rdf:type rdf:resource="http://www.w3.org/2004/02/skos/core#Concept"/>
    <skos:definition xml:lang="fr">Un acrostiche, du grec akrostikhos (akros, haut, élevé et stikhos, le vers), est un poème, une strophe ou une série de strophes fondés sur une forme poétique consistant en ce que, lues verticalement de haut en bas, la première lettre ou, parfois, les premiers mots d'une suite de vers composent un mot ou une expression en lien avec le poème. <![CDATA[<a href="#_dbpedia_2017">(DBpedia, 2017)</a>]]></skos:definition>
    <prov:derivedFrom rdf:resource="http://dbpedia.org/resource/Acrostic"/>
    <rdfs:comment xml:lang="en">The description for this term is indebted to DBpedia. </rdfs:comment>
    <rdfs:comment xml:lang="fr">La description de ce terme est basée sur celle de DBPedia.</rdfs:comment>

    <skos:definition xml:lang="en">Short poems or prose compositions in which text is arranged so that the first letters of each line form a word, phrase, or motto. <![CDATA[<a href="#_getty_2017">(Getty, 2017)</a>]]></skos:definition>
    <skos:definition xml:lang="de">Kurzes Gedicht oder Prosakomposition, bei der der Text so angeordnet ist, dass die ersten Buchstaben jeder Zeile aneinandergereiht ein Wort, einen Satz oder ein Motto ergeben. <![CDATA[<a href="#_getty_2017">(Getty, 2017)</a>]]></skos:definition>
    <skos:definition xml:lang="nl">Korte gedichten of stukjes proza waarvan de eerste letters van de opeenvolgende regels samen een woord, een zinsnede of een motto vormen. <![CDATA[<a href="#_getty_2017">(Getty, 2017)</a>]]></skos:definition>
    <skos:definition xml:lang="es">Poemas cortos o composiciones en prosa en los que el texto es ordenado de tal manera que las primeras letras de cada línea forman una palabra, frase o máxima. <![CDATA[<a href="#_getty_2017">(Getty, 2017)</a>]]></skos:definition>
    <skos:definition xml:lang="zh-hant">各行首字母可組成一個字、詞，或座右銘的短詩或散文作品。 <![CDATA[<a href="#_getty_2017">(Getty, 2017)</a>]]></skos:definition>
    <prov:derivedFrom rdf:resource="http://vocab.getty.edu/aat/300256198"/>
    <rdfs:comment xml:lang="en">The description for this term is indebted to the Getty Art &amp; Architecture Thesaurus.</rdfs:comment>
  </genre:Genre>
  <genre:Genre rdf:about="#genreAdaptation">
    <rdf:value>ADAPTATION</rdf:value>
    <rdfs:label xml:lang="en">adaptation</rdfs:label>
    <rdfs:label xml:lang="fr">adaptation</rdfs:label>
    <rdfs:isDefinedBy rdf:resource="http://sparql.cwrc.ca/ontologies/genre-ONTOLOGY_DATE"/>
    <void:inDataset rdf:resource="#datasetdefinition"/>
    <skos:inScheme rdf:resource="#Genre"/>
    <rdf:type rdf:resource="http://www.w3.org/2004/02/skos/core#Concept"/>
    <skos:definition xml:lang="en">Written works or works derived from written works, where the second work is an alteration or amendment a text to make it suitable for another purpose. An example of an adaptation is a version of an earlier text made to better agree with a philosophy other than that intended by the original. Other examples are written works adapted for another medium, such as film, broadcasting, or stage production. For visual works adapted from another work, use &quot;adaptations (derivative objects).&quot;</skos:definition>
    <prov:derivedFrom rdf:resource="http://vocab.getty.edu/aat/300410356"/>
    <rdfs:comment xml:lang="en">The description for this term is indebted to the Getty Art &amp; Architecture Thesaurus.</rdfs:comment>
  </genre:Genre>
  <genre:Genre rdf:about="#genreAdventurewriting">
    <rdf:value>ADVENTUREWRITING</rdf:value>
    <rdfs:label xml:lang="en">adventure writing</rdfs:label>
    <rdfs:label xml:lang="fr">roman d'aventure</rdfs:label> 
    <rdfs:isDefinedBy rdf:resource="http://sparql.cwrc.ca/ontologies/genre-ONTOLOGY_DATE"/>
    <void:inDataset rdf:resource="#datasetdefinition"/>
    <skos:inScheme rdf:resource="#Genre"/>
    <rdf:type rdf:resource="http://www.w3.org/2004/02/skos/core#Concept"/>
  </genre:Genre>
  <genre:Genre rdf:about="#genreAdvertisingcopy">
    <rdf:value>ADVERTISINGCOPY</rdf:value>
    <rdfs:label xml:lang="en">advertising copy</rdfs:label>
    <rdfs:label xml:lang="fr"/>
    <rdfs:isDefinedBy rdf:resource="http://sparql.cwrc.ca/ontologies/genre-ONTOLOGY_DATE"/>
    <void:inDataset rdf:resource="#datasetdefinition"/>
    <skos:inScheme rdf:resource="#Genre"/>
    <rdf:type rdf:resource="http://www.w3.org/2004/02/skos/core#Concept"/>
  </genre:Genre>
  <genre:Genre rdf:about="#genreAfterpiece">
    <rdf:value>AFTERPIECE</rdf:value>
    <rdfs:label xml:lang="en">afterpiece</rdfs:label>
    <rdfs:label xml:lang="fr"/>
    <rdfs:isDefinedBy rdf:resource="http://sparql.cwrc.ca/ontologies/genre-ONTOLOGY_DATE"/>
    <void:inDataset rdf:resource="#datasetdefinition"/>
    <skos:inScheme rdf:resource="#Genre"/>
    <rdf:type rdf:resource="http://www.w3.org/2004/02/skos/core#Concept"/>
  </genre:Genre>
  <genre:Genre rdf:about="#genreAfterword">
    <rdf:value>AFTERWORD</rdf:value>
    <rdfs:label xml:lang="en">afterword</rdfs:label>
    <rdfs:label xml:lang="fr">postface</rdfs:label>
    <rdfs:isDefinedBy rdf:resource="http://sparql.cwrc.ca/ontologies/genre-ONTOLOGY_DATE"/>
    <void:inDataset rdf:resource="#datasetdefinition"/>
    <skos:inScheme rdf:resource="#Genre"/>
    <rdf:type rdf:resource="http://www.w3.org/2004/02/skos/core#Concept"/>
  </genre:Genre>
  <genre:Genre rdf:about="#genreAgitprop">
    <rdf:value>AGITPROP</rdf:value>
    <rdfs:label xml:lang="en">agitprop</rdfs:label>
    <rdfs:label xml:lang="fr">agitprop</rdfs:label>
    <rdfs:isDefinedBy rdf:resource="http://sparql.cwrc.ca/ontologies/genre-ONTOLOGY_DATE"/>
    <void:inDataset rdf:resource="#datasetdefinition"/>
    <skos:inScheme rdf:resource="#Genre"/>
    <rdf:type rdf:resource="http://www.w3.org/2004/02/skos/core#Concept"/>
    <skos:definition xml:lang="en">Derived from agitation propaganda, meaning intended to inspire political action. With reference to visual art, refers to the specific art movement arising in Soviet Russia following the Bolshevik revolution. <![CDATA[<a href="#_getty_2017">(Getty, 2017)</a>]]></skos:definition>
    <skos:definition xml:lang="es">Derivado de propaganda de agitación, cuyo objetivo es inspirar acción política. En referencia a las artes visuales, úsese para el movimiento artísitico específico surgido en la Rusia Sovietica tras la revolución Bolchevique. <![CDATA[<a href="#_getty_2017">(Getty, 2017)</a>]]></skos:definition>
    <skos:definition xml:lang="nl">Ontleend aan de agitatie en propaganda, bedoeld om politieke actie te inspireren. Voor de beeldende kunsten te gebruiken voor de specifieke kunstbeweging in het voormalig Sovjet Unie na de bolsjewistische revolutie. <![CDATA[<a href="#_getty_2017">(Getty, 2017)</a>]]></skos:definition>
    <skos:definition xml:lang="zh-hant">概念來自煽動性宣傳活動，意指刻意激起政治性活動。若指涉視覺藝術方面，則指在布爾什維克革命後的蘇聯發起的特定藝術運動。  <![CDATA[<a href="#_getty_2017">(Getty, 2017)</a>]]></skos:definition>
    <prov:derivedFrom rdf:resource="http://vocab.getty.edu/aat/300055540"/>
    <rdfs:comment xml:lang="en">The description for this term is indebted to the Getty Art &amp; Architecture Thesaurus.</rdfs:comment>
  </genre:Genre>
  <genre:Genre rdf:about="#genreAllegory">
    <rdf:value>ALLEGORY</rdf:value>
    <rdfs:label xml:lang="en">allegory</rdfs:label>
    <rdfs:label xml:lang="fr">allégorie</rdfs:label>
    <rdfs:isDefinedBy rdf:resource="http://sparql.cwrc.ca/ontologies/genre-ONTOLOGY_DATE"/>
    <void:inDataset rdf:resource="#datasetdefinition"/>
    <skos:inScheme rdf:resource="#Genre"/>
    <rdf:type rdf:resource="http://www.w3.org/2004/02/skos/core#Concept"/>
    <skos:definition xml:lang="fr">Une allégorie (du grec : ἄλλον / állon, « autre chose », et ἀγορεύειν / agoreúein, « parler en public ») est une forme de représentation indirecte qui emploie une chose (une personne, un être animé ou inanimé, une action) comme signe d'une autre chose, cette dernière étant souvent une idée abstraite ou une notion morale difficile à représenter directement. Elle représente donc une idée abstraite par du concret. En littérature, l'allégorie est une figure rhétorique qui consiste à exprimer une idée en utilisant une histoire ou une représentation qui doit servir de support comparatif. La signification étymologique est : « une autre manière de dire », au moyen d'une image figurative ou figurée. <![CDATA[<a href="#_dbpedia_2017">(DBpedia, 2017)</a>]]></skos:definition>
    <prov:derivedFrom rdf:resource="http://dbpedia.org/resource/Allegory"/>
    <rdfs:comment xml:lang="en">The description for this term is indebted to DBpedia. </rdfs:comment>
    <rdfs:comment xml:lang="fr">La description de ce terme est basée sur celle de DBPedia.</rdfs:comment>

    <skos:definition xml:lang="en">Literary works, art works, or other creative works that employ allegory to express complex abstract ideas, for example works that employ symbolic, fictional figures and actions to express truths or generalizations about human conduct or experience. <![CDATA[<a href="#_getty_2017">(Getty, 2017)</a>]]></skos:definition>
    <skos:definition xml:lang="de">Literarisches Werk, Kunstwerk oder anderes künstlerisches Werk, das allegorische Darstellungsformen benutzt, um komplexe abstrakte Ideen auszudrücken, zum Beispiel ein Werk, das symbolhafte, fiktionale Bilder und Handlungen verwendet, um Wahrheiten oder Verallgemeinerungen über menschliches Verhalten oder Erfahrungen zum Ausdruck zu bringen. <![CDATA[<a href="#_getty_2017">(Getty, 2017)</a>]]></skos:definition>
    <skos:definition xml:lang="es">Obras literarias que emplean personajes y acciones ficticias simbólicas para expresar verdades o generalizaciones acerca de conductas o experiencias humanas. <![CDATA[<a href="#_getty_2017">(Getty, 2017)</a>]]></skos:definition>
    <skos:definition xml:lang="nl">Literaire werken waarin met behulp van fictionele, symbolische figuren en handelingen waarheden of generalisaties omtrent menselijk gedrag of menselijke ervaringen worden gedebiteerd. <![CDATA[<a href="#_getty_2017">(Getty, 2017)</a>]]></skos:definition>
    <prov:derivedFrom rdf:resource="http://vocab.getty.edu/aat/300202507"/>
    <rdfs:comment xml:lang="en">The description for this term is indebted to the Getty Art &amp; Architecture Thesaurus.</rdfs:comment>
  </genre:Genre>
  <genre:Genre rdf:about="#genreAnagram">
    <rdf:value>ANAGRAM</rdf:value>
    <rdfs:label xml:lang="en">anagram</rdfs:label>
    <rdfs:label xml:lang="fr">anagramme</rdfs:label>
    <rdfs:isDefinedBy rdf:resource="http://sparql.cwrc.ca/ontologies/genre-ONTOLOGY_DATE"/>
    <void:inDataset rdf:resource="#datasetdefinition"/>
    <skos:inScheme rdf:resource="#Genre"/>
    <rdf:type rdf:resource="http://www.w3.org/2004/02/skos/core#Concept"/>
    <skos:definition xml:lang="en">Anagrammatic poetry is poetry with the constrained form that either each line or each verse is an anagram of all other lines or verses in the poem. A poet that specializes in anagrams is an anagrammarian. Writing anagrammatic poetry is a form of a constrained writing similar to writing pangrams or long alliterations. <![CDATA[<a href="#_dbpedia_2017">(DBpedia, 2017)</a>]]></skos:definition>
    <prov:derivedFrom rdf:resource="http://dbpedia.org/resource/Anagrammatic_poem"/>
    <rdfs:comment xml:lang="en">The description for this term is indebted to DBpedia. </rdfs:comment>
    <skos:definition xml:lang="en">Words or phrases made by transposing the letters of other words or phrases. <![CDATA[<a href="#_getty_2017">(Getty, 2017)</a>]]></skos:definition>
    <skos:definition xml:lang="es">Palabras o frases que resultan de la transposición de las letras de otras palabras o frases. <![CDATA[<a href="#_getty_2017">(Getty, 2017)</a>]]></skos:definition>
    <skos:definition xml:lang="nl">Woorden of zinnen die worden gevormd door de letters van andere woorden of zinnen om te zetten. <![CDATA[<a href="#_getty_2017">(Getty, 2017)</a>]]></skos:definition>
    <skos:definition xml:lang="zh-hant">將其他字或詞的字母調換位置，所組成的字或詞。 <![CDATA[<a href="#_getty_2017">(Getty, 2017)</a>]]></skos:definition>
    <prov:derivedFrom rdf:resource="http://vocab.getty.edu/aat/300202515"/>
    <rdfs:comment xml:lang="en">The description for this term is indebted to the Getty Art &amp; Architecture Thesaurus.</rdfs:comment>
  </genre:Genre>
  <genre:Genre rdf:about="#genreAnnotation">
    <rdf:value>ANNOTATION</rdf:value>
    <rdfs:label xml:lang="en">annotation</rdfs:label>
    <rdfs:label xml:lang="fr">annotation</rdfs:label>
    <rdfs:isDefinedBy rdf:resource="http://sparql.cwrc.ca/ontologies/genre-ONTOLOGY_DATE"/>
    <void:inDataset rdf:resource="#datasetdefinition"/>
    <skos:inScheme rdf:resource="#Genre"/>
    <rdf:type rdf:resource="http://www.w3.org/2004/02/skos/core#Concept"/>
    <skos:definition xml:lang="en">Notes added as comment or explanation, such as those accompanying an entry in a bibliography, reading list, or catalogue intended to describe, explain, or evaluate the publication referred to. <![CDATA[<a href="#_getty_2017">(Getty, 2017)</a>]]></skos:definition>
    <skos:definition xml:lang="de">Ergänzung, die als Kommentar oder Erklärung hinzugefügt wird, wie beispielsweise jene, die einem Titel in einer Bibliografie, einer Leseliste oder einem Katalog beigefügt ist und die betreffende Publikation beschreiben, erklären oder bewerten soll. <![CDATA[<a href="#_getty_2017">(Getty, 2017)</a>]]></skos:definition>
    <skos:definition xml:lang="es">Notas agregadas como comentarios o explicaciones. <![CDATA[<a href="#_getty_2017">(Getty, 2017)</a>]]></skos:definition>
    <skos:definition xml:lang="nl">Verklarende aantekeningen. <![CDATA[<a href="#_getty_2017">(Getty, 2017)</a>]]></skos:definition>
    <prov:derivedFrom rdf:resource="http://vocab.getty.edu/aat/300026100"/>
    <rdfs:comment xml:lang="en">The description for this term is indebted to the Getty Art &amp; Architecture Thesaurus.</rdfs:comment>
  </genre:Genre>
  <genre:Genre rdf:about="#genreAnswer">
    <rdf:value>ANSWER</rdf:value>
    <rdfs:label xml:lang="en">answer</rdfs:label>
    <rdfs:label xml:lang="fr">réponse</rdfs:label>
    <rdfs:isDefinedBy rdf:resource="http://sparql.cwrc.ca/ontologies/genre-ONTOLOGY_DATE"/>
    <void:inDataset rdf:resource="#datasetdefinition"/>
    <skos:inScheme rdf:resource="#Genre"/>
    <rdf:type rdf:resource="http://www.w3.org/2004/02/skos/core#Concept"/>
  </genre:Genre>
  <genre:Genre rdf:about="#genreAnthem">
    <rdf:value>ANTHEM</rdf:value>
    <rdfs:label xml:lang="en">anthem</rdfs:label>
    <rdfs:label xml:lang="fr">hymne</rdfs:label>
    <rdfs:isDefinedBy rdf:resource="http://sparql.cwrc.ca/ontologies/genre-ONTOLOGY_DATE"/>
    <void:inDataset rdf:resource="#datasetdefinition"/>
    <skos:inScheme rdf:resource="#Genre"/>
    <rdf:type rdf:resource="http://www.w3.org/2004/02/skos/core#Concept"/>
  </genre:Genre>
  <genre:Genre rdf:about="#genreAnthology">
    <rdf:value>ANTHOLOGY</rdf:value>
    <rdfs:label xml:lang="en">anthology</rdfs:label>
    <rdfs:label xml:lang="fr">anthologie</rdfs:label>
    <rdfs:isDefinedBy rdf:resource="http://sparql.cwrc.ca/ontologies/genre-ONTOLOGY_DATE"/>
    <void:inDataset rdf:resource="#datasetdefinition"/>
    <skos:inScheme rdf:resource="#Genre"/>
    <rdf:type rdf:resource="http://www.w3.org/2004/02/skos/core#Concept"/>
    <skos:definition xml:lang="en">Collections of choice extracts, from the writings of one author, or various authors, and usually having a common characteristic such as subject matter or literary form. <![CDATA[<a href="#_getty_2017">(Getty, 2017)</a>]]></skos:definition>
    <skos:definition xml:lang="de">Sammlung von Auszügen aus den Schriften eines Autors oder verschiedenen Autoren; in der Regel mit einem gemeinsamen Merkmal wie Motiv oder literarischer Form. <![CDATA[<a href="#_getty_2017">(Getty, 2017)</a>]]></skos:definition>
    <skos:definition xml:lang="es">Colecciones de piezas escogidas de las obras de un autor, o varios autores, y generalmente teniendo una característica común, tal como un tema central o una forma literaria. <![CDATA[<a href="#_getty_2017">(Getty, 2017)</a>]]></skos:definition>
    <skos:definition xml:lang="nl">Verzamelingen van passages gekozen uit het geschreven werk van één auteur of verscheidene auteurs, meestal met een gemeenschappelijk kenmerk, zoals het onderwerp of de literaire vorm. <![CDATA[<a href="#_getty_2017">(Getty, 2017)</a>]]></skos:definition>
    <prov:derivedFrom rdf:resource="http://vocab.getty.edu/aat/300026037"/>
    <rdfs:comment xml:lang="en">The description for this term is indebted to the Getty Art &amp; Architecture Thesaurus.</rdfs:comment>
  </genre:Genre>
  <genre:Genre rdf:about="#genreAntiromance">
    <rdf:value>ANTIROMANCE</rdf:value>
    <rdfs:label xml:lang="en">antiromance</rdfs:label>
    <rdfs:label xml:lang="fr"/>
    <rdfs:isDefinedBy rdf:resource="http://sparql.cwrc.ca/ontologies/genre-ONTOLOGY_DATE"/>
    <void:inDataset rdf:resource="#datasetdefinition"/>
    <skos:inScheme rdf:resource="#Genre"/>
    <rdf:type rdf:resource="http://www.w3.org/2004/02/skos/core#Concept"/>
  </genre:Genre>
  <genre:Genre rdf:about="#genreAphorism">
    <rdf:value>APHORISM</rdf:value>
    <rdfs:label xml:lang="en">aphorism</rdfs:label>
    <rdfs:label xml:lang="fr">aphorisme</rdfs:label>
    <rdfs:isDefinedBy rdf:resource="http://sparql.cwrc.ca/ontologies/genre-ONTOLOGY_DATE"/>
    <void:inDataset rdf:resource="#datasetdefinition"/>
    <skos:inScheme rdf:resource="#Genre"/>
    <rdf:type rdf:resource="http://www.w3.org/2004/02/skos/core#Concept"/>
    <rdfs:comment xml:lang="en">The description for this term is indebted to the Getty Art &amp; Architecture Thesaurus.</rdfs:comment>
    <skos:definition xml:lang="en">Short, pithy statements of principle or precepts, often of known authorship; distinguished from &quot;proverbs&quot; which are statements repeated colloquially and which often embody the folk wisdom of a group or nation. <![CDATA[<a href="#_getty_2017">(Getty, 2017)</a>]]></skos:definition>
    <skos:definition xml:lang="de">Kurze, prägnante Erklärung eines Prinzips oder Grundsatzes, häufig mit bekannter Urheberschaft; zu unterscheiden vom &quot;Sprichwort&quot;, einer in der Alltagssprache wiederholten Äußerung, die häufig Volksweisheiten einer Gruppe oder eines Landes enthält. <![CDATA[<a href="#_getty_2017">(Getty, 2017)</a>]]></skos:definition>
    <skos:definition xml:lang="es">Sentencias cortas y concisas de principios o preceptos, a menudo de conocida autoría, diferentes de los &quot;proverbios&quot; que son sentencias que se repiten coloquialmente y que a menudo encarnan la sabiduría popular de un grupo o nación. <![CDATA[<a href="#_getty_2017">(Getty, 2017)</a>]]></skos:definition>
    <skos:definition xml:lang="nl">Korte, bondige formuleringen van principes of voorschriften, waarvan de auteur dikwijls bekend is; te onderscheiden van 'spreekwoorden', hetgeen uitdrukkingen zijn die in de omgangstaal zijn ingeburgerd en dikwijls een volkswijsheid van een groep mensen of een volk uitdrukken. <![CDATA[<a href="#_getty_2017">(Getty, 2017)</a>]]></skos:definition>
    <prov:derivedFrom rdf:resource="http://vocab.getty.edu/aat/300253001"/>
    <rdfs:comment xml:lang="en">The description for this term is indebted to the Getty Art &amp; Architecture Thesaurus.</rdfs:comment>
  </genre:Genre>
  <genre:Genre rdf:about="#genreApology">
    <rdf:value>APOLOGY</rdf:value>
    <rdfs:label xml:lang="en">apology</rdfs:label>
    <rdfs:label xml:lang="fr">apologie</rdfs:label>
    <rdfs:isDefinedBy rdf:resource="http://sparql.cwrc.ca/ontologies/genre-ONTOLOGY_DATE"/>
    <void:inDataset rdf:resource="#datasetdefinition"/>
    <skos:inScheme rdf:resource="#Genre"/>
    <rdf:type rdf:resource="http://www.w3.org/2004/02/skos/core#Concept"/>
  </genre:Genre>
  <genre:Genre rdf:about="#genreArtcriticism">
    <rdf:value>ARTCRITICISM</rdf:value>
    <rdfs:label xml:lang="en">art criticism</rdfs:label>
    <rdfs:label xml:lang="fr">critique d'art</rdfs:label>
    <rdfs:isDefinedBy rdf:resource="http://sparql.cwrc.ca/ontologies/genre-ONTOLOGY_DATE"/>
    <void:inDataset rdf:resource="#datasetdefinition"/>
    <skos:inScheme rdf:resource="#Genre"/>
    <rdf:type rdf:resource="http://www.w3.org/2004/02/skos/core#Concept"/>
  </genre:Genre>
  <genre:Genre rdf:about="#genreAutobiography">
    <rdf:value>AUTOBIOGRAPHY</rdf:value>
    <rdfs:label xml:lang="en">autobiography</rdfs:label>
    <rdfs:label xml:lang="fr">autobiographie</rdfs:label>
    <rdfs:isDefinedBy rdf:resource="http://sparql.cwrc.ca/ontologies/genre-ONTOLOGY_DATE"/>
    <void:inDataset rdf:resource="#datasetdefinition"/>
    <skos:inScheme rdf:resource="#Genre"/>
    <rdf:type rdf:resource="http://www.w3.org/2004/02/skos/core#Concept"/>
    <skos:definition xml:lang="en">Documents of any type that are biographies of individuals written by themselves. For the overall genre, use &quot;autobiography (genre).&quot;<![CDATA[<a href="#_getty_2017">(Getty, 2017)</a>]]></skos:definition>
    <skos:definition xml:lang="es">Biografías de individuos escritas por ellos mismos. <![CDATA[<a href="#_getty_2017">(Getty, 2017)</a>]]></skos:definition>
    <skos:definition xml:lang="nl">Biografieën met de auteur zelf als onderwerp. <![CDATA[<a href="#_getty_2017">(Getty, 2017)</a>]]></skos:definition>
    <skos:definition xml:lang="de">Biographie einer Person, die von ihr selbst verfasst wurde. <![CDATA[<a href="#_getty_2017">(Getty, 2017)</a>]]></skos:definition>
    <prov:derivedFrom rdf:resource="http://vocab.getty.edu/aat/300080104"/>
    <rdfs:comment xml:lang="en">The description for this term is indebted to the Getty Art &amp; Architecture Thesaurus.</rdfs:comment>
  </genre:Genre>
  <genre:Genre rdf:about="#genreBallade">
    <rdf:value>BALLAD</rdf:value>
    <rdf:value>BALLADE</rdf:value>
    <rdf:value>BALLAD</rdf:value>
    <rdfs:label xml:lang="en">ballade</rdfs:label>
    <rdfs:label xml:lang="fr">ballade</rdfs:label>
    <rdfs:isDefinedBy rdf:resource="http://sparql.cwrc.ca/ontologies/genre-ONTOLOGY_DATE"/>
    <void:inDataset rdf:resource="#datasetdefinition"/>
    <skos:inScheme rdf:resource="#Genre"/>
    <rdf:type rdf:resource="http://www.w3.org/2004/02/skos/core#Concept"/>
    <skos:definition xml:lang="en">A ballade (from French ballade, [baˈlad], and German Ballade, [baˈlaːdə], both being words for &quot;ballad&quot;), in classical music since the late 18th century, refers to a setting of a literary ballad, a narrative poem, in the musical tradition of the Lied, or to a one-movement instrumental piece with lyrical and dramatic narrative qualities reminiscent of such a song setting, especially a piano ballad. <![CDATA[<a href="#_dbpedia_2017">(DBpedia, 2017)</a>]]></skos:definition>
    <skos:definition xml:lang="de">Die Ballade ist in der Klaviermusik eine Gattung des 19. Jahrhunderts, die ähnlich wie das Charakterstück oder das Lied ohne Worte formal nicht festgelegt ist. Gelegentlich lassen sich die Komponisten von Dichtungen (z. B. Chopin und Brahms) oder Stimmungen inspirieren. Zu den Vorläufern der Klavierballade zählen die Rhapsodien der beiden tschechischen Komponisten Václav Jan Křtitel Tomášek und Jan Václav Voříšek. <![CDATA[<a href="#_dbpedia_2017">(DBpedia, 2017)</a>]]></skos:definition>
    <skos:definition xml:lang="es">El término balada se ha utilizado de formas muy diferentes en la historia de la música. En los siglos XIV y XV la palabra francesa ballade designaba un tipo de canción, habitualmente con tres estrofas de siete u ocho versos de los que el último servía de estribillo. La forma musical era la denominada &quot;forma bar&quot; (AAB): la melodía de los dos primeros versos se repetía en el tercero y cuarto; el resto se cantaban con melodía diferente. Las ballades eran habitualmente polifónicas, a dos o, con más frecuencia, tres voces: la voz superior (cantus) era la melodía principal; las otras voces podían ser cantadas o interpretadas con instrumentos. En Italia, en el Trecento (siglo XIV), el término ballata designaba un tipo diferente de canción, similar al virelay francés: un estribillo alternaba con estrofas divididas en dos secciones: la primera repetía dos veces una melodía, con final abierto y cerrado; la segunda se cantaba con la melodía del estribillo. En el siglo XIX, el título fue dado por Frédéric Chopin a cuatro importantes obras a gran escala para piano (Opus 23, 38, 47 y 52), la primera aplicación significativa del término en la música instrumental. Subsecuentemente otros compositores han usado el título para sus obras para piano: Johannes Brahms (la tercera de sus Klavierstücke opus 118, y las cuatro del opus 10), Edvard Grieg (opus 24, un conjunto de variaciones), Franz Liszt (que escribió dos) y Gabriel Fauré (opus 19, posteriormente arreglada para piano y orquesta). Sin embargo, hay que destacar que también se han escrito baladas para otros instrumentos. <![CDATA[<a href="#_dbpedia_2017">(DBpedia, 2017)</a>]]></skos:definition>
    <prov:derivedFrom rdf:resource="http://dbpedia.org/resource/Ballade_(classical_music)"/>
    <rdfs:comment xml:lang="en">The description for this term is indebted to DBpedia. </rdfs:comment>
    <rdfs:comment xml:lang="fr">La description de ce terme est basée sur celle de DBPedia.</rdfs:comment>

  </genre:Genre>
  <genre:Genre rdf:about="#genreBalladopera">
    <rdf:value>BALLADOPERA</rdf:value>
    <rdfs:label xml:lang="en">ballad opera</rdfs:label>
    <rdfs:label xml:lang="fr">opéra-ballade</rdfs:label>
    <rdfs:isDefinedBy rdf:resource="http://sparql.cwrc.ca/ontologies/genre-ONTOLOGY_DATE"/>
    <void:inDataset rdf:resource="#datasetdefinition"/>
    <skos:inScheme rdf:resource="#Genre"/>
    <rdf:type rdf:resource="http://www.w3.org/2004/02/skos/core#Concept"/>
  </genre:Genre>
  <genre:Genre rdf:about="#genreBallet">
    <rdf:value>BALLET</rdf:value>
    <rdfs:label xml:lang="en">ballet</rdfs:label>
    <rdfs:label xml:lang="fr">ballet</rdfs:label>
    <rdfs:isDefinedBy rdf:resource="http://sparql.cwrc.ca/ontologies/genre-ONTOLOGY_DATE"/>
    <void:inDataset rdf:resource="#datasetdefinition"/>
    <skos:inScheme rdf:resource="#Genre"/>
    <rdf:type rdf:resource="http://www.w3.org/2004/02/skos/core#Concept"/>
  </genre:Genre>
  <genre:Genre rdf:about="#genreBergamasque">
    <rdf:value>BERGAMASQUE</rdf:value>
    <rdfs:label xml:lang="en">bergamasque</rdfs:label>
    <rdfs:label xml:lang="fr">bergamasque</rdfs:label>
    <rdfs:isDefinedBy rdf:resource="http://sparql.cwrc.ca/ontologies/genre-ONTOLOGY_DATE"/>
    <void:inDataset rdf:resource="#datasetdefinition"/>
    <skos:inScheme rdf:resource="#Genre"/>
    <rdf:type rdf:resource="http://www.w3.org/2004/02/skos/core#Concept"/>
  </genre:Genre>
  <genre:Genre rdf:about="#genreBestiary">
    <rdf:value>BESTIARY</rdf:value>
    <rdfs:label xml:lang="en">bestiary</rdfs:label>
    <rdfs:label xml:lang="fr">bestiaire</rdfs:label>
    <rdfs:isDefinedBy rdf:resource="http://sparql.cwrc.ca/ontologies/genre-ONTOLOGY_DATE"/>
    <void:inDataset rdf:resource="#datasetdefinition"/>
    <skos:inScheme rdf:resource="#Genre"/>
    <rdf:type rdf:resource="http://www.w3.org/2004/02/skos/core#Concept"/>
    <skos:definition xml:lang="en">Collections of moralized fables, especially as written in the Middle Ages, about actual or mythical animals. <![CDATA[<a href="#_getty_2017">(Getty, 2017)</a>]]></skos:definition>
    <skos:definition xml:lang="de">Sammlung moralischer Fabeln, insbesondere solcher, die im Mittelalter über wirkliche oder mythische Tiere verfasst wurden. <![CDATA[<a href="#_getty_2017">(Getty, 2017)</a>]]></skos:definition>
    <skos:definition xml:lang="nl">Verzamelingen moraliserende vertellingen, zoals die in de middeleeuwen veel werden geschreven, over bestaande of mythische dieren. <![CDATA[<a href="#_getty_2017">(Getty, 2017)</a>]]></skos:definition>
    <skos:definition xml:lang="es">Colecciones de fábulas moralizadoras, especialmente como aquellas escritas de la Edad Media, acerca de animales actuales o míticos. <![CDATA[<a href="#_getty_2017">(Getty, 2017)</a>]]></skos:definition>
    <skos:definition xml:lang="zh-hant">描寫真實或虛構的動物，具道德教訓的寓言集，尤指中世紀之著作。 <![CDATA[<a href="#_getty_2017">(Getty, 2017)</a>]]></skos:definition>
    <prov:derivedFrom rdf:resource="http://vocab.getty.edu/aat/300201056"/>
    <rdfs:comment xml:lang="en">The description for this term is indebted to the Getty Art &amp; Architecture Thesaurus.</rdfs:comment>
  </genre:Genre>
  <genre:Genre rdf:about="#genreBiblicalparaphrase">
    <rdf:value>BIBLICALPARAPHRASE</rdf:value>
    <rdfs:label xml:lang="en">biblical paraphrase</rdfs:label>
    <rdfs:label xml:lang="fr">paraphrase biblique </rdfs:label>
    <rdfs:isDefinedBy rdf:resource="http://sparql.cwrc.ca/ontologies/genre-ONTOLOGY_DATE"/>
    <void:inDataset rdf:resource="#datasetdefinition"/>
    <skos:inScheme rdf:resource="#Genre"/>
    <rdf:type rdf:resource="http://www.w3.org/2004/02/skos/core#Concept"/>
  </genre:Genre>
  <genre:Genre rdf:about="#genreBildungsroman">
    <rdf:value>BILDUNGSROMAN</rdf:value>
    <rdfs:label xml:lang="en">bildungsroman</rdfs:label>
    <rdfs:label xml:lang="fr">bildungsroman</rdfs:label>
    <rdfs:isDefinedBy rdf:resource="http://sparql.cwrc.ca/ontologies/genre-ONTOLOGY_DATE"/>
    <void:inDataset rdf:resource="#datasetdefinition"/>
    <skos:inScheme rdf:resource="#Genre"/>
    <rdf:type rdf:resource="http://www.w3.org/2004/02/skos/core#Concept"/>
    <skos:definition xml:lang="fr">Le roman d'apprentissage, appelé aussi roman de formation ou roman d’éducation, est un genre littéraire romanesque né en Allemagne au XVIIIe siècle (à ne pas confondre avec le roman de jeunesse). Il s'oppose cependant à la fonction première du romanesque qui est de nous transporter dans un monde de rêve et d'évasion. On parle ainsi de « roman initiatique » ou de « conte initiatique ». En allemand, le roman de formation est nommé « Bildungsroman ». Ce terme est dû au philologue allemand Johann Carl Simon Morgenstern, qui voyait dans le Bildungsroman « l'essence du roman par opposition au récit épique ». On emploie aussi l'expression « Entwicklungsroman » (roman de développement personnel). Un roman d'apprentissage a pour thème le cheminement évolutif d'un héros, souvent jeune, jusqu'à ce qu'il atteigne l'idéal de l'homme accompli et cultivé. Le héros découvre en général un domaine particulier dans lequel il fait ses armes. Mais en réalité, c'est une conception de la vie en elle-même qu'il se forge progressivement. En effet, derrière l'apprentissage d'un domaine, le jeune héros découvre les grands événements de l'existence (la mort, l'amour, la haine, l'altérité, pour prendre quelques exemples). Ainsi, dans L'Éducation sentimentale (Flaubert, 1869), le jeune Frédéric connaît les premiers émois de l'amour : et réfléchissant sur les sentiments qu'il porte à Mme Arnoux, Frédéric se construit une idée de l'existence. Le roman d'apprentissage est un roman qui décrit la maturation du héros. Il manque d'expérience au départ et traverse des obstacles ou des épreuves afin de mûrir et d'en tirer des leçons. <![CDATA[<a href="#_dbpedia_2017">(DBpedia, 2017)</a>]]></skos:definition>
    <skos:definition xml:lang="es">La novela de formación o novela de aprendizaje es un género literario que retrata la transición de la niñez a la vida adulta. El término alemán original, Bildungsroman () significa literalmente novela de formación o novela de educación y fue acuñado por el filólogo Johann Carl Simon Morgenstern en 1819. La temática de esta novela es la evolución y el desarrollo físico, moral, psicológico y social de un personaje, generalmente desde su infancia hasta la madurez. En esta evolución se suelen diferenciar tres etapas: la primera es el aprendizaje de juventud (&quot;Jugendlehre&quot;), la segunda son los años de peregrinación (&quot;Wanderjahre&quot;) y por último el perfeccionamiento (&quot;Läuterung&quot;). A pesar de que existen rasgos de la novela de aprendizaje en obras clásicas o medievales (en las obras moralizantes, por ejemplo), es plausible situar en el Renacimiento el embrión de este tipo de novela, especialmente en el género picaresco. Por ejemplo, El lazarillo de Tormes muestra el proceso por el que el protagonista, Lázaro, aprende a defenderse en la vida tras sufrir sirviendo a distintos amos abusivos. Convencionalmente se considera que el género surge dentro de la corriente del Romanticismo alemán con Los años de aprendizaje de Wilhelm Meister (Wilhem Meister Lehrjahre, 1795/1796) de Wolfgang Goethe. La traducción al inglés de esta novela, realizada por Thomas Carlyle, contribuyó a expandir este género nacido en Alemania al resto de Europa y luego al resto del mundo. A medida que ha ido avanzando el género, nos podemos encontrar con negativos Bildungsromane en los que se cuentan los fracasos de los personajes como, por ejemplo, en &quot;Anton Reiser&quot; de Karl Philip Moritz y modernos Bildungsromane, como Carta breve para un largo adiós (Der Kurze Brief zum langen Abschied, 1972) de Peter Handke. Muchas de las grandes novelas de los siglos XIX y XX, sin ser estrictamente Bildungsroman, comparten alguna de sus características. Por ejemplo, Marcel Proust en En busca del tiempo perdido narra el proceso de aprendizaje del protagonista, Marcel; lo mismo sucede en Retrato del artista adolescente, de James Joyce, en el Moll Flanders de Defoe o en La montaña mágica, de Thomas Mann. Bajo las ruedas, de Hermann Hesse, es un Bildungsroman en sentido aún más estricto. A pesar de que la novela de aprendizaje parece haber perdido peso desde la segunda mitad del siglo XX, muchos de sus elementos aún perviven en novelas como El guardián entre el centeno de J. D. Salinger o en numerosas películas contemporáneas. La sombra del viento (2001), del barcelonés Carlos Ruiz Zafón, narra el tránsito de la infancia a la madurez de Daniel Sempere a través del misterio y del amor a los libros y podría ser considerado un Bildungsroman del siglo XXI. <![CDATA[<a href="#_dbpedia_2017">(DBpedia, 2017)</a>]]></skos:definition>
    <prov:derivedFrom rdf:resource="http://dbpedia.org/resource/Bildungsroman"/>
    <rdfs:comment xml:lang="en">The description for this term is indebted to DBpedia. </rdfs:comment>
    <rdfs:comment xml:lang="fr">La description de ce terme est basée sur celle de DBPedia.</rdfs:comment>

    <skos:definition xml:lang="en">Novels of a traditional German genre that focuses on the spiritual development or formative years of an individual. Now in broad use to refer to this type of novel written in any language or in any culture. <![CDATA[<a href="#_getty_2017">(Getty, 2017)</a>]]></skos:definition>
    <skos:definition xml:lang="de">Traditionelle deutsche Romanform, bei der das Hauptaugenmerk auf der geistigen Entwicklung oder die prägenden Jahre einer Person liegt. Wird inzwischen weitgehend für diesen Romantypus verwendet, egal in welcher Sprache er geschrieben wurde oder aus welcher Kultur er stammt.  <![CDATA[<a href="#_getty_2017">(Getty, 2017)</a>]]></skos:definition>
    <skos:definition xml:lang="nl">Romans van een traditioneel Duits genre met daarin een beschrijving van de geestelijke ontwikkeling of vormende jaren van een persoon. De term gebruikt men nu in algemene zin voor romans van dit type, ongeacht de betreffende taal of cultuur. <![CDATA[<a href="#_getty_2017">(Getty, 2017)</a>]]></skos:definition>
    <skos:definition xml:lang="zh-hant">傳統德國類型之小說，著重於主角的精神發展或構成的年代。而今廣泛用於指以任何語言或於任何文化背景寫作之此一種類的小說。 <![CDATA[<a href="#_getty_2017">(Getty, 2017)</a>]]></skos:definition>
    <prov:derivedFrom rdf:resource="http://vocab.getty.edu/aat/300297857"/>
    <rdfs:comment xml:lang="en">The description for this term is indebted to the Getty Art &amp; Architecture Thesaurus.</rdfs:comment>
  </genre:Genre>
  <genre:Genre rdf:about="#genreBiographicaldictionary">
    <rdf:value>BIOGRAPHICALDICTIONARY</rdf:value>
    <rdfs:label xml:lang="en">biographical dictionary</rdfs:label>
    <rdfs:label xml:lang="fr"/>
    <rdfs:isDefinedBy rdf:resource="http://sparql.cwrc.ca/ontologies/genre-ONTOLOGY_DATE"/>
    <void:inDataset rdf:resource="#datasetdefinition"/>
    <skos:inScheme rdf:resource="#Genre"/>
    <rdf:type rdf:resource="http://www.w3.org/2004/02/skos/core#Concept"/>
  </genre:Genre>
  <genre:Genre rdf:about="#genreBiography">
    <rdf:value>BIOGRAPHY</rdf:value>
    <rdfs:label xml:lang="en">biography</rdfs:label>
    <rdfs:label xml:lang="fr">biographie </rdfs:label>
    <rdfs:isDefinedBy rdf:resource="http://sparql.cwrc.ca/ontologies/genre-ONTOLOGY_DATE"/>
    <void:inDataset rdf:resource="#datasetdefinition"/>
    <skos:inScheme rdf:resource="#Genre"/>
    <rdf:type rdf:resource="http://www.w3.org/2004/02/skos/core#Concept"/>
    <skos:definition xml:lang="en">Brief profiles of a people's life or work. <![CDATA[<a href="#_getty_2017">(Getty, 2017)</a>]]></skos:definition>
    <prov:derivedFrom rdf:resource="http://vocab.getty.edu/aat/300404015"/>
    <rdfs:comment xml:lang="en">The description for this term is indebted to the Getty Art &amp; Architecture Thesaurus.</rdfs:comment>
    <skos:definition xml:lang="fr">Une biographie (une bio), du grec ancien βίος, « la vie » et γραφή, « écrire », est un écrit qui a pour objet l'histoire d'une vie particulière. Elle peut être écrite par la personne elle-même (autobiographie) ou par une autre personne. <![CDATA[<a href="#_dbpedia_2017">(DBpedia, 2017)</a>]]></skos:definition>
    <skos:definition xml:lang="de">Eine Biografie, auch Biographie (griechisch βιογραφία, von βίος, bíos „Leben“ und -graphie von γράφω, gráphō „ritzen, malen, schreiben“) ist die Lebensbeschreibung einer Person. Die Biografie ist die mündliche oder schriftliche Präsentation des Lebenslaufes eines anderen Menschen; ein Sonderfall der Biografie ist die Autobiografie: Sie hat der Betreffende selbst (heute allerdings häufig mit der Unterstützung eines Ghostwriters) über seine eigenen Lebenserfahrungen verfasst. Im Familienverbund werden Autobiografien manchmal dem Testament beigefügt. Es soll vom Leben eine Spur übrig bleiben – die Nachkommen sollen wissen, was war. Den Lebenslauf zu beschreiben, bedeutete auch eine nachträgliche Konstruktion einer bestimmten Sinnhaftigkeit des beschriebenen Lebens. Dies führt weiter zur Frage nach dem subjektiv verstandenen und dem objektiven Leben. Jeder Mensch entwirft seine eigene Biografie in unterschiedlichen Lebenssituationen (beim Bewerbungsgespräch, bei der Aufnahme persönlicher Beziehungen oder allgemeiner bei der eigenen Lebensrückschau, z. B. beim Psychologen oder Psychiater). Biografien bilden auch ein wichtiges Instrument der Erinnerung an andere Personen. Sie sind daher Gegenstand der Literatur- und Geschichtswissenschaft, der Soziologie, der Pädagogik, der Psychologie, der Medizin und der Theologie. Die einzelnen Arbeitsfelder und Arbeitsgegenstände der Biografieforschung sind sehr heterogen und haben eigene Forschungstraditionen entwickelt. <![CDATA[<a href="#_dbpedia_2017">(DBpedia, 2017)</a>]]></skos:definition>
    <skos:definition xml:lang="es">La biografía (del griego βίος [bíos], ‘vida’ y γράφειν [grafein], ‘escribir’) es la historia de la vida de una persona narrada desde su nacimiento hasta su muerte, consignando sus hechos logrados, fracasos, sucesos relevantes de su vida, así como todo lo que pueda interesar de la misma. <![CDATA[<a href="#_dbpedia_2017">(DBpedia, 2017)</a>]]></skos:definition>
    <skos:definition xml:lang="nl">Een biografie (Grieks: βιος leven) is een op schrift gestelde (en doorgaans gepubliceerde) levensbeschrijving van een persoon. De term wordt meestal gebruikt voor non-fictie, dat wil zeggen werken waarin iemand het werkelijke leven van een werkelijk bestaand, veelal beroemd, persoon probeert te beschrijven. Een biografie is wel verhalend en probeert op die manier een beter inzicht te geven in de persoonlijkheid en karakter van de beschreven persoon dan een droge opsomming van feiten zou doen. Een biografie van een heilige heet een hagiografie. Deze term wordt ook gebruikt als de schrijver zijn onderwerp onkritisch behandelt. Als de schrijver van een biografie ook het onderwerp van de biografie is, heet dit een autobiografie. <![CDATA[<a href="#_dbpedia_2017">(DBpedia, 2017)</a>]]></skos:definition>
    <prov:derivedFrom rdf:resource="http://dbpedia.org/resource/Biography"/>
    <rdfs:comment xml:lang="en">The description for this term is indebted to DBpedia. </rdfs:comment>
    <rdfs:comment xml:lang="fr">La description de ce terme est basée sur celle de DBPedia.</rdfs:comment>

    <skos:definition xml:lang="en">The genre of nonfiction that concerns accounts of the lives of individuals. For examples of this genre, prefer &quot;biographies (documents).&quot; <![CDATA[<a href="#_getty_2017">(Getty, 2017)</a>]]></skos:definition>
    <skos:definition xml:lang="es">El género de no ficción que compete a narraciones escritas de la vida de individuos. <![CDATA[<a href="#_getty_2017">(Getty, 2017)</a>]]></skos:definition>
    <skos:definition xml:lang="nl">Het non-fictie genre dat zich bezighoudt met geschreven beschrijvingen van het leven van een persoon. <![CDATA[<a href="#_getty_2017">(Getty, 2017)</a>]]></skos:definition>
    <skos:definition xml:lang="zh-hant">關於個人生活之非小說類型。 <![CDATA[<a href="#_getty_2017">(Getty, 2017)</a>]]></skos:definition>
    <prov:derivedFrom rdf:resource="http://vocab.getty.edu/aat/300055908"/>
    <rdfs:comment xml:lang="en">The description for this term is indebted to the Getty Art &amp; Architecture Thesaurus.</rdfs:comment>
  </genre:Genre>
  <genre:Genre rdf:about="#genreBisexualfiction">
    <rdf:value>BISEXUALFICTION</rdf:value>
    <rdfs:label xml:lang="en">bisexual fiction</rdfs:label>
    <rdfs:label xml:lang="fr"/>
    <rdfs:isDefinedBy rdf:resource="http://sparql.cwrc.ca/ontologies/genre-ONTOLOGY_DATE"/>
    <void:inDataset rdf:resource="#datasetdefinition"/>
    <skos:inScheme rdf:resource="#Genre"/>
    <rdf:type rdf:resource="http://www.w3.org/2004/02/skos/core#Concept"/>
  </genre:Genre>
  <genre:Genre rdf:about="#genreBlackcomedy">
    <rdf:value>BLACKCOMEDY</rdf:value>
    <rdfs:label xml:lang="en">black comedy</rdfs:label>
    <rdfs:label xml:lang="fr">humour noir</rdfs:label>
    <rdfs:isDefinedBy rdf:resource="http://sparql.cwrc.ca/ontologies/genre-ONTOLOGY_DATE"/>
    <void:inDataset rdf:resource="#datasetdefinition"/>
    <skos:inScheme rdf:resource="#Genre"/>
    <rdf:type rdf:resource="http://www.w3.org/2004/02/skos/core#Concept"/>
    <skos:definition xml:lang="en">A black comedy (or dark comedy) is a comic work that employs morbid humor, which, in its simplest form, is humor that makes light of subject matter usually considered taboo. Black humor corresponds to the earlier concept of gallows humor. Black comedy is often controversial due to its subject matter. <![CDATA[<a href="#_dbpedia_2017">(DBpedia, 2017)</a>]]></skos:definition>
    <skos:definition xml:lang="fr">L’humour noir est une forme d’humour qui souligne avec cruauté, amertume et parfois désespoir l’absurdité du monde, face à laquelle il constitue quelques fois une forme de défense. <![CDATA[<a href="#_dbpedia_2017">(DBpedia, 2017)</a>]]></skos:definition>
    <skos:definition xml:lang="de">Als schwarzer Humor wird Humor bezeichnet, der Verbrechen, Krankheit, Tod und ähnliche Themen, für die gewöhnlich eine Abhandlung in ernster Form erwartet wird, in satirischer oder bewusst verharmlosender Weise verwendet. Oft bezieht er sich auf Zeitthemen. Schwarzer Humor bedient sich häufig paradoxer Stilfiguren. Nicht selten löst er Kontroversen aus darüber, ob man sich über die genannten Dinge lustig machen dürfe und wo die Grenzen des guten Geschmacks lägen; besonders ist dies der Fall, wenn religiöse und sexuelle Themen und tragische Ereignisse zum Gegenstand genommen werden. In der darstellenden Kunst nennt man auf schwarzen Humor setzende Werke schwarze Komödien. <![CDATA[<a href="#_dbpedia_2017">(DBpedia, 2017)</a>]]></skos:definition>
    <skos:definition xml:lang="es">El humor negro es un tipo de humor que se ejerce a propósito de cosas que suscitarían, contempladas desde otra perspectiva, piedad, terror, lástima o emociones parecidas. Cuestiona situaciones sociales que generalmente son serias mediante la sátira. El asunto más recurrente en el humor negro es la muerte y todo lo que está relacionado con ella. Atañe los temas más oscuros y dolorosos para el ser humano y que, por norma general, suelen resultar controvertidos y polémicos para la sociedad porque están relacionados con la moral. Algunos ejemplos pueden ser: las grandes tragedias, las normas sociales, la sexualidad, los asesinatos, el suicidio, las enfermedades, la pobreza, la locura, el terrorismo, el racismo, la drogadicción, la violación, las discapacidades, la guerra, la religión, la política, la discriminación, etc., pero representados en forma cómica. <![CDATA[<a href="#_dbpedia_2017">(DBpedia, 2017)</a>]]></skos:definition>
    <skos:definition xml:lang="nl">Zwarte humor is een vorm van humor, gebaseerd op het leed van anderen met als doel te spotten en te amuseren. Hierbij is er een zekere overeenkomst met het (psychologisch) cynisme, waarbij een negatieve houding tegenover (een deel van) de maatschappij tot uiting komt. Vaak wordt deze, meestal overdreven, vorm van humor gebruikt om het leed te relativeren of een reactie bij de toeschouwer te ontlokken. Zwarte humor draait vaak rond taboe-onderwerpen die over het algemeen erg gevoelig liggen bij de meeste mensen, zoals dood, geweld, ziekte, moord, zelfmoord, natuurrampen, ongevallen, handicaps, drugs, mishandeling, hongersnood, armoede, kindermisbruik, verkrachting, racisme, discriminatie, genocide, de holocaust en de Tweede Wereldoorlog. In normale omstandigheden wordt humor rond deze deprimerende thema's afgekeurd of bijzonder smakeloos gevonden. Veel mensen die gebruikmaken van zwarte humor proberen hun publiek hiermee dan ook ongemakkelijk te maken of te choqueren. Op het juiste moment en in de juiste omstandigheden kan deze vorm van humor echter ook helpen om spanningen weg te nemen of het leed te relativeren. Doordat echter elk individu zijn eigen morele en ethische grenzen heeft is de reactie bij het publiek niet altijd in te schatten. <![CDATA[<a href="#_dbpedia_2017">(DBpedia, 2017)</a>]]></skos:definition>
    <prov:derivedFrom rdf:resource="http://dbpedia.org/resource/Black_comedy"/>
    <rdfs:comment xml:lang="en">The description for this term is indebted to DBpedia. </rdfs:comment>
    <rdfs:comment xml:lang="fr">La description de ce terme est basée sur celle de DBPedia.</rdfs:comment>

  </genre:Genre>
  <genre:Genre rdf:about="#genreBoutsrimes">
    <rdf:value>BOUTSRIMES</rdf:value>
    <rdfs:label xml:lang="en">bouts-rimés</rdfs:label>
    <rdfs:label xml:lang="fr">bout-rimé</rdfs:label>
    <rdfs:isDefinedBy rdf:resource="http://sparql.cwrc.ca/ontologies/genre-ONTOLOGY_DATE"/>
    <void:inDataset rdf:resource="#datasetdefinition"/>
    <skos:inScheme rdf:resource="#Genre"/>
    <rdf:type rdf:resource="http://www.w3.org/2004/02/skos/core#Concept"/>
  </genre:Genre>
  <genre:Genre rdf:about="#genreBroadside">
    <rdf:value>BROADSIDE</rdf:value>
    <rdfs:label xml:lang="en">broadside</rdfs:label>
    <rdfs:label xml:lang="fr"/>
    <rdfs:isDefinedBy rdf:resource="http://sparql.cwrc.ca/ontologies/genre-ONTOLOGY_DATE"/>
    <void:inDataset rdf:resource="#datasetdefinition"/>
    <skos:inScheme rdf:resource="#Genre"/>
    <rdf:type rdf:resource="http://www.w3.org/2004/02/skos/core#Concept"/>
  </genre:Genre>
  <genre:Genre rdf:about="#genreBurletta">
    <rdf:value>BURLETTA</rdf:value>
    <rdfs:label xml:lang="en">burletta</rdfs:label>
    <rdfs:label xml:lang="fr">burletta</rdfs:label>
    <rdfs:isDefinedBy rdf:resource="http://sparql.cwrc.ca/ontologies/genre-ONTOLOGY_DATE"/>
    <void:inDataset rdf:resource="#datasetdefinition"/>
    <skos:inScheme rdf:resource="#Genre"/>
    <rdf:type rdf:resource="http://www.w3.org/2004/02/skos/core#Concept"/>
  </genre:Genre>
  <genre:Genre rdf:about="#genreCabaret">
    <rdf:value>CABARET</rdf:value>
    <rdfs:label xml:lang="en">cabaret</rdfs:label>
    <rdfs:label xml:lang="fr">cabaret</rdfs:label>
    <rdfs:isDefinedBy rdf:resource="http://sparql.cwrc.ca/ontologies/genre-ONTOLOGY_DATE"/>
    <void:inDataset rdf:resource="#datasetdefinition"/>
    <skos:inScheme rdf:resource="#Genre"/>
    <rdf:type rdf:resource="http://www.w3.org/2004/02/skos/core#Concept"/>
  </genre:Genre>
  <genre:Genre rdf:about="#genreCaptivitynarrative">
    <rdf:value>CAPTIVITYNARRATIVE</rdf:value>
    <rdfs:label xml:lang="en">captivity narrative</rdfs:label>
    <rdfs:label xml:lang="fr">récit de captivité</rdfs:label>
    <rdfs:isDefinedBy rdf:resource="http://sparql.cwrc.ca/ontologies/genre-ONTOLOGY_DATE"/>
    <void:inDataset rdf:resource="#datasetdefinition"/>
    <skos:inScheme rdf:resource="#Genre"/>
    <rdf:type rdf:resource="http://www.w3.org/2004/02/skos/core#Concept"/>
    <skos:definition xml:lang="en">Captivity narratives are usually stories of people captured by enemies whom they consider uncivilized, or whose beliefs and customs they oppose. The best-known captivity narratives are those concerning the indigenous peoples of North America. These narratives (and questions about their accuracy) have an enduring place in literature, history, ethnography, and the study of Native peoples. However, captivity narratives have also come to play a major role in the study of contemporary religious movements, thanks to scholars of religion like David G. Bromley and James R. Lewis. In this article, both main types of captivity narratives are considered. Traditionally, historians have made limited use of certain captivity narratives. They have regarded the genre with suspicion because of its ideological underpinnings. As a result of new scholarly approaches, historians with a more certain grasp of Native American cultures are distinguishing between plausible statements of fact and value-laden judgements in order to study the narratives as rare sources from &quot;inside&quot; Native societies. Contemporary historians such as Linda Colley and anthropologists such as Pauline Turner Strong have also found the narratives useful in analyzing how the colonists constructed the &quot;other&quot;, as well as what the narratives reveal about the settlers' sense of themselves and their culture, and the experience of crossing the line to another. Colley has studied the long history of English captivity in other cultures, both the Barbary pirate captives who preceded those in North America, and British captives in cultures such as India, after the North American experience. Certain North American captivity narratives involving Native peoples were published from the 18th through the 19th centuries, but they reflected a well-established genre in English literature. There had already been English accounts of captivity by Barbary pirates, or in the Middle East, which established some of the major elements of the form. Following the American experience, additional accounts were written after British people were captured during exploration and settlement in India and East Asia. Other types of captivity narratives, such as those recounted by apostates from religious movements (i.e. &quot;cult survivor&quot; tales), have remained an enduring feature of modern media, and currently appear in books, periodicals, film, and television. The unifying factor in most captivity narratives, whether they stem from geopolitical or religious conflicts, is that the captive portrays the captors' way of life as alien, undesirable, and incompatible with the captive's own (typically dominant) culture. This underscores the utility of captivity narratives in garnering support for social control measures, such as removing Native Americans to &quot;reservations&quot;, or stigmatizing participation in religious movements – whether Catholicism in the nineteenth century, or ISKCON in the twentieth. Captivity narratives tend to be culturally chauvinistic, viewing an &quot;alien&quot; culture through the lens of the narrator's preferred culture, thus making (possibly unfair) value judgements like &quot;Puritans good, Indians bad.&quot; <![CDATA[<a href="#_dbpedia_2017">(DBpedia, 2017)</a>]]></skos:definition>
    <skos:definition xml:lang="de">Der Ausdruck captivity narrative bezeichnet ein eigenständiges Genre der amerikanischen Literatur, das die Erfahrungen weißer Siedler in Nordamerika, zumeist Frauen, in indianischer Gefangenschaft schildert. Captivity narratives hatten im 17. Jahrhundert einen erheblichen Einfluss sowohl auf die autobiografische Literatur als auch später auf den amerikanischen Roman. Bekannt in diesem Zusammenhang wurden u.a. die Schicksale von Mary Rowlandson (1637–1711), Elizabeth Hanson (1684–1737) oder Cynthia Ann Parker (1826–1870). <![CDATA[<a href="#_dbpedia_2017">(DBpedia, 2017)</a>]]></skos:definition>
    <prov:derivedFrom rdf:resource="http://dbpedia.org/resource/Captivity_narrative"/>
    <rdfs:comment xml:lang="en">The description for this term is indebted to DBpedia. </rdfs:comment>
  </genre:Genre>
  <genre:Genre rdf:about="#genreCatechism">
    <rdf:value>CATECHISM</rdf:value>
    <rdfs:label xml:lang="en">catechism</rdfs:label>
    <rdfs:label xml:lang="fr">catéchisme</rdfs:label>
    <rdfs:isDefinedBy rdf:resource="http://sparql.cwrc.ca/ontologies/genre-ONTOLOGY_DATE"/>
    <void:inDataset rdf:resource="#datasetdefinition"/>
    <skos:inScheme rdf:resource="#Genre"/>
    <rdf:type rdf:resource="http://www.w3.org/2004/02/skos/core#Concept"/>
    <skos:definition xml:lang="en">A catechism (/ˈkætəˌkizəm/; from Greek: κατηχέω, to teach orally), is a summary or exposition of doctrine and served as a learning introduction to the Sacraments traditionally used in catechesis, or Christian religious teaching of children and adult converts. Catechisms are doctrinal manuals - often in the form of questions followed by answers to be memorised - a format in non-religious or secular contexts as well. The term catechumen refers to the designated recipient of the catechetical work or instruction. In the Catholic Church, catachumens were usually placed separately during Holy Mass from those who received the Sacrament of Baptism. Early catecheticals emerged from Graeco-Roman mystery religions, especially the late cult of Mithras meant to educate their members into the secretive teachings, which competed with the Christian Church as an underground religion in the 1st to 4th centuries CE and allegedly shared its many ritual practices. Today, they are characteristic of Western Christianity but are also present in Eastern Christianity. <![CDATA[<a href="#_dbpedia_2017">(DBpedia, 2017)</a>]]></skos:definition>
    <skos:definition xml:lang="fr">Dans la religion chrétienne, le catéchisme désigne l'instruction des doctrines de la foi chrétienne, particulièrement destinée aux enfants. Il prend souvent la forme d'une exposé officiel des articles de la foi, servant d'outil de base pour la catéchèse, qui est l'ensemble des actions destinées à éduquer des enfants, des jeunes et des adultes à la doctrine chrétienne. La catéchèse est une des composantes de la mission évangélique du christianisme. <![CDATA[<a href="#_dbpedia_2017">(DBpedia, 2017)</a>]]></skos:definition>
    <skos:definition xml:lang="de">Der Katechismus ist seit dem Beginn der Neuzeit ein Handbuch der Unterweisung in den Grundfragen des christlichen Glaubens. Mit dem Wort Katechismus wurde auch die Taufkatechese für die Erwachsenen und seit der Einführung der Kindertaufe das Glaubensexamen der Taufpaten bezeichnet. <![CDATA[<a href="#_dbpedia_2017">(DBpedia, 2017)</a>]]></skos:definition>
    <skos:definition xml:lang="es">El catecismo (del griego κατηχισμός, de kata [«abajo»] + echein [«sonar»], literalmente «sonar abajo» (dentro de los oídos), es decir, «adoctrinar») es el texto en el que se presenta una exposición orgánica y sintética de los contenidos esenciales y fundamentales de la doctrina cristiana tanto sobre la fe como sobre la moral. A lo largo de la historia han existido diversos tipos de catecismos, y la mayoría de iglesias y denominaciones cristianas cuentan con sus propias ediciones. En el caso de la Iglesia católica, sus catecismos se basan principalmente en la Tradición de la Iglesia interpretada a la luz del Concilio Vaticano II. Sus fuentes principales son la Sagrada Escritura, los Santos Padres, la Liturgia y el Magisterio de la Iglesia. Está destinado a servir &quot;como un punto de referencia para los catecismos o compendios que sean compuestos en los diversos países&quot; (Sínodo de los Obispos 1985. Relación final II B A 4). Existe una versión in extenso promulgada el 11 de octubre de 1992 por Juan Pablo II y el Compendio, promulgado por el Papa Benedicto XVI el 28 de junio de 2005, que es una síntesis fiel y segura del Catecismo de la Iglesia católica. Contiene, de modo conciso, todos los elementos esenciales y fundamentales de la fe de la Iglesia, de manera tal que constituye, de acuerdo a lo descrito en su presentación por el Papa &quot;una especie de vademécum, a través del cual las personas, creyentes o no, pueden abarcar con una sola mirada de conjunto el panorama completo de la fe católica&quot;. <![CDATA[<a href="#_dbpedia_2017">(DBpedia, 2017)</a>]]></skos:definition>
    <skos:definition xml:lang="nl">Een catechismus (van het Griekse: Κατήχησις, katechesis = onderricht) is een opsomming van de leer van een bepaald kerkgenootschap waarin al zijn dogma's systematisch en voor leken begrijpelijk worden gegeven en uitgelegd. Omdat ze een middel zijn bij de catechese, worden ze vaak in vraag- en antwoordvorm uitgegeven. <![CDATA[<a href="#_dbpedia_2017">(DBpedia, 2017)</a>]]></skos:definition>
    <prov:derivedFrom rdf:resource="http://dbpedia.org/resource/Catechism"/>
    <rdfs:comment xml:lang="en">The description for this term is indebted to DBpedia. </rdfs:comment>
    <rdfs:comment xml:lang="fr">La description de ce terme est basée sur celle de DBPedia.</rdfs:comment>

    <skos:definition xml:lang="en">Manuals or guides for instructing through a series of questions and answers, especially for religious instruction. <![CDATA[<a href="#_getty_2017">(Getty, 2017)</a>]]></skos:definition>
    <skos:definition xml:lang="de">Handbuch oder Leitfaden, der durch Fragen und Antworten lehrreich ist, insbesondere für die religiöse Unterweisung. <![CDATA[<a href="#_getty_2017">(Getty, 2017)</a>]]></skos:definition>
    <skos:definition xml:lang="nl">Handboeken of richtsnoeren voor onderwijs aan de hand van een reeks vragen en antwoorden, met name voor religieus onderwijs. <![CDATA[<a href="#_getty_2017">(Getty, 2017)</a>]]></skos:definition>
    <skos:definition xml:lang="es">Manuales o guías para instruir a través de una serie de preguntas y respuestas, especialmente para instrucción religiosa. <![CDATA[<a href="#_getty_2017">(Getty, 2017)</a>]]></skos:definition>
    <skos:definition xml:lang="zh-hant">藉由一系列問題與答案來教學的手冊或指南，尤其是宗教教育。 <![CDATA[<a href="#_getty_2017">(Getty, 2017)</a>]]></skos:definition>
    <prov:derivedFrom rdf:resource="http://vocab.getty.edu/aat/300026460"/>
    <rdfs:comment xml:lang="en">The description for this term is indebted to the Getty Art &amp; Architecture Thesaurus.</rdfs:comment>
  </genre:Genre>
  <genre:Genre rdf:about="#genreChapbook">
    <rdf:value>CHAPBOOK</rdf:value>
    <rdfs:label xml:lang="en">chapbook</rdfs:label>
    <rdfs:label xml:lang="fr">chapbook</rdfs:label>
    <rdfs:isDefinedBy rdf:resource="http://sparql.cwrc.ca/ontologies/genre-ONTOLOGY_DATE"/>
    <void:inDataset rdf:resource="#datasetdefinition"/>
    <skos:inScheme rdf:resource="#Genre"/>
    <rdf:type rdf:resource="http://www.w3.org/2004/02/skos/core#Concept"/>
    <skos:definition xml:lang="en">Small books or pamphlets, usually cheaply printed and containing such texts as popular tales, treatises, ballads, or nursery rhymes, formerly peddled by chapmen. <![CDATA[<a href="#_getty_2017">(Getty, 2017)</a>]]></skos:definition>
    <skos:definition xml:lang="de">Kleines Buch oder Broschüre, in der Regel kostengünstig gedruckt. Es enthält Texte wie Volksmärchen, Abhandlungen, Balladen oder Kinderreime, die früher von Hausierern verbreitet wurden. <![CDATA[<a href="#_getty_2017">(Getty, 2017)</a>]]></skos:definition>
    <skos:definition xml:lang="nl">Kleine boeken of pamfletten, meestal goedkoop gedrukt en met teksten als volksverhalen, verhandelingen, ballades of kinderversjes, vroeger gevent door marskramers. <![CDATA[<a href="#_getty_2017">(Getty, 2017)</a>]]></skos:definition>
    <skos:definition xml:lang="es">Libros pequeños o folletos, generalmente de impresión barata y conteniendo textos tales como cuentos populares, tratados, baladas o rimas infantiles, anteriormente vendidos por vendedores ambulantes. <![CDATA[<a href="#_getty_2017">(Getty, 2017)</a>]]></skos:definition>
    <skos:definition xml:lang="zh-hant">小本書或小冊子，通常為廉價印刷，內容為受歡迎的故事、論文、民謠，或童謠等，從前由小販沿街叫賣。 <![CDATA[<a href="#_getty_2017">(Getty, 2017)</a>]]></skos:definition>
    <prov:derivedFrom rdf:resource="http://vocab.getty.edu/aat/300152367"/>
    <rdfs:comment xml:lang="en">The description for this term is indebted to the Getty Art &amp; Architecture Thesaurus.</rdfs:comment>
  </genre:Genre>
  <genre:Genre rdf:about="#genreCharacter">
    <rdf:value>CHARACTER</rdf:value>
    <rdfs:label xml:lang="en">character</rdfs:label>
    <rdfs:label xml:lang="fr">personnage</rdfs:label>
    <rdfs:isDefinedBy rdf:resource="http://sparql.cwrc.ca/ontologies/genre-ONTOLOGY_DATE"/>
    <void:inDataset rdf:resource="#datasetdefinition"/>
    <skos:inScheme rdf:resource="#Genre"/>
    <rdf:type rdf:resource="http://www.w3.org/2004/02/skos/core#Concept"/>
    <skos:definition xml:lang="en">Any representation of an individual being presented in a dramatic or narrative work through extended dramatic or verbal representation. The reader can interpret characters as endowed with moral and dispositional qualities expressed in what they say (dialogue) and what they do (action). <![CDATA[<a href="#_wheeler_2017">(L. K Wheeler, 2017)</a>]]></skos:definition>
    <prov:derivedFrom rdf:resource="http://web.cn.edu/kwheeler/lit_terms_c.html"/>
    <rdfs:comment xml:lang="en">The description for this term is indebted to Dr. L. Kip Wheeler of Carson-Newman University. </rdfs:comment>
  </genre:Genre>
  <genre:Genre rdf:about="#genreCharade">
    <rdf:value>CHARADE</rdf:value>
    <rdfs:label xml:lang="en">charade</rdfs:label>
    <rdfs:label xml:lang="fr">charade</rdfs:label>
    <rdfs:isDefinedBy rdf:resource="http://sparql.cwrc.ca/ontologies/genre-ONTOLOGY_DATE"/>
    <void:inDataset rdf:resource="#datasetdefinition"/>
    <skos:inScheme rdf:resource="#Genre"/>
    <rdf:type rdf:resource="http://www.w3.org/2004/02/skos/core#Concept"/>
  </genre:Genre>
  <genre:Genre rdf:about="#genreChildrensLiterature">
    <rdf:value>CHILDRENSLITERATURE</rdf:value>
    <rdfs:label xml:lang="en">childrens literature</rdfs:label>
    <rdfs:label xml:lang="fr">littérature pour enfants</rdfs:label>
    <rdfs:isDefinedBy rdf:resource="http://sparql.cwrc.ca/ontologies/genre-ONTOLOGY_DATE"/>
    <void:inDataset rdf:resource="#datasetdefinition"/>
    <skos:inScheme rdf:resource="#Genre"/>
    <rdf:type rdf:resource="http://www.w3.org/2004/02/skos/core#Concept"/>
    <skos:definition xml:lang="en">Literature written and published for children. <![CDATA[<a href="#_getty_2017">(Getty, 2017)</a>]]></skos:definition>
    <skos:definition xml:lang="es">Literatura escrita y publicada para niños. <![CDATA[<a href="#_getty_2017">(Getty, 2017)</a>]]></skos:definition>
    <skos:definition xml:lang="nl">Literatuur die wordt geschreven en uitgegeven voor kinderen. <![CDATA[<a href="#_getty_2017">(Getty, 2017)</a>]]></skos:definition>
    <skos:definition xml:lang="zh-hant">為兒童寫作、出版的文學。 <![CDATA[<a href="#_getty_2017">(Getty, 2017)</a>]]></skos:definition>
    <prov:derivedFrom rdf:resource="http://vocab.getty.edu/aat/300263209"/>
    <rdfs:comment xml:lang="en">The description for this term is indebted to the Getty Art &amp; Architecture Thesaurus.</rdfs:comment>
  </genre:Genre>
  <genre:Genre rdf:about="#genreClerihew">
    <rdf:value>CLERIHEW</rdf:value>
    <rdfs:label xml:lang="en">clerihew</rdfs:label>
    <rdfs:label xml:lang="fr"/>
    <rdfs:isDefinedBy rdf:resource="http://sparql.cwrc.ca/ontologies/genre-ONTOLOGY_DATE"/>
    <void:inDataset rdf:resource="#datasetdefinition"/>
    <skos:inScheme rdf:resource="#Genre"/>
    <rdf:type rdf:resource="http://www.w3.org/2004/02/skos/core#Concept"/>
    <skos:definition xml:lang="en">A clerihew is a whimsical, four-line biographical poem invented by Edmund Clerihew Bentley. The first line is the name of the poem's subject, usually a famous person put in an absurd light. The rhyme scheme is AABB, and the rhymes are often forced. The line length and metre are irregular. Bentley invented the clerihew in school and then popularized it in books. <![CDATA[<a href="#_dbpedia_2017">(DBpedia, 2017)</a>]]></skos:definition>
    <skos:definition xml:lang="de">Ein Clerihew ist ein kurzer scherzhafter pseudobiographischer Vierzeiler, eine Gedichtform, die von Edmund Clerihew Bentley (1875–1956) erfunden wurde. Er besteht aus zwei Reimpaaren mit ungleichmäßiger Länge und mehr oder weniger freiem Rhythmus. Der Name der historischen Person steht dabei meist am Ende der ersten oder der zweiten Verszeile. Der Clerihew ist eher wunderlich und schrullig als satirisch.Die Verszeilen sind auf komische Weise irregulär (unregelmäßige Verslänge, unregelmäßiger – nicht aber freier – Rhythmus). <![CDATA[<a href="#_dbpedia_2017">(DBpedia, 2017)</a>]]></skos:definition>
    <skos:definition xml:lang="nl">De clerihew is een zogenaamd light verse (gedicht) bedacht door Edmund Clerihew Bentley (1875-1956). De volgende regels zijn van toepassing op een clerihew: Voorbeeld in het Engels:Our art teacher, Mr. Shaw, Really knows how to draw. But his awful paintings Have caused many faintings. Voorbeeld van Drs. P:Karel IXWou dat het koppen regendeToen de Bartolomeusnacht werd afgeflotenZei hij zelfs: Ik heb (Hu!) genoten! <![CDATA[<a href="#_dbpedia_2017">(DBpedia, 2017)</a>]]></skos:definition>
    <prov:derivedFrom rdf:resource="http://dbpedia.org/resource/Clerihew"/>
    <rdfs:comment xml:lang="en">The description for this term is indebted to DBpedia. </rdfs:comment>
  </genre:Genre>
  <genre:Genre rdf:about="#genreClosetdrama">
    <rdf:value>CLOSETDRAMA</rdf:value>
    <rdfs:label xml:lang="en">closetdrama</rdfs:label>
    <rdfs:label xml:lang="fr">pièce en chambre</rdfs:label>
    <rdfs:isDefinedBy rdf:resource="http://sparql.cwrc.ca/ontologies/genre-ONTOLOGY_DATE"/>
    <void:inDataset rdf:resource="#datasetdefinition"/>
    <skos:inScheme rdf:resource="#Genre"/>
    <rdf:type rdf:resource="http://www.w3.org/2004/02/skos/core#Concept"/>
  </genre:Genre>
  <genre:Genre rdf:about="#genreColouringbook">
    <rdf:value>COLOURINGBOOK</rdf:value>
    <rdfs:label xml:lang="en">colouring book</rdfs:label>
    <rdfs:label xml:lang="fr">livre de coloriage</rdfs:label>
    <rdfs:isDefinedBy rdf:resource="http://sparql.cwrc.ca/ontologies/genre-ONTOLOGY_DATE"/>
    <void:inDataset rdf:resource="#datasetdefinition"/>
    <skos:inScheme rdf:resource="#Genre"/>
    <rdf:type rdf:resource="http://www.w3.org/2004/02/skos/core#Concept"/>
    <skos:definition xml:lang="en">Books containing outline drawings, for coloring in with crayons, watercolor, colored pencils, or other media, usually intended for use by children. <![CDATA[<a href="#_getty_2017">(Getty, 2017)</a>]]></skos:definition>
    <skos:definition xml:lang="de">Buch mit Umrisszeichnungen zum farbigen Ausmalen mit Wachsstiften, Wasserfarben, Buntstiften oder anderen Medien, in der Regel für Kinder gedacht. <![CDATA[<a href="#_getty_2017">(Getty, 2017)</a>]]></skos:definition>
    <skos:definition xml:lang="nl">Boeken met omtrektekeningen die kunnen worden ingekleurd met tekenstiften, aquarelverf, kleurpotloden of andere middelen, gewoonlijk bedoeld voor kinderen. <![CDATA[<a href="#_getty_2017">(Getty, 2017)</a>]]></skos:definition>
    <skos:definition xml:lang="es">Libros que contienen dibujos de contornos, para ser coloreados con lápices de cera, acuarelas, lápices de colores, u otros medios, generalmente destinados a niños. <![CDATA[<a href="#_getty_2017">(Getty, 2017)</a>]]></skos:definition>
    <skos:definition xml:lang="zh-hant">內含圖畫輪廓的書本，可用蠟筆、水彩、彩色鉛筆、或其他材料，加以著色，使用對象通常為兒童。 <![CDATA[<a href="#_getty_2017">(Getty, 2017)</a>]]></skos:definition>
    <prov:derivedFrom rdf:resource="http://vocab.getty.edu/aat/300026449"/>
    <rdfs:comment xml:lang="en">The description for this term is indebted to the Getty Art &amp; Architecture Thesaurus.</rdfs:comment>
  </genre:Genre>
  <genre:Genre rdf:about="#genreComedy">
    <rdf:value>COMEDY</rdf:value>
    <rdfs:label xml:lang="en">comedy</rdfs:label>
    <rdfs:label xml:lang="fr">comédie</rdfs:label>
    <rdfs:isDefinedBy rdf:resource="http://sparql.cwrc.ca/ontologies/genre-ONTOLOGY_DATE"/>
    <void:inDataset rdf:resource="#datasetdefinition"/>
    <skos:inScheme rdf:resource="#Genre"/>
    <rdf:type rdf:resource="http://www.w3.org/2004/02/skos/core#Concept"/>
    <skos:definition xml:lang="en">Genre encompassing forms of theatre, literature, and improvisation with the basic objective to amuse, humor, and induce laughter. In general, it is often contrasted with tragedy and can be applied in the form of social criticism through satire and political or intellectual wit or applied in the form of pure spectacle through farce or burlesque. <![CDATA[<a href="#_getty_2017">(Getty, 2017)</a>]]></skos:definition>
    <skos:definition xml:lang="es">Género que engloba formas de teatro, literatura e improvisación con el objetivo básico de entretener, complacer e inducir a la risa. En general, y es a menudo contrastado con la tragedia, puede ser aplicado en la forma de crítica social o sátira intelectual o aplicado en la forma de espectáculo puro a través de la farsa o parodia. <![CDATA[<a href="#_getty_2017">(Getty, 2017)</a>]]></skos:definition>
    <skos:definition xml:lang="nl">Genre waaronder theater-, literatuur- en improvisatievormen vallen waarvan het belangrijkste doel is mensen te amuseren en aan het lachen te maken. Tragedie wordt in het algemeen vaak ter contrastering gebruikt. Komedie kan een maatschappijkritische vorm krijgen door middel van satire en politieke of intellectuele spitsvondigheid, of kan puur spektakel zijn in de vorm van klucht of burleske. <![CDATA[<a href="#_getty_2017">(Getty, 2017)</a>]]></skos:definition>
    <prov:derivedFrom rdf:resource="http://vocab.getty.edu/aat/300055911"/>
    <rdfs:comment xml:lang="en">The description for this term is indebted to the Getty Art &amp; Architecture Thesaurus.</rdfs:comment>
  </genre:Genre>
  <genre:Genre rdf:about="#genreComedyofintrigue">
    <rdf:value>COMEDYOFINTRIGUE</rdf:value>
    <rdfs:label xml:lang="en">comedy of intrigue</rdfs:label>
    <rdfs:label xml:lang="fr">comédie d'intrigue</rdfs:label>
    <rdfs:isDefinedBy rdf:resource="http://sparql.cwrc.ca/ontologies/genre-ONTOLOGY_DATE"/>
    <void:inDataset rdf:resource="#datasetdefinition"/>
    <skos:inScheme rdf:resource="#Genre"/>
    <rdf:type rdf:resource="http://www.w3.org/2004/02/skos/core#Concept"/>
    <skos:broaderTransitive rdf:resource="#genreComedy"/>
  </genre:Genre>
  <genre:Genre rdf:about="#genreComedyofmanners">
    <rdf:value>COMEDYOFMANNERS</rdf:value>
    <rdfs:label xml:lang="en">comedy of manners</rdfs:label>
    <rdfs:label xml:lang="fr"/>
    <rdfs:isDefinedBy rdf:resource="http://sparql.cwrc.ca/ontologies/genre-ONTOLOGY_DATE"/>
    <void:inDataset rdf:resource="#datasetdefinition"/>
    <skos:inScheme rdf:resource="#Genre"/>
    <rdf:type rdf:resource="http://www.w3.org/2004/02/skos/core#Concept"/>
    <skos:definition xml:lang="en">The comedy of manners is an entertainment form which satirizes the manners and affectations of a social class or of multiple classes, often represented by stereotypical stock characters. For example, the miles gloriosus (&quot;boastful soldier&quot;) in ancient times, the fop and the rake during the English Restoration, or an old person pretending to be young. Restoration comedy is used as a synonym for &quot;comedy of manners&quot;. The plot of the comedy, often concerned with scandal, is generally less important than its witty dialogue. A great writer of comedies of manners was Oscar Wilde, his most famous play being The Importance of Being Earnest. The comedy of manners was first developed in the new comedy of the Ancient Greek playwright Menander. His style, elaborate plots, and stock characters were imitated by the Roman playwrights Plautus and Terence, whose comedies were widely known and copied during the Renaissance. The best-known comedies of manners, however, may well be those of the French playwright Molière, who satirized the hypocrisy and pretension of the ancien régime in such plays as L'École des femmes (The School for Wives, 1662), Le Misanthrope (The Misanthrope, 1666), and most famously Tartuffe (1664). <![CDATA[<a href="#_dbpedia_2017">(DBpedia, 2017)</a>]]></skos:definition>
    <skos:definition xml:lang="fr">La comédie de mœurs est un sous-genre de la comédie qui se développe à partir du XVIe siècle. Y sont dénoncés les travers d'une époque, d'un groupe ou d'une classe sociale, généralement dominante. La comédie de mœurs est souvent caractérisée par une critique sociale qui reste superficielle. Généralement la dimension satirique ne vise qu'un travers particulier ou une convention risible très ciblée de la communauté dépeinte. En ce sens, la comédie de mœurs ne remet souvent rien de fondamental en cause dans la structure sociale ni dans la représentation dominante de l'époque. La critique s'efface vite et devient récupérable par l'ordre en place, comme dans les pièces d'Émile Augier ou d'Alexandre Dumas fils. Cependant, le dénouement peut aussi être impressionnant, comme celui des Affaires sont les affaires du libertaire Octave Mirbeau (1903), parfois qualifié de &quot;shakespearien&quot;. Plusieurs comédies très connues de Molière sont des comédies de mœurs : Les Précieuses ridicules ou encore Les Femmes savantes mais aussi L'École des femmes. Pour Molière, la comédie de mœurs représente un lieu privilégié pour la satire sociale. <![CDATA[<a href="#_dbpedia_2017">(DBpedia, 2017)</a>]]></skos:definition>
    <skos:definition xml:lang="de">Ein Konversationsstück, auch Gesellschaftsstück, ist eine Form der Komödie. Im Vordergrund eines Konversationsstückes steht der geistreiche, witzig-pointierte Dialog. Theaterstücke, die als Konversationsstücke gelten, entstanden vor allem in der zweiten Hälfte des 19. Jahrhunderts, seltener im 20. Jahrhundert in England und Frankreich. Der Literaturwissenschaftler Péter Szondi beschrieb den Begriff, indem er das Konversationsstück als „Rettungsversuch des Dramas durch die Rettung des Dialogs, der allerdings zur bloßen Konvention wird“ charakterisierte. Die Handlung, die in den höheren Gesellschaftskreisen spielt, wird durch von außen kommende Ereignisse vorangetrieben. Themen sind unter anderem das Frauenstimmrecht, die freie Liebe, die Mesalliance oder der Sozialismus. Bedeutende Vertreter des Konversationsstückes sind in Frankreich Eugène Scribe, Victorien Sardou und Sacha Guitry, in Großbritannien Oscar Wilde, George Bernhard Shaw und Thomas Stearns Eliot. Im deutschsprachigen Raum fehlte für die Ausbildung typischer Konversationsstücke weitgehend der gesellschaftliche Hintergrund. Werke von Hermann Bahr und Arthur Schnitzler können dem Genre noch am ehesten zugerechnet werden. Hugo von Hofmannsthal schuf 1921 mit Der Schwierige, wo die inhaltsleere Konversation selbst zum Thema wird, ein Zerrbild des Konversationsstücks. <![CDATA[<a href="#_dbpedia_2017">(DBpedia, 2017)</a>]]></skos:definition>
    <skos:definition xml:lang="es">La comedia de costumbres es un subgénero dramático que describe con ironía y agudeza la vida cotidiana de una época o de una clase social concreta, por lo general la clase media o burguesa. El Diccionario Oxford la describe como &quot;Comedia cuyo asunto principal es la presentación de la forma de conducta de los personajes y la descripción de ambientes de la vida social cotidiana&quot;. Trata siempre de los actos comunes de la vida social ordinaria, tanto en el plano egocéntrico (familia, amistades, centro de trabajo...) como en el sociocéntrico (vida política, relaciones institucionales...). Se halla emparentada con el llamado costumbrismo literario o cuadro de costumbres y se destina a un público que suele ser el mismo que aparece caricaturizado, reflejando la destreza o torpeza con que ciertos personajes siguen las pautas convencionales de comportamiento de su entorno, pautas que pueden ser tan rigurosas o banales moralmente cuanto su público pueda soportar, ya que su crítica social suele ser y de hecho es superficial, no toca a los pilares fundamentales de la sociedad y se suele desvanecer fácilmente. Lope de Vega (El perro del hortelano), Molière (Las preciosas ridículas, La escuela de las mujeres), Manuel Bretón de los Herreros (El pelo de la dehesa) y Jacinto Benavente (Pepa Doncel) destacaron escribiendo este tipo de comedias. La trama suele ser algún romance no permitido o algún otro asunto escandaloso, pero es menos importante que los diálogos ingeniosos, los comentarios punzantes sobre las flaquezas humanas y la atmósfera llena de susceptibilidades de la obra. Lope de Vega, Tirso de Molina, Agustín Moreto y otros dramaturgos del s. XVII español fueron los primeros creadores de este tipo de comedias que fueron imitadas y desarrolladas en el XVIII por los franceses (Molière especialmente) e italianos (Carlo Goldoni, quien la imbricó con la Commedia dell'Arte); en Inglaterra se desarrolló a través de las piezas de William Congreve, Oliver Goldsmith y Richard Brinsley Sheridan, y ya en el XIX con las de Óscar Wilde; en el siglo XX destacan las de Noël Coward. En Francia siguieron el género en el XIX Dumas hijo, Eugène Scribe y Victorien Sardou entre otros y, ya en el siglo XX, Sacha Guitry. <![CDATA[<a href="#_dbpedia_2017">(DBpedia, 2017)</a>]]></skos:definition>
    <prov:derivedFrom rdf:resource="http://dbpedia.org/resource/Comedy_of_manners"/>
    <rdfs:comment xml:lang="en">The description for this term is indebted to DBpedia. </rdfs:comment>
    <skos:broaderTransitive rdf:resource="#genreComedy"/>
  </genre:Genre>
  <genre:Genre rdf:about="#genreComedyofmenace">
    <rdf:value>COMEDYOFMENACE</rdf:value>
    <rdfs:label xml:lang="en">comedy of menace</rdfs:label>
    <rdfs:label xml:lang="fr"/>
    <rdfs:isDefinedBy rdf:resource="http://sparql.cwrc.ca/ontologies/genre-ONTOLOGY_DATE"/>
    <void:inDataset rdf:resource="#datasetdefinition"/>
    <skos:inScheme rdf:resource="#Genre"/>
    <rdf:type rdf:resource="http://www.w3.org/2004/02/skos/core#Concept"/>
    <skos:broaderTransitive rdf:resource="#genreComedy"/>
  </genre:Genre>
  <genre:Genre rdf:about="#genreComicbook">
    <rdf:value>COMICBOOK</rdf:value>
    <rdfs:label xml:lang="en">comicbook</rdfs:label>
    <rdfs:label xml:lang="fr">bande dessinée</rdfs:label> 
    <rdfs:isDefinedBy rdf:resource="http://sparql.cwrc.ca/ontologies/genre-ONTOLOGY_DATE"/>
    <void:inDataset rdf:resource="#datasetdefinition"/>
    <skos:inScheme rdf:resource="#Genre"/>
    <rdf:type rdf:resource="http://www.w3.org/2004/02/skos/core#Concept"/>
    <skos:definition xml:lang="en">Sequence of illustrations containing a story or stories (called &quot;comics,&quot; because some are humorous), often serialized, published in booklet form. <![CDATA[<a href="#_getty_2017">(Getty, 2017)</a>]]></skos:definition>
    <skos:definition xml:lang="de">Abfolge von Bildern, die eine Geschichte oder Geschichten beinhalten (&quot;Comics&quot; genannt, weil manche lustig sind), häufig als Fortsetzungsgeschichte und in Heftform veröffentlicht. <![CDATA[<a href="#_getty_2017">(Getty, 2017)</a>]]></skos:definition>
    <skos:definition xml:lang="nl">Strips die vaak in verschillende delen, in pamfletvorm worden uitgegeven. <![CDATA[<a href="#_getty_2017">(Getty, 2017)</a>]]></skos:definition>
    <skos:definition xml:lang="es">Cómics, a menudo como series, publicados en forma de folletos. <![CDATA[<a href="#_getty_2017">(Getty, 2017)</a>]]></skos:definition>
    <skos:definition xml:lang="zh-hant">以小書冊形式出版的漫畫，常連載刊登。 <![CDATA[<a href="#_getty_2017">(Getty, 2017)</a>]]></skos:definition>
    <prov:derivedFrom rdf:resource="http://vocab.getty.edu/aat/300203177"/>
    <rdfs:comment xml:lang="en">The description for this term is indebted to the Getty Art &amp; Architecture Thesaurus.</rdfs:comment>
  </genre:Genre>
  <genre:Genre rdf:about="#genreComingout">
    <rdf:value>COMINGOUT</rdf:value>
    <rdfs:label xml:lang="en">coming out</rdfs:label>
    <rdfs:label xml:lang="fr"/>
    <rdfs:isDefinedBy rdf:resource="http://sparql.cwrc.ca/ontologies/genre-ONTOLOGY_DATE"/>
    <void:inDataset rdf:resource="#datasetdefinition"/>
    <skos:inScheme rdf:resource="#Genre"/>
    <rdf:type rdf:resource="http://www.w3.org/2004/02/skos/core#Concept"/>
  </genre:Genre>
  <genre:Genre rdf:about="#genreCommonplacebook">
    <rdf:value>COMMONPLACEBOOK</rdf:value>
    <rdfs:label xml:lang="en">common place book</rdfs:label>
    <rdfs:label xml:lang="fr"/>
    <rdfs:isDefinedBy rdf:resource="http://sparql.cwrc.ca/ontologies/genre-ONTOLOGY_DATE"/>
    <void:inDataset rdf:resource="#datasetdefinition"/>
    <skos:inScheme rdf:resource="#Genre"/>
    <rdf:type rdf:resource="http://www.w3.org/2004/02/skos/core#Concept"/>
    <skos:definition xml:lang="en">Books in which noteworthy literary passages, cogent quotations, poems, comments, recipes, prescriptions, and other miscellaneous document types are written. <![CDATA[<a href="#_getty_2017">(Getty, 2017)</a>]]></skos:definition>
    <skos:definition xml:lang="de">Buch, in das bemerkenswerte literarische Passagen, treffende Zitate, Gedichte, Kommentare, Rezepte, Belehrungen und diverse andere Textsorten geschrieben werden. <![CDATA[<a href="#_getty_2017">(Getty, 2017)</a>]]></skos:definition>
    <skos:definition xml:lang="nl">Boeken waarin bijzondere of beroemde passages, citaten, gedichten, commentaren, recepten, voorschriften en allerlei soorten andere documenten bijeen zijn gebracht. <![CDATA[<a href="#_getty_2017">(Getty, 2017)</a>]]></skos:definition>
    <skos:definition xml:lang="es">Libros en los cuales están escritos pasajes literarios dignos de mención, citas válidas, poemas, comentarios, recetas de cocina, de remedios y otros tipos misceláneos de documentos. <![CDATA[<a href="#_getty_2017">(Getty, 2017)</a>]]></skos:definition>
    <skos:definition xml:lang="zh-hant">記錄值得注意的文章段落、名言佳句、詩、評論、食譜、醫療處方、和其他五花八門文件類型的本子。 <![CDATA[<a href="#_getty_2017">(Getty, 2017)</a>]]></skos:definition>
    <prov:derivedFrom rdf:resource="http://vocab.getty.edu/aat/300027093"/>
    <rdfs:comment xml:lang="en">The description for this term is indebted to the Getty Art &amp; Architecture Thesaurus.</rdfs:comment>
  </genre:Genre>
  <genre:Genre rdf:about="#genreCompanion">
    <rdf:value>COMPANION</rdf:value>
    <rdfs:label xml:lang="en">companion</rdfs:label>
    <rdfs:label xml:lang="fr"/>
    <rdfs:isDefinedBy rdf:resource="http://sparql.cwrc.ca/ontologies/genre-ONTOLOGY_DATE"/>
    <void:inDataset rdf:resource="#datasetdefinition"/>
    <skos:inScheme rdf:resource="#Genre"/>
    <rdf:type rdf:resource="http://www.w3.org/2004/02/skos/core#Concept"/>
  </genre:Genre>
  <genre:Genre rdf:about="#genreComputerprogram">
    <rdf:value>COMPUTERPROGRAM</rdf:value>
    <rdfs:label xml:lang="en">computer program</rdfs:label>
    <rdfs:label xml:lang="fr"/>
    <rdfs:isDefinedBy rdf:resource="http://sparql.cwrc.ca/ontologies/genre-ONTOLOGY_DATE"/>
    <void:inDataset rdf:resource="#datasetdefinition"/>
    <skos:inScheme rdf:resource="#Genre"/>
    <rdf:type rdf:resource="http://www.w3.org/2004/02/skos/core#Concept"/>
    <skos:definition xml:lang="en">A compilation of coded instructions or sequence of code that, when run, achieves a certain task in a mechanism, usually a computer. <![CDATA[<a href="#_getty_2017">(Getty, 2017)</a>]]></skos:definition>
    <skos:definition xml:lang="de">Ein Kompilat kodierter Anweisungen oder Codesequenzen, das bei Ausführung innerhalb eines Systems, in der Regel einem Computer, eine bestimmte Aufgabe verrichtet. <![CDATA[<a href="#_getty_2017">(Getty, 2017)</a>]]></skos:definition>
    <skos:definition xml:lang="nl">Een reeks gecodeerde instructies die door een apparaat of mechanisme, gewoonlijk een computer, kunnen worden uitgevoerd zodat ze een bepaalde taak uitvoeren. <![CDATA[<a href="#_getty_2017">(Getty, 2017)</a>]]></skos:definition>
    <prov:derivedFrom rdf:resource="http://vocab.getty.edu/aat/300312188"/>
    <rdfs:comment xml:lang="en">The description for this term is indebted to the Getty Art &amp; Architecture Thesaurus.</rdfs:comment>
  </genre:Genre>
  <genre:Genre rdf:about="#genreConditionofenglandnovel">
    <rdf:value>CONDITIONOFENGLANDNOVEL</rdf:value>
    <rdfs:label xml:lang="en">condition of england novel</rdfs:label>
    <rdfs:label xml:lang="fr"/>
    <rdfs:isDefinedBy rdf:resource="http://sparql.cwrc.ca/ontologies/genre-ONTOLOGY_DATE"/>
    <void:inDataset rdf:resource="#datasetdefinition"/>
    <skos:inScheme rdf:resource="#Genre"/>
    <rdf:type rdf:resource="http://www.w3.org/2004/02/skos/core#Concept"/>
    <skos:broaderTransitive rdf:resource="#genreNovel"/>
  </genre:Genre>
  <genre:Genre rdf:about="#genreConductliterature">
    <rdf:value>CONDUCTLITERATURE</rdf:value>
    <rdfs:label xml:lang="en">conduct literature</rdfs:label>
    <rdfs:label xml:lang="fr"/>
    <rdfs:isDefinedBy rdf:resource="http://sparql.cwrc.ca/ontologies/genre-ONTOLOGY_DATE"/>
    <void:inDataset rdf:resource="#datasetdefinition"/>
    <skos:inScheme rdf:resource="#Genre"/>
    <rdf:type rdf:resource="http://www.w3.org/2004/02/skos/core#Concept"/>
  </genre:Genre>
  <genre:Genre rdf:about="#genreCookbook">
    <rdf:value>COOKBOOK</rdf:value>
    <rdfs:label xml:lang="en">cookbook</rdfs:label>
    <rdfs:label xml:lang="fr"/>
    <rdfs:isDefinedBy rdf:resource="http://sparql.cwrc.ca/ontologies/genre-ONTOLOGY_DATE"/>
    <void:inDataset rdf:resource="#datasetdefinition"/>
    <skos:inScheme rdf:resource="#Genre"/>
    <rdf:type rdf:resource="http://www.w3.org/2004/02/skos/core#Concept"/>
    <skos:definition xml:lang="en">A cookbook (sometimes cookery book in Commonwealth English or cook book) is a kitchen reference publication that typically contains a collection of recipes. Modern versions may also include colorful illustrations and advice on purchasing quality ingredients or making substitutions. Cookbooks can also cover a wide variety of topics, including cooking techniques for the home, recipes and commentary from famous chefs, institutional kitchen manuals, and cultural commentary. <![CDATA[<a href="#_dbpedia_2017">(DBpedia, 2017)</a>]]></skos:definition>
    <skos:definition xml:lang="fr">Un livre de cuisine est un recueil de recettes ou de considérations gastronomiques. <![CDATA[<a href="#_dbpedia_2017">(DBpedia, 2017)</a>]]></skos:definition>
    <skos:definition xml:lang="de">Kochbücher beschreiben in Rezepten die Zubereitung von Speisen. Sie sind grob in drei Kategorien zu unterteilen: Der Begriff „Rezept“ für die Kochanweisung weist auf die Verbindung zwischen Heilkunst und Ernährung hin. Auch in der chemischen Industrie steht „Rezeptur“ für eine Liste chemischer Stoffe zur Bereitung eines anderen chemischen Stoffes. So schrieben Ärzte im alten Griechenland nicht nur Rezepte für Medikamente, sondern auch für Gerichte (Diät). <![CDATA[<a href="#_dbpedia_2017">(DBpedia, 2017)</a>]]></skos:definition>
    <skos:definition xml:lang="es">El libro de cocina (también recetario) es una colección de recetas de cocina elaboradas por un cocinero famoso que suele exponer algunos trucos culinarios y diferentes experiencias personales. Uno de los más antiguos en lengua europea distinta del latín es el Llibre de Sent Soví, del que se conserva un manuscrito de 1313 o antes, pudiendo ser de 1024. También hay otros, como el escrito por Guillaume Tirel (1326 - 1395) durante la Gastronomía de la Edad Media, cuyo alias fue Taillevent. <![CDATA[<a href="#_dbpedia_2017">(DBpedia, 2017)</a>]]></skos:definition>
    <skos:definition xml:lang="nl">In een kookboek vindt men recepten voor de bereiding van voedsel, en informatie over het bereiden van voedsel in het algemeen. Kookboeken worden soms ware bestsellers, zoals de boeken van Jamie Oliver. In een kookboek staan, behalve recepten, informatie over het gebruik van een oven, definities of omschrijvingen van bereidingstechnieken en gewichtstabellen. Kookboeken zijn meestal opgedeeld in verschillende hoofdstukken, die ieder een andere gerechtsoort behandelen (voorgerechten, hoofdgerechten, nagerechten). Westerse kookboeken categoriseren de recepten voor hoofdgerechten meestal op basis van ingrediënten. In Japanse kookboeken worden de gerechten vaak gegroepeerd per kooktechniek (bijvoorbeeld braden, grillen en stomen). <![CDATA[<a href="#_dbpedia_2017">(DBpedia, 2017)</a>]]></skos:definition>
    <prov:derivedFrom rdf:resource="http://dbpedia.org/resource/Cookbook"/>
    <rdfs:comment xml:lang="en">The description for this term is indebted to DBpedia. </rdfs:comment>
    <skos:definition xml:lang="en">Reference publications containing collections of recipes with ancillary content on selection of ingredients or the broader context of the types of cooking presented. Contemporary cookbooks may  focus on cultural or regional themes. <![CDATA[<a href="#_getty_2017">(Getty, 2017)</a>]]></skos:definition>
    <prov:derivedFrom rdf:resource="http://vocab.getty.edu/aat/300026109"/>
    <rdfs:comment xml:lang="en">The description for this term is indebted to the Getty Art &amp; Architecture Thesaurus.</rdfs:comment>
  </genre:Genre>
  <genre:Genre rdf:about="#genreCourtshipfiction">
    <rdf:value>COURTSHIPFICTION</rdf:value>
    <rdfs:label xml:lang="en">courtshipfiction</rdfs:label>
    <rdfs:label xml:lang="fr"/>
    <rdfs:isDefinedBy rdf:resource="http://sparql.cwrc.ca/ontologies/genre-ONTOLOGY_DATE"/>
    <void:inDataset rdf:resource="#datasetdefinition"/>
    <skos:inScheme rdf:resource="#Genre"/>
    <rdf:type rdf:resource="http://www.w3.org/2004/02/skos/core#Concept"/>
  </genre:Genre>
  <genre:Genre rdf:about="#genreCriminology">
    <rdf:value>CRIMINOLOGY</rdf:value>
    <rdfs:label xml:lang="en">criminology</rdfs:label>
    <rdfs:label xml:lang="fr"/>
    <rdfs:isDefinedBy rdf:resource="http://sparql.cwrc.ca/ontologies/genre-ONTOLOGY_DATE"/>
    <void:inDataset rdf:resource="#datasetdefinition"/>
    <skos:inScheme rdf:resource="#Genre"/>
    <rdf:type rdf:resource="http://www.w3.org/2004/02/skos/core#Concept"/>
  </genre:Genre>
  <genre:Genre rdf:about="#genreDedication">
    <rdf:value>DEDICATION</rdf:value>
    <rdfs:label xml:lang="en">dedication</rdfs:label>
    <rdfs:label xml:lang="fr"/>
    <rdfs:isDefinedBy rdf:resource="http://sparql.cwrc.ca/ontologies/genre-ONTOLOGY_DATE"/>
    <void:inDataset rdf:resource="#datasetdefinition"/>
    <skos:inScheme rdf:resource="#Genre"/>
    <rdf:type rdf:resource="http://www.w3.org/2004/02/skos/core#Concept"/>
    <skos:definition xml:lang="en">A short bit of text conventionally appearing before the start of a novel or poem in which the author or poet addresses some individual, invoking his or her gratitude or thanks to that individual. Frequently, the dedication is to a spouse, friend, loved one, child, mentor, or individual who inspired the work. Several of the Inklings dedicated specific fictional works to each other (or in the case of C.S. Lewis, to children of fellow Inklings). Among scholars, one of the most significant types of dedications is a festschrift. A festschrift is a collection of essays or studies in book form, dedicated to a former teacher or professor in his or her advanced age. The individual scholarly writings come from his or her students, who typically collaborate to organize the work and contact the publisher, and they present the collection to the teacher upon its publication. <![CDATA[<a href="#_wheeler_2017">(L. K Wheeler, 2017)</a>]]></skos:definition>
    <prov:derivedFrom rdf:resource="http://web.cn.edu/kwheeler/lit_terms_d.html"/>
    <rdfs:comment xml:lang="en">The description for this term is indebted to Dr. L. Kip Wheeler of Carson-Newman University. </rdfs:comment>
  </genre:Genre>
  <genre:Genre rdf:about="#genreDetective">
    <rdf:value>DETECTIVE</rdf:value>
    <rdfs:label xml:lang="en">detective</rdfs:label>
    <rdfs:label xml:lang="fr">policier</rdfs:label>
    <rdfs:isDefinedBy rdf:resource="http://sparql.cwrc.ca/ontologies/genre-ONTOLOGY_DATE"/>
    <void:inDataset rdf:resource="#datasetdefinition"/>
    <skos:inScheme rdf:resource="#Genre"/>
    <rdf:type rdf:resource="http://www.w3.org/2004/02/skos/core#Concept"/>
    <skos:definition xml:lang="en">Detective fiction is a subgenre of crime fiction and mystery fiction in which an investigator or a detective—either professional or amateur—investigates a crime, often murder.</skos:definition>
    <skos:definition xml:lang="es">Ficción detectivesca o ficción con detectives o detectives en la literatura (en inglés detective fiction) es un subgénero de la novela negra y de la ficción de misterio y de suspense, en el que un investigador (muy a menudo un detective, ya sea profesional o amateur, ya sea o no integrante de las fuerzas oficiales) investiga un determinado crimen, a menudo un asesinato.</skos:definition>
    <prov:derivedFrom rdf:resource="http://dbpedia.org/resource/Detective_fiction"/>
    <skos:definition xml:lang="fr">Le genre policier, ou polar, est un genre caractérisant certaines œuvres narratives et qui se distingue par sa mise en scène d'une énigme que le protagoniste tente de résoudre, souvent par une enquête de police. En ressortent notamment, en littérature le roman policier, au cinéma le film policier et à la télévision la série télévisée policière.</skos:definition>
    <prov:derivedFrom rdf:resource="http://dbpedia.org/resource/Crime_fiction"/>
    <rdfs:comment xml:lang="en">The description for this term is indebted to DBpedia. </rdfs:comment>
  </genre:Genre>
  <genre:Genre rdf:about="#genreDevotional">
    <rdf:value>DEVOTIONAL</rdf:value>
    <rdfs:label xml:lang="en">devotional</rdfs:label>
    <rdfs:label xml:lang="fr">dévotional</rdfs:label>
    <rdfs:isDefinedBy rdf:resource="http://sparql.cwrc.ca/ontologies/genre-ONTOLOGY_DATE"/>
    <void:inDataset rdf:resource="#datasetdefinition"/>
    <skos:inScheme rdf:resource="#Genre"/>
    <rdf:type rdf:resource="http://www.w3.org/2004/02/skos/core#Concept"/>
    <skos:definition xml:lang="en">Christian devotional literature (also called devotionals or Christian living literature) is religious writing that is neither doctrinal nor theological, but designed for individuals to read for their personal edification and spiritual formation. Theologian Karl Holl has suggested that devotional literature came into full development at the time of Pietism during the second half of the 17th century. <![CDATA[<a href="#_dbpedia_2017">(DBpedia, 2017)</a>]]></skos:definition>
    <skos:definition xml:lang="de">Der Begriff Erbauungsliteratur, der erstmals um das 14. Jahrhundert erwähnt wird, beschreibt ursprünglich volksnahe Schriften mit religiöser Motivation. Bei der Erbauungsliteratur handelt es sich nicht um theologische Literatur, da sie keine wissenschaftlichen Diskurse verfolgt und keine dogmatischen Absichten besitzt. Vielmehr war mit den Veränderungen der Neuzeit eine Konzentration auf die Innerlichkeit zu verzeichnen, die sich im Bereich der Religion in der Beobachtung der Frömmigkeit Gestalt schuf. Es handelte sich um eine Anleitung für ein tugendhaftes Leben, die emotional den Geist erbauen sollte. Eine Wurzel hat die Erbauungsliteratur in der Heiligenlegende. Weitere Formen sind Andachtsbuch, Gebetbuch, Stundenbuch oder Sammlungen von Predigten. Erbauungsliteratur war jahrhundertelang weit verbreitet, einzelne Ausgaben wurden sogar über Konfessionsgrenzen hinweg gelesen. Sie trat anfänglich auf in Gestalt religiöser Biografien oder Bekehrungsgeschichten, aber auch in Gestalt von Kirchenliedern, die nicht selten zu diesem Zweck geschaffen wurden. Das 17. Jahrhundert schuf zahlreiche literarisch bedeutende Schriften von bekannten Barockdichtern wie Johann Arndt, Johann Michael Dilherr, Jeremias Drexel, Paul Gerhardt, Johannes Lassenius, Joachim Meichel, Martin Moller, Heinrich Müller und Christian Scriver. Aufgrund der bewussten Schlichtheit der Inhalte wurde der Begriff in späterer Zeit auch negativ wertend gebraucht. Im 19. Jahrhundert verstand man deshalb unter Erbauungsliteratur auch kitschige oder einfältige Literatur. Mit der Industrialisierung des Buchdrucks erwuchs zunächst in den 100.000-fach vertriebenen erbaulichen Traktaten eine eigene Literaturform. Begonnen mit den im angelsächsischen Bereich entstehenden Traktatgesellschaften, verbunden mit dem Aufkommen des Kolportagehandels setzte sich diese Vertriebsform rasch im gesamten europäischen Raum durch. Bahnbrecher des Vertriebs von Erbauungsliteratur im deutschsprachigen Raum waren damals u.a. das Haus Bertelsmann sowie der Christliche Verein im nördlichen Deutschland. Im 19. Jahrhundert wurde Erbauungsliteratur zunehmend durch die Unterhaltungsliteratur verdrängt. <![CDATA[<a href="#_dbpedia_2017">(DBpedia, 2017)</a>]]></skos:definition>
    <prov:derivedFrom rdf:resource="http://dbpedia.org/resource/Christian_devotional_literature"/>
    <rdfs:comment xml:lang="en">The description for this term is indebted to DBpedia. </rdfs:comment>
  </genre:Genre>
  <genre:Genre rdf:about="#genreDialogueofthedead">
    <rdf:value>DIALOGUEOFTHEDEAD</rdf:value>
    <rdfs:label xml:lang="en">dialogue of the dead</rdfs:label>
    <rdfs:label xml:lang="fr"/>
    <rdfs:isDefinedBy rdf:resource="http://sparql.cwrc.ca/ontologies/genre-ONTOLOGY_DATE"/>
    <void:inDataset rdf:resource="#datasetdefinition"/>
    <skos:inScheme rdf:resource="#Genre"/>
    <rdf:type rdf:resource="http://www.w3.org/2004/02/skos/core#Concept"/>
  </genre:Genre>
  <genre:Genre rdf:about="#genreDialogueordebate">
    <rdf:value>DIALOGUEORDEBATE</rdf:value>
    <rdfs:label xml:lang="en">dialogue or debate</rdfs:label>
    <rdfs:label xml:lang="fr"/>
    <rdfs:isDefinedBy rdf:resource="http://sparql.cwrc.ca/ontologies/genre-ONTOLOGY_DATE"/>
    <void:inDataset rdf:resource="#datasetdefinition"/>
    <skos:inScheme rdf:resource="#Genre"/>
    <rdf:type rdf:resource="http://www.w3.org/2004/02/skos/core#Concept"/>
  </genre:Genre>
  <genre:Genre rdf:about="#genreDiary">
    <rdf:value>DIARY</rdf:value>
    <rdfs:label xml:lang="en">diary</rdfs:label>
    <rdfs:label xml:lang="fr"/>
    <rdfs:isDefinedBy rdf:resource="http://sparql.cwrc.ca/ontologies/genre-ONTOLOGY_DATE"/>
    <void:inDataset rdf:resource="#datasetdefinition"/>
    <skos:inScheme rdf:resource="#Genre"/>
    <rdf:type rdf:resource="http://www.w3.org/2004/02/skos/core#Concept"/>
    <skos:definition xml:lang="en">Refers to books containing the daily, personal accounts of the writer's own experiences, attitudes, and observations. Use &quot;journals (accounts)&quot; when referring to an individual's or an organization's account of occurrences or transactions. <![CDATA[<a href="#_getty_2017">(Getty, 2017)</a>]]></skos:definition>
    <skos:definition xml:lang="es">Úsese para libros que contienen los relatos personales diarios de las experiencias, actitudes y observaciones del escritor. Use &quot;jornal (cuenta)&quot; para referirse al relato de los acontecimientos o transacciones de un individuo u organización. <![CDATA[<a href="#_getty_2017">(Getty, 2017)</a>]]></skos:definition>
    <skos:definition xml:lang="nl">Wordt gebruikt voor boeken die het dagelijkse, persoonlijke verslag bevatten van de eigen ervaringen, standpunten en observaties van de schrijver. Gebruik `journalen (verslagen)' wanneer het gaat om het verslag van de activiteiten of de transacties van personen of organisaties. <![CDATA[<a href="#_getty_2017">(Getty, 2017)</a>]]></skos:definition>
    <skos:definition xml:lang="zh-hant">指內含筆者每日自身經驗、態度，與觀察之個人記述的本子。記述個人或組織所發生的事件或業務進行時，稱為「日誌（記述）」。 <![CDATA[<a href="#_getty_2017">(Getty, 2017)</a>]]></skos:definition>
    <prov:derivedFrom rdf:resource="http://vocab.getty.edu/aat/300027112"/>
    <rdfs:comment xml:lang="en">The description for this term is indebted to the Getty Art &amp; Architecture Thesaurus.</rdfs:comment>
  </genre:Genre>
  <genre:Genre rdf:about="#genreDictionary">
    <rdf:value>DICTIONARY</rdf:value>
    <rdfs:label xml:lang="en">dictionary</rdfs:label>
    <rdfs:label xml:lang="fr"/>
    <rdfs:isDefinedBy rdf:resource="http://sparql.cwrc.ca/ontologies/genre-ONTOLOGY_DATE"/>
    <void:inDataset rdf:resource="#datasetdefinition"/>
    <skos:inScheme rdf:resource="#Genre"/>
    <rdf:type rdf:resource="http://www.w3.org/2004/02/skos/core#Concept"/>
    <skos:definition xml:lang="en">Reference sources containing alphabetical lists of words with information given for each word; generally including meanings, pronunciation, etymology, and often usage guidance. <![CDATA[<a href="#_getty_2017">(Getty, 2017)</a>]]></skos:definition>
    <skos:definition xml:lang="es">Fuentes referenciales que contiene listas alfabéticas de palabras con información proporcionada para cada una; generalmente incluyendo significados, pronunciación, etimología y a menudo orientando su uso. <![CDATA[<a href="#_getty_2017">(Getty, 2017)</a>]]></skos:definition>
    <skos:definition xml:lang="nl">Naslagwerken die alfabetisch gerangschikte lijsten woorden omvatten met daarbij informatie over ieder weergegeven woord. Meestal geven ze betekenis, uitspraak en etymologie, en bevatten ook informatie over het gebruik van een woord. <![CDATA[<a href="#_getty_2017">(Getty, 2017)</a>]]></skos:definition>
    <prov:derivedFrom rdf:resource="http://vocab.getty.edu/aat/300026186"/>
    <rdfs:comment xml:lang="en">The description for this term is indebted to the Getty Art &amp; Architecture Thesaurus.</rdfs:comment>
  </genre:Genre>
  <genre:Genre rdf:about="#genreDidactic">
    <rdf:value>DIDACTIC</rdf:value>
    <rdfs:label xml:lang="en">didactic</rdfs:label>
    <rdfs:label xml:lang="fr"/>
    <rdfs:isDefinedBy rdf:resource="http://sparql.cwrc.ca/ontologies/genre-ONTOLOGY_DATE"/>
    <void:inDataset rdf:resource="#datasetdefinition"/>
    <skos:inScheme rdf:resource="#Genre"/>
    <rdf:type rdf:resource="http://www.w3.org/2004/02/skos/core#Concept"/>
    <skos:definition xml:lang="en">Writing that is &quot;preachy&quot; or seeks overtly to convince a reader of a particular point or lesson. Medieval homilies and Victorian moral essays are often held up as examples of didactic literature, but one might argue that all literature is didactic to one extent or another since the written word frequently implies or suggests an authorial attitude. Sometimes, the lesson is overtly religious, as in the case of sermons or in literature like Milton's Paradise Lost, which seeks to &quot;justify God's ways to men.&quot; In a more subtle way, much of Romantic literature hints at a critique of urbanized and mechanized life in 19th-century London. <![CDATA[<a href="#_wheeler_2017">(L. K Wheeler, 2017)</a>]]></skos:definition>
    <prov:derivedFrom rdf:resource="http://web.cn.edu/kwheeler/lit_terms_d.html"/>
    <rdfs:comment xml:lang="en">The description for this term is indebted to Dr. L. Kip Wheeler of Carson-Newman University. </rdfs:comment>
  </genre:Genre>
  <genre:Genre rdf:about="#genreDirectory">
    <rdf:value>DIRECTORY</rdf:value>
    <rdfs:label xml:lang="en">directory</rdfs:label>
    <rdfs:label xml:lang="fr"/>
    <rdfs:isDefinedBy rdf:resource="http://sparql.cwrc.ca/ontologies/genre-ONTOLOGY_DATE"/>
    <void:inDataset rdf:resource="#datasetdefinition"/>
    <skos:inScheme rdf:resource="#Genre"/>
    <rdf:type rdf:resource="http://www.w3.org/2004/02/skos/core#Concept"/>
    <skos:definition xml:lang="en">Enumerations of names, addresses, and other data about specific groups of persons or organizations; may appear in alphabetic or graphic format. <![CDATA[<a href="#_getty_2017">(Getty, 2017)</a>]]></skos:definition>
    <skos:definition xml:lang="es">Enumeraciones de nombres, direcciones y otras informaciones acerca de un grupo específico de personas u organizaciones; puede aparecer en formato alfabético o gráfico. <![CDATA[<a href="#_getty_2017">(Getty, 2017)</a>]]></skos:definition>
    <skos:definition xml:lang="nl">Opsommingen van namen, adressen en andere gegevens van specifieke groepen personen of organisaties; komen voor in alfabetische of grafische vorm. <![CDATA[<a href="#_getty_2017">(Getty, 2017)</a>]]></skos:definition>
    <skos:definition xml:lang="zh-hant">特定群體或組織之姓名、地址，與其他資料的細目；可能依字母順序或圖像格式出現。 <![CDATA[<a href="#_getty_2017">(Getty, 2017)</a>]]></skos:definition>
    <prov:derivedFrom rdf:resource="http://vocab.getty.edu/aat/300026234"/>
    <rdfs:comment xml:lang="en">The description for this term is indebted to the Getty Art &amp; Architecture Thesaurus.</rdfs:comment>
  </genre:Genre>
  <genre:Genre rdf:about="#genreDissertation">
    <rdf:value>DISSERTATION</rdf:value>
    <rdfs:label xml:lang="en">dissertation</rdfs:label>
    <rdfs:label xml:lang="fr"/>
    <rdfs:isDefinedBy rdf:resource="http://sparql.cwrc.ca/ontologies/genre-ONTOLOGY_DATE"/>
    <void:inDataset rdf:resource="#datasetdefinition"/>
    <skos:inScheme rdf:resource="#Genre"/>
    <rdf:type rdf:resource="http://www.w3.org/2004/02/skos/core#Concept"/>
  </genre:Genre>
  <genre:Genre rdf:about="#genreDocumentary">
    <rdf:value>DOCUMENTARY</rdf:value>
    <rdfs:label xml:lang="en">documentary</rdfs:label>
    <rdfs:label xml:lang="fr"/>
    <rdfs:isDefinedBy rdf:resource="http://sparql.cwrc.ca/ontologies/genre-ONTOLOGY_DATE"/>
    <void:inDataset rdf:resource="#datasetdefinition"/>
    <skos:inScheme rdf:resource="#Genre"/>
    <rdf:type rdf:resource="http://www.w3.org/2004/02/skos/core#Concept"/>
  </genre:Genre>
  <genre:Genre rdf:about="#genreDomestic">
    <rdf:value>DOMESTIC</rdf:value>
    <rdfs:label xml:lang="en">domestic</rdfs:label>
    <rdfs:label xml:lang="fr"/>
    <rdfs:isDefinedBy rdf:resource="http://sparql.cwrc.ca/ontologies/genre-ONTOLOGY_DATE"/>
    <void:inDataset rdf:resource="#datasetdefinition"/>
    <skos:inScheme rdf:resource="#Genre"/>
    <rdf:type rdf:resource="http://www.w3.org/2004/02/skos/core#Concept"/>
    <skos:definition xml:lang="en">Domestic realism normally refers to the genre of nineteenth-century novels popular with women readers. This body of writing is also known as &quot;sentimental fiction&quot; or &quot;woman's fiction&quot;. The genre is mainly reflected in the novel though short-stories and non-fiction works such as Harriet Beecher Stowe's &quot;Our Country Neighbors&quot; and The New Housekeeper's Manual written by Stowe and her sister-in-law Catharine Beecher are works of domestic realism. The style's particular characteristics are: &quot;1. Plot focuses on a heroine who embodies one of two types of exemplar: the angel and the practical woman (Reynolds) who sometimes exist in the same work. Baym says that this heroine is contrasted with the passive woman (incompetent, cowardly, ignorant; often the heroine's mother is this type) and the &quot;belle,&quot; who is deprived of a proper education. 2. The heroine struggles for self-mastery, learning the pain of conquering her own passions (Tompkins, Sensational Designs, 172). 3. The heroine learns to balance society's demands for self-denial with her own desire for autonomy, a struggle often addressed in terms of religion. 4. She suffers at the hands of abusers of power before establishing a network of surrogate kin. 5. The plots &quot;repeatedly identify immersion in feeling as one of the great temptations and dangers for a developing woman. They show that feeling must be controlled. . . &quot; (Baym 25). Frances Cogan notes that the heroines thus undergo a full education within which to realize feminine obligations (The All-American Girl). 6. The tales generally end with marriage, usually one of two possible kinds: A. Reforming the bad or &quot;wild&quot; male, as in Augusta Evans's St. Elmo (1867) B. Marrying the solid male who already meets her qualifications.Examples: Maria Cummins, The Lamplighter (1854) and Susan Warner, The Wide, Wide World (1850) 7. The novels may use a &quot;language of tears&quot; that evokes sympathy from the readers. 8. Richard Brodhead (Cultures of Letters) sees class as an important issue, as the ideal family or heroine is poised between a lower-class family exemplifying poverty and domestic disorganization and upper-class characters exemplifying an idle, frivolous existence (94).&quot; An example of this style of novel is Jane Smiley's A Thousand Acres in which the main character's confinement is emphasized in such a way. Some early exponents of the genre of domestic realism were Jane Austen and Elizabeth Barrett Browning. <![CDATA[<a href="#_dbpedia_2017">(DBpedia, 2017)</a>]]></skos:definition>
    <prov:derivedFrom rdf:resource="http://dbpedia.org/resource/Domestic_realism"/>
    <rdfs:comment xml:lang="en">The description for this term is indebted to DBpedia. </rdfs:comment>
  </genre:Genre>
  <genre:Genre rdf:about="#genreDrama">
    <rdf:value>DRAMA</rdf:value>
    <rdfs:label xml:lang="en">drama</rdfs:label>
    <rdfs:label xml:lang="fr">drame</rdfs:label>
    <rdfs:isDefinedBy rdf:resource="http://sparql.cwrc.ca/ontologies/genre-ONTOLOGY_DATE"/>
    <void:inDataset rdf:resource="#datasetdefinition"/>
    <skos:inScheme rdf:resource="#Genre"/>
    <rdf:type rdf:resource="http://www.w3.org/2004/02/skos/core#Concept"/>
    <skos:definition xml:lang="en">A composition in prose or verse presenting, in pantomime and dialogue, a narrative involving conflict between a character or characters and some external or internal force (see conflict). Playwrights usually design dramas for presentation on a stage in front of an audience. Aristotle called drama &quot;imitated human action.&quot; Drama may have originated in religious ceremonies. Thespis of Attica (sixth century BCE) was the first recorded composer of a tragedy. Tragedies in their earliest stage were performed by a single actor who interacted with the chorus. The playwright Aeschylus added a second actor on the stage (deuteragonist) to allow additional conflict and dialogue. Sophocles and Euripides added a third (tritagonist). Medieval drama may have evolved independently from rites commemorating the birth and death of Christ. During the late medieval period and the early Renaissance, drama gradually altered to the form we know today. The mid-sixteenth century in England in particular was one of the greatest periods of world drama. In traditional Greek drama, as defined by Aristotle, a play was to consist of five acts and follow the three dramatic unities. In more recent drama (i.e., during the last two centuries), plays have frequently consisted of three acts, and playwrights have felt more comfortable disregarding the confines of Aristotelian rules involving verisimilitude. See also unities, comedy, tragedy, revenge play, miracle play, morality play, and mystery play. An individual work of drama is called a play. DRAMATIC CONVENTION: See convention. DRAMATIC IRONY: See irony. DRAMATIC<![CDATA[<a href="#_wheeler_2017">(L. K Wheeler, 2017)</a>]]></skos:definition>
    <prov:derivedFrom rdf:resource="http://web.cn.edu/kwheeler/lit_terms_d.html"/>
    <rdfs:comment xml:lang="en">The description for this term is indebted to Dr. L. Kip Wheeler of Carson-Newman University. </rdfs:comment>
  </genre:Genre>
  <genre:Genre rdf:about="#genreDramaticmonologue">
    <rdf:value>DRAMATICMONOLOGUE</rdf:value>
    <rdfs:label xml:lang="en">dramatic monologue</rdfs:label>
    <rdfs:label xml:lang="fr"/>
    <rdfs:isDefinedBy rdf:resource="http://sparql.cwrc.ca/ontologies/genre-ONTOLOGY_DATE"/>
    <void:inDataset rdf:resource="#datasetdefinition"/>
    <skos:inScheme rdf:resource="#Genre"/>
    <rdf:type rdf:resource="http://www.w3.org/2004/02/skos/core#Concept"/>
    <skos:definition xml:lang="en">Dramatic monologue, also known as a persona poem, is a type of poetry written in the form of a speech of an individual character. M.H. Abrams notes the following three features of the dramatic monologue as it applies to poetry. <![CDATA[<a href="#_dbpedia_2017">(DBpedia, 2017)</a>]]></skos:definition>
    <skos:definition xml:lang="fr">Un monologue dramatique est en France, à la fin du Moyen Âge, un type de poème comique à vocation scénique. À l’instar des jongleurs, l’acteur seul en scène incarnait plusieurs personnages stéréotypés. Il est considéré comme un des quatre grands genres comiques de la fin du Moyen Âge avec la sotie, le sermon joyeux et la farce. Dans l'Angleterre du XIXe siècle, le terme monologue dramatique (dramatic mononologue) désignait un type de poème, fort apprécié par de nombreux poètes de l'époque victorienne, dans lequel un personnage, de fiction ou historique, exprime ses sentiments, ses actions ou ses motifs dans un monologue. Celui-ci, dont les paroles sont souvent influencées par le contexte critique dans lequel elles sont prononcées, s'adresse en général à un auditoire silencieux.Des exemples de monologues dramatiques sont My Last Duchess de Robert Browning, The Captain of the 1984 Top of the Form Team de Carol Ann Duffy, ou encore Lady Lazarus de Sylvia Plath. <![CDATA[<a href="#_dbpedia_2017">(DBpedia, 2017)</a>]]>
</skos:definition>
    <skos:definition xml:lang="es">El monólogo dramático puede ser dos cosas: <![CDATA[<a href="#_dbpedia_2017">(DBpedia, 2017)</a>]]></skos:definition>
    <prov:derivedFrom rdf:resource="http://dbpedia.org/resource/Dramatic_monologue"/>
    <rdfs:comment xml:lang="en">The description for this term is indebted to DBpedia. </rdfs:comment>
  </genre:Genre>
  <genre:Genre rdf:about="#genreDreamvision">
    <rdf:value>DREAMVISION</rdf:value>
    <rdfs:label xml:lang="en">dreamvision</rdfs:label>
    <rdfs:label xml:lang="fr"/>
    <rdfs:isDefinedBy rdf:resource="http://sparql.cwrc.ca/ontologies/genre-ONTOLOGY_DATE"/>
    <void:inDataset rdf:resource="#datasetdefinition"/>
    <skos:inScheme rdf:resource="#Genre"/>
    <rdf:type rdf:resource="http://www.w3.org/2004/02/skos/core#Concept"/>
  </genre:Genre>
  <genre:Genre rdf:about="#genreDystopia">
    <rdf:value>DYSTOPIA</rdf:value>
    <rdfs:label xml:lang="en">dystopia</rdfs:label>
    <rdfs:label xml:lang="fr"/>
    <rdfs:isDefinedBy rdf:resource="http://sparql.cwrc.ca/ontologies/genre-ONTOLOGY_DATE"/>
    <void:inDataset rdf:resource="#datasetdefinition"/>
    <skos:inScheme rdf:resource="#Genre"/>
    <rdf:type rdf:resource="http://www.w3.org/2004/02/skos/core#Concept"/>
    <skos:definition xml:lang="en">(from Greek, dys topos, &quot;bad place&quot;): The opposite of a utopia, a dystopia is an imaginary society in fictional writing that represents, as M. H. Abrams puts it, &quot;a very unpleasant imaginary world in which ominous tendencies of our present social, political, and technological order are projected in some disastrous future culmination&quot; (Glossary 218). For instance, while a utopia presents readers with a place where all the citizens are happy and ruled by a virtuous, efficient, rational government, a dystopia presents readers with a world where all citizens are universally unhappy, manipulated, and repressed by a sinister, sadistic totalitarian state. This government exists at best to further its own power and at worst seeks actively to destroy its own citizens' creativity, health, and happiness. Examples of fictional dystopias include Aldous Huxley's Brave New World, George Orwell's 1984, Margaret Atwood's The Handmaid's Tale, and Ursula Le Guin's The Dispossessed. <![CDATA[<a href="#_wheeler_2017">(L. K Wheeler, 2017)</a>]]></skos:definition>
    <prov:derivedFrom rdf:resource="http://web.cn.edu/kwheeler/lit_terms_d.html"/>
    <rdfs:comment xml:lang="en">The description for this term is indebted to Dr. L. Kip Wheeler of Carson-Newman University. </rdfs:comment>
  </genre:Genre>
  <genre:Genre rdf:about="#genreEclogue">
    <rdf:value>ECLOGUE</rdf:value>
    <rdfs:label xml:lang="en">eclogue</rdfs:label>
    <rdfs:label xml:lang="fr"/>
    <rdfs:isDefinedBy rdf:resource="http://sparql.cwrc.ca/ontologies/genre-ONTOLOGY_DATE"/>
    <void:inDataset rdf:resource="#datasetdefinition"/>
    <skos:inScheme rdf:resource="#Genre"/>
    <rdf:type rdf:resource="http://www.w3.org/2004/02/skos/core#Concept"/>
    <skos:definition xml:lang="en">An eclogue is a poem in a classical style on a pastoral subject. Poems in the genre are sometimes also called bucolics. <![CDATA[<a href="#_dbpedia_2017">(DBpedia, 2017)</a>]]>
</skos:definition>
    <skos:definition xml:lang="fr">Une églogue est un poème de style classique consacré à un sujet pastoral. Les poèmes de ce genre littéraire sont parfois qualifiés de « bucoliques ». <![CDATA[<a href="#_dbpedia_2017">(DBpedia, 2017)</a>]]>
</skos:definition>
    <skos:definition xml:lang="de">Die Ekloge (griechisch ἐκλογή eklogḗ „Auswahl“ oder „Wahl“, latinisiert ecloga) ist ein Begriff aus der antiken Literatur. Die Grundbedeutung ist „Auswahl“, das heißt „das Ausgewählte“. Gemeint ist ursprünglich ein ausgewähltes Stück (Auszug, Zitat) aus einem längeren literarischen Text oder ein einzelnes Gedicht von mäßiger Länge, das aus einer Sammlung von Gedichten oder aus dem Werk eines Dichters herausgegriffen wurde. Der Begriff Ekloge bezeichnet im eigentlichen Wortsinn ein „ausgewähltes“ Gedicht, wurde aber im Humanismus als Gattungsbezeichnung missverstanden. Im Plural bezeichnet eclogae in der römischen Lyrik ursprünglich nur „ausgewählte“ Gedichte, in späterem Sprachgebrauch sind gewöhnlich ländliche oder Hirtengedichte (bukolische Dichtung) gemeint. Daher wird der Begriff Ekloge oft als Synonym von „bukolisches Gedicht“ verwendet. Die bekanntesten Gedichte, für die heute die Bezeichnung Eklogen (Eclogae) gängig ist, sind die Eclogae (oder auch Bucolica) von Vergil. Bereits im 1. Jahrhundert bezeichnet Statius einzelne Gedichte aus seinen Silvae mit dem Ausdruck egloga; er ist der erste römische Dichter, der den Begriff für seine eigenen Werke verwendet. In der deutschen Literatur waren bis ins 18. Jahrhundert Ekloge, Schäfer- bzw. Hirtengedicht und Idylle synonym verwendete Begriffe und bezeichneten lyrisch-dramatische Hirtengesänge oder allgemein kürzere Hirtendichtung, siehe etwa Georg Rodolf Weckherlin Eclogen oder Hürtengedichte (1641) oder Johann Christoph Gottscheds Von Idyllen, Eklogen oder Schäfergedichten (in Critische Dichtkunst, 1730).Durch den Erfolg von Salomon Gessners Idyllen (1756) wurde aber Idylle der gebräuchliche Begriff für diese Gattung. <![CDATA[<a href="#_dbpedia_2017">(DBpedia, 2017)</a>]]>
</skos:definition>
    <skos:definition xml:lang="es">La égloga es un subgénero de la poesía lírica que se dialoga a veces como una pequeña pieza teatral en un acto. De tema amoroso, uno o varios pastores lo desarrollan contándolo en un ambiente campesino donde la naturaleza es paradisíaca y tiene un gran protagonismo la música. Como subgénero lírico se desarrolla a veces mediante un monólogo pastoril o, más frecuentemente, con un diálogo. La égloga es una composición en la que el poeta, encarnado en uno o varios pastores, expresa su amor en un marco idealizado, lleno de belleza y amor. Las primeras églogas fueron los Idilios (en griego, &quot;poemitas&quot; o &quot;pequeños cantos&quot;) de Teócrito; luego los escribieron Mosco, Bión de Esmirna y otros autores bajo su influencia. El escritor latino Virgilio (siglo I a. C.) con sus Églogas (en griego, &quot;selecciones&quot;) o Bucólicas añadió elementos autobiográficos, haciendo de cada pastor un personaje imaginario que encubría a un personaje real: Cayo Cilnio Mecenas, Augusto, etc. Algunas de ellas llegaron a escenificarse en Roma. Otros autores latinos escribieron también églogas, como Nemesiano, Calpurnio Sículo o Ausonio. Esta innovación pasó a la bucólica posterior, de forma que algunas veces los personajes de las églogas representaban personajes reales. A través de Giovanni Boccaccio y con el Renacimiento y la Arcadia de Jacopo Sannazaro el género se volvió a recuperar mezclándose las composiciones en verso en un marco narrativo en prosa, y se difundió por todo el mundo occidental, bien en verso, bien como églogas intercaladas en una novela pastoril cualquiera. En la literatura castellana, escribieron églogas Juan del Encina, Lucas Fernández, Garcilaso de la Vega, Juan Boscán, Lope de Vega, Pedro Soto de Rojas, Bernardo de Balbuena y Juan Meléndez Valdés. <![CDATA[<a href="#_dbpedia_2017">(DBpedia, 2017)</a>]]>
</skos:definition>
    <skos:definition xml:lang="nl">Ecloge – ook wel: ekloge (Griekse spelling) en ecloga (Latijnse spelling) - is een benaming voor een herdersdicht en maakt deel uit van de bucolische poëzie. Het woord ecloge kennen we vooral van de tien herdersdichten (Bucolica) die Vergilius in 38 v.Chr. publiceerde en die doorgaans Eclogae worden genoemd. Het uit het Grieks afkomstige woord ekloge (ἑκλογή) betekent eigenlijk ‘keus’. Het is waarschijnlijk dat Vergilius niet zelf de naam ecloga gebruikte, maar dat die door latere grammatici aan zijn gedichten is gegeven. De Eclogae of Eclogen van Vergilius zijn tien herdersdichten, die Vergilius dichtte naar het voorbeeld van Theocritus, de uitvinder van het herdersdicht. Ze zijn geschreven in dactylische hexameters en variëren in lengte van 63 tot 111 regels. De meeste zijn gesprekken tussen herders. Sinds Vergilius is de naam ecloge een algemeen gebruikte naam voor dit soort gedichten. We kennen verder zeven eclogen die ene Calpurnius Siculus schreef in de tijd van Nero, en van de derde-eeuwse dichter Nemesianus zijn vier eclogen overgeleverd. Zeer invloedrijk werd in later eeuwen Vergilius’ vierde ecloge, waarin de komst van een bijzonder kind wordt aangekondigd die een nieuwe tijd zal inluiden. Dit werd al snel uitgelegd als een aankondiging van de geboorte van Christus. In de middeleeuwse Latijnse literatuur werd het genre van het herdersdicht niet altijd begrepen. Zo schreef bisschop Radboud ca. 900 een Ecloga pro St. Lebuino, waarin hij de kerstenende activiteiten van Lebuïnus beschrijft. In de Neolatijnse literatuur werd het genre van de ecloga veel beoefend. Het woord werd door de neolatinisten ook wel gespeld als (a)egloga, omdat men dacht dat het verwant was met αἱγ- (aeg), het Griekse woord voor ‘geit’. Geleidelijk ontstonden er enkele varianten op het genre. Zo schreef Iacopo Sannazaro (1458-1530) vijf Eclogae piscatoriae, waarin hij de herders verving door vissers, en schreef de Franse jezuïet René Rapin christelijke eclogen: Eclogae Sacrae (1659). <![CDATA[<a href="#_dbpedia_2017">(DBpedia, 2017)</a>]]></skos:definition>
    <prov:derivedFrom rdf:resource="http://dbpedia.org/resource/Eclogue"/>
    <rdfs:comment xml:lang="en">The description for this term is indebted to DBpedia. </rdfs:comment>
  </genre:Genre>
  <genre:Genre rdf:about="#genreElegy">
    <rdf:value>ELEGY</rdf:value>
    <rdfs:label xml:lang="en">elegy</rdfs:label>
    <rdfs:label xml:lang="fr">élégie</rdfs:label>
    <rdfs:isDefinedBy rdf:resource="http://sparql.cwrc.ca/ontologies/genre-ONTOLOGY_DATE"/>
    <void:inDataset rdf:resource="#datasetdefinition"/>
    <skos:inScheme rdf:resource="#Genre"/>
    <rdf:type rdf:resource="http://www.w3.org/2004/02/skos/core#Concept"/>
    <skos:definition xml:lang="en">Mournful, melancholy, or plaintive poems, especially funeral songs or laments for the dead. <![CDATA[<a href="#_getty_2017">(Getty, 2017)</a>]]></skos:definition>
    <skos:definition xml:lang="es">Poemas tristes, melancólicos o quejumbrosos, especialmente cantos fúnebres o lamentos por los muertos. <![CDATA[<a href="#_getty_2017">(Getty, 2017)</a>]]></skos:definition>
    <skos:definition xml:lang="nl">Sombere, melancholieke of treurige gedichten, met name klaagliederen of liederen die bij een begrafenisplechtigheid ten gehore worden gebracht. <![CDATA[<a href="#_getty_2017">(Getty, 2017)</a>]]></skos:definition>
    <skos:definition xml:lang="de">Schwermütiges, melancholisches oder trauriges Gedicht, insbesondere Begräbnislied oder Totenklage. <![CDATA[<a href="#_getty_2017">(Getty, 2017)</a>]]></skos:definition>
    <prov:derivedFrom rdf:resource="http://vocab.getty.edu/aat/300026285"/>
    <rdfs:comment xml:lang="en">The description for this term is indebted to the Getty Art &amp; Architecture Thesaurus.</rdfs:comment>
    <skos:definition xml:lang="fr">L’élégie (en grec ancien ἐλεγεία / elegeía, signifiant « chant de mort ») fut une forme de poème dans l'Antiquité, avant de devenir un genre poétique à partir de la Renaissance. Dans l’Antiquité, était appelé « élégie » tout poème alternant hexamètres et pentamètres en distiques : ce sont les vers élégiaques. De nos jours, l’élégie est considérée comme un genre au sein de la poésie lyrique, en tant que poème de longueur et de forme variables caractérisé par son ton plaintif particulièrement adapté à l’évocation d’un mort ou à l’expression d’une souffrance amoureuse due à un abandon ou à une absence. <![CDATA[<a href="#_dbpedia_2017">(DBpedia, 2017)</a>]]></skos:definition>
    <prov:derivedFrom rdf:resource="http://dbpedia.org/resource/Elegy"/>
    <rdfs:comment xml:lang="en">The description for this term is indebted to DBpedia. </rdfs:comment>
  </genre:Genre>
  <genre:Genre rdf:about="#genreEncyclopaedia">
    <rdf:value>ENCYCLOPAEDIA</rdf:value>
    <rdfs:label xml:lang="en">encyclopaedia</rdfs:label>
    <rdfs:label xml:lang="fr"/>
    <rdfs:isDefinedBy rdf:resource="http://sparql.cwrc.ca/ontologies/genre-ONTOLOGY_DATE"/>
    <void:inDataset rdf:resource="#datasetdefinition"/>
    <skos:inScheme rdf:resource="#Genre"/>
    <rdf:type rdf:resource="http://www.w3.org/2004/02/skos/core#Concept"/>
    <skos:definition xml:lang="en">Books, set of books, or disks, containing informational articles on subjects in every field of knowledge, or limited to a special field or subject, usually arranged in alphabetical order. <![CDATA[<a href="#_getty_2017">(Getty, 2017)</a>]]></skos:definition>
    <prov:derivedFrom rdf:resource="http://vocab.getty.edu/aat/300129439"/>
    <rdfs:comment xml:lang="en">The description for this term is indebted to the Getty Art &amp; Architecture Thesaurus.</rdfs:comment>
  </genre:Genre>
  <genre:Genre rdf:about="#genreEpic">
    <rdf:value>EPIC</rdf:value>
    <rdfs:label xml:lang="en">epic</rdfs:label>
    <rdfs:label xml:lang="fr"/>
    <rdfs:isDefinedBy rdf:resource="http://sparql.cwrc.ca/ontologies/genre-ONTOLOGY_DATE"/>
    <void:inDataset rdf:resource="#datasetdefinition"/>
    <skos:inScheme rdf:resource="#Genre"/>
    <rdf:type rdf:resource="http://www.w3.org/2004/02/skos/core#Concept"/>
    <skos:definition xml:lang="en">Meaning extended from &quot;epic poetry,&quot; in modern usage refers to literary art forms, such as prose, poetry, plays, films, and other works where the story has a theme of grandeur and heroism.  <![CDATA[<a href="#_getty_2017">(Getty, 2017)</a>]]></skos:definition>
    <prov:derivedFrom rdf:resource="http://vocab.getty.edu/aat/300404209"/>
    <rdfs:comment xml:lang="en">The description for this term is indebted to the Getty Art &amp; Architecture Thesaurus.</rdfs:comment>
  </genre:Genre>
  <genre:Genre rdf:about="#genreEpigram">
    <rdf:value>EPIGRAM</rdf:value>
    <rdfs:label xml:lang="en">epigram</rdfs:label>
    <rdfs:label xml:lang="fr"/>
    <rdfs:isDefinedBy rdf:resource="http://sparql.cwrc.ca/ontologies/genre-ONTOLOGY_DATE"/>
    <void:inDataset rdf:resource="#datasetdefinition"/>
    <skos:inScheme rdf:resource="#Genre"/>
    <rdf:type rdf:resource="http://www.w3.org/2004/02/skos/core#Concept"/>
    <skos:definition xml:lang="fr">À l’origine, une épigramme, du grec ancien ἐπίγραμμα (epígramma), « inscription », est une inscription, d’abord en prose, puis en vers, qu’on gravait sur les monuments, les statues, les tombeaux et les trophées, pour perpétuer le souvenir d’un héros ou d’un événement. À partir du IVe siècleav. J.-C., l’épigramme devient une petite pièce de poésie sur un sujet quelconque, imitant par sa brièveté les inscriptions, offrant une pensée ingénieuse ou délicate exprimée avec grâce et précision. Enfin, à partir du XVIe siècle, le genre se spécialise dans le mot d’esprit : l’épigramme renferme généralement une pointe grivoise ou assassine. Les plus anciennes épigrammes ne revêtent qu'un caractère pratique, visant à identifier le propriétaire ou la personne dédiant l’objet. Le premier auteur d’épigrammes, selon la tradition grecque, est Simonide de Céos (Hérodote, VII, 228, 4), qui vit à la fin du VIe siècleav. J.-C. C'est de cette même époque que date la première épigramme signée connue ; il s'agit d’une dédicace d’Ion de Chios à Delphes. <![CDATA[<a href="#_dbpedia_2017">(DBpedia, 2017)</a>]]></skos:definition>
    <prov:derivedFrom rdf:resource="http://dbpedia.org/resource/Epigram"/>
    <rdfs:comment xml:lang="en">The description for this term is indebted to DBpedia. </rdfs:comment>
    <skos:definition xml:lang="en">Refers to short satiric poems or any similar pointed sayings. <![CDATA[<a href="#_getty_2017">(Getty, 2017)</a>]]></skos:definition>
    <skos:definition xml:lang="de">Bezeichnet ein kurzes satirisches Gedicht oder jede ähnlich pointierte Redensart. <![CDATA[<a href="#_getty_2017">(Getty, 2017)</a>]]></skos:definition>
    <skos:definition xml:lang="es">Úsese para poemas satíricos cortos u otros refranes mordaces similares. <![CDATA[<a href="#_getty_2017">(Getty, 2017)</a>]]></skos:definition>
    <skos:definition xml:lang="nl">Wordt gebruikt voor korte, satirische gedichten of vergelijkbare puntige gezegdes. <![CDATA[<a href="#_getty_2017">(Getty, 2017)</a>]]></skos:definition>
    <prov:derivedFrom rdf:resource="http://vocab.getty.edu/aat/300202533"/>
    <rdfs:comment xml:lang="en">The description for this term is indebted to the Getty Art &amp; Architecture Thesaurus.</rdfs:comment>
  </genre:Genre>
  <genre:Genre rdf:about="#genreEpilogue">
    <rdf:value>EPILOGUE</rdf:value>
    <rdfs:label xml:lang="en">epilogue</rdfs:label>
    <rdfs:label xml:lang="fr">épilogue</rdfs:label>
    <rdfs:isDefinedBy rdf:resource="http://sparql.cwrc.ca/ontologies/genre-ONTOLOGY_DATE"/>
    <void:inDataset rdf:resource="#datasetdefinition"/>
    <skos:inScheme rdf:resource="#Genre"/>
    <rdf:type rdf:resource="http://www.w3.org/2004/02/skos/core#Concept"/>
    <skos:definition xml:lang="en">A conclusion added to a literary work such as a novel, play, or long poem. It is the opposite of a prologue. Often, the epilogue refers to the moral of a fable. Sometimes, it is a speech made by one of the actors at the end of a play asking for the indulgence of the critics and the audience. Shakespeare's A Midsummer Night's Dream contains one of the most famous epilogues. Contrast with prologue. Do not confuse the term with eclogue. <![CDATA[<a href="#_wheeler_2017">(L. K Wheeler, 2017)</a>]]></skos:definition>
    <prov:derivedFrom rdf:resource="http://web.cn.edu/kwheeler/lit_terms_e.html"/>
    <rdfs:comment xml:lang="en">The description for this term is indebted to Dr. L. Kip Wheeler of Carson-Newman University. </rdfs:comment>
  </genre:Genre>
  <genre:Genre rdf:about="#genreEpistle">
    <rdf:value>EPISTLE</rdf:value>
    <rdfs:label xml:lang="en">epistle</rdfs:label>
    <rdfs:label xml:lang="fr">épître&gt;</rdfs:label>
    <rdfs:isDefinedBy rdf:resource="http://sparql.cwrc.ca/ontologies/genre-ONTOLOGY_DATE"/>
    <void:inDataset rdf:resource="#datasetdefinition"/>
    <skos:inScheme rdf:resource="#Genre"/>
    <rdf:type rdf:resource="http://www.w3.org/2004/02/skos/core#Concept"/>
    <skos:definition xml:lang="fr">Le terme épître, issu du latin epistula, du grec επιστολη (epistolē), désigne une lettre (au sens de correspondance).Il a pris le sens aujourd'hui d'un court traité philosophique ou religieux exposé sous forme épistolaire. Ce sont de courts traités le plus souvent philosophiques. Ce peuvent être aussi des « conversations en l'absence » de l'interlocuteur sur des aspects sociaux ou moraux de l'existence. Au fil du temps, l’épître devient, en littérature, un discours en vers du genre académique ou didactique. Elle prend rapidement le sens d’épigramme nettement moins acerbe que la satire.Le mot « épître » est un nom commun féminin. Le Nouveau Testament contient plusieur <![CDATA[<a href="#_dbpedia_2017">(DBpedia, 2017)</a>]]>
s épîtres.</skos:definition>
    <skos:definition xml:lang="de">Epistel (griech. ἐπιστολή, epistolē; lat. epistola, epistula) ist ein über das Lateinische aus dem Griechischen entlehntes Wort für „Brief“, das für Brieftexte gehobenen Anspruchs (Sendschreiben, Versepistel) verwendet wird, insbesondere für die Apostelbriefe der Bibel. Als liturgische Kurzbezeichnung bezieht sich der Begriff auf bestimmte im Gottesdienst zu lesende Abschnitte der Bibel. <![CDATA[<a href="#_dbpedia_2017">(DBpedia, 2017)</a>]]>
</skos:definition>
    <skos:definition xml:lang="es">Epístola (del griego: ἐπιστολή, epistolē) es un sinónimo de carta: un texto cuya función principal es la comunicación entre el remitente o emisor (el escritor que la redacta y envía) y el destinatario o receptor que la debe recibir. El uso del término suele implicar un registro culto o un contexto literario (el género epistolar). En la actualidad es un término arcaico, por lo general restringido en su uso a las cartas didáctica sobre ética o religión; y particularmente para referirse a los libros del Nuevo Testamento que reciben el nombre de &quot;epístolas&quot;, y donde se recogen las escritas por algunos apóstoles destinadas a las comunidades cristianas primitivas. Las tradicionalmente atribuidas a Pablo de Tarso se conocen como &quot;epístolas paulinas&quot; y el resto con el nombre genérico de &quot;epístolas católicas&quot; (es decir, &quot;universales&quot; o &quot;generales&quot;). El género epistolar fue común en el Antiguo Egipto como parte del trabajo de los escribas, y están recogidas bajo el nombre de Sebayt (instrucciones), estando datadas las más antiguas en el siglo XXV a. C. También nos han llegado de la Antigüedad las Epístolas de Horacio, del siglo I a. C. Una de ellas, Epistula ad Pisones, recibe el nombre de Arte poética, y ha sido durante siglos considerada como la normativa de principios literarios. <![CDATA[<a href="#_dbpedia_2017">(DBpedia, 2017)</a>]]>
</skos:definition>
    <skos:definition xml:lang="nl">Een epistel is een schrijven gericht aan een persoon of een groep personen, meestal in de vorm van een erg formele brief, vaak didactisch van aard en elegant geformuleerd. De brieven van de apostelen aan verscheidene joodse gemeenschappen in de wereld, opgenomen in het Nieuwe Testament, worden vaak epistels genoemd. <![CDATA[<a href="#_dbpedia_2017">(DBpedia, 2017)</a>]]></skos:definition>
    <prov:derivedFrom rdf:resource="http://dbpedia.org/resource/Epistle"/>
    <rdfs:comment xml:lang="en">The description for this term is indebted to DBpedia. </rdfs:comment>
    <skos:definition xml:lang="en">Literary genre taking the form of letters, usually of a literary, formal, or public nature. Examples are the epistles in the Biblical New Testament. <![CDATA[<a href="#_getty_2017">(Getty, 2017)</a>]]></skos:definition>
    <prov:derivedFrom rdf:resource="http://vocab.getty.edu/aat/300404697"/>
    <rdfs:comment xml:lang="en">The description for this term is indebted to the Getty Art &amp; Architecture Thesaurus.</rdfs:comment>
  </genre:Genre>
  <genre:Genre rdf:about="#genreEpistolary">
    <rdf:value>EPISTOLARY</rdf:value>
    <rdfs:label xml:lang="en">epistolary</rdfs:label>
    <rdfs:label xml:lang="fr"/>
    <rdfs:isDefinedBy rdf:resource="http://sparql.cwrc.ca/ontologies/genre-ONTOLOGY_DATE"/>
    <void:inDataset rdf:resource="#datasetdefinition"/>
    <skos:inScheme rdf:resource="#Genre"/>
    <rdf:type rdf:resource="http://www.w3.org/2004/02/skos/core#Concept"/>
    <skos:definition xml:lang="en">Novels written by using the device of a series of letters, diary entries, newspaper clippings, or other documents. <![CDATA[<a href="#_getty_2017">(Getty, 2017)</a>]]></skos:definition>
    <prov:derivedFrom rdf:resource="http://vocab.getty.edu/aat/300410324"/>
    <rdfs:comment xml:lang="en">The description for this term is indebted to the Getty Art &amp; Architecture Thesaurus.</rdfs:comment>
    <skos:definition xml:lang="de">Briefgedicht ist eine Sammelbezeichnung für alle Arten von in Gedichtform verfassten echten oder fingierten Briefen. Beispiele für Briefgedichte reichen bis in die Antike zurück, am bekanntesten sind Ovids Heroides, in elegischen Distichen verfasste fingierte Briefe mythologischer Frauen an ihre männlichen Partner, in denen sie sich über Vernachlässigung und/oder schlechte Behandlung beklagen, sowie die in Hexametern verfassten Epistulae des Horaz. Aus dem Mittelalter sind spezielle Formen der Minnebrief, ein in Reimpaaren verfasster Liebesgruß an die Geliebte und im Frankreich der Trobadore der Salut d’amour.Im Barock wird von Hofmannswaldau die Ovidsche Form wieder aufgenommen (Helden-Briefe 1664), weitere Beispiele finden sich im französischen Rokoko und der deutschen Anakreontik bei Goeckingk, Gleim, Rabener und Wieland. In der Weimarer Klassik sind die Briefgedichte Goethes an Frau von Stein, Augusta zu Stolberg, Marianne von Willemer und Bettina Brentano die bedeutendsten Beispiele der Gattung in der deutschen Literatur und zugleich Muster einer Gelegenheitsdichtung auf hohem Niveau. Als Beispiel Goethes Gedicht an Charlotte von Stein: Nach der Klassik finden sich vereinzelt Briefgedichte bei Heinrich Heine, Clemens Brentano, Friedrich de la Motte Fouqué, Annette von Droste-Hülshoff, Theodor Fontane, Detlev von Liliencron, Rainer Maria Rilke (Briefwechsel mit Erika Mitterer) und Joachim Ringelnatz. In der französischen Literatur finden sich Briefgedichte bei Clément Marot und in der englischen unter anderem bei John Donne, John Dryden, Alexander Pope und John Keats. <![CDATA[<a href="#_dbpedia_2017">(DBpedia, 2017)</a>]]></skos:definition>
    <prov:derivedFrom rdf:resource="http://dbpedia.org/resource/Epistolary_poem"/>
    <rdfs:comment xml:lang="en">The description for this term is indebted to DBpedia. </rdfs:comment>
  </genre:Genre>
  <genre:Genre rdf:about="#genreEpitaph">
    <rdf:value>EPITAPH</rdf:value>
    <rdfs:label xml:lang="en">epitaph</rdfs:label>
    <rdfs:label xml:lang="fr"/>
    <rdfs:isDefinedBy rdf:resource="http://sparql.cwrc.ca/ontologies/genre-ONTOLOGY_DATE"/>
    <void:inDataset rdf:resource="#datasetdefinition"/>
    <skos:inScheme rdf:resource="#Genre"/>
    <rdf:type rdf:resource="http://www.w3.org/2004/02/skos/core#Concept"/>
    <skos:definition xml:lang="en">Inscriptions on sepulchral monuments in the memory of those buried in the tomb or grave. <![CDATA[<a href="#_getty_2017">(Getty, 2017)</a>]]></skos:definition>
    <skos:definition xml:lang="de">Inschrift auf einem Grabmal in Erinnerung an die in der Grabstätte Beerdigten. <![CDATA[<a href="#_getty_2017">(Getty, 2017)</a>]]></skos:definition>
    <skos:definition xml:lang="nl">Inscripties op grafmonumenten ter nagedachtenis aan personen die in het betreffende graf of de betreffende tombe zijn begraven. <![CDATA[<a href="#_getty_2017">(Getty, 2017)</a>]]></skos:definition>
    <skos:definition xml:lang="es">Inscripciones en mausoleos en memoria de quienes se encuentran enterrados en la tumba o sepulcro. <![CDATA[<a href="#_getty_2017">(Getty, 2017)</a>]]></skos:definition>
    <skos:definition xml:lang="zh-hant">墓碑上的銘文，以紀念埋葬於墳地或墓穴者。 <![CDATA[<a href="#_getty_2017">(Getty, 2017)</a>]]></skos:definition>
    <prov:derivedFrom rdf:resource="http://vocab.getty.edu/aat/300028729"/>
    <rdfs:comment xml:lang="en">The description for this term is indebted to the Getty Art &amp; Architecture Thesaurus.</rdfs:comment>
  </genre:Genre>
  <genre:Genre rdf:about="#genreEpithalamium">
    <rdf:value>EPITHALAMIUM</rdf:value>
    <rdfs:label xml:lang="en">epithalamium</rdfs:label>
    <rdfs:label xml:lang="fr"/>
    <rdfs:isDefinedBy rdf:resource="http://sparql.cwrc.ca/ontologies/genre-ONTOLOGY_DATE"/>
    <void:inDataset rdf:resource="#datasetdefinition"/>
    <skos:inScheme rdf:resource="#Genre"/>
    <rdf:type rdf:resource="http://www.w3.org/2004/02/skos/core#Concept"/>
    <skos:definition xml:lang="en">An epithalamiumLatin form of Greek ἐπιθαλάμιον epithalamion from ἐπί epi &quot;upon,&quot; and θάλαμος thalamos nuptial chamber) is a poem written specifically for the bride on the way to her marital chamber. This form continued in popularity through the history of the classical world; the Roman poet Catullus wrote a famous epithalamium, which was translated from or at least inspired by a now-lost work of Sappho. According to Origen, Song of Songs, might be an epithalamium on the marriage of Solomon with Pharaoh’s daughter. <![CDATA[<a href="#_dbpedia_2017">(DBpedia, 2017)</a>]]></skos:definition>
    <skos:definition xml:lang="fr">L'épithalame (en grec ancien ἐπιθαλάμιον / epithalámion) est une sorte de poème lyrique composé chez les Anciens à l'occasion d'un mariage et à la louange des nouveaux époux. En Grèce, il était chanté par un chœur, soit de jeunes vierges seules, soit de jeunes filles[réf. nécessaire] et de jeunes garçons, avec accompagnement de danses. On le nommait aussi catakoemèse (de catakoimân, envoyer dormir). <![CDATA[<a href="#_dbpedia_2017">(DBpedia, 2017)</a>]]></skos:definition>
    <skos:definition xml:lang="de">Ein Epithalamion (von griech. έπί epi bei und ϑάλαμος thálamos Schlafgemach; lat. epithalamium; dt. Hochzeitsgedicht, Brautlied; Plural: -ien) ist ein üblicherweise pastorales Gelegenheitsgedicht, verfasst und meist chorisch vorgetragen zur Feier einer Hochzeit. <![CDATA[<a href="#_dbpedia_2017">(DBpedia, 2017)</a>]]></skos:definition>
    <skos:definition xml:lang="es">El epitalamio es una poesía lírica, subgénero lírico griego imitado después por los romanos, consistente en un canto de boda. El nombre epitalamio es griego, compuesto sobre y tálamo (en griego θάλαμος) lecho nupcial. Se cantaba regularmente a la puerta de la habitación de los novios por coros de jóvenes y doncellas acompañados de flautas o de otros instrumentos suaves y armónicos. Entre quienes compusieron epitalamios en la antigüedad, se encuentra los poetas griegos Safo y Calímaco y el romano Catulo. <![CDATA[<a href="#_dbpedia_2017">(DBpedia, 2017)</a>]]></skos:definition>
    <prov:derivedFrom rdf:resource="http://dbpedia.org/resource/Epithalamium"/>
    <rdfs:comment xml:lang="en">The description for this term is indebted to DBpedia. </rdfs:comment>
  </genre:Genre>
  <genre:Genre rdf:about="#genreEpyllion">
    <rdf:value>EPYLLION</rdf:value>
    <rdfs:label xml:lang="en">epyllion</rdfs:label>
    <rdfs:label xml:lang="fr"/>
    <rdfs:isDefinedBy rdf:resource="http://sparql.cwrc.ca/ontologies/genre-ONTOLOGY_DATE"/>
    <void:inDataset rdf:resource="#datasetdefinition"/>
    <skos:inScheme rdf:resource="#Genre"/>
    <rdf:type rdf:resource="http://www.w3.org/2004/02/skos/core#Concept"/>
    <skos:definition xml:lang="en">Brief narrative poems in dactylic hexameter of ancient Greece, imitated by Romans and others. Usually dealing with mythological and romantic themes. They are characterized by lively description, miniaturistic attitude, scholarly allusion, and an elevated tone similar to that of the elegy. <![CDATA[<a href="#_getty_2017">(Getty, 2017)</a>]]></skos:definition>
    <prov:derivedFrom rdf:resource="http://vocab.getty.edu/aat/300410360"/>
    <rdfs:comment xml:lang="en">The description for this term is indebted to the Getty Art &amp; Architecture Thesaurus.</rdfs:comment>
  </genre:Genre>
  <genre:Genre rdf:about="#genreEroticapornography">
    <rdf:value>EROTICAPORNOGRAPHY</rdf:value>
    <rdfs:label xml:lang="en">erotica pornography</rdfs:label>
    <rdfs:label xml:lang="fr"/>
    <rdfs:isDefinedBy rdf:resource="http://sparql.cwrc.ca/ontologies/genre-ONTOLOGY_DATE"/>
    <void:inDataset rdf:resource="#datasetdefinition"/>
    <skos:inScheme rdf:resource="#Genre"/>
    <rdf:type rdf:resource="http://www.w3.org/2004/02/skos/core#Concept"/>
  </genre:Genre>
  <genre:Genre rdf:about="#genreEssay">
    <rdf:value>ESSAY</rdf:value>
    <rdfs:label xml:lang="en">essay</rdfs:label>
    <rdfs:label xml:lang="fr">essai</rdfs:label>
    <rdfs:isDefinedBy rdf:resource="http://sparql.cwrc.ca/ontologies/genre-ONTOLOGY_DATE"/>
    <void:inDataset rdf:resource="#datasetdefinition"/>
    <skos:inScheme rdf:resource="#Genre"/>
    <rdf:type rdf:resource="http://www.w3.org/2004/02/skos/core#Concept"/>
    <skos:definition xml:lang="fr">En littérature, un essai est une œuvre de réflexion portant sur les sujets les plus divers et exposée de manière personnelle, voire subjective par l'auteur. Contrairement à l'étude, l'essai peut être polémique ou partisan. C'est un texte littéraire qui se prête bien à la réflexion philosophique, mais aussi à d'autres domaines : essais historiques, essais scientifiques, essais politiques, etc. L'auteur d’un essai est appelé « essayiste ». Le terme « essai » est dérivé du latin exagium, un poids ou appareil de mesure. <![CDATA[<a href="#_dbpedia_2017">(DBpedia, 2017)</a>]]></skos:definition>
    <prov:derivedFrom rdf:resource="http://dbpedia.org/resource/Essay"/>
    <rdfs:comment xml:lang="en">The description for this term is indebted to DBpedia. </rdfs:comment>
    <skos:definition xml:lang="en">Short literary compositions on single subjects, often presenting the personal view of the author. <![CDATA[<a href="#_getty_2017">(Getty, 2017)</a>]]></skos:definition>
    <skos:definition xml:lang="de">Kurzer literarischer Aufsatz über ein Einzelthema, gibt häufig die persönliche Meinung des Autors wieder. <![CDATA[<a href="#_getty_2017">(Getty, 2017)</a>]]></skos:definition>
    <skos:definition xml:lang="nl">Korte literaire verhandelingen over één onderwerp, waarin de auteur dikwijls een persoonlijk standpunt verwoordt. <![CDATA[<a href="#_getty_2017">(Getty, 2017)</a>]]></skos:definition>
    <skos:definition xml:lang="es">Breves composiciones literarias sobre temas específicos, a menudo presentando el punto de vista personal del autor. <![CDATA[<a href="#_getty_2017">(Getty, 2017)</a>]]></skos:definition>
    <skos:definition xml:lang="zh-hant">單一主題的簡短文學作品，常表述作者之個人觀點。 <![CDATA[<a href="#_getty_2017">(Getty, 2017)</a>]]></skos:definition>
    <prov:derivedFrom rdf:resource="http://vocab.getty.edu/aat/300026291"/>
    <rdfs:comment xml:lang="en">The description for this term is indebted to the Getty Art &amp; Architecture Thesaurus.</rdfs:comment>
  </genre:Genre>
  <genre:Genre rdf:about="#genreEulogy">
    <rdf:value>EULOGY</rdf:value>
    <rdfs:label xml:lang="en">eulogy</rdfs:label>
    <rdfs:label xml:lang="fr"/>
    <rdfs:isDefinedBy rdf:resource="http://sparql.cwrc.ca/ontologies/genre-ONTOLOGY_DATE"/>
    <void:inDataset rdf:resource="#datasetdefinition"/>
    <skos:inScheme rdf:resource="#Genre"/>
    <rdf:type rdf:resource="http://www.w3.org/2004/02/skos/core#Concept"/>
    <skos:definition xml:lang="en">A eulogy (from εὐλογία, eulogia, Classical Greek for &quot;praise&quot;) is a speech or writing in praise of a person(s) or thing(s), especially one who recently died or retired or as a term of endearment. Eulogies may be given as part of funeral services. They take place in a funeral home during or after a wake. However, some denominations either discourage or do not permit eulogies at services to maintain respect for traditions. Eulogies can also praise people who are still alive. This normally takes place on special occasions like birthdays, office parties, retirement celebrations, etc. Eulogies should not be confused with elegies, which are poems written in tribute to the dead; nor with obituaries, which are published biographies recounting the lives of those who have recently died; nor with obsequies, which refer generally to the rituals surrounding funerals. Catholic priests are prohibited by the rubrics of the Mass from presenting a eulogy for the deceased in place of a homily during a funeral Mass. The modern use of the word eulogy was first documented in the 15th century and came from the Medieval Latin term “eulogium” (Merriam-Webster 2012). “Eulogium” at that time has since turned into the shorter “eulogy” of today. Eulogies are usually delivered by a family member or a close family friend in the case of a dead person. For a living eulogy given in such cases as a retirement, a senior colleague could perhaps deliver it. On occasions, eulogies are given to those who are severely ill or elderly in order to express words of love and gratitude before they die. Eulogies are not limited to merely people, however; Places or things can also be given eulogies (which anyone can deliver), but these are less common than those delivered to people, whether living or deceased.</skos:definition>
    <skos:definition xml:lang="fr">L’éloge (masculin du latin elogium, avec l’influence du grec εὐλογία) est un genre littéraire hérité de l'Antiquité, où il est très présent, qui consiste à vanter les mérites d'un individu ou d'une institution. Il s'agit d'un discours public ou donné comme tel, destiné à l'édification commune ; à cette fin, il recourt à l'exploitation des ressources du discours épidictique héritées de la rhétorique classique. Il existe plusieurs sortes d'éloges:</skos:definition>
    <skos:definition xml:lang="es">El encomio es un texto de alabanza en honor a algo o alguien. Junto a su opuesto, que es el vituperio, textos insultantes, compone el género epidíctico cuyo objetivo práctico es argumentar y que se incluye dentro de la retórica. Podía realizarse en lírica o prosa, según el tono deseado. El encomio era un importante ejercicio de oratoria.</skos:definition>
    <skos:definition xml:lang="nl">Een eulogie (uit het Grieks εὐλογία, letterlijk: goed woord) is een lofrede of lofdicht uitgesproken bij een speciale gelegenheid zoals een verjaardag. Het begrip moet niet verward worden met een elegie, die geschreven wordt als eerbetoon aan een overleden persoon. <![CDATA[<a href="#_dbpedia_2017">(DBpedia, 2017)</a>]]></skos:definition>
    <prov:derivedFrom rdf:resource="http://dbpedia.org/resource/Eulogy"/>
    <rdfs:comment xml:lang="en">The description for this term is indebted to DBpedia. </rdfs:comment>
  </genre:Genre>
  <genre:Genre rdf:about="#genreExhibitioncatalogue">
    <rdf:value>EXHIBITIONCATALOGUE</rdf:value>
    <rdfs:label xml:lang="en">exhibition catalogue</rdfs:label>
    <rdfs:label xml:lang="fr"/>
    <rdfs:isDefinedBy rdf:resource="http://sparql.cwrc.ca/ontologies/genre-ONTOLOGY_DATE"/>
    <void:inDataset rdf:resource="#datasetdefinition"/>
    <skos:inScheme rdf:resource="#Genre"/>
    <rdf:type rdf:resource="http://www.w3.org/2004/02/skos/core#Concept"/>
    <skos:definition xml:lang="en">Publications that document the works displayed in an exhibition. <![CDATA[<a href="#_getty_2017">(Getty, 2017)</a>]]></skos:definition>
    <skos:definition xml:lang="de">Druckwerk, das die in einer Ausstellung gezeigten Werke dokumentiert. <![CDATA[<a href="#_getty_2017">(Getty, 2017)</a>]]></skos:definition>
    <prov:derivedFrom rdf:resource="http://vocab.getty.edu/aat/300026096"/>
    <rdfs:comment xml:lang="en">The description for this term is indebted to the Getty Art &amp; Architecture Thesaurus.</rdfs:comment>
  </genre:Genre>
  <genre:Genre rdf:about="#genreFable">
    <rdf:value>FABLE</rdf:value>
    <rdfs:label xml:lang="en">fable</rdfs:label>
    <rdfs:label xml:lang="fr"/>
    <rdfs:isDefinedBy rdf:resource="http://sparql.cwrc.ca/ontologies/genre-ONTOLOGY_DATE"/>
    <void:inDataset rdf:resource="#datasetdefinition"/>
    <skos:inScheme rdf:resource="#Genre"/>
    <rdf:type rdf:resource="http://www.w3.org/2004/02/skos/core#Concept"/>
    <skos:definition xml:lang="en">Fictitious narratives usually with animals or inanimate objects as protagonists, intended to convey a hidden meaning regarding human conduct. <![CDATA[<a href="#_getty_2017">(Getty, 2017)</a>]]></skos:definition>
    <skos:definition xml:lang="de">Fiktionale Erzählung, deren Protagonisten in der Regel Tiere oder unbelebte Objekte sind, mit dem Ziel, unterschwellig menschliches Verhalten darzustellen. <![CDATA[<a href="#_getty_2017">(Getty, 2017)</a>]]></skos:definition>
    <skos:definition xml:lang="es">Narraciones imaginarias que generalmente tienen como protagonistas a animales u objetos inanimados, destinadas a transmitir un mensaje oculto relativo a la conducta humana. <![CDATA[<a href="#_getty_2017">(Getty, 2017)</a>]]></skos:definition>
    <skos:definition xml:lang="nl">Verzonnen verhalen, meestal met dieren of levenloze voorwerpen als hoofdpersonen, waarin gewoonlijk een boodschap met betrekking tot menselijk gedrag wordt verborgen. <![CDATA[<a href="#_getty_2017">(Getty, 2017)</a>]]></skos:definition>
    <prov:derivedFrom rdf:resource="http://vocab.getty.edu/aat/300055917"/>
    <rdfs:comment xml:lang="en">The description for this term is indebted to the Getty Art &amp; Architecture Thesaurus.</rdfs:comment>
    <skos:definition xml:lang="en">A brief story illustrating human tendencies through animal characters. Unlike the parables, fables often include talking animals or animated objects as the principal characters. The interaction of these animals or objects reveals general truths about human nature, i.e., a person can learn practical lessons from the fictional antics in a fable. However, unlike a parable, the lesson learned is not necessarily allegorical. Each animal is not necessarily a symbol for something else. Instead, the reader learns the lesson as an exemplum--an example of what one should or should not do. The sixth century (BCE) Greek writer Aesop is most credited as an author of fables, but Phaedrus and Babrius in the first century (CE) expanded on his works to produce the tales we know today. A famous collection of Indian fables was the Sanskrit Bidpai (circa 300 CE), and in the medieval period, Marie de France (c. 1200 CE) composed 102 fables in verse. After the 1600s, fables increasingly became common as a form of children's literature. See also allegory, beast fable, and parable. Click here for a PDF handout discussing the difference between fables and parables. <![CDATA[<a href="#_wheeler_2017">(L. K Wheeler, 2017)</a>]]></skos:definition>
    <prov:derivedFrom rdf:resource="http://web.cn.edu/kwheeler/lit_terms_f.html"/>
    <rdfs:comment xml:lang="en">The description for this term is indebted to Dr. L. Kip Wheeler of Carson-Newman University. </rdfs:comment>
  </genre:Genre>
  <genre:Genre rdf:about="#genreFabliau">
    <rdf:value>FABLIAU</rdf:value>
    <rdfs:label xml:lang="en">fabliau</rdfs:label>
    <rdfs:label xml:lang="fr"/>
    <rdfs:isDefinedBy rdf:resource="http://sparql.cwrc.ca/ontologies/genre-ONTOLOGY_DATE"/>
    <void:inDataset rdf:resource="#datasetdefinition"/>
    <skos:inScheme rdf:resource="#Genre"/>
    <rdf:type rdf:resource="http://www.w3.org/2004/02/skos/core#Concept"/>
    <skos:definition xml:lang="en">plural, fabliaux): A humorous, frequently ribald or &quot;dirty&quot; narrative popular with French poets, who traditionally wrote the story in octosyllabic couplets. The tales frequently revolve around trickery, practical jokes, sexual mishaps, scatology, mistaken identity, and bodily humor. Chaucer included several fabliaux in The Canterbury Tales, including the stories of the Shipman, the Friar, the Miller, the Reeve, and the Cook. Examples from French literature include Les Quatre Souhais Saint Martin, Audigier, and Beranger au Long Cul (Beranger of the Long Ass). <![CDATA[<a href="#_wheeler_2017">(L. K Wheeler, 2017)</a>]]></skos:definition>
    <prov:derivedFrom rdf:resource="http://web.cn.edu/kwheeler/lit_terms_f.html"/>
    <rdfs:comment xml:lang="en">The description for this term is indebted to Dr. L. Kip Wheeler of Carson-Newman University. </rdfs:comment>
  </genre:Genre>
  <genre:Genre rdf:about="#genreFairytale">
    <rdf:value>FAIRYTALE</rdf:value>
    <rdfs:label xml:lang="en">fairytale</rdfs:label>
    <rdfs:label xml:lang="fr"/>
    <rdfs:isDefinedBy rdf:resource="http://sparql.cwrc.ca/ontologies/genre-ONTOLOGY_DATE"/>
    <void:inDataset rdf:resource="#datasetdefinition"/>
    <skos:inScheme rdf:resource="#Genre"/>
    <rdf:type rdf:resource="http://www.w3.org/2004/02/skos/core#Concept"/>
    <skos:definition xml:lang="en">Fairytale fantasy is distinguished from other subgenres of fantasy by the works' heavy use of motifs, and often plots, from folklore. <![CDATA[<a href="#_dbpedia_2017">(DBpedia, 2017)</a>]]></skos:definition>
    <prov:derivedFrom rdf:resource="http://dbpedia.org/resource/Fairytale_fantasy"/>
    <rdfs:comment xml:lang="en">The description for this term is indebted to DBpedia. </rdfs:comment>
    <skos:definition xml:lang="en">Narratives set in the distant past recounting events impossible in the real world, often magical and with fairies, but with humans as heroes and heroines. <![CDATA[<a href="#_getty_2017">(Getty, 2017)</a>]]></skos:definition>
    <skos:definition xml:lang="de">Erzählung, die in der entfernten Vergangenheit spielt und von Ereignissen berichtet, die nicht in der realen Welt geschehen, häufig mit magischen Elementen und Feen, aber mit menschlichen Helden und Heldinnen. <![CDATA[<a href="#_getty_2017">(Getty, 2017)</a>]]></skos:definition>
    <skos:definition xml:lang="nl">Verhalen die zich afspelen in een ver verleden en waarin gebeurtenissen worden beschreven die in de echte wereld onmogelijk zouden kunnen plaatsvinden.  Hoewel het vaak magische verhalen zijn waarin allerlei fantasiefiguren voorkomen, worden de hoofdrollen door mensen vertolkt. <![CDATA[<a href="#_getty_2017">(Getty, 2017)</a>]]></skos:definition>
    <skos:definition xml:lang="es">Conjunto de narraciones situadas en el pasado distante que narran sucesos imposibles en el mundo real, a veces mágicos y con hadas, pero con seres humanos como héroes o heroínas. <![CDATA[<a href="#_getty_2017">(Getty, 2017)</a>]]></skos:definition>
    <skos:definition xml:lang="zh-hant">背景設定在遙遠的過去，敘述在真實世界不可能發生的故事。常有魔法與仙女，但男女主角為人類。 <![CDATA[<a href="#_getty_2017">(Getty, 2017)</a>]]></skos:definition>
    <prov:derivedFrom rdf:resource="http://vocab.getty.edu/aat/300185684"/>
    <rdfs:comment xml:lang="en">The description for this term is indebted to the Getty Art &amp; Architecture Thesaurus.</rdfs:comment>
  </genre:Genre>
  <genre:Genre rdf:about="#genreFantasy">
    <rdf:value>FANTASY</rdf:value>
    <rdfs:label xml:lang="en">fantasy</rdfs:label>
    <rdfs:label xml:lang="fr"/>
    <rdfs:isDefinedBy rdf:resource="http://sparql.cwrc.ca/ontologies/genre-ONTOLOGY_DATE"/>
    <void:inDataset rdf:resource="#datasetdefinition"/>
    <skos:inScheme rdf:resource="#Genre"/>
    <rdf:type rdf:resource="http://www.w3.org/2004/02/skos/core#Concept"/>
    <skos:definition xml:lang="en">Literary genre in which works are of a whimsical or visionary nature, having suppositions that are speculation or resting on no solid grounds. <![CDATA[<a href="#_getty_2017">(Getty, 2017)</a>]]></skos:definition>
    <prov:derivedFrom rdf:resource="http://vocab.getty.edu/aat/300380290"/>
    <rdfs:comment xml:lang="en">The description for this term is indebted to the Getty Art &amp; Architecture Thesaurus.</rdfs:comment>
    <skos:definition xml:lang="fr">La fantasy, ou fantasie (terme issu de l’anglais fantasy : « imagination » ; à ne pas confondre avec la fantaisie musicale, ni avec le terme allemand phantasie qui désigne le concept psychologique de fantasme), est un genre littéraire présentant un ou plusieurs éléments surnaturels qui relèvent souvent du mythe et qui sont souvent incarnés par l’irruption ou l’utilisation de la magie. La fantasy fait partie des littératures de l'imaginaire. Dans la fantasy comme dans le merveilleux, le surnaturel est généralement accepté, voire utilisé pour définir les règles d'un monde imaginaire, et n'est pas nécessairement objet de doute ou de peur. Cela distingue la fantasy du fantastique où le surnaturel fait intrusion dans les règles du monde habituel, et de l'horreur où il suscite peur et angoisse. Par extension, à partir du genre littéraire, on parle aussi de fantasy à propos d'illustrations, de bandes dessinées, de films, de jeux, etc.</skos:definition>
    <skos:definition xml:lang="de">Fantasy (von engl. fantasy „Phantasie“) ist ein Genre der Phantastik, dessen Wurzeln sich in der Mythologie und den Sagen finden. Ähnlich wie die benachbarten Genres Science-Fiction und Horror, findet Fantasy ihre wichtigsten Ausprägungen in Literatur und Film, außerdem aber auch in Musik und bildender Kunst sowie im Bereich der Gesellschaftsspiele, Computerspiele sowie Pen-&amp;-Paper- und Live-Rollenspiele.</skos:definition>
    <skos:definition xml:lang="es">El género fantástico, comúnmente llamado fantasía, es un género artístico en el cual los elementos principales del argumento son imaginarios, irreales y sobrenaturales. En su sentido más amplio, el género fantástico se halla presente en la literatura, cinematografía, historieta, videojuegos, juegos de rol, pintura, escultura, drama y, sobre todo, en la mitología y relatos antiguos, donde tuvo su origen. Se caracteriza por no dar prioridad a una representación realista que respete las leyes de funcionamiento del mundo real. En ese sentido se suele decir que el género fantástico es subversivo, pues viola las normas de la realidad. Generalmente se lo distingue de otras formas artísticas como la ciencia ficción –en la que también se subvierten los mecanismos de funcionamiento de la realidad conocida– aduciendo que la causa de los fenómenos observados en obras de corte fantástico siempre tienen que ver con fuerzas sobrenaturales mientras que en la ciencia ficción hay causas “cientifizadas”, con explicaciones que buscan la racionalidad dentro de su ruptura con el orden conocido. Por eso, algunos autores opinan que la diferencia entre el relato fantástico y el de ciencia-ficción radica no tanto en los hechos sobrenaturales sino en el modo en que el autor presenta y explica los mismos.</skos:definition>
    <skos:definition xml:lang="nl">Fantasy is een apart genre binnen diverse media-, kunst- en cultuurvormen zoals films, televisie, literatuur, computerspellen, festivals, muziek, en dergelijke. Het is een genre dat zich kenmerkt door het gebruik van fictieve verhalen, verzonnen wezens en imaginaire werelden. Bovendien spelen magie en andere bovennatuurlijke elementen veelal een belangrijke rol in het genre. Toch is fantasy meestal duidelijk te onderscheiden van aanverwante genres als sciencefiction en horror, die de meeste van de bovenstaande kenmerken ook kunnen bezitten. Dit onderscheid is vooral te vinden in de toon, de stijl en de manier waarop diverse thema's behandeld worden. Daarnaast focussen sciencefiction en horror zich respectievelijk op bepaalde elementen als 'toekomst en techniek' en 'angst en mysterie', terwijl in fantasy de bovengenoemde kenmerken centraal staan. Vaak lijken fantasy-verhalen zich af te spelen in een onbestemd en mythisch verleden, waarin &quot;bovennatuurlijke&quot; verschijnselen of een daarmee samenhangende sfeer alledaags lijken (zoals tovenarij), terwijl het met name bij sciencefiction daarentegen veelal gaat om een setting in een al dan niet onbestemd &quot;futuristisch&quot; verschiet, waarin technisch vernuft een belangrijke rol speelt (zoals ruimtereizen). <![CDATA[<a href="#_dbpedia_2017">(DBpedia, 2017)</a>]]></skos:definition>
    <prov:derivedFrom rdf:resource="http://dbpedia.org/resource/Fantasy"/>
    <rdfs:comment xml:lang="en">The description for this term is indebted to DBpedia. </rdfs:comment>
  </genre:Genre>
  <genre:Genre rdf:about="#genreFarce">
    <rdf:value>FARCE</rdf:value>
    <rdfs:label xml:lang="en">farce</rdfs:label>
    <rdfs:label xml:lang="fr"/>
    <rdfs:isDefinedBy rdf:resource="http://sparql.cwrc.ca/ontologies/genre-ONTOLOGY_DATE"/>
    <void:inDataset rdf:resource="#datasetdefinition"/>
    <skos:inScheme rdf:resource="#Genre"/>
    <rdf:type rdf:resource="http://www.w3.org/2004/02/skos/core#Concept"/>
    <skos:definition xml:lang="en">(from Latin Farsus, &quot;stuffed&quot;): A farce is a form of low comedy designed to provoke laughter through highly exaggerated caricatures of people in improbable or silly situations. Traits of farce include (1) physical bustle such as slapstick, (2) sexual misunderstandings and mix-ups, and (3) broad verbal humor such as puns. Many literary critics (especially in the Victorian period) have tended to view farce as inferior to &quot;high comedy&quot; that involves brilliant dialogue. Many of Shakespeare's early works, such as The Taming of the Shrew, are considered farces. Contrast with comedy of manners. <![CDATA[<a href="#_wheeler_2017">(L. K Wheeler, 2017)</a>]]></skos:definition>
    <prov:derivedFrom rdf:resource="http://web.cn.edu/kwheeler/lit_terms_f.html"/>
    <rdfs:comment xml:lang="en">The description for this term is indebted to Dr. L. Kip Wheeler of Carson-Newman University. </rdfs:comment>
  </genre:Genre>
  <genre:Genre rdf:about="#genreFeminist">
    <rdf:value>FEMINIST</rdf:value>
    <rdfs:label xml:lang="en">feminist</rdfs:label>
    <rdfs:label xml:lang="fr"/>
    <rdfs:isDefinedBy rdf:resource="http://sparql.cwrc.ca/ontologies/genre-ONTOLOGY_DATE"/>
    <void:inDataset rdf:resource="#datasetdefinition"/>
    <skos:inScheme rdf:resource="#Genre"/>
    <rdf:type rdf:resource="http://www.w3.org/2004/02/skos/core#Concept"/>
    <skos:definition xml:lang="en">Writing concerned with the unique experience of being a woman or alternatively writing designed to challenge existing preconceptions of gender. Examples of feminist writings include Christine de Pisan's medieval work, The City of Ladies; Aemilia Lanyer's Renaissance treatise, Salve Deus, Rex Judaeorum (which presented the then-shocking idea that Adam was just as much to blame for the fall of man as Eve was in the Genesis account); Mary Wollstonecraft's Vindication, and Susan B. Anthony's nineteenth-century essays (which presented the equally shocking idea that women in America and Canada should have the right to vote). Many female students in my class preface their discussions of feminist writings by stating, &quot;I'm not a feminist, but ...&quot; This tendency always puzzled me, since it implies that feminism is something negative, radical, or always liberal. Worse yet, it implies that it's bad for women to want crazy, misguided things like education, equal health insurance, similar pay to what men earn in similar professions, freedom from harassment, and funding for medical problems concerning women, such as breast and uterine cancer research, which are the primary concerns of feminism. Somewhere toward the end of the twentieth-century, detractors of such writers have caricatured these demands as &quot;man-hating&quot; or &quot;anti-family.&quot; As an antidote to such thinking, keep in mind the broader definition: a feminist is anyone who thinks that women are people too.<![CDATA[<a href="#_wheeler_2017">(L. K Wheeler, 2017)</a>]]></skos:definition>
    <prov:derivedFrom rdf:resource="http://web.cn.edu/kwheeler/lit_terms_f.html"/>
    <rdfs:comment xml:lang="en">The description for this term is indebted to Dr. L. Kip Wheeler of Carson-Newman University. </rdfs:comment>
  </genre:Genre>
  <genre:Genre rdf:about="#genreFeministtheory">
    <rdf:value>FEMINISTTHEORY</rdf:value>
    <rdfs:label xml:lang="en">feminist theory</rdfs:label>
    <rdfs:label xml:lang="fr"/>
    <rdfs:isDefinedBy rdf:resource="http://sparql.cwrc.ca/ontologies/genre-ONTOLOGY_DATE"/>
    <void:inDataset rdf:resource="#datasetdefinition"/>
    <skos:inScheme rdf:resource="#Genre"/>
    <rdf:type rdf:resource="http://www.w3.org/2004/02/skos/core#Concept"/>
  </genre:Genre>
  <genre:Genre rdf:about="#genreFiction">
    <rdf:value>FICTION</rdf:value>
    <rdfs:label xml:lang="en">fiction</rdfs:label>
    <rdfs:label xml:lang="fr">fiction</rdfs:label>
    <rdfs:isDefinedBy rdf:resource="http://sparql.cwrc.ca/ontologies/genre-ONTOLOGY_DATE"/>
    <void:inDataset rdf:resource="#datasetdefinition"/>
    <skos:inScheme rdf:resource="#Genre"/>
    <rdf:type rdf:resource="http://www.w3.org/2004/02/skos/core#Concept"/>
    <skos:definition xml:lang="en">Poetic or prosaic literary forms derived from medieval narratives of love, legendary or heroic adventures, and chivalry. Extends to narratives about important religious figures, or fantastic or supernatural events. <![CDATA[<a href="#_getty_2017">(Getty, 2017)</a>]]></skos:definition>
    <skos:definition xml:lang="nl">Vertellingen in proza of versvorm, zich vaak afspelend in de middeleeuwen, waarin grootse, fantastische of bovennatuurlijke gebeurtenissen worden beschreven. <![CDATA[<a href="#_getty_2017">(Getty, 2017)</a>]]></skos:definition>
    <skos:definition xml:lang="es">Narraciones en verso o prosa que relatan sucesos heroicos, fantásticos o sobrenaturales que a menudo transcurren en tiempos medievales. <![CDATA[<a href="#_getty_2017">(Getty, 2017)</a>]]></skos:definition>
    <skos:definition xml:lang="zh-hant">描述英雄事蹟、幻想，或超自然事件的詩文或散文體記敘文，常設定於中世紀時期。 <![CDATA[<a href="#_getty_2017">(Getty, 2017)</a>]]></skos:definition>
    <prov:derivedFrom rdf:resource="http://vocab.getty.edu/aat/300191065"/>
    <rdfs:comment xml:lang="en">The description for this term is indebted to the Getty Art &amp; Architecture Thesaurus.</rdfs:comment>
  </genre:Genre>
  <genre:Genre rdf:about="#genreFilmtvscript">
    <rdf:value>FILMTVSCRIPT</rdf:value>
    <rdfs:label xml:lang="en">film tv script</rdfs:label>
    <rdfs:label xml:lang="fr"/>
    <rdfs:isDefinedBy rdf:resource="http://sparql.cwrc.ca/ontologies/genre-ONTOLOGY_DATE"/>
    <void:inDataset rdf:resource="#datasetdefinition"/>
    <skos:inScheme rdf:resource="#Genre"/>
    <rdf:type rdf:resource="http://www.w3.org/2004/02/skos/core#Concept"/>
  </genre:Genre>
  <genre:Genre rdf:about="#genreFolksong">
    <rdf:value>FOLKSONG</rdf:value>
    <rdfs:label xml:lang="en">folksong</rdfs:label>
    <rdfs:label xml:lang="fr"/>
    <rdfs:isDefinedBy rdf:resource="http://sparql.cwrc.ca/ontologies/genre-ONTOLOGY_DATE"/>
    <void:inDataset rdf:resource="#datasetdefinition"/>
    <skos:inScheme rdf:resource="#Genre"/>
    <rdf:type rdf:resource="http://www.w3.org/2004/02/skos/core#Concept"/>
  </genre:Genre>
  <genre:Genre rdf:about="#genreGardeningbook">
    <rdf:value>GARDENINGBOOK</rdf:value>
    <rdfs:label xml:lang="en">gardening book</rdfs:label>
    <rdfs:label xml:lang="fr"/>
    <rdfs:isDefinedBy rdf:resource="http://sparql.cwrc.ca/ontologies/genre-ONTOLOGY_DATE"/>
    <void:inDataset rdf:resource="#datasetdefinition"/>
    <skos:inScheme rdf:resource="#Genre"/>
    <rdf:type rdf:resource="http://www.w3.org/2004/02/skos/core#Concept"/>
  </genre:Genre>
  <genre:Genre rdf:about="#genreGenealogy">
    <rdf:value>GENEALOGY</rdf:value>
    <rdfs:label xml:lang="en">genealogy</rdfs:label>
    <rdfs:label xml:lang="fr"/>
    <rdfs:isDefinedBy rdf:resource="http://sparql.cwrc.ca/ontologies/genre-ONTOLOGY_DATE"/>
    <void:inDataset rdf:resource="#datasetdefinition"/>
    <skos:inScheme rdf:resource="#Genre"/>
    <rdf:type rdf:resource="http://www.w3.org/2004/02/skos/core#Concept"/>
    <skos:definition xml:lang="en">Accounts or histories of the descent of persons, families, or other groups, from an ancestor or ancestors; enumerations of ancestors and their descendants in the natural order of succession. <![CDATA[<a href="#_getty_2017">(Getty, 2017)</a>]]></skos:definition>
    <skos:definition xml:lang="es">Documentos o historias de la ascendencia de personas, familias u otros grupos, desde un antepasado o antepasados, enumeraciones de antepasados y su descendencia en el orden natural de sucesión. <![CDATA[<a href="#_getty_2017">(Getty, 2017)</a>]]></skos:definition>
    <skos:definition xml:lang="nl">Verslagen van of verhalen over de afkomst van personen, families of andere groepen mensen beginnende bij één of meer gemeenschappelijke voorouders; opsommingen van voorouders en hun afstammelingen in volgorde van nakomelingschap. <![CDATA[<a href="#_getty_2017">(Getty, 2017)</a>]]></skos:definition>
    <skos:definition xml:lang="de">Bericht oder Chronik über die Abstammung von Personen, Familien oder anderen Gruppen von einem oder mehreren Vorfahren; Auflistung der Vorfahren und ihrer Nachkommen in natürlicher Abfolge. <![CDATA[<a href="#_getty_2017">(Getty, 2017)</a>]]></skos:definition>
    <skos:definition xml:lang="zh-hant">從一位祖先或諸位祖先開始的個人、家庭，或其他群體之記述或歷史；依繼承自然順序列舉祖先與其後裔。 <![CDATA[<a href="#_getty_2017">(Getty, 2017)</a>]]></skos:definition>
    <prov:derivedFrom rdf:resource="http://vocab.getty.edu/aat/300027015"/>
    <rdfs:comment xml:lang="en">The description for this term is indebted to the Getty Art &amp; Architecture Thesaurus.</rdfs:comment>
  </genre:Genre>
  <genre:Genre rdf:about="#genreGeorgic">
    <rdf:value>GEORGIC</rdf:value>
    <rdfs:label xml:lang="en">georgic</rdfs:label>
    <rdfs:label xml:lang="fr"/>
    <rdfs:isDefinedBy rdf:resource="http://sparql.cwrc.ca/ontologies/genre-ONTOLOGY_DATE"/>
    <void:inDataset rdf:resource="#datasetdefinition"/>
    <skos:inScheme rdf:resource="#Genre"/>
    <rdf:type rdf:resource="http://www.w3.org/2004/02/skos/core#Concept"/>
  </genre:Genre>
  <genre:Genre rdf:about="#genreGhoststory">
    <rdf:value>GHOSTSTORY</rdf:value>
    <rdfs:label xml:lang="en">ghost story</rdfs:label>
    <rdfs:label xml:lang="fr"/>
    <rdfs:isDefinedBy rdf:resource="http://sparql.cwrc.ca/ontologies/genre-ONTOLOGY_DATE"/>
    <void:inDataset rdf:resource="#datasetdefinition"/>
    <skos:inScheme rdf:resource="#Genre"/>
    <rdf:type rdf:resource="http://www.w3.org/2004/02/skos/core#Concept"/>
    <skos:definition xml:lang="fr">Les histoires de fantôme sont un sous-genre du fantastique. Dans ces histoires, le fantôme est souvent le héros et a une personnalité et une identité bien à lui. Le genre peut aussi donner lieu à des récits centrés uniquement sur les fantômes ou les morts. <![CDATA[<a href="#_dbpedia_2017">(DBpedia, 2017)</a>]]></skos:definition>
    <prov:derivedFrom rdf:resource="http://dbpedia.org/resource/Ghost_story"/>
    <rdfs:comment xml:lang="en">The description for this term is indebted to DBpedia. </rdfs:comment>
    <skos:definition xml:lang="en">Prose tales of the supernatural in which the living encounter manifestations of the spirits of the dead. <![CDATA[<a href="#_getty_2017">(Getty, 2017)</a>]]></skos:definition>
    <skos:definition xml:lang="de">Prosaerzählung vom Übernatürlichen, in der die Lebenden den Geistern der Toten begegnen. <![CDATA[<a href="#_getty_2017">(Getty, 2017)</a>]]></skos:definition>
    <skos:definition xml:lang="nl">Prozavertellingen over het bovennatuurlijke, waarin levende figuren in aanraking komen met verschijningen van de geesten van doden. <![CDATA[<a href="#_getty_2017">(Getty, 2017)</a>]]></skos:definition>
    <skos:definition xml:lang="es">Cuentos sobrenaturales en prosa en los que seres vivos tienen encuentros con manifestaciones de los espíritus de los muertos. <![CDATA[<a href="#_getty_2017">(Getty, 2017)</a>]]></skos:definition>
    <skos:definition xml:lang="zh-hant">超自然的散文體故事，敘述活人與死者現形的靈魂相遇。 <![CDATA[<a href="#_getty_2017">(Getty, 2017)</a>]]></skos:definition>
    <prov:derivedFrom rdf:resource="http://vocab.getty.edu/aat/300254823"/>
    <rdfs:comment xml:lang="en">The description for this term is indebted to the Getty Art &amp; Architecture Thesaurus.</rdfs:comment>
  </genre:Genre>
  <genre:Genre rdf:about="#genreGiftbook">
    <rdf:value>GIFTBOOK</rdf:value>
    <rdfs:label xml:lang="en">giftbook</rdfs:label>
    <rdfs:label xml:lang="fr"/>
    <rdfs:isDefinedBy rdf:resource="http://sparql.cwrc.ca/ontologies/genre-ONTOLOGY_DATE"/>
    <void:inDataset rdf:resource="#datasetdefinition"/>
    <skos:inScheme rdf:resource="#Genre"/>
    <rdf:type rdf:resource="http://www.w3.org/2004/02/skos/core#Concept"/>
    <skos:definition xml:lang="en">Books, usually illustrated literary anthologies, intended to be given as gifts and often published annually; popular in the 19th century. For works produced to mark an occasion, use &quot;keepsakes (books).&quot; <![CDATA[<a href="#_getty_2017">(Getty, 2017)</a>]]></skos:definition>
    <skos:definition xml:lang="es">Úsese para libros, generalmente antologías literarias ilustradas, para ser obsequiados y a menudo publicados anualmente; populares en el siglo XIX. Para obras producidas para destacar una ocasión, use &quot;recuerdo (libros)&quot;. <![CDATA[<a href="#_getty_2017">(Getty, 2017)</a>]]></skos:definition>
    <skos:definition xml:lang="nl">Wordt gebruikt voor boeken, meestal geïllustreerde literaire bloemlezingen, die bedoeld zijn om cadeau te worden gedaan en die vaak jaarlijks worden uitgegeven. Dergelijke boeken waren met name tijdens de 19e eeuw in zwang. Gebruik `gedenkschriften' voor werken die worden opgesteld ter gedachtenis van een bepaalde gebeurtenis. <![CDATA[<a href="#_getty_2017">(Getty, 2017)</a>]]></skos:definition>
    <skos:definition xml:lang="zh-hant">通常附插圖的文學選集。流行於十九世紀，往往一年出版一次，大多作為贈禮用。為標誌某重大時刻而製作的作品，則使用「紀念品（書）」一詞。 <![CDATA[<a href="#_getty_2017">(Getty, 2017)</a>]]></skos:definition>
    <prov:derivedFrom rdf:resource="http://vocab.getty.edu/aat/300202541"/>
    <rdfs:comment xml:lang="en">The description for this term is indebted to the Getty Art &amp; Architecture Thesaurus.</rdfs:comment>
  </genre:Genre>
  <genre:Genre rdf:about="#genreGothic">
    <rdf:value>GOTHIC</rdf:value>
    <rdfs:label xml:lang="en">gothic</rdfs:label>
    <rdfs:label xml:lang="fr">gothique</rdfs:label>
    <rdfs:isDefinedBy rdf:resource="http://sparql.cwrc.ca/ontologies/genre-ONTOLOGY_DATE"/>
    <void:inDataset rdf:resource="#datasetdefinition"/>
    <skos:inScheme rdf:resource="#Genre"/>
    <rdf:type rdf:resource="http://www.w3.org/2004/02/skos/core#Concept"/>
    <skos:definition xml:lang="en">Romantic fictions having a prevailing atmosphere of mystery and terror, often combined with a love story. The genre was introduced in England ca. 1765, but soon became popular elsewhere in Europe, reaching its heyday in the 1790s. The genre has undergone frequent revivals in subsequent centuries. It is called &quot;Gothic&quot; because the early examples were often set in part among medieval buildings and ruins, such as castles or monasteries. <![CDATA[<a href="#_getty_2017">(Getty, 2017)</a>]]></skos:definition>
    <skos:definition xml:lang="de">Romantische Prosa, die in einer Atmosphäre des Mysteriösen und Schreckensvollen spielt, häufig im Zusammenhang mit einer Liebesgeschichte. Das Genre wurde ca. 1765 in England entwickelt, wurde aber bald in ganz Europa beliebt und erreichte in den 1790er Jahren seine Blütezeit. In den nachfolgenden Jahrhunderten hat das Genre viele Wiederbelebungen erfahren. Es wird im Emglischen &quot;Gothic&quot; genannt, weil die frühen Beispiele oftmals zu Teilen in mittelalterlichen Bauten und Ruinen spielten, wie beispielsweise in Burgen oder Klöstern. <![CDATA[<a href="#_getty_2017">(Getty, 2017)</a>]]></skos:definition>
    <skos:definition xml:lang="zh-hant">瀰漫神秘與恐怖氛圍的浪漫小說，常與愛情故事結合。此一文類約於1765年始自英國，但迅即在歐洲其他地區流行，於1790年代達到顛峰。爾後本類型文體經歷頻繁的復興。稱「哥德體」係因早期作品常有部份設定於城堡或修道院之類的中世紀建築與遺跡裡。 <![CDATA[<a href="#_getty_2017">(Getty, 2017)</a>]]></skos:definition>
    <skos:definition xml:lang="nl">Romans met een combinatie van mystery, romantiek en horror. Dit genre ontstond in circa 1765 in Engeland, maar werd ook elders in Europa al snel populair, met het hoogtepunt in de jaren negentig van de achttiende eeuw. Het genre beleefde in de daaropvolgende eeuwen regelmatig een wederopbloei. Men noemde dit soort romans ���gotisch' omdat ze zich aanvankelijk vaak gedeeltelijk afspeelden in middeleeuwse ruïnes en gebouwen, zoals kastelen en kloosters. <![CDATA[<a href="#_getty_2017">(Getty, 2017)</a>]]></skos:definition>
    <prov:derivedFrom rdf:resource="http://vocab.getty.edu/aat/300266777"/>
    <rdfs:comment xml:lang="en">The description for this term is indebted to the Getty Art &amp; Architecture Thesaurus.</rdfs:comment>
  </genre:Genre>
  <genre:Genre rdf:about="#genreGovernmentreport">
    <rdf:value>GOVERNMENTREPORT</rdf:value>
    <rdfs:label xml:lang="en">government report</rdfs:label>
    <rdfs:label xml:lang="fr"/>
    <rdfs:isDefinedBy rdf:resource="http://sparql.cwrc.ca/ontologies/genre-ONTOLOGY_DATE"/>
    <void:inDataset rdf:resource="#datasetdefinition"/>
    <skos:inScheme rdf:resource="#Genre"/>
    <rdf:type rdf:resource="http://www.w3.org/2004/02/skos/core#Concept"/>
  </genre:Genre>
  <genre:Genre rdf:about="#genreGrammar">
    <rdf:value>GRAMMAR</rdf:value>
    <rdfs:label xml:lang="en">grammar</rdfs:label>
    <rdfs:label xml:lang="fr"/>
    <rdfs:isDefinedBy rdf:resource="http://sparql.cwrc.ca/ontologies/genre-ONTOLOGY_DATE"/>
    <void:inDataset rdf:resource="#datasetdefinition"/>
    <skos:inScheme rdf:resource="#Genre"/>
    <rdf:type rdf:resource="http://www.w3.org/2004/02/skos/core#Concept"/>
    <skos:definition xml:lang="en">GRAMMAR: Another term for transformational grammar. <![CDATA[<a href="#_wheeler_2017">(L. K Wheeler, 2017)</a>]]></skos:definition>
    <prov:derivedFrom rdf:resource="http://web.cn.edu/kwheeler/lit_terms_g.html"/>
    <rdfs:comment xml:lang="en">The description for this term is indebted to Dr. L. Kip Wheeler of Carson-Newman University. </rdfs:comment>
  </genre:Genre>
  <genre:Genre rdf:about="#genreGraveyardpoetry">
    <rdf:value>GRAVEYARDPOETRY</rdf:value>
    <rdfs:label xml:lang="en">graveyard poetry</rdfs:label>
    <rdfs:label xml:lang="fr"/>
    <rdfs:isDefinedBy rdf:resource="http://sparql.cwrc.ca/ontologies/genre-ONTOLOGY_DATE"/>
    <void:inDataset rdf:resource="#datasetdefinition"/>
    <skos:inScheme rdf:resource="#Genre"/>
    <rdf:type rdf:resource="http://www.w3.org/2004/02/skos/core#Concept"/>
    <skos:broaderTransitive rdf:resource="#genrePoetry"/>
  </genre:Genre>
  <genre:Genre rdf:about="#genreGuidebook">
    <rdf:value>GUIDEBOOK</rdf:value>
    <rdfs:label xml:lang="en">guidebook</rdfs:label>
    <rdfs:label xml:lang="fr"/>
    <rdfs:isDefinedBy rdf:resource="http://sparql.cwrc.ca/ontologies/genre-ONTOLOGY_DATE"/>
    <void:inDataset rdf:resource="#datasetdefinition"/>
    <skos:inScheme rdf:resource="#Genre"/>
    <rdf:type rdf:resource="http://www.w3.org/2004/02/skos/core#Concept"/>
    <skos:definition xml:lang="en">Handbooks for the guidance of strangers or visitors in a district, town, building, etc., giving a description of the roads, places, or objects of interest to be found there. <![CDATA[<a href="#_getty_2017">(Getty, 2017)</a>]]></skos:definition>
    <skos:definition xml:lang="de">Handbuch für Fremde oder Reisende mit Informationen über ein Gebiet, eine Stadt, ein Gebäude usw., in dem Straßen, Plätze, oder Sehenswürdigkeiten beschrieben werden. <![CDATA[<a href="#_getty_2017">(Getty, 2017)</a>]]></skos:definition>
    <skos:definition xml:lang="es">Manuales con direcciones e informaciones, por ejemplo para viajeros. <![CDATA[<a href="#_getty_2017">(Getty, 2017)</a>]]></skos:definition>
    <skos:definition xml:lang="nl">Handleidingen met aanwijzingen en informatie, bijvoorbeeld voor reizigers. <![CDATA[<a href="#_getty_2017">(Getty, 2017)</a>]]></skos:definition>
    <prov:derivedFrom rdf:resource="http://vocab.getty.edu/aat/300026300"/>
    <rdfs:comment xml:lang="en">The description for this term is indebted to the Getty Art &amp; Architecture Thesaurus.</rdfs:comment>
  </genre:Genre>
  <genre:Genre rdf:about="#genreHagiography">
    <rdf:value>HAGIOGRAPHY</rdf:value>
    <rdfs:label xml:lang="en">hagiography</rdfs:label>
    <rdfs:label xml:lang="fr"/>
    <rdfs:isDefinedBy rdf:resource="http://sparql.cwrc.ca/ontologies/genre-ONTOLOGY_DATE"/>
    <void:inDataset rdf:resource="#datasetdefinition"/>
    <skos:inScheme rdf:resource="#Genre"/>
    <rdf:type rdf:resource="http://www.w3.org/2004/02/skos/core#Concept"/>
    <skos:definition xml:lang="en">Biographies of saints, usually written, but includes oral or visual works as well.</skos:definition>
    <skos:definition xml:lang="nl">Biografieën van heiligen.</skos:definition>
    <skos:definition xml:lang="es">Biografías de santos.</skos:definition>
    <skos:definition xml:lang="de">Biografie eines Heiligen. <![CDATA[<a href="#_getty_2017">(Getty, 2017)</a>]]></skos:definition>
    <prov:derivedFrom rdf:resource="http://vocab.getty.edu/aat/300201063"/>
    <rdfs:comment xml:lang="en">The description for this term is indebted to the Getty Art &amp; Architecture Thesaurus.</rdfs:comment>
    <skos:definition xml:lang="fr">L’hagiographie (du grec ancien ἅγιος / hágios (« saint ») et γράφειν / gráphein (« écrire »)) est l'écriture de la vie et / ou de l'œuvre des saints. Pour un texte particulier, on ne parle que rarement d'« une hagiographie » (sauf dans le sens figuré), mais plutôt d'un texte hagiographique ou tout simplement d'une vie de saint. Le texte hagiographique étant destiné à être lu, soit lors de l'office des moines soit en public dans le cadre de la prédication, on lui donne souvent le nom de légende (du latin legenda, « ce qui doit être lu », terme utilisé dans son acception la plus littérale et non dans son sens péjoratif actuel de récit dépourvu de tout enracinement dans l'histoire événementielle). Un texte hagiographique recouvre plusieurs genres littéraires ou artistiques parmi lesquels on compte en premier lieu la vita, c'est-à-dire le récit biographique de la vie du saint. Une fresque à épisode est également une hagiographie, de même qu'une simple notice résumant la vie du bienheureux. Par rapport à une biographie, l'hagiographie est un genre littéraire qui veut mettre en avant le caractère de sainteté du personnage dont on raconte la vie. L'écrivain, l'hagiographe n'a pas d'abord une démarche d'historien, surtout lorsque le genre hagiographique s'est déployé. Aussi les hagiographies anciennes sont parsemées de passages merveilleux à l'historicité douteuse. De plus, des typologies de saints existaient au Moyen Âge, ce qui a conduit les hagiographes à se conformer à ces modèles et à faire de nombreux emprunts à des récits antérieurs. L'hagiographie est ainsi un récit fortement stéréotypé dont la fonction pastorale est de servir à l'instruction et l'édification religieuse, mais qui peut avoir aussi une fonction normative, politique et de propagande religieuse. D'une manière plus polémique, on parle aussi d'hagiographie pour désigner un écrit (une biographie, l'analyse d'un système philosophique, etc.) trop favorable à son objet, c'est-à-dire manquant de recul et/ou ne laissant guère de place à la critique. <![CDATA[<a href="#_dbpedia_2017">(DBpedia, 2017)</a>]]></skos:definition>
    <prov:derivedFrom rdf:resource="http://dbpedia.org/resource/Hagiography"/>
    <rdfs:comment xml:lang="en">The description for this term is indebted to DBpedia. </rdfs:comment>
    <skos:definition xml:lang="en">Saints' lives as a branch of literature or legend. <![CDATA[<a href="#_getty_2017">(Getty, 2017)</a>]]></skos:definition>
    <prov:derivedFrom rdf:resource="http://vocab.getty.edu/aat/300055909"/>
    <rdfs:comment xml:lang="en">The description for this term is indebted to the Getty Art &amp; Architecture Thesaurus.</rdfs:comment>
  </genre:Genre>
  <genre:Genre rdf:about="#genreHaiku">
    <rdf:value>HAIKU</rdf:value>
    <rdfs:label xml:lang="en">haiku</rdfs:label>
    <rdfs:label xml:lang="fr"/>
    <rdfs:isDefinedBy rdf:resource="http://sparql.cwrc.ca/ontologies/genre-ONTOLOGY_DATE"/>
    <void:inDataset rdf:resource="#datasetdefinition"/>
    <skos:inScheme rdf:resource="#Genre"/>
    <rdf:type rdf:resource="http://www.w3.org/2004/02/skos/core#Concept"/>
    <skos:definition xml:lang="en">(plural: haiku, from archaic Japanese): The term haiku is a fairly late addition to Japanese poetry. The poet Shiki coined the term in the nineteenth century from a longer, more traditional phrase, haikai renga no hokku (&quot;the introductory lines of light linked verse&quot;). To understand the haiku's history as a genre, peruse the vocabulary entries for its predecessors, the hokku and the haikai renga or renku. The haiku follows several conventions: Many Japanese poets have used the form, the two acknowledged masters being Bashó (a nom de plume for Matsuo Munefusa, 1644-94); and Kobayashi Issa (a nom de plume for Kobayashi Nobuyuki). The Imagist Movement in 20th century English literature has been profoundly influenced by haiku. The list of poets who attempted the haiku or admired the genre includes Ezra Pound, Amy Lowell, Robert Frost, Conrad Aiken, and W. B. Yeats. Contrast haiku with the tanka and the senryu. See also hokku, below, and haikai, above. See also kigo and imagism. You can click here to download a PDF handout summarizing this discussion of haiku, or you can click here to download PDF samples of haiku. <![CDATA[<a href="#_wheeler_2017">(L. K Wheeler, 2017)</a>]]></skos:definition>
    <prov:derivedFrom rdf:resource="http://web.cn.edu/kwheeler/lit_terms_h.html"/>
    <rdfs:comment xml:lang="en">The description for this term is indebted to Dr. L. Kip Wheeler of Carson-Newman University. </rdfs:comment>
  </genre:Genre>
  <genre:Genre rdf:about="#genreHarlequinade">
    <rdf:value>HARLEQUINADE</rdf:value>
    <rdfs:label xml:lang="en">harlequinade</rdfs:label>
    <rdfs:label xml:lang="fr"/>
    <rdfs:isDefinedBy rdf:resource="http://sparql.cwrc.ca/ontologies/genre-ONTOLOGY_DATE"/>
    <void:inDataset rdf:resource="#datasetdefinition"/>
    <skos:inScheme rdf:resource="#Genre"/>
    <rdf:type rdf:resource="http://www.w3.org/2004/02/skos/core#Concept"/>
  </genre:Genre>
  <genre:Genre rdf:about="#genreHeroic">
    <rdf:value>HEROIC</rdf:value>
    <rdfs:label xml:lang="en">heroic</rdfs:label>
    <rdfs:label xml:lang="fr"/>
    <rdfs:isDefinedBy rdf:resource="http://sparql.cwrc.ca/ontologies/genre-ONTOLOGY_DATE"/>
    <void:inDataset rdf:resource="#datasetdefinition"/>
    <skos:inScheme rdf:resource="#Genre"/>
    <rdf:type rdf:resource="http://www.w3.org/2004/02/skos/core#Concept"/>
    <skos:definition xml:lang="en">Form of poetry comprising long narratives celebrating on a grand scale the adventures and deeds of one or more heroic figures, ordinarily concerning a serious subject significant to a culture or nation. Classical epic poetry employs dactylic hexameter and recounts a journey. <![CDATA[<a href="#_getty_2017">(Getty, 2017)</a>]]></skos:definition>
    <prov:derivedFrom rdf:resource="http://vocab.getty.edu/aat/300404208"/>
    <rdfs:comment xml:lang="en">The description for this term is indebted to the Getty Art &amp; Architecture Thesaurus.</rdfs:comment>
  </genre:Genre>
  <genre:Genre rdf:about="#genreHistorical">
    <rdf:value>HISTORICAL</rdf:value>
    <rdfs:label xml:lang="en">historical</rdfs:label>
    <rdfs:label xml:lang="fr">historique</rdfs:label>
    <rdfs:isDefinedBy rdf:resource="http://sparql.cwrc.ca/ontologies/genre-ONTOLOGY_DATE"/>
    <void:inDataset rdf:resource="#datasetdefinition"/>
    <skos:inScheme rdf:resource="#Genre"/>
    <rdf:type rdf:resource="http://www.w3.org/2004/02/skos/core#Concept"/>
    <skos:definition xml:lang="en">Refers to maps that indicate political administrative boundaries or other characteristics of a region at periods of time before the present. They typically include historical names for places, historical population dispositions, and the historical state of physical features. <![CDATA[<a href="#_getty_2017">(Getty, 2017)</a>]]></skos:definition>
    <skos:definition xml:lang="de">Bezieht sich auf eine Karte, die politische Verwaltungsgrenzen oder andere Charakteristiken eines Gebietes zu einem Zeitpunkt darstellt, der vor der Gegenwart liegt. In der Regel beinhaltet sie historische Ortsnamen, die historische Bevölkerungsentwicklung und den historischen Zustand geografischer Merkmale. <![CDATA[<a href="#_getty_2017">(Getty, 2017)</a>]]></skos:definition>
    <skos:definition xml:lang="nl">Verwijst naar kaarten waarop politieke bestuurlijke grenzen of andere kenmerken van een regio uit het verleden zijn weergegeven. Meestal bevatten ze historische namen van plaatsen, de historische spreiding van bevolkingsgroepen en de historische situatie van fysieke kenmerken. <![CDATA[<a href="#_getty_2017">(Getty, 2017)</a>]]></skos:definition>
    <skos:definition xml:lang="es">Se refiere a mapas que indican las fronteras político- administrativas u otras características de una región en períodos anteriores al presente. Incluyen generalmente los nombres históricos de lugares, las conductas históricas de las poblaciones, y el estado histórico de las características físicas. <![CDATA[<a href="#_getty_2017">(Getty, 2017)</a>]]></skos:definition>
    <skos:definition xml:lang="zh-hant">標明一區域在過往時期的政治行政界線或其他特點的地圖。通常包括地方的歷史名稱、歷史上的人口排列、與地表特徵的歷史狀態等。 <![CDATA[<a href="#_getty_2017">(Getty, 2017)</a>]]></skos:definition>
    <prov:derivedFrom rdf:resource="http://vocab.getty.edu/aat/300028233"/>
    <rdfs:comment xml:lang="en">The description for this term is indebted to the Getty Art &amp; Architecture Thesaurus.</rdfs:comment>
  </genre:Genre>
  <genre:Genre rdf:about="#genreHistory">
    <rdf:value>HISTORY</rdf:value>
    <rdfs:label xml:lang="en">history</rdfs:label>
    <rdfs:label xml:lang="fr"/>
    <rdfs:isDefinedBy rdf:resource="http://sparql.cwrc.ca/ontologies/genre-ONTOLOGY_DATE"/>
    <void:inDataset rdf:resource="#datasetdefinition"/>
    <skos:inScheme rdf:resource="#Genre"/>
    <rdf:type rdf:resource="http://www.w3.org/2004/02/skos/core#Concept"/>
    <skos:definition xml:lang="en">Chronological records of significant events, as of the life or development of a people, country, or institution, often with an explanation of the causes. <![CDATA[<a href="#_getty_2017">(Getty, 2017)</a>]]></skos:definition>
    <skos:definition xml:lang="de">Chronologische Aufzeichnung bedeutungsvoller Ereignisse, wie beispielsweise das Leben oder die Entwicklung eines Volkes, Landes oder einer Institution, häufig mit einer Erklärung des Geschehens. <![CDATA[<a href="#_getty_2017">(Getty, 2017)</a>]]></skos:definition>
    <skos:definition xml:lang="nl">Aanduiding voor chronologische verslagen van gebeurtenissen, zoals het leven of de ontwikkeling van een volk, land of instituut. <![CDATA[<a href="#_getty_2017">(Getty, 2017)</a>]]></skos:definition>
    <skos:definition xml:lang="es">Úsese para designar registros cronológicos de sucesos, como de la vida o el desarrollo de un pueblo, país o institución. <![CDATA[<a href="#_getty_2017">(Getty, 2017)</a>]]></skos:definition>
    <skos:definition xml:lang="zh-hant">依時間先後排列的事件紀錄，例如一個民族、國家、或社會組織的生活或其發展。 <![CDATA[<a href="#_getty_2017">(Getty, 2017)</a>]]></skos:definition>
    <prov:derivedFrom rdf:resource="http://vocab.getty.edu/aat/300026358"/>
    <rdfs:comment xml:lang="en">The description for this term is indebted to the Getty Art &amp; Architecture Thesaurus.</rdfs:comment>
  </genre:Genre>
  <genre:Genre rdf:about="#genreHymn">
    <rdf:value>HYMN</rdf:value>
    <rdfs:label xml:lang="en">hymn</rdfs:label>
    <rdfs:label xml:lang="fr"/>
    <rdfs:isDefinedBy rdf:resource="http://sparql.cwrc.ca/ontologies/genre-ONTOLOGY_DATE"/>
    <void:inDataset rdf:resource="#datasetdefinition"/>
    <skos:inScheme rdf:resource="#Genre"/>
    <rdf:type rdf:resource="http://www.w3.org/2004/02/skos/core#Concept"/>
    <skos:definition xml:lang="en">A religious song consisting of one or more repeating rhythmical stanzas. In classical Roman literature, hymns to Minerva and Jupiter survive. The Greek poet Sappho wrote a number of hymns to Aphrodite. More recently a vast number of hymns appear in Catholic and Protestant religious lyrics. A particularly vibrant tradition of hymn-writing comes from the South's African-American population during the nineteenth century. In the realm of fiction, C.S. Lewis creates hymns for the Solid Ones in The Great Divorce, and Tolkien creates Elvish hymns such as &quot;O Elbereth&quot; in The Lord of the Rings, typically with quatrain structure alternating with couplet stanzas. In the example of &quot;O Elbereth,&quot; the hymn honors one of the Maiar spirits. See also paean. <![CDATA[<a href="#_wheeler_2017">(L. K Wheeler, 2017)</a>]]></skos:definition>
    <prov:derivedFrom rdf:resource="http://web.cn.edu/kwheeler/lit_terms_h.html"/>
    <rdfs:comment xml:lang="en">The description for this term is indebted to Dr. L. Kip Wheeler of Carson-Newman University. </rdfs:comment>
  </genre:Genre>
  <genre:Genre rdf:about="#genreImitation">
    <rdf:value>IMITATION</rdf:value>
    <rdfs:label xml:lang="en">imitation</rdfs:label>
    <rdfs:label xml:lang="fr"/>
    <rdfs:isDefinedBy rdf:resource="http://sparql.cwrc.ca/ontologies/genre-ONTOLOGY_DATE"/>
    <void:inDataset rdf:resource="#datasetdefinition"/>
    <skos:inScheme rdf:resource="#Genre"/>
    <rdf:type rdf:resource="http://www.w3.org/2004/02/skos/core#Concept"/>
  </genre:Genre>
  <genre:Genre rdf:about="#genreIndustrialnovel">
    <rdf:value>INDUSTRIALNOVEL</rdf:value>
    <rdfs:label xml:lang="en">industrial novel</rdfs:label>
    <rdfs:label xml:lang="fr"/>
    <rdfs:isDefinedBy rdf:resource="http://sparql.cwrc.ca/ontologies/genre-ONTOLOGY_DATE"/>
    <void:inDataset rdf:resource="#datasetdefinition"/>
    <skos:inScheme rdf:resource="#Genre"/>
    <rdf:type rdf:resource="http://www.w3.org/2004/02/skos/core#Concept"/>
    <skos:broaderTransitive rdf:resource="#genreNovel"/>
  </genre:Genre>
  <genre:Genre rdf:about="#genreIntroduction">
    <rdf:value>INTRODUCTION</rdf:value>
    <rdfs:label xml:lang="en">introduction</rdfs:label>
    <rdfs:label xml:lang="fr"/>
    <rdfs:isDefinedBy rdf:resource="http://sparql.cwrc.ca/ontologies/genre-ONTOLOGY_DATE"/>
    <void:inDataset rdf:resource="#datasetdefinition"/>
    <skos:inScheme rdf:resource="#Genre"/>
    <rdf:type rdf:resource="http://www.w3.org/2004/02/skos/core#Concept"/>
  </genre:Genre>
  <genre:Genre rdf:about="#genreJournalism">
    <rdf:value>JOURNALISM</rdf:value>
    <rdfs:label xml:lang="en">journalism</rdfs:label>
    <rdfs:label xml:lang="fr"/>
    <rdfs:isDefinedBy rdf:resource="http://sparql.cwrc.ca/ontologies/genre-ONTOLOGY_DATE"/>
    <void:inDataset rdf:resource="#datasetdefinition"/>
    <skos:inScheme rdf:resource="#Genre"/>
    <rdf:type rdf:resource="http://www.w3.org/2004/02/skos/core#Concept"/>
  </genre:Genre>
  <genre:Genre rdf:about="#genreJuvenilia">
    <rdf:value>JUVENILIA</rdf:value>
    <rdfs:label xml:lang="en">juvenilia</rdfs:label>
    <rdfs:label xml:lang="fr"/>
    <rdfs:isDefinedBy rdf:resource="http://sparql.cwrc.ca/ontologies/genre-ONTOLOGY_DATE"/>
    <void:inDataset rdf:resource="#datasetdefinition"/>
    <skos:inScheme rdf:resource="#Genre"/>
    <rdf:type rdf:resource="http://www.w3.org/2004/02/skos/core#Concept"/>
    <skos:definition xml:lang="en">Literary or artistic works produced by persons in their childhood or youth; usually used to set those works apart from later, mature works. <![CDATA[<a href="#_getty_2017">(Getty, 2017)</a>]]></skos:definition>
    <skos:definition xml:lang="de">schriftstellerisches oder künstlerisches Werk aus der Kindheit oder der Jugend einer Person; in der Regel verwendet, um diese Werke von den später entstandenen,  reifen Werken abzusetzen. <![CDATA[<a href="#_getty_2017">(Getty, 2017)</a>]]></skos:definition>
    <skos:definition xml:lang="nl">Literair of artistiek werk dat de maker heeft vervaardigd in zijn kindertijd of jeugd; wordt meestal gebruikt om deze werken te onderscheiden van later, volwassen werk. <![CDATA[<a href="#_getty_2017">(Getty, 2017)</a>]]></skos:definition>
    <skos:definition xml:lang="es">Obras literarias o artísticas producidas por personas en su niñez o juventud; usualmente usadas para ubicar aquellas obras aparte de las posteriores, obras maduras. <![CDATA[<a href="#_getty_2017">(Getty, 2017)</a>]]></skos:definition>
    <skos:definition xml:lang="zh-hant">指個人在童年或青少年時期創作的文學或藝術作品，一般用以區別較後期的成熟作品。 <![CDATA[<a href="#_getty_2017">(Getty, 2017)</a>]]></skos:definition>
    <prov:derivedFrom rdf:resource="http://vocab.getty.edu/aat/300028883"/>
    <rdfs:comment xml:lang="en">The description for this term is indebted to the Getty Art &amp; Architecture Thesaurus.</rdfs:comment>
  </genre:Genre>
  <genre:Genre rdf:about="#genreKitchensinkdrama">
    <rdf:value>KITCHENSINKDRAMA</rdf:value>
    <rdfs:label xml:lang="en">kitchensink drama</rdfs:label>
    <rdfs:label xml:lang="fr"/>
    <rdfs:isDefinedBy rdf:resource="http://sparql.cwrc.ca/ontologies/genre-ONTOLOGY_DATE"/>
    <void:inDataset rdf:resource="#datasetdefinition"/>
    <skos:inScheme rdf:resource="#Genre"/>
    <rdf:type rdf:resource="http://www.w3.org/2004/02/skos/core#Concept"/>
  </genre:Genre>
  <genre:Genre rdf:about="#genreKunstlerroman">
    <rdf:value>KUNSTLERROMAN</rdf:value>
    <rdfs:label xml:lang="en">kunstlerroman</rdfs:label>
    <rdfs:label xml:lang="fr"/>
    <rdfs:isDefinedBy rdf:resource="http://sparql.cwrc.ca/ontologies/genre-ONTOLOGY_DATE"/>
    <void:inDataset rdf:resource="#datasetdefinition"/>
    <skos:inScheme rdf:resource="#Genre"/>
    <rdf:type rdf:resource="http://www.w3.org/2004/02/skos/core#Concept"/>
  </genre:Genre>
  <genre:Genre rdf:about="#genreLais">
    <rdf:value>LAIS</rdf:value>
    <rdfs:label xml:lang="en">lais</rdfs:label>
    <rdfs:label xml:lang="fr"/>
    <rdfs:isDefinedBy rdf:resource="http://sparql.cwrc.ca/ontologies/genre-ONTOLOGY_DATE"/>
    <void:inDataset rdf:resource="#datasetdefinition"/>
    <skos:inScheme rdf:resource="#Genre"/>
    <rdf:type rdf:resource="http://www.w3.org/2004/02/skos/core#Concept"/>
    <skos:definition xml:lang="en">A laisse is a type of stanza, of varying length, found in medieval French literature, specifically medieval French epic poetry (the chanson de geste), such as The Song of Roland. In early works, each laisse was made up of (mono) assonanced verses, although the appearance of (mono) rhymed laisses was increasingly common in later poems. Within a poem, the length of each separate laisse is variable (whereas the metric length of the verses is invariable, each verse having the same syllable length, typically decasyllables or, occasionally, alexandrines. The laisse is characterized by stereotyped phrases and formulas and frequently repeated themes and motifs, including repetitions of material from one laisse to another. Such repetitions and formulaic structures are common of orality and oral-formulaic composition. When medieval poets repeated content (with different wording or assonance/rhyme) from one laisse to another, such &quot;similar&quot; laisses are called laisses similaires in French. <![CDATA[<a href="#_dbpedia_2017">(DBpedia, 2017)</a>]]></skos:definition>
    <prov:derivedFrom rdf:resource="http://dbpedia.org/resource/Laisse"/>
    <rdfs:comment xml:lang="en">The description for this term is indebted to DBpedia. </rdfs:comment>
  </genre:Genre>
  <genre:Genre rdf:about="#genreLampoon">
    <rdf:value>LAMPOON</rdf:value>
    <rdfs:label xml:lang="en">lampoon</rdfs:label>
    <rdfs:label xml:lang="fr"/>
    <rdfs:isDefinedBy rdf:resource="http://sparql.cwrc.ca/ontologies/genre-ONTOLOGY_DATE"/>
    <void:inDataset rdf:resource="#datasetdefinition"/>
    <skos:inScheme rdf:resource="#Genre"/>
    <rdf:type rdf:resource="http://www.w3.org/2004/02/skos/core#Concept"/>
    <skos:definition xml:lang="en">A coarse or crude satire ridiculing the appearance or character of another person. <![CDATA[<a href="#_wheeler_2017">(L. K Wheeler, 2017)</a>]]></skos:definition>
    <prov:derivedFrom rdf:resource="http://web.cn.edu/kwheeler/lit_terms_l.html"/>
    <rdfs:comment xml:lang="en">The description for this term is indebted to Dr. L. Kip Wheeler of Carson-Newman University. </rdfs:comment>
  </genre:Genre>
  <genre:Genre rdf:about="#genreLegalwriting">
    <rdf:value>LEGALWRITING</rdf:value>
    <rdfs:label xml:lang="en">legal writing</rdfs:label>
    <rdfs:label xml:lang="fr"/>
    <rdfs:isDefinedBy rdf:resource="http://sparql.cwrc.ca/ontologies/genre-ONTOLOGY_DATE"/>
    <void:inDataset rdf:resource="#datasetdefinition"/>
    <skos:inScheme rdf:resource="#Genre"/>
    <rdf:type rdf:resource="http://www.w3.org/2004/02/skos/core#Concept"/>
  </genre:Genre>
  <genre:Genre rdf:about="#genreLegendFolktale">
    <rdf:value>LEGENDFOLKTALE</rdf:value>
    <rdfs:label xml:lang="en">legend folktale</rdfs:label>
    <rdfs:label xml:lang="fr">légende et conte de fée</rdfs:label>
    <rdfs:isDefinedBy rdf:resource="http://sparql.cwrc.ca/ontologies/genre-ONTOLOGY_DATE"/>
    <void:inDataset rdf:resource="#datasetdefinition"/>
    <skos:inScheme rdf:resource="#Genre"/>
    <rdf:type rdf:resource="http://www.w3.org/2004/02/skos/core#Concept"/>
  </genre:Genre>
  <genre:Genre rdf:about="#genreLesbian">
    <rdf:value>LESBIAN</rdf:value>
    <rdfs:label xml:lang="en">lesbian</rdfs:label>
    <rdfs:label xml:lang="fr"/>
    <rdfs:isDefinedBy rdf:resource="http://sparql.cwrc.ca/ontologies/genre-ONTOLOGY_DATE"/>
    <void:inDataset rdf:resource="#datasetdefinition"/>
    <skos:inScheme rdf:resource="#Genre"/>
    <rdf:type rdf:resource="http://www.w3.org/2004/02/skos/core#Concept"/>
    <skos:definition xml:lang="en">Azalea: A Magazine by Third World Lesbians was a quarterly periodical for black, Asian, Latina, and Native American lesbians published between 1977 and 1983 by the Salsa Soul Sisters, Third World Wimmin Inc Collective. The Collective also published the Salsa Soul Sisters/Third World Women's Gay-zette (c. 1982). <![CDATA[<a href="#_dbpedia_2017">(DBpedia, 2017)</a>]]></skos:definition>
    <prov:derivedFrom rdf:resource="http://dbpedia.org/resource/Azalea:_A_Magazine_by_Third_World_Lesbians"/>
    <rdfs:comment xml:lang="en">The description for this term is indebted to DBpedia. </rdfs:comment>
  </genre:Genre>
  <genre:Genre rdf:about="#genreLetter">
    <rdf:value>LETTER</rdf:value>
    <rdfs:label xml:lang="en">letter</rdfs:label>
    <rdfs:label xml:lang="fr"/>
    <rdfs:isDefinedBy rdf:resource="http://sparql.cwrc.ca/ontologies/genre-ONTOLOGY_DATE"/>
    <void:inDataset rdf:resource="#datasetdefinition"/>
    <skos:inScheme rdf:resource="#Genre"/>
    <rdf:type rdf:resource="http://www.w3.org/2004/02/skos/core#Concept"/>
    <skos:definition xml:lang="en-gb">Letters written to a newspaper or magazine to present a position, make a correction, or respond to another story or letter. <![CDATA[<a href="#_getty_2017">(Getty, 2017)</a>]]></skos:definition>
    <prov:derivedFrom rdf:resource="http://vocab.getty.edu/aat/300343729"/>
    <rdfs:comment xml:lang="en">The description for this term is indebted to the Getty Art &amp; Architecture Thesaurus.</rdfs:comment>
  </genre:Genre>
  <genre:Genre rdf:about="#genreLettersfromthedeadtotheliving">
    <rdf:value>LETTERSFROMTHEDEADTOTHELIVING</rdf:value>
    <rdfs:label xml:lang="en">letters from the dead to the living</rdfs:label>
    <rdfs:label xml:lang="fr"/>
    <rdfs:isDefinedBy rdf:resource="http://sparql.cwrc.ca/ontologies/genre-ONTOLOGY_DATE"/>
    <void:inDataset rdf:resource="#datasetdefinition"/>
    <skos:inScheme rdf:resource="#Genre"/>
    <rdf:type rdf:resource="http://www.w3.org/2004/02/skos/core#Concept"/>
  </genre:Genre>
  <genre:Genre rdf:about="#genreLibretto">
    <rdf:value>LIBRETTO</rdf:value>
    <rdfs:label xml:lang="en">libretto</rdfs:label>
    <rdfs:label xml:lang="fr"/>
    <rdfs:isDefinedBy rdf:resource="http://sparql.cwrc.ca/ontologies/genre-ONTOLOGY_DATE"/>
    <void:inDataset rdf:resource="#datasetdefinition"/>
    <skos:inScheme rdf:resource="#Genre"/>
    <rdf:type rdf:resource="http://www.w3.org/2004/02/skos/core#Concept"/>
    <skos:definition xml:lang="en">Books or booklets containing the text or words of an opera or similar extended musical composition. <![CDATA[<a href="#_getty_2017">(Getty, 2017)</a>]]></skos:definition>
    <skos:definition xml:lang="de">Buch oder Heft mit dem Text einer Oper oder einer ähnlich umfänglichen musikalischen Komposition. <![CDATA[<a href="#_getty_2017">(Getty, 2017)</a>]]></skos:definition>
    <skos:definition xml:lang="es">Libros o folletos que contienen el texto o letras de una ópera o de una composición musical de similar extensión. <![CDATA[<a href="#_getty_2017">(Getty, 2017)</a>]]></skos:definition>
    <skos:definition xml:lang="nl">Boeken of boekjes waarin de tekst of de woorden van een opera of een vergelijkbaar, uitgewerkt muziekstuk staan. <![CDATA[<a href="#_getty_2017">(Getty, 2017)</a>]]></skos:definition>
    <prov:derivedFrom rdf:resource="http://vocab.getty.edu/aat/300026424"/>
    <rdfs:comment xml:lang="en">The description for this term is indebted to the Getty Art &amp; Architecture Thesaurus.</rdfs:comment>
  </genre:Genre>
  <genre:Genre rdf:about="#genreLiteraryCriticism">
    <rdf:value>LITERARYCRITICISM</rdf:value>
    <rdfs:label xml:lang="en">literary criticism</rdfs:label>
    <rdfs:label xml:lang="fr">critiquelittéraire</rdfs:label>
    <rdfs:isDefinedBy rdf:resource="http://sparql.cwrc.ca/ontologies/genre-ONTOLOGY_DATE"/>
    <void:inDataset rdf:resource="#datasetdefinition"/>
    <skos:inScheme rdf:resource="#Genre"/>
    <rdf:type rdf:resource="http://www.w3.org/2004/02/skos/core#Concept"/>
  </genre:Genre>
  <genre:Genre rdf:about="#genreLiturgy">
    <rdf:value>LITURGY</rdf:value>
    <rdfs:label xml:lang="en">liturgy</rdfs:label>
    <rdfs:label xml:lang="fr"/>
    <rdfs:isDefinedBy rdf:resource="http://sparql.cwrc.ca/ontologies/genre-ONTOLOGY_DATE"/>
    <void:inDataset rdf:resource="#datasetdefinition"/>
    <skos:inScheme rdf:resource="#Genre"/>
    <rdf:type rdf:resource="http://www.w3.org/2004/02/skos/core#Concept"/>
  </genre:Genre>
  <genre:Genre rdf:about="#genreLove">
    <rdf:value>LOVE</rdf:value>
    <rdfs:label xml:lang="en">love</rdfs:label>
    <rdfs:label xml:lang="fr"/>
    <rdfs:isDefinedBy rdf:resource="http://sparql.cwrc.ca/ontologies/genre-ONTOLOGY_DATE"/>
    <void:inDataset rdf:resource="#datasetdefinition"/>
    <skos:inScheme rdf:resource="#Genre"/>
    <rdf:type rdf:resource="http://www.w3.org/2004/02/skos/core#Concept"/>
    <prov:derivedFrom rdf:resource="http://dbpedia.org/resource/Christo"/>
    <rdfs:comment xml:lang="en">The description for this term is indebted to DBpedia. </rdfs:comment>
  </genre:Genre>
  <genre:Genre rdf:about="#genreLyric">
    <rdf:value>LYRIC</rdf:value>
    <rdfs:label xml:lang="en">lyric</rdfs:label>
    <rdfs:label xml:lang="fr">lyrique</rdfs:label>
    <rdfs:isDefinedBy rdf:resource="http://sparql.cwrc.ca/ontologies/genre-ONTOLOGY_DATE"/>
    <void:inDataset rdf:resource="#datasetdefinition"/>
    <skos:inScheme rdf:resource="#Genre"/>
    <rdf:type rdf:resource="http://www.w3.org/2004/02/skos/core#Concept"/>
    <skos:definition xml:lang="en">Lyric Essay is a subgenre of essay writing, which combines qualities of poetry, essay, memoir, and research writing. The lyric essay is considered high art, and often requires work and association on behalf of the reader. Proponents of the lyric essay classification insist it differs from prose poetry in its reliance on association rather than line breaks and juxtaposition. <![CDATA[<a href="#_dbpedia_2017">(DBpedia, 2017)</a>]]></skos:definition>
    <prov:derivedFrom rdf:resource="http://dbpedia.org/resource/Lyric_essay"/>
    <rdfs:comment xml:lang="en">The description for this term is indebted to DBpedia. </rdfs:comment>
  </genre:Genre>
  <genre:Genre rdf:about="#genreMagicrealist">
    <rdf:value>MAGICREALIST</rdf:value>
    <rdfs:label xml:lang="en">magic realist</rdfs:label>
    <rdfs:label xml:lang="fr"/>
    <rdfs:isDefinedBy rdf:resource="http://sparql.cwrc.ca/ontologies/genre-ONTOLOGY_DATE"/>
    <void:inDataset rdf:resource="#datasetdefinition"/>
    <skos:inScheme rdf:resource="#Genre"/>
    <rdf:type rdf:resource="http://www.w3.org/2004/02/skos/core#Concept"/>
  </genre:Genre>
  <genre:Genre rdf:about="#genreManifesto">
    <rdf:value>MANIFESTO</rdf:value>
    <rdfs:label xml:lang="en">manifesto</rdfs:label>
    <rdfs:label xml:lang="fr"/>
    <rdfs:isDefinedBy rdf:resource="http://sparql.cwrc.ca/ontologies/genre-ONTOLOGY_DATE"/>
    <void:inDataset rdf:resource="#datasetdefinition"/>
    <skos:inScheme rdf:resource="#Genre"/>
    <rdf:type rdf:resource="http://www.w3.org/2004/02/skos/core#Concept"/>
    <skos:definition xml:lang="en">Formal written declarations, promulgated by a sovereign or by the executive authority of a state or nation, such as to proclaim its reasons and motives for declaring a war, or other international action; also public declarations or proclamations of political, social, artistic, or other principles. <![CDATA[<a href="#_getty_2017">(Getty, 2017)</a>]]></skos:definition>
    <skos:definition xml:lang="es">Declaraciones formales escritas, promulgadas por un soberano o por la autoridad ejecutiva de un estado o nación, como aquellas que proclaman las razones y motivos para declarar una guerra u otra acción internacional; también declaraciones públicas o proclamaciones de principios políticos, sociales, artísticos y otros. <![CDATA[<a href="#_getty_2017">(Getty, 2017)</a>]]></skos:definition>
    <skos:definition xml:lang="nl">Formele, schriftelijke afkondigingen die worden uitgevaardigd door een vorst of door de uitvoerende autoriteiten van een staat of een natie, en waarin, bijvoorbeeld, de motieven voor een oorlogsverklaring, of een andere internationale actie bekend worden gemaakt. Wordt ook gebruikt voor openbare verklaringen of proclamaties van politieke, sociale, artistieke of andere beginselen. <![CDATA[<a href="#_getty_2017">(Getty, 2017)</a>]]></skos:definition>
    <prov:derivedFrom rdf:resource="http://vocab.getty.edu/aat/300026393"/>
    <rdfs:comment xml:lang="en">The description for this term is indebted to the Getty Art &amp; Architecture Thesaurus.</rdfs:comment>
  </genre:Genre>
  <genre:Genre rdf:about="#genreManual">
    <rdf:value>MANUAL</rdf:value>
    <rdfs:label xml:lang="en">manual</rdfs:label>
    <rdfs:label xml:lang="fr"/>
    <rdfs:isDefinedBy rdf:resource="http://sparql.cwrc.ca/ontologies/genre-ONTOLOGY_DATE"/>
    <void:inDataset rdf:resource="#datasetdefinition"/>
    <skos:inScheme rdf:resource="#Genre"/>
    <rdf:type rdf:resource="http://www.w3.org/2004/02/skos/core#Concept"/>
    <skos:definition xml:lang="en">Books or treatises, often compendious, containing rules or instructions needed to perform tasks, operations, processes, occupations, arts, or studies, and intended to be used as reference while the task or study is performed. <![CDATA[<a href="#_getty_2017">(Getty, 2017)</a>]]></skos:definition>
    <skos:definition xml:lang="de">Buch oder Abhandlung, oft in kompakter Form, mit Regeln oder Anweisungen, die für Ablauf oder Verrichtung einer Aufgabe, Arbeit, eines Prozesses oder einer Tätigkeit, für die Kunst oder wissenschaftliche Untersuchungen gebraucht werden und die während des Ablaufs einer Arbeit oder Untersuchung als Referenz dienen sollen. <![CDATA[<a href="#_getty_2017">(Getty, 2017)</a>]]></skos:definition>
    <skos:definition xml:lang="es">Libros, generalmente compactos, que contienen información concisa, a menudo las reglas o instrucciones necesarias para realizar tareas o procesos. <![CDATA[<a href="#_getty_2017">(Getty, 2017)</a>]]></skos:definition>
    <skos:definition xml:lang="nl">Wordt gebruikt voor, meestal compacte, boeken die beknopte informatie bevatten. Meestal gaat het om regels of aanwijzingen die men nodig heeft om bepaalde taken of processen te kunnen uitvoeren. <![CDATA[<a href="#_getty_2017">(Getty, 2017)</a>]]></skos:definition>
    <prov:derivedFrom rdf:resource="http://vocab.getty.edu/aat/300026395"/>
    <rdfs:comment xml:lang="en">The description for this term is indebted to the Getty Art &amp; Architecture Thesaurus.</rdfs:comment>
  </genre:Genre>
  <genre:Genre rdf:about="#genreMap">
    <rdf:value>MAP</rdf:value>
    <rdfs:label xml:lang="en">map</rdfs:label>
    <rdfs:label xml:lang="fr"/>
    <rdfs:isDefinedBy rdf:resource="http://sparql.cwrc.ca/ontologies/genre-ONTOLOGY_DATE"/>
    <void:inDataset rdf:resource="#datasetdefinition"/>
    <skos:inScheme rdf:resource="#Genre"/>
    <rdf:type rdf:resource="http://www.w3.org/2004/02/skos/core#Concept"/>
  </genre:Genre>
  <genre:Genre rdf:about="#genreMasque">
    <rdf:value>MASQUE</rdf:value>
    <rdfs:label xml:lang="en">masque</rdfs:label>
    <rdfs:label xml:lang="fr"/>
    <rdfs:isDefinedBy rdf:resource="http://sparql.cwrc.ca/ontologies/genre-ONTOLOGY_DATE"/>
    <void:inDataset rdf:resource="#datasetdefinition"/>
    <skos:inScheme rdf:resource="#Genre"/>
    <rdf:type rdf:resource="http://www.w3.org/2004/02/skos/core#Concept"/>
    <skos:definition xml:lang="en">Not to be confused with a masquerade, a masque is a type of elaborate court entertainment popular in the times of Queen Elizabeth I, King James I, and Charles I--i.e., the early 17th Century after Queen Elizabeth's death. The masque as a performance grew out of medieval plays, but it was more spectacle than drama proper. The content was suitable for amateur actors rather than professional performers. The masques tended to use long speeches and little action. They combined poetic drama, singing, dancing, music, and splendid costumes and settings. The imagery was influential on later poets and poems, such as Andrew Marvell, who makes use of masque-imagery in &quot;Upon Appleton House.&quot;<![CDATA[<a href="#_wheeler_2017">(L. K Wheeler, 2017)</a>]]></skos:definition>
    <prov:derivedFrom rdf:resource="http://web.cn.edu/kwheeler/lit_terms_m.html"/>
    <rdfs:comment xml:lang="en">The description for this term is indebted to Dr. L. Kip Wheeler of Carson-Newman University. </rdfs:comment>
  </genre:Genre>
  <genre:Genre rdf:about="#genreMedicalwriting">
    <rdf:value>MEDICALWRITING</rdf:value>
    <rdfs:label xml:lang="en">medical writing</rdfs:label>
    <rdfs:label xml:lang="fr"/>
    <rdfs:isDefinedBy rdf:resource="http://sparql.cwrc.ca/ontologies/genre-ONTOLOGY_DATE"/>
    <void:inDataset rdf:resource="#datasetdefinition"/>
    <skos:inScheme rdf:resource="#Genre"/>
    <rdf:type rdf:resource="http://www.w3.org/2004/02/skos/core#Concept"/>
  </genre:Genre>
  <genre:Genre rdf:about="#genreMelodrama">
    <rdf:value>MELODRAMA</rdf:value>
    <rdfs:label xml:lang="en">melodrama</rdfs:label>
    <rdfs:label xml:lang="fr"/>
    <rdfs:isDefinedBy rdf:resource="http://sparql.cwrc.ca/ontologies/genre-ONTOLOGY_DATE"/>
    <void:inDataset rdf:resource="#datasetdefinition"/>
    <skos:inScheme rdf:resource="#Genre"/>
    <rdf:type rdf:resource="http://www.w3.org/2004/02/skos/core#Concept"/>
    <skos:definition xml:lang="en">A dramatic form characterized by excessive sentiment, exaggerated emotion, sensational and thrilling action, and an artificially happy ending. Melodramas originally referred to romantic plays featuring music, singing, and dancing, but by the eighteenth century they connoted simplified and coincidental plots, bathos, and happy endings. These melodramatic traits are present in Gothic novels, western stories, popular films, and television crime shows, to name but a few more recent examples. <![CDATA[<a href="#_wheeler_2017">(L. K Wheeler, 2017)</a>]]></skos:definition>
    <prov:derivedFrom rdf:resource="http://web.cn.edu/kwheeler/lit_terms_m.html"/>
    <rdfs:comment xml:lang="en">The description for this term is indebted to Dr. L. Kip Wheeler of Carson-Newman University. </rdfs:comment>
  </genre:Genre>
  <genre:Genre rdf:about="#genreMixedmedia">
    <rdf:value>MIXEDMEDIA</rdf:value>
    <rdfs:label xml:lang="en">mixed media</rdfs:label>
    <rdfs:label xml:lang="fr"/>
    <rdfs:isDefinedBy rdf:resource="http://sparql.cwrc.ca/ontologies/genre-ONTOLOGY_DATE"/>
    <void:inDataset rdf:resource="#datasetdefinition"/>
    <skos:inScheme rdf:resource="#Genre"/>
    <rdf:type rdf:resource="http://www.w3.org/2004/02/skos/core#Concept"/>
  </genre:Genre>
  <genre:Genre rdf:about="#genreMockforms">
    <rdf:value>MOCKFORMS</rdf:value>
    <rdfs:label xml:lang="en">mockforms</rdfs:label>
    <rdfs:label xml:lang="fr"/>
    <rdfs:isDefinedBy rdf:resource="http://sparql.cwrc.ca/ontologies/genre-ONTOLOGY_DATE"/>
    <void:inDataset rdf:resource="#datasetdefinition"/>
    <skos:inScheme rdf:resource="#Genre"/>
    <rdf:type rdf:resource="http://www.w3.org/2004/02/skos/core#Concept"/>
  </genre:Genre>
  <genre:Genre rdf:about="#genreMonologue">
    <rdf:value>MONOLOGUE</rdf:value>
    <rdfs:label xml:lang="en">monologue</rdfs:label>
    <rdfs:label xml:lang="fr"/>
    <rdfs:isDefinedBy rdf:resource="http://sparql.cwrc.ca/ontologies/genre-ONTOLOGY_DATE"/>
    <void:inDataset rdf:resource="#datasetdefinition"/>
    <skos:inScheme rdf:resource="#Genre"/>
    <rdf:type rdf:resource="http://www.w3.org/2004/02/skos/core#Concept"/>
    <skos:definition xml:lang="en">In theatre, a monologue (from Greek μονόλογος from μόνος mónos, &quot;alone, solitary&quot; and λόγος lógos, &quot;speech&quot;) is a speech presented by a single character, most often to express their mental thoughts aloud, though sometimes also to directly address another character or the audience. Monologues are common across the range of dramatic media (plays, films, etc.), as well as in non-dramatic media such as poetry. Monologues share much in common with several other literary devices including soliloquies, apostrophes, and aside. There are, however, distinctions between each of these devices. <![CDATA[<a href="#_dbpedia_2017">(DBpedia, 2017)</a>]]></skos:definition>
    <skos:definition xml:lang="fr">Un monologue (du grec mono : &quot;un seul&quot;, et logos : &quot;discours&quot;) est une ou plusieurs phrases auto-adressées à haute voix, rapportant les pensées du locuteur au style direct.Il faut distinguer le véritable monologue non seulement, cela va de soi, du roman autobiographique à la première personne, qui suppose un décalage de temps, même minime (&quot;Aujourd'hui maman est morte&quot;) entre la narration et le narré, mais aussi d'une forme d'écriture fictionnelle moderne, la représentation du flux intérieur sous la forme je ou tu. <![CDATA[<a href="#_dbpedia_2017">(DBpedia, 2017)</a>]]></skos:definition>
    <skos:definition xml:lang="de">Der Monolog (gr. μόνος mónos „allein“ und -log; lat. Soliloquium) ist im Gegensatz zum Dialog ein Selbstgespräch und findet vor allem im Drama Verwendung. Er richtet sich nicht direkt an einen Zuhörer, sondern an eine imaginäre Person. Faktisch ist das Publikum Adressat des Monologisierenden. Eine Sonderform des Monologs ist der Innere Monolog in der Erzählprosa. Der Ausdruck Monolog bezeichnet auch eine Rede, die so formuliert ist, als sei sie nicht an einen Zuhörer oder Gesprächspartner gerichtet. Oftmals wird damit nicht das alltägliche Selbstgespräch bezeichnet, sondern der bewusste Einsatz des alleinigen Redens, in der Kunst, vor allem im Theater und in der Literatur, zusammen mit Gesten. Dort dient der Monolog häufig dazu, Gedanken und seelische Vorgänge einer Person hörbar oder lesbar nach außen zu tragen und damit für Zuschauer oder Leser deutlich werden zu lassen. In vielen Theaterstücken bilden Monologe einen dramatischen Höhepunkt oder bezeichnen einen Wendepunkt der Handlung. Ein bekanntes Beispiel dafür ist der Hamlet-Monolog von Shakespeare. Im Englischen, Französischen und anderen Sprachen wird in der Literaturwissenschaft noch eine wichtige Sonderform des Monologs unterschieden. Diese Sonderform wird als (engl.) Soliloquy bezeichnet und erlaubt im Drama – im Gegensatz zum Monolog – Zuhörer. in gewisser Weise handelt es sich um ein meist dramatisches Selbstgespräch. <![CDATA[<a href="#_dbpedia_2017">(DBpedia, 2017)</a>]]></skos:definition>
    <skos:definition xml:lang="es">Monólogo (del griego mono: uno; y logo: palabra) es un discurso que emite una sola persona tanto para un solo ente receptor como para hacia otros receptores (personajes, lectores, auditorio, a una cosa, a un personaje o a un narrador). El monólogo es un recurso utilizado en todos los géneros literarios que puede encontrarse tanto en poesía, cuento, periodismo, discusión, teatro, como en novela. <![CDATA[<a href="#_dbpedia_2017">(DBpedia, 2017)</a>]]></skos:definition>
    <skos:definition xml:lang="nl">Een monoloog is alleenspraak; een betoog van één persoon die aan het woord is (en blijft), vaak zonder dat er toehoorders zijn. Monoloog komt van het Grieks, waar μονος (monos) één en alleen betekent, en λογος (logos) woord of idee betekent. In het theater is het een toneeloptreden van één acteur binnen een toneelstuk. Daarvoor wordt vaak de term soliloque gebruikt. In een gesprek op een bijeenkomst betekent een monoloog dat de andere aanwezigen niet aan het woord kunnen of mogen komen. Een toespraak dus. Het is het tegengestelde van een dialoog. <![CDATA[<a href="#_dbpedia_2017">(DBpedia, 2017)</a>]]></skos:definition>
    <prov:derivedFrom rdf:resource="http://dbpedia.org/resource/Monologue"/>
    <rdfs:comment xml:lang="en">The description for this term is indebted to DBpedia. </rdfs:comment>
  </genre:Genre>
  <genre:Genre rdf:about="#genreMoralitymysteryplay">
    <rdf:value>MORALITYMYSTERYPLAY</rdf:value>
    <rdfs:label xml:lang="en">morality mystery play</rdfs:label>
    <rdfs:label xml:lang="fr"/>
    <rdfs:isDefinedBy rdf:resource="http://sparql.cwrc.ca/ontologies/genre-ONTOLOGY_DATE"/>
    <void:inDataset rdf:resource="#datasetdefinition"/>
    <skos:inScheme rdf:resource="#Genre"/>
    <rdf:type rdf:resource="http://www.w3.org/2004/02/skos/core#Concept"/>
  </genre:Genre>
  <genre:Genre rdf:about="#genreMultimedia">
    <rdf:value>MULTIMEDIA</rdf:value>
    <rdfs:label xml:lang="en">multimedia</rdfs:label>
    <rdfs:label xml:lang="fr"/>
    <rdfs:isDefinedBy rdf:resource="http://sparql.cwrc.ca/ontologies/genre-ONTOLOGY_DATE"/>
    <void:inDataset rdf:resource="#datasetdefinition"/>
    <skos:inScheme rdf:resource="#Genre"/>
    <rdf:type rdf:resource="http://www.w3.org/2004/02/skos/core#Concept"/>
  </genre:Genre>
  <genre:Genre rdf:about="#genreMusicology">
    <rdf:value>MUSICOLOGY</rdf:value>
    <rdfs:label xml:lang="en">musicology</rdfs:label>
    <rdfs:label xml:lang="fr"/>
    <rdfs:isDefinedBy rdf:resource="http://sparql.cwrc.ca/ontologies/genre-ONTOLOGY_DATE"/>
    <void:inDataset rdf:resource="#datasetdefinition"/>
    <skos:inScheme rdf:resource="#Genre"/>
    <rdf:type rdf:resource="http://www.w3.org/2004/02/skos/core#Concept"/>
  </genre:Genre>
  <genre:Genre rdf:about="#genreMystery">
    <rdf:value>MYSTERY</rdf:value>
    <rdfs:label xml:lang="en">mystery</rdfs:label>
    <rdfs:label xml:lang="fr"/>
    <rdfs:isDefinedBy rdf:resource="http://sparql.cwrc.ca/ontologies/genre-ONTOLOGY_DATE"/>
    <void:inDataset rdf:resource="#datasetdefinition"/>
    <skos:inScheme rdf:resource="#Genre"/>
    <rdf:type rdf:resource="http://www.w3.org/2004/02/skos/core#Concept"/>
    <skos:definition xml:lang="en">A novel focused on suspense and solving a mystery--especially a murder, theft, kidnapping, or some other crime. The protagonist faces inexplicable events, threats, assaults, and unknown forces or antagonists. Conventionally, the hero is a keenly observant individual (such as Sherlock Holmes) and the police are depicted as incompetent or incapable of solving the crime by themselves. Many of the works of Sir Arthur Conan Doyle, Edgar Allan Poe, and Agatha Christie are mystery novels.<![CDATA[<a href="#_wheeler_2017">(L. K Wheeler, 2017)</a>]]></skos:definition>
    <prov:derivedFrom rdf:resource="http://web.cn.edu/kwheeler/lit_terms_m.html"/>
    <rdfs:comment xml:lang="en">The description for this term is indebted to Dr. L. Kip Wheeler of Carson-Newman University. </rdfs:comment>
  </genre:Genre>
  <genre:Genre rdf:about="#genreMyth">
    <rdf:value>MYTH</rdf:value>
    <rdfs:label xml:lang="en">myth</rdfs:label>
    <rdfs:label xml:lang="fr"/>
    <rdfs:isDefinedBy rdf:resource="http://sparql.cwrc.ca/ontologies/genre-ONTOLOGY_DATE"/>
    <void:inDataset rdf:resource="#datasetdefinition"/>
    <skos:inScheme rdf:resource="#Genre"/>
    <rdf:type rdf:resource="http://www.w3.org/2004/02/skos/core#Concept"/>
    <skos:definition xml:lang="en">Legendary stories without a determinable basis of fact or natural explanation, typically concerning a being, hero, deity, or event and explains some practice, rite, or phenomenon of nature. <![CDATA[<a href="#_getty_2017">(Getty, 2017)</a>]]></skos:definition>
    <skos:definition xml:lang="de">Sagenhafte Geschichte ohne bestimmbare Faktengrundlage oder natürliche Erklärung, die in der Regel ein Wesen, einen Helden, eine Gottheit oder ein Ereignis zum Thema hat und eine bestimmte Praxis, einen Ritus oder ein Naturphänomen erklärt. <![CDATA[<a href="#_getty_2017">(Getty, 2017)</a>]]></skos:definition>
    <prov:derivedFrom rdf:resource="http://vocab.getty.edu/aat/300201023"/>
    <rdfs:comment xml:lang="en">The description for this term is indebted to the Getty Art &amp; Architecture Thesaurus.</rdfs:comment>
    <skos:definition xml:lang="fr">Un mythe est un récit qui se veut explicatif et surtout fondateur d'une pratique sociale. Il est porté à l'origine par une tradition orale, qui propose une explication pour certains aspects fondamentaux du monde et de la société qui a forgé ou qui véhicule ces mythes : L'étude des mythes est appelée mythologie. Le terme mythe est souvent employé pour désigner une croyance manifestement erronée au premier abord, mais qui peut se rapporter à des éléments concrets exprimés de façon symbolique et partagée par un nombre significatif de personnes. Le mythe se distingue de la légende (qui suppose quelques faits historiques identifiables), du conte (qui se veut inventif sans expliquer), et du roman (qui &quot;explique&quot; avec peu de fondements). <![CDATA[<a href="#_dbpedia_2017">(DBpedia, 2017)</a>]]></skos:definition>
    <skos:definition xml:lang="es">Un mito (del griego μῦθος, mythos, «relato», «cuento») es un relato tradicional que se refiere a acontecimientos prodigiosos, protagonizados por seres sobrenaturales o extraordinarios, tales como dioses, semidioses, héroes, monstruos o personajes fantásticos, los cuales buscan dar una explicación a un hecho o fenómeno. <![CDATA[<a href="#_dbpedia_2017">(DBpedia, 2017)</a>]]></skos:definition>
    <skos:definition xml:lang="nl">Mythe (Grieks: mythos; μυθος) betekende oorspronkelijk in het Grieks gesproken woord, verhaal.De betekenis is afhankelijk van de context: In tegenstelling tot wat bij sagen, sprookjes en fabels meestal het geval is, gaan mythen in hoofdzaak over goden en halfgoden. <![CDATA[<a href="#_dbpedia_2017">(DBpedia, 2017)</a>]]></skos:definition>
    <prov:derivedFrom rdf:resource="http://dbpedia.org/resource/Myth"/>
    <rdfs:comment xml:lang="en">The description for this term is indebted to DBpedia. </rdfs:comment>
  </genre:Genre>
  <genre:Genre rdf:about="#genreNarrativepoetry">
    <rdf:value>NARRATIVEPOETRY</rdf:value>
    <rdfs:label xml:lang="en">narrative poetry</rdfs:label>
    <rdfs:label xml:lang="fr"/>
    <rdfs:isDefinedBy rdf:resource="http://sparql.cwrc.ca/ontologies/genre-ONTOLOGY_DATE"/>
    <void:inDataset rdf:resource="#datasetdefinition"/>
    <skos:inScheme rdf:resource="#Genre"/>
    <rdf:type rdf:resource="http://www.w3.org/2004/02/skos/core#Concept"/>
    <skos:definition xml:lang="en">Narrative poetry is a form of poetry that tells a story, often making use of the voices of a narrator and characters as well; the entire story is usually written in metred verse. Narrative poems do not have to follow rhythmic patterns. The poems that make up this genre may be short or long, and the story it relates to may be complex. It is usually well it normally dramatic, with objectives, diverse characters, and metre. Narrative poems include epics, ballads, idylls, and lays. Some narrative poetry takes the form of a novel in verse. An example of this is The Ring and the Book by Robert Browning. In terms of narrative poetry, a romance is a narrative poem that tells a story of chivalry. Examples include the Romance of the Rose or Tennyson's Idylls of the King. Although these examples use medieval and Arthurian materials, romances may also tell stories from classical mythology. Shorter narrative poems are often similar in style to the short story. Sometimes these short narratives are collected into interrelated groups, as with Chaucer's The Canterbury Tales. Some literatures contain prose naose narratives, and the Old Norse sagas include both incidental poetry and the biographies of poets. An example is &quot;The Cremation of Sam McGee&quot; by Robert Service. <![CDATA[<a href="#_dbpedia_2017">(DBpedia, 2017)</a>]]></skos:definition>
    <skos:definition xml:lang="fr">La poésie narrative est un courant de la poésie italienne contemporaine dont les principaux représentants sont Carlo Bordini, Mauro Fabi et Andrea di Consoli. Cette poésie, qui sans renoncer à sa dimension expérimentale ou à une certaine forme de lyrisme exploite des matériaux divers - en usant du collage ou en incluant des fragments discursifs ou narratifs - et s'appuie sur le rythme et l'oralité non pour cacher le sens, mais pour le révéler. <![CDATA[<a href="#_dbpedia_2017">(DBpedia, 2017)</a>]]></skos:definition>
    <skos:definition xml:lang="de">Narrative Poesie ist dadurch gekennzeichnet, dass in ihr Handlung eine wesentliche Rolle spielt und dass sie weitgehend in Versen geschrieben ist. In der Poetik des Aristoteles war dieser Bereich allein durch das Epos abgedeckt, heute rechnen eine große Zahl von Mischformen dazu. In der Ballade finden sich oft Elemente aus allen drei Dichtungsgattungen erzählende, lyrische und dramatische. Idyllen und Lais haben meist primär erzählenden Charakter. Versromane unterscheiden sich vom modernen Roman nicht nur durch die Verwendung des Metrums, sondern haben auch inhaltliche Gemeinsamkeiten mit dem antiken Epos (Heldenreise). Das gilt auch für die Romanzen. In der Versnovelle, Beispiele sind Meier Helmbrecht und insbesondere Chaucers Canterbury Tales, sind dagegen kaum Unterschiede zu der zeitlich parallelen Prosa zu finden. Bei Chaucer stehen Prosa und Verserzählung nebeneinander. In manchen Dichtungsformen ist die Prosaerzählung stark von Versen durchsetzt, so in den altnordischen Sagas und in der Dichtung irischer Barden. <![CDATA[<a href="#_dbpedia_2017">(DBpedia, 2017)</a>]]></skos:definition>
    <skos:definition xml:lang="es">La narrativa poética o poesía narrativa es aquella que narra una historia. La longitud del poema y la complejidad de la historia varía de un poema a otro, no hay un criterio establecido. Por norma general, no suelen ser dramáticos, presentan versos objetivos y un esquema métrico y rima regular. Entre los poemas narrativos se encuentran la poesía épica, la poesía lírica, la balada y la égloga. Los poemas narrativos son una forma de arte. La poesía narrativa es uno de los más antiguos géneros dentro de la poesía. En la mayoría de las primeras obras literarias que se conocen, desde la epopeya de Gilgamesh hasta los poemas homéricos, tanto en la literatura en inglés antiguo como en la poesía en nórdico antiguo, así como la epopeya en sánscrito titulada Mahábharata, aparecen poemas narrativos. Muchos estudiosos de Homero, desde Quinto de Esmirna en adelante, han llegado a la conclusión de que los cuentos de la Ilíada y la Odisea fueron creados a partir de recopilaciones de poemas narrativos cortos que narraban historias individuales, las cuales resultaban más adecuadas para ser contadas alrededor de una hoguera. Algunos poemas narrativos deben ser considerados novelas en verso, como el extenso poema The Ring and the Book de Robert Browning. En cuanto a la poesía narrativa, un romance es un poema narrativo que cuentan historias de caballería. Algunos ejemplos son el Roman de la Rose, de Guillaume de Lorris, o los Idilios del rey, de Lord Tennyson. Aunque estos ejemplos describen historias medievales y leyendas artúricas, los romances también puede contar historias basadas en la [[mitología clásica. Los poemas narrativos más cortos tener un estilo literario similar al de los cuentos. A veces, estas narraciones breves se recogen compilaciones, como los Los cuentos de Canterbury de Chaucer. Algunas obras literarias contienen prosa narrativa, en la que se incluyen poemas e interludios poéticos.Un ejemplo de esta modalidad es la Vita Nuova de Dante Alighierl. pero el existió pero hace mucho mucho tiempo</skos:definition>
    <skos:definition xml:lang="nl">Narratieve poëzie (ook verhalende dichtkunst of epische poëzie genoemd) is poëzie die een verhaal vertelt. Het is een poëziegenre waartoe zowel korte als langere gedichten kunnen behoren en waarbij het verhaal eenvoudig of complex kan zijn. Meestal wordt een regelmatig rijmschema en metrum gehanteerd. Voorbeelden van verhalende gedichten zijn heldendichten, balladen, idylles en lays. Het oudste overgeleverd verhalend gedicht is het Babylonische epos van Gilgamesj dat dateert uit het 2e millennium v.Chr. In de Middelnederlandse literatuur zijn de ballade 'Heer Halewijn zong een liedekijn' en het Arthurverhaal Ferguut bekende voorbeelden. In sommige gevallen wordt verhalende poëzie gepresenteerd in de vorm van een roman in verzen. Een voorbeeld hiervan is The Ring and the Book van Robert Browning. Een romance is een verhalend gedicht dat een verhaal vertelt over ridderlijkheid. Voorbeelden hiervan zijn Romance of the Rose van Alfred Tennyson. Romancedichters behandelen vaak idyllisch voorgestelde taferelen uit de middeleeuwen en uit de klassieke mythologie of inspireren zich op verhalen over de legendarische koning Arthur. Kortere verhalende gedichten vertonen vaak stilistische gelijkenissen met korte verhalen. Soms zijn deze korte verhalen verzameld in aan elkaar verwante groepen, zoals bij Chaucers Canterbury Tales. Sommige vormen van literatuur bevatten prozaverhalen waarin ook gedichten en poëtische intermezzo's zijn opgenomen. Zo is veel oude Ierse poëzie opgenomen in prozaverhalen, en de oude Noordse sagen omvatten zowel incidentele poëzie als biografieën van dichters. Een voorbeeld is &quot;The Cremation of Sam McGee&quot; door Robert Service. <![CDATA[<a href="#_dbpedia_2017">(DBpedia, 2017)</a>]]></skos:definition>
    <prov:derivedFrom rdf:resource="http://dbpedia.org/resource/Narrative_poetry"/>
    <rdfs:comment xml:lang="en">The description for this term is indebted to DBpedia. </rdfs:comment>
    <skos:broaderTransitive rdf:resource="#genrePoetry"/>
  </genre:Genre>
  <genre:Genre rdf:about="#genreNationaltale">
    <rdf:value>NATIONALTALE</rdf:value>
    <rdfs:label xml:lang="en">national tale</rdfs:label>
    <rdfs:label xml:lang="fr"/>
    <rdfs:isDefinedBy rdf:resource="http://sparql.cwrc.ca/ontologies/genre-ONTOLOGY_DATE"/>
    <void:inDataset rdf:resource="#datasetdefinition"/>
    <skos:inScheme rdf:resource="#Genre"/>
    <rdf:type rdf:resource="http://www.w3.org/2004/02/skos/core#Concept"/>
  </genre:Genre>
  <genre:Genre rdf:about="#genreNotebook">
    <rdf:value>NOTEBOOK</rdf:value>
    <rdfs:label xml:lang="en">notebook</rdfs:label>
    <rdfs:label xml:lang="fr"/>
    <rdfs:isDefinedBy rdf:resource="http://sparql.cwrc.ca/ontologies/genre-ONTOLOGY_DATE"/>
    <void:inDataset rdf:resource="#datasetdefinition"/>
    <skos:inScheme rdf:resource="#Genre"/>
    <rdf:type rdf:resource="http://www.w3.org/2004/02/skos/core#Concept"/>
    <skos:definition xml:lang="en">Notebook is a style of writing where people jot down what they have thought or heard at the spur of moment. The contents of a notebook are unorganized, and the number of subjects covered in a notebook are unlimited: a paragraph of autobiography can be followed immediately by one on astronomy or one on history. Some famous authors are also famous for the notebooks they left. The Italian poet Giacomo Leopardi kept a notebook, called Zibaldone, from 1817 to 1832. The idea of keeping that, which contains no fewer than 4,526 pages, was possibly suggested by a priest who fled from the French Revolution and came to live in the poet's hometown. The priest suggested that &quot;every literary man should have a written chaos such as this: notebook containing sottiseries, adrersa, excerpta, pugillares, commentaria... the store-house out of which fine literature of every kind may come, as the sun, moon, and stars issued out of chaos.&quot; There are writers who earned their posthumous fame solely by their notebooks, such as the German scientist and humorous writer Georg Lichtenberg. He called his notebooks &quot;waste book,&quot; using the English book-keeping term. He explains the purpose of his &quot;waste book&quot; in his notebook E: The notebooks of scientists, such as those of Michael Faraday and Charles Darwin, can reveal the development of their scientific theories. On the other hand, the notebooks used by scientists for recording their experiments are called lab notebooks. The notebooks used by artists are usually referred as sketchbooks, which may contain more than sketches. Leonardo da Vinci's notebooks contain his writings on painting, sculpture, architecture, anatomy, mining, inventions and music, as well as his sketches, his grocery lists and the names of people who owed him money. In Chinese literature, &quot;notebook&quot; or biji is a distinct genre, and has a broader meaning. <![CDATA[<a href="#_dbpedia_2017">(DBpedia, 2017)</a>]]></skos:definition>
    <skos:definition xml:lang="de">Pinselnotizen oder Pinselaufzeichnungen (chinesisch 筆記 / 笔记, Pinyin bǐjì) sind eine schwer abgrenzbare Gattung von Kurzprosa überwiegend aus der klassischen chinesischen Literatur. Das Wort lässt sich grob mit „Notizbuch“ oder „Aufzeichnungen“ übersetzen (als Schreibmaterial diente der Schreibpinsel). Pinselnotizen bestehen meist aus kurzen Gedankenskizzen, Literaturkritik, Tagebuchaufzeichnungen, Anekdoten, Zitaten, auch Reiseberichten, Abenteuer- und Geistergeschichten, Witzen, Rätseln und Kleinprosa jeglicher Art. Das Genre bildete sich während der Wei- und Jin-Dynastie in der Zeit der Sechs Dynastien heraus und reifte in der Zeit der Tang-Dynastie heran. In voller Blüte stand die Biji-Literatur während der Zeit der Song-Dynastie. Auch in späteren Epochen wurde diese Literaturgattung ausgiebig gepflegt. Die Prosastücke wurden oft in Sammlungen herausgegeben und sind heute als wertvolle kulturgeschichtliche Quellen geschätzt. Berühmte Pinselnotizen sind die Werke Shishuo xinyu (世說新語) von Liu Yiqing (劉義慶) (Song-Dynastie der Südlichen Dynastien), Youyang zazu (酉陽雜俎) von Duan Chengshi (Tang-Dynastie), Song Jingwen biji (宋景文笔记) von Song Qi (宋祁) (Song-Dynastie), Chouchi biji (仇池笔记) von Su Shi (苏轼), Mengxi bitan (夢溪筆談) von Shen Kuo (auch: Shen Gua) (沈括) (Song-Dynastie) und Rongzhai suibi (容齋隨筆) von Hong Mai (Song-Dynastie), Dongjing meng Hua lu (東京夢華錄) von Meng Yuanlao (孟元老) (Südliche Song-Dynastie), Shanju xinhua (山居新话) von Yang Yu (杨瑀) Yuan-Dynastie, Wuli xiaoshi (物理小識) von Fang Yizhi (Ming-Dynastie), Yuewei caotang biji (閱微草堂筆記) von Ji Yun (紀昀) (Qing-Dynastie). Viele Pinselnotizen sind in sogenannten congshu („Sammelwerken“) überliefert, wie beispielsweise dem Shuofu (说郛), oder für spätere Epochen den Sammelwerken Ming Qing biji congkan (明清笔记丛刊) oder „Qingdai biji congkan“ (清代笔记丛刊). <![CDATA[<a href="#_dbpedia_2017">(DBpedia, 2017)</a>]]></skos:definition>
    <prov:derivedFrom rdf:resource="http://dbpedia.org/resource/Notebook_(style)"/>
    <rdfs:comment xml:lang="en">The description for this term is indebted to DBpedia. </rdfs:comment>
  </genre:Genre>
  <genre:Genre rdf:about="#genreNovel">
    <rdf:value>NOVEL</rdf:value>
    <rdfs:label xml:lang="en">novel</rdfs:label>
    <rdfs:label xml:lang="fr">roman</rdfs:label>
    <rdfs:isDefinedBy rdf:resource="http://sparql.cwrc.ca/ontologies/genre-ONTOLOGY_DATE"/>
    <void:inDataset rdf:resource="#datasetdefinition"/>
    <skos:inScheme rdf:resource="#Genre"/>
    <rdf:type rdf:resource="http://www.w3.org/2004/02/skos/core#Concept"/>
    <skos:definition xml:lang="en">Invented prose narratives of considerable length and a certain complexity that deal imaginatively with human experience through a connected sequence of events involving a group of persons in a specific setting. <![CDATA[<a href="#_getty_2017">(Getty, 2017)</a>]]></skos:definition>
    <skos:definition xml:lang="de">Fiktionale Prosaerzählung beträchtlichen Umfangs und einiger Komplexität, die auf fantasievolle Weise menschliche Erfahrungen durch eine verknüpfte Reihe von Ereignissen mit einer Gruppe von Personen in einem bestimmten Umfeld schildert. <![CDATA[<a href="#_getty_2017">(Getty, 2017)</a>]]></skos:definition>
    <skos:definition xml:lang="nl">Verzonnen prozaverhalen van aanzienlijke lengte en een zekere complexiteit die op verbeeldingsrijke wijze de menselijke ervaring behandelen aan de hand van een reeks onderling verbonden gebeurtenissen rond een groep personen in een specifieke omgeving. <![CDATA[<a href="#_getty_2017">(Getty, 2017)</a>]]></skos:definition>
    <skos:definition xml:lang="es">Narraciones ficticias en prosa de considerable extensión y una cierta complejidad que tratan imaginativamente sobre experiencias humanas a través de una secuencia relacionada de sucesos que involucran a un grupo de personas en un escenario específico. <![CDATA[<a href="#_getty_2017">(Getty, 2017)</a>]]></skos:definition>
    <skos:definition xml:lang="zh-hant">具相當長度與一定程度複雜性的虛構散文體記敘文，藉由與一群人，於一特定背景中相關聯的一連串事件，於想像中處理人類經驗。 <![CDATA[<a href="#_getty_2017">(Getty, 2017)</a>]]></skos:definition>
    <prov:derivedFrom rdf:resource="http://vocab.getty.edu/aat/300202580"/>
    <rdfs:comment xml:lang="en">The description for this term is indebted to the Getty Art &amp; Architecture Thesaurus.</rdfs:comment>
  </genre:Genre>
  <genre:Genre rdf:about="#genreNovella">
    <rdf:value>NOVELLA</rdf:value>
    <rdfs:label xml:lang="en">novella</rdfs:label>
    <rdfs:label xml:lang="fr"/>
    <rdfs:isDefinedBy rdf:resource="http://sparql.cwrc.ca/ontologies/genre-ONTOLOGY_DATE"/>
    <void:inDataset rdf:resource="#datasetdefinition"/>
    <skos:inScheme rdf:resource="#Genre"/>
    <rdf:type rdf:resource="http://www.w3.org/2004/02/skos/core#Concept"/>
    <skos:definition xml:lang="en">Short prose tales popular in the Renaissance and for later prose narratives intermediate between novels and short stories. <![CDATA[<a href="#_getty_2017">(Getty, 2017)</a>]]></skos:definition>
    <skos:definition xml:lang="de">Kurze, in der Renaissance beliebte Prosageschichte und in späteren Zeiten Prosaerzählung, zwischen Roman und Kurzgeschichte einzuordnen. <![CDATA[<a href="#_getty_2017">(Getty, 2017)</a>]]></skos:definition>
    <skos:definition xml:lang="nl">Wordt gebruikt voor korte prozaverhalen die in de renaissance populair waren en voor moderne prozavertellingen die korter zijn dan romans maar langer dan korte verhalen. <![CDATA[<a href="#_getty_2017">(Getty, 2017)</a>]]></skos:definition>
    <skos:definition xml:lang="es">Úsese para cuentos cortos en prosa populares en el Renacimiento y para narraciones en prosa posteriores que se ubican entre la novela y el cuento breve. <![CDATA[<a href="#_getty_2017">(Getty, 2017)</a>]]></skos:definition>
    <skos:definition xml:lang="zh-hant">指文藝復興時期流行的短篇散文體故事，並指後來介於長篇小說與短篇故事之間的散文體記敘文。 <![CDATA[<a href="#_getty_2017">(Getty, 2017)</a>]]></skos:definition>
    <prov:derivedFrom rdf:resource="http://vocab.getty.edu/aat/300202569"/>
    <rdfs:comment xml:lang="en">The description for this term is indebted to the Getty Art &amp; Architecture Thesaurus.</rdfs:comment>
  </genre:Genre>
  <genre:Genre rdf:about="#genreNurseryrhyme">
    <rdf:value>NURSERYRHYME</rdf:value>
    <rdfs:label xml:lang="en">nurseryrhyme</rdfs:label>
    <rdfs:label xml:lang="fr"/>
    <rdfs:isDefinedBy rdf:resource="http://sparql.cwrc.ca/ontologies/genre-ONTOLOGY_DATE"/>
    <void:inDataset rdf:resource="#datasetdefinition"/>
    <skos:inScheme rdf:resource="#Genre"/>
    <rdf:type rdf:resource="http://www.w3.org/2004/02/skos/core#Concept"/>
    <skos:definition xml:lang="en">Tales in rhymed verse for children. <![CDATA[<a href="#_getty_2017">(Getty, 2017)</a>]]></skos:definition>
    <skos:definition xml:lang="de">Eine Geschichte für Kinder in gereimten Versen. <![CDATA[<a href="#_getty_2017">(Getty, 2017)</a>]]></skos:definition>
    <skos:definition xml:lang="nl">Kinderverhaaltjes op rijm. <![CDATA[<a href="#_getty_2017">(Getty, 2017)</a>]]></skos:definition>
    <skos:definition xml:lang="es">Cuentos en verso rimado para niños. <![CDATA[<a href="#_getty_2017">(Getty, 2017)</a>]]></skos:definition>
    <skos:definition xml:lang="zh-hant">以兒童為對象，用押韻詩文講述的故事。 <![CDATA[<a href="#_getty_2017">(Getty, 2017)</a>]]></skos:definition>
    <prov:derivedFrom rdf:resource="http://vocab.getty.edu/aat/300202593"/>
    <rdfs:comment xml:lang="en">The description for this term is indebted to the Getty Art &amp; Architecture Thesaurus.</rdfs:comment>
  </genre:Genre>
  <genre:Genre rdf:about="#genreObituary">
    <rdf:value>OBITUARY</rdf:value>
    <rdfs:label xml:lang="en">obituary</rdfs:label>
    <rdfs:label xml:lang="fr"/>
    <rdfs:isDefinedBy rdf:resource="http://sparql.cwrc.ca/ontologies/genre-ONTOLOGY_DATE"/>
    <void:inDataset rdf:resource="#datasetdefinition"/>
    <skos:inScheme rdf:resource="#Genre"/>
    <rdf:type rdf:resource="http://www.w3.org/2004/02/skos/core#Concept"/>
    <skos:definition xml:lang="en">Obituary poetry, in the broad sense, includes any poem that commemorates a person or group of people's death: an elegy. In its stricter sense, though, it refers to a genre of popular verse or folk poetry that had its greatest popularity in the nineteenth century, especially in the United States of America. The genre consists largely of sentimental narrative verse that tells the story of the demise of its typically named subjects, and seeks to console their mourners with descriptions of their happy afterlife. The genre achieved its peak of popularity in the decade of the 1870s. While usually full chiefly of conventional pious sentiments, the obituary poets in one sense continue the program of meditations on death begun by the eighteenth-century graveyard poets, such as Edward Young's Night Thoughts, and as such continue one of the themes that went into literary Romanticism. <![CDATA[<a href="#_dbpedia_2017">(DBpedia, 2017)</a>]]></skos:definition>
    <prov:derivedFrom rdf:resource="http://dbpedia.org/resource/Obituary_poetry"/>
    <rdfs:comment xml:lang="en">The description for this term is indebted to DBpedia. </rdfs:comment>
  </genre:Genre>
  <genre:Genre rdf:about="#genreOccasionalpoetry">
    <rdf:value>OCCASIONALPOETRY</rdf:value>
    <rdfs:label xml:lang="en">occasional poetry</rdfs:label>
    <rdfs:label xml:lang="fr"/>
    <rdfs:isDefinedBy rdf:resource="http://sparql.cwrc.ca/ontologies/genre-ONTOLOGY_DATE"/>
    <void:inDataset rdf:resource="#datasetdefinition"/>
    <skos:inScheme rdf:resource="#Genre"/>
    <rdf:type rdf:resource="http://www.w3.org/2004/02/skos/core#Concept"/>
    <skos:definition xml:lang="en">Occasional poetry is poetry composed for a particular occasion. In the history of literature, it is often studied in connection with orality, performance, and patronage.</skos:definition>
    <skos:definition xml:lang="de">Der Ausdruck Gelegenheitsdichtung (Casualpoesie sowie parallele Wortbildungen auf -lyrik) bezeichnet in der Literaturwissenschaft Dichtung, die meist unter kommerziellen Gesichtspunkten auf einen speziellen Anlass hin verfasst wird (Gelegenheitsschrift). Goethe verwendet in Dichtung und Wahrheit und in den Gesprächen mit Eckermann den Ausdruck „Gelegenheitsgedicht“ auch in einem weniger abschätzigen Sinn für Gedichte, die sich der Inspiration eines Augenblicks verdanken, der nun im Gedicht festgehalten ist. <![CDATA[<a href="#_dbpedia_2017">(DBpedia, 2017)</a>]]></skos:definition>
    <prov:derivedFrom rdf:resource="http://dbpedia.org/resource/Occasional_poetry"/>
    <rdfs:comment xml:lang="en">The description for this term is indebted to DBpedia. </rdfs:comment>
    <skos:broaderTransitive rdf:resource="#genrePoetry"/>
  </genre:Genre>
  <genre:Genre rdf:about="#genreOde">
    <rdf:value>ODE</rdf:value>
    <rdfs:label xml:lang="en">ode</rdfs:label>
    <rdfs:label xml:lang="fr"/>
    <rdfs:isDefinedBy rdf:resource="http://sparql.cwrc.ca/ontologies/genre-ONTOLOGY_DATE"/>
    <void:inDataset rdf:resource="#datasetdefinition"/>
    <skos:inScheme rdf:resource="#Genre"/>
    <rdf:type rdf:resource="http://www.w3.org/2004/02/skos/core#Concept"/>
    <skos:definition xml:lang="en">Lyric poems of exalted emotion devoted to the praise or celebration of its subject; often employing complex or irregular metrical form. <![CDATA[<a href="#_getty_2017">(Getty, 2017)</a>]]></skos:definition>
    <skos:definition xml:lang="nl">Geëxalteerde lyrische gedichten waarin een verheven onderwerp wordt bezongen, vaak met gebruikmaking van complexe of onregelmatige metrische patronen. <![CDATA[<a href="#_getty_2017">(Getty, 2017)</a>]]></skos:definition>
    <skos:definition xml:lang="es">Poemas líricos de sentimientos elevados destinados al elogio o celebración del tema tratado, a menudo empleando formas métricas complejas o irregulares. <![CDATA[<a href="#_getty_2017">(Getty, 2017)</a>]]></skos:definition>
    <skos:definition xml:lang="de">Lyrisches Gedicht von erhabener Haltung zur Ehre oder Feier seines Gegenstandes; häufig in komplexer oder unregelmäßiger metrischer Form. <![CDATA[<a href="#_getty_2017">(Getty, 2017)</a>]]></skos:definition>
    <prov:derivedFrom rdf:resource="http://vocab.getty.edu/aat/300253045"/>
    <rdfs:comment xml:lang="en">The description for this term is indebted to the Getty Art &amp; Architecture Thesaurus.</rdfs:comment>
  </genre:Genre>
  <genre:Genre rdf:about="#genreOneactplay">
    <rdf:value>ONEACTPLAY</rdf:value>
    <rdfs:label xml:lang="en">one act play</rdfs:label>
    <rdfs:label xml:lang="fr"/>
    <rdfs:isDefinedBy rdf:resource="http://sparql.cwrc.ca/ontologies/genre-ONTOLOGY_DATE"/>
    <void:inDataset rdf:resource="#datasetdefinition"/>
    <skos:inScheme rdf:resource="#Genre"/>
    <rdf:type rdf:resource="http://www.w3.org/2004/02/skos/core#Concept"/>
  </genre:Genre>
  <genre:Genre rdf:about="#genreOpera">
    <rdf:value>OPERA</rdf:value>
    <rdfs:label xml:lang="en">opera</rdfs:label>
    <rdfs:label xml:lang="fr"/>
    <rdfs:isDefinedBy rdf:resource="http://sparql.cwrc.ca/ontologies/genre-ONTOLOGY_DATE"/>
    <void:inDataset rdf:resource="#datasetdefinition"/>
    <skos:inScheme rdf:resource="#Genre"/>
    <rdf:type rdf:resource="http://www.w3.org/2004/02/skos/core#Concept"/>
  </genre:Genre>
  <genre:Genre rdf:about="#genreOratorio">
    <rdf:value>ORATORIO</rdf:value>
    <rdfs:label xml:lang="en">oratorio</rdfs:label>
    <rdfs:label xml:lang="fr"/>
    <rdfs:isDefinedBy rdf:resource="http://sparql.cwrc.ca/ontologies/genre-ONTOLOGY_DATE"/>
    <void:inDataset rdf:resource="#datasetdefinition"/>
    <skos:inScheme rdf:resource="#Genre"/>
    <rdf:type rdf:resource="http://www.w3.org/2004/02/skos/core#Concept"/>
  </genre:Genre>
  <genre:Genre rdf:about="#genreOriental">
    <rdf:value>ORIENTAL</rdf:value>
    <rdfs:label xml:lang="en">oriental</rdfs:label>
    <rdfs:label xml:lang="fr"/>
    <rdfs:isDefinedBy rdf:resource="http://sparql.cwrc.ca/ontologies/genre-ONTOLOGY_DATE"/>
    <void:inDataset rdf:resource="#datasetdefinition"/>
    <skos:inScheme rdf:resource="#Genre"/>
    <rdf:type rdf:resource="http://www.w3.org/2004/02/skos/core#Concept"/>
  </genre:Genre>
  <genre:Genre rdf:about="#genrePageant">
    <rdf:value>PAGEANT</rdf:value>
    <rdfs:label xml:lang="en">pageant</rdfs:label>
    <rdfs:label xml:lang="fr"/>
    <rdfs:isDefinedBy rdf:resource="http://sparql.cwrc.ca/ontologies/genre-ONTOLOGY_DATE"/>
    <void:inDataset rdf:resource="#datasetdefinition"/>
    <skos:inScheme rdf:resource="#Genre"/>
    <rdf:type rdf:resource="http://www.w3.org/2004/02/skos/core#Concept"/>
  </genre:Genre>
  <genre:Genre rdf:about="#genrePanegyric">
    <rdf:value>PANEGYRIC</rdf:value>
    <rdfs:label xml:lang="en">panegyric</rdfs:label>
    <rdfs:label xml:lang="fr"/>
    <rdfs:isDefinedBy rdf:resource="http://sparql.cwrc.ca/ontologies/genre-ONTOLOGY_DATE"/>
    <void:inDataset rdf:resource="#datasetdefinition"/>
    <skos:inScheme rdf:resource="#Genre"/>
    <rdf:type rdf:resource="http://www.w3.org/2004/02/skos/core#Concept"/>
    <skos:definition xml:lang="en">A speech or poem designed to praise another person or group. In ancient Greek and Roman rhetoric, it was one branch of public speaking, with established rules and conventions found in the works of Menander and Hermogenes. Famous examples include Pliny's eulogy on Emperor Trajan and Isocrates' oration on the Olympic games of 380. <![CDATA[<a href="#_wheeler_2017">(L. K Wheeler, 2017)</a>]]></skos:definition>
    <prov:derivedFrom rdf:resource="http://web.cn.edu/kwheeler/lit_terms_p.html"/>
    <rdfs:comment xml:lang="en">The description for this term is indebted to Dr. L. Kip Wheeler of Carson-Newman University. </rdfs:comment>
  </genre:Genre>
  <genre:Genre rdf:about="#genrePantomime">
    <rdf:value>PANTOMIME</rdf:value>
    <rdfs:label xml:lang="en">pantomime</rdfs:label>
    <rdfs:label xml:lang="fr"/>
    <rdfs:isDefinedBy rdf:resource="http://sparql.cwrc.ca/ontologies/genre-ONTOLOGY_DATE"/>
    <void:inDataset rdf:resource="#datasetdefinition"/>
    <skos:inScheme rdf:resource="#Genre"/>
    <rdf:type rdf:resource="http://www.w3.org/2004/02/skos/core#Concept"/>
  </genre:Genre>
  <genre:Genre rdf:about="#genreParable">
    <rdf:value>PARABLE</rdf:value>
    <rdfs:label xml:lang="en">parable</rdfs:label>
    <rdfs:label xml:lang="fr"/>
    <rdfs:isDefinedBy rdf:resource="http://sparql.cwrc.ca/ontologies/genre-ONTOLOGY_DATE"/>
    <void:inDataset rdf:resource="#datasetdefinition"/>
    <skos:inScheme rdf:resource="#Genre"/>
    <rdf:type rdf:resource="http://www.w3.org/2004/02/skos/core#Concept"/>
    <skos:definition xml:lang="en">Short, fictitious stories that illustrate a moral attitude or religious principle. <![CDATA[<a href="#_getty_2017">(Getty, 2017)</a>]]></skos:definition>
    <skos:definition xml:lang="nl">Wordt gebruikt voor korte, verzonnen verhalen waarin een moreel standpunt of religieus principe wordt toegelicht. <![CDATA[<a href="#_getty_2017">(Getty, 2017)</a>]]></skos:definition>
    <skos:definition xml:lang="es">Úsese para relatos cortos imaginarios que ilustran una actitud moral o un principio religioso. <![CDATA[<a href="#_getty_2017">(Getty, 2017)</a>]]></skos:definition>
    <skos:definition xml:lang="de">Kurze, fiktive Geschichte, die eine moralische Haltung oder ein religiöses Prinzip veranschaulicht. <![CDATA[<a href="#_getty_2017">(Getty, 2017)</a>]]></skos:definition>
    <prov:derivedFrom rdf:resource="http://vocab.getty.edu/aat/300185342"/>
    <rdfs:comment xml:lang="en">The description for this term is indebted to the Getty Art &amp; Architecture Thesaurus.</rdfs:comment>
    <skos:definition xml:lang="fr">Une parabole (du grec παραϐολή, « rapprochement, comparaison ») est une des variétés de l’allégorie. La parabole est une figure de rhétorique consistant en une courte histoire qui utilise les événements quotidiens pour illustrer un enseignement, une morale ou une doctrine. Tandis que celle-ci, en général, présente directement le fait qu’elle a en vue, la parabole offre, sous ses couleurs véritables, un fait qui doit servir à la démonstration d’une vérité d’un autre ordre, avec laquelle elle a une relation plus ou moins facile à saisir. « Substituez dans la parabole, dit l’abbé Girard, le véritable fait à celui qu’elle expose, vous changerez le fond du discours : substituez dans l’allégorie les véritables couleurs à celles qu’elle emprunte, vous ne changerez que la forme. » On la trouve également dans le discours argumentatif lorsqu’un récit illustre la thèse défendue pour faciliter la compréhension du lecteur. La parabole est également un récit allégorique qui permet de dispenser un enseignement moral ou religieux. Présente dans la Bible où elle joue le rôle de l’apologue et de la fable, surtout les Évangiles, qui l'ont empruntée au midrash hébreu, la parabole est reprise dans les sermons des orateurs chrétiens. Le Nouveau Testament en contient un très grand nombre : le grain de sénevé ou l’Église, le Bon Samaritain ou l’amour de l’humanité, le levain ou la grâce, les loups ravisseurs sous des peaux d’agneaux ou les instituteurs de fausses doctrines, le travail des ouvriers de la vigne ou les œuvres du salut, le mauvais riche ou l’obligation de l’aumône, le bon pasteur, etc. Les paraboles sont plus fréquentes encore dans la littérature bouddhique ; les Avadanas, le Hitopadekas donnent à peine l’idée des recueils plus vastes dont ils sont extraits et dont l’un s’appelle le Yu-Lin, c’est-à-dire la « Forêt de comparaisons». Dans les littératures modernes, les Allemands ont surtout cultivé la parabole ; Lessing, Herder, Krummacher y ont particulièrement réussi. Dans le Bouc émissaire, page 270, René Girard remarque que « paraballo signifie jeter quelque chose en pâture à la foule pour apaiser son appétit de violence, de préférence une victime, un condamné à mort ; c'est ainsi qu'on se tire soi-même d'une situation épineuse, de toute évidence. C'est pour empêcher la foule de se retourner contre l'orateur que celui-ci recourt à la parabole, c'est-à-dire à la métaphore. » <![CDATA[<a href="#_dbpedia_2017">(DBpedia, 2017)</a>]]></skos:definition>
    <prov:derivedFrom rdf:resource="http://dbpedia.org/resource/Parable"/>
    <rdfs:comment xml:lang="en">The description for this term is indebted to DBpedia. </rdfs:comment>
    <skos:definition xml:lang="en">Short, fictitious stories that illustrate a moral attitude or religious principle. <![CDATA[<a href="#_getty_2017">(Getty, 2017)</a>]]></skos:definition>
    <skos:definition xml:lang="de">Kurze, fiktive Geschichte, die eine moralische Haltung oder ein religiöses Prinzip veranschaulicht. <![CDATA[<a href="#_getty_2017">(Getty, 2017)</a>]]></skos:definition>
    <skos:definition xml:lang="es">Úsese para relatos cortos imaginarios que ilustran una actitud moral o un principio religioso. <![CDATA[<a href="#_getty_2017">(Getty, 2017)</a>]]></skos:definition>
    <skos:definition xml:lang="nl">Wordt gebruikt voor korte, verzonnen verhalen waarin een moreel standpunt of religieus principe wordt toegelicht. <![CDATA[<a href="#_getty_2017">(Getty, 2017)</a>]]></skos:definition>
    <prov:derivedFrom rdf:resource="http://vocab.getty.edu/aat/300185342"/>
    <rdfs:comment xml:lang="en">The description for this term is indebted to the Getty Art &amp; Architecture Thesaurus.</rdfs:comment>
  </genre:Genre>
  <genre:Genre rdf:about="#genreParatexts">
    <rdf:value>PARATEXTS</rdf:value>
    <rdfs:label xml:lang="en">paratexts</rdfs:label>
    <rdfs:label xml:lang="fr">paratextes</rdfs:label>
    <rdfs:isDefinedBy rdf:resource="http://sparql.cwrc.ca/ontologies/genre-ONTOLOGY_DATE"/>
    <void:inDataset rdf:resource="#datasetdefinition"/>
    <skos:inScheme rdf:resource="#Genre"/>
    <rdf:type rdf:resource="http://www.w3.org/2004/02/skos/core#Concept"/>
  </genre:Genre>
  <genre:Genre rdf:about="#genreParody">
    <rdf:value>PARODY</rdf:value>
    <rdfs:label xml:lang="en">parody</rdfs:label>
    <rdfs:label xml:lang="fr"/>
    <rdfs:isDefinedBy rdf:resource="http://sparql.cwrc.ca/ontologies/genre-ONTOLOGY_DATE"/>
    <void:inDataset rdf:resource="#datasetdefinition"/>
    <skos:inScheme rdf:resource="#Genre"/>
    <rdf:type rdf:resource="http://www.w3.org/2004/02/skos/core#Concept"/>
    <skos:definition xml:lang="en">A parody (/ˈpærədi/; also called spoof, send-up, take-off or lampoon), in use, is a work created to imitate, make fun of, or comment on an original work, its subject, author, style, or some other target, by means of satiric or ironic imitation. As the literary theorist Linda Hutcheon puts it, &quot;parody … is imitation, not always at the expense of the parodied text.&quot; Another critic, Simon Dentith, defines parody as &quot;any cultural practice which provides a relatively polemical allusive imitation of another cultural production or practice.&quot;Parody may be found in art or culture, including literature, music (although &quot;parody&quot; in music has an earlier, somewhat different meaning than for other art forms), animation, gaming and film. The writer and critic John Gross observes in his Oxford Book of Parodies, that parody seems to flourish on territory somewhere between pastiche (&quot;a composition in another artist's manner, without satirical intent&quot;) and burlesque (which &quot;fools around with the material of high literature and adapts it to low ends&quot;). Meanwhile, the Encyclopédie of Denis Diderot distinguishes between the parody and the burlesque, &quot;A good parody is a fine amusement, capable of amusing and instructing the most sensible and polished minds; the burlesque is a miserable buffoonery which can only please the populace.&quot; Historically, when a formula grows tired, as in the case of the moralistic melodramas in the 1910s, it retains value only as a parody, as demonstrated by the Buster Keaton shorts that mocked that genre. In his 1960 anthology of parody from the 14th through 20th centuries, critic Dwight Macdonald offered this metaphor: &quot;Parody is making a new wine that tastes like the old but has a slightly lethal effect.&quot; <![CDATA[<a href="#_dbpedia_2017">(DBpedia, 2017)</a>]]></skos:definition>
    <skos:definition xml:lang="fr">La parodie est une forme d'humour qui utilise le cadre, les personnages, le style et le fonctionnement d'une œuvre ou une institution pour s'en moquer. Elle se base entre autres sur l'inversion et l'exagération des caractéristiques appartenant au sujet parodié. Selon Dominique Maingueneau, la parodie constitue une « stratégie de réinvestissement d'un texte ou d'un genre de discours dans d'autres » : il s'agit d'une stratégie de « subversion », visant à disqualifier l'auteur du texte ou du genre source, tandis que la stratégie opposée (la « captation », imitation positive) permet de « transférer sur le discours réinvestisseur l'autorité attachée au texte ou au genre source ». <![CDATA[<a href="#_dbpedia_2017">(DBpedia, 2017)</a>]]></skos:definition>
    <skos:definition xml:lang="de">Eine Parodie (griechisch παρῳδία parōdía „Gegenlied“ oder „verstellt gesungenes Lied“) ist eine verzerrende, übertreibende oder verspottende Nachahmung. <![CDATA[<a href="#_dbpedia_2017">(DBpedia, 2017)</a>]]></skos:definition>
    <skos:definition xml:lang="es">La parodia (del griego, παρώδïα, παρα, en contra de o al lado de, y ώδή, oda) es una obra satírica que caracteriza o interpreta humorísticamente otra obra de arte, un autor o un tema, mediante la emulación o alusión irónica. Modernamente, la parodia no implica necesariamente la burla del texto parodiado. En el sentido de en contra del canto, la parodia se refiere a imitaciones burlonas de la forma de cantar o recitar, mientras en el real sentido de al lado del canto implica repetición con diferencia, sin necesariamente burla. La parodia existe en todos los géneros, incluyendo la literatura, la música , el cine y la televisión. Un acontecimiento político, social o cultural puede ser asimismo parodiado. La parodia es la recreación de un personaje o un hecho, empleando recursos irónicos para emitir una opinión generalmente transgresora sobre la persona o el acontecimiento parodiado. <![CDATA[<a href="#_dbpedia_2017">(DBpedia, 2017)</a>]]></skos:definition>
    <skos:definition xml:lang="nl">Een parodie of persiflage is een spottende nabootsing van een gedicht, lied, film, toneelstuk, verhaal of andere uiting. Vaak worden hierbij herkenbare eigenschappen van het origineel overdreven of uitvergroot. <![CDATA[<a href="#_dbpedia_2017">(DBpedia, 2017)</a>]]></skos:definition>
    <prov:derivedFrom rdf:resource="http://dbpedia.org/resource/Parody"/>
    <rdfs:comment xml:lang="en">The description for this term is indebted to DBpedia. </rdfs:comment>
  </genre:Genre>
  <genre:Genre rdf:about="#genrePastoral">
    <rdf:value>PASTORAL</rdf:value>
    <rdfs:label xml:lang="en">pastoral</rdfs:label>
    <rdfs:label xml:lang="fr"/>
    <rdfs:isDefinedBy rdf:resource="http://sparql.cwrc.ca/ontologies/genre-ONTOLOGY_DATE"/>
    <void:inDataset rdf:resource="#datasetdefinition"/>
    <skos:inScheme rdf:resource="#Genre"/>
    <rdf:type rdf:resource="http://www.w3.org/2004/02/skos/core#Concept"/>
    <skos:definition xml:lang="en">Genre that depicts or evokes idyllic life in the country; in works of pictorial art, often scenes of shepherds and shepherdesses in idealized arcadian landscapes. <![CDATA[<a href="#_getty_2017">(Getty, 2017)</a>]]></skos:definition>
    <skos:definition xml:lang="es">Género que representa o evoca la vida idilica en un país; en obras de arte pictórico, a menudo escenas de pastores o pastoras en paisajes rurales idealizados. <![CDATA[<a href="#_getty_2017">(Getty, 2017)</a>]]></skos:definition>
    <skos:definition xml:lang="nl">Genre dat het idyllische leven op het platteland oproept of afbeeldt; vaak scènes in beeldende kunstwerken met herders en herderinnetjes in geïdealiseerde arcadische landschappen. <![CDATA[<a href="#_getty_2017">(Getty, 2017)</a>]]></skos:definition>
    <skos:definition xml:lang="zh-hant">描繪或令人憶起鄉村田園詩情畫意般生活的藝術類型。在繪畫作品中，常常是在理想化的阿卡笛亞(古希臘傳說的聖地)田園風景中，有牧羊人與牧羊女的場景。 <![CDATA[<a href="#_getty_2017">(Getty, 2017)</a>]]></skos:definition>
    <prov:derivedFrom rdf:resource="http://vocab.getty.edu/aat/300250491"/>
    <rdfs:comment xml:lang="en">The description for this term is indebted to the Getty Art &amp; Architecture Thesaurus.</rdfs:comment>
  </genre:Genre>
  <genre:Genre rdf:about="#genrePedagogy">
    <rdf:value>PEDAGOGY</rdf:value>
    <rdfs:label xml:lang="en">pedagogy</rdfs:label>
    <rdfs:label xml:lang="fr"/>
    <rdfs:isDefinedBy rdf:resource="http://sparql.cwrc.ca/ontologies/genre-ONTOLOGY_DATE"/>
    <void:inDataset rdf:resource="#datasetdefinition"/>
    <skos:inScheme rdf:resource="#Genre"/>
    <rdf:type rdf:resource="http://www.w3.org/2004/02/skos/core#Concept"/>
  </genre:Genre>
  <genre:Genre rdf:about="#genrePerformancepoetry">
    <rdf:value>PERFORMANCEPOETRY</rdf:value>
    <rdfs:label xml:lang="en">performance poetry</rdfs:label>
    <rdfs:label xml:lang="fr"/>
    <rdfs:isDefinedBy rdf:resource="http://sparql.cwrc.ca/ontologies/genre-ONTOLOGY_DATE"/>
    <void:inDataset rdf:resource="#datasetdefinition"/>
    <skos:inScheme rdf:resource="#Genre"/>
    <rdf:type rdf:resource="http://www.w3.org/2004/02/skos/core#Concept"/>
    <skos:definition xml:lang="en">Performance poetry is poetry that is specifically composed for or during a performance before an audience. During the 1980s, the term came into popular usage to describe poetry written or composed for performance rather than print distribution. <![CDATA[<a href="#_dbpedia_2017">(DBpedia, 2017)</a>]]></skos:definition>
    <skos:definition xml:lang="fr">La lecture performée ou lecture-performance est une lecture publique de textes poétiques ou littéraires effectuée le plus souvent par son auteur dans un esprit qui s'apparente à celui de la performance et qui peut convoquer tous les arts et techniques du théâtre et de la scène où la poésie et la littérature sont cependant toujours au premier plan. Christian Prigent, Serge Pey et Charles Pennequin en sont les premiers représentants. Édith Azam est aujourd'hui la conseillère lecture-performance au festival Voix de la Méditerranée de Lodève. <![CDATA[<a href="#_dbpedia_2017">(DBpedia, 2017)</a>]]></skos:definition>
    <prov:derivedFrom rdf:resource="http://dbpedia.org/resource/Performance_poetry"/>
    <rdfs:comment xml:lang="en">The description for this term is indebted to DBpedia. </rdfs:comment>
    <skos:broaderTransitive rdf:resource="#genrePoetry"/>
  </genre:Genre>
  <genre:Genre rdf:about="#genrePeriodical">
    <rdf:value>PERIODICAL</rdf:value>
    <rdfs:label xml:lang="en">periodical</rdfs:label>
    <rdfs:label xml:lang="fr"/>
    <rdfs:isDefinedBy rdf:resource="http://sparql.cwrc.ca/ontologies/genre-ONTOLOGY_DATE"/>
    <void:inDataset rdf:resource="#datasetdefinition"/>
    <skos:inScheme rdf:resource="#Genre"/>
    <rdf:type rdf:resource="http://www.w3.org/2004/02/skos/core#Concept"/>
    <skos:definition xml:lang="en">Publications issued at regular intervals, but not daily, containing articles on various subjects by different authors for the general reader. <![CDATA[<a href="#_getty_2017">(Getty, 2017)</a>]]></skos:definition>
    <skos:definition xml:lang="de">Regelmäßige, jedoch nicht tägliche, Veröffenlichung, mit Artikeln zu verschiedenen Themen von verschiedenen Autoren für die allgemeine Öffentlichkeit. <![CDATA[<a href="#_getty_2017">(Getty, 2017)</a>]]></skos:definition>
    <skos:definition xml:lang="es">Publicaciones editadas en intervalos regulares de más de un día. <![CDATA[<a href="#_getty_2017">(Getty, 2017)</a>]]></skos:definition>
    <skos:definition xml:lang="nl">Publikaties die regelmatig worden uitgegeven met tussenpozen van meer dan één dag. <![CDATA[<a href="#_getty_2017">(Getty, 2017)</a>]]></skos:definition>
    <prov:derivedFrom rdf:resource="http://vocab.getty.edu/aat/300026657"/>
    <rdfs:comment xml:lang="en">The description for this term is indebted to the Getty Art &amp; Architecture Thesaurus.</rdfs:comment>
  </genre:Genre>
  <genre:Genre rdf:about="#genrePetition">
    <rdf:value>PETITION</rdf:value>
    <rdfs:label xml:lang="en">petition</rdfs:label>
    <rdfs:label xml:lang="fr"/>
    <rdfs:isDefinedBy rdf:resource="http://sparql.cwrc.ca/ontologies/genre-ONTOLOGY_DATE"/>
    <void:inDataset rdf:resource="#datasetdefinition"/>
    <skos:inScheme rdf:resource="#Genre"/>
    <rdf:type rdf:resource="http://www.w3.org/2004/02/skos/core#Concept"/>
    <skos:definition xml:lang="en">Includes any written requests and lists of signatures submitted to an authority to appeal for the performance of specific action. <![CDATA[<a href="#_getty_2017">(Getty, 2017)</a>]]></skos:definition>
    <skos:definition xml:lang="es">Incluye toda solicitud escrita y listas de firmas entregadas a una autoridad para pedir la realización de una acción específica. <![CDATA[<a href="#_getty_2017">(Getty, 2017)</a>]]></skos:definition>
    <skos:definition xml:lang="nl">Hieronder vallen alle mogelijke verzoekschriften en handtekeningenlijsten die aan een bevoegde autoriteit worden uitgereikt, en waarin om het nemen of nalaten van een of andere maatregel wordt verzocht <![CDATA[<a href="#_getty_2017">(Getty, 2017)</a>]]></skos:definition>
    <skos:definition xml:lang="zh-hant">任何呈交給當局附署名列表的書面請求，用於懇求當局履行特定行動。 <![CDATA[<a href="#_getty_2017">(Getty, 2017)</a>]]></skos:definition>
    <prov:derivedFrom rdf:resource="http://vocab.getty.edu/aat/300027219"/>
    <rdfs:comment xml:lang="en">The description for this term is indebted to the Getty Art &amp; Architecture Thesaurus.</rdfs:comment>
  </genre:Genre>
  <genre:Genre rdf:about="#genrePhilosophical">
    <rdf:value>PHILOSOPHICAL</rdf:value>
    <rdfs:label xml:lang="en">philosophical</rdfs:label>
    <rdfs:label xml:lang="fr"/>
    <rdfs:isDefinedBy rdf:resource="http://sparql.cwrc.ca/ontologies/genre-ONTOLOGY_DATE"/>
    <void:inDataset rdf:resource="#datasetdefinition"/>
    <skos:inScheme rdf:resource="#Genre"/>
    <rdf:type rdf:resource="http://www.w3.org/2004/02/skos/core#Concept"/>
  </genre:Genre>
  <genre:Genre rdf:about="#genrePhilosophy">
    <rdf:value>PHILOSOPHY</rdf:value>
    <rdfs:label xml:lang="en">philosophy</rdfs:label>
    <rdfs:label xml:lang="fr"/>
    <rdfs:isDefinedBy rdf:resource="http://sparql.cwrc.ca/ontologies/genre-ONTOLOGY_DATE"/>
    <void:inDataset rdf:resource="#datasetdefinition"/>
    <skos:inScheme rdf:resource="#Genre"/>
    <rdf:type rdf:resource="http://www.w3.org/2004/02/skos/core#Concept"/>
    <skos:definition xml:lang="en">(Greek, &quot;Love of wisdom&quot;): The methodical and systematic exploration of what we know, how we know it, and why it is important that we know it. Too frequently, students use the term somewhat nebulously. They often mistakenly state, &quot;My philosophy about X is . . .&quot; when they really mean, &quot;My opinion about X is . . .&quot; or &quot;My attitude toward X is . . .&quot; Traditional areas of Western philosophic inquiry include the following areas. <![CDATA[<a href="#_wheeler_2017">(L. K Wheeler, 2017)</a>]]></skos:definition>
    <prov:derivedFrom rdf:resource="http://web.cn.edu/kwheeler/lit_terms_p.html"/>
    <rdfs:comment xml:lang="en">The description for this term is indebted to Dr. L. Kip Wheeler of Carson-Newman University. </rdfs:comment>
  </genre:Genre>
  <genre:Genre rdf:about="#genrePicaresque">
    <rdf:value>PICARESQUE</rdf:value>
    <rdfs:label xml:lang="en">picaresque</rdfs:label>
    <rdfs:label xml:lang="fr"/>
    <rdfs:isDefinedBy rdf:resource="http://sparql.cwrc.ca/ontologies/genre-ONTOLOGY_DATE"/>
    <void:inDataset rdf:resource="#datasetdefinition"/>
    <skos:inScheme rdf:resource="#Genre"/>
    <rdf:type rdf:resource="http://www.w3.org/2004/02/skos/core#Concept"/>
    <skos:definition xml:lang="en">The picaresque novel (Spanish: &quot;picaresca,&quot; from &quot;pícaro,&quot; for &quot;rogue&quot; or &quot;rascal&quot;) is a genre of prose fiction which depicts the adventures of a roguish hero of low social class who lives by his wits in a corrupt society. Picaresque novels typically adopt a realistic style, with elements of comedy and satire. This style of novel originated in 16th-century Spain and flourished throughout Europe in the 17th and 18th centuries. It continues to influence modern literature. According to the traditional view of Thrall and Hibbard (first published in 1936), seven qualities distinguish the picaresque novel or narrative form, all or some of which may be employed for effect by the author. (1) A picaresque narrative is usually written in first person as an autobiographical account. (2) The main character is often of low character or social class. He or she gets by with wit and rarely deigns to hold a job. (3) There is no plot. The story is told in a series of loosely connected adventures or episodes. (4) There is little if any character development in the main character. Once a picaro, always a picaro. His or her circumstances may change but they rarely result in a change of heart. (5) The picaro's story is told with a plainness of language or realism. (6) Satire might sometimes be a prominent element. (7) The behavior of a picaresque hero or heroine stops just short of criminality. Carefree or immoral rascality positions the picaresque hero as a sympathetic outsider, untouched by the false rules of society. However, Trall and Hibbert's thesis has been questioned by scholars[specify] interested in how genre functions, rather than how it looks on the surface. <![CDATA[<a href="#_dbpedia_2017">(DBpedia, 2017)</a>]]></skos:definition>
    <skos:definition xml:lang="fr">Le roman picaresque (de l'espagnol pícaro, « misérable », « futé ») est un genre littéraire né en Espagne au XVIe siècle et qui a connu sa plus florissante époque dans ce pays. Un roman picaresque se compose d'un récit sur le mode autobiographique de l’histoire de héros miséreux, généralement des jeunes gens vivant en marge de la société et à ses dépens. Au cours d’aventures souvent extravagantes supposées plus pittoresques et surtout plus variées que celles des honnêtes gens, qui sont autant de prétextes à présenter des tableaux de la vie vulgaire et des scènes de mœurs, le héros entre en contact avec toutes les couches de la société. <![CDATA[<a href="#_dbpedia_2017">(DBpedia, 2017)</a>]]></skos:definition>
    <skos:definition xml:lang="de">Der Schelmenroman oder pikarischer/pikaresker Roman (aus dem Spanischen: pícaro = Schelm) , dessen Ursprung im 16. Jahrhundert in Spanien liegt, schildert aus der Perspektive seines Helden, wie sich dieser in einer Reihe von Abenteuern durchs Leben schlägt. Der Schelm stammt aus den unteren gesellschaftlichen Schichten, ist deshalb ungebildet, aber „bauernschlau“. Er durchläuft alle gesellschaftlichen Schichten und wird zu deren Spiegel. Der Held hat keinen Einfluss auf die Geschehnisse um ihn herum, schafft es aber immer wieder, sich aus allen brenzligen Situationen zu retten. Traditionell ist der Schelmenroman eine (fingierte) Autobiographie. Sie beginnt oft mit einer Desillusionierung des Helden, der die Schlechtigkeit der Welt erst hier erkennt. Er begibt sich, sei es freiwillig, sei es unfreiwillig, auf Reisen. Die dabei erlebten Abenteuer sind episodenhaft, d. h. sie hängen nicht voneinander ab und können beliebig erweitert werden, was bei Übersetzungen oft der Fall war. Das Ende ist meist eine „Bekehrung“ des Schelms, nach der er zu einem geregelten Leben findet. Es besteht auch die Möglichkeit einer Flucht aus der Welt, also aus der Realität. <![CDATA[<a href="#_dbpedia_2017">(DBpedia, 2017)</a>]]></skos:definition>
    <skos:definition xml:lang="es">Novela picaresca es un género literario narrativo en prosa muy característico de la literatura española, aunque trascendió a la europea en general. Surgió en los años de transición entre el Renacimiento y el Barroco, durante el llamado Siglo de Oro de las letras españolas. <![CDATA[<a href="#_dbpedia_2017">(DBpedia, 2017)</a>]]></skos:definition>
    <skos:definition xml:lang="nl">De schelmenroman is een literair genre dat in Spanje ontstond in de 16e en 17e eeuw. Schelmenromans worden ook picareske romans genoemd (naar het Spaanse picaro, dat schelm betekent). De schelmenroman is een subtype van de roman. <![CDATA[<a href="#_dbpedia_2017">(DBpedia, 2017)</a>]]></skos:definition>
    <prov:derivedFrom rdf:resource="http://dbpedia.org/resource/Picaresque_novel"/>
    <rdfs:comment xml:lang="en">The description for this term is indebted to DBpedia. </rdfs:comment>
  </genre:Genre>
  <genre:Genre rdf:about="#genrePindaric">
    <rdf:value>PINDARIC</rdf:value>
    <rdfs:label xml:lang="en">pindaric</rdfs:label>
    <rdfs:label xml:lang="fr"/>
    <rdfs:isDefinedBy rdf:resource="http://sparql.cwrc.ca/ontologies/genre-ONTOLOGY_DATE"/>
    <void:inDataset rdf:resource="#datasetdefinition"/>
    <skos:inScheme rdf:resource="#Genre"/>
    <rdf:type rdf:resource="http://www.w3.org/2004/02/skos/core#Concept"/>
  </genre:Genre>
  <genre:Genre rdf:about="#genrePoetry">
    <rdf:value>POETRY</rdf:value>
    <rdfs:label xml:lang="en">poetry</rdfs:label>
    <rdfs:label xml:lang="fr">poésie</rdfs:label>
    <rdfs:isDefinedBy rdf:resource="http://sparql.cwrc.ca/ontologies/genre-ONTOLOGY_DATE"/>
    <void:inDataset rdf:resource="#datasetdefinition"/>
    <skos:inScheme rdf:resource="#Genre"/>
    <rdf:type rdf:resource="http://www.w3.org/2004/02/skos/core#Concept"/>
    <skos:definition xml:lang="en">Poetry is a form of literature that uses aesthetic and rhythmic qualities of language—such as phonaesthetics, sound symbolism, and metre—to evoke meanings in addition to, or in place of, the prosaic ostensible meaning. <![CDATA[<a href="#_dbpedia_2017">(DBpedia, 2017)</a>]]></skos:definition>
    <skos:definition xml:lang="fr">La poésie est un genre littéraire très ancien aux formes variées, écrites généralement en vers, mais qui admettent aussi la prose, et qui privilégient l'expressivité de la forme, les mots disant plus qu'eux-mêmes par leur choix (sens et sonorités) et leur agencement (rythmes, métrique, figures de style). Sa définition se révèle difficile et varie selon les époques, au point que chaque siècle a pu lui trouver une fonction et une expression différente, à quoi s'ajoute l'approche propre à la personnalité de chaque poète. Le terme « poésie » et ses dérivés viennent du grec ancien ποίησις, et s'écrivait, jusqu'en 1878 poësie (le tréma marquait une disjonction entre les voyelles o et e). ποιεῖν (poiein) signifie « faire, créer » : le poète est donc un créateur, un inventeur de formes expressives, ce que révèlent aussi les termes du Moyen Âge, comme trouvère et troubadour. Le poète, héritier d'une longue tradition orale, privilégie la musicalité et le rythme, d'où, dans la plupart des textes poétiques, le recours à une forme versifiée qui confère de la densité à la langue. Le poète recherche aussi l'expressivité par le poids accordé aux mots comme par l'utilisation des figures de style et au premier chef des images et des figures d'analogie, recherchées pour leur force suggestive. La poésie s'est constamment renouvelée au cours des siècles avec des orientations différentes selon les époques, les civilisations et les individus. On peut par exemple distinguer le poète artiste soucieux d'abord de beauté formelle, le poète « lyrique » qui cultive le « chant de l'âme », le poète prophète, découvreur du monde et « voyant » ou le poète engagé, sans cependant réduire un créateur à une étiquette simplificatrice. <![CDATA[<a href="#_dbpedia_2017">(DBpedia, 2017)</a>]]></skos:definition>
    <skos:definition xml:lang="de">Das Wort Poesie (von gr. ποίησις poiesis, „Erschaffung“) bezeichnet erstens einen Textbereich, dessen Produktion traditionell nach den poetischen Gattungen geteilt wird. Nach Aristotelischer Poetik (so das Wort für die Theorie der Poesie) sind dies Drama, Epos und kleinere lyrische Gattungen. Im Deutschen wird seit dem 19. Jahrhundert eher von Literatur und literarischen Gattungen gesprochen. Allenfalls kurze Gedichte behielten das Wort, so etwa im Falle des Poesiealbums. Der Begriff bezeichnet im übertragenen Sinn ferner eine bestimmte Qualität. So spricht man etwa von der „Poesie eines Moments“ oder einem „poetischen Film“ und meint damit in der Regel, dass von dem Bezeichneten eine sich der Sprache entziehende, oder über sie hinausgehende Wirkung ausgeht, etwas Stilles, ähnlich wie von einem Gedicht, das eine sich der Alltagssprache entziehende Wirkung entfaltet. <![CDATA[<a href="#_dbpedia_2017">(DBpedia, 2017)</a>]]></skos:definition>
    <skos:definition xml:lang="es">La poesía (del griego ποίησις 'acción, creación; adopción; fabricación; composición, poesía; poema'  ποιέω 'hacer, fabricar; engendrar, dar a luz; obtener; causar; crear') se define como un género literario considerado como una manifestación de la belleza o del sentimiento estético por medio de la palabra, en verso o en prosa. Los griegos entendían que podría haber tres tipos de poesía, la lírica o canción cantada con acompañamiento de lira o arpa de mano, que es el significado que luego se generalizó para la palabra, incluso sin música; la dramática o teatral y la épica o narrativa. Por eso se suele entender generalmente hoy como poesía la poesía lírica. También es encuadrable como una «modalidad textual» (esto es, como un tipo de texto). Es frecuente, en la actualidad, utilizar el término «poesía» como sinónimo de «poesía lírica» o de «lírica», aunque, desde un punto de vista histórico y cultural, esta es un subgénero o subtipo de la poesía. <![CDATA[<a href="#_dbpedia_2017">(DBpedia, 2017)</a>]]></skos:definition>
    <skos:definition xml:lang="nl">Poëzie of dichtkunst (van het Griekse 'poiesis'/ποίησις: maken, scheppen, vormen) is een vorm van literatuur die de esthetische en ritmische eigenschappen van taal zoals metrum en geluidssymboliek benut om betekenissen te genereren ter aanvulling, vervanging of ondermijning van de prozaïsche, ogenschijnlijke betekenis. Poëzie heeft een lange geschiedenis die teruggaat tot het Soemerische epos Gilgamesj. Vroege gedichten ontwikkelden zich uit volksliederen zoals de Chinese Sjijing, of uit de noodzaak om orale epiek steeds opnieuw te vertellen, zoals in de Veda's uit het Sanskriet, het Zoroastrische Gathas en de Homerische epossen Ilias en Odyssee. Antieke pogingen om poëzie te omschrijven, zoals de Poetica van Aristoteles, benadrukten het spraakgebruik in retorica, drama, lied en komedie. Latere pogingen concentreerden zich op kenmerken als herhaling, versvorm en rijm en benadrukten de esthetica die poëzie onderscheidt van meer objectief informatieve, prozaïsche vormen van schrift. Vanaf het midden der twintigste eeuw wordt de dichtkunst soms meer algemeen beschouwd als een wezenlijk creatieve handeling waarbij taal gebruikt wordt. In poëzie worden vormen en conventies gebruikt om een andere interpretatie van woorden te suggereren, of om een gevoelsmatige respons teweeg te brengen. Middelen zoals assonantie, alliteratie, onomatopeeën en ritme worden soms gebruikt om bezwerende of muzikale effecten te bereiken. Het gebruik van ambiguïteit, symboliek, ironie en andere stilistische elementen van de poëtische voordracht maken vaak een veelheid van interpretaties mogelijk. Op dezelfde wijze schept beeldspraak zoals metafoor, vergelijking (al dan niet Homerisch) en metonymie resonantie tussen anderszins ongelijksoortige beelden - een gelaagdheid van betekenissen waarbij niet eerder waargenomen connecties worden gevormd. Tussen individuele versregels kunnen verwante vormen van resonantie aanwezig zijn in hun patronen van rijm of ritme. De genoegens die de poëzie aan lezer of luisteraar verschaft, worden teweeggebracht door de bijzondere combinatie van vorm, klank en betekenis die eigen is aan het vers, en deze genoegens kunnen van emotionele (bijvoorbeeld ontroering of bezwering), intellectuele (bijvoorbeeld inzicht of nuancering) of humoristische aard zijn. Ontvankelijkheid voor poëzie of versgevoeligheid is mede afhankelijk van de mate waarin deze wordt gecultiveerd. Poëzie heeft een lange geschiedenis, vanaf de vroegste mondeling gereciteerde en gezongen verzen tot de hedendaagse schriftelijke, al dan niet gestructureerde vormen van dichtkunst. <![CDATA[<a href="#_dbpedia_2017">(DBpedia, 2017)</a>]]></skos:definition>
    <prov:derivedFrom rdf:resource="http://dbpedia.org/resource/Poetry"/>
    <rdfs:comment xml:lang="en">The description for this term is indebted to DBpedia. </rdfs:comment>
  </genre:Genre>
  <genre:Genre rdf:about="#genrePolemic">
    <rdf:value>POLEMIC</rdf:value>
    <rdfs:label xml:lang="en">polemic</rdfs:label>
    <rdfs:label xml:lang="fr"/>
    <rdfs:isDefinedBy rdf:resource="http://sparql.cwrc.ca/ontologies/genre-ONTOLOGY_DATE"/>
    <void:inDataset rdf:resource="#datasetdefinition"/>
    <skos:inScheme rdf:resource="#Genre"/>
    <rdf:type rdf:resource="http://www.w3.org/2004/02/skos/core#Concept"/>
    <skos:definition xml:lang="fr">Le terme de polémique (du grec πολεμικός, polêmikôs « qui concerne la guerre », « disposé à la guerre », polêmikon museion, musée de la guerre, « batailleur, querelleur ») désigne une discussion, un débat, une controverse qui traduit de façon violente ou passionnée, et le plus souvent par écrit, des opinions contraires sur toutes espèces de sujets (politique, scientifique, littéraire, religieux, etc.). Il fait aujourd'hui l'objet d'emplois multiples. <![CDATA[<a href="#_dbpedia_2017">(DBpedia, 2017)</a>]]></skos:definition>
    <prov:derivedFrom rdf:resource="http://dbpedia.org/resource/Polemic"/>
    <rdfs:comment xml:lang="en">The description for this term is indebted to DBpedia. </rdfs:comment>
    <skos:definition xml:lang="en">Aggressive, forcefully presented arguments, often disputing a policy or opinion. <![CDATA[<a href="#_getty_2017">(Getty, 2017)</a>]]></skos:definition>
    <skos:definition xml:lang="de">Scharfes und mit Nachdruck vorgebrachtes Argument, das häufig gegen eine bestimmte Politik oder Meinung gerichtet ist. <![CDATA[<a href="#_getty_2017">(Getty, 2017)</a>]]></skos:definition>
    <skos:definition xml:lang="es">Argumentos presentados en forma agresiva y enérgica, a menudo para discutir una política u opinión. <![CDATA[<a href="#_getty_2017">(Getty, 2017)</a>]]></skos:definition>
    <skos:definition xml:lang="nl">Agressieve, scherp geformuleerde twistgeschriften, waarin dikwijls een beleid of een mening wordt betwist. <![CDATA[<a href="#_getty_2017">(Getty, 2017)</a>]]></skos:definition>
    <prov:derivedFrom rdf:resource="http://vocab.getty.edu/aat/300252982"/>
    <rdfs:comment xml:lang="en">The description for this term is indebted to the Getty Art &amp; Architecture Thesaurus.</rdfs:comment>
  </genre:Genre>
  <genre:Genre rdf:about="#genrePoliticalwriting">
    <rdf:value>POLITICALWRITING</rdf:value>
    <rdfs:label xml:lang="en">political writing</rdfs:label>
    <rdfs:label xml:lang="fr"/>
    <rdfs:isDefinedBy rdf:resource="http://sparql.cwrc.ca/ontologies/genre-ONTOLOGY_DATE"/>
    <void:inDataset rdf:resource="#datasetdefinition"/>
    <skos:inScheme rdf:resource="#Genre"/>
    <rdf:type rdf:resource="http://www.w3.org/2004/02/skos/core#Concept"/>
  </genre:Genre>
  <genre:Genre rdf:about="#genrePopular">
    <rdf:value>POPULAR</rdf:value>
    <rdfs:label xml:lang="en">popular</rdfs:label>
    <rdfs:label xml:lang="fr"/>
    <rdfs:isDefinedBy rdf:resource="http://sparql.cwrc.ca/ontologies/genre-ONTOLOGY_DATE"/>
    <void:inDataset rdf:resource="#datasetdefinition"/>
    <skos:inScheme rdf:resource="#Genre"/>
    <rdf:type rdf:resource="http://www.w3.org/2004/02/skos/core#Concept"/>
    <skos:definition xml:lang="en">Visual arts produced by or for the general public, often reflecting fads and as a response to the daily environment; works produced for mass audiences as distinct from fine art and folk art. <![CDATA[<a href="#_getty_2017">(Getty, 2017)</a>]]></skos:definition>
    <prov:derivedFrom rdf:resource="http://vocab.getty.edu/aat/300311927"/>
    <rdfs:comment xml:lang="en">The description for this term is indebted to the Getty Art &amp; Architecture Thesaurus.</rdfs:comment>
  </genre:Genre>
  <genre:Genre rdf:about="#genrePrayer">
    <rdf:value>PRAYER</rdf:value>
    <rdfs:label xml:lang="en">prayer</rdfs:label>
    <rdfs:label xml:lang="fr"/>
    <rdfs:isDefinedBy rdf:resource="http://sparql.cwrc.ca/ontologies/genre-ONTOLOGY_DATE"/>
    <void:inDataset rdf:resource="#datasetdefinition"/>
    <skos:inScheme rdf:resource="#Genre"/>
    <rdf:type rdf:resource="http://www.w3.org/2004/02/skos/core#Concept"/>
    <skos:definition xml:lang="en">Documents containing prayers that are associated with donning official priestly vestments or transfer of vestments, most commonly in Christian contexts.</skos:definition>
    <skos:definition xml:lang="nl">Gebed dat de priester uitspreekt bij het aantrekken van een liturgisch gewaad en bij de overhandiging van de liturgische gewaden bij de priesterwijding. Het gebed staat soms ingelijst in de sacristie, bijvoorbeeld op de credens. <![CDATA[<a href="#_getty_2017">(Getty, 2017)</a>]]></skos:definition>
    <prov:derivedFrom rdf:resource="http://vocab.getty.edu/aat/300391080"/>
    <rdfs:comment xml:lang="en">The description for this term is indebted to the Getty Art &amp; Architecture Thesaurus.</rdfs:comment>
  </genre:Genre>
  <genre:Genre rdf:about="#genrePrefatorypiece">
    <rdf:value>PREFATORYPIECE</rdf:value>
    <rdfs:label xml:lang="en">prefatory piece</rdfs:label>
    <rdfs:label xml:lang="fr">préfixe</rdfs:label>
    <rdfs:isDefinedBy rdf:resource="http://sparql.cwrc.ca/ontologies/genre-ONTOLOGY_DATE"/>
    <void:inDataset rdf:resource="#datasetdefinition"/>
    <skos:inScheme rdf:resource="#Genre"/>
    <rdf:type rdf:resource="http://www.w3.org/2004/02/skos/core#Concept"/>
  </genre:Genre>
  <genre:Genre rdf:about="#genreProletarianwriting">
    <rdf:value>PROLETARIANWRITING</rdf:value>
    <rdfs:label xml:lang="en">proletarianwriting</rdfs:label>
    <rdfs:label xml:lang="fr"/>
    <rdfs:isDefinedBy rdf:resource="http://sparql.cwrc.ca/ontologies/genre-ONTOLOGY_DATE"/>
    <void:inDataset rdf:resource="#datasetdefinition"/>
    <skos:inScheme rdf:resource="#Genre"/>
    <rdf:type rdf:resource="http://www.w3.org/2004/02/skos/core#Concept"/>
  </genre:Genre>
  <genre:Genre rdf:about="#genrePrologue">
    <rdf:value>PROLOGUE</rdf:value>
    <rdfs:label xml:lang="en">prologue</rdfs:label>
    <rdfs:label xml:lang="fr"/>
    <rdfs:isDefinedBy rdf:resource="http://sparql.cwrc.ca/ontologies/genre-ONTOLOGY_DATE"/>
    <void:inDataset rdf:resource="#datasetdefinition"/>
    <skos:inScheme rdf:resource="#Genre"/>
    <rdf:type rdf:resource="http://www.w3.org/2004/02/skos/core#Concept"/>
    <skos:definition xml:lang="en">(1) In original Greek tragedy, the prologue was either the action or a set of introductory speeches before the first entry (parados) of the chorus. Here, a single actor's monologue or a dialogue between two actors would establish the play's background events. (2) In later literature, a prologue is a section of any introductory material before the first chapter or the main material of a prose work, or any such material before the first stanza of a poetic work. <![CDATA[<a href="#_wheeler_2017">(L. K Wheeler, 2017)</a>]]></skos:definition>
    <prov:derivedFrom rdf:resource="http://web.cn.edu/kwheeler/lit_terms_p.html"/>
    <rdfs:comment xml:lang="en">The description for this term is indebted to Dr. L. Kip Wheeler of Carson-Newman University. </rdfs:comment>
  </genre:Genre>
  <genre:Genre rdf:about="#genrePropaganda">
    <rdf:value>PROPAGANDA</rdf:value>
    <rdfs:label xml:lang="en">propaganda</rdfs:label>
    <rdfs:label xml:lang="fr"/>
    <rdfs:isDefinedBy rdf:resource="http://sparql.cwrc.ca/ontologies/genre-ONTOLOGY_DATE"/>
    <void:inDataset rdf:resource="#datasetdefinition"/>
    <skos:inScheme rdf:resource="#Genre"/>
    <rdf:type rdf:resource="http://www.w3.org/2004/02/skos/core#Concept"/>
    <skos:definition xml:lang="en">Ideas, facts, or allegations spread deliberately to support one cause or individual or to damage another. <![CDATA[<a href="#_getty_2017">(Getty, 2017)</a>]]></skos:definition>
    <skos:definition xml:lang="es">Ideas, hechos o alegatos difundidos deliberadamente para soportar una causa o individuo o para dañar a otro. <![CDATA[<a href="#_getty_2017">(Getty, 2017)</a>]]></skos:definition>
    <skos:definition xml:lang="nl">Ideeën, feiten of beweringen die met opzet zijn verspreid om het ene doel of individu te ondersteunen en het andere te schaden. <![CDATA[<a href="#_getty_2017">(Getty, 2017)</a>]]></skos:definition>
    <skos:definition xml:lang="zh-hant">蓄意傳播思想、事實、主張以支持或詆毀某個理想或個人。 <![CDATA[<a href="#_getty_2017">(Getty, 2017)</a>]]></skos:definition>
    <prov:derivedFrom rdf:resource="http://vocab.getty.edu/aat/300055539"/>
    <rdfs:comment xml:lang="en">The description for this term is indebted to the Getty Art &amp; Architecture Thesaurus.</rdfs:comment>
    <skos:definition xml:lang="en">(Latin, &quot;things that must be sent forth&quot;): In its original use, the term referred to a committee of cardinals the Roman Catholic church founded in 1622 (the Congregatio de propaganda fide). This group established specific educational materials to be sent with priests-in-training for foreign missions . The term is today used to refer to information, rumors, ideas, and artwork spread deliberately to help or harm another specific group, movement, belief, institution, or government. The term's connotations are mostly negative. When literature or journalism is propaganda and when it is not is hotly debated. For instance, the Roman Emperor Augustus commissioned Virgil to write The Aeneid for specific goals. He wanted Virgil to glorify Rome's greatness, instill public pride in Rome's past, and cultivate traditional Roman virtues such as loyalty to the family, the Empire, and the gods. Is this propaganda? Or patriotism? Typically, readers claim a work is propaganda when it sets forth an argument with which they personally disagree. In other cases, readers will call a work propagandistic if they can perceive that the characters or the author advances particular doctrines or principles. Harry Shaw notes: &quot;Propaganda is attacked by most critics and general readers because it is an attempt to influence opinions and actions deliberately, but by this definition all education and most literature are propagandistic&quot; (220). <![CDATA[<a href="#_wheeler_2017">(L. K Wheeler, 2017)</a>]]></skos:definition>
    <prov:derivedFrom rdf:resource="http://web.cn.edu/kwheeler/lit_terms_p.html"/>
    <rdfs:comment xml:lang="en">The description for this term is indebted to Dr. L. Kip Wheeler of Carson-Newman University. </rdfs:comment>
  </genre:Genre>
  <genre:Genre rdf:about="#genreProphecy">
    <rdf:value>PROPHECY</rdf:value>
    <rdfs:label xml:lang="en">prophecy</rdfs:label>
    <rdfs:label xml:lang="fr"/>
    <rdfs:isDefinedBy rdf:resource="http://sparql.cwrc.ca/ontologies/genre-ONTOLOGY_DATE"/>
    <void:inDataset rdf:resource="#datasetdefinition"/>
    <skos:inScheme rdf:resource="#Genre"/>
    <rdf:type rdf:resource="http://www.w3.org/2004/02/skos/core#Concept"/>
    <skos:definition xml:lang="en">Prophecy involves a process in which one or more messages allegedly communicated to a prophet are then communicated to other people. Such messages typically involve] inspiration, interpretation, or revelation of events to come (compare divine knowledge). Historically, clairvoyance has been used[by whom?] as an adjunct to prophecy. <![CDATA[<a href="#_dbpedia_2017">(DBpedia, 2017)</a>]]></skos:definition>
    <skos:definition xml:lang="fr">Dans les religions abrahamiques, une prophétie consiste en des paroles ou des écrits divinement inspirés qu'une personne reçoit par révélation. Pour les chrétiens, le témoignage de Jésus est l'esprit de la prophétie (Apocalypse 19:10). Une prophétie peut avoir trait au passé, au présent ou à l'avenir. Quand une personne prophétise, elle dit ou écrit ce que Dieu veut qu'elle sache, pour son propre bien ou pour le bien des autres. La prophétie n'est pas l'apanage des prophètes. Une personne peut recevoir une prophétie ou une révélation pour sa vie personnelle. <![CDATA[<a href="#_dbpedia_2017">(DBpedia, 2017)</a>]]></skos:definition>
    <skos:definition xml:lang="de">Als Prophezeiung – auch Weissagung oder Verheißung – bezeichnet man in religiösen Kontexten eine Prognose von Ereignissen in der Zukunft. Der Oberbegriff für gesammelte mündliche oder schriftliche Prophezeiungen, meist einer Einzelperson, ist Prophetie. Dieser Ausdruck stammt vom altgriechischen propheteía für „aussprechen“, „aussagen“ oder „für jemanden sprechen“ (altgriechisch φηµί phēmí „ich spreche“; pro „für, heraus, anstelle“). Prophezeiungen kommen in vielen Religionen in unterschiedlichsten Zusammenhängen, aus verschiedenen Anlässen und aufgrund verschiedener Empfangsweisen der prophezeiten Botschaft vor. Die altorientalischen Kulte kennen vielfältige Arten von Orakeln, regelmäßigen Befragungen an Opferstätten oder vor Schlachten, ekstatischen Ausnahmebotschaften, Traumvisionen, als Prophezeiung gedeuteten Medien wie Tierorganen, Vogelflug, Verzückung oder Audition usw. Die klassische Schriftprophetie im Judentum kennt solche Formen jedoch kaum. Hier bildet in der Regel eine Berufung eines Propheten durch den Gott Israels Ausgangspunkt von Wortbotschaften, die sich auf die Geschichte Gesamtisraels beziehen. Im Christentum werden Prophezeiungen seit der Jerusalemer Urgemeinde erwähnt. In der Folgezeit sind Prophezeiungen ein beliebtes Thema der Literatur geworden. In den Geschichtswissenschaften wird eine Prophezeiung auch als Vatizinium (Plural „Vatizinien“; von lateinisch vates „Weissager“, „Prophet“) bezeichnet. Insbesondere nennt man Prophezeiungen im Nachhinein Vaticinium ex eventu. <![CDATA[<a href="#_dbpedia_2017">(DBpedia, 2017)</a>]]></skos:definition>
    <skos:definition xml:lang="es">Una profecía (del latín prophetīa, y este del griego προφητεία, o quizá del griego φαινος, aparición) es, en la primera acepción del Diccionario de la lengua española de la Real Academia Española, un «don sobrenatural que consiste en conocer por inspiración divina las cosas distantes o futuras». Podría considerarse la existencia de diferencias entre los términos profecía y predicción. El Diccionario de la lengua española de la Real Academia Española no marca límites tan precisos en el sentido de la palabra predicción, al señalar que predecir significa «anunciar por revelación, ciencia o conjetura algo que ha de suceder». Por lo tanto, la predicción puede involucrar un don sobrenatural, un proceso lógico-racional, o un juicio más o menos subjetivo basado en indicios u observaciones. Por el contrario, la mayoría de las acepciones del citado diccionario referidas a la palabra profecía señalan que se trataría de un «don sobrenatural», es decir, que sería «inspirada por Dios». Así, se sitúa a las profecías mayormente en el ámbito de la fe, sin ligarlas necesariamente a un razonamiento en la previsión del resultado predicho. En grados diversos y formas variables, las religiones de la antigüedad hicieron referencia a hombres «inspirados» que afirmaban hablar en nombre de su dios.Pero en las grandes religiones monoteístas (judaísmo, cristianismo, islam), las manifestaciones extraordinarias nunca constituyen lo esencial en los profetas, que se distinguen claramente de otros exaltados o simuladores por tener simplemente carácter de mensajeros. Las profecías eran, pues, consideradas simples indicadores del designio de Dios. Hasta la fecha, más allá de las evidencias científicas que puedan o no resultar suficientes para unos u otros, muchos seguidores de estas grandes religiones históricas afirman que, en buena medida, las profecías de sus libros sagrados se han cumplido. <![CDATA[<a href="#_dbpedia_2017">(DBpedia, 2017)</a>]]></skos:definition>
    <skos:definition xml:lang="nl">Het woord profetie is afgeleid van het Griekse woord propheteía, dat uitspreken of voor iemand anders spreken betekent. In algemene zin wordt met 'profetie' gewoonlijk een voorspellende uitspraak over gebeurtenissen in de toekomst bedoeld. <![CDATA[<a href="#_dbpedia_2017">(DBpedia, 2017)</a>]]></skos:definition>
    <prov:derivedFrom rdf:resource="http://dbpedia.org/resource/Prophecy"/>
    <rdfs:comment xml:lang="en">The description for this term is indebted to DBpedia. </rdfs:comment>
  </genre:Genre>
  <genre:Genre rdf:about="#genrePsalm">
    <rdf:value>PSALM</rdf:value>
    <rdfs:label xml:lang="en">psalm</rdfs:label>
    <rdfs:label xml:lang="fr"/>
    <rdfs:isDefinedBy rdf:resource="http://sparql.cwrc.ca/ontologies/genre-ONTOLOGY_DATE"/>
    <void:inDataset rdf:resource="#datasetdefinition"/>
    <skos:inScheme rdf:resource="#Genre"/>
    <rdf:type rdf:resource="http://www.w3.org/2004/02/skos/core#Concept"/>
  </genre:Genre>
  <genre:Genre rdf:about="#genrePsychoanalytical">
    <rdf:value>PSYCHOANALYTICAL</rdf:value>
    <rdfs:label xml:lang="en">psychoanalytical</rdfs:label>
    <rdfs:label xml:lang="fr"/>
    <rdfs:isDefinedBy rdf:resource="http://sparql.cwrc.ca/ontologies/genre-ONTOLOGY_DATE"/>
    <void:inDataset rdf:resource="#datasetdefinition"/>
    <skos:inScheme rdf:resource="#Genre"/>
    <rdf:type rdf:resource="http://www.w3.org/2004/02/skos/core#Concept"/>
  </genre:Genre>
  <genre:Genre rdf:about="#genreQuiz">
    <rdf:value>QUIZ</rdf:value>
    <rdfs:label xml:lang="en">quiz</rdfs:label>
    <rdfs:label xml:lang="fr"/>
    <rdfs:isDefinedBy rdf:resource="http://sparql.cwrc.ca/ontologies/genre-ONTOLOGY_DATE"/>
    <void:inDataset rdf:resource="#datasetdefinition"/>
    <skos:inScheme rdf:resource="#Genre"/>
    <rdf:type rdf:resource="http://www.w3.org/2004/02/skos/core#Concept"/>
  </genre:Genre>
  <genre:Genre rdf:about="#genreRadiodrama">
    <rdf:value>RADIODRAMA</rdf:value>
    <rdfs:label xml:lang="en">radio drama</rdfs:label>
    <rdfs:label xml:lang="fr"/>
    <rdfs:isDefinedBy rdf:resource="http://sparql.cwrc.ca/ontologies/genre-ONTOLOGY_DATE"/>
    <void:inDataset rdf:resource="#datasetdefinition"/>
    <skos:inScheme rdf:resource="#Genre"/>
    <rdf:type rdf:resource="http://www.w3.org/2004/02/skos/core#Concept"/>
  </genre:Genre>
  <genre:Genre rdf:about="#genreRealist">
    <rdf:value>REALIST</rdf:value>
    <rdfs:label xml:lang="en">realist</rdfs:label>
    <rdfs:label xml:lang="fr">réaliste</rdfs:label>
    <rdfs:isDefinedBy rdf:resource="http://sparql.cwrc.ca/ontologies/genre-ONTOLOGY_DATE"/>
    <void:inDataset rdf:resource="#datasetdefinition"/>
    <skos:inScheme rdf:resource="#Genre"/>
    <rdf:type rdf:resource="http://www.w3.org/2004/02/skos/core#Concept"/>
    <skos:definition xml:lang="en">General term for a quality of art works in which the depiction is based on or seems to be based on the direct observation of the external world, including or even emphasizing flaws and imperfections rather than the beauty or idealized characteristics. Although a work may be both realistic and naturalistic, naturalism may somewhat idealize the flaws or ugliness of the subject depicted. <![CDATA[<a href="#_getty_2017">(Getty, 2017)</a>]]></skos:definition>
     <prov:derivedFrom rdf:resource="http://vocab.getty.edu/aat/300056550"/>
    <rdfs:comment xml:lang="en">The description for this term is indebted to the Getty Art &amp; Architecture Thesaurus.</rdfs:comment>
  </genre:Genre>
  <genre:Genre rdf:about="#genreRegional">
    <rdf:value>REGIONAL</rdf:value>
    <rdfs:label xml:lang="en">regional</rdfs:label>
    <rdfs:label xml:lang="fr"/>
    <rdfs:isDefinedBy rdf:resource="http://sparql.cwrc.ca/ontologies/genre-ONTOLOGY_DATE"/>
    <void:inDataset rdf:resource="#datasetdefinition"/>
    <skos:inScheme rdf:resource="#Genre"/>
    <rdf:type rdf:resource="http://www.w3.org/2004/02/skos/core#Concept"/>
  </genre:Genre>
  <genre:Genre rdf:about="#genreReligious">
    <rdf:value>RELIGIOUS</rdf:value>
    <rdfs:label xml:lang="en">religious</rdfs:label>
    <rdfs:label xml:lang="fr">religieux</rdfs:label>
    <rdfs:isDefinedBy rdf:resource="http://sparql.cwrc.ca/ontologies/genre-ONTOLOGY_DATE"/>
    <void:inDataset rdf:resource="#datasetdefinition"/>
    <skos:inScheme rdf:resource="#Genre"/>
    <rdf:type rdf:resource="http://www.w3.org/2004/02/skos/core#Concept"/>
  </genre:Genre>
  <genre:Genre rdf:about="#genreReview">
    <rdf:value>REVIEW</rdf:value>
    <rdfs:label xml:lang="en">review</rdfs:label>
    <rdfs:label xml:lang="fr"/>
    <rdfs:isDefinedBy rdf:resource="http://sparql.cwrc.ca/ontologies/genre-ONTOLOGY_DATE"/>
    <void:inDataset rdf:resource="#datasetdefinition"/>
    <skos:inScheme rdf:resource="#Genre"/>
    <rdf:type rdf:resource="http://www.w3.org/2004/02/skos/core#Concept"/>
  </genre:Genre>
  <genre:Genre rdf:about="#genreRevue">
    <rdf:value>REVUE</rdf:value>
    <rdfs:label xml:lang="en">revue</rdfs:label>
    <rdfs:label xml:lang="fr"/>
    <rdfs:isDefinedBy rdf:resource="http://sparql.cwrc.ca/ontologies/genre-ONTOLOGY_DATE"/>
    <void:inDataset rdf:resource="#datasetdefinition"/>
    <skos:inScheme rdf:resource="#Genre"/>
    <rdf:type rdf:resource="http://www.w3.org/2004/02/skos/core#Concept"/>
    <skos:definition xml:lang="en">Periodicals, reports, or essays giving critical estimates and appraisals of art, a performance, or event. For other critical descriptions and analyses, prefer &quot;criticism.&quot; <![CDATA[<a href="#_getty_2017">(Getty, 2017)</a>]]></skos:definition>
    <skos:definition xml:lang="de">Zeitschrift, Bericht oder Essay mit kritischen Urteilen und Einschätzungen zu Kunst, Theater oder Veranstaltungen. Für kritische Beschreibungen und Analysen anderer Art, siehe &quot;Kritik&quot;. <![CDATA[<a href="#_getty_2017">(Getty, 2017)</a>]]></skos:definition>
    <skos:definition xml:lang="es">Informes o ensayos que dan una estimación crítica de un trabajo, desempeño o suceso relativamente reciente. Para otras descripciones críticas y otros análisis críticos, prefiera &quot;crítica&quot;. <![CDATA[<a href="#_getty_2017">(Getty, 2017)</a>]]></skos:definition>
    <skos:definition xml:lang="nl">Verslagen of essays die kritische beoordelingen geven van een relatief recent werk, voorstelling of gebeurtenis. Voor andere kritische beschrijvingen en analyses wordt de voorkeur gegeven aan 'kritieken' <![CDATA[<a href="#_getty_2017">(Getty, 2017)</a>]]></skos:definition>
    <prov:derivedFrom rdf:resource="http://vocab.getty.edu/aat/300026480"/>
    <rdfs:comment xml:lang="en">The description for this term is indebted to the Getty Art &amp; Architecture Thesaurus.</rdfs:comment>
  </genre:Genre>
  <genre:Genre rdf:about="#genreRiddle">
    <rdf:value>RIDDLE</rdf:value>
    <rdfs:label xml:lang="en">riddle</rdfs:label>
    <rdfs:label xml:lang="fr">énigme</rdfs:label>
    <rdfs:isDefinedBy rdf:resource="http://sparql.cwrc.ca/ontologies/genre-ONTOLOGY_DATE"/>
    <void:inDataset rdf:resource="#datasetdefinition"/>
    <skos:inScheme rdf:resource="#Genre"/>
    <rdf:type rdf:resource="http://www.w3.org/2004/02/skos/core#Concept"/>
    <skos:definition xml:lang="en">(from Old English roedel, from roedan meaning &quot;to give council&quot; or &quot;to read&quot;): A universal form of literature in which a puzzling question or a conundrum is presented to the reader. The reader is often challenged to solve this enigma, which requires ingenuity in discovering the hidden meaning. A riddle may involve puns, symbolism, synecdoche, personification (especially prosopopoeia), or unusual imagery. For instance, a Norse riddle asks, &quot;Tell me what I am. Thirty white horses round a red hill. First they champ. Then they stamp. Now they stand still.&quot; The answer is the speaker's teeth; these thirty white horses circle the &quot;red hill&quot; of the tongue; they champ and stamp while the riddler speaks, but stand still at the end of his riddle. Another famous example is the riddle of the sphinx from Sophocles' Oedipus Trilogy. The sphinx asks Oedipus, &quot;What goes on four feet, on two feet, and then three. But the more feet it goes on, the weaker is he?&quot; The answer is a human being, which crawls as an infant, walks erect on two feet as an adult, and totters on a staff (the third leg) in old age. The earliest known English riddles are recorded in the Exeter Book, and they probably date back to the 8th century. Examples, however, can be found in Greek, Sanskrit, Hebrew, Arabic, Persian, and Chinese, and many other languages. Authors of Anglo-Latin riddles include Aldhelm of Sherborne, Archbishop Tatwine of Canterbury, and Abbot Eusebius of Wearmouth. A large Renaissance collection can also be found in Nicolas Reusner's Aenigmatographia (1602). <![CDATA[<a href="#_wheeler_2017">(L. K Wheeler, 2017)</a>]]></skos:definition>
    <prov:derivedFrom rdf:resource="http://web.cn.edu/kwheeler/lit_terms_r.html"/>
    <rdfs:comment xml:lang="en">The description for this term is indebted to Dr. L. Kip Wheeler of Carson-Newman University. </rdfs:comment>
  </genre:Genre>
  <genre:Genre rdf:about="#genreRomance">
    <rdf:value>ROMANCE</rdf:value>
    <rdfs:label xml:lang="en">romance</rdfs:label>
    <rdfs:label xml:lang="fr"/>
    <rdfs:isDefinedBy rdf:resource="http://sparql.cwrc.ca/ontologies/genre-ONTOLOGY_DATE"/>
    <void:inDataset rdf:resource="#datasetdefinition"/>
    <skos:inScheme rdf:resource="#Genre"/>
    <rdf:type rdf:resource="http://www.w3.org/2004/02/skos/core#Concept"/>
    <skos:definition xml:lang="en">Poetic or prosaic literary forms derived from medieval narratives of love, legendary or heroic adventures, and chivalry. Extends to narratives about important religious figures, or fantastic or supernatural events. <![CDATA[<a href="#_getty_2017">(Getty, 2017)</a>]]></skos:definition>
    <skos:definition xml:lang="es">Narraciones en verso o prosa que relatan sucesos heroicos, fantásticos o sobrenaturales que a menudo transcurren en tiempos medievales. <![CDATA[<a href="#_getty_2017">(Getty, 2017)</a>]]></skos:definition>
    <skos:definition xml:lang="nl">Vertellingen in proza of versvorm, zich vaak afspelend in de middeleeuwen, waarin grootse, fantastische of bovennatuurlijke gebeurtenissen worden beschreven. <![CDATA[<a href="#_getty_2017">(Getty, 2017)</a>]]></skos:definition>
    <skos:definition xml:lang="zh-hant">描述英雄事蹟、幻想，或超自然事件的詩文或散文體記敘文，常設定於中世紀時期。 <![CDATA[<a href="#_getty_2017">(Getty, 2017)</a>]]></skos:definition>
    <prov:derivedFrom rdf:resource="http://vocab.getty.edu/aat/300191065"/>
    <rdfs:comment xml:lang="en">The description for this term is indebted to the Getty Art &amp; Architecture Thesaurus.</rdfs:comment>
  </genre:Genre>
  <genre:Genre rdf:about="#genreSagewriting">
    <rdf:value>SAGEWRITING</rdf:value>
    <rdfs:label xml:lang="en">sage writing</rdfs:label>
    <rdfs:label xml:lang="fr"/>
    <rdfs:isDefinedBy rdf:resource="http://sparql.cwrc.ca/ontologies/genre-ONTOLOGY_DATE"/>
    <void:inDataset rdf:resource="#datasetdefinition"/>
    <skos:inScheme rdf:resource="#Genre"/>
    <rdf:type rdf:resource="http://www.w3.org/2004/02/skos/core#Concept"/>
    <skos:definition xml:lang="en">Sage writing was a genre of creative nonfiction popular in the Victorian era. The concept originates with John Holloway's 1953 book The Victorian Sage: Studies in Argument. Sage writing is a development from ancient wisdom literature in which the writer chastises and instructs the reader about contemporary social issues, often utilizing discourses of philosophy, history, politics, and economics in non-technical ways. Prominent examples of the genre include writings by Thomas Carlyle, Matthew Arnold, John Ruskin, and Henry David Thoreau. Some 20th-century writers, such as Joan Didion and New Journalists such as Norman Mailer and Tom Wolfe, have also been identified as sage writers. <![CDATA[<a href="#_dbpedia_2017">(DBpedia, 2017)</a>]]></skos:definition>
    <prov:derivedFrom rdf:resource="http://dbpedia.org/resource/Sage_writing"/>
    <rdfs:comment xml:lang="en">The description for this term is indebted to DBpedia. </rdfs:comment>
  </genre:Genre>
  <genre:Genre rdf:about="#genreSatire">
    <rdf:value>SATIRE</rdf:value>
    <rdfs:label xml:lang="en">satire</rdfs:label>
    <rdfs:label xml:lang="fr">satire</rdfs:label>
    <rdfs:isDefinedBy rdf:resource="http://sparql.cwrc.ca/ontologies/genre-ONTOLOGY_DATE"/>
    <void:inDataset rdf:resource="#datasetdefinition"/>
    <skos:inScheme rdf:resource="#Genre"/>
    <rdf:type rdf:resource="http://www.w3.org/2004/02/skos/core#Concept"/>
    <skos:definition xml:lang="fr">Une satire est une œuvre dont l'objectif est une critique moqueuse de son sujet (des individus, des organisations, des États, etc.), souvent dans l'intention de provoquer, prévenir un changement ou de porter à réfléchir. On attribue généralement la paternité de ce genre littéraire (satura, c'est-à-dire pot-pourri) au poète archaïque latin Lucilius. <![CDATA[<a href="#_dbpedia_2017">(DBpedia, 2017)</a>]]></skos:definition>
    <prov:derivedFrom rdf:resource="http://dbpedia.org/resource/Satire"/>
    <rdfs:comment xml:lang="en">The description for this term is indebted to DBpedia. </rdfs:comment>
    <skos:definition xml:lang="en">Literary compositions in verse or prose, or ideas expressed as the subjects of art works, in which human folly and vice are held up to scorn, derision, or ridicule. <![CDATA[<a href="#_getty_2017">(Getty, 2017)</a>]]></skos:definition>
    <skos:definition xml:lang="de">Werk der Literatur in Versen oder in Prosa, oder eine in einem Kunstwerk ausgedrückte Idee, in denen menschliche Torheit oder Laster lächerlich gemacht oder mit Hohn und Spott überzogen werden. <![CDATA[<a href="#_getty_2017">(Getty, 2017)</a>]]></skos:definition>
    <skos:definition xml:lang="nl">Literaire werken in versvorm of proza waarin menselijke dwaasheden en ondeugden op spottende wijze aan de kaak worden gesteld. <![CDATA[<a href="#_getty_2017">(Getty, 2017)</a>]]></skos:definition>
    <skos:definition xml:lang="es">Composiciones literarias en verso o prosa en las cuales la locura y los vicios humanos son presentados con desprecio, escarnio o burla. <![CDATA[<a href="#_getty_2017">(Getty, 2017)</a>]]></skos:definition>
    <skos:definition xml:lang="zh-hant">指用韻文或散文創作之文學作品，作品凸顯人類的愚蠢與惡習，而加以奚落、嘲弄、或揶揄。 <![CDATA[<a href="#_getty_2017">(Getty, 2017)</a>]]></skos:definition>
    <prov:derivedFrom rdf:resource="http://vocab.getty.edu/aat/300251297"/>
    <rdfs:comment xml:lang="en">The description for this term is indebted to the Getty Art &amp; Architecture Thesaurus.</rdfs:comment>
  </genre:Genre>
  <genre:Genre rdf:about="#genreScholarship">
    <rdf:value>SCHOLARSHIP</rdf:value>
    <rdfs:label xml:lang="en">scholarship</rdfs:label>
    <rdfs:label xml:lang="fr"/>
    <rdfs:isDefinedBy rdf:resource="http://sparql.cwrc.ca/ontologies/genre-ONTOLOGY_DATE"/>
    <void:inDataset rdf:resource="#datasetdefinition"/>
    <skos:inScheme rdf:resource="#Genre"/>
    <rdf:type rdf:resource="http://www.w3.org/2004/02/skos/core#Concept"/>
  </genre:Genre>
  <genre:Genre rdf:about="#genreSchoolfiction">
    <rdf:value>SCHOOLFICTION</rdf:value>
    <rdfs:label xml:lang="en">school fiction</rdfs:label>
    <rdfs:label xml:lang="fr"/>
    <rdfs:isDefinedBy rdf:resource="http://sparql.cwrc.ca/ontologies/genre-ONTOLOGY_DATE"/>
    <void:inDataset rdf:resource="#datasetdefinition"/>
    <skos:inScheme rdf:resource="#Genre"/>
    <rdf:type rdf:resource="http://www.w3.org/2004/02/skos/core#Concept"/>
  </genre:Genre>
  <genre:Genre rdf:about="#genreSciencefiction">
    <rdf:value>SCIENCEFICTION</rdf:value>
    <rdfs:label xml:lang="en">science fiction</rdfs:label>
    <rdfs:label xml:lang="fr"/>
    <rdfs:isDefinedBy rdf:resource="http://sparql.cwrc.ca/ontologies/genre-ONTOLOGY_DATE"/>
    <void:inDataset rdf:resource="#datasetdefinition"/>
    <skos:inScheme rdf:resource="#Genre"/>
    <rdf:type rdf:resource="http://www.w3.org/2004/02/skos/core#Concept"/>
    <skos:definition xml:lang="en">Science fiction is a genre of speculative fiction dealing with imaginative concepts such as futuristic settings, futuristic science and technology, space travel, time travel, faster than light travel, parallel universes and extraterrestrial life. Science fiction often explores the potential consequences of scientific and other innovations, and has been called a &quot;literature of ideas.&quot; It usually eschews the supernatural, and unlike the related genre of fantasy, historically science fiction stories were intended to have at least a faint grounding in science-based fact or theory at the time the story was created, but this connection has become tenuous or non-existent in much of science fiction. <![CDATA[<a href="#_dbpedia_2017">(DBpedia, 2017)</a>]]></skos:definition>
    <skos:definition xml:lang="fr">La science-fiction est un genre narratif, principalement un genre littéraire et un genre cinématographique. Il est structuré par des hypothèses sur ce que pourrait être le futur ou ce qu'aurait pu être le présent voire le passé (planètes éloignées, mondes parallèles, uchronie...), en partant des connaissances actuelles (scientifiques, technologiques, ethnologiques...). Elle se distingue du fantastique qui inclut une dimension inexplicable et de la fantasy qui fait souvent intervenir la magie. <![CDATA[<a href="#_dbpedia_2017">(DBpedia, 2017)</a>]]></skos:definition>
    <skos:definition xml:lang="de">Science-Fiction [ˌsaɪəns ˈfɪkʃən̩] (engl. science „Wissenschaft“, fiction „Fiktion“) ist ein Genre der Literatur und des Films, aber auch anderer Bereiche wie etwa der bildenden Kunst oder der Videospiele, das den Einzelnen, die Gesellschaft oder die Umwelt in (oft radikal) alternativen Konstellationen betrachtet. Science-Fiction entwirft – häufig in die Zukunft verlegte, teilweise auch räumlich entfernte – Konstellationen des Möglichen und beschreibt deren Auswirkungen. Dabei werden reale wissenschaftliche und technische Möglichkeiten mit fiktionalen Spekulationen angereichert. <![CDATA[<a href="#_dbpedia_2017">(DBpedia, 2017)</a>]]></skos:definition>
    <skos:definition xml:lang="es">Ciencia ficción es la denominación popular con que se conoce a uno de los géneros derivados de la literatura de ficción, junto con la literatura fantástica y la narrativa de terror. Nacida como subgénero literario distinguido en la década de 1920 (aunque hay obras reconocibles muy anteriores) y exportada posteriormente a otros medios, como el cinematográfico, historietístico y televisivo, gozó de un gran auge en la segunda mitad del sigloxx debido al interés popular acerca del futuro que despertó el espectacular avance tanto científico como tecnológico alcanzado durante todos estos años. Es un género especulativo que relata acontecimientos posibles desarrollados en un marco puramente imaginario, cuya verosimilitud se fundamenta narrativamente en los campos de las ciencias físicas, naturales y sociales. La acción puede girar en torno a un abanico grande de posibilidades (viajes interestelares, conquista del espacio, consecuencias de una hecatombe terrestre o cósmica, evolución humana a causa de mutaciones, evolución de los robots, realidad virtual, existencia de civilizaciones alienígenas, etc.). Esta acción puede tener lugar en un tiempo pasado, presente o futuro, o, incluso, en tiempos alternativos ajenos a la realidad conocida, y tener por escenario espacios físicos (reales o imaginarios, terrestres o extraterrestres) o el espacio interno de la mente. Los personajes son igualmente diversos: a partir del patrón natural humano, recorre y explota modelos antropomórficos hasta desembocar en la creación de entidades artificiales de forma humana (robot, androide, cíborg) o en criaturas no antropomórficas. <![CDATA[<a href="#_dbpedia_2017">(DBpedia, 2017)</a>]]></skos:definition>
    <skos:definition xml:lang="nl">Sciencefiction (afgekort sf, scifi of essef, in het Engels als science fiction gespeld), is tegenwoordig een belangrijk genre dat vooral opgeld heeft gedaan in literatuur, stripverhalen, films, televisieseries, hoorspelen en computerspellen. Het Engelse &quot;science fiction&quot; betekent letterlijk vertaald &quot;wetenschapsfictie&quot;, en dit is dan ook de betekenis die de bedenker van de term, Hugo Gernsback, eraan heeft willen geven. Voor Gernsback was de sciencefiction vooral bedoeld als een middel tot popularisatie van de wetenschap en van wetenschappelijke ontdekkingen, maar de geschiedenis ervan laat zien dat deze gedachte door latere schrijvers slechts beperkt is nagestreefd. In het genre worden tegenwoordig vooral toekomstbeelden met verzonnen technologische vooruitgang en wetenschappelijke ontwikkelingen gebruikt. <![CDATA[<a href="#_dbpedia_2017">(DBpedia, 2017)</a>]]></skos:definition>
    <prov:derivedFrom rdf:resource="http://dbpedia.org/resource/Science_fiction"/>
    <rdfs:comment xml:lang="en">The description for this term is indebted to DBpedia. </rdfs:comment>
  </genre:Genre>
  <genre:Genre rdf:about="#genreScientificwriting">
    <rdf:value>SCIENTIFICWRITING</rdf:value>
    <rdfs:label xml:lang="en">scientific writing</rdfs:label>
    <rdfs:label xml:lang="fr"/>
    <rdfs:isDefinedBy rdf:resource="http://sparql.cwrc.ca/ontologies/genre-ONTOLOGY_DATE"/>
    <void:inDataset rdf:resource="#datasetdefinition"/>
    <skos:inScheme rdf:resource="#Genre"/>
    <rdf:type rdf:resource="http://www.w3.org/2004/02/skos/core#Concept"/>
  </genre:Genre>
  <genre:Genre rdf:about="#genreScrapbook">
    <rdf:value>SCRAPBOOK</rdf:value>
    <rdfs:label xml:lang="en">scrapbook</rdfs:label>
    <rdfs:label xml:lang="fr"/>
    <rdfs:isDefinedBy rdf:resource="http://sparql.cwrc.ca/ontologies/genre-ONTOLOGY_DATE"/>
    <void:inDataset rdf:resource="#datasetdefinition"/>
    <skos:inScheme rdf:resource="#Genre"/>
    <rdf:type rdf:resource="http://www.w3.org/2004/02/skos/core#Concept"/>
  </genre:Genre>
  <genre:Genre rdf:about="#genreSensationnovel">
    <rdf:value>SENSATIONNOVEL</rdf:value>
    <rdfs:label xml:lang="en">sensation novel</rdfs:label>
    <rdfs:label xml:lang="fr"/>
    <rdfs:isDefinedBy rdf:resource="http://sparql.cwrc.ca/ontologies/genre-ONTOLOGY_DATE"/>
    <void:inDataset rdf:resource="#datasetdefinition"/>
    <skos:inScheme rdf:resource="#Genre"/>
    <rdf:type rdf:resource="http://www.w3.org/2004/02/skos/core#Concept"/>
    <skos:definition xml:lang="en">The sensation novel was a literary genre of fiction popular in Great Britain in the 1860s and 1870s, following on from earlier melodramatic novels and the Newgate novels, which focused on tales woven around criminal biographies. It also drew on the gothic and romantic genres of fiction. The sensation novel's appearance notably follows the Industrial Revolution, which made books available on a mass scale for people of all social standings and increased the sensation novel's popularity. Sensation novels used both modes of romance and realism to the extreme where in the past they had traditionally been contradictory modes of literature. The sensation novelists commonly wrote stories that were allegorical and abstract; the abstract nature of the stories gave the authors room to explore scenarios that wrestled with the social anxieties of the Victorian Era. The loss of identity is seen in many sensation fiction stories because this was a common social anxiety; in Britain, there was an increased use in record keeping and therefore people questioned the meaning and permanence of identity. The social anxiety regarding identity is reflected in stories, such as, The Woman in White and Lady Audley's Secret. The genre of sensation fiction was established by the publications of the following novels The Woman in White by Wilkie Collins in 1859; East Lynne by Ellen Wood in 1861; Lady Audley's Secret by Mary Elizabeth Braddon in 1862. Perhaps the earliest use of the term, sensation fiction, as a name for such novels appears in the 1861 edition of the Saunders, Otley, &amp; co.'s Literary Budget. The neo-Victorian novel of New Zealand author Eleanor Catton, The Luminaries, which won the 2013 Man Booker Prize, has been described as being heavily based on sensation literature, with its plot devices of &quot;suspect wills and forged documents, secret marriages, illegitimacy and opium&quot; <![CDATA[<a href="#_dbpedia_2017">(DBpedia, 2017)</a>]]></skos:definition>
    <skos:definition xml:lang="fr">Le roman à sensation est un genre littéraire né dans la deuxième moitié du XIXe siècle en Grande-Bretagne. Ce genre littéraire est une évolution des romans mélodramatiques, qui utilisaient un ensemble de personnages stéréotypés, et des romans Newgate, qui avaient pour thème principal la vie de célèbres criminels. East Lynne de Ellen Wood's, paru en 1861, fut le premier roman à être étiqueté comme roman à sensation par la critique. Le courant comprend trois auteurs majeurs : Ellen Woods, Wilkie Collins (La Femme en blanc, 1859; La Pierre de lune, 1868) et Mary Elizabeth Braddon (Le secret de Lady Audley, 1862). Les romans à sensation avaient pour thèmes des sujets choquants comme l'adultère, le vol, l'enlèvement, la bigamie, la fabrication de fausse monnaie, la séduction et le meurtre. Le genre se distinguait des autres mouvements de l'époque, comme le mouvement Gothique, par l'utilisation de ces thèmes dans un contexte domestique, voire familial, allant ainsi à l'encontre de l'idée largement répandue à l'époque victorienne que les événements sensationnels étaient totalement étrangers à la vie confortable des classes moyennes qui composaient la plus grande partie du lectorat de l'époque. William S. Gilbert fit une satire du genre en 1871 avec son opéra comique A Sensation Novel. <![CDATA[<a href="#_dbpedia_2017">(DBpedia, 2017)</a>]]></skos:definition>
    <prov:derivedFrom rdf:resource="http://dbpedia.org/resource/Sensation_novel"/>
    <rdfs:comment xml:lang="en">The description for this term is indebted to DBpedia. </rdfs:comment>
    <skos:broaderTransitive rdf:resource="#genreNovel"/>
  </genre:Genre>
  <genre:Genre rdf:about="#genreSentimental">
    <rdf:value>SENTIMENTAL</rdf:value>
    <rdfs:label xml:lang="en">sentimental</rdfs:label>
    <rdfs:label xml:lang="fr"/>
    <rdfs:isDefinedBy rdf:resource="http://sparql.cwrc.ca/ontologies/genre-ONTOLOGY_DATE"/>
    <void:inDataset rdf:resource="#datasetdefinition"/>
    <skos:inScheme rdf:resource="#Genre"/>
    <rdf:type rdf:resource="http://www.w3.org/2004/02/skos/core#Concept"/>
    <skos:definition xml:lang="en">The sentimental novel or the novel of sensibility is an 18th-century literary genre which celebrates the emotional and intellectual concepts of sentiment, sentimentalism, and sensibility. Sentimentalism, which is to be distinguished from sensibility, was a fashion in both poetry and prose fiction beginning in the eighteenth century in reaction to the rationalism of the Augustan Age. Sentimental novels relied on emotional response, both from their readers and characters. They feature scenes of distress and tenderness, and the plot is arranged to advance both emotions and actions. The result is a valorization of &quot;fine feeling,&quot; displaying the characters as a model for refined, sensitive emotional effect. The ability to display feelings was thought to show character and experience, and to shape social life and relations. <![CDATA[<a href="#_dbpedia_2017">(DBpedia, 2017)</a>]]></skos:definition>
    <skos:definition xml:lang="es">La novela sentimental es un subgénero literario histórico que se desarrolla entre el Prerrenacimiento del siglo XV y el Renacimiento de la primera mitad del siglo XVI. Se incluye dentro del género épico o narrativo y se compone en prosa con versos intercalados, a veces en forma epistolar; posee temática amorosa, frecuentemente dentro de las leyes del llamado amor cortés. <![CDATA[<a href="#_dbpedia_2017">(DBpedia, 2017)</a>]]></skos:definition>
    <prov:derivedFrom rdf:resource="http://dbpedia.org/resource/Sentimental_novel"/>
    <rdfs:comment xml:lang="en">The description for this term is indebted to DBpedia. </rdfs:comment>
  </genre:Genre>
  <genre:Genre rdf:about="#genreSequel">
    <rdf:value>SEQUEL</rdf:value>
    <rdfs:label xml:lang="en">sequel</rdfs:label>
    <rdfs:label xml:lang="fr"/>
    <rdfs:isDefinedBy rdf:resource="http://sparql.cwrc.ca/ontologies/genre-ONTOLOGY_DATE"/>
    <void:inDataset rdf:resource="#datasetdefinition"/>
    <skos:inScheme rdf:resource="#Genre"/>
    <rdf:type rdf:resource="http://www.w3.org/2004/02/skos/core#Concept"/>
    <skos:definition xml:lang="en">(from Latin sequi, to follow): A literary work complete in itself, but continuing the narrative of an earlier work. It is a new story that extends or develops characters and situations found in an earlier work. Two sequels following an original work (together) are called a trilogy. Three sequels following an original work together are called a tetralogy.Often sequels have a reputation for inferior artistry compared to the original publication since they are often hastily written from the desire to capitalize on earlier financial success. Examples include Mark Twain's Tom Sawyer Abroad, which is a sequel to The Adventures of Tom Sawyer, and Alexandra Ripley's Scarlett, which is a sequel to Mitchell's Gone With the Wind. In the late twentieth century, it became common retroactively to write &quot;prequels,&quot; a later book with the same geographic setting or characters, but which takes place in an earlier time. <![CDATA[<a href="#_wheeler_2017">(L. K Wheeler, 2017)</a>]]></skos:definition>
    <prov:derivedFrom rdf:resource="http://web.cn.edu/kwheeler/lit_terms_s.html"/>
    <rdfs:comment xml:lang="en">The description for this term is indebted to Dr. L. Kip Wheeler of Carson-Newman University. </rdfs:comment>
  </genre:Genre>
  <genre:Genre rdf:about="#genreSermon">
    <rdf:value>SERMON</rdf:value>
    <rdfs:label xml:lang="en">sermon</rdfs:label>
    <rdfs:label xml:lang="fr"/>
    <rdfs:isDefinedBy rdf:resource="http://sparql.cwrc.ca/ontologies/genre-ONTOLOGY_DATE"/>
    <void:inDataset rdf:resource="#datasetdefinition"/>
    <skos:inScheme rdf:resource="#Genre"/>
    <rdf:type rdf:resource="http://www.w3.org/2004/02/skos/core#Concept"/>
    <skos:definition xml:lang="en">A sermon is an oration, lecture, or talk by a member of a religious institution or clergy. Sermons address a Biblical, theological, religious, or moral topic, usually expounding on a type of belief, law or behavior within both past and present contexts. Elements of the sermon often include exposition, exhortation and practical application. In Christianity, a sermon (also known as a homily within some churches) is usually delivered in a place of worship from an elevated architectural feature, variously known as a pulpit, a lectern, or an ambo. The word &quot;sermon&quot; comes from a Middle English word which was derived from Old French, which in turn came from the Latin word sermō meaning &quot;discourse&quot;. The word can mean &quot;conversation&quot;, which could mean that early sermons were delivered in the form of question and answer, and that only later did it come to mean a monologue. However, the Bible contains many speeches without interlocution, which some take to be sermons: Moses in Deuteronomy 1-33 ; Jesus' sermon on the mount in Matthew 5-7 (though the gospel writers do not specifically call it a sermon; the popular descriptor for Christ's speech there came much later); Peter after Pentecost in Acts 2:14-40 (though this speech was delivered to nonbelievers and as such is not quite parallel to the popular definition of a sermon). In modern language, the word &quot;sermon&quot; is used in secular terms, pejoratively, to describe a lengthy or tedious speech delivered with great passion, by any person, to an uninterested audience. A sermonette is a short sermon (usually associated with television broadcasting, as stations would present a sermonette before signing off for the night). <![CDATA[<a href="#_dbpedia_2017">(DBpedia, 2017)</a>]]></skos:definition>
    <skos:definition xml:lang="fr">Le sermon est un discours de prédication prononcé dans des circonstances religieuses. <![CDATA[<a href="#_dbpedia_2017">(DBpedia, 2017)</a>]]></skos:definition>
    <skos:definition xml:lang="de">Predigt (lat. praedicatio), auf Englisch und Französisch sermon (von lat. sermo ‚Wechselrede, Gespräch; Vortrag) ist eine Rede mit religiösem Inhalt oder eine Rede im Kontext einer religiösen Feier. Die Predigt hat einen besonderen Stellenwert im Neuen Testament und im christlichen Gottesdienst. In der christlichen Theologie wird die Lehre von der Predigt als Homiletik bezeichnet. <![CDATA[<a href="#_dbpedia_2017">(DBpedia, 2017)</a>]]></skos:definition>
    <skos:definition xml:lang="es">Se denomina sermón u homilía al género de la oratoria que consiste en un discurso de tema religioso, por lo general pronunciado durante el culto cristiano. El sermón se pronunciaba, en la primera liturgia cristiana, en latín, pero después, en vista de que el pueblo ya no entendía el latín culto, empezó a pronunciarse en lengua vernácula, mientras que el resto de la liturgia continuaba pronunciándose en latín. Algunos autores piensan que ese fue el origen de cierto transvase de voces, proverbios y cuentecillos cultos a la lengua vulgar, dando origen a buena parte de la literatura folclórica. El sermón podría ser dogmático, místico, ascético o parenético. Era dogmático si trataba de dogmas; los que explicaban los misterios, eran los sermones místicos; los que trataban sobre las prácticas religiosas, se denominaban ascéticos y los que versaban sobre cuestiones morales, parenéticos. Estos últimos se subdividían a su vez en homilías, pláticas y sermones propiamente dichos. También existe el fervorín (antes de comulgar), la oración fúnebre (glosando las virtudes de un difunto) y el panegírico (en honor de un santo). <![CDATA[<a href="#_dbpedia_2017">(DBpedia, 2017)</a>]]></skos:definition>
    <skos:definition xml:lang="nl">De preek of prediking is een belangrijk onderdeel van de eredienst in verschillende godsdiensten. De leer van het doordenken, maken en geven van een preek of homilie heet homiletiek. <![CDATA[<a href="#_dbpedia_2017">(DBpedia, 2017)</a>]]></skos:definition>
    <prov:derivedFrom rdf:resource="http://dbpedia.org/resource/Sermon"/>
    <rdfs:comment xml:lang="en">The description for this term is indebted to DBpedia. </rdfs:comment>
  </genre:Genre>
  <genre:Genre rdf:about="#genreSexualawakeningfiction">
    <rdf:value>SEXUALAWAKENINGFICTION</rdf:value>
    <rdfs:label xml:lang="en">sexual awakening fiction</rdfs:label>
    <rdfs:label xml:lang="fr"/>
    <rdfs:isDefinedBy rdf:resource="http://sparql.cwrc.ca/ontologies/genre-ONTOLOGY_DATE"/>
    <void:inDataset rdf:resource="#datasetdefinition"/>
    <skos:inScheme rdf:resource="#Genre"/>
    <rdf:type rdf:resource="http://www.w3.org/2004/02/skos/core#Concept"/>
  </genre:Genre>
  <genre:Genre rdf:about="#genreShortstory">
    <rdf:value>SHORTSTORY</rdf:value>
    <rdfs:label xml:lang="en">short story</rdfs:label>
    <rdfs:label xml:lang="fr">nouvelle</rdfs:label>
    <rdfs:isDefinedBy rdf:resource="http://sparql.cwrc.ca/ontologies/genre-ONTOLOGY_DATE"/>
    <void:inDataset rdf:resource="#datasetdefinition"/>
    <skos:inScheme rdf:resource="#Genre"/>
    <rdf:type rdf:resource="http://www.w3.org/2004/02/skos/core#Concept"/>
    <skos:definition xml:lang="en">Relatively brief invented prose narratives. <![CDATA[<a href="#_getty_2017">(Getty, 2017)</a>]]></skos:definition>
    <skos:definition xml:lang="de">Verhältnismäßig kurze fiktionale Prosaerzählung. <![CDATA[<a href="#_getty_2017">(Getty, 2017)</a>]]></skos:definition>
    <skos:definition xml:lang="nl">Betrekkelijk korte, verzonnen prozavertellingen. <![CDATA[<a href="#_getty_2017">(Getty, 2017)</a>]]></skos:definition>
    <skos:definition xml:lang="es">Narraciones ficticias en prosa, relativamente breves. <![CDATA[<a href="#_getty_2017">(Getty, 2017)</a>]]></skos:definition>
    <skos:definition xml:lang="zh-hant">篇幅相對較短的虛構性散文體記敘文。 <![CDATA[<a href="#_getty_2017">(Getty, 2017)</a>]]></skos:definition>
    <prov:derivedFrom rdf:resource="http://vocab.getty.edu/aat/300202607"/>
    <rdfs:comment xml:lang="en">The description for this term is indebted to the Getty Art &amp; Architecture Thesaurus.</rdfs:comment>
  </genre:Genre>
  <genre:Genre rdf:about="#genreSilverforknovel">
    <rdf:value>SILVERFORKNOVEL</rdf:value>
    <rdfs:label xml:lang="en">silverfork novel</rdfs:label>
    <rdfs:label xml:lang="fr"/>
    <rdfs:isDefinedBy rdf:resource="http://sparql.cwrc.ca/ontologies/genre-ONTOLOGY_DATE"/>
    <void:inDataset rdf:resource="#datasetdefinition"/>
    <skos:inScheme rdf:resource="#Genre"/>
    <rdf:type rdf:resource="http://www.w3.org/2004/02/skos/core#Concept"/>
    <skos:broaderTransitive rdf:resource="#genreNovel"/>
  </genre:Genre>
  <genre:Genre rdf:about="#genreSketch">
    <rdf:value>SKETCH</rdf:value>
    <rdfs:label xml:lang="en">sketch</rdfs:label>
    <rdfs:label xml:lang="fr"/>
    <rdfs:isDefinedBy rdf:resource="http://sparql.cwrc.ca/ontologies/genre-ONTOLOGY_DATE"/>
    <void:inDataset rdf:resource="#datasetdefinition"/>
    <skos:inScheme rdf:resource="#Genre"/>
    <rdf:type rdf:resource="http://www.w3.org/2004/02/skos/core#Concept"/>
    <skos:definition xml:lang="en">Short literary compositions on single subjects, often presenting the personal view of the author. <![CDATA[<a href="#_getty_2017">(Getty, 2017)</a>]]></skos:definition>
    <skos:definition xml:lang="es">Breves composiciones literarias sobre temas específicos, a menudo presentando el punto de vista personal del autor. <![CDATA[<a href="#_getty_2017">(Getty, 2017)</a>]]></skos:definition>
    <skos:definition xml:lang="nl">Korte literaire verhandelingen over één onderwerp, waarin de auteur dikwijls een persoonlijk standpunt verwoordt. <![CDATA[<a href="#_getty_2017">(Getty, 2017)</a>]]></skos:definition>
    <skos:definition xml:lang="de">Kurzer literarischer Aufsatz über ein Einzelthema, gibt häufig die persönliche Meinung des Autors wieder. <![CDATA[<a href="#_getty_2017">(Getty, 2017)</a>]]></skos:definition>
    <skos:definition xml:lang="zh-hant">單一主題的簡短文學作品，常表述作者之個人觀點。<![CDATA[<a href="#_getty_2017">(Getty, 2017)</a>]]></skos:definition>
    <prov:derivedFrom rdf:resource="http://vocab.getty.edu/aat/300026291"/>
    <rdfs:comment xml:lang="en">The description for this term is indebted to the Getty Art &amp; Architecture Thesaurus.</rdfs:comment>
  </genre:Genre>
  <genre:Genre rdf:about="#genreSketchbook">
    <rdf:value>SKETCHBOOK</rdf:value>
    <rdfs:label xml:lang="en">sketch book</rdfs:label>
    <rdfs:label xml:lang="fr"/>
    <rdfs:isDefinedBy rdf:resource="http://sparql.cwrc.ca/ontologies/genre-ONTOLOGY_DATE"/>
    <void:inDataset rdf:resource="#datasetdefinition"/>
    <skos:inScheme rdf:resource="#Genre"/>
    <rdf:type rdf:resource="http://www.w3.org/2004/02/skos/core#Concept"/>
    <skos:definition xml:lang="en">Books or pads of blank sheets used or intended for sketching, which are informal or rough drawings. <![CDATA[<a href="#_getty_2017">(Getty, 2017)</a>]]></skos:definition>
    <skos:definition xml:lang="es">Libros o blocs de hojas en blanco usadas o para ser usadas en bosquejos. <![CDATA[<a href="#_getty_2017">(Getty, 2017)</a>]]></skos:definition>
    <skos:definition xml:lang="nl">Boeken of blokken blanco papier die worden gebruikt of zijn bedoeld om op te schetsen. <![CDATA[<a href="#_getty_2017">(Getty, 2017)</a>]]></skos:definition>
    <prov:derivedFrom rdf:resource="http://vocab.getty.edu/aat/300027354"/>
    <rdfs:comment xml:lang="en">The description for this term is indebted to the Getty Art &amp; Architecture Thesaurus.</rdfs:comment>
  </genre:Genre>
  <genre:Genre rdf:about="#genreSlavenarrative">
    <rdf:value>SLAVENARRATIVE</rdf:value>
    <rdfs:label xml:lang="en">slave narrative</rdfs:label>
    <rdfs:label xml:lang="fr"/>
    <rdfs:isDefinedBy rdf:resource="http://sparql.cwrc.ca/ontologies/genre-ONTOLOGY_DATE"/>
    <void:inDataset rdf:resource="#datasetdefinition"/>
    <skos:inScheme rdf:resource="#Genre"/>
    <rdf:type rdf:resource="http://www.w3.org/2004/02/skos/core#Concept"/>
  </genre:Genre>
  <genre:Genre rdf:about="#genreSocialscience">
    <rdf:value>SOCIALSCIENCE</rdf:value>
    <rdfs:label xml:lang="en">social science</rdfs:label>
    <rdfs:label xml:lang="fr"/>
    <rdfs:isDefinedBy rdf:resource="http://sparql.cwrc.ca/ontologies/genre-ONTOLOGY_DATE"/>
    <void:inDataset rdf:resource="#datasetdefinition"/>
    <skos:inScheme rdf:resource="#Genre"/>
    <rdf:type rdf:resource="http://www.w3.org/2004/02/skos/core#Concept"/>
  </genre:Genre>
  <genre:Genre rdf:about="#genreSong">
    <rdf:value>SONG</rdf:value>
    <rdfs:label xml:lang="en">song</rdfs:label>
    <rdfs:label xml:lang="fr"/>
    <rdfs:isDefinedBy rdf:resource="http://sparql.cwrc.ca/ontologies/genre-ONTOLOGY_DATE"/>
    <void:inDataset rdf:resource="#datasetdefinition"/>
    <skos:inScheme rdf:resource="#Genre"/>
    <rdf:type rdf:resource="http://www.w3.org/2004/02/skos/core#Concept"/>
    <skos:definition xml:lang="en">A lyric poem with a number of repeating stanzas (called refrains), written to be set to music in either vocal performance or with accompaniment of musical instruments. See dawn song and lyric, above and stanza, below. <![CDATA[<a href="#_wheeler_2017">(L. K Wheeler, 2017)</a>]]></skos:definition>
    <prov:derivedFrom rdf:resource="http://web.cn.edu/kwheeler/lit_terms_s.html"/>
    <rdfs:comment xml:lang="en">The description for this term is indebted to Dr. L. Kip Wheeler of Carson-Newman University. </rdfs:comment>
  </genre:Genre>
  <genre:Genre rdf:about="#genreSonnet">
    <rdf:value>SONNET</rdf:value>
    <rdfs:label xml:lang="en">sonnet</rdfs:label>
    <rdfs:label xml:lang="fr"/>
    <rdfs:isDefinedBy rdf:resource="http://sparql.cwrc.ca/ontologies/genre-ONTOLOGY_DATE"/>
    <void:inDataset rdf:resource="#datasetdefinition"/>
    <skos:inScheme rdf:resource="#Genre"/>
    <rdf:type rdf:resource="http://www.w3.org/2004/02/skos/core#Concept"/>
    <skos:definition xml:lang="en">Poems consisting of 14 decasyllabic lines, often in a rhyming scheme. The sonnet form is considered to be of Italian origin, appearing in the 13th century in Sicily, after which it spread to Tuscany, where Petrarch perfected the form with his Canzioniere, a series of 317 sonnets to his idealized love, Laura. The Petrarchian sonnet has historically been the most widely used of the form, although the Elizabethan form (3 quatrains, with a final rhyming couplet) is also common. <![CDATA[<a href="#_getty_2017">(Getty, 2017)</a>]]></skos:definition>
    <skos:definition xml:lang="de">Gedicht, das aus 14 zehnsilbigen Verszeilen besteht, häufig mit Reimschema. Die Sonettform stammt vermutlich aus Italien, wo sie im 13. Jahrhundert in Sizilien aufkam und sich dann bis in die Toskana ausbreitete, wo Petrarca sie mit seinem Canzoniere perfektionierte, einer Sammlung aus 317 Sonetten, die an Laura, seine idealisierte Geliebte, gerichtet sind. Das petrarkische Sonett ist die historisch am weitesten verbreitete Form, obwohl die elisabethanische Form (3 Quartette mit einem Paarreim am Schluss) ebenfalls häufig anzutreffen ist. <![CDATA[<a href="#_getty_2017">(Getty, 2017)</a>]]></skos:definition>
    <skos:definition xml:lang="zh-hant">由十四行十音節詩行所組成的詩，常押韻。十四行詩形式被認為源於義大利，13世紀於西西里島出現，爾後傳播至多斯加尼(或譯托斯卡尼)，佩脫拉克在此完成Canzioniere集，一系列共317首十四行詩，獻給其理想愛人蘿拉，將此一形式臻於完美。史上該形式最廣為使用佩脫拉克式十四行詩，但伊莉莎白式十四行詩（3段四行詩，加上最後押韻的對句）也很常見。<![CDATA[<a href="#_getty_2017">(Getty, 2017)</a>]]></skos:definition>
    <skos:definition xml:lang="nl">Gedicht van veertien regels met tien lettergrepen, vaak met een rijmschema. Men denkt dat het sonnet oorspronkelijk uit Italië komt. De eerste sonnetten verschenen in de dertiende eeuw op Sicilië. Daarna verspreidden ze zich naar Toscane, waar Petrarca de vorm perfectioneerde in zijn Canzioniere, een serie van 317 sonnetten voor zijn geïdealiseerde geliefde Laura. Het petrarkische sonnet is historisch gezien het meest gebruikte sonnet, hoewel het shakespearesonnet (drie kwatrijnen en twee slotregels met gepaard rijm) ook veel voorkomt. <![CDATA[<a href="#_getty_2017">(Getty, 2017)</a>]]></skos:definition>
    <prov:derivedFrom rdf:resource="http://vocab.getty.edu/aat/300266382"/>
    <rdfs:comment xml:lang="en">The description for this term is indebted to the Getty Art &amp; Architecture Thesaurus.</rdfs:comment>
  </genre:Genre>
  <genre:Genre rdf:about="#genreSpeech">
    <rdf:value>SPEECH</rdf:value>
    <rdfs:label xml:lang="en">speech</rdfs:label>
    <rdfs:label xml:lang="fr"/>
    <rdfs:isDefinedBy rdf:resource="http://sparql.cwrc.ca/ontologies/genre-ONTOLOGY_DATE"/>
    <void:inDataset rdf:resource="#datasetdefinition"/>
    <skos:inScheme rdf:resource="#Genre"/>
    <rdf:type rdf:resource="http://www.w3.org/2004/02/skos/core#Concept"/>
    <skos:definition xml:lang="en">Documents containing the text of any public address or talk <![CDATA[<a href="#_getty_2017">(Getty, 2017)</a>]]></skos:definition>
    <prov:derivedFrom rdf:resource="http://vocab.getty.edu/aat/300026671"/>
    <rdfs:comment xml:lang="en">The description for this term is indebted to the Getty Art &amp; Architecture Thesaurus.</rdfs:comment>
  </genre:Genre>
  <genre:Genre rdf:about="#genreTestimony">
    <rdf:value>TESTIMONY</rdf:value>
    <rdfs:label xml:lang="en">testimony</rdfs:label>
    <rdfs:label xml:lang="fr"/>
    <rdfs:isDefinedBy rdf:resource="http://sparql.cwrc.ca/ontologies/genre-ONTOLOGY_DATE"/>
    <void:inDataset rdf:resource="#datasetdefinition"/>
    <skos:inScheme rdf:resource="#Genre"/>
    <rdf:type rdf:resource="http://www.w3.org/2004/02/skos/core#Concept"/>
    <skos:definition xml:lang="en">Solemn declarations, written or verbal; usually made orally by a witness under oath in response to interrogation by a lawyer or authorized public official, then reduced to writing for the record. <![CDATA[<a href="#_getty_2017">(Getty, 2017)</a>]]></skos:definition>
    <skos:definition xml:lang="es">Declaraciones solemnes, generalmente hechas oralmente por un testigo bajo juramento en respuesta al interrogatorio de un abogado o funcionario público autorizado, en su versión escrita. <![CDATA[<a href="#_getty_2017">(Getty, 2017)</a>]]></skos:definition>
    <skos:definition xml:lang="nl">Plechtige verklaringen, meestal mondeling afgelegd door een getuige onder ede als antwoord op een ondervraging door een advocaat of een gemachtigde functionaris en teruggebracht tot een geschreven stuk. <![CDATA[<a href="#_getty_2017">(Getty, 2017)</a>]]></skos:definition>
    <prov:derivedFrom rdf:resource="http://vocab.getty.edu/aat/300027861"/>
    <rdfs:comment xml:lang="en">The description for this term is indebted to the Getty Art &amp; Architecture Thesaurus.</rdfs:comment>
  </genre:Genre>
  <genre:Genre rdf:about="#genreTextbook">
    <rdf:value>TEXTBOOK</rdf:value>
    <rdfs:label xml:lang="en">textbook</rdfs:label>
    <rdfs:label xml:lang="fr"/>
    <rdfs:isDefinedBy rdf:resource="http://sparql.cwrc.ca/ontologies/genre-ONTOLOGY_DATE"/>
    <void:inDataset rdf:resource="#datasetdefinition"/>
    <skos:inScheme rdf:resource="#Genre"/>
    <rdf:type rdf:resource="http://www.w3.org/2004/02/skos/core#Concept"/>
    <skos:definition xml:lang="en">Books used as standard works for the formal study of a particular subject. <![CDATA[<a href="#_getty_2017">(Getty, 2017)</a>]]></skos:definition>
    <skos:definition xml:lang="de">Buch, das für das Studium eines bestimmten Themas als Standardwerk gilt. <![CDATA[<a href="#_getty_2017">(Getty, 2017)</a>]]></skos:definition>
    <skos:definition xml:lang="nl">Boeken die bij uitstek worden gebruikt bij de studie van een bepaald onderwerp of een bepaalde wetenschap. <![CDATA[<a href="#_getty_2017">(Getty, 2017)</a>]]></skos:definition>
    <skos:definition xml:lang="es">Libros usados como obras oficiales para el estudio formal de alguna materia en particular. <![CDATA[<a href="#_getty_2017">(Getty, 2017)</a>]]></skos:definition>
    <skos:definition xml:lang="zh-hant">某特定學科之正規標準學習用書籍。 <![CDATA[<a href="#_getty_2017">(Getty, 2017)</a>]]></skos:definition>
    <prov:derivedFrom rdf:resource="http://vocab.getty.edu/aat/300026384"/>
    <rdfs:comment xml:lang="en">The description for this term is indebted to the Getty Art &amp; Architecture Thesaurus.</rdfs:comment>
  </genre:Genre>
  <genre:Genre rdf:about="#genreTheatreofcruelty">
    <rdf:value>THEATREOFCRUELTY</rdf:value>
    <rdfs:label xml:lang="en">theatre of cruelty</rdfs:label>
    <rdfs:label xml:lang="fr"/>
    <rdfs:isDefinedBy rdf:resource="http://sparql.cwrc.ca/ontologies/genre-ONTOLOGY_DATE"/>
    <void:inDataset rdf:resource="#datasetdefinition"/>
    <skos:inScheme rdf:resource="#Genre"/>
    <rdf:type rdf:resource="http://www.w3.org/2004/02/skos/core#Concept"/>
  </genre:Genre>
  <genre:Genre rdf:about="#genreTheatreoftheabsurd">
    <rdf:value>THEATREOFTHEABSURD</rdf:value>
    <rdfs:label xml:lang="en">theatre of the absurd</rdfs:label>
    <rdfs:label xml:lang="fr"/>
    <rdfs:isDefinedBy rdf:resource="http://sparql.cwrc.ca/ontologies/genre-ONTOLOGY_DATE"/>
    <void:inDataset rdf:resource="#datasetdefinition"/>
    <skos:inScheme rdf:resource="#Genre"/>
    <rdf:type rdf:resource="http://www.w3.org/2004/02/skos/core#Concept"/>
  </genre:Genre>
  <genre:Genre rdf:about="#genreTheology">
    <rdf:value>THEOLOGY</rdf:value>
    <rdfs:label xml:lang="en">theology</rdfs:label>
    <rdfs:label xml:lang="fr"/>
    <rdfs:isDefinedBy rdf:resource="http://sparql.cwrc.ca/ontologies/genre-ONTOLOGY_DATE"/>
    <void:inDataset rdf:resource="#datasetdefinition"/>
    <skos:inScheme rdf:resource="#Genre"/>
    <rdf:type rdf:resource="http://www.w3.org/2004/02/skos/core#Concept"/>
  </genre:Genre>
  <genre:Genre rdf:about="#genreThesaurus">
    <rdf:value>THESAURUS</rdf:value>
    <rdfs:label xml:lang="en">thesaurus</rdfs:label>
    <rdfs:label xml:lang="fr"/>
    <rdfs:isDefinedBy rdf:resource="http://sparql.cwrc.ca/ontologies/genre-ONTOLOGY_DATE"/>
    <void:inDataset rdf:resource="#datasetdefinition"/>
    <skos:inScheme rdf:resource="#Genre"/>
    <rdf:type rdf:resource="http://www.w3.org/2004/02/skos/core#Concept"/>
  </genre:Genre>
  <genre:Genre rdf:about="#genreThriller">
    <rdf:value>THRILLER</rdf:value>
    <rdfs:label xml:lang="en">thriller</rdfs:label>
    <rdfs:label xml:lang="fr"/>
    <rdfs:isDefinedBy rdf:resource="http://sparql.cwrc.ca/ontologies/genre-ONTOLOGY_DATE"/>
    <void:inDataset rdf:resource="#datasetdefinition"/>
    <skos:inScheme rdf:resource="#Genre"/>
    <rdf:type rdf:resource="http://www.w3.org/2004/02/skos/core#Concept"/>
  </genre:Genre>
  <genre:Genre rdf:about="#genreTopographicalpoetry">
    <rdf:value>TOPOGRAPHICALPOETRY</rdf:value>
    <rdfs:label xml:lang="en">topographical poetry</rdfs:label>
    <rdfs:label xml:lang="fr"/>
    <rdfs:isDefinedBy rdf:resource="http://sparql.cwrc.ca/ontologies/genre-ONTOLOGY_DATE"/>
    <void:inDataset rdf:resource="#datasetdefinition"/>
    <skos:inScheme rdf:resource="#Genre"/>
    <rdf:type rdf:resource="http://www.w3.org/2004/02/skos/core#Concept"/>
    <skos:definition xml:lang="en">Topographical poetry or loco-descriptive poetry is a genre of poetry that describes, and often praises, a landscape or place. John Denham's 1642 poem &quot;Cooper's Hill&quot; established the genre, which peaked in popularity in 18th-century England. Examples of topographical verse date, however, to the late classical period, and can be found throughout the medieval era and during the Renaissance. Though the earliest examples come mostly from continental Europe, the topographical poetry in the tradition originating with Denham concerns itself with the classics, and many of the various types of topographical verse, such as river, ruin, or hilltop poems were established by the early 17th century. Alexander Pope's &quot;Windsor Forest&quot; (1713) and John Dyer's &quot;Grongar Hill' (1762) are two other oft-mentioned examples. More recently, Matthew Arnold's &quot;The Scholar Gipsy&quot; (1853) praises the Oxfordshire countryside, and W. H. Auden's &quot;In Praise of Limestone&quot; (1948) uses a limestone landscape as an allegory. Subgenres of topographical poetry include the country house poem, written in 17th-century England to compliment a wealthy patron, and the prospect poem, describing the view from a distance or a temporal view into the future, with the sense of opportunity or expectation. When understood broadly as landscape poetry and when assessed from its establishment to the present, topographical poetry can take on many formal situations and types of places. Kenneth Baker identifies 37 varieties and compiles poems from the 16th through the 20th centuries—from Edmund Spenser to Sylvia Plath—correspondent to each type, from &quot;Walks and Surveys,&quot; to &quot;Mountains, Hills, and the View from Above,&quot; to &quot;Violation of Nature and the Landscape,&quot; to &quot;Spirits and Ghosts.&quot; Common aesthetic registers of which topographical poetry make use include pastoral imagery, the sublime, and the picturesque. These latter two registers subsume imagery of rivers, ruins, moonlight, birdsong, and clouds, peasants, mountains, caves, and waterscapes. <![CDATA[<a href="#_dbpedia_2017">(DBpedia, 2017)</a>]]></skos:definition>
    <prov:derivedFrom rdf:resource="http://dbpedia.org/resource/Topographical_poetry"/>
    <rdfs:comment xml:lang="en">The description for this term is indebted to DBpedia. </rdfs:comment>
    <skos:broaderTransitive rdf:resource="#genrePoetry"/>
  </genre:Genre>
  <genre:Genre rdf:about="#genreTractpamphlet">
    <rdf:value>TRACTPAMPHLET</rdf:value>
    <rdfs:label xml:lang="en">tract pamphlet</rdfs:label>
    <rdfs:label xml:lang="fr"/>
    <rdfs:isDefinedBy rdf:resource="http://sparql.cwrc.ca/ontologies/genre-ONTOLOGY_DATE"/>
    <void:inDataset rdf:resource="#datasetdefinition"/>
    <skos:inScheme rdf:resource="#Genre"/>
    <rdf:type rdf:resource="http://www.w3.org/2004/02/skos/core#Concept"/>
  </genre:Genre>
  <genre:Genre rdf:about="#genreTragedy">
    <rdf:value>TRAGEDY</rdf:value>
    <rdfs:label xml:lang="en">tragedy</rdfs:label>
    <rdfs:label xml:lang="fr">tragédie</rdfs:label>
    <rdfs:isDefinedBy rdf:resource="http://sparql.cwrc.ca/ontologies/genre-ONTOLOGY_DATE"/>
    <void:inDataset rdf:resource="#datasetdefinition"/>
    <skos:inScheme rdf:resource="#Genre"/>
    <rdf:type rdf:resource="http://www.w3.org/2004/02/skos/core#Concept"/>
    <skos:definition xml:lang="en">Literary works of serious and dignified character that reach disastrous or sorrowful conclusions. <![CDATA[<a href="#_getty_2017">(Getty, 2017)</a>]]></skos:definition>
    <skos:definition xml:lang="nl">Literaire werken met een ernstig en plechtig karakter die toewerken naar een rampzalig of droevig slot. <![CDATA[<a href="#_getty_2017">(Getty, 2017)</a>]]></skos:definition>
    <skos:definition xml:lang="es">Trabajos literarios de carácter serio y solemne que terminan en desenlaces funestos o lamentables. <![CDATA[<a href="#_getty_2017">(Getty, 2017)</a>]]></skos:definition>
    <skos:definition xml:lang="de">Literarisches Werk mit ernstem und würdevollem Charakter, das katastrophal oder unglücklich endet. <![CDATA[<a href="#_getty_2017">(Getty, 2017)</a>]]></skos:definition>
    <prov:derivedFrom rdf:resource="http://vocab.getty.edu/aat/300201026"/>
    <rdfs:comment xml:lang="en">The description for this term is indebted to the Getty Art &amp; Architecture Thesaurus.</rdfs:comment>
    <skos:definition xml:lang="fr">La tragédie est un genre théâtral dont l’origine remonte au théâtre grec antique. Contrairement à la comédie, elle met en scène des personnages de rangs élevés et se dénoue très souvent par la mort d’un ou de plusieurs personnages.Elle a un rôle cathartique (prévenir les gens de ne pas faire le Mal en suscitant terreur et pitié). <![CDATA[<a href="#_dbpedia_2017">(DBpedia, 2017)</a>]]></skos:definition>
    <prov:derivedFrom rdf:resource="http://dbpedia.org/resource/Tragedy"/>
    <rdfs:comment xml:lang="en">The description for this term is indebted to DBpedia. </rdfs:comment>
  </genre:Genre>
  <genre:Genre rdf:about="#genreTragicomedy">
    <rdf:value>TRAGICOMEDY</rdf:value>
    <rdfs:label xml:lang="en">tragicomedy</rdfs:label>
    <rdfs:label xml:lang="fr"/>
    <rdfs:isDefinedBy rdf:resource="http://sparql.cwrc.ca/ontologies/genre-ONTOLOGY_DATE"/>
    <void:inDataset rdf:resource="#datasetdefinition"/>
    <skos:inScheme rdf:resource="#Genre"/>
    <rdf:type rdf:resource="http://www.w3.org/2004/02/skos/core#Concept"/>
    <skos:definition xml:lang="en">Tragicomedy is a literary genre that blends aspects of both tragic and comic forms. Most often seen in dramatic literature, the term can variously describe either a tragic play which contains enough comic elements to lighten the overall mood or a serious play with a happy ending. <![CDATA[<a href="#_dbpedia_2017">(DBpedia, 2017)</a>]]></skos:definition>
    <skos:definition xml:lang="fr">La tragi-comédie est une forme théâtrale caractérisée par une action romanesque, des personnages de haute extraction, un dénouement heureux et un refus des règles de la tragédie. Le terme est apparu en France chez le dramaturge Robert Garnier vers la fin du XVIe siècle, orthographié tragecomedie ; le terme nous vient de Plaute, qui désigne son Amphitryon comme une &quot;tragi-comoedia&quot; (au vers 59). Ce genre a connu un très grand succès en France dans les années 1630-1640. Il est assez difficile de définir les limites de la tragi-comédie à cette époque parce que les auteurs revendiquaient le refus de toute règle. On pouvait alors voir dans la tragi-comédie une sorte de tragédie à fin heureuse parce que la tragédie n'était définie que par son personnel noble et mythologique. Dans les années 1640, les partisans d'un théâtre beaucoup plus normé prennent de plus en plus d'importance et la tragédie répondant aux règles classiques prend le dessus sur la tragi-comédie. Le cas du Le Cid de Corneille est un exemple intéressant à cet égard car il a été publié en 1637 en tant que tragi-comédie et requalifié en tragédie dès 1648 alors que Corneille n'avait pas encore effectué de modification majeure de la pièce. On peut donc considérer que ce n'est pas la pièce mais la perception qu'on avait des différents genres théâtraux qui a évolué entre ces deux dates. En effet, l'intrigue du Cid comporte de nombreux éléments caractéristiques d'une tragi-comédie : il raconte une histoire d'amour dans laquelle un obstacle empêche à un moment donné la réunion des deux amants. À la fin de la pièce, cet obstacle sera levé et le dénouement sera heureux et nuptial ce qui est à l'époque une caractéristique des comédies et des tragi-comédies. La Querelle du Cid aura contribué à fixer les règles de la tragédie même si Le Cid conserve ses caractéristiques à savoir l'accumulation des événements , les coups de théâtre, les changements de décor successif et le dénouement heureux. On a beaucoup reproché à Corneille l'invraisemblance de la fin et un respect très discutable des trois unités. De fait, même s'il est déjà influencé par les règles qui commencent à s'imposer à la fin des années 1630, Corneille conserve dans cette pièce une liberté de composition héritée de la tragi-comédie et que l'on ne trouvera plus dans ses tragédies ultérieures. Pour autant, la pièce annonce la dramaturgie classique parce que les conflits omniprésents qui la constituent ne se manifestent pas à travers de combats spectaculaires sur scène mais à travers le travail du langage. Ainsi le duel entre Rodrigue et Don Gomes s'achève très vite alors que les célébrissimes stances du Cid rendent compte longuement du conflit intérieur qui travaille Rodrigue. Ce refus du spectaculaire au profit d'un travail sur le discours et les sentiments des personnages sera caractéristique de l'esthétique classique et explique que le Cid en soit resté un exemple majeur alors qu'il est encore très influencé par le genre de la tragi-comédie qui s'oppose aux caractéristiques de l'écriture classique. Philippe Quinault , poète et librettiste français, a aussi contribué au succès de ce genre en participant à la création de la tragédie-ballet Psyché en 1671 écrit par Molière aidé de Corneille. Le mélange des genres fut peu représenté par la suite dans le théâtre français, tout au plus trouve-t-on des pièces ou les genres s'alternent sans se mêler. Victor Hugo tente pourtant d'imposer avec son théâtre romantique une écriture entre sublime et grotesque, mais il faudra attendre le XXe siècle et le théâtre de l'absurde pour que le public accepte de concevoir que le rire ne nuit pas obligatoirement à la profondeur dramatique. <![CDATA[<a href="#_dbpedia_2017">(DBpedia, 2017)</a>]]></skos:definition>
    <skos:definition xml:lang="de">Eine Tragikomödie beschreibt ein Drama in der Literatur und im Theater, in dem die Merkmale der Tragödie wie auch der Komödie eng miteinander verknüpft sind. Im weiteren Sinne bezeichnet der Begriff eine Tragödie, welche neben den tragischen auch komische Bestandteile enthält, wie z. B. die alten spanischen und englischen Tragödien. <![CDATA[<a href="#_dbpedia_2017">(DBpedia, 2017)</a>]]></skos:definition>
    <skos:definition xml:lang="es">Una tragicomedia es una gran obra dramática en la que se mezclan los elementos trágicos y cómicos, aunque también hay lugar para el sarcasmo y parodia. También se le conoce como pieza, porque se parece a dicho concepto; generalmente en estos están sintetizadas las características de una clase social, por lo que también se le denomina género psicológico. Una pieza es una obra literaria del tipo realista, en donde la situación y los personajes están claramente presentados. Si bien en lo que se relata y expone hay cambios inesperados, ellos son lógicos y explicables, y el suspenso va en continuo aumento, llegando por momentos a clímax con intensas emociones. La resolución o conclusión de la obra es consecuencia de los actos y de las situaciones planteadas con bastante claridad y sin ambigüedades, donde los actos de los personajes son verosímiles. En la Grecia clásica, el drama satírico o la tragicomedia suele tratar un tema legendario, aunque con efectos cómicos protagonizados, fundamentalmente, por el coro. Los dioses no intervienen en la muerte de los hombres y puede haber más de una acción al mismo tiempo. La tragicomedia principalmente va a mostrar la trayectoria del héroe tragicómico, que tiene un objetivo que perseguir (el amor, la justicia, la ambición, un trono, etc) y de cómo éste lo consigue o no pasando por una serie de obstáculos para llegar a su fin. Si los obstáculos se presentan como positivos, es decir que parece que lo acercan cada vez más a su objetivo, más que obstáculos son como pruebas superadas. Por su parte el final será negativo, si los obstáculos son negativos, y parece que le impiden llegar a su objetivo, aunque por lo general el final será positivo y aunque sea a último minuto alcanzará su objetivo. Su creador fue Lope de Vega cuando rompió las estructuras del teatro aristotélico. Lope se negaba a obedecer las unidades, y entonces creó la tragicomedia. <![CDATA[<a href="#_dbpedia_2017">(DBpedia, 2017)</a>]]></skos:definition>
    <skos:definition xml:lang="nl">Een tragikomedie is een dramavorm die zowel in het theater als in zijn afgeleide, de film, een vermenging hanteert van tragische en komische verhaalelementen. Eén van de eerste auteurs die deze mengvorm beheersten, was Plautus, zo ongeveer in 210 v.Chr., met zijn stuk Amphitruo, dat in de 17e eeuw Molière inspireerde tot het schrijven van zijn Amphitrion (1668). De samenstelling tragikomedie geeft aan dat komedie de hoofdbedoeling is, maar dat er enkele tragische gegevens doorheen lopen. Het begrip is pas tegen het einde van de 16e eeuw echt doorgebroken. De theoreticus van dienst is een zekere Italiaan Battista Guarini met zijn verhandelingen die gebundeld zijn als Compendio della poesia tragicomica (1601). Rond dezelfde tijd vinden we in Shakespeares drama's een hele variëteit clowneske figuren terug: de clown is de tragikomische mens bij uitstek. Een typisch voorbeeld is Le Cid van Pierre Corneille. Enkele van de nevenpersonages sterven hierin, maar voor de twee hoofdpersonages kent het verhaal een gunstige afloop. Aangezien de combinatie tragiek en komedie ook scherp wordt aangevoeld door auteurs die ironie, satire en cynisme gepast kunnen hanteren, vind je in het absurde theater van Samuel Beckett, Eugène Ionesco en Harold Pinter ook veel tragikomische situaties en personages. In de film denke men aan Charlie Chaplin, de hoofdfiguur in zijn eigen stomme films. <![CDATA[<a href="#_dbpedia_2017">(DBpedia, 2017)</a>]]></skos:definition>
    <prov:derivedFrom rdf:resource="http://dbpedia.org/resource/Tragicomedy"/>
    <rdfs:comment xml:lang="en">The description for this term is indebted to DBpedia. </rdfs:comment>
    <skos:definition xml:lang="en">A experimental literary work--either a play or prose piece of fiction--containing elements common to both comedies and tragedies. The genre is marked by characters of both high and low degree, even though classical drama required upper-class characters for tragedy and lower-class characters for comedy. Tragicomedies were of some interest in the Renaissance, but some modern dramas might be considered examples as well. Typically, the early stages of the play resembled those of a tragedy, but an abrupt reversal of circumstance prevent the tragedy. <![CDATA[<a href="#_wheeler_2017">(L. K Wheeler, 2017)</a>]]></skos:definition>
    <prov:derivedFrom rdf:resource="http://web.cn.edu/kwheeler/lit_terms_t.html"/>
    <rdfs:comment xml:lang="en">The description for this term is indebted to Dr. L. Kip Wheeler of Carson-Newman University. </rdfs:comment>
  </genre:Genre>
  <genre:Genre rdf:about="#genreTranslation">
    <rdf:value>TRANSLATION</rdf:value>
    <rdfs:label xml:lang="en">translation</rdfs:label>
    <rdfs:label xml:lang="fr"/>
    <rdfs:isDefinedBy rdf:resource="http://sparql.cwrc.ca/ontologies/genre-ONTOLOGY_DATE"/>
    <void:inDataset rdf:resource="#datasetdefinition"/>
    <skos:inScheme rdf:resource="#Genre"/>
    <rdf:type rdf:resource="http://www.w3.org/2004/02/skos/core#Concept"/>
    <skos:definition xml:lang="en">Translated versions of a text.</skos:definition>
    <skos:definition xml:lang="es">Versiones traducidas de un texto.</skos:definition>
    <skos:definition xml:lang="nl">Vertaalde versies van een tekst.</skos:definition>
    <skos:definition xml:lang="de">Übersetzte Version eines Textes.</skos:definition>
    <skos:definition xml:lang="zh-hant">一文本之翻譯版本。</skos:definition>
    <prov:derivedFrom rdf:resource="http://vocab.getty.edu/aat/300027389"/>
    <rdfs:comment xml:lang="en">The description for this term is indebted to the Getty Art &amp; Architecture Thesaurus.</rdfs:comment>
    <skos:definition xml:lang="en">The act of conveying the meaning of words in one language by attempting to say the same thing in another language, as opposed to paraphrasing, summarizing, and transliteration. <![CDATA[<a href="#_wheeler_2017">(L. K Wheeler, 2017)</a>]]></skos:definition>
    <prov:derivedFrom rdf:resource="http://web.cn.edu/kwheeler/lit_terms_t.html"/>
    <rdfs:comment xml:lang="en">The description for this term is indebted to Dr. L. Kip Wheeler of Carson-Newman University. </rdfs:comment>
  </genre:Genre>
  <genre:Genre rdf:about="#genreTravelwriting">
    <rdf:value>TRAVELWRITING</rdf:value>
    <rdfs:label xml:lang="en">travel writing</rdfs:label>
    <rdfs:label xml:lang="fr"/>
    <rdfs:isDefinedBy rdf:resource="http://sparql.cwrc.ca/ontologies/genre-ONTOLOGY_DATE"/>
    <void:inDataset rdf:resource="#datasetdefinition"/>
    <skos:inScheme rdf:resource="#Genre"/>
    <rdf:type rdf:resource="http://www.w3.org/2004/02/skos/core#Concept"/>
  </genre:Genre>
  <genre:Genre rdf:about="#genreTreatise">
    <rdf:value>TREATISE</rdf:value>
    <rdfs:label xml:lang="en">treatise</rdfs:label>
    <rdfs:label xml:lang="fr"/>
    <rdfs:isDefinedBy rdf:resource="http://sparql.cwrc.ca/ontologies/genre-ONTOLOGY_DATE"/>
    <void:inDataset rdf:resource="#datasetdefinition"/>
    <skos:inScheme rdf:resource="#Genre"/>
    <rdf:type rdf:resource="http://www.w3.org/2004/02/skos/core#Concept"/>
    <skos:definition xml:lang="fr">Un traité est un manuel d'instructions ou un livre standard dans n'importe quelle branche qui forme un sujet d'études. Ils se différencient les uns des autres, aussi bien par le public ciblé que par le sujet abordé. Les traités sont habituellement édités par des imprimeurs spécialisés, dans le but de répondre aux besoins de formation, sur n'importe quel thème susceptible de faire l'objet d'un enseignement. Il s'agit d'un important commerce qui nécessite des ventes massives, afin de rendre ces publications rentables. Bien que la plupart des traités soient uniquement édités sous forme de livres reliés, certains sont désormais consultables sur internet. Les traités sont apparus avec le développement de l'imprimerie de Johannes Gutenberg, sous la forme de méthodes d'enseignement. <![CDATA[<a href="#_dbpedia_2017">(DBpedia, 2017)</a>]]></skos:definition>
    <prov:derivedFrom rdf:resource="http://dbpedia.org/resource/Treatise"/>
    <rdfs:comment xml:lang="en">The description for this term is indebted to DBpedia. </rdfs:comment>
    <skos:definition xml:lang="en">Formal and systematic written expositions of the principles of a subject, generally longer and more detailed than essays. <![CDATA[<a href="#_getty_2017">(Getty, 2017)</a>]]></skos:definition>
    <skos:definition xml:lang="de">Formale und systematische schriftliche Darstellung der Grundgedanken zu einem Thema, im Allgemeinen länger und detaillierter als Essays. <![CDATA[<a href="#_getty_2017">(Getty, 2017)</a>]]></skos:definition>
    <skos:definition xml:lang="es">Exposiciones escritas, formales y sistemáticas de las ideas fundamentales de un tema, generalmente más largas y más detalladas que los ensayos. <![CDATA[<a href="#_getty_2017">(Getty, 2017)</a>]]></skos:definition>
    <skos:definition xml:lang="nl">Schriftelijke documenten waarin een bepaald onderwerp volgens een erkende methode systematisch wordt behandeld. Over het algemeen zijn verhandelingen langer en meer gedetailleerd dan essays. <![CDATA[<a href="#_getty_2017">(Getty, 2017)</a>]]></skos:definition>
    <prov:derivedFrom rdf:resource="http://vocab.getty.edu/aat/300026681"/>
    <rdfs:comment xml:lang="en">The description for this term is indebted to the Getty Art &amp; Architecture Thesaurus.</rdfs:comment>
  </genre:Genre>
  <genre:Genre rdf:about="#genreUtopia">
    <rdf:value>UTOPIA</rdf:value>
    <rdfs:label xml:lang="en">utopia</rdfs:label>
    <rdfs:label xml:lang="fr"/>
    <rdfs:isDefinedBy rdf:resource="http://sparql.cwrc.ca/ontologies/genre-ONTOLOGY_DATE"/>
    <void:inDataset rdf:resource="#datasetdefinition"/>
    <skos:inScheme rdf:resource="#Genre"/>
    <rdf:type rdf:resource="http://www.w3.org/2004/02/skos/core#Concept"/>
    <skos:definition xml:lang="en">An imaginary place or government in which political and social perfection has been reached in the material world as opposed to some spiritual afterlife as discussed in the Christian Bible or the Elysian fields of The Odyssey. The citizens of such utopias are typically universally clean, virtuous, healthy, and happy, or at least those who are criminals are always captured and appropriately punished. A utopian society is one that has cured all social ills. See discussion under Utopian literature, below. Contrast with dystopia. UTOPIAN<![CDATA[<a href="#_wheeler_2017">(L. K Wheeler, 2017)</a>]]></skos:definition>
    <prov:derivedFrom rdf:resource="http://web.cn.edu/kwheeler/lit_terms_u.html"/>
    <rdfs:comment xml:lang="en">The description for this term is indebted to Dr. L. Kip Wheeler of Carson-Newman University. </rdfs:comment>
  </genre:Genre>
  <genre:Genre rdf:about="#genreVersenovel">
    <rdf:value>VERSENOVEL</rdf:value>
    <rdfs:label xml:lang="en">verse novel</rdfs:label>
    <rdfs:label xml:lang="fr"/>
    <rdfs:isDefinedBy rdf:resource="http://sparql.cwrc.ca/ontologies/genre-ONTOLOGY_DATE"/>
    <void:inDataset rdf:resource="#datasetdefinition"/>
    <skos:inScheme rdf:resource="#Genre"/>
    <rdf:type rdf:resource="http://www.w3.org/2004/02/skos/core#Concept"/>
    <skos:definition xml:lang="en">A verse novel is a type of narrative poetry in which a novel-length narrative is told through the medium of poetry rather than prose. Either simple or complex stanzaic verse-forms may be used, but there will usually be a large cast, multiple voices, dialogue, narration, description, and action in a novelistic manner. <![CDATA[<a href="#_dbpedia_2017">(DBpedia, 2017)</a>]]></skos:definition>
    <skos:definition xml:lang="de">Der Versroman ist eine als Roman geschriebene Erzählung in Vers­form; in erster Linie der Ritterroman der höfischen Dichtung des Mittelalters. Dazu zählen beispielsweise: <![CDATA[<a href="#_dbpedia_2017">(DBpedia, 2017)</a>]]></skos:definition>
    <prov:derivedFrom rdf:resource="http://dbpedia.org/resource/Verse_novel"/>
    <rdfs:comment xml:lang="en">The description for this term is indebted to DBpedia. </rdfs:comment>
    <skos:broaderTransitive rdf:resource="#genreNovel"/>
  </genre:Genre>
  <genre:Genre rdf:about="#genreVignette">
    <rdf:value>VIGNETTE</rdf:value>
    <rdfs:label xml:lang="en">vignette</rdfs:label>
    <rdfs:label xml:lang="fr"/>
    <rdfs:isDefinedBy rdf:resource="http://sparql.cwrc.ca/ontologies/genre-ONTOLOGY_DATE"/>
    <void:inDataset rdf:resource="#datasetdefinition"/>
    <skos:inScheme rdf:resource="#Genre"/>
    <rdf:type rdf:resource="http://www.w3.org/2004/02/skos/core#Concept"/>
    <skos:definition xml:lang="en">In theatrical script writing, sketch stories, and poetry, a vignette is a short impressionistic scene that focuses on one moment or gives a trenchant impression about a character, idea, setting, or object.[citation needed] This type of scene is more common in recent postmodern theater, where less emphasis is placed on adhering to the conventions of theatrical structure and story development. Vignettes have been particularly influenced by contemporary notions of a scene as shown in film, video and television scripting. It is also a part of something bigger than itself: for example, a vignette about a house belonging to a collection of vignettes or a whole story, such as The House On Mango Street, by Sandra Cisneros. A blog can provide a form of vignette. <![CDATA[<a href="#_dbpedia_2017">(DBpedia, 2017)</a>]]></skos:definition>
    <skos:definition xml:lang="nl">In proza en poëzie is een vignet een kort, impressionistisch tafereel dat een beeld schetst van een bepaald moment en een bepaalde plaats. Typisch is het de bedoeling om een scherp beeld van een personage, een idee, of een omgeving te geven. Dit type scène komt vaker voor bij het recente postmoderne theater, dat de naleving van de conventies en structuur van een verhaal ter discussie stelt. De manier waarop een scène wordt weergegeven is duidelijk beïnvloed door de hedendaagse snelle beeldcultuur van film, video en televisie. <![CDATA[<a href="#_dbpedia_2017">(DBpedia, 2017)</a>]]></skos:definition>
    <prov:derivedFrom rdf:resource="http://dbpedia.org/resource/Vignette_(literature)"/>
    <rdfs:comment xml:lang="en">The description for this term is indebted to DBpedia. </rdfs:comment>
  </genre:Genre>
  <genre:Genre rdf:about="#genreVillanelle">
    <rdf:value>VILLANELLE</rdf:value>
    <rdfs:label xml:lang="en">villanelle</rdfs:label>
    <rdfs:label xml:lang="fr"/>
    <rdfs:isDefinedBy rdf:resource="http://sparql.cwrc.ca/ontologies/genre-ONTOLOGY_DATE"/>
    <void:inDataset rdf:resource="#datasetdefinition"/>
    <skos:inScheme rdf:resource="#Genre"/>
    <rdf:type rdf:resource="http://www.w3.org/2004/02/skos/core#Concept"/>
    <skos:definition xml:lang="en">A versatile genre of poetry consisting of nineteen lines--five tercets and a concluding quatrain. The form requires that whole lines be repeated in a specific order, and that only two rhyming sounds occur in the course of the poem. A number of English poets, including Oscar Wilde, W. E. Henley, and W. H. Auden have experimented with it. Here is an example of an opening stanza to one poem by W. E. Henley: Probably the most famous English villanelle is Dylan Thomas's &quot;Do Not Go Gentle Into That Good Night.&quot;<![CDATA[<a href="#_wheeler_2017">(L. K Wheeler, 2017)</a>]]></skos:definition>
    <prov:derivedFrom rdf:resource="http://web.cn.edu/kwheeler/lit_terms_v.html"/>
    <rdfs:comment xml:lang="en">The description for this term is indebted to Dr. L. Kip Wheeler of Carson-Newman University. </rdfs:comment>
  </genre:Genre>
  <genre:Genre rdf:about="#genreYoungadultwriting">
    <rdf:value>YOUNGADULTWRITING</rdf:value>
    <rdfs:label xml:lang="en">young adult writing</rdfs:label>
    <rdfs:label xml:lang="fr"/>
    <rdfs:isDefinedBy rdf:resource="http://sparql.cwrc.ca/ontologies/genre-ONTOLOGY_DATE"/>
    <void:inDataset rdf:resource="#datasetdefinition"/>
    <skos:inScheme rdf:resource="#Genre"/>
    <rdf:type rdf:resource="http://www.w3.org/2004/02/skos/core#Concept"/>
  </genre:Genre>
</rdf:RDF>