@prefix rdf: <http://www.w3.org/1999/02/22-rdf-syntax-ns#> .
@prefix cwrc: <http://sparql.cwrc.ca/ontologies/cwrc#> .
@prefix as: <http://www.w3.org/ns/activitystreams#> .
@prefix bio: <http://purl.org/vocab/bio/0.1/> .
@prefix cc: <http://creativecommons.org/ns#> .
@prefix dbpedia: <http://dbpedia.org/resource/> .
@prefix dcterms: <http://purl.org/dc/terms/> .
@prefix doap: <http://usefulinc.com/ns/doap#> .
@prefix foaf: <http://xmlns.com/foaf/0.1/> .
@prefix eurovoc: <http://eurovoc.europa.eu/> .
@prefix geonames: <http://sws.geonames.org/> .
@prefix loc: <http://id.loc.gov/vocabulary/relators/> .
@prefix locl: <http://id.loc.gov/vocabulary/languages/> .
@prefix mil: <http://rdf.muninn-project.org/ontologies/military#> .
@prefix nif: <http://persistence.uni-leipzig.org/nlp2rdf/ontologies/nif-core#> .
@prefix oa: <http://www.w3.org/ns/oa#> .
@prefix owl: <http://www.w3.org/2002/07/owl#> .
@prefix prov: <http://www.w3.org/ns/prov#> .
@prefix rdfs: <http://www.w3.org/2000/01/rdf-schema#> .
@prefix rel: <http://purl.org/vocab/relationship/> .
@prefix skos: <http://www.w3.org/2004/02/skos/core#> .
@prefix skosxl: <http://www.w3.org/2008/05/skos-xl#> .
@prefix time: <http://www.w3.org/2006/time#> .
@prefix vann: <http://purl.org/vocab/vann/> .
@prefix voaf: <http://purl.org/vocommons/voaf#> .
@prefix void: <http://rdfs.org/ns/void#> .
@prefix vs: <http://www.w3.org/2003/06/sw-vocab-status/ns#> .
@prefix xsd: <http://www.w3.org/2001/XMLSchema#> .
@prefix frbr: <http://purl.org/vocab/frbr/core> .
@prefix bibo: <http://purl.org/ontology/bibo/> .
@prefix schema: <http://schema.org/> .

# SOPHIA KING
<http://www.cwrc.ca/cwrcdata/SophiaKing>
    cwrc:hasGender cwrc:woman ;
    cwrc:hasSocialClass cwrc:indigent, cwrc:gentry, cwrc:professional ;
    cwrc:hasGeogHeritage cwrc:portugal ;
    cwrc:hasEthnicity cwrc:jewishEthnicity ;
    cwrc:hasReligion cwrc:judaism ;
    cwrc:hasPoliticalAffiliation cwrc:radical ;
    cwrc:hasNationalitySelfReported cwrc:england ;
    a foaf:Person ;
    foaf:name "Sophia King" .

# Instance of the Cultural Formation for the Ethnicity Context for Sophia King

<http://orlando.cambridge.org/public/svPeople?formname=r&person_id=kingso&heading=c>
    a cwrc:CulturalFormationContext ;
    rdfs:label "Gender Context for Sophia King"@en ;
    oa:hasBody cwrc:woman ;
    oa:hasTarget <http://www.cwrc.ca/cwrcdata/SophiaKing> ;
    prov:derivedFrom <http://www.cwrc.ca/cwrcdata/sophiaKing_Main_Document> .

<http://www.cwrc.ca/cwrcdata/KingCulturalFormation1>
    a cwrc:CulturalFormationContext ;
    rdfs:label "Cultural Formation Context for Sophia King"@en ;
    oa:hasBody cwrc:indigent ;
    oa:hasBody cwrc:gentry ;
    oa:hasBody cwrc:professional ;
    oa:hasBody cwrc:portugal ;
    oa:hasBody cwrc:jewishEthnicity ;
    oa:hasBody cwrc:judaism ;
    oa:hasBody cwrc:radical ;
    oa:hasBody cwrc:england ;
    oa:hasTarget <http://www.cwrc.ca/cwrcdata/SophiaKing> ;
    prov:derivedFrom <http://www.cwrc.ca/cwrcdata/sophiaKing1> .

<http://www.cwrc.ca/cwrcdata/sophiaKing_Main_Document>
    a foaf:Document;
    rdfs:label "Orlando Entry on Sophia King"@en ;
    dcterms:creator cwrc:originalOrlandoAuthor .

# ANNA LEONOWENS
<http://www.cwrc.ca/cwrcdata/AnnaLeonowens>
    cwrc:hasGender cwrc:woman ;
    cwrc:hasReligion cwrc:buddhism, cwrc:presbyterianism, cwrc:hinduism ;
    cwrc:hasNationalHeritage cwrc:welsh ;
    cwrc:hasNationality cwrc:english ;
    cwrc:hasRaceColour cwrc:eurasian ;
    cwrc:hasRaceColourSelfReported cwrc:white ;
    a foaf:Person ;
    foaf:name "Anna Leonowens" .

<http://orlando.cambridge.org/public/svPeople?formname=r&person_id=leonan&heading=c>
    a cwrc:CulturalFormationContext ;
    rdfs:label "Gender Context for Anna Leonowens"@en ;
    oa:hasBody cwrc:woman ;
    oa:hasTarget <http://www.cwrc.ca/cwrcdata/AnnaLeonowens> ;
    prov:derivedFrom <http://www.cwrc.ca/cwrcdata/annaleonowens_Main_Document> .

<http://www.cwrc.ca/cwrcdata/LEONOWENSReligionContext1>
    a cwrc:ReligionContext ;
    rdfs:label "Religion Context for Anna Leonowens"@en ;
    oa:hasBody cwrc:presbyterianism ;
    oa:hasBody cwrc:hinduism ;
    oa:hasBody cwrc:buddhist ;
	oa:hasTarget <http://www.cwrc.ca/cwrcdata/AnnaLeonowens> ;
    prov:derivedFrom <http://www.cwrc.ca/cwrcdata/annaLeonowens1> .

<http://www.cwrc.ca/cwrcdata/LEONOWENSReligionContext2>
    a cwrc:ReligionContext ;
    rdfs:label "Religion Context for Anna Leonowens"@en ;
    oa:hasBody cwrc:buddhist ;
    oa:hasTarget <http://www.cwrc.ca/cwrcdata/AnnaLeonowens> ;
    prov:derivedFrom <http://www.cwrc.ca/cwrcdata/annaleonowens2> .

<http://www.cwrc.ca/cwrcdata/LEONOWENSRaceEthnicityContext1>
    a cwrc:NationalityContext ;
    rdfs:label "Race Ethnicity Context for Anna Leonowens"@en ;
    oa:hasBody cwrc:wales ;
    oa:hasBody cwrc:england ;
    oa:hasBody cwrc:eurasianRace ;
    oa:hasBody cwrc:whiteEthnicity ;
    oa:hasTarget <http://www.cwrc.ca/cwrcdata/AnnaLeonowens> ;
    prov:derivedFrom <http://www.cwrc.ca/cwrcdata/annaleonowens1> .

<http://www.cwrc.ca/cwrcdata/annaLeonowens_Main_Document>
    a foaf:Document;
    rdfs:label "Orlando Markup on Anna Leonowens"@en ;
    dcterms:creator cwrc:originalOrlandoAuthor .

# CHARLOTTE DACRE
<http://www.cwrc.ca/cwrcdata/CharlotteDacre>
    cwrc:hasGender cwrc:woman ;
    cwrc:hasGeogHeritage cwrc:jewishGeographicalHeritage, cwrc:portugal, cwrc:england, cwrc:middlesex, cwrc:london ;
    cwrc:hasEthnicity cwrc:jewishEthnicity ;
    cwrc:hasSocialClass cwrc:entrepreneurial-industrialist, cwrc:gentry, cwrc:indigent;
    cwrc:hasReligion cwrc:anglicanchurch, cwrc:judaism ;
    a foaf:Person ;
    foaf:name "Charlotte Dacre" .

<http://orlando.cambridge.org/public/svPeople?person_id=dacrch>
    a cwrc:CulturalFormationContext ;
    rdfs:label "Gender Context for Charlotte Dacre"@en ;
    oa:hasBody cwrc:woman ;
    oa:hasTarget <http://www.cwrc.ca/cwrcdata/CharlotteDacre> ;
    prov:derivedFrom <http://www.cwrc.ca/cwrcdata/charlotteDacre_Main_Document> .

<http://www.cwrc.ca/cwrcdata/DACRECulturalFormation1>
    a cwrc:CulturalFormationContext ;
    rdfs:label "Cultural Formation Context for Charlotte Dacre"@en ;
    oa:hasBody cwrc:jewishGeographicalHeritage ;
    oa:hasBody cwrc:portugal ;
    oa:hasBody cwrc:england ;
    oa:hasBody cwrc:middlesex ;
    oa:hasBody cwrc:london ;
    oa:hasBody cwrc:jewishEthnicity ;
    oa:hasBody cwrc:entrepreneurial-industrialist ;
    oa:hasBody cwrc:gentry ;
    oa:hasBody cwrc:indigent ;
    oa:hasTarget <http://www.cwrc.ca/cwrcdata/CharlotteDacre> ;
    prov:derivedFrom <http://www.cwrc.ca/cwrcdata/charlotteDacre1> .
    
<http://www.cwrc.ca/cwrcdata/DACREReligionContext1>
    a cwrc:ReligionContext ;
    rdfs:label "Religion Context for Charlotte Dacre"@en ;
    oa:hasBody cwrc:anglicanChurch ;
    oa:hasBody cwrc:judaism ;
    oa:hasTarget <http://www.cwrc.ca/cwrcdata/CharlotteDacre> ;
    prov:derivedFrom <http://www.cwrc.ca/cwrcdata/charlotteDacre1> .

<http://www.cwrc.ca/cwrcdata/DACREReligionContext2>
    a cwrc:ReligionContext ;
    rdfs:label "Religion Context for Charlotte Dacre"@en ;
    oa:hasBody cwrc:anglicanChurch ;
    oa:hasBody cwrc:judaism ;
    oa:hasTarget <http://www.cwrc.ca/cwrcdata/CharlotteDacre> ;
    prov:derivedFrom <http://www.cwrc.ca/cwrcdata/charlotteDacre2> .

<http://www.cwrc.ca/cwrcdata/charlotteDacre_Main_Document>
    a foaf:Document;
    rdfs:label "Orlando Markup on Charlotte Dacre"@en ;
    dcterms:creator cwrc:originalOrlandoAuthor .

#ELIZABETH SARAH GOOCH
<http://www.cwrc.ca/cwrcdata/ElizabethSarahGooch>
    cwrc:hasGender cwrc:genderWomanFemale ;
    cwrc:hasEthnicityHeritage cwrc:jewishEthnicity ;
    cwrc:hasNationalityHeritage cwrc:portugal ;
    cwrc:hasReligionSelfReported cwrc:anglicanChurch ;
    cwrc:hasSocialClassSelfReported cwrc:gentry ;
    a foaf:Person ;
    foaf:name "Elizabeth Sarah Gooch" .

<http://orlando.cambridge.org/public/svPeople?person_id=goocel>
    a cwrc:CulturalFormationContext ;
    rdfs:label "Gender Context for Elizabeth Sarah Gooch"@en ;
    oa:hasBody cwrc:woman ;
    oa:hasTarget <http://www.cwrc.ca/cwrcdata/ElizabethSarahGooch> ;
    prov:derivedFrom <http://www.cwrc.ca/cwrcdata/elizabethSarahGooch_Main_Document> .

<http://www.cwrc.ca/cwrcdata/GOOCHCulturalFormation1>
    a cwrc:CulturalFormationContext ;
    rdfs:label "Cultural Formation for Elizabeth Sarah Gooch"@en ;
    oa:hasBody cwrc:jewishEthnicity ;
    oa:hasBody cwrc:portugal ;
    oa:hasBody cwrc:anglicanChurch ;
    oa:hasBody cwrc:gentry ;
    oa:hasTarget <http://www.cwrc.ca/cwrcdata/ElizabethSarahGooch> ;
    prov:derivedFrom <http://www.cwrc.ca/cwrcdata/elizabethSarahGooch1> .

<http://www.cwrc.ca/cwrcdata/ElizabethSarahGoochFather>
    a foaf:Person ;
    rdfs:label "Father of Elizabeth Sarah Gooch"@en ;
    cwrc:fatherOf <http://www.cwrc.ca/cwrcdata/ElizabethSarahGooch>;
    cwrc:hasReligion cwrc:judaism ;
    prov:derivedFrom <http://www.cwrc.ca/cwrcdata/elizabethSarahGooch1> .

<http://www.cwrc.ca/cwrcdata/elizabethSarahGooch_Main_Document>
    a foaf:Document;
    rdfs:label "Orlando Markup on Elizabeth Sarah Gooch"@en ;
    dcterms:creator cwrc:originalOrlandoAuthor .
 
# GRACE AGUILAR
<http://www.cwrc.ca/cwrcdata/GraceAguilar>
    cwrc:hasGender cwrc:genderWomanFemale ;
    cwrc:hasRaceColourHeritage cwrc:whiteRaceColour ;
    cwrc:hasEthnicity cwrc:jewishEthnicity ;
    cwrc:hasSocialClass cwrc:entrepreneurial-industrialist, cwrc:middleClass ;
    cwrc:hasNationalHeritage cwrc:portugal, cwrc:spain ;
    cwrc:hasNationalitySelfReported cwrc:englishNationalIdentity, cwrc:jewishNationalIdentity ;
    cwrc:hasReligion cwrc:protestantism, cwrc:catholicism ;
    cwrc:hasReligionSelfReported cwrc:judaism ;
    cwrc:hasPoliticalAffiliation cwrc:proto-zionistPoliticalAffiliation ;
    cwrc:hasReligion cwrc:protestantism, cwrc:catholicism, cwrc:christianity, cwrc:judaism ;
    a foaf:Person ;
    owl:sameAs <http://viaf.org/viaf/7628015> ;
    foaf:name "Grace Aguilar" .

<http://orlando.cambridge.org/public/svPeople?person_id=aguigr>
    a cwrc:CulturalFormationContext ;
    rdfs:label "Gender Context for Grace Aguilar"@en ;
    oa:hasBody cwrc:woman ;
    oa:hasTarget <http://www.cwrc.ca/cwrcdata/GraceAguilar> ;
    prov:derivedFrom <http://www.cwrc.ca/cwrcdata/graceAguilar_Main_Document> .
    
<http://www.cwrc.ca/cwrcdata/AGUILARCulturalFormation1>
    a cwrc:CulturalFormationContext ;
    rdfs:label "Cultural Formation Context for Grace Aguilar"@en ;
    oa:hasBody cwrc:whiteRaceColour ;
    oa:hasBody cwrc:entrepreneurial-industrialist ;
    oa:hasBody cwrc:middleClass ;
    oa:hasBody cwrc:portugal ;
    oa:hasBody cwrc:spain ;
    oa:hasBody cwrc:jewishEthnicity ;
    oa:hasBody cwrc:englishNationality ;
    oa:hasBody cwrc:jewishNationality ;
    oa:hasTarget <http://www.cwrc.ca/cwrcdata/GraceAguilar> ;
    prov:derivedFrom <http://www.cwrc.ca/cwrcdata/graceAguilar1> .
    
<http://www.cwrc.ca/cwrcdata/AGUILARCulturalFormation2>
    a cwrc:CulturalFormationContext ;
    rdfs:label "Cultural Formation Context for Grace Aguilar"@en ;
    oa:hasBody cwrc:englishNationality ;
	oa:hasBody cwrc:jewishNationality ;
    oa:hasTarget <http://www.cwrc.ca/cwrcdata/GraceAguilar> ;
    prov:derivedFrom <http://www.cwrc.ca/cwrcdata/graceAguilar2> .

<http://www.cwrc.ca/cwrcdata/AGUILARReligionContext1>
    a cwrc:ReligionContext ;
    rdfs:label "Religion Context for Grace Aguilar"@en ;
    oa:hasBody cwrc:judaism ;
    oa:hasBody cwrc:protestantism ;
    oa:hasBody cwrc:catholicism ;
    oa:hasBody cwrc:proto-zionist ;
    oa:hasTarget <http://www.cwrc.ca/cwrcdata/GraceAguilar> ;
    prov:derivedFrom <http://www.cwrc.ca/cwrcdata/graceAguilar1> .

<http://www.cwrc.ca/cwrcdata/AGUILARReligionContext2>
    a cwrc:ReligionContext ;
    rdfs:label "Religion Context for Grace Aguilar"@en ;
    oa:hasBody cwrc:protestantism ;
    oa:hasBody cwrc:catholicism ;
    oa:hasBody cwrc:christianity ;
    oa:hasBody cwrc:judaism ;
    oa:hasTarget <http://www.cwrc.ca/cwrcdata/GraceAguilar> ;
    prov:derivedFrom <http://www.cwrc.ca/cwrcdata/graceAguilar2> .
    
<http://www.cwrc.ca/cwrcdata/EmanuelAguilar>
    a foaf:Person;
    foaf:name "Emanuel Aguilar" ;
    cwrc:fatherOf <http://www.cwrc.ca/cwrcdata/GraceAguilar> ;
    cwrc:hasNationalHeritage cwrc:portugal ;
    prov:derivedFrom <http://www.cwrc.ca/cwrcdata/graceAguilar1> .

<http://www.cwrc.ca/cwrcdata/SarahDiasFernandesAguilar>
    a foaf:Person ;
    foaf:name "Sarah (Dias Fernandes) Aguilar" ;
    cwrc:motherOf <http://www.cwrc.ca/cwrcdata/GraceAguilar> ;
    cwrc:hasNationalHeritage cwrc:spain ;
    prov:derivedFrom <http://www.cwrc.ca/cwrcdata/graceAguilar1> .

<http://www.cwrc.ca/cwrcdata/graceAguilar_Main_Document>
    a foaf:Document;
    rdfs:label "Orlando Markup on Grace Aguilar"@en ;
    dcterms:creator cwrc:originalOrlandoAuthor .
 
# AMY LEVY
<http://www.cwrc.ca/cwrcdata/AmyLevy>
    cwrc:hasGender cwrc:woman ;
    cwrc:hasSocialClass cwrc:upper-middleClass ;
    cwrc:hasNationalHeritageSelfReported cwrc:english ;
    cwrc:hasReligionSelfReported cwrc:judaism ;
    cwrc:hasReligion cwrc:anglicanism, cwrc:christianity ;
    cwrc:hasSexualIdentity cwrc:lesbian ;
    cwrc:hasEthnicity cwrc:jewishEthnicity ;
    a foaf:Person ;
    owl:sameAs <http://viaf.org/viaf/7628015> ;
    foaf:name "Amy Levy" .

<http://orlando.cambridge.org/public/svPeople?person_id=levyam>
    a cwrc:CulturalFormationContext ;
    rdfs:label "Gender Context for Amy Levy"@en ;
    oa:hasBody cwrc:woman ;
    oa:hasTarget cwrc:AmyLevy ;
    prov:derivedFrom <http://www.cwrc.ca/cwrcdata/amyLevy_Main_Document> .

<http://www.cwrc.ca/cwrcdata/LEVYCulturalFormation1>
    a cwrc:CulturalFormationContext ;
    rdfs:label "Cultural Formation Context for Amy Levy"@en ;
    oa:hasBody cwrc:upper-middleClass ;
    oa:hasBody cwrc:englishNationality ;
    oa:hasBody cwrc:judaism ;
    oa:hasTarget <http://www.cwrc.ca/cwrcdata/AmyLevy> ;
    prov:derivedFrom <http://www.cwrc.ca/cwrcdata/amyLevy1> .

<http://www.cwrc.ca/cwrcdata/LEVYCulturalFormation2>
    a cwrc:CulturalFormationContext ;
    rdfs:label "Cultural Formation Context for Amy Levy"@en ;
    oa:hasBody cwrc:lesbian ;
    oa:hasTarget <http://www.cwrc.ca/cwrcdata/AmyLevy> ;
    prov:derivedFrom <http://www.cwrc.ca/cwrcdata/amyLevy2> .

<http://www.cwrc.ca/cwrcdata/LEVYRaceEthnicityContext3>
    a cwrc:CulturalFormationContext ;
    rdfs:label "Race/Ethnicity Context for Amy Levy"@en ;
    oa:hasBody cwrc:jewishEthnicity ;
    oa:hasTarget <http://www.cwrc.ca/cwrcdata/AmyLevy> ;
    prov:derivedFrom <http://www.cwrc.ca/cwrcdata/amyLevy3> .
    
<http://www.cwrc.ca/cwrcdata/LEVYReligionContext1>
    a cwrc:ReligionContext ;
    rdfs:label "Religion Context for Amy Levy"@en ;
    oa:hasBody cwrc:judaism ;
    oa:hasBody cwrc:anglicanism ;
    oa:hasBody cwrc:christianity ;
    oa:hasTarget <http://www.cwrc.ca/cwrcdata/AmyLevy> ;
    prov:derivedFrom <http://www.cwrc.ca/cwrcdata/amyLevy1> .
    
<http://www.cwrc.ca/cwrcdata/LEVYReligionContext4>
    a cwrc:ReligionContext ;
    rdfs:label "Religion Context for Amy Levy"@en ;
    oa:hasBody cwrc:judaism ;
    oa:hasTarget <http://www.cwrc.ca/cwrcdata/AmyLevy> ;
    prov:derivedFrom <http://www.cwrc.ca/cwrcdata/amyLevy4> .
    
<http://www.cwrc.ca/cwrcdata/amyLevy_Main_Document>
    a foaf:Document;
    rdfs:label "Orlando Markup on Amy Levy"@en ;
    dcterms:creator cwrc:originalOrlandoAuthor .
	     
# CHARLOTTE MONTEFIORE
<http://www.cwrc.ca/cwrcdata/CharlotteMontefiore>
    cwrc:hasGender cwrc:woman ;
    cwrc:hasRaceColour cwrc:whiteRaceColour ;
    cwrc:hasReligionSelfReported cwrc:judaism ;
    cwrc:hasSocialClass cwrc:entrepreneurial-industrialist ;
    cwrc:hasNationalHeritage cwrc:italian ;
    a foaf:Person ;
    foaf:name "Charlotte Montefiore" .

<http://orlando.cambridge.org/public/svPeople?person_id=montc2>
    a cwrc:CulturalFormationContext ;
    rdfs:label "Gender Context for Charlotte Montefiore"@en ;
    oa:hasBody cwrc:woman ;
    oa:hasTarget <http://www.cwrc.ca/cwrcdata/CharlotteMontefiore> ;
    prov:derivedFrom <http://www.cwrc.ca/cwrcdata/charlotteMontefiore_Main_Document> .

<http://www.cwrc.ca/cwrcdata/MONTEFIORECulturalFormation1>
    a cwrc:CulturalFormationContext ;
    rdfs:label "Cultural Formation Context for Charlotte Montefiore"@en ;
    oa:hasBody cwrc:white ;
    oa:hasBody cwrc:judaism ;
    oa:hasBody cwrc:entrepreneurial-industrialist;
    oa:hasBody cwrc:italian ;
    oa:hasTarget <http://www.cwrc.ca/cwrcdata/CharlotteMontefiore> ;
    prov:derivedFrom <http://www.cwrc.ca/cwrcdata/charlotteMontefiore1> .

cwrc:CharlotteMontefioreFather
    a foaf:Person ;
    foaf:name "Abraham Montefiore" ;
    cwrc:fatherOf <http://www.cwrc.ca/cwrcdata/CharlotteMontefiore> ;
    cwrc:hasNationalHeritage cwrc:italian ;
    prov:derivedFrom <http://www.cwrc.ca/cwrcdata/charlotteMontefiore1> .

<http://www.cwrc.ca/cwrcdata/charlotteMontefiore_Main_Document>
    a foaf:Document;
    rdfs:label "Orlando Markup on Charlotte Montefiore"@en ;
    dcterms:creator cwrc:originalOrlandoAuthor .

# JULIA FRANKAU
<http://www.cwrc.ca/cwrcdata/JuliaFrankau>
    cwrc:hasGender cwrc:genderWomanFemale ;
    cwrc:hasEthnicitySelfReported cwrc:jewish ;
    cwrc:hasReligionSelfReported cwrc:judaism ;
    a foaf:Person ;
    foaf:name "Julia Frankau" .

<http://orlando.cambridge.org/public/svPeople?person_id=franju>
    a cwrc:CulturalFormationContext ;
    rdfs:label "Gender Context for Julia Frankau"@en ;
    oa:hasBody cwrc:woman ;
    oa:hasTarget <http://www.cwrc.ca/cwrcdata/JuliaFrankau> ;
    prov:derivedFrom <http://www.cwrc.ca/cwrcdata/juliaFrankau_Main_Document> .

<http://www.cwrc.ca/cwrcdata/FRANKAUEReligionContext1>
    a cwrc:ReligionContext ;
    rdfs:label "Religion Context for Julia Frankau"@en ;
    oa:hasBody cwrc:jewishEthnicity ;
    oa:hasBody cwrc:judaism ;
    oa:hasTarget <http://www.cwrc.ca/cwrcdata/JuliaFrankau> ;
    prov:derivedFrom <http://www.cwrc.ca/cwrcdata/juliaFrankau1> .

<http://www.cwrc.ca/cwrcdata/juliaFrankau_Main_Document>
    a foaf:Document;
    rdfs:label "Orlando Markup on Julia Frankau"@en ;
    dcterms:creator cwrc:originalOrlandoAuthor .

# VITA SACKVILLE-WEST
<http://www.cwrc.ca/cwrcdata/VitaSackvilleWest>
    cwrc:hasGender cwrc:woman ;
    cwrc:hasSocialClass cwrc:nobility ;
    cwrc:hasNationalHeritageSelfReported cwrc:spanish ;
    cwrc:hasEthnicitySelfReported cwrc:gipsy ;
    cwrc:hasNationalHeritageSelfReported cwrc:english ;
    cwrc:hasSexualitySelfReported cwrc:bisexual ;
    cwrc:hasSexualitySelfReported cwrc:lesbian ;
    a foaf:Person ;
    foaf:name "Vita Sackville-West" .
    
<http://orlando.cambridge.org/public/svPeople?person_id=sackvi>
    a cwrc:CulturalFormationContext ;
    rdfs:label "Gender Context for Vita Sackville West"@en ;
    oa:hasBody cwrc:woman ;
    oa:hasTarget <http://www.cwrc.ca/cwrcdata/VitaSackvilleWest> ;
    prov:derivedFrom <http://www.cwrc.ca/cwrcdata/vitaSackvilleWest_Main_Document> .
    
<http://www.cwrc.ca/cwrcdata/SACKVILLEWESTClassIssueContext1>
    a cwrc:ClassIssueContext ;
    rdfs:label "Class Issue Context for Vita Sackville-West"@en ;
    oa:hasBody cwrc:nobility ;
    oa:hasTarget <http://www.cwrc.ca/cwrcdata/VitaSackvilleWest> ;
    prov:derivedFrom <http://www.cwrc.ca/cwrcdata/SackvilleWest1> .
       
<http://www.cwrc.ca/cwrcdata/SACKVILLEWESTRaceEthnicityContext2>
    a cwrc:RaceEthnicityContext ;
    rdfs:label "Race Ethnicity Context for Vita Sackville-West"@en ;
    oa:hasBody cwrc:spanish ;
    oa:hasBody cwrc:english ;
    oa:hasBody cwrc:gipsy ;
    oa:hasTarget <http://www.cwrc.ca/cwrcdata/VitaSackvilleWest> ;
    prov:derivedFrom <http://www.cwrc.ca/cwrcdata/SackvilleWest2> .
    
<http://www.cwrc.ca/cwrcdata/SACKVILLEWESTSexualityContext3>
    a cwrc:SexualityContext ;
    rdfs:label "Sexuality Context for Vita Sackville-West"@en ;
    oa:hasBody cwrc:bisexual ;
    oa:hasBody cwrc:lesbian ;
    oa:hasTarget <http://www.cwrc.ca/cwrcdata/VitaSackvilleWest> ;
    prov:derivedFrom <http://www.cwrc.ca/cwrcdata/SackvilleWest3> .
    
<http://www.cwrc.ca/cwrcdata/JosefaDuran>
    a foaf:Person ;
    foaf:name "Josefa Duran (Pepita)" ;
    cwrc:grandmotherOf <http://www.cwrc.ca/cwrcdata/VitaSackvilleWest> ;
    cwrc:hasNationalIdentity cwrc:spanish ;
    prov:derivedFrom <http://www.cwrc.ca/cwrcdata/SackvilleWest2> .

<http://www.cwrc.ca/cwrcdata/JosefaDuran>
    a foaf:Person ;
    foaf:name "Josefa Duran (Pepita)" ;
    cwrc:grandmotherOf <http://www.cwrc.ca/cwrcdata/VitaSackvilleWest> ;
    cwrc:hasEthnicity cwrc:gipsy ;
    prov:derivedFrom <http://www.cwrc.ca/cwrcdata/SackvilleWest2> .

<http://www.cwrc.ca/cwrcdata/VitaSackvilleWestGrandfather>
    a foaf:Person ;
    foaf:name "Vita Sackville West's grandfather" ;
    cwrc:grandfatherOf <http://www.cwrc.ca/cwrcdata/VitaSackvilleWest> ;
    prov:derivedFrom <http://www.cwrc.ca/cwrcdata/SackvilleWest2> .

# VIRGINIA WOOLF
<http://www.cwrc.ca/cwrcdata/VirginiaWoolf>
    cwrc:hasGender cwrc:woman ;
    cwrc:hasSocialRankSelfReported cwrc:professional ;
    cwrc:hasReligion cwrc:societyOfFriends, cwrc:quakers, cwrc:agnosticism ;
# add cwrc:evangelical once in dataset KM
    cwrc:hasNationality cwrc:englishNationality ;
    cwrc:hasSexualitySelfReported cwrc:bisexual ;
    cwrc:alludesExplicitlyTo <http://www.cwrc.ca/cwrcdata/ElizabethI> ;
    cwrc:respondsTo <http://www.cwrc.ca/cwrcdata/EmbassyLetters> ;
    a foaf:Person ;
    foaf:name "Virginia Woolf" .
    
<http://orlando.cambridge.org/public/svPeople?person_id=woolvi>
    a cwrc:CulturalFormationContext ;
    rdfs:label "Gender Context for Virginia Woolf"@en ;
    oa:hasBody cwrc:woman ;
    oa:hasTarget <http://www.cwrc.ca/cwrcdata/VirginiaWoolf> ;
    prov:derivedFrom <http://www.cwrc.ca/cwrcdata/virginiaWoolf_Main_Document> .
    
<http://www.cwrc.ca/cwrcdata/WOOLFSocialRankSelfReportedProfessional>
    a cwrc:SocialRankContext ;
    rdfs:label "Social Class Context for Virginia Woolf"@en ;
    oa:hasBody cwrc:professional ;
    oa:hasTarget <http://www.cwrc.ca/cwrcdata/VirginiaWoolf> ;
    prov:derivedFrom <http://www.cwrc.ca/cwrcdata/virginiaWoolf1> .

<http://www.cwrc.ca/cwrcdata/WOOLFSexualityContext>
    a cwrc:SexualityContext ;
    rdfs:label "Sexuality Context for Virginia Woolf"@en ;
    oa:hasBody cwrc:bisexual ;
    oa:hasTarget <http://www.cwrc.ca/cwrcdata/VirginiaWoolf> ;
    prov:derivedFrom <http://www.cwrc.ca/cwrcdata/virginiaWoolf1> .
    
<http://www.cwrc.ca/cwrcdata/WOOLFNationalityIssueContext>
    a cwrc:NationalityContext ;
    rdfs:label "Nationality Issue Context for Virginia Woolf"@en ;
    oa:hasBody cwrc:englishNationality ;
    oa:hasTarget <http://www.cwrc.ca/cwrcdata/VirginiaWoolf> ;
    prov:derivedFrom <http://www.cwrc.ca/cwrcdata/virginiaWoolf1> .    

<http://www.cwrc.ca/cwrcdata/virginia_Woolf_Main_Document>
    a foaf:Document;
    rdfs:label "Orlando Markup on Virginia Woolf"@en ;
    dcterms:creator cwrc:originalOrlandoAuthor .
    
 #Works go here   

<http://www.cwrc.ca/cwrcdata/Orlando>
   a frbr:Work, bibo:Book;
   schema:workExample <http://www.cwrc.ca/cwrcdata/OrlandoExpressionOrlando2006> ;
   cwrc:hasGenre cwrc:genreNovel ;
   loc:pub <http://www.cwrc.ca/cwrcdata/HogarthPress> ;
   cwrc:alludesExplicitlyTo <http://www.cwrc.ca/cwrcdata/AlexanderPope> ;
   cwrc:alludesExplicitlyTo <http://www.cwrc.ca/cwrcdata/ElizabethI> ;
   cwrc:relatesByMaterialFeaturesTo <http://www.cwrc.ca/cwrcdata/VitaSackvilleWest> ;
   cwrc:relatesByMaterialFeaturesTo <http://www.cwrc.ca/cwrcdata/KnoleHouse> ;   
   cwrc:contestsGenre cwrc:genreBiography ;
   cwrc:contestsGenre cwrc:genreFiction ;
   cwrc:contestsGenre cwrc:genreMockforms ;
   cwrc:contestsGenre cwrc:genreHistory ;
   cwrc:relatesByCirculationTo <http://www.cwrc.ca/cwrcdata/ToTheLighthouse> ;
   cwrc:relatesByCirculationTo <http://www.cwrc.ca/cwrcdata/HarcourtBrace> ;
   cwrc:relatesByCirculationTo <http://www.cwrc.ca/cwrcdata/RichardKennedy> ;
   cwrc:relatesByManuscriptTo <http://www.cwrc.ca/cwrcdata/VitaSackvilleWest> ;
   cwrc:relatesByArchiveTo <http://www.cwrc.ca/cwrcdata/KnoleHouse> ;
   cwrc:hasSpatialSetting <http://www.cwrc.ca/cwrcdata/Constantinople> ;
   cwrc:respondsTo <http://www.cwrc.ca/cwrcdata/LadyMaryWortleyMontagu> ;
   cwrc:relatesEroticallyTo <http://www.cwrc.ca/cwrcdata/VirginiaWoolf> ;
   cwrc:influences <http://www.cwrc.ca/cwrcdata/ALadyOfQuality> ;
   cwrc:relatesPoliticallyTo <http://www.cwrc.ca/cwrcdata/VirginiaWoolf> ;
   cwrc:relatesTextuallyTo <http://www.cwrc.ca/cwrcdata/HermeticDefinition> ;
   cwrc:relatesEroticallyTo <http://www.cwrc.ca/cwrcdata/VitaSackvilleWest> ;
   cwrc:relatesByReceptionTo <http://www.cwrc.ca/cwrcdata/VitaSackvilleWest> ;
   cwrc:relatesByEducationTo <http://www.cwrc.ca/cwrcdata/HelenDunmore> ;
   dcterms:title "Orlando" ;
   rdfs:label "Orlando (Work)"@en ;
   dcterms:creator <http://www.cwrc.ca/cwrcdata/VirginiaWoolf> .
   
<http://www.cwrc.ca/cwrcdata/ToTheLighthouse>
   a frbr:Work, bibo:Book;
   schema:workExample <http://www.cwrc.ca/cwrcdata/ToTheLighthouse>;
   cwrc:hasGenre cwrc:genreNovel ;  
   dcterms:title "To the Lighthouse" ;
   rdfs:label "To the Lighthouse"@en ;
   dcterms:creator <http://www.cwrc.ca/cwrcdata/VirginiaWoolf> .
   
<http://www.cwrc.ca/cwrcdata/EmbassyLetters>   
   a frbr:Work, bibo:Book;
   schema:workExample <http://www.cwrc.ca/cwrcdata/EmbassyLetters>;
   cwrc:hasGenre cwrc:genreLetter ;
   dcterms:creator <http://www.cwrc.ca/cwrcdata/LadyMaryWortleyMontagu> .
   
<http://www.cwrc.ca/cwrcdata/ALadyofQuality>
   a frbr:Work, bibo:Book;
   schema:workExample <http://cwrc.ca/cwrcdata/ALadyofQuality>;
   cwrc:hasGenre cwrc:genreFiction ;
   cwrc:hasGenre cwrc:genreRomance ;
   cwrc:hasGenre cwrc:genreHistorical ;
   rdfs:label "A Lady of Quality"@en ;   
   dcterms:creator <http://www.cwrc.ca/cwrcdata/FrancesHodgsonBurnett> .
   
<http://www.cwrc.ca/cwrcdata/ToldByAnIdiot>
   a frbr:Work, bibo:Book;
   schema:workExample <http://cwrc.ca/cwrcdata/ToldByAnIdiot>;
   cwrc:hasGenre cwrc:genreNovel ;
   rdfs:label "Told by an Idiot"@en ;
   dcterms:creator <http://www.cwrc.ca/cwrcdata/RoseMacaulay> .  

<http://www.cwrc.ca/cwrcdata/HermeticDefinition>
   a frbr:Work, bibo:Book;
   schema:workExample <http://cwrc.ca/cwrcdata/ALadyofQuality>;
   cwrc:hasGenre cwrc:genrePoetry ;
   rdfs:label "HermeticDefinition"@en ;
   dcterms:creator <http://www.cwrc.ca/cwrcdata/HD> .
   
<http://www.cwrc.ca/cwrcdata/KnoleAndTheSackvilles>
   a frbr:Work, bibo:Book;
   schema:workExample <http://cwrc.ca/cwrcdata/KnoleAndTheSackvilles>;
   cwrc:hasGenre cwrc:genreHistory ;
   cwrc:influences <http://www.cwrc.ca/cwrcdata/Orlando> ;
   dcterms:date "1922";
   rdfs:label "Knole and the Sackvilles"@en ;
   dcterms:creator <http://www.cwrc.ca/cwrcdata/VitaSackvilleWest> .

<http://www.cwrc.ca/cwrcdata/TwelveDays>
   a frbr:Work, bibo:Book;
   schema:workExample <http://cwrc.ca/cwrcdata/TwelveDays>;
   cwrc:hasGenre cwrc:genreHistory ;
   cwrc:hasReceptionRelationTo <http://www.cwrc.ca/cwrcdata/Orlando> ;
   dcterms:date "1922";
   rdfs:label "Twelve Days"@en ;
   dcterms:creator <http://www.cwrc.ca/cwrcdata/VitaSackvilleWest> .
   
<http://www.cwrc.ca/cwrcdata/ABoyAtTheHogarthPress>
   a frbr:Work, bibo:Book;
   schema:workExample <http://www.cwrc.ca/cwrcdata/ABoyAtTheHogarthPress>;
   cwrc:hasGenre cwrc:genreNovel ;  
   dcterms:title "A Boy at the Hogarth Press" ;
   rdfs:label "A Boy at the Hogarth Press"@en ;
   dcterms:creator <http://www.cwrc.ca/cwrcdata/RichardKennedy> .   
   
<http://www.cwrc.ca/cwrcdata/OrlandoFilm>
   a frbr:Work, bibo:Film ;
   cwrc:hasGenre cwrc:genreFilm ; 
   owl:sameAs <http://data.linkedmdb.org/resource/film/1592> ;
   dcterms:creator <http://www.cwrc.ca/cwrcdata/SallyPotter> ;  
   cwrc:adapts <http://www.cwrc.ca/cwrcdata/Orlando> ;
   dcterms:title "Orlando (film)" ;
   rdfs:label "Orlando (film)" .
   
 <http://www.cwrc.ca/cwrcdata/OrlandoPlay>
   a frbr:Work, dbpedia:Play;
   cwrc:hasGenre cwrc:genreDrama ; 
   cwrc:adapts <http://www.cwrc.ca/cwrcdata/Orlando> ;
   dcterms:creator <http://www.cwrc.ca/cwrcdata/SarahRuhl> ;
   dcterms:title "Orlando (play)" ;
   rdfs:label "Orlando (play)" .
 
 <http://www.cwrc.ca/cwrcdata/TheDailyChronicle>
   a frbr:Work, bibo:Newspaper;
   schema:workExample <http://www.cwrc.ca/cwrcdata/TheDailyChronicle>;
   cwrc:hasGenre cwrc:genreNewspaper .
 
 <http://www.cwrc.ca/cwrcdata/TheObserver>
   a frbr:Work, bibo:Newspaper;
   schema:workExample <http://www.cwrc.ca/cwrcdata/TheObserver>;
   cwrc:hasGenre cwrc:genreNewspaper .
 
 <http://www.cwrc.ca/cwrcdata/MorningPost>
   a frbr:Work, bibo:Newspaper;
   schema:workExample <http://www.cwrc.ca/cwrcdata/MorningPost>;
   cwrc:respondsTo <http://www.cwrc.ca/cwrcdata/Orlando> ;
   cwrc:hasGenre cwrc:genreNewspaper .

<http://www.cwrc.ca/cwrcdata/OrlandoExpressionOrlando2006>
   a frbr:Expression, bibo:Book;
   schema:workExample <http://www.cwrc.ca/cwrcdata/Orlando>;
   cwrc:hasGenre cwrc:genreNovel ;
   cwrc:hasMaterialFeaturesRelatedto <http://www.cwrc.ca/cwrcdata/TildaSwinton> ;
   loc:pub <http://www.cwrc.ca/cwrcdata/MarinerBooks> ;
   cwrc:hasMaterialFeaturesRelatedto <http://dbpedia.org/resource/Knole_House>, <http://dbpedia.org/resource/Sevenoaks>, <http://sws.geonames.org/3333158>, <http://sws.geonames.org/6269131>;
   bibo:isbn "978-0156031516";
   dcterms:date "2006";
   bibo:edition "1";
   rdfs:label "Orlando (2006)"@en ;
   dcterms:title "Orlando (2006)" ;
   dcterms:creator <http://www.cwrc.ca/cwrcdata/VirginiaWoolf> .

#Organizations go here

<http://www.cwrc.ca/cwrcdata/MarinerBooks>
   a foaf:Organization;
   foaf:name "Mariner Books"@en ;
   rdfs:label "Mariner Books"@en .
   
<http://www.cwrc.ca/cwrcdata/HogarthPress>
   a foaf:Organization;
   foaf:name "HogarthPress"@en ;
   rdfs:label "HogarthPress"@en ;
   owl:sameAs <http://dbpedia.org/resource/Hogarth_Press> .
   
 <http://www.cwrc.ca/cwrcdata/ClassicStageCompany>
    a foaf:Organization;
    foaf:name "Classic Stage Company"@en ;
    rdfs:label "Classic Stage Company"@en . 
    
#People go here    

<http://www.cwrc.ca/cwrcdata/AlexanderPope>
    cwrc:hasGender cwrc:genderManMale ;
    cwrc:hasNationality cwrc:englishNationalIdentity ;
    a foaf:Person ;
    foaf:name "Alexander Pope" .

<http://www.cwrc.ca/cwrcdata/ElizabethI>
    cwrc:hasGender cwrc:genderWomanFemale ;
    cwrc:hasNationality cwrc:englishNationalIdentity ;
    a foaf:Person ;
    foaf:name "Elizabeth I" .
    
<http://www.cwrc.ca/cwrcdata/TildaSwinton>
    owl:sameAs <http://www.viaf.org/viaf/117443790/#Swinton,_Tilda>;
    a foaf:Person ;
    foaf:name "Tilda Swinton" .
   
<http://www.cwrc.ca/cwrcdata/SallyPotter>
    owl:sameAs <http://www.viaf.org/viaf/78760437/#Potter,_Sally>;
    a foaf:Person ;
    foaf:name "Sally Potter" .
   
<http://www.cwrc.ca/cwrcdata/EdwinMorgan>
    owl:sameAs <http://www.viaf.org/viaf/68969203/#Morgan,_Edwin,_1920-2010>;
    cwrc:alludesExplicitlyTo <http://www.cwrc.ca/cwrcdata/VirginiaWoolf> ;
    a foaf:Person ;
    foaf:name "Edwin Morgan" .
  
<http://www.cwrc.ca/cwrcdata/RichardKennedy>
    owl:sameAs <http://www.viaf.org/viaf/52955138/#Kennedy,_Richard,_1910-1989>;
    a foaf:Person ;
    foaf:name "Richard Kennedy" .
    
#<http://www.cwrc.ca/cwrcdata/SirJohnCollingSquire>
#   a foaf:Person ;
#   foaf:name "Sir John Colling Squire" .
    
<http://www.cwrc.ca/cwrcdata/RebeccaWest>
    owl:sameAs <http://viaf.org/viaf/108321467/#West,_Rebecca,_1892-1983>;
    cwrc:respondsTo <http://www.cwrc.ca/cwrcdata/Orlando> ;
    a foaf:Person ;
    foaf:name "Rebecca West" .    
    
<http://www.cwrc.ca/cwrcdata/DHLawrence>
    owl:sameAs <http://viaf.org/viaf/95150359/#Lawrence,_D._H.,_(David_Herbert),_1885-1930>;
    cwrc:respondsTo <http://www.cwrc.ca/cwrcdata/Orlando> ;
    a foaf:Person ;
    foaf:name "D H Lawrence" .    
    
<http://www.cwrc.ca/cwrcdata/AldousHuxley>
    owl:sameAs <http://viaf.org/viaf/71392434/#Huxley,_Aldous,_1894-1963>;
    cwrc:respondsTo <http://www.cwrc.ca/cwrcdata/Orlando> ;
    a foaf:Person ;
    foaf:name "Aldous Huxley" .  
    
<http://www.cwrc.ca/cwrcdata/JeanetteWinterson>
    owl:sameAs <http://viaf.org/viaf/4961254/#Winterson,_Jeanette,_1959->;
    cwrc:respondsTo <http://www.cwrc.ca/cwrcdata/Orlando> ;
    a foaf:Person ;
    foaf:name "Jeanette Winterson" .
    
<http://www.cwrc.ca/cwrcdata/SarahRuhl>
    owl:sameAs <http://viaf.org/viaf/81312438/#Ruhl,_Sarah,_1974->;
    a foaf:Person ;
    foaf:name "Sarah Ruhl" .    

<http://www.cwrc.ca/cwrcdata/LadyMaryWortleyMonatgu>
    owl:sameAs <http://viaf.org/viaf/7394587/#Montagu,_Mary_Wortley,_Lady,_1689-1762>;
    a foaf:Person ;
    foaf:name "Lady Mary Wortley Montagu" .
    
<http://www.cwrc.ca/cwrcdata/FrancesHodgsonBurnett>
    owl:sameAs <http://viaf.org/viaf/27061925/#Burnett,_Frances_Hodgson,_1849-1924>;
    a foaf:Person ;
    foaf:name "Frances Hodgson Burnett" .   

<http://www.cwrc.ca/cwrcdata/RoseMacaulay>
    owl:sameAs <http://viaf.org/viaf/100194559/#Macaulay,_Rose,_1881-1958>;
    a foaf:Person ;
    foaf:name "Rose Macaulay" .        

<http://www.cwrc.ca/cwrcdata/HD>
    owl:sameAs <http://viaf.org/viaf/4925150/#H.D._(Hilda_Doolittle),_1886-1961>;
    a foaf:Person ;
    foaf:name "H D" .        

#snippets go here

<http://www.cwrc.ca/cwrcdata/sophiaKing1>
    rdfs:label """SK's Sephardic Jewish Portuguese birth, her early years in Judaism, and her father's boyhood as a street urchin and his high-profile but scandalous career (associating with political radicals while lending money to socialites and eventually marrying into the English nobility), made her an outsider in English society."""@en ;
a nif:Context, nif:Sentence ;
    dcterms:partOf <http://www.cwrc.ca/cwrcdata/sophiaKing_Main_Document> ;
    prov:createdBy cwrc:originalOrlandoAuthor .

<http://www.cwrc.ca/cwrcdata/annaLeonowens1>
    rdfs:label """Although AL herself, in attempting to adopt an unequivocally English identity, implicitly claimed that she was white, evidence suggests that while
her father was probably Welsh (he had lived in Middlesex) and presumably white, her mother was quite possibly Eurasian. If this is the case then
AL suppressed her mixed-race origins. Anna was multi-lingual and from childhood could speak Hindustani, English and Guzerati (also called 
Gujarati), which was taught to her by her mother. She also became fluent in Sanskrit,French ,Thai , Malay,  Arabic, Persian, Latin and Pali. 
She knew some Russian from her travels. AL was Presbyterian but also studied Hinduism and Buddhism. She believed that she was too good a Christian 
not to be something of a Buddhist, and too good a Buddhist not to be something of a Christian."""@en ;
    a nif:Context, nif:Sentence ;
    dcterms:partOf <http://www.cwrc.ca/cwrcdata/annaleonowens_Main_Document> ;
    prov:createdBy cwrc:originalOrlandoAuthor .

<http://www.cwrc.ca/cwrcdata/annaLeonowens2>
    rdfs:label """AL often visited the Reclining Buddha at the temple Wat Po in Bangkok. Her Thai teacher gave her frequent instruction on Buddha's teachings. Later in
Siamese Harem Life, Anna recalled that she had learned that the prophet's object was not only a religious but a social revolution. A good deal of what
was venerated as religion he found to be merely social usage, for which a Divine sanction was feigned. [Buddha], without hesitation, rejected all of
this . . . . His greatest blow to the old religion, however, was in his explicit repudiation of caste. He offered his religion to all men alike . . . . 
Buddha boldly expounded to the people that, according to their own books, all men were equal."""@en ;
    a nif:Context, nif:Sentence ;
    dcterms:partOf <http://www.cwrc.ca/cwrcdata/annaleonowens_Main_Document> ;
    prov:createdBy cwrc:originalOrlandoAuthor .

<http://www.cwrc.ca/cwrcdata/charlotteDacre1>
    rdfs:label """CD was a teenager when her Jewish parents divorced; presumably she was brought up in Judaism until this event; probably she completed her upbringing as an gentlewoman. She must have been to a greater or lesser extent an outsider in English society, not only because of her Sephardic Jewish Portuguese heritage but because 
of her father's highly visible but anomalous character, as a Londoner but an outsider, an ex-street-child and boxer, author of inflammatory political pamphlets, 
moving in high society and privy to its financial secrets while not himself a member of it."""@en ;
    a nif:Context, nif:Sentence ;
    dcterms:partOf <http://www.cwrc.ca/cwrcdata/charlotteDacre_Main_Document> ;
    prov:createdBy cwrc:originalOrlandoAuthor .

<http://www.cwrc.ca/cwrcdata/charlotteDacre2>
    rdfs:label """The Anglican baptism of CD's children may—perhaps—represent a final severing of her Jewish roots."""@en ;
    a nif:Context, nif:Sentence ;
    dcterms:partOf <http://www.cwrc.ca/cwrcdata/charlotteDacre_Main_Document> ;
    prov:createdBy cwrc:originalOrlandoAuthor .
    
<http://www.cwrc.ca/cwrcdata/elizabethSarahGooch1>    
    rdfs:label """Despite her clear statement of her father's Jewish ethnicity (and his Portuguese national heritage: she calls herself "the daughter of a Portugueze"),
    she was baptised into the Church of England on 4 October in the year of her birth, aged just over three months. As an orphan, the sole heiress to her 
    late father's wealth, she was a privileged outsider in English society, an unconventional version of a conventional literary heroine."""@en ;
    a nif:Context, nif:Sentence ;
    dcterms:partOf <http://www.cwrc.ca/cwrcdata/elizabethSarahGooch_Main_Document> ;
    prov:createdBy cwrc:originalOrlandoAuthor .

<http://www.cwrc.ca/cwrcdata/graceAguilar1>	
	rdfs:label """Both of GA's parents were presumably white and of Jewish descent; her family belonged to the middle class. Her father's family was from Spain and her mother's 
family was from Portugal. GA was English by birth, and she was full of praise for her country as a land of tolerance and freedom: England offers a rest and home 
of perfect freedom to the exile and oppressed . . . . Much of her writing about Jews served to counter the claims of those such as Thomas Carlyle, who argued that
Jews could not be fully loyal to any country except Zion. GA's writings treat in detail the Jewish faith to which she strongly adhered, and she often focuses on
the persecution and prejudice which Jews suffered throughout the nineteenth century, as well as historically. As critic Michael Galchinsky argues, the practices
and culture of crypto-Judaism, whereby Jews evaded the Inquisition by passing for Catholic while retaining their ancestral faith in private, considerably influenced
both the form and content of her work. Despite her intense commitment to improving the standing of her people through her writing, her friend Anna Maria Hall
avers that she and her husband could only with difficulty get GA to speak on religious topics and were quite unacquainted with her religious habits.
	However, her continuing dedication to Judaism, and her identification of herself with her Sephardic Jewish heritage—which she also considered a nationality
—was obvious to those who knew her, and she may have been a proto-Zionist the natural and unaffected eloquence of her words, when referring to the past history 
of the Jews . . . and the positive radiance of her countenance when she spoke of the gathering of the tribes at Jerusalem, could never be forgotten."""@en ;
    a nif:Context, nif:Sentence ;
    dcterms:partOf <http://www.cwrc.ca/cwrcdata/graceAguilar_Main_Document> ;
    prov:createdBy cwrc:originalOrlandoAuthor .
    
<http://www.cwrc.ca/cwrcdata/graceAguilar2>
	rdfs:label """In Devon she developed the religious tolerance that distinguishes her writing and helped her to bridge the gap between the Jewish and Christian literary 
communities. Here she came into contact with provincial English Protestantism, which she distinguished from the intolerant Catholicism that had 
persecuted her family on the Continent. She made Christian friends with whom she discussed religious issues, attended church—she altered the forms of 
praise and prayer where necessary to accord with her own—and came to the conclusion that Christianity and Judaism had much in common in spirit, even
if they diverged in form. She later argued in Sabbath Thoughts that Christianity was the Kingdom of Iron prophesied by Daniel, which would prepare
for the Jewish messiah. Her lack of adequate religious education meant that she frequently had to rely on Christian texts about Judaism. Critic
Beth-Zion Lask Abrahams joins some contemporary critics in calling her a Jewish Protestant; however, others have argued that though she was reformist,
she was a dedicated Jew nonetheless, and above all."""@en ;
    dcterms:partOf <http://www.cwrc.ca/cwrcdata/graceAguilar_Main_Document> ;
    a nif:Context, nif:Sentence ;
    prov:createdBy cwrc:originalOrlandoAuthor .
    
<http://www.cwrc.ca/cwrcdata/amyLevy1>
	rdfs:label """AL was an upper-middle-class Jew from a family which had been English for over a century, though they travelled the world for career purposes
more freely than most English people. They thought of themselves as wholly assimilated, and seem to have practised the Jewish religion only sketchily. They 
occasionally attended the Reform synagogue in Upper Berkeley Street; the children visited Christian churches with their governess."""@en ;
 	a nif:Context, nif:Sentence ;
    dcterms:partOf <http://www.cwrc.ca/cwrcdata/amyLevy_Main_Document> ;
    prov:createdBy cwrc:originalOrlandoAuthor .

<http://www.cwrc.ca/cwrcdata/amyLevy2>
	rdfs:label """AL early developed strong erotic attachments to women. She wrote of these openly, but may or may not have expressed them physically."""@en ;
 	a nif:Context, nif:Sentence ;
    dcterms:partOf <http://www.cwrc.ca/cwrcdata/amyLevy_Main_Document> ;
    prov:createdBy cwrc:originalOrlandoAuthor .

<http://www.cwrc.ca/cwrcdata/amyLevy3>
	rdfs:label """Being Jewish must have posed problems for AL, problems which seem to have been exacerbated by struggles with an internalised anti-semitism. 
She apparently thought of herself as unattractive to a degree quite at odds with the comments of other people; she drew caricatures, both visual and verbal, 
of Jewish people with exaggeratedly stereotyped racial characteristics. After visiting a synagogue in Dresden she wrote, "the German Hebrew makes me feel, as
 a rule, that the Anti-Semitic movement is a most just & virtuous one."""@en ;
 	a nif:Context, nif:Sentence ;
    dcterms:partOf <http://www.cwrc.ca/cwrcdata/amyLevy_Main_Document> ;
    prov:createdBy cwrc:originalOrlandoAuthor .

<http://www.cwrc.ca/cwrcdata/amyLevy4>
    rdfs:label """Her time in Dresden crystallized her mixed feelings about the practice of her religion. Visiting the synagogue (for Yom Kippur) disgusted her: she said that German Jews made her feel anti-semitic."""@en ;
 	a nif:Context, nif:Sentence ;
    dcterms:partOf <http://www.cwrc.ca/cwrcdata/amyLevy_Main_Document> ;
    prov:createdBy cwrc:originalOrlandoAuthor .
    
<http://www.cwrc.ca/cwrcdata/charlotteMontefiore1> 
	rdfs:label """She was born into a presumably white, Jewish family of the financial 'aristocracy'. Her father was of Italian descent. She and her family were 
members of the 'Cousinhood', "that circle of aristocratic Jewish families who held sway over the community's governance, and who were in contact with MPs on 
issues of emancipation."""@en ;
	a nif:Context, nif:Sentence ;
    dcterms:partOf <http://www.cwrc.ca/cwrcdata/charlotteMontefiore_Main_Document> ;
    prov:createdBy cwrc:originalOrlandoAuthor .
    
<http://www.cwrc.ca/cwrcdata/juliaFrankau1> 
	rdfs:label """Her family, in which literary ability was almost the norm, was Jewish in origin, and her parents practised Reformed Judaism. Commentator Linda 
Gertner Zatlin finds in her "acculturation bordering on assimilation," but she remained a practising Jew until her husband's refusal to circumcise their eldest 
son resulted in their expulsion from their Reform synagogue. JF therefore became assimilated through forces beyond her control."""@en ;
	a nif:Context, nif:Sentence ;
    dcterms:partOf <http://www.cwrc.ca/cwrcdata/juliaFrankau_Main_Document> ;
    prov:createdBy cwrc:originalOrlandoAuthor .

<http://www.cwrc.ca/cwrcdata/vitaSackvilleWest1>
	rdfs:label """She was born into the noble Sackville family, one of the oldest-established in England. Her father, the third Baron Sackville, inherited Knole, 
the estate given to Thomas Sackville by Elizabeth I in 1566. Vita herself could not inherit, owing to the "technical fault" of her sex. As well as being an 
aristocrat, she was a snob: she referred constantly to 'bedints' (a family term for the lower classes, or those whose class status did not pass muster), and 
wrote in 1927: "How I hate the proletariat."""@en ;
 	a nif:Context, nif:Sentence ;
    dcterms:partOf <http://www.cwrc.ca/cwrcdata/vitaSackvilleWest_Main_Document> ;
    prov:createdBy cwrc:originalOrlandoAuthor .
    
<http://www.cwrc.ca/cwrcdata/vitaSackvilleWest2>
	rdfs:label """VSW understood her own 'nature' in terms of a duality of blood created by the union between her maternal grandmother, the Spanish 'gipsy' dancer
Pepita (whose biography she wrote), and the Sackville line (through her grandfather Lionel, second Baron Sackville). She saw the Spanish side of her nature as 
passionate and perverse and the English side of her nature as caring and controlled. Many of her works explore this theme of duality."""@en ;
 	a nif:Context, nif:Sentence ;
    dcterms:partOf <http://www.cwrc.ca/cwrcdata/vitaSackvilleWest_Main_Document> ;
    prov:createdBy cwrc:originalOrlandoAuthor .    

<http://www.cwrc.ca/cwrcdata/vitaSackvilleWest3>
	rdfs:label """VSW was bisexual. She explicitly linked her lesbian desires and behaviour to her Spanish ancestry. She had great magnetism and sexual energy: 
people of both sexes fell in love with her and in some cases developed obsessions with her."""@en ;
 	a nif:Context, nif:Sentence ;
    dcterms:partOf <http://www.cwrc.ca/cwrcdata/vitaSackvilleWest_Main_Document> ;
    prov:createdBy cwrc:originalOrlandoAuthor .
    
<http://www.cwrc.ca/cwrcdata/virginiaWoolf1>
    rdfs:label """Woolf, Virginia Woolf's childhood sexual experience was painful, humiliating, and formative, and her adult sexuality has been much discussed 
since publication of "A Sketch of the Past," "22 Hyde Park Gate," and "Old Bloomsbury" in Moments of Being, 1976. She later shared the principled objections of 
her Bloomsbury friends to the Victorian social management of sexuality, which they saw as based on possessiveness, jealousy, and exploitation. Her own erotic 
relationships were with individuals of both sexes."""@en ;
    a nif:Context, nif:Sentence ;
    dcterms:partOf <http://www.cwrc.ca/cwrcdata/virginiaWoolf_Main_Document> ;
    prov:createdBy cwrc:originalOrlandoAuthor .

#ONTOLOGY 

locl:eng
    a owl:Thing .

<http://sparql.cwrc.ca/ontologies/cwrc>
    loc:ctb cwrc:ConstanceCrompton, cwrc:originalOrlandoAuthor ;
    loc:fnd cwrc:sshrc ;
    loc:pdr cwrc:SusanBrown ;
    dcterms:creator cwrc:AbigelLemak, cwrc:AlliyyaMo, cwrc:ColinFaulkner, cwrc:JadePenancier, cwrc:JohnSimpson, cwrc:KimMartin, cwrc:RobWarren, cwrc:SusanBrown ;
    dcterms:date "2017-08-03"^^xsd:date ;
    dcterms:description "L'Ontologie CWRC est l'ontologie du Collaboratoire scientifique des écrits du Canada."@fr, "The CWRC Ontology is the ontology of the Canadian Writing Research Collaboratory."@en ;
    dcterms:publisher cwrc:cwrc ;
    dcterms:rights <http://creativecommons.org/licenses/by-nc/4.0/> ;
    dcterms:subject <http://id.loc.gov/authorities/subjects/sh2009007122>, <http://id.loc.gov/authorities/subjects/sh85013838>, <http://id.loc.gov/authorities/subjects/sh85019388>, <http://id.loc.gov/authorities/subjects/sh85043777>, <http://id.loc.gov/authorities/subjects/sh85077519> ;
    dcterms:title "L'Ontologie CWRC"@fr, "The CWRC Ontology"@en ;
    vann:preferredNamespacePrefix "cwrc" ;
    vann:preferredNamespaceUri "http://sparql.cwrc.ca/ontology/cwrc#" ;
    void:inDataset cwrc:datasetdefinition ;
    a voaf:Vocabulary, owl:Ontology ;
    rdfs:comment "L'Ontologie CWRC est l'ontologie du Collaboratoire scientifique des écrits du Canada."@fr, "The CWRC Ontology is the ontology of the Canadian Writing Research Collaboratory."@en ;
    rdfs:label "L'Ontologie CWRC"@fr, "The CWRC Ontology"@en ;
    owl:priorVersion <http://sparql.cwrc.ca/ontology/cwrc-2017-06-10> ;
    owl:versionInfo "0.99.3" ;
    vs:term_status "Testing"@en ;
    skos:definition "L'Ontologie CWRC est l'ontologie du Collaboratoire scientifique des écrits du Canada."@fr, "The CWRC Ontology is the ontology of the Canadian Writing Research Collaboratory."@en ;
    foaf:logo <http://sparql.cwrc.ca/images/CWRCLogo-Horz-FullColour.png> ;
    foaf:name "L'Ontologie CWRC"@fr, "The CWRC Ontology"@en .

cwrc:AbigelLemak
    a foaf:Person ;
    foaf:name "Abigel Lemak" .

cwrc:Actor
    void:inDataset cwrc:datasetdefinition ;
    a owl:Class, skos:Concept ;
    rdfs:isDefinedBy <http://sparql.cwrc.ca/ontologies/cwrc-2017-08-03> ;
    rdfs:label "actor"@en ;
    owl:sameAs <http://erlangen-crm.org/current/E39.Actor> ;
    skos:definition "A person performing a certain role within an event."@en .

cwrc:Address
    void:inDataset cwrc:datasetdefinition ;
    a owl:Class, skos:Concept ;
    rdfs:isDefinedBy <http://sparql.cwrc.ca/ontologies/cwrc-2017-08-03> ;
    rdfs:label "address"@en, "adresse"@fr ;
    rdfs:subClassOf cwrc:Place ;
    owl:sameAs <http://schema.org/PostalAddress> ;
    skos:definition "A mailling or street address."@en, "The postal address is the equivalent of a schema.org address and inherits all of the data from that vocabulary to markup a modern postal address."@en, "Une adresse postale ou de rue."@fr .

cwrc:AlliyyaMo
    a foaf:Person ;
    foaf:name "Alliyya Mo" .

cwrc:Androgynous
    void:inDataset cwrc:datasetdefinition ;
    a owl:Class, skos:Concept ;
    rdfs:isDefinedBy <http://sparql.cwrc.ca/ontologies/cwrc-2017-08-03> ;
    rdfs:label "androgyne"@fr, "androgynous"@en .

cwrc:ColinFaulkner
    a foaf:Person ;
    foaf:name "Colin Faulkner" .

cwrc:ConstanceCrompton
    a foaf:Person ;
    foaf:name "Constance Crompton" .

cwrc:Context
    void:inDataset cwrc:datasetdefinition ;
    a owl:Class, skos:Concept, oa:Annotation ;
    rdfs:isDefinedBy <http://sparql.cwrc.ca/ontologies/cwrc-2017-08-03> ;
    rdfs:label "context"@en, "contexte"@fr ;
    skos:definition ""@fr, "A context relates.... "@en .

cwrc:CulturalForm
    void:inDataset cwrc:datasetdefinition ;
    a owl:Class, skos:Concept ;
    rdfs:isDefinedBy <http://sparql.cwrc.ca/ontologies/cwrc-2017-08-03> ;
    rdfs:label "cultural form"@en, "forme culturelle"@fr ;
    skos:definition ""@fr, "Cultural forms refers to the processes of lived social subjectivities of people and is often combined with predicates indicating the identity positions as they relate to the following discursive constructions of Class, Religion, Ethnicity, Gender, GeographicalHeritage, LinguisticAbility, NationalHeritage, NationalIdentity, PoliticalAffiliation, RaceColour, Sexuality. These categories are not understood as transhistorical or isolated categories. Rather, they facilitate analysis of how such situationally contingent, changing, and negotiated labels are assigned to or adopted by a particular individual. The tensions endemic to practices of classification demand critical engagement and inquiry into the situatedness of particular cultural identities."@en .

cwrc:CulturalFormContext
    void:inDataset cwrc:datasetdefinition ;
    a owl:Class, skos:Concept ;
    rdfs:isDefinedBy <http://sparql.cwrc.ca/ontologies/cwrc-2017-08-03> ;
    rdfs:label "contexte culturel"@fr, "cultural form context"@en ;
    rdfs:subClassOf cwrc:Context ;
    skos:definition ""@en, ""@fr .

cwrc:CulturalFormation
    dcterms:isReplacedBy cwrc:CulturalForm ;
    void:inDataset cwrc:datasetdefinition ;
    a owl:DeprecatedClass, skos:Concept ;
    rdfs:comment "Deprecated in favour of class #CulturalForm."@en, "Désapprouver en faveur de la classe #CulturalForm."@fr ;
    rdfs:isDefinedBy <http://sparql.cwrc.ca/ontologies/cwrc-2017-08-03> ;
    rdfs:label "cultural formation "@en, "formation culturelle"@fr ;
    owl:equivalentClass cwrc:CulturalForm ;
    vs:term_status "deprecated"@en ;
    skos:definition ""@fr, "Cultural formation refers to the processes of lived social subjectivities of people and is often combined with predicates indicating the identity positions as they relate to the following discursive constructions of Class, Religion, Ethnicity, Gender, GeographicalHeritage, LinguisticAbility, NationalHeritage, NationalIdentity, PoliticalAffiliation, RaceColour, Sexuality. These categories are not understood as transhistorical or isolated categories. Rather, they facilitate analysis of how such situationally contingent, changing, and negotiated labels are assigned to or adopted by a particular individual. The tensions endemic to practices of classification demand critical engagement and inquiry into the situatedness of particular cultural identities."@en .

cwrc:EnglishLanguage
    dcterms:isReplacedBy locl:eng ;
    void:inDataset cwrc:datasetdefinition ;
    a skos:Concept ;
    rdfs:comment "Deprecated in favour of foreign instance <a href=\"http://id.loc.gov/vocabulary/languages/eng\">eng</a>."@en, "Désapprouver en faveur de l'instance <a href=\"http://id.loc.gov/vocabulary/languages/eng\">eng</a>."@fr ;
    rdfs:isDefinedBy <http://sparql.cwrc.ca/ontologies/cwrc-2017-08-03> ;
    rdfs:label "Anglais"@fr, "English"@en ;
    owl:deprecated true ;
    vs:term_status "deprecated"@en .

cwrc:EnglishNationalHeritage
    dcterms:isReplacedBy cwrc:englishNationalHeritage ;
    void:inDataset cwrc:datasetdefinition ;
    a owl:Thing, skos:Concept ;
    rdfs:comment "Deprecated in favour of instance #englishNationalHeritage."@en, "Désapprouver en faveur de l'instance #englishNationalHeritage."@fr ;
    rdfs:isDefinedBy <http://sparql.cwrc.ca/ontologies/cwrc-2017-08-03> ;
    rdfs:label "Anglais"@fr, "English"@en ;
    owl:deprecated true ;
    vs:term_status "deprecated"@en ;
    skos:definition ""@en, ""@fr .

cwrc:EnglishNationalIdentity
    dcterms:isReplacedBy cwrc:englishNationalIdentity ;
    void:inDataset cwrc:datasetdefinition ;
    a owl:Thing, skos:Concept ;
    rdfs:comment "Deprecated in favour of instance #englishNationalIdentity."@en, "Désapprouver en faveur de l'instance #englishNationalIdentity."@fr ;
    rdfs:isDefinedBy <http://sparql.cwrc.ca/ontologies/cwrc-2017-08-03> ;
    rdfs:label "Anglais"@fr, "English"@en ;
    owl:deprecated true ;
    vs:term_status "deprecated"@en ;
    skos:definition ""@en, ""@fr .

cwrc:Ethnicity
    void:inDataset cwrc:datasetdefinition ;
    a owl:Class, skos:Concept ;
    rdfs:isDefinedBy <http://sparql.cwrc.ca/ontologies/cwrc-2017-08-03> ;
    rdfs:label "ethnicity"@en, "ethnicité"@fr ;
    rdfs:subClassOf cwrc:CulturalForm ;
    skos:definition ""@fr, "Ethnicity is a subclass of CulturalForm that captures information about a person's ethnic position. Ethnicity is a sub-element within culturalFormation and raceAndEthnicity. See raceAndEthnicity for a detailed description of the complexities of this discursive construction and the social practices surrounding it."@en .

cwrc:EthnicityContext
    dcterms:subject cwrc:Ethnicity, cwrc:RaceColour ;
    void:inDataset cwrc:datasetdefinition ;
    a owl:Class, skos:Concept ;
    rdfs:isDefinedBy <http://sparql.cwrc.ca/ontologies/cwrc-2017-08-03> ;
    rdfs:label "contexte racial, de couleur de peau ou d'ethnicité"@fr, "racial, colour or ethnicity context"@en ;
    rdfs:subClassOf cwrc:CulturalFormContext ;
    skos:definition ""@en, ""@fr .

cwrc:Event
    void:inDataset cwrc:datasetdefinition ;
    a owl:Class, skos:Concept, <http://www.w3.org/2006/time/TemporalEntity> ;
    rdfs:isDefinedBy <http://sparql.cwrc.ca/ontologies/cwrc-2017-08-03> ;
    rdfs:label "event"@de, "event (historical)"@en, "évènement (historique)"@fr ;
    owl:sameAs dbpedia:Event, <http://erlangen-crm.org/current/E5.Event>, <http://linkedevents.org/ontology/Event> ;
    skos:definition "An event that occurs in space and time."@en ;
    foaf:name "Event" .

cwrc:FemaleLabel
    void:inDataset cwrc:datasetdefinition ;
    a skosxl:Label ;
    rdf:value "female" ;
    rdfs:comment "Deprecated with no current equivalence."@en, "Désapprouver sans équivalence."@fr ;
    rdfs:isDefinedBy <http://sparql.cwrc.ca/ontologies/cwrc-2017-08-03> ;
    rdfs:label "female"@en, "femelle"@fr ;
    owl:deprecated true ;
    owl:oneOf (cwrc:genderWomanFemale
        cwrc:femaleSex
    ) ;
    vs:term_status "deprecated"@en ;
    skos:definition ""@en, ""@fr ;
    skos:inScheme cwrc:TextLabels ;
    foaf:name "Female (Label)"@en .

cwrc:FrenchLanguage
    dcterms:isReplacedBy locl:fre ;
    void:inDataset cwrc:datasetdefinition ;
    a skos:Concept ;
    rdfs:comment "Deprecated in favour of foreign instance <a href=\"http://id.loc.gov/vocabulary/languages/fre\">fre</a>."@en, "Désapprouver en faveur de l'instance <a href=\"http://id.loc.gov/vocabulary/languages/fre\">fre</a>."@fr ;
    rdfs:isDefinedBy <http://sparql.cwrc.ca/ontologies/cwrc-2017-08-03> ;
    rdfs:label "Français"@fr, "French"@en ;
    owl:deprecated true ;
    vs:term_status "deprecated"@en .

cwrc:Gender
    void:inDataset cwrc:datasetdefinition ;
    a owl:Class, skos:Concept ;
    rdfs:isDefinedBy <http://sparql.cwrc.ca/ontologies/cwrc-2017-08-03> ;
    rdfs:label "gender"@en, "genre"@fr ;
    rdfs:subClassOf cwrc:CulturalForm ;
    skos:definition "A subclass of culturalForms for noting a person's gender whether attributed or self-defined. Although in popular culture gender and biological sex are conflated and understood to be binary, the concept of gender stresses the relationality, constructedness, and performativity of gendered identities and gendered behaviour, whose categories are historically contingent and shifting, and the boundaries between them blurry. Cf. Simone de Beauvoir: \"One is not born, but rather becomes, a woman,\" along with many other theorists of gender including Judith Butler, 1990. Gender is understood as fluid, situational, and sometimes plural, and it is related to though not commensurate with sexual identity and orientation. It is related to but not defined by specific forms of embodiment. Rather than seeing biological sex as a pre-social or natural given, the body is understood as a site of inscription (cf. Elizabeth Grosz 1994) which is also socially constructed and indeed epigenetically shaped by environmental factors (N. Katherine Hayles 2012). This ontology therefore does not provide separate terms for sex as distinct from gender. Instead, the slashes conjoining terms associated with gender and those conventionally associated with sex indicate the constant slippage between gender and sex in the way that these categories circulate through discourses, actions, and institutions. Far from indicating a universal facet of experience, gender intersects with other identity categories and axes of oppression such as class, race or colour, or geographical heritage to produced quite different interests and experiences among people of the same gender, as with the intersection of religion and white masculine identity in the Muscular Christianity movement in nineteenth-century Britain. Being a woman of colour may thus compound the impacts of gender oppression (<a href=\"#crenshaw_demarginalizing_1989\">Kimberlé Crenshaw, 1989</a>)."@en, "Cette  sous-classe de culturalForms indique le genre d’une personne, qu’il soit attribué par cette dernière ou auto-défini. Même si dans la culture populaire le genre et le sexe biologique sont confondus et binaires, le concept de genre souligne la relativité, la constructivité et la performativité des identités et des comportements genrés, réparties en catégories historiquement contingentes, changeantes et aux frontières floues. Cf Simone de Beauvoir: “On ne naît pas femme, on le devient,” et d’autres nombreuses théoriciennes du genre, dont Judith Butler en 1990. Le genre est entendu comme fluide, situationnel, parfois pluriel, et est relié à, l’identité et l’orientation sexuelles même s’ils ne doivent pas être confondus. Il est relié à des formes spécifiques d’incarnation ou à des comportements physiques, sans pour autant être défini par eux. Plutôt que de voir le sexe biologique comme présocial et attribué par nature,  le corps est compris comme un lieu d’inscriptions (cf Elizabeth Grosz 1994) qui est aussi socialement construit et épigénétiquement modelé par des facteurs environnementaux (N. Katherine Hayles 2012). Cette ontologie ne fournit donc pas de termes séparés pour le genre et le sexe. Les barres obliques qui lient les termes associés aux genres et ceux conventionnellement attribués au sexe indiquent plutôt le glissement constant de ces catégories au fil des discours, des actions et des institutions. Loin d’indiquer une part d’expérience universelle, le genre s’entrecroise avec d’autres catégories d’identité et axes d’oppression comme la classe, la race, la couleur, ou l’héritage géographique pour produire des intérêts et des expériences bien différentes pour les personnes d’un même genre. Un exemple est l’intersection de la religion et de l’identité masculine du mouvement de la Chrétienté Musculaire formé au Royaume-Uni au 19ème siècle. Dans ce contexte, être une femme de couleur devait aggraver les oppressions liées au genre (<a href=\"#crenshaw_demarginalizing_1989\">Kimberlé Crenshaw, 1989</a>)."@fr .

cwrc:GenderContext
    dcterms:subject cwrc:Gender ;
    void:inDataset cwrc:datasetdefinition ;
    a owl:Class, skos:Concept ;
    rdfs:isDefinedBy <http://sparql.cwrc.ca/ontologies/cwrc-2017-08-03> ;
    rdfs:label "Contexte de Genre"@fr, "Gender Context"@en ;
    rdfs:subClassOf cwrc:CulturalFormContext ;
    skos:definition ""@en, ""@fr .

cwrc:GenderQueer
    void:inDataset cwrc:datasetdefinition ;
    a owl:Class, skos:Concept ;
    rdfs:isDefinedBy <http://sparql.cwrc.ca/ontologies/cwrc-2017-08-03> ;
    rdfs:label "gender queer"@en, "non-binaire"@fr ;
    skos:note "Listed as non-binary? in french" .

cwrc:GeographicalHeritage
    void:inDataset cwrc:datasetdefinition ;
    a owl:Class, skos:Concept ;
    rdfs:isDefinedBy <http://sparql.cwrc.ca/ontologies/cwrc-2017-08-03> ;
    rdfs:label "geographical heritage"@en, "héritage géographique"@fr ;
    rdfs:subClassOf cwrc:CulturalForm ;
    skos:definition "GeographicalHeritage est une sous-classe de CulturalForm qui contient des informations sur les origines géographiques de la famille d'une personne, ce qui contribue souvent à la compréhension de ses origines ethnique et raciale. Cela permet de saisir l’identité de femmes qui se déclarent “sud-asiatiques” par exemple, quand aucune autre précision n'est fournie concernant l'héritage national. Voir raceEthnicityContext pour un compte-rendu détaillé de la complexité de cet élément."@fr, "GeographicalHeritage is a subclass of CulturalForm that captures information about the geographical origins of a person's family which often contributes to an understanding of their racial and ethnic background. It offers a way to capture women identified as \"South-Asian,\" for example, when no more precise national heritage is indicated. See raceAndEthnicity for a detailed description of the complexities of this element."@en .

cwrc:JadePenancier
    a foaf:Person ;
    foaf:name "Jade Penancier" .

cwrc:JewishEthnicity
    dcterms:isReplacedBy cwrc:jewishEthnicity ;
    void:inDataset cwrc:datasetdefinition ;
    rdfs:comment "Deprecated in favour of instance #jewishEthnicity."@en, "Désapprouver en faveur de l'instance #jewishEthnicity."@fr ;
    rdfs:isDefinedBy <http://sparql.cwrc.ca/ontologies/cwrc-2017-08-03> ;
    rdfs:label "Jewish"@en, "Juif"@fr ;
    owl:deprecated true ;
    vs:term_status "deprecated"@en ;
    skos:broader cwrc:jewishLabel ;
    skos:definition ""@en, ""@fr ;
    foaf:name "Jewish (Ethnicity)"@en .

cwrc:JohnSimpson
    a foaf:Person ;
    foaf:name "John Simpson" .

cwrc:KimMartin
    a foaf:Person ;
    foaf:name "Kim Martin" .

cwrc:Language
    void:inDataset cwrc:datasetdefinition ;
    a owl:Class, skos:Concept ;
    rdfs:isDefinedBy <http://sparql.cwrc.ca/ontologies/cwrc-2017-08-03> ;
    rdfs:label "aptitude linguistique"@fr, "linguistic lbility"@en ;
    rdfs:subClassOf cwrc:CulturalForm ;
    owl:sameAs <http://id.loc.gov/vocabulary/iso639-1/iso639-1_Language> ;
    skos:definition "These terms do not differentiate between spoken and/or written. For operational reasons this class is a direct equivalent to ISO639 language code as published by the Library of Congress."@en, "Écrit ou Parlé. Pour des raisons opérationnelles, cette classe est équivalente à la classe de langage iso639 publiée par le Library of Congress."@fr ;
    foaf:name "linguistic ability"@en .

cwrc:LanguageContext
    dcterms:subject cwrc:Language, cwrc:LinguisticAbility ;
    void:inDataset cwrc:datasetdefinition ;
    a owl:Class, skos:Concept ;
    rdfs:isDefinedBy <http://sparql.cwrc.ca/ontologies/cwrc-2017-08-03> ;
    rdfs:label "contexte linguistique"@fr, "language context"@en ;
    rdfs:subClassOf cwrc:CulturalFormContext ;
    skos:definition ""@en, ""@fr .

cwrc:LinguisticAbility
    void:inDataset cwrc:datasetdefinition ;
    a owl:Class, skos:Concept ;
    rdfs:isDefinedBy <http://sparql.cwrc.ca/ontologies/cwrc-2017-08-03> ;
    rdfs:label "aptitude linguistique (écrit ou parlé)"@fr, "linguistic ability (spoken and/or writen)"@en ;
    rdfs:subClassOf cwrc:CulturalForm ;
    skos:definition ""@en, ""@fr .

cwrc:NationalHeritage
    void:inDataset cwrc:datasetdefinition ;
    a owl:Class, skos:Concept ;
    rdfs:isDefinedBy <http://sparql.cwrc.ca/ontologies/cwrc-2017-08-03> ;
    rdfs:label "Héritage National"@fr, "National Heritage"@en ;
    rdfs:subClassOf cwrc:CulturalForm ;
    skos:definition ""@fr, "A subclass of culturalForms, this escrbes a person's national heritage and is not the same as citizenship."@en .

cwrc:NationalIdentity
    void:inDataset cwrc:datasetdefinition ;
    a owl:Class, skos:Concept ;
    rdfs:isDefinedBy <http://sparql.cwrc.ca/ontologies/cwrc-2017-08-03> ;
    rdfs:label "Nationality"@en, "Nationalité"@fr ;
    rdfs:subClassOf cwrc:CulturalForm ;
    skos:definition "A subclass of Cultural Form, this describes a person's nationalities and is not the same as citizenship."@en, "Une sous-classe de Cultural Form, ceci décrit la nationalité d'une personne et n'est pas sa citoyenneté."@fr .

cwrc:NationalityContext
    dcterms:subject cwrc:GeographicalHeritage, cwrc:NationalHeritage, cwrc:NationalIdentity ;
    void:inDataset cwrc:datasetdefinition ;
    a owl:Class, skos:Concept ;
    rdfs:isDefinedBy <http://sparql.cwrc.ca/ontologies/cwrc-2017-08-03> ;
    rdfs:label "contexte de nationalité"@fr, "nationality context"@en ;
    rdfs:subClassOf cwrc:CulturalFormContext ;
    skos:definition ""@en, ""@fr .

cwrc:Place
    void:inDataset cwrc:datasetdefinition ;
    a owl:Class, skos:Concept ;
    rdfs:isDefinedBy <http://sparql.cwrc.ca/ontologies/cwrc-2017-08-03> ;
    rdfs:label "endroit"@fr, "place"@en ;
    rdfs:subClassOf <http://www.w3.org/2003/01/geo/wgs84_pos#SpatialThing> ;
    owl:equivalentClass <http://dbpedia.org/ontology/Place>, <http://schema.org/Place>, <http://www.geonames.org/ontology#Feature> ;
    owl:sameAs <http://geovocab.org/spatial#Feature>, <http://www.opengis.net/ont/geosparql#Feature> ;
    skos:definition "A named place, wheter incorporated, settled or occupied."@en, "Could be a populated place according to Geonames, but not necessarily so. Some places, such as cross-roads are named without having a population or settlement per say. The geonames is inconsistent in this regards in that a populated place can be abandoned."@en, "Un endroit nommé, qu'il soit déclaré, investi ou occupé."@fr ;
    foaf:name "Endroit"@fr, "Place"@en .

cwrc:PoliticalAffiliation
    void:inDataset cwrc:datasetdefinition ;
    a owl:Class, skos:Concept, skos:ConceptScheme ;
    rdfs:isDefinedBy <http://sparql.cwrc.ca/ontologies/cwrc-2017-08-03> ;
    rdfs:label "affiliation politique"@fr, "political affiliation"@en ;
    rdfs:subClassOf cwrc:CulturalForm ;
    skos:definition ""@fr, "This subclass of CulturalForm tracks the affiliations, connections and associations which designate a person's political involvement. These affiliations can be both formal connections to a party or organization and informal political positions held by the writer. We hope to point our readers towards women writers associated with different political positions and help researchers make links between political beliefs and writing. For this reason, we are defining political affiliations broadly and include things like \"against capital punishment\" or \"strong supporter of the Empire\" in addition to more straightforward affiliations such as \"marxist\" or \"conservative.\""@en .

cwrc:PoliticalContext
    dcterms:subject cwrc:PoliticalAffiliation ;
    void:inDataset cwrc:datasetdefinition ;
    a owl:Class, skos:Concept ;
    rdfs:isDefinedBy <http://sparql.cwrc.ca/ontologies/cwrc-2017-08-03> ;
    rdfs:label "contexte politique"@fr, "political context"@en ;
    rdfs:subClassOf cwrc:CulturalFormContext ;
    skos:definition ""@en, ""@fr .

cwrc:RaceColour
    void:inDataset cwrc:datasetdefinition ;
    a owl:Class, skos:Concept ;
    rdfs:isDefinedBy <http://sparql.cwrc.ca/ontologies/cwrc-2017-08-03> ;
    rdfs:label "race and/or colour"@en, "race et/ou couleur de peau"@fr ;
    rdfs:subClassOf cwrc:CulturalForm ;
    skos:definition ""@en, ""@fr .

cwrc:RaceEthnicity
    void:inDataset cwrc:datasetdefinition ;
    a owl:Class, skos:Concept ;
    rdfs:isDefinedBy <http://sparql.cwrc.ca/ontologies/cwrc-2017-08-03> ;
    rdfs:label "race and/or ethnicity"@en, "race et/ou ethnicité"@fr ;
    rdfs:subClassOf cwrc:CulturalForm ;
    skos:definition ""@en, ""@fr .

cwrc:RaceEthnicityContext
    dcterms:subject cwrc:Ethnicity, cwrc:RaceColour ;
    void:inDataset cwrc:datasetdefinition ;
    a owl:Class, skos:Concept ;
    rdfs:isDefinedBy <http://sparql.cwrc.ca/ontologies/cwrc-2017-08-03> ;
    rdfs:label "contexte racial et/ou ethnique"@fr, "race ethnicity context"@en ;
    rdfs:subClassOf cwrc:CulturalFormContext ;
    skos:definition "raceEthnicityContext est une sous-classe importante de culturalFormContext. Elle indique la présence d’informations et de discussions sur le sujet concernant son appartenance raciale et ethnique, conjointement avec les sous-éléments spécifiques au sujet (raceColour, nationalHeritage, geogHeritage, ethnicity). La discussion qui suit s’applique au contexte discursif général de raceAndEthnicity ainsi qu’aux catégories spécifiques de cette sous-classe. Même si les catégories de race et d'ethnicité sont fréquemment manipulées au service d'intérêts déplorables, elles doivent être prises en compte à cause de leur répercussions idéologiques et matérielles sur la formation identitaire. Ces catégories sont changeantes, historiquement constituées, développées de façon intéressée, doivent être employées en contexte et sont ici entendues comme discursives et représentationnelles. C'est pour ces raisons que l'ontologie ne prétend pas offrir un ensemble de catégories exactes, complètement définies, ou mutuellement exclusives, ce que leur emploi instable et leur chevauchement ne permettent pas. Celles/ceux qui appliquent ces catégories et sous-catégories sont encouragé/es à ne pas faire fonctionner les identités privilégiées comme si elles étaient consensuelles et évidentes, ou à utiliser cette classe seulement pour les marginaux. Celles/ceux préoccupés par le fait que \"blanc\" et \"noir\" sont des catégories homogénéisantes sont encouragés à atteindre la spécificité à travers la multiplicité et les représentations intersectionnelles. RaceAndEthnicity est sous-classe de culturalFormation. Elle a quatre sous-classes qui lui sont liées: raceColour, nationalHeritage, geogHeritage et ethnicity."@fr, "raceEthnicityContext is a significant sub-class within culturalFormContext. It indicates the presence of information and discussions of a person's subject position with regards to race and ethnicity by working in conjunction with subject specific sub-elements (raceColour, nationalHeritage, geogHeritage, ethnicity). The following discussion applies to both the general discursive context of raceAndEthnicity as well as the specific sub-class categories. Despite the ways in which categories of race and ethnicity frequently serve heinous interests, their ideological and material impacts in the formation of identities requires recognition. These are shifting, historically constituted, and interestedly deployed categories whose use must be situated contextually and which are understood here finally as discursive or representational. Because of this this ontology does not try to lay out an exact, fully defined, or mutually exclusive set of categories: this is an impossibility given their shifting use and the overlap among them. Those applying this class and its subclasses are encouraged not to let privileged identities operate as an unspoken given or to use this class solely in relation to the marginalized. Those concerned about \"white\" and \"black\" as homogenizing categories are encouraged to reach for specificity through multiplicity and representations of intersectionality. RaceAndEthnicity is a sub-class within culturalFormation. It has four related content sub-classes: raceColour, nationalHeritage, geogHeritage, and ethnicity."@en .

cwrc:Religion
    void:inDataset cwrc:datasetdefinition ;
    a owl:Class, skos:ConceptScheme ;
    rdfs:isDefinedBy <http://sparql.cwrc.ca/ontologies/cwrc-2017-08-03> ;
    rdfs:label "religion"@en, "religion"@fr ;
    rdfs:subClassOf cwrc:CulturalForm ;
    skos:definition ""@fr, "A subclass of CulturalForm, this describes a person's religion(s) or belief system(s). Note that while atheism denotes the absence of religion, we use the Religion label for convenience."@en .

cwrc:ReligionContext
    dcterms:subject cwrc:Religion ;
    void:inDataset cwrc:datasetdefinition ;
    a owl:Class, skos:Concept ;
    rdfs:isDefinedBy <http://sparql.cwrc.ca/ontologies/cwrc-2017-08-03> ;
    rdfs:label "contexte religieux"@fr, "religious context"@en ;
    rdfs:subClassOf cwrc:CulturalFormContext ;
    skos:definition ""@en, ""@fr .

cwrc:RobWarren
    a foaf:Person ;
    owl:sameAs <http://rdf.muninn-project.org/ww1/2011/11/11/Person/Warren> ;
    foaf:homepage <http://www.muninn-project.org/> ;
    foaf:name "Robert Warren" .

cwrc:SexIdentity
    dcterms:isReplacedBy cwrc:Gender ;
    void:inDataset cwrc:datasetdefinition ;
    a owl:DeprecatedClass, skos:Concept ;
    rdfs:comment "Deprecated in favour of class Gender."@en, "Désapprouver en faveur de la classe Gender."@fr ;
    rdfs:isDefinedBy <http://sparql.cwrc.ca/ontologies/cwrc-2017-08-03> ;
    rdfs:label "identité sexe"@fr, "sex identity"@en ;
    rdfs:subClassOf cwrc:CulturalForm ;
    owl:equivalentClass cwrc:Gender ;
    vs:term_status "deprecated"@en .

cwrc:SexualIdentity
    dcterms:isReplacedBy cwrc:Sexuality ;
    void:inDataset cwrc:datasetdefinition ;
    a owl:DeprecatedClass, skos:Concept ;
    rdfs:comment "Deprecated in favour of #Sexuality term."@en, "Deprecated in favour of class #Sexuality."@en, "Désapprouver en faveur de la classe #Sexuality."@fr ;
    rdfs:isDefinedBy <http://sparql.cwrc.ca/ontologies/cwrc-2017-08-03> ;
    rdfs:label "Identité Sexuelle"@fr, "Sexual Identity"@en ;
    rdfs:subClassOf cwrc:CulturalForm ;
    owl:equivalentClass cwrc:Sexuality ;
    owl:sameAs <http://homosaurus.org/terms/sexualIdentity> ;
    vs:term_status "deprecated"@en .

cwrc:Sexuality
    void:inDataset cwrc:datasetdefinition ;
    a owl:Class, skos:Concept ;
    rdfs:isDefinedBy <http://sparql.cwrc.ca/ontologies/cwrc-2017-08-03> ;
    rdfs:label "sexuality"@en, "sexualité"@fr ;
    rdfs:subClassOf cwrc:CulturalForm ;
    owl:sameAs <http://homosaurus.org/terms/sexualIdentity> ;
    skos:definition "Ces termes identifient en un mot ou en une phrase la sexualité d'un sujet (par exemple “lesbienne”, “monogame”, “hétérosexuel/le”), non pas pour fermer la discussion, mais pour développer l’étude et l’analyse critique de ces catégories. L’association à une sexualité suppose que celle-ci n’est pas vécue de manière essentialiste, mais est plutôt plurielle et fluide; plusieurs désignations peuvent ainsi être appliquées à une seule personne. Le sujet elle/lui-même ou d'autres personnes peuvent émettre des assertions sur son identité sexuelle. Celles-ci peuvent se trouver en tension, se montrer incompatibles, et reflètent le changement du sujet au cours du sa vie. Par exemple, lier le terme “lesbienne” à la classe sexualIdentiy ne signifie pas que le sujet était définitivement lesbienne, car une telle identification est souvent impossible à cause des lacunes et silences historiques. En ce qui concerne les personnes toujours en vie, nous ne nous appuyons que sur des sources ou des déclarations publiques faites par le sujet elle/lui-même afin d’éviter de dévoiler sa sexualité par inadvertance. Voir (<a href=\"#CWRC_ISLANDORA_ID\">Campbell and Cowan 2016</a>)."@fr, "These terms capture in a word or phrase identifications of sexuality (i.e., \"lesbian,\" \"monogamous,\" \"heterosexual\") not as a means of shutting down but advancing investigation and critical analysis of these identifications. The association assumes that sexual identity does not function in an essentialist manner but can be plural and fluid, so multiple designations can be applied to a single person. Assertions of sexual itentity may come from the subject her/himself or from others. They may be in tension or mutually exclusive, and they may reflect different life stages. Linking to the term \"lesbian\" as a sexualIdentity class, for instance, does not signify that the subject was in any definitive sense a lesbian; such identifications are often impossible for reasons of historical gaps and silences. As far as living persons are concerned, our practice is to draw only on widely circulated public sources or disclosures from the subject her/himself in order to avoid inadvertently outing someone. See (<a href=\"#CWRC_ISLANDORA_ID\">Campbell and Cowan 2016</a>)"@en .

cwrc:SexualityContext
    dcterms:subject cwrc:Gender, cwrc:Sexuality ;
    void:inDataset cwrc:datasetdefinition ;
    a owl:Class, skos:Concept ;
    rdfs:isDefinedBy <http://sparql.cwrc.ca/ontologies/cwrc-2017-08-03> ;
    rdfs:label "contexte de sexualité"@fr, "sexuality context"@en ;
    rdfs:subClassOf cwrc:CulturalFormContext ;
    skos:definition "hasSexualityContext is a significant sub-class within culturalFormContext. It indicates the presence of information and discussions of a person's subject position with regards to their sexuality and sexual identity. A subclass of Cultural Formation, hasSexualityContext provides depth to more granual categorizations of a person through hasSexuality or hasSexuality. It is not meant to capture individual sexual experiences and relationships, which are covered by intimateRelationships. Specific relationships may be invoked here to indicate the effect on a subject's life and understanding of her own sexuality. This effort to to contextualize gestures towards some of the complicated issues around sexuality, for example, the politics of outing, the historical specificity of some categories such as \"congenital invert,\" or the multiple forms of relating to one's own sexuality. Capturing discussions of her sexuality within this element, will help users interested in the historical, ideological and gendered constructions of sexuality. There are important politics of privacy with respect to the disclosure of a subject's sexuality, sexual orientation and sexual identity. As far as living persons are concerned, our practice is to draw only on widely circulated public sources or disclosures from the subject her/himself in order to avoid inadvertently outing someone. See Campbell and Cowan 2016"@en, "sexualityContext est une sous-classe importante de culturalFormContext. Elle indique la présence de données ou de discussions sur la subjectivité d’une personne en ce qui concerne sa sexualité et son identité sexuelle. Sous-classe de culturalForms, sexualityContext approfondit la catégorisation granulaire d’une personne à travers hasSexuality ou hasSexuality. Elle n’est pas vouée à répertorier les expériences sexuelles et relations personnelles, qui sont comprises dans intimateRelationships. Des relations spécifiques pourront être évoquées ici pour indiquer les conséquences qu’elles ont eu dans la vie du sujet ou la compréhension de sa propre sexualité. Cet effort de contextualisation est un mouvement vers des questions complexes autours de la sexualité, comme par exemple les politiques de délation autour de la sexualité, la spécificité historique de certaines catégories comme “inversion sexuelle”, ou les multiples formes liées à la sexualité d’une personne. Les utilisatrices/teurs intéressé/es par la construction historique, idéologique et genrée de la sexualité pour se servir de cet élément qui rend compte des débats autour de ce thème. Nous reconnaissons l'importance des politiques de confidentialité au regard de la divulgation de la sexualité, de l’orientation et de l’identité sexuelles du sujet. En ce qui concerne les personnes toujours en vie, notre pratique est de ne nous appuyer que sur des sources ou des déclarations publiques venant du sujet elle/lui-même, afin d’éviter de dévoiler par inadvertance des informations privées sur sa sexualité. Voir Campbell and Cowan 2016. (http://ir.lib.uwo.ca/cgi/viewcontent.cgi?article=1085&context=fimspub). "@fr .

cwrc:SocialClass
    void:inDataset cwrc:datasetdefinition ;
    a owl:Class, skos:Concept, skos:ConceptScheme ;
    rdfs:isDefinedBy <http://sparql.cwrc.ca/ontologies/cwrc-2017-08-03> ;
    rdfs:label "classe sociale"@fr, "social class"@en ;
    rdfs:subClassOf cwrc:CulturalForm ;
    skos:definition "A subclass of culturalForm, socialClass terms associate subjects with a specific social group, recognizing that such categories and their application to individuals are contested and can change over time. The association may be or have been embraced by the subject her/himself or attributed by others. Unlike Notes typed as socialClassContext, which contain detailed discussion of a subject's class position, socialClass links to a word or phrase signifying a particular construction of class, with particular reference to earlier historical periods in the British Isles. Social class has been variously constructed and theorized, and for women is further complicated by the fact that women were understood to take their social status from fathers and/or husbands. The terminology used here reflects quite basic social groupings that intersect with other factors such as wealth."@en, "Une sous-catégorie de culturalForm, les termes de socialClass associent les sujets à des groupes sociaux spécifiques, en prenant en compte le fait que ces catégories et leur application aux individus sont contestables et peuvent changer au fil du temps. L’association à une classe sociale peut ou a pu être assumée par le sujet elle/lui-même ou attribuée par d’autres. Contrairement aux notes comme socialClassContext, qui contiennent les détails des discussions autour de le statut social du sujet, socialClass relie un mot ou une phrase référant à une classe spécifique qui renvoie à des périodes historiques antérieures spécifiques des Îles Britanniques. La notion de classe sociale a été construite et théorisée de diverses manières, et est d’autant plus complexe pour les femmes puisqu’elles étaient censées adopter le statut social de leur père et/ou de leur mari. La terminologie ici utilisée réfère à des groupes sociaux élémentaires qui se recoupent avec d’autres facteurs comme la richesse."@fr .

cwrc:SocialClassContext
    dcterms:subject cwrc:SocialClass ;
    void:inDataset cwrc:datasetdefinition ;
    a owl:Class, skos:Concept ;
    rdfs:isDefinedBy <http://sparql.cwrc.ca/ontologies/cwrc-2017-08-03> ;
    rdfs:label "contexte de classe sociale"@fr, "social class context"@en ;
    rdfs:subClassOf cwrc:CulturalFormContext ;
    skos:definition ""@en, ""@fr .

cwrc:SocialClassIdentity
    dcterms:isReplacedBy cwrc:SocialClass ;
    void:inDataset cwrc:datasetdefinition ;
    a owl:DeprecatedClass, skos:Concept ;
    rdfs:isDefinedBy <http://sparql.cwrc.ca/ontologies/cwrc-2017-08-03> ;
    rdfs:label "identité classe sociale"@fr, "social class identity"@en ;
    rdfs:subClassOf cwrc:CulturalForm ;
    owl:equivalentClass cwrc:SocialClass ;
    vs:term_status "deprecated"@en ;
    skos:definition "A subclass of culturalForms, socialClassIdentity terms associate subjects with a specific social group, recognizing that such categories and their application to individuals are contested and can change over time. The association may be or have been embraced by the subject her/himself or attributed by others. Unlike Notes typed as socialClassContext, which contain detailed discussion of a subject's class position, socialClassIdentity links to a word or phrase signifying a particular construction of class, with particular reference to earlier historical periods in the British Isles. Social class has been variously constructed and theorized, and for women is further complicated by the fact that women were understood to take their social status from fathers and/or husbands. The terminology used here reflects quite basic social groupings that intersect with other factors such as wealth."@en, "Une sous-catégorie de culturalForms, les termes de socialClassIdentity associent les sujets à des groupes sociaux spécifiques, en prenant en compte le fait que ces catégories et leur application aux individus sont contestables et peuvent changer au fil du temps. L’association à une classe sociale peut ou a pu être assumée par le sujet elle/lui-même ou attribuée par d’autres. Contrairement aux notes comme socialClassContext, qui contiennent les détails des discussions autour de le statut social du sujet, socialClassIdentity relie un mot ou une phrase référant à une classe spécifique qui renvoie à des périodes historiques antérieures spécifiques des Îles Britanniques. La notion de classe sociale a été construite et théorisée de diverses manières, et est d’autant plus complexe pour les femmes puisqu’elles étaient censées adopter le statut social de leur père et/ou de leur mari. La terminologie ici utilisée réfère à des groupes sociaux élémentaires qui se recoupent avec d’autres facteurs comme la richesse."@fr .

cwrc:SusanBrown
    a foaf:Person ;
    owl:sameAs <http://orcid.org/0000-0002-0267-7344> ;
    foaf:name "Susan Brown" .

cwrc:TextLabels
    void:inDataset cwrc:datasetdefinition ;
    a skos:ConceptScheme ;
    rdfs:isDefinedBy <http://sparql.cwrc.ca/ontologies/cwrc-2017-08-03> ;
    rdfs:label "text labels"@en, "étiquette"@fr ;
    skos:definition ""@fr, "Collection of all ambiguous labels within the Orlando markup."@en .

cwrc:abolitionism
    void:inDataset cwrc:datasetdefinition ;
    a cwrc:PoliticalAffiliation, skos:Concept ;
    rdf:value "abolition", "abolitionist", "anti-slavery", "integrationism", "sugar boycotter" ;
    rdfs:comment "La description de ce terme est basée sur celle de DBPedia."@fr, "The description for this term is indebted to DBpedia."@en ;
    rdfs:isDefinedBy <http://sparql.cwrc.ca/ontologies/cwrc-2017-08-03> ;
    rdfs:label "Abolitionnisme"@fr, "abolitionism"@en ;
    skos:broaderTransitive cwrc:humanRights, cwrc:racialEquality ;
    skos:definition "Abolitionism is a movement to end slavery, whether formal or informal. In Western Europe and the Americas, abolitionism is a historical movement to end the African and Indian slave trade and set slaves free. King Charles I of Spain, usually known as Emperor Charles V, following the example of the Swedish monarch, passed a law which would have abolished colonial slavery in 1542, although this law was not passed in the largest colonial states, and so was not enforced. In the late 17th century, the Roman Catholic Church, taking up a plea by Lourenco da Silva de Mendouca, officially condemned the slave trade, which was affirmed vehemently by Pope Gregory XVI in 1839. An abolitionist movement only started in the late 18th century, however, when English and American Quakers began to question the morality of slavery. James Oglethorpe was among the first to articulate the Enlightenment case against slavery, banning it in the Province of Georgia on humanist grounds, arguing against it in Parliament, and eventually encouraging his friends Granville Sharp and Hannah More to vigorously pursue the cause. Soon after his death in 1785, they joined with William Wilberforce and others in forming the Clapham Sect. The Somersett Case in 1772, which emancipated a slave in England, helped launch the British movement to abolish slavery. Though anti-slavery sentiments were widespread by the late 18th century, the colonies and emerging nations that used slave labour continued to do so: French, English and Portuguese territories in the West Indies; South America; and the Southern United States. After the American Revolution established the United States, northern states, beginning with Pennsylvania in 1780, passed legislation during the next two decades abolishing slavery, sometimes by gradual emancipation. Massachusetts ratified a constitution that declared all men equal; freedom suits challenging slavery based on this principle brought an end to slavery in the state. Vermont, which existed as an unrecognized state from 1777 to 1791, abolished adult slavery in 1777. In other states, such as Virginia, similar declarations of rights were interpreted by the courts as not applicable to Africans. During the following decades, the abolitionist movement grew in northern states, and Congress regulated the expansion of slavery in new states admitted to the union. David Brion Davis argues that the main driving force was a new moral consciousness, with an intellectual assist from the Enlightenment, and a powerful impulse from religious Quakers and evangelicals. France abolished slavery within the French Kingdom in 1315. Revolutionary France abolished slavery in its colonies in 1794, before it was restored by Napoleon in 1802. Haiti achieved independence from France in 1804 and brought an end to slavery in its territory, establishing the second republic in the New World. The northern states in the U.S. all abolished slavery by 1804. The United Kingdom and the United States outlawed the international slave trade in 1807, after which Britain led efforts to block slave ships. Britain abolished slavery throughout the British Empire with the Slavery Abolition Act 1833, the French colonies abolished it in 1848 and the U.S. in 1865 with the 13th Amendment to the U.S. Constitution. In Eastern Europe, groups organized to abolish the enslavement of the Roma in Wallachia and Moldavia; and to emancipate the serfs in Russia (Emancipation reform of 1861). It was declared illegal in 1948 under the Universal Declaration of Human Rights. The last country to abolish legal slavery was Mauritania, where it was officially abolished by presidential decree in 1981. Today, child and adult slavery and forced labour are illegal in most countries, as well as being against international law, but a high rate of human trafficking for labour and for sexual bondage continues to affect tens of millions of adults and children. <a href=\"#_dbpedia_2017\">(DBpedia, 2017)</a>"@en, "L'abolitionnisme est un courant de pensée qui émerge dans le dernier tiers du XVIIIe siècle dans le monde occidental (notamment en Grande-Bretagne) et vise la suppression de l'esclavage. Par extension, on utilise le terme pour tous les mouvements qui cherchent la suppression d'une tradition, d'une institution ou d'une loi : abolition de la peine de mort, de la torture, du travail, des privilèges, des prisons, de la prostitution, du spécisme, etc. <a href=\"#_dbpedia_2017\">(DBpedia, 2017)</a>"@fr ;
    skos:inScheme cwrc:PoliticalAffiliation ;
    prov:derivedFrom dbpedia:Abolitionism .

cwrc:abrahamicReligions
    void:inDataset cwrc:datasetdefinition ;
    a cwrc:Religion, skos:Concept ;
    rdfs:comment "La description de ce terme est basée sur celle de DBPedia."@fr ;
    rdfs:isDefinedBy <http://sparql.cwrc.ca/ontologies/cwrc-2017-08-03> ;
    rdfs:label "Abrahamic religions"@en, "Religions abrahamiques"@fr ;
    skos:definition "Abrahamic religions, emphasizing and tracing their common origin to the tribal patriarch Abraham or recognizing a spiritual tradition identified with him, comprising one of the major divisions in comparative religion, along with Indian, Iranian, and East Asian religions. Judaism, Christianity and Islam are the largest Abrahamic religions.The largest Abrahamic religions in chronological order of founding are Judaism (2nd millennium BCE), Christianity (1st century CE) and Islam (7th century CE). <a href=\"#_dbpedia_2017\">(DBpedia, 2017)</a>"@en, "L'expression religion abrahamique désigne principalement le judaïsme, le christianisme dont les Saintes Écritures, respectivement le Tanakh, la Bible évoquent la figure d'Abraham et l'islam avec le Coran, celle d'Ibrahim.En français, cette expression est apparue vers 1950 dans des études d'islamologie pour désigner, d'une part, la religion d'Abraham telle qu'elle se conçoit dans l'islam et d'autre part les trois religions que sont le judaïsme, le christianisme et l'islam. <a href=\"#_dbpedia_2017\">(DBpedia, 2017)</a>"@fr ;
    skos:inScheme cwrc:Religion ;
    prov:derivedFrom dbpedia:Abrahamic_religions .

cwrc:agnosticism
    void:inDataset cwrc:datasetdefinition ;
    a cwrc:Religion, skos:Concept ;
    rdfs:isDefinedBy <http://sparql.cwrc.ca/ontologies/cwrc-2017-08-03> ;
    rdfs:label "Agnosticism"@en, "agnosticisme"@fr ;
    skos:definition "Agnosticism is the view that, the truth values of certain claims – especially metaphysical and religious claims such as whether God, the divine or the supernatural exist – are unknown and perhaps unknowable. According to the philosopher William L. Rowe: \"In the popular sense of the term, an agnostic is someone who neither believes nor disbelieves in God, whereas an atheist disbelieves in God.\" Agnosticism is a doctrine or set of tenets rather than a religion as such. Thomas Henry Huxley, an English biologist, coined the word \"agnostic\" in 1869.Earlier thinkers, however, had written works that promoted agnostic points of view, such as Sanjaya Belatthaputta, a 5th-century BCE Indian philosopher who expressed agnosticism about any afterlife; and Protagoras, a 5th-century BCE Greek philosopher who expressed agnosticism about \"the gods\". The Nasadiya Sukta in the Rigveda is agnostic about the origin of the universe. <a href=\"#_dbpedia_2017\">(DBpedia, 2017)</a>"@en, "L’agnosticisme ou pensée de l'interrogation est une attitude de pensée considérant la vérité de certaines propositions concernant notamment l'existence de Dieu ou des dieux comme inconnaissable : à la différence des croyants, considérant probable ou certaine l'existence de telles divinités, ou des athées l'estimant improbable ou impossible, les agnostiques refusent de trancher. Si le degré de scepticisme varie selon les individus, les agnostiques s'accordent pour dire qu'il n'existe pas de preuve définitive en faveur de l'existence ou de l'inexistence du divin, et affirment l'impossibilité de se prononcer. Si les agnostiques refusent de se prononcer quant à l'existence d'une intelligence supérieure, ils n'accordent, en revanche, ou du moins tendent à n'accorder, aucune transcendance et aucune valeur sacrée aux religions (prophète, messie, textes sacrés...) et à leurs institutions (clergé, rituels et prescriptions diverses...). Ceux-ci voient en effet les religions comme de pures constructions sociales et culturelles qui auraient surtout pour fonction historique d'assurer la cohésion et l'ordre dans les sociétés humaines traditionnelles via par exemple la menace de l'enfer, la promesse du paradis ou encore la notion de péché ou par le mécanisme du bouc émissaire. En d'autres termes, les religions, aux yeux d'un agnostique, seraient bien trop « humaines » de par leurs modes de fonctionnement et de par les dynamiques anthropologiques sur lesquelles elles se basent (soutien psychologique face à la mort, analogie très anthropocentrique d'un Dieu bâtisseur de l'univers...) pour qu'elles aient un quelconque lien direct avec toute forme d'intelligence supérieure, tout en n'excluant pas non plus pour certains le fait que ce soit malgré tout possible. D'où cette interrogation constante propre à l'agnostique. <a href=\"#_dbpedia_2017\">(DBpedia, 2017)</a>"@fr ;
    skos:inScheme cwrc:Religion .

cwrc:aidsActivism
    void:inDataset cwrc:datasetdefinition ;
    a cwrc:PoliticalAffiliation, skos:Concept ;
    rdf:value "aids activist" ;
    rdfs:comment "The description for this term is indebted to DBpedia."@en ;
    rdfs:isDefinedBy <http://sparql.cwrc.ca/ontologies/cwrc-2017-08-03> ;
    rdfs:label ""@fr, "AIDS activism"@en ;
    skos:broaderTransitive cwrc:socialReform ;
    skos:definition ""@fr, "Activism related to HIV/AIDS, ranging from addressing attitudes to changing government policies related to treatment and medication. See: <a href=\"https://en.wikipedia.org/wiki/Category:AIDS_activism\">https://en.wikipedia.org/wiki/Category:AIDS_activism</a>"@en ;
    skos:inScheme cwrc:PoliticalAffiliation ;
    prov:derivedFrom <http://dbpedia.org/resource/Category:AIDS_activism> .

cwrc:americanNationalism
    void:inDataset cwrc:datasetdefinition ;
    a cwrc:PoliticalAffiliation, skos:Concept ;
    rdf:value "(us) nationalist", "american nationalist", "us nationalist", "us patriotism" ;
    rdfs:comment "The description for this term is indebted to DBpedia."@en ;
    rdfs:isDefinedBy <http://sparql.cwrc.ca/ontologies/cwrc-2017-08-03> ;
    rdfs:label ""@fr, "American nationalism"@en ;
    skos:broaderTransitive cwrc:nationalism ;
    skos:definition ""@en, ""@fr ;
    skos:inScheme cwrc:PoliticalAffiliation .

cwrc:anarchism
    void:inDataset cwrc:datasetdefinition ;
    cwrc:contraryTo cwrc:nationalism ;
    a cwrc:PoliticalAffiliation, skos:Concept ;
    rdf:value "anarchist" ;
    rdfs:comment "La description de ce terme est basée sur celle de DBPedia."@fr, "The description for this term is indebted to DBpedia."@en ;
    rdfs:isDefinedBy <http://sparql.cwrc.ca/ontologies/cwrc-2017-08-03> ;
    rdfs:label "Anarchisme"@fr, "anarchism"@en ;
    skos:definition "Anarchism is a political philosophy that advocates self-governed societies based on voluntary institutions. These are often described as stateless societies, although several authors have defined them more specifically as institutions based on non-hierarchical free associations. Anarchism holds the state to be undesirable, unnecessary, and harmful. While anti-statism is central, anarchism entails opposing authority or hierarchical organisation in the conduct of all human relations, including, but not limited to, the state system. Anarchism does not offer a fixed body of doctrine from a single particular world view, instead fluxing and flowing as a philosophy. Many types and traditions of anarchism exist, not all of which are mutually exclusive. Anarchist schools of thought can differ fundamentally, supporting anything from extreme individualism to complete collectivism. Strains of anarchism have often been divided into the categories of social and individualist anarchism or similar dual classifications. Anarchism is usually considered a radical left-wing ideology, and much of anarchist economics and anarchist legal philosophy reflect anti-authoritarian interpretations of communism, collectivism, syndicalism, mutualism, or participatory economics. <a href=\"#_dbpedia_2017\">(DBpedia, 2017)</a>"@en, """L'anarchisme est un courant de philosophie politique développé depuis le XIXe siècle sur un ensemble de théories et de pratiques anti-autoritaires d'égalité sociale. Le terme libertaire, souvent utilisé comme synonyme d'anarchisme, est un néologisme créé en 1857 par Joseph Déjacque pour renforcer le caractère égalitaire. Fondé sur la négation du principe d'autorité dans l'organisation sociale et le refus de toute contrainte découlant des institutions basées sur ce principe, l'anarchisme a pour but de développer une société sans domination et sans exploitation, où les individus-producteurs coopèrent librement dans une dynamique d'autogestion et de fédéralisme. Contre l'oppression, l'anarchisme propose une société basée sur la solidarité comme solution aux antagonismes, la complémentarité de la liberté de chacun et celle de la collectivité, l'égalité des conditions de vie et la propriété commune autogérée. Il s'agit donc d'un mode politique qui cherche non pas à résoudre les différences opposant les membres constituants de la société mais à associer des forces autonomes et contradictoires. Le terme « anarchisme » et ses dérivés sont employés tantôt péjorativement, comme synonymes de désordre social dans le sens commun ou courant et qui se rapproche de l’anomie, tantôt comme un but pratique, car l'anarchisme défend l'idée que l'absence d'une structure de pouvoir n'est pas synonyme de désorganisation sociale. Les anarchistes rejettent en général la conception courante de l'anarchie (utilisée par les médias et les pouvoirs politiques). Pour eux, l'ordre naît de la liberté, tandis que les pouvoirs engendrent le désordre. Certains anarchistes useront du terme « acratie » (du grec « kratos », le pouvoir), donc littéralement « absence de pouvoir », plutôt que du terme « anarchie » qui leur semble devenu ambigu. De même, certains anarchistes auront plutôt tendance à utiliser le terme de « libertaires ». Pour ses partisans, l'anarchie n'est justement pas le désordre social. C’est plutôt le contraire, soit l'ordre social absolu, grâce notamment au collectivisme anti-capitaliste. Ce collectivisme, contrairement à l'idée de possessions privées capitalisées, suggère celle de possessions individuelles ne garantissant aucun droit de propriété, notamment celle touchant l'accumulation de biens non utilisés. En outre, ce collectivisme s’exprime par une liberté politique organisée autour du mandatement impératif, de l'autogestion, du fédéralisme et de la démocratie directe. L'anarchie est donc organisée et structurée : c'est l'ordre moins le pouvoir. L'anarchisme est un mouvement pluriel qui embrasse l'ensemble des secteurs de la vie et de la société. Concept philosophique, c’est également « une idée pratique et matérielle, un mode d’être de la vie et des relations entre les êtres qui naît tout autant de la pratique que de la philosophie ; ou pour être plus précis qui naît toujours de la pratique, la philosophie n’étant elle-même qu’une pratique, importante mais parmi d’autres ». En 1928, Sébastien Faure, dans La Synthèse anarchiste, définit quatre grands courants qui cohabitent tout au long de l'histoire du mouvement : 
  *  l'individualisme libertaire qui insiste sur l'autonomie individuelle contre toute autorité ; 
  *  le socialisme libertaire qui propose une gestion collective égalitaire de la société ; 
  *  le communisme libertaire, qui de l'aphorisme « De chacun selon ses moyens, à chacun selon ses besoins » créé par Louis Blanc, veut économiquement partir du besoin des individus, pour ensuite produire le nécessaire pour y répondre ; 
  *  l'anarcho-syndicalisme, qui propose une méthode, le syndicalisme, comme moyen de lutte et d'organisation de la société. Depuis, de nouvelles sensibilités se sont affirmées, telles l'anarcha-féminisme ou l'écologie sociale. La pertinence de cette section est remise en cause, considérez son contenu avec précaution. En discuter ? Pour Vivien Garcia dans L'Anarchisme aujourd'hui (2007), l'anarchisme « ne peut être conçu comme un monument théorique achevé. La réflexion anarchiste n'a rien du système. […] L'anarchisme se constitue comme une nébuleuse de pensées qui peuvent se renvoyer de façon contingente les unes aux autres plutôt que comme une doctrine close » Selon l'historien américain Paul Avrich : « Les anarchistes ont exercé et continuent d'exercer une grande influence. Leur internationalisme rigoureux et leur antimilitarisme, leurs expériences d'autogestion ouvrière, leur lutte pour la libération de la femme et pour l'émancipation sexuelle, leurs écoles et universités libres, leur aspiration écologique à un équilibre entre la ville et la campagne, entre l'homme et la nature, tout cela est d'une actualité criante. » <a href=\"#_dbpedia_2017\">(DBpedia, 2017)</a>"""@fr ;
    skos:inScheme cwrc:PoliticalAffiliation ;
    skos:related cwrc:anti-Monarchism ;
    prov:derivedFrom dbpedia:Anarchism .

cwrc:anglicanism
    void:inDataset cwrc:datasetdefinition ;
    a cwrc:Religion, skos:Concept, foaf:Organization ;
    rdfs:comment "La description de ce terme est basée sur celle de DBPedia."@fr, "The description for this term is indebted to the Getty Art & Architecture Thesaurus."@en ;
    rdfs:isDefinedBy <http://sparql.cwrc.ca/ontologies/cwrc-2017-08-03> ;
    rdfs:label "Anglicaans (kerk van Engeland)"@nl, "Anglicanism"@en, "Anglicanismo"@es, "Iglesia de Inglaterra"@es, "ying guo sheng gong hui"@zh-latn-pinyin-x-notone, "ying kuo sheng kung hui"@zh-latn-wadegile, "yīng guó shèng gōng huì"@zh-latn-pinyin-x-hanyu, "Église d'Angleterre"@fr, "英國聖公會 (英國國教)"@zh-hant ;
    skos:broaderTransitive cwrc:christianity ;
    skos:definition "A Christian denomination having both Protestant and Catholic aspects that originated with Henry VIII's break with the Roman Catholic Church (ca. 1532-34). As the official state Church of England, the monarch of England is still formally considered its head. While at first it remained mainly Catholic in character, reforms came under Edward IV and Elizabeth I who introduced doctrine that was more Protestant in nature, namely new editions of the Book of Common Prayer and the Thirty-nine Articles. Although an overall attitude of toleration exists in the modern Anglican Church, tension remains between its Protestant and Catholic inclinations as well as with newer liberal and evangelical influences. Anglicanism is based on episcopal authority and parish structure is fundamental to the organization of the church. The term is used with regard to the Church of England; with regard to the Episcopal Church in America, use \"Episcopal.\" <a href=\"#_getty_2017\">(Getty, 2017)</a>"@en, "L'anglicanisme est une confession chrétienne présente principalement dans les pays qui ont pu être imprégnés par la culture anglaise incluant notamment, outre l'Angleterre, les anciennes colonies britanniques en Amérique et en Afrique. On retrouve tout de même plusieurs communauté anglicanes dans le monde, notamment en France. L'origine de cette confession remonte à la période antique de l'Église d'Angleterre, lorsque celle-ci était unie canoniquement et juridiquement à l'évêque de Rome. Puis, au XVIe siècle, lorsque le roi d'Angleterre Henri VIII rompit avec le pape de Rome pour causes politiques et théologiques. Ainsi, Henri VIII ne créa rien de nouveau : il extirpa l'autorité du pape de son royaume, sans pour autant modifier ou jeter de nouvelles bases théologiques pour l'Église, et remplaça l'autorité papale par la sienne propre. Depuis la reine Elizabeth Ire, le monarque a le titre de « gouverneur suprême », mais n'a qu'un rôle de maintien de l'ordre et du bon déroulement de la vie ecclésiale, mais aucune réelle autorité décisionnelle comme celle d'un évêque ou d'un synode. L'Archevêque de Canterbury porte le titre de « primat de toute l'Angleterre » et l'archevêque d'York porte quant à lui le titre de « primat de l'Angleterre ». L'Église anglicane, tout comme l'Église orthodoxe, est une communion d'églises autocéphales, mais néanmoins interdépendantes. Bien que plusieurs églises anglicanes existent à travers le monde, comme c'est le cas pour l'Église catholique romaine (présente en France, en Espagne, etc.), ou encore pour l'Église orthodoxe (présente en Russie, en Serbie, etc.), il ne s'agit que d'une seule Église. Elles sont rassemblées dans la Communion anglicane , au sein de laquelle l'Église d'Angleterre et son primat, l'archevêque de Canterbury, ne jouissent que d'une primauté d'honneur. Ces églises sont en pleine communion (doctrinale, spirituelle, épiscopale, sacramentelle) les unes avec les autres et représentent ensemble environ 85 millions de fidèles. Les Églises de la Communion anglicane ont une structure épiscopale. Elles se disent à la fois catholiques et réformées, et l'anglicanisme a souvent été présenté comme une via media entre le catholicisme romain et le protestantisme. Elles se présentent comme des Églises catholiques non romaines, parce qu'elles se veulent en continuité avec la tradition apostolique (ainsi la patristique est très développée dans le monde anglican) et affirment avoir conservé la succession apostolique. L'Église orthodoxe du patriarcat œcuménique de Constantinople a reconnu la validité de la succession apostolique en 1922 ; cependant, d'autres patriarcats, comme celui de Russie, ne saurait reconnaître une quelconque succession apostolique, en autre par le fait de l'ordination épiscopale de femme, depuis janvier 2015. L'Église catholique romaine ne leur reconnait pas cette qualité : ainsi par la lettre apostolique Apostolicae Curae le pape Léon XIII déclare en 1896 « nulles et sans valeur » les ordinations anglicanes (doctrine confirmée par le motu proprio Ad Tuendam Fidem en 1998). Les archevêques anglicans de Canterbury et d'York ont donné leur réponse dans Saepius officio. Pour autant, lors du concile Vatican II est affirmée la « place particulière » des Anglicans, « qui gardent en partie les traditions et les structures catholiques ». Par ailleurs, les Églises anglicanes se disent réformées parce qu'elles ont adhéré à certains principes nouveaux issus de la Réforme protestante en matière de doctrine et de liturgie.À l'origine, la doctrine anglicane est énoncée dans les Trente-neuf articles (Bill of XXXIX articles) qui ont longtemps eu une valeur impérative. L'éventail entre les positions doctrinales s'est ensuite élargi et donne lieu à de nombreuses classifications (Haute Église, Basse Église, Broad Church (en), Anglo-catholicisme, Évangélisme…). Alors que pendant longtemps la coexistence apaisée entre de telles positions divergentes était considérée comme une spécificité de l'anglicanisme, la communion est depuis la fin du XXe siècle soumise à de forts tiraillements sur certaines questions, notamment l'ordination des femmes et la position par rapport à l'homosexualité. <a href=\"#_dbpedia_2017\">(DBpedia, 2017)</a>"@fr, "Te gebruiken om te verwijzen naar de anglicaanse kerk (Church of England); gebruik 'episcopaal' om te verwijzen naar de episcopale kerk in Amerika. De term verwijst naar een christelijke geloofsrichting met zowel protestantse als katholieke elementen die ontstond na de breuk tussen de Engelse koning Hendrik VIII en de rooms-katholieke kerk (circa 1532-34). Het anglicanisme is de officiële Britse staatsgodsdienst, en de Britse soevereine vorst is nog altijd het officiële hoofd van de anglicaanse kerk. Aanvankelijk droeg de kerk nog een overwegend katholiek karakter, maar onder Edward IV en Elizabeth I werden er hervormingen doorgevoerd en werd een meer protestants georiënteerde geloofsleer geïntroduceerd, met een nieuwe versie van het Book of Common Prayer en de Negenendertig Artikelen. Hoewel de huidige anglicaanse kerk in het algemeen wordt gekenmerkt door een tolerante houding, zijn de spanningen tussen protestants en katholiek gezinde stromingen binnen de kerk nooit verdwenen en heerst er weerstand tegen nieuwe vrijzinnige en evangelische invloeden. Het anglicanisme berust op episcopaal gezag en op een structuur van parochies, welke van fundamenteel belang is voor de kerkelijke organisatie. <a href=\"#_getty_2017\">(Getty, 2017)</a>"@nl, "Úsese con referencia a la Iglesia de Inglaterra y también con referencia a la Iglesia Episcopal de Estados Unidos (úsese Iglesia Episcopal). Este término s erefiere a a una denominación cristiana que contiene elementos católicos y protestantes en varios aspectos y que se originó con el rey Enrique VIII quien rompió con la Iglesia Católica Romana (ca. 1532-1534) Es la iglesia oficial de Inglaterra, la Monarquía Inglesa es aún formalmente considerada su cabeza.Mientras en sus comienzos conservaba su carácter católico, con las reformas realizadas bajo Eduardo IV e Isabel I quienes introdujeron una doctrina que está más cerca del protestantismo y que se encuentra contenida en nuevas ediciones del Libro de Oraciones Comunes y en los Treinta y nueve Artículos. Aunque el anglicanismo  tiene actualmente una actitud de total tolerancia, aún persisten tensiones con las iglesias protestantes y católicas así como de últimas influencias liberales y evangélicas.El Anglicanismo está basado en la autoridad episcopal y se sustenta en una estructura de parroquias que resulta fundamental para la organización de la Iglesia. <a href=\"#_getty_2017\">(Getty, 2017)</a>"@es, "英王亨利八世與羅馬天主教教會(西元1532-34年)分裂所創的基督教派別，同時含有新教與天主教元素。作為官方英國國教，其正式教會首腦仍為英國國王。起初較具天主教特色，在愛德華四世與伊莉莎白一世時改革，加入較具新教本質的教條，即：新版的公禱書(Book of Common Prayer)及三十九條信綱(Thirty-nine Articles)。雖然現代的英國聖公會大體上態度已越顯寬容，但教會內的新教派系與天主教派系關係仍緊繃，也仍不樂於接受較新的自由與福音派影響。英國聖公會奠基於主教的權威上，牧師教區的結構對教會組織十分重要。此詞彙用於指稱英國國教；美國區的主教派教會，則稱為「美國聖公會(Episcopal)」。 <a href=\"#_getty_2017\">(Getty, 2017)</a>"@zh-hant ;
    skos:inScheme cwrc:Religion ;
    prov:derivedFrom dbpedia:Anglicanism, <http://vocab.getty.edu/aat/300153822> .

cwrc:animalWelfareAdvocacy
    void:inDataset cwrc:datasetdefinition ;
    a cwrc:PoliticalAffiliation, skos:Concept ;
    rdf:value "animal activist", "animal rights", "animal rights advocate", "animal welfare activist", "anti-blood-sports", "anti-cruelty", "anti-cruelty to animals", "anti-hunting" ;
    rdfs:comment "The description for this term is indebted to DBpedia."@en ;
    rdfs:isDefinedBy <http://sparql.cwrc.ca/ontologies/cwrc-2017-08-03> ;
    rdfs:label ""@fr, "animal welfare advocacy"@en ;
    skos:broaderTransitive cwrc:socialReform ;
    skos:definition ""@fr, "Advocacy, often in the form of activism, for the welfare of animals. See: <a href=\"https://en.wikipedia.org/wiki/Animal_welfare\">https://en.wikipedia.org/wiki/Animal_welfare</a>"@en ;
    skos:inScheme cwrc:PoliticalAffiliation ;
    skos:related cwrc:feminism ;
    prov:derivedFrom dbpedia:Animal_welfare .

cwrc:anti-American
    void:inDataset cwrc:datasetdefinition ;
    a cwrc:PoliticalAffiliation, skos:Concept ;
    rdfs:comment "The description for this term is indebted to DBpedia."@en ;
    rdfs:isDefinedBy <http://sparql.cwrc.ca/ontologies/cwrc-2017-08-03> ;
    rdfs:label ""@fr, "anti-American politics"@en ;
    skos:definition ""@fr, "Opposed to the policies or influence of the United States of America, often with reference to specific government actions. See: <a href=\"https://en.wikipedia.org/wiki/anti-american\">https://en.wikipedia.org/wiki/anti-american</a>"@en ;
    skos:inScheme cwrc:PoliticalAffiliation ;
    prov:derivedFrom dbpedia:anti-american .

cwrc:anti-Antisemitism
    void:inDataset cwrc:datasetdefinition ;
    cwrc:contraryTo cwrc:antisemitism ;
    a cwrc:PoliticalAffiliation, skos:Concept ;
    rdf:value "anti-anti-semitism", "anti-antisemitic", "anti-antisemitist" ;
    rdfs:comment "The description for this term is indebted to DBpedia."@en ;
    rdfs:isDefinedBy <http://sparql.cwrc.ca/ontologies/cwrc-2017-08-03> ;
    rdfs:label ""@fr, "anti-antisemitism"@en ;
    skos:broaderTransitive cwrc:racialEquality ;
    skos:definition ""@fr, "Opposed to anti-semitic attitudes and practices. See <a href=\"https://en.wikipedia.org/wiki/Antisemitism\">https://en.wikipedia.org/wiki/Antisemitism</a>"@en ;
    skos:inScheme cwrc:PoliticalAffiliation ;
    skos:related cwrc:anti-Fascism ;
    prov:derivedFrom dbpedia:Antisemitism .

cwrc:anti-Apartheid
    void:inDataset cwrc:datasetdefinition ;
    a cwrc:PoliticalAffiliation, skos:Concept ;
    rdfs:comment "The description for this term is indebted to DBpedia."@en ;
    rdfs:isDefinedBy <http://sparql.cwrc.ca/ontologies/cwrc-2017-08-03> ;
    rdfs:label ""@fr, "anti-apartheid"@en ;
    skos:broaderTransitive cwrc:humanRights, cwrc:racialEquality, cwrc:socialReform ;
    skos:definition ""@fr, "The Anti-Apartheid Movement (AAM), originally known as the Boycott Movement, was a British organisation that was at the centre of the international movement opposing South Africa's system of apartheid and supporting South Africa's non-whites. <a href=\"#_dbpedia_2017\">(DBpedia, 2017)</a>"@en ;
    skos:inScheme cwrc:PoliticalAffiliation ;
    prov:derivedFrom dbpedia:Anti-Apartheid_Movement .

cwrc:anti-Boer
    void:inDataset cwrc:datasetdefinition ;
    cwrc:contraryTo cwrc:pro-BoerWar ;
    a cwrc:PoliticalAffiliation, skos:Concept ;
    rdfs:comment "The description for this term is indebted to DBpedia."@en ;
    rdfs:isDefinedBy <http://sparql.cwrc.ca/ontologies/cwrc-2017-08-03> ;
    rdfs:label ""@fr, "anti-Boer politics"@en ;
    skos:definition ""@fr, "Opposition to the Second Boer War in Britain was modest when the war began on 11 October 1899 and was always less widespread than support for it, let alone prevailing indifference. However, influential groups formed immediately and ineffectually against the war, including the South African Conciliation Committee and W. T. Stead's Stop the War Committee. <a href=\"#_dbpedia_2017\">(DBpedia, 2017)</a>"@en ;
    skos:inScheme cwrc:PoliticalAffiliation ;
    skos:related cwrc:anti-WarMovement ;
    prov:derivedFrom dbpedia:Opposition_to_the_Second_Boer_War .

cwrc:anti-Bolshevism
    void:inDataset cwrc:datasetdefinition ;
    cwrc:contraryTo cwrc:bolshevism ;
    a cwrc:PoliticalAffiliation, skos:Concept ;
    rdf:value "anti-bolshevik" ;
    rdfs:comment "La description de ce terme est basée sur celle de DBPedia."@fr, "The description for this term is indebted to DBpedia."@en ;
    rdfs:isDefinedBy <http://sparql.cwrc.ca/ontologies/cwrc-2017-08-03> ;
    rdfs:label "Anticommunisme"@fr, "anti-Bolshevism"@en ;
    skos:definition "Anti-communism is opposition to communism. Organized anti-communism developed in reaction to the rise of communism, especially after the 1917 October Revolution in Russia. It reached global dimensions during the Cold War, when America and the Soviet Union engaged in an intense rivalry. Most modern anti-communists reject the concept of historical materialism, which is a central idea in Marxism. Anti-communists reject the Marxist belief that capitalism will be followed by socialism and communism, just as feudalism was followed by capitalism. Anti-communists question the validity of the Marxist claim that the socialist state will \"wither away\" when it becomes unnecessary in a true communist society. Anti-communists also accuse communists of having caused several famines that occurred in 20th-century communist states, such as the Russian Famine of 1921 and the much more severe famine in China during the Great Leap Forward. Some anti-communists refer to both communism and fascism as totalitarianism, seeing similarity between the actions of communist and fascist governments. Opponents argue that communist parties that have come to power have tended to be rigidly intolerant of political opposition. Communist governments have also been accused of creating a new ruling class (a Nomenklatura), with powers and privileges greater than those previously enjoyed by the upper classes in the non-communist regimes. <a href=\"#_dbpedia_2017\">(DBpedia, 2017)</a>"@en, "Le terme d'anticommunisme englobe, au sens large, l'ensemble des attitudes d'opposition ou d'hostilité envers les aspects théoriques ou pratiques du communisme : l'anticommunisme peut se traduire sous forme de simple prise de position, de discours politique structuré, d'action ou de propagande. Son sens est cependant changeant en fonction de celui du « communisme », mot qui recouvre lui-même un ensemble de réalités très différentes les unes des autres en fonction des contextes sociaux, culturels et politiques. Les facteurs distinguant les différents types d'anticommunisme sont notamment la forme de communisme explicitement visée et les motivations qui poussent à s'opposer au communisme ; le terme « anticommunisme » est employé, selon les époques et les contextes, pour qualifier l'opposition aux théories marxistes ou communistes elles-mêmes, ou aux mouvances et partis politiques s'en réclamant, ou bien à la pratique politique des régimes communistes. Le terme d'« anticommunisme » a pu ainsi être utilisé pour qualifier les opposants au stalinisme, que ces derniers aient été ou non anticommunistes au sens strict. Apparu au XIXe siècle en tant que concept, l'anticommunisme s’est largement développé au cours du XXe siècle, à la suite de la prise du pouvoir par les bolcheviks en Russie en octobre 1917, puis à la création de l’URSS : il s’est alors identifié, pour l'essentiel, à l'opposition aux régimes communistes et aux partis communistes d'inspiration léniniste et stalinienne. Après la Seconde Guerre mondiale, l’anticommunisme devient un élément majeur de la politique étrangère et intérieure des États-Unis, opposés à l'URSS dans le contexte de la guerre froide. <a href=\"#_dbpedia_2017\">(DBpedia, 2017)</a>"@fr ;
    skos:inScheme cwrc:PoliticalAffiliation ;
    skos:related cwrc:anti-Communism ;
    prov:derivedFrom dbpedia:Anti-communism .

cwrc:anti-Bonapartism
    void:inDataset cwrc:datasetdefinition ;
    a cwrc:PoliticalAffiliation, skos:Concept ;
    rdf:value "anti-bonapartist" ;
    rdfs:comment "The description for this term is indebted to DBpedia."@en ;
    rdfs:isDefinedBy <http://sparql.cwrc.ca/ontologies/cwrc-2017-08-03> ;
    rdfs:label ""@fr, "anti-Bonapartism"@en ;
    skos:definition ""@fr, "Opposed to the political ideology of Napolean Bonaparte and his followers. See <a href=\"https://en.wikipedia.org/wiki/Bonapartism\">https://en.wikipedia.org/wiki/Bonapartism</a>"@en ;
    skos:inScheme cwrc:PoliticalAffiliation ;
    prov:derivedFrom dbpedia:Bonapartism .

cwrc:anti-British
    void:inDataset cwrc:datasetdefinition ;
    a cwrc:PoliticalAffiliation, skos:Concept ;
    rdfs:comment "The description for this term is indebted to DBpedia."@en ;
    rdfs:isDefinedBy <http://sparql.cwrc.ca/ontologies/cwrc-2017-08-03> ;
    rdfs:label ""@fr, "anti-British politics"@en ;
    skos:definition ""@fr, "Opposed to the policies or influence of the United Kingdom, often with reference to specific government actions. See: <a href=\"https://en.wikipedia.org/wiki/Anti-British_sentiment\">https://en.wikipedia.org/wiki/Anti-British_sentiment</a>"@en ;
    skos:inScheme cwrc:PoliticalAffiliation ;
    prov:derivedFrom dbpedia:Anti-British_sentiment .

cwrc:anti-CapitalPunishment
    void:inDataset cwrc:datasetdefinition ;
    a cwrc:PoliticalAffiliation, skos:Concept ;
    rdf:value "anti-capital-punishment", "opponent of capital punishment" ;
    rdfs:comment "La description de ce terme est basée sur celle de DBPedia."@fr, "The description for this term is indebted to DBpedia."@en ;
    rdfs:isDefinedBy <http://sparql.cwrc.ca/ontologies/cwrc-2017-08-03> ;
    rdfs:label "Peine de mort"@fr, "anti-capital punishment"@en ;
    skos:broaderTransitive cwrc:socialReform ;
    skos:definition "Capital punishment, also known as the death penalty, is a government sanctioned practice whereby a person is put to death by the state as a punishment for a crime. The sentence that someone be punished in such a manner is referred to as a death sentence, whereas the act of carrying out the sentence is known as an execution. Crimes that can result in a death penalty are known as capital crimes or capital offences. The term capital is derived from the Latin capitalis (\"of the head\", referring to execution by beheading). Fifty-eight countries retain capital punishment, 102 countries have completely abolished it de jure for all crimes, six have abolished it for ordinary crimes (while maintaining it for special circumstances such as war crimes), and 32 are abolitionist in practice. Capital punishment is a matter of active controversy in various countries and states, and positions can vary within a single political ideology or cultural region. In the European Union, Article 2 of the Charter of Fundamental Rights of the European Union prohibits the use of capital punishment. Also, the Council of Europe, which has 47 member states, prohibits the use of the death penalty by its members. The United Nations General Assembly has adopted, in 2007, 2008, 2010, 2012 and 2014 non-binding resolutions calling for a global moratorium on executions, with a view to eventual abolition. Although most nations have abolished capital punishment, over 60% of the world's population live in countries where executions take place, such as China, India, the United States and Indonesia. <a href=\"#_dbpedia_2017\">(DBpedia, 2017)</a>"@en, "La peine de mort, ou peine capitale, est une peine prévue par la loi consistant à exécuter une personne ayant été reconnue coupable d'une faute qualifiée de « crime capital ». La sentence est prononcée par l'institution judiciaire à l'issue d'un procès. En l'absence d'un procès, ou dans les cas où celui-ci n'est pas réalisé par une institution reconnue, on parle d'exécution sommaire, d'acte de vengeance ou de justice privée. La peine de mort est diversement considérée selon les époques et les régions géographiques. Elle est prévue dans les textes de loi de 93 pays, mais seuls 22 des 192 pays du globe ont procédé à des exécutions en 2014. Elle est une sanction reconnue bien que réprouvée par les institutions internationales comme l'Organisation des Nations unies (ONU). Les États abolitionnistes sont aujourd'hui majoritaires, mais ils ne représentent encore qu'une minorité de la population mondiale. Parmi les démocraties industrialisées, seules deux la pratiquent : les États-Unis et le Japon. Au plan international, le 18 décembre 2007, l’Assemblée générale de l'ONU a adopté la résolution 62/149 appelant à un moratoire sur les exécutions dans le monde. Cette résolution (comme les autres résolutions de l'ONU) n'a pas de valeur contraignante mais peut être vue comme le signe que la majorité des états souhaite remettre en cause la peine de mort. Cependant huit des dix pays les plus peuplés ont voté contre la résolution. Elle a été renouvelée en 2014. <a href=\"#_dbpedia_2017\">(DBpedia, 2017)</a>"@fr ;
    skos:inScheme cwrc:PoliticalAffiliation ;
    prov:derivedFrom dbpedia:Capital_punishment .

cwrc:anti-Capitalism
    void:inDataset cwrc:datasetdefinition ;
    a cwrc:PoliticalAffiliation, skos:Concept ;
    rdf:value "anti-capitalist" ;
    rdfs:comment "La description de ce terme est basée sur celle de DBPedia."@fr, "The description for this term is indebted to DBpedia."@en ;
    rdfs:isDefinedBy <http://sparql.cwrc.ca/ontologies/cwrc-2017-08-03> ;
    rdfs:label "Anticapitalisme"@fr, "anti-capitalism"@en ;
    skos:definition "Anti-capitalism encompasses a wide variety of movements, ideas and attitudes that oppose capitalism. Anti-capitalists, in the strict sense of the word, are those who wish to replace capitalism with another type of economic system. <a href=\"#_dbpedia_2017\">(DBpedia, 2017)</a>"@en, "L'anticapitalisme regroupe un ensemble de mouvements qui s'opposent au capitalisme. Les aspects visés diffèrent selon les conceptions et peuvent notamment concerner, sans y être limités, le profit et l'importance de l'argent, la spéculation, le salariat, la concurrence économique, les effets considérés comme des effets néfastes du capitalisme sur la société (comme sa supposée « immoralité », ou les inégalités économiques qu'il est censé entraîner), l'environnement, ou les formes sociales de base du capitalisme. Un spectre politique large et très divers s'est réclamé ou se réclame de l'anticapitalisme. <a href=\"#_dbpedia_2017\">(DBpedia, 2017)</a>"@fr ;
    skos:inScheme cwrc:PoliticalAffiliation ;
    skos:related cwrc:communism ;
    prov:derivedFrom dbpedia:Anti-capitalism .

cwrc:anti-Caste
    void:inDataset cwrc:datasetdefinition ;
    a cwrc:PoliticalAffiliation, skos:Concept ;
    rdf:value "worked against the caste system" ;
    rdfs:comment "The description for this term is indebted to DBpedia."@en ;
    rdfs:isDefinedBy <http://sparql.cwrc.ca/ontologies/cwrc-2017-08-03> ;
    rdfs:label ""@fr, "anti-caste movement"@en ;
    skos:broaderTransitive cwrc:feminism, cwrc:socialReform ;
    skos:definition ""@fr, "Advocacy or activism opposing the caste system in India. See <a href=\"https://en.wikipedia.org/wiki/Caste_system_in_India\">https://en.wikipedia.org/wiki/Caste_system_in_India</a>; <a href=\"https://en.wikipedia.org/wiki/Caste_politics\">https://en.wikipedia.org/wiki/Caste_politics</a>; <a href=\"https://en.wikipedia.org/wiki/Dalit\">https://en.wikipedia.org/wiki/Dalit</a>"@en ;
    skos:inScheme cwrc:PoliticalAffiliation ;
    prov:derivedFrom dbpedia:Caste_politics, dbpedia:Caste_system_in_India, dbpedia:Dalit .

cwrc:anti-Catholicism
    void:inDataset cwrc:datasetdefinition ;
    cwrc:contraryTo cwrc:pro-Catholicism ;
    a cwrc:PoliticalAffiliation, skos:Concept ;
    rdf:value "anti-catholic", "anti-catholic-emancipation" ;
    rdfs:comment "La description de ce terme est basée sur celle de DBPedia."@fr, "The description for this term is indebted to DBpedia."@en ;
    rdfs:isDefinedBy <http://sparql.cwrc.ca/ontologies/cwrc-2017-08-03> ;
    rdfs:label "Anticatholicisme"@fr, "anti-catholicism"@en ;
    skos:definition "Anti-Catholicism is hostility towards or opposition to the Catholic Church, its clergy and adherents. After the Reformation and until at least the late 20th Century, majority Protestant states (especially England, Germany, the United States, and Canada) made anti-Catholicism and opposition to the Pope and Catholic rituals major political themes, with anti-Catholic sentiment at times leading to violence and religious discrimination against Catholic individuals (often derogatorily referred to in Anglophone Protestant countries as \"papists\" or \"Romanists\"). Historically, Catholics in Protestant countries were frequently (and almost always baselessly) suspected of conspiring against the state in furtherance of papal interests or to establish a political hegemony under the \"Papacy\", with Protestants sometimes questioning Catholic individuals' loyalty to the state and suspecting Catholics of ultimately maintaining loyalty to the Vatican rather than their domiciled country. In majority Protestant countries with large scale immigration, such as the United States, Canada, and Australia, suspicion or discrimination of Catholic immigrants often overlapped or conflated with nativism, xenophobia, and ethnocentric or racist sentiments (i.e. anti-Italianism, anti-Irish sentiment, hispanophobia, Anti-Quebec sentiment). In the Early modern period, in the face of rising secular powers in Europe, the Catholic Church struggled to maintain its traditional religious and political role in primarily Catholic nations. As a result of these struggles, there arose in some majority Catholic countries (especially among those individuals with certain secular political views) a hostile attitude towards the considerable political, social, spiritual and religious power of the Pope and the clergy in the form of anti-clericalism. <a href=\"#_dbpedia_2017\">(DBpedia, 2017)</a>"@en, "L'anticatholicisme désigne la méfiance, la discrimination, la répression, ou la persécution du catholicisme et des catholiques. <a href=\"#_dbpedia_2017\">(DBpedia, 2017)</a>"@fr ;
    skos:inScheme cwrc:PoliticalAffiliation ;
    prov:derivedFrom dbpedia:Anti-Catholicism .

cwrc:anti-Censorship
    void:inDataset cwrc:datasetdefinition ;
    a cwrc:PoliticalAffiliation, skos:Concept ;
    rdf:value "Freedom of Speech", "anti-censorship", "free speech advocate", "intellectual property activist", "pro free speech", "pro-free speech" ;
    rdfs:comment "The description for this term is indebted to DBpedia."@en ;
    rdfs:isDefinedBy <http://sparql.cwrc.ca/ontologies/cwrc-2017-08-03> ;
    rdfs:label ""@fr, "anti-censorship movement"@en ;
    skos:broaderTransitive cwrc:socialReform ;
    skos:definition ""@fr, "Opposition to censorship. See <a href=\"https://en.wikipedia.org/wiki/Freedom_of_speech\">https://en.wikipedia.org/wiki/Freedom_of_speech</a>"@en ;
    skos:inScheme cwrc:PoliticalAffiliation ;
    skos:related cwrc:anti-Monarchism ;
    prov:derivedFrom dbpedia:Freedom_of_speech .

cwrc:anti-Communism
    void:inDataset cwrc:datasetdefinition ;
    cwrc:contraryTo cwrc:pro-communism ;
    a cwrc:PoliticalAffiliation, skos:Concept ;
    rdf:value "anti-communist" ;
    rdfs:comment "La description de ce terme est basée sur celle de DBPedia."@fr, "The description for this term is indebted to DBpedia."@en ;
    rdfs:isDefinedBy <http://sparql.cwrc.ca/ontologies/cwrc-2017-08-03> ;
    rdfs:label "Anticommunisme"@fr, "anti-communism"@en ;
    skos:definition "Anti-communism is opposition to communism. Organized anti-communism developed in reaction to the rise of communism, especially after the 1917 October Revolution in Russia. It reached global dimensions during the Cold War, when America and the Soviet Union engaged in an intense rivalry. Most modern anti-communists reject the concept of historical materialism, which is a central idea in Marxism. Anti-communists reject the Marxist belief that capitalism will be followed by socialism and communism, just as feudalism was followed by capitalism. Anti-communists question the validity of the Marxist claim that the socialist state will \"wither away\" when it becomes unnecessary in a true communist society. Anti-communists also accuse communists of having caused several famines that occurred in 20th-century communist states, such as the Russian Famine of 1921 and the much more severe famine in China during the Great Leap Forward. Some anti-communists refer to both communism and fascism as totalitarianism, seeing similarity between the actions of communist and fascist governments. Opponents argue that communist parties that have come to power have tended to be rigidly intolerant of political opposition. Communist governments have also been accused of creating a new ruling class (a Nomenklatura), with powers and privileges greater than those previously enjoyed by the upper classes in the non-communist regimes. <a href=\"#_dbpedia_2017\">(DBpedia, 2017)</a>"@en, "Le terme d'anticommunisme englobe, au sens large, l'ensemble des attitudes d'opposition ou d'hostilité envers les aspects théoriques ou pratiques du communisme : l'anticommunisme peut se traduire sous forme de simple prise de position, de discours politique structuré, d'action ou de propagande. Son sens est cependant changeant en fonction de celui du « communisme », mot qui recouvre lui-même un ensemble de réalités très différentes les unes des autres en fonction des contextes sociaux, culturels et politiques. Les facteurs distinguant les différents types d'anticommunisme sont notamment la forme de communisme explicitement visée et les motivations qui poussent à s'opposer au communisme ; le terme « anticommunisme » est employé, selon les époques et les contextes, pour qualifier l'opposition aux théories marxistes ou communistes elles-mêmes, ou aux mouvances et partis politiques s'en réclamant, ou bien à la pratique politique des régimes communistes. Le terme d'« anticommunisme » a pu ainsi être utilisé pour qualifier les opposants au stalinisme, que ces derniers aient été ou non anticommunistes au sens strict. Apparu au XIXe siècle en tant que concept, l'anticommunisme s’est largement développé au cours du XXe siècle, à la suite de la prise du pouvoir par les bolcheviks en Russie en octobre 1917, puis à la création de l’URSS : il s’est alors identifié, pour l'essentiel, à l'opposition aux régimes communistes et aux partis communistes d'inspiration léniniste et stalinienne. Après la Seconde Guerre mondiale, l’anticommunisme devient un élément majeur de la politique étrangère et intérieure des États-Unis, opposés à l'URSS dans le contexte de la guerre froide. <a href=\"#_dbpedia_2017\">(DBpedia, 2017)</a>"@fr ;
    skos:inScheme cwrc:PoliticalAffiliation ;
    prov:derivedFrom dbpedia:Anti-communism .

cwrc:anti-Conscriptionism
    void:inDataset cwrc:datasetdefinition ;
    cwrc:contraryTo cwrc:pro-communism ;
    a cwrc:PoliticalAffiliation, skos:Concept ;
    rdf:value "anti-conscriptionist" ;
    rdfs:comment "The description for this term is indebted to DBpedia."@en ;
    rdfs:isDefinedBy <http://sparql.cwrc.ca/ontologies/cwrc-2017-08-03> ;
    rdfs:label ""@fr, "anti-conscriptionism"@en ;
    skos:definition ""@fr, "Opposition to compulsory enlistment of people in either war or peacetime into a national service, usually military service."@en ;
    skos:inScheme cwrc:PoliticalAffiliation ;
    skos:related cwrc:anti-WarMovement .

cwrc:anti-ContagiousDiseasesAct
    void:inDataset cwrc:datasetdefinition ;
    a cwrc:PoliticalAffiliation, skos:Concept ;
    rdf:value "\"against the Contagious Diseases Acts\" ", "anti-contagious diseases act activist", "anti-contagious diseases acts" ;
    rdfs:comment "The description for this term is indebted to DBpedia."@en ;
    rdfs:isDefinedBy <http://sparql.cwrc.ca/ontologies/cwrc-2017-08-03> ;
    rdfs:label ""@fr, "anti-Contagious Diseases Act"@en ;
    skos:broaderTransitive cwrc:feminism, cwrc:socialReform ;
    skos:definition ""@fr, "Opposition to government regulation of prostitution including the forced physical examination of suspected prostitutes for venereal disease. See: <a href=\"https://en.wikipedia.org/wiki/Contagious_Diseases_Acts\">https://en.wikipedia.org/wiki/Contagious_Diseases_Acts</a>"@en ;
    skos:inScheme cwrc:PoliticalAffiliation ;
    prov:derivedFrom dbpedia:Contagious_Diseases_Acts .

cwrc:anti-CorporalPunishment
    void:inDataset cwrc:datasetdefinition ;
    a cwrc:PoliticalAffiliation, skos:Concept ;
    rdfs:comment "The description for this term is indebted to DBpedia."@en ;
    rdfs:isDefinedBy <http://sparql.cwrc.ca/ontologies/cwrc-2017-08-03> ;
    rdfs:label ""@fr, "anti-corporal punishment"@en ;
    skos:broaderTransitive cwrc:socialReform ;
    skos:definition ""@fr, "Campaigns against corporal punishment aim to reduce or eliminate corporal punishment of minors by instigating legal and cultural changes in the areas where such punishments are practiced. Such campaigns date mostly from the late 20th century, although occasional voices in opposition to corporal punishment existed from ancient times through to the modern era. The UN Committee on the Rights of the Child defines \"corporal punishment\" as: any punishment in which physical force is used and intended to cause some degree of pain or discomfort, however light. Most involves hitting (\"smacking\", \"slapping\", \"spanking\") children, with the hand or with an implement – whip, stick, belt, shoe, wooden spoon, etc. But it can also involve, for example, kicking, shaking or throwing children, scratching, pinching, biting, pulling hair or boxing ears, forcing children to stay in uncomfortable positions, burning, scalding or forced ingestion. <a href=\"#_dbpedia_2017\">(DBpedia, 2017)</a>"@en ;
    skos:inScheme cwrc:PoliticalAffiliation ;
    prov:derivedFrom dbpedia:Campaigns_against_corporal_punishment .

cwrc:anti-European
    void:inDataset cwrc:datasetdefinition ;
    a cwrc:PoliticalAffiliation, skos:Concept ;
    rdfs:comment "The description for this term is indebted to DBpedia."@en ;
    rdfs:isDefinedBy <http://sparql.cwrc.ca/ontologies/cwrc-2017-08-03> ;
    rdfs:label ""@fr, "anti-European politics"@en ;
    skos:definition ""@fr, "Opposed to the existence, policies, or influence of the European Union. On Euroskepticism, see <a href=\"https://en.wikipedia.org/wiki/Euroscepticism\">https://en.wikipedia.org/wiki/Euroscepticism</a>"@en ;
    skos:inScheme cwrc:PoliticalAffiliation ;
    prov:derivedFrom dbpedia:Euroscepticism .

cwrc:anti-Fascism
    void:inDataset cwrc:datasetdefinition ;
    cwrc:contraryTo cwrc:facism ;
    a cwrc:PoliticalAffiliation, skos:Concept ;
    rdf:value "anti-fascist", "anti-nazi" ;
    rdfs:comment "La description de ce terme est basée sur celle de DBPedia."@fr, "The description for this term is indebted to DBpedia."@en ;
    rdfs:isDefinedBy <http://sparql.cwrc.ca/ontologies/cwrc-2017-08-03> ;
    rdfs:label "Antifascisme"@fr, "anti-fascism"@en ;
    skos:definition "Anti-fascism is opposition to fascist ideologies, groups and individuals. The anti-fascist movement began in a few European countries in the 1920s, and eventually spread to other countries around the world. <a href=\"#_dbpedia_2017\">(DBpedia, 2017)</a>"@en, "L'antifascisme est l'opposition organisée au fascisme et, plus largement, à l'extrême droite. Il prend forme dans les années 1920 et se développe conséquemment à la montée du fascisme en Europe. Il a connu un très fort développement au cours des années 1930, étant à l'origine de la formation des Fronts populaires , puis pendant la Seconde Guerre mondiale au sein des résistances contre les dictatures fascistes et nazies ainsi que les régimes de collaboration. L'antifascisme peut désigner dans une acception plus large une idéologie tendant à s'opposer également à la droite dite « dure ». Certains historiens reprochent à l'antifascisme d'avoir été instrumentalisé par le mouvement communiste. <a href=\"#_dbpedia_2017\">(DBpedia, 2017)</a>"@fr ;
    skos:inScheme cwrc:PoliticalAffiliation ;
    skos:related cwrc:anti-Antisemitism ;
    prov:derivedFrom dbpedia:Anti-fascism .

cwrc:anti-Federalism
    void:inDataset cwrc:datasetdefinition ;
    a cwrc:PoliticalAffiliation, skos:Concept ;
    rdf:value "anti-federalist" ;
    rdfs:comment "La description de ce terme est basée sur celle de DBPedia."@fr, "The description for this term is indebted to DBpedia."@en ;
    rdfs:isDefinedBy <http://sparql.cwrc.ca/ontologies/cwrc-2017-08-03> ;
    rdfs:label "Antifédéralisme"@fr, "anti-federalism"@en ;
    skos:definition "Anti-Federalism refers to a movement that opposed the creation of a stronger U.S. federal government and which later opposed the ratification of the 1787 Constitution. The previous constitution, called the Articles of Confederation, gave state governments more authority. Led by Patrick Henry of Virginia, Anti-Federalists worried, among other things, that the position of president, then a novelty, might evolve into a monarchy. <a href=\"#_dbpedia_2017\">(DBpedia, 2017)</a>"@en, """Antifédéralisme fut le nom donné à deux mouvements politiques distincts à la fin du XVIIIe siècle aux États-Unis: 
  *  Le premier mouvement antifédéraliste des années 1780, s'opposa à la création d'un gouvernement national plus fort, tel que le permettait la Constitution et chercha à le conserver tel qu'il était institué dans les Articles de la Confédération de 1777. 
  *  Le second mouvement antifédéraliste se constitua en réaction aux lois fiscales d'Alexander Hamilton lors du premier mandat de George Washington. Ce mouvement est parfois nommé l'Anti-Administration Party qui deviendra plus tard le Parti républicain-démocrate de Thomas Jefferson et James Madison. <a href=\"#_dbpedia_2017\">(DBpedia, 2017)</a>"""@fr ;
    skos:inScheme cwrc:PoliticalAffiliation ;
    prov:derivedFrom dbpedia:Anti-Federalism .

cwrc:anti-Feminism
    void:inDataset cwrc:datasetdefinition ;
    cwrc:contraryTo cwrc:feminism ;
    a cwrc:PoliticalAffiliation, skos:Concept ;
    rdf:value "anti-feminist", "anti-women's liberation", "antifeminist", "gender conservative", "misogynist", "non-feminist" ;
    rdfs:comment "La description de ce terme est basée sur celle de DBPedia."@fr, "The description for this term is indebted to DBpedia."@en ;
    rdfs:isDefinedBy <http://sparql.cwrc.ca/ontologies/cwrc-2017-08-03> ;
    rdfs:label "Antiféminisme"@fr, "anti-feminism"@en ;
    skos:definition "Antifeminism is criticism of some or all feminist ideology, arguing that modern feminism is not practiced in ways that promote true gender equality. This opposition has taken various forms across time and cultures. For example, antifeminists in the late 1800s and early 1900s resisted women's suffrage, while antifeminists in the late 20th century opposed the Equal Rights Amendment. Antifeminism may be motivated by the belief that feminist theories of patriarchy and disadvantages suffered by women in modern society are mischaracterized or exaggerated; that feminism as a movement encourages misandry and results in harm or oppression of men; or driven by general opposition towards women's rights. <a href=\"#_dbpedia_2017\">(DBpedia, 2017)</a>"@en, "L'antiféminisme est un néologisme qualifiant des critiques ou une opposition aux mouvements ou aux thèses féministes, pour des raisons politiques, philosophiques, religieuses, sociologiques ou culturelles. Il s'applique soit à la lutte contre l'émancipation féminine, soit au refus des thèses d'un ou plusieurs mouvements se disant « féministes ». <a href=\"#_dbpedia_2017\">(DBpedia, 2017)</a>"@fr ;
    skos:inScheme cwrc:PoliticalAffiliation ;
    prov:derivedFrom dbpedia:Antifeminism .

cwrc:anti-Globalism
    void:inDataset cwrc:datasetdefinition ;
    a cwrc:PoliticalAffiliation, skos:Concept ;
    rdf:value "anti-globalist" ;
    rdfs:comment "La description de ce terme est basée sur celle de DBPedia."@fr, "The description for this term is indebted to DBpedia."@en ;
    rdfs:isDefinedBy <http://sparql.cwrc.ca/ontologies/cwrc-2017-08-03> ;
    rdfs:label "Mouvement antimondialisation"@fr, "anti-globalism"@en ;
    skos:definition "Le mouvement antimondialisation désigne le mouvement d'opposition à la mondialisation. <a href=\"#_dbpedia_2017\">(DBpedia, 2017)</a>"@fr, "The anti-globalization movement, or counter-globalisation movement, is a social movement critical of the globalization of corporate capitalism. The movement is also commonly referred to as the global justice movement, alter-globalization movement, anti-globalist movement, anti-corporate globalization movement, or movement against neoliberal globalization. Participants base their criticisms on a number of related ideas. What is shared is that participants oppose what they see as large, multi-national corporations having unregulated political power, exercised through trade agreements and deregulated financial markets. Specifically, corporations are accused of seeking to maximize profit at the expense of work safety conditions and standards, labor hiring and compensation standards, environmental conservation principles, and the integrity of national legislative authority, independence and sovereignty. As of January 2012, some commentators have characterized the unprecedented changes in the global economy as \"turbo-capitalism\" (Edward Luttwak), \"market fundamentalism\" (George Soros), \"casino capitalism\" (Susan Strange), and as \"McWorld\" (Benjamin Barber). Many anti-globalization activists call for forms of global integration that better provide democratic representation, advancement of human rights, fair trade and sustainable development and therefore feel the term \"anti-globalization\" is misleading. <a href=\"#_dbpedia_2017\">(DBpedia, 2017)</a>"@en ;
    skos:inScheme cwrc:PoliticalAffiliation ;
    prov:derivedFrom dbpedia:Anti-globalization_movement .

cwrc:anti-Imperialism
    void:inDataset cwrc:datasetdefinition ;
    cwrc:contraryTo cwrc:imperialism ;
    a cwrc:PoliticalAffiliation, skos:Concept ;
    rdf:value "anti-colonial", "anti-colonialism", "anti-colonialist", "anti-imperial", "anti-imperialist" ;
    rdfs:comment "La description de ce terme est basée sur celle de DBPedia."@fr, "The description for this term is indebted to DBpedia."@en ;
    rdfs:isDefinedBy <http://sparql.cwrc.ca/ontologies/cwrc-2017-08-03> ;
    rdfs:label "Anti-impérialisme"@fr, "anti-imperialism"@en ;
    skos:broaderTransitive cwrc:humanRights ;
    skos:definition "\"Anti-imperialism\" in political science and international relations is a term used in a variety of contexts, usually by nationalist movements, who want to secede from a larger polity (usually in the form of an empire, but also in a multi-ethnic sovereign state) or as a specific theory opposed to capitalism in Marxist–Leninist discourse, derived from Vladimir Lenin's work Imperialism, the Highest Stage of Capitalism. A less common usage is by isolationists who oppose an interventionist foreign policy. People who categorise themselves as anti-imperialists, often state that they are opposed to colonialism, colonial empire, hegemony, imperialism, and territorial expansion of a country beyond its established borders. The phrase gained a wide currency after the Second World War and at the onset of the Cold War as political movements in colonies of European powers promoted national sovereignty. Some \"anti-imperialist\" groups who opposed the United States supported the power of the Soviet Union, such as in Guevarism, while in Maoism, this was criticized as \"social imperialism\". In the Arab and Muslim world, the term is often used in the context of Anti-Zionist nationalist and religious movements. <a href=\"#_dbpedia_2017\">(DBpedia, 2017)</a>"@en, "L'anti-impérialisme est une idéologie d’opposition à l'impérialisme, c'est-à-dire la doctrine d'un État ou un groupe d'États à mettre un autre État ou un groupe d'États plus faible sous sa dépendance politique, économique et culturelle par la conquête militaire ou toute autre forme de coercition. Cette idéologie est corollaire au processus de décolonisation, aux mouvements de libération nationale et, dans une certaine mesure, au nationalisme. Bien que le terme impérialisme est utilisé la langue française au cours XIXe siècle pour désigner l'appui au régime napoléonien et le « système de gouvernement et de domination de l'Empire romain », l'anti-impérialisme prend son origine durant la seconde moitié de XIXe siècle de l'anglais imperialism qui désigne d'abord la politique d'extension coloniale de l'Empire britannique sous le premier ministre britannique Benjamin Disraeli au cours des années 1870. Le concept sera approfondi par John Atkinson Hobson en 1902 dans son livre Imperialism: A Study. L'anti-impérialisme est aussi une notions cruciale du marxisme-léninisme. Le concept, qui diffère de l'usage commun, est approfondi dans le livre de 1917 L'Impérialisme, stade suprême du capitalisme de Lénine entre autres. Dans la théorie marxiste, l'impérialisme est un stade du capitalisme au cours duquel le capital financier supplante toutes les autres formes du capital. L'anti-impérialisme a été l'un des principales politique de l'URSS, de la République populaire de Chine, de Cuba et des autres pays communistes depuis la seconde moitié du XXe siècle. La fin du XXe siècle sous l'hégémonie des États-Unis voit la naissance d'un nouvel impérialisme . L'anti-impérialisme, dans ces circonstances, est une part intégrante du mouvement altermondialiste qui s'oppose à la mondialisation libérale et aux grands accords de libre-échange et du mouvement pacifiste qui s'oppose aux invasions militaires. <a href=\"#_dbpedia_2017\">(DBpedia, 2017)</a>"@fr ;
    skos:inScheme cwrc:PoliticalAffiliation ;
    skos:related cwrc:anti-British ;
    prov:derivedFrom dbpedia:Anti-imperialism .

cwrc:anti-Jacobin
    void:inDataset cwrc:datasetdefinition ;
    a cwrc:PoliticalAffiliation, skos:Concept ;
    rdf:value "anti-revolutionary" ;
    rdfs:comment "The description for this term is indebted to DBpedia."@en ;
    rdfs:isDefinedBy <http://sparql.cwrc.ca/ontologies/cwrc-2017-08-03> ;
    rdfs:label ""@fr, "anti-Jacobin"@en ;
    skos:definition ""@fr, "Opposed to Jacobinism. See <a href=\"https://en.wikipedia.org/wiki/Jacobin\">https://en.wikipedia.org/wiki/Jacobin</a>"@en ;
    skos:inScheme cwrc:PoliticalAffiliation ;
    prov:derivedFrom dbpedia:Jacobin .

cwrc:anti-Jacobite
    void:inDataset cwrc:datasetdefinition ;
    cwrc:contraryTo cwrc:jacobitism ;
    a cwrc:PoliticalAffiliation, skos:Concept ;
    rdfs:comment "The description for this term is indebted to DBpedia."@en ;
    rdfs:isDefinedBy <http://sparql.cwrc.ca/ontologies/cwrc-2017-08-03> ;
    rdfs:label ""@fr, "anti-Jacobite"@en ;
    skos:definition ""@fr, "Opposed to Jacobitism. See <a href=\"https://en.wikipedia.org/wiki/Jacobitism\">https://en.wikipedia.org/wiki/Jacobitism</a>"@en ;
    skos:inScheme cwrc:PoliticalAffiliation ;
    prov:derivedFrom dbpedia:Jacobitism .

cwrc:anti-LandLeague
    void:inDataset cwrc:datasetdefinition ;
    a cwrc:PoliticalAffiliation, skos:Concept ;
    rdfs:comment "The description for this term is indebted to DBpedia."@en ;
    rdfs:isDefinedBy <http://sparql.cwrc.ca/ontologies/cwrc-2017-08-03> ;
    rdfs:label ""@fr, "anti-Irish National Land League"@en ;
    skos:definition ""@fr, "Opposed to the Irish Land League movement. See <a href=\"https://en.wikipedia.org/wiki/Irish_National_Land_League\">https://en.wikipedia.org/wiki/Irish_National_Land_League</a>"@en ;
    skos:inScheme cwrc:PoliticalAffiliation ;
    skos:related cwrc:irishUnionism ;
    prov:derivedFrom dbpedia:Irish_National_Land_League .

cwrc:anti-Monarchism
    void:inDataset cwrc:datasetdefinition ;
    cwrc:contraryTo cwrc:monarchism ;
    a cwrc:PoliticalAffiliation, skos:Concept ;
    rdf:value "anti-monarchist" ;
    rdfs:comment "The description for this term is indebted to DBpedia."@en ;
    rdfs:isDefinedBy <http://sparql.cwrc.ca/ontologies/cwrc-2017-08-03> ;
    rdfs:label ""@fr, "anti-monarchism"@en ;
    skos:definition ""@fr, "The abolition of monarchy has occurred throughout history, either through revolutions, coups d'état, wars, or legislative reforms (such as abdications). The founding of the Roman Republic is a noteworthy example and became part of the nation's traditions including as justification for the assassination of Julius Caesar. The twentieth century saw a major acceleration of this process, with many monarchies violently overthrown by revolution or war, or else abolished as part of the process of decolonisation. By contrast, the restoration of monarchies is rare in modern times, with only two major examples, Spain and Cambodia. <a href=\"#_dbpedia_2017\">(DBpedia, 2017)</a>"@en ;
    skos:inScheme cwrc:PoliticalAffiliation ;
    prov:derivedFrom dbpedia:Abolition_of_monarchy .

cwrc:anti-NuclearMovement
    void:inDataset cwrc:datasetdefinition ;
    a cwrc:PoliticalAffiliation, skos:Concept ;
    rdf:value "Campaign for Nuclear Disarmament", "anti-nuclear", "anti-nuclear activist", "anti-nuclear war", "anti-nuclear weapons", "nuclear disarmament", "nuclear disarmament campaigner", "pro nuclear disarmament" ;
    rdfs:comment "La description de ce terme est basée sur celle de DBPedia."@fr, "The description for this term is indebted to DBpedia."@en ;
    rdfs:isDefinedBy <http://sparql.cwrc.ca/ontologies/cwrc-2017-08-03> ;
    rdfs:label "Mouvement antinucléaire"@fr, "anti-nuclear movement"@en ;
    skos:definition "Le mouvement antinucléaire désigne l'ensemble des personnes et organisations (associations, syndicats, partis politiques) qui s'opposent de façon générale à l'utilisation de l'énergie nucléaire. Cette opposition peut s'étendre de la bombe atomique aux armes utilisant l’uranium appauvri, jusqu'à la production d’électricité d’origine nucléaire, l’irradiation des aliments et l’utilisation de la radioactivité. Les opposants au nucléaire soutiennent qu'il existe des solutions alternatives, telles que les économies d'énergie ou les énergies renouvelables et que l'uranium est, de même que les énergies fossiles, une source d'énergie dont l'épuisement est attendu dans quelques décennies. Il existe aussi une opposition spécifique à l'arme nucléaire, que l'on peut qualifier de « mouvement antinucléaire militaire ». Les opposants au nucléaire soutiennent notamment qu'il existe des liens étroits entre le nucléaire civil et militaire, et que le nucléaire civil a une responsabilité lourde dans la prolifération nucléaire. <a href=\"#_dbpedia_2017\">(DBpedia, 2017)</a>"@fr, "The anti-nuclear movement is a social movement that opposes various nuclear technologies. Some direct action groups, environmental groups, and professional organisations have identified themselves with the movement at the local, national, and international level. Major anti-nuclear groups include Campaign for Nuclear Disarmament, Friends of the Earth, Greenpeace, International Physicians for the Prevention of Nuclear War, and the Nuclear Information and Resource Service. The initial objective of the movement was nuclear disarmament, though since the late 1960s opposition has included the use of nuclear power. Many anti-nuclear groups oppose both nuclear power and nuclear weapons. The formation of green parties in the 1970s and 1980s was often a direct result of anti-nuclear politics. Scientists and diplomats have debated nuclear weapons policy since before the atomic bombings of Hiroshima and Nagasaki in 1945. The public became concerned about nuclear weapons testing from about 1954, following extensive nuclear testing in the Pacific. In 1963, many countries ratified the Partial Test Ban Treaty which prohibited atmospheric nuclear testing. Some local opposition to nuclear power emerged in the early 1960s, and in the late 1960s some members of the scientific community began to express their concerns. In the early 1970s, there were large protests about a proposed nuclear power plant in Wyhl, West Germany. The project was cancelled in 1975 and anti-nuclear success at Wyhl inspired opposition to nuclear power in other parts of Europe and North America. Nuclear power became an issue of major public protest in the 1970s. A protest against nuclear power occurred in July 1977 in Bilbao, Spain, with up to 200,000 people in attendance. Following the Three Mile Island accident in 1979, an anti-nuclear protest was held in New York City, involving 200,000 people. In 1981, Germany's largest anti-nuclear power demonstration took place to protest against the Brokdorf Nuclear Power Plant west of Hamburg; some 100,000 people came face to face with 10,000 police officers. The largest protest was held on June 12, 1982, when one million people demonstrated in New York City against nuclear weapons. A 1983 nuclear weapons protest in West Berlin had about 600,000 participants. In May 1986, following the Chernobyl disaster, an estimated 150,000 to 200,000 people marched in Rome to protest against the Italian nuclear program. In the US, public opposition preceded the shutdown of the Shoreham, Yankee Rowe, Millstone 1, Rancho Seco, Maine Yankee, and many other nuclear power plants. For many years after the 1986 Chernobyl disaster nuclear power was off the policy agenda in most countries, and the anti-nuclear power movement seemed to have won its case. Some anti-nuclear groups disbanded. In the 2000s (decade), however, following public relations activities by the nuclear industry, advances in nuclear reactor designs, and concerns about climate change, nuclear power issues came back into energy policy discussions in some countries. The 2011 Japanese nuclear accidents subsequently undermined the nuclear power industry's proposed renaissance and revived nuclear opposition worldwide, putting governments on the defensive. As of 2016, countries such as Australia, Austria, Denmark, Greece, Malaysia, New Zealand, and Norway have no nuclear power stations and remain opposed to nuclear power. Germany, Italy, Spain, Sweden and Switzerland are phasing-out nuclear power.Globally, more nuclear power reactors have closed than opened in recent years. <a href=\"#_dbpedia_2017\">(DBpedia, 2017)</a>"@en ;
    skos:inScheme cwrc:PoliticalAffiliation ;
    prov:derivedFrom dbpedia:Anti-nuclear_movement .

cwrc:anti-Pacifism
    void:inDataset cwrc:datasetdefinition ;
    cwrc:contraryTo cwrc:pacifism ;
    a cwrc:PoliticalAffiliation, skos:Concept ;
    rdf:value "anti-appeasement", "conscriptionist", "war supporter" ;
    rdfs:comment "The description for this term is indebted to DBpedia."@en ;
    rdfs:isDefinedBy <http://sparql.cwrc.ca/ontologies/cwrc-2017-08-03> ;
    rdfs:label ""@fr, "anti-pacifism"@en ;
    skos:definition ""@fr, "Opposed to pacifism. See <a href=\"https://en.wikipedia.org/wiki/Pacifism\">https://en.wikipedia.org/wiki/Pacifism</a>"@en ;
    skos:inScheme cwrc:PoliticalAffiliation ;
    prov:derivedFrom dbpedia:Pacifism .

cwrc:anti-PovertyMovement
    void:inDataset cwrc:datasetdefinition ;
    a cwrc:PoliticalAffiliation, skos:Concept ;
    rdf:value "anti-poverty activist", "anti-poverty movement", "poverty activist" ;
    rdfs:comment "The description for this term is indebted to DBpedia."@en ;
    rdfs:isDefinedBy <http://sparql.cwrc.ca/ontologies/cwrc-2017-08-03> ;
    rdfs:label ""@fr, "anti-poverty movement"@en ;
    skos:definition ""@fr, "Advocacy or activism to reduce poverty. See <a href=\"https://en.wikipedia.org/wiki/Poverty_reduction\">https://en.wikipedia.org/wiki/Poverty_reduction</a>"@en ;
    skos:inScheme cwrc:PoliticalAffiliation ;
    prov:derivedFrom dbpedia:Poverty_reduction .

cwrc:anti-Racism
    void:inDataset cwrc:datasetdefinition ;
    a cwrc:PoliticalAffiliation, skos:Concept ;
    rdf:value "anti-racist" ;
    rdfs:comment "La description de ce terme est basée sur celle de DBPedia."@fr, "The description for this term is indebted to DBpedia."@en ;
    rdfs:isDefinedBy <http://sparql.cwrc.ca/ontologies/cwrc-2017-08-03> ;
    rdfs:label "Antiracisme"@fr, "anti-racism"@en ;
    skos:definition "Anti-racism includes beliefs, actions, movements, and policies adopted or developed to oppose racism. In general, anti-racism is intended to promote an egalitarian society in which people do not face discrimination on the basis of their race, however defined. By its nature, anti-racism tends to promote the view that racism in a particular society is both pernicious and socially pervasive, and that particular changes in political, economic, and/or social life are required to eliminate it. <a href=\"#_dbpedia_2017\">(DBpedia, 2017)</a>"@en, "L'antiracisme inclut les opinions, actions, mouvements et les politiques adoptées ou développée pour s'opposer au racisme. En général l'antiracisme promeut une société dans laquelle les individus ne subissent pas de discrimination sur la base de leur ethnie dont la définition peut varier. De par sa nature, l'antiracisme avance la vision que le racisme dans une société est à la fois pernicieux et socialement pénalisant et que des changements politiques, économiques et/ou sociaux sont nécessaires pour l'éradiquer. La notion d'antiracisme, tout comme les acteurs de la lutte dite antiraciste, ont été critiqués par certains intellectuels notamment pour sa faiblesse conceptuelle, ses utilisations politiques, voire paradoxalement par la réintroduction de la notion de race au sein du débat national. <a href=\"#_dbpedia_2017\">(DBpedia, 2017)</a>"@fr ;
    skos:inScheme cwrc:PoliticalAffiliation ;
    prov:derivedFrom dbpedia:Anti-racism .

cwrc:anti-Socialism
    void:inDataset cwrc:datasetdefinition ;
    cwrc:contraryTo cwrc:socialism ;
    a cwrc:PoliticalAffiliation, skos:Concept ;
    rdf:value "anti-socialist" ;
    rdfs:comment "La description de ce terme est basée sur celle de DBPedia."@fr, "The description for this term is indebted to DBpedia."@en ;
    rdfs:isDefinedBy <http://sparql.cwrc.ca/ontologies/cwrc-2017-08-03> ;
    rdfs:label "Critiques du socialisme"@fr, "anti-socialism"@en ;
    skos:definition "Criticism of socialism refers to any critique of socialist models of economic organization and their feasibility; as well as the political and social implications of adopting such a system. Some criticisms are not directed toward socialism as a system, but are directed toward the socialist movement, socialist political parties or existing socialist states. Some critics consider socialism to be a purely theoretical concept that should be criticized on theoretical grounds (such as in the Socialist calculation debate); others hold that certain historical examples exist and that they can be criticized on practical grounds. Economic liberals and right libertarians view private ownership of the means of production and the market exchange as natural entities or moral rights which are central to their conceptions of freedom and liberty, and view the economic dynamics of capitalism as immutable and absolute. Therefore, they perceive public ownership of the means of production, cooperatives and economic planning as infringements upon liberty. According to the Austrian school economist Ludwig von Mises, an economic system that does not utilize money, financial calculation and market pricing will be unable to effectively value capital goods and coordinate production, and therefore socialism is impossible because it lacks the necessary information to perform economic calculation in the first place. Another central argument leveled against socialist systems based on economic planning is based on the use of dispersed knowledge. Socialism is unfeasible in this view because information cannot be aggregated by a central body and effectively used to formulate a plan for an entire economy, because doing so would result in distorted or absent price signals. Many economic criticisms of socialism focus on the experiences of Soviet-type planned economies. It is argued that a lack of budget constraints in enterprises operating in a planned economy reduces incentives for enterprises to act on information efficiently, thereby reducing overall welfare for society. Other economists criticize models of socialism based on neoclassical economics for their reliance on the faulty and unrealistic assumptions of economic equilibrium and pareto efficiency. Some philosophers have also criticized the aims of socialism, arguing that equality erodes away at individual diversities, and that the establishment of an equal society would have to entail strong coercion. Critics of the socialist political movement often criticize the internal conflicts of the socialist movement as creating a sort of \"responsibility void.\" Because there are many models of socialism, most critiques are only focused on a specific type of socialism. Therefore, the criticisms presented below may not apply to all forms of socialism, and many will focus on the experience of Soviet-type economies. It is also important to note that different models of socialism conflict with each other over questions of property ownership, economic coordination and how socialism is to be achieved - so critics of specific models of socialism might be advocates of a different type of socialism. <a href=\"#_dbpedia_2017\">(DBpedia, 2017)</a>"@en, "Les critiques du socialisme se réfèrent aux critiques des modèles socialistes d'organisation économique, de leurs efficacités et de leurs faisabilités, ainsi que des implications politiques et sociales de tels systèmes. Certaines critiques ne sont pas dirigées vers le socialisme en tant que système, mais sont dirigés vers des mouvements socialistes, des partis politiques socialistes ou des états socialistes existants. Certaines critiques considèrent le socialisme comme un concept purement théorique qui doit être critiqué pour des raisons théoriques, d'autres soutiennent que les expériences socialistes peuvent être critiquées sur les faits. Certains encore veulent englober plusieurs exemples historiques d'États communistes dans une forme de socialisme.Le socialisme est donc une notion large, certaines critiques présentées dans cet article ne s'appliqueront qu'a un modèle spécifique du socialisme qui peuvent différer considérablement des autres types de socialisme. Les libéraux économiques, libertariens, pro-capitalistes et quelques libéraux classiques considèrent l'entreprise privée, la propriété privée des moyens de production et l'échange sur le marché comme des phénomènes naturels ou moraux[pas clair], au centre de leurs conceptions de la liberté. Et par opposition, les membres de ces trois groupes peuvent percevoir la propriété publique des moyens de production, des coopératives et de la planification économique parrainé par l'État comme des atteintes à la liberté[pas clair]. Les membres de l'école néoclassique d'économie critiquent les théories socialistes qui favorisent la participation de l'État ou de la centralisation du capital sur les motifs du manque de motivation au sein des institutions de l'État d'agir sur l'information aussi efficacement que les gestionnaires dans les entreprises capitalistes parce qu'ils n'ont pas de forte contrainte (profit et mécanisme de perte), ce qui réduit le bien-être économique global pour la société. Les membres de l'école autrichienne d'économie soutiennent que les systèmes socialistes basé sur la planification économique sont impossibles parce qu'ils n'ont pas l'information pour effectuer le calcul économique en premier lieu en raison d'un manque de prix libre, qu'ils croient nécessaires pour rationnelle calcul économique. Les membres du mouvement politique socialiste critiquent souvent les conflits internes du mouvement socialiste en créant une sorte de « vide de responsabilité ». <a href=\"#_dbpedia_2017\">(DBpedia, 2017)</a>"@fr ;
    skos:inScheme cwrc:PoliticalAffiliation ;
    prov:derivedFrom dbpedia:Criticisms_of_socialism .

cwrc:anti-Suffrage
    void:inDataset cwrc:datasetdefinition ;
    cwrc:contraryTo cwrc:suffrage ;
    a cwrc:PoliticalAffiliation, skos:Concept ;
    rdf:value "anti-sufffragist", "anti-suffragist" ;
    rdfs:comment "The description for this term is indebted to DBpedia."@en ;
    rdfs:isDefinedBy <http://sparql.cwrc.ca/ontologies/cwrc-2017-08-03> ;
    rdfs:label ""@fr, "anti-suffrage"@en ;
    skos:definition ""@fr, "Anti-suffragism was a political movement composed mainly of women, begun in the late 19th century in order to campaign against women's suffrage in Great Britain and the United States. It was closely associated with \"domestic feminism\", the belief that women had the right to complete freedom within the home. <a href=\"#_dbpedia_2017\">(DBpedia, 2017)</a>"@en ;
    skos:inScheme cwrc:PoliticalAffiliation ;
    prov:derivedFrom dbpedia:Anti-suffragism .

cwrc:anti-Trade-Unionism
    void:inDataset cwrc:datasetdefinition ;
    cwrc:contraryTo cwrc:labourMouvement ;
    a cwrc:PoliticalAffiliation, skos:Concept ;
    rdf:value "anti-trade-unionist" ;
    rdfs:comment "The description for this term is indebted to DBpedia."@en ;
    rdfs:isDefinedBy <http://sparql.cwrc.ca/ontologies/cwrc-2017-08-03> ;
    rdfs:label ""@fr, "anti-trade-unionism"@en ;
    skos:definition ""@fr, "Opposed to trade unions or the trade union movement. See. <a href=\"https://en.wikipedia.org/wiki/Trade_union\">https://en.wikipedia.org/wiki/Trade_union</a>"@en ;
    skos:inScheme cwrc:PoliticalAffiliation ;
    prov:derivedFrom dbpedia:Trade_union .

cwrc:anti-Urbanism
    void:inDataset cwrc:datasetdefinition ;
    a cwrc:PoliticalAffiliation, skos:Concept ;
    rdf:value "pro-countryside" ;
    rdfs:comment "The description for this term is indebted to DBpedia."@en ;
    rdfs:isDefinedBy <http://sparql.cwrc.ca/ontologies/cwrc-2017-08-03> ;
    rdfs:label "anti-urbanism"@en, "antiurbain"@fr ;
    skos:definition "Anti-urbanism is hostility toward the city as opposed to the country, a simple rejection of the city, or a wish to destroy the city. <a href=\"#_dbpedia_2017\">(DBpedia, 2017)</a>"@en, "L’antiurbain est l’hostilité à l’égard de la ville par opposition à la campagne, un rejet pur et simple, une volonté de détruire la ville.  <a href=\"#_dbpedia_2017\">(DBpedia, 2017)</a>"@fr ;
    skos:inScheme cwrc:PoliticalAffiliation ;
    prov:derivedFrom dbpedia:Anti-urbanism .

cwrc:anti-Vaccination
    void:inDataset cwrc:datasetdefinition ;
    a cwrc:PoliticalAffiliation, skos:Concept ;
    rdf:value "movement against compulsory vaccination" ;
    rdfs:comment "The description for this term is indebted to DBpedia."@en ;
    rdfs:isDefinedBy <http://sparql.cwrc.ca/ontologies/cwrc-2017-08-03> ;
    rdfs:label ""@fr, "anti-vaccination movement"@en ;
    skos:definition ""@fr, "Opposition to vaccination, usually compulsory vaccination. See <a href=\"https://en.wikipedia.org/wiki/Vaccine_controversies\">https://en.wikipedia.org/wiki/Vaccine_controversies</a>Also see: <a href=\"https://en.wikipedia.org/wiki/Category:Vaccine_controversies\">https://en.wikipedia.org/wiki/Category:Vaccine_controversies</a>"@en ;
    skos:inScheme cwrc:PoliticalAffiliation ;
    prov:derivedFrom <http://dbpedia.org/resource/Category:Vaccine_controversies>, dbpedia:Vaccine_controversies .

cwrc:anti-Vivisection
    void:inDataset cwrc:datasetdefinition ;
    a cwrc:PoliticalAffiliation, skos:Concept ;
    rdf:value "anti-vivisectionist" ;
    rdfs:comment "The description for this term is indebted to DBpedia."@en ;
    rdfs:isDefinedBy <http://sparql.cwrc.ca/ontologies/cwrc-2017-08-03> ;
    rdfs:label ""@fr, "anti-vivisection"@en ;
    skos:definition ""@fr, "Opposition to experimentation and testing on live animals. See <a href=\"https://en.wikipedia.org/wiki/Category:Anti-vivisection_movement\">https://en.wikipedia.org/wiki/Category:Anti-vivisection_movement</a>Also see <a href=\"https://en.wikipedia.org/wiki/Vivisection\">https://en.wikipedia.org/wiki/Vivisection</a>"@en ;
    skos:inScheme cwrc:PoliticalAffiliation ;
    prov:derivedFrom <http://dbpedia.org/resource/Category:Anti-vivisection_movement>, dbpedia:Vivisection .

cwrc:anti-War
    void:inDataset cwrc:datasetdefinition ;
    a cwrc:PoliticalAffiliation, skos:Concept ;
    rdf:value "anti Vietnam war", "anti-militarism", "anti-militaristic", "anti-war", "anti-war activism", "vietnam war protester" ;
    rdfs:comment "La description de ce terme est basée sur celle de DBPedia."@fr, "The description for this term is indebted to DBpedia."@en ;
    rdfs:isDefinedBy <http://sparql.cwrc.ca/ontologies/cwrc-2017-08-03> ;
    rdfs:label "Antiguerre"@fr, "anti-war movement"@en ;
    skos:broaderTransitive cwrc:pacifism ;
    skos:definition "An anti-war movement (also antiwar) is a social movement, usually in opposition to a particular nation's decision to start or carry on an armed conflict, unconditional of a maybe-existing just cause. The term can also refer to pacifism, which is the opposition to all use of military force during conflicts. Many activists distinguish between anti-war movements and peace movements. Anti-war activists work through protest and other grassroots means to attempt to pressure a government (or governments) to put an end to a particular war or conflict. <a href=\"#_dbpedia_2017\">(DBpedia, 2017)</a>"@en, "Le mouvement antiguerre est un mouvement social[réf. nécessaire] s'opposant aux conflits armés. <a href=\"#_dbpedia_2017\">(DBpedia, 2017)</a>"@fr ;
    skos:inScheme cwrc:PoliticalAffiliation ;
    prov:derivedFrom dbpedia:Anti-war_movement .

cwrc:anti-Zionism
    void:inDataset cwrc:datasetdefinition ;
    cwrc:contraryTo cwrc:zionism ;
    a cwrc:PoliticalAffiliation, skos:Concept ;
    rdf:value "anti-israel", "anti-zionist" ;
    rdfs:comment "La description de ce terme est basée sur celle de DBPedia."@fr, "The description for this term is indebted to DBpedia."@en ;
    rdfs:isDefinedBy <http://sparql.cwrc.ca/ontologies/cwrc-2017-08-03> ;
    rdfs:label "Antisionisme"@fr, "anti-Zionism"@en ;
    skos:definition "Anti-Zionism is opposition to Zionism, broadly defined in the modern era as the opposition to the ethnonationalist and political movement of Jews and Jewish culture that supports the establishment of a Jewish state as a Jewish homeland in the territory defined as the historic Land of Israel (also referred to as Palestine, Canaan or the Holy Land) or to the modern State of Israel as defined as A Jewish and Democratic State. The term is used to describe various religious, moral and political points of view, but their diversity of motivation and expression is sufficiently different that \"anti-Zionism\" cannot be seen as having a single ideology or source. According to many notable Jewish and non-Jewish sources, anti-Zionism has become a cover for modern-day antisemitism, a position that critics have challenged as a tactic to silence criticism of Israeli policies. <a href=\"#_dbpedia_2017\">(DBpedia, 2017)</a>"@en, "L'antisionisme (ou anti-sionisme) désigne historiquement l'opposition au projet sioniste d'établissement d'un foyer national juif en Palestine. Il apparaît d'une part parmi les dirigeants traditionalistes juifs pour des raisons religieuses ou par crainte des Juifs assimiliationistes et d'autre part parmi les dirigeants arabes de Palestine et certains officiers britanniques quand la Grande-Bretagne obtient de la société des Nations un mandat pour administrer le pays. Outre l'opposition politique, l'antisionisme arabe palestinien de l'époque se manifeste lors de la Grande Révolte arabe de 1936-1939 et puis par la Guerre israélo-arabe de 1948. L'antisionisme juif est moins important et d'origine religieuse. Il se réduit fortement à partir de 1921 avec la nomination au grand rabbinat d'Eretz Israel du rabbin Abraham Isaac Kook pour disparaître presque totalement après la Shoah, la Résolution 181 de l'ONU du 30 novembre 1947 qui prévoit le Plan de partage de la Palestine et l'établissement d'un État juif, l'État d'Israël, que les Arabes tentèrent vainement d'empêcher lors de la guerre de 1948 et qui est l'aboutissement du projet sioniste originel. Après la guerre de 1967 et les conquêtes territoriales israéliennes, et en parallèle avec la médiatisation de la cause palestinienne et du problème des réfugiés palestiniens, la notion d'antisionisme évolue et devient plus ambiguë. Le terme peut caractériser des prises de positions aussi éloignées que le simple rejet de la politique israélienne à la revendication de son anéantissement. Ainsi, l'antisionisme est parfois invoqué comme une échappatoire pour voiler une nouvelle forme d'antisémitisme et cette accusation est elle-même dénoncée comme une manipulation visant à empêcher toute critique d'Israël et du sionisme. En Israël même, la situation a engendré les mouvements néosioniste et postsioniste, tous deux en opposition avec le « sionisme séculaire » des « pères fondateurs » mais pas nécessairement antisionistes. <a href=\"#_dbpedia_2017\">(DBpedia, 2017)</a>"@fr ;
    skos:inScheme cwrc:PoliticalAffiliation ;
    prov:derivedFrom dbpedia:Anti-Zionism .

cwrc:antidisestablishmentarianism
    void:inDataset cwrc:datasetdefinition ;
    a cwrc:PoliticalAffiliation, skos:Concept ;
    rdf:value "antidisestablishmentarian" ;
    rdfs:comment "The description for this term is indebted to DBpedia."@en ;
    rdfs:isDefinedBy <http://sparql.cwrc.ca/ontologies/cwrc-2017-08-03> ;
    rdfs:label ""@fr, "antidisestablishmentarianism"@en ;
    skos:definition ""@fr, "Antidisestablishmentarianism (/ˌæn.ti.dɪs.ɪs.tæb.lɪʃ.mənˈtɛə.rɪə.nɪ.zᵊm/, /ˌæn.taɪˌdɪs.ɛsˌtæb.lɪʃ.məntˈɛ.ri.ənˌɪ.zm/) is a political position that developed in 19th-century Britain in opposition to Liberal proposals for the disestablishment of the Church of England—meaning the removal of the Anglican Church's status as the state church of England, Ireland, and Wales. The establishment was maintained in England, but in Ireland the Church of Ireland (Anglican) was disestablished in 1871. In Wales, four Church of England dioceses were disestablished in 1920 and became the Church in Wales. Antidisestablishmentarianism is also one of the longest non-scientific words. The word has also come by analogy to refer to any opposition to those who oppose the establishment, whether the government, in whole or part, or the established society. <a href=\"#_dbpedia_2017\">(DBpedia, 2017)</a>"@en ;
    skos:inScheme cwrc:PoliticalAffiliation ;
    prov:derivedFrom dbpedia:Antidisestablishmentarianism .

cwrc:antisemitism
    void:inDataset cwrc:datasetdefinition ;
    a cwrc:PoliticalAffiliation, skos:Concept ;
    rdf:value "anti-semitism", "antisemitic" ;
    rdfs:comment "La description de ce terme est basée sur celle de DBPedia."@fr, "The description for this term is indebted to DBpedia."@en ;
    rdfs:isDefinedBy <http://sparql.cwrc.ca/ontologies/cwrc-2017-08-03> ;
    rdfs:label "Antisémitisme"@fr, "antisemitism"@en ;
    skos:definition "Antisemitism (also spelled anti-Semitism or anti-semitism) is hostility, prejudice, or discrimination against Jews. A person who holds such positions is called an antisemite. Antisemitism is widely considered to be a form of racism. The root word Semite gives the false impression that antisemitism is directed against all Semitic people. However, the compound word antisemite was popularized in Germany in 1879 as a scientific-sounding term for Judenhass \"Jew-hatred\",and that has been its common use since then. Antisemitism may be manifested in many ways, ranging from expressions of hatred of or discrimination against individual Jews to organized pogroms by mobs, state police, or even military attacks on entire Jewish communities. Although the term did not come into common usage until the 19th century, it is now also applied to historic anti-Jewish incidents. Notable instances of persecution include the Rhineland massacres preceding the First Crusade in 1096, the Edict of Expulsion from England in 1290, the massacres of Spanish Jews in 1391, the persecutions of the Spanish Inquisition, the expulsion from Spain in 1492, the Cossack massacres in Ukraine from 1648 to 1657, various anti-Jewish pogroms in the Russian Empire between 1821 and 1906, the 1894–1906 Dreyfus affair in France, the Holocaust in German-occupied Europe, official Soviet anti-Jewish policies, and Arab and Muslim involvement in the Jewish exodus from Arab and Muslim countries. <a href=\"#_dbpedia_2017\">(DBpedia, 2017)</a>"@en, "L’antisémitisme (originellement : anti-sémitisme) est le nom donné de nos jours à la discrimination et à l'hostilité manifestées à l'encontre des Juifs en tant que groupe ethnique, religieux ou racial. Il s'agit, dans son acception originelle telle que formulée vers la fin du XIXe siècle, d'une forme de racisme dirigée nominalement contre les peuples sémites, regroupés en tant que tels sur base de critères linguistiques, mais ne visant en réalité que les Juifs. Bien que certains historiens comme Jules Isaac insistent pour distinguer antijudaïsme et antisémitisme, le second terme est cependant le plus souvent utilisé aujourd'hui pour qualifier tous les actes d’hostilité anti-juive au cours de l'Histoire, que leurs fondements soient raciaux ou non. Les motifs et mises en pratique de l'antisémitisme incluent divers préjugés, des allégations, des mesures discriminatoires ou d’exclusion socio-économique, des expulsions, voire des massacres d’individus ou de communautés entières. <a href=\"#_dbpedia_2017\">(DBpedia, 2017)</a>"@fr ;
    skos:inScheme cwrc:PoliticalAffiliation ;
    prov:derivedFrom dbpedia:Antisemitism .

cwrc:artsAdvocacy
    void:inDataset cwrc:datasetdefinition ;
    a cwrc:PoliticalAffiliation, skos:Concept ;
    rdf:value "advocate for the arts", "artists' advocate" ;
    rdfs:comment "The description for this term is indebted to DBpedia."@en ;
    rdfs:isDefinedBy <http://sparql.cwrc.ca/ontologies/cwrc-2017-08-03> ;
    rdfs:label ""@fr, "arts advocacy"@en ;
    skos:definition ""@fr, "Advocacy for the fine, performing, or liberal arts."@en ;
    skos:inScheme cwrc:PoliticalAffiliation .

cwrc:atheism
    void:inDataset cwrc:datasetdefinition ;
    a cwrc:Religion, skos:Concept ;
    rdfs:comment "La description de ce terme est basée sur celle de DBPedia."@fr ;
    rdfs:isDefinedBy <http://sparql.cwrc.ca/ontologies/cwrc-2017-08-03> ;
    rdfs:label "Atheism"@en, "athéisme"@fr ;
    skos:definition "Atheism is, in a broad sense, the rejection of belief in the existence of deities. In a narrower sense, atheism is specifically the position that there are no deities. Most inclusively, atheism is the absence of belief that any deities exist. Atheism is contrasted with theism, which, in its most general form, is the belief that at least one deity exists. The term \"atheism\" originated from the Greek ἄθεος (atheos), meaning \"without god(s)\", used as a pejorative term applied to those thought to reject the gods worshiped by the larger society. With the spread of freethought, skeptical inquiry, and subsequent increase in criticism of religion, application of the term narrowed in scope. The first individuals to identify themselves using the word \"atheist\" lived in the 18th century during the Age of Enlightenment. The French Revolution, noted for its \"unprecedented atheism,\" witnessed the first major political movement in history to advocate for the supremacy of human reason. Arguments for atheism range from the philosophical to social and historical approaches. Rationales for not believing in deities include arguments that there is a lack of empirical evidence; the problem of evil; the argument from inconsistent revelations; the rejection of concepts that cannot be falsified; and the argument from nonbelief. Although some atheists have adopted secular philosophies (eg. humanism and skepticism), there is no one ideology or set of behaviors to which all atheists adhere. Many atheists hold that atheism is a more parsimonious worldview than theism and therefore that the burden of proof lies not on the atheist to disprove the existence of God but on the theist to provide a rationale for theism. Since conceptions of atheism vary, accurate estimations of current numbers of atheists are difficult. Several comprehensive global polls on the subject have been conducted by Gallup International: their 2015 poll featured over 64,000 respondents and indicated that 11% were \"convinced atheists\" whereas an earlier 2012 poll found that 13% of respondents were \"convinced atheists.\" An older survey by the BBC, in 2004, recorded atheists as comprising 8% of the world's population. Other older estimates have indicated that atheists comprise 2% of the world's population, while the irreligious add a further 12%. According to these polls, Europe and East Asia are the regions with the highest rates of atheism. In 2015, 61% of people in China reported that they were atheists. The figures for a 2010 Eurobarometer survey in the European Union (EU) reported that 20% of the EU population claimed not to believe in \"any sort of spirit, God or life force\". <a href=\"#_dbpedia_2017\">(DBpedia, 2017)</a>"@en, "L’athéisme est une attitude ou une doctrine qui nie l’existence de quelque dieu ou divinité que ce soit, contrairement, par exemple, au déisme et au théisme qui soutiennent ces existences, ou à l’agnosticisme qui considère que personne ne peut répondre à ces questions. C'est une position philosophique qui peut être formulée ainsi : il n'existe rien qui ressemble de près ou de loin à ce que les croyants appellent un « dieu », ou « Dieu ». <a href=\"#_dbpedia_2017\">(DBpedia, 2017)</a>"@fr ;
    skos:inScheme cwrc:Religion ;
    prov:derivedFrom dbpedia:Atheism .

cwrc:auntOf
    void:inDataset cwrc:datasetdefinition ;
    a owl:ObjectProperty ;
    rdf:value "AUNT" ;
    rdfs:isDefinedBy <http://sparql.cwrc.ca/ontologies/cwrc-2017-08-03> ;
    rdfs:label "aunt of"@en, "tante de"@fr ;
    rdfs:subPropertyOf cwrc:relativeOf .

cwrc:baptistChristianity
    void:inDataset cwrc:datasetdefinition ;
    a cwrc:Religion, skos:Concept ;
    rdfs:comment "La description de ce terme est basée sur celle de DBPedia."@fr, "The description for this term is indebted to the Getty Art & Architecture Thesaurus."@en ;
    rdfs:isDefinedBy <http://sparql.cwrc.ca/ontologies/cwrc-2017-08-03> ;
    rdfs:label "Baptisme"@fr, "Baptisme"@nl, "Baptismo"@es, "Baptist Christianity"@en, "Baptistas"@es, "chin li tsung"@zh-latn-wadegile, "jin li zong"@zh-latn-pinyin-x-notone, "jìn lǐ zōng"@zh-latn-pinyin-x-hanyu, "浸信會"@zh-hant, "浸禮宗"@zh-hant, "浸禮派"@zh-hant ;
    skos:broaderTransitive cwrc:protestantism ;
    skos:definition "Le baptisme est un courant chrétien évangélique issu d'un réveil démarré par les pasteurs anglais John Smyth en Hollande en 1609, puis Thomas Helwys en Angleterre en 1612. Ce mouvement se caractérise par l'importance donnée à la Bible, à la nouvelle naissance, au baptême adulte en tant que témoignage volontaire, un esprit missionnaire, un engagement moral de vie ainsi que par l’autonomie locale des églises, la séparation de l’Église et de l’État, et finalement l’autorité de la congrégation (congrégationalisme). Selon les chiffres du Pew Research Center, en 2011, le mouvement recense 72 millions de croyants. <a href=\"#_dbpedia_2017\">(DBpedia, 2017)</a>"@fr, "Refers to a Protestant denomination centered around the belief that the sacrament of baptism should only be administered to adult members after a personal profession of belief in Jesus Christ. Baptism in this faith is usually done by full immersion. Emphasis is placed on biblical scripture and preaching. The Baptist denomination is primarily derived from early 17th-century England and Wales where it quickly spread although there are some links with the Anabaptists of the 16th century. Baptist churches very rapidly increased in the late 19th century in the United States. <a href=\"#_getty_2017\">(Getty, 2017)</a>"@en, "Se refiere a la religión protestante centrada en torno a la creencia que el sacramento del bautismo debería ser administrado sólo a miembros adultos tras una manifestación personal de creencia en Jesucristo. El bautismo en esta fe es usualmente hecho por inmersión total. El énfasis es puesto en las Escrituras Bíblicas y la oración. La denominación baptista deriva principalmente de la Inglaterra y Gales del siglo XVII en donde rápidamente se difundió a pesar que hay algunas conexiones con los Anabaptistas del siglo XVI. La iglesia baptista creció rápidamente en el siglo XIX en los Estados Unidos. <a href=\"#_getty_2017\">(Getty, 2017)</a>"@es, "Verwijst naar een protestantse gezindte waarbij het geloof centraal staat dat het sacrament van de doop alleen moet worden toegediend aan volwassen leden na een persoonlijke belijdenis van geloof in Jezus Christus. De doop vindt bij deze gezindte doorgaans plaats door volledige onderdompeling. De nadruk ligt op Bijbelse geschriften en preken. Het baptisme is in hoofdzaak ontstaan in de vroege 17de eeuw in Engeland en Wales waar het zich snel verspreidde, hoewel er enige verbanden zijn met de anabaptisten van de 16de eeuw. In de late 19de eeuw nam het aantal baptistische kerken in de Verenigde Staten snel toe. <a href=\"#_getty_2017\">(Getty, 2017)</a>"@nl, "一支新教派別，相信只有親自聲明信仰基督的成人才可受洗。此教的洗禮通常需全身浸洗。重視聖經經文與佈道。浸信會與十六世紀的重浸派有些淵源，但主要源於十七世紀初的英格蘭與威爾斯，在這兩處快速廣傳。其教會於十九世紀末在美國急速增加。 <a href=\"#_getty_2017\">(Getty, 2017)</a>"@zh-hant ;
    skos:inScheme cwrc:Religion ;
    prov:derivedFrom dbpedia:Baptists, <http://vocab.getty.edu/aat/300153825> .

cwrc:baptistChurch
    dcterms:isReplacedBy cwrc:baptistChristianity ;
    void:inDataset cwrc:datasetdefinition ;
    a skos:Concept ;
    rdfs:comment "Deprecated in favour of instance #baptistChristianity."@en, "Désapprouver en faveur de l'instance #baptistChristianity."@fr, "La description de ce terme est basée sur celle de DBPedia."@fr, "The description for this term is indebted to the Getty Art & Architecture Thesaurus."@en ;
    rdfs:isDefinedBy <http://sparql.cwrc.ca/ontologies/cwrc-2017-08-03> ;
    rdfs:label "Baptisme"@fr, "Baptisme"@nl, "Baptismo"@es, "Baptist"@en, "Baptistas"@es, "chin li tsung"@zh-latn-wadegile, "jin li zong"@zh-latn-pinyin-x-notone, "jìn lǐ zōng"@zh-latn-pinyin-x-hanyu, "浸信會"@zh-hant, "浸禮宗"@zh-hant, "浸禮派"@zh-hant ;
    owl:deprecated true ;
    vs:term_status "deprecated"@en ;
    skos:broaderTransitive cwrc:christianity ;
    skos:definition "Le baptisme est un courant chrétien évangélique issu d'un réveil démarré par les pasteurs anglais John Smyth en Hollande en 1609, puis Thomas Helwys en Angleterre en 1612. Ce mouvement se caractérise par l'importance donnée à la Bible, à la nouvelle naissance, au baptême adulte en tant que témoignage volontaire, un esprit missionnaire, un engagement moral de vie ainsi que par l’autonomie locale des églises, la séparation de l’Église et de l’État, et finalement l’autorité de la congrégation (congrégationalisme). Selon les chiffres du Pew Research Center, en 2011, le mouvement recense 72 millions de croyants. <a href=\"#_dbpedia_2017\">(DBpedia, 2017)</a>"@fr, "Refers to a Protestant denomination centered around the belief that the sacrament of baptism should only be administered to adult members after a personal profession of belief in Jesus Christ. Baptism in this faith is usually done by full immersion. Emphasis is placed on biblical scripture and preaching. The Baptist denomination is primarily derived from early 17th-century England and Wales where it quickly spread although there are some links with the Anabaptists of the 16th century. Baptist churches very rapidly increased in the late 19th century in the United States. <a href=\"#_getty_2017\">(Getty, 2017)</a>"@en, "Se refiere a la religión protestante centrada en torno a la creencia que el sacramento del bautismo debería ser administrado sólo a miembros adultos tras una manifestación personal de creencia en Jesucristo. El bautismo en esta fe es usualmente hecho por inmersión total. El énfasis es puesto en las Escrituras Bíblicas y la oración. La denominación baptista deriva principalmente de la Inglaterra y Gales del siglo XVII en donde rápidamente se difundió a pesar que hay algunas conexiones con los Anabaptistas del siglo XVI. La iglesia baptista creció rápidamente en el siglo XIX en los Estados Unidos. <a href=\"#_getty_2017\">(Getty, 2017)</a>"@es, "Verwijst naar een protestantse gezindte waarbij het geloof centraal staat dat het sacrament van de doop alleen moet worden toegediend aan volwassen leden na een persoonlijke belijdenis van geloof in Jezus Christus. De doop vindt bij deze gezindte doorgaans plaats door volledige onderdompeling. De nadruk ligt op Bijbelse geschriften en preken. Het baptisme is in hoofdzaak ontstaan in de vroege 17de eeuw in Engeland en Wales waar het zich snel verspreidde, hoewel er enige verbanden zijn met de anabaptisten van de 16de eeuw. In de late 19de eeuw nam het aantal baptistische kerken in de Verenigde Staten snel toe. <a href=\"#_getty_2017\">(Getty, 2017)</a>"@nl, "一支新教派別，相信只有親自聲明信仰基督的成人才可受洗。此教的洗禮通常需全身浸洗。重視聖經經文與佈道。浸信會與十六世紀的重浸派有些淵源，但主要源於十七世紀初的英格蘭與威爾斯，在這兩處快速廣傳。其教會於十九世紀末在美國急速增加。 <a href=\"#_getty_2017\">(Getty, 2017)</a>"@zh-hant ;
    skos:inScheme cwrc:Religion ;
    prov:derivedFrom dbpedia:Baptists, <http://vocab.getty.edu/aat/300153825> .

cwrc:birthControlActivism
    void:inDataset cwrc:datasetdefinition ;
    a cwrc:PoliticalAffiliation, skos:Concept ;
    rdf:value "birth control activist", "birth control campaigner", "birth-control activist", "contraceptionist", "pro birth control", "pro-birth control", "pro-contraception" ;
    rdfs:comment "The description for this term is indebted to DBpedia."@en ;
    rdfs:isDefinedBy <http://sparql.cwrc.ca/ontologies/cwrc-2017-08-03> ;
    rdfs:label ""@fr, "birth control activism"@en ;
    skos:definition ""@fr, "Promotion of birth control awareness, practices, and resources. See: <a href=\"https://en.wikipedia.org/wiki/Birth_control_movement_in_the_United_States\">https://en.wikipedia.org/wiki/Birth_control_movement_in_the_United_States  Also see: </a><a href=\"https://en.wikipedia.org/wiki/Category:Birth_control\">https://en.wikipedia.org/wiki/Category:Birth_control</a>"@en ;
    skos:inScheme cwrc:PoliticalAffiliation ;
    prov:derivedFrom dbpedia:Birth_control_movement_in_the_United_States, <http://dbpedia.org/resource/Category:Birth_control> .

cwrc:black
    void:inDataset cwrc:datasetdefinition ;
    a cwrc:RaceColour ;
    rdfs:isDefinedBy <http://sparql.cwrc.ca/ontologies/cwrc-2017-08-03> ;
    rdfs:label "black (race)"@en, "noir (race)"@fr ;
    skos:definition ""@en, ""@fr .

cwrc:blackAnti-Oppression
    void:inDataset cwrc:datasetdefinition ;
    a cwrc:PoliticalAffiliation, skos:Concept ;
    rdf:value "anti-segregationist", "black activist", "black liberation", "black liberationist", "black power", "black pride" ;
    rdfs:comment "The description for this term is indebted to DBpedia."@en ;
    rdfs:isDefinedBy <http://sparql.cwrc.ca/ontologies/cwrc-2017-08-03> ;
    rdfs:label ""@fr, "black anti-oppression movement"@en ;
    skos:definition ""@fr, "Opposition to the social, institutional, and political oppression of people defined as black, which varies historically and geographically.  See <a href=\"https://en.wikipedia.org/wiki/Racism_in_the_United_Kingdom\">https://en.wikipedia.org/wiki/Racism_in_the_United_Kingdom</a> and <a href=\"https://en.wikipedia.org/wiki/African-American_Civil_Rights_Movement_(1954%E2%80%931968)\">https://en.wikipedia.org/wiki/African-American_Civil_Rights_Movement_(1954%E2%80%931968)</a>"@en ;
    skos:inScheme cwrc:PoliticalAffiliation ;
    skos:related cwrc:abolitionism ;
    prov:derivedFrom <http://dbpedia.org/resource/African-American_Civil_Rights_Movement_(1954%E2%80%931968)>, dbpedia:Racism_in_the_United_Kingdom .

cwrc:blackLabel
    void:inDataset cwrc:datasetdefinition ;
    a skos:Concept, skosxl:Label ;
    rdfs:isDefinedBy <http://sparql.cwrc.ca/ontologies/cwrc-2017-08-03> ;
    rdfs:label "black"@en, "noir"@fr ;
    skos:definition ""@en, ""@fr ;
    skos:inScheme cwrc:TextLabels ;
    foaf:name "black"@en .

cwrc:bloodRelativeOf
    void:inDataset cwrc:datasetdefinition ;
    a owl:ObjectProperty ;
    rdfs:isDefinedBy <http://sparql.cwrc.ca/ontologies/cwrc-2017-08-03> ;
    rdfs:label "blood relative of"@en, "liens de sang"@fr ;
    rdfs:subPropertyOf cwrc:relativeOf .

cwrc:bolshevism
    void:inDataset cwrc:datasetdefinition ;
    a cwrc:PoliticalAffiliation, skos:Concept ;
    rdf:value "Bolshevist", "pro-bolshevik" ;
    rdfs:comment "La description de ce terme est basée sur celle de DBPedia."@fr, "The description for this term is indebted to DBpedia."@en ;
    rdfs:isDefinedBy <http://sparql.cwrc.ca/ontologies/cwrc-2017-08-03> ;
    rdfs:label "Bolcheviks"@fr, "Bolshevism"@en ;
    skos:definition "Les bolcheviks, bolcheviques ou bolchéviques sont les membres d'une fraction du Parti ouvrier social-démocrate de Russie, créée en 1903 sous la direction de Lénine, devenue un parti indépendant en 1912. Après la révolution russe de février 1917, les bolcheviks prennent le pouvoir au nom des soviets en octobre 1917 dans le cadre de la République socialiste fédérative soviétique de Russie. En 1918, le Parti bolchévique est renommé Parti communiste. Après la mise en place de l'URSS (1922), il devient le Parti communiste de l'Union soviétique (PCUS), ajoutant jusqu'en 1952 à ce nom l'adjectif bolchevik (placé entre parenthèses). <a href=\"#_dbpedia_2017\">(DBpedia, 2017)</a>"@fr, "The Bolsheviks, originally also Bolshevists or Bolsheviki (Russian: большевики, большевик (singular); IPA: [bəlʲʂɨˈvʲik]; derived from большинство bol'shinstvo, \"majority\", literally meaning \"one of the majority\") were a faction of the Marxist Russian Social Democratic Labour Party (RSDLP) which split apart from the Menshevik faction at the Second Party Congress in 1903. The RSDLP was a revolutionary socialist political party formed in 1898 in Minsk to unite the various revolutionary organisations of the Russian Empire into one party. In the Second Party Congress vote, the Bolsheviks won on the majority of important issues, hence their name. They ultimately became the Communist Party of the Soviet Union. The Bolsheviks or Reds came to power in Russia during the October Revolution phase of the Russian Revolution of 1917, and founded the Russian Soviet Federative Socialist Republic (RSFSR). With the Reds defeating the Whites, and others during the Russian Civil War of 1917–1922, the RSFSR became the chief constituent of the Soviet Union in December 1922. The Bolsheviks, founded by Vladimir Lenin and Alexander Bogdanov, were by 1905 a major organization consisting primarily of workers under a democratic internal hierarchy governed by the principle of democratic centralism, who considered themselves the leaders of the revolutionary working class of Russia. Their beliefs and practices were often referred to as Bolshevism. <a href=\"#_dbpedia_2017\">(DBpedia, 2017)</a>"@en ;
    skos:inScheme cwrc:PoliticalAffiliation ;
    prov:derivedFrom dbpedia:Bolsheviks .

cwrc:bonapartism
    void:inDataset cwrc:datasetdefinition ;
    a cwrc:PoliticalAffiliation, skos:Concept ;
    rdf:value "pro-bonapartist" ;
    rdfs:comment "La description de ce terme est basée sur celle de DBPedia."@fr, "The description for this term is indebted to DBpedia."@en ;
    rdfs:isDefinedBy <http://sparql.cwrc.ca/ontologies/cwrc-2017-08-03> ;
    rdfs:label "Bonapartism"@en, "Bonapartisme"@fr ;
    skos:definition "Bonapartism is the political ideology of Napoleon Bonaparte and his followers and successors. It was later used to refer to persons who hoped to restore the House of Bonaparte and its style of government. After Napoleon, the term was applied to the French politicians who seized power in the coup of 18 Brumaire, ruling in the French Consulate and subsequently in the First and Second French Empires under the House of Bonaparte (the family of Bonaparte and his nephew Louis). The term was used more generally for a political movement that advocated a dictatorship or authoritarian centralized state, with a strongman charismatic leader based on anti-elitist rhetoric, army support, and conservatism. Marxism and Leninism developed a vocabulary of political terms that included Bonapartism, derived from their analysis of the career of Napoleon Bonaparte. Karl Marx was a student of Jacobinism and the French Revolution, and was a contemporary critic of the Second Republic and Second Empire. He used \"Bonapartism\" to refer to a situation in which counter-revolutionary military officers seize power from revolutionaries, and use selective reforms to co-opt the radicalism of the popular classes. Marx argued that in the process, Bonapartists preserve and mask the power of a narrower ruling class. According to his essay \"The Eighteenth Brumaire of Louis Napoleon\" (1852), Marx believed that both Bonaparte and his nephew Napoleon III had corrupted revolutions in France in this way. In this document, he drew attention to what he calls the phenomenon's repetitive history by saying: \"History repeats itself, first as tragedy, then as farce.\" More generally, \"Bonapartism\" may be used to describe the replacement of civilian leadership by military leadership within revolutionary movements or governments. Many modern-day Trotskyists and other leftists use the phrase \"left Bonapartist\" to describe those, such as Stalin and Mao, who controlled 20th-century bureaucratic socialist regimes. In addition, Leon Trotsky was accused of using his position as commander of the Red Army to gain top-level power after Lenin's death. Noted political scientists and historians greatly differ on the definition and interpretation of Bonapartism. Sudhir Hazareesingh's book The Legend of Napoleon explores numerous interpretations of the term. He says that it refers to a \"popular national leader confirmed by popular election, above party politics, promoting equality, progress, and social change, with a belief in religion as an adjunct to the State, a belief that the central authority can transform society and a belief in the 'nation' and its glory and a fundamental belief in national unity.\" Hazareesingh believes that although recent research shows Napoleon used forced conscription of French troops, some men must have fought believing in Napoleon's ideals. He says that to argue Bonapartism co-opted the masses is an example of the Marxist perspective of false consciousness: the idea that the masses can be manipulated by a few determined leaders in the pursuit of ends. Scholar Raymond Hinnebusch has characterized Hafez al-Asad's regime in Syria as Bonapartist. <a href=\"#_dbpedia_2017\">(DBpedia, 2017)</a>"@en, """Le bonapartisme est une famille de pensée politique française, qui s'inspire de l'action de l'empereur Napoléon Ier. Le terme a deux acceptions : 
  * au sens strict, le bonapartisme vise à établir un régime républicain impérial en France à la tête duquel serait placé un membre de la famille de Napoléon Bonaparte ; 
  * au sens large, le bonapartisme vise à établir un État national à exécutif fort et centralisé mais d'essence républicaine et assis sur la consultation régulière du peuple par le biais de plébiscites. Le bonapartisme n'implique donc pas forcément l'adhésion à un système d'organisation politique héréditaire mais peut au contraire s'accommoder d'une forme républicaine de gouvernement. Il repose sur la fusion des élites et l'adhésion populaire. Ces deux facettes peuvent être distinctes ou confondues, selon les personnes et périodes. <a href=\"#_dbpedia_2017\">(DBpedia, 2017)</a>"""@fr ;
    skos:inScheme cwrc:PoliticalAffiliation ;
    prov:derivedFrom dbpedia:Bonapartism .

cwrc:boulangism
    void:inDataset cwrc:datasetdefinition ;
    a cwrc:PoliticalAffiliation, skos:Concept ;
    rdf:value "boulangist" ;
    rdfs:comment "The description for this term is indebted to DBpedia."@en ;
    rdfs:isDefinedBy <http://sparql.cwrc.ca/ontologies/cwrc-2017-08-03> ;
    rdfs:label ""@fr, "boulangism"@en ;
    skos:definition ""@fr, "Followed the three principles of \"revenge on Germany\", \"revision of the constitution\", and \"the return to monarchy\" in frustration with French conservatism. Based on the politics of Georges Ernest Boulanger. See: <a href=\"https://en.wikipedia.org/wiki/Georges_Ernest_Boulanger\">https://en.wikipedia.org/wiki/Georges_Ernest_Boulanger</a>"@en ;
    skos:inScheme cwrc:PoliticalAffiliation ;
    prov:derivedFrom dbpedia:Georges_Ernest_Boulanger .

cwrc:britishNationalism
    void:inDataset cwrc:datasetdefinition ;
    a cwrc:PoliticalAffiliation, skos:Concept ;
    rdf:value "british nationalist" ;
    rdfs:comment "The description for this term is indebted to DBpedia."@en ;
    rdfs:isDefinedBy <http://sparql.cwrc.ca/ontologies/cwrc-2017-08-03> ;
    rdfs:label ""@fr, "British nationalism"@en ;
    skos:definition ""@fr, "British nationalism asserts that the British are a nation and promotes the cultural unity of the British, in a definition of Britishness that may include people of English, Scottish, Welsh, Ulster Scots and Irish descent. British nationalism is closely associated with British unionism, which seeks to uphold the political union that is the United Kingdom, or strengthen the links between the countries of the United Kingdom. British nationalism's unifying identity descends from the ancient Britons who dwelt on the island of Great Britain. British nationalism grew to include people outside Great Britain, in Ireland, because of the 1542 Crown of Ireland Act, which declared that the crown of Ireland was to be held by the ruling monarch of England as well as Anglo-Irish calls for unity with Britain. It is characterised as a \"powerful but ambivalent force in British politics\". In its moderate form, British nationalism has been a civic nationalism, emphasizing both cohesion and diversity of the people of the United Kingdom, its dependencies, and its former colonies. Recently however, nativist nationalism has arisen based on fear of Britain being swamped by immigrants; this anti-immigrant nativist nationalism has manifested politically in the British National Party and other nativist nationalist movements. Politicians, such as British Prime Minister David Cameron of the Conservative Party and his direct predecessor Gordon Brown of the Labour Party, have sought to promote British nationalism as a progressive cause. <a href=\"#_dbpedia_2017\">(DBpedia, 2017)</a>"@en ;
    skos:inScheme cwrc:PoliticalAffiliation ;
    prov:derivedFrom dbpedia:British_nationalism .

cwrc:buddhism
    void:inDataset cwrc:datasetdefinition ;
    a cwrc:Religion, skos:Concept ;
    rdfs:comment "La description de ce terme est basée sur celle de DBPedia."@fr, "The description for this term is indebted to the Getty Art & Architecture Thesaurus."@en ;
    rdfs:isDefinedBy <http://sparql.cwrc.ca/ontologies/cwrc-2017-08-03> ;
    rdfs:label "Boeddhisme"@nl, "Bouddhisme"@fr, "Buddhism"@en, "Budismo"@es, "fo chiao"@zh-latn-wadegile, "fo jiao"@zh-latn-pinyin-x-notone, "fó jiào"@zh-latn-pinyin-x-hanyu, "佛教"@zh-hant ;
    skos:altLabel "Buddhist"@en ;
    skos:definition "Le bouddhisme est, selon les points de vue en Occident, une religion (notamment une religion d'État) ou une philosophie, voire les deux, dont les origines remontent en Inde au Ve siècleav. J.-C. à la suite de l'éveil de Siddhartha Gautama et de son enseignement. Le bouddhisme comptait en 2005 entre 230 millions et 500 millions d'adeptes, ce qui en fait la quatrième religion mondiale, derrière (dans l'ordre décroissant) le christianisme, l'islam, et l'hindouisme. Le bouddhisme présente un ensemble ramifié de pratiques méditatives, de pratiques éthiques, de théories psychologiques, philosophiques, cosmogoniques et cosmologiques, abordées dans la perspective de la bodhi, « l'éveil ». À l'instar du jaïnisme, le bouddhisme est à l'origine une tradition shramana, et non brahmanique comme l'est l'hindouisme. Les notions de dieu et de divinité dans le bouddhisme sont particulières : bien que le bouddhisme soit souvent perçu comme une religion sans dieu créateur, la notion étant absente de la plupart des formes du bouddhisme, la vénération et le culte du Bouddha historique Siddhartha Gautama en tant que bhagavat joue un rôle important dans le Theravāda et également dans le Mahāyāna, dans lesquels il est un être éveillé ayant trois aspects ou manifestations (trikāya). <a href=\"#_dbpedia_2017\">(DBpedia, 2017)</a>"@fr, "Refers to the philosophy and religion based on the enlightenment and teachings of the Buddha Gautama in the early sixth century BCE in the northeastern region of modern India. Playing dominant roles in the art and culture of Southeast Asia and East Asia, this religion is based on the transcendence of human suffering and pain through the acceptance of the limitations of individuality, the surrender of worldly desires and cravings that cause disappointment and sorrow, and the deliverance from the impermanence of living and individual ego based on wealth, social position, or family through the process of enlightenment (nirvana). The religion also centers around 'anatman', or no-self, the idea that the self is in a state of action or a series of changing manifestations rather than in a state of fixed, metaphysical substance. The structure of the religion is based on the Triratna (\"Three Jewels\" of Buddha), a tripartite schematic for living based on three elements: Buddha (the teacher), dharma (the teaching), and sangha (community). <a href=\"#_getty_2017\">(Getty, 2017)</a>"@en, "Se refiere a la filosofía y religión basada en la iluminación y enseñanza del Buddha Gautama en el siglo VI a.C temprano en la región nordeste de la India Moderna. Jugando un rol dominante en el arte y la cultura del Asia Sudeste y Asia Oriental, esta religión está basada en la trascendencia del sufrimiento y dolor humano a través de la aceptación de las limitaciones de individualidad, la rendición de deseos mundanos y anhelos que causan desilusión y aflicción y la liberación desde la transitoriedad of living and individual ego based on wealth, social position, or family through the process of enlightenment (nirvana). The religion also centers around anatman, or no-self, the idea that the self is in a state of action or a series of changing manifestations rather than in a state of fixed, metaphysical substance. The structure of the religion is based on the Triratna (\"Three Jewels\" of Buddha), a tripartite schematic for living based on three elements: Buddha (the teacher), dharma (the teaching), and sangha (community). <a href=\"#_getty_2017\">(Getty, 2017)</a>"@es, "Verwijst naar de filosofie en religie die zijn gebaseerd op de verlichting en leer van Boeddha Gautama in de vroege 6de eeuw v. Chr. in het Noord-Oosten van het moderne India. Deze religie, die een dominante rol speelt in de kunst en cultuur van Zuidoost-Azië en Oost-Azië, is gebaseerd op het overstijgen van menselijk lijden en pijn door het accepteren van de grenzen van de individualiteit, het opgeven van wereldse verlangens en wensen die voor teleurstellingen en verdriet zorgen en het loslaten van het niet-permanente van het leven en het afzonderlijke ego met de bijbehorende welvaart, sociale positie of familierelaties, allemaal door het proces van de verlichting (nirvana). Bij deze religie staat ook 'anatman' centraal, het idee dat 'het zelf' altijd in ontwikkeling is of deel uitmaakt van een reeks veranderende verschijningsvormen in plaats van een vaste, metafysische substantie. De structuur van de religie is gebaseerd op de Triratna ('drie juwelen' van boeddha), een drieledige structuur voor het leven gebaseerd op drie elementen: boeddha (de leraar), dharma (de leer) en sangha (de gemeenschap). <a href=\"#_getty_2017\">(Getty, 2017)</a>"@nl, "根據釋迦牟尼佛之開悟與教誨的哲學和宗教，在西元前六世紀初起源於現今印度東北部。佛教於東南亞及東亞的藝術與文化層面扮演主要角色，相信透過接受自身的局限，以及放棄會引起失望與悲傷的世俗欲求及渴望，能夠使人類的苦痛得以昇華，而在開悟（涅盤）過程中得以從短暫的生命以及建築在財富、社會地位與家庭上的個人自尊中獲得解脫。此宗教的中心思想為「無我」，認為自我是處於活動狀態或是一連串的形式改變，而非固定的形上實體狀態。佛教的架構奠基於「三寶」，即生命三元素：佛(老師)、法(規範)、僧(眾)。 <a href=\"#_getty_2017\">(Getty, 2017)</a>"@zh-hant ;
    skos:inScheme cwrc:Religion ;
    prov:derivedFrom dbpedia:Buddhism, <http://vocab.getty.edu/aat/300073738> .

cwrc:catholicChurch
    dcterms:isReplacedBy cwrc:catholicism ;
    void:inDataset cwrc:datasetdefinition ;
    a skos:Concept ;
    rdfs:comment "Deprecated in favour of instance #catholicism."@en, "Désapprouver en faveur de l'instance #catholicism."@fr, "La description de ce terme est basée sur celle de DBPedia."@fr, "The description for this term is indebted to the Getty Art & Architecture Thesaurus."@en ;
    rdfs:isDefinedBy <http://sparql.cwrc.ca/ontologies/cwrc-2017-08-03> ;
    rdfs:label "Catholicisme"@fr, "Catolicismo"@es, "Catolicismo Romano"@es, "Katholicisme"@nl, "Katholiek"@nl, "Roman Catholic"@en, "Rooms-Katholicisme"@nl ;
    owl:deprecated true ;
    vs:term_status "deprecated"@en ;
    skos:broaderTransitive cwrc:christianity ;
    skos:definition "L’Église catholique, ou Église catholique, apostolique et romaine, est la plus grande Église chrétienne avec plus d'un milliard de fidèles. Elle réunit l’ensemble des chrétiens en communion avec le pape et les évêques qui sont considérés par les catholiques comme étant les successeurs des apôtres de Jésus-Christ. L'Église catholique est l'une des plus vieilles institutions religieuses au monde et a joué un rôle important dans l'histoire, surtout du monde occidental. La foi de l'Église catholique est résumée par le symbole de Nicée et elle se caractérise par la célébration des sept sacrements dont le plus important est l'Eucharistie célébré liturgiquement durant la messe. Selon son propre catéchisme, l'Église catholique est composée de trois parties qui ne forment qu'une seule Église placée sous Jésus-Christ : l'Église militante, l'Église triomphante et l'Église souffrante correspondant respectivement à l'ensemble des fidèles sur terre, l'ensemble des saints qui sont au ciel et l'ensemble des âmes qui sont au purgatoire. L'Église catholique sur terre se conçoit comme une communion d'Églises locales ou particulières, c'est-à-dire ayant chacune un territoire et un évêque à sa tête. Celles-ci sont chacune pleinement l'Église catholique dans la mesure où elles sont en communion avec le pape, qui est l'évêque de Rome et considéré comme étant le successeur de saint Pierre, et en communion les unes avec les autres. L'Église catholique se définit comme une institution à la fois humaine et divine : « société parfaite en dépit de l'imperfection de ses membres ». En plus d'être l'ensemble des baptisés, elle est aussi une institution et un clergé organisés de façon hiérarchique. Une très grande majorité des catholiques (au moins 98 %) sont de l'Église latine, mais il existe aussi des catholiques de différentes Églises catholiques orientales. <a href=\"#_dbpedia_2017\">(DBpedia, 2017)</a>"@fr, "Refers to the branch of Christianity characterized by a uniform, highly developed ritual canon and organizational structure with doctrinal roots based in the teachings of the Apostles of Jesus Christ in the first century, in the Alexandrian school of theology, and in Augustinian thought. In this religious branch, faith is considered an acceptance of revelation; revelation appears as doctrine. In juridical terms, it refers to the branch of Christianity distinguished as a unified, monolithic sacramental system under the governance of papal authority. Throughout much of its history, the seat of the Pope has been in Rome, thus \"Roman Catholicism\" is often used to distinguish this concept from the Orthodox Catholic church. <a href=\"#_getty_2017\">(Getty, 2017)</a>"@en, "Se refiere a la rama del cristianismo caracterizada por un canon ritual uniforme y altamente desarrollado y una estructura organizacional con raíces doctrinales basadas en las enseñanzas de los Apostoles de Jesucristo en la primera centuria, en la Escuela Alejandrina de teología, y en el pensamiento agustiniano. En esta rama de la religión, la fe es considerada como una aceptación de revelación; la revelación aparece como doctrina. Se refiere a la rama del cristianismo caracterizada por un canon ritual uniforme y altamente desarrollado y una estructura organizacional con raíces doctrinales basadas en las enseñanzas de los Apóstoles de Jesucristo en el primer siglo, en la Escuela Alejandrina de teología, y en el pensamiento agustiniano. En esta rama de la religión, la fe es considerada como una aceptación de revelación; la revelación aparece como doctrina. En términos jurídicos, se refiere a la rama del Cristianismo distinguido como sistema sacramental unificado, monolítico bajo gobierno de la autoridad papal. A través de la mayor parte de su historia, \"la silla del papal” ha estado en Roma, mediante este concepto el Catolicismo Romano se distingue de la Iglesia Católica Ortodoxa. <a href=\"#_getty_2017\">(Getty, 2017)</a>"@es, "Verwijst naar de richting van het christendom die zich kenmerkt door een uniforme, hoogontwikkelde rituele canon en organisatiestructuur met een doctrine die wortelt in de leer van de apostelen van Jezus Christus in de 1ste eeuw, in de theologie van de Alexandrijnse school en in het augustijner gedachtegoed. In deze godsdienstige richting wordt het geloof beschouwd als een aanvaarding van de openbaring; de openbaring heeft de vorm van een doctrine. In juridische zin verwijst de term naar de richting van het christendom die zich onderscheidt als een verenigd, monolithisch sacramenteel systeem onder het bestuur van het pauselijk gezag. Gedurende het grootste deel van de geschiedenis van dit systeem was de paus gevestigd in Rome en daarom wordt 'rooms-katholicisme' vaak gebruikt om dit begrip te onderscheiden van de orthodoxe katholieke kerk. <a href=\"#_getty_2017\">(Getty, 2017)</a>"@nl ;
    skos:inScheme cwrc:Religion ;
    prov:derivedFrom dbpedia:Catholic_Church, <http://vocab.getty.edu/aat/300073730> .

cwrc:catholicism
    void:inDataset cwrc:datasetdefinition ;
    a cwrc:Religion, skos:Concept ;
    rdfs:comment "La description de ce terme est basée sur celle de DBPedia."@fr, "The description for this term is indebted to the Getty Art & Architecture Thesaurus."@en ;
    rdfs:isDefinedBy <http://sparql.cwrc.ca/ontologies/cwrc-2017-08-03> ;
    rdfs:label "Catholicisme"@fr, "Catolicismo"@es, "Catolicismo Romano"@es, "Katholicisme"@nl, "Katholiek"@nl, "Roman Catholicism"@en, "Rooms-Katholicisme"@nl ;
    skos:broaderTransitive cwrc:christianity ;
    skos:definition "L’Église catholique, ou Église catholique, apostolique et romaine, est la plus grande Église chrétienne avec plus d'un milliard de fidèles. Elle réunit l’ensemble des chrétiens en communion avec le pape et les évêques qui sont considérés par les catholiques comme étant les successeurs des apôtres de Jésus-Christ. L'Église catholique est l'une des plus vieilles institutions religieuses au monde et a joué un rôle important dans l'histoire, surtout du monde occidental. La foi de l'Église catholique est résumée par le symbole de Nicée et elle se caractérise par la célébration des sept sacrements dont le plus important est l'Eucharistie célébré liturgiquement durant la messe. Selon son propre catéchisme, l'Église catholique est composée de trois parties qui ne forment qu'une seule Église placée sous Jésus-Christ : l'Église militante, l'Église triomphante et l'Église souffrante correspondant respectivement à l'ensemble des fidèles sur terre, l'ensemble des saints qui sont au ciel et l'ensemble des âmes qui sont au purgatoire. L'Église catholique sur terre se conçoit comme une communion d'Églises locales ou particulières, c'est-à-dire ayant chacune un territoire et un évêque à sa tête. Celles-ci sont chacune pleinement l'Église catholique dans la mesure où elles sont en communion avec le pape, qui est l'évêque de Rome et considéré comme étant le successeur de saint Pierre, et en communion les unes avec les autres. L'Église catholique se définit comme une institution à la fois humaine et divine : « société parfaite en dépit de l'imperfection de ses membres ». En plus d'être l'ensemble des baptisés, elle est aussi une institution et un clergé organisés de façon hiérarchique. Une très grande majorité des catholiques (au moins 98 %) sont de l'Église latine, mais il existe aussi des catholiques de différentes Églises catholiques orientales. <a href=\"#_dbpedia_2017\">(DBpedia, 2017)</a>"@fr, "Refers to the branch of Christianity characterized by a uniform, highly developed ritual canon and organizational structure with doctrinal roots based in the teachings of the Apostles of Jesus Christ in the first century, in the Alexandrian school of theology, and in Augustinian thought. In this religious branch, faith is considered an acceptance of revelation; revelation appears as doctrine. In juridical terms, it refers to the branch of Christianity distinguished as a unified, monolithic sacramental system under the governance of papal authority. Throughout much of its history, the seat of the Pope has been in Rome, thus \"Roman Catholicism\" is often used to distinguish this concept from the Orthodox Catholic church. <a href=\"#_getty_2017\">(Getty, 2017)</a>"@en, "Se refiere a la rama del cristianismo caracterizada por un canon ritual uniforme y altamente desarrollado y una estructura organizacional con raíces doctrinales basadas en las enseñanzas de los Apostoles de Jesucristo en la primera centuria, en la Escuela Alejandrina de teología, y en el pensamiento agustiniano. En esta rama de la religión, la fe es considerada como una aceptación de revelación; la revelación aparece como doctrina. Se refiere a la rama del cristianismo caracterizada por un canon ritual uniforme y altamente desarrollado y una estructura organizacional con raíces doctrinales basadas en las enseñanzas de los Apóstoles de Jesucristo en el primer siglo, en la Escuela Alejandrina de teología, y en el pensamiento agustiniano. En esta rama de la religión, la fe es considerada como una aceptación de revelación; la revelación aparece como doctrina. En términos jurídicos, se refiere a la rama del Cristianismo distinguido como sistema sacramental unificado, monolítico bajo gobierno de la autoridad papal. A través de la mayor parte de su historia, \"la silla del papal” ha estado en Roma, mediante este concepto el Catolicismo Romano se distingue de la Iglesia Católica Ortodoxa. <a href=\"#_getty_2017\">(Getty, 2017)</a>"@es, "Verwijst naar de richting van het christendom die zich kenmerkt door een uniforme, hoogontwikkelde rituele canon en organisatiestructuur met een doctrine die wortelt in de leer van de apostelen van Jezus Christus in de 1ste eeuw, in de theologie van de Alexandrijnse school en in het augustijner gedachtegoed. In deze godsdienstige richting wordt het geloof beschouwd als een aanvaarding van de openbaring; de openbaring heeft de vorm van een doctrine. In juridische zin verwijst de term naar de richting van het christendom die zich onderscheidt als een verenigd, monolithisch sacramenteel systeem onder het bestuur van het pauselijk gezag. Gedurende het grootste deel van de geschiedenis van dit systeem was de paus gevestigd in Rome en daarom wordt 'rooms-katholicisme' vaak gebruikt om dit begrip te onderscheiden van de orthodoxe katholieke kerk. <a href=\"#_getty_2017\">(Getty, 2017)</a>"@nl ;
    skos:inScheme cwrc:Religion ;
    prov:derivedFrom dbpedia:Catholic_Church, <http://vocab.getty.edu/aat/300073730> .

cwrc:childOf
    void:inDataset cwrc:datasetdefinition ;
    a owl:ObjectProperty ;
    rdfs:isDefinedBy <http://sparql.cwrc.ca/ontologies/cwrc-2017-08-03> ;
    rdfs:label "child of"@en, "enfant de"@fr ;
    rdfs:subPropertyOf cwrc:relativeOf .

cwrc:childrensWelfare
    void:inDataset cwrc:datasetdefinition ;
    a cwrc:PoliticalAffiliation, skos:Concept ;
    rdf:value "campaigner against child prostitution", "children's rights", "children's rights activist", "children's rights advocate" ;
    rdfs:comment "The description for this term is indebted to DBpedia."@en ;
    rdfs:isDefinedBy <http://sparql.cwrc.ca/ontologies/cwrc-2017-08-03> ;
    rdfs:label ""@fr, "children's welfare"@en ;
    skos:definition ""@fr, "Advocacy or activism for the rights or welfare of children. See: <a href=\"https://en.wikipedia.org/wiki/Category:Child_welfare\">https://en.wikipedia.org/wiki/Category:Child_welfare</a>"@en ;
    skos:inScheme cwrc:PoliticalAffiliation ;
    prov:derivedFrom <http://dbpedia.org/resource/Category:Child_welfare> .

cwrc:christianPacifism
    void:inDataset cwrc:datasetdefinition ;
    a cwrc:PoliticalAffiliation, skos:Concept ;
    rdf:value "christian pacifist" ;
    rdfs:comment "La description de ce terme est basée sur celle de DBPedia."@fr, "The description for this term is indebted to DBpedia."@en ;
    rdfs:isDefinedBy <http://sparql.cwrc.ca/ontologies/cwrc-2017-08-03> ;
    rdfs:label "Christian pacifism"@en, "Pacifisme chrétien"@fr ;
    skos:broaderTransitive cwrc:pacifism ;
    skos:definition "Christian pacifism is the theological and ethical position that any form of violence is incompatible with the Christian faith. Christian pacifists state that Jesus himself was a pacifist who taught and practiced pacifism and that his followers must do likewise. Notable Christian pacifists include Martin Luther King, Jr., Leo Tolstoy, and Ammon Hennacy. Hennacy believed that adherence to Christianity required not just pacifism but, because governments inevitably threatened or used force to resolve conflicts, anarchism. However, most Christian pacifists, including the peace churches, Christian Peacemaker Teams and individuals such as John Howard Yoder, make no claim to be anarchists. <a href=\"#_dbpedia_2017\">(DBpedia, 2017)</a>"@en, "Le pacifisme chrétien est un courant de pensée et d'action à l'intérieur du christianisme. Il désigne, a minima, le refus de la participation à la mise à mort d'un être humain à la guerre pour motif de conscience, et plus largement, le refus d'utiliser des moyens violents pour se défendre, parvenir à ses fins ou opposer une résistance. Bien qu'étant la position d'origine des premiers chrétiens , le pacifisme est considéré comme la position minoritaire au sein des Églises chrétiennes, la position dominante dans l'histoire de l'Église étant la doctrine de la guerre juste. Ce refus d'attenter à la vie de la personne humaine se fonde sur l'un ou plusieurs les aspects bibliques-théologiques suivants : l'être humain comme créature et image de Dieu à ne pas tuer (Ge 1.27 ; Ge 9.5-6)la parole du Décalogue (Ex 20,13) : « Tu ne tueras point », et l'extension de son champ d'applicationl'enseignement du Christ (« Ne vous opposez pas [violemment] au mal » (Mt 5.39) ; « Aimez vos ennemis » (Mt 5.44)l'exemple de la vie du Christ (1 Pi 2.21-23)la mort du Christ interprétée comme don de soi et comme manière de répondre au mal (Rm 5.6-10)la résurrection du Christ vue comme la justification par Dieu de la manière de vivre du Messie (Phil 2.6-11)l'enseignement des apôtres (« Soyez en paix avec tous » (Rm 12.18) ; « Sois vainqueur du mal par le bien » (Rm 12.21) Le pacifisme chrétien rejoint aujourd'hui l'ensemble de ce qui peut se désigner par le vocable de non-violence et qui se décline en dialogue, résolution de conflits, médiation, protestation non-violence, justice restaurative, etc. Le pacifisme chrétien et la non-violence sont notamment connu en milieu catholique à travers les efforts de pacification de la communauté de Sant'Egidio et les nombreuses missions diplomatiques de Jean-Paul II[réf. nécessaire]. Au sein du protestantisme, la résistance spirituelle au nazisme suscitée par le pasteur André Trocmé autour du Chambon-sur-Lignon, le combat de Martin Luther King pour les droits civiques, les Équipes chrétiennes d’action pour la paix (en) (Christian Peacemaker Teams), ou encore le pardon accordé par la communauté amish après la tuerie dans l'école de Nickel Mines en Pennsylvanie ont largement popularisé la non-violence. <a href=\"#_dbpedia_2017\">(DBpedia, 2017)</a>"@fr ;
    skos:inScheme cwrc:PoliticalAffiliation ;
    prov:derivedFrom dbpedia:Christian_pacifism .

cwrc:christianScience
    void:inDataset cwrc:datasetdefinition ;
    a cwrc:Religion, skos:Concept ;
    rdfs:comment "La description de ce terme est basée sur celle de DBPedia."@fr, "The description for this term is indebted to the Getty Art & Architecture Thesaurus."@en ;
    rdfs:isDefinedBy <http://sparql.cwrc.ca/ontologies/cwrc-2017-08-03> ;
    rdfs:label "Christenwetenschap"@nl, "Christian Science"@en, "Ciencia Cristiana"@es, "Science CHRÉTIENNE"@fr ;
    skos:broaderTransitive cwrc:christianity ;
    skos:definition "La Science chrétienne (ou Christian Science en anglais) se définit elle-même comme la « Science du Christ ». Sa fondatrice, la théologienne américaine Mary Baker Eddy, estime avoir redécouvert en 1866 les lois appliquées par Jésus dans la guérison des malades et la résolution des aléas de la vie, lois toujours démontrables aujourd'hui. Son observation des guérisons et résolutions diverses obtenues sur la base de sa théorie en prouve, selon elle, la validité. Ainsi, la Science chrétienne est « chrétienne » en ce sens qu’elle repose sur les enseignements de Jésus de Nazareth, tels qu'exposés dans le Nouveau Testament. La Science chrétienne se veut une religion pratique permettant l'application de lois divines démontrables. Afin d'assurer la diffusion de cette science, Mary Baker Eddy fonde en 1879 une Église sans credo, appelée « Église du Christ, Scientiste » (en anglais The First Church of Christ, Scientist), rassemblant de nos jours 1 800 églises dans 82 pays et quelques centaines de milliers de pratiquants, principalement aux États-Unis. Reconnue comme association cultuelle dans de nombreux pays, notamment aux États-Unis, la Science chrétienne précise que, malgré la confusion possible entre les deux noms, elle n’a rien de commun avec l’Église de Scientologie; de plus, bien qu'elle partage nombre de concepts métaphysiques avec les églises de la Nouvelle Pensée comme Unité, la Science divine et la Science religieuse, ce qui amène certains historiens et sociologues à les aborder ensemble dans leurs travaux, la Science chrétienne et ces églises ne se reconnaissent pas mutuellement comme faisant partie de la même mouvance. La principale critique de la Science chrétienne est qu'elle a un caractère alternatif et non complémentaire au traitement médical. Ainsi, les guérisons alléguées sont obtenues en dehors de tout contrôle médical. Ses guérisons de maladies fonctionnelles ou organiques sont considérées comme relevant de l’effet placebo par les détracteurs de la Science chrétienne (ce qui n’est d’ailleurs pas tellement en contradiction avec la Science chrétienne, qui ne considère la maladie que comme le résultat de simples croyances erronées, qu’il faudrait donc corriger pour recouvrer la santé.). La principale défense de la Science chrétienne est que chacun est libre de choisir la méthode de guérison qu'il juge la plus efficace et qu'il n'existe aucune contrainte à ce sujet. Les sympathisants mettent en avant les guérisons qu’ils disent avoir obtenues et réfutent toute idée de rejet de la médecine conventionnelle. <a href=\"#_dbpedia_2017\">(DBpedia, 2017)</a>"@fr, "Refers to a Christian denomination and movement founded by Mary Baker Eddy (1821-1910) that seeks to reinstate the Christian message of salvation from all evil, including sickness and disease as well as sin. Eddy, a semi-invalid who was interested in cures not involving medicine, claimed a recovery from a bad injury without medical assistance in 1866. Afterwards, she devoted herself to restoring the healing emphasis of early Christianity. In 1875 she finished writing the first edition of the 'Science and Health with Key to the Scriptures.' This work and the Bible are the principal texts of the movement and importance has been laid on establishing reading rooms where these works can make their own appeal to readers. The 'Christian Science Monitor' is also published by the denomination. Christian Science believes that ignorance is at the root of human unease and thus 'dis-ease.' Instead of seeking medical treatment, special Christian Science healers are to be consulted for spiritual healing. Health, happiness, and holiness can be restored by applying to all aspects of life practices and attitudes in keeping with the principal of divine harmony. The first Church of Christ, Scientist was founded in 1879 in Boston and its headquarters remain there. <a href=\"#_getty_2017\">(Getty, 2017)</a>"@en, "Se refiere a una secta y movimiento cristiano fundado por Mary Baker Eddy (1821-1910) que busca reincorporar el mensaje cristiano de salvación de todo mal, incluso la enfermedad y padecimiento así como el pecado. Eddy, un semi-inválido que estaba interesado en curas que no involucraran medicina, afirmó que se había recuperado de una lesión grave sin la ayuda médica en 1866. Después, se consagró a restaurar el énfasis curativo de la primera cristiandad. En 1875 ella terminó escribiendo la primera edición del \"la Ciencia y Salud con Llave a las Escrituras\". Este trabajo y la Biblia son los textos principales del movimiento y importancia se ha puesto en establecer salas de lectura donde estos trabajos pueden hacer su propia apelación a los lectores. El \"Instructivo de ciencia cristiano\" también fue publicado por la secta. La Ciencia Cristiana cree que la ignorancia es la raíz de los padecimientos humanos y por lo tanto de la enfermedad. En lugar de buscar tratamiento médico, los sanadores de la Ciencia Cristiana especiales serán consultados para la curación espiritual. La salud, felicidad, y santidad pueden ser restauradas aplicando a todos los aspectos de la vida prácticas y actitudes en concordancia con la armonía divina. La primera Iglesia Científica de Cristo, se fundó en 1879 en Boston y su centro principal permanece allí. <a href=\"#_getty_2017\">(Getty, 2017)</a>"@es, "Verwijst naar een christelijke gezindte en beweging die is gesticht door Mary Baker Eddy (1821-1910) en die streeft naar herbevestiging van de christelijke boodschap van verlossing van al het kwaad, met inbegrip van ziekte en zonde. Eddy, die half invalide was en geïnteresseerd in genezing zonder medicijnen, beweerde dat zij in 1866 zonder medische hulp was hersteld van zwaar letsel. Daarna wijdde zij zich aan het herstel van de nadruk op gebedsgenezing die het vroege christendom had gekenmerkt. In 1875 voltooide zij de eerste editie van haar boek 'Science and Health with Key to the Scriptures'. Dit werk en de Bijbel zijn de voornaamste geschriften van de beweging, die veel belang hecht aan de inrichting van leesruimten waar deze boeken een eigen beroep op de lezers kunnen doen. Ook de 'Christian Science Monitor' wordt door het kerkgenootschap uitgegeven. Volgens de leer van Christian Science is onwetendheid de wortel van het menselijk ongemak, de menselijke ziekte. In plaats van medische behandeling te zoeken moet men gebedsgenezers van Christian Science raadplegen voor spirituele genezing. Gezondheid, geluk en heiligheid kunnen worden hersteld door alle aspecten van de levenspraktijk en -houding aan te spreken in overeenstemming met het beginsel van goddelijke harmonie. De eerste Church of Christ, Scientist werd in 1879 in Boston gesticht en het hoofdkwartier van de beweging is daar nog altijd gevestigd. <a href=\"#_getty_2017\">(Getty, 2017)</a>"@nl ;
    skos:inScheme cwrc:Religion ;
    prov:derivedFrom dbpedia:Christian_Science, <http://vocab.getty.edu/aat/300264476> .

cwrc:christianSocialism
    void:inDataset cwrc:datasetdefinition ;
    a cwrc:PoliticalAffiliation, skos:Concept ;
    rdf:value "christian socialist" ;
    rdfs:comment "The description for this term is indebted to DBpedia."@en ;
    rdfs:isDefinedBy <http://sparql.cwrc.ca/ontologies/cwrc-2017-08-03> ;
    rdfs:label ""@fr, "Christian socialism"@en ;
    skos:broaderTransitive cwrc:socialism ;
    skos:definition ""@fr, "Christian socialism is a form of religious socialism based on the teachings of Jesus of Nazareth. Many Christian socialists believe capitalism to be idolatrous and rooted in greed, which some Christian denominations consider a mortal sin. Christian socialists identify the cause of inequality to be the greed that they associate with capitalism. Christian socialism became a major movement in the United Kingdom beginning in the 1960s through the Christian Socialist Movement, since 2013 known as Christians on the Left. Other earlier figures are also viewed as Christian socialists, such as the nineteenth century writers Frederick Denison Maurice (The Kingdom of Christ, 1838), John Ruskin (Unto This Last, 1862), Charles Kingsley (The Water-Babies, 1863), Thomas Hughes (Tom Brown's Schooldays, 1857), Frederick James Furnivall (co-creator of the Oxford English Dictionary), Adin Ballou (Practical Christian Socialism, 1854), and Francis Bellamy (a Baptist minister and the author of the United States' Pledge of Allegiance). <a href=\"#_dbpedia_2017\">(DBpedia, 2017)</a>"@en ;
    skos:inScheme cwrc:PoliticalAffiliation ;
    prov:derivedFrom dbpedia:Christian_socialism .

cwrc:christianity
    void:inDataset cwrc:datasetdefinition ;
    a cwrc:Religion, skos:Concept ;
    rdfs:comment "La description de ce terme est basée sur celle de DBPedia."@fr, "The description for this term is indebted to the Getty Art & Architecture Thesaurus."@en ;
    rdfs:isDefinedBy <http://sparql.cwrc.ca/ontologies/cwrc-2017-08-03> ;
    rdfs:label "Christelijk"@nl, "Christendom"@nl, "Christianisme"@fr, "Christianity"@en, "Cristianismo"@es, "chi tu chiao"@zh-latn-wadegile, "ji du jiao"@zh-latn-pinyin-x-notone, "jī dū jiāo"@zh-latn-pinyin-x-hanyu, "基督教"@zh-hant ;
    skos:broaderTransitive cwrc:abrahamicReligions ;
    skos:definition "Le christianisme est une religion abrahamique fondée sur l'enseignement, la personne et la vie de Jésus de Nazareth tels qu'ils sont interprétés par la tradition chrétienne à partir du Nouveau Testament de la Bible. Il s'agit d'une religion du salut considérant Jésus-Christ comme le Messie annoncé par les prophètes dans l'Ancien Testament qui vient sauver l'humanité du Mal et la faire participer à la vie de Dieu. La foi en la résurrection de Jésus est au cœur du christianisme car elle signifie le début d'une humanité nouvelle libérée du Mal. Les premières communautés chrétiennes naissent au Ier siècle en Judée et dans les grandes villes de la diaspora juive telles que Rome, Éphèse, Antioche et Alexandrie. Le christianisme se développe dès le IIe siècle dans l'Empire romain, dont il devient la religion officielle au IVe siècle, mais aussi en Perse, en Inde et en Éthiopie. Au Moyen-Âge, le christianisme devint majoritaire en Europe, tandis qu'il s'amenuise face à l'islam dans les régions où il est né. Depuis le XVIe siècle, il est devenu la religion la plus importante de la planète par son expansion en Amérique et, plus tard, en Afrique. Il est actuellement présent dans tous les pays du monde. Les Églises chrétiennes sont classiquement regroupées en trois principales branches : le catholicisme, le christianisme orthodoxe et le protestantisme représentant respectivement 50%, 12% et 37% du total des chrétiens en 2010. À la mi-2015, le nombre total de chrétiens dans le monde est évalué à 2,419 milliards, ce qui en fait la religion comptant le plus grand nombre de fidèles au monde devant l'islam qui en compte environ 1,6 milliard. <a href=\"#_dbpedia_2017\">(DBpedia, 2017)</a>"@fr, "Refers to the world religion and culture that developed in the first century CE, driven by the teachings of Jesus Christ of Nazareth. Its roots are in the Judaic tradition and the Old Testament. The tenets include a belief in the death and redemptive resurrection of Jesus. The religion incorporates a tradition of faith, ritual, and a form of church authority or leadership. <a href=\"#_getty_2017\">(Getty, 2017)</a>"@en, "Se refiere a la religión y cultura que se desarrolló en la primera centuria, guiado por la creencia y reverencia por la vida, enseñanza, muerte y resurrección redentiva de Jesucristo de Nazaret. La religión incorpora una tradición de fe, ritual y una forma de iglesia de autoridad y liderazgo. <a href=\"#_getty_2017\">(Getty, 2017)</a>"@es, "Verwijst naar de wereldreligie en -cultuur die in de eerste eeuw n. Chr. tot ontwikkeling kwam op basis van de leer van Jezus Christus van Nazareth. De wortels van deze religie liggen in de joodse traditie en het Oude Testament. Een van de kenmerkende grondbeginselen is het geloof in de dood en wederopstanding van Jezus. De religie omvat een traditie van geloof, rituelen en een vorm van kerkelijke autoriteit of leiderschap. <a href=\"#_getty_2017\">(Getty, 2017)</a>"@nl, "發展於西元一世紀的世界宗教與文化，跟隨拿薩勒(Nazareth)耶穌基督的教誨。源於猶太傳統及舊約聖經。教義包括相信耶穌之死與救贖復活。此教融合信仰傳統、儀式，及某種形式的教會權威或領導。 <a href=\"#_getty_2017\">(Getty, 2017)</a>"@zh-hant ;
    skos:inScheme cwrc:Religion ;
    prov:derivedFrom dbpedia:Christianity, <http://vocab.getty.edu/aat/300073711> .

cwrc:churchOfChristianScience
    dcterms:isReplacedBy cwrc:christianScience ;
    void:inDataset cwrc:datasetdefinition ;
    a skos:Concept ;
    rdfs:comment "Deprecated in favour of instance #christianScience."@en, "Désapprouver en faveur de l'instance #christianScience."@fr, "La description de ce terme est basée sur celle de DBPedia."@fr, "The description for this term is indebted to the Getty Art & Architecture Thesaurus."@en ;
    rdfs:isDefinedBy <http://sparql.cwrc.ca/ontologies/cwrc-2017-08-03> ;
    rdfs:label "Christenwetenschap"@nl, "Christian Science"@en, "Ciencia Cristiana"@es, "Science CHRÉTIENNE"@fr ;
    owl:deprecated true ;
    vs:term_status "deprecated"@en ;
    skos:broaderTransitive cwrc:christianity ;
    skos:definition "La Science chrétienne (ou Christian Science en anglais) se définit elle-même comme la « Science du Christ ». Sa fondatrice, la théologienne américaine Mary Baker Eddy, estime avoir redécouvert en 1866 les lois appliquées par Jésus dans la guérison des malades et la résolution des aléas de la vie, lois toujours démontrables aujourd'hui. Son observation des guérisons et résolutions diverses obtenues sur la base de sa théorie en prouve, selon elle, la validité. Ainsi, la Science chrétienne est « chrétienne » en ce sens qu’elle repose sur les enseignements de Jésus de Nazareth, tels qu'exposés dans le Nouveau Testament. La Science chrétienne se veut une religion pratique permettant l'application de lois divines démontrables. Afin d'assurer la diffusion de cette science, Mary Baker Eddy fonde en 1879 une Église sans credo, appelée « Église du Christ, Scientiste » (en anglais The First Church of Christ, Scientist), rassemblant de nos jours 1 800 églises dans 82 pays et quelques centaines de milliers de pratiquants, principalement aux États-Unis. Reconnue comme association cultuelle dans de nombreux pays, notamment aux États-Unis, la Science chrétienne précise que, malgré la confusion possible entre les deux noms, elle n’a rien de commun avec l’Église de Scientologie; de plus, bien qu'elle partage nombre de concepts métaphysiques avec les églises de la Nouvelle Pensée comme Unité, la Science divine et la Science religieuse, ce qui amène certains historiens et sociologues à les aborder ensemble dans leurs travaux, la Science chrétienne et ces églises ne se reconnaissent pas mutuellement comme faisant partie de la même mouvance. La principale critique de la Science chrétienne est qu'elle a un caractère alternatif et non complémentaire au traitement médical. Ainsi, les guérisons alléguées sont obtenues en dehors de tout contrôle médical. Ses guérisons de maladies fonctionnelles ou organiques sont considérées comme relevant de l’effet placebo par les détracteurs de la Science chrétienne (ce qui n’est d’ailleurs pas tellement en contradiction avec la Science chrétienne, qui ne considère la maladie que comme le résultat de simples croyances erronées, qu’il faudrait donc corriger pour recouvrer la santé.). La principale défense de la Science chrétienne est que chacun est libre de choisir la méthode de guérison qu'il juge la plus efficace et qu'il n'existe aucune contrainte à ce sujet. Les sympathisants mettent en avant les guérisons qu’ils disent avoir obtenues et réfutent toute idée de rejet de la médecine conventionnelle. <a href=\"#_dbpedia_2017\">(DBpedia, 2017)</a>"@fr, "Refers to a Christian denomination and movement founded by Mary Baker Eddy (1821-1910) that seeks to reinstate the Christian message of salvation from all evil, including sickness and disease as well as sin. Eddy, a semi-invalid who was interested in cures not involving medicine, claimed a recovery from a bad injury without medical assistance in 1866. Afterwards, she devoted herself to restoring the healing emphasis of early Christianity. In 1875 she finished writing the first edition of the 'Science and Health with Key to the Scriptures.' This work and the Bible are the principal texts of the movement and importance has been laid on establishing reading rooms where these works can make their own appeal to readers. The 'Christian Science Monitor' is also published by the denomination. Christian Science believes that ignorance is at the root of human unease and thus 'dis-ease.' Instead of seeking medical treatment, special Christian Science healers are to be consulted for spiritual healing. Health, happiness, and holiness can be restored by applying to all aspects of life practices and attitudes in keeping with the principal of divine harmony. The first Church of Christ, Scientist was founded in 1879 in Boston and its headquarters remain there. <a href=\"#_getty_2017\">(Getty, 2017)</a>"@en, "Se refiere a una secta y movimiento cristiano fundado por Mary Baker Eddy (1821-1910) que busca reincorporar el mensaje cristiano de salvación de todo mal, incluso la enfermedad y padecimiento así como el pecado. Eddy, un semi-inválido que estaba interesado en curas que no involucraran medicina, afirmó que se había recuperado de una lesión grave sin la ayuda médica en 1866. Después, se consagró a restaurar el énfasis curativo de la primera cristiandad. En 1875 ella terminó escribiendo la primera edición del \"la Ciencia y Salud con Llave a las Escrituras\". Este trabajo y la Biblia son los textos principales del movimiento y importancia se ha puesto en establecer salas de lectura donde estos trabajos pueden hacer su propia apelación a los lectores. El \"Instructivo de ciencia cristiano\" también fue publicado por la secta. La Ciencia Cristiana cree que la ignorancia es la raíz de los padecimientos humanos y por lo tanto de la enfermedad. En lugar de buscar tratamiento médico, los sanadores de la Ciencia Cristiana especiales serán consultados para la curación espiritual. La salud, felicidad, y santidad pueden ser restauradas aplicando a todos los aspectos de la vida prácticas y actitudes en concordancia con la armonía divina. La primera Iglesia Científica de Cristo, se fundó en 1879 en Boston y su centro principal permanece allí. <a href=\"#_getty_2017\">(Getty, 2017)</a>"@es, "Verwijst naar een christelijke gezindte en beweging die is gesticht door Mary Baker Eddy (1821-1910) en die streeft naar herbevestiging van de christelijke boodschap van verlossing van al het kwaad, met inbegrip van ziekte en zonde. Eddy, die half invalide was en geïnteresseerd in genezing zonder medicijnen, beweerde dat zij in 1866 zonder medische hulp was hersteld van zwaar letsel. Daarna wijdde zij zich aan het herstel van de nadruk op gebedsgenezing die het vroege christendom had gekenmerkt. In 1875 voltooide zij de eerste editie van haar boek 'Science and Health with Key to the Scriptures'. Dit werk en de Bijbel zijn de voornaamste geschriften van de beweging, die veel belang hecht aan de inrichting van leesruimten waar deze boeken een eigen beroep op de lezers kunnen doen. Ook de 'Christian Science Monitor' wordt door het kerkgenootschap uitgegeven. Volgens de leer van Christian Science is onwetendheid de wortel van het menselijk ongemak, de menselijke ziekte. In plaats van medische behandeling te zoeken moet men gebedsgenezers van Christian Science raadplegen voor spirituele genezing. Gezondheid, geluk en heiligheid kunnen worden hersteld door alle aspecten van de levenspraktijk en -houding aan te spreken in overeenstemming met het beginsel van goddelijke harmonie. De eerste Church of Christ, Scientist werd in 1879 in Boston gesticht en het hoofdkwartier van de beweging is daar nog altijd gevestigd. <a href=\"#_getty_2017\">(Getty, 2017)</a>"@nl ;
    skos:inScheme cwrc:Religion ;
    prov:derivedFrom dbpedia:Christian_Science, <http://vocab.getty.edu/aat/300264476> .

cwrc:churchOfEngland
    void:inDataset cwrc:datasetdefinition ;
    a cwrc:Religion, skos:Concept, foaf:Organization ;
    rdfs:isDefinedBy <http://sparql.cwrc.ca/ontologies/cwrc-2017-08-03> ;
    rdfs:label ""@fr, "Church of England"@en ;
    skos:broaderTransitive cwrc:christianity ;
    skos:definition ""@en, ""@fr ;
    skos:inScheme cwrc:Religion .

cwrc:churchOfIreland
    void:inDataset cwrc:datasetdefinition ;
    a cwrc:Religion, skos:Concept, foaf:Organization ;
    rdfs:comment "La description de ce terme est basée sur celle de DBPedia."@fr ;
    rdfs:isDefinedBy <http://sparql.cwrc.ca/ontologies/cwrc-2017-08-03> ;
    rdfs:label "Church of Ireland"@en, "Église d'Irlande"@fr ;
    skos:broaderTransitive cwrc:anglicanism ;
    skos:definition "L'Église d'Irlande (irlandais : Eaglais na hÉireann, anglais : Church of Ireland) est une communauté religieuse autonome de la communion anglicane, dont le rayon d'action touche la République d'Irlande et l'Irlande du Nord. Comme d'autres Églises anglicanes, elle s'affirme « catholique » et « réformée ». Quand l'Église d'Angleterre rompt avec le Pape et l'Église catholique romaine, l'Église d'Irlande évolue également vers la Réforme, gardant son statut juridique et ses possessions, si sa doctrine change. Ainsi, de nos jours, l'Église, dans ses cathédrales et ses églises, conserve largement l'héritage des constructions médiévales de l'île. La nouvelle Église indépendante n'est cependant pas suivie par la majorité de la population ; l'Église catholique romaine conserve le soutien de la plus grande partie des habitants, et ce jusqu'à aujourd'hui. En dépit de son caractère minoritaire, cependant, l'Église d'Irlande conserve le statut de religion d'État jusqu'au désétablissement de 1869, quand Gladstone abolit l'Acte d'établissement. Le nombre d'églises est tombé brusquement au cours du XXe siècle, particulièrement en République d'Irlande, après l'indépendance ; le dernier recensement de la République montre un exemple rare de résistance à la crise de la foi. Aujourd'hui, l'Église d'Irlande est, après l'Église catholique, la deuxième plus importante Église de l'île d'Irlande. C'est également la plus importante Église protestante de la République d'Irlande et le deuxième plus importante d'Irlande du Nord, après l'Église presbytérienne d'Irlande. Elle est gouvernée par un synode général du clergé et des laïcs et organisée en douze diocèses. Elle a à sa tête l'archevêque d'Armagh, qui porte le titre de \"Primat de toute l'Irlande\". L'archevêque actuel est Richard Clarke qui a succédé le à Alan Harper ; l'autre archevêque est celui de Dublin John Neill. <a href=\"#_dbpedia_2017\">(DBpedia, 2017)</a>"@fr, "The Church of Ireland (Irish: Eaglais na hÉireann Scots: Kirk o Airlann) is a Christian church in Ireland and an autonomous province of the Anglican Communion. It is organised on an all-Ireland basis and is the second-largest Christian church on the island after the Catholic Church. Like other Anglican churches, it has retained elements of pre-Reformation practice, notably its episcopal polity, while rejecting the primacy of the Bishop of Rome. Nevertheless, in theological and liturgical matters, it incorporates many principles of the Reformation, particularly those espoused during the English Reformation. The church self identifies as being both Catholic and Reformed. Within the church, differences exist between those members who are more Catholic-leaning (high church) and those who are more Protestant-leaning (low church or evangelical). For historical and cultural reasons, the Church of Ireland is generally identified as a Protestant church. The Church of Ireland is the second-largest in the Republic of Ireland, with around 130,000 members, and the third-largest in Northern Ireland, with around 260,000 members. <a href=\"#_dbpedia_2017\">(DBpedia, 2017)</a>"@en ;
    skos:inScheme cwrc:Religion ;
    prov:derivedFrom dbpedia:Church_of_Ireland .

cwrc:civilLibertarianism
    void:inDataset cwrc:datasetdefinition ;
    a cwrc:PoliticalAffiliation, skos:Concept ;
    rdf:value "civil libertarian" ;
    rdfs:comment "The description for this term is indebted to DBpedia."@en ;
    rdfs:isDefinedBy <http://sparql.cwrc.ca/ontologies/cwrc-2017-08-03> ;
    rdfs:label ""@fr, "civil libertarianism"@en ;
    skos:definition ""@fr, "Civil libertarianism is a strain of political thought that supports civil liberties, or which emphasizes the supremacy of individual rights and personal freedoms over and against any kind of authority (such as a state, a corporation, social norms imposed through peer pressure, etc.). Civil libertarianism is not a complete ideology; rather, it is a collection of views on the specific issues of civil liberties and civil rights. <a href=\"#_dbpedia_2017\">(DBpedia, 2017)</a>"@en ;
    skos:inScheme cwrc:PoliticalAffiliation ;
    prov:derivedFrom dbpedia:Civil_libertarianism .

cwrc:civilRights
    void:inDataset cwrc:datasetdefinition ;
    a cwrc:PoliticalAffiliation, skos:Concept ;
    rdf:value "civil rights", "civil rights activist", "personal rights advocate", "pro civil rights" ;
    rdfs:comment "La description de ce terme est basée sur celle de DBPedia."@fr, "The description for this term is indebted to DBpedia."@en ;
    rdfs:isDefinedBy <http://sparql.cwrc.ca/ontologies/cwrc-2017-08-03> ;
    rdfs:label "Droits civiques"@fr, "civil rights movement"@en ;
    skos:definition "Civil and political rights are a class of rights that protect individuals' freedom from infringement by governments, social organizations, and private individuals. They ensure one's ability to participate in the civil and political life of the society and state without discrimination or repression. Civil rights include the ensuring of peoples' physical and mental integrity, life, and safety; protection from discrimination on grounds such as race, gender, national origin, colour, age, political affiliation, ethnicity, religion, or disability; and individual rights such as privacy and the freedoms of thought, speech, religion, press, assembly, and movement. Political rights include natural justice (procedural fairness) in law, such as the rights of the accused, including the right to a fair trial; due process; the right to seek redress or a legal remedy; and rights of participation in civil society and politics such as freedom of association, the right to assemble, the right to petition, the right of self-defense, and the right to vote. Civil and political rights form the original and main part of international human rights. They comprise the first portion of the 1948 Universal Declaration of Human Rights (with economic, social, and cultural rights comprising the second portion). The theory of three generations of human rights considers this group of rights to be \"first-generation rights\", and the theory of negative and positive rights considers them to be generally negative rights. <a href=\"#_dbpedia_2017\">(DBpedia, 2017)</a>"@en, "Les droits civiques désignent les protections et privilèges des libertés fondamentales accordés à tous les citoyens par la loi contre toutes les discriminations. <a href=\"#_dbpedia_2017\">(DBpedia, 2017)</a>"@fr ;
    skos:inScheme cwrc:PoliticalAffiliation ;
    prov:derivedFrom dbpedia:Civil_and_political_rights .

cwrc:co-operativeMovement
    void:inDataset cwrc:datasetdefinition ;
    a cwrc:PoliticalAffiliation, skos:Concept ;
    rdfs:comment "The description for this term is indebted to DBpedia."@en ;
    rdfs:isDefinedBy <http://sparql.cwrc.ca/ontologies/cwrc-2017-08-03> ;
    rdfs:label ""@fr, "co-operative movement"@en ;
    skos:definition ""@fr, "Supporter of the co-operative movement. <a href=\"https://en.wikipedia.org/wiki/History_of_the_cooperative_movement\">https://en.wikipedia.org/wiki/History_of_the_cooperative_movement</a>"@en ;
    skos:inScheme cwrc:PoliticalAffiliation ;
    prov:derivedFrom dbpedia:History_of_the_cooperative_movement .

cwrc:communalism
    void:inDataset cwrc:datasetdefinition ;
    a cwrc:PoliticalAffiliation, skos:Concept ;
    rdf:value "communalist" ;
    rdfs:comment "The description for this term is indebted to DBpedia."@en ;
    rdfs:isDefinedBy <http://sparql.cwrc.ca/ontologies/cwrc-2017-08-03> ;
    rdfs:label ""@fr, "communalism"@en ;
    skos:definition ""@fr, "Communalism usually refers to a system that integrates communal ownership and federations of highly localised independent communities. A prominent libertarian socialist, Murray Bookchin, defines communalism as \"a theory of government or a system of government in which independent communes participate in a federation\", as well as \"the principles and practice of communal ownership\". This usage of communalism appears to have emerged during the late 20th century to distinguish commune-based systems from other political movements and/or governments espousing (if not actually practicing) similar ideas. In particular, earlier communities and movements advocating such practices that were often described as \"anarchist\", \"socialist\" and/or \"communist\". Many historical communities practicing utopian socialism or anarchist communism did implement internal rules of communalist property ownership in the context of federated communalism. It is at least theoretically possible for a federation of communes to include communes which do not practice communalist rules of property, which is to say, that the overall national government may be a federation of communes, but that private property rather than communalist property is the order within each such commune. Karl Marx, often viewed as the founder of modern communism, criticized older forms, including primitive communism and/or utopian socialism, as poorly conceived and/or prone to disintegration in practise. Communalism in the form described above is distinct from the predominant usage in South Asian forms of English: allegiance to a particular ethnic and/or religious group rather than to a broader society. As such, this usage is synonymous with sectarianism and associated with communal violence. <a href=\"#_dbpedia_2017\">(DBpedia, 2017)</a>"@en ;
    skos:inScheme cwrc:PoliticalAffiliation ;
    prov:derivedFrom dbpedia:Communalism .

cwrc:communism
    void:inDataset cwrc:datasetdefinition ;
    a cwrc:PoliticalAffiliation, skos:Concept ;
    rdf:value "christian communist", "communist" ;
    rdfs:comment "La description de ce terme est basée sur celle de DBPedia."@fr, "The description for this term is indebted to DBpedia."@en ;
    rdfs:isDefinedBy <http://sparql.cwrc.ca/ontologies/cwrc-2017-08-03> ;
    rdfs:label "Communisme"@fr, "communism"@en ;
    skos:definition "In political and social sciences, communism (from Latin communis, \"common, universal\") is a social, political, and economic ideology and movement whose ultimate goal is the establishment of the communist society, which isa socioeconomic order structured upon the common ownership of the means of production and the absence of social classes, money, and the state. Communism includes a variety of schools of thought, which broadly include Marxism, anarchism (anarchist communism), and the political ideologies grouped around both. All these hold in common the analysis that the current order of society stems from its economic system, capitalism, that in this system, there are two major social classes: the working class – who must work to survive, and who make up a majority of society – and the capitalist class – a minority who derive profit from employing the proletariat, through private ownership of the means of production (the physical and institutional means with which commodities are produced and distributed), and that political, social and economic conflict between these two classes will trigger a fundamental change in the economic system, and by extension a wide-ranging transformation of society. The primary element which will enable this transformation, according to this analysis, is the social ownership of the means of production. <a href=\"#_dbpedia_2017\">(DBpedia, 2017)</a>"@en, "Le communisme (du latin communis – commun, universel) est un ensemble de doctrines politiques issues du socialisme et, pour la plupart, du marxisme, opposées au capitalisme et visant à l'instauration d'une société sans classes sociales. Plus largement, ce terme est associé au mouvement communiste international né après la Première Guerre mondiale, fruit d'une scission de la IIe Internationale provoquée par les bolcheviks. Il renvoie également, dans le contexte de la guerre froide, à une alliance géopolitique (bloc communiste) dominée par l'Union soviétique, ainsi qu'au régime politique à parti unique, dictatorial ou totalitaire, en vigueur dans les pays du bloc communiste. Dans son sens d'origine, le communisme est une forme d'organisation sociale sans classes, sans État et sans monnaie, où les biens matériels seraient partagés. Au XIXe siècle, le mot « communisme » entre dans le vocabulaire du socialisme. Il se rattache en particulier à l'œuvre de Karl Marx et Friedrich Engels - qui le reprennent à leur compte en 1848 dans le Manifeste du Parti communiste - et, par extension, à l'école de pensée marxiste. En 1917, les bolcheviks, dirigés par Lénine, prennent le pouvoir en Russie lors de la Révolution d'Octobre. Cet évènement change radicalement le sens du mot communisme : il désigne désormais un mouvement politique international, né d'une scission du socialisme, et qui se reconnaît dans le courant révolutionnaire incarné par les bolcheviks comme dans l'interprétation du marxisme par Lénine. Le communisme se présente désormais comme la véritable expression politique du mouvement ouvrier, au détriment de la social-démocratie dont il est issu. Selon cette acception, le communisme constitue l'un des phénomènes les plus importants du XXe siècle, qui a pu être qualifié de « siècle du communisme » tant cette idéologie y a tenu un rôle moteur. Lénine et ses partisans créent en 1919 l'Internationale communiste (dite Troisième Internationale, ou Komintern) afin de regrouper à l'échelle internationale les partisans de la Russie soviétique. L'Union des républiques socialistes soviétiques (URSS), fondée en 1922 pour fédérer les territoires de l'ex-empire russe, dirige via le Komintern les activités des partis communistes du monde entier : elle domine ainsi la mouvance communiste, malgré l'existence de courants dissidents. Après la mort de Lénine, Joseph Staline s'impose comme le maître absolu de l'URSS et du mouvement communiste mondial. En 1941, durant la Seconde Guerre mondiale, l'URSS est attaquée par l'Allemagne nazie avec laquelle elle avait conclu un pacte deux ans plus tôt. Les troupes soviétiques jouent alors un rôle déterminant dans la défaite du nazisme. Après-guerre, l'URSS accède au rang de superpuissance : elle occupe militairement l'essentiel de l'Europe de l'Est, dont les pays deviennent des États communistes, formant le bloc de l'Est. La Chine bascule également dans le camp communiste en 1949. Le Rideau de fer qui sépare l'Europe et la progression spectaculaire du communisme amènent le monde à se diviser en « blocs » rivaux : la guerre froide oppose ainsi durant plusieurs décennies les pays communistes au « monde libre », au sein duquel les États-Unis constituent la superpuissance rivale de l'URSS. La Chine de Mao occupe quant à elle une place à part après la rupture sino-soviétique. À l'apogée de l'influence du communisme dans le monde, un quart de l'humanité vit dans des pays communistes. Dans les années 1980, l'URSS tente de remédier à sa sclérose économique et politique en lançant un mouvement de réformes, la perestroïka : mais ce processus aboutit à l'effondrement général des régimes communistes européens entre 1989 et 1991. Par la suite, bien qu'en net déclin, le communisme ne disparaît pas : si des partis anciennement communistes ont adopté d'autres identités, d'autres ont conservé leur nom et sont associés au pouvoir dans certains pays. À Cuba, au Viêt Nam, au Laos et en Corée du Nord, des pays communistes existent encore, sans se conformer à un mode de gouvernement unique. La République populaire de Chine, pays le plus peuplé de la planète, est toujours dirigée par un Parti communiste ; convertie à l'économie de marché, elle est aujourd'hui l'une des principales puissances mondiales. En tant que dictatures à parti unique, les régimes communistes se sont tous rendus coupables de violations des droits de l'homme ; certains, comme l'URSS sous Staline et la Chine sous Mao, se sont livrés à des crimes de masse, le nombre de leurs victimes s'élevant à plusieurs millions de morts. Le bilan historique du communisme, qui englobe un ensemble de réalités très différentes les unes des autres, demeure cependant, du fait même de sa complexité, contrasté et polémique. Le communisme a fait l'objet de diverses approches historiographiques concurrentes, longtemps handicapées par la difficulté d'accès aux documents et par les contextes politiques nationaux et internationaux. La fin de la guerre froide et l'ouverture des archives du bloc de l'Est ont depuis bouleversé le champ des études sur le communisme, sans mettre fin à toutes les controverses autour du sujet. <a href=\"#_dbpedia_2017\">(DBpedia, 2017)</a>"@fr ;
    skos:inScheme cwrc:PoliticalAffiliation ;
    prov:derivedFrom dbpedia:Communism .

cwrc:congregationalChurch
    dcterms:isReplacedBy cwrc:congragationalism ;
    void:inDataset cwrc:datasetdefinition ;
    a skos:Concept ;
    rdfs:comment "Deprecated in favour of instance #congregationalism."@en, "Désapprouver en faveur de l'instance #congragationalism."@fr, "La description de ce terme est basée sur celle de DBPedia."@fr ;
    rdfs:isDefinedBy <http://sparql.cwrc.ca/ontologies/cwrc-2017-08-03> ;
    rdfs:label "Congregational Church"@en, "Églises congrégationalistes"@fr ;
    owl:deprecated true ;
    vs:term_status "deprecated"@en ;
    skos:broaderTransitive cwrc:christianity ;
    skos:definition "Congregational churches are Protestant Christian churches practicing congregationalist church governance, in which each congregation independently and autonomously runs its own affairs. Congregationalism is often considered to be a part of the wider Reformed tradition. Many Congregational churches claim their descent from Protestant denominations formed on a theory of union published by the theologian Robert Browne in 1582. These arose from the ideas of nonconforming Protestants during the Puritan Reformation of the Church of England. In Great Britain, the early Congregationalists were called Separatists or Independents to distinguish them from the similarly Calvinistic Presbyterians. Congregational churches were widely established in the Plymouth Colony and the Massachusetts Bay Colony (later New England), and together wrote the Cambridge Platform of 1648 which described the autonomy of the church and its association with others. Within the United States, the model of Congregational churches was carried by migrating settlers from New England into New York, then into the Old North West, and further. With their insistence on independent local bodies, they became important in many social reform movements, including abolitionism, temperance, and women's suffrage. Modern Congregationalism in the United States is largely split into three bodies: the United Church of Christ, the National Association of Congregational Christian Churches and the Conservative Congregational Christian Conference, which is the most theologically conservative. Congregationalism, as defined by the Pew Research Center, is estimated to represent 0.5% of the worldwide Protestant population. <a href=\"#_dbpedia_2017\">(DBpedia, 2017)</a>"@en, "Les Églises congrégationalistes sont des églises protestantes de tradition réformée, pratiquant une forme d’organisation d’église où chaque paroisse se gère de manière entièrement autonome et indépendante. Le congrégationalisme se caractérise plus comme un mouvement que comme une dénomination chrétienne en raison de sa conviction fondamentale en faveur de l’autonomie complète de chaque paroisse. Malgré la forte diversité théologique inhérente à leur forme d'organisation, la plupart des congrégationalistes se considèrent d'abord comme des réformés, soit traditionnels soit néo-orthodoxes (barthiens). Les congrégationalistes, selon la définition du centre de recherche indépendant Pew Research Center, représentent environ 0,5% de la population protestante mondiale, soit 4 millions de chrétiens répartis essentiellement dans les grands pays anglophones (Royaume-Uni, États-Unis, Canada, Australie, Afrique du sud, Irlande) et dans quelques « terres de mission » (Argentine, Bulgarie, Îles Samoa). Leur rôle historique et leur influence, notamment aux États-Unis, excèdent largement ces chiffres. <a href=\"#_dbpedia_2017\">(DBpedia, 2017)</a>"@fr ;
    skos:inScheme cwrc:Religion ;
    prov:derivedFrom dbpedia:Congregational_church .

cwrc:congregationalism
    void:inDataset cwrc:datasetdefinition ;
    a cwrc:Religion, skos:Concept ;
    rdfs:comment "La description de ce terme est basée sur celle de DBPedia."@fr ;
    rdfs:isDefinedBy <http://sparql.cwrc.ca/ontologies/cwrc-2017-08-03> ;
    rdfs:label "Congregationalism"@en, "Églises congrégationalistes"@fr ;
    skos:broaderTransitive cwrc:protestantism ;
    skos:definition "Congregational churches are Protestant Christian churches practicing congregationalist church governance, in which each congregation independently and autonomously runs its own affairs. Congregationalism is often considered to be a part of the wider Reformed tradition. Many Congregational churches claim their descent from Protestant denominations formed on a theory of union published by the theologian Robert Browne in 1582. These arose from the ideas of nonconforming Protestants during the Puritan Reformation of the Church of England. In Great Britain, the early Congregationalists were called Separatists or Independents to distinguish them from the similarly Calvinistic Presbyterians. Congregational churches were widely established in the Plymouth Colony and the Massachusetts Bay Colony (later New England), and together wrote the Cambridge Platform of 1648 which described the autonomy of the church and its association with others. Within the United States, the model of Congregational churches was carried by migrating settlers from New England into New York, then into the Old North West, and further. With their insistence on independent local bodies, they became important in many social reform movements, including abolitionism, temperance, and women's suffrage. Modern Congregationalism in the United States is largely split into three bodies: the United Church of Christ, the National Association of Congregational Christian Churches and the Conservative Congregational Christian Conference, which is the most theologically conservative. Congregationalism, as defined by the Pew Research Center, is estimated to represent 0.5% of the worldwide Protestant population. <a href=\"#_dbpedia_2017\">(DBpedia, 2017)</a>"@en, "Les Églises congrégationalistes sont des églises protestantes de tradition réformée, pratiquant une forme d’organisation d’église où chaque paroisse se gère de manière entièrement autonome et indépendante. Le congrégationalisme se caractérise plus comme un mouvement que comme une dénomination chrétienne en raison de sa conviction fondamentale en faveur de l’autonomie complète de chaque paroisse. Malgré la forte diversité théologique inhérente à leur forme d'organisation, la plupart des congrégationalistes se considèrent d'abord comme des réformés, soit traditionnels soit néo-orthodoxes (barthiens). Les congrégationalistes, selon la définition du centre de recherche indépendant Pew Research Center, représentent environ 0,5% de la population protestante mondiale, soit 4 millions de chrétiens répartis essentiellement dans les grands pays anglophones (Royaume-Uni, États-Unis, Canada, Australie, Afrique du sud, Irlande) et dans quelques « terres de mission » (Argentine, Bulgarie, Îles Samoa). Leur rôle historique et leur influence, notamment aux États-Unis, excèdent largement ces chiffres. <a href=\"#_dbpedia_2017\">(DBpedia, 2017)</a>"@fr ;
    skos:inScheme cwrc:Religion ;
    prov:derivedFrom dbpedia:Congregational_church .

cwrc:conscientiousObjection
    void:inDataset cwrc:datasetdefinition ;
    a cwrc:PoliticalAffiliation, skos:Concept ;
    rdfs:comment "The description for this term is indebted to DBpedia."@en ;
    rdfs:isDefinedBy <http://sparql.cwrc.ca/ontologies/cwrc-2017-08-03> ;
    rdfs:label ""@fr, "conscientious objection"@en ;
    skos:broaderTransitive cwrc:pacifism ;
    skos:definition ""@fr, "A conscientious objector is an \"individual who has claimed the right to refuse to perform military service\" on the grounds of freedom of thought, conscience, disability or religion. In general, conscientious objector status is considered only in the context of military conscription and is not applicable to volunteer military forces. In some countries, conscientious objectors are assigned to an alternative civilian service as a substitute for conscription or military service. Some conscientious objectors consider themselves pacifist, non-interventionist, non-resistant, non-aggressionist, or antimilitarist. On March 8, 1995 the United Nations Commission on Human Rights resolution 1995/83 stated that \"persons performing military service should not be excluded from the right to have conscientious objections to military service.\" This was re-affirmed in 1998, when resolution 1998/77 recognized that \"persons [already] performing military service may develop conscientious objections.\". A number of organizations around the world celebrate the principle on May 15 as International Conscientious Objectors Day. The term has also been extended to objecting to working for the military-industrial complex due to a crisis of conscience. <a href=\"#_dbpedia_2017\">(DBpedia, 2017)</a>"@en ;
    skos:inScheme cwrc:PoliticalAffiliation ;
    prov:derivedFrom dbpedia:Conscientious_objector .

cwrc:conservatism
    void:inDataset cwrc:datasetdefinition ;
    a cwrc:PoliticalAffiliation, skos:Concept ;
    rdf:value "conservative" ;
    rdfs:comment "La description de ce terme est basée sur celle de DBPedia."@fr, "The description for this term is indebted to DBpedia."@en ;
    rdfs:isDefinedBy <http://sparql.cwrc.ca/ontologies/cwrc-2017-08-03> ;
    rdfs:label "Conservatisme"@fr, "conservatism"@en ;
    skos:definition "Conservatism as a political and social philosophy promotes retaining traditional social institutions in the context of culture and civilization. Some conservatives seek to preserve things as they are, emphasizing stability and continuity, while others, called reactionaries, oppose modernism and seek a return to \"the way things were\". The first established use of the term in a political context originated with François-René de Chateaubriand in 1818, during the period of Bourbon restoration that sought to roll back the policies of the French Revolution. The term, historically associated with right-wing politics, has since been used to describe a wide range of views. There is no single set of policies that are universally regarded as conservative, because the meaning of conservatism depends on what is considered traditional in a given place and time. Thus conservatives from different parts of the world—each upholding their respective traditions—may disagree on a wide range of issues. Edmund Burke, an 18th-century politician who opposed the French Revolution but supported the American Revolution, is credited as one of the main theorists of conservatism in Britain in the 1790s. According to Quintin Hogg, the chairman of the British Conservative Party in 1959, \"Conservatism is not so much a philosophy as an attitude, a constant force, performing a timeless function in the development of a free society, and corresponding to a deep and permanent requirement of human nature itself.\" <a href=\"#_dbpedia_2017\">(DBpedia, 2017)</a>"@en, "Le conservatisme est une philosophie politique qui est en faveur des valeurs traditionnelles et qui s'oppose au progressisme. Les cultures ayant chacune des valeurs différentes, les conservateurs selon leur culture ont des buts différents. Mais tous les conservateurs promeuvent la défense (statu quo) ou le retour à des valeurs établies (statu quo ante). Pour Michael Freeden, le conservatisme croit seulement en un changement limité de ce qui est naturel ou organique ; aussi, pour lui, l'ordre social est indépendant de la volonté humaine. Le terme vient de « conserver » ; du latin conservare, « maintenir, observer (une loi, une coutume) » composé de servare « préserver, garder ». Bien que ce ne soit pas une idéologie en soi, le conservatisme est une philosophie politique dont les idées sont en grande partie liées à leur contexte d'existence. Il est défini en partie par l'accent mis sur la tradition comme source de sagesse, bien au-delà de ce qui peut être démontré ou explicitement établi. Il se fonde sur la conservation d'un ordre préétabli, selon les conventions, chacun à sa place. <a href=\"#_dbpedia_2017\">(DBpedia, 2017)</a>"@fr ;
    skos:inScheme cwrc:PoliticalAffiliation ;
    prov:derivedFrom dbpedia:Conservatism .

cwrc:conservativeFeminism
    void:inDataset cwrc:datasetdefinition ;
    a cwrc:PoliticalAffiliation, skos:Concept ;
    rdf:value "conservative feminism" ;
    rdfs:comment "The description for this term is indebted to DBpedia."@en ;
    rdfs:isDefinedBy <http://sparql.cwrc.ca/ontologies/cwrc-2017-08-03> ;
    rdfs:label ""@fr, "conservative feminism"@en ;
    skos:broaderTransitive cwrc:feminism ;
    skos:definition ""@fr, "Feminism that tends towards social conservativism. See <a href=\"https://en.wikipedia.org/wiki/Feminism\">https://en.wikipedia.org/wiki/Feminism</a>"@en ;
    skos:inScheme cwrc:PoliticalAffiliation ;
    prov:derivedFrom dbpedia:Feminism .

cwrc:conservativePartyUk
    void:inDataset cwrc:datasetdefinition ;
    a cwrc:PoliticalAffiliation, skos:Concept ;
    rdf:value "conservative party" ;
    rdfs:comment "The description for this term is indebted to DBpedia."@en ;
    rdfs:isDefinedBy <http://sparql.cwrc.ca/ontologies/cwrc-2017-08-03> ;
    rdfs:label ""@fr, "Conservative Party (UK)"@en ;
    skos:definition ""@fr, "The Tories were members of two political parties which existed, sequentially, in the Kingdom of England, the Kingdom of Great Britain and later the United Kingdom of Great Britain and Ireland from the 17th to the early 19th centuries. The first Tories emerged in 1678 in England, when they opposed the Whig-supported Exclusion Bill which set out to disinherit the heir presumptive James, Duke of York (who eventually became James II of England and VII of Scotland). This party ceased to exist as an organised political entity in the early 1760s, although it was used as a term of self-description by some political writers. A few decades later, a new Tory party would rise to establish a hold on government between 1783 and 1830, with William Pitt the Younger followed by Robert Jenkinson, 2nd Earl of Liverpool. The Earl of Liverpool was succeeded by fellow Tory Arthur Wellesley, 1st Duke of Wellington, whose term included the Catholic Emancipation, which occurred mostly due to the election of Daniel O'Connell as a Catholic MP from Ireland. When the Whigs subsequently regained control, the Representation of the People Act 1832 removed the rotten boroughs, many of which were controlled by Tories. In the following general election, the Tory ranks were reduced to 180 MPs. Under the leadership of Robert Peel, the Tamworth Manifesto was issued, which began to transform the Tories into the Conservative Party. However, Peel lost many of his supporters by repealing the Corn Laws, causing the party to break apart. One faction, led by the Earl of Derby and Benjamin Disraeli, survived to become the modern Conservative Party, whose members are commonly still referred to as Tories. <a href=\"#_dbpedia_2017\">(DBpedia, 2017)</a>"@en ;
    skos:inScheme cwrc:PoliticalAffiliation ;
    skos:related cwrc:toryPartyUk ;
    prov:derivedFrom <http://dbpedia.org/resource/Tories_(British_political_party)> .

cwrc:constitutionalism
    void:inDataset cwrc:datasetdefinition ;
    a cwrc:PoliticalAffiliation, skos:Concept ;
    rdf:value "constitutional feminist", "constitutionalist" ;
    rdfs:comment "La description de ce terme est basée sur celle de DBPedia."@fr, "The description for this term is indebted to DBpedia."@en ;
    rdfs:isDefinedBy <http://sparql.cwrc.ca/ontologies/cwrc-2017-08-03> ;
    rdfs:label "Constitutionnalisme"@fr, "constitutionalism"@en ;
    skos:definition "Constitutionalism is \"a complex of ideas, attitudes, and patterns of behavior elaborating the principle that the authority of government derives from and is limited by a body of fundamental law\". Political organizations are constitutional to the extent that they \"contain institutionalized mechanisms of power control for the protection of the interests and liberties of the citizenry, including those that may be in the minority\". As described by political scientist and constitutional scholar David Fellman: Constitutionalism is descriptive of a complicated concept, deeply embedded in historical experience, which subjects the officials who exercise governmental powers to the limitations of a higher law. Constitutionalism proclaims the desirability of the rule of law as opposed to rule by the arbitrary judgment or mere fiat of public officials…. Throughout the literature dealing with modern public law and the foundations of statecraft the central element of the concept of constitutionalism is that in political society government officials are not free to do anything they please in any manner they choose; they are bound to observe both the limitations on power and the procedures which are set out in the supreme, constitutional law of the community. It may therefore be said that the touchstone of constitutionalism is the concept of limited government under a higher law. <a href=\"#_dbpedia_2017\">(DBpedia, 2017)</a>"@en, "Le constitutionnalisme est une théorie du droit qui insiste sur le rôle et la fonction de la Constitution dans la hiérarchie des normes par rapport à la loi, ainsi que sur le contrôle de constitutionnalité des lois. On l'oppose parfois au légicentrisme, qui défend la suprématie de la loi, émanation de la souveraineté populaire. En droit international, le constitutionnalisme est une conception qui tend à s'opposer au pluralisme juridique. <a href=\"#_dbpedia_2017\">(DBpedia, 2017)</a>"@fr ;
    skos:inScheme cwrc:PoliticalAffiliation ;
    prov:derivedFrom dbpedia:Constitutionalism .

cwrc:contraryTo
    void:inDataset cwrc:datasetdefinition ;
    a owl:ObjectProperty ;
    rdfs:isDefinedBy <http://sparql.cwrc.ca/ontologies/cwrc-2017-08-03> ;
    rdfs:label "contraire à"@fr, "contrary to"@en .

cwrc:covenanters
    void:inDataset cwrc:datasetdefinition ;
    a cwrc:PoliticalAffiliation, skos:Concept ;
    rdfs:comment "La description de ce terme est basée sur celle de DBPedia."@fr, "The description for this term is indebted to DBpedia."@en ;
    rdfs:isDefinedBy <http://sparql.cwrc.ca/ontologies/cwrc-2017-08-03> ;
    rdfs:label "Covenantaire"@fr, "Covenanters"@en ;
    skos:definition "Les Covenantaires formèrent un important mouvement religieux et politique en Écosse au XVIIe siècle. Du point de vue religieux, ce mouvement s'attacha surtout à promouvoir et à développer le presbytérianisme, et à en faire une forme de gouvernement souhaitée par le peuple, en opposition avec l'Épiscopalisme, qui avait les faveurs de la couronne. Du point de vue politique, ce mouvement vit d'importantes évolutions du caractère et du fonctionnement du Parlement écossais, qui commença à se démarquer progressivement de ses origines médiévales. Dans son ensemble, ce mouvement était essentiellement conservateur dans le ton, mais il amorça une révolution qui embrasa l'Écosse, l'Angleterre et l'Irlande, et qui fut appelée les guerres des Trois Royaumes. Le nom Covenantaire provient de « covenant », qui est un mot de l'ancien français, passé dans le moyen anglais, qui signifiait à l'origine convention, chose convenue, et qui désigna, dans la loi anglaise, un accord formel, une promesse solennelle. En Écosse, le terme prit le sens biblique d'« Alliance » ou de « Promesse ». Le premier engagement de ce genre fut signé par les Écossais de toutes les classes, en 1588, lorsque Philippe II menaçait l'Angleterre et la Réforme par sa fameuse Invincible Armada. Il contenait une profession de foi protestante, une réprobation de l'Église romaine et un serment de défense mutuelle et d'union. La destruction de la flotte espagnole rendit cette confédération sans objet. Au siècle suivant, le « National Covenant » de 1638, qui prit comme base des documents précédents du même genre, était surtout intéressé à préserver la Réforme de toute innovation issue de la couronne britannique. Son document jumeau de 1643, « Solemn League and Covenant », se préoccupait également de religion, même s'il s'agissait principalement d'un traité d'alliance entre les covenantaires d'Écosse et le Parlement d'Angleterre, soucieux de se soutenir lors de la guerre civile de plus en plus violente contre le roi Charles Ier. <a href=\"#_dbpedia_2017\">(DBpedia, 2017)</a>"@fr, "The Covenanters were a Scottish Presbyterian movement that played an important part in the history of Scotland, and to a lesser extent that of England and Ireland, during the 17th century. Presbyterian denominations tracing their history to the Covenanters and often incorporating the name continue the ideas and traditions in Scotland and internationally. They derive their name from the term covenant after the Covenant between God and the Israelites in the Old Testament. There were two important covenants in Scottish history, the National Covenant and the Solemn League and Covenant. <a href=\"#_dbpedia_2017\">(DBpedia, 2017)</a>"@en ;
    skos:inScheme cwrc:PoliticalAffiliation ;
    prov:derivedFrom dbpedia:Covenanter .

cwrc:cwrc
    a foaf:Organization ;
    foaf:homepage <http://www.cwrc.ca/> ;
    foaf:logo <http://sparql.cwrc.ca/images/CWRCLogo-Horz-FullColour.png> ;
    foaf:name "Le Collaboratoire scientifique des écrits du Canada"@fr, "The Canadian Writing Research Collaboratory"@en .

cwrc:datasetdefinition
    cc:Jurisdiction dbpedia:Canada ;
    cc:attributionURL <http://www.cwrc.ca/> ;
    cc:license <http://creativecommons.org/licenses/by-nc/4.0/> ;
    loc:ctb cwrc:ConstanceCrompton, cwrc:originalOrlandoAuthor ;
    loc:fnd cwrc:sshrc ;
    loc:pdr cwrc:SusanBrown ;
    dcterms:creator cwrc:AbiLemak, cwrc:AlliyyaMo, cwrc:ColinFaulkner, cwrc:JadePenancier, cwrc:JohnSimpson, cwrc:KimMartin, cwrc:RobWarren, cwrc:SusanBrown ;
    dcterms:description "L'Ontologie CWRC est l'ontologie du Collaboratoire scientifique des écrits du Canada."@fr, "The CWRC Ontology is the ontology of the Canadian Writing Research Collaboratory."@en ;
    dcterms:publisher cwrc:cwrc ;
    dcterms:subject <http://id.loc.gov/authorities/subjects/sh2009007122>, <http://id.loc.gov/authorities/subjects/sh85013838>, <http://id.loc.gov/authorities/subjects/sh85019388>, <http://id.loc.gov/authorities/subjects/sh85043777>, <http://id.loc.gov/authorities/subjects/sh85077519> ;
    dcterms:title "L'Ontologie CWRC"@fr, "The CWRC Ontology"@en ;
    void:entities "389" ;
    void:triples "4691" ;
    a void:Dataset ;
    rdfs:comment "L'Ontologie CWRC est l'ontologie du Collaboratoire scientifique des écrits du Canada."@fr, "The CWRC Ontology is the ontology of the Canadian Writing Research Collaboratory."@en ;
    rdfs:isDefinedBy <http://sparql.cwrc.ca/ontologies/cwrc-2017-08-03> ;
    rdfs:label "L'Ontologie CWRC"@fr, "The CWRC Ontology"@en ;
    skos:definition "L'Ontologie CWRC est l'ontologie du Collaboratoire scientifique des écrits du Canada."@fr, "The CWRC Ontology is the ontology of the Canadian Writing Research Collaboratory."@en ;
    foaf:logo <http://www.cwrc.ca/wp-content/uploads/2010/11/CWRC_logo_v074.gif> ;
    foaf:name "L'Ontologie CWRC"@fr, "The CWRC Ontology"@en .

cwrc:daughterOf
    void:inDataset cwrc:datasetdefinition ;
    a owl:ObjectProperty ;
    rdfs:isDefinedBy <http://sparql.cwrc.ca/ontologies/cwrc-2017-08-03> ;
    rdfs:label "daughter of"@en, "fille de"@fr ;
    rdfs:subPropertyOf cwrc:childOf .

cwrc:disestablismentarianism
    void:inDataset cwrc:datasetdefinition ;
    a cwrc:PoliticalAffiliation, skos:Concept ;
    rdf:value "anti-anglican", "anti-episcopal", "anti-episcopalian", "anti-tithes" ;
    rdfs:comment "The description for this term is indebted to DBpedia."@en ;
    rdfs:isDefinedBy <http://sparql.cwrc.ca/ontologies/cwrc-2017-08-03> ;
    rdfs:label ""@fr, "disestablismentarianism"@en ;
    skos:definition ""@fr, "Disestablishmentarianism refers to campaigns to sever links between church and state, particularly in relation to the Church of England as an established church. It was initially a movement in the United Kingdom in the 18th century. The established churches in Wales and Ireland could not count on even nominal adherence by a majority of the population of those countries. In Ireland, the predominantly Roman Catholic population campaigned against the position of the established Anglican Church of Ireland - eventually disestablished in Ireland from 1 January 1871. In England there was a campaign by Liberals, dissenters and nonconformists to disestablish the Church of England in the 19th century. The campaigners were called \"Liberationists\" (the \"Liberation Society\" was founded by Edward Miall in 1844). This campaign failed, but nearly all of the legal disabilities of nonconformists were gradually dismantled. The campaign for disestablishment was revived in the 20th century when Parliament rejected the 1929 revision of the Book of Common Prayer, leading to calls for separation of Church and State to prevent political interference in matters of worship. In the late 20th century, reform of the House of Lords also brought into question the position of the Lords Spiritual. Nick Clegg, the former Deputy Prime Minister of the United Kingdom and Leader of the Liberal Democrats, said in April 2014 that he thought the Church of England and the British state should be separated \"in the long run\". Prime Minister David Cameron, responding to Clegg's comments, said that disestablishmentarianism is \"a long-term Liberal idea, but it is not a Conservative one\" and that he believed having an established church works well. The Church of England was disestablished in Wales in 1920, becoming the Church in Wales. An Act of the British Parliament enabling the disestablishment of the Church of Ireland was passed in 1869, coming into effect on 1 January 1871. The Church of Scotland was disestablished in 1929 but remains the largest church in Scotland. <a href=\"#_dbpedia_2017\">(DBpedia, 2017)</a>"@en ;
    skos:inScheme cwrc:PoliticalAffiliation ;
    prov:derivedFrom dbpedia:Disestablishmentarianism .

cwrc:dissentProtestant
    void:inDataset cwrc:datasetdefinition ;
    a cwrc:Religion, skos:Concept ;
    rdfs:isDefinedBy <http://sparql.cwrc.ca/ontologies/cwrc-2017-08-03> ;
    rdfs:label "Dissent (Protestant)"@en, "dissidents (ou non-conformistes)"@fr ;
    skos:broaderTransitive cwrc:churchOfEngland ;
    skos:definition "In English church history, a nonconformist was a Protestant who did not \"conform\" to the governance and usages of the established Church of England. Broad use of the term was precipitated after the Restoration of the British monarchy in 1660, when the Act of Uniformity 1662 re-established the opponents of reform within the Church of England. By the late 19th-century the term specifically included the Reformed Christians (Presbyterians, Congregationalists and other Calvinist sects), plus the Baptists and Methodists. The English Dissenters such as the Puritans who violated the Act of Uniformity 1559 — typically by practising radical, sometimes separatist, dissent — were retrospectively labelled as nonconformists.<a href=\"#_dbpedia_2017\">(DBpedia, 2017)</a>"@en, "Les non-conformistes, appelés aussi Dissidents (dissenters), étaient ceux qui, en Angleterre, refusaient de suivre la doctrine de l'Église anglicane. Il s'agissait notamment des Puritains, des Presbytériens, des Anabaptistes ou des Calvinistes. On oppose les non-conformistes aux Conformistes.<a href=\"#_dbpedia_2017\">(DBpedia, 2017)</a>"@fr ;
    skos:inScheme cwrc:Religion ;
    prov:derivedFrom dbpedia:English_Dissenters, dbpedia:Nonconformist .

cwrc:dissenters
    dcterms:isReplacedBy cwrc:dissentProtestant ;
    void:inDataset cwrc:datasetdefinition ;
    a skos:Concept ;
    rdfs:comment "Deprecated in favour of instance #dissentProtestant."@en, "Désapprouver en faveur de l'instance #dissentProtestant."@fr ;
    rdfs:isDefinedBy <http://sparql.cwrc.ca/ontologies/cwrc-2017-08-03> ;
    rdfs:label "Dissenters"@en, "dissidents (ou non-conformistes)"@fr ;
    owl:deprecated true ;
    vs:term_status "deprecated"@en ;
    skos:broaderTransitive cwrc:churchOfEngland ;
    skos:definition ""@fr, "\"One who dissents or disagrees in matters of opinion, belief, &c. The term 'dissenter' is, however, practically restricted to the special sense of a member of a religious body in England which has, for one reason or another, separated from the Established Church. Strictly, the term includes the English Roman Catholics, who in the original draft of the Relief Act of 1791 were styled “Protesting Catholic Dissenters.” It is in practice, however, restricted to the “Protestant Dissenters” referred to in sec. ii. of the Toleration Act of 1688.\"<a href=\"#_britannica_1911\">(Encyclopedia Britannica, 1911)</a>"@en ;
    skos:inScheme cwrc:Religion .

cwrc:dissentingChristianity
    void:inDataset cwrc:datasetdefinition ;
    a cwrc:Religion, skos:Concept ;
    rdfs:isDefinedBy <http://sparql.cwrc.ca/ontologies/cwrc-2017-08-03> ;
    rdfs:label "Dissenting Christianity"@en, "Dissidence anglaise"@fr ;
    skos:broaderTransitive cwrc:protestantism ;
    skos:definition "\"Les Dissidents anglais (en anglais : English Dissenters ou nonconformists) sont des protestants anglais qui firent sécession de l'Église d'Angleterre. Ils s'opposaient à l'interférence de l'État dans les affaires religieuses et fondèrent leurs propres communautés du XVIe au XVIIIe siècle. Les Dissidents triomphèrent un temps lors du gouvernement d'Oliver Cromwell, mais après la Restauration de la monarchie, en 1660, l'épiscopat fut rétabli et les droits civiques des Dissidents limités, dès les années 1660, par une série de lois dont l’Act of Uniformity, le Corporation Act et le Test Act. Ce n'est qu'en 1828 que ces lois discriminatoires sont abrogées. Parmi les Dissidents les plus connus, on peut citer le fondateur de la secte des Puritains Henry Jacob (en) (1563-1624), l'éditeur Joseph Johnson (1738-1809), la mystique Jane Leade (1623-1704), le philosophe Richard Price (1723-1791), ou encore le chimiste et théologien Joseph Priestley (1733-1804), ainsi que le fondateur d'une académie dissidente à Kendal (Cumbria), le révérend Caleb Rotherham, qui instruisit l'un des pères de la Révolution industrielle, le fondeur et beau-frère de Joseph Priestley, John Wilkinson.\"<a href=\"#_dbpedia_2017\">(DBpedia, 2017)</a>"@fr, "\"One who dissents or disagrees in matters of opinion, belief, &c. The term 'dissenter' is, however, practically restricted to the special sense of a member of a religious body in England which has, for one reason or another, separated from the Established Church. Strictly, the term includes the English Roman Catholics, who in the original draft of the Relief Act of 1791 were styled “Protesting Catholic Dissenters.” It is in practice, however, restricted to the “Protestant Dissenters” referred to in sec. ii. of the Toleration Act of 1688.\"<a href=\"#_britannica_1911\">(Encyclopedia Britannica, 1911)</a>"@en ;
    skos:inScheme cwrc:Religion .

cwrc:dissentingChurches
    dcterms:isReplacedBy cwrc:dissentProtestant ;
    void:inDataset cwrc:datasetdefinition ;
    a skos:Concept ;
    rdfs:comment "Deprecated in favour of instance #dissentProtestant."@en, "Désapprouver en faveur de l'instance #dissentProtestant."@fr ;
    rdfs:isDefinedBy <http://sparql.cwrc.ca/ontologies/cwrc-2017-08-03> ;
    rdfs:label "Dissenting Churches"@en, "Églises dissidentes"@fr ;
    owl:deprecated true ;
    vs:term_status "deprecated"@en ;
    skos:broaderTransitive cwrc:churchOfEngland ;
    skos:definition "English Dissenters were Christians who separated from the Church of England in the 16th, 17th and 18th centuries. A dissenter (from the Latin dissentire, “to disagree”) is one who disagrees in matters of opinion, belief, etc. English Dissenters opposed state interference in religious matters, and founded their own churches, educational establishments, and communities; some emigrated to the New World. They originally agitated for a wide-reaching Protestant Reformation of the Established Church, and triumphed briefly under Oliver Cromwell.<a href=\"#_dbpedia_2017\">(DBpedia, 2017)</a>"@en, "Les Dissidents anglais (en anglais : English Dissenters ou nonconformists) sont des protestants anglais qui firent sécession de l'Église d'Angleterre1. Ils s'opposaient à l'interférence de l'État dans les affaires religieuses et fondèrent leurs propres communautés du xvie au xviiie siècle. Les Dissidents triomphèrent un temps lors du gouvernement d'Oliver Cromwell, mais après la Restauration de la monarchie, en 1660, l'épiscopat fut rétabli et les droits civiques des Dissidents limités, dès les années 1660, par une série de lois dont l’Act of Uniformity, le Corporation Act et le Test Act. Ce n'est qu'en 1828 que ces lois discriminatoires sont abrogées.<a href=\"#_dbpedia_2017\">(DBpedia, 2017)</a>"@fr ;
    skos:inScheme cwrc:Religion ;
    prov:derivedFrom dbpedia:English_Dissenters .

cwrc:dressReform
    void:inDataset cwrc:datasetdefinition ;
    a cwrc:PoliticalAffiliation, skos:Concept ;
    rdf:value "dress reformer" ;
    rdfs:comment "The description for this term is indebted to DBpedia."@en ;
    rdfs:isDefinedBy <http://sparql.cwrc.ca/ontologies/cwrc-2017-08-03> ;
    rdfs:label ""@fr, "dress reform"@en ;
    skos:definition ""@fr, "Victorian dress reform was an objective of the Victorian dress reform movement (also known as the rational dress movement) of the middle and late Victorian era, comprising various reformers who proposed, designed, and wore clothing considered more practical and comfortable than the fashions of the time. Dress reformists were largely middle class women involved in the first wave of feminism in the United States and in Britain, from the 1850s through the 1890s. The movement emerged in the Progressive Era along with calls for temperance, women's education, suffrage and moral purity. Dress reform called for emancipation from the \"dictates of fashion\", expressed a desire to “cover the limbs as well as the torso adequately,” and promoted \"rational dress\". The movement had its greatest success in the reform of women's undergarments, which could be modified without exposing the wearer to social ridicule. Dress reformers were also influential in persuading women to adopt simplified garments for athletic activities such as bicycling or swimming. The movement was much less concerned with men's clothing, although it initiated the widespread adoption of knitted wool union suits or long johns. Some proponents of the movement established dress reform parlors, or storefronts, where women could buy sewing patterns for the newfangled garments, or buy them directly. <a href=\"#_dbpedia_2017\">(DBpedia, 2017)</a>"@en ;
    skos:inScheme cwrc:PoliticalAffiliation ;
    prov:derivedFrom dbpedia:Victorian_dress_reform .

cwrc:dreyfusard
    void:inDataset cwrc:datasetdefinition ;
    cwrc:contraryTo cwrc:antisematism ;
    a cwrc:PoliticalAffiliation, skos:Concept ;
    rdfs:comment "The description for this term is indebted to DBpedia."@en ;
    rdfs:isDefinedBy <http://sparql.cwrc.ca/ontologies/cwrc-2017-08-03> ;
    rdfs:label ""@fr, "Dreyfusard"@en ;
    skos:broaderTransitive cwrc:humanRights ;
    skos:definition ""@fr, "Supporters of Captain Alfred Dreyfus in his prosecution by the French military. See: <a href=\"https://en.wikipedia.org/wiki/Dreyfus_affair\">https://en.wikipedia.org/wiki/Dreyfus_affair</a>"@en ;
    skos:inScheme cwrc:PoliticalAffiliation ;
    skos:related cwrc:anti-Antisemitism ;
    prov:derivedFrom dbpedia:Dreyfus_affair .

cwrc:educationReform
    void:inDataset cwrc:datasetdefinition ;
    a cwrc:PoliticalAffiliation, skos:Concept ;
    rdf:value "education reformer", "educational reform", "educational reformer", "educationalist", "state education movement" ;
    rdfs:comment "The description for this term is indebted to DBpedia."@en ;
    rdfs:isDefinedBy <http://sparql.cwrc.ca/ontologies/cwrc-2017-08-03> ;
    rdfs:label ""@fr, "education reform"@en ;
    skos:definition ""@fr, "Education reform is the name given to the goal of changing public education. Historically, reforms have taken different forms because the motivations of reformers have differed. However, since the 1980s, education reform has been focused on changing the existing system from one focused on inputs to one focused on outputs (i.e., student achievement). In the United States, education reform acknowledges and encourages public education as the primary source of K-12 education for American youth. Education reformers desire to make public education into a market (in the form of an input-output system), where accountability creates high-stakes from curriculum standards tied to standardized tests.As a result of this input-output system, equality has been conceptualized as an end point, which is often evidenced by an achievement gap among diverse populations. This conceptualization of education reform is based on the market-logic of competition. As a consequence, competition creates inequality which has continued to drive the market-logic of equality at an end point by reproduce the achievement gap among diverse youth. Overall, education reform has and continues to be used as a substitute for needed economic reforms in the United States. The one constant for all forms of education reform includes the idea that small changes in education will have large social returns in citizen health, wealth and well-being. For example, a stated motivation has been to reduce cost to students and society. From ancient times until the 1800s, one goal was to reduce the expense of a classical education. Ideally, classical education is undertaken with a highly educated full-time (extremely expensive) personal tutor. Historically, this was available only to the most wealthy. Encyclopedias, public libraries and grammar schools are examples of innovations intended to lower the cost of a classical education. Related reforms attempted to develop similar classical results by concentrating on \"why\", and \"which\" questions neglected by classical education. Abstract, introspective answers to these questions can theoretically compress large amounts of facts into relatively few principles. This path was taken by some Transcendentalist educators, such as Amos Bronson Alcott.In the early modern age, Victorian schools were reformed to teach commercially useful topics, such as modern languages and mathematics, rather than classical subjects, such as Latin and Greek. Many reformers focused on reforming society by reforming education on more scientific, humanistic, pragmatic or democratic principles. John Dewey and Anton Makarenko are prominent examples of such reformers. Some reformers incorporated several motivations, e.g. Maria Montessori, who both \"educated for peace\" (a social goal), and to \"meet the needs of the child\" (A humanistic goal). In historic Prussia, an important motivation for the invention of Kindergarten was to foster national unity by teaching a national language while children were young enough that learning a language was easy. Reform has taken many forms and directions. Throughout history and the present day, the meaning and methods of education have changed through debates over what content or experiences result in an educated individual or an educated society. Changes may be implemented by individual educators and/or by broad-based school organization and/or by curriculum changes with performance evaluations. <a href=\"#_dbpedia_2017\">(DBpedia, 2017)</a>"@en ;
    skos:inScheme cwrc:PoliticalAffiliation ;
    prov:derivedFrom dbpedia:Education_reform .

cwrc:egalitarianism
    void:inDataset cwrc:datasetdefinition ;
    a cwrc:PoliticalAffiliation, skos:Concept ;
    rdf:value "egalitarian" ;
    rdfs:comment "La description de ce terme est basée sur celle de DBPedia."@fr, "The description for this term is indebted to DBpedia."@en ;
    rdfs:isDefinedBy <http://sparql.cwrc.ca/ontologies/cwrc-2017-08-03> ;
    rdfs:label "egalitarianism"@en, "Égalitarisme"@fr ;
    skos:definition "Egalitarianism (from French  égal, meaning \"equal\")—or equalitarianism—is a trend of thought that favors equality for all people. Egalitarian doctrines maintain that all humans are equal in fundamental worth or social status, according to the Stanford Encyclopedia of Philosophy. According to the Merriam-Webster Dictionary, the term has two distinct definitions in modern English: either as a political doctrine that all people should be treated as equals and have the same political, economic, social, and civil rights; or as a social philosophy advocating the removal of economic inequalities among people, economic egalitarianism, or the decentralization of power. Some sources define egalitarianism as the point of view that equality reflects the natural state of humanity. <a href=\"#_dbpedia_2017\">(DBpedia, 2017)</a>"@en, "L'égalitarisme est une doctrine politique prônant l'égalité des citoyens en matière politique, économique et/ou sociale, selon les contextes. Dans le sens vulgaire, l'égalitarisme désigne plus particulièrement la doctrine qui a pour valeur politique suprême l'égalité matérielle de tous. <a href=\"#_dbpedia_2017\">(DBpedia, 2017)</a>"@fr ;
    skos:inScheme cwrc:PoliticalAffiliation ;
    skos:related cwrc:feminism ;
    prov:derivedFrom dbpedia:Egalitarianism .

cwrc:egyptianNationalism
    void:inDataset cwrc:datasetdefinition ;
    a cwrc:PoliticalAffiliation, skos:Concept ;
    rdfs:comment "The description for this term is indebted to DBpedia."@en ;
    rdfs:isDefinedBy <http://sparql.cwrc.ca/ontologies/cwrc-2017-08-03> ;
    rdfs:label ""@fr, "Egyptian nationalism"@en ;
    skos:definition ""@fr, "Egyptian nationalism refers to the nationalism of Egyptians and Egyptian culture. Egyptian nationalism has typically been a civic nationalism that has emphasized the unity of Egyptians regardless of ethnicity or religion. Egyptian nationalism first manifested itself in Pharaonism beginning in the 19th century that identified Egypt as being a unique and independent political unit in the world since the era of the Pharaohs in ancient Egypt. Both the Arabic language spoken in modern Egypt and the ancient Egyptian language are Afroasiatic languages. The rule of Muhammad Ali of Egypt led Egypt into an advanced level of socioeconomic development in comparison with Egypt's neighbours, which along with the discoveries of relics of ancient Egyptian civilization, helped to foster Egyptian identity and Egyptian nationalism. The Urabi movement in the 1870s and 1880s was the first major Egyptian nationalist movement that demanded an end to the alleged despotism of the Muhammed Ali family and demanded curbing the growth of European influence in Egypt, it campaigned under the nationalist slogan of \"Egypt for Egyptians\". After the British occupation of Egypt in 1882, Egyptian nationalism became focused upon ending British colonial rule. Egyptian nationalism reached its peak in popularity in 1919 when revolution against British rule took place in response to wartime deprivations imposed by the British upon Egypt during World War I. Three years of protest and political turmoil followed until Britain unilaterally declared the independence of Egypt in 1922 that was a monarchy, though Britain reserved several areas for British supervision. During the period of the Kingdom of Egypt, Egyptian nationalists remained determined to terminate the remaining British presence in Egypt. Though Arab nationalism rose as a political force in the 1930s, there remained a strong regional attachment to Egypt by those who advocated cooperation with other Arab or Muslim neighbours. After the Egyptian Revolution of 1952 that overthrew the monarchy and established a republic, Gamal Abdel Nasser rose to power on themes that mixed Arab and Egyptian nationalism. Nasser saw Egypt as the leader of the Arab states and saw Egypt's role as promoting Arab solidarity against both the West and Israel. Egypt was briefly united with Syria from 1958 until 1961 when Syria abandoned the union. Nasser's successors, Anwar Sadat and Hosni Mubarak de-emphasized Arab nationalism and re-emphasized Egyptian nationalism based on Egypt's distinctiveness within the Arab world. Sadat and Mubarak also abandoned Nasser's Arab nationalist conflict with Israel and the West. The Arab Spring in Egypt in 2011 that forced the resignation of Mubarak from power and resulted in multiparty elections, has raised questions over the future of Egyptian nationalism. In particular the previous secular regimes of Nasser, Sadat, and Mubarak avoided direct religious conflicts between the majority Muslims and the minority Coptic Christians through their emphasis on secular Egyptian nationalist culture, while concerns have been raised on whether this Egyptian nationalist culture will remain with the political changes caused by the Arab Spring. This has especially become an issue after a series of episodes of Muslim-Christian violence erupted in Egypt in 2011. <a href=\"#_dbpedia_2017\">(DBpedia, 2017)</a>"@en ;
    skos:inScheme cwrc:PoliticalAffiliation ;
    prov:derivedFrom dbpedia:Egyptian_nationalism .

cwrc:elderRights
    void:inDataset cwrc:datasetdefinition ;
    a cwrc:PoliticalAffiliation, skos:Concept ;
    rdf:value "elder care activist" ;
    rdfs:comment "The description for this term is indebted to DBpedia."@en ;
    rdfs:isDefinedBy <http://sparql.cwrc.ca/ontologies/cwrc-2017-08-03> ;
    rdfs:label ""@fr, "elder rights"@en ;
    skos:definition ""@fr, "Elder rights are the rights of the aged, who in the United States are not recognized as a constitutionally protected class. Common rights issues faced by elders include age-related job discrimination (such as forced age of retirement), lack of access to medical treatments because of age or age-related obstacles, societal perceptions of ability/disability due to age, and vulnerability to abuse, including financial, physical, psychological, social, and sexual because of diminished capacity and lack of access to/ability to use technology. <a href=\"#_dbpedia_2017\">(DBpedia, 2017)</a>"@en ;
    skos:inScheme cwrc:PoliticalAffiliation ;
    prov:derivedFrom dbpedia:Elder_rights .

cwrc:england
    void:inDataset cwrc:datasetdefinition ;
    a cwrc:GeographicalHeritage, owl:Thing ;
    rdfs:isDefinedBy <http://sparql.cwrc.ca/ontologies/cwrc-2017-08-03> ;
    rdfs:label "Angleterre"@fr, "England"@en ;
    owl:sameAs <http://eurovoc.europa.eu/5438> ;
    skos:broader cwrc:englishLabel ;
    skos:definition ""@en, ""@fr ;
    foaf:name "England (Geographical Heritage)"@en .

cwrc:englandLabel
    void:inDataset cwrc:datasetdefinition ;
    a skos:Concept, skosxl:Label ;
    rdfs:isDefinedBy <http://sparql.cwrc.ca/ontologies/cwrc-2017-08-03> ;
    rdfs:label "Angleterre"@fr, "England"@en ;
    owl:oneOf (cwrc:england
    ) ;
    skos:definition ""@en, ""@fr ;
    skos:inScheme cwrc:TextLabels ;
    foaf:name "England"@en .

cwrc:englishLabel
    void:inDataset cwrc:datasetdefinition ;
    a skos:Concept, skosxl:Label ;
    rdf:value "english" ;
    rdfs:isDefinedBy <http://sparql.cwrc.ca/ontologies/cwrc-2017-08-03> ;
    rdfs:label "englais"@fr, "english"@en ;
    owl:oneOf (cwrc:EnglishNationalHeritage
        locl:eng
        cwrc:EnglishNationalIdentity
        cwrc:england
    ) ;
    skos:definition ""@en, ""@fr ;
    skos:inScheme cwrc:TextLabels ;
    skos:narrower locl:eng ;
    foaf:name "english"@en .

cwrc:englishNationalHeritage
    void:inDataset cwrc:datasetdefinition ;
    a cwrc:NationalHeritage, skos:Concept ;
    rdfs:isDefinedBy <http://sparql.cwrc.ca/ontologies/cwrc-2017-08-03> ;
    rdfs:label "Anglais"@fr, "English"@en ;
    owl:sameAs <http://sws.geonames.org/6269131/> ;
    skos:broader cwrc:englishLabel ;
    skos:definition ""@en, ""@fr .

cwrc:englishNationalIdentity
    void:inDataset cwrc:datasetdefinition ;
    a cwrc:NationalIdentity, skos:Concept ;
    rdfs:isDefinedBy <http://sparql.cwrc.ca/ontologies/cwrc-2017-08-03> ;
    rdfs:label "Anglais"@fr, "English"@en ;
    owl:sameAs <http://eurovoc.europa.eu/5438> ;
    skos:broader cwrc:englishLabel ;
    skos:definition ""@en, ""@fr .

cwrc:entrepreneurial-industrialism
    dcterms:isReplacedBy cwrc:entrepreneurial-industrialist ;
    void:inDataset cwrc:datasetdefinition ;
    a skos:Concept ;
    rdfs:comment "Deprecated in favour of instance #entrepreneurial."@en, "Désapprouver en faveur de l'instance #entrepreneurial."@fr ;
    rdfs:isDefinedBy <http://sparql.cwrc.ca/ontologies/cwrc-2017-08-03> ;
    rdfs:label "entrepreneurial industrialism"@en, "entrepreneuriat industriel"@fr ;
    owl:deprecated true ;
    vs:term_status "deprecated"@en ;
    skos:definition ""@en, ""@fr .

cwrc:entrepreneurial-industrialist
    void:inDataset cwrc:datasetdefinition ;
    a cwrc:SocialClass, skos:Concept ;
    rdfs:isDefinedBy <http://sparql.cwrc.ca/ontologies/cwrc-2017-08-03> ;
    rdfs:label "entrepreneur"@fr, "entrepreneurial"@en ;
    skos:definition ""@fr, "Involves larges-scale enterprises such as running factories, or backing such enterprises through investing money, for instance, Elizabeth Montagu or Beatrice Webb."@en ;
    skos:inScheme cwrc:SocialClass .

cwrc:environmentalism
    void:inDataset cwrc:datasetdefinition ;
    a cwrc:PoliticalAffiliation, skos:Concept ;
    rdf:value "ecologist", "environmentalist", "nature conservationist" ;
    rdfs:comment "La description de ce terme est basée sur celle de DBPedia."@fr, "The description for this term is indebted to DBpedia."@en ;
    rdfs:isDefinedBy <http://sparql.cwrc.ca/ontologies/cwrc-2017-08-03> ;
    rdfs:label "environmentalism"@en, "Écologisme"@fr ;
    skos:definition "Environmentalism or environmental rights is a broad philosophy, ideology, and social movement regarding concerns for environmental protection and improvement of the health of the environment, particularly as the measure for this health seeks to incorporate the concerns of non-human elements. Environmentalism advocates the lawful preservation, restoration and/or improvement of the natural environment, and may be referred to as a movement to control pollution or protect plant and animal diversity. For this reason, concepts such as a land ethic, environmental ethics, biodiversity, ecology, and the biophilia hypothesis figure predominantly. At its crux, environmentalism is an attempt to balance relations between humans and the various natural systems on which they depend in such a way that all the components are accorded a proper degree of sustainability. The exact measures and outcomes of this balance is controversial and there are many different ways for environmental concerns to be expressed in practice. Environmentalism and environmental concerns are often represented by the color green, but this association has been appropriated by the marketing industries for the tactic known as greenwashing. Environmentalism is opposed by anti-environmentalism, which says that the Earth is less fragile than some environmentalists maintain, and portrays environmentalism as overreacting to the human contribution to climate change or opposing human advancement. <a href=\"#_dbpedia_2017\">(DBpedia, 2017)</a>"@en, "L'écologisme, ou environnementalisme, est à la fois un courant de pensée (idéologie ou philosophie), un corpus de valeurs et de propositions incluant notamment celles du mouvement écologiste. L'orientation de l'activité politique ou parapolitique vise au respect, à la protection, la préservation ou la restauration de l'environnement dans une forme très poussée. James Lovelock, père de la théorie Gaïa, est l'un des représentants les plus célèbres de cette doctrine. Ce mouvement éco-centrique a comme projet la conservation de la nature et le « respect » des équilibres naturels. L'environnementalisme et le mouvement écologiste ont parmi leurs priorités : la conservation des ressources naturelles, la préservation de la « vie sauvage » (wilderness), la lutte contre la dégradation, la fragmentation et la destruction des habitats et des écosystèmes au sens le plus large. Ils définissent de nouveaux rapports territoriaux dans les milieux habités par l'humain, dont les milieux urbains considérés comme les habitats potentiels de substitution et comme cadre de vie d'une part grandissante de l'humanité. Ces différentes demandes sociales et politiques, ou même protestations s'expriment dès le début du XXe siècle : en 1902, une convention internationale pour la protection des oiseaux utiles était signée entre 11 pays d'Europe, et en 1913, le congrès de Berne réclamait une « Protection mondiale de la nature », principalement du constat de la dégradation de la nature par l'homme, notamment par la chasse et la surexploitation de la nature, puis par la pollution et la destruction à grande échelle de milieux naturels (forêts tropicales) notamment. <a href=\"#_dbpedia_2017\">(DBpedia, 2017)</a>"@fr ;
    skos:inScheme cwrc:PoliticalAffiliation ;
    prov:derivedFrom dbpedia:Environmentalism .

cwrc:eugenics
    void:inDataset cwrc:datasetdefinition ;
    a cwrc:PoliticalAffiliation, skos:Concept ;
    rdf:value "eugenicist" ;
    rdfs:comment "La description de ce terme est basée sur celle de DBPedia."@fr, "The description for this term is indebted to DBpedia."@en ;
    rdfs:isDefinedBy <http://sparql.cwrc.ca/ontologies/cwrc-2017-08-03> ;
    rdfs:label "Eugénisme"@fr, "eugenics"@en ;
    skos:definition "Eugenics (/juːˈdʒɛnɪks/; from Greek εὐγενής eugenes \"well-born\" from εὖ eu, \"good, well\" and γένος genos, \"race, stock, kin\") is a set of beliefs and practices that aims at improving the genetic quality of the human population. It is a social philosophy advocating the improvement of human genetic traits through the promotion of higher rates of sexual reproduction for people with desired traits (positive eugenics), or reduced rates of sexual reproduction and sterilization of people with less-desired or undesired traits (negative eugenics), or both. Alternatively, gene selection rather than \"people selection\" has recently been made possible through advances in genome editing (e.g. CRISPR). The exact definition of eugenics has been a matter of debate since the term was coined. The definition of it as a \"social philosophy\"—that is, a philosophy with implications for social order—is not universally accepted, and was taken from Frederick Osborn's 1937 journal article \"Development of a Eugenic Philosophy\". While eugenic principles have been practiced as far back in world history as Ancient Greece, the modern history of eugenics began in the early 20th century when a popular eugenics movement emerged in the United Kingdom and spread to many countries, including the United States, Canada and most European countries. In this period, eugenic ideas were espoused across the political spectrum. Consequently, many countries adopted eugenic policies meant to improve the genetic stock of their countries. Such programs often included both \"positive\" measures, such as encouraging individuals deemed particularly \"fit\" to reproduce, and \"negative\" measures such as marriage prohibitions and forced sterilization of people deemed unfit for reproduction. People deemed unfit to reproduce often included people with mental or physical disabilities, people who scored in the low ranges of different IQ tests, criminals and deviants, and members of disfavored minority groups. The eugenics movement became negatively associated with Nazi Germany and the Holocaust when many of the defendants at the Nuremberg trials attempted to justify their human rights abuses by claiming there was little difference between the Nazi eugenics programs and the US eugenics programs.In the decades following World War II, with the institution of human rights, many countries gradually abandoned eugenics policies, although some Western countries, among them the United States, continued to carry out forced sterilizations. Since the 1980s and 1990s when new assisted reproductive technology procedures became available, such as gestational surrogacy (available since 1985), preimplantation genetic diagnosis (available since 1989) and cytoplasmic transfer (first performed in 1996), fear about a possible future revival of eugenics and a widening of the gap between the rich and the poor has emerged. A major criticism of eugenics policies is that, regardless of whether \"negative\" or \"positive\" policies are used, they are vulnerable to abuse because the criteria of selection are determined by whichever group is in political power. Furthermore, negative eugenics in particular is considered by many to be a violation of basic human rights, which include the right to reproduction. Another criticism is that eugenic policies eventually lead to a loss of genetic diversity, resulting in inbreeding depression instead due to a low genetic variation. <a href=\"#_dbpedia_2017\">(DBpedia, 2017)</a>"@en, "L’eugénisme peut être défini comme l’ensemble des méthodes et pratiques visant à intervenir sur le patrimoine génétique de l’espèce humaine, dans le but de le faire tendre vers un idéal déterminé, du moins tel que conçu à l'époque en cours. Il peut être le fruit d’une politique délibérément menée par un État. Il peut aussi être le résultat collectif d’une somme de décisions individuelles convergentes prises par les futurs parents, dans une culture qui valoriserait la recherche de l’« enfant parfait ». Le terme eugenics a été employé pour la première fois en 1883 par le scientifique britannique Francis Galton. Les travaux de celui-ci participèrent à la constitution et à la diffusion de la mouvance eugéniste. Mené par des scientifiques et des médecins, le mouvement de promotion de l'eugénisme qui se met en place au tournant du XXe siècle milite en faveur de politiques volontaristes d'éradication des caractères jugés handicapants ou dans le but de favoriser des caractères jugés bénéfiques. Son influence sur la législation s’est traduite principalement dans trois domaines : la mise en place de programmes de stérilisations contraintes là où la culture dominante le permettait, un durcissement de l’encadrement juridique du mariage et des mesures de restriction ou promotion de tel ou tel type d’immigration. Dans la période contemporaine, les progrès du génie génétique et le développement des techniques de procréation médicalement assistée ont ouvert de nouvelles possibilités médicales (diagnostic prénatal, diagnostic préimplantatoire…) qui ont nourri les débats éthiques concernant la convergence des techniques biomédicales et des pratiques sélectives. Singapour a mis en place, ainsi que la Chine, un système qualifié d'eugéniste. <a href=\"#_dbpedia_2017\">(DBpedia, 2017)</a>"@fr ;
    skos:inScheme cwrc:PoliticalAffiliation ;
    prov:derivedFrom dbpedia:Eugenics .

cwrc:eurasianLabel
    void:inDataset cwrc:datasetdefinition ;
    a skos:Concept, skosxl:Label ;
    rdfs:isDefinedBy <http://sparql.cwrc.ca/ontologies/cwrc-2017-08-03> ;
    rdfs:label "eurasian"@en, "eurasian"@fr ;
    skos:definition ""@en, ""@fr ;
    skos:inScheme cwrc:TextLabels ;
    skos:narrower cwrc:eurasianRace .

cwrc:eurasianRace
    void:inDataset cwrc:datasetdefinition ;
    a cwrc:RaceColour, skos:Concept ;
    rdfs:isDefinedBy <http://sparql.cwrc.ca/ontologies/cwrc-2017-08-03> ;
    rdfs:label "eurasian"@en, "eurasien"@fr ;
    rdfs:subClassOf cwrc:eurasianLabel ;
    skos:broader cwrc:eurasianLabel ;
    skos:definition ""@en, ""@fr ;
    prov:derivedFrom <http://dbpedia.org/resource/Eurasian_(mixed_ancestry)> ;
    foaf:name "eurasian (race colour)"@en .

cwrc:existentialism
    void:inDataset cwrc:datasetdefinition ;
    a cwrc:PoliticalAffiliation, skos:Concept ;
    rdf:value "existentialist" ;
    rdfs:comment "La description de ce terme est basée sur celle de DBPedia."@fr, "The description for this term is indebted to DBpedia."@en ;
    rdfs:isDefinedBy <http://sparql.cwrc.ca/ontologies/cwrc-2017-08-03> ;
    rdfs:label "Existentialisme"@fr, "existentialism"@en ;
    skos:definition "Existentialism (/ɛɡzɪˈstɛnʃəlɪzəm/) is a term applied to the work of certain late-19th- and 20th-century European philosophers who, despite profound doctrinal differences, shared the belief that philosophical thinking begins with the human subject—not merely the thinking subject, but the acting, feeling, living human individual. While the predominant value of existentialist thought is commonly acknowledged to be freedom, its primary virtue is authenticity. In the view of the existentialist, the individual's starting point is characterized by what has been called \"the existential attitude\", or a sense of disorientation and confusion in the face of an apparently meaningless or absurd world. Many existentialists have also regarded traditional systematic or academic philosophies, in both style and content, as too abstract and remote from concrete human experience. Søren Kierkegaard is generally considered to have been the first existentialist philosopher, though he did not use the term existentialism. He proposed that each individual—not society or religion—is solely responsible for giving meaning to life and living it passionately and sincerely, or \"authentically\". Existentialism became popular in the years following World War II, and strongly influenced many disciplines besides philosophy, including theology, drama, art, literature, and psychology. <a href=\"#_dbpedia_2017\">(DBpedia, 2017)</a>"@en, "L’existentialisme est un courant philosophique ainsi que littéraire qui postule que l'être humain forme l'essence de sa vie par ses propres actions, celles-ci n'étant pas prédéterminées par des doctrines théologiques, philosophiques ou morales. L'existentialisme considère chaque personne comme un être unique maître de ses actes, de son destin et des valeurs qu'il décide d'adopter. Bien qu'il existe des tendances communes entre les penseurs existentialistes, des différences subsistent : il y a notamment un fossé entre les existentialistes athées comme Jean-Paul Sartre et les philosophes existentiels chrétiens comme Søren Kierkegaard, Paul Tillich ou Gabriel Marcel, sans oublier la philosophie juive de l'existence de Martin Buber et Emmanuel Levinas ou encore musulmane d'Abdennour Bidar. Certains auteurs tels que Albert Camus ou Martin Heidegger ont même refusé d'être étiquetés comme existentialistes. Sartre a livré quant à lui sa propre définition et conception de l'existentialisme et a donné une conférence sur le sujet : L'existentialisme est un humanisme. <a href=\"#_dbpedia_2017\">(DBpedia, 2017)</a>"@fr ;
    skos:inScheme cwrc:PoliticalAffiliation ;
    prov:derivedFrom dbpedia:Existentialism .

cwrc:fascism
    void:inDataset cwrc:datasetdefinition ;
    a cwrc:PoliticalAffiliation, skos:Concept ;
    rdf:value "fascist", "fascist party", "pro-fascist" ;
    rdfs:comment "La description de ce terme est basée sur celle de DBPedia."@fr, "The description for this term is indebted to DBpedia."@en ;
    rdfs:isDefinedBy <http://sparql.cwrc.ca/ontologies/cwrc-2017-08-03> ;
    rdfs:label "Fascisme"@fr, "fascism"@en ;
    skos:definition "Fascism /ˈfæʃɪzəm/ is a form of radical authoritarian nationalism that came to prominence in early 20th-century Europe, influenced by national syndicalism. Fascism originated in Italy during World War I and spread to other European countries. Fascism opposes liberalism, Marxism and anarchism and is usually placed on the far-right within the traditional left–right spectrum. Fascists saw World War I as a revolution that brought massive changes in the nature of war, society, the state, and technology. The advent of total war and total mass mobilization of society had broken down the distinction between civilian and combatant. A \"military citizenship\" arose in which all citizens were involved with the military in some manner during the war. The war had resulted in the rise of a powerful state capable of mobilizing millions of people to serve on the front lines and providing economic production and logistics to support them, as well as having unprecedented authority to intervene in the lives of citizens. Fascists believe that liberal democracy is obsolete, and they regard the complete mobilization of society under a totalitarian one-party state as necessary to prepare a nation for armed conflict and to respond effectively to economic difficulties. Such a state is led by a strong leader—such as a dictator and a martial government composed of the members of the governing fascist party—to forge national unity and maintain a stable and orderly society. Fascism rejects assertions that violence is automatically negative in nature, and views political violence, war, and imperialism as means that can achieve national rejuvenation. Fascists advocate a mixed economy, with the principal goal of achieving autarky through protectionist and interventionist economic policies. Since the end of World War II in 1945, few parties have openly described themselves as fascist, and the term is instead now usually used pejoratively by political opponents. The descriptions neo-fascist or post-fascist are sometimes applied more formally to describe parties of the far right with ideologies similar to, or rooted in, 20th century fascist movements. <a href=\"#_dbpedia_2017\">(DBpedia, 2017)</a>"@en, "Le terme fascisme (prononcé [fa.ʃism], calque de la prononciation italienne [faˈʃizmo] ; ou plus rarement [fa.sism]) s'applique au sens étroit à la période mussolinienne de l'histoire italienne et au sens large à un système politique aux caractéristiques inspirées par l'exemple italien mais qui a pu prendre des aspects différents selon les pays. Des débats existent entre les historiens quant à la qualification de certains régimes (France de Vichy, Espagne franquiste...). Le terme même (en italien fascismo) vient du mot « fascio » (« faisceau ») désignant le rassemblement des fusils au repos ou l'attribut du licteur dans la Rome antique. La différence entre fascisme et totalitarisme fait l'objet de nombreux débats. Le fascisme est un système politique autoritaire qui associe populisme, nationalisme et totalitarisme au nom d'un idéal collectif suprême. À la fois révolutionnaire et conservateur, il s'oppose frontalement à la démocratie parlementaire et à l'État libéral garant des droits individuels. Issu de diverses composantes de la philosophie européenne du XIXe siècle, le fascisme a trouvé dans les circonstances économiques et historiques de l'après-première guerre mondiale le contexte qui lui a permis d'accéder au pouvoir, d'abord en Italie dans les années 1920 avec Mussolini, puis sous une variante accentuée, militariste et terroriste, en Allemagne dans les années 1930 avec le nazisme et Hitler. Niant l'individu et la démocratie au nom de la masse incarnée dans un chef providentiel, le fascisme embrigade les groupes sociaux (jeunesse, milices) et justifie la violence d'État menée contre les opposants assimilés à des ennemis intérieurs, l'unité de la nation devant dépasser et résoudre les antagonismes des classes sociales dans un parti unique. Dans le domaine économique, l'état conduit une politique dirigiste mais maintient la propriété privée et capitaliste.En même temps il rejette la notion d'égalité au nom d'un ordre hiérarchique naturel : il définit un « homme nouveau », un idéal de pureté nationale et raciale qui nourrit en particulier l'antisémitisme, l'homophobie, l'exclusion des personnes atteintes d'un handicap et exalte les corps régénérés ainsi que les vertus de la terre, du sang et de la tradition, tout comme il affirme une hiérarchie entre les peuples forts et les peuples faibles qui doivent être soumis. De façon générale le fascisme exalte la force et s’appuie sur les valeurs traditionnelles de la masculinité, reléguant les femmes dans leur rôle maternel. Il célèbre dans cet esprit les vertus guerrières en développant une esthétique héroïque et grandiose. Révélateur d'une crise de la modernité et luttant contre le sentiment de décadence de la civilisation, le fascisme s'appuie aussi sur la mystique romantique du passé et sur l'émotion collective qu'il met en scène dans la théâtralité dynamique d'une religion civile (culte du chef, uniformes, rassemblements, propagande) et suscite ainsi une fascination idéologique et esthétique avérée. Dans son acception la plus large, le terme est employé pour disqualifier l'ennemi politique (par exemple par les Soviétiques durant la Guerre froide ou certains partis politiques sur l'échiquier politique dans les démocraties libérales), cependant, le fascisme est encore revendiqué par certaines mouvances d'extrême droite (les néofascistes). <a href=\"#_dbpedia_2017\">(DBpedia, 2017)</a>"@fr ;
    skos:inScheme cwrc:PoliticalAffiliation ;
    prov:derivedFrom dbpedia:Fascism .

cwrc:fatherOf
    void:inDataset cwrc:datasetdefinition ;
    a owl:ObjectProperty ;
    rdf:value "FATHER" ;
    rdfs:isDefinedBy <http://sparql.cwrc.ca/ontologies/cwrc-2017-08-03> ;
    rdfs:label "father of"@en, "père de"@fr ;
    rdfs:subPropertyOf cwrc:parentOf .

cwrc:femaleSex
    dcterms:isReplacedBy cwrc:genderWomanFemale ;
    void:inDataset cwrc:datasetdefinition ;
    a owl:Thing, skos:Concept ;
    rdfs:comment "Deprecated in favour of instance #genderWomanFemale."@en, "Désapprouver en faveur de l'instance #genderWomanFemale."@fr ;
    rdfs:isDefinedBy <http://sparql.cwrc.ca/ontologies/cwrc-2017-08-03> ;
    rdfs:label "Female"@en, "Femelle"@fr ;
    owl:deprecated true ;
    vs:term_status "deprecated"@en ;
    skos:definition ""@en, ""@fr ;
    foaf:name "Female (Sex)"@en .

cwrc:feminism
    void:inDataset cwrc:datasetdefinition ;
    a cwrc:PoliticalAffiliation, skos:Concept ;
    rdf:value "activist for women and children", "anti-sexist", "equal rights", "feminist", "gender egalitarian", "health activist", "moderate feminist", "pro-family", "proto-feminist", "salary reform", "women's rights" ;
    rdfs:comment "La description de ce terme est basée sur celle de DBPedia."@fr, "The description for this term is indebted to DBpedia."@en ;
    rdfs:isDefinedBy <http://sparql.cwrc.ca/ontologies/cwrc-2017-08-03> ;
    rdfs:label "Féminisme"@fr, "feminism"@en ;
    skos:definition "Feminism is a range of political movements, ideologies, and social movements that share a common goal: to define, establish, and achieve political, economic, personal, and social rights for women that are equal to those of men. This includes seeking to establish equal opportunities for women in education and employment. Feminist movements have campaigned and continue to campaign for women's rights, including the right to vote, to hold public office, to work, to earn fair wages or equal pay, to own property, to receive education, to enter contracts, to have equal rights within marriage, and to have maternity leave. Feminists have also worked to promote bodily autonomy and integrity, and to protect women and girls from rape, sexual harassment, and domestic violence. Feminist campaigns are generally considered to be one of the main forces behind major historical societal changes for women's rights, particularly in the West, where they are near-universally credited with having achieved women's suffrage, gender neutrality in English, reproductive rights for women (including access to contraceptives and abortion), and the right to enter into contracts and own property. Although feminist advocacy is, and has been, mainly focused on women's rights, some feminists, including bell hooks, argue for the inclusion of men's liberation within its aims because men are also harmed by traditional gender roles.Feminist theory, which emerged from feminist movements, aims to understand the nature of gender inequality by examining women's social roles and lived experience; it has developed theories in a variety of disciplines in order to respond to issues concerning gender. Numerous feminist movements and ideologies have developed over the years and represent different viewpoints and aims. Some forms of feminism have been criticized for taking into account only white, middle class, and educated perspectives. This criticism led to the creation of ethnically specific or multicultural forms of feminism, including black feminism and intersectional feminism. <a href=\"#_dbpedia_2017\">(DBpedia, 2017)</a>"@en, "Le féminisme est un ensemble de mouvements et d'idées politiques, philosophiques et sociales, qui partagent un but commun : définir, établir et atteindre l'égalité politique, économique, culturelle, personnelle, sociale et juridique entre les femmes et les hommes. Le féminisme a donc pour objectif d'abolir, dans ces différents domaines, les inégalités homme-femme dont les femmes sont les principales victimes, et ainsi de promouvoir les droits des femmes dans la société civile et dans la sphère privée. Si le terme « féminisme » ne prend son sens actuel qu'à la fin du XIXe siècle, les idées de libération de la femme prennent leurs racines dans le siècle des Lumières et se réclament de mouvements plus anciens ou de combats menés dans d'autres contextes historiques. L’objectif principal de la première vague féministe est de réformer les institutions, de sorte que les hommes et les femmes deviennent égaux devant la loi : droit à l'éducation, droit au travail, droit à la maîtrise de leurs biens et droit de vote des femmes constituent les revendications principales de cette période. Le mouvement féministe a produit une grande diversité d'analyses sociologiques et philosophiques. La deuxième vague féministe, qui intervient à la fin des années 1960 avec la naissance du Mouvement de libération des femmes (MLF) et du Women's Lib, a ainsi élaboré plusieurs concepts qui entendent rendre compte de la spécificité du rapport de domination exercé sur les femmes. C'est à cette période qu'est reformulé le concept de patriarcat, élaboré celui de sexisme et que l'accent est mis sur la sphère privée comme lieu privilégié de la domination masculine : le « privé est politique ». Les revendications touchant au contrôle de leur corps par les femmes (avortement, contraception) sont placées au premier plan mais, plus largement, c'est à la construction de nouveaux rapports sociaux de sexe qu'appellent les féministes de cette deuxième vague. Dans cette perspective, la notion de « genre » entend « dénaturaliser » les rapports entre les sexes. Sous le nom de troisième vague féministe, on désigne à partir des années 1990, un large ensemble de revendications exprimées par des militantes féministes issues de groupes minoritaires, dans le sillage du Black feminism. <a href=\"#_dbpedia_2017\">(DBpedia, 2017)</a>"@fr ;
    skos:inScheme cwrc:PoliticalAffiliation ;
    prov:derivedFrom dbpedia:Feminism .

cwrc:feministAnti-ViolenceActivism
    void:inDataset cwrc:datasetdefinition ;
    a cwrc:PoliticalAffiliation, skos:Concept ;
    rdf:value "anti-female-genital-mutilation" ;
    rdfs:comment "The description for this term is indebted to DBpedia."@en ;
    rdfs:isDefinedBy <http://sparql.cwrc.ca/ontologies/cwrc-2017-08-03> ;
    rdfs:label ""@fr, "feminist anti-violence activism"@en ;
    skos:broaderTransitive cwrc:feminism ;
    skos:definition ""@fr, "Activism opposing violence from a feminist perspective, often but not exclusively violence against women and children, including sexual and domestic violence and female genital mutilation."@en ;
    skos:inScheme cwrc:PoliticalAffiliation .

cwrc:feministInternationalism
    void:inDataset cwrc:datasetdefinition ;
    a cwrc:PoliticalAffiliation, skos:Concept ;
    rdfs:comment "The description for this term is indebted to DBpedia."@en ;
    rdfs:isDefinedBy <http://sparql.cwrc.ca/ontologies/cwrc-2017-08-03> ;
    rdfs:label ""@fr, "feminist internationalism"@en ;
    skos:broaderTransitive cwrc:feminism, cwrc:internationalism ;
    skos:definition ""@fr, "Feminist participant in the internationalism movement.  See <a href=\"https://en.wikipedia.org/wiki/Internationalism_(politics)\">https://en.wikipedia.org/wiki/Internationalism_(politics)</a>"@en ;
    skos:inScheme cwrc:PoliticalAffiliation ;
    prov:derivedFrom <http://dbpedia.org/resource/Internationalism_(politics)> .

cwrc:feministPacifism
    void:inDataset cwrc:datasetdefinition ;
    a cwrc:PoliticalAffiliation, skos:Concept ;
    rdfs:comment "The description for this term is indebted to DBpedia."@en ;
    rdfs:isDefinedBy <http://sparql.cwrc.ca/ontologies/cwrc-2017-08-03> ;
    rdfs:label ""@fr, "feminist pacifism"@en ;
    skos:broaderTransitive cwrc:feminism, cwrc:pacifism ;
    skos:definition ""@fr, "Feminist participant in the pacifist movement.  See <a href=\"https://en.wikipedia.org/wiki/Internationalism_(politics\">https://en.wikipedia.org/wiki/Internationalism_(politics) Also see: </a><a href=\"https://en.wikipedia.org/wiki/Pacifism\">https://en.wikipedia.org/wiki/Pacifism</a>"@en ;
    skos:inScheme cwrc:PoliticalAffiliation ;
    prov:derivedFrom <http://dbpedia.org/resource/Internationalism_(politics>, dbpedia:Pacifism .

cwrc:fifthMonarchists
    void:inDataset cwrc:datasetdefinition ;
    a cwrc:Religion, skos:Concept, foaf:Organization ;
    rdfs:comment "La description de ce terme est basée sur celle de DBPedia."@fr ;
    rdfs:isDefinedBy <http://sparql.cwrc.ca/ontologies/cwrc-2017-08-03> ;
    rdfs:label "Cinquièmes Monarchistes"@fr, "Fifth Monarchists"@en ;
    skos:broaderTransitive cwrc:dissenters, cwrc:millenarianism ;
    skos:definition "Les hommes de la Cinquième Monarchie, ou Cinquièmes Monarchistes (Fifth Monarchy Men ou Fifth Monarchists en anglais) sont une faction idéologique de la Première Révolution anglaise, active de 1649 à 1661. Ils tiennent leur nom de leur croyance en la fondation prochaine d'un royaume planétaire par Jésus retournant sur terre. <a href=\"#_dbpedia_2017\">(DBpedia, 2017)</a>"@fr, "The Fifth Monarchists or Fifth Monarchy Men were active from 1649 to 1660 during the Interregnum, following the English Civil Wars of the 17th century. They took their name from a prophecy in the Book of Daniel that four ancient monarchies (Babylonian, Persian, Macedonian, and Roman) would precede the kingdom of Christ. They also referred to the year 1666 and its relationship to the biblical Number of the Beast indicating the end of earthly rule by carnal human beings. They were one of a number of nonconformist dissenting groups that emerged around this time. <a href=\"#_dbpedia_2017\">(DBpedia, 2017)</a>"@en ;
    skos:inScheme cwrc:Religion ;
    prov:derivedFrom dbpedia:Fifth_Monarchists .

cwrc:freeTradeMovement
    void:inDataset cwrc:datasetdefinition ;
    a cwrc:PoliticalAffiliation, skos:Concept ;
    rdf:value "free trader" ;
    rdfs:comment "The description for this term is indebted to DBpedia."@en ;
    rdfs:isDefinedBy <http://sparql.cwrc.ca/ontologies/cwrc-2017-08-03> ;
    rdfs:label ""@fr, "free trade movement"@en ;
    skos:definition ""@fr, "Free Trader was a political label used in the United Kingdom by several candidates in the 1906 general election and January 1910 general election. Its candidates were in university constituencies, led by John Eldon Gorst, who had been previously elected as a Conservative Party but had split from the party in 1902. The group was in favour of limited social reforms, and in particular of free trade. While several of its candidates received substantial votes, none were elected, and in 1910 Gorst stood instead as a Liberal Party candidate, the remainder of the grouping soon petering out. <a href=\"#_dbpedia_2017\">(DBpedia, 2017)</a>"@en ;
    skos:inScheme cwrc:PoliticalAffiliation ;
    prov:derivedFrom dbpedia:Free_Trader .

cwrc:frenchNationalism
    void:inDataset cwrc:datasetdefinition ;
    a cwrc:PoliticalAffiliation, skos:Concept ;
    rdfs:comment "La description de ce terme est basée sur celle de DBPedia."@fr, "The description for this term is indebted to DBpedia."@en ;
    rdfs:isDefinedBy <http://sparql.cwrc.ca/ontologies/cwrc-2017-08-03> ;
    rdfs:label "French nationalism"@en, "Nationalisme en France"@fr ;
    skos:definition "French nationalism is the nationalism that asserts that the French are a nation and promotes the cultural unity of the French. <a href=\"#_dbpedia_2017\">(DBpedia, 2017)</a>"@en, "Le nationalisme en France est apparu au cours du XVIIIe siècle dans la bourgeoisie, sous la plume des philosophes des Lumières. Le nationalisme signifiait pour eux, à cette époque, que c'est le peuple qui incarne le pays, par opposition à la vision de l'ancien régime pour lequel le pays est incarné par le Roi de France. Au XIXe siècle, le nationalisme devient une opposition aux autres nations, voire aux autres peuples, cette idée prenant clairement forme à la fin de ce siècle, dans les mouvements politiques entrant en jeu dans le système démocratique français, est née en 1870, avec la Troisième République. À cette époque, tous les partis manifestent ostensiblement de telles idées nationalistes et anti-allemandes : la Prusse venait de gagner une guerre et avait pris l'Alsace-Lorraine. <a href=\"#_dbpedia_2017\">(DBpedia, 2017)</a>"@fr ;
    skos:inScheme cwrc:PoliticalAffiliation ;
    prov:derivedFrom dbpedia:French_nationalism .

cwrc:gayRights
    void:inDataset cwrc:datasetdefinition ;
    a cwrc:PoliticalAffiliation, skos:Concept ;
    rdf:value "gay rights advocate", "pro-sexual preference" ;
    rdfs:comment "La description de ce terme est basée sur celle de DBPedia."@fr, "The description for this term is indebted to DBpedia."@en ;
    rdfs:isDefinedBy <http://sparql.cwrc.ca/ontologies/cwrc-2017-08-03> ;
    rdfs:label "Mouvement LGBT"@fr, "gay rights movement"@en ;
    skos:definition "Le mouvement lesbien, gay, bisexuel et transsexuel (LGBT) désigne l'ensemble des mouvements et actions individuelles ou collectives qui cherchent à faire évoluer la perception sociale des minorités sexuelles, de l'homosexualité, de la bisexualité et de la transsexualité. Un objectif fréquemment avancé par ces mouvements est l'égalité des droits civils et sociaux pour les personnes LGBT et, parfois, la construction de communautés LGBT ou la libération de l'ensemble de la société de la biphobie, de l'homophobie et de la transphobie. Il n'existe pas d'organisation qui regroupe l'ensemble des LGBT et de nombreuses structures existent dans différents pays à travers le monde. Le mouvement se concrétise notamment par des actions militantes, culturelles et artistiques ou des manifestations de rue telle que la Marche des fiertés. <a href=\"#_dbpedia_2017\">(DBpedia, 2017)</a>"@fr, "Lesbian, gay, bisexual, transgender, and queer (LGBTQ) social movements are social movements that advocate for the equalized acceptance of LGBT people in society. In these movements, LGBTQ people and their allies have a long history of campaigning for what is now generally called LGBTQ rights, sometimes also called gay rights or gay and lesbian rights. Although there is not a primary or an overarching central organization that represents all LGBT people and their interests, numerous LGBT rights organizations are active worldwide. The earliest organizations to support LGBT rights were formed in the 19th century. A commonly stated goal among these movements is social equality for LGBT people. Some have also focused on building LGBT communities or worked towards liberation for the broader society from biphobia, homophobia, and transphobia. LGBT movements organized today are made up of a wide range of political activism and cultural activity, including lobbying, street marches, social groups, media, art, and research. <a href=\"#_dbpedia_2017\">(DBpedia, 2017)</a>"@en ;
    skos:inScheme cwrc:PoliticalAffiliation ;
    prov:derivedFrom dbpedia:LGBT_social_movements .

cwrc:genderManMale
    dcterms:isReplacedBy cwrc:man ;
    void:inDataset cwrc:datasetdefinition ;
    a owl:Thing, skos:Concept ;
    rdfs:comment "Deprecated in favour of instance #man."@en, "Désapprouver en faveur de l'instance #man."@fr ;
    rdfs:isDefinedBy <http://sparql.cwrc.ca/ontologies/cwrc-2017-08-03> ;
    rdfs:label "homme/mâle"@fr, "man/male"@en ;
    owl:deprecated true ;
    vs:term_status "deprecated"@en ;
    skos:definition ""@en ;
    foaf:name "man/male (gender)"@en .

cwrc:genderTransMan
    dcterms:isReplacedBy cwrc:transMan ;
    void:inDataset cwrc:datasetdefinition ;
    a skos:Concept ;
    rdfs:comment "Deprecated in favour of instance #transMan."@en, "Désapprouver en faveur de l'instance #transMan."@fr ;
    rdfs:isDefinedBy <http://sparql.cwrc.ca/ontologies/cwrc-2017-08-03> ;
    rdfs:label "Homme Trans"@fr, "Transman/Transmale"@en ;
    owl:deprecated true ;
    vs:term_status "deprecated"@en ;
    skos:definition ""@en ;
    foaf:name "Transman/Transmale (gender)"@en .

cwrc:genderTransWoman
    dcterms:isReplacedBy cwrc:transWoman ;
    void:inDataset cwrc:datasetdefinition ;
    a skos:Concept ;
    rdfs:comment "Deprecated in favour of instance #transWoman."@en, "Désapprouver en faveur de l'instance #transWoman."@fr ;
    rdfs:isDefinedBy <http://sparql.cwrc.ca/ontologies/cwrc-2017-08-03> ;
    rdfs:label "Femme Trans"@fr, "Transwoman/Transfemale"@en ;
    owl:deprecated true ;
    vs:term_status "deprecated"@en ;
    skos:definition ""@en ;
    foaf:name "Transwoman/Transfemale (gender)"@en .

cwrc:genderWomanFemale
    dcterms:isReplacedBy cwrc:woman ;
    void:inDataset cwrc:datasetdefinition ;
    a owl:Thing, skos:Concept ;
    rdfs:comment "Deprecated in favour of instance #woman."@en, "Désapprouver en faveur de l'instance #woman."@fr ;
    rdfs:isDefinedBy <http://sparql.cwrc.ca/ontologies/cwrc-2017-08-03> ;
    rdfs:label "Femme/Femelle"@fr, "Woman/Female"@en ;
    owl:deprecated true ;
    vs:term_status "deprecated"@en ;
    skos:definition ""@en ;
    foaf:name "Woman/Female (gender)"@en .

cwrc:gentry
    void:inDataset cwrc:datasetdefinition ;
    a cwrc:SocialClass, skos:Concept ;
    rdfs:isDefinedBy <http://sparql.cwrc.ca/ontologies/cwrc-2017-08-03> ;
    rdfs:label "gentry"@en, "noblesse non titrée"@fr ;
    owl:sameAs dbpedia:Gentry ;
    skos:definition "Gentry indicates someone who is property-owning or related to the same; property can be land or stocks and bonds. It begins in the idea of owning arms and having a coat of arms. but is distinguished from nobility in so far as money is not necessarily related to blood and title. Disinterested gentlemen are of this class (i.e. Mr. Bennett in Jane Austen). Gentlewomen belong to this class, even thought they may not themselves own much property but instead be supported by a father or brother, or they may be distressed, which is to say, impoverished gentlewomen, as in the case of Jane Eyre or Austen's Jane Fairfax. <a href=\"#_dbpedia_2017\">(DBpedia, 2017)</a>"@en, "La landed gentry est le nom donné à la bonne société anglaise, et en particulier à la noblesse non titrée. Elle est de bonne éducation et « a des valeurs ». Les membres de la gentry sont légalement des gentlemen, esquire, et peuvent recevoir des décorations, titres de noblesses, héréditaires ou viagier (chevaliers, baronnets). Cette classe, composée à la fois de la haute bourgeoisie et de la noblesse titrée ou non, se développe au XVIe siècle, à une époque de mobilité sociale accentuée. À l'origine, ce sont des notables provinciaux, propriétaires, qui s'enrichissent grâce à leurs domaines (qu'ils n'exploitent pas directement). Du point de vue juridique, la gentry n'a pas un statut comparable à celui qu'a eu la noblesse continentale au cours des siècles, et on ne parle donc pas légalement de nobility (sauf en Écosse qui a un système plus proche du système continental). En effet, en Angleterre (au sens strict), seuls les pairs ont légalement le titre de noble et tous les attributs légaux qui vont avec. Ainsi, dans une famille qui descend d'un pair du royaume, seul le chef de famille est légalement « noble », les autres sont gentry. Néanmoins, la gentry a tous les attributs sociaux de la noblesse, et est donc reconnue comme noble au sens complet par la CILANE (« Commission d'information et de liaison des associations nobles d'Europe », voir Association d'entraide de la noblesse française). Le statut juridique de la gentility est donné par la lettre patente donnée par les rois d'armes par délégation du souverain. C'est cette lettre patente qui leur donne à eux seuls le droit de porter des armoiries, de se déclarer « of gentle birth. » Dans la distinction traditionnelle nobilitas maior et nobilitas minor, les pairs représentent le premier groupe, la gentry le second. <a href=\"#_dbpedia_2017\">(DBpedia, 2017)</a>"@fr ;
    skos:inScheme cwrc:SocialClass .

cwrc:germanNationalism
    void:inDataset cwrc:datasetdefinition ;
    a cwrc:PoliticalAffiliation, skos:Concept ;
    rdfs:comment "The description for this term is indebted to DBpedia."@en ;
    rdfs:isDefinedBy <http://sparql.cwrc.ca/ontologies/cwrc-2017-08-03> ;
    rdfs:label ""@fr, "German nationalism"@en ;
    skos:definition ""@fr, "German nationalism is the idea that asserts that Germans are a nation and promotes the cultural unity of Germans. The earliest origins of German nationalism began with the birth of Romantic nationalism during the Napoleonic Wars when Pan-Germanism started to rise. Advocacy of a German nation began to become an important political force in response to the invasion of German territories by France under Napoleon. After the rise and fall of Nazi Germany during World War II, German nationalism has been generally viewed in the country as taboo. However, during the Cold War, German nationalism arose that supported the reunification of East and West Germany that was achieved in 1990. German nationalism has faced difficulties in promoting a united German identity as well as facing opposition within Germany. The Catholic-Protestant divide in Germany at times created extreme tension and hostility between Catholic and Protestant Germans after 1871, such as in response to the policy of Kulturkampf in Prussia by German Chancellor and Prussian Prime Minister Otto von Bismarck, that sought to dismantle Catholic culture in Prussia, that provoked outrage amongst Germany's Catholics and resulted in the rise of the pro-Catholic Centre Party and the Bavarian People's Party. There have been rival nationalists within Germany, particularly Bavarian nationalists who claim that the terms that Bavaria entered into Germany in 1871 were controversial and have claimed the German government has long intruded into the domestic affairs of Bavaria. Outside of modern-day Germany in Austria, there are Austrian nationalists who have rejected unification of Austria with Germany on the basis of preserving Austrians' Catholic religious identity from the potential danger posed by being part of a Protestant-majority Germany. <a href=\"#_dbpedia_2017\">(DBpedia, 2017)</a>"@en ;
    skos:inScheme cwrc:PoliticalAffiliation ;
    prov:derivedFrom dbpedia:German_nationalism .

cwrc:girondin
    void:inDataset cwrc:datasetdefinition ;
    a cwrc:PoliticalAffiliation, skos:Concept ;
    rdfs:comment "La description de ce terme est basée sur celle de DBPedia."@fr, "The description for this term is indebted to DBpedia."@en ;
    rdfs:isDefinedBy <http://sparql.cwrc.ca/ontologies/cwrc-2017-08-03> ;
    rdfs:label "Gironde (Révolution française)"@fr, "Girondin"@en ;
    skos:definition "Certains Girondins, comme Condorcet, Brissot, Roland, Guadet, Vergniaud, Isnard, Ducos et Buzot étaient des républicains convaincus. Ses membres, pour la plupart inscrits au club des Jacobins à Paris ou en province, constituaient l'aile la plus avancée de l'Assemblée législative, avant de représenter l'aile droite de la Convention nationale face aux Montagnards, qui étaient en force parmi les députés de Paris, et incarnés par les figures de Robespierre, Danton ou Marat. Les affrontements violents entre Girondins et Montagnards dominent les premiers mois de la Convention. <a href=\"#_dbpedia_2017\">(DBpedia, 2017)</a>"@fr, "The Girondins or Girondists were members of the Gironba, a political group operating in France from 1791 to 1795 during the French Revolution. The Girondins were active within the Legislative Assembly and the National Convention. They were part of the Jacobin movement, though not every Girondin was a member of the Jacobin Club. The Girondins campaigned for the end of the monarchy but then resisted the spiraling momentum of the Revolution. They came into conflict with The Mountain (Montagnards), a radical faction within the Jacobin Club. This conflict eventually led to the fall of the Girondins and their mass execution, the beginning of the Reign of Terror. The Girondins comprised a group of loosely affiliated individuals rather than an organized political party, and the name was at first informally applied because the most prominent exponents of their point of view were deputies to the Legislative Assembly from the department of Gironde in southwest France. The term became standard with Lamartine's history in 1847. Girondin leader Jacques-Pierre Brissot proposed an ambitious military plan to spread the Revolution—one that Napoleon later achieved. He called on the Convention to dominate Western Europe by conquering the Rhineland, Poland, and Holland, with a goal of creating a protective ring of satellite republics in Britain, Spain and Italy by 1795. The Girondins were thus the war party in 1792–93. Other prominent Girondins included Jean Marie Roland and his wife Madame Roland. They had an ally in the English-born, sometime American, activist Thomas Paine. Brissot and Madame Roland were executed and Jean Roland (who had gone into hiding) committed suicide when he learned what had transpired. Paine was arrested and imprisoned but narrowly escaped execution. The famous painting Death of Marat depicts the killing of the fiery radical journalist (and denouncer of the Girondins) Jean-Paul Marat by the Girondin sympathizer Charlotte Corday, who was executed. <a href=\"#_dbpedia_2017\">(DBpedia, 2017)</a>"@en ;
    skos:inScheme cwrc:PoliticalAffiliation ;
    prov:derivedFrom dbpedia:Girondins .

cwrc:grandFatherOf
    void:inDataset cwrc:datasetdefinition ;
    a owl:ObjectProperty ;
    rdf:value "GRANDFATHER" ;
    rdfs:isDefinedBy <http://sparql.cwrc.ca/ontologies/cwrc-2017-08-03> ;
    rdfs:label "grand father of"@en, "grand-père de"@fr ;
    rdfs:subPropertyOf cwrc:grandParentOf .

cwrc:grandMotherOf
    void:inDataset cwrc:datasetdefinition ;
    a owl:ObjectProperty ;
    rdf:value "GRANDMOTHER" ;
    rdfs:isDefinedBy <http://sparql.cwrc.ca/ontologies/cwrc-2017-08-03> ;
    rdfs:label "grand mother of"@en, "grand-mère de"@fr ;
    rdfs:subPropertyOf cwrc:grandParentOf .

cwrc:grandParentOf
    void:inDataset cwrc:datasetdefinition ;
    a owl:ObjectProperty ;
    rdf:value "GRANDPARENTS" ;
    rdfs:isDefinedBy <http://sparql.cwrc.ca/ontologies/cwrc-2017-08-03> ;
    rdfs:label "grand parent de"@fr, "grand parent of"@en ;
    rdfs:subPropertyOf cwrc:relativeOf .

cwrc:greekNationalist
    void:inDataset cwrc:datasetdefinition ;
    a cwrc:PoliticalAffiliation, skos:Concept ;
    rdfs:comment "The description for this term is indebted to DBpedia."@en ;
    rdfs:isDefinedBy <http://sparql.cwrc.ca/ontologies/cwrc-2017-08-03> ;
    rdfs:label ""@fr, "Greek nationalist"@en ;
    skos:broaderTransitive cwrc:nationalism ;
    skos:definition ""@fr, "Greek nationalism (or Hellenic nationalism) refers to the nationalism of Greeks and Greek culture. As an ideology, Greek nationalism originated and evolved in pre-modern times. It became a major political movement beginning in the 18th century, which culminated in the Greek War of Independence (1821–1829) against the Ottoman Empire. It became a potent movement in Greece shortly prior to, and during World War I under the leadership of nationalist figure Eleutherios Venizelos who pursued the Megali Idea and managed to liberate Greece in the Balkan Wars and after World War I, briefly annexed the region of Izmir before it was retaken by Turkey. Today Greek nationalism remains important in the Greco-Turkish dispute over Cyprus. <a href=\"#_dbpedia_2017\">(DBpedia, 2017)</a>"@en ;
    skos:inScheme cwrc:PoliticalAffiliation ;
    prov:derivedFrom dbpedia:Greek_nationalism .

cwrc:guelphPartyFlorence
    void:inDataset cwrc:datasetdefinition ;
    a cwrc:PoliticalAffiliation, skos:Concept ;
    rdfs:comment "La description de ce terme est basée sur celle de DBPedia."@fr, "The description for this term is indebted to DBpedia."@en ;
    rdfs:isDefinedBy <http://sparql.cwrc.ca/ontologies/cwrc-2017-08-03> ;
    rdfs:label "Guelfes et gibelins"@fr, "Guelph party (Florence)"@en ;
    skos:definition "Les guelfes et les gibelins sont deux factions (parti ou, plus souvent, brigate ou sette) médiévales qui s'opposèrent militairement, politiquement et culturellement dans l'Italie des Duecento et Trecento. À l'origine, elles soutenaient respectivement deux dynasties qui se disputaient le trône du Saint-Empire : la pars Guelfa appuyait les prétentions de la dynastie des « Welfs » et de la papauté, puis de la maison d'Anjou, la pars Gebellina, celles des Hohenstaufen, et au-delà celles du Saint-Empire. Conflit en apparence limité au Saint-Empire, l'opposition entre Guelfes et Gibelins va se transporter dans diverses parties d'Europe, principalement dans les villes de la péninsule italienne. Dans cette bipolarisation, parfois surestimée, les allégeances dynastiques sont parfois secondaires, les adhésions fluctuantes, et il faut attendre le règne de Frédéric II pour que papauté et empire deviennent des symboles forts de ralliement et que se construise une véritable division antithétique. Ce clivage trouve des manifestations dans le domaine civique et religieux et cristallise les tensions entre les villes italiennes, au sein de leurs élites et parfois entre la ville et son contado. L'écho du conflit se manifeste à des époques ultérieures, en revêtant de nouveaux caractères et en stigmatisant des oppositions idéologiques nouvelles. <a href=\"#_dbpedia_2017\">(DBpedia, 2017)</a>"@fr, "The Guelphs and Ghibellines were factions supporting the Pope and the Holy Roman Emperor, respectively, in the Italian city-states of Central and Northern Italy. During the 12th and 13th centuries, rivalry between these two parties formed a particularly important aspect of the internal politics of medieval Italy. The struggle for power between the Papacy and the Holy Roman Empire had arisen with the Investiture Controversy, which began in 1075 and ended with the Concordat of Worms in 1122. The division between the Guelphs and Ghibellines in Italy, however, persisted until the 15th century."@en ;
    skos:inScheme cwrc:PoliticalAffiliation ;
    skos:related cwrc:pro-Catholicism ;
    prov:derivedFrom dbpedia:Guelphs_and_Ghibellines .

cwrc:hanoverian
    void:inDataset cwrc:datasetdefinition ;
    a cwrc:PoliticalAffiliation, skos:Concept ;
    rdf:value "House of Hanover" ;
    rdfs:comment "La description de ce terme est basée sur celle de DBPedia."@fr, "The description for this term is indebted to DBpedia."@en ;
    rdfs:isDefinedBy <http://sparql.cwrc.ca/ontologies/cwrc-2017-08-03> ;
    rdfs:label "Hanoverian"@en, "Maison de Hanovre"@fr ;
    skos:definition "La Maison de Hanovre est une dynastie royale allemande qui a régné sur le duché de Brunswick-Lunebourg (en allemand Braunschweig-Lüneburg), le royaume de Hanovre, le royaume de Grande-Bretagne, puis du Royaume-Uni. Elle succède à la Maison Stuart sur le trône britannique en 1714 et s'y maintient jusqu'à la mort de Victoria en 1901. Elle est parfois appelée Maison de Brunswick-Lüneburg. À la mort de Victoria, le trône du Royaume-Uni est passé dans la maison de Saxe-Cobourg-Gotha en la personne d'Édouard VII du Royaume-Uni, devenue la maison Windsor en 1917. <a href=\"#_dbpedia_2017\">(DBpedia, 2017)</a>"@fr, "The House of Hanover is a German royal dynasty that ruled the Electorate and then the Kingdom of Hanover, and that also provided monarchs of Great Britain and Ireland from 1714 and ruled the United Kingdom until the death of Queen Victoria in 1901. The House of Hanover was formally named the House of Brunswick-Lüneburg, Hanover line, as it was originally a cadet branch of the House of Brunswick-Lüneburg. The senior branch became extinct in 1884, and the House of Hanover is now the only surviving branch of the House of Welf, which is the senior branch of the House of Este. The current head of the House of Hanover is Ernst August, Prince of Hanover. <a href=\"#_dbpedia_2017\">(DBpedia, 2017)</a>"@en ;
    skos:inScheme cwrc:PoliticalAffiliation ;
    prov:derivedFrom dbpedia:House_of_Hanover .

cwrc:hasActor
    void:inDataset cwrc:datasetdefinition ;
    a owl:ObjectProperty, skos:Concept ;
    rdfs:isDefinedBy <http://sparql.cwrc.ca/ontologies/cwrc-2017-08-03> ;
    rdfs:label "has actor"@en ;
    rdfs:range cwrc:Actor, cwrc:Event ;
    skos:definition "An Actor in this event."@en .

cwrc:hasCulturalForm
    void:inDataset cwrc:datasetdefinition ;
    a owl:ObjectProperty ;
    rdfs:isDefinedBy <http://sparql.cwrc.ca/ontologies/cwrc-2017-08-03> ;
    rdfs:label "a une forme culturelle"@fr, "has a cultural form"@en ;
    skos:definition "Associe des concepts et des catégories spécifiques au processus de formation identitaire à travers les processus culturels. Le sujet elle/lui-même peut ou a pu s’approprier de telles associations, ou d’autres personnes les lui ont attribuées. Les concepts et les catégories classés dans culturalForms se chevauchent en théorie et en terme d'étiquettes utilisés."@fr, "This associates specific concepts and categories with the process of identity formation through cultural processes. Such associations may be or have been embraced by the subject her/himself or attributed by others. The concepts and categories classed as culturalForms are understood to overlap with each other conceptually and in terms of the labels used."@en .

cwrc:hasCulturalForms
    dcterms:isReplacedBy cwrc:hasCulturalForm ;
    void:inDataset cwrc:datasetdefinition ;
    a owl:DeprecatedProperty ;
    rdfs:comment "Deprecated in favour of object property #hasCulturalForm."@en, "Désapprouver en faveur de la propriété #hasCulturalForm."@fr ;
    rdfs:isDefinedBy <http://sparql.cwrc.ca/ontologies/cwrc-2017-08-03> ;
    rdfs:label "a une forme culturelle"@fr, "has a cultural form"@en ;
    owl:equivalentProperty cwrc:hasCulturalForm ;
    vs:term_status "deprecated"@en ;
    skos:definition "Cette sous-classe de culturalFormation associe des concepts et des catégories spécifiques au processus de formation identitaire à travers les processus culturels. Le sujet elle/lui-même peut ou a pu s’approprier de telles associations, ou d’autres personnes les lui ont attribuées. Les concepts et les catégories classés dans culturalForms se chevauchent en théorie et en terme d'étiquettes utilisés."@fr, "This sub-class of culturalFormation associates specific concepts and categories with the process of identity formation through cultural processes. Such associations may be or have been embraced by the subject her/himself or attributed by others. The concepts and categories classed as culturalForms are understood to overlap with each other conceptually and in terms of the labels used."@en .

cwrc:hasEthnicity
    void:inDataset cwrc:datasetdefinition ;
    a owl:ObjectProperty ;
    rdfs:isDefinedBy <http://sparql.cwrc.ca/ontologies/cwrc-2017-08-03> ;
    rdfs:label "d'ethnicité"@fr, "has ethnicity"@en ;
    rdfs:range cwrc:Ethnicity ;
    rdfs:subPropertyOf cwrc:personalProperty ;
    skos:definition ""@en, ""@fr .

cwrc:hasEthnicitySelfDefined
    dcterms:isReplacedBy cwrc:hasEthnicitySelfReported ;
    void:inDataset cwrc:datasetdefinition ;
    rdfs:comment "Deprecated in favour of instance #hasEthnicitySelfReported."@en, "Désapprouver en faveur de l'instance #hasEthnicitySelfReported."@fr ;
    rdfs:isDefinedBy <http://sparql.cwrc.ca/ontologies/cwrc-2017-08-03> ;
    rdfs:label "d'ethnicité (autodéclarée)"@fr, "has ethnicity (self defined)"@en ;
    rdfs:range cwrc:Ethnicity ;
    rdfs:subPropertyOf cwrc:personalPropertySelfDefined ;
    owl:deprecated true ;
    vs:term_status "deprecated"@en ;
    skos:definition ""@en, ""@fr .

cwrc:hasEthnicitySelfReported
    void:inDataset cwrc:datasetdefinition ;
    a owl:ObjectProperty ;
    rdfs:isDefinedBy <http://sparql.cwrc.ca/ontologies/cwrc-2017-08-03> ;
    rdfs:label "d'ethnicité (autodéclarée)"@fr, "has ethnicity (self reported)"@en ;
    rdfs:range cwrc:Ethnicity ;
    rdfs:subPropertyOf cwrc:personalPropertySelfReported .

cwrc:hasGender
    void:inDataset cwrc:datasetdefinition ;
    a owl:ObjectProperty ;
    rdfs:isDefinedBy <http://sparql.cwrc.ca/ontologies/cwrc-2017-08-03> ;
    rdfs:label "est de genre"@fr, "has gender"@en ;
    rdfs:range cwrc:Gender ;
    rdfs:subPropertyOf cwrc:personalProperty ;
    skos:definition ""@en, ""@fr .

cwrc:hasGenderSelfDeclared
    dcterms:isReplacedBy cwrc:hasGenderSelfReported ;
    void:inDataset cwrc:datasetdefinition ;
    rdfs:comment "Deprecated in favour of instance #hasGenderSelfReported."@en, "Désapprouver en faveur de l'instance #hasGenderSelfReported."@fr ;
    rdfs:isDefinedBy <http://sparql.cwrc.ca/ontologies/cwrc-2017-08-03> ;
    rdfs:label "est de genre (autodéclaré)"@fr, "has gender (self declared)"@en ;
    rdfs:range cwrc:Gender ;
    rdfs:subPropertyOf cwrc:personalPropertySelfDeclared ;
    owl:deprecated true ;
    vs:term_status "deprecated"@en ;
    skos:definition ""@en, ""@fr .

cwrc:hasGenderSelfReported
    void:inDataset cwrc:datasetdefinition ;
    a owl:ObjectProperty ;
    rdfs:isDefinedBy <http://sparql.cwrc.ca/ontologies/cwrc-2017-08-03> ;
    rdfs:label "est de genre (autodéclaré)"@fr, "has gender (self reported)"@en ;
    rdfs:range cwrc:Gender ;
    rdfs:subPropertyOf cwrc:personalPropertySelfReported .

cwrc:hasGeographicHeritage
    void:inDataset cwrc:datasetdefinition ;
    a owl:ObjectProperty ;
    rdfs:isDefinedBy <http://sparql.cwrc.ca/ontologies/cwrc-2017-08-03> ;
    rdfs:label "A un héritage géographique"@fr, "has Geographic Heritage"@en ;
    rdfs:range cwrc:GeographicHeritage ;
    rdfs:subPropertyOf cwrc:personalProperty ;
    skos:definition ""@en, ""@fr .

cwrc:hasGeographicHeritageSelfDeclared
    dcterms:isReplacedBy cwrc:hasGeographicHeritageSelfReported ;
    void:inDataset cwrc:datasetdefinition ;
    rdfs:comment "Deprecated in favour of instance #hasGeographicHeritageSelfReported."@en, "Désapprouver en faveur de l'instance #hasGeographicHeritageSelfReported."@fr ;
    rdfs:isDefinedBy <http://sparql.cwrc.ca/ontologies/cwrc-2017-08-03> ;
    rdfs:label "a un héritage géographique (autodéclaré)"@fr, "has geographic heritage (self declared)"@en ;
    rdfs:range cwrc:GeographicHeritage ;
    rdfs:subPropertyOf cwrc:personalProperty ;
    owl:deprecated true ;
    vs:term_status "deprecated"@en ;
    skos:definition ""@en, ""@fr .

cwrc:hasGeographicHeritageSelfReported
    void:inDataset cwrc:datasetdefinition ;
    a owl:ObjectProperty ;
    rdfs:isDefinedBy <http://sparql.cwrc.ca/ontologies/cwrc-2017-08-03> ;
    rdfs:label "a un héritage géographique (autodéclaré)"@fr, "has geographic heritage (self reported)"@en ;
    rdfs:range cwrc:GeographicHeritage ;
    rdfs:subPropertyOf cwrc:personalPropertySelfReported .

cwrc:hasLinguisticAbility
    void:inDataset cwrc:datasetdefinition ;
    a owl:ObjectProperty ;
    rdfs:isDefinedBy <http://sparql.cwrc.ca/ontologies/cwrc-2017-08-03> ;
    rdfs:label "connait la langue"@fr, "language known"@en ;
    rdfs:range cwrc:LinguisticAbility ;
    rdfs:subPropertyOf cwrc:personalProperty ;
    skos:definition ""@fr, "Knowlege of the language for writing or reading."@en .

cwrc:hasLinguisticAbilitySelfDeclared
    dcterms:isReplacedBy cwrc:hasLinguisticAbilitySelfReported ;
    void:inDataset cwrc:datasetdefinition ;
    rdfs:comment "Deprecated in favour of instance #hasLinguisticAbilitySelfReported."@en, "Désapprouver en faveur de l'instance #hasLinguisticAbilitySelfReported."@fr ;
    rdfs:isDefinedBy <http://sparql.cwrc.ca/ontologies/cwrc-2017-08-03> ;
    rdfs:label "connait la langue (autodéclaré)"@fr, "language known (self declared)"@en ;
    rdfs:range cwrc:LinguisticAbility ;
    rdfs:subPropertyOf cwrc:personalPropertySelfDeclared ;
    owl:deprecated true ;
    vs:term_status "deprecated"@en ;
    skos:definition ""@en, ""@fr .

cwrc:hasLinguisticAbilitySelfReported
    void:inDataset cwrc:datasetdefinition ;
    a owl:ObjectProperty ;
    rdfs:isDefinedBy <http://sparql.cwrc.ca/ontologies/cwrc-2017-08-03> ;
    rdfs:label "connait la langue (autodéclaré)"@fr, "language known (self reported)"@en ;
    rdfs:range cwrc:LinguisticAbility ;
    rdfs:subPropertyOf cwrc:personalPropertySelfReported .

cwrc:hasNationality
    void:inDataset cwrc:datasetdefinition ;
    a owl:ObjectProperty ;
    rdfs:isDefinedBy <http://sparql.cwrc.ca/ontologies/cwrc-2017-08-03> ;
    rdfs:label "de nationalité"@fr, "has nationality"@en ;
    rdfs:range cwrc:NationalIdentity ;
    rdfs:subPropertyOf cwrc:personalProperty ;
    skos:definition ""@en, ""@fr .

cwrc:hasNationalitySelfDeclared
    dcterms:isReplacedBy cwrc:hasNationalitySelfReported ;
    void:inDataset cwrc:datasetdefinition ;
    rdfs:comment "Deprecated in favour of instance #hasNationalitySelfReported."@en, "Désapprouver en faveur de l'instance #hasNationalitySelfReported."@fr ;
    rdfs:isDefinedBy <http://sparql.cwrc.ca/ontologies/cwrc-2017-08-03> ;
    rdfs:label "de nationalité (autodéclarée)"@fr, "has nationality (self declared)"@en ;
    rdfs:range cwrc:NationalIdentity ;
    rdfs:subPropertyOf cwrc:personalPropertySelfDeclared ;
    owl:deprecated true ;
    vs:term_status "deprecated"@en ;
    skos:definition ""@en, ""@fr .

cwrc:hasNationalitySelfReported
    void:inDataset cwrc:datasetdefinition ;
    a owl:ObjectProperty ;
    rdfs:isDefinedBy <http://sparql.cwrc.ca/ontologies/cwrc-2017-08-03> ;
    rdfs:label "de nationalité (autodéclarée)"@fr, "has nationality (self reported)"@en ;
    rdfs:range cwrc:NationalIdentity ;
    rdfs:subPropertyOf cwrc:personalPropertySelfReported .

cwrc:hasNativeLinguisticAbility
    void:inDataset cwrc:datasetdefinition ;
    a owl:ObjectProperty ;
    rdfs:isDefinedBy <http://sparql.cwrc.ca/ontologies/cwrc-2017-08-03> ;
    rdfs:label "a une langue maternelle"@fr, "natively known language"@en ;
    rdfs:range cwrc:LinguisticAbility ;
    rdfs:subPropertyOf cwrc:hasLinguisticAbility ;
    skos:definition ""@fr, "Knowledge of the language for writing or reading."@en .

cwrc:hasNativeLinguisticAbilitySelfDeclared
    dcterms:isReplacedBy cwrc:hasLinguisticAbilitySelfReported ;
    void:inDataset cwrc:datasetdefinition ;
    rdfs:comment "Deprecated in favour of instance #hasLinguisticAbilitySelfReported."@en, "Désapprouver en faveur de l'instance #hasLinguisticAbilitySelfReported."@fr ;
    rdfs:isDefinedBy <http://sparql.cwrc.ca/ontologies/cwrc-2017-08-03> ;
    rdfs:label "a une langue maternelle (autodéclaré)"@fr, "natively known language (self declared)"@en ;
    rdfs:range cwrc:LinguisticAbility ;
    rdfs:subPropertyOf cwrc:hasLinguisticAbilitySelfDeclared ;
    owl:deprecated true ;
    vs:term_status "deprecated"@en ;
    skos:definition ""@en, ""@fr .

cwrc:hasNativeLinguisticAbilitySelfReported
    void:inDataset cwrc:datasetdefinition ;
    a owl:ObjectProperty ;
    rdfs:isDefinedBy <http://sparql.cwrc.ca/ontologies/cwrc-2017-08-03> ;
    rdfs:label "a une langue maternelle (autodéclaré)"@fr, "natively known language (self reported)"@en ;
    rdfs:range cwrc:LinguisticAbility ;
    rdfs:subPropertyOf cwrc:hasLinguisticAbilitySelfReported .

cwrc:hasRaceColour
    void:inDataset cwrc:datasetdefinition ;
    a owl:ObjectProperty ;
    rdfs:isDefinedBy <http://sparql.cwrc.ca/ontologies/cwrc-2017-08-03> ;
    rdfs:label "est de race"@fr, "has race"@en ;
    rdfs:range cwrc:RaceColour ;
    rdfs:subPropertyOf cwrc:personalProperty ;
    skos:definition ""@fr, "A subclass of raceEthnicityContext, this describes a person's racial identity."@en .

cwrc:hasRaceColourSelfDeclared
    dcterms:isReplacedBy cwrc:hasNationalitySelfReported ;
    void:inDataset cwrc:datasetdefinition ;
    rdfs:comment "Deprecated in favour of instance #hasNationalitySelfReported."@en, "Désapprouver en faveur de l'instance #hasNationalitySelfReported."@fr ;
    rdfs:isDefinedBy <http://sparql.cwrc.ca/ontologies/cwrc-2017-08-03> ;
    rdfs:label "est de race (autodéclarée)"@fr, "has race (self declared)"@en ;
    rdfs:range cwrc:Race ;
    rdfs:subPropertyOf cwrc:personalPropertySelfDeclared ;
    owl:deprecated true ;
    vs:term_status "deprecated"@en ;
    skos:definition "This describes a person's self-reported racial identity."@en .

cwrc:hasRaceColourSelfReported
    void:inDataset cwrc:datasetdefinition ;
    a owl:ObjectProperty ;
    rdfs:isDefinedBy <http://sparql.cwrc.ca/ontologies/cwrc-2017-08-03> ;
    rdfs:label "est de race (autodéclarée)"@fr, "has race (self reported)"@en ;
    rdfs:range cwrc:Race ;
    rdfs:subPropertyOf cwrc:personalPropertySelfReported ;
    skos:definition "This describes a person's self-reported racial identity."@en .

cwrc:hasReligion
    void:inDataset cwrc:datasetdefinition ;
    a owl:ObjectProperty ;
    rdfs:isDefinedBy <http://sparql.cwrc.ca/ontologies/cwrc-2017-08-03> ;
    rdfs:label "est de confession"@fr, "has religious affiliation"@en ;
    rdfs:range cwrc:Religion ;
    rdfs:subPropertyOf cwrc:personalProperty ;
    skos:definition ""@en, ""@fr .

cwrc:hasReligionSelfDefined
    dcterms:isReplacedBy cwrc:hasReligionSelfReported ;
    void:inDataset cwrc:datasetdefinition ;
    rdfs:comment "Deprecated in favour of instance #hasReligionSelfReported."@en, "Désapprouver en faveur de l'instance #hasReligionSelfReported."@fr ;
    rdfs:isDefinedBy <http://sparql.cwrc.ca/ontologies/cwrc-2017-08-03> ;
    rdfs:label "has religious affilication (self defined)"@en, "religion (autodéclarée)"@fr ;
    rdfs:range cwrc:Religion ;
    rdfs:subPropertyOf cwrc:personalPropertySelfDefined ;
    owl:deprecated true ;
    vs:term_status "deprecated"@en ;
    skos:definition ""@en, ""@fr .

cwrc:hasReligionSelfReported
    void:inDataset cwrc:datasetdefinition ;
    a owl:ObjectProperty ;
    rdfs:isDefinedBy <http://sparql.cwrc.ca/ontologies/cwrc-2017-08-03> ;
    rdfs:label "has religious affiliation (self reported)"@en, "religion (autodéclarée)"@fr ;
    rdfs:range cwrc:Religion ;
    rdfs:subPropertyOf cwrc:personalPropertySelfReported .

cwrc:hasSexuality
    void:inDataset cwrc:datasetdefinition ;
    a owl:ObjectProperty ;
    rdfs:isDefinedBy <http://sparql.cwrc.ca/ontologies/cwrc-2017-08-03> ;
    rdfs:label "a une orientation sexuelle"@fr, "has sexual orientation"@en ;
    rdfs:range cwrc:Sexuality ;
    rdfs:subPropertyOf cwrc:personalProperty ;
    skos:definition ""@en, ""@fr .

cwrc:hasSexualitySelfDeclared
    dcterms:isReplacedBy cwrc:hasSexualitySelfReported ;
    void:inDataset cwrc:datasetdefinition ;
    rdfs:comment "Deprecated in favour of instance #hasSexualitySelfReported."@en, "Désapprouver en faveur de l'instance #hasSexualitySelfReported."@fr ;
    rdfs:isDefinedBy <http://sparql.cwrc.ca/ontologies/cwrc-2017-08-03> ;
    rdfs:label "a une orientation sexuelle (autodéclarée)"@fr, "has sexual orientation (self declared)"@en ;
    rdfs:range cwrc:Sexuality ;
    rdfs:subPropertyOf cwrc:personalPropertySelfDeclared ;
    owl:deprecated true ;
    vs:term_status "deprecated"@en ;
    skos:definition ""@en, ""@fr .

cwrc:hasSexualitySelfReported
    void:inDataset cwrc:datasetdefinition ;
    a owl:ObjectProperty ;
    rdfs:isDefinedBy <http://sparql.cwrc.ca/ontologies/cwrc-2017-08-03> ;
    rdfs:label "a une orientation sexuelle (autodéclarée)"@fr, "has sexual orientation (self reported)"@en ;
    rdfs:range cwrc:Sexuality ;
    rdfs:subPropertyOf cwrc:personalPropertySelfReported ;
    skos:definition ""@en, ""@fr .

cwrc:hasSocialClass
    void:inDataset cwrc:datasetdefinition ;
    a owl:ObjectProperty ;
    rdfs:isDefinedBy <http://sparql.cwrc.ca/ontologies/cwrc-2017-08-03> ;
    rdfs:label "de classe sociale"@fr, "has social class"@en ;
    rdfs:range cwrc:SocialClass ;
    rdfs:subPropertyOf cwrc:personalProperty ;
    skos:definition ""@en, ""@fr .

cwrc:hasSocialClassSelfDefined
    dcterms:isReplacedBy cwrc:hasSocialClassSelfReported ;
    void:inDataset cwrc:datasetdefinition ;
    rdfs:comment "Deprecated in favour of instance #hasSocialClassSelfReported."@en, "Désapprouver en faveur de l'instance #hasSocialClassSelfReported."@fr ;
    rdfs:isDefinedBy <http://sparql.cwrc.ca/ontologies/cwrc-2017-08-03> ;
    rdfs:label "de classe sociale (autodéclarés)"@fr, "has social class (self defined)"@en ;
    rdfs:range cwrc:SocialClass ;
    rdfs:subPropertyOf cwrc:personalPropertySelfDefined ;
    owl:deprecated true ;
    vs:term_status "deprecated"@en ;
    skos:definition ""@en, ""@fr .

cwrc:hasSocialClassSelfReported
    void:inDataset cwrc:datasetdefinition ;
    a owl:ObjectProperty ;
    rdfs:isDefinedBy <http://sparql.cwrc.ca/ontologies/cwrc-2017-08-03> ;
    rdfs:label "de classe sociale (autodéclarés)"@fr, "has social class (self reported)"@en ;
    rdfs:range cwrc:SocialClass ;
    rdfs:subPropertyOf cwrc:personalPropertySelfReported .

cwrc:heterosexual
    void:inDataset cwrc:datasetdefinition ;
    a cwrc:Sexuality, skos:Concept ;
    rdfs:isDefinedBy <http://sparql.cwrc.ca/ontologies/cwrc-2017-08-03> ;
    rdfs:label "heterosexual"@en, "hétérosexuelle"@fr ;
    owl:sameAs <http://homosaurus.org/terms/heterosexualIdentity> ;
    skos:definition ""@en, ""@fr ;
    foaf:name "heterosexual (sexual identity)"@en .

cwrc:hinduism
    void:inDataset cwrc:datasetdefinition ;
    a cwrc:Religion, skos:Concept ;
    rdfs:comment "La description de ce terme est basée sur celle de DBPedia."@fr, "The description for this term is indebted to the Getty Art & Architecture Thesaurus."@en ;
    rdfs:isDefinedBy <http://sparql.cwrc.ca/ontologies/cwrc-2017-08-03> ;
    rdfs:label "Hindoeïsme"@nl, "Hindou"@fr, "Hinduism"@en, "Hinduismo"@es, "hindouisme"@fr, "yin du jiao"@zh-latn-pinyin-x-notone, "yin tu chiao"@zh-latn-wadegile, "yìn dù jiào"@zh-latn-pinyin-x-hanyu, "印度教"@zh-hant ;
    skos:definition "General term for the set of intellectual and philosophical tenets and highly diverse beliefs and practices that define the civilization, art, literature, society, and politics of the Indian subcontinent. Hinduism is not a common set of rigid beliefs , but varies significantly between different regions; it includes Shaivism, Vaishnavism, Srauta, and numerous other traditions. Among other practices and philosophies, Hinduism includes a wide spectrum of laws and prescriptions of \"daily morality\" based on karma, dharma, and societal norms. The highest divine powers are seen as complementary to one another and not exclusive. Hinduism does not have a particular founder or central authority. Hindu literature is rich and varied, with no one text considered uniquely authoritative. The Vedas, dating to the Vedic period (ca. 1200-500 BCE), are the earliest extant writings. Religious law books and epics such as the Ramayana and the Mahabharata have been and continue to be highly influential. <a href=\"#_getty_2017\">(Getty, 2017)</a>"@en, "L’hindouisme (hindi : hindu dharm ; devanāgarī : हिन्दू धर्म ; « religion hindoue »), ou Sanatana Dharma (sanskrit IAST : sanātanadharma ; devanāgarī : सनातनधर्म ; « Loi Éternelle »), est l'une des plus vieilles religions du monde encore pratiquées, qui n'a ni fondateur ni Église. Avec près d'un milliard de fidèles dans 84 pays, c'est actuellement la troisième religion la plus pratiquée dans le monde après le christianisme et l'islam. Elle est issue du sous-continent indien qui reste son principal foyer de peuplement. La particularité de l'hindouisme est de n'avoir ni prophètes ni dogmes centraux. Cependant, les hindous contemporains croient en l'autorité du Veda, qui, selon la tradition, fut révélé aux hommes, grâce à la « vision » des Rishi. Le terme persan hindu (du sanskrit Sindhu) désignait au départ, pour les musulmans qui pénétrèrent en Inde, les habitants du bassin de l'Indus. L'hindouisme se présente comme un ensemble de concepts philosophiques issus d'une tradition remontant à la protohistoire indienne, la pratique hindouiste étant sans doute issue d'une tradition orale très ancienne, proche de l'animisme. On retient parfois une tripartition historique qui fait de l'hindouisme la dernière phase du développement des religions en Inde, après le védisme aryen (~1500 à 900 av. J.-C.) et le brahmanisme (~900 à 400 av. J.-C.). Au-delà du syncrétisme théologique, l'hindouisme d'avant les invasions islamiques et le colonialisme européen qui soumirent l'Inde à leur autorité était un vecteur pour toutes les sciences : le droit, la politique, l'architecture, l'astronomie, la philosophie, la médecine, etc., comme d'autres savoirs qui avaient en commun le substrat religieux. <a href=\"#_dbpedia_2017\">(DBpedia, 2017)</a>"@fr, "Se refiere al conjunto de creencias y prácticas altamente diversas que generalmente denotan la civilización y cultura India de los dos mil últimos años. La religión influye fuertemente en el arte, la literatura, la política y al sociedad hinduista. Presenta la creencia y la práctica de ritos mágicos, cultos animales, creencia en demonios, cultos a deidades, incluyendo dioses locales y dioses centrales, misticismo, ascetismo y una apreciación y respeto por otras formas de cultos o creencias religiosas. La verdad de la religión no esta concebida como un término dogmático, sino que la verdad supera toda definición verbal. En vez de un sistema de doctrinas, el énfasis se pone en la manera correcta de vivir (dharma). Hay variaciones significativas entre diversas regiones. La mayoría de las formas de hinduismo enfatizan el concepto del reencarnación o de la transmigración; la liberación (moksha) desde el ciclo del samsara es la última meta espiritual del hindú. Brahma, Vishnu y Shiva son las deidades hindúes principales, juntos forman la tríada, el Trimurti. Existen muchos otros deidades de menor rango. El Hinduismo no tiene un fundador en particular o un iniciado, allí no hay una autoridad central. La literatura hindú es rica y variada, sin un texto considerado únicamente autoritario. El Vedas, fechando en el período de Vedic (ca. 1200-500 a. C), es la escritura más temprana existente. Los libros de ley y las epopeyas religiosas tales como el Ramayana y el Mahabharata han sido y continúan siendo altamente influyentes. <a href=\"#_getty_2017\">(Getty, 2017)</a>"@es, "Verwijst naar de reeks uiterst diverse geloven en gebruiken die in het algemeen verwijzen naar de Indiase beschaving en cultuur van de afgelopen tweeduizend jaar. De religie heeft een sterke invloed op de Indiase kunst, literatuur, maatschappij en politiek. Het hindoeïsme omvat diverse religieuze geloven en gebruiken en in plaats van andere goden, andere godsdiensten en andere religieuze concepten als fout of onverenigbaar te zien, worden de hoogste goddelijke machten gezien als elkaar aanvullend. De religieuze waarheid wordt niet gezien in dogmatische termen aangezien wordt geloofd dat de waarheid alle woordelijke definities overstijgt. In plaats van op een reeks doctrines ligt de nadruk op de juiste manier van leven (dharma). Er zijn aanzienlijke verschillen per regio. In de meeste vormen van het hindoeïsme ligt de nadruk op het concept van reïncarnatie of zielsverhuizing; de bevrijding (moksha) van de cyclus van samsara is het uiteindelijke spirituele doel van hindoes. Brahma, Visjnoe en Shiva zijn de belangrijkste hindoeïstische godheden en vormen gezamenlijk een drie-eenheid, de Trimurti. Verder is er een groot aantal lagere goden. Het hindoeïsme heeft geen specifieke oprichter of ontstaansmoment en er is geen centrale autoriteit. De hindoeïstische literatuur is erg rijk en gevarieerd en geen enkele specifieke tekst wordt als gezaghebbend beschouwd. De Veda's, die afkomstig zijn uit de Vedische periode (ca. 1200-500 v. Chr.), zijn de oudste overgebleven geschriften. Religieuze wetboeken en heldendichten zoals de Ramayana en de Mahabharata zijn altijd erg invloedrijk geweest. <a href=\"#_getty_2017\">(Getty, 2017)</a>"@nl, "代表過去兩千年來印度文明與文化的一套極多樣的信仰與實踐方式。此宗教對印度藝術、文學、社會與政治有極大影響。印度教包含多元的宗教信仰及實踐方式，因此不會認為其他的神明、其他形式的敬拜及宗教觀是錯誤或者互不相容，反而認為最高的神力是彼此互補的。他們相信真理超越所有言語定義，因此不應武斷認定何謂宗教真理。重視生活的正確方式(法)，而非一連串的教條。不同宗教之間差異甚鉅。大部分的印度教形式強調輪迴觀念；從生死疾苦等輪迴中解脫是印度教徒最終的心靈目標。婆羅摩、毗濕奴、濕婆是印度教主要的三個神明(三相神) 。還有很多其他小神。印度教沒有確切的建立者及開始時間，也沒有中央權威。印度教文學豐富且多樣，但沒有哪一部作品被認為是權威。追溯自吠陀時期(西元前500年到西元1200年)的吠陀經是現存最早的經典。宗教法律典籍及史詩如《羅摩耶那史詩》及《摩訶婆羅達》仍舊極具影響力。 <a href=\"#_getty_2017\">(Getty, 2017)</a>"@zh-hant ;
    skos:inScheme cwrc:Religion ;
    prov:derivedFrom dbpedia:Hinduism, <http://vocab.getty.edu/aat/300073727> .

cwrc:homosexual
    void:inDataset cwrc:datasetdefinition ;
    a cwrc:Sexuality, skos:Concept ;
    rdfs:isDefinedBy <http://sparql.cwrc.ca/ontologies/cwrc-2017-08-03> ;
    rdfs:label "homosexual"@en, "homosexuelle"@fr ;
    skos:definition ""@en, ""@fr ;
    foaf:name "homosexual (sexual identity)"@en .

cwrc:housingMovement
    void:inDataset cwrc:datasetdefinition ;
    a cwrc:PoliticalAffiliation, skos:Concept ;
    rdf:value "housing activism", "housing charity" ;
    rdfs:comment "The description for this term is indebted to DBpedia."@en ;
    rdfs:isDefinedBy <http://sparql.cwrc.ca/ontologies/cwrc-2017-08-03> ;
    rdfs:label ""@fr, "housing movement"@en ;
    skos:definition ""@fr, "Advocacy or activism related to housing for the poor or otherwise disadvantaged."@en ;
    skos:inScheme cwrc:PoliticalAffiliation .

cwrc:humanRights
    void:inDataset cwrc:datasetdefinition ;
    a cwrc:PoliticalAffiliation, skos:Concept ;
    rdf:value "human rights activist", "humanitarian" ;
    rdfs:comment "The description for this term is indebted to DBpedia."@en ;
    rdfs:isDefinedBy <http://sparql.cwrc.ca/ontologies/cwrc-2017-08-03> ;
    rdfs:label ""@fr, "human rights"@en ;
    skos:definition ""@fr, "Advocacy or activism in support of human rights. <a href=\"https://en.wikipedia.org/wiki/Human_rights\">https://en.wikipedia.org/wiki/Human_rights</a>"@en ;
    skos:inScheme cwrc:PoliticalAffiliation ;
    prov:derivedFrom dbpedia:Human_rights .

cwrc:humanism
    void:inDataset cwrc:datasetdefinition ;
    a cwrc:PoliticalAffiliation, skos:Concept ;
    rdf:value "humanist" ;
    rdfs:comment "La description de ce terme est basée sur celle de DBPedia."@fr, "The description for this term is indebted to DBpedia."@en ;
    rdfs:isDefinedBy <http://sparql.cwrc.ca/ontologies/cwrc-2017-08-03> ;
    rdfs:label "Humanisme"@fr, "humanism"@en ;
    skos:definition "Humanism is a philosophical and ethical stance that emphasizes the value and agency of human beings, individually and collectively, and generally prefers critical thinking and evidence (rationalism, empiricism) over acceptance of dogma or superstition. The meaning of the term humanism has fluctuated according to the successive intellectual movements which have identified with it. The term was coined by theologian Friedrich Niethammer at the beginning of the 19th century. Generally, however, humanism refers to a perspective that affirms some notion of human freedom and progress. In modern times, humanist movements are typically aligned with secularism, and today humanism typically refers to a non-theistic life stance centred on human agency and looking to science rather than revelation from a supernatural source to understand the world. <a href=\"#_dbpedia_2017\">(DBpedia, 2017)</a>"@en, "L’humanisme est un courant culturel européen, trouvant ses origines en Italie, principalement autour de la Toscane, qui s'est développé à la Renaissance. Renouant avec la civilisation gréco-romaine, les intellectuels de l'époque manifestent un vif appétit de savoir (philologie notamment). Considérant que l’Homme est en possession de capacités intellectuelles potentiellement illimitées, ils considèrent la quête du savoir et la maîtrise des diverses disciplines comme nécessaires au bon usage de ces facultés. Ils prônent la vulgarisation de tous les savoirs, dont religieux ; la parole divine doit être accessible à toute personne, quelles que soient ses origines ou sa langue (traduction de la Bible par Jacques Lefèvre d'Étaples en 1523). Ainsi, cet humanisme vise à diffuser plus clairement le patrimoine culturel. L’individu, correctement instruit, reste libre et pleinement responsable de ses actes dans la croyance de son choix. Les notions de liberté ou libre arbitre, de tolérance, d’indépendance, d’ouverture et de curiosité sont, de ce fait, indissociables de la théorie humaniste classique. Par extension, on désigne par « humaniste » toute pensée qui met au premier plan de ses préoccupations le développement des qualités essentielles de l'être humain. Une vaste catégorie de philosophies portant sur l'éthique affirme la dignité et la valeur de tous les individus, fondée sur la capacité de déterminer le bien et le mal par le recours à des qualités humaines universelles, en particulier la rationalité. L'humanisme implique un engagement à la recherche de la vérité et de la moralité par l'intermédiaire des moyens humains, en particulier les sciences, en solidarité avec l'humanité. En mettant l'accent sur la capacité d'auto-détermination, l'humanisme rejette la validité des justifications transcendantes de l'époque, alors éloignée des questions phénoménologiques du XXe siècle, jugées comme une dépendance à l'égard du surnaturel et de la croyance, tels certains textes présentés comme d'origine divine. Les humanistes développent une morale universelle fondée sur la communauté de la condition humaine. L'humanisme est composante d'une variété de systèmes philosophiques plus spécifiques et de plusieurs écoles de pensée religieuse. Bien avant d’être un concept galvaudé par la politique, l’humanisme est avant tout un terme de l’histoire de la philosophie renvoyant à la Renaissance, et plus particulièrement au mouvement d’Erasme, Michel de Montaigne ou encore Budé, lesquels ont remis à l’honneur à la fois la littérature de l’Antiquité gréco-latine et la réflexion personnelle. <a href=\"#_dbpedia_2017\">(DBpedia, 2017)</a>"@fr ;
    skos:inScheme cwrc:PoliticalAffiliation ;
    prov:derivedFrom dbpedia:Humanism .

cwrc:identity
    void:inDataset cwrc:datasetdefinition ;
    a owl:ObjectProperty, skos:Concept ;
    rdfs:domain cwrc:Actor ;
    rdfs:isDefinedBy <http://sparql.cwrc.ca/ontologies/cwrc-2017-08-03> ;
    rdfs:label "identity"@en ;
    rdfs:range cwrc:Person ;
    skos:definition "The identity of the person who committed the act."@en .

cwrc:imperialism
    void:inDataset cwrc:datasetdefinition ;
    a cwrc:PoliticalAffiliation, skos:Concept ;
    rdf:value "colonialist", "commonwealth supporter", "imperialist" ;
    rdfs:comment "La description de ce terme est basée sur celle de DBPedia."@fr, "The description for this term is indebted to DBpedia."@en ;
    rdfs:isDefinedBy <http://sparql.cwrc.ca/ontologies/cwrc-2017-08-03> ;
    rdfs:label "Impérialisme"@fr, "imperialism"@en ;
    skos:definition "Imperialism means \"to extend a country's power through military and diplomacy\". Its name originated from the Latin word imperium, which means to rule over large territories. Imperialism is \"a policy of extending a country's power and influence through colonization, use of military force, or other means\". It has also allowed for the rapid spread of technologies and ideas. The term imperialism has been applied to Western (and Japanese) political and economic dominance especially in Asia and Africa in the 19th and 20th centuries. Its precise meaning continues to be debated by scholars. Some writers, such as Edward Said, use the term more broadly to describe any system of domination and subordination organised with an imperial center and a periphery. Imperialism is defined as \"A policy of extending a country’s power and influence through diplomacy or military force.\" Imperialism is particularly focused on the control that one group, often a state power, has on another group of people. This is often through various forms of \"othering\" (see other) based on racial, religious, or cultural stereotypes. There are \"formal\" or \"informal\" imperialisms. \"Formal imperialism\" is defined as \"physical control or full-fledged colonial rule\". \"Informal imperialism\" is less direct; however, it is still a powerful form of dominance. The definition of imperialism has not been finalized for centuries and was confusedly seen to represent the policies of major powers, or simply, general-purpose aggressiveness. Further on, some writers used the term imperialism, in slightly more discriminating fashion, to mean all kinds of domination or control by a group of people over another. To clear out this confusion about the definition of imperialism one could speak of \"formal\" and \"informal\" imperialism, the first meaning physical control or \"full-fledged colonial rule\" while the second implied less direct rule though still containing perceivable kinds of dominance. Informal rule is generally less costly than taking over territories formally. This is because, with informal rule, the control is spread more subtly through technological superiority, enforcing land officials into large debts that cannot be repaid, ownership of private industries thus expanding the controlled area, or having countries agree to uneven trade agreements forcefully. It is mostly accepted that modern-day colonialism is an expression of imperialism and cannot exist without the latter. The extent to which \"informal\" imperialism with no formal colonies is properly described remains a controversial topic among historians. Both colonization and imperialism have been described by Tom Nairn and Paul James as early forms of globalization: Even if a particular empire does not have a \"global reach\" as we would define it today, empires by their nature still tend to contribute to processes of globalization because of the way that imperial power tends to generate counter-power at its edge-lands and send out reverberations far beyond the territories of their immediate control. The word imperialism became common in Great Britain during the 1870s and was used with a negative connotation. In Great Britain, the word had until then mostly been used to refer to the politics of Napoleon III in obtaining favorable public opinion in France through foreign military interventions. <a href=\"#_dbpedia_2017\">(DBpedia, 2017)</a>"@en, "L'impérialisme est une stratégie ou une doctrine politique de conquête, visant la formation d'un empire ou d'une domination. Pour John Atkinson Hobson, la nouveauté dans l'impérialisme de la fin du XIXe siècle et du début du XXe siècle, c'est qu'il n'est plus lié à l'idée d'un empire couvrant le monde connu, comme c'était le cas dans le cadre de la Pax Romana. Au contraire, à la suite de la montée du nationalisme au XIXe siècle, cet impérialisme donne lieu à une lutte entre empires concurrents (Empire allemand, Empire britannique, Empire russe, etc.). Au niveau économique, l'impérialisme est alors de nature protectionniste et s'oppose au libre-échange. Par ailleurs, ses liens avec certaines formes de capitalisme monopolistique sont mis en avant par de nombreux auteurs marxistes. De nos jours, ce terme est employé de façon large pour désigner tout rapport de domination établi par une nation ou pays sur un ou plusieurs autres pays. <a href=\"#_dbpedia_2017\">(DBpedia, 2017)</a>"@fr ;
    skos:inScheme cwrc:PoliticalAffiliation ;
    prov:derivedFrom dbpedia:Imperialism .

cwrc:inRole
    void:inDataset cwrc:datasetdefinition ;
    a owl:ObjectProperty, skos:Concept ;
    rdfs:domain cwrc:Actor ;
    rdfs:isDefinedBy <http://sparql.cwrc.ca/ontologies/cwrc-2017-08-03> ;
    rdfs:label "in role"@en ;
    rdfs:range cwrc:Role ;
    skos:definition "The role taken on by this actor."@en .

cwrc:indianIndependence
    void:inDataset cwrc:datasetdefinition ;
    a cwrc:PoliticalAffiliation, skos:Concept ;
    rdf:value "indian nationalist", "pro-independence (indian)" ;
    rdfs:comment "La description de ce terme est basée sur celle de DBPedia."@fr, "The description for this term is indebted to DBpedia."@en ;
    rdfs:isDefinedBy <http://sparql.cwrc.ca/ontologies/cwrc-2017-08-03> ;
    rdfs:label "Indian independence movement"@en, "Mouvement pour l'indépendance de l'Inde"@fr ;
    skos:broaderTransitive cwrc:humanRights ;
    skos:definition "45xCe modèle est-il pertinent ? Cliquez pour en voir d'autres.Cet article ne cite pas suffisamment ses sources (mai 2015). Si vous disposez d'ouvrages ou d'articles de référence ou si vous connaissez des sites web de qualité traitant du thème abordé ici, merci de compléter l'article en donnant les références utiles à sa vérifiabilité et en les liant à la section « Notes et références » (modifier l'article, comment ajouter mes sources ?). Le mouvement pour l'indépendance de l'Inde recouvre un ensemble complexe englobant diverses campagnes nationales et régionales, des troubles et des tentatives inspirés d'une philosophie à la fois non-violente et militante, et a impliqué une gamme étendue d'organismes, de philosophies et de mouvements politiques indiens ayant eu pour but commun de mettre fin à l'autorité coloniale britannique aussi bien que celle d'autres administrations coloniales dans le sous-continent indien. <a href=\"#_dbpedia_2017\">(DBpedia, 2017)</a>"@fr, "The Indian Independence Movement encompassed activities and ideas aiming to end the East India Company rule (1757–1858) and the British Raj (1858–1947) in the Indian subcontinent. The Movement spanned a total of 190 years (1757-1947). The very first organised militant movements were in Bengal, but they later took movement in the then newly formed Indian National Congress with prominent moderate leaders seeking only their basic right to appear for Indian Civil Service examinations, as well as more rights, economic in nature, for the people of the soil. The early part of the 20th century saw a more radical approach towards political self-rule proposed by leaders such as the Lal, Bal, Pal and Aurobindo Ghosh, V. O. Chidambaram Pillai. The last stages of the self-rule struggle from the 1920s onwards saw Congress adopt Mohandas Karamchand Gandhi's policy of nonviolence and civil resistance, Muhammad Ali Jinnah's constitutional struggle for the rights of minorities in India, and several other campaigns. Activists Netaji Subhas Chandra Bose and Bhagat Singh preached armed revolution to achieve self-rule. Poets and writers such as Rabindranath Tagore, Subramaniya Bharathi, Allama Iqbal, Josh Malihabadi, Mohammad Ali Jouhar, Bankim Chandra Chattopadhyay and Kazi Nazrul Islam used literature, poetry and speech as a tool for political awareness. Feminists such as Sarojini Naidu and Begum Rokeya promoted the emancipation of Indian women and their participation in national politics. Babasaheb Ambedkar championed the cause of the disadvantaged sections of Indian society within the larger self-rule movement. The period of the Second World War saw the peak of the campaigns by the Quit India movement led by Mahatma Gandhi and the Indian National Army movement led by Netaji Subhas Chandra Bose. The Indian self-rule movement was a mass-based movement that encompassed various sections of society. It also underwent a process of constant ideological evolution. Although the basic ideology of the movement was anti-colonial, it was supported by a vision of independent capitalist economic development coupled with a secular, democratic, republican, and civil-libertarian political structure. After the 1930s, the movement took on a strong socialist orientation, due to the increasing influence of left-wing elements in the Congress as well as the rise and growth of the Communist Party of India. The All-India Muslim League was formed in 1906 as a separate Muslim party which later in 1940 called for separate state of Pakistan. The work of these various movements led ultimately to the Indian Independence Act 1947, which ended the suzerainty in India and the creation of Pakistan. India remained a Dominion of the Crown until 26 January 1950, when the Constitution of India came into force, establishing the Republic of India; Pakistan was a dominion until 1956, when it adopted its first republican constitution. In 1971, East Pakistan declared independence as the People's Republic of Bangladesh. <a href=\"#_dbpedia_2017\">(DBpedia, 2017)</a>"@en ;
    skos:inScheme cwrc:PoliticalAffiliation ;
    prov:derivedFrom dbpedia:Indian_independence_movement .

cwrc:indigenousRights
    void:inDataset cwrc:datasetdefinition ;
    a cwrc:PoliticalAffiliation, skos:Concept ;
    rdfs:comment "The description for this term is indebted to DBpedia."@en ;
    rdfs:isDefinedBy <http://sparql.cwrc.ca/ontologies/cwrc-2017-08-03> ;
    rdfs:label ""@fr, "Indigenous rights movement"@en ;
    skos:definition ""@fr, "Advocacy or activism in support of human rights. <a href=\"https://en.wikipedia.org/wiki/Indigenous_rights\">https://en.wikipedia.org/wiki/Indigenous_rights</a>"@en ;
    skos:inScheme cwrc:PoliticalAffiliation ;
    prov:derivedFrom dbpedia:Indigenous_rights .

cwrc:indigent
    void:inDataset cwrc:datasetdefinition ;
    a cwrc:SocialClass, skos:Concept ;
    rdfs:isDefinedBy <http://sparql.cwrc.ca/ontologies/cwrc-2017-08-03> ;
    rdfs:label "indigent"@en, "indigents"@fr ;
    skos:definition ""@fr, "This social group is poor, destitute, unemployed, supported by charity, or on social security."@en ;
    skos:inScheme cwrc:SocialClass .

cwrc:individualism
    void:inDataset cwrc:datasetdefinition ;
    a cwrc:PoliticalAffiliation, skos:Concept ;
    rdf:value "individualist" ;
    rdfs:comment "La description de ce terme est basée sur celle de DBPedia."@fr, "The description for this term is indebted to DBpedia."@en ;
    rdfs:isDefinedBy <http://sparql.cwrc.ca/ontologies/cwrc-2017-08-03> ;
    rdfs:label "Individualisme"@fr, "individualism"@en ;
    skos:definition "Individualism is the moral stance, political philosophy, ideology, or social outlook that emphasizes the moral worth of the individual. Individualists promote the exercise of one's goals and desires and so value independence and self-reliance and advocate that interests of the individual should achieve precedence over the state or a social group, while opposing external interference upon one's own interests by society or institutions such as the government. Individualism is often defined in contrast to totalitarianism, collectivism and more corporate social forms. Individualism makes the individual its focus and so starts \"with the fundamental premise that the human individual is of primary importance in the struggle for liberation.\" Classical Liberalism, existentialism, and anarchism are examples of movements that take the human individual as a central unit of analysis. Individualism thus involves \"the right of the individual to freedom and self-realization\". It has also been used as a term denoting \"The quality of being an individual; individuality\" related to possessing \"An individual characteristic; a quirk.\" Individualism is thus also associated with artistic and bohemian interests and lifestyles where there is a tendency towards self-creation and experimentation as opposed to tradition or popular mass opinions and behaviors as so also with humanist philosophical positions and ethics. <a href=\"#_dbpedia_2017\">(DBpedia, 2017)</a>"@en, "L'individualisme est une conception philosophique, politique, sociale et morale qui tend à privilégier les droits, les intérêts et la valeur de l'individu par rapport à ceux du groupe. Il prône l'autonomie individuelle face aux diverses institutions sociales et politiques (la famille, le clan, la corporation, la caste...) qui exercent sur lui de multiples pressions. Il ne faut pas confondre individualisme et égoïsme. Contrairement à la compréhension populaire, ce n'est que péjorativement que l'individualisme peut se rapprocher de l'égoïsme et se définir comme une tendance à ne vivre que pour soi. L'individualisme est apparu vers la fin du Moyen Âge et s'est développé à partir de la Renaissance sous l'effet de multiples facteurs, tels que l'invention de l'imprimerie au XVe siècle, qui a favorisé l'activité individuelle de la lecture. <a href=\"#_dbpedia_2017\">(DBpedia, 2017)</a>"@fr ;
    skos:inScheme cwrc:PoliticalAffiliation ;
    prov:derivedFrom dbpedia:Individualism .

cwrc:internationalism
    void:inDataset cwrc:datasetdefinition ;
    a cwrc:PoliticalAffiliation, skos:Concept ;
    rdf:value "internationalist" ;
    rdfs:comment "La description de ce terme est basée sur celle de DBPedia."@fr, "The description for this term is indebted to DBpedia."@en ;
    rdfs:isDefinedBy <http://sparql.cwrc.ca/ontologies/cwrc-2017-08-03> ;
    rdfs:label "Internationalisme institutionnel"@fr, "internationalism"@en ;
    skos:definition "Internationalism is a political principle which advocates a greater political or economic cooperation among nations and peoples, and whose ideological roots can be traced to both socialism and liberalism. Supporters of this principle are referred to as internationalists, and generally believe that the people of the world should unite across national, political, cultural, racial, or class boundaries to advance their common interests, or that the governments of the world should cooperate because their mutual long-term interests are of greater importance than their short-term disputes. Internationalism is, in general, opposed to nationalism, jingoism or chauvinism, and war, and proponents can include supporters of any of the four socialist Internationals and organizations such as the United Nations or the World Federalist Movement. <a href=\"#_dbpedia_2017\">(DBpedia, 2017)</a>"@en, "L’internationalisme institutionnel est un concept de la théorie des relations internationales, désignant un supranationalisme qui prône le développement de la coopération institutionnelle entre États-nations. <a href=\"#_dbpedia_2017\">(DBpedia, 2017)</a>"@fr ;
    skos:inScheme cwrc:PoliticalAffiliation ;
    prov:derivedFrom <http://dbpedia.org/resource/Internationalism_(politics)> .

cwrc:irishHomeRuleMovement
    void:inDataset cwrc:datasetdefinition ;
    a cwrc:PoliticalAffiliation, skos:Concept ;
    rdf:value "home ruler", "home ruler (ireland)", "irish home ruler" ;
    rdfs:comment "The description for this term is indebted to DBpedia."@en ;
    rdfs:isDefinedBy <http://sparql.cwrc.ca/ontologies/cwrc-2017-08-03> ;
    rdfs:label ""@fr, "Irish Home Rule Movement"@en ;
    skos:definition ""@fr, "The Irish Home Rule movement was a movement that agitated for self-government for Ireland within the United Kingdom of Great Britain and Ireland. It was the dominant political movement of Irish nationalism from 1870 to the end of World War I. Isaac Butt founded the Home Government Association in 1870. This was succeeded in 1873 by the Home Rule League, and in 1882 by the Irish Parliamentary Party. These organisations campaigned for home rule in the British House of Commons. Under the leadership of Charles Stewart Parnell, the movement came close to success when the Liberal government under William Ewart Gladstone introduced the First Home Rule Bill in 1886, but the bill was defeated in the House of Commons after a split in the Liberal Party. After Parnell's death, Gladstone introduced the Second Home Rule Bill in 1893; it passed the Commons but was defeated in the House of Lords. After the removal of the Lords' veto in 1911, the Third Home Rule Bill was introduced in 1912, leading to the Home Rule Crisis. On the outbreak of World War I it was enacted, but suspended until the conclusion of the war. Following the Easter Rising of 1916, public support shifted from the Home Rule movement to the more radical Sinn Féin party. In the 1918 General Election the Irish Parliamentary Party suffered a crushing defeat, only a handful of MP's surviving. This was effectively the death of the Home Rule movement. The elected Sinn Féin MPs had no interest in home rule, instead setting up their own legislature, Dáil Éireann, and declaring the independence of Ireland as a republic. Britain passed a Fourth Home Rule Bill, the Government of Ireland Act 1920, aimed at creating separate parliaments for Northern Ireland and Southern Ireland. The former was established in 1921, and the state continues to this day, but the latter never functioned. Following the Treaty that ended the Anglo-Irish War, the 26 southern counties of Ireland gained independence as the Irish Free State. <a href=\"#_dbpedia_2017\">(DBpedia, 2017)</a>"@en ;
    skos:inScheme cwrc:PoliticalAffiliation ;
    prov:derivedFrom dbpedia:Irish_Home_Rule_movement .

cwrc:irishNationalism
    void:inDataset cwrc:datasetdefinition ;
    a cwrc:PoliticalAffiliation, skos:Concept ;
    rdf:value "cultural nationalist", "irish nationalist", "irish patriotism", "parnellite" ;
    rdfs:comment "La description de ce terme est basée sur celle de DBPedia."@fr, "The description for this term is indebted to DBpedia."@en ;
    rdfs:isDefinedBy <http://sparql.cwrc.ca/ontologies/cwrc-2017-08-03> ;
    rdfs:label "Irish nationalism"@en, "Nationalisme irlandais"@fr ;
    skos:definition "Irish nationalism asserts that the Irish people are a nation. Since the partition of Ireland, the term generally refers to support for a united Ireland. Irish nationalists assert that rule from London has been to the detriment of Irish interests. <a href=\"#_dbpedia_2017\">(DBpedia, 2017)</a>"@en, "Le nationalisme irlandais est né avec l'occupation précoce de l'île par les Anglais. Le nationalisme culturel irlandais vise à rétablir la culture gaélique des Irlandais en combattant, notamment, l'impérialisme culturel anglais. Il s'oppose historiquement aux privilèges accordés à l'aristocratie protestante, qui imposait le serment du test et interdisait aux catholiques de siéger au parlement. <a href=\"#_dbpedia_2017\">(DBpedia, 2017)</a>"@fr ;
    skos:inScheme cwrc:PoliticalAffiliation ;
    skos:related cwrc:irishRepublicanism ;
    prov:derivedFrom dbpedia:Irish_nationalism .

cwrc:irishRepublicanism
    void:inDataset cwrc:datasetdefinition ;
    a cwrc:PoliticalAffiliation, skos:Concept ;
    rdf:value "anti-unionist", "irish independence", "irish republic", "irish republican", "irish republicanism", "irish resistance" ;
    rdfs:comment "La description de ce terme est basée sur celle de DBPedia."@fr, "The description for this term is indebted to DBpedia."@en ;
    rdfs:isDefinedBy <http://sparql.cwrc.ca/ontologies/cwrc-2017-08-03> ;
    rdfs:label "Irish republicanism"@en, "Républicanisme irlandais"@fr ;
    skos:definition "Irish republicanism (Irish: poblachtánachas Éireannach) is an ideology based on the belief that all of Ireland should be an independent republic. The development of nationalist and democratic sentiment throughout Europe in the eighteenth and nineteenth centuries was reflected in Ireland in the emergence of republicanism, in opposition to British rule. This followed hundreds of years of British conquest and Irish resistance through rebellion. Discrimination against Catholics and Non-conformists, attempts by the British administration to suppress Irish culture, and the belief that Ireland was economically disadvantaged as a result of the Act of Union were among the specific factors leading to such opposition. The Society of United Irishmen, formed in the 1780s and led primarily by liberal Protestants, evolved into a revolutionary republican organisation, inspired by the American Revolution and allied with Revolutionary France. It launched the 1798 Rebellion with the help of French troops. The rebellion had some success, especially in County Wexford, before it was suppressed. A second rising in 1803, led by Robert Emmet, was quickly put down, and Emmet was hanged. The Young Ireland movement, formed in the 1830s, was initially a part of the Repeal Association of Daniel O'Connell, but broke with O'Connell on the issue of the legitimacy of the use of violence. Primarily a political and cultural organisation, some members of Young Ireland staged an abortive rising, the Young Irelander Rebellion of 1848. Its leaders were transported to Van Diemen's Land. Some of these escaped to the United States, where they linked up with other Irish exiles to form the Fenian Brotherhood. Together with the Irish Republican Brotherhood, founded in Ireland by James Stephens and others in 1858, they made up a movement commonly known as \"Fenians\" which was dedicated to the overthrow of British imperial rule in Ireland. They staged another rising, the Fenian Rising, in 1867, and a dynamite campaign in England in the 1880s. In the early 20th century IRB members, in particular Tom Clarke and Seán MacDermott, began planning another rising. The Easter Rising took place from 24 to 30 April 1916, when members of the Irish Volunteers and Irish Citizen Army seized the centre of Dublin, proclaimed a republic and held off British forces for almost a week. The execution of the Rising's leaders, including Clarke, MacDermott, Patrick Pearse and James Connolly, led to a surge of support for republicanism in Ireland. In 1917 the Sinn Féin party stated as its aim the \"securing the international recognition of Ireland as an independent Irish Republic\", and in the general election of 1918 Sinn Féin took 73 of the 105 Irish seats in the British House of Commons. The elected members did not take their seats but instead set up the First Dáil. Between 1919 and 1921 the Irish Republican Army (IRA), who were loyal to the Dáil, fought the British Army and Royal Irish Constabulary (RIC) in the Irish War of Independence. Talks between the British and Irish in late 1921 led to a treaty by which the British conceded, not a 32-county Irish Republic, but a 26-county Irish Free State with Dominion status. This led to the Irish Civil War, in which the republicans were defeated by their former comrades. The Free State became an independent constitutional monarchy following the Balfour Declaration of 1926 and the Statute of Westminster 1931 and formally became a republic with the passage of the Republic of Ireland Act 1948. That same year, the republican movement took the decision to focus on Northern Ireland thereafter. The Border Campaign, which lasted from 1956 to 1962, involved bombings and attacks on Royal Ulster Constabulary barracks. The failure of this campaign led the republican leadership to concentrate on political action, and to move to the left. Following the outbreak of The Troubles in 1968-9, the movement split between Officials (leftists) and Provisionals (traditionalists) at the beginning of 1970. Both sides were initially involved in an armed campaign against the British state, but the Officials gradually moved into mainstream politics after the Official IRA ceasefire of 1972; the associated \"Official Sinn Féin\" eventually renamed itself the Workers' Party. The Provisional IRA, except during brief ceasefires in 1972 and 1975, kept up a campaign of violence for nearly thirty years, directed against security forces and civilian targets (especially businesses). While the Social Democratic and Labour Party (SDLP) represented the nationalists of Northern Ireland in initiatives such as the 1973 Sunningdale Agreement, republicans took no part in these, believing that a withdrawal of British troops and a commitment to a united Ireland was a necessary precondition of any settlement. This began to change with a landmark speech by Danny Morrison in 1981, advocating what became known as the Armalite and ballot box strategy. Under the leadership of Gerry Adams, Sinn Féin began to focus on the search for a political settlement. When the party voted in 1986 to take seats in legislative bodies within Ireland, there was a walk-out of die-hard republicans, who set up Republican Sinn Féin and the Continuity IRA. Following the Hume–Adams dialogue, Sinn Féin took part in the Northern Ireland peace process which led to the IRA ceasefires of 1994 and 1997 and the Good Friday Agreement of 1998. After elections to the Northern Ireland Assembly, republicans sat in government in Northern Ireland for the first time when Martin McGuinness and Bairbre de Brún were elected to the Northern Ireland Executive. However, another split occurred, with anti-Agreement republicans setting up the 32 County Sovereignty Movement and the Real IRA. Today, Irish republicanism is divided between those who support the institutions set up under the Good Friday Agreement and the later St Andrews Agreement, and those who oppose them. The latter are often referred to as \"dissident\" republicans. <a href=\"#_dbpedia_2017\">(DBpedia, 2017)</a>"@en, "Le républicanisme irlandais est une idéologie politique opposée à la présence britannique en Irlande et prônant l'unification de l'île en une République égalitariste. Le fondateur du républicanisme irlandais est le protestant Theobald Wolfe Tone et son mouvement, les United Irishmen. À la fin du XVIIIe siècle, cette idée est portée à la fois par la bourgeoisie libérale protestante d'Irlande et par la paysannerie catholique. Après l'échec de la rébellion irlandaise de 1798, la bourgeoisie protestante devint réactionnaire et se rangea du côté anglais. Révolutionnaires et égalitaristes, inspirés par les révolutions française et américaine, les républicains irlandais se veulent aussi confessionnels, mythifiant l'ancienne union entre catholiques et protestants, sentiment symbolisé par le drapeau irlandais, union du vert des Irlandais et de l'orange des Orangistes. L'action armée tient une place importante dans la tradition républicaine irlandaise, son histoire s'émaillant de soulèvements et de groupes armés clandestins. <a href=\"#_dbpedia_2017\">(DBpedia, 2017)</a>"@fr ;
    skos:inScheme cwrc:PoliticalAffiliation ;
    skos:related cwrc:irishNationalism ;
    prov:derivedFrom dbpedia:Irish_republicanism .

cwrc:irishUnionism
    void:inDataset cwrc:datasetdefinition ;
    a cwrc:PoliticalAffiliation, skos:Concept ;
    rdf:value "anti-home rule", "anti-home ruler", "anti-irish", "anti-irish nationalist", "unionist" ;
    rdfs:comment "La description de ce terme est basée sur celle de DBPedia."@fr, "The description for this term is indebted to DBpedia."@en ;
    rdfs:isDefinedBy <http://sparql.cwrc.ca/ontologies/cwrc-2017-08-03> ;
    rdfs:label "Irish unionism"@en, "Unionisme en Irlande"@fr ;
    skos:definition " Pour les articles homonymes, voir unionisme. L'unionisme en Irlande est une idéologie politique prônant le maintien d'une forme d'union politique entre la province d'Irlande du Nord et le Royaume-Uni. <a href=\"#_dbpedia_2017\">(DBpedia, 2017)</a>"@fr, "Unionism in Ireland is a political ideology that favours the continuation of some form of political union between the islands of Ireland and Great Britain. Since the partition of Ireland, unionism in Ireland has focused on maintaining and preserving the place of Northern Ireland within the United Kingdom. In this context, a distinction may be made between the unionism in the province of Ulster and unionism elsewhere in Ireland. Today in Northern Ireland, Unionist ideology is expressed in a number of different ways: through preferences for particular newspapers or sports team, participation in unionist culture and by voting for political candidates who espouse unionism. Irish nationalism is opposed to the ideology of unionism. Most unionists come from Protestant backgrounds; most nationalists come from a Roman Catholic background. Exceptions to these generalisations exist; there are Protestant nationalists and there are Catholic unionists. <a href=\"#_dbpedia_2017\">(DBpedia, 2017)</a>"@en ;
    skos:inScheme cwrc:PoliticalAffiliation ;
    skos:related cwrc:irishNationalism, cwrc:irishRepublicanism ;
    prov:derivedFrom dbpedia:Unionism_in_Ireland .

cwrc:islam
    void:inDataset cwrc:datasetdefinition ;
    a cwrc:Religion, skos:Concept ;
    rdfs:comment "La description de ce terme est basée sur celle de DBPedia."@fr, "The description for this term is indebted to the Getty Art & Architecture Thesaurus."@en ;
    rdfs:isDefinedBy <http://sparql.cwrc.ca/ontologies/cwrc-2017-08-03> ;
    rdfs:label "Islam"@es, "Islam"@nl, "Islamism"@en, "Islamismo"@es, "Mahométisme"@fr, "Religion Mahométane"@fr, "i ssu lan chiao"@zh-latn-wadegile, "islam"@fr, "yi si lan jiao"@zh-latn-pinyin-x-notone, "yī sī lán jiāo"@zh-latn-pinyin-x-hanyu, "伊斯蘭教"@zh-hant, "回教"@zh-hant ;
    skos:broaderTransitive cwrc:abrahamicReligions ;
    skos:definition "L'islam (arabe : الإسلام) est une religion abrahamique s'appuyant sur le dogme du monothéisme absolu (l'adoration du Dieu unique sans lui attribuer aucun associé) et prenant sa source dans le Coran, considéré comme le recueil de la parole de Dieu (arabe : الله, Allah) révélée à Mahomet, proclamé par les adhérents de l'islam comme étant le dernier prophète de Dieu, au VIIe siècle en Arabie. Un adepte de l'islam est appelé un musulman. L'islam revendique pour fondement et enseignement principal le tawhid (monothéisme, unicité et indivisibilité), c'est-à-dire le monothéisme le plus épuré où le culte est voué exclusivement à Dieu, sans lui attribuer aucun fils. Les musulmans croient que Dieu est un et incomparable et que le but de l'existence est d'adorer Dieu. Les musulmans croient également que l'islam est la version complète et universelle d'une foi primordiale qui a été révélée à plusieurs reprises par le passé à travers les prophètes, incluant Adam, Noé, Abraham, Moïse et Jésus. Ainsi, elle se présente comme un retour sur les pas d'Abraham (appelé, en arabe, Ibrahim par les musulmans) du point de vue de la croyance, le Coran le définissant comme étant l'étalon-pied, la lieue de la Kaaba, le mille d'Abraham (milla ta Ibrahim), c'est-à-dire une soumission exclusive à la volonté d'Allah. Le Coran reconnaît l'origine divine de l'ensemble des livres sacrés du judaïsme et du christianisme, tout en estimant qu'ils seraient, dans leurs interprétations actuelles, le résultat d'une falsification partielle : le Suhuf-i-Ibrahim (les Feuillets d'Abraham), la Tawrat (le Pentateuque ou la Torah), le Zabur de David et Salomon (identifié au Livre des Psaumes) et l'Injil (l'Évangile). Outre le Coran, la majorité des musulmans se réfèrent à des transmissions de paroles, actes et approbations de Mahomet, récits appelés hadîths, pour l'établissement de règles juridiques (fiqh) permettant la compréhension et l'accomplissement des adorations du musulman au quotidien. Les différentes branches de l'islam ne s'accordent pas sur les compilations de hadiths à retenir comme authentiques. Le Coran et les hadiths dits « recevables » sont deux des quatre sources de la loi islamique, la charia, les deux autres étant l'unanimité (ijma’) et l'analogie (qiyas). En 2010, le nombre de musulmans dans le monde est estimé à 1,6 milliard, soit 23,4 % de la population mondiale, ce qui fait de l'islam la deuxième religion du monde après le christianisme et devant l'hindouisme. C’est, chronologiquement parlant, le troisième grand courant monothéiste de la famille des religions abrahamiques, après le judaïsme et le christianisme avec lesquels il possède un certain nombre d'éléments communs. L’islam se répartit en différents courants, dont les principaux sont le sunnisme, qui représente entre 80 et 85 % des musulmans, et le chiisme, rencontré principalement en Irak et en Iran. <a href=\"#_dbpedia_2017\">(DBpedia, 2017)</a>"@fr, "Refers to the religious beliefs and social practices founded in the seventh century by the Arabian Prophet Muhammad, held to be the last of a series of major prophets, which include, according to Islamic dogma, Adam, Noah, and Jesus. It later spread throughout the Middle East, Africa, Europe, and parts of Asia. It is characterized by the belief in the fundamental idea that a devotee 'surrenders' and submits his will to Allah, the prime creator and sustainer of the universe and all creation. In Islam, God is unique and has no partner or intermediary as in the Christian Trinity. Social service and the active alleviation of suffering in others is considered the only path to salvation and prayer and sacred ritual alone are inadequate forms of submission to Allah. The Qur'an (Koran), the sacred text of the religion, is a compilation of revelations from Allah believed to have been received by Muhammad. <a href=\"#_getty_2017\">(Getty, 2017)</a>"@en, "Se refiere a creencias religiosas y prácticas sociales fundadas en el siglo VII por el Profeta árabe Mahoma, supuestamente el último de una serie de grandes profetas, incluídos, de acuerdo al dogma Islámico, Adán, Noé y Jesús. Posteriormente se difundió a través del Medio Oriente, África, Europa y parte de Asia. Se caracteriza por la creencia en la idea fundamental que un devoto se \"rinde\" y somete la voluntad de Alá, el principal creador y mantenedor del universo y toda creación. En el Islam, Dios es único y no tiene parentesco o intermediario como la trinidad cristiana. El servicio social y las actividades que alivian el sufrimiento de otros es considerado el único camino a la salvación y la oración y ritual sagrado a solas es una inadecuado forma de sumisión para Alá. El Coran (Koran), consagrado el texto de las religiones, es una compilación relevante de las creencias de Alá que fueron recibidas de Mahoma. <a href=\"#_getty_2017\">(Getty, 2017)</a>"@es, "Verwijst naar het samenstel van religieuze overtuigingen en sociale gebruiken dat in de 7de eeuw is ontstaan op basis van de leer van de Arabische profeet Mohammed, die wordt beschouwd als de laatste in een reeks van grote profeten; volgens de islamitische leer zijn dit onder anderen Adam, Noach en Jezus. De islam heeft zich later verspreid in het Midden-Oosten, Afrika, Europa en delen van Azië. De islam wordt gekenmerkt door het geloof in het fundamentele idee dat een gelovige zich 'overgeeft' en zich onderwerpt aan Allah, de schepper van het universum en de schepping als geheel. God is uniek en heeft geen partner of tussenpersoon zoals bij de christelijke drie-eenheid. Maatschappelijke dienstbaarheid en het actief verlichten van het lijden van anderen wordt beschouwd als de enige weg naar verlossing en gebeden en heilige rituelen zijn op zichzelf onvoldoende vormen van overgave aan Allah. De Qur'an (Koran), het heilige geschrift van de religie, is een verzameling onthullingen die, zo gelooft men, door Allah aan Mohammed zijn geopenbaard. <a href=\"#_getty_2017\">(Getty, 2017)</a>"@nl, "由阿拉伯先知穆罕默德於七世紀創建的宗教信仰與社會實踐方式。根據伊斯蘭教條，穆罕默德是繼亞當、挪亞、耶穌後最後一個主要的先知。此教之後廣傳中東、非洲、歐洲、及部份亞洲。基本思想為信徒交出自己的意志給阿拉(宇宙及所有創造物的最高造物者與支撐者)。就伊斯蘭教而言，神是獨一無二的，且并非如基督教三位一體的觀點般有夥伴或是媒介。社會服務及積極幫助受苦者被認為是通往救贖的唯一路徑，若只有祈禱及神聖儀式則不算完全奉獻予阿拉。可蘭經是此教的聖典，記載穆罕默德從阿拉得來的神示。 <a href=\"#_getty_2017\">(Getty, 2017)</a>"@zh-hant ;
    skos:inScheme cwrc:Religion ;
    prov:derivedFrom dbpedia:Islam, <http://vocab.getty.edu/aat/300073715> .

cwrc:italianNationalism
    void:inDataset cwrc:datasetdefinition ;
    a cwrc:PoliticalAffiliation, skos:Concept ;
    rdf:value "italian nationalist", "italian risorgimento", "mazzinian" ;
    rdfs:comment "The description for this term is indebted to DBpedia."@en ;
    rdfs:isDefinedBy <http://sparql.cwrc.ca/ontologies/cwrc-2017-08-03> ;
    rdfs:label ""@fr, "Italian nationalism"@en ;
    skos:broaderTransitive cwrc:nationalism ;
    skos:definition ""@fr, "Support for the unification of Italy as a single nation or of Italian nationalism. See <a href=\"https://en.wikipedia.org/wiki/Italian_nationalism\">https://en.wikipedia.org/wiki/Italian_nationalism</a><a href=\"https://en.wikipedia.org/wiki/Italian_unification\">https://en.wikipedia.org/wiki/Italian_unification</a>"@en ;
    skos:inScheme cwrc:PoliticalAffiliation ;
    prov:derivedFrom dbpedia:Italian_nationalism, dbpedia:Italian_unification .

cwrc:jacobism
    void:inDataset cwrc:datasetdefinition ;
    a cwrc:PoliticalAffiliation, skos:Concept ;
    rdfs:comment "La description de ce terme est basée sur celle de DBPedia."@fr, "The description for this term is indebted to DBpedia."@en ;
    rdfs:isDefinedBy <http://sparql.cwrc.ca/ontologies/cwrc-2017-08-03> ;
    rdfs:label "Club des Jacobins"@fr, "Jacobism"@en ;
    skos:definition "La Société des amis de la Constitution, plus connue ensuite sous le nom de club des Jacobins, est le plus célèbre des clubs de la Révolution française. « C’est ici que s’est préparée la Révolution, dit Georges Couthon en 1793, c’est ici qu’elle s’est faite, c’est ici que se sont préparés tous les grands événements ». Appelé d'abord Club breton, le club tient son nom du couvent des Jacobins de la rue Saint-Honoré (Collège des Jacobins) où il s’est installé en 1789, dans une salle louée par le couvent de l'Annonciation, fondé entre 1611 et 1613 par Sébastien Michaëlis comme extension du Couvent des Jacobins de la rue Saint-Jacques (Jacobus en latin). Le Club des Jacobins est une société de pensée qui a constitué, pendant la Révolution française, à la fois un groupe de pression et un réseau d’une remarquable efficacité. L’action du club, essentielle dès le début de 1790, devient dominante entre 1792 et 1794. À cette époque, l’adjectif « jacobin » signifie partisan de la politique du Comité de salut public. À la fin de 1793, environ 6 000 sociétés de même type sont en correspondance avec lui dans toute la France. La chute de Robespierre marque la fin du grand rôle politique exercé par le club et entraîne sa dissolution en novembre 1794. Depuis cette époque, le nom et l’adjectif s’appliquent à un homme, une femme ou un courant politique hostile à toute idée d’affaiblissement et de démembrement de l’État. <a href=\"#_dbpedia_2017\">(DBpedia, 2017)</a>"@fr, "The Society of the Friends of the Constitution, after 1792 renamed Society of the Jacobins, Friends of Freedom and Equality (French: Société des Jacobins, amis de la liberté et de l'égalité), commonly known as the Jacobin Club (Club des Jacobins) or just collectively Jacobins, was the most famous and influential political club in the development of the French Revolution. Initially founded by anti-Royalist deputies from Brittany, the Club grew into a nationwide republican movement, with a membership estimated at a half million or more. The Jacobin Club was heterogeneous and included both prominent parliamentary factions of the early 1790s, the radical Mountain and the more moderate Girondists. In 1792–3, the Girondists (led by Brissot and including Thomas Paine) dominated the Jacobin Club and led the country. Believing that revolutionary France would not be accepted by its neighbours, they called for an aggressive foreign policy and forced war on Austria. The Girondists were the dominant faction when the Jacobins overthrew the monarchy and created the republic. When the Republic failed to deliver the unrealistic gains that had been expected, they lost popularity. The Girondists sought to curb fanatical revolutionary violence, and were therefore accused by the Mountain of being royalist sympathisers. The National Guard eventually switched its support from the Girondists to the Mountain, allowing the Mountain to stage a coup d'etat. In May 1793, led by Maximilien de Robespierre, the leaders of the Mountain faction succeeded in sidelining the Girondist faction and controlled the government until July 1794. Their time in government was characterized by radically progressive legislation imposed with very high levels of political violence. In June 1793, they approved the Constitution of Year 1 which introduced universal male suffrage for the first time in history. In September 1793, twenty-one prominent Girondists were guillotined, beginning the Reign of Terror. In October, during the Terror, the new constitution was ratified in a referendum which most eligible voters avoided participating in. The Mountain executed tens of thousands of opponents nationwide, ostensibly to suppress the Vendée insurrection and the Federalist insurrections, and to prevent any other insurrections, during the War of the First Coalition. In 1794, the fall of Robespierre pushed the Mountain out of power. The Jacobin Club was closed and many of its remaining leaders, notably Robespierre, were themselves executed. Today, Jacobin and Jacobinism are used in a variety of senses. In Britain, where the term \"Jacobin\" has been linked primarily to the Mountain, it is sometimes used as a pejorative for radical, left-wing revolutionary politics, especially when it exhibits dogmatism and violent repression. In France, \"Jacobin\" now generally indicates a supporter of a centralized republican state and strong central government powers and/or supporters of extensive government intervention to transform society. It is also used in other related senses, indicating proponents of a state education system which strongly promotes and inculcates civic values, and proponents of a strong nation-state capable of resisting any undesirable foreign interference. <a href=\"#_dbpedia_2017\">(DBpedia, 2017)</a>"@en ;
    skos:inScheme cwrc:PoliticalAffiliation ;
    prov:derivedFrom dbpedia:Jacobin .

cwrc:jacobitism
    void:inDataset cwrc:datasetdefinition ;
    a cwrc:PoliticalAffiliation, skos:Concept ;
    rdf:value "jacobite" ;
    rdfs:comment "La description de ce terme est basée sur celle de DBPedia."@fr, "The description for this term is indebted to DBpedia."@en ;
    rdfs:isDefinedBy <http://sparql.cwrc.ca/ontologies/cwrc-2017-08-03> ;
    rdfs:label "Jacobitism"@en, "Jacobitisme"@fr ;
    skos:definition "Jacobitism (/ˈdʒækəbaɪˌtɪzm/ JAK-ə-beye-TIZ-əm;Irish: Seacaibíteachas, Séamusachas, Scottish Gaelic: Seumasachas) was a political movement in Great Britain and Ireland that aimed to restore the Roman Catholic Stuart King James VII of Scotland, II of England and Ireland, and his heirs to the thrones of England, Scotland and Ireland. The movement took its name from Jacobus, the Renaissance Latin form of Iacomus, the original Latin form of James. Adherents rebelled against the British government on several occasions between 1688 and 1746. After James II was deposed in 1688 and replaced by his daughter Mary II, ruling jointly with her husband and first cousin (James's nephew) William III, the Stuarts lived in exile, occasionally attempting to regain the throne. The strongholds of Jacobitism were parts of the Scottish Highlands and the lowland north-east of Scotland, Ireland, and parts of Northern England (mostly within the counties of Northumberland and Lancashire). Significant support also existed in Wales and South-West England. The Jacobites believed that parliamentary interference with the line of succession to the English and Scottish thrones was illegal. Catholics also hoped the Stuarts would end recusancy. In Scotland, the Jacobite cause became intertwined with the last throes of the warrior clan system. The emblem of the Jacobites is the White Cockade. White Rose Day is celebrated on 10 June, the anniversary of the birth of the Old Pretender in 1688. <a href=\"#_dbpedia_2017\">(DBpedia, 2017)</a>"@en, "Le « jacobitisme » historique est un mouvement politique proche des Tories entre 1688 et 1807, composé de ceux qui soutenaient la dynastie détrônée des Stuarts et considéraient comme usurpateurs tous les rois et les reines britanniques ayant régné pendant cette période. Soutenu par les monarchies catholiques françaises et espagnoles, il était surtout implanté en Irlande et dans les Highlands d'Écosse qui furent le théâtre de plusieurs révoltes soutenues par la France. Plus marginalement, le jacobitisme disposait également d'un certain nombre de partisans dans le nord de l'Angleterre et au Pays de Galles. En 1688, le roi Jacques II d'Angleterre et d'Irlande et VII d'Écosse (1633-1701) fut détrôné par un coup d’État, appelé par les historiens Glorieuse Révolution, mené par une armée hollandaise de 25 000 hommes, dont plus de 7 000 huguenots français. Le roi est chassé et une bonne partie de ses pouvoirs transmis au parlement, où les lois seront élaborées par le parti whig. Les royalistes britanniques qui lui étaient restés fidèles, de même qu'à ses successeurs, sont connus sous le nom de jacobites car le prénom du roi, en latin, est « Jacobus ». Les historiens évaluent à 40 000 le nombre de réfugiés jacobites en France, qui ont émigré après la Glorieuse Révolution, dont environ 60 % étaient irlandais, 34 % anglais et 6 % écossais. Parmi eux, 40 % étaient de familles aristocratiques, dont un grand nombre d'officiers de l'armée du roi. En France, ils ont constitué la Cour jacobite de Saint-Germain en Laye et la puissante communauté des Irlandais de Nantes. Apparu plus tard, le jacobitisme dit « moderne » est un mouvement très marginal composé de ceux qui considèrent qu'étaient illégitimes tous les rois et les reines ayant régné sur les pays de l'Empire britannique et du Commonwealth après 1688, en particulier parce que ces souverains ont abdiqué une grande part de leur pouvoir en faveur du parlement. Les jacobites modernes considèrent que la reine Elisabeth II (née en 1926, reine depuis 1952) n'est que « la princesse Philippe de Schleswig-Holstein-Sonderbourg-Glücksbourg ». <a href=\"#_dbpedia_2017\">(DBpedia, 2017)</a>"@fr ;
    skos:inScheme cwrc:PoliticalAffiliation ;
    prov:derivedFrom dbpedia:Jacobitism .

cwrc:jewishEmancipation
    void:inDataset cwrc:datasetdefinition ;
    a cwrc:PoliticalAffiliation, skos:Concept ;
    rdfs:comment "La description de ce terme est basée sur celle de DBPedia."@fr, "The description for this term is indebted to DBpedia."@en ;
    rdfs:isDefinedBy <http://sparql.cwrc.ca/ontologies/cwrc-2017-08-03> ;
    rdfs:label "Jewish emancipation"@en, "Émancipation des Juifs"@fr ;
    skos:definition "Jewish emancipation was the external (and internal) process in various nations in Europe of eliminating Jewish disabilities, e.g. Jewish quotas, to which Jewish people were then subject, and the recognition of Jews as entitled to equality and citizenship rights on a communal, not merely individual, basis. It included efforts within the community to integrate into their societies as citizens. It occurred gradually between the late 18th century and the early 20th century. Jewish emancipation followed the Age of Enlightenment and the concurrent Jewish enlightenment. Various nations repealed or superseded previous discriminatory laws applied specifically against Jews where they resided. Before the emancipation, most Jews were isolated in residential areas from the rest of the society; emancipation was a major goal of European Jews of that time, who worked within their communities to achieve integration in the majority societies and broader education. Many became active politically and culturally within wider European civil society as Jews gained full citizenship. They emigrated to countries offering better social and economic opportunities, such as the Russian Empire and France. Some European Jews turned to Socialism, others to Jewish nationalism: Zionism. <a href=\"#_dbpedia_2017\">(DBpedia, 2017)</a>"@en, "L'émancipation des Juifs désigne le processus de libération des Juifs en Europe et dans le monde, qui leur a permis d'obtenir la citoyenneté et la pleine égalité de leurs droits avec leurs concitoyens. Si la France a été la première à attribuer la pleine égalité de droits aux Juifs par le vote de l'Assemblée constituante en 1791 au début de la Révolution française, il faut rappeler que le processus d'émancipation a débuté juridiquement avec l'Édit de tolérance de Joseph II d'Autriche (1781) qui accorde la liberté de culte aux Protestants comme aux Juifs, l'Édit de tolérance de Louis XVI (1787) et en Allemagne avec la conjonction de la philosophie des Lumières et de la Haskalah (dont le plus illustre représentant est Moïse Mendelssohn). L'émancipation se traduit par une série d'actes législatifs par laquelle les états ont reconnu la citoyenneté aux Juifs. En France, la Terreur a empêché un temps chrétiens et juifs de pratiquer leur religion, mais l'égalité de droits a été confirmée sous Napoléon Ier. Dans le reste de l'Europe, l'émancipation qui s'est faite au XIXe siècle, a conduit à la disparition au moins formelle des ghettos et à l'égalité des chances pour les Juifs, en Europe occidentale et en Amérique. Là où elle s'est heurtée à une plus grande opposition, dans l'Empire russe particulièrement, les Juifs se sont plus volontiers tournés vers les mouvements révolutionnaires ou le sionisme. <a href=\"#_dbpedia_2017\">(DBpedia, 2017)</a>"@fr ;
    skos:inScheme cwrc:PoliticalAffiliation ;
    prov:derivedFrom dbpedia:Jewish_emancipation .

cwrc:jewishEthnicity
    void:inDataset cwrc:datasetdefinition ;
    a cwrc:Ethnicity, owl:Thing ;
    rdfs:isDefinedBy <http://sparql.cwrc.ca/ontologies/cwrc-2017-08-03> ;
    rdfs:label "Jewish"@en, "Juif"@fr ;
    skos:broader cwrc:jewishLabel ;
    skos:definition ""@en, ""@fr ;
    foaf:name "Jewish (Ethnicity)"@en .

cwrc:jewishGeographicalHeritage
    void:inDataset cwrc:datasetdefinition ;
    a cwrc:GeographicalHeritage, owl:Thing ;
    rdfs:isDefinedBy <http://sparql.cwrc.ca/ontologies/cwrc-2017-08-03> ;
    rdfs:label "Jewish"@en, "Juif"@fr ;
    skos:broader cwrc:jewishLabel ;
    skos:definition ""@en, ""@fr ;
    foaf:name "Jewish (Geographical Heritage)"@en .

cwrc:jewishLabel
    void:inDataset cwrc:datasetdefinition ;
    a skos:Concept, skosxl:Label ;
    rdfs:isDefinedBy <http://sparql.cwrc.ca/ontologies/cwrc-2017-08-03> ;
    rdfs:label "Jewish"@en, "Juif"@fr ;
    owl:oneOf (cwrc:judaism
        cwrc:jewishEthnicity
        cwrc:jewishGeographicalHeritage
        cwrc:jewishNationalIdentity
    ) ;
    skos:definition ""@en, ""@fr ;
    skos:inScheme cwrc:TextLabels ;
    foaf:name "Jewish"@en .

cwrc:jewishNationalIdentity
    void:inDataset cwrc:datasetdefinition ;
    a cwrc:NationalIdentity, owl:Thing, skos:Concept ;
    rdfs:isDefinedBy <http://sparql.cwrc.ca/ontologies/cwrc-2017-08-03> ;
    rdfs:label "Jewish"@en, "Juif"@fr ;
    skos:broader cwrc:jewishlabel ;
    skos:definition ""@en, ""@fr .

cwrc:jewishReligion
    dcterms:isReplacedBy cwrc:judaism ;
    void:inDataset cwrc:datasetdefinition ;
    a skos:Concept ;
    rdfs:comment "Deprecated in favour of instance #judaism."@en, "Désapprouver en faveur de l'instance #judaism."@fr, "La description de ce terme est basée sur celle de DBPedia."@fr, "The description for this term is indebted to the Getty Art & Architecture Thesaurus."@en ;
    rdfs:isDefinedBy <http://sparql.cwrc.ca/ontologies/cwrc-2017-08-03> ;
    rdfs:label "Jewish"@en, "Jodendom"@nl, "Joods"@nl, "Judaísmo"@es, "Judaïsme"@fr, "you tai jiao"@zh-latn-pinyin-x-notone, "yu t'ai chiao"@zh-latn-wadegile, "yóu tài jiāo"@zh-latn-pinyin-x-hanyu, "猶太教"@zh-hant ;
    owl:deprecated true ;
    vs:term_status "deprecated"@en ;
    skos:broader cwrc:jewishLabel ;
    skos:broaderTransitive cwrc:abrahamicReligions ;
    skos:definition "Pour l'Encyclopædia Britannica, le mot judaïsme recouvre la religion des Juifs, ainsi que la théologie, la loi et les traditions culturelles du peuple juif, constitué des descendants des Israélites provenant de l'antique terre d'Israël et des quelques minorités les ayant rejoints par la conversion et s'étant mélangées à eux au fil de leur diaspora de deux millénaires. Pour un juif orthodoxe comme Daniel Boyarin, le judaïsme est « l'ensemble des rituels et des autres pratiques, des croyances et des valeurs, des loyautés historiques et politiques qui constituent l'allégeance au peuple d'Israël », mais le judaïsme n’est ni une religion ni une foi, selon Boyarin. Ainsi Bernard-Henri Lévy affirme que « la tâche des Juifs comme tels est d’être irréligieux », dans la mesure où la religion, telle qu'on la conçoit en théologie, édifiée par une croyance, par des dogmes, par une instance suprême, centrale et doctrinale, n’appartient pas à l’esprit du judaïsme, selon lui. Le judaïsme comporte des éléments religieux, mais ne s'y limite pas puisqu'il contient des coutumes non spécifiquement religieuses – outre des codes de conduite, des lois, des rites – et qu’il fonde plus largement encore une « culture juive ». Néanmoins, par convention, on parle habituellement du judaïsme comme d’une « religion », mais il ne faut pas l’entendre au sens strict, selon des historiens des religions comme Simon Claude Mimouni ou Daniel Boyarin, ou des philosophes comme Léo Strauss ou Bernard-Henri Lévy. Selon ses textes fondateurs, en particulier le Tanakh, la foi des anciens Israélites et de leurs descendants les Juifs, est fondée sur une alliance contractée entre Dieu et Abraham, qui a ensuite été renouvelée entre Dieu et Moïse. Les juifs fondent le judaïsme sur la religion abrahamique qui fleurira ensuite dans la Loi mosaïque (la Torah, les Nevi'im et les Ketouvim), collectivement désignés par l'acronyme Tanakh, dont le texte constitue la Miqra ou Bible hébraïque. Cette religion se fonde sur le culte du Dieu d'Abraham, d'Isaac et de Jacob, au Nom ineffable, qu'elle conçoit comme une Essence éternelle (YHWH), qui détient tous les pouvoirs (Elohim), transcendant le Seigneur des Seigneurs (Adonaï) qu'elle considère Un et Unique et qu'elle qualifie ainsi : omnipotent, omniscient, omniprésent, juste et miséricordieux. Cette religion professe aussi que le rassemblement de toutes les puissances (Elohim) manifesta le créateur du monde qui continue de s'impliquer dans sa destinée en faisant irruption dans l'Histoire dont il révèle la dimension d'Histoire Sainte, comme lorsqu'il fit sortir d'Égypte les enfants d'Israël. Les cohanim, ou prêtres, du Temple de Jérusalem, par deux fois détruit, assuraient son culte. Certains groupes juifs, comme les Ésséniens, s'opposaient à la centralité du culte à Jérusalem. La seconde destruction du Temple de Jérusalem et la dispersion des juifs dans le monde donna naissance à plusieurs traditions religieuses juives. Si la majorité des juifs se regroupèrent autour de l'élaboration du Talmud par les rabbanim, un mouvement strictement scripturaliste, dit Karaïsme, s'opposa à la codification de la tradition orale, tandis que d'autres groupes éloignés, comme les Beta d'Israël en Éthiopie, ignorèrent cette évolution et se développèrent en vase clos. Le judaïsme est l'une des plus anciennes traditions religieuses du monothéisme exclusif encore pratiquées aujourd'hui. Les valeurs et l'histoire du peuple juif sont à la source des deux autres religions abrahamiques, le christianisme et l'islam. Il n'est toutefois pas à la base du samaritanisme, qui est une tradition israélite très tôt distincte du judaïsme de Jérusalem, ni du zoroastrisme, lui-même issu du mazdéisme. <a href=\"#_dbpedia_2017\">(DBpedia, 2017)</a>"@fr, "Refers to the monotheistic religion of the Jewish people, central to which is the belief that the ancient Israelites experienced God's presence in human events. Jews believe that the one God delivered the Israelites out of bondage in Egypt, revealed the structure of communal and individual life to them, and chose them to be a holy nation of people able to set an example for all humankind. The Hebrew Bible and Talmud are the two primary sources for Judaism's spiritual and ethical principles. The religion, which traces its origins to Abraham, places more emphasis on expressing beliefs through ritual rather than through abstract doctrine. The Sabbath, beginning on sunset on Friday and ending at sunset on Saturday, is the central religious observance; there is also an annual cycle of religious festivals and days of fasting. Judaism has had a diverse history of development over almost 4000 years, with a number of resulting branches in modern times, namely Orthodox, Conservative, and Reform. <a href=\"#_getty_2017\">(Getty, 2017)</a>"@en, "Se refiere a la religión monoteista del pueblo judío, para los cuales es central la creencia que los antiguos israelitas experimentaron la presencia de Dios en los eventos humanos. Los judíos creen que el Dios único salvó los israelistas de la esclavitud en Egipto, revelándoles la estructura de la vida comunal e individual y eligiéndolos para ser una nación sagrada de personas capaces de dar un ejemplo para toda la humanidad. La Biblia Hebrea y el Talmud son dos fuentes primarias de la espiritualidad judía y de los principios éticos.Los orígenes de la religión se remontan a los tiempos de Abraham, poniendo mayor énfasis en expresar la creencia con rituales más bien que con doctrinas abstractas. El Shabbat, que comienza con la puesta de sol del viernes y termina con la puesta de sol del sábado, es la observancia religiosa central; hay también un ciclo anual de fiestas religiosas y días de ayuno. El judaísmo ha tenido un desarrollo diverso a lo largo de la historia de casi 4.000 años, con un gran número de ramas resultantes en épocas modernas, concretamente ortodoxas, conservadoras, y reformistas. <a href=\"#_getty_2017\">(Getty, 2017)</a>"@es, "Verwijst naar de monotheïstische religie van het joodse volk, waarbij het geloof centraal staat dat de oude Israëlieten de aanwezigheid van God ervoeren in menselijke gebeurtenissen. Joden geloven dat één God de Israëlieten uit hun gevangenschap in Egypte heeft bevrijd, de structuur van een gemeenschappelijk en individueel leven aan hen heeft onthuld en hen heeft uitverkoren als een heilig volk dat als voorbeeld moest dienen voor de gehele mensheid. De Hebreeuwse bijbel en de Talmoed zijn de belangrijkste bronnen voor de spirituele en ethische principes van het jodendom. Deze religie, waarvan de oorsprong teruggaat naar de tijd van Abraham, legt meer de nadruk op het tot uitdrukking brengen van het geloof in de vorm van rituelen dan in de vorm van abstracte doctrines. De sabbat, die begint bij zonsondergang op vrijdag en eindigt bij zonsondergang op zaterdag, is een centraal element van de religie; er is ook een jaarlijkse cyclus van religieuze feestdagen en vastendagen. Het jodendom heeft een zeer uiteenlopende ontwikkelingsgeschiedenis die bijna 4000 jaar beslaat en is uitgemond in diverse stromingen: de orthodoxe, conservatieve en reformistische stroming. <a href=\"#_getty_2017\">(Getty, 2017)</a>"@nl, "猶太人的一神論宗教，相信古代以色列人於人類事件中體驗到神的存在。猶太人相信這唯一的神使他們脫離埃及的奴役，向他們揭示公共及個人生活的結構，並選擇他們為聖國子民，以為全人類樹立榜樣。《希伯來聖經(Hebrew Bible)》與《塔爾穆德(Talmud)》為猶太教精神與道德原則的兩大來源。猶太教源於亞伯拉罕，較強調以儀式而非抽象的教條表達信仰。遵循信仰的重心為安息日，從週五的日落開始到週日的日出結束；另外每年還有宗教節慶和齋戒日。猶太教經過將近四千年的發展，衍生出許多現代的分支，即正統派猶太教(Orthodox)、保守派猶太教(Conservative)，與改革派猶太教(Reform.)。 <a href=\"#_getty_2017\">(Getty, 2017)</a>"@zh-hant ;
    skos:inScheme cwrc:Religion ;
    prov:derivedFrom dbpedia:Judaism, <http://vocab.getty.edu/aat/300073723> .

cwrc:judaism
    void:inDataset cwrc:datasetdefinition ;
    a cwrc:Religion, owl:Thing, skos:Concept ;
    rdfs:comment "La description de ce terme est basée sur celle de DBPedia."@fr, "The description for this term is indebted to the Getty Art & Architecture Thesaurus."@en ;
    rdfs:isDefinedBy <http://sparql.cwrc.ca/ontologies/cwrc-2017-08-03> ;
    rdfs:label "Jodendom"@nl, "Joods"@nl, "Judaism"@en, "Judaísmo"@es, "Judaïsme"@fr, "you tai jiao"@zh-latn-pinyin-x-notone, "yu t'ai chiao"@zh-latn-wadegile, "yóu tài jiāo"@zh-latn-pinyin-x-hanyu, "猶太教"@zh-hant ;
    skos:broader cwrc:jewishLabel ;
    skos:broaderTransitive cwrc:abrahamicReligions ;
    skos:definition "Pour l'Encyclopædia Britannica, le mot judaïsme recouvre la religion des Juifs, ainsi que la théologie, la loi et les traditions culturelles du peuple juif, constitué des descendants des Israélites provenant de l'antique terre d'Israël et des quelques minorités les ayant rejoints par la conversion et s'étant mélangées à eux au fil de leur diaspora de deux millénaires. Pour un juif orthodoxe comme Daniel Boyarin, le judaïsme est « l'ensemble des rituels et des autres pratiques, des croyances et des valeurs, des loyautés historiques et politiques qui constituent l'allégeance au peuple d'Israël », mais le judaïsme n’est ni une religion ni une foi, selon Boyarin. Ainsi Bernard-Henri Lévy affirme que « la tâche des Juifs comme tels est d’être irréligieux », dans la mesure où la religion, telle qu'on la conçoit en théologie, édifiée par une croyance, par des dogmes, par une instance suprême, centrale et doctrinale, n’appartient pas à l’esprit du judaïsme, selon lui. Le judaïsme comporte des éléments religieux, mais ne s'y limite pas puisqu'il contient des coutumes non spécifiquement religieuses – outre des codes de conduite, des lois, des rites – et qu’il fonde plus largement encore une « culture juive ». Néanmoins, par convention, on parle habituellement du judaïsme comme d’une « religion », mais il ne faut pas l’entendre au sens strict, selon des historiens des religions comme Simon Claude Mimouni ou Daniel Boyarin, ou des philosophes comme Léo Strauss ou Bernard-Henri Lévy. Selon ses textes fondateurs, en particulier le Tanakh, la foi des anciens Israélites et de leurs descendants les Juifs, est fondée sur une alliance contractée entre Dieu et Abraham, qui a ensuite été renouvelée entre Dieu et Moïse. Les juifs fondent le judaïsme sur la religion abrahamique qui fleurira ensuite dans la Loi mosaïque (la Torah, les Nevi'im et les Ketouvim), collectivement désignés par l'acronyme Tanakh, dont le texte constitue la Miqra ou Bible hébraïque. Cette religion se fonde sur le culte du Dieu d'Abraham, d'Isaac et de Jacob, au Nom ineffable, qu'elle conçoit comme une Essence éternelle (YHWH), qui détient tous les pouvoirs (Elohim), transcendant le Seigneur des Seigneurs (Adonaï) qu'elle considère Un et Unique et qu'elle qualifie ainsi : omnipotent, omniscient, omniprésent, juste et miséricordieux. Cette religion professe aussi que le rassemblement de toutes les puissances (Elohim) manifesta le créateur du monde qui continue de s'impliquer dans sa destinée en faisant irruption dans l'Histoire dont il révèle la dimension d'Histoire Sainte, comme lorsqu'il fit sortir d'Égypte les enfants d'Israël. Les cohanim, ou prêtres, du Temple de Jérusalem, par deux fois détruit, assuraient son culte. Certains groupes juifs, comme les Ésséniens, s'opposaient à la centralité du culte à Jérusalem. La seconde destruction du Temple de Jérusalem et la dispersion des juifs dans le monde donna naissance à plusieurs traditions religieuses juives. Si la majorité des juifs se regroupèrent autour de l'élaboration du Talmud par les rabbanim, un mouvement strictement scripturaliste, dit Karaïsme, s'opposa à la codification de la tradition orale, tandis que d'autres groupes éloignés, comme les Beta d'Israël en Éthiopie, ignorèrent cette évolution et se développèrent en vase clos. Le judaïsme est l'une des plus anciennes traditions religieuses du monothéisme exclusif encore pratiquées aujourd'hui. Les valeurs et l'histoire du peuple juif sont à la source des deux autres religions abrahamiques, le christianisme et l'islam. Il n'est toutefois pas à la base du samaritanisme, qui est une tradition israélite très tôt distincte du judaïsme de Jérusalem, ni du zoroastrisme, lui-même issu du mazdéisme. <a href=\"#_dbpedia_2017\">(DBpedia, 2017)</a>"@fr, "Refers to the monotheistic religion of the Jewish people, central to which is the belief that the ancient Israelites experienced God's presence in human events. Jews believe that the one God delivered the Israelites out of bondage in Egypt, revealed the structure of communal and individual life to them, and chose them to be a holy nation of people able to set an example for all humankind. The Hebrew Bible and Talmud are the two primary sources for Judaism's spiritual and ethical principles. The religion, which traces its origins to Abraham, places more emphasis on expressing beliefs through ritual rather than through abstract doctrine. The Sabbath, beginning on sunset on Friday and ending at sunset on Saturday, is the central religious observance; there is also an annual cycle of religious festivals and days of fasting. Judaism has had a diverse history of development over almost 4000 years, with a number of resulting branches in modern times, namely Orthodox, Conservative, and Reform. <a href=\"#_getty_2017\">(Getty, 2017)</a>"@en, "Se refiere a la religión monoteista del pueblo judío, para los cuales es central la creencia que los antiguos israelitas experimentaron la presencia de Dios en los eventos humanos. Los judíos creen que el Dios único salvó los israelistas de la esclavitud en Egipto, revelándoles la estructura de la vida comunal e individual y eligiéndolos para ser una nación sagrada de personas capaces de dar un ejemplo para toda la humanidad. La Biblia Hebrea y el Talmud son dos fuentes primarias de la espiritualidad judía y de los principios éticos.Los orígenes de la religión se remontan a los tiempos de Abraham, poniendo mayor énfasis en expresar la creencia con rituales más bien que con doctrinas abstractas. El Shabbat, que comienza con la puesta de sol del viernes y termina con la puesta de sol del sábado, es la observancia religiosa central; hay también un ciclo anual de fiestas religiosas y días de ayuno. El judaísmo ha tenido un desarrollo diverso a lo largo de la historia de casi 4.000 años, con un gran número de ramas resultantes en épocas modernas, concretamente ortodoxas, conservadoras, y reformistas. <a href=\"#_getty_2017\">(Getty, 2017)</a>"@es, "Verwijst naar de monotheïstische religie van het joodse volk, waarbij het geloof centraal staat dat de oude Israëlieten de aanwezigheid van God ervoeren in menselijke gebeurtenissen. Joden geloven dat één God de Israëlieten uit hun gevangenschap in Egypte heeft bevrijd, de structuur van een gemeenschappelijk en individueel leven aan hen heeft onthuld en hen heeft uitverkoren als een heilig volk dat als voorbeeld moest dienen voor de gehele mensheid. De Hebreeuwse bijbel en de Talmoed zijn de belangrijkste bronnen voor de spirituele en ethische principes van het jodendom. Deze religie, waarvan de oorsprong teruggaat naar de tijd van Abraham, legt meer de nadruk op het tot uitdrukking brengen van het geloof in de vorm van rituelen dan in de vorm van abstracte doctrines. De sabbat, die begint bij zonsondergang op vrijdag en eindigt bij zonsondergang op zaterdag, is een centraal element van de religie; er is ook een jaarlijkse cyclus van religieuze feestdagen en vastendagen. Het jodendom heeft een zeer uiteenlopende ontwikkelingsgeschiedenis die bijna 4000 jaar beslaat en is uitgemond in diverse stromingen: de orthodoxe, conservatieve en reformistische stroming. <a href=\"#_getty_2017\">(Getty, 2017)</a>"@nl, "猶太人的一神論宗教，相信古代以色列人於人類事件中體驗到神的存在。猶太人相信這唯一的神使他們脫離埃及的奴役，向他們揭示公共及個人生活的結構，並選擇他們為聖國子民，以為全人類樹立榜樣。《希伯來聖經(Hebrew Bible)》與《塔爾穆德(Talmud)》為猶太教精神與道德原則的兩大來源。猶太教源於亞伯拉罕，較強調以儀式而非抽象的教條表達信仰。遵循信仰的重心為安息日，從週五的日落開始到週日的日出結束；另外每年還有宗教節慶和齋戒日。猶太教經過將近四千年的發展，衍生出許多現代的分支，即正統派猶太教(Orthodox)、保守派猶太教(Conservative)，與改革派猶太教(Reform.)。 <a href=\"#_getty_2017\">(Getty, 2017)</a>"@zh-hant ;
    skos:inScheme cwrc:Religion ;
    prov:derivedFrom dbpedia:Judaism, <http://vocab.getty.edu/aat/300073723> .

cwrc:labourMovement
    void:inDataset cwrc:datasetdefinition ;
    cwrc:contraryTo cwrc:anti-Trade-Unionism ;
    a cwrc:PoliticalAffiliation, skos:Concept ;
    rdf:value "anti-sweated labour", "factory reformer", "labour activism", "labour activist", "labour advocate", "labour feminist", "labour organizer", "women's labour activist" ;
    rdfs:comment "La description de ce terme est basée sur celle de DBPedia."@fr, "The description for this term is indebted to DBpedia."@en ;
    rdfs:isDefinedBy <http://sparql.cwrc.ca/ontologies/cwrc-2017-08-03> ;
    rdfs:label "Mouvement ouvrier"@fr, "labour movement"@en ;
    skos:definition "Le terme de mouvement ouvrier désigne l'ensemble des mouvements et partis organisés, à partir de l'époque de la révolution industrielle, pour améliorer les conditions d'existence de la classe ouvrière. Cette définition inclut principalement le syndicalisme, mais aussi les partis politiques en étant issus ou s'en étant réclamés et plus largement les différentes formes d'action politique et sociale ayant représenté, ou estimé représenter, les intérêts de la classe ouvrière (coopératisme, mutualisme). Plus particulièrement, au XIXe siècle, la mouvance socialiste — qui adopte dans une partie des pays européens l'appellation de social-démocrate — se pose en représentant du mouvement ouvrier. La nature des liens entre syndicalisme et partis politiques est cependant variable selon les pays : au Royaume-Uni, la précocité du développement industriel a entraîné l'antériorité des syndicats sur le Parti travailliste. Après la scission de la mouvance socialiste au début du XXe siècle, les partis communistes et, prise au sens large, la mouvance communiste dans son ensemble, se sont présentés comme les représentants authentiques du mouvement ouvrier. Les anarchistes ont également pu revendiquer la représentation des intérêts du monde ouvrier, notamment via des phénomènes comme l'anarcho-syndicalisme. <a href=\"#_dbpedia_2017\">(DBpedia, 2017)</a>"@fr, "The Labour movement or Labor movement (see spelling differences), or, respectively, labourism or laborism, are general terms for the collective organization of working people developed to represent and campaign for better working conditions and treatment from their employers and, by the implementation of labour and employment laws, their governments. The standard unit of organization is the trade union. In some countries, especially the United Kingdom and Australia, the labour movement is understood to include a formal political wing, usually as a political party known as a \"labour party\" or \"workers' party\". Many individuals and political groups otherwise considered to represent ruling classes may be part of and active in the labour movement. Contemporary labourism developed in response to the depredations of industrial capitalism at about the same time as socialism. However, while the goal of labourism was to protect and strengthen the interests of labour within capitalism, the goal of socialism was to replace the capitalist system entirely. <a href=\"#_dbpedia_2017\">(DBpedia, 2017)</a>"@en ;
    skos:inScheme cwrc:PoliticalAffiliation ;
    prov:derivedFrom dbpedia:Labour_movement .

cwrc:left-Wing
    void:inDataset cwrc:datasetdefinition ;
    a cwrc:PoliticalAffiliation, skos:Concept ;
    rdf:value "anti-conservative", "leftist" ;
    rdfs:comment "La description de ce terme est basée sur celle de DBPedia."@fr, "The description for this term is indebted to DBpedia."@en ;
    rdfs:isDefinedBy <http://sparql.cwrc.ca/ontologies/cwrc-2017-08-03> ;
    rdfs:label "Gauche (politique)"@fr, "left-wing"@en ;
    skos:definition "En politique, l'usage consiste à diviser les partis politiques en catégories générales qui formalisent une division bipartisane : la droite et la gauche, auxquelles on peut ajouter le centre. Dans l'ensemble du champ politique, les forces politiques sont triples : droite, gauche et forces révolutionnaires (extrême-gauche) hors partis. La notion de gauche et celle de droite en politique est une construction progressive entre la fin du XVIIIe siècle et le début du XXe siècle. La gauche désigne la partie gauche de l'hémicycle d'une assemblée parlementaire et les personnes et partis qui y siègent habituellement. De ce fait, la notion de gauche (comme celle de droite) ne possède pas un contenu idéologique fixe et a priori : par exemple, l'orléanisme est à gauche du légitimisme, le bourgeois libéral est à gauche du bourgeois monarchiste, et ce qui était à gauche à une époque se retrouve souvent à droite à une autre époque, ainsi le bourgeois libéral est aujourd’hui généralement à droite, alors qu'il est de gauche du temps de Benjamin Constant. De nos jours, les partis de gauche se rassemblent généralement dans la promotion d'idéaux progressistes et d'égalité, la critique de l'ordre social et le souci d'une plus grande justice sociale. Elle comprend la social-démocratie, le radicalisme, le socialisme, le communisme et certains courants de l'anarchisme.Le terme n'est pas utilisé que pour les partis, on utilise parfois le terme de gauche syndicale ou plus rarement de gauche associative. <a href=\"#_dbpedia_2017\">(DBpedia, 2017)</a>"@fr, "Left-wing politics supports social equality and egalitarianism, often in opposition to social hierarchy and social inequality. It typically involves a concern for those in society whom its adherents perceive as disadvantaged relative to others (prioritarianism), as well as a belief that there are unjustified inequalities that need to be reduced or abolished (by advocating for social justice). The term left wing can also refer to \"the radical, reforming, or socialist section of a political party or system\". The political terms Left and Right were coined during the French Revolution (1789–1799), referring to the seating arrangement in the Estates General: those who sat on the left generally opposed the monarchy and supported the revolution, including the creation of a republic and secularization, while those on the right were supportive of the traditional institutions of the Old Regime. Use of the term \"Left\" became more prominent after the restoration of the French monarchy in 1815 when it was applied to the \"Independents\". The word \"wing\" was appended to Left and Right in the late 19th century, usually with disparaging intent, and \"left-wing\" was applied to those who were unorthodox in their religious or political views. The term was later applied to a number of movements, especially republicanism during the French Revolution in the 18th century, followed by socialism, communism, anarchism, and social democracy in the 19th and 20th centuries. Since then, the term left-wing has been applied to a broad range of movements including civil rights movements, feminist movements, anti-war movements, and environmental movements, as well as a wide range of parties. According to author Barry Clark, \"Leftists [...] claim that human development flourishes when individuals engage in cooperative, mutually respectful relations that can thrive only when excessive differences in status, power, and wealth are eliminated.\". <a href=\"#_dbpedia_2017\">(DBpedia, 2017)</a>"@en ;
    skos:inScheme cwrc:PoliticalAffiliation ;
    prov:derivedFrom dbpedia:Left-wing_politics .

cwrc:lesbian
    void:inDataset cwrc:datasetdefinition ;
    a cwrc:Sexuality, skos:Concept ;
    rdfs:isDefinedBy <http://sparql.cwrc.ca/ontologies/cwrc-2017-08-03> ;
    rdfs:label "lesbian"@en, "lesbienne"@fr ;
    owl:sameAs <http://homosaurus.org/terms/lesbianIdentity> ;
    skos:definition ""@en, ""@fr ;
    foaf:name "lesbian (sexual identity)"@en .

cwrc:liberalUnionistParty
    void:inDataset cwrc:datasetdefinition ;
    a cwrc:PoliticalAffiliation, skos:Concept ;
    rdf:value "liberal unionist" ;
    rdfs:comment "La description de ce terme est basée sur celle de DBPedia."@fr, "The description for this term is indebted to DBpedia."@en ;
    rdfs:isDefinedBy <http://sparql.cwrc.ca/ontologies/cwrc-2017-08-03> ;
    rdfs:label "Liberal Unionist Party"@en, "Parti libéral unioniste"@fr ;
    skos:definition """Le Liberal Unionist Party est un parti politique britannique qui se sépara du Parti libéral en 1886. Dirigé par Spencer Cavendish (Lord Hartington, et plus tard duc du Devonshire) et Joseph Chamberlain, le parti a formé une alliance politique avec le Parti conservateur dans l'opposition à l’Home Rule de l'Irlande. Les deux partis ont formé un gouvernement de coalition en 1895, mais gardèrent un fonctionnement séparés jusqu'à une fusion complète en mai 1912. 
  * Portail de la politique britannique Portail de la politique britannique <a href=\"#_dbpedia_2017\">(DBpedia, 2017)</a>"""@fr, "The Liberal Unionist Party was a British political party that was formed in 1886 by a faction that broke away from the Liberal Party. Led by Lord Hartington (later the Duke of Devonshire) and Joseph Chamberlain, the party formed a political alliance with the Conservative Party in opposition to Irish Home Rule. The two parties formed the ten-year-long, coalition Unionist Government 1895–1905 but kept separate political funds and their own party organisations until a complete merger was agreed in May 1912. <a href=\"#_dbpedia_2017\">(DBpedia, 2017)</a>"@en ;
    skos:inScheme cwrc:PoliticalAffiliation ;
    prov:derivedFrom dbpedia:Liberal_Unionist_Party .

cwrc:liberalism
    void:inDataset cwrc:datasetdefinition ;
    a cwrc:PoliticalAffiliation, skos:Concept ;
    rdf:value "liberal" ;
    rdfs:comment "La description de ce terme est basée sur celle de DBPedia."@fr, "The description for this term is indebted to DBpedia."@en ;
    rdfs:isDefinedBy <http://sparql.cwrc.ca/ontologies/cwrc-2017-08-03> ;
    rdfs:label "Libéralisme"@fr, "liberalism"@en ;
    skos:definition "Le libéralisme est une doctrine de philosophie politique qui affirme la liberté comme principe politique suprême ainsi que son corollaire de responsabilité individuelle, et revendique la limitation du pouvoir du souverain. Le mot libéralisme fait son apparition au début du XIXe siècle. Les racines du libéralisme sont plus anciennes. L'opposition à l'absolutisme du souverain s'est développée dans l’Europe des Lumières (XVIIIe siècle), mais aussi auparavant par la scolastique de l'École de Salamanque (XVIe siècle) faisant obligation morale au souverain de respecter les droits fondamentaux de chaque être humain au motif de sa nature de créature de Dieu, ou plus anciennement par les chartes médiévales (telles la Magna Carta) introduisant des droits fondamentaux dont le respect est exigé du souverain, ou encore par certains pans de la philosophie thomiste, eux-mêmes précédés par le principe de justice naturelle d'Aristote. La date des débuts formels du libéralisme ou de ses composantes politiques, économiques ou religieuses diffère selon les auteurs. De nombreux auteurs font commencer le libéralisme avec la Lettre sur la tolérance de John Locke (1689) qui complète les racines préexistantes. Le libéralisme repose sur l’idée que chaque être humain possède des droits fondamentaux naturels précédant toute association et qu'aucun pouvoir n'a le droit de violer. En conséquence, les libéraux veulent limiter les obligations sociales imposées par le pouvoir et plus généralement le système social, telles que la morale, au profit du libre choix et de l'intérêt de chaque individu indépendamment des autres. La question de l'articulation entre « libéralisme économique » et « libéralisme politique » reçoit des réponses variées. Le libéralisme prône la liberté d'expression des individus. Dans le domaine économique, il défend notamment l'initiative privée, la libre concurrence et son corollaire l'économie de marché ; dans le domaine politique, il accepte des pouvoirs politiques encadrés par une loi librement débattue, défend un État de droit et des contre-pouvoirs. Au libéralisme classique, fondé davantage sur la liberté en tant que droit négatif, s'oppose entre autres le libéralisme social fondé sur la liberté en tant que droit positif (protection exigée du souverain contre la misère matérielle ou la pression morale communautaire, quitte à accorder au souverain un droit de coercition sociale à cette fin). Ainsi le libéralisme peut se manifester de façons fort diverses, voire opposées. Le « libéral » peut être suivant le cas celui qui exige de l'État qu'il brise une tradition qui contraint la liberté de l'individu (caste, statuts, discriminations et privilèges…), celui qui défend la liberté de pratiquer ou non une religion ou une tradition, celui qui demande que l'État intervienne pour redonner une véritable capacité d'action économique (bridée par un monopole, la pauvreté, le manque d'éducation, de crédit ou autre), ou encore celui qui s'oppose à l'intervention du pouvoir (dans le respect de l'initiative privée, de la libre concurrence, de l’égalité de traitement…). Les limites à fixer à l'action de l'État, ainsi que les modalités de l'action publique, notamment aux rôles respectifs de l'action administrative et de la loi, sont donc sujets à débat au sein même du libéralisme. La plupart des libéraux considèrent que l'action de l'État est nécessaire à la protection des libertés individuelles, dans le cadre de ses fonctions régaliennes, et nombre d'entre eux (comme Adam Smith, Raymond Aron, Karl Popper ou Benedetto Croce) acceptent et même recommandent certaines interventions de l'État dans l'économie, notamment en matière de contrôle et de régulation. À l'opposé, les libertariens de tendance anarcho-capitaliste refusent à l'État toute légitimité dans quelque domaine que ce soit. <a href=\"#_dbpedia_2017\">(DBpedia, 2017)</a>"@fr, "Liberalism is a political philosophy or worldview founded on ideas of liberty and equality. Whereas classical liberalism emphasises the role of liberty, social liberalism stresses the importance of equality. Liberals espouse a wide array of views depending on their understanding of these principles, but generally they support ideas and programmes such as freedom of speech, freedom of the press, freedom of religion, free markets, civil rights, democratic societies, secular governments, gender equality and international cooperation. Liberalism first became a distinct political movement during the Age of Enlightenment, when it became popular among philosophers and economists in the Western world. Liberalism rejected the prevailing social and political norms of hereditary privilege, state religion, absolute monarchy, and the Divine Right of Kings. The 17th-century philosopher John Locke is often credited with founding liberalism as a distinct philosophical tradition. Locke argued that each man has a natural right to life, liberty and property, while adding that governments must not violate these rights based on the social contract. Liberals opposed traditional conservatism and sought to replace absolutism in government with representative democracy and the rule of law. Prominent revolutionaries in the Glorious Revolution, the American Revolution, and the French Revolution used liberal philosophy to justify the armed overthrow of what they saw as tyrannical rule. Liberalism started to spread rapidly especially after the French Revolution. The 19th century saw liberal governments established in nations across Europe, South America, and North America. In this period, the dominant ideological opponent of classical liberalism was conservatism, but liberalism later survived major ideological challenges from new opponents, such as fascism and communism. During the 20th century, liberal ideas spread even further as liberal democracies found themselves on the winning side in both world wars. In Europe and North America, the establishment of social liberalism became a key component in the expansion of the welfare state. Today, liberal parties continue to wield power and influence throughout the world. <a href=\"#_dbpedia_2017\">(DBpedia, 2017)</a>"@en ;
    skos:inScheme cwrc:PoliticalAffiliation ;
    prov:derivedFrom dbpedia:Liberalism .

cwrc:libertarianism
    void:inDataset cwrc:datasetdefinition ;
    a cwrc:PoliticalAffiliation, skos:Concept ;
    rdf:value "libertarian", "religious libertarian" ;
    rdfs:comment "La description de ce terme est basée sur celle de DBPedia."@fr, "The description for this term is indebted to DBpedia."@en ;
    rdfs:isDefinedBy <http://sparql.cwrc.ca/ontologies/cwrc-2017-08-03> ;
    rdfs:label "Libertarianism"@en, "Libertarianisme"@fr ;
    skos:definition "Le libertarianisme, aussi appelé libertarisme (à ne pas confondre avec libertarisme de gauche et Libertaire) est une philosophie politique qui conçoit la société juste comme une société dont les institutions respectent et protègent la liberté de chaque individu d’exercer son plein droit de propriété sur lui-même et les droits de propriété qu’il a légitimement acquis sur des objets extérieurs. Issue du libéralisme elle prône donc, au sein d'un système de propriété et de marché universel, la liberté individuelle en tant que droit naturel. La liberté est conçue par le libertarianisme comme une valeur fondamentale des rapports sociaux, des échanges économiques et du système politique. Les libertariens se fondent sur le principe de non-agression qui affirme que nul ne peut prendre l'initiative de la force physique contre un individu, sa personne, sa liberté ou sa propriété. De fait, ses partisans, les libertariens, sont favorables à une réduction voire à la disparition de l'État (antiétatisme) en tant que système fondé sur la coercition, au profit d'une coopération libre et volontaire entre les individus, avec un État limité à des fonctions régaliennes. Robert Nozick (1938-2002), Murray Rothbard (1926-1995) et Charles Murray (1943-) font partie des principaux auteurs nourrissant cette doctrine. <a href=\"#_dbpedia_2017\">(DBpedia, 2017)</a>"@fr, "Libertarianism (Latin: liber, \"free\") is a collection of political philosophies that uphold liberty. Libertarians seek to maximize autonomy and freedom of choice, emphasizing political freedom, voluntary association, and the primacy of individual judgment. Libertarians generally share a skepticism of authority; however, they diverge on the scope of their opposition to existing political and economic systems. Various schools of libertarian thought offer a range of views regarding the legitimate functions of state and private power, often calling to restrict or to dissolve coercive social institutions. Some libertarians advocate laissez-faire capitalism and strong private property rights, such as in land, infrastructure, and natural resources. Others, notably libertarian socialists, seek to abolish capitalism and private ownership of the means of production in favor of their common or cooperative ownership and management. An additional line of division is between minarchists and anarchists. While minarchists think that a minimal centralized government is necessary, anarchists propose to completely eliminate the state. <a href=\"#_dbpedia_2017\">(DBpedia, 2017)</a>"@en ;
    skos:inScheme cwrc:PoliticalAffiliation ;
    prov:derivedFrom dbpedia:Libertarianism .

cwrc:lollards
    dcterms:isReplacedBy cwrc:lollardy ;
    void:inDataset cwrc:datasetdefinition ;
    a skos:Concept ;
    rdfs:comment "Deprecated in favour of instance #lollardy."@en, "Désapprouver en faveur de l'instance #lollardy."@fr, "La description de ce terme est basée sur celle de DBPedia."@fr ;
    rdfs:isDefinedBy <http://sparql.cwrc.ca/ontologies/cwrc-2017-08-03> ;
    rdfs:label "Lollards"@en, "Lollards"@fr ;
    owl:deprecated true ;
    vs:term_status "deprecated"@en ;
    skos:broaderTransitive cwrc:catholicChurch ;
    skos:definition "Les Lollards sont les membres ou sympathisants d'un mouvement de contestation religieuse et sociale apparu en Angleterre au XIVe siècle. — John Ball <a href=\"#_dbpedia_2017\">(DBpedia, 2017)</a> "@fr, "Lollardy (Lollardry, Lollardism) was a political and religious movement that existed from the mid-14th century to the English Reformation. It was initially led by John Wycliffe, a prominent theologian who was dismissed from the University of Oxford in 1381 for criticism of the Church, especially in his doctrine on the Eucharist. The Lollards' demands were primarily for reform of Western Christianity. <a href=\"#_dbpedia_2017\">(DBpedia, 2017)</a>"@en ;
    skos:inScheme cwrc:Religion ;
    prov:derivedFrom dbpedia:Lollardy .

cwrc:lollardy
    void:inDataset cwrc:datasetdefinition ;
    a cwrc:Religion, skos:Concept ;
    rdfs:comment "La description de ce terme est basée sur celle de DBPedia."@fr ;
    rdfs:isDefinedBy <http://sparql.cwrc.ca/ontologies/cwrc-2017-08-03> ;
    rdfs:label "Lollardy"@en, "Lollardy"@fr ;
    skos:broaderTransitive cwrc:catholicChurch ;
    skos:definition "Les Lollards sont les membres ou sympathisants d'un mouvement de contestation religieuse et sociale apparu en Angleterre au XIVe siècle. — John Ball <a href=\"#_dbpedia_2017\">(DBpedia, 2017)</a> "@fr, "Lollardy (Lollardry, Lollardism) was a political and religious movement that existed from the mid-14th century to the English Reformation. It was initially led by John Wycliffe, a prominent theologian who was dismissed from the University of Oxford in 1381 for criticism of the Church, especially in his doctrine on the Eucharist. The Lollards' demands were primarily for reform of Western Christianity. <a href=\"#_dbpedia_2017\">(DBpedia, 2017)</a>"@en ;
    skos:inScheme cwrc:Religion ;
    prov:derivedFrom dbpedia:Lollardy .

cwrc:lowerMiddleClass
    void:inDataset cwrc:datasetdefinition ;
    a cwrc:SocialClass, skos:Concept ;
    rdfs:isDefinedBy <http://sparql.cwrc.ca/ontologies/cwrc-2017-08-03> ;
    rdfs:label "classe-moyenne inférieure"@fr, "lower-middle class"@en ;
    skos:definition ""@fr, "Employees, clerical workers, teachers, governesses. Note, however, that some teachers go into Professions (<a href=\"https://en.wikipedia.org/wiki/Goodbye,_Mr._Chips_(1939_film)\">Mr. Chips from the 1939 film of that name</a>) and women starting schools and then managing them also go into Professions."@en ;
    skos:inScheme cwrc:SocialClass .

cwrc:maleLabel
    void:inDataset cwrc:datasetdefinition ;
    a skosxl:Label ;
    rdf:value "male" ;
    rdfs:comment "Deprecated with no current equivalence.."@en, "Désapprouver sans équivalence."@fr ;
    rdfs:isDefinedBy <http://sparql.cwrc.ca/ontologies/cwrc-2017-08-03> ;
    rdfs:label "male"@en, "male"@fr ;
    owl:deprecated true ;
    owl:oneOf (cwrc:genderManMale
        cwrc:maleSex
    ) ;
    vs:term_status "deprecated"@en ;
    skos:definition ""@en, ""@fr ;
    skos:inScheme cwrc:TextLabels ;
    foaf:name "Male (Label)"@en .

cwrc:maleSex
    dcterms:isReplacedBy cwrc:genderManMale ;
    void:inDataset cwrc:datasetdefinition ;
    a owl:Thing, skos:Concept ;
    rdfs:comment "Deprecated in favour of instance #genderManMale."@en, "Désapprouver en faveur de l'instance #genderManMale."@fr ;
    rdfs:isDefinedBy <http://sparql.cwrc.ca/ontologies/cwrc-2017-08-03> ;
    rdfs:label "Male"@en, "Mâle"@fr ;
    owl:deprecated true ;
    vs:term_status "deprecated"@en ;
    skos:definition ""@en, ""@fr ;
    foaf:name "Male (Sex)"@en .

cwrc:man
    void:inDataset cwrc:datasetdefinition ;
    a cwrc:Gender, owl:Thing, skos:Concept ;
    rdfs:isDefinedBy <http://sparql.cwrc.ca/ontologies/cwrc-2017-08-03> ;
    rdfs:label "homme"@fr, "man"@en ;
    skos:definition ""@en ;
    foaf:name "man (gender)"@en .

cwrc:manLabel
    void:inDataset cwrc:datasetdefinition ;
    a skos:Concept, skosxl:Label ;
    rdf:value "man" ;
    rdfs:isDefinedBy <http://sparql.cwrc.ca/ontologies/cwrc-2017-08-03> ;
    rdfs:label "homme"@fr, "man"@en ;
    owl:oneOf (cwrc:man
    ) ;
    skos:definition ""@en, ""@fr ;
    skos:inScheme cwrc:TextLabels ;
    foaf:name "Man (Label)"@en .

cwrc:managerial
    void:inDataset cwrc:datasetdefinition ;
    a cwrc:SocialClass, skos:Concept ;
    rdfs:isDefinedBy <http://sparql.cwrc.ca/ontologies/cwrc-2017-08-03> ;
    rdfs:label "gestionnaire"@fr, "managerial"@en ;
    skos:definition ""@fr, "Someone whose station in life comes from the fact that they are running something but not putting their money into it, e.g. salaried civil service, bankers, hospital administrators."@en ;
    skos:inScheme cwrc:SocialClass .

cwrc:maoism
    void:inDataset cwrc:datasetdefinition ;
    a cwrc:PoliticalAffiliation, skos:Concept ;
    rdf:value "chinese communism" ;
    rdfs:comment "La description de ce terme est basée sur celle de DBPedia."@fr, "The description for this term is indebted to DBpedia."@en ;
    rdfs:isDefinedBy <http://sparql.cwrc.ca/ontologies/cwrc-2017-08-03> ;
    rdfs:label "Maoism"@en, "Maoïsme"@fr ;
    skos:definition "Le maoïsme (en chinois : 毛泽东思想, pinyin : Máo Zédōng sīxiǎng, « pensée Mao-Zedong ») est un courant du communisme développé au XXe siècle par Mao Zedong, chef du Parti communiste chinois, qui arrive au pouvoir en Chine en 1949, au terme d'une longue guerre civile contre le Guomindang. Comme Lénine dit avoir adapté les théories de Karl Marx à la Russie, Mao déclare adapter les théories de Marx et de Lénine à la situation politique et économique de la Chine du XXe siècle. Au sortir de la Seconde Guerre mondiale, Mao affirme vouloir émanciper la population chinoise à la fois de l'impérialisme occidental et du confucianisme. Au moment de la rupture sino-soviétique, Mao se réclame d'une lecture « anti-révisionniste » du marxisme-léninisme et refuse de suivre un processus parallèle à la déstalinisation, poussant la Chine encore plus loin sur la voie du quadrillage total de la société par le Parti et du culte de sa personnalité. Le maoïsme, même si la tendance pro-soviétique reste largement majoritaire au sein du communisme mondial, commence alors à la concurrencer, et de multiples groupes à travers le monde se réclament de Mao et de sa vision tiers-mondiste et « anti-impérialiste ». L'Albanie d'Enver Hoxha devient même un pays satellite de la Chine. Après la mort de Mao en 1976, le maoïsme est, en République populaire de Chine, progressivement vidé de sa substance idéologique même si le PCC continue de se réclamer officiellement de la « pensée Mao-Zedong ». En revanche, des groupes maoïstes, d'importance très inégale, continuent d'exister à travers le monde, notamment des groupes armés de l'Inde, du Népal et d'Amérique latine. En Occident, le maoïsme intellectuel a fait long feu, ses adeptes (dont le philosophe Jean-Paul Sartre) ayant dans leur immense majorité changé d'opinions après la mort de Mao ; il est considéré par les historiens d'aujourd'hui comme une idéologie totalitaire comparable au stalinisme. <a href=\"#_dbpedia_2017\">(DBpedia, 2017)</a>"@fr, "Mao Zedong Thought (simplified Chinese: 毛泽东思想; traditional Chinese: 毛澤東思想; pinyin: Máo Zédōng Sīxiǎng), or Maoism, is a political theory derived from the teachings of the Chinese political leader Mao Zedong (1893–1976). Its followers, known as Maoists, consider it an anti-Revisionist form of Marxism–Leninism. Developed from the 1950s until the Deng Xiaoping reforms in the 1970s, it was widely applied as the guiding political and military ideology of the Communist Party of China (CPC), and as theory guiding revolutionary movements around the world. The essential difference between Maoism and other forms of Marxism is that Mao claimed that peasants should be the essential revolutionary class in China, because, contrary to their industrial working \"comrades,\" they were more suited to establishing a successful revolution and socialist society in China. <a href=\"#_dbpedia_2017\">(DBpedia, 2017)</a>"@en ;
    skos:inScheme cwrc:PoliticalAffiliation ;
    prov:derivedFrom dbpedia:Maoism .

cwrc:marriageLawReform
    void:inDataset cwrc:datasetdefinition ;
    a cwrc:PoliticalAffiliation, skos:Concept ;
    rdf:value "custody rights", "divorce reform activist", "divorce reformer", "marriage law reformer", "marriage reformer", "married women's property supporter", "maternal wage activist" ;
    rdfs:comment "The description for this term is indebted to DBpedia."@en ;
    rdfs:isDefinedBy <http://sparql.cwrc.ca/ontologies/cwrc-2017-08-03> ;
    rdfs:label ""@fr, "marriage law reform"@en ;
    skos:definition ""@fr, "Advocacy or activism related to the reform of laws related to marriage and divorce, including education, marital rape, wages for housework and childrearing, property law, child custody, and civil rights."@en ;
    skos:inScheme cwrc:PoliticalAffiliation .

cwrc:marxism
    void:inDataset cwrc:datasetdefinition ;
    a cwrc:PoliticalAffiliation, skos:Concept ;
    rdf:value "marxist" ;
    rdfs:comment "La description de ce terme est basée sur celle de DBPedia."@fr, "The description for this term is indebted to DBpedia."@en ;
    rdfs:isDefinedBy <http://sparql.cwrc.ca/ontologies/cwrc-2017-08-03> ;
    rdfs:label "Marxism"@en, "Marxisme"@fr ;
    skos:definition "Le marxisme est un courant de pensée politique, sociologique et économique fondé sur les idées de Karl Marx (et dans une moindre mesure de Friedrich Engels) et de ses continuateurs. Politiquement, le marxisme repose sur la participation au mouvement réel de la lutte des classes, afin d'arriver à une société sans classes en tant qu'alternative au capitalisme. En effet, Karl Marx considère que « l’émancipation des travailleurs doit être l’œuvre des travailleurs eux-mêmes ». <a href=\"#_dbpedia_2017\">(DBpedia, 2017)</a>"@fr, "Marxism is a method of socioeconomic analysis that analyzes class relations and societal conflict using a materialist interpretation of historical development and a dialectical view of social transformation. It originates from the mid-to-late 19th century works of German philosophers Karl Marx and Friedrich Engels. Marxist methodology originally used a method of economic and sociopolitical inquiry known as historical materialism to analyze and critique the development of capitalism and the role of class struggle in systemic economic change. According to Marxist perspective, class conflict within capitalism arises due to intensifying contradictions between the highly productive mechanized and socialized production performed by the proletariat, and the private ownership and appropriation of the surplus product (profit) by a small minority of the population who are private owners called the bourgeoisie. As the contradiction becomes apparent to the proletariat through the alienation of labor, social unrest between the two antagonistic classes will intensify, until it culminates in social revolution. The eventual long-term outcome of this revolution would be the establishment of socialism – a socioeconomic system based on social ownership of the means of production, distribution based on one's contribution, and production organized directly for use. As the productive forces and technology continued to advance, Marx hypothesized that socialism would eventually give way to a communist stage of social development, which would be a classless, stateless, humane society erected on common ownership and the principle of \"From each according to his ability, to each according to his needs\". Marxism has since developed into different branches and schools of thought, and there is now no single definitive Marxist theory. Different Marxian schools place a greater emphasis on certain aspects of classical Marxism while de-emphasizing or rejecting other aspects, and sometimes combine Marxist analysis with non-Marxian concepts; as a result, they might reach contradictory conclusions from each other. Lately, however, there is movement toward the recognition that the main aspect of Marxism is philosophy of dialectical materialism and historicism, which should result to more agreement between different schools. Marxist analyses and methodologies have influenced multiple political ideologies and social movements, and Marxist understandings of history and society have been adopted by some academics in the disciplines of archaeology, anthropology, media studies, political science, theater, history, sociology, art history and theory, cultural studies, education, economics, geography, literary criticism, aesthetics, critical psychology, and philosophy. <a href=\"#_dbpedia_2017\">(DBpedia, 2017)</a>"@en ;
    skos:inScheme cwrc:PoliticalAffiliation ;
    prov:derivedFrom dbpedia:Marxism .

cwrc:methodism
    void:inDataset cwrc:datasetdefinition ;
    a cwrc:Religion, skos:Concept ;
    rdfs:isDefinedBy <http://sparql.cwrc.ca/ontologies/cwrc-2017-08-03> ;
    rdfs:label "Methodism"@en, "Église méthodiste"@fr ;
    skos:broaderTransitive cwrc:protestantism ;
    skos:definition ""@fr, "\"Or United Methodists, an English Nonconformist community formed in 1907 by the union of the Methodist New Connexion (1797), the Bible Christians (1815), and the United Methodist Free Churches (1857). The act of parliament which enabled this amalgamation received the royal assent on the 26th of July 1907, and authorized the union “to deal with real and personal property belonging to the said three churches or denominations, to provide for the vesting of the said property in trust for the United Church so formed and for the assimilation of the trusts thereof, and for other purposes.” The union was completed on the 16th of September 1907 in Wesley's Chapel, City Road, London.\"<a href=\"#_britannica_1911\">(Encyclopedia Britannica, 1911)</a>"@en ;
    skos:inScheme cwrc:Religion .

cwrc:millenarianism
    void:inDataset cwrc:datasetdefinition ;
    a cwrc:Religion, skos:Concept, foaf:Organization ;
    rdfs:comment "La description de ce terme est basée sur celle de DBPedia."@fr ;
    rdfs:isDefinedBy <http://sparql.cwrc.ca/ontologies/cwrc-2017-08-03> ;
    rdfs:label "Millenarianism"@en, "millénarisme, ou chiliasme"@fr ;
    skos:definition "Le millénarisme, ou chiliasme (ou encore, mais de façon erronée, chialisme), est une doctrine religieuse qui soutient l'idée d'un règne terrestre du Messie, après que celui-ci aura chassé l'Antéchrist et préalablement au Jugement dernier.Cette pensée est présente dans certains courants du judaïsme, dans l'Apocalypse de Jean, dans les écrits des Pères apostoliques et dans l'islam sunnite et chiite.Toujours par extension, le mot peut servir à désigner dans le langage courant des types de pensée non plus religieuses mais politiques. <a href=\"#_dbpedia_2017\">(DBpedia, 2017)</a>"@fr, "Millenarianism (also millenarism), from Latin mīllēnārius \"containing a thousand\", is the belief by a religious, social, or political group or movement in a coming major transformation of society, after which all things will be changed. Millenarianism is a concept or theme that exists in many cultures and religions. <a href=\"#_dbpedia_2017\">(DBpedia, 2017)</a>"@en ;
    skos:inScheme cwrc:Religion ;
    prov:derivedFrom dbpedia:Millenarianism .

cwrc:monarchism
    void:inDataset cwrc:datasetdefinition ;
    a cwrc:PoliticalAffiliation, skos:Concept ;
    rdf:value "monarchist", "royalist" ;
    rdfs:comment "La description de ce terme est basée sur celle de DBPedia."@fr, "The description for this term is indebted to DBpedia."@en ;
    rdfs:isDefinedBy <http://sparql.cwrc.ca/ontologies/cwrc-2017-08-03> ;
    rdfs:label "Monarchisme"@fr, "monarchism"@en ;
    skos:definition "Le monarchisme est une doctrine politique qui prône la monarchie, c’est-à-dire une forme de gouvernement dans laquelle une seule personne fonde l'autorité de l'État. Le mode de désignation du monarque n'est pas nécessairement héréditaire : il peut dans de rares cas être élu, comme les empereurs du Saint-Empire romain germanique, les doges de la République de Venise ou (encore actuellement) les Papes de l'Église catholique romaine. Cependant, les mots monarque et monarchisme sont presque toujours utilisés à la place de ceux de roi et royalisme, en particulier dans les textes de ceux qui critiquaient la royauté sous l'Ancien Régime. On parle aussi, avec le présidentialisme, de monarchie républicaine. <a href=\"#_dbpedia_2017\">(DBpedia, 2017)</a>"@fr, "Monarchism is the advocacy of a monarch or monarchical rule. A monarchist is an individual who supports this form of government, independent of any specific monarch; one who espouses a particular monarch is a royalist. Conversely, the opposition to monarchical rule is sometimes referred to as republicanism. Depending on the country, a monarchist may advocate for the rule of the person who sits on the throne, a pretender, or someone who would otherwise occupy the throne but has been deposed. <a href=\"#_dbpedia_2017\">(DBpedia, 2017)</a>"@en ;
    skos:inScheme cwrc:PoliticalAffiliation ;
    prov:derivedFrom dbpedia:Monarchism .

cwrc:motherOf
    void:inDataset cwrc:datasetdefinition ;
    a owl:ObjectProperty ;
    rdf:value "MOTHER" ;
    rdfs:isDefinedBy <http://sparql.cwrc.ca/ontologies/cwrc-2017-08-03> ;
    rdfs:label "mother of"@en, "mère de"@fr ;
    rdfs:subPropertyOf cwrc:parentOf .

cwrc:multiculturalism
    void:inDataset cwrc:datasetdefinition ;
    a cwrc:PoliticalAffiliation, skos:Concept ;
    rdf:value "multiculturalist" ;
    rdfs:comment "La description de ce terme est basée sur celle de DBPedia."@fr, "The description for this term is indebted to DBpedia."@en ;
    rdfs:isDefinedBy <http://sparql.cwrc.ca/ontologies/cwrc-2017-08-03> ;
    rdfs:label "Multiculturalisme"@fr, "multiculturalism"@en ;
    skos:definition """Le multiculturalisme est un terme sujet à diverses interprétations. Il peut simplement désigner la coexistence de différentes cultures (ethniques, religieuses, etc.) au sein d'un même ensemble (pays, par exemple). Il peut aussi désigner différentes politiques volontaristes : 
  *  anti-discriminatoires, visant à assurer un statut social égal aux membres des diverses cultures ; 
  *  communautaires, permettant l'existence de statuts (légaux, administratifs…) spécifiques aux membres de telle ou telle communauté culturelle ;  
  *  identitaires, visant à favoriser l'expression des particularités des diverses cultures ; 
  *  et aujourd’hui le multiculturalisme se centre sur le thème religieux (pluralisme). Multiculturalisme s’oppose à interculturalisme. Dans une société interculturelle les immigrés ou leurs descendants participent à l’ensemble des activités de la société d’accueil. Une intégration culturelle réussie nécessite l’abandon d’une partie de la culture d’origine qui ne serait pas compatible avec les valeurs de la société d’accueil. <a href=\"#_dbpedia_2017\">(DBpedia, 2017)</a>"""@fr, "Multiculturalism describes the existence, acceptance, and/or promotion of multiple cultural traditions within a single jurisdiction, usually considered in terms of the culture associated with an aboriginal ethnic group and foreigner ethnic groups. This can happen when a jurisdiction is created or expanded by amalgamating areas with two or more different cultures (e.g. French Canada and English Canada) or through immigration from different jurisdictions around the world (e.g. Australia, Canada, United States, United Kingdom, and many other countries). Multicultural ideologies and policies vary widely, ranging from the advocacy of equal respect to the various cultures in a society, to a policy of promoting the maintenance of cultural diversity, to policies in which people of various ethnic and religious groups are addressed by the authorities as defined by the group to which they belong. Multiculturalism that promotes maintaining the distinctiveness of multiple cultures is often contrasted to other settlement policies such as social integration, cultural assimilation and racial segregation. Multiculturalism has been described as a \"salad bowl\" and \"cultural mosaic\". Two different and seemingly inconsistent strategies have developed through different government policies and strategies. The first focuses on interaction and communication between different cultures; this approach is also often known as interculturalism. The second centers on diversity and cultural uniqueness which can sometimes result in intercultural competition over jobs among other things and may lead to ethnic conflict. Cultural isolation can protect the uniqueness of the local culture of a nation or area and also contribute to global cultural diversity. A common aspect of many policies following the second approach is that they avoid presenting any specific ethnic, religious, or cultural community values as central. <a href=\"#_dbpedia_2017\">(DBpedia, 2017)</a>"@en ;
    skos:inScheme cwrc:PoliticalAffiliation ;
    prov:derivedFrom dbpedia:Multiculturalism .

cwrc:multiracialism
    void:inDataset cwrc:datasetdefinition ;
    a cwrc:PoliticalAffiliation, skos:Concept ;
    rdf:value "multi-racialist" ;
    rdfs:comment "The description for this term is indebted to DBpedia."@en ;
    rdfs:isDefinedBy <http://sparql.cwrc.ca/ontologies/cwrc-2017-08-03> ;
    rdfs:label ""@fr, "multiracialism"@en ;
    skos:definition ""@fr, "Multiracialism is a concept or ideology that promotes a society composed of various races, while accepting and respecting different cultural backgrounds. It is a society that consists of a diverse mix of people, whether it be relative to their ethnicity, language, culture, religion, or traditions. <a href=\"#_dbpedia_2017\">(DBpedia, 2017)</a>"@en ;
    skos:inScheme cwrc:PoliticalAffiliation ;
    prov:derivedFrom dbpedia:Multiracialism .

cwrc:nationalism
    void:inDataset cwrc:datasetdefinition ;
    a cwrc:PoliticalAffiliation, skos:Concept ;
    rdfs:comment "La description de ce terme est basée sur celle de DBPedia."@fr, "The description for this term is indebted to DBpedia."@en ;
    rdfs:isDefinedBy <http://sparql.cwrc.ca/ontologies/cwrc-2017-08-03> ;
    rdfs:label "Nationalisme"@fr, "nationalism"@en ;
    skos:definition "Le nationalisme est un principe politique, né à la fin du XVIIIe siècle, tendant à légitimer l'existence d'un État-nation pour chaque peuple (initialement par opposition à la royauté, régime politique qui en France sera ensuite nommé Ancien Régime). Ce principe politique s'est progressivement imposé en Europe au cours du XIXe siècle et au début du XXe siècle. Les historiens ne présentent pas ce nationalisme, en général, comme une idéologie, car il est peu et mal argumenté ou justifié par des intellectuels. Depuis son avènement il est en revanche facilement présenté comme une évidence dans la vie politique et sociale. Ce terme désigne aussi des mouvements politiques déclarant vouloir exalter une nation sous toutes ses formes (État, culture, religion, traditions, préférence nationale pour l'emploi...), par opposition aux autres nations et populations. Cette deuxième variante du mouvement s'est développée à partir de la fin du XIXe siècle, vers 1870 : chauvine et xénophobe, elle trouvait alors ses militants principalement dans la petite bourgeoisie. Le nationalisme apparaît aussi, à partir du milieu du XIXe siècle, comme un sentiment national plus ou moins répandu et exalté au sein de la population d'un pays, et s'invitant (surtout au XXe siècle) au sein de multiples doctrines ou idéologies politiques, allant du communisme (par exemple le concept de Patriotisme anti-impérialiste de Mao Zedong) et du fascisme (concept de Totalitarisme anticapitaliste de Benito Mussolini) jusqu'aux démocraties parlementaires, en passant par la Troisième Internationale léniniste. Ainsi il a souvent servi de justification aux épurations ethniques du XXe siècle, peut-être parce que le sentiment national est devenu « puissamment mobilisateur », comme l'avaient compris dès le printemps des peuples de 1848 certains conseillers de dynasties européennes. On distingue en général trois formes principales de nationalisme, le nationalisme ethnique, ou ethnonationalisme, qui est la forme de nationalisme dans lequel la « nation » est défini en termes d'appartenance ethnique (« biologique »), le nationalisme civique, le plus souvent inspiré par des notions issues du droit du sol et le nationalisme culturel, position intermédiaire entres les deux autres formes et dans lequel la nation est définie par une culture commune. <a href=\"#_dbpedia_2017\">(DBpedia, 2017)</a>"@fr, "Nationalism is a shared group feeling in the significance of a geographical and sometimes demographic region seeking independence for its culture or ethnicity that holds that group together. This can be expressed as a belief or political ideology that involves an individual identifying with or becoming attached to one's nation. Nationalism involves national identity, by contrast with the related concept of patriotism, which involves the social conditioning and personal behaviours that support a state's decisions and actions. From a political or sociological perspective, there are two main perspectives on the origins and basis of nationalism. One is the primordialist perspective that describes nationalism as a reflection of the ancient and perceived evolutionary tendency of humans to organize into distinct groupings based on an affinity of birth. The other is the modernist perspective that describes nationalism as a recent phenomenon that requires the structural conditions of modern society in order to exist. An alternative perspective to both of these lineages comes out of engaged theory, and argues that while the form of nationalism is modern, the content and subjective reach of nationalism depends upon 'primordial' sentiments. There are various definitions for what constitutes a nation, however, which leads to several different strands of nationalism. It can be a belief that citizenship in a state should be limited to one ethnic, cultural, religious, or identity group, or that multinationality in a single state should necessarily comprise the right to express and exercise national identity even by minorities.The adoption of national identity in terms of historical development has commonly been the result of a response by influential groups unsatisfied with traditional identities due to inconsistency between their defined social order and the experience of that social order by its members, resulting in a situation of anomie that nationalists seek to resolve. This anomie results in a society or societies reinterpreting identity, retaining elements that are deemed acceptable and removing elements deemed unacceptable, in order to create a unified community. This development may be the result of internal structural issues or the result of resentment by an existing group or groups towards other communities, especially foreign powers that are or are deemed to be controlling them. National flags, national anthems and other symbols of national identity are commonly considered highly important symbols of the national community. <a href=\"#_dbpedia_2017\">(DBpedia, 2017)</a>"@en ;
    skos:inScheme cwrc:PoliticalAffiliation ;
    prov:derivedFrom dbpedia:Nationalism .

cwrc:nazism
    void:inDataset cwrc:datasetdefinition ;
    a cwrc:PoliticalAffiliation, skos:Concept ;
    rdf:value "nazi", "pro-nazi" ;
    rdfs:comment "La description de ce terme est basée sur celle de DBPedia."@fr, "The description for this term is indebted to DBpedia."@en ;
    rdfs:isDefinedBy <http://sparql.cwrc.ca/ontologies/cwrc-2017-08-03> ;
    rdfs:label "Nazism"@en, "Nazisme"@fr ;
    skos:definition "Le national-socialisme (en allemand : Nationalsozialismus), plus couramment désigné en français sous l'abréviation nazisme, est l'idéologie politique du Parti national-socialiste des travailleurs allemands (NSDAP), parti politique d'extrême droite fondé en Allemagne en 1920 et dirigé par Adolf Hitler. Cette idéologie théorise une hiérarchie au sein d'une espèce humaine divisée en « races », au sommet de laquelle elle place la « race aryenne ». Le nazisme est le seul type de fascisme incorporant à la fois racisme biologique et antisémitisme. Par extension, le terme nazisme désigne le régime politique inspiré de cette idéologie, dictature totalitaire et expansionniste dirigée par Adolf Hitler de 1933 à 1945 et connue sous les noms de Troisième Reich et d'Allemagne nazie. En tant que sujet de science politique, les définitions du nazisme varient selon les historiens. En particulier, reste ouverte la question de savoir si le nazisme ne fut que l'une des formes du fascisme ou, parce qu'ayant fait du racisme une doctrine d'État, le nazisme doit être considéré comme un phénomène historique unique. En effet, l'antisémitisme officiel du régime nazi, dès 1933, l'élimination des personnes handicapées et la persécution des opposants politiques, des Juifs, des homosexuels, des Roms, etc., se concrétisèrent par la mise en place, dès 1933, des premiers camps de concentration en Allemagne. Cette politique ne fit que s'amplifier du début de la Seconde Guerre mondiale, qui vit la création des camps d’extermination nazis, jusqu'à la défaite militaire du nazisme en 1945. Ainsi près de six millions de personnes, dont une majorité de Juifs, périrent dans les camps de concentration et d'extermination nazi ou par la Shoah par balles (voir Shoah). Le régime nazi, censé « durer mille ans », en dura douze et laissa l'Allemagne en ruine. <a href=\"#_dbpedia_2017\">(DBpedia, 2017)</a>"@fr, "National Socialism (German: Nationalsozialismus), more commonly known as Nazism (/ˈnɑːtsɪzəm, ˈnæ-/), is the ideology and practice associated with the 20th-century German Nazi Party and Nazi state, as well as other far-right groups. Usually characterized as a form of fascism that incorporates scientific racism and antisemitism, Nazism developed out of the influences of Pan-Germanism, the Völkisch German nationalist movement and the anti-communist Freikorps paramilitary groups that emerged during the Weimar Republic after German defeat in World War I. Nazism subscribed to theories of racial hierarchy and Social Darwinism, identifying Germans as part of what Nazis regarded as an Aryan or Nordic master race. It aimed to overcome social divisions and create a homogeneous society, unified on the basis of \"racial purity\" (Volksgemeinschaft). The Nazis aimed to unite all Germans living in historically German territory, as well as gain additional lands for German expansion under the doctrine of Lebensraum, while excluding those deemed either to be community aliens or belonging to an \"inferior\" race. The term \"National Socialism\" arose out of attempts to create a nationalist redefinition of \"socialism\", as an alternative to both international socialism and free market capitalism. Nazism rejected the Marxist concept of class struggle, opposed cosmopolitan internationalism, and sought to convince all parts of a new German society to subordinate their personal interests to the \"common good\" and to accept the priority of political interests in economic organisation. The Nazi Party was founded as the Pan-German nationalist and antisemitic German Workers' Party on 5 January 1919. By the early 1920s, Adolf Hitler assumed control of the organization and renamed it the National Socialist German Workers' Party (Nationalsozialistische Deutsche Arbeiterpartei, NSDAP) to broaden its appeal. The National Socialist Program, adopted in 1920, called for a united Greater Germany that would deny citizenship to Jews or those of Jewish descent, while also supporting land reform and the nationalization of some industries. In Mein Kampf, written in 1924, Hitler outlined the antisemitism and anti-communism at the heart of his political philosophy, as well as his disdain for parliamentary democracy and his belief in Germany’s right to territorial expansion. In 1933, with the support of traditional conservative nationalists, Hitler was appointed Chancellor of Germany and the Nazis gradually established a one-party state, under which Jews, political opponents and other \"undesirable\" elements were marginalized, with several millions eventually imprisoned and killed. Hitler purged the party’s more socially and economically radical factions in the mid-1934 Night of the Long Knives and, after the death of President Hindenburg, political power was concentrated in his hands, as Führer or \"leader\". Following the Holocaust and German defeat in World War II, only a few fringe racist groups, usually referred to as neo-Nazis, still describe themselves as following National Socialism. <a href=\"#_dbpedia_2017\">(DBpedia, 2017)</a>"@en ;
    skos:inScheme cwrc:PoliticalAffiliation ;
    prov:derivedFrom dbpedia:Nazism .

cwrc:neo-Conservatism
    void:inDataset cwrc:datasetdefinition ;
    a cwrc:PoliticalAffiliation, skos:Concept ;
    rdfs:comment "La description de ce terme est basée sur celle de DBPedia."@fr, "The description for this term is indebted to DBpedia."@en ;
    rdfs:isDefinedBy <http://sparql.cwrc.ca/ontologies/cwrc-2017-08-03> ;
    rdfs:label "Néo-conservatisme"@fr, "neo-conservatism"@en ;
    skos:broaderTransitive cwrc:conservatism ;
    skos:definition "Le néo-conservatisme ou néoconservatisme est un courant de pensée politique d'origine américaine apparu à la fin du XXe siècle. Il s'agit d'une conception qui a émergé aux États-Unis par opposition au relativisme culturel et à la contre-culture de la Nouvelle gauche (« New Left ») des années 1960. Cette philosophie a influencé les politiques menées par George W. Bush, signifiant un réalignement de la politique américaine, et le passage de quelques libéraux sociaux à la droite du spectre politique, d'où le terme qui fait référence aux « nouveaux » conservateurs. À l'origine, le terme néo-conservateur était utilisé pour critiquer les sociaux-libéraux qui sont passés du côté du Parti républicain. Michael Harrington, un social-démocrate, a forgé l'usage du mot néo-conservateur en 1973 dans Dissent, un magazine sur les politiques de protection sociale. Selon E. J. Dionne, le néo-conservatisme est né sur le principe que le social-libéralisme a échoué. Le premier théoricien néo-conservateur à avoir adopté ce mot et qui est considéré comme le fondateur de cette idéologie est Irving Kristol et père de William Kristol, fondateur du think-tank « néo-conservateur » Project for the New American Century. Irving Kristol a été un militant trotskyste actif pendant sa jeunesse et a exposé ses vues néoconservatrices en 1979 dans l'article Confessions of a True, Self-Confessed 'Neoconservative'. Les idées de Kristol sont influentes depuis les années 1950 quand il a cofondé et édité le magazine Encounter. Un autre idéologue de ce mouvement était Norman Podhoretz, éditeur au magazine Commentary de 1960 à 1995. En 1982, Podhoretz se désignait déjà comme un néo-conservateur dans un article du New York Times Magazine intitulé The Neoconservative Anguish over Reagan's Foreign Policy. La doctrine Reagan était considérée comme anticommuniste et en opposition avec l'influence mondiale de l'URSS. Elle était au centre de la politique étrangère américaine jusqu'à la fin de la Guerre froide, un peu avant que Clinton ne devienne président. L'influence néo-conservatrice sur la politique étrangère américaine sera un peu plus tard au premier plan de la doctrine Bush. Les journaux néo-conservateurs prééminents sont Commentary et The Weekly Standard. Il existe aussi des cercles de réflexion néo-conservateurs sur la politique étrangère dont notamment American Enterprise Institute (AEI), le The Heritage Foundation, JINSA (Jewish Institute for National Security Affairs) et enfin Project for the New American Century (PNAC). <a href=\"#_dbpedia_2017\">(DBpedia, 2017)</a>"@fr, "Neoconservatism (commonly shortened to neocon) is a political movement born in the United States during the 1960s among conservative leaning Democrats who became disenchanted with the party's foreign policy. Many of its adherents became politically famous during the Republican presidential administrations of the 1970s, 1980s, 1990s and 2000s. Neoconservatives peaked in influence during the administration of George W. Bush, when they played a major role in promoting and planning the 2003 invasion of Iraq. Prominent neoconservatives in the George W. Bush administration included Paul Wolfowitz, John Bolton, Elliott Abrams, Richard Perle and Paul Bremer. Senior officials Vice President Dick Cheney and Secretary of Defense Donald Rumsfeld, while not identifying as neoconservatives, listened closely to neoconservative advisers regarding foreign policy, especially the defense of Israel and the promotion of democracy in the Middle East. The term \"neoconservative\" refers to those who made the ideological journey from the anti-Stalinist Left to the camp of American conservatism. Neoconservatives typically advocate the promotion of democracy and promotion of American national interest in international affairs, including by means of military force and are known for espousing disdain for communism and for political radicalism. The movement had its intellectual roots in the Jewish monthly review magazine Commentary, published by the American Jewish Committee. They spoke out against the New Left and in that way helped define the movement. C. Bradley Thompson, a professor at Clemson University, claims that most influential neoconservatives refer explicitly to the theoretical ideas in the philosophy of Leo Strauss (1899–1973),though in doing so they may draw upon meaning that Strauss himself did not endorse. <a href=\"#_dbpedia_2017\">(DBpedia, 2017)</a>"@en ;
    skos:inScheme cwrc:PoliticalAffiliation ;
    prov:derivedFrom dbpedia:Neoconservatism .

cwrc:neo-thomism
    void:inDataset cwrc:datasetdefinition ;
    a cwrc:Religion, skos:Concept ;
    rdfs:comment "La description de ce terme est basée sur celle de DBPedia."@fr ;
    rdfs:isDefinedBy <http://sparql.cwrc.ca/ontologies/cwrc-2017-08-03> ;
    rdfs:label "Neo-thomism"@en, "néothomisme"@fr ;
    skos:broaderTransitive cwrc:catholicChurch ;
    skos:definition "\"Courant de pensée philosophico-théologique de type thomiste, développé à partir XIXe siècle pour répondre aux objections posées au christianisme catholique par la modernité.\"<a href=\"#_dbpedia_2017\">(DBpedia, 2017)</a>"@fr, "Neo-Scholasticism (also known as neo-scholastic Thomism or neo-Thomism because of the great influence of the writings of St. Thomas Aquinas on the movement), is a revival and development of medieval scholasticism in Roman Catholic theology and philosophy which began in the second half of the 19th century.<a href=\"#_dbpedia_2017\">(DBpedia, 2017)</a>"@en ;
    skos:inScheme cwrc:Religion ;
    prov:derivedFrom dbpedia:Neo-Scholasticism .

cwrc:newDealer
    void:inDataset cwrc:datasetdefinition ;
    a cwrc:PoliticalAffiliation, skos:Concept ;
    rdfs:comment "The description for this term is indebted to DBpedia."@en ;
    rdfs:isDefinedBy <http://sparql.cwrc.ca/ontologies/cwrc-2017-08-03> ;
    rdfs:label ""@fr, "new dealer"@en ;
    skos:definition ""@fr, "Supporter of New Deal policies. See <a href=\"https://en.wikipedia.org/wiki/New_Deal\">https://en.wikipedia.org/wiki/New_Deal</a>"@en ;
    skos:inScheme cwrc:PoliticalAffiliation ;
    prov:derivedFrom dbpedia:New_Deal .

cwrc:nihilism
    void:inDataset cwrc:datasetdefinition ;
    a cwrc:PoliticalAffiliation, skos:Concept ;
    rdf:value "nihilist" ;
    rdfs:comment "La description de ce terme est basée sur celle de DBPedia."@fr, "The description for this term is indebted to DBpedia."@en ;
    rdfs:isDefinedBy <http://sparql.cwrc.ca/ontologies/cwrc-2017-08-03> ;
    rdfs:label "Nihilisme"@fr, "nihilism"@en ;
    skos:definition "Le nihilisme (du latin nihil, « rien ») est une doctrine ou attitude, fondée sur la négation de toutes valeurs, croyances ou réalités substantielles. Souvent associé au pessimisme ou au scepticisme radical, le nihilisme nie ou émet des doutes, quant aux causalités, intentionnalités et normativités de l'existence. Cette notion est applicable à différents domaines : politique, littéraire, religieux et philosophique. Un mouvement révolutionnaire nihiliste et anarchiste apparut en Russie dans la seconde moitié du XIXe siècle. Il rejetait l'autorité de l'État, de l'Église orthodoxe et de la famille et revendiquait une organisation de la société basée sur le rationalisme et le matérialisme. Il aboutit vers 1870 au terrorisme radical. <a href=\"#_dbpedia_2017\">(DBpedia, 2017)</a>"@fr, "Nihilism is a philosophical doctrine that suggests the lack of belief in one or more reputedly meaningful aspects of life. Most commonly, nihilism is presented in the form of existential nihilism, which argues that life is without objective meaning, purpose, or intrinsic value. Moral nihilists assert that morality does not inherently exist, and that any established moral values are abstractly contrived. Nihilism can also take epistemological, ontological, or metaphysical forms, meaning respectively that, in some aspect, knowledge is not possible, or that reality does not actually exist. The term is sometimes used in association with anomie to explain the general mood of despair at a perceived pointlessness of existence that one may develop upon realising there are no necessary norms, rules, or laws. Movements such as Futurism and deconstruction, among others, have been identified by commentators as \"nihilistic\". Nihilism is also a characteristic that has been ascribed to time periods: for example, Jean Baudrillard and others have called postmodernity a nihilistic epoch, and some Christian theologians and figures of religious authority have asserted that postmodernity and many aspects of modernity represent a rejection of theism, and that such rejection of their theistic doctrine entails nihilism. <a href=\"#_dbpedia_2017\">(DBpedia, 2017)</a>"@en ;
    skos:inScheme cwrc:PoliticalAffiliation ;
    prov:derivedFrom dbpedia:Nihilism .

cwrc:nobility
    void:inDataset cwrc:datasetdefinition ;
    a cwrc:SocialClass, skos:Concept ;
    rdfs:isDefinedBy <http://sparql.cwrc.ca/ontologies/cwrc-2017-08-03> ;
    rdfs:label "nobility"@en, "noblesse"@fr ;
    skos:definition ""@fr, "This group refers to those holding a title or of close family relation to someone holding a title (such as Lady Mary Wortley Montagu, Lord Byron, or Nancy Mitford)."@en ;
    skos:inScheme cwrc:SocialClass .

cwrc:nonjurorsMovement
    void:inDataset cwrc:datasetdefinition ;
    a cwrc:PoliticalAffiliation, skos:Concept ;
    rdfs:comment "The description for this term is indebted to DBpedia."@en ;
    rdfs:isDefinedBy <http://sparql.cwrc.ca/ontologies/cwrc-2017-08-03> ;
    rdfs:label ""@fr, "nonjurors movement"@en ;
    skos:broaderTransitive cwrc:jacobitism ;
    skos:definition ""@fr, "The nonjuring schism was a split in the Anglican churches of England, Scotland and Ireland in the aftermath of the Glorious Revolution of 1688, over whether William III and Mary II could legally be recognised as sovereigns. The word \"nonjuring\" means \"not swearing [an oath]\", from the Latin word iuro or juro meaning \"to swear an oath\". Many of the Anglican clergy felt legally bound by their previous oaths of allegiance to James II and, though they could accept William as regent, they could not accept him as king. It was not necessarily a split on matters of religious doctrine, but more of a political issue and a matter of conscience, though most of the nonjurors were high church Anglicans. Thus, latitudinarian Anglicans were handed control of the Church of England, while Presbyterians took control of the Church of Scotland. The nonjurors thus were nominally Jacobite, although they generally did not actively support the Jacobite rebellions in 1715 or 1745. <a href=\"#_dbpedia_2017\">(DBpedia, 2017)</a>"@en ;
    skos:inScheme cwrc:PoliticalAffiliation ;
    prov:derivedFrom dbpedia:Nonjuring_schism .

cwrc:occultism
    void:inDataset cwrc:datasetdefinition ;
    a cwrc:Religion, skos:Concept ;
    rdfs:isDefinedBy <http://sparql.cwrc.ca/ontologies/cwrc-2017-08-03> ;
    rdfs:label "Occultism/Theosophism"@en, "occultisme"@fr ;
    skos:definition ""@fr, "Any religious or philosophic ideology based on mystical insight into the nature of God and/or divine truth. This insight is attained only through direct experience of the divine. The term is sometimes used to specifically refer to the principles of the Theosophical Society founded in New York in 1875 by Madame Blavatsky and H. S. Olcott which incorporated aspects of Buddhism and Brahmanism.<a href=\"#_getty_2017\">(Getty, 2017)</a>"@en ;
    skos:inScheme cwrc:Religion ;
    prov:derivedFrom <http://vocab.getty.edu/aat/300056000> .

cwrc:originalOrlandoAuthor
    void:inDataset cwrc:datasetdefinition ;
    a skos:Concept, foaf:Group ;
    rdfs:isDefinedBy <http://sparql.cwrc.ca/ontologies/cwrc-2017-08-03> ;
    rdfs:label "Les membres du projet Orlando"@fr, "Members of the Orlando Project"@en ;
    skos:definition "La collection de tous les auteurs du Projet Orlando."@fr, "The collection of all persons having written entries for The Orlando Project."@en ;
    foaf:homepage <http://orlando.cambridge.org/public/svDocumentation?formname=t&d_id=CREDITSANDACKNOWLEDGEMENTS> ;
    foaf:name "Les membres du projet Orlando"@fr, "Members of the Orlando Project."@en .

cwrc:pacifism
    void:inDataset cwrc:datasetdefinition ;
    a cwrc:PoliticalAffiliation, skos:Concept ;
    rdf:value "pacifist", "pacifist supporter", "peace movement" ;
    rdfs:comment "La description de ce terme est basée sur celle de DBPedia."@fr, "The description for this term is indebted to DBpedia."@en ;
    rdfs:isDefinedBy <http://sparql.cwrc.ca/ontologies/cwrc-2017-08-03> ;
    rdfs:label "Pacifisme"@fr, "pacifism"@en ;
    skos:definition "Le pacifisme possède deux acceptions possibles incluant l'action des partisans de la paix, ou une doctrine de la non-violence. Bien que reliés, les deux concepts se distinguent du point de vue de la théorie et de la pratique. Le pacifisme est la doctrine et l'action des partisans de la paix ou du rétablissement de la paix. Les socialistes d'avant 1914 (Jean Jaurès), les Zimmerwaldiens durant la Première Guerre mondiale, les opposants aux guerres coloniales ou les partisans de la paix professent un pacifisme qui n'est pas toujours assimilable à la non-violence. La vision du pacifisme associé à une personne refusant le recours à toutes formes de violence est par contre beaucoup plus répandue. La doctrine de la non-violence voit de nombreux courants philosophiques bannir le recours à toute forme de violence en vertu d'un pacifisme radical. Vision portée par de nombreux mouvements et courants de pensée à vocation générale (courants de pensée humaniste, plusieurs tendances inspirées de l'hindouisme, courants chrétiens, etc.). <a href=\"#_dbpedia_2017\">(DBpedia, 2017)</a>"@fr, "Pacifism is opposition to war, militarism, or violence. The word pacifism was coined by the French peace campaigner Émile Arnaud (1864–1921) and adopted by other peace activists at the tenth Universal Peace Congress in Glasgow in 1901. A related term is ahimsa (to do no harm), which is a core philosophy in Buddhism, Jainism, and Hinduism. While modern connotations are recent, having been explicated since the 19th century, ancient references abound. In Christianity, Jesus Christ's injunction to \"love your enemies\" and asking for forgiveness for his crucifiers \"for they know not what they do\" have been interpreted as calling for pacifism. In modern times, interest was revived by Leo Tolstoy in his late works, particularly in The Kingdom of God Is Within You. Mohandas Gandhi (1869–1948) propounded the practice of steadfast nonviolent opposition which he called \"satyagraha\", instrumental in its role in the Indian Independence Movement. Its effectiveness served as inspiration to Martin Luther King Jr., James Lawson, James Bevel, Thich Nhat Hanh and many others in the Civil Rights Movement. Pacifism was widely associated with the much publicized image of Tiananmen Square Protests of 1989 with the \"Tank Man\", where one protester stood in nonviolent opposition to a column of tanks. <a href=\"#_dbpedia_2017\">(DBpedia, 2017)</a>"@en ;
    skos:inScheme cwrc:PoliticalAffiliation ;
    prov:derivedFrom dbpedia:Pacifism .

cwrc:pagan
    dcterms:isReplacedBy cwrc:paganism ;
    void:inDataset cwrc:datasetdefinition ;
    a skos:Concept ;
    rdfs:comment "Deprecated in favour of instance #paganism."@en, "Désapprouver en faveur de l'instance #paganism."@fr ;
    rdfs:isDefinedBy <http://sparql.cwrc.ca/ontologies/cwrc-2017-08-03> ;
    rdfs:label "Pagan"@en, "païen (ou payen)"@fr ;
    owl:deprecated true ;
    vs:term_status "deprecated"@en ;
    skos:broaderTransitive cwrc:occultism ;
    skos:definition "Paganism is a term that developed among the Christian community of southern Europe during late antiquity to describe religions other than their own, Judaism, or Islam–the three Abrahamic religions. Throughout Christendom, it continued to be used, typically in a derogatory sense. In the 19th century, it was re-adopted as a self-descriptor by members of various artistic groups inspired by the ancient world. In the 20th century, it came to be applied as a self-description by practitioners of contemporary pagan, or neo-pagan, religious movements. There has been much scholarly argument as to the origin of the term paganism. Paganism has also been understood by some[who?] to include any non-Abrahamic religions, but this is generally[who?] seen as insulting by adherents of those religions. While paganism is often considered to exclude monotheism and to express a worldview that is pantheistic, polytheistic, or animistic, there are some monotheistic pagans. Once monotheistic religions, such as Christianity and Islam, started to become more prominent (in processes known as Christianization and Islamization), names to encompass polytheistic worshipers started to develop; some of these include Hellene, pagan, and heathen, and at times these names were used as slurs. Modern knowledge of old pagan religions comes from several sources, including: anthropological field research records, the evidence of archaeological artifacts, and the historical accounts of ancient writers regarding cultures known to the classical world. Before the rise of monotheistic religions, most people practiced some type of polytheism. Many of these religions started to die out, and eventually they became extinct. In some cases, elements of polytheistic belief systems continued to exist in folklore. Paganism would later be studied during the Renaissance and Romantic era. Forms of these religions, influenced by various historical pagan beliefs of pre-modern Europe, exist today and are known as contemporary or modern paganism, also referred to as Neo-paganism. <a href=\"#_dbpedia_2017\">(DBpedia, 2017)</a>"@en, "Paganisme est un terme générique employé depuis le VIe siècle par des chrétiens pour désigner la religion de ceux qui ne sont ni chrétiens, ni juifs, ni musulmans. Il remonte au latin paganus (païen). Au VIe siècle, ce mot pouvait servir à désigner les habitants des campagnes par opposition à ceux des villes ou bien les civils par opposition aux militaires. D'abord employé comme sobriquet populaire par des chrétiens pour désigner ceux qui ne sont pas baptisés, le terme a ensuite été adopté dans la littérature chrétienne. Même s'il y désigne toujours ceux qui ne sont pas chrétiens, son acception y est cependant ambiguë. Il est parfois employé de façon péjorative pour désigner ceux qui sont tenus pour être des ignorants, parfois de façon neutre pour désigner les philosophes grecs, parfois encore pour désigner des chrétiens jugés mal convertis ou tièdes dans leur foi. À partir de 370, des lois impériales regroupées au Ve siècle dans le code théodosien emploient le terme paganus pour désigner ceux qui pratiquent la magie, ceux qui sont considérés comme superstitieux ou dans l'erreur. Le terme a depuis conservé une connotation péjorative. De nombreux Pères de l'Église ayant écrit « contre les païens », le paganisme a eu une première existence sous forme de fiction littéraire, comme s'il s'agissait de la religion de ceux qui ne sont pas chrétiens. Le paganisme tel qu'il a été exposé par les Pères de l'Église n'était cependant pas à proprement parler une religion, il s'agit plutôt de l'ensemble sans homogénéité des positions philosophiques et des croyances rejetées par les Pères de l'Église. Le paganisme est ainsi, dans l'antiquité tardive, une attitude combattue par des chrétiens puis par les autorités, mais elle n'est revendiquée par personne. C'est surtout à l'époque moderne, avec l'essor de l'histoire des religions que le paganisme commence à être perçu et étudié comme une religion parmi d'autres. Le paganisme peut aujourd'hui être revendiqué sous forme de néo-paganisme, ou bien comme une position philosophique tel que l'a fait Marc Augé dans Le génie du paganisme. Le mot paganus n'a pas son correspondant chez les écrivains chrétiens de langue grecque qui utilisent le terme moins péjoratif de « nations » ou « religions nationales » (ethnikoï) (décalque de l'hébreu). <a href=\"#_dbpedia_2017\">(DBpedia, 2017)</a>"@fr ;
    skos:inScheme cwrc:Religion .

cwrc:paganism
    void:inDataset cwrc:datasetdefinition ;
    a cwrc:Religion, skos:Concept ;
    rdfs:isDefinedBy <http://sparql.cwrc.ca/ontologies/cwrc-2017-08-03> ;
    rdfs:label "Paganism"@en, "Paganisme"@fr ;
    skos:definition "Paganism is a term that developed among the Christian community of southern Europe during late antiquity to describe religions other than their own, Judaism, or Islam–the three Abrahamic religions. Throughout Christendom, it continued to be used, typically in a derogatory sense. In the 19th century, it was re-adopted as a self-descriptor by members of various artistic groups inspired by the ancient world. In the 20th century, it came to be applied as a self-description by practitioners of contemporary pagan, or neo-pagan, religious movements. There has been much scholarly argument as to the origin of the term paganism. Paganism has also been understood by some[who?] to include any non-Abrahamic religions, but this is generally[who?] seen as insulting by adherents of those religions. While paganism is often considered to exclude monotheism and to express a worldview that is pantheistic, polytheistic, or animistic, there are some monotheistic pagans. Once monotheistic religions, such as Christianity and Islam, started to become more prominent (in processes known as Christianization and Islamization), names to encompass polytheistic worshipers started to develop; some of these include Hellene, pagan, and heathen, and at times these names were used as slurs. Modern knowledge of old pagan religions comes from several sources, including: anthropological field research records, the evidence of archaeological artifacts, and the historical accounts of ancient writers regarding cultures known to the classical world. Before the rise of monotheistic religions, most people practiced some type of polytheism. Many of these religions started to die out, and eventually they became extinct. In some cases, elements of polytheistic belief systems continued to exist in folklore. Paganism would later be studied during the Renaissance and Romantic era. Forms of these religions, influenced by various historical pagan beliefs of pre-modern Europe, exist today and are known as contemporary or modern paganism, also referred to as Neo-paganism. <a href=\"#_dbpedia_2017\">(DBpedia, 2017)</a>"@en, "Paganisme est un terme générique employé depuis le VIe siècle par des chrétiens pour désigner la religion de ceux qui ne sont ni chrétiens, ni juifs, ni musulmans. Il remonte au latin paganus (païen). Au VIe siècle, ce mot pouvait servir à désigner les habitants des campagnes par opposition à ceux des villes ou bien les civils par opposition aux militaires. D'abord employé comme sobriquet populaire par des chrétiens pour désigner ceux qui ne sont pas baptisés, le terme a ensuite été adopté dans la littérature chrétienne. Même s'il y désigne toujours ceux qui ne sont pas chrétiens, son acception y est cependant ambiguë. Il est parfois employé de façon péjorative pour désigner ceux qui sont tenus pour être des ignorants, parfois de façon neutre pour désigner les philosophes grecs, parfois encore pour désigner des chrétiens jugés mal convertis ou tièdes dans leur foi. À partir de 370, des lois impériales regroupées au Ve siècle dans le code théodosien emploient le terme paganus pour désigner ceux qui pratiquent la magie, ceux qui sont considérés comme superstitieux ou dans l'erreur. Le terme a depuis conservé une connotation péjorative. De nombreux Pères de l'Église ayant écrit « contre les païens », le paganisme a eu une première existence sous forme de fiction littéraire, comme s'il s'agissait de la religion de ceux qui ne sont pas chrétiens. Le paganisme tel qu'il a été exposé par les Pères de l'Église n'était cependant pas à proprement parler une religion, il s'agit plutôt de l'ensemble sans homogénéité des positions philosophiques et des croyances rejetées par les Pères de l'Église. Le paganisme est ainsi, dans l'antiquité tardive, une attitude combattue par des chrétiens puis par les autorités, mais elle n'est revendiquée par personne. C'est surtout à l'époque moderne, avec l'essor de l'histoire des religions que le paganisme commence à être perçu et étudié comme une religion parmi d'autres. Le paganisme peut aujourd'hui être revendiqué sous forme de néo-paganisme, ou bien comme une position philosophique tel que l'a fait Marc Augé dans Le génie du paganisme. Le mot paganus n'a pas son correspondant chez les écrivains chrétiens de langue grecque qui utilisent le terme moins péjoratif de « nations » ou « religions nationales » (ethnikoï) (décalque de l'hébreu). <a href=\"#_dbpedia_2017\">(DBpedia, 2017)</a>"@fr ;
    skos:inScheme cwrc:Religion .

cwrc:parentOf
    void:inDataset cwrc:datasetdefinition ;
    a owl:ObjectProperty ;
    rdf:value "PARENTS" ;
    rdfs:isDefinedBy <http://sparql.cwrc.ca/ontologies/cwrc-2017-08-03> ;
    rdfs:label "parent de"@fr, "parent of"@en ;
    rdfs:subPropertyOf cwrc:relativeOf .

cwrc:parliamentarianism
    void:inDataset cwrc:datasetdefinition ;
    a cwrc:PoliticalAffiliation, skos:Concept ;
    rdf:value "parliamentarian", "parliamentarianism", "pro-parliamentarian" ;
    rdfs:comment "The description for this term is indebted to DBpedia."@en ;
    rdfs:isDefinedBy <http://sparql.cwrc.ca/ontologies/cwrc-2017-08-03> ;
    rdfs:label ""@fr, "parliamentarianism"@en ;
    skos:definition ""@fr, "Advocacy for parliamentary systems in government. See: <a href=\"https://en.wikipedia.org/wiki/Parliamentary_system\">https://en.wikipedia.org/wiki/Parliamentary_system</a>"@en ;
    skos:inScheme cwrc:PoliticalAffiliation ;
    prov:derivedFrom dbpedia:Parliamentary_system .

cwrc:parliamentaryReform
    void:inDataset cwrc:datasetdefinition ;
    a cwrc:PoliticalAffiliation, skos:Concept ;
    rdf:value "parliamentary reformer", "pro-reform" ;
    rdfs:comment "The description for this term is indebted to DBpedia."@en ;
    rdfs:isDefinedBy <http://sparql.cwrc.ca/ontologies/cwrc-2017-08-03> ;
    rdfs:label ""@fr, "parliamentary reform"@en ;
    skos:definition ""@fr, "Support for reform of the parliamentary system of the United Kingdom. See <a href=\"https://en.wikipedia.org/wiki/Reform_Bills\">https://en.wikipedia.org/wiki/Reform_Bills</a>; <a href=\"https://en.wikipedia.org/wiki/Category:Representation_of_the_People_Acts\">https://en.wikipedia.org/wiki/Category:Representation_of_the_People_Acts</a>; <a href=\"https://en.wikipedia.org/wiki/Electoral_reform\">https://en.wikipedia.org/wiki/Electoral_reform</a>"@en ;
    skos:inScheme cwrc:PoliticalAffiliation ;
    prov:derivedFrom <http://dbpedia.org/resource/Category:Representation_of_the_People_Acts>, dbpedia:Electoral_reform, dbpedia:Reform_Bills .

cwrc:patriotism
    void:inDataset cwrc:datasetdefinition ;
    a cwrc:PoliticalAffiliation, skos:Concept ;
    rdf:value "patriot", "patriotic", "patriotism" ;
    rdfs:comment "La description de ce terme est basée sur celle de DBPedia."@fr, "The description for this term is indebted to DBpedia."@en ;
    rdfs:isDefinedBy <http://sparql.cwrc.ca/ontologies/cwrc-2017-08-03> ;
    rdfs:label "Patriotisme"@fr, "patriotism"@en ;
    skos:definition "Le patriotisme désigne le dévouement d'un individu envers son pays qu'il reconnait comme étant sa patrie. <a href=\"#_dbpedia_2017\">(DBpedia, 2017)</a>"@fr, "Patriotism is an emotional attachment to a nation which an individual recognizes as their homeland. This attachment, also known as national feeling or national pride, can be viewed in terms of different features relating to one's own nation, including ethnic, cultural, political or historical aspects. It encompasses a set of concepts closely related to those of nationalism. An excess of patriotism in the defense of a nation is called chauvinism; another related term is jingoism. The English term patriot is first attested in the Elizabethan era, via Middle French from Late Latin (6th century) patriota, meaning \"countryman\", ultimately from Greek  πατριώτης (patriōtēs), meaning \"from the same country\", from  πατρίς (patris), meaning \"fatherland\". The abstract noun patriotism appears in the early 18th century. <a href=\"#_dbpedia_2017\">(DBpedia, 2017)</a>"@en ;
    skos:inScheme cwrc:PoliticalAffiliation ;
    prov:derivedFrom dbpedia:Patriotism .

cwrc:personalProperty
    void:inDataset cwrc:datasetdefinition ;
    a owl:ObjectProperty ;
    rdfs:isDefinedBy <http://sparql.cwrc.ca/ontologies/cwrc-2017-08-03> ;
    rdfs:label "personal property"@en, "propriété de la personne"@fr ;
    skos:definition ""@en, ""@fr .

cwrc:personalPropertySelfDeclared
    dcterms:isReplacedBy cwrc:personalPropertySelfReported ;
    void:inDataset cwrc:datasetdefinition ;
    rdfs:comment "Deprecated in favour of instance #personalPropertySelfReported."@en, "Désapprouver en faveur de l'instance #personalPropertySelfReported."@fr ;
    rdfs:isDefinedBy <http://sparql.cwrc.ca/ontologies/cwrc-2017-08-03> ;
    rdfs:label "personal property (self reported)"@en, "propriété de la personne (autodéclarée)"@fr ;
    rdfs:subPropertyOf cwrc:personalProperty ;
    owl:deprecated true ;
    vs:term_status "deprecated"@en .

cwrc:personalPropertySelfReported
    void:inDataset cwrc:datasetdefinition ;
    a owl:ObjectProperty ;
    rdfs:isDefinedBy <http://sparql.cwrc.ca/ontologies/cwrc-2017-08-03> ;
    rdfs:label "personal property (self reported)"@en, "propriété de la personne (autodéclarée)"@fr ;
    rdfs:subPropertyOf cwrc:personalProperty .

cwrc:plymouthBrethren
    void:inDataset cwrc:datasetdefinition ;
    a cwrc:Religion, skos:Concept ;
    rdfs:comment "La description de ce terme est basée sur celle de DBPedia."@fr ;
    rdfs:isDefinedBy <http://sparql.cwrc.ca/ontologies/cwrc-2017-08-03> ;
    rdfs:label "Assemblées de Frères"@fr, "Frères de Schwarzenau"@fr, "Plymouth Brethren"@en ;
    skos:broaderTransitive cwrc:protestantism ;
    skos:definition "Le courant des Assemblées de Frères ou Plymouth Brethren ou encore Frères de Plymouth constitue l'une des branches du protestantisme évangélique. Ce mouvement est né à Dublin et en Grande-Bretagne vers 1830 et a connu une importante scission en 1848 qui a abouti à distinguer un courant « ouvert » d'une part, les « Open Brethren », et un courant « exclusif » d'autre part, appelé aussi « darbyste ». La branche la plus « étroite » a suivi John Nelson Darby et la branche plus ouverte des leaders comme George Müller et Henry Craik. Ces deux courants se sont développés dans le monde et notamment en France pour faire partie des cinq principales dénominations évangéliques sur quarante-trois significatives. <a href=\"#_dbpedia_2017\">(DBpedia, 2017)</a>"@fr, "The Plymouth Brethren are a conservative, low church, nonconformist, Evangelical Christian movement whose history can be traced to Dublin, Ireland in the late 1820s, originating from Anglicanism. Among other beliefs, the group emphasizes sola scriptura, the belief that the Bible is the supreme authority for church doctrine and practice over and above \"the [mere] tradition of men\" (Mark 7:8). Brethren generally see themselves not as a denomination but as a network, or even as a collection of overlapping networks, of like-minded independent churches. (The Brethren would generally prefer that their gatherings be referred to as \"assemblies\" rather than \"churches\" but, in the interests of simplicity, this article uses both terms interchangeably.) The movement refused for many years to take any denominational name to itself, a stance that some still maintain. The title \"The Brethren,\" however, is one that many of their number are comfortable with, in that the Bible designates all believers as \"brethren\". (\"[O]ne is your Master, even Christ; and all ye are brethren.\" Matthew 23:8)<a href=\"#_dbpedia_2017\">(DBpedia, 2017)</a>"@en ;
    skos:inScheme cwrc:Religion ;
    prov:derivedFrom dbpedia:Plymouth_Brethren .

cwrc:polishNationalism
    void:inDataset cwrc:datasetdefinition ;
    a cwrc:PoliticalAffiliation, skos:Concept ;
    rdf:value "Polish nationalism", "polish nationalist" ;
    rdfs:comment "The description for this term is indebted to DBpedia."@en ;
    rdfs:isDefinedBy <http://sparql.cwrc.ca/ontologies/cwrc-2017-08-03> ;
    rdfs:label ""@fr, "Polish nationalism"@en ;
    skos:broaderTransitive cwrc:nationalism ;
    skos:definition ""@fr, "Polish nationalism is the nationalism that asserts that Poles are a Polish nation, and promotes the cultural unity of Poles. Norman Davies, in the context of Polish nationalism, defined nationalism in general as \"a doctrine ... to create a nation by arousing people's awareness of their nationality, and to mobilize their feelings into a vehicle for political action\". The old Polish protonationalism of the Polish-Lithuanian Commonwealth based on the Polish-Lithuanian identity was multi-ethnic and multi-religious. The nationalist ideology developed soon after the Partitions was initially free of \"ethnic nationalism\" of any kind. It was a Romantic movement for the restoration of the Polish sovereign state. Polish Romantic nationalism was described by Maurycy Mochnacki as \"the essence of the nation\" no longer defined by borders but by ideas, feelings, and thoughts resulting from the past. The birth of modern nationalism under foreign rule coincided with the November Uprising of 1830 and the subsequent Spring of Nations. However, the defeat suffered by the Poles also broke the Polish revolutionary spirit. Many intellectuals turned to social Darwinism of Herbert Spencer, blaming the Romantic philosophy for the loss of their property, mass destruction, and ultimately the loss of the nation. With the advent of Positivism between 1860 and 1890 Polish nationalism became an elitist cause. Because the partitioning powers could not have identified themselves with the Polish nation, therefore the ideology became more restrictive in terms of ethnicity and religion. <a href=\"#_dbpedia_2017\">(DBpedia, 2017)</a>"@en ;
    skos:inScheme cwrc:PoliticalAffiliation ;
    prov:derivedFrom dbpedia:Polish_nationalism .

cwrc:poorAdvocacy
    void:inDataset cwrc:datasetdefinition ;
    a cwrc:PoliticalAffiliation, skos:Concept ;
    rdf:value "advocate for the poor" ;
    rdfs:comment "The description for this term is indebted to DBpedia."@en ;
    rdfs:isDefinedBy <http://sparql.cwrc.ca/ontologies/cwrc-2017-08-03> ;
    rdfs:label ""@fr, "poor advocacy"@en ;
    skos:definition ""@fr, "Advocacy for the poor."@en ;
    skos:inScheme cwrc:PoliticalAffiliation .

cwrc:poorLawReform
    void:inDataset cwrc:datasetdefinition ;
    a cwrc:PoliticalAffiliation, skos:Concept ;
    rdf:value "Poor Law reform" ;
    rdfs:comment "The description for this term is indebted to DBpedia."@en ;
    rdfs:isDefinedBy <http://sparql.cwrc.ca/ontologies/cwrc-2017-08-03> ;
    rdfs:label ""@fr, "poor law reform"@en ;
    skos:definition ""@fr, "From the reign of Elizabeth I until the passage of the Poor Law Amendment Act in 1834 relief of the poor in England was administered on the basis of a Poor Law enacted in 1601. From the start of the nineteenth century the basic concept of providing poor relief was criticised as misguided by leading political economists and in southern agricultural counties the burden of poor-rates was felt to be excessive (especially where poor-rates were used to supplement low wages (the 'allowance' or Speenhamland system)). Opposition to the Elizabethan Poor Law led to a Royal Commission on poor relief, which recommended that poor relief could not in the short term be abolished; however it should be curtailed, and administered on such terms that none but the desperate would claim it. Relief should only be administered in workhouses, whose inhabitants were to be confined, 'classified' (men, women, boys, girls) and segregated. The Poor Law Amendment Act allowed these changes to be implemented by a Poor Law Commission largely unaccountable to Parliament. The Act was passed by large majorities in Parliament, but the regime it was intended to bring about was denounced by its critics as (variously) un-Christian, un-English, unconstitutional, and impracticable for the great manufacturing districts of Northern England. The Act itself did not introduce the regime, but introduced a framework by which it might easily be brought in. Opposition to the New Poor Law strictly speaking was resistance to the introduction of the New Poor Law administrative framework; this was chiefly encountered in the industrial North in 1837–9 and overcome after a few riots by a judicious mixture of legal threats and deployment of the military. Opposition to the New Poor Law in the looser sense of resistance to (and criticism of) key features of the regime recommended by the Royal Commission persisted and eventually became orthodoxy: for example outdoor relief was never abolished in much of the industrial North. When a prominent West Riding opponent of the New Poor Law died in 1858, the Huddersfield Chronicle wrote \"..the controversy closed and English common sense has settled down on the poor-law question somewhat nearer to the views of Oastler and Pitkethly than those of their opponents.\" <a href=\"#_dbpedia_2017\">(DBpedia, 2017)</a>"@en ;
    skos:inScheme cwrc:PoliticalAffiliation ;
    prov:derivedFrom dbpedia:Opposition_to_the_English_Poor_Laws .

cwrc:presbyterianism
    void:inDataset cwrc:datasetdefinition ;
    a cwrc:Religion, skos:Concept ;
    rdfs:comment "La description de ce terme est basée sur celle de DBPedia."@fr, "The description for this term is indebted to the Getty Art & Architecture Thesaurus."@en ;
    rdfs:isDefinedBy <http://sparql.cwrc.ca/ontologies/cwrc-2017-08-03> ;
    rdfs:label "Prebyteriaan"@nl, "Presbiterianismo"@es, "Presbytarianisme"@fr, "Presbyterianism"@en, "Presbyterianisme"@nl, "chang lao tsung"@zh-latn-wadegile, "zhang lao zong"@zh-latn-pinyin-x-notone, "zhǎng lǎo zōng"@zh-latn-pinyin-x-hanyu, "長老制"@zh-hant, "長老宗"@zh-hant, "長老教會"@zh-hant ;
    skos:broaderTransitive cwrc:protestantism ;
    skos:definition "Een van de belangrijkste protestantse groeperingen die voortkwamen uit de 16de-eeuwse Reformatie. In het algemeen hebben moderne presbyteriaanse kerken hun oorsprong in de calvinistische kerken op de Britse eilanden, waarvan de Europese tegenhangers bekend zijn geworden onder de meer algemene naam 'gereformeerden'. De term 'presbyteriaans' verwijst ook naar een collegiaal type kerkbestuur onder leiding van pastors en leken die ouderlingen of presbyters worden genoemd. Strikt genomen maken alle presbyteriaanse kerken deel uit van de gereformeerde of calvinistische traditie, maar zijn niet alle gereformeerde kerken presbyteriaans in hun bestuursvorm. <a href=\"#_getty_2017\">(Getty, 2017)</a>"@nl, "Le presbytérianisme est une forme du protestantisme liée à l'Écosse. <a href=\"#_dbpedia_2017\">(DBpedia, 2017)</a>"@fr, "One of the main Protestant groups that arose out of the 16th-century Reformation. Generally speaking, modern Presbyterian churches trace their origins to the Calvinist churches of the British Isles, the European counterparts of which came to be known by the more inclusive name of Reformed. The term presbyterian also denotes a collegiate type of church government led by pastors and lay leaders called elders or presbyters. Strictly speaking, all Presbyterian churches are a part of the Reformed, or Calvinist, tradition, although not all Reformed churches are presbyterian in their form of government. <a href=\"#_getty_2017\">(Getty, 2017)</a>"@en, "Uno de los principales grupos protestantes que surgió de la Reforma del siglo XVI. Hablando en general, las Iglesias Presbiterianas modernas señalan sus orígenes en las iglesias calvinistas de las Islas Británicas, la contraparte Europea la que fue conocida por el nombre más global de \"Reformada\". El término presbiterianismo también denota un tipo colegiado de gobierno de iglesia liderado por el pastor y lideres laicos llamados ancianos o presbiteros. Estrictamente hablando, todas las iglesias presbiterianas son parte de la Iglesia .El término presbiterianismo también denota un tipo colegiado de gobierno de iglesia liderado por el pastor y lideres laicos llamados ancianos o presbiteros. Estrictamente hablando, todas las iglesias presbiterianas son parte de la Reforma o Calvinismo, tradición, aunque no todas las iglesias Reformadas son presbiterianas en su gubernamentalidad. <a href=\"#_getty_2017\">(Getty, 2017)</a>"@es, "自十六世紀宗教改革興起的主要新教團體的一派。一般說來，現代的長老教會可追溯至不列顛群島的喀爾文(Calvinis)教派，其在歐洲的對應教派則被稱為較具涵蓋性的歸正派(Reformed)。長老教會一詞，亦表示其管理方式如同大學，由稱作長老或教士的牧師及信徒領導。嚴格來說，所有長老教會皆為歸正派或喀爾文教派傳統的一部分，但並非所有歸正教會的管理方式皆如同長老教會一般。 <a href=\"#_getty_2017\">(Getty, 2017)</a>"@zh-hant ;
    skos:inScheme cwrc:Religion ;
    prov:derivedFrom dbpedia:Presbyterianism, <http://vocab.getty.edu/aat/300153854> .

cwrc:prisonReform
    void:inDataset cwrc:datasetdefinition ;
    a cwrc:PoliticalAffiliation, skos:Concept ;
    rdf:value "prison reform" ;
    rdfs:comment "The description for this term is indebted to DBpedia."@en ;
    rdfs:isDefinedBy <http://sparql.cwrc.ca/ontologies/cwrc-2017-08-03> ;
    rdfs:label ""@fr, "prison reform"@en ;
    skos:definition ""@fr, "Prison reform is the attempt to improve conditions inside prisons, establish a more effective penal system, or implement alternatives to incarceration. <a href=\"#_dbpedia_2017\">(DBpedia, 2017)</a>"@en ;
    skos:inScheme cwrc:PoliticalAffiliation ;
    prov:derivedFrom dbpedia:Prison_reform .

cwrc:pro-American
    void:inDataset cwrc:datasetdefinition ;
    a cwrc:PoliticalAffiliation, skos:Concept ;
    rdfs:comment "The description for this term is indebted to DBpedia."@en ;
    rdfs:isDefinedBy <http://sparql.cwrc.ca/ontologies/cwrc-2017-08-03> ;
    rdfs:label ""@fr, "pro-American"@en ;
    skos:definition ""@en, ""@fr ;
    skos:inScheme cwrc:PoliticalAffiliation ;
    skos:related cwrc:nationalism .

cwrc:pro-BoerWar
    void:inDataset cwrc:datasetdefinition ;
    a cwrc:PoliticalAffiliation, skos:Concept ;
    rdfs:comment "The description for this term is indebted to DBpedia."@en ;
    rdfs:isDefinedBy <http://sparql.cwrc.ca/ontologies/cwrc-2017-08-03> ;
    rdfs:label ""@fr, "pro-Boer War"@en ;
    skos:definition ""@fr, "Support of the First or Second Boer War. See <a href=\"https://en.wikipedia.org/wiki/First_Boer_War\">https://en.wikipedia.org/wiki/First_Boer_War</a>; <a href=\"https://en.wikipedia.org/wiki/Second_Boer_War\">https://en.wikipedia.org/wiki/Second_Boer_War</a>"@en ;
    skos:inScheme cwrc:PoliticalAffiliation ;
    prov:derivedFrom dbpedia:First_Boer_War, dbpedia:Second_Boer_War .

cwrc:pro-Catholicism
    void:inDataset cwrc:datasetdefinition ;
    a cwrc:PoliticalAffiliation, skos:Concept ;
    rdf:value "catholic", "non-compounder", "roman catholic" ;
    rdfs:comment "The description for this term is indebted to DBpedia."@en ;
    rdfs:isDefinedBy <http://sparql.cwrc.ca/ontologies/cwrc-2017-08-03> ;
    rdfs:label ""@fr, "pro-Catholicism"@en ;
    skos:definition ""@fr, "Favouring the political re-establishment of Catholicism as a component of the state or the extension of civil rights to Catholics. See <a href=\"https://en.wikipedia.org/wiki/Category:Catholicism-related_controversies\">https://en.wikipedia.org/wiki/Category:Catholicism-related_controversies</a>"@en ;
    skos:inScheme cwrc:PoliticalAffiliation ;
    prov:derivedFrom <http://dbpedia.org/resource/Category:Catholicism-related_controversies> .

cwrc:pro-Choice
    void:inDataset cwrc:datasetdefinition ;
    a cwrc:PoliticalAffiliation, skos:Concept ;
    rdfs:comment "La description de ce terme est basée sur celle de DBPedia."@fr, "The description for this term is indebted to DBpedia."@en ;
    rdfs:isDefinedBy <http://sparql.cwrc.ca/ontologies/cwrc-2017-08-03> ;
    rdfs:label "Mouvement pro-choix"@fr, "pro-choice"@en ;
    skos:definition " Pour l’article homonyme, voir ProChoix. Le mouvement pro-choix (en anglais pro-choice, c'est-à-dire « pour le choix ») désigne en Amérique du Nord l'ensemble des mouvements qui défendent l'idée politique et éthique que les femmes devraient avoir le contrôle de leur grossesse et de leur fertilité. S'y ajoutent notamment la liberté sexuelle, le droit au recours à l'avortement légal et encadré, et le libre choix de la contraception. On l'oppose dans ce contexte aux mouvements pro-vie, pour lesquels la liberté des femmes ne peut pas être utilisée comme argument pour contester le droit à la vie de l'embryon. Par extension, on utilise pro-choix pour évoquer tous les mouvements de défense des libertés individuelles, telles que la liberté de culte et l'euthanasie. Ce terme provient d'une justification des actes en fonction de leurs modalités d'exécution (choisi/imposé). <a href=\"#_dbpedia_2017\">(DBpedia, 2017)</a>"@fr, "Abortion-rights movements advocate for legal access to induced abortion services. The issue of induced abortion remains divisive in public life, with recurring arguments to liberalize or to restrict access to legal abortion services. Abortion-rights supporters themselves are frequently divided as to the types of abortion services that should be available and to the circumstances, for example different periods in the pregnancy such as late term abortions, in which access may be restricted. <a href=\"#_dbpedia_2017\">(DBpedia, 2017)</a>"@en ;
    skos:inScheme cwrc:PoliticalAffiliation ;
    prov:derivedFrom dbpedia:Abortion-rights_movements .

cwrc:pro-European
    void:inDataset cwrc:datasetdefinition ;
    a cwrc:PoliticalAffiliation, skos:Concept ;
    rdfs:comment "The description for this term is indebted to DBpedia."@en ;
    rdfs:isDefinedBy <http://sparql.cwrc.ca/ontologies/cwrc-2017-08-03> ;
    rdfs:label ""@fr, "pro-European"@en ;
    skos:definition ""@fr, "Supportive of the existence, policies, or influence of the European Union. See <a href=\"https://en.wikipedia.org/wiki/Pro-Europeanism\">https://en.wikipedia.org/wiki/Pro-Europeanism</a>"@en ;
    skos:inScheme cwrc:PoliticalAffiliation ;
    prov:derivedFrom dbpedia:Pro-Europeanism .

cwrc:pro-Slavery
    void:inDataset cwrc:datasetdefinition ;
    a cwrc:PoliticalAffiliation, skos:Concept ;
    rdfs:comment "The description for this term is indebted to DBpedia."@en ;
    rdfs:isDefinedBy <http://sparql.cwrc.ca/ontologies/cwrc-2017-08-03> ;
    rdfs:label ""@fr, "pro-slavery"@en ;
    skos:definition ""@fr, "Proslavery is an ideology that perceives slavery as a positive good. <a href=\"#_dbpedia_2017\">(DBpedia, 2017)</a>"@en ;
    skos:inScheme cwrc:PoliticalAffiliation ;
    prov:derivedFrom dbpedia:Proslavery .

cwrc:professional
    void:inDataset cwrc:datasetdefinition ;
    a cwrc:SocialClass, skos:Concept ;
    rdfs:isDefinedBy <http://sparql.cwrc.ca/ontologies/cwrc-2017-08-03> ;
    rdfs:label "professional"@en, "professionnel"@fr ;
    skos:definition ""@fr, "Includes doctors, lawyers, guild members, and those of high calling such as members of the clergy (Church of England). It implies social respect and intellectual requirements. Examples are Ann Hunter, who was married to a surgeon, and Virginia Woolf, daughter of an intellectual."@en ;
    skos:inScheme cwrc:SocialClass .

cwrc:propertyLawReform
    void:inDataset cwrc:datasetdefinition ;
    a cwrc:PoliticalAffiliation, skos:Concept ;
    rdf:value "illegitimacy reformer", "land reform", "land reformer", "property reform" ;
    rdfs:comment "The description for this term is indebted to DBpedia."@en ;
    rdfs:isDefinedBy <http://sparql.cwrc.ca/ontologies/cwrc-2017-08-03> ;
    rdfs:label ""@fr, "property law reform"@en ;
    skos:definition ""@fr, "Support for reform of the laws regarding real or personal property. See <a href=\"https://en.wikipedia.org/wiki/Property_law\">https://en.wikipedia.org/wiki/Property_law</a>"@en ;
    skos:inScheme cwrc:PoliticalAffiliation ;
    prov:derivedFrom dbpedia:Property_law .

cwrc:protestantRule
    void:inDataset cwrc:datasetdefinition ;
    a cwrc:PoliticalAffiliation, skos:Concept ;
    rdf:value "protestant", "protestantism" ;
    rdfs:comment "The description for this term is indebted to DBpedia."@en ;
    rdfs:isDefinedBy <http://sparql.cwrc.ca/ontologies/cwrc-2017-08-03> ;
    rdfs:label ""@fr, "Protestant rule"@en ;
    skos:definition ""@fr, "Support for protestant rule in the United Kingdom. See <a href=\"https://en.wikipedia.org/wiki/English_Reformation\">https://en.wikipedia.org/wiki/English_Reformation</a>"@en ;
    skos:inScheme cwrc:PoliticalAffiliation ;
    prov:derivedFrom dbpedia:English_Reformation .

cwrc:protestantism
    void:inDataset cwrc:datasetdefinition ;
    a cwrc:Religion, skos:Concept ;
    rdfs:comment "The description for this term is indebted to the Getty Art & Architecture Thesaurus."@en ;
    rdfs:isDefinedBy <http://sparql.cwrc.ca/ontologies/cwrc-2017-08-03> ;
    rdfs:label "Protestantism"@en, "hsin chiao"@zh-latn-wadegile, "protestant"@nl, "protestantisme"@fr, "protestantisme"@nl, "protestantismo"@es, "xin jiao"@zh-latn-pinyin-x-notone, "xīn jiāo"@zh-latn-pinyin-x-hanyu, "抗羅宗"@zh-hant, "新教"@zh-hant ;
    skos:broaderTransitive cwrc:christianity ;
    skos:definition "De algemene term voor typen christelijk geloof die zijn ontstaan tijdens de Reformatie. Hoewel de vroegste vormen van protestantisme werden beoefend door de volgelingen van Luther, Calvijn en Zwingli, wordt de term tegenwoordig gebruikt voor de meeste overtuigingen die niet rooms-katholiek of orthodox zijn. Protestanten willen dichter bij de geloofsstijl van de vroege kerk staan, die volgens hen in de katholieke praktijk overschaduwd is geraakt. De term is afkomstig van het woord 'protestari', wat niet alleen 'protesteren' betekent, maar ook 'belijden'. Enkele algemene kenmerken van het protestantisme zijn: rechtvaardiging door het geloof alleen, de berusting van alle gezag bij de Bijbel en de leer dat alle gelovigen zelf hun zonden aan God kunnen belijden, waarbij het aanhoren van de biecht niet alleen aan priesters is voorbehouden. <a href=\"#_getty_2017\">(Getty, 2017)</a>"@nl, "El término general para tipos de fe cristiana originadas a partir de la Reforma. Aunque las formas tempranas del protestantismo fueron aquellas que obedecían a Lutero, Calvino y Zwinglio, el término ahora incluye la mayoría de las denominaciones no Romanas o no Ortodoxas. El caracter común de los protestantes incluye la justificación de la fe por la fe, la autoridad de la sagrada escritura  y el sacerdocio de todos los fieles, por el que cada creyente puede oir la confesión de los pecados, no siendo exclusivo del clero. protestantes quieren estar cerca al estilo de fe de la primera Iglesia el cual sienten ha sido opacado en las prácticas católicas. El término deriva desde la palabra \"protestari\" que significa no sólo protestar sino que reconocer o confesar. Característica común. <a href=\"#_getty_2017\">(Getty, 2017)</a>"@es, "Le protestantisme est l'une des principales branches du christianisme avec le catholicisme et l'orthodoxie. Entendu largement, le protestantisme est l'ensemble des groupements « issus, directement ou non, de la Réforme et qui rejettent l'autorité du pape ». Selon cette perspective, le protestantisme englobe des mouvements variés allant des luthériens passant par les évangéliques, jusqu'aux quakers. <a href=\"#_getty_2017\">(DBpedia, 2017)</a>"@fr, "The general term for types of Christian faith originating from the Reformation. Although the early forms of Protestantism were those who followed Luther, Calvin, and Zwingli, the term now includes most non-Roman Catholic or non-Orthodox denominations. Protestants want to be closer to the style of faith of the early Church which they feel has been obscured in Catholic practices. The term derives from the word 'protestari' which means not only to protest but to avow or confess. Common characteristics of Protestantism include the justification by faith alone, the authority of scripture, and the priesthood of all believers, in which not only the clergy are able to hear the confession of sin. <a href=\"#_getty_2017\">(Getty, 2017)</a>"@en, "泛稱源自宗教改革的各式基督信仰。雖然早期的新教形式是指遵循路德(Luther)、喀爾文(Calvin)，以及茨溫利(Zwingli)的派別，但現在新教這個詞彙包含了大部分非羅馬天主教或非正教的派別。新教徒希望能更接近早期教會信仰，認為天主教將之變得晦澀難解。本詞彙衍生自”protestari”，不僅意指抗議，更要坦白或懺悔。新教的常見特色包括因純信而稱義、經典的權威性、信徒皆牧師，所以不是只有牧師才能聽取認罪懺悔。 <a href=\"#_getty_2017\">(Getty, 2017)</a>"@zh-hant ;
    skos:inScheme cwrc:Religion ;
    prov:derivedFrom dbpedia:Protestantism, <http://vocab.getty.edu/aat/300073735> .

cwrc:quakerism
    void:inDataset cwrc:datasetdefinition ;
    a cwrc:Religion, skos:Concept ;
    rdfs:comment "La description de ce terme est basée sur celle de DBPedia."@fr ;
    rdfs:isDefinedBy <http://sparql.cwrc.ca/ontologies/cwrc-2017-08-03> ;
    rdfs:label "Quakerism"@en, "quaker"@fr ;
    skos:broaderTransitive cwrc:dissenters, cwrc:protestantism ;
    skos:definition "Het Religieus Genootschap der Vrienden, beter bekend als quakers, verouderd Nederlands kwakers, vormt een groep ondogmatische gelovigen, die zijn wortels vindt in de christelijke traditie. Het leven en de overgeleverde uitspraken van Jezus vormen een belangrijke inspiratiebron. <a href=\"#_dbpedia_2017\">(DBpedia, 2017)</a>"@nl, "La Société religieuse des Amis est un mouvement religieux fondé en Angleterre au XVIIe siècle par des dissidents de l'Église anglicane. Les membres de ce mouvement sont communément connus sous le nom de quakers () mais ils se nomment entre eux « Amis » et « Amies ». Le mouvement est souvent nommé simplement Société des Amis et le surnom de « quaker » apparaît le plus souvent dans la dénomination officielle, sous la forme Société religieuse des Amis (quakers). Les historiens s'accordent à désigner George Fox comme le principal fondateur ou le plus important meneur des débuts du mouvement. Depuis sa création en Angleterre, le mouvement s'est d'abord répandu dans les pays de colonisation anglo-saxonne. Au XXe siècle, des missionnaires quakers ont propagé leur religion en Amérique latine et en Afrique. Aujourd'hui, les quakers déclarent être au nombre d'environ 350 000 dans le monde. La Société des Amis se différencie de la plupart des autres groupes issus du christianisme par l'absence de credo et de toute structure hiérarchique. Pour les quakers, la croyance religieuse appartient à la sphère personnelle et chacun est libre de ses convictions. Le concept de « lumière intérieure » (inner light) est cependant partagé par la plupart d'entre eux, quelle que soit la signification donnée à ces mots. De nombreux quakers reconnaissent le christianisme mais ne ressentent pas leur foi comme entrant dans les catégories chrétiennes traditionnelles. On trouve aujourd'hui dans la Société des Amis des pratiques très diverses, y compris un large courant évangélique. <a href=\"#_dbpedia_2017\">(DBpedia, 2017)</a>"@fr, "Quakers (or Friends) are members of a group of religious Christian movements which is known as the Religious Society of Friends in Europe, Australia, New Zealand and parts of North America; and known as the Friends Church in Africa, Asia, South America and parts of the US. The movements were originally, and are still predominantly based on Christianity. Members of the movements profess the priesthood of all believers, a doctrine derived from the First Epistle of Peter. They include those with evangelical, holiness, liberal, and traditional Quaker understandings of Christianity. To differing extents, the different movements that make up the Religious Society of Friends/Friends Church avoid creeds and hierarchical structures. In 2007, there were approximately 359,000 adult Quakers. <a href=\"#_dbpedia_2017\">(DBpedia, 2017)</a>"@en ;
    skos:inScheme cwrc:Religion ;
    prov:derivedFrom dbpedia:Quakers .

cwrc:quakers
    dcterms:isReplacedBy cwrc:quakerism ;
    void:inDataset cwrc:datasetdefinition ;
    a skos:Concept ;
    rdfs:comment "Deprecated in favour of instance #quakerism."@en, "Désapprouver en faveur de l'instance #quakerism."@fr, "La description de ce terme est basée sur celle de DBPedia."@fr ;
    rdfs:isDefinedBy <http://sparql.cwrc.ca/ontologies/cwrc-2017-08-03> ;
    rdfs:label "Quaker"@en, "quaker"@fr ;
    owl:deprecated true ;
    vs:term_status "deprecated"@en ;
    skos:broaderTransitive cwrc:churchOfEngland, cwrc:dissenters ;
    skos:definition "Het Religieus Genootschap der Vrienden, beter bekend als quakers, verouderd Nederlands kwakers, vormt een groep ondogmatische gelovigen, die zijn wortels vindt in de christelijke traditie. Het leven en de overgeleverde uitspraken van Jezus vormen een belangrijke inspiratiebron. <a href=\"#_dbpedia_2017\">(DBpedia, 2017)</a>"@nl, "La Société religieuse des Amis est un mouvement religieux fondé en Angleterre au XVIIe siècle par des dissidents de l'Église anglicane. Les membres de ce mouvement sont communément connus sous le nom de quakers () mais ils se nomment entre eux « Amis » et « Amies ». Le mouvement est souvent nommé simplement Société des Amis et le surnom de « quaker » apparaît le plus souvent dans la dénomination officielle, sous la forme Société religieuse des Amis (quakers). Les historiens s'accordent à désigner George Fox comme le principal fondateur ou le plus important meneur des débuts du mouvement. Depuis sa création en Angleterre, le mouvement s'est d'abord répandu dans les pays de colonisation anglo-saxonne. Au XXe siècle, des missionnaires quakers ont propagé leur religion en Amérique latine et en Afrique. Aujourd'hui, les quakers déclarent être au nombre d'environ 350 000 dans le monde. La Société des Amis se différencie de la plupart des autres groupes issus du christianisme par l'absence de credo et de toute structure hiérarchique. Pour les quakers, la croyance religieuse appartient à la sphère personnelle et chacun est libre de ses convictions. Le concept de « lumière intérieure » (inner light) est cependant partagé par la plupart d'entre eux, quelle que soit la signification donnée à ces mots. De nombreux quakers reconnaissent le christianisme mais ne ressentent pas leur foi comme entrant dans les catégories chrétiennes traditionnelles. On trouve aujourd'hui dans la Société des Amis des pratiques très diverses, y compris un large courant évangélique. <a href=\"#_dbpedia_2017\">(DBpedia, 2017)</a>"@fr, "Quakers (or Friends) are members of a group of religious Christian movements which is known as the Religious Society of Friends in Europe, Australia, New Zealand and parts of North America; and known as the Friends Church in Africa, Asia, South America and parts of the US. The movements were originally, and are still predominantly based on Christianity. Members of the movements profess the priesthood of all believers, a doctrine derived from the First Epistle of Peter. They include those with evangelical, holiness, liberal, and traditional Quaker understandings of Christianity. To differing extents, the different movements that make up the Religious Society of Friends/Friends Church avoid creeds and hierarchical structures. In 2007, there were approximately 359,000 adult Quakers. <a href=\"#_dbpedia_2017\">(DBpedia, 2017)</a>"@en ;
    skos:inScheme cwrc:Religion ;
    prov:derivedFrom dbpedia:Quakers .

cwrc:racialEquality
    void:inDataset cwrc:datasetdefinition ;
    a cwrc:PoliticalAffiliation, skos:Concept ;
    rdf:value "activist for racial equality", "race equality", "racial equality activist", "racial integration", "racial integrationist" ;
    rdfs:comment "The description for this term is indebted to DBpedia."@en ;
    rdfs:isDefinedBy <http://sparql.cwrc.ca/ontologies/cwrc-2017-08-03> ;
    rdfs:label ""@fr, "racial equality"@en ;
    skos:definition ""@fr, "Racial equality is an equal regard to all races. It can refer to a belief in biological equality of all human races, and it can also refer to social equality for people of different races. Racial equality is a stated goal of most current political movements. The divergence of any particular society from a state of racial equality is often contested by members of that society of different races. In today's society, there is more diversity and more integration among races. However, attaining equality has been difficult for African Americans, Asians, and Latinos, especially in schools. <a href=\"#_dbpedia_2017\">(DBpedia, 2017)</a>"@en ;
    skos:inScheme cwrc:PoliticalAffiliation ;
    prov:derivedFrom dbpedia:Racial_equality .

cwrc:racism
    void:inDataset cwrc:datasetdefinition ;
    a cwrc:PoliticalAffiliation, skos:Concept ;
    rdf:value "racist" ;
    rdfs:comment "La description de ce terme est basée sur celle de DBPedia."@fr, "The description for this term is indebted to DBpedia."@en ;
    rdfs:isDefinedBy <http://sparql.cwrc.ca/ontologies/cwrc-2017-08-03> ;
    rdfs:label "Racisme"@fr, "racism"@en ;
    skos:definition "Le racisme est une idéologie qui, partant du postulat de l'existence de races au sein de l'espèce humaine, considère que certaines catégories de personnes sont intrinsèquement supérieures à d'autres. Cette idéologie peut entraîner une attitude d'hostilité ou de sympathie systématique à l'égard d'une catégorie déterminée de personnes. Cette hostilité envers une autre appartenance culturelle et ethnique se traduit par des formes de xénophobie ou d'ethnocentrisme. Certaines formes d'expression du racisme, comme les injures racistes, la diffamation raciale, la discrimination, sont considérées comme des délits dans un certain nombre de pays. Les idéologies racistes ont servi de fondement à des doctrines politiques conduisant à pratiquer des discriminations raciales, des ségrégations ethniques et à commettre des injustices et des violences, allant jusqu'au génocide. Le Petit Larousse définit aussi le racisme comme « une attitude d'hostilité répétée voire systématique à l'égard d'une catégorie déterminée de personnes ». <a href=\"#_dbpedia_2017\">(DBpedia, 2017)</a>"@fr, "Racism is a product of the complex interaction in a given society of a race-based worldview with prejudice, stereotyping, and discrimination. Racism can be present in social actions, practices, or political systems (e.g., apartheid) that support the expression of prejudice or aversion in discriminatory practices. The ideology underlying racist practices often includes the idea that humans can be subdivided into distinct groups that are different in their social behavior and innate capacities and that can be ranked as inferior or superior. Racist ideology can become manifest in many aspects of social life. Associated social actions may include xenophobia, otherness, segregation, hierarchical ranking, supremacism, and related social phenomena. While race and ethnicity are considered to be separate in contemporary social science, the two terms have a long history of equivalence in popular usage and older social science literature. \"Ethnicity\" is often used in a sense close to one traditionally attributed to \"race\": the division of human groups based on qualities assumed to be essential or innate to the group (e.g. shared ancestry or shared behavior). Racism and racial discrimination are often used to describe discrimination on an ethnic or cultural basis, independent of whether these differences are described as racial. According to a United Nations convention, there is no distinction between the terms \"racial\" and \"ethnic\" discrimination. The UN convention further concludes that superiority based on racial differentiation is scientifically false, morally condemnable, socially unjust and dangerous, and there is no justification for racial discrimination, anywhere, in theory or in practice. Today, the use of the term \"racism\" does not easily fall under a single definition. It is usually found in, but usage is not limited to, law, the social and behavioral sciences, humanities, and popular culture. <a href=\"#_dbpedia_2017\">(DBpedia, 2017)</a>"@en ;
    skos:inScheme cwrc:PoliticalAffiliation ;
    prov:derivedFrom dbpedia:Racism .

cwrc:radicalism
    void:inDataset cwrc:datasetdefinition ;
    a cwrc:PoliticalAffiliation, skos:Concept ;
    rdf:value "radical" ;
    rdfs:comment "The description for this term is indebted to DBpedia."@en ;
    rdfs:isDefinedBy <http://sparql.cwrc.ca/ontologies/cwrc-2017-08-03> ;
    rdfs:label ""@fr, "radicalism"@en ;
    skos:definition ""@fr, "The term political radicalism (or simply, in political science, radicalism) denotes political principles focused on altering social structures through revolutionary means and changing value systems in fundamental ways. Derived from the Latin radix (root), the denotation of radical has changed since its eighteenth-century coinage to comprehend the entire political spectrum—yet retains the \"change at the root\" connotation fundamental to revolutionary societal change. Historically, radicalism has referred exclusively to the radical left (under the single category of far-left politics) and rarely incorporating far-right politics, though these may have revolutionary elements; the prominent exception is in the United States where some consider radicalism to include both political extremes of the radical left and the radical right. In traditional labels of the spectrum of political thought, the opposite of radical on the \"right\" of the political spectrum is termed reactionary. The nineteenth-century Cyclopaedia of Political Science (1881, 1889) reports that \"radicalism is characterized less by its principles than by the manner of their application\". Conservatives often used the term radical pejoratively, whereas contemporary left radicals used the term conservative derogatorily; thus contemporary denotations of radical, radicalism, and political radicalism comprehend far left (hard left, radical left), and far right (hard right, radical right). The Encyclopædia Britannica records the first political usage of radical as ascribed to the British Whig Party parliamentarian Charles James Fox, who, in 1797, proposed a \"radical reform\" of the electoral system, franchise to provide universal manhood suffrage, thereby, idiomatically establishing radical to denote supporters of the reformation of the British Parliament. Throughout the nineteenth century, the term was combined with political notions and doctrines, thus working class radicalism, middle class-, philosophic-, democratic- bourgeois-, Tory-, and plebeian radicalism. In the event, politically influential radical leaders give rise to their own trend of political radicalism, e.g. Spencean radicalism and Carlilean radicalism. Philosophically, the French political scientist Jean-Jacques Rousseau (1712–78), is the principal theoretician proposing political radicalism as feasible in republican political philosophy, viz the French Revolution (1789–99), and other modern revolutions—the antithesis to the liberalism of John Locke. <a href=\"#_dbpedia_2017\">(DBpedia, 2017)</a>"@en ;
    skos:inScheme cwrc:PoliticalAffiliation ;
    prov:derivedFrom dbpedia:Political_radicalism .

cwrc:rationalDissenter
    dcterms:isReplacedBy cwrc:dissentingChristianity ;
    void:inDataset cwrc:datasetdefinition ;
    a skos:Concept ;
    rdfs:comment "Deprecated in favour of instance #dissentingChristianity."@en, "Désapprouver en faveur de l'instance #dissentingChristianity."@fr ;
    rdfs:isDefinedBy <http://sparql.cwrc.ca/ontologies/cwrc-2017-08-03> ;
    rdfs:label ""@fr, "Rational Dissenter"@en ;
    owl:deprecated true ;
    vs:term_status "deprecated"@en ;
    skos:broaderTransitive cwrc:dissenters ;
    skos:definition ""@fr, "An 18th-century, group much \"closer to the Anglicanism of their day than other Dissenting sects; however, they believed that state religions impinged on the freedom of conscience. They were fiercely opposed to the hierarchical structure of the Established Church and the financial ties between it and the government.\"<a href=\"#_dbpedia_2017\">(DBpedia, 2017)</a>"@en ;
    skos:inScheme cwrc:Religion ;
    prov:derivedFrom <http://dbpedia.org/resource/English_Dissenters#Rational_Dissenters> .

cwrc:rationalism
    void:inDataset cwrc:datasetdefinition ;
    a cwrc:PoliticalAffiliation, skos:Concept ;
    rdf:value "rationalist" ;
    rdfs:comment "La description de ce terme est basée sur celle de DBPedia."@fr, "The description for this term is indebted to DBpedia."@en ;
    rdfs:isDefinedBy <http://sparql.cwrc.ca/ontologies/cwrc-2017-08-03> ;
    rdfs:label "Rationalisme"@fr, "rationalism"@en ;
    skos:definition "In epistemology, rationalism is the view that \"regards reason as the chief source and test of knowledge\" or \"any view appealing to reason as a source of knowledge or justification\". More formally, rationalism is defined as a methodology or a theory \"in which the criterion of the truth is not sensory but intellectual and deductive\". In an old controversy, rationalism was opposed to empiricism, where the rationalists believed that reality has an intrinsically logical structure. Because of this, the rationalists argued that certain truths exist and that the intellect can directly grasp these truths. That is to say, rationalists asserted that certain rational principles exist in logic, mathematics, ethics, and metaphysics that are so fundamentally true that denying them causes one to fall into contradiction. The rationalists had such a high confidence in reason that empirical proof and physical evidence were regarded as unnecessary to ascertain certain truths – in other words, \"there are significant ways in which our concepts and knowledge are gained independently of sense experience\". Different degrees of emphasis on this method or theory lead to a range of rationalist standpoints, from the moderate position \"that reason has precedence over other ways of acquiring knowledge\" to the more extreme position that reason is \"the unique path to knowledge\". Given a pre-modern understanding of reason, rationalism is identical to philosophy, the Socratic life of inquiry, or the zetetic (skeptical) clear interpretation of authority (open to the underlying or essential cause of things as they appear to our sense of certainty). In recent decades, Leo Strauss sought to revive \"Classical Political Rationalism\" as a discipline that understands the task of reasoning, not as foundational, but as maieutic. In politics, Rationalism, since the Enlightenment, historically emphasized a \"politics of reason\" centered upon rational choice, utilitarianism, secularism, and irreligion – the latter aspect's antitheism later ameliorated by utilitarian adoption of pluralistic rationalist methods practicable regardless of religious or irreligious ideology. In this regard, the philosopher John Cottingham noted how rationalism, a methodology, became socially conflated with atheism, a worldview: In the past, particularly in the 17th and 18th centuries, the term 'rationalist' was often used to refer to free thinkers of an anti-clerical and anti-religious outlook, and for a time the word acquired a distinctly pejorative force (thus in 1670 Sanderson spoke disparagingly of 'a mere rationalist, that is to say in plain English an atheist of the late edition...'). The use of the label 'rationalist' to characterize a world outlook which has no place for the supernatural is becoming less popular today; terms like 'humanist' or 'materialist' seem largely to have taken its place. But the old usage still survives. <a href=\"#_dbpedia_2017\">(DBpedia, 2017)</a>"@en, "Le rationalisme est la doctrine qui pose la raison discursive comme seule source possible de toute connaissance réelle. Autrement dit, le réel ne serait connaissable qu'en vertu d'une explication par la raison déterminante, suffisante et nécessaire. Ainsi, le rationalisme s'entend de toute doctrine qui attribue à la seule raison humaine la capacité de connaître et d'établir la vérité. Dans son acception classique, il s'agit de postuler que le raisonnement consiste à déterminer que certains effets résultent de certaines causes, uniquement à partir de principes logiques ; à la manière dont les théorèmes mathématiques résultent des hypothèses admises au départ. De plus, et en particulier, les principes logiques eux-mêmes utilisés dans le raisonnement ont été connus par déduction. <a href=\"#_dbpedia_2017\">(DBpedia, 2017)</a>"@fr ;
    skos:inScheme cwrc:PoliticalAffiliation ;
    prov:derivedFrom dbpedia:Rationalism .

cwrc:relativeOf
    void:inDataset cwrc:datasetdefinition ;
    a owl:ObjectProperty ;
    rdf:value "FAMILY" ;
    rdfs:isDefinedBy <http://sparql.cwrc.ca/ontologies/cwrc-2017-08-03> ;
    rdfs:label "liens de famille"@fr, "relative of"@en .

cwrc:republicanism
    void:inDataset cwrc:datasetdefinition ;
    a cwrc:PoliticalAffiliation, skos:Concept ;
    rdfs:comment "La description de ce terme est basée sur celle de DBPedia."@fr, "The description for this term is indebted to DBpedia."@en ;
    rdfs:isDefinedBy <http://sparql.cwrc.ca/ontologies/cwrc-2017-08-03> ;
    rdfs:label "Républicanisme"@fr, "republicanism"@en ;
    skos:definition "Le républicanisme est une idéologie politique selon laquelle l'objectif d'un État et le sens de son existence, comme de ses décisions, doivent être le bien commun (en latin, res publica : « la chose publique »). Selon le républicanisme, les détenteurs du pouvoir doivent être nommés par d'autres moyens que l'hérédité, c'est-à-dire être élus par le peuple ou par une partie de celui-ci. La notion de souveraineté populaire découle donc en partie de cette idéologie, mais elle ne lui est pas nécessairement attachée. La notion de « république » remonte à l'Antiquité grecque et romaine, et l'idéologie républicaine moderne a pris des formes légèrement différentes selon qu'elle a été développée aux États-Unis, en France ou en Irlande. À l'époque moderne, le républicanisme s'oppose à d'autres idéologies politiques telles que le monarchisme, l'autoritarisme ou le despotisme. Dans les débats contemporains, c'est principalement au libéralisme politique qu'il s'oppose. <a href=\"#_dbpedia_2017\">(DBpedia, 2017)</a>"@fr, "Republicanism is an ideology of being a citizen in a state as a republic under which the people hold popular sovereignty. Many countries are \"republics\" in the sense that they are not monarchies. However, this article covers only the ideology of republicanism. The word, republic, derives from the Latin, res publica, which referred to the system of government that emerged in the 6th century BCE following the expulsion of the kings from Rome by Lucius Junius Brutus and Collatinus. This form of government collapsed in the latter part of the 1st century BCE, giving way to what was a monarchy in form, if not in name. Republics revived subsequently, with, for example, Renaissance Florence or early modern Britain. The concept of a republic became a powerful force in Britain's North American colonies where it led to the American Revolution. In Europe it gained enormous influence through the French Revolution. <a href=\"#_dbpedia_2017\">(DBpedia, 2017)</a>"@en ;
    skos:inScheme cwrc:PoliticalAffiliation ;
    prov:derivedFrom dbpedia:Republicanism .

cwrc:revolutionaryPolitics
    void:inDataset cwrc:datasetdefinition ;
    a cwrc:PoliticalAffiliation, skos:Concept ;
    rdf:value "pro-revolutionary" ;
    rdfs:comment "The description for this term is indebted to DBpedia."@en ;
    rdfs:isDefinedBy <http://sparql.cwrc.ca/ontologies/cwrc-2017-08-03> ;
    rdfs:label ""@fr, "revolutionary"@en ;
    skos:definition ""@fr, "A revolutionary is a person who either actively participates in, or advocates revolution. Also, when used as an adjective, the term revolutionary refers to something that has a major, sudden impact on society or on some aspect of human endeavor. <a href=\"#_dbpedia_2017\">(DBpedia, 2017)</a>"@en ;
    skos:inScheme cwrc:PoliticalAffiliation ;
    prov:derivedFrom dbpedia:Revolutionary .

cwrc:rural-unskilled
    void:inDataset cwrc:datasetdefinition ;
    a cwrc:SocialClass, skos:Concept ;
    rdfs:isDefinedBy <http://sparql.cwrc.ca/ontologies/cwrc-2017-08-03> ;
    rdfs:label "rural unskilled"@en, "travailleurs ruraux non qualifiés"@fr ;
    skos:definition ""@fr, "This generally indicates farm laborers, mostly male in earlier periods, and includes migrant farm workers."@en ;
    skos:inScheme cwrc:SocialClass .

cwrc:sabbatarianism
    void:inDataset cwrc:datasetdefinition ;
    a cwrc:PoliticalAffiliation, skos:Concept ;
    rdfs:comment "The description for this term is indebted to DBpedia."@en ;
    rdfs:isDefinedBy <http://sparql.cwrc.ca/ontologies/cwrc-2017-08-03> ;
    rdfs:label ""@fr, "Sabbatarianism"@en ;
    skos:definition ""@fr, "Sabbatarianism is a movement within Protestantism whose proponents advocate that certain observances, specifically enumerated in a code of behavior or law, are required for Christians to properly observe the Sabbath or Sabbath principles. Its historical origins lie in Puritan Sabbatarianism, which delineated precepts for keeping Sunday holy in observance of Sabbath commandment principles. This observance of Sunday is the purest form of first-day Sabbatarianism, a movement which diminished and largely disappeared in the 18th century, though traces and influences remain today. Today, seventh-day Sabbatarianism is the most prominent type, a movement that generally embraces a literal reading of the Sabbath commandment that provides for both worship and rest on the seventh day of the week. Seventh-day Baptists leave most other Sabbath considerations of observance to individual conscience. The Seventh-day Adventist Church and Church of God (Seventh Day) have similar views, but maintain the original, scriptural duration as Friday sunset through Saturday sunset. Non-Sabbatarianism is the view opposing all Sabbatarianism, declaring Christians to be free of mandates to follow such specific observances. It upholds the principle in Christian church doctrine that the church is not bound by such law or code, but is free to set in place and time such observances as uphold Sabbath principles according to its doctrine: to establish a day of rest, or not, and to establish a day of worship, or not, whether on Saturday or on Sunday or on some other day. It includes all Catholics and Orthodox, and most Protestant denominations. <a href=\"#_dbpedia_2017\">(DBpedia, 2017)</a>"@en ;
    skos:inScheme cwrc:PoliticalAffiliation ;
    prov:derivedFrom dbpedia:Sabbatarianism .

cwrc:sanitaryMovement
    void:inDataset cwrc:datasetdefinition ;
    a cwrc:PoliticalAffiliation, skos:Concept ;
    rdfs:comment "The description for this term is indebted to DBpedia."@en ;
    rdfs:isDefinedBy <http://sparql.cwrc.ca/ontologies/cwrc-2017-08-03> ;
    rdfs:label ""@fr, "sanitary movement"@en ;
    skos:definition ""@fr, "Promotion of sanitary practices and conditions, often directed at the poor or the reform of urban sanitation, through charitable or political activities. See <a href=\"https://en.wikipedia.org/wiki/Sanitation#History\">https://en.wikipedia.org/wiki/Sanitation#History</a>; "@en ;
    skos:inScheme cwrc:PoliticalAffiliation ;
    skos:related cwrc:urbanReform ;
    prov:derivedFrom <http://dbpedia.org/resource/Sanitation#History> .

cwrc:scottishNationalism
    void:inDataset cwrc:datasetdefinition ;
    a cwrc:PoliticalAffiliation, skos:Concept ;
    rdf:value "scots nationalist", "scottish nationalist" ;
    rdfs:comment "La description de ce terme est basée sur celle de DBPedia."@fr, "The description for this term is indebted to DBpedia."@en ;
    rdfs:isDefinedBy <http://sparql.cwrc.ca/ontologies/cwrc-2017-08-03> ;
    rdfs:label "Nationalisme écossais"@fr, "Scottish nationalism"@en ;
    skos:broaderTransitive cwrc:nationalism ;
    skos:definition "Le nationalisme écossais moderne naît dans l'entre-deux-guerres, même si des éléments nationalistes sont depuis plusieurs siècles au cœur de l'identité écossaise. L'article examine le contexte historique et politique qui a vu l'éclosion d'un nationalisme politique en Écosse, depuis la création du SNP (Scottish National Party) en 1934 jusqu'à la mise en place d'un régime de dévolution à l'Écosse à partir de 1999. <a href=\"#_dbpedia_2017\">(DBpedia, 2017)</a>"@fr, "Scottish nationalism promotes the idea that the Scottish people form a cohesive nation and national identity and is closely linked to the cause of Scottish home rule and Scottish independence, the ideology of the Scottish National Party, the party forming the Scottish Government. It is often described as a form of civic nationalism rather than ethnic nationalism. The Acts of Union merged the independent kingdoms of Scotland and England into Great Britain in 1707, but a separate legal system and distinct Scottish institutions continued to exist. Linguistic independence was an important part of the twentieth century Scottish Renaissance, associated with the nationalist impetus provided by Hugh MacDiarmid. <a href=\"#_dbpedia_2017\">(DBpedia, 2017)</a>"@en ;
    skos:inScheme cwrc:PoliticalAffiliation ;
    prov:derivedFrom dbpedia:Scottish_nationalism .

cwrc:secularism
    void:inDataset cwrc:datasetdefinition ;
    a cwrc:PoliticalAffiliation, skos:Concept ;
    rdf:value "secularist" ;
    rdfs:comment "La description de ce terme est basée sur celle de DBPedia."@fr, "The description for this term is indebted to DBpedia."@en ;
    rdfs:isDefinedBy <http://sparql.cwrc.ca/ontologies/cwrc-2017-08-03> ;
    rdfs:label "Laïcité"@fr, "secularism"@en ;
    skos:definition "La laïcité ou le sécularisme est le « principe de séparation dans l'État de la société civile et de la société religieuse» et « d'impartialité ou de neutralité de l'État à l'égard des confessions religieuses». Le mot désigne par extension le caractère des « institutions, publiques ou privées, qui sont indépendantes du clergé et des églises». La laïcité s'oppose à la reconnaissance d'une religion d'État. Toutefois, le principe de séparation entre l'État et les religions peut trouver des applications différentes selon les pays. <a href=\"#_dbpedia_2017\">(DBpedia, 2017)</a>"@fr, "Secularism is the principle of the separation of government institutions and persons mandated to represent the state from religious institutions and religious dignitaries. One manifestation of secularism is asserting the right to be free from religious rule and teachings, or, in a state declared to be neutral on matters of belief, from the imposition by government of religion or religious practices upon its people. Another manifestation of secularism is the view that public activities and decisions, especially political ones, should be uninfluenced by religious beliefs and/or practices. Secularism draws its intellectual roots from Greek and Roman philosophers such as Epicurus and Marcus Aurelius; from Enlightenment thinkers such as John Locke, Denis Diderot, Voltaire, Baruch Spinoza, James Madison, Thomas Jefferson, and Thomas Paine; and from more recent freethinkers and atheists such as Robert Ingersoll and Bertrand Russell. The purposes and arguments in support of secularism vary widely. In European laicism, it has been argued that secularism is a movement toward modernization, and away from traditional religious values (also known as secularization). This type of secularism, on a social or philosophical level, has often occurred while maintaining an official state church or other state support of religion. In the United States, some argue that  has served to a greater extent to protect religion and the religious from governmental interference, while secularism on a social level is less prevalent. Within countries as well, differing political movements support secularism for varying reasons. <a href=\"#_dbpedia_2017\">(DBpedia, 2017)</a>"@en ;
    skos:inScheme cwrc:PoliticalAffiliation ;
    prov:derivedFrom dbpedia:Secularism .

cwrc:servants
    void:inDataset cwrc:datasetdefinition ;
    a cwrc:SocialClass, skos:Concept ;
    rdfs:isDefinedBy <http://sparql.cwrc.ca/ontologies/cwrc-2017-08-03> ;
    rdfs:label "domestiques"@fr, "servants"@en ;
    skos:definition ""@fr, "Domestic servants typically live in the home with the family or institution that employs them, although the lowest class of servants might work only casually and hence not receive room and board. This type of labour, very common before the twentieth century, is distinct from that of service positions such as shop assistants, flight attendances, and restaurant workers."@en ;
    skos:inScheme cwrc:SocialClass .

cwrc:sexualReform
    void:inDataset cwrc:datasetdefinition ;
    a cwrc:PoliticalAffiliation, skos:Concept ;
    rdf:value "sex-trade activist", "sex-trade reformer", "sexual liberationist", "sexual libertarian", "sexual reformer" ;
    rdfs:comment "The description for this term is indebted to DBpedia."@en ;
    rdfs:isDefinedBy <http://sparql.cwrc.ca/ontologies/cwrc-2017-08-03> ;
    rdfs:label ""@fr, "sexual reform"@en ;
    skos:definition ""@fr, "Advocacy or activism related to the reform of attitudes, practices and laws related to sex, including autonomy, age of consent, trafficking, and sex work."@en ;
    skos:inScheme cwrc:PoliticalAffiliation .

cwrc:shopkeepers
    void:inDataset cwrc:datasetdefinition ;
    a cwrc:SocialClass, skos:Concept ;
    rdfs:isDefinedBy <http://sparql.cwrc.ca/ontologies/cwrc-2017-08-03> ;
    rdfs:label "commerçants"@fr, "shopkeepers"@en ;
    skos:definition ""@fr, "Owns and runs a pub or shop. Similar to an industrialist but to a lesser degree of magnitude."@en ;
    skos:inScheme cwrc:SocialClass .

cwrc:skilledCraftpersonArtisan
    void:inDataset cwrc:datasetdefinition ;
    a cwrc:SocialClass, skos:Concept ;
    rdfs:isDefinedBy <http://sparql.cwrc.ca/ontologies/cwrc-2017-08-03> ;
    rdfs:label "artisan"@fr, "skilled craftperson/artisan"@en ;
    skos:definition ""@fr, "Goldsmith, tailor, shoemaker, milliner, dressmaker."@en ;
    skos:inScheme cwrc:SocialClass .

cwrc:socialPurity
    void:inDataset cwrc:datasetdefinition ;
    a cwrc:PoliticalAffiliation, skos:Concept ;
    rdf:value "purity movement" ;
    rdfs:comment "The description for this term is indebted to DBpedia."@en ;
    rdfs:isDefinedBy <http://sparql.cwrc.ca/ontologies/cwrc-2017-08-03> ;
    rdfs:label ""@fr, "social purity"@en ;
    skos:definition ""@fr, "The social purity movement was a late 19th-century social movement that sought to abolish prostitution and other sexual activities that were considered immoral according to Christian morality. Composed primarily of women, the movement was active in English-speaking nations from the late 1860s to about 1910, exerting an important influence on the contemporaneous feminist, eugenics, and birth control movements. The movement helped to shape feminist views on prostitution. The roots of the social purity movement lay in early 19th-century moral reform movements, such as radical utopianism, abolitionism, and the temperance movement. In the late 19th century, \"social\" was a euphemism for \"sexual\"; the movement first formed in opposition to the legalization and regulation of prostitution, and quickly spread to other sex-related issues such as raising the age of consent, sexually segregating prisons, eliminating abortion, opposing contraception, and censoring pornography. <a href=\"#_dbpedia_2017\">(DBpedia, 2017)</a>"@en ;
    skos:inScheme cwrc:PoliticalAffiliation ;
    prov:derivedFrom dbpedia:Social_purity_movement .

cwrc:socialReform
    void:inDataset cwrc:datasetdefinition ;
    a cwrc:PoliticalAffiliation, skos:Concept ;
    rdf:value "progressivism", "reform", "reformer", "reformers", "reformist", "social reformer", "social welfare" ;
    rdfs:comment "The description for this term is indebted to DBpedia."@en ;
    rdfs:isDefinedBy <http://sparql.cwrc.ca/ontologies/cwrc-2017-08-03> ;
    rdfs:label ""@fr, "social reform"@en ;
    skos:definition ""@fr, "A reform movement is the kind of social movement that aims to make gradual change, or change in certain aspects of society, rather than rapid or fundamental changes. A reform movement is distinguished from more radical social movements such as revolutionary movements. Reformists' ideas are often grounded in liberalism, although they may be rooted in socialist (specifically, social democratic) or religious concepts. Some rely on personal transformation; others rely on small collectives, such as Mahatma Gandhi's spinning wheel and the self-sustaining village economy, as a mode of social change. Reactionary movements, which can arise against any of these, attempt to put things back the way they were before any successes the new reform movement(s) enjoyed, or to prevent any such successes. <a href=\"#_dbpedia_2017\">(DBpedia, 2017)</a>"@en ;
    skos:inScheme cwrc:PoliticalAffiliation ;
    prov:derivedFrom dbpedia:Reform_movement .

cwrc:socialism
    void:inDataset cwrc:datasetdefinition ;
    a cwrc:PoliticalAffiliation, skos:Concept ;
    rdf:value "militant socialist", "owenite socialism", "socialist", "socialist and feminist", "socialist feminist" ;
    rdfs:comment "La description de ce terme est basée sur celle de DBPedia."@fr, "The description for this term is indebted to DBpedia."@en ;
    rdfs:isDefinedBy <http://sparql.cwrc.ca/ontologies/cwrc-2017-08-03> ;
    rdfs:label ""@en, "Socialisme"@fr ;
    skos:definition "Le mot socialisme recouvre un ensemble très divers de courants de pensée et de mouvements politiques, dont le point commun est de rechercher une organisation sociale et économique plus juste. Le but originel du socialisme est d'obtenir l'égalité sociale, ou du moins une réduction des inégalités, et notamment pour les courants d'inspiration marxiste, d'établir une société sans classes sociales. Plus largement, le socialisme peut être défini comme une tendance politique, historiquement marquée à gauche, dont le principe de base est l'aspiration à un monde meilleur, fondé sur une organisation sociale harmonieuse et sur la lutte contre les injustices. Selon les contextes, le mot socialisme ou l'adjectif socialiste peuvent qualifier une idéologie, un parti politique, un régime politique ou une organisation sociale. Le mot socialisme lui-même entre dans le langage courant à partir des années 1820, dans le contexte de la révolution industrielle et de l'urbanisation qui l'accompagne : il désigne alors un ensemble de revendications et d'idées visant à améliorer le sort des ouvriers, et plus largement de la population, via le remplacement du capitalisme par une société supposée plus juste. L'idée socialiste, sous de multiples formes, se développe au long du XIXe siècle et donne naissance dans le monde entier à des partis politiques s'en réclamant sous diverses dénominations (socialiste, mais également social-démocrate, travailliste, etc.). Dans la seconde moitié du XIXe siècle, le marxisme supplante l'approche dite du « socialisme utopique », ainsi que le « socialisme libertaire » des anarchistes : le courant de pensée marxiste se veut porteur d'une forme « scientifique » de socialisme, fondé sur une analyse du capitalisme, du dépassement de celui-ci par le biais de la lutte des classes et du passage à la propriété sociale des moyens de production. Dans les dernières années du siècle, une partie du socialisme européen s'oriente cependant dans les faits vers le réformisme. À la fin de la Première Guerre mondiale, la famille politique socialiste connaît un schisme avec la naissance du courant communiste, qui continue de se réclamer du socialisme dont il affirme revenir à la tradition révolutionnaire. Les partis socialistes connaissent dans le monde entier des scissions au cours des années 1920 ; ils se trouvent dès lors en compétition avec des partis communistes qui se réclament du « socialisme réel » (ou « socialisme réellement existant ») appliqué par l'Union des républiques socialistes soviétiques (URSS), ce dernier pays étant proclamé « patrie du socialisme ». La plupart des partis socialistes européens accélèrent, notamment après la Seconde Guerre mondiale, leur évolution vers un réformisme éloigné du marxisme, tandis que les régimes communistes alignés sur l'URSS, et qui se disent eux-mêmes socialistes, se multiplient dans le monde. Le socialisme démocratique, c'est-à-dire un socialisme converti à la démocratie libérale et respectueux du jeu parlementaire, représente aujourd'hui la tendance majoritaire des partis socialistes, qui n'envisagent plus la rupture avec l'économie de marché. La notion de socialisme démocratique est par ailleurs désormais associée à celle de social-démocratie qui tend, notamment en Europe, à en devenir un synonyme. Outre les diversités liées à ses variations idéologiques, le socialisme connaît également de nombreux avatars liés aux contextes géographiques et culturels, comme le socialisme arabe ou le socialisme africain. La mouvance socialiste, prise au sens large, demeure aujourd'hui l'une des plus importantes de la vie politique mondiale, bien que le mot socialisme continue de recouvrir un ensemble de réalités, de pratiques politiques, et de formes de pensée extrêmement diverses et parfois contradictoires entre elles, allant des partis travaillistes aux diverses variétés de « gauchisme », en passant par les partis et régimes communistes actuels. La majorité des principaux partis se réclamant du socialisme se réunit, au niveau international, au sein de l'Internationale socialiste et, au niveau européen, au sein du Parti socialiste européen. Ces organisations n'ont cependant pas le monopole de l'usage de l'appellation socialiste. <a href=\"#_dbpedia_2017\">(DBpedia, 2017)</a>"@fr, "Socialism is a range of economic and social systems characterised by social ownership and democratic control of the means of production; as well as the political ideologies, theories, and movements that aim at their establishment. Social ownership may refer to forms of public, collective, or cooperative ownership; to citizen ownership of equity; or to any combination of these. Although there are many varieties of socialism and there is no single definition encapsulating all of them, social ownership is the common element shared by its various forms. Socialist economic systems can be divided into both non-market and market forms. Non-market socialism involves the substitution of factor markets and money with engineering and technical criteria based on calculation performed in-kind, thereby producing an economic mechanism that functions according to different economic laws from those of capitalism. Non-market socialism aims to circumvent the inefficiencies and crises traditionally associated with capital accumulation and the profit system. By contrast, market socialism retains the use of monetary prices, factor markets, and, in some cases, the profit motive with respect to the operation of socially owned enterprises and the allocation of capital goods between them. Profits generated by these firms would be controlled directly by the workforce of each firm or accrue to society at large in the form of a social dividend. The feasibility and exact methods of resource allocation and calculation for a socialist system are the subjects of the socialist calculation debate. The socialist political movement includes a diverse array of political philosophies that originated amid the revolutionary movements of the mid-to-late 1700s and of a general concern for the social problems that were associated with capitalism. In addition to the debate over markets and planning, the varieties of socialism differ in their form of social ownership, how management is to be organized within productive institutions, and the role of the state in constructing socialism. Core dichotomies associated with these concerns include reformism versus revolutionary socialism, and state socialism versus libertarian socialism. Socialist politics has been both centralist and decentralized; internationalist and nationalist in orientation; organized through political parties and opposed to party politics; at times overlapping with trade unions and at other times independent of, and critical of, unions; and present in both industrialized and developing countries. While all tendencies of socialism consider themselves democratic, the term \"democratic socialism\" is often used to highlight its advocates' high value for democratic processes in the economy and democratic political systems, usually to draw contrast to tendencies they may perceive to be undemocratic in their approach. The term is frequently used to draw contrast to the political system of the Soviet Union, which operated in an authoritarian fashion. By the late 19th century, and after further articulation and advancement by Karl Marx and his collaborator Friedrich Engels as the culmination of technological development outstripping the economic dynamics of capitalism, \"socialism\" had come to signify opposition to capitalism and advocacy for a post-capitalist system based on some form of social ownership of the means of production. By the 1920s, social democracy and communism became the two dominant political tendencies within the international socialist movement. Socialism proceeded to emerge as the most influential secular political-economic worldview of the twentieth century, and while the emergence of the Soviet Union as the world's first nominally socialist state led to socialism's widespread association with the Soviet economic model, many economists and intellectuals have argued that in practice the model functioned as a form of state capitalism, or a non-planned administrative or command economy. Socialist parties and ideas remain a political force with varying degrees of power and influence in all continents, heading national governments in many countries around the world. Today, some socialists have also adopted the causes of other social movements, such as environmentalism, feminism and liberalism. <a href=\"#_dbpedia_2017\">(DBpedia, 2017)</a>"@en ;
    skos:inScheme cwrc:PoliticalAffiliation ;
    skos:related cwrc:communism, cwrc:socialReform ;
    prov:derivedFrom dbpedia:Socialism .

cwrc:societyOfFriends
    dcterms:isReplacedBy cwrc:quakerism ;
    void:inDataset cwrc:datasetdefinition ;
    a cwrc:PoliticalAffiliation, skos:Concept ;
    rdf:value "pro-toleration" ;
    rdfs:comment "Deprecated in favour of instance #quakerism."@en, "Désapprouver en faveur de l'instance #quakerism."@fr, "La description de ce terme est basée sur celle de DBPedia."@fr, "The description for this term is indebted to DBpedia."@en ;
    rdfs:isDefinedBy <http://sparql.cwrc.ca/ontologies/cwrc-2017-08-03> ;
    rdfs:label "Society of Friends"@en, "Société religieuse des Amis"@fr ;
    owl:deprecated true ;
    vs:term_status "deprecated"@en ;
    skos:broaderTransitive cwrc:christianity, cwrc:humanRights ;
    skos:definition ""@en, ""@fr, "La Société religieuse des Amis est un mouvement religieux fondé en Angleterre au XVIIe siècle par des dissidents de l'Église anglicane. Les membres de ce mouvement sont communément connus sous le nom de quakers () mais ils se nomment entre eux « Amis » et « Amies ». Le mouvement est souvent nommé simplement Société des Amis et le surnom de « quaker » apparaît le plus souvent dans la dénomination officielle, sous la forme Société religieuse des Amis (quakers). Les historiens s'accordent à désigner George Fox comme le principal fondateur ou le plus important meneur des débuts du mouvement. Depuis sa création en Angleterre, le mouvement s'est d'abord répandu dans les pays de colonisation anglo-saxonne. Au XXe siècle, des missionnaires quakers ont propagé leur religion en Amérique latine et en Afrique. Aujourd'hui, les quakers déclarent être au nombre d'environ 350 000 dans le monde. La Société des Amis se différencie de la plupart des autres groupes issus du christianisme par l'absence de credo et de toute structure hiérarchique. Pour les quakers, la croyance religieuse appartient à la sphère personnelle et chacun est libre de ses convictions. Le concept de « lumière intérieure » (inner light) est cependant partagé par la plupart d'entre eux, quelle que soit la signification donnée à ces mots. De nombreux quakers reconnaissent le christianisme mais ne ressentent pas leur foi comme entrant dans les catégories chrétiennes traditionnelles. On trouve aujourd'hui dans la Société des Amis des pratiques très diverses, y compris un large courant évangélique. <a href=\"#_dbpedia_2017\">(DBpedia, 2017)</a>"@fr, "Quakers (or Friends) are members of a historically Christian group of religious movements generally known as the Religious Society of Friends. Members of the various Quaker movements are all generally united in a belief in the ability of each human being to experientially access \"that of God in every person,\" and therefore they profess the priesthood of all believers, a doctrine derived from the First Epistle of Peter. They include those with evangelical, holiness, liberal, and traditional Quaker understandings of Christianity. To differing extents, the different movements that make up the Religious Society of Friends/Friends Church avoid creeds and hierarchical structures. In 2007, there were approximately 359,000 adult Quakers. In 2012, there were 377,055 adult Quakers. Around 79% of Quakers worldwide belong to the \"evangelical\" and \"programmed\" branches of Quakerism—these Quakers worship in services with singing and a prepared message from the Bible, coordinated by a pastor. Around 11% of Friends practice waiting worship, or unprogrammed worship (more commonly known today as Meeting for Worship), where the order of service is not planned in advance, is predominantly silent, and may include unprepared vocal ministry from those present. Some meetings of both types have Recorded Ministers in their meetings—Friends recognised for their gift of vocal ministry. The first Quakers lived in mid-17th century England. The movement arose from the Legatine-Arians and other dissenting Protestant groups, breaking away from the established Church of England. The Quakers, especially the ones known as the Valiant Sixty, attempted to convert others to their understanding of Christianity, travelling both throughout Great Britain and overseas, preaching the gospel of Jesus Christ. Some of these early Quaker ministers were women. They based their message on the religious belief that \"Christ has come to teach his people himself\", stressing the importance of a direct relationship with God through Jesus Christ, and a direct religious belief in the universal priesthood of all believers. They emphasized a personal and direct religious experience of Christ, acquired through both direct religious experience and the reading and studying of the Bible. Quakers focused their private life on developing behaviour and speech reflecting emotional purity and the light of God. In the past, Quakers were known for their use of thee as an ordinary pronoun, refusal to participate in war, plain dress, refusal to swear oaths, opposition to slavery, and teetotalism. Described as \"natural capitalists\" by the BBC, some Quakers founded banks and financial institutions, including Barclays, Lloyds, and Friends Provident; manufacturing companies, including shoe retailer C. & J. Clark and the big three British confectionery makers Cadbury, Rowntree and Fry's; and philanthropic efforts, including abolition of slavery, prison reform, and social justice projects. <a href=\"#_dbpedia_2017\">(DBpedia, 2017)</a>"@en ;
    skos:inScheme cwrc:PoliticalAffiliation, cwrc:Religion ;
    skos:related cwrc:abolitionism, cwrc:feminism ;
    prov:derivedFrom dbpedia:Quakers .

cwrc:sonOf
    void:inDataset cwrc:datasetdefinition ;
    a owl:ObjectProperty ;
    rdfs:isDefinedBy <http://sparql.cwrc.ca/ontologies/cwrc-2017-08-03> ;
    rdfs:label "fil de"@fr, "son of"@en ;
    rdfs:subPropertyOf cwrc:childOf .

cwrc:spanishRepublicanism
    void:inDataset cwrc:datasetdefinition ;
    a cwrc:PoliticalAffiliation, skos:Concept ;
    rdf:value "spanish republican", "spanish republican supporter" ;
    rdfs:comment "The description for this term is indebted to DBpedia."@en ;
    rdfs:isDefinedBy <http://sparql.cwrc.ca/ontologies/cwrc-2017-08-03> ;
    rdfs:label ""@fr, "Spanish republicanism"@en ;
    skos:definition ""@fr, "There has existed in the Kingdom of Spain a persistent trend of republican thought, especially throughout the 19th, 20th, and 21st centuries, that has manifested itself in diverse political parties and movements over the entire course of the history of Spain. While these movements have shared the objective of establishing a republic in Spain, during these three centuries there have surged distinct schools of thought on the form republicans would want to give to the Spanish State: unitary (centralized) or federal. Despite the country's long-lasting schools of republican movements, the government of Spain has been organized as a republic during only two very short periods in its history, which totaled less than 10 years of republican government in the entirety of Spanish history. The First Spanish Republic lasted from February 1873 to December 1874, and the Second Spanish Republic lasted from April 1931 to April 1939. Currently there are movements and political parties throughout the entire political spectrum that advocate for a Third Spanish Republic, including almost all of the Spanish left, as well as liberal, right-winged, and nationalist parties. <a href=\"#_dbpedia_2017\">(DBpedia, 2017)</a>"@en ;
    skos:inScheme cwrc:PoliticalAffiliation ;
    prov:derivedFrom dbpedia:Republicanism_in_Spain .

cwrc:spiritualism
    void:inDataset cwrc:datasetdefinition ;
    a cwrc:Religion, skos:Concept ;
    rdfs:isDefinedBy <http://sparql.cwrc.ca/ontologies/cwrc-2017-08-03> ;
    rdfs:label "Spiritualism"@en, "Spritisme"@fr ;
    rdfs:subClassOf dbpedia:Spiritualism ;
    skos:definition ""@fr, "Spiritualism is the belief that the spirits of the dead have both the ability and the inclination to communicate with the living. The afterlife, or the \"spirit world\", is seen by spiritualists, not as a static place, but as one in which spirits continue to evolve. These two beliefs: that contact with spirits is possible, and that spirits are more advanced than humans, lead spiritualists to a third belief, that spirits are capable of providing useful knowledge about moral and ethical issues, as well as about the nature of God. Some spiritualists will speak of a concept which they refer to as \"spirit guides\"—specific spirits, often contacted, who are relied upon for spiritual guidance. Spiritism, a branch of spiritualism developed by Allan Kardec and today practiced mostly in Continental Europe and Latin America, especially in Brazil, emphasizes reincarnation.<a href=\"#_dbpedia_2017\">(DBpedia, 2017)</a>"@en ;
    skos:inScheme cwrc:Religion ;
    prov:derivedFrom dbpedia:Spiritualism .

cwrc:sshrc
    a foaf:Organization ;
    foaf:name "Conseil de recherches en sciences humaines"@fr, "Social Sciences and Humanities Research Council"@en ;
    foaf:nick "SSHRC" .

cwrc:stalinism
    void:inDataset cwrc:datasetdefinition ;
    a cwrc:PoliticalAffiliation, skos:Concept ;
    rdf:value "stalinist", "totalitarian" ;
    rdfs:comment "La description de ce terme est basée sur celle de DBPedia."@fr, "The description for this term is indebted to DBpedia."@en ;
    rdfs:isDefinedBy <http://sparql.cwrc.ca/ontologies/cwrc-2017-08-03> ;
    rdfs:label "Stalinism"@en, "Stalinisme"@fr ;
    skos:broaderTransitive cwrc:communism ;
    skos:definition "Le mot stalinisme désigne l’idéologie et la pratique politique des partis communistes ayant adopté la ligne politique définie par les partisans de Joseph Staline, secrétaire général du Parti communiste de l'Union soviétique. Par extension, ces partis et leurs membres ont été qualifiés de staliniens. Le stalinisme est caractérisé par le centralisme et l'emploi de la force et de la terreur comme mode de gouvernement, accompagnés d'un culte de la personnalité organisé autour du principal dirigeant de chaque Parti communiste. Les régimes staliniens se caractérisent par une économie planifiée par l'état. Par extension, le terme de stalinisme et les adjectifs stalinien ou, plus rarement, staliniste sont parfois utilisés pour qualifier l'ensemble des régimes basés sur le modèle soviétique, ainsi que les partis politiques les soutenant. Après la déstalinisation (1956), l'Union soviétique cesse de se réclamer de Staline, mais le terme stalinisme et l'adjectif stalinien continuent d'être utilisés, dans le cadre de discours critiques ou polémiques, pour qualifier l'URSS, l'ensemble des pays du bloc de l'Est et plus largement l'ensemble des régimes dictatoriaux communistes. En Europe après la déstalinisation, seule la République populaire socialiste d'Albanie s'est réclamée de la continuité stalinienne. En Asie en revanche, ce fut encore, durant des décennies, le cas des régimes communistes chinois, vietnamien, laotien, cambodgien et surtout coréen qui, au XXIe siècle, est parfois qualifiée de « dernier régime stalinien ». <a href=\"#_dbpedia_2017\">(DBpedia, 2017)</a>"@fr, "Stalinism is the means of governing and related policies implemented by Joseph Stalin. Stalinist policies in the Soviet Union included state terror, rapid industrialization, the theory of socialism in one country, a centralized state, collectivization of agriculture, cult of personality in leadership, and subordination of interests of foreign communist parties to those of the Communist Party of the Soviet Union—deemed by Stalinism to be the most forefront vanguard party of communist revolution at the time. Stalinism promoted the escalation of class conflict, utilizing state violence to forcibly purge society of claimed supporters of the bourgeoisie, regarding them as threats to the pursuit of the communist revolution that resulted in substantial political violence and persecution of such people. These included not only bourgeois people but also working-class people accused of counter-revolutionary sympathies. Stalinist industrialization was officially designed to accelerate the development towards communism, stressing that such rapid industrialization was needed because the country was previously economically backward in comparison with other countries; and that it was needed in order to face the challenges posed by internal and external enemies of communism. Rapid industrialization was accompanied with mass collectivization of agriculture and rapid urbanization. Rapid urbanization converted many small villages into industrial cities. To accelerate the development of industrialization, Stalin pragmatically created joint venture contracts with major American private enterprises, such as Ford Motor Company, that under state supervision assisted in developing the basis of industry of the Soviet economy from the late 1920s to 1930s. After the American private enterprises completed their tasks, Soviet state enterprises took over. <a href=\"#_dbpedia_2017\">(DBpedia, 2017)</a>"@en ;
    skos:inScheme cwrc:PoliticalAffiliation ;
    prov:derivedFrom dbpedia:Stalinism .

cwrc:suffrage
    void:inDataset cwrc:datasetdefinition ;
    cwrc:contraryTo cwrc:anti-Feminism ;
    a cwrc:PoliticalAffiliation, skos:Concept ;
    rdf:value "christian suffragist", "female suffrage", "moderate suffragist", "non-militant suffragist", "suffrage", "suffragism", "suffragist", "women's suffrage" ;
    rdfs:comment "La description de ce terme est basée sur celle de DBPedia."@fr, "The description for this term is indebted to DBpedia."@en ;
    rdfs:isDefinedBy <http://sparql.cwrc.ca/ontologies/cwrc-2017-08-03> ;
    rdfs:label "Droit de vote"@fr, "suffrage movement"@en ;
    skos:broaderTransitive cwrc:feminism, cwrc:socialReform ;
    skos:definition "Le droit de vote permet aux citoyens d'un État de voter pour exprimer leur volonté, à l'occasion d'un scrutin. Dans son application contemporaine, il pose un choix et permet, soit d'élire des gouvernants à but représentatif, soit de répondre à une question posée par la gouvernance, sous forme de plébiscite ou de référendum. Les démocraties modernes présentent le droit de vote comme un droit civique fondamental. À partir du XIXe siècle, le vote devient un synonyme de démocratie, alors qu'auparavant il désignait un régime aristocratique ou oligarchique. <a href=\"#_dbpedia_2017\">(DBpedia, 2017)</a>"@fr, "Suffrage, political franchise, or simply franchise is the right to vote in public, political elections (although the term is sometimes used for any right to vote). The right to run for office is sometimes called candidate eligibility, and the combination of both rights is sometimes called full suffrage. In many languages, the right to vote is called the active right to vote and the right to run for office is called the passive right to vote. In English, these are sometimes called active suffrage and passive suffrage. Suffrage is often conceived in terms of elections for representatives. However, suffrage applies equally to referenda and initiatives. Suffrage describes not only the legal right to vote, but also the practical question of whether a question will be put to a vote. The utility of suffrage is reduced when important questions are decided unilaterally by elected or non-elected representatives. In most democracies, eligible voters can vote in elections of representatives. Voting on issues by referendum may also be available. For example, in Switzerland this is permitted at all levels of government. In the United States, some states such as California and Washington have exercised their shared sovereignty to offer citizens the opportunity to write, propose, and vote on referendums and initiatives; other states have not. The United States federal government does not offer any initiatives at all. Suffrage is granted to qualifying citizens once they have reached the voting age. What constitutes a qualifying citizen depends on the government's decision, but most democracies no longer extend differing rights to vote on the basis of sex or race. Resident non-citizens can vote in some countries, which may be restricted to citizens of closely linked countries (e.g., Commonwealth citizens and European Union citizens). <a href=\"#_dbpedia_2017\">(DBpedia, 2017)</a>"@en ;
    skos:inScheme cwrc:PoliticalAffiliation ;
    prov:derivedFrom dbpedia:Suffrage .

cwrc:taxResistance
    void:inDataset cwrc:datasetdefinition ;
    a cwrc:PoliticalAffiliation, skos:Concept ;
    rdf:value "tax resister", "tax withholder" ;
    rdfs:comment "La description de ce terme est basée sur celle de DBPedia."@fr, "The description for this term is indebted to DBpedia."@en ;
    rdfs:isDefinedBy <http://sparql.cwrc.ca/ontologies/cwrc-2017-08-03> ;
    rdfs:label "Résistance fiscale"@fr, "tax resistance"@en ;
    skos:definition "La résistance fiscale (ou résistance à l'imposition ou désobéissance fiscale) est un acte politique consistant à refuser de participer à la fiscalité de son pays au nom de valeurs morales. C'est une forme de résistance non-violente. <a href=\"#_dbpedia_2017\">(DBpedia, 2017)</a>"@fr, "Tax resistance is the refusal to pay tax because of opposition to the government that is imposing the tax or to government policy or as opposition to the concept of taxation in itself. Tax resistance is a form of direct action and if in violation of the tax regulations, a form of civil disobedience. Examples of tax resistance campaigns include those advocating home rule, such as the Salt March led by Mahatma Gandhi, and those promoting women's suffrage, such as the Women's Tax Resistance League. War tax resistance is the refusal to pay some or all taxes that pay for war and a form of nonviolent resistance. War tax resistance may be practiced by conscientious objectors, pacifists, or those protesting against a particular war. As a percentage of income tax funds military expenditure, war tax resisters may avoid or refuse to pay some or all income tax. For example, war resisters may choose to avoid taxes by living simply below the income tax threshold. Tax resisters are distinct from tax protesters who deny that the legal obligation to pay taxes exists or applies. Tax resisters may accept that some law commands them to pay taxes but they still choose to resist taxation. <a href=\"#_dbpedia_2017\">(DBpedia, 2017)</a>"@en ;
    skos:inScheme cwrc:PoliticalAffiliation ;
    skos:related cwrc:anti-Monarchism ;
    prov:derivedFrom dbpedia:Tax_resistance .

cwrc:temperanceMovement
    void:inDataset cwrc:datasetdefinition ;
    a cwrc:PoliticalAffiliation, skos:Concept ;
    rdf:value "temperance", "temperance activist", "temperance supporter" ;
    rdfs:comment "La description de ce terme est basée sur celle de DBPedia."@fr, "The description for this term is indebted to DBpedia."@en ;
    rdfs:isDefinedBy <http://sparql.cwrc.ca/ontologies/cwrc-2017-08-03> ;
    rdfs:label "Ligue de tempérance"@fr, "temperance movement"@en ;
    skos:definition "The temperance movement is a social movement against the consumption of alcoholic beverages. Temperance movements typically criticize excessive alcohol consumption, promote complete abstinence (teetotalism), or use its political influence to press the government to enact alcohol laws to regulate the availability of alcohol or even its complete prohibition. <a href=\"#_dbpedia_2017\">(DBpedia, 2017)</a>"@en, "Une Ligue de tempérance est une association formée pour s'opposer à la consommation d'alcools. Son fondement est souvent d'ordre religieux ou moral : la plupart des mouvements du XXe siècle en Occident sont également associés au mouvement féministe, l'alcool étant souvent la cause de violences conjugales et absorbant une part substantielle des revenus des familles à bas revenus. <a href=\"#_dbpedia_2017\">(DBpedia, 2017)</a>"@fr ;
    skos:inScheme cwrc:PoliticalAffiliation ;
    prov:derivedFrom dbpedia:Temperance_movement .

cwrc:toryPartyBritain
    void:inDataset cwrc:datasetdefinition ;
    cwrc:contraryTo cwrc:whiggism ;
    a cwrc:PoliticalAffiliation, skos:Concept ;
    rdf:value "tory" ;
    rdfs:comment "The description for this term is indebted to DBpedia."@en ;
    rdfs:isDefinedBy <http://sparql.cwrc.ca/ontologies/cwrc-2017-08-03> ;
    rdfs:label ""@fr, "Tory Party (Britain)"@en ;
    skos:definition ""@fr, "The Tories were members of two political parties which existed, sequentially, in the Kingdom of England, the Kingdom of Great Britain and later the United Kingdom of Great Britain and Ireland from the 17th to the early 19th centuries. The first Tories emerged in 1678 in England, when they opposed the Whig-supported Exclusion Bill which set out to disinherit the heir presumptive James, Duke of York (who eventually became James II of England and VII of Scotland). This party ceased to exist as an organised political entity in the early 1760s, although it was used as a term of self-description by some political writers. A few decades later, a new Tory party would rise to establish a hold on government between 1783 and 1830, with William Pitt the Younger followed by Robert Jenkinson, 2nd Earl of Liverpool. The Earl of Liverpool was succeeded by fellow Tory Arthur Wellesley, 1st Duke of Wellington, whose term included the Catholic Emancipation, which occurred mostly due to the election of Daniel O'Connell as a Catholic MP from Ireland. When the Whigs subsequently regained control, the Representation of the People Act 1832 removed the rotten boroughs, many of which were controlled by Tories. In the following general election, the Tory ranks were reduced to 180 MPs. Under the leadership of Robert Peel, the Tamworth Manifesto was issued, which began to transform the Tories into the Conservative Party. However, Peel lost many of his supporters by repealing the Corn Laws, causing the party to break apart. One faction, led by the Earl of Derby and Benjamin Disraeli, survived to become the modern Conservative Party, whose members are commonly still referred to as Tories. <a href=\"#_dbpedia_2017\">(DBpedia, 2017)</a>"@en ;
    skos:inScheme cwrc:PoliticalAffiliation ;
    skos:related cwrc:conservatism ;
    prov:derivedFrom <http://dbpedia.org/resource/Tories_(British_political_party)> .

cwrc:tractarianMovement
    void:inDataset cwrc:datasetdefinition ;
    a cwrc:Religion, skos:Concept ;
    rdfs:isDefinedBy <http://sparql.cwrc.ca/ontologies/cwrc-2017-08-03> ;
    rdfs:label "Tractarian Movement"@en, "tractarianisme"@fr ;
    rdfs:subClassOf dbpedia:Oxford_Movement ;
    skos:broaderTransitive cwrc:churchOfEngland ;
    skos:definition ""@fr, "The Oxford Movement was a movement of High Church members of the Church of England which eventually developed into Anglo-Catholicism. The movement, whose original devotees were mostly associated with the University of Oxford, argued for the reinstatement of some older Christian traditions of faith and their inclusion into Anglican liturgy and theology. They thought of Anglicanism as one of three branches of the One, Holy, Catholic, and Apostolic Church. The movement's philosophy was known as Tractarianism after its series of publications, the Tracts for the Times, published from 1833 to 1841. Tractarians were also disparagingly referred to as \"Newmanites\" (before 1845) and \"Puseyites\" (after 1845) after two prominent Tractarians, John Henry Newman and Edward Bouverie Pusey. Other well-known Tractarians included John Keble, Charles Marriott, Richard Froude, Robert Wilberforce, Isaac Williams and William Palmer.<a href=\"#_dbpedia_2017\">(DBpedia, 2017)</a>"@en ;
    skos:inScheme cwrc:Religion ;
    prov:derivedFrom dbpedia:Oxford_Movement .

cwrc:tradeUnionism
    void:inDataset cwrc:datasetdefinition ;
    a cwrc:PoliticalAffiliation, skos:Concept ;
    rdf:value "trade unionist", "union movement", "unionism" ;
    rdfs:comment "The description for this term is indebted to DBpedia."@en ;
    rdfs:isDefinedBy <http://sparql.cwrc.ca/ontologies/cwrc-2017-08-03> ;
    rdfs:label ""@fr, "trade unionism"@en ;
    skos:broaderTransitive cwrc:socialReform ;
    skos:definition ""@fr, "In support of the formation of a trade union. See <a href=\"https://en.wikipedia.org/wiki/Trade_union\">https://en.wikipedia.org/wiki/Trade_union</a>"@en ;
    skos:inScheme cwrc:PoliticalAffiliation ;
    prov:derivedFrom dbpedia:Trade_union .

cwrc:transMan
    void:inDataset cwrc:datasetdefinition ;
    a cwrc:Gender, skos:Concept ;
    rdfs:isDefinedBy <http://sparql.cwrc.ca/ontologies/cwrc-2017-08-03> ;
    rdfs:label "homme trans"@fr, "transman/transmale"@en ;
    skos:definition ""@en ;
    foaf:name "transman/transmale (gender)"@en .

cwrc:transWoman
    void:inDataset cwrc:datasetdefinition ;
    a cwrc:Gender, skos:Concept ;
    rdfs:isDefinedBy <http://sparql.cwrc.ca/ontologies/cwrc-2017-08-03> ;
    rdfs:label "femme trans"@fr, "transwoman/transfemale"@en ;
    skos:definition ""@en ;
    foaf:name "transwoman/transfemale (gender)"@en .

cwrc:uncleOf
    void:inDataset cwrc:datasetdefinition ;
    a owl:ObjectProperty ;
    rdf:value "UNCLE" ;
    rdfs:isDefinedBy <http://sparql.cwrc.ca/ontologies/cwrc-2017-08-03> ;
    rdfs:label "oncle de"@fr, "uncle of"@en ;
    rdfs:subPropertyOf cwrc:relativeOf .

cwrc:unitarianChurch
    dcterms:isReplacedBy cwrc:unitarianism ;
    void:inDataset cwrc:datasetdefinition ;
    a skos:Concept ;
    rdf:value "unitarianChurch" ;
    rdfs:comment "Deprecated in favour of instance #unitarianism."@en, "Désapprouver en faveur de l'instance #unitarianism."@fr, "La description de ce terme est basée sur celle de DBPedia."@fr ;
    rdfs:isDefinedBy <http://sparql.cwrc.ca/ontologies/cwrc-2017-08-03> ;
    rdfs:label "Unitarian Church"@en, "Église unitarienne"@fr ;
    owl:deprecated true ;
    vs:term_status "deprecated"@en ;
    skos:broaderTransitive cwrc:christianity ;
    skos:definition ""@fr, "Unitarian church usually refers to a church (either a single church or a group of churches and/or its followers) which follows Unitarianism, a Christian theology. It can also more broadly refer to a church which is a member of an umbrella group with \"Unitarian\" in its title, such as the Unitarian Universalist Association in the U.S., the Canadian Unitarian Council, and similar bodies. <a href=\"#_dbpedia_2017\">(DBpedia, 2017)</a>"@en ;
    prov:derivedFrom dbpedia:Unitarian_church .

cwrc:unitarianism
    void:inDataset cwrc:datasetdefinition ;
    a cwrc:Religion, skos:Concept ;
    rdf:value "unitarianMovement" ;
    rdfs:comment "La description de ce terme est basée sur celle de DBPedia."@fr, "The description for this term is indebted to the Getty Art & Architecture Thesaurus."@en ;
    rdfs:isDefinedBy <http://sparql.cwrc.ca/ontologies/cwrc-2017-08-03> ;
    rdfs:label "Unitarianism"@en, "unitarios"@es, "unitarisme"@fr, "unitarisme"@nl, "unitarismo"@es ;
    rdfs:subClassOf dbpedia:Unitarianism ;
    skos:altLabel "Unitarian"@en, "Unitarian Church"@en, "Unitarian Movement"@en ;
    skos:broaderTransitive cwrc:protestantism ;
    skos:definition "In het bijzonder te gebruiken voor de vrijzinnig protestantse beweging die in Europa opkwam tijdens de Reformatie in de 16de eeuw, werd belichaamd door een kerk in Transsylvanië en een confessionele status verkreeg in Groot-Brittannië, de Verenigde Staten en Canada tijdens de 19de eeuw. De beweging wordt gekenmerkt door de afwijzing van de orthodox christelijke leer van de Drie-eenheid en de goddelijke Christus, het vrije gebruik van de rede in religieuze zaken en het geloof dat God bestaat in één persoon. In 1961 fuseerde deze beweging in de Verenigde Staten en Canada met de universalistische beweging, waardoor het ‘unitaristisch universalisme’ ontstond. Ook in het algemeen te gebruiken voor de theologische leer van de eenheid van God en het mens-zijn van Jezus, zoals voor het eerst verwoord in het monarchisme van de 2de en 3de eeuw en in de leer van Arius in de 3de en 4de eeuw, en later in de leer van de radicale neoplatonisten uit de Reformatie zoals Michael Servetus, Faustus Socinus en Ferenc David. <a href=\"#_getty_2017\">(Getty, 2017)</a>"@nl, "L’unitarisme est une doctrine qui affirme que le Dieu du christianisme est une seule personne, et non pas une seule nature ou \"ousie\" en trois hypostases comme l'affirme le dogme de la Trinité : Père, Fils et Esprit. Selon le dogme de la Trinité, ces trois personnes divines participent d'une seule nature divine unique . Le « trinitarisme » est la doctrine officielle du christianisme depuis le premier concile de Nicée (325) et le concile de Chalcédoine (451). <a href=\"#_dbpedia_2017\">(DBpedia, 2017)</a>"@fr, "The liberal Protestant movement that arose in Europe during the 16th century Reformation, was embodied in a church in Transylvania, and achieved denominational status in the 19th century in the United Kingdom, the United States, and Canada. It is characterized by a denial of the orthodox Christian doctrines of the Trinity and the divinity of Jesus, the free use of reason in religion, and the belief that God exists in one person. In 1961, in the United States and Canada, it merged with the Universalist denomination to form \"Unitarian Universalism.\"  Use also generally for the theological doctrines of the unified nature of God and the humanity of Jesus, first expressed in second- and third-century monarchism and in the teachings of Arius in the third and fourth centuries, and later in the radical Neoplatonist thinkers of the Reformation such as Michael Servetus, Faustus Socinus, and Ferenc David. <a href=\"#_getty_2017\">(Getty, 2017)</a>"@en, "Úsese específicamente para el movimiento protestante liberal que surgió en Europa durante la Reforma del siglo XVI, que tuvo su manifestación en una iglesia en Transilvania, y que logró un estatus confesional en el siglo XIX en el Reino Unido, los Estados Unidos y Canadá. Es caracterizado por una desaprobación de las doctrinas cristianas ortodoxas de la Trinidad y la divinidad de Jesús, el libre uso de la razón en la religión y la creencia que Dios existe en una persona. En 1961, en los Estados Unidos y Canadá s <a href=\"#_getty_2017\">(Getty, 2017)</a>"@es ;
    skos:inScheme cwrc:Religion ;
    prov:derivedFrom dbpedia:Unitarianism, <http://vocab.getty.edu/aat/300263305> .

cwrc:unknownSex
    void:inDataset cwrc:datasetdefinition ;
    a skos:Concept ;
    rdfs:comment "Deprecated with no current equivalence."@en ;
    rdfs:isDefinedBy <http://sparql.cwrc.ca/ontologies/cwrc-2017-08-03> ;
    rdfs:label "Inconnue"@fr, "Unknown"@en ;
    owl:deprecated true ;
    vs:term_status "deprecated"@en ;
    skos:definition ""@en, ""@fr ;
    foaf:name "Unknown (Sex)"@en .

cwrc:upper-middleClass
    void:inDataset cwrc:datasetdefinition ;
    a cwrc:SocialClass, skos:Concept ;
    rdfs:comment "This term is a CWRC specific addition not in the original Orlando tag set."@en ;
    rdfs:isDefinedBy <http://sparql.cwrc.ca/ontologies/cwrc-2017-08-03> ;
    rdfs:label "classe moyenne supérieure"@fr, "upper-middle class"@en ;
    skos:definition ""@en, ""@fr ;
    skos:inScheme cwrc:SocialClass .

cwrc:urban-industrialUnskilled
    void:inDataset cwrc:datasetdefinition ;
    a cwrc:SocialClass, skos:Concept ;
    rdfs:isDefinedBy <http://sparql.cwrc.ca/ontologies/cwrc-2017-08-03> ;
    rdfs:label "ouvrier non qualifié"@fr, "urban unskilled"@en ;
    skos:definition ""@fr, "This category includes factory workers and workers in urban or large-scale industries without defined trades or professional qualifications, and those in low-wage and low-status service sector jobs, such as the restaurant or fast-food industry, in industrial or post-industrial societies."@en ;
    skos:inScheme cwrc:SocialClass .

cwrc:urbanReform
    void:inDataset cwrc:datasetdefinition ;
    a cwrc:PoliticalAffiliation, skos:Concept ;
    rdf:value "urban reformer" ;
    rdfs:comment "The description for this term is indebted to DBpedia."@en ;
    rdfs:isDefinedBy <http://sparql.cwrc.ca/ontologies/cwrc-2017-08-03> ;
    rdfs:label ""@fr, "urban reform"@en ;
    skos:broaderTransitive cwrc:socialReform ;
    skos:definition ""@fr, "Advocacy or activism in support of reforming the urban environment, often in support of alleviating poverty. See <a href=\"https://en.wikipedia.org/wiki/Urban_renewal\">https://en.wikipedia.org/wiki/Urban_renewal</a>"@en ;
    skos:inScheme cwrc:PoliticalAffiliation ;
    prov:derivedFrom dbpedia:Urban_renewal .

cwrc:vegetarianism
    void:inDataset cwrc:datasetdefinition ;
    a cwrc:PoliticalAffiliation, skos:Concept ;
    rdf:value "vegetarian" ;
    rdfs:comment "La description de ce terme est basée sur celle de DBPedia."@fr, "The description for this term is indebted to DBpedia."@en ;
    rdfs:isDefinedBy <http://sparql.cwrc.ca/ontologies/cwrc-2017-08-03> ;
    rdfs:label "Végétarisme"@fr, "vegetarianism"@en ;
    skos:definition "Le végétarisme est une pratique alimentaire qui exclut la consommation de chair animale. Sa définition la plus large correspond à l'ovo-lacto-végétarisme, qui consiste à consommer des végétaux, des champignons et des aliments d'origine animale (comme le miel, les œufs, le lait ainsi que leurs produits dérivés). Il s'agit du végétarisme occidental classique dont les pratiquants étaient appelés « pythagoréens / pythagoriciens » jusqu'en 1847. Le végétarisme indien (hindou et sikh), basé sur l'ahimsâ, autorise la consommation de produits laitiers mais exclut les œufs (les Lois de Manu excluent aussi la consommation des champignons). Le végétarisme est adopté pour des motivations diverses. Certains deviennent végétariens pour des raisons éthiques, religieuses, culturelles ou liées à la santé. D'autres facteurs peuvent motiver l'adoption d'un régime végétarien : la critique des méthodes de traçabilité, d'élevage et d'abattage, l'accès aux denrées alimentaires, l'impact environnemental des modes de production et de prélèvement de ces dernières (les économies d'énergies et d'eau) ou encore le refus par principe de l'exploitation animale. Plusieurs études tendent à montrer qu'une alimentation végétarienne aurait un effet bénéfique sur la santé — diminution des risques de maladies cardiovasculaires et de diabète notamment — et sur l'espérance de vie. Pour autant, cet avantage des régimes sans viande est moins important lorsqu'on les compare avec des régimes omnivores sains. Dans le langage courant, toutes les pratiques alimentaires excluant la chair animale mais incluant la consommation d'autres produits d'origine animale sont appelées « végétarisme » et leurs pratiquants « végétariens ». D'autres pratiques alimentaires influencées par le végétarisme existent, comme le pesco-végétarisme (ou « pescétarisme ») qui inclut la consommation de poisson, de mollusques et de crustacés aquatiques, ou le flexitarisme, souvent qualifié de « semi-végétarisme », qui inclut une consommation de viande occasionnelle. Le végétalisme quant à lui exclut la totalité des produits d'origine animale. <a href=\"#_dbpedia_2017\">(DBpedia, 2017)</a>"@fr, "Vegetarianism /vɛdʒɪˈtɛəriənɪzəm/ is the practice of abstaining from the consumption of meat (red meat, poultry, seafood, and the flesh of any other animal), and may also include abstention from by-products of animal slaughter. Vegetarianism can be adopted for different reasons. Many object to eating meat out of respect for sentient life. Such ethical motivations have been codified under various religious beliefs, along with animal rights. Other motivations for vegetarianism are health-related, political, environmental, cultural, aesthetic, economic, or personal preference. There are varieties of the diet as well: an ovo-vegetarian diet includes eggs but not dairy products, a lacto-vegetarian diet includes dairy products but not eggs, and an ovo-lacto vegetarian diet includes both eggs and dairy products. A vegan diet excludes all animal products, including eggs, dairy, and honey. Some vegans also avoid other animal products such as beeswax, leather or silk clothing, and goose-fat shoe polish. Various packaged or processed foods, including cake, cookies, candies, chocolate, yogurt and marshmallows, often contain unfamiliar animal ingredients, and may be a special concern for vegetarians due to the likelihood of such additions. Often, products are reviewed by vegetarians for animal-derived ingredients prior to purchase or consumption. Vegetarians vary in their feelings regarding these ingredients, however. For example, while some vegetarians may be unaware of animal-derived rennet's role in the usual production of cheese and may therefore unknowingly consume the product, other vegetarians may not take issue with its consumption. Semi-vegetarian diets consist largely of vegetarian foods, but may include fish or poultry, or sometimes other meats, on an infrequent basis. Those with diets containing fish or poultry may define meat only as mammalian flesh and may identify with vegetarianism. This is because earlier dictionaries included fish as part of the definition whereas the current versions do not. A pescetarian diet has been described as \"fish but no other meat\". The common use association between such diets and vegetarianism has led vegetarian groups such as the Vegetarian Society to state that diets containing these ingredients are not vegetarian, because fish and birds are also animals. <a href=\"#_dbpedia_2017\">(DBpedia, 2017)</a>"@en ;
    skos:inScheme cwrc:PoliticalAffiliation ;
    skos:related cwrc:animalWelfareAdvocacy ;
    prov:derivedFrom dbpedia:Vegetarianism .

cwrc:welshNationalHeritage
    void:inDataset cwrc:datasetdefinition ;
    a cwrc:NationalHeritage, skos:Concept ;
    rdfs:isDefinedBy <http://sparql.cwrc.ca/ontologies/cwrc-2017-08-03> ;
    rdfs:label "Gallois"@fr, "Welsh"@en ;
    owl:sameAs <http://sws.geonames.org/2634895/> ;
    skos:broader cwrc:welshLabel ;
    skos:definition ""@en, ""@fr .

cwrc:welshNationalism
    void:inDataset cwrc:datasetdefinition ;
    a cwrc:PoliticalAffiliation, skos:Concept ;
    rdf:value "welsh nationalist" ;
    rdfs:comment "La description de ce terme est basée sur celle de DBPedia."@fr, "The description for this term is indebted to DBpedia."@en ;
    rdfs:isDefinedBy <http://sparql.cwrc.ca/ontologies/cwrc-2017-08-03> ;
    rdfs:label "Nationalisme gallois"@fr, "Welsh nationalism"@en ;
    skos:broaderTransitive cwrc:nationalism ;
    skos:definition """Le nationalisme gallois consiste dans le projet de défense de l'identité du Pays de Galles, de la culture et de la langue galloise. Ses revendications vont de l'autonomisme, visant à obtenir des pouvoirs accrus pour l'Assemblée nationale du Pays de Galles et le gouvernement gallois, à l'indépendantisme, défendu notamment par le parti Plaid Cymru. 
  * Portail de la politique britannique Portail de la politique britannique   
  * Portail du pays de Galles Portail du pays de Galles <a href=\"#_dbpedia_2017\">(DBpedia, 2017)</a>"""@fr, "Welsh nationalism (Welsh: Cenedlaetholdeb Cymreig) emphasises the distinctiveness of Welsh language, culture, and history, and calls for more self-determination for Wales, which might include more devolved powers for the Welsh Assembly or full independence from the United Kingdom. <a href=\"#_dbpedia_2017\">(DBpedia, 2017)</a>"@en ;
    skos:inScheme cwrc:PoliticalAffiliation ;
    prov:derivedFrom dbpedia:Welsh_nationalism .

cwrc:whiggism
    void:inDataset cwrc:datasetdefinition ;
    a cwrc:PoliticalAffiliation, skos:Concept ;
    rdf:value "dissident whig", "foxite whig", "opposition whig", "pittite whig", "whig", "whigs", "williamite" ;
    rdfs:comment "The description for this term is indebted to DBpedia."@en ;
    rdfs:isDefinedBy <http://sparql.cwrc.ca/ontologies/cwrc-2017-08-03> ;
    rdfs:label ""@fr, "whiggism"@en ;
    skos:definition ""@fr, "Whiggism, sometimes spelled Whigism, is a historical political philosophy that grew out of the Parliamentarian faction in the Wars of the Three Kingdoms (1639–1651). The whigs' key policy positions were the supremacy of Parliament (as opposed to that of the king), tolerance of Protestant dissenters, and opposition to a Catholic (especially a Stuart) on the throne. After the huge success of the Glorious Revolution of 1688–1689, Whiggism dominated English and British politics until about 1760, although in practice it splintered into different factions. After 1760 the Whigs lost power, apart from sharing it in a few short-lived coalitions, but Whiggism fashioned itself into a generalized belief system that emphasized innovation and liberty and was strongly held by about half of the leading families in England and Scotland, as well as most merchants, Dissenters and professionals. The opposing Tory position was held by the other great families, the Church of England, and most of the landed gentry and officers of the army and the navy. Whigs who opposed Robert Walpole often called themselves \"Old Whigs\" and comprised part of the Country Party. Whiggism referred originally to the Whigs of the British Isles, but in its \"Old Whig\" form was largely adopted by the American Patriots in the Thirteen Colonies. American Whiggism was known as republicanism. One meaning of 'whiggism' given by the Oxford English Dictionary is \"moderate or antiquated Liberalism\". <a href=\"#_dbpedia_2017\">(DBpedia, 2017)</a>"@en ;
    skos:inScheme cwrc:PoliticalAffiliation ;
    skos:related cwrc:left-Wing, cwrc:liberalism ;
    prov:derivedFrom dbpedia:Whiggism .

cwrc:whiteEthnicity
    void:inDataset cwrc:datasetdefinition ;
    a cwrc:Ethnicity, owl:Thing ;
    rdfs:isDefinedBy <http://sparql.cwrc.ca/ontologies/cwrc-2017-08-03> ;
    rdfs:label "blanc"@fr, "white"@en ;
    skos:broader cwrc:whiteLabel ;
    skos:definition ""@en, ""@fr ;
    foaf:name "white (ethnicity)"@en .

cwrc:whiteLabel
    void:inDataset cwrc:datasetdefinition ;
    a skos:Concept, skosxl:Label ;
    rdfs:isDefinedBy <http://sparql.cwrc.ca/ontologies/cwrc-2017-08-03> ;
    rdfs:label "blanc"@fr, "white"@en ;
    owl:oneOf (cwrc:whiteEthnicity
        cwrc:whiteRace
    ) ;
    skos:definition ""@en, ""@fr ;
    skos:inScheme cwrc:TextLabels ;
    foaf:name "white"@en .

cwrc:whiteRace
    dcterms:isReplacedBy cwrc:whiteRaceColour ;
    void:inDataset cwrc:datasetdefinition ;
    a owl:Thing, skos:Concept ;
    rdfs:comment "Deprecated in favour of instance #whiteRaceColour."@en, "Désapprouver en faveur de l'instance #whiteRaceColour."@fr ;
    rdfs:isDefinedBy <http://sparql.cwrc.ca/ontologies/cwrc-2017-08-03> ;
    rdfs:label "blanc"@fr, "white"@en ;
    rdfs:subClassOf cwrc:whiteLabel ;
    owl:deprecated true ;
    vs:term_status "deprecated"@en ;
    skos:definition ""@en, ""@fr ;
    foaf:name "White (Race Colour)"@en .

cwrc:whiteRaceColour
    void:inDataset cwrc:datasetdefinition ;
    a cwrc:RaceColour, skos:Concept ;
    rdfs:isDefinedBy <http://sparql.cwrc.ca/ontologies/cwrc-2017-08-03> ;
    rdfs:label "blanc"@fr, "white"@en ;
    skos:broader <http://rdf.muninn-project.org/ontologies/appearances#SkinColorSimpleWhite>, cwrc:whiteLabel ;
    skos:definition ""@en, ""@fr ;
    foaf:name "white (race colour)"@en .

cwrc:wilkite
    void:inDataset cwrc:datasetdefinition ;
    a cwrc:PoliticalAffiliation, skos:Concept ;
    rdfs:comment "The description for this term is indebted to DBpedia."@en ;
    rdfs:isDefinedBy <http://sparql.cwrc.ca/ontologies/cwrc-2017-08-03> ;
    rdfs:label ""@fr, "Wilkite"@en ;
    skos:broaderTransitive cwrc:socialReform ;
    skos:definition ""@fr, "A view of the law, in support of John Wilkes. Focused on government accountability and right to trial by jury. See: <a href=\"https://en.wikipedia.org/wiki/John_Wilkes\">https://en.wikipedia.org/wiki/John_Wilkes</a>"@en ;
    skos:inScheme cwrc:PoliticalAffiliation ;
    prov:derivedFrom dbpedia:John_Wilkes .

cwrc:woman
    void:inDataset cwrc:datasetdefinition ;
    a cwrc:Gender, owl:Thing, skos:Concept ;
    rdfs:isDefinedBy <http://sparql.cwrc.ca/ontologies/cwrc-2017-08-03> ;
    rdfs:label "femme"@fr, "woman"@en ;
    skos:definition ""@en ;
    foaf:name "woman (gender)"@en .

cwrc:womanLabel
    void:inDataset cwrc:datasetdefinition ;
    a skos:Concept, skosxl:Label ;
    rdf:value "woman" ;
    rdfs:isDefinedBy <http://sparql.cwrc.ca/ontologies/cwrc-2017-08-03> ;
    rdfs:label "femme"@fr, "woman"@en ;
    owl:oneOf (cwrc:woman
    ) ;
    skos:definition ""@en, ""@fr ;
    skos:inScheme cwrc:TextLabels ;
    foaf:name "Woman (Label)"@en .

cwrc:womanism
    void:inDataset cwrc:datasetdefinition ;
    cwrc:contraryTo cwrc:anti-feminism ;
    a cwrc:PoliticalAffiliation, skos:Concept ;
    rdf:value "womanist" ;
    rdfs:comment "The description for this term is indebted to DBpedia."@en ;
    rdfs:isDefinedBy <http://sparql.cwrc.ca/ontologies/cwrc-2017-08-03> ;
    rdfs:label ""@fr, "womanism"@en ;
    skos:broaderTransitive cwrc:feminism ;
    skos:definition ""@fr, "Womanism is a social theory deeply rooted in the racial and gender-based oppression of black women. There are varying interpretations on what the term \"womanist\" means, and efforts to provide a concise and all encompassing definition have only been marginally successful. The ambiguity within the theory allows for its continuous expansion of its basic tenets, though this ambiguity is also widely considered its greatest weakness. At its core, womanism is a social change perspective based upon the everyday problems and experiences of black women and other women of minority demographics, but more broadly seeks methods to eradicate inequalities not just for black women, but for all people. <a href=\"#_dbpedia_2017\">(DBpedia, 2017)</a>"@en ;
    skos:inScheme cwrc:PoliticalAffiliation ;
    prov:derivedFrom dbpedia:Womanism .

cwrc:womensEducationReform
    void:inDataset cwrc:datasetdefinition ;
    cwrc:contraryTo cwrc:anti-feminism ;
    a cwrc:PoliticalAffiliation, skos:Concept ;
    rdf:value "activist for women's education", "campaigner for women's education", "female education", "female education advocate", "women's education reformer", "women's higher education", "women's medical education" ;
    rdfs:comment "The description for this term is indebted to DBpedia."@en ;
    rdfs:isDefinedBy <http://sparql.cwrc.ca/ontologies/cwrc-2017-08-03> ;
    rdfs:label ""@fr, "women's education reform"@en ;
    skos:broaderTransitive cwrc:educationReform ;
    skos:definition ""@fr, "Reform of education for women. See <a href=\"https://en.wikipedia.org/wiki/Female_education\">https://en.wikipedia.org/wiki/Female_education</a>; <a href=\"https://en.wikipedia.org/wiki/Category:Women_and_education\">https://en.wikipedia.org/wiki/Category:Women_and_education</a>"@en ;
    skos:inScheme cwrc:PoliticalAffiliation ;
    prov:derivedFrom <http://dbpedia.org/resource/Category:Women_and_education>, dbpedia:Female_education .

cwrc:womensEmploymentReform
    void:inDataset cwrc:datasetdefinition ;
    cwrc:contraryTo cwrc:anti-feminism ;
    a cwrc:PoliticalAffiliation, skos:Concept ;
    rdf:value "employment activist", "equal rights in the work place", "female employment", "women's employment reformer" ;
    rdfs:comment "The description for this term is indebted to DBpedia."@en ;
    rdfs:isDefinedBy <http://sparql.cwrc.ca/ontologies/cwrc-2017-08-03> ;
    rdfs:label ""@fr, "women's employment reform"@en ;
    skos:broaderTransitive cwrc:feminism, cwrc:socialReform ;
    skos:definition ""@fr, "Advocacy or activism related to women's employment including training, opportunities, wages, and working conditions. See <a href=\"https://en.wikipedia.org/wiki/Women_in_the_workforce\">https://en.wikipedia.org/wiki/Women_in_the_workforce</a>"@en ;
    skos:inScheme cwrc:PoliticalAffiliation ;
    prov:derivedFrom dbpedia:Women_in_the_workforce .

cwrc:yeoman-farmer
    void:inDataset cwrc:datasetdefinition ;
    a cwrc:SocialClass, skos:Concept ;
    rdfs:isDefinedBy <http://sparql.cwrc.ca/ontologies/cwrc-2017-08-03> ;
    rdfs:label "agriculteur vivrier"@fr, "yeoman farmer"@en ;
    skos:definition ""@fr, "Own just enough land to support themselves if they do most of the work themselves (ie Elizabeth Ham, Mary Webb)."@en ;
    skos:inScheme cwrc:SocialClass .

cwrc:zionism
    void:inDataset cwrc:datasetdefinition ;
    a cwrc:PoliticalAffiliation, skos:Concept ;
    rdf:value "zionist" ;
    rdfs:comment "La description de ce terme est basée sur celle de DBPedia."@fr, "The description for this term is indebted to DBpedia."@en ;
    rdfs:isDefinedBy <http://sparql.cwrc.ca/ontologies/cwrc-2017-08-03> ;
    rdfs:label "Sionisme"@fr, "Zionism"@en ;
    skos:broaderTransitive cwrc:nationalism ;
    skos:definition "Le sionisme est une idéologie politique fondée sur un sentiment national juif, décrite comme nationaliste par les uns et comme émancipatrice par les autres, prônant l'existence d'un centre territorial ou étatique peuplé par les Juifs en Terre d'Israël (Eretz Israël). À la naissance du mouvement, à la fin du XIXe siècle, ce territoire correspondait à la Palestine ottomane, puis après la Première Guerre mondiale à la partie occidentale de la Palestine mandataire. Sur un plan idéologique et institutionnel, le sionisme entend œuvrer à donner ou redonner aux Juifs un statut perdu depuis l'annexion du Royaume d'Israël par l'Empire assyrien en -720, à savoir celui d'un peuple disposant d'un territoire. Il faut le différencier du post-sionisme, qui veut donner une orientation laïque à l'État d'Israël, normaliser les relations avec les Palestiniens, et du néo-sionisme, qui milite pour la migration des Palestiniens et des Arabes israéliens vers les autres pays arabes. Le mouvement sioniste est né parmi les communautés ashkénazes d'Europe centrale et orientale sous la pression des pogroms, mais aussi en Europe occidentale, à la suite du choc causé par l'affaire Dreyfus – qui compte parmi les motifs du lancement du Congrès sioniste par Theodor Herzl. Bien qu'ayant des caractères spécifiques du fait de la dispersion des Juifs, cette idéologie est contemporaine de l'affirmation d'autres nationalismes en Europe. <a href=\"#_dbpedia_2017\">(DBpedia, 2017)</a>"@fr, "Zionism is a nationalist political movement of Jews and Jewish culture that supports the re-establishment of a Jewish homeland in the territory defined as the historic Land of Israel (roughly corresponding to Palestine, Canaan or the Holy Land). Zionism emerged in the late 19th century in central and eastern Europe as a national revival movement, in reaction to anti-Semitic and exclusionary nationalist movements in Europe. Soon after this, most leaders of the movement associated the main goal with creating the desired state in Palestine, then an area controlled by the Ottoman Empire. Until 1948, the primary goals of Zionism were the re-establishment of Jewish sovereignty in the Land of Israel, ingathering of the exiles, and liberation of Jews from the antisemitic discrimination and persecution that they experienced during their diaspora. Since the establishment of the State of Israel in 1948, Zionism continues primarily to advocate on behalf of Israel and address threats to its continued existence and security. A religious variety of Zionism supports Jews upholding their Jewish identity defined as adherence to religious Judaism, opposes the assimilation of Jews into other societies, and has advocated the return of Jews to Israel as a means for Jews to be a majority nation in their own state. A variety of Zionism, called cultural Zionism, founded and represented most prominently by Ahad Ha'am, fostered a secular vision of a Jewish \"spiritual center\" in Israel. Unlike Herzl, the founder of political Zionism, Ahad Ha'am strived for Israel to be \"a Jewish state and not merely a state of Jews\". Advocates of Zionism view it as a national liberation movement for the repatriation of a persecuted people residing as minorities in a variety of nations to their ancestral homeland. Critics of Zionism view it as a colonialist, racist and exceptionalist ideology that led advocates to violence during Mandatory Palestine, followed by the forced exodus of Palestinians, and the subsequent denial of their human rights. <a href=\"#_dbpedia_2017\">(DBpedia, 2017)</a>"@en ;
    skos:inScheme cwrc:PoliticalAffiliation ;
    skos:related cwrc:anti-Antisemitism ;
    prov:derivedFrom dbpedia:Zionism .

prov:derivedFrom
    rdfs:range cwrc:Context .

